@prefix rdf: <http://www.w3.org/1999/02/22-rdf-syntax-ns#>.
@prefix rdfs: <http://www.w3.org/2000/01/rdf-schema#>.
@prefix xsd: <http://www.w3.org/2001/XMLSchema#>.
@prefix cc: <http://creativecommons.org/ns#>.
@prefix dcterms: <http://purl.org/dc/terms/>.
@prefix owl: <http://www.w3.org/2002/07/owl#>.
@prefix foaf: <http://xmlns.com/foaf/0.1/>.
@prefix ql: <http://semweb.mmlab.be/ns/ql#>.
@prefix rml: <http://semweb.mmlab.be/ns/rml#>.
@prefix rmlt: <http://semweb.mmlab.be/ns/rml-target#>.
@prefix rr: <http://www.w3.org/ns/r2rml#>.
@prefix vann: <http://purl.org/vocab/vann/>.
@prefix xml: <http://www.w3.org/XML/1998/namespace>.
@prefix : <http://semweb.mmlab.be/ns/rml#>.

{
    _:autos189 foaf:name "Anastasia Dimou".
    _:autos190 foaf:name "Miel Vander Sande".
    _:autos191 a owl:Class;
               owl:intersectionOf _:autos192.
    _:autos192 rdf:first rr:ObjectMap;
               rdf:rest _:autos193.
    _:autos193 rdf:first _:autos194;
               rdf:rest rdf:nil.
    _:autos194 a owl:Restriction;
               owl:maxQualifiedCardinality "0"^^xsd:nonNegativeInteger;
               owl:onDataRange xsd:string;
               owl:onProperty rml:reference.
    _:autos195 a owl:Class;
               owl:intersectionOf _:autos196.
    _:autos196 rdf:first rr:PredicateMap;
               rdf:rest _:autos197.
    _:autos197 rdf:first _:autos198;
               rdf:rest rdf:nil.
    _:autos198 a owl:Restriction;
               owl:maxQualifiedCardinality "0"^^xsd:nonNegativeInteger;
               owl:onDataRange xsd:string;
               owl:onProperty rml:reference.
    _:autos199 a owl:Class;
               owl:intersectionOf _:autos200.
    _:autos200 rdf:first rr:SubjectMap;
               rdf:rest _:autos201.
    _:autos201 rdf:first _:autos202;
               rdf:rest rdf:nil.
    _:autos202 a owl:Restriction;
               owl:maxQualifiedCardinality "0"^^xsd:nonNegativeInteger;
               owl:onDataRange xsd:string;
               owl:onProperty rml:reference.
    _:autos203 a owl:Restriction;
               owl:minQualifiedCardinality "1"^^xsd:nonNegativeInteger;
               owl:onClass rml:LogicalSource;
               owl:onProperty rml:logicalSource.
    _:autos204 a owl:Restriction;
               owl:onClass rr:SubjectMap;
               owl:onProperty rr:subjectMap;
               owl:qualifiedCardinality "1"^^xsd:nonNegativeInteger.
    _:autos205 a owl:Restriction;
               owl:onProperty rml:referenceFormulation;
               owl:qualifiedCardinality "1"^^xsd:nonNegativeInteger.
    _:autos206 a owl:Restriction;
               owl:maxQualifiedCardinality "1"^^xsd:nonNegativeInteger;
               owl:onProperty rml:iterator.
    _:autos207 a owl:Restriction;
               owl:minQualifiedCardinality "1"^^xsd:nonNegativeInteger;
               owl:onProperty rml:source.
    ql:CSS3 ql:specification <http://www.w3.org/TR/css3-selectors/>;
            a rml:ReferenceFormulation,
              owl:NamedIndividual;
            rdfs:comment "Denotes the selectors, namely the patterns that match against elements in a tree and are used in CSS and other thechnolgies to select elements in HTML or XML documents.";
            rdfs:label "Selectors Level 3".
    ql:CSV ql:specification <http://tools.ietf.org/html/rfc4180>;
           a rml:ReferenceFormulation,
             owl:NamedIndividual;
           rdfs:comment "Denotes that the CSV file's column names are used for referring to extracts of CSV resources."@en;
           rdfs:label "CSV".
    ql:JSONPath a rml:ReferenceFormulation,
                  owl:NamedIndividual;
                rdfs:comment "Denotes the JSONPath reference formulation, used for referring to extracts of JSON sources."@en;
                rdfs:label "JSONPath".
    ql:XPath ql:specification <http://www.w3.org/TR/xpath20/>;
             rml:version "2.0";
             a rml:ReferenceFormulation,
               owl:NamedIndividual;
             rdfs:comment "Denotes the XPath reference formulation, used for referring to extracts of XML sources."@en;
             rdfs:label "XPath".
    rml: cc:license <http://creativecommons.org/licenses/by/3.0/>;
         dcterms:creator _:autos189,
                         _:autos190;
         dcterms:description "Generic Mapping Language for RDF (RDB/CSV/TSV/XML/JSON/... to RDF) - Vocabulary description"@en;
         dcterms:issued "2013-07-01"^^xsd:date;
         dcterms:modified "2014-09-10"^^xsd:date;
         dcterms:title "RML: Generic Mapping Language for RDF"@en;
         vann:preferredNamespacePrefix "rml";
         vann:preferredNamespaceUri "http://semweb.mmlab.be/ns/rml#";
         a <http://purl.org/vocommons/voaf#Vocabulary>,
           owl:Ontology;
         owl:imports rr:.
    rml:BaseSource a owl:Class;
                   rdfs:comment "Base Source",
                                "Represents a base source."@en;
                   rdfs:label "Base Source";
                   rdfs:subClassOf rml:LogicalSource.
    rml:LogicalSource a owl:Class;
                      rdfs:comment "Represents a logical source."@en;
                      rdfs:label "Logical Source";
                      rdfs:subClassOf _:autos205,
                                      _:autos206,
                                      _:autos207,
                                      owl:Thing.
    rml:ReferenceFormulation a owl:Class;
                             rdfs:comment "Represents a Reference Formulation."@en;
                             rdfs:label "Reference Formulation".
    rml:TriplesMap rdfs:comment "Represents a triples map."@en;
                   rdfs:subClassOf _:autos203,
                                   _:autos204,
                                   owl:Thing.
    rml:iterator a owl:DatatypeProperty;
                 rdfs:comment "an expression qualified according to the reference formulation specified for pointing to an extract of the source data. "@en;
                 rdfs:domain rml:LogicalSource;
                 rdfs:label "iterator";
                 rdfs:range xsd:string.
    rml:logicalSource a owl:ObjectProperty;
                      rdfs:comment "Represents the logical source to be mapped. This can be a pointer to any dataset."@en;
                      rdfs:domain rr:TriplesMap;
                      rdfs:label "logical source";
                      rdfs:range rml:LogicalSource.
    rml:logicalTarget a owl:ObjectProperty;
                      rdfs:comment "Represents the logical target to where triples are exported to. This can be a pointer to any dataset."@en;
                      rdfs:domain rr:TriplesMap;
                      rdfs:label "logical target";
                      rdfs:range rmlt:LogicalTarget.
    rml:query a owl:DatatypeProperty;
              rdfs:comment "A valid query."@en;
              rdfs:domain rml:LogicalSource.
    rml:reference a owl:DatatypeProperty;
                  rdfs:comment "A valid expression that selects values from the source data. The reference should confront to the syntax rules/grammar of the specified Reference Formulation. "@en;
                  rdfs:domain rr:TermMap;
                  rdfs:label "reference";
                  rdfs:range xsd:string.
    rml:referenceFormulation a owl:ObjectProperty;
                             rdfs:comment "The reference formulation used to refer to extracts of the source data. "@en;
                             rdfs:domain rml:LogicalSource;
                             rdfs:label "reference formulation";
                             rdfs:range rml:ReferenceFormulation.
    rml:source a rdf:Property;
               rdfs:comment "qualified name of the source data."@en;
               rdfs:domain rml:LogicalSource;
               rdfs:label "source".
    rml:version a owl:DatatypeProperty;
                rdfs:comment "It defines the version of the reference Formulation used. "@en;
                rdfs:domain rml:LogicalSource;
                rdfs:label "version";
                rdfs:range xsd:string.
    rr:LogicalTable rdfs:subClassOf rml:LogicalSource.
    rr:TriplesMap rdfs:subClassOf rml:TriplesMap.
    rr:column rdfs:subPropertyOf rml:reference.
    rr:object rdfs:domain _:autos191.
    rr:predicate rdfs:domain _:autos195.
    rr:sqlQuery rdfs:subPropertyOf rml:query.
    rr:sqlVersion rdfs:subPropertyOf rml:version.
    rr:subject rdfs:domain _:autos199.
    rr:tableName rdfs:subPropertyOf rml:source.
}

