@prefix rdf: <http://www.w3.org/1999/02/22-rdf-syntax-ns#>.
@prefix rdfs: <http://www.w3.org/2000/01/rdf-schema#>.
@prefix xsd: <http://www.w3.org/2001/XMLSchema#>.
@prefix solid: <http://www.w3.org/ns/solid/terms#>.
@prefix owl: <http://www.w3.org/2002/07/owl#>.
@prefix dc: <http://purl.org/dc/terms/>.
@prefix foaf: <http://xmlns.com/foaf/0.1/>.
@prefix ldp: <http://www.w3.org/ns/ldp#>.
@prefix log: <http://www.w3.org/2000/10/swap/log#>.
@prefix vann: <http://purl.org/vocab/vann/>.
@prefix ws: <http://www.w3.org/ns/pim/space#>.

solid: dc:issued "2015-11-16"^^xsd:date;
       dc:license <https://creativecommons.org/publicdomain/zero/1.0/>;
       vann:preferredNamespacePrefix "solid";
       vann:preferredNamespaceUri "http://www.w3.org/ns/solid/terms#"^^xsd:anyURI;
       a owl:Ontology;
       rdfs:comment "The Solid Terms vocabulary defines terms referenced in Solid specifications."@en;
       rdfs:isDefinedBy solid:;
       rdfs:label "Solid Terms"@en;
       owl:versionInfo [dc:date "2020-12-22"^^xsd:date ; 
                        dc:replaces <https://raw.githubusercontent.com/solid/vocab/46a5e2a8df1df48cd21a6ecdd422a37d29d39cbe/solid-terms.ttl> ; 
                        rdfs:seeAlso <https://github.com/solid/vocab/pull/67>].
solid:Account dc:issued "2016-05-17"^^xsd:date;
              a rdfs:Class;
              rdfs:comment "A Solid account."@en;
              rdfs:isDefinedBy solid:;
              rdfs:label "Account"@en.
solid:Inbox dc:issued "2015-11-16"^^xsd:date;
            dc:modified "2018-10-24"^^xsd:date;
            a rdfs:Class;
            rdfs:comment "A resource containing notifications."@en;
            rdfs:isDefinedBy solid:;
            rdfs:label "Inbox"@en.
solid:InsertDeletePatch dc:issued "2022-05-03"^^xsd:date;
                        a rdfs:Class;
                        rdfs:comment "A class of patch expressing insertions, deletions, and conditional modifications to a resource that has an RDF-based representation."@en;
                        rdfs:isDefinedBy solid:;
                        rdfs:label "Insert/delete patch"@en;
                        rdfs:seeAlso <https://solidproject.org/TR/2021/protocol-20211217#server-patch-n3-type>;
                        rdfs:subClassOf solid:Patch.
solid:ListedDocument dc:issued "2015-11-16"^^xsd:date;
                     dc:modified "2018-01-24"^^xsd:date;
                     a rdfs:Class;
                     rdfs:comment "Listed Type Index is a registry of resources that are publicly discoverable by outside users and applications."@en;
                     rdfs:isDefinedBy solid:;
                     rdfs:label "Listed Type Index"@en.
solid:Notification dc:issued "2015-12-18"^^xsd:date;
                   dc:modified "2015-12-20"^^xsd:date,
                               "2018-10-25"^^xsd:date;
                   a rdfs:Class;
                   rdfs:comment "A notification resource."@en;
                   rdfs:isDefinedBy solid:;
                   rdfs:label "Notification"@en.
solid:Patch dc:issued "2017-08-17"^^xsd:date;
            a rdfs:Class;
            rdfs:comment "A patch expresses conditional modifications to a resource that has an RDF-based representation."@en;
            rdfs:isDefinedBy solid:;
            rdfs:label "Patch"@en.
solid:Timeline dc:issued "2016-01-04"^^xsd:date;
               a rdfs:Class;
               rdfs:comment "A resource containing time ordered items and sub-containers.  Sub-containers may be desirable in file based systems to split the timeline into logical components e.g. /yyyy-mm-dd/ as used in ISO 8061."@en;
               rdfs:isDefinedBy solid:;
               rdfs:label "Timeline"@en.
solid:TypeIndex dc:issued "2016-02-05"^^xsd:date;
                a rdfs:Class;
                rdfs:comment "A index of type registries for resources. Applications can register the RDF type they use and list them in the index resource."@en;
                rdfs:isDefinedBy solid:;
                rdfs:label "Type index"@en.
solid:TypeRegistration dc:issued "2018-01-24"^^xsd:date;
                       a rdfs:Class;
                       rdfs:comment "The registered types that map a RDF classes/types to their locations using either `instance` or `instanceContainer` property."@en;
                       rdfs:isDefinedBy solid:;
                       rdfs:label "Type Registration"@en.
solid:UnlistedDocument dc:issued "2018-01-24"^^xsd:date;
                       a rdfs:Class;
                       rdfs:comment "Unlisted Type Index is a registry of resources that are private to the user and their apps, for types that are not publicly discoverable."@en;
                       rdfs:isDefinedBy solid:;
                       rdfs:label "Unlisted Type Index"@en.
solid:account dc:issued "2016-05-17"^^xsd:date;
              dc:modified "2018-01-24"^^xsd:date;
              a rdf:Property;
              rdfs:comment "A solid account belonging to an Agent."@en;
              rdfs:isDefinedBy solid:;
              rdfs:label "account"@en.
solid:deletes dc:issued "2017-08-17"^^xsd:date;
              a rdf:Property,
                owl:FunctionalProperty,
                owl:ObjectProperty;
              rdfs:comment "The triple patterns this patch removes from the document."@en;
              rdfs:domain solid:Patch;
              rdfs:isDefinedBy solid:;
              rdfs:label "deletes"@en;
              rdfs:range log:Formula.
solid:forClass dc:issued "2018-01-24"^^xsd:date;
               a rdf:Property;
               rdfs:comment "A class that is used to map an listed or unlisted type index."@en;
               rdfs:isDefinedBy solid:;
               rdfs:label "registry class"@en.
solid:inbox dc:issued "2015-11-16"^^xsd:date;
            dc:modified "2016-02-05"^^xsd:date,
                        "2018-10-25"^^xsd:date;
            a rdf:Property;
            rdfs:comment "Deprecated pointer to a Linked Data Notifications inbox; please use http://www.w3.org/ns/ldp#inbox instead."@en;
            rdfs:isDefinedBy solid:;
            rdfs:label "inbox (deprecated)"@en;
            rdfs:subPropertyOf ldp:inbox;
            owl:deprecated true;
            owl:equivalentProperty ldp:inbox.
solid:inserts dc:issued "2017-08-17"^^xsd:date;
              a rdf:Property,
                owl:FunctionalProperty,
                owl:ObjectProperty;
              rdfs:comment "The triple patterns this patch adds to the document."@en;
              rdfs:domain solid:Patch;
              rdfs:isDefinedBy solid:;
              rdfs:label "inserts"@en;
              rdfs:range log:Formula.
solid:instance dc:issued "2018-01-24"^^xsd:date;
               a rdf:Property;
               rdfs:comment "Maps a type to an individual resource, typically an index or a directory listing resource."@en;
               rdfs:isDefinedBy solid:;
               rdfs:label "instance"@en.
solid:instanceContainer dc:issued "2018-01-24"^^xsd:date;
                        a rdf:Property;
                        rdfs:comment "Maps a type to a container which the client would have to list to get the instances of that type."@en;
                        rdfs:isDefinedBy solid:;
                        rdfs:label "instance container"@en.
solid:loginEndpoint dc:issued "2015-11-16"^^xsd:date;
                    a rdf:Property;
                    rdfs:comment "The login URI of a given server."@en;
                    rdfs:isDefinedBy solid:;
                    rdfs:label "loginEndpoint"@en.
solid:logoutEndpoint dc:issued "2015-11-16"^^xsd:date;
                     a rdf:Property;
                     rdfs:comment "The logout URI of a given server."@en;
                     rdfs:isDefinedBy solid:;
                     rdfs:label "logoutEndpoint"@en.
solid:notification dc:issued "2016-03-11"^^xsd:date;
                   dc:modified "2018-10-25"^^xsd:date;
                   a rdf:Property;
                   rdfs:comment "Notification resource for an inbox."@en;
                   rdfs:isDefinedBy solid:;
                   rdfs:label "notification"@en.
solid:oidcIssuer dc:issued "2017-08-15"^^xsd:date;
                 dc:modified "2017-08-16"^^xsd:date;
                 a rdf:Property;
                 rdfs:comment "The preferred OpenID Connect issuer URI for a given WebID."@en;
                 rdfs:isDefinedBy solid:;
                 rdfs:label "OIDC issuer"@en;
                 rdfs:subPropertyOf <http://openid.net/specs/connect/1.0/issuer>.
solid:owner dc:issued "2021-05-19"^^xsd:date;
            a rdf:Property;
            rdfs:comment "A person or social entity that is considered to have control, rights, and responsibilities over a data storage."@en;
            rdfs:isDefinedBy solid:;
            rdfs:label "owner"@en;
            rdfs:range foaf:Agent.
solid:patches dc:issued "2017-08-17"^^xsd:date;
              a rdf:Property,
                owl:ObjectProperty;
              rdfs:comment "The document to which this patch applies."@en;
              rdfs:domain solid:Patch;
              rdfs:isDefinedBy solid:;
              rdfs:label "patches"@en;
              rdfs:range rdfs:Resource.
solid:privateLabelIndex dc:issued "2023-10-04"^^xsd:date;
                        a rdf:Property;
                        rdfs:comment "Points to an unlisted label index resource."@en;
                        rdfs:isDefinedBy solid:;
                        rdfs:label "private label index"@en;
                        rdfs:range solid:UnlistedDocument.
solid:privateTypeIndex dc:issued "2018-01-24"^^xsd:date;
                       a rdf:Property;
                       rdfs:comment "Points to an unlisted type index resource."@en;
                       rdfs:isDefinedBy solid:;
                       rdfs:label "private type index"@en;
                       rdfs:range solid:UnlistedDocument.
solid:publicTypeIndex dc:issued "2018-01-24"^^xsd:date;
                      a rdf:Property;
                      rdfs:comment "Points to a listed type index resource."@en;
                      rdfs:isDefinedBy solid:;
                      rdfs:label "public type index"@en;
                      rdfs:range solid:ListedDocument;
                      rdfs:subPropertyOf solid:typeIndex.
solid:read dc:issued "2015-12-18"^^xsd:date;
           a rdf:Property;
           rdfs:comment "Indicates if a message has been read or not. This property should have a boolean datatype."@en;
           rdfs:domain <http://rdfs.org/sioc/ns#Post>;
           rdfs:isDefinedBy solid:;
           rdfs:label "read"@en.
solid:storageDescription dc:issued "2024-12-28"^^xsd:date;
                         a rdf:Property,
                           owl:ObjectProperty;
                         rdfs:comment "Refers to the resource that provides a description of the storage containing this resource."@en;
                         rdfs:isDefinedBy solid:;
                         rdfs:label "storage description"@en;
                         rdfs:seeAlso <https://solidproject.org/TR/2024/protocol-20240512#server-storage-description>.
solid:storageQuota dc:issued "2018-10-26"^^xsd:date;
                   dc:modified "2018-11-07"^^xsd:date,
                               "2019-01-22"^^xsd:date;
                   a rdf:Property,
                     owl:DatatypeProperty;
                   rdfs:comment "The quota of non-volatile memory that is available for the account (in bytes)"@en;
                   rdfs:domain solid:Account;
                   rdfs:isDefinedBy solid:;
                   rdfs:label "Non-volatile memory quota"@en.
solid:storageUsage dc:issued "2019-01-22"^^xsd:date;
                   a rdf:Property,
                     owl:DatatypeProperty;
                   rdfs:comment "The amount of non-volatile memory that the account have used (in bytes)"@en;
                   rdfs:domain solid:Account;
                   rdfs:isDefinedBy solid:;
                   rdfs:label "Non-volatile memory usage"@en.
solid:timeline dc:issued "2016-01-04"^^xsd:date;
               a rdf:Property;
               rdfs:comment "Timeline for a given resource."@en;
               rdfs:isDefinedBy solid:;
               rdfs:label "timeline"@en.
solid:typeIndex dc:issued "2016-02-05"^^xsd:date;
                a rdf:Property;
                rdfs:comment "Points to a TypeIndex resource."@en;
                rdfs:isDefinedBy solid:;
                rdfs:label "type index"@en;
                rdfs:range solid:TypeIndex.
solid:where dc:issued "2017-08-17"^^xsd:date;
            a rdf:Property,
              owl:FunctionalProperty,
              owl:ObjectProperty;
            rdfs:comment "The conditions the document and the inserted and deleted triple patterns need to satisfy in order for the patch to be applied."@en;
            rdfs:domain solid:Patch;
            rdfs:isDefinedBy solid:;
            rdfs:label "where"@en;
            rdfs:range log:Formula.
