# this namespace

# baseURI: http://jazz.net/ns/aspice#
@prefix jazz_aspice: <http://jazz.net/ns/aspice#> .

# general namespaces
@prefix dcterms: <http://purl.org/dc/terms/> .
@prefix owl: <http://www.w3.org/2002/07/owl#> .
@prefix rdf: <http://www.w3.org/1999/02/22-rdf-syntax-ns#> .
@prefix rdfs: <http://www.w3.org/2000/01/rdf-schema#> .
@prefix xsd: <http://www.w3.org/2001/XMLSchema#> .

# OSLC namespaces
@prefix oslc_rm: <http://open-services.net/ns/rm#> .
@prefix oslc_cm: <http://open-services.net/ns/cm#> .
@prefix oslc_qm: <http://open-services.net/ns/qm#> .

# Jazz namespaces
@prefix jazz_ccm: <http://jazz.net/ns/ccm#> .
@prefix jazz_rm: <http://jazz.net/ns/rm#> .
@prefix jazz_rqm: <http://jazz.net/ns/qm/rqm#> .
@prefix jazz_esa: <http://jazz.net/ns/enterprise_agile#> .
@prefix jazz_sse: <http://jazz.net/ns/sse#> .
@prefix jazz_fusa: <http://jazz.net/ns/functional_safety#> .

# Other namespaces
@prefix skos: <http://www.w3.org/2004/02/skos/core#> .

# the ontology
jazz_aspice:
    a owl:Ontology ;
    dcterms:title "IBM ASPICE Compliance Vocabulary" ;
    dcterms:description "Vocabulary terms describing resources related to the automotive regulations specific to ASPICE." ;
    rdfs:label "ASPICE core" ;
    dcterms:source <https://jazz.net/wiki/pub/LinkedData/AspiceVocabulary/aspice-vocabulary.ttl> ;
    dcterms:license <https://jazz.net/ns/license.html> ;
    dcterms:dateCopyrighted "2020" ;
    .

## Note: In most of these definitions, "resource" connotes an RDF resource unless explicitly defined otherwise

### ---------------------------------------------------

#   RM Class definitions (types)

### ---------------------------------------------------
# jazz_sse defines: Actor, Free-Form Diagram, Heading, Information, Release Collection, Stakeholder Requirement, Stakeholder Requirements Module,
#      Hardware Requirement, Hardware Requirements Module, Software Requirement, Software Requirements Module, System Requirement, System Requirements Module,
#      Term, Use Case, Use Case Module, Vision

jazz_aspice:LegalAdministrativeDocument a rdfs:Class ;
    rdfs:comment "This artifact is used to specify relevant Legal and Administrative Document in a central Register (Module). It is derived from Automotive SPICE ACQ.12. Legal and Administrative Requirements." ;
    rdfs:isDefinedBy jazz_aspice: ;
    rdfs:label "Legal and Administrative Document" .

jazz_aspice:LegalAdministrativeRequirement a rdfs:Class ;
    rdfs:comment "This artifact is used for capturing a Legal or Administrative Requirement of a Regulatory. It is derived from Automotive SPICE ACQ.12. Legal and Administrative Requirements." ;
    rdfs:isDefinedBy jazz_aspice: ;
    rdfs:label "Legal and Administrative Requirement" .

jazz_aspice:Document a rdfs:Class ;
    rdfs:comment "This artifact is used for specific documents required for ASPICE compliance." ;
    rdfs:isDefinedBy jazz_aspice: ;
    rdfs:label "Document" .

jazz_aspice:Finding a rdfs:Class ;
    rdfs:comment "This artifact represents information discovered as a result of an investigation during a review, inspection, analysis, etc.." ;
    rdfs:isDefinedBy jazz_aspice: ;
    rdfs:label "Finding" .

jazz_aspice:FindingsModule a jazz_rm:Module ;
    rdfs:comment "A module containing Findings." ;
    rdfs:isDefinedBy jazz_aspice: ;
    rdfs:seeAlso jazz_aspice:Finding ;
    rdfs:label "Findings Module" .

# Added in 7.0.2
	
jazz_aspice:LegalAdministrativeModule a jazz_rm:Module ;
    rdfs:comment "A module containing Legal and Administrative Requirements. It is derived from Automotive SPICE ACQ.12. Legal and Administrative Requirements." ;
    rdfs:isDefinedBy jazz_aspice: ;
    rdfs:label "Legal and Administrative Module" .

jazz_aspice:LegalAdministrativeRegister a jazz_rm:Module ;
    rdfs:comment "A module containing a central registry that collates Legal and Administrative documents. It is derived from Automotive SPICE ACQ.12. Legal and Administrative Requirements." ;
    rdfs:isDefinedBy jazz_aspice: ;
    rdfs:label "Legal and Administrative Register" .


## ---------------
#  RM Link types
## ---------------
# jazz_esa defines illustrates
# jazz_sse defines: constrains, dependsOn, derivesFrom, impacts, integratesWith, mitigates, satisfies

#################################################
# -- State / status
#################################################

#  Status Values is oscl_cm:State and custom property values
#  oslc_cm:State defines oslc_cm:Closed, oslc_cm:Inprogress, oslc_cm:Fixed, oslc_cm:Approved, oslc_cm:Reviewed, and oslc_cm:Verified
#  jazz_sse and jazz_esa: Defines the general-purpose and SAFe-specific states to be reused here
#  Note: State property values can be reused across all domains, so this section includes CM states also

#oscl_cm:Inprogress States

jazz_aspice:StateVerifying a oslc_cm:State ;
    rdfs:comment "A Problem is in the process of being verified." ;
    rdfs:isDefinedBy jazz_aspice: ;
    skos:narrower oslc_cm:Inprogress ;
    rdfs:label "Verifying" .

# --------------------------------------

# RM Properties

# ---------------------------------------

# ----  RM enum definitions  ------
# ---------------------------------------

# -- Affected Domain type values
jazz_aspice:AffectedDomainTypes a rdfs:Class ;
    rdfs:comment "Defines the types of domains that could be affected by a requirement." ;
    rdfs:isDefinedBy jazz_aspice: ;
    rdfs:label "Affected Domain Types" .

jazz_aspice:AffectedDomainTypesSystem a jazz_aspice:AffectedDomainTypes ;
    rdfs:comment "Specifies a System domain." ;
    rdfs:isDefinedBy jazz_aspice: ;
    rdfs:label "System" .

jazz_aspice:AffectedDomainTypesSoftware a jazz_aspice:AffectedDomainTypes ;
    rdfs:comment "Specifies a Software domain." ;
    rdfs:isDefinedBy jazz_aspice: ;
    rdfs:label "Software" .

jazz_aspice:AffectedDomainTypesHardware a jazz_aspice:AffectedDomainTypes ;
    rdfs:comment "Specifies a Hardware domain." ;
    rdfs:isDefinedBy jazz_aspice: ;
    rdfs:label "Hardware" .

jazz_aspice:AffectedDomainTypesMechanical a jazz_aspice:AffectedDomainTypes ;
    rdfs:comment "Specifies a Mechanical domain." ;
    rdfs:isDefinedBy jazz_aspice: ;
    rdfs:label "Mechanical" .

# -- Approval type values
jazz_aspice:ApprovalTypes a rdfs:Class ;
    rdfs:comment "Defines the types of approvals for a requirement change review." ;
    rdfs:isDefinedBy jazz_aspice: ;
    rdfs:label "Approval Types" .

jazz_aspice:ApprovalTypeNotStarted a jazz_aspice:ApprovalTypes ;
    rdfs:comment "Specifies that a requirement change review has not been started." ;
    rdfs:isDefinedBy jazz_aspice: ;
    rdfs:label "Not Started" .

jazz_aspice:ApprovalTypeInAnalysisReview a jazz_aspice:ApprovalTypes ;
    rdfs:comment "Specifies that a change to a requirement is in analysis or review." ;
    rdfs:isDefinedBy jazz_aspice: ;
    rdfs:label "In Analysis/Review" .

jazz_aspice:ApprovalTypeApproved a jazz_aspice:ApprovalTypes ;
    rdfs:comment "Specifies that a change to requirement has been approved." ;
    rdfs:isDefinedBy jazz_aspice: ;
    rdfs:label "Approved" .

jazz_aspice:ApprovalTypeNotApproved a jazz_aspice:ApprovalTypes ;
    rdfs:comment "Specifies that a change to a rquirement has not been approved." ;
    rdfs:isDefinedBy jazz_aspice: ;
    rdfs:label "Not Approved" .

# -- Finding type values
jazz_aspice:FindingTypes a rdfs:Class ;
    rdfs:comment "Defines the types of for a Finding." ;
    rdfs:isDefinedBy jazz_aspice: ;
    rdfs:label "Finding Types" .

jazz_aspice:FindingTypesEditorial a jazz_aspice:FindingTypes ;
    rdfs:comment "Specifies that a Finding reflects an editorial comment." ;
    rdfs:isDefinedBy jazz_aspice: ;
    rdfs:label "Editorial" .

jazz_aspice:FindingTypesTechnical a jazz_aspice:FindingTypes ;
    rdfs:comment "Specifies that a Finding reflects an technical comment." ;
    rdfs:isDefinedBy jazz_aspice: ;
    rdfs:label "Technical" .

# -- Maturity type values
jazz_aspice:MaturityTypes a rdfs:Class ;
    rdfs:comment "Defines the levels of maturity an Automotive OEM would use to describe the desired state of requirement delivery." ;
    rdfs:isDefinedBy jazz_aspice: ;
    rdfs:label "Maturity Types" .

jazz_aspice:MaturityTypesConcept a jazz_aspice:MaturityTypes ;
    rdfs:comment "Specifies that requirement delivery is in the Concept state." ;
    rdfs:isDefinedBy jazz_aspice: ;
    rdfs:label "Concept" .

jazz_aspice:MaturityTypesPrototype a jazz_aspice:MaturityTypes ;
    rdfs:comment "Specifies that requirement delivery is in the Prototype state." ;
    rdfs:isDefinedBy jazz_aspice: ;
    rdfs:label "Prototype" .

jazz_aspice:MaturityTypesBetaTested a jazz_aspice:MaturityTypes ;
    rdfs:comment "Specifies that requirement delivery has been Beta-tested." ;
    rdfs:isDefinedBy jazz_aspice: ;
    rdfs:label "Beta-tested" .

jazz_aspice:MaturityTypesProductionReady a jazz_aspice:MaturityTypes ;
    rdfs:comment "Specifies that requirement delivery is Production-ready." ;
    rdfs:isDefinedBy jazz_aspice: ;
    rdfs:label "Production-ready" .

# -- Requirement type values
jazz_aspice:RequirementTypes a rdfs:Class ;
    rdfs:comment "Defines the types of requirement." ;
    rdfs:isDefinedBy jazz_aspice: ;
    rdfs:label "Requirement Types" .

jazz_aspice:RequirementTypeFunctional a jazz_aspice:RequirementTypes ;
    rdfs:comment "Specifies a requirement as a functional requirement." ;
    rdfs:isDefinedBy jazz_aspice: ;
    rdfs:label "Functional" .

jazz_aspice:RequirementTypeNonFunctional a jazz_aspice:RequirementTypes ;
    rdfs:comment "Specifies a requirement as a non-functional requirement." ;
    rdfs:isDefinedBy jazz_aspice: ;
    rdfs:label "Non-Functional" .

jazz_aspice:RequirementTypeSafety a jazz_aspice:RequirementTypes ;
    rdfs:comment "Specifies a requirement as a safety requirement." ;
    rdfs:isDefinedBy jazz_aspice: ;
    rdfs:label "Safety" .

# -- System Requirement Verification type enum values

jazz_aspice:SysReqVerificationLevels a rdfs:Class ;
    rdfs:comment "Defines the levels of verification specifically for System Requirements." ;
    rdfs:isDefinedBy jazz_aspice: ;
    rdfs:label "System Requirement Verification Levels" .

jazz_aspice:SysReqVerificationSystemIntegrationTest a jazz_aspice:SysReqVerificationLevels ;
    rdfs:comment "Indicates requirement will be verified during system integration test." ;
    rdfs:isDefinedBy jazz_aspice: ;
    rdfs:label "System Integration Test" .

jazz_aspice:SysReqVerificationSystemQualificationTest a jazz_aspice:SysReqVerificationLevels ;
    rdfs:comment "Indicates requirement will be verified during system qualification test." ;
    rdfs:isDefinedBy jazz_aspice: ;
    rdfs:label "System Qualification Test" .

# -- Verification level enum values

jazz_aspice:VerificationLevels a rdfs:Class ;
    rdfs:comment "Defines the levels of verification." ;
    rdfs:isDefinedBy jazz_aspice: ;
    rdfs:label "Verification Levels" .

jazz_aspice:VerificationUnitTest a jazz_aspice:VerificationLevels ;
    rdfs:comment "Indicates requirement will be verified during unit test." ;
    rdfs:isDefinedBy jazz_aspice: ;
    rdfs:label "Unit Test" .

jazz_aspice:VerificationIntegrationTest a jazz_aspice:VerificationLevels ;
    rdfs:comment "Indicates requirement will be verified during integration test." ;
    rdfs:isDefinedBy jazz_aspice: ;
    rdfs:label "Integration Test" .

jazz_aspice:VerificationQualificationTest a jazz_aspice:VerificationLevels ;
    rdfs:comment "Indicates requirement will be verified during qualification test." ;
    rdfs:isDefinedBy jazz_aspice: ;
    rdfs:label "Qualification Test" .

# -- Verification method enum values

jazz_aspice:VerifyByMethod a rdfs:Class ;
	rdfs:comment "Defines the methods that can be used for verification." ;
	rdfs:isDefinedBy jazz_aspice: ;
	rdfs:label "Verification Methods" .

jazz_aspice:VerifyByUnassigned a jazz_aspice:VerifyByMethod ;
    rdfs:comment "The verification method is unassigned." ;
    rdfs:isDefinedBy jazz_aspice: ;
    rdfs:label "Unassigned".
	
jazz_aspice:VerifyByAnalysis a jazz_aspice:VerifyByMethod ; 
	rdfs:comment "Indicates the verification method is by analysis." ;
	rdfs:isDefinedBy jazz_aspice: ;
	rdfs:label "Analysis" .

jazz_aspice:VerifyByAudit a jazz_aspice:VerifyByMethod ;
    rdfs:comment "Indicates the verification method is by audit." ;
    rdfs:isDefinedBy jazz_aspice: ;
    rdfs:label "Audit".
	
jazz_aspice:VerifyByComparison a jazz_aspice:VerifyByMethod ; 
	rdfs:comment "Indicates the verification method is by comparison." ;
	rdfs:isDefinedBy jazz_aspice: ;
	rdfs:label "Comparison" .	
	
jazz_aspice:VerifyByDemonstration a jazz_aspice:VerifyByMethod ; 
	rdfs:comment "Indicates the verification method is by demonstration." ;
	rdfs:isDefinedBy jazz_aspice: ;
	rdfs:label "Demonstration" .
	
jazz_aspice:VerifyByInspection a jazz_aspice:VerifyByMethod ; 
	rdfs:comment "Indicates the verification method is by inspection." ;
	rdfs:isDefinedBy jazz_aspice: ;
	rdfs:label "Inspection" .

jazz_aspice:VerifyByPeerReview a jazz_aspice:VerifyByMethod ;
    rdfs:comment "Indicates the verification method is by peer review." ;
    rdfs:isDefinedBy jazz_aspice: ;
    rdfs:label "Peer Review".
	
jazz_aspice:VerifyByTest a jazz_aspice:VerifyByMethod ; 
	rdfs:comment "Indicates the verification method is by test." ;
	rdfs:isDefinedBy jazz_aspice: ;
	rdfs:label "Test" .

jazz_aspice:VerifyByWalkthrough a jazz_aspice:VerifyByMethod ;
    rdfs:comment "Indicates the verification method is by walkthrough." ;
    rdfs:isDefinedBy jazz_aspice: ;
    rdfs:label "Walkthrough".
	

# -- requirement levels enum values
# Added in 7.0.2

jazz_aspice:RequirementLevels a rdfs:Class ;
    rdfs:comment "Defines levels of system requirements." ;
    rdfs:isDefinedBy jazz_aspice: ;
    rdfs:label "Requirement Levels" .

jazz_aspice:RequirementLevelFunctional a jazz_aspice:RequirementLevels ;
    rdfs:comment "Functional requirements level." ;
    rdfs:isDefinedBy jazz_aspice: ;
    rdfs:label "Functional" .

jazz_aspice:RequirementLevelTechnical a jazz_aspice:RequirementLevels ;
    rdfs:comment "Technical requirements level." ;
    rdfs:isDefinedBy jazz_aspice: ;
    rdfs:label "Technical" .


## ----   State values ---------

#  oslc_cm:State defines oslc_cm:Closed, oslc_cm:Inprogress, oslc_cm:Fixed, oslc_cm:Approved, oslc_cm:Reviewed, and oslc_cm:Verified
#  jazz_sse defines Draft, Under Review, Approved, Rejected, Deprecated
#  Note: State property values can be reused across all domains


#oscl_cm:Inprogress States

jazz_aspice:StateReadyForReview a oslc_cm:State ;
    rdfs:comment "The artifact is ready for a review." ;
    rdfs:isDefinedBy jazz_aspice: ;
    skos:narrower oslc_cm:Inprogress ;
    rdfs:label "Ready for Review" .

jazz_aspice:StateScheduled a oslc_cm:State ;
    rdfs:comment "The artifact is scheduled." ;
    rdfs:isDefinedBy jazz_aspice: ;
    skos:narrower oslc_cm:Inprogress ;
    rdfs:label "Scheduled" .

#oscl_cm:Closed States

jazz_aspice:StateCanceled a oslc_cm:State ;
    rdfs:comment "The artifact has been canceled." ;
    rdfs:isDefinedBy jazz_aspice: ;
    skos:narrower oslc_cm:Closed ;
    rdfs:label "Canceled" .

# ---------------------------------
#  RM non-enum artifact properties
# ---------------------------------

jazz_aspice:affectedDomain a rdf:Property;
    rdfs:comment "Used to specify the domain level of the requirement." ;
    rdfs:isDefinedBy jazz_aspice: ;
    rdfs:label "Affected Domain" ;
    rdfs:seeAlso jazz_aspice:AffectedDomainTypes .

jazz_aspice:docVersion  a rdf:Property ;
    rdfs:comment "The version of a document.";
    rdfs:isDefinedBy jazz_aspice: ;
    rdfs:label "Document Version" .

jazz_aspice:findingType a rdf:Property;
    rdfs:comment "Specifies the nature of a finding." ;
    rdfs:isDefinedBy jazz_aspice: ;
    rdfs:label "Finding Type" ;
    rdfs:seeAlso jazz_aspice:FindingTypes .

jazz_aspice:legalEntity a rdf:Property;
    rdfs:comment "Derived from ACQ.12. Legal and Administrative Requirements. Describes the Legal Entity releasing a Legal and Administrative Requirement e.g. ISO." ;
    rdfs:isDefinedBy jazz_aspice: ;
    rdfs:label "Legal Entity" .

jazz_aspice:maturity a rdf:Property;
    rdfs:comment "Used by Automotive OEMs to indicate the level of maturity of requirement delivery." ;
    rdfs:isDefinedBy jazz_aspice: ;
    rdfs:label "Maturity" ;
    rdfs:seeAlso jazz_aspice:MaturityTypes .

jazz_aspice:need a rdf:Property;
    rdfs:comment "Indicates the degree of need for this requirement." ;
    rdfs:isDefinedBy jazz_aspice: ;
    rdfs:label "Need" ;
    rdfs:seeAlso jazz_aspice:NeedValues .

jazz_aspice:offlineComments a rdf:Property;
    rdfs:comment "Comments submitted offline." ;
    rdfs:isDefinedBy jazz_aspice: ;
    rdfs:label "Offline Comments" .

jazz_aspice:paragraph a rdf:Property;
    rdfs:comment "Derived from Automotive SPICE ACQ.12. Legal and Administrative Requirements. Needed to specify the Paragraph in a Legal and Administrative Requirement." ;
    rdfs:isDefinedBy jazz_aspice: ;
    rdfs:label "Paragraph" .

jazz_aspice:requirementType  a rdf:Property;
    rdfs:comment "The type of requirement." ;
    rdfs:isDefinedBy jazz_aspice: ;
    rdfs:label "Requirement Type" ;
    rdfs:seeAlso jazz_aspice:RequirementTypes .

jazz_aspice:reviewer a rdf:Property;
    rdfs:comment "The user reviewing a case and presenting a finding." ;
    rdfs:isDefinedBy jazz_aspice: ;
    rdfs:label "Reviewer" .

jazz_aspice:systemReqVerificationLevel a rdf:Property ;
    rdfs:comment "Level of testing at which the system requirement should be verified. Can be expressed as a value of type jazz_aspice:VerificationLevel." ;
    rdfs:isDefinedBy jazz_aspice: ;
    rdfs:seeAlso jazz_aspice:VerificationLevels ;
    rdfs:label "System Req Verification Level" .

jazz_aspice:verificationLevel  a rdf:Property;
    rdfs:comment "Level of testing at which the requirement should be verified. Can be expressed as a value of type jazz_aspice:VerificationLevel." ;
    rdfs:isDefinedBy jazz_aspice: ;
    rdfs:seeAlso jazz_aspice:VerificationLevels ;
    rdfs:label "Verification Level" .

jazz_aspice:verificationMethod  a rdf:Property; 
	rdfs:comment "Method to be used to verify the artifact. Can be expressed as a value of type jazz_aspice:VerifyByMethod." ;
	rdfs:isDefinedBy jazz_aspice: ;
	rdfs:seeAlso jazz_aspice:VerifyByMethod ;
	rdfs:label "Verification Method" .	

# Added in 7.0.2
	
jazz_aspice:requirementLevel a rdf:Property;
    rdfs:comment "This value defines the level of abstraction of the system requirement. Expressed of type jazz_aspice:RequirementLevels.";
    rdfs:isDefinedBy jazz_aspice:;
    rdfs:seeAlso jazz_aspice:RequirementLevels ;
    rdfs:label "Requirement Level".

## -----------------------------------
#   CM Classes
## ------------------------------------
#  oslc_cm:ChangeNotice, oslc_cm:ChangeRequest, oslc_cm:Defect, oslc_cm:Enhancement, oslc_cm:ReviewTask, oslc_cm:Task;
#  oslc_cm:Priority, oslc_cm:Severity property values defined along with oslc_cm:priority, oslc_cm:severity attributes
#  jazz_ccm:Complexity, jazz_ccm:Impact property values, but Impact is not the same as Risk Impact
#  jazz_sse:RiskImpact, jazz_sse:RiskProbability, jazz_sse:RiskCategory property values
#  jazz_sse:complexity, jazz_sse:impact, jazz_sse:probability, jazz_sse:riskCategory attributes

# ---------------------
#  CM enum definitions
# ----------------------

# -  Risk Area values

jazz_aspice:RiskArea a rdfs:Class ;
    rdfs:comment "Defines the aspect of delivery to which the Risk applies." ;
    rdfs:isDefinedBy jazz_aspice: ;
    rdfs:label "Risk Area".

jazz_aspice:RiskAreaUnassigned a jazz_aspice:RiskArea ;
    rdfs:comment "The Risk area is unassigned." ;
    rdfs:isDefinedBy jazz_aspice: ;
    rdfs:label "Unassigned".

jazz_aspice:RiskAreaTechnical a jazz_aspice:RiskArea ;
    rdfs:comment "The Risk relates to a technical issue." ;
    rdfs:isDefinedBy jazz_aspice: ;
    rdfs:label "Technical".

jazz_aspice:RiskAreaCost a jazz_aspice:RiskArea ;
    rdfs:comment "The Risk relates to a cost issue." ;
    rdfs:isDefinedBy jazz_aspice: ;
    rdfs:label "Cost".

jazz_aspice:RiskAreaTiming a jazz_aspice:RiskArea ;
    rdfs:comment "The Risk relates to a timing or schedule issue." ;
    rdfs:isDefinedBy jazz_aspice: ;
    rdfs:label "Timing".

jazz_aspice:RiskAreaResource a jazz_aspice:RiskArea ;
    rdfs:comment "The Risk relates to a resource issue." ;
    rdfs:isDefinedBy jazz_aspice: ;
    rdfs:label "Resource".

jazz_aspice:RiskAreaEffort a jazz_aspice:RiskArea ;
    rdfs:comment "The Risk relates to an issue with effort, such as estimated effort is too low or there is no capacity." ;
    rdfs:isDefinedBy jazz_aspice: ;
    rdfs:label "Effort".

jazz_aspice:RiskAreaCompliance a jazz_aspice:RiskArea ;
    rdfs:comment "The Risk relates to an internal or external compliance issue." ;
    rdfs:isDefinedBy jazz_aspice: ;
    rdfs:label "Compliance".

# -  Risk Type values

jazz_aspice:RiskType a rdfs:Class ;
    rdfs:comment "Defines the type of Risk." ;
    rdfs:isDefinedBy jazz_aspice: ;
    rdfs:label "Risk Type".

jazz_aspice:RiskTypeUnassigned a jazz_aspice:RiskType ;
    rdfs:comment "The Risk type is unassigned." ;
    rdfs:isDefinedBy jazz_aspice: ;
    rdfs:label "Unassigned".

jazz_aspice:RiskTypeManagement a jazz_aspice:RiskType ;
    rdfs:comment "The Risk type is related to management." ;
    rdfs:isDefinedBy jazz_aspice: ;
    rdfs:label "Management".

jazz_aspice:RiskTypeFMEA a jazz_aspice:RiskType ;
    rdfs:comment "The Risk type is related to FMEA." ;
    rdfs:isDefinedBy jazz_aspice: ;
    rdfs:label "FMEA".

jazz_aspice:RiskTypeFunctional a jazz_aspice:RiskType ;
    rdfs:comment "The Risk type is related to functional analysis." ;
    rdfs:isDefinedBy jazz_aspice: ;
    rdfs:label "Functional Analysis".

jazz_aspice:RiskTypeSimulation a jazz_aspice:RiskType ;
    rdfs:comment "The Risk type is relatd to simulation." ;
    rdfs:isDefinedBy jazz_aspice: ;
    rdfs:label "Simulation".

# -- Problem "how found" values --

jazz_aspice:ProblemHowFoundValue a rdfs:Class ;
    rdfs:comment "Describes whether a problem was found internally or externally." ;
    rdfs:isDefinedBy jazz_aspice: ;
    rdfs:label "How Found" .

jazz_aspice:ProblemHowFoundInternal a jazz_aspice:ProblemHowFoundValue ;
    rdfs:comment "Indicates a problem was found internally." ;
    rdfs:isDefinedBy jazz_aspice: ;
    rdfs:label "Internal" .

jazz_aspice:ProblemHowFoundExternal a jazz_aspice:ProblemHowFoundValue ;
    rdfs:comment "Indicates a problem was found externally." ;
    rdfs:isDefinedBy jazz_aspice: ;
    rdfs:label "External" .

# -- Process Group values --

jazz_aspice:ProcessGroups a rdfs:Class ;
    rdfs:comment "Defines the ASPICE process groups to which work can be associated." ;
    rdfs:isDefinedBy jazz_aspice: ;
    rdfs:label "Process Groups" .

jazz_aspice:ProcessSYS1 a jazz_aspice:ProcessGroups ;
    rdfs:comment "The work is associated with requirements elicitation." ;
    rdfs:isDefinedBy jazz_aspice: ;
    rdfs:label "SYS.1 Requirements Elicitation" .

jazz_aspice:ProcessSYS2 a jazz_aspice:ProcessGroups ;
    rdfs:comment "The work is associated with requirements analysis." ;
    rdfs:isDefinedBy jazz_aspice: ;
    rdfs:label "SYS.2 System Requirements Analysis" .

jazz_aspice:ProcessSYS3 a jazz_aspice:ProcessGroups ;
    rdfs:comment "The work is associated with system architectural design." ;
    rdfs:isDefinedBy jazz_aspice: ;
    rdfs:label "SYS.3 System Architectural Design" .

jazz_aspice:ProcessSYS4 a jazz_aspice:ProcessGroups ;
    rdfs:comment "The work is associated with system integration and integration test." ;
    rdfs:isDefinedBy jazz_aspice: ;
    rdfs:label "SYS.4 System Integration and Integration Test" .

jazz_aspice:ProcessSYS5 a jazz_aspice:ProcessGroups ;
    rdfs:comment "The work is associated with system qualification test." ;
    rdfs:isDefinedBy jazz_aspice: ;
    rdfs:label "SYS.5 System Qualification Test" .

jazz_aspice:ProcessSWE1 a jazz_aspice:ProcessGroups ;
    rdfs:comment "The work is associated with software requirements analysis." ;
    rdfs:isDefinedBy jazz_aspice: ;
    rdfs:label "SWE.1 Software Requirements Analysis" .

jazz_aspice:ProcessSWE2 a jazz_aspice:ProcessGroups ;
    rdfs:comment "The work is associated with software architectural design." ;
    rdfs:isDefinedBy jazz_aspice: ;
    rdfs:label "SWE.2 Software Architectural Design" .

jazz_aspice:ProcessSWE3 a jazz_aspice:ProcessGroups ;
    rdfs:comment "The work is associated with software detailed design and unit construction." ;
    rdfs:isDefinedBy jazz_aspice: ;
    rdfs:label "SWE.3 Software Detailed Design and Unit Construction" .

jazz_aspice:ProcessSWE4 a jazz_aspice:ProcessGroups ;
    rdfs:comment "The work is associated with software unit verification." ;
    rdfs:isDefinedBy jazz_aspice: ;
    rdfs:label "SWE.4 Software Unit Verification" .

jazz_aspice:ProcessSWE5 a jazz_aspice:ProcessGroups ;
    rdfs:comment "The work is associated with software integration and integration test." ;
    rdfs:isDefinedBy jazz_aspice: ;
    rdfs:label "SWE.5 Software Integration and Integration Test" .

jazz_aspice:ProcessSWE6 a jazz_aspice:ProcessGroups ;
    rdfs:comment "The work is associated with software qualification test." ;
    rdfs:isDefinedBy jazz_aspice: ;
    rdfs:label "SWE.6 Software Qualification Test" .

jazz_aspice:ProcessSUP10 a jazz_aspice:ProcessGroups ;
    rdfs:comment "The work is associated with change request management." ;
    rdfs:isDefinedBy jazz_aspice: ;
    rdfs:label "SUP.10 Change Request Management" .

jazz_aspice:ProcessSUP1 a jazz_aspice:ProcessGroups ;
    rdfs:comment "The work is associated with quality assurance." ;
    rdfs:isDefinedBy jazz_aspice: ;
    rdfs:label "SUP.1 Quality Assurance" .

jazz_aspice:ProcessSUP8 a jazz_aspice:ProcessGroups ;
    rdfs:comment "The work is associated with configuration management." ;
    rdfs:isDefinedBy jazz_aspice: ;
    rdfs:label "SUP.8 Configuration Management" .

jazz_aspice:ProcessSUP9 a jazz_aspice:ProcessGroups ;
    rdfs:comment "The work is associated with problem resolution management." ;
    rdfs:isDefinedBy jazz_aspice: ;
    rdfs:label "SUP.9 Problem Resolution Management" .

jazz_aspice:ProcessMAN3 a jazz_aspice:ProcessGroups ;
    rdfs:comment "The work is associated with project management." ;
    rdfs:isDefinedBy jazz_aspice: ;
    rdfs:label "MAN.3 Project Management" .

jazz_aspice:ProcessACQ4 a jazz_aspice:ProcessGroups ;
    rdfs:comment "The work is associated with supplier monitoring." ;
    rdfs:isDefinedBy jazz_aspice: ;
    rdfs:label "ACQ.4 Supplier Monitoring" .

jazz_aspice:ProcessNone a jazz_aspice:ProcessGroups ;
    rdfs:comment "The work is not associated with any ASPICE-specific process group." ;
    rdfs:isDefinedBy jazz_aspice: ;
    rdfs:label "No ASPICE Process" .

# -- Event type values

jazz_aspice:EventTypes a rdfs:Class ;
    rdfs:comment "Designates the values that define the type of an Event." ;
    rdfs:isDefinedBy jazz_aspice: ;
    rdfs:label "Event Types" .

jazz_aspice:EventMeeting a jazz_aspice:EventTypes ;
    rdfs:comment "The Event is a meeting." ;
    rdfs:isDefinedBy jazz_aspice: ;
    rdfs:label "Meeting" .

jazz_aspice:EventPlanning a jazz_aspice:EventTypes ;
    rdfs:comment "The Event is a for planning." ;
    rdfs:isDefinedBy jazz_aspice: ;
    rdfs:label "Planning Event" .

jazz_aspice:EventMilestone a jazz_aspice:EventTypes ;
    rdfs:comment "The Event is a milestone." ;
    rdfs:isDefinedBy jazz_aspice: ;
    rdfs:label "Milestone" .

jazz_aspice:EventRetrospective a jazz_aspice:EventTypes ;
    rdfs:comment "The Event is a retrospective." ;
    rdfs:isDefinedBy jazz_aspice: ;
    rdfs:label "Retrospective" .

# -- Problem category values
# The difference between Defect and Issue is that Defect comes directly out of testing, whereas Issue has more of a general-purpose source.

jazz_aspice:ProblemCategories a rdfs:Class ;
    rdfs:comment "Designates the values for category of a Problem." ;
    rdfs:isDefinedBy jazz_aspice: ;
    rdfs:label "Problem Categories" .

jazz_aspice:CategoryDefect a jazz_aspice:ProblemCategories ;
    rdfs:comment "The Problem category is a defect." ;
    rdfs:isDefinedBy jazz_aspice: ;
    rdfs:label "Defect" .

jazz_aspice:CategoryIssue a jazz_aspice:ProblemCategories ;
    rdfs:comment "The Problem category is an issue." ;
    rdfs:isDefinedBy jazz_aspice: ;
    rdfs:label "Issue" .

# -------------------------------
#  CM attributes
# -----------------------------------

# -- Change Request

jazz_aspice:hardwareImpactAnalysis a rdf:Property ;
    rdfs:comment "Describes the analysis of hardware impact as a result of the change reuqest.";
    rdfs:isDefinedBy jazz_aspice: ;
    rdfs:label "Hardware Impact Analysis" .

jazz_aspice:howFound a rdf:Property ;
    rdfs:comment "Describes whether the change request or problem is from an internal or external source. Typically expressed as a value of type jazz_aspice:HowFoundValue.";
    rdfs:isDefinedBy jazz_aspice: ;
        rdfs:seeAlso jazz_aspice:HowFoundValue ;
    rdfs:label "How Found" .

jazz_aspice:manufacturingImpactAnalysis a rdf:Property ;
    rdfs:comment "Describes the analysis of manufacturing impact as a result of the change request.";
    rdfs:isDefinedBy jazz_aspice: ;
    rdfs:label "Manufacturing Impact Analysis" .

jazz_aspice:mechanicalImpactAnalysis a rdf:Property ;
    rdfs:comment "Describes the analysis of mechanical impact as a result of the change request.";
    rdfs:isDefinedBy jazz_aspice: ;
    rdfs:label "Mechanical Impact Analysis" .

jazz_aspice:qualityImpactAnalysis a rdf:Property ;
    rdfs:comment "Describes the analysis of quality impact as a result of the change request.";
    rdfs:isDefinedBy jazz_aspice: ;
    rdfs:label "Quality Impact Analysis" .

jazz_aspice:scheduleImpactAnalysis a rdf:Property ;
    rdfs:comment "Describes the analysis of schedule impact as a result of the change request.";
    rdfs:isDefinedBy jazz_aspice: ;
    rdfs:label "Schedule Impact Analysis" .

jazz_aspice:softwareImpactAnalysis a rdf:Property ;
    rdfs:comment "Describes the analysis of software impact as a result of the change request.";
    rdfs:isDefinedBy jazz_aspice: ;
    rdfs:label "Software Impact Analysis" .

jazz_aspice:systemImpactAnalysis a rdf:Property ;
    rdfs:comment "Describes the analysis of system impact as a result of the change request.";
    rdfs:isDefinedBy jazz_aspice: ;
    rdfs:label "System Impact Analysis" .

# --- Problem

jazz_aspice:detectedDuring a rdf:Property ;
    rdfs:comment "The problem was detected during the phase of the lifecycle described by a Process Group. Typically expressed as a value of type jazz_aspice:ProcessGroups.";
    rdfs:isDefinedBy jazz_aspice: ;
    rdfs:seeAlso jazz_aspice:ProcessGroups ;
    rdfs:label "Detected During" .

jazz_aspice:introducedIn a rdf:Property ;
    rdfs:comment "The problem was introduced during the phase of the lifecycle described by a Process Group. Typically expressed as a value of type jazz_aspice:ProcessGroups.";
    rdfs:isDefinedBy jazz_aspice: ;
    rdfs:seeAlso jazz_aspice:ProcessGroups ;
    rdfs:label "Introduced In" .

jazz_aspice:lessonsLearned a rdf:Property ;
    rdfs:comment "Indicates whether or not the Problem leads to lessons learned documentation.";
    rdfs:isDefinedBy jazz_aspice: ;
    rdfs:label "Lessons Learned" .

jazz_aspice:partyHighImpact a rdf:Property ;
    rdfs:comment "Indicates whether or not the Problem has an impact on another party.";
    rdfs:isDefinedBy jazz_aspice: ;
    rdfs:label "High Impact on Other Party" .

jazz_aspice:systemHighImpact a rdf:Property ;
    rdfs:comment "Indicates whether or not the Problem has an impact on another system.";
    rdfs:isDefinedBy jazz_aspice: ;
    rdfs:label "High Impact on Other System" .

jazz_aspice:problemCategory a rdf:Property ;
    rdfs:comment "Specifies the category of the problem. Typically expressed as a value of type jazz_aspice:ProblemCategories.";
    rdfs:isDefinedBy jazz_aspice: ;
    rdfs:seeAlso jazz_aspice:ProblemCategories ;
    rdfs:label "Problem Category" .

jazz_aspice:problemDescription a rdf:Property ;
    rdfs:comment "Description of the problem.";
    rdfs:isDefinedBy jazz_aspice: ;
    rdfs:label "Problem Description" .

# --- Review

jazz_aspice:improvementSuggestions a rdf:Property ;
    rdfs:comment "Suggestions for improvements in the reviewed artifacts or system." ;
    rdfs:isDefinedBy jazz_aspice: ;
    rdfs:label "Improvement Suggestions" .

jazz_aspice:mandatoryReviewers a rdf:Property ;
    rdfs:comment "Identifies the mandatory reviewers." ;
    rdfs:isDefinedBy jazz_aspice: ;
    rdfs:label "Mandatory Reviewers" .

jazz_aspice:nonConformities a rdf:Property ;
    rdfs:comment "Identifies any non-conformities as a result of the review." ;
    rdfs:isDefinedBy jazz_aspice: ;
    rdfs:label "Non-Conformities" .

jazz_aspice:optionalReviewers a rdf:Property ;
    rdfs:comment "Identifies the optional reviewers." ;
    rdfs:isDefinedBy jazz_aspice: ;
    rdfs:label "Optional Reviewers" .

jazz_aspice:processGroup a rdf:Property ;
    rdfs:comment "Specifies the process group associated with the review. Typically expressed as a value of type jazz_aspice:ProcessGroups.";
    rdfs:isDefinedBy jazz_aspice: ;
    rdfs:seeAlso jazz_aspice:ProcessGroups ;
    rdfs:label "Process Group" .

jazz_aspice:reviewFindings a rdf:Property ;
    rdfs:comment "Identifies any findings as a result of the review." ;
    rdfs:isDefinedBy jazz_aspice: ;
    rdfs:label "Review Findings" .

jazz_aspice:verificationCriteria a rdf:Property ;
    rdfs:comment "Identifies the critieria used for the review." ;
    rdfs:isDefinedBy jazz_aspice: ;
    rdfs:label "Verification Criteria" .

# -- Risk

jazz_aspice:riskArea a rdf:Property ;
    rdfs:comment "Aspect of delivery to which the Risk applies. Typically expressed as a value of type jazz_aspice:RiskArea." ;
    rdfs:isDefinedBy jazz_aspice: ;
    rdfs:seeAlso jazz_aspice:RiskArea ;
    rdfs:label "Risk Area" .

jazz_aspice:riskConsequence a rdf:Property ;
    rdfs:comment "Consequences associated with the risk." ;
    rdfs:isDefinedBy jazz_aspice: ;
    rdfs:label "Risk Consequence" .

jazz_aspice:riskType a rdf:Property ;
    rdfs:comment "Identifies the type of Risk. Typically expressed as a value of type jazz_aspice:RiskType." ;
    rdfs:isDefinedBy jazz_aspice: ;
    rdfs:seeAlso jazz_aspice:RiskType ;
    rdfs:label "Risk Type" .

# -- Event attributes

jazz_aspice:eventType a rdf:Property ;
    rdfs:comment "The type of event. Typically expressed as a value of type jazz_aspice:EventTypes." ;
    rdfs:isDefinedBy jazz_aspice: ;
    rdfs:seeAlso jazz_aspice:EventTypes ;
    rdfs:label "Event Type" .

jazz_aspice:externalParticipants a rdf:Property ;
    rdfs:comment "Identifies the external participants for an Event." ;
    rdfs:isDefinedBy jazz_aspice: ;
    rdfs:label "External Participants" .

jazz_aspice:internalParticipants a rdf:Property ;
    rdfs:comment "Identifies the interna participants for an Event." ;
    rdfs:isDefinedBy jazz_aspice: ;
    rdfs:label "Internal Participants" .

## -----------------------------------------------
#     QM Properties
## -----------------------------------------------

# Artifact Categories

# -- Test Phase (used in Test Plan, Test Case, Test Script and Test Suite Categories) 

jazz_aspice:testCategoryTestPhase a rdf:Property ;
    rdfs:comment "Category indicating the phase of testing in the ASPICE process to which the test artifact applies." ;
    rdfs:isDefinedBy jazz_aspice: ;
    rdfs:label "Test Level" .

jazz_aspice:testPhaseSystemQualification a rdf:Property ;
    rdfs:comment "Category indicating the test artifact is associated with the ASPICE System Qualification Test phase." ;
    rdfs:isDefinedBy jazz_aspice: ;
    rdfs:label "System Qualification Test" .

jazz_aspice:testPhaseSystemIntegration a rdf:Property ;
    rdfs:comment "Category indicating the test artifact is associated with the ASPICE System Integration and Integration Test phase." ;
    rdfs:isDefinedBy jazz_aspice: ;
    rdfs:label "System Integration and Integration Test" .

jazz_aspice:testPhaseSoftwareQualification a rdf:Property ;
    rdfs:comment "Category indicating the test artifact is associated with the ASPICE Software Qualification Test phase." ;
    rdfs:isDefinedBy jazz_aspice: ;
    rdfs:label "Software Qualification Test" .

jazz_aspice:testPhaseSoftwareIntegration a rdf:Property ;
    rdfs:comment "Category indicating the test artifact is associated with the ASPICE Software Integration and Integration Test phase." ;
    rdfs:isDefinedBy jazz_aspice: ;
    rdfs:label "Software Integration and Integration Test" .

jazz_aspice:testPhaseUnitTest a rdf:Property ;
    rdfs:comment "Category indicating the test artifact is associated with the ASPICE Software Integration and Integration Test phase." ;
    rdfs:isDefinedBy jazz_aspice: ;
    rdfs:label "Unit Test" .

jazz_aspice:testPhaseUAT a rdf:Property ;
    rdfs:comment "Category indicating the test artifact is associated with the ASPICE Software Integration and Integration Test phase." ;
    rdfs:isDefinedBy jazz_aspice: ;
    rdfs:label "User Acceptance Test" .
	
# Added in 7.0.2
jazz_aspice:testPhaseSafetyValidation a rdf:Property ;
    rdfs:comment "Category indicating the test artifact is associated with the ASPICE Software Integration and Integration Test phase." ;
    rdfs:isDefinedBy jazz_aspice: ;
    rdfs:label "Safety Validation Test" .


# -- Test Case Categories

jazz_aspice:testCaseCategoryRequiredForRegression a rdf:Property ;
    rdfs:comment "Category indicating whether a Test Case is required for regression testing." ;
    rdfs:isDefinedBy jazz_aspice: ;
    rdfs:label "Required for Regression" .

jazz_aspice:requiredForRegression a rdf:Property ;
    rdfs:comment "Indicates the Test Case is required for regression testing." ;
    rdfs:isDefinedBy jazz_aspice: ;
    rdfs:label "Required" .

jazz_aspice:notRequiredForRegression a rdf:Property ;
    rdfs:comment "Indicates the Test Case is not required for regression testing." ;
    rdfs:isDefinedBy jazz_aspice: ;
    rdfs:label "Not Required" .

# -- Test Script Categories

jazz_aspice:testScriptCategoryAutomationStatus a rdf:Property ;
    rdfs:comment "Category indicating whether a Test Script is automated, manual, or to be automated." ;
    rdfs:isDefinedBy jazz_aspice: ;
    rdfs:label "Automation" .

jazz_aspice:statusAutomated a rdf:Property ;
    rdfs:comment "Indicates the Test Script is automated." ;
    rdfs:isDefinedBy jazz_aspice: ; 
    rdfs:label "Automated" .

jazz_aspice:statusNotAutomated a rdf:Property ;
    rdfs:comment "Indicates the Test Script is not automated." ;
    rdfs:isDefinedBy jazz_aspice: ;
    rdfs:label "Not Automated" .

jazz_aspice:statusAutomationPlanned a rdf:Property ;
    rdfs:comment "Indicates the Test Script is in the process of or planned to be automated." ;
    rdfs:isDefinedBy jazz_aspice: ;
    rdfs:label "Automation Planned" .