@prefix rdf: <http://www.w3.org/1999/02/22-rdf-syntax-ns#>.
@prefix rdfs: <http://www.w3.org/2000/01/rdf-schema#>.
@prefix xsd: <http://www.w3.org/2001/XMLSchema#>.
@prefix jazz_aspice: <http://jazz.net/ns/aspice#>.
@prefix dcterms: <http://purl.org/dc/terms/>.
@prefix owl: <http://www.w3.org/2002/07/owl#>.
@prefix oslc_rm: <http://open-services.net/ns/rm#>.
@prefix oslc_cm: <http://open-services.net/ns/cm#>.
@prefix oslc_qm: <http://open-services.net/ns/qm#>.
@prefix jazz_ccm: <http://jazz.net/ns/ccm#>.
@prefix jazz_rm: <http://jazz.net/ns/rm#>.
@prefix jazz_rqm: <http://jazz.net/ns/qm/rqm#>.
@prefix jazz_esa: <http://jazz.net/ns/enterprise_agile#>.
@prefix jazz_sse: <http://jazz.net/ns/sse#>.
@prefix jazz_fusa: <http://jazz.net/ns/functional_safety#>.
@prefix skos: <http://www.w3.org/2004/02/skos/core#>.

{
    jazz_aspice: dcterms:dateCopyrighted "2020";
                 dcterms:description "Vocabulary terms describing resources related to the automotive regulations specific to ASPICE.";
                 dcterms:license <https://jazz.net/ns/license.html>;
                 dcterms:source <https://jazz.net/wiki/pub/LinkedData/AspiceVocabulary/aspice-vocabulary.ttl>;
                 dcterms:title "IBM ASPICE Compliance Vocabulary";
                 a owl:Ontology;
                 rdfs:label "ASPICE core".
    jazz_aspice:AffectedDomainTypes a rdfs:Class;
                                    rdfs:comment "Defines the types of domains that could be affected by a requirement.";
                                    rdfs:isDefinedBy jazz_aspice:;
                                    rdfs:label "Affected Domain Types".
    jazz_aspice:AffectedDomainTypesHardware a jazz_aspice:AffectedDomainTypes;
                                            rdfs:comment "Specifies a Hardware domain.";
                                            rdfs:isDefinedBy jazz_aspice:;
                                            rdfs:label "Hardware".
    jazz_aspice:AffectedDomainTypesMechanical a jazz_aspice:AffectedDomainTypes;
                                              rdfs:comment "Specifies a Mechanical domain.";
                                              rdfs:isDefinedBy jazz_aspice:;
                                              rdfs:label "Mechanical".
    jazz_aspice:AffectedDomainTypesSoftware a jazz_aspice:AffectedDomainTypes;
                                            rdfs:comment "Specifies a Software domain.";
                                            rdfs:isDefinedBy jazz_aspice:;
                                            rdfs:label "Software".
    jazz_aspice:AffectedDomainTypesSystem a jazz_aspice:AffectedDomainTypes;
                                          rdfs:comment "Specifies a System domain.";
                                          rdfs:isDefinedBy jazz_aspice:;
                                          rdfs:label "System".
    jazz_aspice:ApprovalTypeApproved a jazz_aspice:ApprovalTypes;
                                     rdfs:comment "Specifies that a change to requirement has been approved.";
                                     rdfs:isDefinedBy jazz_aspice:;
                                     rdfs:label "Approved".
    jazz_aspice:ApprovalTypeInAnalysisReview a jazz_aspice:ApprovalTypes;
                                             rdfs:comment "Specifies that a change to a requirement is in analysis or review.";
                                             rdfs:isDefinedBy jazz_aspice:;
                                             rdfs:label "In Analysis/Review".
    jazz_aspice:ApprovalTypeNotApproved a jazz_aspice:ApprovalTypes;
                                        rdfs:comment "Specifies that a change to a rquirement has not been approved.";
                                        rdfs:isDefinedBy jazz_aspice:;
                                        rdfs:label "Not Approved".
    jazz_aspice:ApprovalTypeNotStarted a jazz_aspice:ApprovalTypes;
                                       rdfs:comment "Specifies that a requirement change review has not been started.";
                                       rdfs:isDefinedBy jazz_aspice:;
                                       rdfs:label "Not Started".
    jazz_aspice:ApprovalTypes a rdfs:Class;
                              rdfs:comment "Defines the types of approvals for a requirement change review.";
                              rdfs:isDefinedBy jazz_aspice:;
                              rdfs:label "Approval Types".
    jazz_aspice:CategoryDefect a jazz_aspice:ProblemCategories;
                               rdfs:comment "The Problem category is a defect.";
                               rdfs:isDefinedBy jazz_aspice:;
                               rdfs:label "Defect".
    jazz_aspice:CategoryIssue a jazz_aspice:ProblemCategories;
                              rdfs:comment "The Problem category is an issue.";
                              rdfs:isDefinedBy jazz_aspice:;
                              rdfs:label "Issue".
    jazz_aspice:Document a rdfs:Class;
                         rdfs:comment "This artifact is used for specific documents required for ASPICE compliance.";
                         rdfs:isDefinedBy jazz_aspice:;
                         rdfs:label "Document".
    jazz_aspice:EventMeeting a jazz_aspice:EventTypes;
                             rdfs:comment "The Event is a meeting.";
                             rdfs:isDefinedBy jazz_aspice:;
                             rdfs:label "Meeting".
    jazz_aspice:EventMilestone a jazz_aspice:EventTypes;
                               rdfs:comment "The Event is a milestone.";
                               rdfs:isDefinedBy jazz_aspice:;
                               rdfs:label "Milestone".
    jazz_aspice:EventPlanning a jazz_aspice:EventTypes;
                              rdfs:comment "The Event is a for planning.";
                              rdfs:isDefinedBy jazz_aspice:;
                              rdfs:label "Planning Event".
    jazz_aspice:EventRetrospective a jazz_aspice:EventTypes;
                                   rdfs:comment "The Event is a retrospective.";
                                   rdfs:isDefinedBy jazz_aspice:;
                                   rdfs:label "Retrospective".
    jazz_aspice:EventTypes a rdfs:Class;
                           rdfs:comment "Designates the values that define the type of an Event.";
                           rdfs:isDefinedBy jazz_aspice:;
                           rdfs:label "Event Types".
    jazz_aspice:Finding a rdfs:Class;
                        rdfs:comment "This artifact represents information discovered as a result of an investigation during a review, inspection, analysis, etc..";
                        rdfs:isDefinedBy jazz_aspice:;
                        rdfs:label "Finding".
    jazz_aspice:FindingTypes a rdfs:Class;
                             rdfs:comment "Defines the types of for a Finding.";
                             rdfs:isDefinedBy jazz_aspice:;
                             rdfs:label "Finding Types".
    jazz_aspice:FindingTypesEditorial a jazz_aspice:FindingTypes;
                                      rdfs:comment "Specifies that a Finding reflects an editorial comment.";
                                      rdfs:isDefinedBy jazz_aspice:;
                                      rdfs:label "Editorial".
    jazz_aspice:FindingTypesTechnical a jazz_aspice:FindingTypes;
                                      rdfs:comment "Specifies that a Finding reflects an technical comment.";
                                      rdfs:isDefinedBy jazz_aspice:;
                                      rdfs:label "Technical".
    jazz_aspice:FindingsModule a jazz_rm:Module;
                               rdfs:comment "A module containing Findings.";
                               rdfs:isDefinedBy jazz_aspice:;
                               rdfs:label "Findings Module";
                               rdfs:seeAlso jazz_aspice:Finding.
    jazz_aspice:LegalAdministrativeDocument a rdfs:Class;
                                            rdfs:comment "This artifact is used to specify relevant Legal and Administrative Document in a central Register (Module). It is derived from Automotive SPICE ACQ.12. Legal and Administrative Requirements.";
                                            rdfs:isDefinedBy jazz_aspice:;
                                            rdfs:label "Legal and Administrative Document".
    jazz_aspice:LegalAdministrativeModule a jazz_rm:Module;
                                          rdfs:comment "A module containing Legal and Administrative Requirements. It is derived from Automotive SPICE ACQ.12. Legal and Administrative Requirements.";
                                          rdfs:isDefinedBy jazz_aspice:;
                                          rdfs:label "Legal and Administrative Module".
    jazz_aspice:LegalAdministrativeRegister a jazz_rm:Module;
                                            rdfs:comment "A module containing a central registry that collates Legal and Administrative documents. It is derived from Automotive SPICE ACQ.12. Legal and Administrative Requirements.";
                                            rdfs:isDefinedBy jazz_aspice:;
                                            rdfs:label "Legal and Administrative Register".
    jazz_aspice:LegalAdministrativeRequirement a rdfs:Class;
                                               rdfs:comment "This artifact is used for capturing a Legal or Administrative Requirement of a Regulatory. It is derived from Automotive SPICE ACQ.12. Legal and Administrative Requirements.";
                                               rdfs:isDefinedBy jazz_aspice:;
                                               rdfs:label "Legal and Administrative Requirement".
    jazz_aspice:MaturityTypes a rdfs:Class;
                              rdfs:comment "Defines the levels of maturity an Automotive OEM would use to describe the desired state of requirement delivery.";
                              rdfs:isDefinedBy jazz_aspice:;
                              rdfs:label "Maturity Types".
    jazz_aspice:MaturityTypesBetaTested a jazz_aspice:MaturityTypes;
                                        rdfs:comment "Specifies that requirement delivery has been Beta-tested.";
                                        rdfs:isDefinedBy jazz_aspice:;
                                        rdfs:label "Beta-tested".
    jazz_aspice:MaturityTypesConcept a jazz_aspice:MaturityTypes;
                                     rdfs:comment "Specifies that requirement delivery is in the Concept state.";
                                     rdfs:isDefinedBy jazz_aspice:;
                                     rdfs:label "Concept".
    jazz_aspice:MaturityTypesProductionReady a jazz_aspice:MaturityTypes;
                                             rdfs:comment "Specifies that requirement delivery is Production-ready.";
                                             rdfs:isDefinedBy jazz_aspice:;
                                             rdfs:label "Production-ready".
    jazz_aspice:MaturityTypesPrototype a jazz_aspice:MaturityTypes;
                                       rdfs:comment "Specifies that requirement delivery is in the Prototype state.";
                                       rdfs:isDefinedBy jazz_aspice:;
                                       rdfs:label "Prototype".
    jazz_aspice:ProblemCategories a rdfs:Class;
                                  rdfs:comment "Designates the values for category of a Problem.";
                                  rdfs:isDefinedBy jazz_aspice:;
                                  rdfs:label "Problem Categories".
    jazz_aspice:ProblemHowFoundExternal a jazz_aspice:ProblemHowFoundValue;
                                        rdfs:comment "Indicates a problem was found externally.";
                                        rdfs:isDefinedBy jazz_aspice:;
                                        rdfs:label "External".
    jazz_aspice:ProblemHowFoundInternal a jazz_aspice:ProblemHowFoundValue;
                                        rdfs:comment "Indicates a problem was found internally.";
                                        rdfs:isDefinedBy jazz_aspice:;
                                        rdfs:label "Internal".
    jazz_aspice:ProblemHowFoundValue a rdfs:Class;
                                     rdfs:comment "Describes whether a problem was found internally or externally.";
                                     rdfs:isDefinedBy jazz_aspice:;
                                     rdfs:label "How Found".
    jazz_aspice:ProcessACQ4 a jazz_aspice:ProcessGroups;
                            rdfs:comment "The work is associated with supplier monitoring.";
                            rdfs:isDefinedBy jazz_aspice:;
                            rdfs:label "ACQ.4 Supplier Monitoring".
    jazz_aspice:ProcessGroups a rdfs:Class;
                              rdfs:comment "Defines the ASPICE process groups to which work can be associated.";
                              rdfs:isDefinedBy jazz_aspice:;
                              rdfs:label "Process Groups".
    jazz_aspice:ProcessMAN3 a jazz_aspice:ProcessGroups;
                            rdfs:comment "The work is associated with project management.";
                            rdfs:isDefinedBy jazz_aspice:;
                            rdfs:label "MAN.3 Project Management".
    jazz_aspice:ProcessNone a jazz_aspice:ProcessGroups;
                            rdfs:comment "The work is not associated with any ASPICE-specific process group.";
                            rdfs:isDefinedBy jazz_aspice:;
                            rdfs:label "No ASPICE Process".
    jazz_aspice:ProcessSUP1 a jazz_aspice:ProcessGroups;
                            rdfs:comment "The work is associated with quality assurance.";
                            rdfs:isDefinedBy jazz_aspice:;
                            rdfs:label "SUP.1 Quality Assurance".
    jazz_aspice:ProcessSUP10 a jazz_aspice:ProcessGroups;
                             rdfs:comment "The work is associated with change request management.";
                             rdfs:isDefinedBy jazz_aspice:;
                             rdfs:label "SUP.10 Change Request Management".
    jazz_aspice:ProcessSUP8 a jazz_aspice:ProcessGroups;
                            rdfs:comment "The work is associated with configuration management.";
                            rdfs:isDefinedBy jazz_aspice:;
                            rdfs:label "SUP.8 Configuration Management".
    jazz_aspice:ProcessSUP9 a jazz_aspice:ProcessGroups;
                            rdfs:comment "The work is associated with problem resolution management.";
                            rdfs:isDefinedBy jazz_aspice:;
                            rdfs:label "SUP.9 Problem Resolution Management".
    jazz_aspice:ProcessSWE1 a jazz_aspice:ProcessGroups;
                            rdfs:comment "The work is associated with software requirements analysis.";
                            rdfs:isDefinedBy jazz_aspice:;
                            rdfs:label "SWE.1 Software Requirements Analysis".
    jazz_aspice:ProcessSWE2 a jazz_aspice:ProcessGroups;
                            rdfs:comment "The work is associated with software architectural design.";
                            rdfs:isDefinedBy jazz_aspice:;
                            rdfs:label "SWE.2 Software Architectural Design".
    jazz_aspice:ProcessSWE3 a jazz_aspice:ProcessGroups;
                            rdfs:comment "The work is associated with software detailed design and unit construction.";
                            rdfs:isDefinedBy jazz_aspice:;
                            rdfs:label "SWE.3 Software Detailed Design and Unit Construction".
    jazz_aspice:ProcessSWE4 a jazz_aspice:ProcessGroups;
                            rdfs:comment "The work is associated with software unit verification.";
                            rdfs:isDefinedBy jazz_aspice:;
                            rdfs:label "SWE.4 Software Unit Verification".
    jazz_aspice:ProcessSWE5 a jazz_aspice:ProcessGroups;
                            rdfs:comment "The work is associated with software integration and integration test.";
                            rdfs:isDefinedBy jazz_aspice:;
                            rdfs:label "SWE.5 Software Integration and Integration Test".
    jazz_aspice:ProcessSWE6 a jazz_aspice:ProcessGroups;
                            rdfs:comment "The work is associated with software qualification test.";
                            rdfs:isDefinedBy jazz_aspice:;
                            rdfs:label "SWE.6 Software Qualification Test".
    jazz_aspice:ProcessSYS1 a jazz_aspice:ProcessGroups;
                            rdfs:comment "The work is associated with requirements elicitation.";
                            rdfs:isDefinedBy jazz_aspice:;
                            rdfs:label "SYS.1 Requirements Elicitation".
    jazz_aspice:ProcessSYS2 a jazz_aspice:ProcessGroups;
                            rdfs:comment "The work is associated with requirements analysis.";
                            rdfs:isDefinedBy jazz_aspice:;
                            rdfs:label "SYS.2 System Requirements Analysis".
    jazz_aspice:ProcessSYS3 a jazz_aspice:ProcessGroups;
                            rdfs:comment "The work is associated with system architectural design.";
                            rdfs:isDefinedBy jazz_aspice:;
                            rdfs:label "SYS.3 System Architectural Design".
    jazz_aspice:ProcessSYS4 a jazz_aspice:ProcessGroups;
                            rdfs:comment "The work is associated with system integration and integration test.";
                            rdfs:isDefinedBy jazz_aspice:;
                            rdfs:label "SYS.4 System Integration and Integration Test".
    jazz_aspice:ProcessSYS5 a jazz_aspice:ProcessGroups;
                            rdfs:comment "The work is associated with system qualification test.";
                            rdfs:isDefinedBy jazz_aspice:;
                            rdfs:label "SYS.5 System Qualification Test".
    jazz_aspice:RequirementLevelFunctional a jazz_aspice:RequirementLevels;
                                           rdfs:comment "Functional requirements level.";
                                           rdfs:isDefinedBy jazz_aspice:;
                                           rdfs:label "Functional".
    jazz_aspice:RequirementLevelTechnical a jazz_aspice:RequirementLevels;
                                          rdfs:comment "Technical requirements level.";
                                          rdfs:isDefinedBy jazz_aspice:;
                                          rdfs:label "Technical".
    jazz_aspice:RequirementLevels a rdfs:Class;
                                  rdfs:comment "Defines levels of system requirements.";
                                  rdfs:isDefinedBy jazz_aspice:;
                                  rdfs:label "Requirement Levels".
    jazz_aspice:RequirementTypeFunctional a jazz_aspice:RequirementTypes;
                                          rdfs:comment "Specifies a requirement as a functional requirement.";
                                          rdfs:isDefinedBy jazz_aspice:;
                                          rdfs:label "Functional".
    jazz_aspice:RequirementTypeNonFunctional a jazz_aspice:RequirementTypes;
                                             rdfs:comment "Specifies a requirement as a non-functional requirement.";
                                             rdfs:isDefinedBy jazz_aspice:;
                                             rdfs:label "Non-Functional".
    jazz_aspice:RequirementTypeSafety a jazz_aspice:RequirementTypes;
                                      rdfs:comment "Specifies a requirement as a safety requirement.";
                                      rdfs:isDefinedBy jazz_aspice:;
                                      rdfs:label "Safety".
    jazz_aspice:RequirementTypes a rdfs:Class;
                                 rdfs:comment "Defines the types of requirement.";
                                 rdfs:isDefinedBy jazz_aspice:;
                                 rdfs:label "Requirement Types".
    jazz_aspice:RiskArea a rdfs:Class;
                         rdfs:comment "Defines the aspect of delivery to which the Risk applies.";
                         rdfs:isDefinedBy jazz_aspice:;
                         rdfs:label "Risk Area".
    jazz_aspice:RiskAreaCompliance a jazz_aspice:RiskArea;
                                   rdfs:comment "The Risk relates to an internal or external compliance issue.";
                                   rdfs:isDefinedBy jazz_aspice:;
                                   rdfs:label "Compliance".
    jazz_aspice:RiskAreaCost a jazz_aspice:RiskArea;
                             rdfs:comment "The Risk relates to a cost issue.";
                             rdfs:isDefinedBy jazz_aspice:;
                             rdfs:label "Cost".
    jazz_aspice:RiskAreaEffort a jazz_aspice:RiskArea;
                               rdfs:comment "The Risk relates to an issue with effort, such as estimated effort is too low or there is no capacity.";
                               rdfs:isDefinedBy jazz_aspice:;
                               rdfs:label "Effort".
    jazz_aspice:RiskAreaResource a jazz_aspice:RiskArea;
                                 rdfs:comment "The Risk relates to a resource issue.";
                                 rdfs:isDefinedBy jazz_aspice:;
                                 rdfs:label "Resource".
    jazz_aspice:RiskAreaTechnical a jazz_aspice:RiskArea;
                                  rdfs:comment "The Risk relates to a technical issue.";
                                  rdfs:isDefinedBy jazz_aspice:;
                                  rdfs:label "Technical".
    jazz_aspice:RiskAreaTiming a jazz_aspice:RiskArea;
                               rdfs:comment "The Risk relates to a timing or schedule issue.";
                               rdfs:isDefinedBy jazz_aspice:;
                               rdfs:label "Timing".
    jazz_aspice:RiskAreaUnassigned a jazz_aspice:RiskArea;
                                   rdfs:comment "The Risk area is unassigned.";
                                   rdfs:isDefinedBy jazz_aspice:;
                                   rdfs:label "Unassigned".
    jazz_aspice:RiskType a rdfs:Class;
                         rdfs:comment "Defines the type of Risk.";
                         rdfs:isDefinedBy jazz_aspice:;
                         rdfs:label "Risk Type".
    jazz_aspice:RiskTypeFMEA a jazz_aspice:RiskType;
                             rdfs:comment "The Risk type is related to FMEA.";
                             rdfs:isDefinedBy jazz_aspice:;
                             rdfs:label "FMEA".
    jazz_aspice:RiskTypeFunctional a jazz_aspice:RiskType;
                                   rdfs:comment "The Risk type is related to functional analysis.";
                                   rdfs:isDefinedBy jazz_aspice:;
                                   rdfs:label "Functional Analysis".
    jazz_aspice:RiskTypeManagement a jazz_aspice:RiskType;
                                   rdfs:comment "The Risk type is related to management.";
                                   rdfs:isDefinedBy jazz_aspice:;
                                   rdfs:label "Management".
    jazz_aspice:RiskTypeSimulation a jazz_aspice:RiskType;
                                   rdfs:comment "The Risk type is relatd to simulation.";
                                   rdfs:isDefinedBy jazz_aspice:;
                                   rdfs:label "Simulation".
    jazz_aspice:RiskTypeUnassigned a jazz_aspice:RiskType;
                                   rdfs:comment "The Risk type is unassigned.";
                                   rdfs:isDefinedBy jazz_aspice:;
                                   rdfs:label "Unassigned".
    jazz_aspice:StateCanceled a oslc_cm:State;
                              rdfs:comment "The artifact has been canceled.";
                              rdfs:isDefinedBy jazz_aspice:;
                              rdfs:label "Canceled";
                              skos:narrower oslc_cm:Closed.
    jazz_aspice:StateReadyForReview a oslc_cm:State;
                                    rdfs:comment "The artifact is ready for a review.";
                                    rdfs:isDefinedBy jazz_aspice:;
                                    rdfs:label "Ready for Review";
                                    skos:narrower oslc_cm:Inprogress.
    jazz_aspice:StateScheduled a oslc_cm:State;
                               rdfs:comment "The artifact is scheduled.";
                               rdfs:isDefinedBy jazz_aspice:;
                               rdfs:label "Scheduled";
                               skos:narrower oslc_cm:Inprogress.
    jazz_aspice:StateVerifying a oslc_cm:State;
                               rdfs:comment "A Problem is in the process of being verified.";
                               rdfs:isDefinedBy jazz_aspice:;
                               rdfs:label "Verifying";
                               skos:narrower oslc_cm:Inprogress.
    jazz_aspice:SysReqVerificationLevels a rdfs:Class;
                                         rdfs:comment "Defines the levels of verification specifically for System Requirements.";
                                         rdfs:isDefinedBy jazz_aspice:;
                                         rdfs:label "System Requirement Verification Levels".
    jazz_aspice:SysReqVerificationSystemIntegrationTest a jazz_aspice:SysReqVerificationLevels;
                                                        rdfs:comment "Indicates requirement will be verified during system integration test.";
                                                        rdfs:isDefinedBy jazz_aspice:;
                                                        rdfs:label "System Integration Test".
    jazz_aspice:SysReqVerificationSystemQualificationTest a jazz_aspice:SysReqVerificationLevels;
                                                          rdfs:comment "Indicates requirement will be verified during system qualification test.";
                                                          rdfs:isDefinedBy jazz_aspice:;
                                                          rdfs:label "System Qualification Test".
    jazz_aspice:VerificationIntegrationTest a jazz_aspice:VerificationLevels;
                                            rdfs:comment "Indicates requirement will be verified during integration test.";
                                            rdfs:isDefinedBy jazz_aspice:;
                                            rdfs:label "Integration Test".
    jazz_aspice:VerificationLevels a rdfs:Class;
                                   rdfs:comment "Defines the levels of verification.";
                                   rdfs:isDefinedBy jazz_aspice:;
                                   rdfs:label "Verification Levels".
    jazz_aspice:VerificationQualificationTest a jazz_aspice:VerificationLevels;
                                              rdfs:comment "Indicates requirement will be verified during qualification test.";
                                              rdfs:isDefinedBy jazz_aspice:;
                                              rdfs:label "Qualification Test".
    jazz_aspice:VerificationUnitTest a jazz_aspice:VerificationLevels;
                                     rdfs:comment "Indicates requirement will be verified during unit test.";
                                     rdfs:isDefinedBy jazz_aspice:;
                                     rdfs:label "Unit Test".
    jazz_aspice:VerifyByAnalysis a jazz_aspice:VerifyByMethod;
                                 rdfs:comment "Indicates the verification method is by analysis.";
                                 rdfs:isDefinedBy jazz_aspice:;
                                 rdfs:label "Analysis".
    jazz_aspice:VerifyByAudit a jazz_aspice:VerifyByMethod;
                              rdfs:comment "Indicates the verification method is by audit.";
                              rdfs:isDefinedBy jazz_aspice:;
                              rdfs:label "Audit".
    jazz_aspice:VerifyByComparison a jazz_aspice:VerifyByMethod;
                                   rdfs:comment "Indicates the verification method is by comparison.";
                                   rdfs:isDefinedBy jazz_aspice:;
                                   rdfs:label "Comparison".
    jazz_aspice:VerifyByDemonstration a jazz_aspice:VerifyByMethod;
                                      rdfs:comment "Indicates the verification method is by demonstration.";
                                      rdfs:isDefinedBy jazz_aspice:;
                                      rdfs:label "Demonstration".
    jazz_aspice:VerifyByInspection a jazz_aspice:VerifyByMethod;
                                   rdfs:comment "Indicates the verification method is by inspection.";
                                   rdfs:isDefinedBy jazz_aspice:;
                                   rdfs:label "Inspection".
    jazz_aspice:VerifyByMethod a rdfs:Class;
                               rdfs:comment "Defines the methods that can be used for verification.";
                               rdfs:isDefinedBy jazz_aspice:;
                               rdfs:label "Verification Methods".
    jazz_aspice:VerifyByPeerReview a jazz_aspice:VerifyByMethod;
                                   rdfs:comment "Indicates the verification method is by peer review.";
                                   rdfs:isDefinedBy jazz_aspice:;
                                   rdfs:label "Peer Review".
    jazz_aspice:VerifyByTest a jazz_aspice:VerifyByMethod;
                             rdfs:comment "Indicates the verification method is by test.";
                             rdfs:isDefinedBy jazz_aspice:;
                             rdfs:label "Test".
    jazz_aspice:VerifyByUnassigned a jazz_aspice:VerifyByMethod;
                                   rdfs:comment "The verification method is unassigned.";
                                   rdfs:isDefinedBy jazz_aspice:;
                                   rdfs:label "Unassigned".
    jazz_aspice:VerifyByWalkthrough a jazz_aspice:VerifyByMethod;
                                    rdfs:comment "Indicates the verification method is by walkthrough.";
                                    rdfs:isDefinedBy jazz_aspice:;
                                    rdfs:label "Walkthrough".
    jazz_aspice:affectedDomain a rdf:Property;
                               rdfs:comment "Used to specify the domain level of the requirement.";
                               rdfs:isDefinedBy jazz_aspice:;
                               rdfs:label "Affected Domain";
                               rdfs:seeAlso jazz_aspice:AffectedDomainTypes.
    jazz_aspice:detectedDuring a rdf:Property;
                               rdfs:comment "The problem was detected during the phase of the lifecycle described by a Process Group. Typically expressed as a value of type jazz_aspice:ProcessGroups.";
                               rdfs:isDefinedBy jazz_aspice:;
                               rdfs:label "Detected During";
                               rdfs:seeAlso jazz_aspice:ProcessGroups.
    jazz_aspice:docVersion a rdf:Property;
                           rdfs:comment "The version of a document.";
                           rdfs:isDefinedBy jazz_aspice:;
                           rdfs:label "Document Version".
    jazz_aspice:eventType a rdf:Property;
                          rdfs:comment "The type of event. Typically expressed as a value of type jazz_aspice:EventTypes.";
                          rdfs:isDefinedBy jazz_aspice:;
                          rdfs:label "Event Type";
                          rdfs:seeAlso jazz_aspice:EventTypes.
    jazz_aspice:externalParticipants a rdf:Property;
                                     rdfs:comment "Identifies the external participants for an Event.";
                                     rdfs:isDefinedBy jazz_aspice:;
                                     rdfs:label "External Participants".
    jazz_aspice:findingType a rdf:Property;
                            rdfs:comment "Specifies the nature of a finding.";
                            rdfs:isDefinedBy jazz_aspice:;
                            rdfs:label "Finding Type";
                            rdfs:seeAlso jazz_aspice:FindingTypes.
    jazz_aspice:hardwareImpactAnalysis a rdf:Property;
                                       rdfs:comment "Describes the analysis of hardware impact as a result of the change reuqest.";
                                       rdfs:isDefinedBy jazz_aspice:;
                                       rdfs:label "Hardware Impact Analysis".
    jazz_aspice:howFound a rdf:Property;
                         rdfs:comment "Describes whether the change request or problem is from an internal or external source. Typically expressed as a value of type jazz_aspice:HowFoundValue.";
                         rdfs:isDefinedBy jazz_aspice:;
                         rdfs:label "How Found";
                         rdfs:seeAlso jazz_aspice:HowFoundValue.
    jazz_aspice:improvementSuggestions a rdf:Property;
                                       rdfs:comment "Suggestions for improvements in the reviewed artifacts or system.";
                                       rdfs:isDefinedBy jazz_aspice:;
                                       rdfs:label "Improvement Suggestions".
    jazz_aspice:internalParticipants a rdf:Property;
                                     rdfs:comment "Identifies the interna participants for an Event.";
                                     rdfs:isDefinedBy jazz_aspice:;
                                     rdfs:label "Internal Participants".
    jazz_aspice:introducedIn a rdf:Property;
                             rdfs:comment "The problem was introduced during the phase of the lifecycle described by a Process Group. Typically expressed as a value of type jazz_aspice:ProcessGroups.";
                             rdfs:isDefinedBy jazz_aspice:;
                             rdfs:label "Introduced In";
                             rdfs:seeAlso jazz_aspice:ProcessGroups.
    jazz_aspice:legalEntity a rdf:Property;
                            rdfs:comment "Derived from ACQ.12. Legal and Administrative Requirements. Describes the Legal Entity releasing a Legal and Administrative Requirement e.g. ISO.";
                            rdfs:isDefinedBy jazz_aspice:;
                            rdfs:label "Legal Entity".
    jazz_aspice:lessonsLearned a rdf:Property;
                               rdfs:comment "Indicates whether or not the Problem leads to lessons learned documentation.";
                               rdfs:isDefinedBy jazz_aspice:;
                               rdfs:label "Lessons Learned".
    jazz_aspice:mandatoryReviewers a rdf:Property;
                                   rdfs:comment "Identifies the mandatory reviewers.";
                                   rdfs:isDefinedBy jazz_aspice:;
                                   rdfs:label "Mandatory Reviewers".
    jazz_aspice:manufacturingImpactAnalysis a rdf:Property;
                                            rdfs:comment "Describes the analysis of manufacturing impact as a result of the change request.";
                                            rdfs:isDefinedBy jazz_aspice:;
                                            rdfs:label "Manufacturing Impact Analysis".
    jazz_aspice:maturity a rdf:Property;
                         rdfs:comment "Used by Automotive OEMs to indicate the level of maturity of requirement delivery.";
                         rdfs:isDefinedBy jazz_aspice:;
                         rdfs:label "Maturity";
                         rdfs:seeAlso jazz_aspice:MaturityTypes.
    jazz_aspice:mechanicalImpactAnalysis a rdf:Property;
                                         rdfs:comment "Describes the analysis of mechanical impact as a result of the change request.";
                                         rdfs:isDefinedBy jazz_aspice:;
                                         rdfs:label "Mechanical Impact Analysis".
    jazz_aspice:need a rdf:Property;
                     rdfs:comment "Indicates the degree of need for this requirement.";
                     rdfs:isDefinedBy jazz_aspice:;
                     rdfs:label "Need";
                     rdfs:seeAlso jazz_aspice:NeedValues.
    jazz_aspice:nonConformities a rdf:Property;
                                rdfs:comment "Identifies any non-conformities as a result of the review.";
                                rdfs:isDefinedBy jazz_aspice:;
                                rdfs:label "Non-Conformities".
    jazz_aspice:notRequiredForRegression a rdf:Property;
                                         rdfs:comment "Indicates the Test Case is not required for regression testing.";
                                         rdfs:isDefinedBy jazz_aspice:;
                                         rdfs:label "Not Required".
    jazz_aspice:offlineComments a rdf:Property;
                                rdfs:comment "Comments submitted offline.";
                                rdfs:isDefinedBy jazz_aspice:;
                                rdfs:label "Offline Comments".
    jazz_aspice:optionalReviewers a rdf:Property;
                                  rdfs:comment "Identifies the optional reviewers.";
                                  rdfs:isDefinedBy jazz_aspice:;
                                  rdfs:label "Optional Reviewers".
    jazz_aspice:paragraph a rdf:Property;
                          rdfs:comment "Derived from Automotive SPICE ACQ.12. Legal and Administrative Requirements. Needed to specify the Paragraph in a Legal and Administrative Requirement.";
                          rdfs:isDefinedBy jazz_aspice:;
                          rdfs:label "Paragraph".
    jazz_aspice:partyHighImpact a rdf:Property;
                                rdfs:comment "Indicates whether or not the Problem has an impact on another party.";
                                rdfs:isDefinedBy jazz_aspice:;
                                rdfs:label "High Impact on Other Party".
    jazz_aspice:problemCategory a rdf:Property;
                                rdfs:comment "Specifies the category of the problem. Typically expressed as a value of type jazz_aspice:ProblemCategories.";
                                rdfs:isDefinedBy jazz_aspice:;
                                rdfs:label "Problem Category";
                                rdfs:seeAlso jazz_aspice:ProblemCategories.
    jazz_aspice:problemDescription a rdf:Property;
                                   rdfs:comment "Description of the problem.";
                                   rdfs:isDefinedBy jazz_aspice:;
                                   rdfs:label "Problem Description".
    jazz_aspice:processGroup a rdf:Property;
                             rdfs:comment "Specifies the process group associated with the review. Typically expressed as a value of type jazz_aspice:ProcessGroups.";
                             rdfs:isDefinedBy jazz_aspice:;
                             rdfs:label "Process Group";
                             rdfs:seeAlso jazz_aspice:ProcessGroups.
    jazz_aspice:qualityImpactAnalysis a rdf:Property;
                                      rdfs:comment "Describes the analysis of quality impact as a result of the change request.";
                                      rdfs:isDefinedBy jazz_aspice:;
                                      rdfs:label "Quality Impact Analysis".
    jazz_aspice:requiredForRegression a rdf:Property;
                                      rdfs:comment "Indicates the Test Case is required for regression testing.";
                                      rdfs:isDefinedBy jazz_aspice:;
                                      rdfs:label "Required".
    jazz_aspice:requirementLevel a rdf:Property;
                                 rdfs:comment "This value defines the level of abstraction of the system requirement. Expressed of type jazz_aspice:RequirementLevels.";
                                 rdfs:isDefinedBy jazz_aspice:;
                                 rdfs:label "Requirement Level";
                                 rdfs:seeAlso jazz_aspice:RequirementLevels.
    jazz_aspice:requirementType a rdf:Property;
                                rdfs:comment "The type of requirement.";
                                rdfs:isDefinedBy jazz_aspice:;
                                rdfs:label "Requirement Type";
                                rdfs:seeAlso jazz_aspice:RequirementTypes.
    jazz_aspice:reviewFindings a rdf:Property;
                               rdfs:comment "Identifies any findings as a result of the review.";
                               rdfs:isDefinedBy jazz_aspice:;
                               rdfs:label "Review Findings".
    jazz_aspice:reviewer a rdf:Property;
                         rdfs:comment "The user reviewing a case and presenting a finding.";
                         rdfs:isDefinedBy jazz_aspice:;
                         rdfs:label "Reviewer".
    jazz_aspice:riskArea a rdf:Property;
                         rdfs:comment "Aspect of delivery to which the Risk applies. Typically expressed as a value of type jazz_aspice:RiskArea.";
                         rdfs:isDefinedBy jazz_aspice:;
                         rdfs:label "Risk Area";
                         rdfs:seeAlso jazz_aspice:RiskArea.
    jazz_aspice:riskConsequence a rdf:Property;
                                rdfs:comment "Consequences associated with the risk.";
                                rdfs:isDefinedBy jazz_aspice:;
                                rdfs:label "Risk Consequence".
    jazz_aspice:riskType a rdf:Property;
                         rdfs:comment "Identifies the type of Risk. Typically expressed as a value of type jazz_aspice:RiskType.";
                         rdfs:isDefinedBy jazz_aspice:;
                         rdfs:label "Risk Type";
                         rdfs:seeAlso jazz_aspice:RiskType.
    jazz_aspice:scheduleImpactAnalysis a rdf:Property;
                                       rdfs:comment "Describes the analysis of schedule impact as a result of the change request.";
                                       rdfs:isDefinedBy jazz_aspice:;
                                       rdfs:label "Schedule Impact Analysis".
    jazz_aspice:softwareImpactAnalysis a rdf:Property;
                                       rdfs:comment "Describes the analysis of software impact as a result of the change request.";
                                       rdfs:isDefinedBy jazz_aspice:;
                                       rdfs:label "Software Impact Analysis".
    jazz_aspice:statusAutomated a rdf:Property;
                                rdfs:comment "Indicates the Test Script is automated.";
                                rdfs:isDefinedBy jazz_aspice:;
                                rdfs:label "Automated".
    jazz_aspice:statusAutomationPlanned a rdf:Property;
                                        rdfs:comment "Indicates the Test Script is in the process of or planned to be automated.";
                                        rdfs:isDefinedBy jazz_aspice:;
                                        rdfs:label "Automation Planned".
    jazz_aspice:statusNotAutomated a rdf:Property;
                                   rdfs:comment "Indicates the Test Script is not automated.";
                                   rdfs:isDefinedBy jazz_aspice:;
                                   rdfs:label "Not Automated".
    jazz_aspice:systemHighImpact a rdf:Property;
                                 rdfs:comment "Indicates whether or not the Problem has an impact on another system.";
                                 rdfs:isDefinedBy jazz_aspice:;
                                 rdfs:label "High Impact on Other System".
    jazz_aspice:systemImpactAnalysis a rdf:Property;
                                     rdfs:comment "Describes the analysis of system impact as a result of the change request.";
                                     rdfs:isDefinedBy jazz_aspice:;
                                     rdfs:label "System Impact Analysis".
    jazz_aspice:systemReqVerificationLevel a rdf:Property;
                                           rdfs:comment "Level of testing at which the system requirement should be verified. Can be expressed as a value of type jazz_aspice:VerificationLevel.";
                                           rdfs:isDefinedBy jazz_aspice:;
                                           rdfs:label "System Req Verification Level";
                                           rdfs:seeAlso jazz_aspice:VerificationLevels.
    jazz_aspice:testCaseCategoryRequiredForRegression a rdf:Property;
                                                      rdfs:comment "Category indicating whether a Test Case is required for regression testing.";
                                                      rdfs:isDefinedBy jazz_aspice:;
                                                      rdfs:label "Required for Regression".
    jazz_aspice:testCategoryTestPhase a rdf:Property;
                                      rdfs:comment "Category indicating the phase of testing in the ASPICE process to which the test artifact applies.";
                                      rdfs:isDefinedBy jazz_aspice:;
                                      rdfs:label "Test Level".
    jazz_aspice:testPhaseSafetyValidation a rdf:Property;
                                          rdfs:comment "Category indicating the test artifact is associated with the ASPICE Software Integration and Integration Test phase.";
                                          rdfs:isDefinedBy jazz_aspice:;
                                          rdfs:label "Safety Validation Test".
    jazz_aspice:testPhaseSoftwareIntegration a rdf:Property;
                                             rdfs:comment "Category indicating the test artifact is associated with the ASPICE Software Integration and Integration Test phase.";
                                             rdfs:isDefinedBy jazz_aspice:;
                                             rdfs:label "Software Integration and Integration Test".
    jazz_aspice:testPhaseSoftwareQualification a rdf:Property;
                                               rdfs:comment "Category indicating the test artifact is associated with the ASPICE Software Qualification Test phase.";
                                               rdfs:isDefinedBy jazz_aspice:;
                                               rdfs:label "Software Qualification Test".
    jazz_aspice:testPhaseSystemIntegration a rdf:Property;
                                           rdfs:comment "Category indicating the test artifact is associated with the ASPICE System Integration and Integration Test phase.";
                                           rdfs:isDefinedBy jazz_aspice:;
                                           rdfs:label "System Integration and Integration Test".
    jazz_aspice:testPhaseSystemQualification a rdf:Property;
                                             rdfs:comment "Category indicating the test artifact is associated with the ASPICE System Qualification Test phase.";
                                             rdfs:isDefinedBy jazz_aspice:;
                                             rdfs:label "System Qualification Test".
    jazz_aspice:testPhaseUAT a rdf:Property;
                             rdfs:comment "Category indicating the test artifact is associated with the ASPICE Software Integration and Integration Test phase.";
                             rdfs:isDefinedBy jazz_aspice:;
                             rdfs:label "User Acceptance Test".
    jazz_aspice:testPhaseUnitTest a rdf:Property;
                                  rdfs:comment "Category indicating the test artifact is associated with the ASPICE Software Integration and Integration Test phase.";
                                  rdfs:isDefinedBy jazz_aspice:;
                                  rdfs:label "Unit Test".
    jazz_aspice:testScriptCategoryAutomationStatus a rdf:Property;
                                                   rdfs:comment "Category indicating whether a Test Script is automated, manual, or to be automated.";
                                                   rdfs:isDefinedBy jazz_aspice:;
                                                   rdfs:label "Automation".
    jazz_aspice:verificationCriteria a rdf:Property;
                                     rdfs:comment "Identifies the critieria used for the review.";
                                     rdfs:isDefinedBy jazz_aspice:;
                                     rdfs:label "Verification Criteria".
    jazz_aspice:verificationLevel a rdf:Property;
                                  rdfs:comment "Level of testing at which the requirement should be verified. Can be expressed as a value of type jazz_aspice:VerificationLevel.";
                                  rdfs:isDefinedBy jazz_aspice:;
                                  rdfs:label "Verification Level";
                                  rdfs:seeAlso jazz_aspice:VerificationLevels.
    jazz_aspice:verificationMethod a rdf:Property;
                                   rdfs:comment "Method to be used to verify the artifact. Can be expressed as a value of type jazz_aspice:VerifyByMethod.";
                                   rdfs:isDefinedBy jazz_aspice:;
                                   rdfs:label "Verification Method";
                                   rdfs:seeAlso jazz_aspice:VerifyByMethod.
}

