@prefix rdf: <http://www.w3.org/1999/02/22-rdf-syntax-ns#>.
@prefix rdfs: <http://www.w3.org/2000/01/rdf-schema#>.
@prefix xsd: <http://www.w3.org/2001/XMLSchema#>.
@prefix jazz_sse: <http://jazz.net/ns/sse#>.
@prefix dcterms: <http://purl.org/dc/terms/>.
@prefix owl: <http://www.w3.org/2002/07/owl#>.
@prefix oslc: <http://open-services.net/ns/core#>.
@prefix oslc_rm: <http://open-services.net/ns/rm#>.
@prefix oslc_cm: <http://open-services.net/ns/cm#>.
@prefix oslc_qm: <http://open-services.net/ns/qm#>.
@prefix jazz_ccm: <http://jazz.net/ns/ccm#>.
@prefix jazz_rm: <http://jazz.net/ns/rm#>.
@prefix jazz_rqm: <http://jazz.net/ns/qm/rqm#>.
@prefix jazz_esa: <http://jazz.net/ns/enterprise_agile#>.
@prefix jazz_fusa: <http://jazz.net/ns/functional_safety#>.
@prefix jazz_aspice: <http://jazz.net/ns/aspice#>.
@prefix skos: <http://www.w3.org/2004/02/skos/core#>.

{
    jazz_sse: dcterms:dateCopyrighted "2019";
              dcterms:description "Vocabulary terms describing typical resources used for software and systems engineering.";
              dcterms:license <https://jazz.net/ns/license.html>;
              dcterms:source <https://jazz.net/wiki/pub/LinkedData/SseVocabulary/sse-vocabulary.ttl>;
              dcterms:title "IBM Software and Systems Engineering Vocabulary";
              a owl:Ontology;
              rdfs:label "Software and Systems engineering core".
    jazz_sse:Actor a rdfs:Class;
                   rdfs:comment "Represents a role that a human, hardware device, or another system can play in a use case or scenario.";
                   rdfs:isDefinedBy jazz_sse:;
                   rdfs:label "Actor".
    jazz_sse:ApprovalTypeApproved a jazz_sse:ApprovalTypes;
                                  rdfs:comment "Registers approval.";
                                  rdfs:isDefinedBy jazz_sse:;
                                  rdfs:label "Approved".
    jazz_sse:ApprovalTypeInAnalysisReview a jazz_sse:ApprovalTypes;
                                          rdfs:comment "The approval is in analysis/review.";
                                          rdfs:isDefinedBy jazz_sse:;
                                          rdfs:label "In Analysis/Review".
    jazz_sse:ApprovalTypeNotApproved a jazz_sse:ApprovalTypes;
                                     rdfs:comment "Registers lack of approval.";
                                     rdfs:isDefinedBy jazz_sse:;
                                     rdfs:label "Not Approved".
    jazz_sse:ApprovalTypeNotStarted a jazz_sse:ApprovalTypes;
                                    rdfs:comment "The approval is not yet started (default).";
                                    rdfs:isDefinedBy jazz_sse:;
                                    rdfs:label "Not Started".
    jazz_sse:ApprovalTypes a rdfs:Class;
                           rdfs:comment "Types of approvals.";
                           rdfs:isDefinedBy jazz_sse:;
                           rdfs:label "Approval Types".
    jazz_sse:ArtifactCollection a rdfs:Class;
                                rdfs:comment "A logical grouping of related artifacts.";
                                rdfs:isDefinedBy jazz_sse:;
                                rdfs:label "Collection".
    jazz_sse:ArtifactModule a rdfs:Class;
                            rdfs:comment "A hiearchy of requirements.";
                            rdfs:isDefinedBy jazz_sse:;
                            rdfs:label "Module".
    jazz_sse:CheckItem a rdfs:Class;
                       rdfs:comment "A check item is an item on a checklist that needs to be verified for purpose of checking.";
                       rdfs:isDefinedBy jazz_sse:;
                       rdfs:label "Check Item".
    jazz_sse:CheckItemStatusTypes a rdfs:Class;
                                  rdfs:comment "Indicates the status of a check item in a checklist.";
                                  rdfs:isDefinedBy jazz_sse:;
                                  rdfs:label "Check Item Status Types".
    jazz_sse:CheckItemStatusTypesNotApplicable a jazz_sse:CheckItemStatus;
                                               rdfs:comment "The check item is not applicable to the review or artifact.";
                                               rdfs:isDefinedBy jazz_sse:;
                                               rdfs:label "Not Applicable".
    jazz_sse:CheckItemStatusTypesNotStarted a jazz_sse:CheckItemStatus;
                                            rdfs:comment "The check item review has not started (default).";
                                            rdfs:isDefinedBy jazz_sse:;
                                            rdfs:label "Not Started".
    jazz_sse:CheckItemStatusTypesRejected a jazz_sse:CheckItemStatus;
                                          rdfs:comment "The check item has been rejected.";
                                          rdfs:isDefinedBy jazz_sse:;
                                          rdfs:label "Rejected".
    jazz_sse:CheckItemStatusTypesRework a jazz_sse:CheckItemStatus;
                                        rdfs:comment "The check item has recommended rework.";
                                        rdfs:isDefinedBy jazz_sse:;
                                        rdfs:label "Rework".
    jazz_sse:CheckItemStatusTypesVerified a jazz_sse:CheckItemStatus;
                                          rdfs:comment "The check item has been verified.";
                                          rdfs:isDefinedBy jazz_sse:;
                                          rdfs:label "Verified".
    jazz_sse:ChecklistModule a jazz_rm:Module;
                             rdfs:comment "A check item is an item on a checklist that needs to be verified for purpose of checking. A checklist module is used to create checklists composed of check items. This is used along with reviews to ensure that all aspects of the review have been covered.";
                             rdfs:isDefinedBy jazz_sse:;
                             rdfs:label "Checklist Module".
    jazz_sse:DefectDisposition a rdfs:Class;
                               rdfs:comment "Disposition of the resolved defect.";
                               rdfs:isDefinedBy jazz_sse:;
                               rdfs:label "Disposition".
    jazz_sse:DefectDispositionDuplicate a jazz_sse:DefectDisposition;
                                        rdfs:comment "Duplicate of another defect.";
                                        rdfs:isDefinedBy jazz_sse:;
                                        rdfs:label "Duplicate".
    jazz_sse:DefectDispositionFixed a jazz_sse:DefectDisposition;
                                    rdfs:comment "Defect has been corrected.";
                                    rdfs:isDefinedBy jazz_sse:;
                                    rdfs:label "Fixed".
    jazz_sse:DefectDispositionFixedUpstream a jazz_sse:DefectDisposition;
                                            rdfs:comment "Defect has been corrected as part of another change.";
                                            rdfs:isDefinedBy jazz_sse:;
                                            rdfs:label "Fixed Upstream".
    jazz_sse:DefectDispositionInvalid a jazz_sse:DefectDisposition;
                                      rdfs:comment "Not valid.";
                                      rdfs:isDefinedBy jazz_sse:;
                                      rdfs:label "Invalid".
    jazz_sse:DefectDispositionNotReproducible a jazz_sse:DefectDisposition;
                                              rdfs:comment "Defect cannot be reproduced.";
                                              rdfs:isDefinedBy jazz_sse:;
                                              rdfs:label "Not Reproducible".
    jazz_sse:DefectDispositionWontFix a jazz_sse:DefectDisposition;
                                      rdfs:comment "Defect will not be fixed.";
                                      rdfs:isDefinedBy jazz_sse:;
                                      rdfs:label "Won't Fix".
    jazz_sse:DefectDispositionWorksAsDesigned a jazz_sse:DefectDisposition;
                                              rdfs:comment "Working as designed.";
                                              rdfs:isDefinedBy jazz_sse:;
                                              rdfs:label "Works as Designed".
    jazz_sse:DefectDispositionWorksForMe a jazz_sse:DefectDisposition;
                                         rdfs:comment "Unable to reproduce.";
                                         rdfs:isDefinedBy jazz_sse:;
                                         rdfs:label "Works for Me".
    jazz_sse:FreeFormDiagram a rdfs:Class;
                             rdfs:comment "A diagram to help illustrate or communicate a solution or requirement.";
                             rdfs:isDefinedBy jazz_sse:;
                             rdfs:label "Free-Form Diagram".
    jazz_sse:HMLScale a rdfs:Class;
                      rdfs:comment "Ordinal scale (high/medium/low) for rating properties. Typically expressed as a value of type oslc_cm:Priority.";
                      rdfs:isDefinedBy jazz_sse:;
                      rdfs:label "Rating scale (High/Medium/Low)";
                      rdfs:seeAlso oslc_cm:High,
                                   oslc_cm:Low,
                                   oslc_cm:Medium.
    jazz_sse:HMLUnassigned a jazz_sse:HMLScale;
                           rdf:value 0 ;
                           rdfs:comment "Unassigned ordinal scale value.";
                           rdfs:isDefinedBy jazz_sse:;
                           rdfs:label "Unassigned".
    jazz_sse:HardwareRequirement a rdfs:Class;
                                 rdfs:comment "A requirement allocated to hardware.";
                                 rdfs:isDefinedBy jazz_sse:;
                                 rdfs:label "Hardware Requirement".
    jazz_sse:HardwareRequirementsModule a jazz_rm:Module;
                                        rdfs:comment "A module for hardware requirements.";
                                        rdfs:isDefinedBy jazz_sse:;
                                        rdfs:label "Hardware Requirements Module".
    jazz_sse:Heading a rdfs:Class;
                     rdfs:comment "An artifact used as a heading in a strucured module.";
                     rdfs:isDefinedBy jazz_sse:;
                     rdfs:label "Heading".
    jazz_sse:HowFoundCustomer a jazz_sse:HowFoundValue;
                              rdfs:comment "Indicates a customer found the defect or issue.";
                              rdfs:isDefinedBy jazz_sse:;
                              rdfs:label "Customer".
    jazz_sse:HowFoundDevelopment a jazz_sse:HowFoundValue;
                                 rdfs:comment "Indicates the development team found the defect or issue.";
                                 rdfs:isDefinedBy jazz_sse:;
                                 rdfs:label "Development".
    jazz_sse:HowFoundTest a jazz_sse:HowFoundValue;
                          rdfs:comment "Indicates the test or QA team found the defect or issue.";
                          rdfs:isDefinedBy jazz_sse:;
                          rdfs:label "Test".
    jazz_sse:HowFoundUnknown a jazz_sse:HowFoundValue;
                             rdfs:comment "Indicates that the origin of the defect is not known or not defined.";
                             rdfs:isDefinedBy jazz_sse:;
                             rdfs:label "Unknown".
    jazz_sse:HowFoundValue a rdfs:Class;
                           rdfs:comment "Describes how a defect was found.";
                           rdfs:isDefinedBy jazz_sse:;
                           rdfs:label "How Found".
    jazz_sse:Information a rdfs:Class;
                         rdfs:comment "Artifact used to contain non-requirement content, such as instructions related to managing requirements or modules.";
                         rdfs:isDefinedBy jazz_sse:;
                         rdfs:label "Information".
    jazz_sse:NonFunctionalAccessibility a jazz_sse:NonFunctionalType;
                                        rdfs:comment "Requirement related to accessibility.";
                                        rdfs:isDefinedBy jazz_sse:;
                                        rdfs:label "Accessibility".
    jazz_sse:NonFunctionalAvailability a jazz_sse:NonFunctionalType;
                                       rdfs:comment "Requirement related to availability.";
                                       rdfs:isDefinedBy jazz_sse:;
                                       rdfs:label "Availability".
    jazz_sse:NonFunctionalCapacity a jazz_sse:NonFunctionalType;
                                   rdfs:comment "Requirement related to capacity.";
                                   rdfs:isDefinedBy jazz_sse:;
                                   rdfs:label "Capacity".
    jazz_sse:NonFunctionalCompliance a jazz_sse:NonFunctionalType;
                                     rdfs:comment "Requirement related to compliance.";
                                     rdfs:isDefinedBy jazz_sse:;
                                     rdfs:label "Compliance".
    jazz_sse:NonFunctionalInteroperability a jazz_sse:NonFunctionalType;
                                           rdfs:comment "Requirement related to interoperability.";
                                           rdfs:isDefinedBy jazz_sse:;
                                           rdfs:label "Interoperability".
    jazz_sse:NonFunctionalPerformance a jazz_sse:NonFunctionalType;
                                      rdfs:comment "Requirement related to performance.";
                                      rdfs:isDefinedBy jazz_sse:;
                                      rdfs:label "Performance".
    jazz_sse:NonFunctionalReliability a jazz_sse:NonFunctionalType;
                                      rdfs:comment "Requirement related to reliability.";
                                      rdfs:isDefinedBy jazz_sse:;
                                      rdfs:label "Reliability".
    jazz_sse:NonFunctionalRequirement a rdfs:Class;
                                      rdfs:comment "The Non-Functional Requirement (NFR) describes system attributes such as security, reliability, maintainability, scalability and usability (i.e. 'Utilities').";
                                      rdfs:isDefinedBy jazz_sse:;
                                      rdfs:label "Non-Functional Requirement".
    jazz_sse:NonFunctionalScalability a jazz_sse:NonFunctionalType;
                                      rdfs:comment "Requirement related to scalability.";
                                      rdfs:isDefinedBy jazz_sse:;
                                      rdfs:label "Scalability".
    jazz_sse:NonFunctionalSecurity a jazz_sse:NonFunctionalType;
                                   rdfs:comment "Requirement related to security.";
                                   rdfs:isDefinedBy jazz_sse:;
                                   rdfs:label "Security".
    jazz_sse:NonFunctionalSupportability a jazz_sse:NonFunctionalType;
                                         rdfs:comment "Requirement related to supportability.";
                                         rdfs:isDefinedBy jazz_sse:;
                                         rdfs:label "Supportability".
    jazz_sse:NonFunctionalType a rdfs:Class;
                               rdfs:comment "Types of non-functional requirements.";
                               rdfs:isDefinedBy jazz_sse:;
                               rdfs:label "Non-Functional Requirement Types".
    jazz_sse:NonfunctionalRequirementsModule a jazz_rm:Module;
                                             rdfs:comment "A module for nonfunctional requirements.";
                                             rdfs:isDefinedBy jazz_sse:;
                                             rdfs:label "Nonfunctional Requirements Module".
    jazz_sse:OriginCompetitiveAnalysis a jazz_sse:OriginValue;
                                       rdfs:comment "Originated from competition or competitive analysis.";
                                       rdfs:isDefinedBy jazz_sse:;
                                       rdfs:label "Competitive Analysis".
    jazz_sse:OriginCustomer a jazz_sse:OriginValue;
                            rdfs:comment "Originated from a customer.";
                            rdfs:isDefinedBy jazz_sse:;
                            rdfs:label "Customer".
    jazz_sse:OriginDevelopment a jazz_sse:OriginValue;
                               rdfs:comment "Originated from the development team.";
                               rdfs:isDefinedBy jazz_sse:;
                               rdfs:label "Development".
    jazz_sse:OriginLegal a jazz_sse:OriginValue;
                         rdfs:comment "Originated from a standard or legal contraint.";
                         rdfs:isDefinedBy jazz_sse:;
                         rdfs:label "Standards/Legal".
    jazz_sse:OriginMarketAnalysis a jazz_sse:OriginValue;
                                  rdfs:comment "Originated from marketing or market analysis.";
                                  rdfs:isDefinedBy jazz_sse:;
                                  rdfs:label "Market Analysis".
    jazz_sse:OriginPartner a jazz_sse:OriginValue;
                           rdfs:comment "Originated from one or more business partners.";
                           rdfs:isDefinedBy jazz_sse:;
                           rdfs:label "Partner".
    jazz_sse:OriginQA a jazz_sse:OriginValue;
                      rdfs:comment "Originated from the Quality assurance team.";
                      rdfs:isDefinedBy jazz_sse:;
                      rdfs:label "Quality Assurance".
    jazz_sse:OriginServices a jazz_sse:OriginValue;
                            rdfs:comment "Originated from the services team.";
                            rdfs:isDefinedBy jazz_sse:;
                            rdfs:label "Services".
    jazz_sse:OriginSupport a jazz_sse:OriginValue;
                           rdfs:comment "Originated from the Help Desk or support team.";
                           rdfs:isDefinedBy jazz_sse:;
                           rdfs:label "Support".
    jazz_sse:OriginValue a rdfs:Class;
                         rdfs:comment "Origin of a requirement or request.";
                         rdfs:isDefinedBy jazz_sse:;
                         rdfs:label "Origin".
    jazz_sse:ReleaseCollection a rdfs:Class;
                               rdfs:comment "A logical grouping of related artifacts specifically associated with a release.";
                               rdfs:isDefinedBy jazz_sse:;
                               rdfs:label "Release Collection".
    jazz_sse:RequestForChange a oslc_cm:ChangeRequest;
                              rdfs:comment "Request for a change to some aspect of the product.";
                              rdfs:isDefinedBy jazz_sse:;
                              rdfs:label "Change Request".
    jazz_sse:ReviewAnalysis a jazz_sse:ReviewMethod;
                            rdfs:comment "Review to be verified by analysis.";
                            rdfs:isDefinedBy jazz_sse:;
                            rdfs:label "Analysis".
    jazz_sse:ReviewAudit a jazz_sse:ReviewMethod;
                         rdfs:comment "Review to be verified by audit.";
                         rdfs:isDefinedBy jazz_sse:;
                         rdfs:label "Audit".
    jazz_sse:ReviewInspection a jazz_sse:ReviewMethod;
                              rdfs:comment "Review to be verified by inspection.";
                              rdfs:isDefinedBy jazz_sse:;
                              rdfs:label "Inspection".
    jazz_sse:ReviewMethod a rdfs:Class;
                          rdfs:comment "Verification methods used in review activities.";
                          rdfs:isDefinedBy jazz_sse:;
                          rdfs:label "Review Verification Methods".
    jazz_sse:ReviewPeer a jazz_sse:ReviewMethod;
                        rdfs:comment "Review to be verified by peer review.";
                        rdfs:isDefinedBy jazz_sse:;
                        rdfs:label "Peer review".
    jazz_sse:ReviewUnassigned a jazz_sse:ReviewMethod;
                              rdfs:comment "Review verification method has not been assigned.";
                              rdfs:isDefinedBy jazz_sse:;
                              rdfs:label "Unassigned".
    jazz_sse:ReviewWalkthrough a jazz_sse:ReviewMethod;
                               rdfs:comment "Review to be verified by a walkthrough.";
                               rdfs:isDefinedBy jazz_sse:;
                               rdfs:label "Walkthrough".
    jazz_sse:RiskCategory a rdfs:Class;
                          rdfs:comment "Category values for risks.";
                          rdfs:isDefinedBy jazz_sse:;
                          rdfs:label "Risk Categories".
    jazz_sse:RiskCompetitive a jazz_sse:RiskCategory;
                             rdfs:comment "Competitive risk.";
                             rdfs:isDefinedBy jazz_sse:;
                             rdfs:label "Competitive".
    jazz_sse:RiskDisposition a rdfs:Class;
                             rdfs:comment "Disposition of the resolved risk.";
                             rdfs:isDefinedBy jazz_sse:;
                             rdfs:label "Disposition".
    jazz_sse:RiskDispositionAvoided a jazz_sse:RiskDisposition;
                                    rdfs:comment "The risk has been avoided.";
                                    rdfs:isDefinedBy jazz_sse:;
                                    rdfs:label "Avoided".
    jazz_sse:RiskDispositionInvalid a jazz_sse:RiskDisposition;
                                    rdfs:comment "The risk is invalid.";
                                    rdfs:isDefinedBy jazz_sse:;
                                    rdfs:label "Invalid".
    jazz_sse:RiskDispositionTransferredShared a jazz_sse:RiskDisposition;
                                              rdfs:comment "The risk is transferred or shared with another team.";
                                              rdfs:isDefinedBy jazz_sse:;
                                              rdfs:label "Transferred/Shared".
    jazz_sse:RiskEconomic a jazz_sse:RiskCategory;
                          rdfs:comment "Economic risk.";
                          rdfs:isDefinedBy jazz_sse:;
                          rdfs:label "Economic".
    jazz_sse:RiskImpact a rdfs:Class;
                        rdfs:comment "Impact values associated with risks.";
                        rdfs:isDefinedBy jazz_sse:;
                        rdfs:label "Impact";
                        rdfs:seeAlso jazz_ccm:Impact.
    jazz_sse:RiskImpactBlocker a jazz_sse:RiskImpact;
                               rdfs:comment "The Risk is a blocker.";
                               rdfs:isDefinedBy jazz_sse:;
                               rdfs:label "100% - Blocker";
                               rdfs:seeAlso jazz_ccm:ImpactSignificant.
    jazz_sse:RiskImpactCritical a jazz_sse:RiskImpact;
                                rdfs:comment "The Risk has significant or critical impact.";
                                rdfs:isDefinedBy jazz_sse:;
                                rdfs:label "80% - Critical";
                                rdfs:seeAlso jazz_ccm:ImpactSignificant.
    jazz_sse:RiskImpactMajor a jazz_sse:RiskImpact;
                             rdfs:comment "The Risk has major impact.";
                             rdfs:isDefinedBy jazz_sse:;
                             rdfs:label "60% - Major";
                             rdfs:seeAlso jazz_ccm:ImpactMajor.
    jazz_sse:RiskImpactMinor a jazz_sse:RiskImpact;
                             rdfs:comment "The Risk has minor impact.";
                             rdfs:isDefinedBy jazz_sse:;
                             rdfs:label "20% - Minor";
                             rdfs:seeAlso jazz_ccm:ImpactMinor.
    jazz_sse:RiskImpactModerate a jazz_sse:RiskImpact;
                                rdfs:comment "The Risk has moderate impact.";
                                rdfs:isDefinedBy jazz_sse:;
                                rdfs:label "40% - Moderate";
                                rdfs:seeAlso jazz_ccm:ImpactModerate.
    jazz_sse:RiskMarket a jazz_sse:RiskCategory;
                        rdfs:comment "Market risk.";
                        rdfs:isDefinedBy jazz_sse:;
                        rdfs:label "Market".
    jazz_sse:RiskPolitical a jazz_sse:RiskCategory;
                           rdfs:comment "Political risk.";
                           rdfs:isDefinedBy jazz_sse:;
                           rdfs:label "Political".
    jazz_sse:RiskProbability a rdfs:Class;
                             rdfs:comment "Probability values for a risk occurring.";
                             rdfs:isDefinedBy jazz_sse:;
                             rdfs:label "Probability".
    jazz_sse:RiskProbabilityHigh a jazz_sse:RiskProbability;
                                 rdfs:comment "High probability that the risk will occur.";
                                 rdfs:isDefinedBy jazz_sse:;
                                 rdfs:label "80% - High".
    jazz_sse:RiskProbabilityLow a jazz_sse:RiskProbability;
                                rdfs:comment "Low probability that the risk will occur.";
                                rdfs:isDefinedBy jazz_sse:;
                                rdfs:label "40% - Low".
    jazz_sse:RiskProbabilityModerate a jazz_sse:RiskProbability;
                                     rdfs:comment "Moderate probability that the risk will occur.";
                                     rdfs:isDefinedBy jazz_sse:;
                                     rdfs:label "60% - Moderate".
    jazz_sse:RiskProbabilityVeryHigh a jazz_sse:RiskProbability;
                                     rdfs:comment "Very high probability that the risk will occur.";
                                     rdfs:isDefinedBy jazz_sse:;
                                     rdfs:label "100% - Very High".
    jazz_sse:RiskProbabilityVeryLow a jazz_sse:RiskProbability;
                                    rdfs:comment "Very low probability that the risk will occur.";
                                    rdfs:isDefinedBy jazz_sse:;
                                    rdfs:label "20% - Very Low".
    jazz_sse:RiskRegulatoryLegal a jazz_sse:RiskCategory;
                                 rdfs:comment "Regulatory/legal risk.";
                                 rdfs:isDefinedBy jazz_sse:;
                                 rdfs:label "Regulatory/legal".
    jazz_sse:RiskSocioCultural a jazz_sse:RiskCategory;
                               rdfs:comment "Socio-cultural risk.";
                               rdfs:isDefinedBy jazz_sse:;
                               rdfs:label "Socio-cultural".
    jazz_sse:RiskTechnology a jazz_sse:RiskCategory;
                            rdfs:comment "Technology risk.";
                            rdfs:isDefinedBy jazz_sse:;
                            rdfs:label "Technology".
    jazz_sse:RiskUncertainty a jazz_sse:RiskCategory;
                             rdfs:comment "Uncertainty risk.";
                             rdfs:isDefinedBy jazz_sse:;
                             rdfs:label "Uncertainty".
    jazz_sse:Role a rdfs:Class;
                  rdfs:comment "Describes a role that performs activities within the context of a scenario, for example, Systems Engineer, Product Owner, Architect, Software Engineer, Hardware Engineer.";
                  rdfs:isDefinedBy jazz_sse:;
                  rdfs:label "Role".
    jazz_sse:SoftwareArchitectureDesign a rdfs:Class;
                                        rdfs:comment "Represents the architectural design for the software of a system or product.";
                                        rdfs:isDefinedBy jazz_sse:;
                                        rdfs:label "Software Architecture Design".
    jazz_sse:SoftwareDetailedDesign a rdfs:Class;
                                    rdfs:comment "Represents the detailed architectural design for the software of a system or product.";
                                    rdfs:isDefinedBy jazz_sse:;
                                    rdfs:label "Software Detailed Design".
    jazz_sse:SoftwareRequirement a rdfs:Class;
                                 rdfs:comment "A requirement for software.";
                                 rdfs:isDefinedBy jazz_sse:;
                                 rdfs:label "Software Requirement".
    jazz_sse:SoftwareRequirementsModule a jazz_rm:Module;
                                        rdfs:comment "A module for software requirements.";
                                        rdfs:isDefinedBy jazz_sse:;
                                        rdfs:label "Software Requirements Module".
    jazz_sse:StakeholderRequirement a rdfs:Class;
                                    rdfs:comment "A requirement from the business or enterprise operations level (users, acquirers, customers, other stakeholders) as they relate to the problem or opportunity, that describe the solution required.";
                                    rdfs:isDefinedBy jazz_sse:;
                                    rdfs:label "Stakeholder Requirement".
    jazz_sse:StakeholderRequirementsModule a jazz_rm:Module;
                                           rdfs:comment "A module for stakeholder requirements.";
                                           rdfs:isDefinedBy jazz_sse:;
                                           rdfs:label "Stakeholder Requirements Module".
    jazz_sse:Standard a rdfs:Class;
                      rdfs:comment "A specific type of requirement that defines a regulatory or system constraint.";
                      rdfs:isDefinedBy jazz_sse:;
                      rdfs:label "Standard".
    jazz_sse:StateAccepted a oslc_cm:State;
                           rdfs:comment "Work has been successfully implemented and tested, and accepted by the business owner/stakeholder.";
                           rdfs:isDefinedBy jazz_sse:;
                           rdfs:label "Accepted";
                           skos:narrower oslc_cm:Approved.
    jazz_sse:StateAnalyzing a oslc_cm:State;
                            rdfs:comment "The artifact is being analyzed to understand vision, feasibility, cost, impact, iterative delivery and benefit.";
                            rdfs:isDefinedBy jazz_sse:;
                            rdfs:label "Analyzing";
                            skos:narrower oslc_cm:Inprogress.
    jazz_sse:StateDeprecated a oslc_cm:State;
                             rdfs:comment "The artifact or work defined has been deprecated and there might be a newer version of it.";
                             rdfs:isDefinedBy jazz_sse:;
                             rdfs:label "Deprecated";
                             skos:narrower oslc_cm:Closed.
    jazz_sse:StateDone a oslc_cm:State;
                       rdfs:comment "The artifact or work defined is completed and delivered.";
                       rdfs:isDefinedBy jazz_sse:;
                       rdfs:label "Done";
                       skos:narrower oslc_cm:Closed.
    jazz_sse:StateDraft a oslc_cm:State;
                        rdfs:comment "Initial state of the artifact.";
                        rdfs:isDefinedBy jazz_sse:;
                        rdfs:label "Draft";
                        skos:narrower oslc_cm:Inprogress.
    jazz_sse:StateImplementing a oslc_cm:State;
                               rdfs:comment "Work is allocated to one or more Value Streams or Programs.";
                               rdfs:isDefinedBy jazz_sse:;
                               rdfs:label "Implementing";
                               skos:narrower oslc_cm:Inprogress.
    jazz_sse:StateInDevelopment a oslc_cm:State;
                                rdfs:comment "Development work has started.";
                                rdfs:isDefinedBy jazz_sse:;
                                rdfs:label "In Development";
                                skos:narrower oslc_cm:Inprogress.
    jazz_sse:StateInTest a oslc_cm:State;
                         rdfs:comment "Development tasks are complete and code is delivered for testing.";
                         rdfs:isDefinedBy jazz_sse:;
                         rdfs:label "In Test";
                         skos:narrower oslc_cm:Inprogress.
    jazz_sse:StateInvalid a oslc_cm:State;
                          rdfs:comment "The artifact or work defined is not valid.";
                          rdfs:isDefinedBy jazz_sse:;
                          rdfs:label "Invalid";
                          skos:narrower oslc_cm:Closed.
    jazz_sse:StateNew a oslc_cm:State;
                      rdfs:comment "Initial state of the artifact.";
                      rdfs:isDefinedBy jazz_sse:;
                      rdfs:label "New";
                      skos:narrower oslc_cm:Inprogress.
    jazz_sse:StateObsolete a oslc_cm:State;
                           rdfs:comment "The artifact or work defined is obsolete.";
                           rdfs:isDefinedBy jazz_sse:;
                           rdfs:label "Obsolete";
                           skos:narrower oslc_cm:Closed.
    jazz_sse:StatePostponed a oslc_cm:State;
                            rdfs:comment "The artifact or work defined is postponed.";
                            rdfs:isDefinedBy jazz_sse:;
                            rdfs:label "Postponed";
                            skos:narrower oslc_cm:Closed.
    jazz_sse:StateReadyForApproval a oslc_cm:State;
                                   rdfs:comment "Analysis is completed and the epic is submitted for approval.";
                                   rdfs:isDefinedBy jazz_sse:;
                                   rdfs:label "Ready (for Approval)";
                                   skos:narrower oslc_cm:Inprogress.
    jazz_sse:StateRejected a oslc_cm:State;
                           rdfs:comment "The artifact or work defined is rejected and no further work will be done.";
                           rdfs:isDefinedBy jazz_sse:;
                           rdfs:label "Rejected";
                           skos:narrower oslc_cm:Closed.
    jazz_sse:StateResolved a oslc_cm:State;
                           rdfs:comment "The artifact or work defined is resolved.";
                           rdfs:isDefinedBy jazz_sse:;
                           rdfs:label "Resolved";
                           skos:narrower oslc_cm:Closed.
    jazz_sse:StateRetired a oslc_cm:State;
                          rdfs:comment "The artifact or work defined has been retired and is now closed.";
                          rdfs:isDefinedBy jazz_sse:;
                          rdfs:label "Retired";
                          skos:narrower oslc_cm:Closed.
    jazz_sse:StateReviewing a oslc_cm:State;
                            rdfs:comment "The artifact is being reviewed.";
                            rdfs:isDefinedBy jazz_sse:;
                            rdfs:label "Reviewing";
                            skos:narrower oslc_cm:Inprogress.
    jazz_sse:StateUnderReview a oslc_cm:State;
                              rdfs:comment "The artifact is under review reviewed.";
                              rdfs:isDefinedBy jazz_sse:;
                              rdfs:label "Under Review";
                              skos:narrower oslc_cm:Inprogress.
    jazz_sse:StateVerifying a oslc_cm:State;
                            rdfs:comment "A problem is in the process of being verified.";
                            rdfs:isDefinedBy jazz_sse:;
                            rdfs:label "Verifying";
                            skos:narrower oslc_cm:Inprogress.
    jazz_sse:SupportingResource a rdfs:Class;
                                rdfs:comment "An artifact that does not fit one of the other categories. A supporting resource will often be leveraged when uploading artifacts where one of the artifact types does not apply.";
                                rdfs:isDefinedBy jazz_sse:;
                                rdfs:label "Supporting Resource".
    jazz_sse:SystemArchitecture a rdfs:Class;
                                rdfs:comment "Represents the architecture of the overall system.";
                                rdfs:isDefinedBy jazz_sse:;
                                rdfs:label "System Architecture".
    jazz_sse:SystemRequirement a rdfs:Class;
                               rdfs:comment "An requirement describing a function that the system as a whole should fulfill to satisfy the stakeholder needs and requirements.";
                               rdfs:isDefinedBy jazz_sse:;
                               rdfs:label "System Requirement".
    jazz_sse:SystemRequirementsModule a jazz_rm:Module;
                                      rdfs:comment "A module for system requirements.";
                                      rdfs:isDefinedBy jazz_sse:;
                                      rdfs:label "System Requirements Module".
    jazz_sse:Term a rdfs:Class;
                  rdfs:comment "Captures phrases or words that require a description.";
                  rdfs:isDefinedBy jazz_sse:;
                  rdfs:label "Term".
    jazz_sse:UCPropertyAlternateFlow a jazz_sse:UseCasePropertyValues;
                                     rdfs:comment "Alternate flow property for a use case.";
                                     rdfs:isDefinedBy jazz_sse:;
                                     rdfs:label "Alternate Flow".
    jazz_sse:UCPropertyBasicFlow a jazz_sse:UseCasePropertyValues;
                                 rdfs:comment "Basic flow property for a use case.";
                                 rdfs:isDefinedBy jazz_sse:;
                                 rdfs:label "Basic Flow".
    jazz_sse:UCPropertyDescription a jazz_sse:UseCasePropertyValues;
                                   rdfs:comment "Brief description property for a use case.";
                                   rdfs:isDefinedBy jazz_sse:;
                                   rdfs:label "Brief Description".
    jazz_sse:UCPropertyName a jazz_sse:UseCasePropertyValues;
                            rdfs:comment "Name property for a use case.";
                            rdfs:isDefinedBy jazz_sse:;
                            rdfs:label "Name".
    jazz_sse:UCPropertyPostCondition a jazz_sse:UseCasePropertyValues;
                                     rdfs:comment "Post-condition property for a use case.";
                                     rdfs:isDefinedBy jazz_sse:;
                                     rdfs:label "Post-Condition".
    jazz_sse:UCPropertyPreCondition a jazz_sse:UseCasePropertyValues;
                                    rdfs:comment "Pre-condition property for a use case.";
                                    rdfs:isDefinedBy jazz_sse:;
                                    rdfs:label "Pre-Condition".
    jazz_sse:UCPropertySpecialRequirement a jazz_sse:UseCasePropertyValues;
                                          rdfs:comment "Special requirement property for a use case.";
                                          rdfs:isDefinedBy jazz_sse:;
                                          rdfs:label "Special Requirement".
    jazz_sse:UseCase a rdfs:Class;
                     rdfs:comment "The set of actions performed by a system, which yeilds an observable result that is, typically of value for one or more actors or other stakeholders of the system.";
                     rdfs:isDefinedBy jazz_sse:;
                     rdfs:label "Use Case".
    jazz_sse:UseCaseModule a jazz_rm:Module;
                           rdfs:comment "A module describing a particular use case.";
                           rdfs:isDefinedBy jazz_sse:;
                           rdfs:label "Use Case Module".
    jazz_sse:UseCasePropertyValues a rdfs:Class;
                                   rdfs:comment "Values for a use case property.";
                                   rdfs:isDefinedBy jazz_sse:;
                                   rdfs:label "Use Case Property Values".
    jazz_sse:UserRequirement a rdfs:Class;
                             rdfs:comment "A User Requirement specifically describes a capability required by end-users or customers. User Requirements are typically implemented by Features or Stories.";
                             rdfs:isDefinedBy jazz_sse:;
                             rdfs:label "User Requirement".
    jazz_sse:Vision a rdfs:Class;
                    rdfs:comment "The Vision is a description of the future state of the Solution under development. It reflects Customer and stakeholder needs, as well as the Feature and Capabilities, proposed to meet those needs.";
                    rdfs:isDefinedBy jazz_sse:;
                    rdfs:label "Vision".
    jazz_sse:accepted a rdf:Property;
                      rdfs:comment "Indicates whether or not the requirement or work has been accepted. Typically expressed as a boolean value.";
                      rdfs:isDefinedBy jazz_sse:;
                      rdfs:label "Accepted".
    jazz_sse:approvedBy a rdf:Property;
                        rdfs:comment "Approver of the artifact.";
                        rdfs:isDefinedBy jazz_sse:;
                        rdfs:label "Approved By".
    jazz_sse:approverPosition a rdf:Property;
                              rdfs:comment "Position of the person approving the artifact.";
                              rdfs:isDefinedBy jazz_sse:;
                              rdfs:label "Approver Position".
    jazz_sse:benefits a rdf:Property;
                      rdfs:comment "Benefits to be gained by implementing a change or cabability.";
                      rdfs:isDefinedBy jazz_sse:;
                      rdfs:label "Benefits".
    jazz_sse:changeReason a rdf:Property;
                          rdfs:comment "Reason for requesting a change.";
                          rdfs:isDefinedBy jazz_sse:;
                          rdfs:label "Change Reason".
    jazz_sse:checkItemStatus a rdf:Property;
                             rdfs:comment "The status of a check item in a checklist.";
                             rdfs:isDefinedBy jazz_sse:;
                             rdfs:label "Check Item Status";
                             rdfs:seeAlso jazz_sse:CheckItemStatusTypes.
    jazz_sse:constrains oslc:inverseLabel "Constrained By";
                        a rdf:Property;
                        rdfs:comment "Link type indicating that a requirement constrains another. For example, a non-functional requirement constrains a system requirement.";
                        rdfs:isDefinedBy jazz_sse:;
                        rdfs:label "Constrains".
    jazz_sse:contingencyPlan a rdf:Property;
                             rdfs:comment "Contingency plan for a risk.";
                             rdfs:isDefinedBy jazz_sse:;
                             rdfs:label "Contingency Plan".
    jazz_sse:customerApprovalStatus a rdf:Property;
                                    rdfs:comment "The approval status for a customer.";
                                    rdfs:isDefinedBy jazz_sse:;
                                    rdfs:label "Customer Approval Status";
                                    rdfs:seeAlso jazz_sse:ApprovalTypes.
    jazz_sse:defectDisposition a rdf:Property;
                               rdfs:comment "Indicates the disposition of a resolved defect (how it was resolved). Typically expressed as a value of type jazz_sse:DefectDisposition.";
                               rdfs:isDefinedBy jazz_sse:;
                               rdfs:label "Disposition";
                               rdfs:seeAlso jazz_sse:DefectDisposition.
    jazz_sse:dependsOn oslc:inverseLabel "Blocks";
                       a rdf:Property;
                       rdfs:comment "Shows dependency between requirements.";
                       rdfs:isDefinedBy jazz_sse:;
                       rdfs:label "Depends On".
    jazz_sse:derivesFrom oslc:inverseLabel "Derives To";
                         a rdf:Property;
                         rdfs:comment "Shows the derivation of lower level requirements from higher level requirements.";
                         rdfs:isDefinedBy jazz_sse:;
                         rdfs:label "Is Derived From".
    jazz_sse:estimatedCost a rdf:Property;
                           rdfs:comment "Estimated cost of delivery.";
                           rdfs:isDefinedBy jazz_sse:;
                           rdfs:label "Estimated Cost".
    jazz_sse:exposure a rdf:Property;
                      rdfs:comment "The risk exposure to the plan as a result of the risk identified.";
                      rdfs:isDefinedBy jazz_sse:;
                      rdfs:label "Exposure (%)".
    jazz_sse:howFound a rdf:Property;
                      rdfs:comment "Indicates how the defect was found. Typically expressed as a value of type jazz_sse:HowFound.";
                      rdfs:isDefinedBy jazz_sse:;
                      rdfs:label "How Found";
                      rdfs:seeAlso jazz_sse:HowFound.
    jazz_sse:identificationDate a rdf:Property;
                                rdfs:comment "Date when the risk was identified.";
                                rdfs:isDefinedBy jazz_sse:;
                                rdfs:label "Identification Date".
    jazz_sse:impact a rdf:Property;
                    rdfs:comment "Impact associated with a risk or change. Typically expressed as a value of type jazz_sse:RiskImpact.";
                    rdfs:isDefinedBy jazz_sse:;
                    rdfs:label "Impact";
                    rdfs:seeAlso jazz_sse:RiskImpact.
    jazz_sse:impactAssessment a rdf:Property;
                              rdfs:comment "Description of the impact of making the change.";
                              rdfs:isDefinedBy jazz_sse:;
                              rdfs:label "Impact Assessment".
    jazz_sse:impacts oslc:inverseLabel "Impacted By";
                     a rdf:Property;
                     rdfs:comment "Shows impacts, for example of a system requirement on other elements of the operating environment.";
                     rdfs:isDefinedBy jazz_sse:;
                     rdfs:label "Impacts".
    jazz_sse:integratesWith oslc:inverseLabel "Integrates with Software";
                            a rdf:Property;
                            rdfs:comment "Shows integration relationship between hardware and software requirements.";
                            rdfs:isDefinedBy jazz_sse:;
                            rdfs:label "Integrates with Hardware".
    jazz_sse:isBlocked a rdf:Property;
                       rdfs:comment "Indicates a 'soft dependency', that the work is blocked by some other required work.";
                       rdfs:isDefinedBy jazz_sse:;
                       rdfs:label "Blocked".
    jazz_sse:maturity a rdf:Property;
                      rdfs:comment "Assessed maturity of the artifact.";
                      rdfs:isDefinedBy jazz_sse:;
                      rdfs:label "Maturity";
                      rdfs:seeAlso jazz_sse:HMLScale.
    jazz_sse:mitigates oslc:inverseLabel "Mitigated By";
                       a rdf:Property;
                       rdfs:comment "Shows that a requirement mitigates another, such as in the case of a hazard or risk.";
                       rdfs:isDefinedBy jazz_sse:;
                       rdfs:label "Mitigates".
    jazz_sse:mitigationPlan a rdf:Property;
                            rdfs:comment "Plan to mitigate the risk.";
                            rdfs:isDefinedBy jazz_sse:;
                            rdfs:label "Mitigation Plan".
    jazz_sse:nonfunctionalType a rdf:Property;
                               rdfs:comment "Type or category of non-functional requirement, for example, usability, performance, serviceability. Can be expressed as a value of type jazz_sse:NonFunctionalType.";
                               rdfs:isDefinedBy jazz_sse:;
                               rdfs:label "Nonfunctional Type";
                               rdfs:seeAlso jazz_sse:NonFunctionalType.
    jazz_sse:occurrenceDate a rdf:Property;
                            rdfs:comment "Date when the risk actually occurred.";
                            rdfs:isDefinedBy jazz_sse:;
                            rdfs:label "Occurrence Date".
    jazz_sse:origin a rdf:Property;
                    rdfs:comment "Indicates where the requirement originated. Can be expressed as a value of type jazz_sse:OriginValue.";
                    rdfs:isDefinedBy jazz_sse:;
                    rdfs:label "Origin";
                    rdfs:seeAlso jazz_sse:OriginValue.
    jazz_sse:owner a rdf:Property;
                   rdfs:comment "Owner or responsible party for the artifact or action.";
                   rdfs:isDefinedBy jazz_sse:;
                   rdfs:label "Owner".
    jazz_sse:probability a rdf:Property;
                         rdfs:comment "Probability that a risk will occur. Typically expressed as a value of type jazz_sse:RiskProbability.";
                         rdfs:isDefinedBy jazz_sse:;
                         rdfs:label "Probability";
                         rdfs:seeAlso jazz_sse:RiskProbability.
    jazz_sse:reasonForBlock a rdf:Property;
                            rdfs:comment "Explanation of the 'soft dependency' that is blocking the work.";
                            rdfs:isDefinedBy jazz_sse:;
                            rdfs:label "Reason".
    jazz_sse:resourceRequirements a rdf:Property;
                                  rdfs:comment "Resources required to address a change request.";
                                  rdfs:isDefinedBy jazz_sse:;
                                  rdfs:label "Resource Requirements".
    jazz_sse:reviewCriteria a rdf:Property;
                            rdfs:comment "Specifies the verification criteria used to conduct a review.";
                            rdfs:isDefinedBy jazz_sse:;
                            rdfs:label "Verification Criteria".
    jazz_sse:reviewFindings a rdf:Property;
                            rdfs:comment "Documents any discovery or new findings as a result of a review.";
                            rdfs:isDefinedBy jazz_sse:;
                            rdfs:label "Review Findings".
    jazz_sse:reviewMethod a rdf:Property;
                          rdfs:comment "Indicates the method of review to be used. Can be expressed as a value of type jazz_sse:ReviewMethod.";
                          rdfs:isDefinedBy jazz_sse:;
                          rdfs:label "Verification Method";
                          rdfs:seeAlso jazz_sse:ReviewMethod.
    jazz_sse:reviewStakeholders a rdf:Property;
                                rdfs:comment "Parties who are interested in the review and its outcome, but are not reviewers.";
                                rdfs:isDefinedBy jazz_sse:;
                                rdfs:label "Review Stakeholders".
    jazz_sse:reviewers a rdf:Property;
                       rdfs:comment "Participants in the review.";
                       rdfs:isDefinedBy jazz_sse:;
                       rdfs:label "Reviewers".
    jazz_sse:riskCategory a rdf:Property;
                          rdfs:comment "Category or classification of the type of risk. Typically expressed as a value of type jazz_sse:RiskCategory.";
                          rdfs:isDefinedBy jazz_sse:;
                          rdfs:label "Risk Category";
                          rdfs:seeAlso jazz_sse:RiskCategory.
    jazz_sse:satisfies oslc:inverseLabel "Mitigated By";
                       a rdf:Property;
                       rdfs:comment "Shows that a requirement satisfies another requirement.";
                       rdfs:isDefinedBy jazz_sse:;
                       rdfs:label "Mitigates".
    jazz_sse:schedulingIssues a rdf:Property;
                              rdfs:comment "Scheduling issues associated with a change request.";
                              rdfs:isDefinedBy jazz_sse:;
                              rdfs:label "Scheduling Issues".
    jazz_sse:stability a rdf:Property;
                       rdfs:comment "Assessment of how stable the requirement is, as opposed to likely to change.";
                       rdfs:isDefinedBy jazz_sse:;
                       rdfs:label "Stability";
                       rdfs:seeAlso jazz_sse:HMLScale.
    jazz_sse:supplierApprovalStatus a rdf:Property;
                                    rdfs:comment "The approval status for a supplier.";
                                    rdfs:isDefinedBy jazz_sse:;
                                    rdfs:label "Supplier Approval Status";
                                    rdfs:seeAlso jazz_sse:ApprovalTypes.
    jazz_sse:testCaseCategoryTestType a rdf:Property;
                                      rdfs:comment "Category that indicates the type of the Test Case.";
                                      rdfs:isDefinedBy jazz_sse:;
                                      rdfs:label "Test Type".
    jazz_sse:testLevelIntegration a rdf:Property;
                                  rdfs:comment "Category that indicates testing is at the Integration Test level.";
                                  rdfs:isDefinedBy jazz_sse:;
                                  rdfs:label "Integration".
    jazz_sse:testLevelSystem a rdf:Property;
                             rdfs:comment "Category that indicates testing is at the System Test level.";
                             rdfs:isDefinedBy jazz_sse:;
                             rdfs:label "System".
    jazz_sse:testLevelUnit a rdf:Property;
                           rdfs:comment "Category that indicates testing is at the Unit Test level.";
                           rdfs:isDefinedBy jazz_sse:;
                           rdfs:label "Unit".
    jazz_sse:testLevelUserAcceptance a rdf:Property;
                                     rdfs:comment "Category that indicates testing is at the User Acceptance Test level.";
                                     rdfs:isDefinedBy jazz_sse:;
                                     rdfs:label "User Acceptance".
    jazz_sse:testObjectiveFinal a rdf:Property;
                                rdfs:comment "Category that indicates the Test Suite is for final testing.";
                                rdfs:isDefinedBy jazz_sse:;
                                rdfs:label "Final".
    jazz_sse:testObjectiveInitial a rdf:Property;
                                  rdfs:comment "Category that indicates the Test Suite is for initial testing.";
                                  rdfs:isDefinedBy jazz_sse:;
                                  rdfs:label "Initial".
    jazz_sse:testObjectiveRegression a rdf:Property;
                                     rdfs:comment "Category that indicates the Test Suite is for regression testing.";
                                     rdfs:isDefinedBy jazz_sse:;
                                     rdfs:label "Regression".
    jazz_sse:testObjectiveSmoke a rdf:Property;
                                rdfs:comment "Category that indicates the Test Suite is for smoke testing.";
                                rdfs:isDefinedBy jazz_sse:;
                                rdfs:label "Smoke".
    jazz_sse:testPlanCategoryTestLevel a rdf:Property;
                                       rdfs:comment "Category that indicates the level of testing involved.";
                                       rdfs:isDefinedBy jazz_sse:;
                                       rdfs:label "Test Level".
    jazz_sse:testSuiteCategoryTestObjective a rdf:Property;
                                            rdfs:comment "Category that indicates the objective of the Test Suites.";
                                            rdfs:isDefinedBy jazz_sse:;
                                            rdfs:label "Test Objective".
    jazz_sse:testTypeFunctional a rdf:Property;
                                rdfs:comment "Category that indicates a Functional Test Case.";
                                rdfs:isDefinedBy jazz_sse:;
                                rdfs:label "Functional".
    jazz_sse:testTypePerformance a rdf:Property;
                                 rdfs:comment "Category that indicates a Performance Test Case.";
                                 rdfs:isDefinedBy jazz_sse:;
                                 rdfs:label "Performance".
    jazz_sse:testTypeReliability a rdf:Property;
                                 rdfs:comment "Category that indicates a Reliability Test Case.";
                                 rdfs:isDefinedBy jazz_sse:;
                                 rdfs:label "Reliability".
    jazz_sse:testTypeSupportability a rdf:Property;
                                    rdfs:comment "Category that indicates a Supportability Test Case.";
                                    rdfs:isDefinedBy jazz_sse:;
                                    rdfs:label "Supportability".
    jazz_sse:testTypeUsability a rdf:Property;
                               rdfs:comment "Category that indicates a Usability Test Case.";
                               rdfs:isDefinedBy jazz_sse:;
                               rdfs:label "Usability".
    jazz_sse:ucProperty a rdf:Property;
                        rdfs:comment "Property of a use case. Typically expressed as a value of type jazz_sse:UseCasePropertyValues.";
                        rdfs:isDefinedBy jazz_sse:;
                        rdfs:label "Use Case Property";
                        rdfs:seeAlso jazz_sse:UseCasePropertyValues.
}

