@prefix : <http://www.semanticweb.org/owl/owlapi/turtle#> .
@prefix dc: <http://purl.org/dc/elements/1.1/> .
@prefix ex: <http://example.org/> .
@prefix om: <http://www.ontology-of-units-of-measure.org/resource/om-2/> .
@prefix sd: <http://www.w3.org/ns/sparql-service-description#> .
@prefix lis: <http://rds.posccaesar.org/ontology/lis14/rdl/> .
@prefix owl: <http://www.w3.org/2002/07/owl#> .
@prefix pav: <http://purl.org/pav/> .
@prefix pca: <http://data.posccaesar.org/rdl/> .
@prefix rdf: <http://www.w3.org/1999/02/22-rdf-syntax-ns#> .
@prefix rdl: <http://rds.posccaesar.org/ontology/plm/rdl/> .
@prefix req: <https://w3id.org/requirement-ontology/rdl/> .
@prefix xml: <http://www.w3.org/XML/1998/namespace> .
@prefix xsd: <http://www.w3.org/2001/XMLSchema#> .
@prefix foaf: <http://xmlns.com/foaf/0.1/> .
@prefix ntpl: <http://norsok.org/templates/> .
@prefix ottr: <http://ns.ottr.xyz/0.4/> .
@prefix rdfs: <http://www.w3.org/2000/01/rdf-schema#> .
@prefix rrdl: <http://w3id.org/readi/rdl/> .
@prefix rstr: <http://tpl.ottr.xyz/owl/restriction/0.1/> .
@prefix skos: <http://www.w3.org/2004/02/skos/core#> .
@prefix vann: <http://purl.org/vocab/vann/> .
@prefix void: <http://rdfs.org/ns/void#> .
@prefix o-rdf: <http://tpl.ottr.xyz/rdf/0.1/> .
@prefix orcid: <https://orcid.org/> .
@prefix listpl: <http://rds.posccaesar.org/ontology/lis14/tpl/0.1/> .
@prefix o-rdfs: <http://tpl.ottr.xyz/rdfs/0.1/> .
@prefix plmtpl: <http://rds.posccaesar.org/ontology/plm/tpl/0.1/> .
@prefix reqtpl: <http://w3id.org/requirement-ontology/tpl/0.1/> .
@prefix dcterms: <http://purl.org/dc/terms/> .
@prefix o-docttr: <http://tpl.ottr.xyz/p/docttr/0.1/> .
@prefix o-owl-ax: <http://tpl.ottr.xyz/owl/axiom/0.1/> .
@prefix o-owl-ma: <http://tpl.ottr.xyz/owl/macro/0.1/> .
@prefix o-owl-re: <http://tpl.ottr.xyz/owl/restriction/0.1/> .
@prefix o-owl-ut: <http://tpl.ottr.xyz/owl/util/0.1/> .
@prefix o-owl-dec: <http://tpl.ottr.xyz/owl/declaration/0.1/> .
@base <http://rds.posccaesar.org/ontology/plm/ont/norsok-z001> .

<http://rds.posccaesar.org/ontology/plm/ont/norsok-z001> rdf:type owl:Ontology ;
                                                          owl:versionIRI <http://rds.posccaesar.org/ontology/plm/ont/norsok-z001/0.1.1> ;
                                                          owl:imports <http://rds.posccaesar.org/ontology/plm/ont/document> ;
                                                          ottr:status ottr:incomplete ;
                                                          dc:creator <https://orcid.org/0000-0002-7167-7321> ;
                                                          dc:description "NORSOK Z-001 Information Item ontology" ;
                                                          dc:title "norsok-z001" ;
                                                          dcterms:issued "2022-05-02"^^xsd:date ;
                                                          dcterms:modified "2022-09-26"^^xsd:date ;
                                                          dcterms:publisher <http://www.posccaesar.org/> ;
                                                          pav:createdBy <https://orcid.org/0000-0002-7167-7321> ;
                                                          pav:hasPreviousVersion <http://rds.posccaesar.org/ontology/plm/ont/norsok-z001/0.1.0> ;
                                                          pav:lastUpdateOn "2022-09-26T23:40:00Z"^^xsd:dateTime ;
                                                          vann:preferredNamespacePrefix "rdl" ;
                                                          vann:preferredNamespaceUri rdl: ;
                                                          void:feature <http://www.w3.org/ns/formats/JSON-LD> ,
                                                                       <http://www.w3.org/ns/formats/N-Triples> ,
                                                                       <http://www.w3.org/ns/formats/OWL_Manchester> ,
                                                                       <http://www.w3.org/ns/formats/RDF_XML> ,
                                                                       <http://www.w3.org/ns/formats/Turtle> ;
                                                          void:sparqlEndpoint <https://rds.posccaesar.org/ontology/sparql> ;
                                                          rdfs:comment "NORSOK Z-001 Information Item ontology" ;
                                                          rdfs:label "norsok-z001" ;
                                                          owl:versionInfo "0.1.1" ;
                                                          skos:changeNote "Z-001 Item collection" .

#################################################################
#    Annotation properties
#################################################################

###  http://www.w3.org/2004/02/skos/core#broadMatch
skos:broadMatch rdf:type owl:AnnotationProperty .


###  http://www.w3.org/2004/02/skos/core#broader
skos:broader rdf:type owl:AnnotationProperty .


###  http://www.w3.org/2004/02/skos/core#member
skos:member rdf:type owl:AnnotationProperty .


#################################################################
#    Classes
#################################################################

###  http://rds.posccaesar.org/ontology/plm/rdl/PCA_100006078
rdl:PCA_100006078 rdf:type owl:Class ;
                  rdfs:subClassOf rdl:PCA_100004908 ;
                  rdl:PCA_100006763 "The documentation enabling visualisation of design and easier verification of design, dimensions, space (envelopes) and interfaces." ;
                  rdl:PCA_100006764 "The model must be complete in order to check interface and possible interference with other equipments. All final dimensions and external geometry must be defined in the 3D model. Weight and center of gravity shall be defined in the 3D model and in the assembly drawing." ;
                  rdl:PCA_100006766 rdl:PCA_100006656 ;
                  rdl:PCA_100006768 "The 3D model shall be prepared according to Company's requirements." ;
                  rdfs:comment "The 3D model shall be prepared according to Company's requirements." ;
                  rdfs:label "3D CAD model - offshore, onshore and subsea" ;
                  skos:broadMatch rdl:PCA_100006707 ,
                                  rdl:PCA_100006708 ,
                                  rdl:PCA_100006709 ,
                                  rdl:PCA_100006710 ,
                                  rdl:PCA_100006731 ,
                                  rdl:PCA_100006732 ;
                  skos:broader rdl:PCA_100006738 .


###  http://rds.posccaesar.org/ontology/plm/rdl/PCA_100006079
rdl:PCA_100006079 rdf:type owl:Class ;
                  rdfs:subClassOf rdl:PCA_100004908 ;
                  rdl:PCA_100006765 rrdl:CFIHOS-20000010 ,
                                    rrdl:CFIHOS-20000011 ,
                                    rrdl:CFIHOS-20000013 ;
                  rdl:PCA_100006766 rdl:PCA_100006656 ;
                  rdl:PCA_100006768 "The Noise Simulation Model shall include all noise sources, piping and reflection from adjacent equipment and structure (walls, floor, ceiling, etc). Noise reducing measures, as absorption, noise hoods, etc. shall be included in the simulation model. The software to be used requires use of point sources, line sources, areas sources and box sources, both directly from sources and from reflections. The handover format to be agreed. All necessary files to run the model shall be handed over, including maps and/or plot plans." ;
                  rdfs:comment "The Noise Simulation Model shall include all noise sources, piping and reflection from adjacent equipment and structure (walls, floor, ceiling, etc). Noise reducing measures, as absorption, noise hoods, etc. shall be included in the simulation model. The software to be used requires use of point sources, line sources, areas sources and box sources, both directly from sources and from reflections. The handover format to be agreed. All necessary files to run the model shall be handed over, including maps and/or plot plans." ;
                  rdfs:label "3D noise simulation model" ;
                  skos:broadMatch rdl:PCA_100006707 ,
                                  rdl:PCA_100006708 ,
                                  rdl:PCA_100006709 ,
                                  rdl:PCA_100006710 ,
                                  rdl:PCA_100006731 ,
                                  rdl:PCA_100006732 ;
                  skos:broader rdl:PCA_100006738 .


###  http://rds.posccaesar.org/ontology/plm/rdl/PCA_100006080
rdl:PCA_100006080 rdf:type owl:Class ;
                  rdfs:subClassOf rdl:PCA_100004908 ;
                  rdl:PCA_100006766 rdl:PCA_100006656 ;
                  rdl:PCA_100006768 "A view model in as-built status of all structures in adequate details, including panels, pipeline, cabling,\ntees, wyes and valves, for intervention/inspection activities during operations shall be delivered" ;
                  rdfs:comment "A view model in as-built status of all structures in adequate details, including panels, pipeline, cabling,\ntees, wyes and valves, for intervention/inspection activities during operations shall be delivered" ;
                  rdfs:label "3D view model" ;
                  skos:broadMatch rdl:PCA_100006732 ;
                  skos:broader rdl:PCA_100006738 .


###  http://rds.posccaesar.org/ontology/plm/rdl/PCA_100006081
rdl:PCA_100006081 rdf:type owl:Class ;
                  rdfs:subClassOf rdl:PCA_100004908 ;
                  rdl:PCA_100006763 "These drawings shall be based on equipment layout drawings or architectural layout drawings and shall include acoustic insulation, thermal insulation and fire protection details" ;
                  rdl:PCA_100006765 rrdl:CFIHOS-20000003 ;
                  rdl:PCA_100006766 rdl:PCA_100006654 ;
                  rdl:PCA_100006768 "These drawings shall be based on equipment layout drawings or architectural layout drawings and shall include acoustic insulation, thermal insulation and fire protection details as follows: \n - All doors and windows;\n - All insulation in ceiling, floors and walls;\n - Blast/fire walls;\n - All penetrations in blast/fire wall." ;
                  rdfs:comment "These drawings shall be based on equipment layout drawings or architectural layout drawings and shall include acoustic insulation, thermal insulation and fire protection details as follows: \n - All doors and windows;\n - All insulation in ceiling, floors and walls;\n - Blast/fire walls;\n - All penetrations in blast/fire wall." ;
                  rdfs:label "Acoustic/thermal insulation and fire protection plan" ;
                  skos:broadMatch rdl:PCA_100006707 ,
                                  rdl:PCA_100006729 ;
                  skos:broader rdl:PCA_100006753 .


###  http://rds.posccaesar.org/ontology/plm/rdl/PCA_100006082
rdl:PCA_100006082 rdf:type owl:Class ;
                  rdfs:subClassOf rdl:PCA_100004908 ;
                  rdl:PCA_100006763 "Documentation shall be in accordance with requirements in ISO21905." ;
                  rdl:PCA_100006765 rrdl:CFIHOS-20000021 ,
                                    rrdl:CFIHOS-20000022 ,
                                    rrdl:CFIHOS-20000023 ;
                  rdfs:label "Additional documentation for gas turbine exhaust systems" .


###  http://rds.posccaesar.org/ontology/plm/rdl/PCA_100006083
rdl:PCA_100006083 rdf:type owl:Class ;
                  rdfs:subClassOf rdl:PCA_100004908 ;
                  rdl:PCA_100006766 rdl:PCA_100006654 ;
                  rdl:PCA_100006768 "All additional studies required for the specific scope for the project/plant shall be delivered. This may include:\n - Technology qualification studies;\n - 3rd party studies, e.g. special studies and verification studies.\nThese studies shall be delivered as LCI also when performed in project phases prior to the execution phase." ;
                  rdfs:comment "All additional studies required for the specific scope for the project/plant shall be delivered. This may include:\n - Technology qualification studies;\n - 3rd party studies, e.g. special studies and verification studies.\nThese studies shall be delivered as LCI also when performed in project phases prior to the execution phase." ;
                  rdfs:label "Additional studies" .


###  http://rds.posccaesar.org/ontology/plm/rdl/PCA_100006084
rdl:PCA_100006084 rdf:type owl:Class ;
                  rdfs:subClassOf rdl:PCA_100004908 ;
                  rdl:PCA_100006763 "Air distribution diagrams (HVAC flow diagrams) shall be provided per system" ;
                  rdl:PCA_100006765 rrdl:CFIHOS-20000019 ;
                  rdl:PCA_100006766 rdl:PCA_100006650 ;
                  rdl:PCA_100006768 "Air distribution diagrams (HVAC flow diagrams) shall be provided per system and include the following information: \n - Tag codes for supply and extract fans (air handling units);\n - Flow rates for supply and extract fans (air handling units);\n - Flow rates for all serviced areas and air flows necessary for system balancing;\n - Temperature range requirements for all serviced areas;\n - Air change rates for all serviced areas;\n - HVAC noise range requirements for all serviced areas;\n - Area code and description for fan rooms and serviced areas;\n - Notes regarding main design parameters, such as fan standby philosophy, emergency operation, shall be given." ;
                  rdfs:comment "Air distribution diagrams (HVAC flow diagrams) shall be provided per system and include the following information: \n - Tag codes for supply and extract fans (air handling units);\n - Flow rates for supply and extract fans (air handling units);\n - Flow rates for all serviced areas and air flows necessary for system balancing;\n - Temperature range requirements for all serviced areas;\n - Air change rates for all serviced areas;\n - HVAC noise range requirements for all serviced areas;\n - Area code and description for fan rooms and serviced areas;\n - Notes regarding main design parameters, such as fan standby philosophy, emergency operation, shall be given." ;
                  rdfs:label "Air flow diagrams" ;
                  skos:broadMatch rdl:PCA_100006696 ;
                  skos:broader rdl:PCA_100006745 .


###  http://rds.posccaesar.org/ontology/plm/rdl/PCA_100006085
rdl:PCA_100006085 rdf:type owl:Class ;
                  rdfs:subClassOf rdl:PCA_100004908 ;
                  rdl:PCA_100006763 "The context and hiding charts shall be prepared as a matrix between initiating and actuated elements to be hidden. Both initiating and hidden elements shall be identified by ENS tag numbers." ;
                  rdl:PCA_100006765 rrdl:CFIHOS-20000015 ;
                  rdl:PCA_100006766 rdl:PCA_100006626 ,
                                    rdl:PCA_100006627 ,
                                    rdl:PCA_100006628 ,
                                    rdl:PCA_100006633 ;
                  rdl:PCA_100006768 "The context and hiding charts shall be prepared as a matrix between initiating and actuated elements to be hidden. Both initiating and hidden elements shall be identified by ENS tag numbers." ;
                  rdfs:comment "The context and hiding charts shall be prepared as a matrix between initiating and actuated elements to be hidden. Both initiating and hidden elements shall be identified by ENS tag numbers." ;
                  rdfs:label "Alarm C&H (context & hiding)" ;
                  skos:broadMatch rdl:PCA_100006699 ;
                  skos:broader rdl:PCA_100006748 .


###  http://rds.posccaesar.org/ontology/plm/rdl/PCA_100006086
rdl:PCA_100006086 rdf:type owl:Class ;
                  rdfs:subClassOf rdl:PCA_100004908 ;
                  rdl:PCA_100006763 "A list containing necessary information for alarm handling such that it can be understood and handled in time for required safe operations of equipment." ;
                  rdl:PCA_100006765 rrdl:CFIHOS-20000015 ,
                                    rrdl:CFIHOS-20000031 ;
                  rdl:PCA_100006766 rdl:PCA_100006626 ,
                                    rdl:PCA_100006627 ,
                                    rdl:PCA_100006628 ,
                                    rdl:PCA_100006633 ,
                                    rdl:PCA_100006634 ,
                                    rdl:PCA_100006635 ,
                                    rdl:PCA_100006636 ,
                                    rdl:PCA_100006637 ,
                                    rdl:PCA_100006638 ,
                                    rdl:PCA_100006639 ,
                                    rdl:PCA_100006640 ,
                                    rdl:PCA_100006641 ;
                  rdl:PCA_100006768 "A list suggesting alarms and alarm priorities based on signals from equipment. Alarms shall be documented in accordance with IEC 62682 Ch 9 Rationalization." ;
                  rdfs:comment "A list suggesting alarms and alarm priorities based on signals from equipment. Alarms shall be documented in accordance with IEC 62682 Ch 9 Rationalization." ;
                  rdfs:label "Alarm classification" ;
                  skos:broadMatch rdl:PCA_100006700 ;
                  skos:broader rdl:PCA_100006748 .


###  http://rds.posccaesar.org/ontology/plm/rdl/PCA_100006087
rdl:PCA_100006087 rdf:type owl:Class ;
                  rdfs:subClassOf rdl:PCA_100004908 ;
                  rdl:PCA_100006763 "The ALARP register should be established to keep track of identification, evaluation and decision regarding risk reducing measures." ;
                  rdl:PCA_100006765 rrdl:CFIHOS-20000010 ,
                                    rrdl:CFIHOS-20000011 ,
                                    rrdl:CFIHOS-20000013 ;
                  rdl:PCA_100006766 rdl:PCA_100006626 ,
                                    rdl:PCA_100006627 ,
                                    rdl:PCA_100006628 ,
                                    rdl:PCA_100006629 ,
                                    rdl:PCA_100006630 ,
                                    rdl:PCA_100006631 ,
                                    rdl:PCA_100006632 ,
                                    rdl:PCA_100006633 ;
                  rdl:PCA_100006768 "An ALARP register could contain the following information fields:\n - Unique identification number;\n - Source of identification, e.g. Hazop;\n - Cross reference to other databases/registers, for instance the uncertainty management register;\n - Description of the hazard/risk to be prevented or mitigated;\n - Description of the risk reducing measure;\n - Relevant DSHA(s);\n - Relevant safety barrier(s);\n - Coarse risk evaluation;\n - Decision based on coarse risk evaluation;\n - Date and signature for coarse risk evaluation/decision;\n - Detailed risk evaluation, if applicable;\n - Decision based on detailed risk evaluation, if applicable;\n - Date and signature for detailed risk evaluation/decision, if applicable." ;
                  rdfs:comment "An ALARP register could contain the following information fields:\n - Unique identification number;\n - Source of identification, e.g. Hazop;\n - Cross reference to other databases/registers, for instance the uncertainty management register;\n - Description of the hazard/risk to be prevented or mitigated;\n - Description of the risk reducing measure;\n - Relevant DSHA(s);\n - Relevant safety barrier(s);\n - Coarse risk evaluation;\n - Decision based on coarse risk evaluation;\n - Date and signature for coarse risk evaluation/decision;\n - Detailed risk evaluation, if applicable;\n - Decision based on detailed risk evaluation, if applicable;\n - Date and signature for detailed risk evaluation/decision, if applicable." ;
                  rdfs:label "ALARP register" ;
                  skos:broadMatch rdl:PCA_100006726 ,
                                  rdl:PCA_100006727 ;
                  skos:broader rdl:PCA_100006748 .


###  http://rds.posccaesar.org/ontology/plm/rdl/PCA_100006088
rdl:PCA_100006088 rdf:type owl:Class ;
                  rdfs:subClassOf rdl:PCA_100004908 ;
                  rdl:PCA_100006763 "The report or collection of reports shall contain the final documentation of the anchors." ;
                  rdl:PCA_100006765 rrdl:CFIHOS-20000033 ;
                  rdl:PCA_100006766 rdl:PCA_100006647 ;
                  rdl:PCA_100006768 "Anchor design reports shall be delivered. The report or collection of reports shall contain the final documentation of the anchors. The report shall typically contain: \n - Geotechnical report;\n - Structural design report;\n - Arrangement and detail drawings." ;
                  rdfs:comment "Anchor design reports shall be delivered. The report or collection of reports shall contain the final documentation of the anchors. The report shall typically contain: \n - Geotechnical report;\n - Structural design report;\n - Arrangement and detail drawings." ;
                  rdfs:label "Anchor design reports" ;
                  skos:broadMatch rdl:PCA_100006691 ,
                                  rdl:PCA_100006698 ;
                  skos:broader rdl:PCA_100006756 .


###  http://rds.posccaesar.org/ontology/plm/rdl/PCA_100006089
rdl:PCA_100006089 rdf:type owl:Class ;
                  rdfs:subClassOf rdl:PCA_100004908 ;
                  rdl:PCA_100006763 "To give an overview of location of the anodes on equipment" ;
                  rdl:PCA_100006765 rrdl:CFIHOS-20000006 ;
                  rdl:PCA_100006766 rdl:PCA_100006653 ;
                  rdl:PCA_100006768 "Drawing of anodes shall be provided for the structural discipline with the following information: \n - Location where the anode is attached;\n - Number off;\n - Type/weight/dimension;\n - Attachment to structure." ;
                  rdfs:comment "Drawing of anodes shall be provided for the structural discipline with the following information: \n - Location where the anode is attached;\n - Number off;\n - Type/weight/dimension;\n - Attachment to structure." ;
                  rdfs:label "Anode details and layout" ;
                  skos:broadMatch rdl:PCA_100006732 ,
                                  rdl:PCA_100006733 ,
                                  rdl:PCA_100006734 ;
                  skos:broader rdl:PCA_100006746 .


###  http://rds.posccaesar.org/ontology/plm/rdl/PCA_100006090
rdl:PCA_100006090 rdf:type owl:Class ;
                  rdfs:subClassOf rdl:PCA_100004908 ;
                  rdl:PCA_100006763 "An index describing the scope of Anodes for an installation, and reference related information." ;
                  rdl:PCA_100006765 rrdl:CFIHOS-20000031 ;
                  rdl:PCA_100006766 rdl:PCA_100006653 ;
                  rdl:PCA_100006768 "An anode/reference electrode index shall be provided containing the following information:\n - Anode/ref. electrode type (unique reference to applicable anode/ref. electrode datasheet);\n - Data sheet number (data sheet to include details of dimensions, weight, Ex. cert., potential (max/min), sacrificial material, steel insert quality;\n - PO number;\n - Manufacturer;\n - Manufacturer type;\n - Location;\n - Identification reference; cross reference to layout drawing for anode/ref. electrode;\n - Layout drawing number." ;
                  rdfs:comment "An anode/reference electrode index shall be provided containing the following information:\n - Anode/ref. electrode type (unique reference to applicable anode/ref. electrode datasheet);\n - Data sheet number (data sheet to include details of dimensions, weight, Ex. cert., potential (max/min), sacrificial material, steel insert quality;\n - PO number;\n - Manufacturer;\n - Manufacturer type;\n - Location;\n - Identification reference; cross reference to layout drawing for anode/ref. electrode;\n - Layout drawing number." ;
                  rdfs:label "Anode index" ;
                  skos:broadMatch rdl:PCA_100006716 ,
                                  rdl:PCA_100006717 ,
                                  rdl:PCA_100006718 ;
                  skos:broader rdl:PCA_100006748 .


###  http://rds.posccaesar.org/ontology/plm/rdl/PCA_100006091
rdl:PCA_100006091 rdf:type owl:Class ;
                  rdfs:subClassOf rdl:PCA_100004908 ;
                  rdl:PCA_100006765 rrdl:CFIHOS-20000030 ;
                  rdl:PCA_100006766 rdl:PCA_100006653 ;
                  rdl:PCA_100006768 "Antenna tower layout drawings shall be provided. Drawings shall include location of antennas in antenna tower, the type of antenna, associated equipment and the vertical and horizontal distance between the different antennas." ;
                  rdfs:comment "Antenna tower layout drawings shall be provided. Drawings shall include location of antennas in antenna tower, the type of antenna, associated equipment and the vertical and horizontal distance between the different antennas." ;
                  rdfs:label "Antenna tower layout drawings" ;
                  skos:broadMatch rdl:PCA_100006710 ;
                  skos:broader rdl:PCA_100006746 .


###  http://rds.posccaesar.org/ontology/plm/rdl/PCA_100006092
rdl:PCA_100006092 rdf:type owl:Class ;
                  rdfs:subClassOf rdl:PCA_100004908 ;
                  rdl:PCA_100006765 rrdl:CFIHOS-20000003 ;
                  rdl:PCA_100006766 rdl:PCA_100006656 ;
                  rdl:PCA_100006768 "Architectural layout drawings (plans and elevations) shall be produced for all architectural areas (living quarters, CCR, stores, workshops, etc.). The drawing scale shall normally be 1:100 on A3 format. However larger scales can be selected if required. The drawings shall include stairs, walls, doors, windows, furniture, access and escape routes and all tagged equipment.\n\nMain dimensions shall be included. Elevations of all floors and platforms etc. shall be shown. Room areas shall be included. The area shall be noted in m2 and be positioned adjacent to or directly under the room or area name. A key plan, grid lines with north and east references and match lines with drawing references shall be included. Drawings from adjacent areas shall be referenced." ;
                  rdfs:comment "Architectural layout drawings (plans and elevations) shall be produced for all architectural areas (living quarters, CCR, stores, workshops, etc.). The drawing scale shall normally be 1:100 on A3 format. However larger scales can be selected if required. The drawings shall include stairs, walls, doors, windows, furniture, access and escape routes and all tagged equipment.\n\nMain dimensions shall be included. Elevations of all floors and platforms etc. shall be shown. Room areas shall be included. The area shall be noted in m2 and be positioned adjacent to or directly under the room or area name. A key plan, grid lines with north and east references and match lines with drawing references shall be included. Drawings from adjacent areas shall be referenced." ;
                  rdfs:label "Architectural layout drawings" ;
                  skos:broadMatch rdl:PCA_100006710 ;
                  skos:broader rdl:PCA_100006746 .


###  http://rds.posccaesar.org/ontology/plm/rdl/PCA_100006093
rdl:PCA_100006093 rdf:type owl:Class ;
                  rdfs:subClassOf rdl:PCA_100004908 ;
                  rdl:PCA_100006764 "Area classification drawings should be based on Safety layout drawings" ;
                  rdl:PCA_100006765 rrdl:CFIHOS-20000010 ,
                                    rrdl:CFIHOS-20000011 ,
                                    rrdl:CFIHOS-20000013 ;
                  rdl:PCA_100006766 rdl:PCA_100006656 ;
                  rdl:PCA_100006768 "Fire walls, other gas tight barriers, hazardous area classification of zones and each fire area to be shown with fire area identification. All air intakes and ventilation air outlets to/from all areas shall be shown on the area classification drawings. All sources of releases shall be identified. Area classification drawings shall be scaled and prepared in accordance with regulatory requirements for area classification." ;
                  rdfs:comment "Fire walls, other gas tight barriers, hazardous area classification of zones and each fire area to be shown with fire area identification. All air intakes and ventilation air outlets to/from all areas shall be shown on the area classification drawings. All sources of releases shall be identified. Area classification drawings shall be scaled and prepared in accordance with regulatory requirements for area classification." ;
                  rdfs:label "Area classification drawings" ;
                  skos:broadMatch rdl:PCA_100006727 ;
                  skos:broader rdl:PCA_100006746 .


###  http://rds.posccaesar.org/ontology/plm/rdl/PCA_100006094
rdl:PCA_100006094 rdf:type owl:Class ;
                  rdfs:subClassOf rdl:PCA_100004908 ;
                  rdl:PCA_100006765 rrdl:CFIHOS-20000010 ,
                                    rrdl:CFIHOS-20000011 ,
                                    rrdl:CFIHOS-20000013 ;
                  rdl:PCA_100006766 rdl:PCA_100006656 ;
                  rdl:PCA_100006768 "The Area classification source of release shall describe all sources of release, medium causing hazardous area, extent of hazardous area from the release source, ventilation conditions for the area. The Area classification source of release shall be prepared in accordance with recognized area classification standards.  Examples of Area classification source of release can be found in IEC60079 and IP15." ;
                  rdfs:comment "The Area classification source of release shall describe all sources of release, medium causing hazardous area, extent of hazardous area from the release source, ventilation conditions for the area. The Area classification source of release shall be prepared in accordance with recognized area classification standards.  Examples of Area classification source of release can be found in IEC60079 and IP15." ;
                  rdfs:label "Area classification source of release" ;
                  skos:broadMatch rdl:PCA_100006687 ,
                                  rdl:PCA_100006727 ;
                  skos:broader rdl:PCA_100006756 .


###  http://rds.posccaesar.org/ontology/plm/rdl/PCA_100006095
rdl:PCA_100006095 rdf:type owl:Class ;
                  rdfs:subClassOf rdl:PCA_100004908 ;
                  rdl:PCA_100006765 rrdl:CFIHOS-20000019 ;
                  rdl:PCA_100006766 rdl:PCA_100006650 ;
                  rdl:PCA_100006768 "The complete Area Duct & and Instrumentation Diagrams (D&ID) shall be in accordance with the plants’ process typicals and drafting standard.\n\nThe level of detail within packages shall be identical to that outside.\nTag number shall be shown for all tagged components including manual valves.\n\nArea Duct & Instrumentation Diagram (D&ID) shall be provided by area and include the following information:\n - All relevant HVAC system within the defined area;\n - All HVAC equipment with their tag number and all HVAC bulk items with their item number;\n - Equipment data summary with tag number for all equipment such as filters, fans, coils, etc.;\n - All ductwork identified with system no., sizes, duct classes, insulation classes;\n - All inline equipment;\n - Air flow to all serviced areas;\n - Area breaks and duct class breaks;\n - All areas/rooms served to be identified;\n - All instrument locations shall be indicated and completed with tag numbers;\n - Connections to other systems e.g. sea water, heating, cooling, drain, etc.;\n - Airflow in and out of diagram with references;\n - Fire partitions with fire rating." ;
                  rdfs:comment "The complete Area Duct & and Instrumentation Diagrams (D&ID) shall be in accordance with the plants’ process typicals and drafting standard.\n\nThe level of detail within packages shall be identical to that outside.\nTag number shall be shown for all tagged components including manual valves.\n\nArea Duct & Instrumentation Diagram (D&ID) shall be provided by area and include the following information:\n - All relevant HVAC system within the defined area;\n - All HVAC equipment with their tag number and all HVAC bulk items with their item number;\n - Equipment data summary with tag number for all equipment such as filters, fans, coils, etc.;\n - All ductwork identified with system no., sizes, duct classes, insulation classes;\n - All inline equipment;\n - Air flow to all serviced areas;\n - Area breaks and duct class breaks;\n - All areas/rooms served to be identified;\n - All instrument locations shall be indicated and completed with tag numbers;\n - Connections to other systems e.g. sea water, heating, cooling, drain, etc.;\n - Airflow in and out of diagram with references;\n - Fire partitions with fire rating." ;
                  rdfs:label "Area duct & and instrumentation diagrams (D&ID)" ;
                  skos:broadMatch rdl:PCA_100006696 ;
                  skos:broader rdl:PCA_100006745 .


###  http://rds.posccaesar.org/ontology/plm/rdl/PCA_100006096
rdl:PCA_100006096 rdf:type owl:Class ;
                  rdfs:subClassOf rdl:PCA_100004908 ;
                  rdl:PCA_100006763 "Drawing documenting the changes between issued for construction and as- built version of the product. Not used for standard and non-engineered products." ;
                  rdl:PCA_100006764 "An As-built drawing is a red-marked up and stamped copy of the IFC version of an drawing, that will be part of the MRB." ;
                  rdl:PCA_100006765 rrdl:CFIHOS-20000031 ;
                  rdl:PCA_100006766 rdl:PCA_100006653 ;
                  rdl:PCA_100006768 "To document actual manufacturing with reference to individual serial number." ;
                  rdfs:comment "To document actual manufacturing with reference to individual serial number." ;
                  rdfs:label "As-built drawings (info)" ;
                  skos:broadMatch rdl:PCA_100006733 ;
                  skos:broader rdl:PCA_100006746 .


###  http://rds.posccaesar.org/ontology/plm/rdl/PCA_100006097
rdl:PCA_100006097 rdf:type owl:Class ;
                  rdfs:subClassOf rdl:PCA_100004908 ;
                  rdl:PCA_100006763 "A drawing including an overview of main parts of the equipment used for manufacturing. The drawing includes reference to sub-assemblies, dimensions, interface information, weights, service supply details and reference to design documents." ;
                  rdl:PCA_100006765 rrdl:CFIHOS-20000031 ;
                  rdl:PCA_100006766 rdl:PCA_100006653 ;
                  rdl:PCA_100006768 "Provides overview of the main parts of the equipment including part numbers and references to specifications and other design documentation. Drawing is used for manufacturing of assemblies." ;
                  rdfs:comment "Provides overview of the main parts of the equipment including part numbers and references to specifications and other design documentation. Drawing is used for manufacturing of assemblies." ;
                  rdfs:label "Assembly drawing" ;
                  skos:broadMatch rdl:PCA_100006734 ;
                  skos:broader rdl:PCA_100006746 .


###  http://rds.posccaesar.org/ontology/plm/rdl/PCA_100006098
rdl:PCA_100006098 rdf:type owl:Class ;
                  rdfs:subClassOf rdl:PCA_100004908 ;
                  rdl:PCA_100006763 "Procedure for assembly of individual components." ;
                  rdl:PCA_100006764 "The Assembly Procedure shall describe all actions, equipments and tools required to perform assembly of equipments including any lubricants or service materials.\nThis procedure shall include all HSE and safety precautions necessary to ensure safe operation." ;
                  rdl:PCA_100006765 rrdl:CFIHOS-20000031 ;
                  rdl:PCA_100006766 rdl:PCA_100006653 ;
                  rdl:PCA_100006768 "Provide the assembly site with sufficient information to assemble the equipment correctly." ;
                  rdfs:comment "Provide the assembly site with sufficient information to assemble the equipment correctly." ;
                  rdfs:label "Assembly procedure" ;
                  skos:broadMatch rdl:PCA_100006688 ;
                  skos:broader rdl:PCA_100006751 .


###  http://rds.posccaesar.org/ontology/plm/rdl/PCA_100006099
rdl:PCA_100006099 rdf:type owl:Class ;
                  rdfs:subClassOf rdl:PCA_100004908 ;
                  rdl:PCA_100006763 "The document shall be result of a systematic mapping of all potential ignition sources both electrical and non-electrical, including risk assessment and risk reduction measures in order to reduce ignition probability of an explosive atmosphere occurring in both hazardous and non-hazardous areas. The equipment shall be categorized as non-essential, essential and safety critical equipment respectively." ;
                  rdl:PCA_100006765 rrdl:CFIHOS-20000010 ,
                                    rrdl:CFIHOS-20000011 ,
                                    rrdl:CFIHOS-20000013 ;
                  rdl:PCA_100006766 rdl:PCA_100006626 ,
                                    rdl:PCA_100006627 ,
                                    rdl:PCA_100006628 ,
                                    rdl:PCA_100006629 ,
                                    rdl:PCA_100006630 ,
                                    rdl:PCA_100006631 ,
                                    rdl:PCA_100006632 ,
                                    rdl:PCA_100006633 ,
                                    rdl:PCA_100006634 ,
                                    rdl:PCA_100006635 ,
                                    rdl:PCA_100006636 ,
                                    rdl:PCA_100006637 ,
                                    rdl:PCA_100006638 ,
                                    rdl:PCA_100006639 ,
                                    rdl:PCA_100006640 ,
                                    rdl:PCA_100006641 ,
                                    rdl:PCA_100006642 ;
                  rdl:PCA_100006768 "A complete list to identify of all potential ignition sources that could come into contact with explosive atmosphere and the likelihood of occurrence of the potential ignition source to become effective.  \n\nReference is made to EN 1127-1." ;
                  rdfs:comment "A complete list to identify of all potential ignition sources that could come into contact with explosive atmosphere and the likelihood of occurrence of the potential ignition source to become effective.  \n\nReference is made to EN 1127-1." ;
                  rdfs:label "ATEX ignition source mapping report" ;
                  skos:broadMatch rdl:PCA_100006716 ,
                                  rdl:PCA_100006717 ,
                                  rdl:PCA_100006718 ;
                  skos:broader rdl:PCA_100006756 .


###  http://rds.posccaesar.org/ontology/plm/rdl/PCA_100006100
rdl:PCA_100006100 rdf:type owl:Class ;
                  rdfs:subClassOf rdl:PCA_100004908 ;
                  rdl:PCA_100006763 "Test reports for Audio and video entertainment distribution network (coaxial cable) shall be provided. Test per outlet." ;
                  rdl:PCA_100006765 rrdl:CFIHOS-20000030 ;
                  rdl:PCA_100006766 rdl:PCA_100006653 ;
                  rdfs:label "Audio and video entertainment distribution network (coaxial cable) test report" ;
                  skos:broadMatch rdl:PCA_100006722 ;
                  skos:broader rdl:PCA_100006756 .


###  http://rds.posccaesar.org/ontology/plm/rdl/PCA_100006101
rdl:PCA_100006101 rdf:type owl:Class ;
                  rdfs:subClassOf rdl:PCA_100004908 ;
                  rdl:PCA_100006763 "To detailed the design and the implementation of the control and monitoring system." ;
                  rdl:PCA_100006765 rrdl:CFIHOS-20000015 ;
                  rdl:PCA_100006766 rdl:PCA_100006626 ,
                                    rdl:PCA_100006627 ,
                                    rdl:PCA_100006628 ,
                                    rdl:PCA_100006629 ,
                                    rdl:PCA_100006633 ;
                  rdl:PCA_100006768 "Individual Functional Specifications (FS) shall be developed for each process system to be controlled and/or monitored. A separate FS shall be developed for the control system itself." ;
                  rdfs:comment "Individual Functional Specifications (FS) shall be developed for each process system to be controlled and/or monitored. A separate FS shall be developed for the control system itself." ;
                  rdfs:label "Automation functional specifications" ;
                  skos:broadMatch rdl:PCA_100006687 ;
                  skos:broader rdl:PCA_100006757 .


###  http://rds.posccaesar.org/ontology/plm/rdl/PCA_100006102
rdl:PCA_100006102 rdf:type owl:Class ;
                  rdfs:subClassOf rdl:PCA_100004908 ;
                  rdl:PCA_100006763 "This document shall support verification of component or system function according to company/project requirements." ;
                  rdl:PCA_100006765 rrdl:CFIHOS-20000021 ;
                  rdl:PCA_100006766 rdl:PCA_100006653 ;
                  rdl:PCA_100006768 "Sufficient information to demonstrate balancing of delivered equipment" ;
                  rdfs:comment "Sufficient information to demonstrate balancing of delivered equipment" ;
                  rdfs:label "Balancing report" ;
                  skos:broadMatch rdl:PCA_100006722 ;
                  skos:broader rdl:PCA_100006756 .


###  http://rds.posccaesar.org/ontology/plm/rdl/PCA_100006103
rdl:PCA_100006103 rdf:type owl:Class ;
                  rdfs:subClassOf rdl:PCA_100004908 ;
                  rdl:PCA_100006763 "An overview of all barriers to prevent hazardous event, and barriers to control consequences and effects for a pipeline system is needed for safe operation. Reference is given to DNV-RP-F116:2019, figure I-1." ;
                  rdl:PCA_100006765 rrdl:CFIHOS-20000018 ;
                  rdl:PCA_100006766 rdl:PCA_100006657 ;
                  rdl:PCA_100006768 "A spreadsheet shall be prepared. This shall include all barrier system /element given in DNV-RP-F116:2019, table I-7. The spreadsheet shall also include function, reliability and robustness per barrier element/threat. (Template available in Equinor, however needs to be updated). ." ;
                  rdfs:comment "A spreadsheet shall be prepared. This shall include all barrier system /element given in DNV-RP-F116:2019, table I-7. The spreadsheet shall also include function, reliability and robustness per barrier element/threat. (Template available in Equinor, however needs to be updated). ." ;
                  rdfs:label "Barrier matrix" ;
                  skos:broadMatch rdl:PCA_100006699 ;
                  skos:broader rdl:PCA_100006753 .


###  http://rds.posccaesar.org/ontology/plm/rdl/PCA_100006104
rdl:PCA_100006104 rdf:type owl:Class ;
                  rdfs:subClassOf rdl:PCA_100004908 ;
                  rdl:PCA_100006763 "A description of the overall pipeline system 'pig trap to pig trap' is needed to ensure a common understanding of where documentation will be authorized during the pipeline lifetime, including an overview of battery limits." ;
                  rdl:PCA_100006765 rrdl:CFIHOS-20000018 ;
                  rdl:PCA_100006766 rdl:PCA_100006654 ;
                  rdl:PCA_100006768 "Drawing covering interfaces towards elements such as, plants, platforms and other pipelines (tees/wyes), and other pipeline operators. Changes in standards, codes and authority requirements and testing interfaces along the pipeline system shall be included." ;
                  rdfs:comment "Drawing covering interfaces towards elements such as, plants, platforms and other pipelines (tees/wyes), and other pipeline operators. Changes in standards, codes and authority requirements and testing interfaces along the pipeline system shall be included." ;
                  rdfs:label "Battery limit drawings" ;
                  skos:broadMatch rdl:PCA_100006713 ;
                  skos:broader rdl:PCA_100006746 ,
                               rdl:PCA_100006753 .


###  http://rds.posccaesar.org/ontology/plm/rdl/PCA_100006105
rdl:PCA_100006105 rdf:type owl:Class ;
                  rdfs:subClassOf rdl:PCA_100004908 ;
                  rdl:PCA_100006763 "Quality assurance of the product (incl. dimensions and materials)" ;
                  rdl:PCA_100006765 rrdl:CFIHOS-20000027 ;
                  rdl:PCA_100006766 rdl:PCA_100006653 ;
                  rdl:PCA_100006768 "Describe parameters for bending, and expected bending results" ;
                  rdfs:comment "Describe parameters for bending, and expected bending results" ;
                  rdfs:label "Bending procedure" ;
                  skos:broadMatch rdl:PCA_100006722 ;
                  skos:broader rdl:PCA_100006751 .


###  http://rds.posccaesar.org/ontology/plm/rdl/PCA_100006106
rdl:PCA_100006106 rdf:type owl:Class ;
                  rdfs:subClassOf rdl:PCA_100004908 ;
                  rdl:PCA_100006763 "A list of parts, components and sub-assemblies for equipment with part numbers, item numbers, quantities, material designations and references to specifications." ;
                  rdl:PCA_100006765 rrdl:CFIHOS-20000031 ;
                  rdl:PCA_100006766 rdl:PCA_100006653 ;
                  rdl:PCA_100006768 "Provide purchase information on key parts of an assembly. Gives reference to sub-level parts. The BOM is used as part of the documents for manufacturing and accompanies the assembly drawings." ;
                  rdfs:comment "Provide purchase information on key parts of an assembly. Gives reference to sub-level parts. The BOM is used as part of the documents for manufacturing and accompanies the assembly drawings." ;
                  rdfs:label "Bill of material (BOM)" ;
                  skos:broadMatch rdl:PCA_100006715 ;
                  skos:broader rdl:PCA_100006748 .


###  http://rds.posccaesar.org/ontology/plm/rdl/PCA_100006107
rdl:PCA_100006107 rdf:type owl:Class ;
                  rdfs:subClassOf rdl:PCA_100004908 ;
                  rdl:PCA_100006763 "To describe the complete sequence starting with \"black\" platform/plant and ending with main power established." ;
                  rdl:PCA_100006765 rrdl:CFIHOS-20000008 ;
                  rdl:PCA_100006766 rdl:PCA_100006634 ,
                                    rdl:PCA_100006635 ,
                                    rdl:PCA_100006636 ,
                                    rdl:PCA_100006637 ,
                                    rdl:PCA_100006638 ,
                                    rdl:PCA_100006639 ;
                  rdl:PCA_100006768 "All involved auxiliary systems shall be included." ;
                  rdfs:comment "All involved auxiliary systems shall be included." ;
                  rdfs:label "Black start philosophy" ;
                  skos:broadMatch rdl:PCA_100006687 ,
                                  rdl:PCA_100006688 ;
                  skos:broader rdl:PCA_100006752 .


###  http://rds.posccaesar.org/ontology/plm/rdl/PCA_100006108
rdl:PCA_100006108 rdf:type owl:Class ;
                  rdfs:subClassOf rdl:PCA_100004908 ;
                  rdl:PCA_100006763 "This document shall support verification of component function according to company/project requirements.\n\nThis document gives an input to DAL" ;
                  rdl:PCA_100006765 rrdl:CFIHOS-20000013 ;
                  rdl:PCA_100006766 rdl:PCA_100006653 ;
                  rdl:PCA_100006768 "This calculation documents that the combined unit has sufficient strength for the explosion loads specified" ;
                  rdfs:comment "This calculation documents that the combined unit has sufficient strength for the explosion loads specified" ;
                  rdfs:label "Blast load calculation" ;
                  skos:broadMatch rdl:PCA_100006687 ;
                  skos:broader rdl:PCA_100006741 .


###  http://rds.posccaesar.org/ontology/plm/rdl/PCA_100006109
rdl:PCA_100006109 rdf:type owl:Class ;
                  rdfs:subClassOf rdl:PCA_100004908 ;
                  rdl:PCA_100006763 "Required for system understanding, functionality, and troubleshooting" ;
                  rdl:PCA_100006764 "This is a schematic diagram which shows connections between simple figures (rectangles etc.) in order to set out the sequence of pieces of equipment or functions. It includes the \"Process block diagram\".\nNOTE! This type of block diagrams shall not be used to present logic." ;
                  rdl:PCA_100006765 rrdl:CFIHOS-20000031 ;
                  rdl:PCA_100006766 rdl:PCA_100006653 ;
                  rdl:PCA_100006768 "Show configuration of a system/package and subsystems or relevant interfaces to give a functional understanding." ;
                  rdfs:comment "Show configuration of a system/package and subsystems or relevant interfaces to give a functional understanding." ;
                  rdfs:label "Block diagram" ;
                  skos:broadMatch rdl:PCA_100006695 ;
                  skos:broader rdl:PCA_100006745 .


###  http://rds.posccaesar.org/ontology/plm/rdl/PCA_100006110
rdl:PCA_100006110 rdf:type owl:Class ;
                  rdfs:subClassOf rdl:PCA_100004908 ;
                  rdl:PCA_100006765 rrdl:CFIHOS-20000003 ;
                  rdl:PCA_100006766 rdl:PCA_100006656 ;
                  rdl:PCA_100006768 "Architectural layout drawings (plans, elevations) and cross sections and details of all architectural components shall be produced.\n\nDrawings showing extent and details for thermal and acoustic insulation and fire protection shall be included. All penetrations including windows and doors shall be shown.\n\nLocation, direction and type of signpost shall be shown on architectural layout drawings.\n\nThe drawing scale for architectural layout drawings shall normally be 1:100 in A3 format. However different scales can be used on A1 format if readable when reduced to A3 format. The drawings shall include stairs, walls, doors, windows, furniture, access and escape routes and all tagged equipment.\n\nMain dimensions shall be included. Elevations of all floors and platforms etc. shall be shown. A key plan, grid lines with north and east references and match lines with drawing references shall be included. Relevant civil, structural, HVAC, etc. drawings be referenced. The drawings shall have a title block which contains all the information necessary to identify the drawing and its purpose." ;
                  rdfs:comment "Architectural layout drawings (plans, elevations) and cross sections and details of all architectural components shall be produced.\n\nDrawings showing extent and details for thermal and acoustic insulation and fire protection shall be included. All penetrations including windows and doors shall be shown.\n\nLocation, direction and type of signpost shall be shown on architectural layout drawings.\n\nThe drawing scale for architectural layout drawings shall normally be 1:100 in A3 format. However different scales can be used on A1 format if readable when reduced to A3 format. The drawings shall include stairs, walls, doors, windows, furniture, access and escape routes and all tagged equipment.\n\nMain dimensions shall be included. Elevations of all floors and platforms etc. shall be shown. A key plan, grid lines with north and east references and match lines with drawing references shall be included. Relevant civil, structural, HVAC, etc. drawings be referenced. The drawings shall have a title block which contains all the information necessary to identify the drawing and its purpose." ;
                  rdfs:label "Buildings architectural drawings" ;
                  skos:broadMatch rdl:PCA_100006710 ;
                  skos:broader rdl:PCA_100006746 .


###  http://rds.posccaesar.org/ontology/plm/rdl/PCA_100006111
rdl:PCA_100006111 rdf:type owl:Class ;
                  rdfs:subClassOf rdl:PCA_100004908 ;
                  rdl:PCA_100006765 rrdl:CFIHOS-20000008 ;
                  rdl:PCA_100006766 rdl:PCA_100006656 ;
                  rdl:PCA_100006768 "For the following, individual layout drawings shall be provided:   Cable ladders/trays > =300 mm" ;
                  rdfs:comment "For the following, individual layout drawings shall be provided:   Cable ladders/trays > =300 mm" ;
                  rdfs:label "Cable ladder/trays >=300 mm layout drawings" ;
                  skos:broadMatch rdl:PCA_100006709 ;
                  skos:broader rdl:PCA_100006746 .


###  http://rds.posccaesar.org/ontology/plm/rdl/PCA_100006112
rdl:PCA_100006112 rdf:type owl:Class ;
                  rdfs:subClassOf rdl:PCA_100004908 ;
                  rdl:PCA_100006765 rrdl:CFIHOS-20000008 ,
                                    rrdl:CFIHOS-20000015 ,
                                    rrdl:CFIHOS-20000030 ,
                                    rrdl:CFIHOS-20000031 ;
                  rdl:PCA_100006766 rdl:PCA_100006656 ;
                  rdl:PCA_100006768 "Cable route and changes to network shall be delivered.\n\nCable routing shall document the following:\n - Cable route network:\n   - Cable ladder/tray >=300mm;\n   - Cable tray <300 mm if purpose to connect Cable ladders >=300mm;\n   - Penetrations;\n   - Unsupported Jump between cable ladders;\n - Cables routed on network." ;
                  rdfs:comment "Cable route and changes to network shall be delivered.\n\nCable routing shall document the following:\n - Cable route network:\n   - Cable ladder/tray >=300mm;\n   - Cable tray <300 mm if purpose to connect Cable ladders >=300mm;\n   - Penetrations;\n   - Unsupported Jump between cable ladders;\n - Cables routed on network." ;
                  rdfs:label "Cable routing" ;
                  skos:broadMatch rdl:PCA_100006708 ,
                                  rdl:PCA_100006709 ;
                  skos:broader rdl:PCA_100006762 .


###  http://rds.posccaesar.org/ontology/plm/rdl/PCA_100006113
rdl:PCA_100006113 rdf:type owl:Class ;
                  rdfs:subClassOf rdl:PCA_100004908 ;
                  rdl:PCA_100006763 "Characteristics and functional parameters shall be documented and performance shall be shown to be probable. This shall include but not be limited to calculations, curves, tables, reference to similar applications and test data. This shall as a minimum be at a level customary for the equipment and to the extent such data are of importance for interfaces to plant and system." ;
                  rdl:PCA_100006768 "Lateral analyses and torsion analyses for compressors; performance curves for pumps and compressors. \n\nStrength calculations, thermal performance and vibration calculations for heat exchangers/pressure vessels." ;
                  rdfs:comment "Lateral analyses and torsion analyses for compressors; performance curves for pumps and compressors. \n\nStrength calculations, thermal performance and vibration calculations for heat exchangers/pressure vessels." ;
                  rdfs:label "Calculations, curves and tables" ;
                  skos:broadMatch rdl:PCA_100006687 ;
                  skos:broader rdl:PCA_100006741 .


###  http://rds.posccaesar.org/ontology/plm/rdl/PCA_100006114
rdl:PCA_100006114 rdf:type owl:Class ;
                  rdfs:subClassOf rdl:PCA_100004908 ;
                  rdl:PCA_100006763 "A document containing data which records compliance with specified requirements." ;
                  rdl:PCA_100006765 rrdl:CFIHOS-20000015 ;
                  rdl:PCA_100006766 rdl:PCA_100006653 ;
                  rdl:PCA_100006768 "Provides details about out-of-tolerance conditions, special measurement conditions, standard used, date and approvals etc. Each certificate includes a serial number that associates one calibration with one instrument." ;
                  rdfs:comment "Provides details about out-of-tolerance conditions, special measurement conditions, standard used, date and approvals etc. Each certificate includes a serial number that associates one calibration with one instrument." ;
                  rdfs:label "Calibration certificate" ;
                  skos:broadMatch rdl:PCA_100006722 ;
                  skos:broader rdl:PCA_100006743 .


###  http://rds.posccaesar.org/ontology/plm/rdl/PCA_100006115
rdl:PCA_100006115 rdf:type owl:Class ;
                  rdfs:subClassOf rdl:PCA_100004908 ;
                  rdl:PCA_100006763 "The purpose of Cause & Effect (C&E) Diagram is to define logic control and shutdown functions." ;
                  rdl:PCA_100006765 rrdl:CFIHOS-20000015 ,
                                    rrdl:CFIHOS-20000031 ;
                  rdl:PCA_100006766 rdl:PCA_100006626 ,
                                    rdl:PCA_100006627 ,
                                    rdl:PCA_100006628 ,
                                    rdl:PCA_100006633 ,
                                    rdl:PCA_100006634 ,
                                    rdl:PCA_100006635 ,
                                    rdl:PCA_100006636 ,
                                    rdl:PCA_100006637 ,
                                    rdl:PCA_100006638 ,
                                    rdl:PCA_100006639 ,
                                    rdl:PCA_100006640 ,
                                    rdl:PCA_100006641 ;
                  rdl:PCA_100006768 "The C&E Diagram shall be prepared as a matrix between initiating (input) and actuated elements (output) performing the corrective action. Both input and output shall be identified by ENS tag numbers. In addition, the following information shall be given for each input/output:\n - Tag number, Initiator/Actuator, Value, Note, Service description.\n - Reference drawing number (e.g. Piping & instrument diagram).\n\nNote: The cause and effect for the fire and gas detection system is included in the Fire protection data sheet (FPDS)." ;
                  rdfs:comment "The C&E Diagram shall be prepared as a matrix between initiating (input) and actuated elements (output) performing the corrective action. Both input and output shall be identified by ENS tag numbers. In addition, the following information shall be given for each input/output:\n - Tag number, Initiator/Actuator, Value, Note, Service description.\n - Reference drawing number (e.g. Piping & instrument diagram).\n\nNote: The cause and effect for the fire and gas detection system is included in the Fire protection data sheet (FPDS)." ;
                  rdfs:label "Cause & effect (C&E)" ;
                  skos:broadMatch rdl:PCA_100006699 ;
                  skos:broader rdl:PCA_100006742 .


###  http://rds.posccaesar.org/ontology/plm/rdl/PCA_100006116
rdl:PCA_100006116 rdf:type owl:Class ;
                  rdfs:subClassOf rdl:PCA_100004908 ;
                  rdl:PCA_100006763 "The purpose of the Cause and Effect (C&E) is to give an overview over interlock and intertrip between IED / breakers." ;
                  rdl:PCA_100006765 rrdl:CFIHOS-20000015 ;
                  rdl:PCA_100006768 "IEC 61850 / GOOSE address shall be included if relevant. Logical diagrams shall be included as part of Cause and Effect, or reference to relevant documents shall be given. There shall be one sheet per IED / breaker." ;
                  rdfs:comment "IEC 61850 / GOOSE address shall be included if relevant. Logical diagrams shall be included as part of Cause and Effect, or reference to relevant documents shall be given. There shall be one sheet per IED / breaker." ;
                  rdfs:label "Cause & effect (C&E) for interlock and intertrip" ;
                  skos:broadMatch rdl:PCA_100006699 ;
                  skos:broader rdl:PCA_100006742 .


###  http://rds.posccaesar.org/ontology/plm/rdl/PCA_100006117
rdl:PCA_100006117 rdf:type owl:Class ;
                  rdfs:subClassOf rdl:PCA_100004908 ;
                  rdl:PCA_100006763 "Lifting appliances shall be accompanied by a certificate issued by an enterprise of competence prior to use in accordance with ILO C152 or Annex H of NORSOK R-003, or NORSOK R-005, as applicable.\n\nThis also includes manufacturers' ILO based certificates for loose Gear (hooks, hooks block, \nwire, shackles, links, etc.)." ;
                  rdfs:label "Certificate for use - lifting appliances" ;
                  skos:broadMatch rdl:PCA_100006722 ;
                  skos:broader rdl:PCA_100006743 .


###  http://rds.posccaesar.org/ontology/plm/rdl/PCA_100006118
rdl:PCA_100006118 rdf:type owl:Class ;
                  rdfs:subClassOf rdl:PCA_100004908 ;
                  rdl:PCA_100006763 "A Certificate where Contractor/supplier confirms/verifies that the requirements in the contract/purchase order for design, calculations, production, testing and traceability requirements have been met;" ;
                  rdl:PCA_100006765 rrdl:CFIHOS-20000008 ,
                                    rrdl:CFIHOS-20000031 ;
                  rdl:PCA_100006766 rdl:PCA_100006634 ,
                                    rdl:PCA_100006635 ,
                                    rdl:PCA_100006636 ,
                                    rdl:PCA_100006637 ,
                                    rdl:PCA_100006638 ,
                                    rdl:PCA_100006639 ,
                                    rdl:PCA_100006640 ,
                                    rdl:PCA_100006641 ,
                                    rdl:PCA_100006642 ;
                  rdl:PCA_100006768 "One document shall cover the complete contract/purchase order." ;
                  rdfs:comment "One document shall cover the complete contract/purchase order." ;
                  rdfs:label "Certificate of conformance" ;
                  skos:broadMatch rdl:PCA_100006722 ;
                  skos:broader rdl:PCA_100006743 .


###  http://rds.posccaesar.org/ontology/plm/rdl/PCA_100006119
rdl:PCA_100006119 rdf:type owl:Class ;
                  rdfs:subClassOf rdl:PCA_100004908 ;
                  rdl:PCA_100006763 "Description of chemical treatment strategy for the project/asset, including strategy for modifications & tie-ins;" ;
                  rdl:PCA_100006765 rrdl:CFIHOS-20000026 ;
                  rdl:PCA_100006766 rdl:PCA_100006654 ;
                  rdl:PCA_100006768 "Each field/plant should have a Chemical Management Plan that describes as a minimum:\n - Contact details for key personnel;\n - Roles & Responsibilities;\n - Contract references;\n - Risk reviews;\n - Description of each and every chemical used (past, present and future), including:\n   - Reason for use;\n   - Mechanism & application;\n   - Imitations;\n   - Injection system;\n   - Monitoring programme\n   - Troubleshooting guide;\n   - HSE summary;\n   - Supply chain description;\n - Description of processes where chemicals are currently not used, and why;\n - Description of data management;\n - Report references;\n - Reference to governing documents;\n - Reference to substitution plans;\n - Reference to improvement plans;\n - Key Performance Indicators." ;
                  rdfs:comment "Each field/plant should have a Chemical Management Plan that describes as a minimum:\n - Contact details for key personnel;\n - Roles & Responsibilities;\n - Contract references;\n - Risk reviews;\n - Description of each and every chemical used (past, present and future), including:\n   - Reason for use;\n   - Mechanism & application;\n   - Imitations;\n   - Injection system;\n   - Monitoring programme\n   - Troubleshooting guide;\n   - HSE summary;\n   - Supply chain description;\n - Description of processes where chemicals are currently not used, and why;\n - Description of data management;\n - Report references;\n - Reference to governing documents;\n - Reference to substitution plans;\n - Reference to improvement plans;\n - Key Performance Indicators." ;
                  rdfs:label "Chemical management plan" ;
                  skos:broadMatch rdl:PCA_100006726 ,
                                  rdl:PCA_100006728 ,
                                  rdl:PCA_100006729 ;
                  skos:broader rdl:PCA_100006753 .


###  http://rds.posccaesar.org/ontology/plm/rdl/PCA_100006120
rdl:PCA_100006120 rdf:type owl:Class ;
                  rdfs:subClassOf rdl:PCA_100004908 ;
                  rdl:PCA_100006763 "The circuit/wiring diagram shall be sufficient for all testing, troubleshooting and maintenance.\n\nThe principles of the circuit/wiring diagrams shall be in accordance with IEC 61082.\n\nNOTE: For customized documentation, handover format shall be native 2D CAD (Z-005) + PDF.\n\nThe power circuit shall be shown to the extent necessary for the understanding of the circuit functions and for understanding how the components are wired. Contactor and terminal blocks shall be included. This means also including references to equipment not being part of scope of work. The documentation shall reflect the actual internal wiring. Terminal blocks and external references shall be included. Reference shall be made to the supplier's equipment and terminal marking." ;
                  rdl:PCA_100006765 rrdl:CFIHOS-20000008 ;
                  rdl:PCA_100006766 rdl:PCA_100006634 ,
                                    rdl:PCA_100006635 ,
                                    rdl:PCA_100006636 ,
                                    rdl:PCA_100006637 ,
                                    rdl:PCA_100006638 ,
                                    rdl:PCA_100006639 ;
                  rdl:PCA_100006768 "Circuit/wiring diagram shall typically include the following (as relevant for the equipment):\n - All internal connections for control, alarms, protection, interlocks, trip functions, monitoring, etc.;\n - Component list for all internal components including control and protection units;\n - Switchgear/-board tag code;\n - Cubicle number;\n - Consumer tag code;\n - Type of external signals (fire and gas trip signal, etc.);\n - Power and current rating;\n - Terminal block/socket number;\n - Terminal/pin number (including spares);\n - Internal cable numbers with pair and core colour details;\n - Destination for internal cables;\n - Earthing details;\n - Equipment and equipment connections;\n - External cable numbers with pair and core colour details;\n - Signal tag number;\n - Reference drawings (Company document number);\n - Reference to loop database for signal interfaced to instrument/automation and telecommunication systems." ;
                  rdfs:comment "Circuit/wiring diagram shall typically include the following (as relevant for the equipment):\n - All internal connections for control, alarms, protection, interlocks, trip functions, monitoring, etc.;\n - Component list for all internal components including control and protection units;\n - Switchgear/-board tag code;\n - Cubicle number;\n - Consumer tag code;\n - Type of external signals (fire and gas trip signal, etc.);\n - Power and current rating;\n - Terminal block/socket number;\n - Terminal/pin number (including spares);\n - Internal cable numbers with pair and core colour details;\n - Destination for internal cables;\n - Earthing details;\n - Equipment and equipment connections;\n - External cable numbers with pair and core colour details;\n - Signal tag number;\n - Reference drawings (Company document number);\n - Reference to loop database for signal interfaced to instrument/automation and telecommunication systems." ;
                  rdfs:label "Circuit / wiring diagram" ;
                  skos:broadMatch rdl:PCA_100006702 ,
                                  rdl:PCA_100006712 ;
                  skos:broader rdl:PCA_100006745 .


###  http://rds.posccaesar.org/ontology/plm/rdl/PCA_100006121
rdl:PCA_100006121 rdf:type owl:Class ;
                  rdfs:subClassOf rdl:PCA_100004908 ;
                  rdl:PCA_100006763 "Verification of cleanness off hydraulic system." ;
                  rdl:PCA_100006766 rdl:PCA_100006653 ;
                  rdl:PCA_100006768 "Documentation of cleanness according to specification." ;
                  rdfs:comment "Documentation of cleanness according to specification." ;
                  rdfs:label "Cleanness documentation" .


###  http://rds.posccaesar.org/ontology/plm/rdl/PCA_100006122
rdl:PCA_100006122 rdf:type owl:Class ;
                  rdfs:subClassOf rdl:PCA_100004908 ;
                  rdl:PCA_100006763 "Verification of suppliers compliance with surface protection and coating requirements.\n\n(This document provides a procedure for coating operator to ensure repeatability and formalism and hence prove the quality of the coating work.)" ;
                  rdl:PCA_100006764 "Requirements related to assurance and check of quality in manufacturing phase will very much depend on Purchaser’s knowledge of supplier. Well known supplier, with proven track record, delivering products based on industry standards, will typically deliver less verification documentation to Purchaser than unknown/new supplier delivering the same product. Therefore, this deliverable should be evaluated as candidate for being available in digital format to Purchaser, for information only." ;
                  rdl:PCA_100006765 rrdl:CFIHOS-20000028 ;
                  rdl:PCA_100006766 rdl:PCA_100006653 ;
                  rdl:PCA_100006768 "This document details the work process and how the defined requirements to surface treatment, application and quality control shall be met. \n\nA procedure may cover wet paint, powder coating, or metallic coatings. The document shall include reference to applied standards and the information about revision of the applied standard." ;
                  rdfs:comment "This document details the work process and how the defined requirements to surface treatment, application and quality control shall be met. \n\nA procedure may cover wet paint, powder coating, or metallic coatings. The document shall include reference to applied standards and the information about revision of the applied standard." ;
                  rdfs:label "Coating procedure" ;
                  skos:broadMatch rdl:PCA_100006722 ;
                  skos:broader rdl:PCA_100006751 .


###  http://rds.posccaesar.org/ontology/plm/rdl/PCA_100006123
rdl:PCA_100006123 rdf:type owl:Class ;
                  rdfs:subClassOf rdl:PCA_100004908 ;
                  rdl:PCA_100006763 "This document is used for verification of compliance with surface protection and coating requirements." ;
                  rdl:PCA_100006764 "Requirements related to assurance and check of quality in manufacturing phase will very much depend on Purchaser’s knowledge of supplier. Well known supplier, with proven track record, delivering products based on industry standards, will typically deliver less verification documentation to Purchaser than unknown/new supplier delivering the same product. Therefore, this deliverable should be evaluated as candidate for being available in digital format to Purchaser, for information only." ;
                  rdl:PCA_100006765 rrdl:CFIHOS-20000028 ;
                  rdl:PCA_100006766 rdl:PCA_100006653 ;
                  rdl:PCA_100006768 "Document containing records of performed surface protection and coating work." ;
                  rdfs:comment "Document containing records of performed surface protection and coating work." ;
                  rdfs:label "Coating report" ;
                  skos:broadMatch rdl:PCA_100006722 ;
                  skos:broader rdl:PCA_100006756 .


###  http://rds.posccaesar.org/ontology/plm/rdl/PCA_100006124
rdl:PCA_100006124 rdf:type owl:Class ;
                  rdfs:subClassOf rdl:PCA_100004908 ;
                  rdl:PCA_100006765 rrdl:CFIHOS-20000030 ;
                  rdl:PCA_100006766 rdl:PCA_100006653 ;
                  rdl:PCA_100006768 "Test reports for coaxial cables (for radio systems) shall be provided." ;
                  rdfs:comment "Test reports for coaxial cables (for radio systems) shall be provided." ;
                  rdfs:label "Coaxial cable test reports" ;
                  skos:broadMatch rdl:PCA_100006722 ;
                  skos:broader rdl:PCA_100006756 .


###  http://rds.posccaesar.org/ontology/plm/rdl/PCA_100006125
rdl:PCA_100006125 rdf:type owl:Class ;
                  rdfs:subClassOf rdl:PCA_100004908 ;
                  rdl:PCA_100006763 "Certificate to confirm compliance with contract / purchase order with reference to standards, technical specifications and requirements for the product." ;
                  rdl:PCA_100006765 rrdl:CFIHOS-20000031 ;
                  rdl:PCA_100006766 rdl:PCA_100006653 ;
                  rdl:PCA_100006768 "The manufacture’s or other party’s confirmation that the product is designed, manufactured and tested as specified." ;
                  rdfs:comment "The manufacture’s or other party’s confirmation that the product is designed, manufactured and tested as specified." ;
                  rdfs:label "COC - certificate of conformance" ;
                  skos:broadMatch rdl:PCA_100006724 ;
                  skos:broader rdl:PCA_100006743 .


###  http://rds.posccaesar.org/ontology/plm/rdl/PCA_100006126
rdl:PCA_100006126 rdf:type owl:Class ;
                  rdfs:subClassOf rdl:PCA_100004908 ;
                  rdl:PCA_100006763 "Instruction providing information on the commissioning of the product. Instructions for commissioning are provided especially for large and highly complex products and for large industrial installations. The purpose of such instructions is to provide the user with the information needed for initial setting-up and start-up of the product." ;
                  rdl:PCA_100006766 rdl:PCA_100006653 ;
                  rdl:PCA_100006768 "These instructions should contain for example:\n\n - download program, software instructions according to IEC 61506\n - checking instructions\n - checks to be performed before connection to the supply network and before first operation\n - details of specifications to apply to acceptance, inspection and performance tests." ;
                  rdfs:comment "These instructions should contain for example:\n\n - download program, software instructions according to IEC 61506\n - checking instructions\n - checks to be performed before connection to the supply network and before first operation\n - details of specifications to apply to acceptance, inspection and performance tests." ;
                  rdfs:label "Commissioning instruction" ;
                  skos:broadMatch rdl:PCA_100006688 .


###  http://rds.posccaesar.org/ontology/plm/rdl/PCA_100006127
rdl:PCA_100006127 rdf:type owl:Class ;
                  rdfs:subClassOf rdl:PCA_100004908 ;
                  rdl:PCA_100006763 "Document the performance of the CP system" ;
                  rdl:PCA_100006765 rrdl:CFIHOS-20000018 ;
                  rdl:PCA_100006766 rdl:PCA_100006657 ;
                  rdl:PCA_100006768 "Commissioning report shall be according to ISO15589-1 Section 13.2" ;
                  rdfs:comment "Commissioning report shall be according to ISO15589-1 Section 13.2" ;
                  rdfs:label "Commissioning report CP system (close out report)" ;
                  skos:broadMatch rdl:PCA_100006663 ;
                  skos:broader rdl:PCA_100006756 .


###  http://rds.posccaesar.org/ontology/plm/rdl/PCA_100006128
rdl:PCA_100006128 rdf:type owl:Class ;
                  rdfs:subClassOf rdl:PCA_100004908 ;
                  rdl:PCA_100006765 rrdl:CFIHOS-20000006 ;
                  rdl:PCA_100006766 rdl:PCA_100006656 ;
                  rdl:PCA_100006768 "The following concrete detail drawings shall be delivered: \n - General Arrangements;\n - Typicals;\n - Sections and details;\n - Main Mechanical Outfitting (MMO) drawings.\n\nThe concrete detail drawings shall contain:\n - Concrete dimensions;\n - All reinforcement types (tensile-, shear, pretension reinforcement, other if applicable);\n - Reinforcement dimensions, quantity and location in concrete structure;\n - Material properties (concrete and reinforcement)." ;
                  rdfs:comment "The following concrete detail drawings shall be delivered: \n - General Arrangements;\n - Typicals;\n - Sections and details;\n - Main Mechanical Outfitting (MMO) drawings.\n\nThe concrete detail drawings shall contain:\n - Concrete dimensions;\n - All reinforcement types (tensile-, shear, pretension reinforcement, other if applicable);\n - Reinforcement dimensions, quantity and location in concrete structure;\n - Material properties (concrete and reinforcement)." ;
                  rdfs:label "Concrete detail drawings" ;
                  skos:broadMatch rdl:PCA_100006731 ;
                  skos:broader rdl:PCA_100006746 .


###  http://rds.posccaesar.org/ontology/plm/rdl/PCA_100006129
rdl:PCA_100006129 rdf:type owl:Class ;
                  rdfs:subClassOf rdl:PCA_100004908 ;
                  rdl:PCA_100006764 "Structural design reports and input files/parameters shall be delivered. The report or collection of reports shall be self-contained, i.e. provide all information required to reproduce the results.\n\nThe static analysis and calculations shall have specific and detailed references to drawings and relevant part of regulations and referenced standards." ;
                  rdl:PCA_100006765 rrdl:CFIHOS-20000007 ;
                  rdl:PCA_100006766 rdl:PCA_100006656 ;
                  rdl:PCA_100006768 "Ref. generic design report" ;
                  rdfs:comment "Ref. generic design report" ;
                  rdfs:label "Concrete structural design report" ;
                  skos:broadMatch rdl:PCA_100006691 ,
                                  rdl:PCA_100006698 ;
                  skos:broader rdl:PCA_100006756 .


###  http://rds.posccaesar.org/ontology/plm/rdl/PCA_100006130
rdl:PCA_100006130 rdf:type owl:Class ;
                  rdfs:subClassOf rdl:PCA_100004908 ;
                  rdl:PCA_100006765 rrdl:CFIHOS-20000006 ;
                  rdl:PCA_100006768 "The following detail drawings shall be delivered\n - General Arrangements \n - Typicals \n - Sections and details \n - Concrete dimensions \n - Material properties \nDetails related to embedded items, block-outs, pre-stressing and post-tensioning of structures shall be included. \nFor embedded items for lifting operations documentation of certificates shall be included. Structural load plans shall also be included." ;
                  rdfs:comment "The following detail drawings shall be delivered\n - General Arrangements \n - Typicals \n - Sections and details \n - Concrete dimensions \n - Material properties \nDetails related to embedded items, block-outs, pre-stressing and post-tensioning of structures shall be included. \nFor embedded items for lifting operations documentation of certificates shall be included. Structural load plans shall also be included." ;
                  rdfs:label "Concrete structures geometry drawings" ;
                  skos:broadMatch rdl:PCA_100006731 ,
                                  rdl:PCA_100006732 ,
                                  rdl:PCA_100006733 ,
                                  rdl:PCA_100006734 ;
                  skos:broader rdl:PCA_100006746 .


###  http://rds.posccaesar.org/ontology/plm/rdl/PCA_100006131
rdl:PCA_100006131 rdf:type owl:Class ;
                  rdfs:subClassOf rdl:PCA_100004908 ;
                  rdl:PCA_100006764 "The following drawings shall be delivered:\n - All reinforcement types (tensile-, shear, pretension reinforcement, other if applicable);\n - Reinforcement dimensions, quantity and location in concrete structure;\n - Material properties." ;
                  rdl:PCA_100006765 rrdl:CFIHOS-20000007 ;
                  rdl:PCA_100006766 rdl:PCA_100006656 ;
                  rdl:PCA_100006768 "Ref. generic general arrangement drawing" ;
                  rdfs:comment "Ref. generic general arrangement drawing" ;
                  rdfs:label "Concrete structures reinforcement drawings" ;
                  skos:broadMatch rdl:PCA_100006707 ,
                                  rdl:PCA_100006731 ,
                                  rdl:PCA_100006732 ;
                  skos:broader rdl:PCA_100006746 .


###  http://rds.posccaesar.org/ontology/plm/rdl/PCA_100006132
rdl:PCA_100006132 rdf:type owl:Class ;
                  rdfs:subClassOf rdl:PCA_100004908 ;
                  rdl:PCA_100006763 "Diagram providing information about the physical connections among components or units." ;
                  rdl:PCA_100006764 "Separate diagrams shall be made for hydraulic, pneumatic and electrical connections, unless deemed not appropriate." ;
                  rdl:PCA_100006766 rdl:PCA_100006653 ;
                  rdl:PCA_100006768 "(IEC 61082-1) Diagram providing information about the physical connections among components or units\nMandatory content of information:\n - Conductor or cable type information (e.g. recognized type designation, catalogue or part number, material, construction, size, insulation, voltage rating, colour, number of conductors, other technical data);\n - Reference designation or conductor or cable number;\n - Identification or representation of the connected objects (e.g. reference and/or terminal designation)." ;
                  rdfs:comment "(IEC 61082-1) Diagram providing information about the physical connections among components or units\nMandatory content of information:\n - Conductor or cable type information (e.g. recognized type designation, catalogue or part number, material, construction, size, insulation, voltage rating, colour, number of conductors, other technical data);\n - Reference designation or conductor or cable number;\n - Identification or representation of the connected objects (e.g. reference and/or terminal designation)." ;
                  rdfs:label "Connection diagram" ;
                  skos:broadMatch rdl:PCA_100006712 ,
                                  rdl:PCA_100006713 ;
                  skos:broader rdl:PCA_100006745 .


###  http://rds.posccaesar.org/ontology/plm/rdl/PCA_100006133
rdl:PCA_100006133 rdf:type owl:Class ;
                  rdfs:subClassOf rdl:PCA_100004908 ;
                  rdl:PCA_100006763 "There shall be a consequence analysis document for each individual logic solver.\n\nThis document shall give information about which process unit is affected if the logic solver is switched off." ;
                  rdl:PCA_100006765 rrdl:CFIHOS-20000015 ;
                  rdl:PCA_100006766 rdl:PCA_100006626 ,
                                    rdl:PCA_100006633 ;
                  rdl:PCA_100006768 "Description of consequences of switching off the logic solver, including both hardwired signals and software communicated signals, and suggestion to operational mitigating actions to avoid the consequences described to avoid further loss of plant operation covering both switching off and start-up. The document shall describe the general precautions and consequences and describe in detail signals found to be critical (regularity, safety and environmental) and the effect on these signals after switching off the logic solver." ;
                  rdfs:comment "Description of consequences of switching off the logic solver, including both hardwired signals and software communicated signals, and suggestion to operational mitigating actions to avoid the consequences described to avoid further loss of plant operation covering both switching off and start-up. The document shall describe the general precautions and consequences and describe in detail signals found to be critical (regularity, safety and environmental) and the effect on these signals after switching off the logic solver." ;
                  rdfs:label "Consequence analysis logic solver" ;
                  skos:broadMatch rdl:PCA_100006698 ;
                  skos:broader rdl:PCA_100006756 .


###  http://rds.posccaesar.org/ontology/plm/rdl/PCA_100006134
rdl:PCA_100006134 rdf:type owl:Class ;
                  rdfs:subClassOf rdl:PCA_100004908 ;
                  rdl:PCA_100006763 "A document stating the normal and maximum consumption of the equipment." ;
                  rdl:PCA_100006765 rrdl:CFIHOS-20000031 ;
                  rdl:PCA_100006766 rdl:PCA_100006653 ;
                  rdl:PCA_100006768 "The document provides input for sizing relevant supplying sources such as e.g. electrical, air." ;
                  rdfs:comment "The document provides input for sizing relevant supplying sources such as e.g. electrical, air." ;
                  rdfs:label "Consumption/utilities list" ;
                  skos:broadMatch rdl:PCA_100006716 ;
                  skos:broader rdl:PCA_100006748 .


###  http://rds.posccaesar.org/ontology/plm/rdl/PCA_100006135
rdl:PCA_100006135 rdf:type owl:Class ;
                  rdfs:subClassOf rdl:PCA_100004908 ;
                  rdl:PCA_100006763 "A document to describe the method and timeline to deliver the required LCI during project execution and final handover to operations,  in accordance with Client LCI requirments." ;
                  rdl:PCA_100006765 rrdl:CFIHOS-20000001 ;
                  rdl:PCA_100006766 rdl:PCA_100006654 ;
                  rdl:PCA_100006768 "LCI strategy shall as a minimum include the following:\n - Contractor’s Life Cycle information management organization;\n - An overall strategy for interaction between internal parties, such as procurement and engineering.;\n - An overall integration strategy of life cycle information from all parties involved such as external contractors, subcontractors and suppliers;\n - Contractor shall describe their systems portfolio related to the production and administration of LCI including integration capabilities with the Company systems;\n - Training strategy of staff in both Company’s and Contractor's LCI tools;\n - LCI Handover strategy from MC to Commissioning;\n - Strategy for Material control and SPIR handling;\n - Contractor's method for LCI quality control and systematic correction of quality issues;\n - Contractor's method for ensuring delivery of 3D CAD design models throughout the project in compliance with Company’s requirements;\n - LCI procedures (including):\n   - Procedure for collection, storage, processing, transfer and sharing of LCI;\n   - The procedure for standard documentation handling;\n   - Work procedures for 3D handling as described in Company’s requirements;\n   - The procedure shall include transfer methods, information logistics, systems involved, responsibilities, milestones, quality control, error reporting and rectification;\n   - The procedure for tag scoping for supplier packages;\n   - The procedure for tag scoping for engineering;\n   - List containing Contractors planned deliveries of LCI according to Company's requirements;\n   - Time schedules showing LCI deliveries including 3D;\n   - Procedures or method to ensure special attention to identify early access and QC milestones. The schedules shall reflect the project execution plan and time schedules;\n   - Procedure for LCI progress reporting according to LCI time schedules;\n   - Procedures and checklists to ensure quality and completeness of the LCI delivery including maintenance of LCI during MC & commissioning;\n   - Procedure for handling of \"mark-ups\" from construction and MC & commissioning.\n\nDescribe work process for continuous transfer of LCI covering:\n - Project revisions of documents and drawings;\n - Tag information (including tag-doc references);\n - Continuous updates of 3D CAD information according to Company’s requirements;\n - Before issuing safety critical documents and single line diagram in IFC revision, tag information (in Company’s LCI systems) for tags shown on document/drawing shall as a minimum include tag no, description, area, discipline, system and PO references, cross references tag/tag, tag/doc relation." ;
                  rdfs:comment "LCI strategy shall as a minimum include the following:\n - Contractor’s Life Cycle information management organization;\n - An overall strategy for interaction between internal parties, such as procurement and engineering.;\n - An overall integration strategy of life cycle information from all parties involved such as external contractors, subcontractors and suppliers;\n - Contractor shall describe their systems portfolio related to the production and administration of LCI including integration capabilities with the Company systems;\n - Training strategy of staff in both Company’s and Contractor's LCI tools;\n - LCI Handover strategy from MC to Commissioning;\n - Strategy for Material control and SPIR handling;\n - Contractor's method for LCI quality control and systematic correction of quality issues;\n - Contractor's method for ensuring delivery of 3D CAD design models throughout the project in compliance with Company’s requirements;\n - LCI procedures (including):\n   - Procedure for collection, storage, processing, transfer and sharing of LCI;\n   - The procedure for standard documentation handling;\n   - Work procedures for 3D handling as described in Company’s requirements;\n   - The procedure shall include transfer methods, information logistics, systems involved, responsibilities, milestones, quality control, error reporting and rectification;\n   - The procedure for tag scoping for supplier packages;\n   - The procedure for tag scoping for engineering;\n   - List containing Contractors planned deliveries of LCI according to Company's requirements;\n   - Time schedules showing LCI deliveries including 3D;\n   - Procedures or method to ensure special attention to identify early access and QC milestones. The schedules shall reflect the project execution plan and time schedules;\n   - Procedure for LCI progress reporting according to LCI time schedules;\n   - Procedures and checklists to ensure quality and completeness of the LCI delivery including maintenance of LCI during MC & commissioning;\n   - Procedure for handling of \"mark-ups\" from construction and MC & commissioning.\n\nDescribe work process for continuous transfer of LCI covering:\n - Project revisions of documents and drawings;\n - Tag information (including tag-doc references);\n - Continuous updates of 3D CAD information according to Company’s requirements;\n - Before issuing safety critical documents and single line diagram in IFC revision, tag information (in Company’s LCI systems) for tags shown on document/drawing shall as a minimum include tag no, description, area, discipline, system and PO references, cross references tag/tag, tag/doc relation." ;
                  rdfs:label "Contractor's LCI execution strategy" ;
                  skos:broadMatch rdl:PCA_100006666 ,
                                  rdl:PCA_100006667 ;
                  skos:broader rdl:PCA_100006759 .


###  http://rds.posccaesar.org/ontology/plm/rdl/PCA_100006136
rdl:PCA_100006136 rdf:type owl:Class ;
                  rdfs:subClassOf rdl:PCA_100004908 ;
                  rdl:PCA_100006763 "A compound document containing information on capabilities, design details, features, and limitations of software." ;
                  rdl:PCA_100006765 rrdl:CFIHOS-20000031 ;
                  rdl:PCA_100006766 rdl:PCA_100006653 ;
                  rdl:PCA_100006768 "A document describing logical and communicative functions including interfaces for a software system." ;
                  rdfs:comment "A document describing logical and communicative functions including interfaces for a software system." ;
                  rdfs:label "Control system software documentation" ;
                  skos:broadMatch rdl:PCA_100006703 ;
                  skos:broader rdl:PCA_100006761 .


###  http://rds.posccaesar.org/ontology/plm/rdl/PCA_100006137
rdl:PCA_100006137 rdf:type owl:Class ;
                  rdfs:subClassOf rdl:PCA_100004908 ;
                  rdl:PCA_100006765 rrdl:CFIHOS-20000020 ;
                  rdl:PCA_100006766 rdl:PCA_100006654 ;
                  rdl:PCA_100006768 "The stress critical lines shall be listed in the document. The list shall include:\n - Line number;\n - Stress ISO document number (typically referenced on piping ISOs/support drawings);\n - Pipe size;\n - Pipe class;\n - Service;\n - Max design temp;\n - Min design temp;\n - Design pressure;\n - PED category (applicable for installations that require conformity with Pressure Equipment Directive);\n - P&ID document number;\n - Pipe stress report document number;\n - Piping stress isometric drawing number;" ;
                  rdfs:comment "The stress critical lines shall be listed in the document. The list shall include:\n - Line number;\n - Stress ISO document number (typically referenced on piping ISOs/support drawings);\n - Pipe size;\n - Pipe class;\n - Service;\n - Max design temp;\n - Min design temp;\n - Design pressure;\n - PED category (applicable for installations that require conformity with Pressure Equipment Directive);\n - P&ID document number;\n - Pipe stress report document number;\n - Piping stress isometric drawing number;" ;
                  rdfs:label "Critical line list" ;
                  skos:broadMatch rdl:PCA_100006716 ,
                                  rdl:PCA_100006717 ;
                  skos:broader rdl:PCA_100006748 .


###  http://rds.posccaesar.org/ontology/plm/rdl/PCA_100006138
rdl:PCA_100006138 rdf:type owl:Class ;
                  rdfs:subClassOf rdl:PCA_100004908 ;
                  rdl:PCA_100006763 "Report documenting seabed intervention required for separation between crossing pipeline, riser or umbilical and provides input to routing design." ;
                  rdl:PCA_100006765 rrdl:CFIHOS-20000031 ;
                  rdl:PCA_100006766 rdl:PCA_100006653 ;
                  rdl:PCA_100006768 "To detail how crossings will be performed." ;
                  rdfs:comment "To detail how crossings will be performed." ;
                  rdfs:label "Crossing design report" ;
                  skos:broadMatch rdl:PCA_100006686 ;
                  skos:broader rdl:PCA_100006756 .


###  http://rds.posccaesar.org/ontology/plm/rdl/PCA_100006139
rdl:PCA_100006139 rdf:type owl:Class ;
                  rdfs:subClassOf rdl:PCA_100004908 ;
                  rdl:PCA_100006763 "Overview of pipeline crossings" ;
                  rdl:PCA_100006765 rrdl:CFIHOS-20000018 ;
                  rdl:PCA_100006766 rdl:PCA_100006654 ;
                  rdl:PCA_100006768 "List of all crossings (pipelines, roads, road allowances, rivers, power line, cables, railway lines etc.) in chronological order along the pipeline (KP) with geographical position, type of crossing and crossing method. Also include reference to relevant crossing design drawings. Owner and content of the crossed object." ;
                  rdfs:comment "List of all crossings (pipelines, roads, road allowances, rivers, power line, cables, railway lines etc.) in chronological order along the pipeline (KP) with geographical position, type of crossing and crossing method. Also include reference to relevant crossing design drawings. Owner and content of the crossed object." ;
                  rdfs:label "Crossing lists" ;
                  skos:broadMatch rdl:PCA_100006720 ;
                  skos:broader rdl:PCA_100006748 .


###  http://rds.posccaesar.org/ontology/plm/rdl/PCA_100006140
rdl:PCA_100006140 rdf:type owl:Class ;
                  rdfs:subClassOf rdl:PCA_100004908 ;
                  rdl:PCA_100006763 "To show internals. Used in engineering and operations." ;
                  rdl:PCA_100006765 rrdl:CFIHOS-20000031 ;
                  rdl:PCA_100006766 rdl:PCA_100006653 ;
                  rdl:PCA_100006768 "A view or drawing that shows what the inside of equipment looks like after a cross-sectional cut has been made, including key parameter capacities for the cross- section." ;
                  rdfs:comment "A view or drawing that shows what the inside of equipment looks like after a cross-sectional cut has been made, including key parameter capacities for the cross- section." ;
                  rdfs:label "Cross-sectional drawing" ;
                  skos:broadMatch rdl:PCA_100006732 ;
                  skos:broader rdl:PCA_100006746 .


###  http://rds.posccaesar.org/ontology/plm/rdl/PCA_100006141
rdl:PCA_100006141 rdf:type owl:Class ;
                  rdfs:subClassOf rdl:PCA_100004908 ;
                  rdl:PCA_100006763 "To document compliance with the PSA facilities regulations § 62 and NMA Regulations No. 878 in addition to IMO instruments and Class requirements, as applicable." ;
                  rdl:PCA_100006765 rrdl:CFIHOS-20000033 ;
                  rdl:PCA_100006766 rdl:PCA_100006657 ;
                  rdl:PCA_100006768 "The damage control plan and damage control booklet are intended to provide information for actions to mitigate the loss of stability in the event of a damage causing flooding. The damage control booklet should include the same information as the damage control plan in addition to general instructions for controlling the effects of damage." ;
                  rdfs:comment "The damage control plan and damage control booklet are intended to provide information for actions to mitigate the loss of stability in the event of a damage causing flooding. The damage control booklet should include the same information as the damage control plan in addition to general instructions for controlling the effects of damage." ;
                  rdfs:label "Damage control booklet" .


###  http://rds.posccaesar.org/ontology/plm/rdl/PCA_100006142
rdl:PCA_100006142 rdf:type owl:Class ;
                  rdfs:subClassOf rdl:PCA_100004908 ;
                  rdl:PCA_100006763 "To document compliance with the PSA facilities regulations § 62 and NMA Regulations No. 878 in addition to IMO instruments and Class requirements, as applicable." ;
                  rdl:PCA_100006765 rrdl:CFIHOS-20000033 ;
                  rdl:PCA_100006766 rdl:PCA_100006657 ;
                  rdl:PCA_100006768 "The damage control plan and damage control booklet are intended to provide information for actions to mitigate the loss of stability in the event of a damage causing flooding. The damage control plan should include inboard profile, plan views of each deck and transverse sections to the extent necessary to show amongst others watertight subdivision and equipment related to maintaining the boundaries and effectiveness of the subdivision." ;
                  rdfs:comment "The damage control plan and damage control booklet are intended to provide information for actions to mitigate the loss of stability in the event of a damage causing flooding. The damage control plan should include inboard profile, plan views of each deck and transverse sections to the extent necessary to show amongst others watertight subdivision and equipment related to maintaining the boundaries and effectiveness of the subdivision." ;
                  rdfs:label "Damage control plan" ;
                  skos:broadMatch rdl:PCA_100006707 ;
                  skos:broader rdl:PCA_100006753 .


###  http://rds.posccaesar.org/ontology/plm/rdl/PCA_100006143
rdl:PCA_100006143 rdf:type owl:Class ;
                  rdfs:subClassOf rdl:PCA_100004908 ;
                  rdl:PCA_100006765 rrdl:CFIHOS-20000030 ;
                  rdl:PCA_100006766 rdl:PCA_100006653 ;
                  rdl:PCA_100006768 "Test reports for Data and telephone cabling network (category type copper cables) shall be provided. Test per outlet." ;
                  rdfs:comment "Test reports for Data and telephone cabling network (category type copper cables) shall be provided. Test per outlet." ;
                  rdfs:label "Data and telephone cabling network test reports" ;
                  skos:broadMatch rdl:PCA_100006722 ;
                  skos:broader rdl:PCA_100006756 .


###  http://rds.posccaesar.org/ontology/plm/rdl/PCA_100006144
rdl:PCA_100006144 rdf:type owl:Class ;
                  rdfs:subClassOf rdl:PCA_100004908 ;
                  rdl:PCA_100006763 "Document providing information on technical data and characteristics about material, products or systems and their environment for proper implementation." ;
                  rdl:PCA_100006766 rdl:PCA_100006653 ;
                  rdl:PCA_100006768 "This document provides structured data form containing part number/model, design information,\noperational data and limitations of the equipment. \nDocument shall provide information on technical data and characteristics about material, products or systems and their environment for proper implementation." ;
                  rdfs:comment "This document provides structured data form containing part number/model, design information,\noperational data and limitations of the equipment. \nDocument shall provide information on technical data and characteristics about material, products or systems and their environment for proper implementation." ;
                  rdfs:label "Data sheet" ;
                  skos:broadMatch rdl:PCA_100006686 ;
                  skos:broader rdl:PCA_100006747 .


###  http://rds.posccaesar.org/ontology/plm/rdl/PCA_100006145
rdl:PCA_100006145 rdf:type owl:Class ;
                  rdfs:subClassOf rdl:PCA_100004908 ;
                  rdl:PCA_100006763 "The equipment supplier standard datasheet shall be delivered." ;
                  rdl:PCA_100006765 rrdl:CFIHOS-20000010 ,
                                    rrdl:CFIHOS-20000011 ;
                  rdl:PCA_100006768 "The datasheet shall as a minimum contain the information specified in the datasheet template. \n\nC999-ST-R-DS-0041 Template - Noise data sheet" ;
                  rdfs:comment "The datasheet shall as a minimum contain the information specified in the datasheet template. \n\nC999-ST-R-DS-0041 Template - Noise data sheet" ;
                  rdfs:label "Data sheet - Noise" ;
                  skos:broadMatch rdl:PCA_100006686 ;
                  skos:broader rdl:PCA_100006747 .


###  http://rds.posccaesar.org/ontology/plm/rdl/PCA_100006146
rdl:PCA_100006146 rdf:type owl:Class ;
                  rdfs:subClassOf rdl:PCA_100004908 ;
                  rdl:PCA_100006763 "This document shall support verification of compliance and provide necessary information" ;
                  rdl:PCA_100006766 rdl:PCA_100006653 ;
                  rdl:PCA_100006768 "Hose data, including pressure, medium, materials" ;
                  rdfs:comment "Hose data, including pressure, medium, materials" ;
                  rdfs:label "Data sheets - Hose" ;
                  skos:broadMatch rdl:PCA_100006686 ;
                  skos:broader rdl:PCA_100006747 .


###  http://rds.posccaesar.org/ontology/plm/rdl/PCA_100006147
rdl:PCA_100006147 rdf:type owl:Class ;
                  rdfs:subClassOf rdl:PCA_100004908 ;
                  rdl:PCA_100006765 rrdl:CFIHOS-20000042 ;
                  rdl:PCA_100006768 "The equipment supplier standard datasheet shall be delivered. · The datasheet shall as a minimum contain the information specified in the applicable datasheet template · Plant specific information (e.g. P.O. number, tag number, P&ID, etc.) is not required · The data sheet shall only describe one equipment type and shall be identified by one document number" ;
                  rdfs:comment "The equipment supplier standard datasheet shall be delivered. · The datasheet shall as a minimum contain the information specified in the applicable datasheet template · Plant specific information (e.g. P.O. number, tag number, P&ID, etc.) is not required · The data sheet shall only describe one equipment type and shall be identified by one document number" ;
                  rdfs:label "Data sheets - Well completion equipment" ;
                  skos:broadMatch rdl:PCA_100006686 ;
                  skos:broader rdl:PCA_100006747 .


###  http://rds.posccaesar.org/ontology/plm/rdl/PCA_100006148
rdl:PCA_100006148 rdf:type owl:Class ;
                  rdfs:subClassOf rdl:PCA_100004908 ;
                  rdl:PCA_100006768 "Content according to ISO 19901-5 ‘Weight control during engineering and construction’, Class A. For equipment packages, separate weight data sheets shall be issued for each piece of equipment shipped and installed separately comprising the total equipment package." ;
                  rdfs:comment "Content according to ISO 19901-5 ‘Weight control during engineering and construction’, Class A. For equipment packages, separate weight data sheets shall be issued for each piece of equipment shipped and installed separately comprising the total equipment package." ;
                  rdfs:label "Data sheets -Weight" ;
                  skos:broadMatch rdl:PCA_100006686 ;
                  skos:broader rdl:PCA_100006747 .


###  http://rds.posccaesar.org/ontology/plm/rdl/PCA_100006149
rdl:PCA_100006149 rdf:type owl:Class ;
                  rdfs:subClassOf rdl:PCA_100004908 ;
                  rdl:PCA_100006763 "Shall be provided for equipment and / or assemblies covered by EU Directives, delivered to projects within the EEA, according to requirements of the relevant EU - directives wrt conformity assessment procedures and eventual necessary involvements of Notified Bodies i.e for EU type examinations thereto , e.g.: EU Directive: 2006/42/EC Machinery Directive EU Directive: 2004/22/EC (MID) Measuring Instruments EU Directive: 2014/68/EU (PED) Pressure Equipment Directive EU Directive: 2014/34/EU (ATEX) Product Directive, EU Directive: 2014/30/EU (EMC) Electromagnetic Compatibility EU Directive: 89/686/EEC (PPE) Personal Protective Equipment EU Regulation: No 1272/2008 (CLP) on classification, labelling and packaging of substances and mixtures, amending and repealing Directives 67/548/EEC and 1999/45/EC, and amending Regulation (EC) No 1907/2006 LVD (2014/35-EU) The guidance of relevant directive shall be considered by the manufacturer when compiling the DoC." ;
                  rdl:PCA_100006765 rrdl:CFIHOS-20000027 ;
                  rdl:PCA_100006768 "The declaration of conformity shall be written up by the manufacturer of the equipment or component, as the legal binding document from the manufacturer / vendor to the purchaser / user ensuring conformity with the relevant EU directive( s). \n\nLocal language: YES for lifting appliances" ;
                  rdfs:comment "The declaration of conformity shall be written up by the manufacturer of the equipment or component, as the legal binding document from the manufacturer / vendor to the purchaser / user ensuring conformity with the relevant EU directive( s). \n\nLocal language: YES for lifting appliances" ;
                  rdfs:label "Declaration of conformity" ;
                  skos:broadMatch rdl:PCA_100006724 ;
                  skos:broader rdl:PCA_100006756 .


###  http://rds.posccaesar.org/ontology/plm/rdl/PCA_100006150
rdl:PCA_100006150 rdf:type owl:Class ;
                  rdfs:subClassOf rdl:PCA_100004908 ;
                  rdl:PCA_100006763 "The document shall describe all inspection and maintenance to be performed to the DEH equipment to ensure safe, reliable and economical operation." ;
                  rdl:PCA_100006765 rrdl:CFIHOS-20000018 ;
                  rdl:PCA_100006766 rdl:PCA_100006657 ;
                  rdl:PCA_100006768 "Proposed maintenance interval and method is to be outlined. In addition, the document shall describe the repair philosophy for the cables with illustrating sketches." ;
                  rdfs:comment "Proposed maintenance interval and method is to be outlined. In addition, the document shall describe the repair philosophy for the cables with illustrating sketches." ;
                  rdfs:label "DEH maintenance and repair procedure" ;
                  skos:broadMatch rdl:PCA_100006688 ;
                  skos:broader rdl:PCA_100006751 .


###  http://rds.posccaesar.org/ontology/plm/rdl/PCA_100006151
rdl:PCA_100006151 rdf:type owl:Class ;
                  rdfs:subClassOf rdl:PCA_100004908 ;
                  rdl:PCA_100006763 "Documentation of ratings" ;
                  rdl:PCA_100006765 rrdl:CFIHOS-20000018 ;
                  rdl:PCA_100006766 rdl:PCA_100006657 ;
                  rdl:PCA_100006768 "The DEH rating report shall give the electrical and thermal rating of the DEH system. Parameters such as current, voltage, system impedance and power are to be calculated for all design modes. Similarly, the thermal performance shall be documented for both steady state and transient conditions." ;
                  rdfs:comment "The DEH rating report shall give the electrical and thermal rating of the DEH system. Parameters such as current, voltage, system impedance and power are to be calculated for all design modes. Similarly, the thermal performance shall be documented for both steady state and transient conditions." ;
                  rdfs:label "DEH rating report" ;
                  skos:broadMatch rdl:PCA_100006686 ;
                  skos:broader rdl:PCA_100006756 .


###  http://rds.posccaesar.org/ontology/plm/rdl/PCA_100006152
rdl:PCA_100006152 rdf:type owl:Class ;
                  rdfs:subClassOf rdl:PCA_100004908 ;
                  rdl:PCA_100006763 "Documentation of the systems" ;
                  rdl:PCA_100006765 rrdl:CFIHOS-20000018 ;
                  rdl:PCA_100006766 rdl:PCA_100006657 ;
                  rdl:PCA_100006768 "Drawing of the DEH system showing all the building blocks the system consists of." ;
                  rdfs:comment "Drawing of the DEH system showing all the building blocks the system consists of." ;
                  rdfs:label "DEH system overview (delivery overview)" ;
                  skos:broadMatch rdl:PCA_100006695 ,
                                  rdl:PCA_100006705 ;
                  skos:broader rdl:PCA_100006746 .


###  http://rds.posccaesar.org/ontology/plm/rdl/PCA_100006153
rdl:PCA_100006153 rdf:type owl:Class ;
                  rdfs:subClassOf rdl:PCA_100004908 ;
                  rdfs:label "Design accidental load report" ;
                  skos:broadMatch rdl:PCA_100006726 ,
                                  rdl:PCA_100006727 ,
                                  rdl:PCA_100006729 ;
                  skos:broader rdl:PCA_100006756 .


###  http://rds.posccaesar.org/ontology/plm/rdl/PCA_100006154
rdl:PCA_100006154 rdf:type owl:Class ;
                  rdfs:subClassOf rdl:PCA_100004908 ;
                  rdl:PCA_100006763 "Accidential load chosen to be used as basis for design. In the design phase, the design accidental load could be more conservative (higher) than the dimensioning accidental load, but should never be lower." ;
                  rdl:PCA_100006765 rrdl:CFIHOS-20000018 ;
                  rdl:PCA_100006766 rdl:PCA_100006654 ;
                  rdl:PCA_100006768 "Covering all possible loads along the pipeline route such as 3rd party activities (e.g. anchoring, trawling, construction, traffic). Could be a part of pipeline desig report." ;
                  rdfs:comment "Covering all possible loads along the pipeline route such as 3rd party activities (e.g. anchoring, trawling, construction, traffic). Could be a part of pipeline desig report." ;
                  rdfs:label "Design accidental loads report" ;
                  skos:broadMatch rdl:PCA_100006686 ;
                  skos:broader rdl:PCA_100006756 .


###  http://rds.posccaesar.org/ontology/plm/rdl/PCA_100006155
rdl:PCA_100006155 rdf:type owl:Class ;
                  rdfs:subClassOf rdl:PCA_100004908 ;
                  rdl:PCA_100006763 "A report providing calculations of the load cases defined for the equipment with reference to applicable standards. The report shall contain loads and load cases as per design basis." ;
                  rdl:PCA_100006766 rdl:PCA_100006653 ;
                  rdl:PCA_100006768 "A report providing calculations of the load cases defined for the equipment with reference to applicable standards." ;
                  rdfs:comment "A report providing calculations of the load cases defined for the equipment with reference to applicable standards." ;
                  rdfs:label "Design calculations and analyses report" ;
                  skos:broader rdl:PCA_100006741 .


###  http://rds.posccaesar.org/ontology/plm/rdl/PCA_100006156
rdl:PCA_100006156 rdf:type owl:Class ;
                  rdfs:subClassOf rdl:PCA_100004908 ;
                  rdl:PCA_100006765 rrdl:CFIHOS-20000018 ;
                  rdl:PCA_100006766 rdl:PCA_100006654 ;
                  rdl:PCA_100006768 "Design documentation (analysis and drawings) of all permanent installation used for construction and installation along the pipeline, such as, but not limited to, turn point and foundation for winches." ;
                  rdfs:comment "Design documentation (analysis and drawings) of all permanent installation used for construction and installation along the pipeline, such as, but not limited to, turn point and foundation for winches." ;
                  rdfs:label "Design documentation of permanent auxiliary installations" ;
                  skos:broadMatch rdl:PCA_100006686 ;
                  skos:broader rdl:PCA_100006741 ,
                               rdl:PCA_100006746 .


###  http://rds.posccaesar.org/ontology/plm/rdl/PCA_100006157
rdl:PCA_100006157 rdf:type owl:Class ;
                  rdfs:subClassOf rdl:PCA_100004908 ;
                  rdl:PCA_100006763 "A report verifying conformance to design specifications." ;
                  rdl:PCA_100006764 "If on System level, (i.e. System Design Report): \nThe objective of the system design report is to give sufficient details arguing the reason for choice of design related to system parameters. This shall apply to all disciplines within all systems. Typical content may be:\n - System description\n - Operational data and limitations\n - Composition of medium\n - Material choice\n - Corrosion evaluations\n - Bases for choice and use of corrosion inhibitors\n - Location of injection points\n - Location of sampling points for analyses\n - Location of areas for corrosion control equipment\n - Project specific features and solutions\n - Hydraulic analysis (fire protection systems)\n - Seabed preparation and intervention work" ;
                  rdl:PCA_100006765 rrdl:CFIHOS-20000031 ;
                  rdl:PCA_100006766 rdl:PCA_100006653 ;
                  rdl:PCA_100006768 "A report containing design analysis/calculations, including loads and load cases. It further summarizes design parameters, system integrity and operational limitations according to design specifications as given by the design basis." ;
                  rdfs:comment "A report containing design analysis/calculations, including loads and load cases. It further summarizes design parameters, system integrity and operational limitations according to design specifications as given by the design basis." ;
                  rdfs:label "Design report" ;
                  skos:broadMatch rdl:PCA_100006686 ;
                  skos:broader rdl:PCA_100006756 .


###  http://rds.posccaesar.org/ontology/plm/rdl/PCA_100006158
rdl:PCA_100006158 rdf:type owl:Class ;
                  rdfs:subClassOf rdl:PCA_100004908 ;
                  rdl:PCA_100006763 "For installation specific requirements to newbuilds and modifications." ;
                  rdl:PCA_100006765 rrdl:CFIHOS-20000026 ;
                  rdl:PCA_100006766 rdl:PCA_100006654 ;
                  rdl:PCA_100006768 "In general, requirements applicable for design of the plant are defined by design basis, Company specifications and international standard." ;
                  rdfs:comment "In general, requirements applicable for design of the plant are defined by design basis, Company specifications and international standard." ;
                  rdfs:label "Design requirements for process and utility systems" ;
                  skos:broadMatch rdl:PCA_100006693 ,
                                  rdl:PCA_100006695 ,
                                  rdl:PCA_100006696 ,
                                  rdl:PCA_100006698 ;
                  skos:broader rdl:PCA_100006757 .


###  http://rds.posccaesar.org/ontology/plm/rdl/PCA_100006159
rdl:PCA_100006159 rdf:type owl:Class ;
                  rdfs:subClassOf rdl:PCA_100004908 ;
                  rdl:PCA_100006763 "Give instructions concerning design requirements." ;
                  rdl:PCA_100006765 rrdl:CFIHOS-20000031 ;
                  rdl:PCA_100006766 rdl:PCA_100006653 ;
                  rdl:PCA_100006768 "Specification for design requirements used for equipment and components." ;
                  rdfs:comment "Specification for design requirements used for equipment and components." ;
                  rdfs:label "Design specification" ;
                  skos:broadMatch rdl:PCA_100006687 ;
                  skos:broader rdl:PCA_100006757 .


###  http://rds.posccaesar.org/ontology/plm/rdl/PCA_100006160
rdl:PCA_100006160 rdf:type owl:Class ;
                  rdfs:subClassOf rdl:PCA_100004908 ;
                  rdl:PCA_100006763 "A detail and cross sectional drawing with parts list to facilitate dismantling, repair and assembly of parts and components shall be included. Relevant for assemblies and smaller components within assemblies." ;
                  rdl:PCA_100006766 rdl:PCA_100006653 ;
                  rdl:PCA_100006768 "A view or drawing that shows what the inside of equipment looks like after a cross-sectional cut has been made.\nThe manufacturer's standard detail cross sectional drawing shall be delivered.\nTypical information may be:\n - Items list with reference to supplier’s  part number.\n - Material definition with reference to relevant  standards" ;
                  rdfs:comment "A view or drawing that shows what the inside of equipment looks like after a cross-sectional cut has been made.\nThe manufacturer's standard detail cross sectional drawing shall be delivered.\nTypical information may be:\n - Items list with reference to supplier’s  part number.\n - Material definition with reference to relevant  standards" ;
                  rdfs:label "Detail cross sectional drawings with parts list" ;
                  skos:broadMatch rdl:PCA_100006732 ;
                  skos:broader rdl:PCA_100006746 .


###  http://rds.posccaesar.org/ontology/plm/rdl/PCA_100006161
rdl:PCA_100006161 rdf:type owl:Class ;
                  rdfs:subClassOf rdl:PCA_100004908 ;
                  rdl:PCA_100006763 "This document shall support verification of supplier’s design with regards to functionality and material selection.\n\nThis document also supports other documents where a cross-sectional view or part list is necessary for clarity." ;
                  rdl:PCA_100006766 rdl:PCA_100006653 ;
                  rdl:PCA_100006768 "A view or drawing that shows what the inside of equipment looks like after a cross-sectional cut has been made.\n\nThe manufacturer's standard detail cross sectional drawing shall be delivered, following content requirements are:\n - Part list with material description.\n - Part numbers can be included or delivered through recommended spare parts list, and is thus not required for all parts. \n - Material definition shall include reference to relevant national/international standards - and material data sheet numbers if additional requirements applies\n - Top Work details in a separate view or sheet shall be included for on/off valves with intended use for gear box or actuator, and if applicable for control valves.\n - Bolt up torque table for pressure containing parts shall be included if not a part of IOM." ;
                  rdfs:comment "A view or drawing that shows what the inside of equipment looks like after a cross-sectional cut has been made.\n\nThe manufacturer's standard detail cross sectional drawing shall be delivered, following content requirements are:\n - Part list with material description.\n - Part numbers can be included or delivered through recommended spare parts list, and is thus not required for all parts. \n - Material definition shall include reference to relevant national/international standards - and material data sheet numbers if additional requirements applies\n - Top Work details in a separate view or sheet shall be included for on/off valves with intended use for gear box or actuator, and if applicable for control valves.\n - Bolt up torque table for pressure containing parts shall be included if not a part of IOM." ;
                  rdfs:label "Detail drawing with parts list" ;
                  skos:broadMatch rdl:PCA_100006732 ;
                  skos:broader rdl:PCA_100006746 .


###  http://rds.posccaesar.org/ontology/plm/rdl/PCA_100006162
rdl:PCA_100006162 rdf:type owl:Class ;
                  rdfs:subClassOf rdl:PCA_100004908 ;
                  rdl:PCA_100006763 "The Design, Fabrication and Installation (DFI) resumés shall provide Operations with a general summary of the installation based on the most relevant information from the design, fabrication and installation phases, and contain information required for plant integrity management and maintenance planning of the facilities throughout the entire lifetime of the installation.\n\nThe document shall also serve as an aid in the consideration of measures to be taken if the condition monitoring reveals that the installation is damaged or deviates from the acceptance criteria." ;
                  rdl:PCA_100006765 rrdl:CFIHOS-20000006 ,
                                    rrdl:CFIHOS-20000031 ;
                  rdl:PCA_100006766 rdl:PCA_100006653 ;
                  rdl:PCA_100006768 "DFI resumes shall be produced in English and in accordance with this standard. The requirement for DFI resume applies to all locations.\n\nIndependent resumes to be made for each major unit or system of the installation, dependant of size and complexity. The Contractor shall incorporate relevant material from their sub-contractors. \n\nThe Fabrication- and Installation-parts shall mainly concentrate on non-conformances from design/fabrication criteria, specifications, etc. Further, areas should be highlighted where special attention in the operational phase is recommended due to e.g. difficult repairs, unexpected large loads or other unforeseen events. Only a brief description of the work performed shall be included.\n\nInformation of foundation performance during installation being relevant for lifetime extension and/or removal shall be included. The required information will depend on foundation system (e.g. pile driving records, suction during penetration, drag lengths vs. tension, penetration during pre-loading).\n\nDFI resumés shall be prepared for:\n - Load bearing structures, such as: Jackets, Gravity Based Structures, Tension Leg Platforms, Semi submersibles, Ships, Jack-Ups, Spars, Subsea structures, Module Support Frames, Modules, Living quarters, Integrated Topsides, Derricks, Flares, Riser support systems and Mooring systems.\n - Pipeline System, including submarine and connected onshore pipelines and risers transporting hydrocarbons and other commodities, with associated safety systems, valves, tool launchers/receivers, internal and external corrosion protection systems, other accessory equipment, and all applied intervention works." ;
                  rdfs:comment "DFI resumes shall be produced in English and in accordance with this standard. The requirement for DFI resume applies to all locations.\n\nIndependent resumes to be made for each major unit or system of the installation, dependant of size and complexity. The Contractor shall incorporate relevant material from their sub-contractors. \n\nThe Fabrication- and Installation-parts shall mainly concentrate on non-conformances from design/fabrication criteria, specifications, etc. Further, areas should be highlighted where special attention in the operational phase is recommended due to e.g. difficult repairs, unexpected large loads or other unforeseen events. Only a brief description of the work performed shall be included.\n\nInformation of foundation performance during installation being relevant for lifetime extension and/or removal shall be included. The required information will depend on foundation system (e.g. pile driving records, suction during penetration, drag lengths vs. tension, penetration during pre-loading).\n\nDFI resumés shall be prepared for:\n - Load bearing structures, such as: Jackets, Gravity Based Structures, Tension Leg Platforms, Semi submersibles, Ships, Jack-Ups, Spars, Subsea structures, Module Support Frames, Modules, Living quarters, Integrated Topsides, Derricks, Flares, Riser support systems and Mooring systems.\n - Pipeline System, including submarine and connected onshore pipelines and risers transporting hydrocarbons and other commodities, with associated safety systems, valves, tool launchers/receivers, internal and external corrosion protection systems, other accessory equipment, and all applied intervention works." ;
                  rdfs:label "DFI resumes" ;
                  skos:broader rdl:PCA_100006749 .


###  http://rds.posccaesar.org/ontology/plm/rdl/PCA_100006163
rdl:PCA_100006163 rdf:type owl:Class ;
                  rdfs:subClassOf rdl:PCA_100004908 ;
                  rdl:PCA_100006763 "Provide clear instructions for how to perform dimensional control including acceptance criteria and reporting." ;
                  rdl:PCA_100006765 rrdl:CFIHOS-20000031 ;
                  rdl:PCA_100006766 rdl:PCA_100006653 ;
                  rdl:PCA_100006768 "A procedure describing the dimensional control methods for different equipment." ;
                  rdfs:comment "A procedure describing the dimensional control methods for different equipment." ;
                  rdfs:label "Dimensional control procedure" ;
                  skos:broadMatch rdl:PCA_100006688 ;
                  skos:broader rdl:PCA_100006751 .


###  http://rds.posccaesar.org/ontology/plm/rdl/PCA_100006164
rdl:PCA_100006164 rdf:type owl:Class ;
                  rdfs:subClassOf rdl:PCA_100004908 ;
                  rdl:PCA_100006763 "Report including verification of critical dimensions specified on drawings." ;
                  rdl:PCA_100006764 "The Dimensional Control Report shall document and verify that specified dimensional and tolerance requirements has been met. The control of dimensions is fundamental to the mechanical engineering discipline, and without which no mechanism could work, no parts would be interchangeable. It is achieved by specifying tolerances – limits to the deviation from nominal dimension. No mechanical drawing is complete without tolerances on all dimensions, limits and fits on mating parts, and flatness tolerances on surfaces." ;
                  rdl:PCA_100006765 rrdl:CFIHOS-20000031 ;
                  rdl:PCA_100006766 rdl:PCA_100006653 ;
                  rdl:PCA_100006768 "The Dimensional Control Report shall document and verify that specified dimensional and tolerance requirements has been met." ;
                  rdfs:comment "The Dimensional Control Report shall document and verify that specified dimensional and tolerance requirements has been met." ;
                  rdfs:label "Dimensional control reports" ;
                  skos:broadMatch rdl:PCA_100006722 ;
                  skos:broader rdl:PCA_100006756 .


###  http://rds.posccaesar.org/ontology/plm/rdl/PCA_100006165
rdl:PCA_100006165 rdf:type owl:Class ;
                  rdfs:subClassOf rdl:PCA_100004908 ;
                  rdl:PCA_100006763 "Verification of tolerances" ;
                  rdl:PCA_100006766 rdl:PCA_100006653 ;
                  rdl:PCA_100006768 "Measured real dimensions" ;
                  rdfs:comment "Measured real dimensions" ;
                  rdfs:label "Dimensional report" ;
                  skos:broadMatch rdl:PCA_100006722 ;
                  skos:broader rdl:PCA_100006756 .


###  http://rds.posccaesar.org/ontology/plm/rdl/PCA_100006166
rdl:PCA_100006166 rdf:type owl:Class ;
                  rdfs:subClassOf rdl:PCA_100004908 ;
                  rdl:PCA_100006763 "A compound document typically containing the following;packing lists, instructions for transport, handling, lifting and preservation, instructions for unpacking if applicable, completed applicable forms for mechanical completion, certificate of conformity, data sheets, preservation log, certificate for lifting equipment, material certificates." ;
                  rdl:PCA_100006765 rrdl:CFIHOS-20000031 ;
                  rdl:PCA_100006766 rdl:PCA_100006653 ;
                  rdl:PCA_100006768 "A document shipped with equipment, enabling correct handling, transport, receipt, storage and preservation. Normally is the dispatch dossier a short version of the full MRB." ;
                  rdfs:comment "A document shipped with equipment, enabling correct handling, transport, receipt, storage and preservation. Normally is the dispatch dossier a short version of the full MRB." ;
                  rdfs:label "Dispatch dossier" ;
                  skos:broadMatch rdl:PCA_100006668 ;
                  skos:broader rdl:PCA_100006762 .


###  http://rds.posccaesar.org/ontology/plm/rdl/PCA_100006167
rdl:PCA_100006167 rdf:type owl:Class ;
                  rdfs:subClassOf rdl:PCA_100004908 ;
                  rdl:PCA_100006763 "The supplier shall supply the documentation needed to enable the customer to evaluate the dispatch and make plans for receipt, storage and installation of the equipment. \n\nDocumentation shall be available to the customer prior to dispatch. Documentation for preservation, packing and transportation method shall be available to the customer prior to dispatch of the equipment." ;
                  rdl:PCA_100006765 rrdl:CFIHOS-20000029 ;
                  rdl:PCA_100006768 "Documentation available to recipient prior to delivery The following documentation shall be available to the recipient prior to delivery of the equipment:\n - Procedure for receiving inspection required by the supplier\n - Guidelines for lifting and handling\n - Requirements for storage and preservation \n\nDocumentation available to recipient at delivery The following documentation shall be available to the recipient no later than at delivery of the equipment:\n - Packing lists\n - Instructions for unpacking, if special precautions are required during unpacking\n - Completed forms for mechanical completion. This applies only if the order includes a clause stating that the supplier shall complete forms forming a part of the purchaser’s system for mechanical completion\n - Preservation log, if this is specified in the order\n - Certificate for temporary lifting equipment" ;
                  rdfs:comment "Documentation available to recipient prior to delivery The following documentation shall be available to the recipient prior to delivery of the equipment:\n - Procedure for receiving inspection required by the supplier\n - Guidelines for lifting and handling\n - Requirements for storage and preservation \n\nDocumentation available to recipient at delivery The following documentation shall be available to the recipient no later than at delivery of the equipment:\n - Packing lists\n - Instructions for unpacking, if special precautions are required during unpacking\n - Completed forms for mechanical completion. This applies only if the order includes a clause stating that the supplier shall complete forms forming a part of the purchaser’s system for mechanical completion\n - Preservation log, if this is specified in the order\n - Certificate for temporary lifting equipment" ;
                  rdfs:label "Documentation for dispatch, receipt, storage and preservation" ;
                  skos:broadMatch rdl:PCA_100006668 ;
                  skos:broader rdl:PCA_100006749 .


###  http://rds.posccaesar.org/ontology/plm/rdl/PCA_100006168
rdl:PCA_100006168 rdf:type owl:Class ;
                  rdfs:subClassOf rdl:PCA_100004908 ;
                  rdl:PCA_100006763 "Documentation of installed cathodic protection equipment to ensure safe operation" ;
                  rdl:PCA_100006765 rrdl:CFIHOS-20000018 ;
                  rdl:PCA_100006766 rdl:PCA_100006657 ;
                  rdl:PCA_100006768 "The drawings for transformer rectifiers units, testposts and belonging components for onshore CP-system shall cover geometry, dimensions, materials, cable routing, cable penetrations for foundation and cabinets." ;
                  rdfs:comment "The drawings for transformer rectifiers units, testposts and belonging components for onshore CP-system shall cover geometry, dimensions, materials, cable routing, cable penetrations for foundation and cabinets." ;
                  rdfs:label "Drawings for onshore cp-system" ;
                  skos:broadMatch rdl:PCA_100006732 ;
                  skos:broader rdl:PCA_100006746 .


###  http://rds.posccaesar.org/ontology/plm/rdl/PCA_100006169
rdl:PCA_100006169 rdf:type owl:Class ;
                  rdfs:subClassOf rdl:PCA_100004908 ;
                  rdl:PCA_100006763 "Survey reports and data shall comply with requirements for Onshore/Offshore surveys." ;
                  rdl:PCA_100006765 rrdl:CFIHOS-20000018 ;
                  rdl:PCA_100006766 rdl:PCA_100006656 ;
                  rdl:PCA_100006768 "Data to be delivered in accordance with Companys' requirements" ;
                  rdfs:comment "Data to be delivered in accordance with Companys' requirements" ;
                  rdfs:label "Dredging, trenching and ploughing survey reports and data" ;
                  skos:broadMatch rdl:PCA_100006705 ;
                  skos:broader rdl:PCA_100006756 ,
                               rdl:PCA_100006762 .


###  http://rds.posccaesar.org/ontology/plm/rdl/PCA_100006170
rdl:PCA_100006170 rdf:type owl:Class ;
                  rdfs:subClassOf rdl:PCA_100004908 ;
                  rdl:PCA_100006763 "To determine maximum sea state for installation of equipment." ;
                  rdl:PCA_100006765 rrdl:CFIHOS-20000031 ;
                  rdl:PCA_100006766 rdl:PCA_100006653 ;
                  rdl:PCA_100006768 "Report documenting all calculations and analysis performed for dynamic installation load cases." ;
                  rdfs:comment "Report documenting all calculations and analysis performed for dynamic installation load cases." ;
                  rdfs:label "Dynamic (installation) load case analysis" ;
                  skos:broadMatch rdl:PCA_100006687 ;
                  skos:broader rdl:PCA_100006741 .


###  http://rds.posccaesar.org/ontology/plm/rdl/PCA_100006171
rdl:PCA_100006171 rdf:type owl:Class ;
                  rdfs:subClassOf rdl:PCA_100004908 ;
                  rdl:PCA_100006763 "Give clear instructions for testing of interfaces between different assemblies and equipment and to verify the sub-system performance and functionality." ;
                  rdl:PCA_100006765 rrdl:CFIHOS-20000031 ;
                  rdl:PCA_100006766 rdl:PCA_100006653 ;
                  rdl:PCA_100006768 "Extended factory acceptance test (EFAT) procedure contains detailed instructions and descriptions for test setup, methods, steps, activities and acceptance criteria for sub-systems. EFAT covers sub-system functionality and equipment interface testing." ;
                  rdfs:comment "Extended factory acceptance test (EFAT) procedure contains detailed instructions and descriptions for test setup, methods, steps, activities and acceptance criteria for sub-systems. EFAT covers sub-system functionality and equipment interface testing." ;
                  rdfs:label "EFAT procedure" ;
                  skos:broadMatch rdl:PCA_100006688 ;
                  skos:broader rdl:PCA_100006751 .


###  http://rds.posccaesar.org/ontology/plm/rdl/PCA_100006172
rdl:PCA_100006172 rdf:type owl:Class ;
                  rdfs:subClassOf rdl:PCA_100004908 ;
                  rdl:PCA_100006763 "Document the tests performed in accordance with the procedure." ;
                  rdl:PCA_100006765 rrdl:CFIHOS-20000031 ;
                  rdl:PCA_100006766 rdl:PCA_100006653 ;
                  rdl:PCA_100006768 "Report containing results from the EFAT including check records and pictures from the procedure steps." ;
                  rdfs:comment "Report containing results from the EFAT including check records and pictures from the procedure steps." ;
                  rdfs:label "EFAT report" ;
                  skos:broadMatch rdl:PCA_100006722 ;
                  skos:broader rdl:PCA_100006756 .


###  http://rds.posccaesar.org/ontology/plm/rdl/PCA_100006173
rdl:PCA_100006173 rdf:type owl:Class ;
                  rdfs:subClassOf rdl:PCA_100004908 ;
                  rdl:PCA_100006763 "Electrical block diagram shall show configuration of an electrical system/package and subsystems or relevant interfaces to give a functional understanding." ;
                  rdl:PCA_100006765 rrdl:CFIHOS-20000008 ;
                  rdl:PCA_100006766 rdl:PCA_100006634 ,
                                    rdl:PCA_100006635 ,
                                    rdl:PCA_100006636 ,
                                    rdl:PCA_100006637 ,
                                    rdl:PCA_100006638 ,
                                    rdl:PCA_100006639 ,
                                    rdl:PCA_100006640 ,
                                    rdl:PCA_100006641 ,
                                    rdl:PCA_100006642 ;
                  rdl:PCA_100006768 "Electrical block diagram typical contents shall be:\n - All related systems and subsystems or eventual packages and interfaces represented by blocks;\n - Short description;\n - Location of equipment;\n - Tag number (when applicable);\n - Interface cabling between blocks within the package and all interface cables towards other packages shall be indicated." ;
                  rdfs:comment "Electrical block diagram typical contents shall be:\n - All related systems and subsystems or eventual packages and interfaces represented by blocks;\n - Short description;\n - Location of equipment;\n - Tag number (when applicable);\n - Interface cabling between blocks within the package and all interface cables towards other packages shall be indicated." ;
                  rdfs:label "Electrical block diagrams" ;
                  skos:broadMatch rdl:PCA_100006695 ,
                                  rdl:PCA_100006696 ,
                                  rdl:PCA_100006699 ;
                  skos:broader rdl:PCA_100006740 .


###  http://rds.posccaesar.org/ontology/plm/rdl/PCA_100006174
rdl:PCA_100006174 rdf:type owl:Class ;
                  rdfs:subClassOf rdl:PCA_100004908 ;
                  rdl:PCA_100006763 "Electrical calculations / analyses are required to be done according to IEC 61892-2 to confirm the design of the electrical system and corresponding ratings of the equipment:\n\nGeneral EMC planning shall be in accordance with IEC 60533, Annex B(Offshore) or IEC 61000-2-5 (onshore).\n\nArc flash study is required to be done according to IEEE Std 1584 to calculate arc incident energy." ;
                  rdl:PCA_100006764 "The following studies are required to be done:\n - Electrical load study:\n     - The electrical load study shall be done to determine major equipment ratings.\n     - An allowance and contingency multiplication factor shall be applied to the estimated load to select the rating of generators and transformers.\n - Load flow calculations:\n     - Load flow calculations shall be done to check the voltage profile and circuit loading under steady state conditions. Calculations shall include:\n     - All general modes (such as main power mode, essential mode, emergency mode).\n           - Different network configuration (such as open bus tie breaker, closed bus tie breaker with single incomer supply).\n           - Different load scenarios (maximum load, no load).\n - Short circuit analysis calculations:\n     - Short circuit calculations shall be done to determine maximum stresses during fault conditions. The results shall be used for specifying equipment ratings and to determine setting of protection.\n - Protection and discrimination study:\n     - The protection and discrimination study shall be done to provide correct protection and discrimination.\n     - The study shall include the following main subjects:\n           - Network description.\n           - Short overview of plant, with a subchapter per voltage level and system.\n           - Operational modes description.\n           - Full production mode, drilling mode, essential mode, emergency mode, UPS mode.\n           - Protection relays and functions per circuit type.\n           - Description of each individual protective device for the plant.\n           - Fuse selection.\n           - Fuse selection criteria, short circuit protection of consumer and contactor in starter/feeder, starting current versus starting time, load current and overload protection.\n           - Protection principles.\n           - Protection principles per system and operational mode.\n           - This to include phase-phase faults and phase-earth faults in separate subsections.\n           - Coordination of earth fault relays with different operating characteristic to be handled especially.\n           - Protection principles per equipment type (equipment protection).\n           - Protection relay templates.\n           - Template per make/type of protection and per type of equipment to be protected.\n           - Setting tables.\n           - All individual setting parameters to be included. This shall also include protective relay settings on mechanical packages (e.g. firefighting system).\n           - Current - time diagrams.\n           - Logarithms current versus time curves (for visually documenting selectivity in the system and proper protection of equipment and cables).\n           - All cases where curves indicate conflict with defined principles or criteria shall be explained.\n - Power system dynamic study:\n     - The dynamic study shall be done to analyse the transient and dynamic performance of the power system.\n     - Calculations shall include (as applicable) the dynamic performance when:\n           - Starting/ energising largest motor/ consumer at each main switchboard.\n           - Stopping/deenergising the largest possible group of consumers (due to e.g. process shut down).\n           - Trip of one generator (or power source), with and without load shedding.\n           - Short circuit in the primary distribution system, cleared by short circuit protection.\n           - Other as required.\n           - Calculations shall be done for different preconditions as follows:\n           - All power modes (such as main power mode, essential mode, emergency mode, testing of the essential and emergency generator).\n           - Different network configuration (especially those giving the extreme dynamic disturbance conditions).\n - Calculations of harmonic voltages:\n     - Calculations shall be done to verify that harmonic distortions in all operating modes are within defined limitations.\n - Switching/equipment insulation study:\n     - A switching/equipment insulation study shall when necessary be performed in order to specify the correct equipment insulation levels and to determine whether additional protections are required.\n - Electromagnetic compatibility (EMC):\n \n     - The above referred standards as well as the manufacturer’s and supplier’s instructions with regards to EMC shall be followed and taken into account in the design.\n - Cable selection and sizing criteria:\n     - An electrical cable sizing study shall be performed in order to establish cable sizing criteria.\n     - The following subjects shall be taken into account when making general cable sizing criteria:\n           - Consumer/ circuit nominal current.\n           - Motor start current (motor circuits).\n           - For voltage drop from generator terminals (in primary distribution system) or transformer secondary terminals (in secondary distribution system), stationary and transient.\n           - Cables’ short circuits withstand capabilities (both mechanical and thermal). To be coordinated with short circuit protection.\n           - Short circuit (phase to phase) at the end of the power cable supplying small power and lighting should cause instantaneous trip of the protective device.\n           - The type of cable to be used for each purpose and area shall be fully described (e.g. mud/oil resistant, fire resistant etc.).\n           - Current ratings for cables and de-rating factors for ambient temperature and cable grouping.\n           - The study shall as a minimum summarise the following results:\n                 - Cable current capacity (maximum current) per type and size of cable.\n                 \nStudies shall be done according to relevant IEC standards and more detailed company specific requirements. \n\nIf electrical power system design and simulation software is used, all modified or new files shall be transferred to Company as files of the software that is used. The report from the system study shall be delivered as a text file." ;
                  rdl:PCA_100006765 rrdl:CFIHOS-20000008 ;
                  rdl:PCA_100006766 rdl:PCA_100006634 ,
                                    rdl:PCA_100006635 ,
                                    rdl:PCA_100006636 ,
                                    rdl:PCA_100006637 ,
                                    rdl:PCA_100006638 ,
                                    rdl:PCA_100006639 ;
                  rdfs:label "Electrical calculations / analyses" ;
                  skos:broadMatch rdl:PCA_100006687 ;
                  skos:broader rdl:PCA_100006741 .


###  http://rds.posccaesar.org/ontology/plm/rdl/PCA_100006175
rdl:PCA_100006175 rdf:type owl:Class ;
                  rdfs:subClassOf rdl:PCA_100004908 ;
                  rdl:PCA_100006764 "The equipment supplier standard drawing to be delivered. The external connection diagram should typically include:\n - Terminal/pin number\n - Earthing details \nInternal wiring diagrams shall be supplied when relevant e.g. to show the wiring between different electrical equipment within a package, and should typically include: \n - Terminal block/socket number\n - Terminal/pin number (including spares)\n - Internal cable numbers with pair and core colour details\n - Destination for internal cables\n - Earthing details\n - Equipment and equipment connections\n - External cables with pair and core colour details" ;
                  rdl:PCA_100006765 rrdl:CFIHOS-20000008 ;
                  rdfs:label "Electrical connection and wiring diagram - instrument" ;
                  skos:broadMatch rdl:PCA_100006702 ,
                                  rdl:PCA_100006712 ;
                  skos:broader rdl:PCA_100006745 .


###  http://rds.posccaesar.org/ontology/plm/rdl/PCA_100006176
rdl:PCA_100006176 rdf:type owl:Class ;
                  rdfs:subClassOf rdl:PCA_100004908 ;
                  rdl:PCA_100006764 "The external connection diagram shall typically include:\n - Tag number of equipment\n - External cable tag number\n - Earthing details\nInternal wiring diagrams shall be supplied when relevant e.g. to show the wiring between different electrical equipment within a package, and shall typically include:\n - Terminal block/socket number\n - Destination for internal cables\n - Earthing details" ;
                  rdl:PCA_100006765 rrdl:CFIHOS-20000008 ;
                  rdfs:label "Electrical connection and wiring diagram – well completion" ;
                  skos:broadMatch rdl:PCA_100006702 ,
                                  rdl:PCA_100006712 ;
                  skos:broader rdl:PCA_100006745 .


###  http://rds.posccaesar.org/ontology/plm/rdl/PCA_100006177
rdl:PCA_100006177 rdf:type owl:Class ;
                  rdfs:subClassOf rdl:PCA_100004908 ;
                  rdl:PCA_100006763 "The diagram shall show the electrical connection between different electrical equipment and components within a package. The diagram shall also identify all connections to Company’s power supply and instrumented systems." ;
                  rdl:PCA_100006764 "Electrical connection diagram shall typical include the following:\n - Tag number of equipment to which the cable ends are terminated;\n - Signal tag number;\n - External cable tag number;\n - External cables with pair or wire number and core colour details;\n - Terminal block/socket number;\n - Earthing details;\n - Reference drawings." ;
                  rdl:PCA_100006765 rrdl:CFIHOS-20000008 ,
                                    rrdl:CFIHOS-20000030 ,
                                    rrdl:CFIHOS-20000031 ;
                  rdl:PCA_100006766 rdl:PCA_100006634 ,
                                    rdl:PCA_100006635 ,
                                    rdl:PCA_100006636 ,
                                    rdl:PCA_100006637 ,
                                    rdl:PCA_100006638 ,
                                    rdl:PCA_100006639 ,
                                    rdl:PCA_100006640 ,
                                    rdl:PCA_100006641 ,
                                    rdl:PCA_100006642 ;
                  rdfs:label "Electrical connection diagram" ;
                  skos:broadMatch rdl:PCA_100006702 ,
                                  rdl:PCA_100006712 ;
                  skos:broader rdl:PCA_100006745 .


###  http://rds.posccaesar.org/ontology/plm/rdl/PCA_100006178
rdl:PCA_100006178 rdf:type owl:Class ;
                  rdfs:subClassOf rdl:PCA_100004908 ;
                  rdl:PCA_100006765 rrdl:CFIHOS-20000008 ;
                  rdl:PCA_100006766 rdl:PCA_100006656 ;
                  rdl:PCA_100006768 "At least one field equipment layout drawing for each area or module deck level shall be produced. The size of the facility will determine the scale of the drawing, but normally a scale of 1:100 on A3 format shall be aimed for. If required several drawings per area can be necessary to achieve this scale. Equipment which is covered by platforms above shall be shown dotted or shown in separate figures.\n\nThe following content shall be included on the drawings:\n - Platform/plant northing and orientation with respect of true north;\n - Gridlines with north and east references;\n - Key plan;\n - Scale bar;\n - Match lines with drawing references;\n - Deck/area elevations;\n - Location of electrical field equipment as identified in MEL;\n - Equipment shall be tagged according to MEL." ;
                  rdfs:comment "At least one field equipment layout drawing for each area or module deck level shall be produced. The size of the facility will determine the scale of the drawing, but normally a scale of 1:100 on A3 format shall be aimed for. If required several drawings per area can be necessary to achieve this scale. Equipment which is covered by platforms above shall be shown dotted or shown in separate figures.\n\nThe following content shall be included on the drawings:\n - Platform/plant northing and orientation with respect of true north;\n - Gridlines with north and east references;\n - Key plan;\n - Scale bar;\n - Match lines with drawing references;\n - Deck/area elevations;\n - Location of electrical field equipment as identified in MEL;\n - Equipment shall be tagged according to MEL." ;
                  rdfs:label "Electrical field equipment layout drawings" ;
                  skos:broadMatch rdl:PCA_100006710 ;
                  skos:broader rdl:PCA_100006746 .


###  http://rds.posccaesar.org/ontology/plm/rdl/PCA_100006179
rdl:PCA_100006179 rdf:type owl:Class ;
                  rdfs:subClassOf rdl:PCA_100004908 ;
                  rdl:PCA_100006763 "See requirements to load study, ref. (Z-001-0052 - Electrical calculations / analyses). \nThe purpose of this document is to define the electrical loading of the electrical power system." ;
                  rdl:PCA_100006765 rrdl:CFIHOS-20000008 ;
                  rdl:PCA_100006766 rdl:PCA_100006634 ,
                                    rdl:PCA_100006635 ,
                                    rdl:PCA_100006636 ,
                                    rdl:PCA_100006637 ,
                                    rdl:PCA_100006638 ,
                                    rdl:PCA_100006639 ;
                  rdl:PCA_100006768 "An electrical load list shall be worked out based on the Main Equipment List and emergency and/or essential consumers clearly marked as such in the list. Load list shall include individual consumers on high and low voltage switchboards (motor control centers) as well as assumed sum load on 400/230 V level. Sum UPS load per UPS system shall be listed. Allowance and contingency requirements for the load list shall be applied." ;
                  rdfs:comment "An electrical load list shall be worked out based on the Main Equipment List and emergency and/or essential consumers clearly marked as such in the list. Load list shall include individual consumers on high and low voltage switchboards (motor control centers) as well as assumed sum load on 400/230 V level. Sum UPS load per UPS system shall be listed. Allowance and contingency requirements for the load list shall be applied." ;
                  rdfs:label "Electrical load list" ;
                  skos:broadMatch rdl:PCA_100006716 ,
                                  rdl:PCA_100006717 ;
                  skos:broader rdl:PCA_100006748 .


###  http://rds.posccaesar.org/ontology/plm/rdl/PCA_100006180
rdl:PCA_100006180 rdf:type owl:Class ;
                  rdfs:subClassOf rdl:PCA_100004908 ;
                  rdl:PCA_100006763 "Power System Philosophy shall outline the design and operation of the electrical power supply and distribution systems. The document shall be the guideline for the electrical system detail design, supplier equipment and software deliveries to the power systems like switchboards, generators, variable speed drives etc." ;
                  rdl:PCA_100006765 rrdl:CFIHOS-20000008 ;
                  rdl:PCA_100006766 rdl:PCA_100006634 ,
                                    rdl:PCA_100006635 ,
                                    rdl:PCA_100006636 ,
                                    rdl:PCA_100006637 ,
                                    rdl:PCA_100006638 ,
                                    rdl:PCA_100006639 ,
                                    rdl:PCA_100006641 ;
                  rdl:PCA_100006768 "The document shall include an overview of:\n - The overall power system;\n - The hardwired electrical interlock/inter-tripping principles throughout the electrical distribution system;\n - An overview of the control philosophy;\n - The general principles for the Power Distribution Control System (PDCS);\n - The power management functions;\n - The operating requirements and interface between control facilities and electrical equipment;\n - The principles for remote access and monitoring of the electrical equipment.\n\nThe document shall further describe the various operating modes of the power system like:\n - Normal modes;\n - Emergency modes;\n - Maintenance modes;\n - Others (as applicable).\n\nThe reliability of the grid supply shall be assessed (if applicable)." ;
                  rdfs:comment "The document shall include an overview of:\n - The overall power system;\n - The hardwired electrical interlock/inter-tripping principles throughout the electrical distribution system;\n - An overview of the control philosophy;\n - The general principles for the Power Distribution Control System (PDCS);\n - The power management functions;\n - The operating requirements and interface between control facilities and electrical equipment;\n - The principles for remote access and monitoring of the electrical equipment.\n\nThe document shall further describe the various operating modes of the power system like:\n - Normal modes;\n - Emergency modes;\n - Maintenance modes;\n - Others (as applicable).\n\nThe reliability of the grid supply shall be assessed (if applicable)." ;
                  rdfs:label "Electrical power system philosophy" ;
                  skos:broadMatch rdl:PCA_100006695 ,
                                  rdl:PCA_100006698 ;
                  skos:broader rdl:PCA_100006752 .


###  http://rds.posccaesar.org/ontology/plm/rdl/PCA_100006181
rdl:PCA_100006181 rdf:type owl:Class ;
                  rdfs:subClassOf rdl:PCA_100004908 ;
                  rdl:PCA_100006763 "Illustrate electrical equipment with lines and connections." ;
                  rdl:PCA_100006764 "Electrical Circuit/Schematics shall be prepared for all feeders and control circuits (except for small components ). This diagram shall include all internal\nconnections for control, alarms, protection, interlocks, trip functions, monitoring, etc." ;
                  rdl:PCA_100006765 rrdl:CFIHOS-20000031 ;
                  rdl:PCA_100006766 rdl:PCA_100006653 ;
                  rdl:PCA_100006768 "A diagram showing electrical and fiber optical connections between different equipment and components." ;
                  rdfs:comment "A diagram showing electrical and fiber optical connections between different equipment and components." ;
                  rdfs:label "Electrical schematics" ;
                  skos:broadMatch rdl:PCA_100006702 ;
                  skos:broader rdl:PCA_100006745 .


###  http://rds.posccaesar.org/ontology/plm/rdl/PCA_100006182
rdl:PCA_100006182 rdf:type owl:Class ;
                  rdfs:subClassOf rdl:PCA_100004908 ;
                  rdl:PCA_100006763 "For electrical and fiber-optical downhole instruments the supplier shall work out hook-up drawings. The drawing shall visualize the instrumentation in an entire well." ;
                  rdl:PCA_100006764 "A typical hook-up drawing shall indicate details such as:\n - All instruments/type installed by Supplier\n - Location in well relative to zones/branches\n - Measuring point relative to tubing/annulus (gauges only)\n - Connections and interconnections of signal lines\nThe drawing shall indicate split of responsibilities between Supplier and Purchaser." ;
                  rdl:PCA_100006765 rrdl:CFIHOS-20000008 ;
                  rdfs:label "Electrical/fiberoptical hook-up drawing - well completion" ;
                  skos:broadMatch rdl:PCA_100006712 ,
                                  rdl:PCA_100006731 ,
                                  rdl:PCA_100006732 ;
                  skos:broader rdl:PCA_100006746 .


###  http://rds.posccaesar.org/ontology/plm/rdl/PCA_100006183
rdl:PCA_100006183 rdf:type owl:Class ;
                  rdfs:subClassOf rdl:PCA_100004908 ;
                  rdl:PCA_100006763 "The Emergency preparedness analysis report shall reflect the current operating conditions and experience and be written in a way to facilitate the use by the operating organization. See NORSOK Z-013 for further details." ;
                  rdl:PCA_100006765 rrdl:CFIHOS-20000010 ,
                                    rrdl:CFIHOS-20000011 ,
                                    rrdl:CFIHOS-20000013 ;
                  rdl:PCA_100006766 rdl:PCA_100006654 ;
                  rdfs:label "Emergency preparedness analysis" ;
                  skos:broadMatch rdl:PCA_100006729 ;
                  skos:broader rdl:PCA_100006756 .


###  http://rds.posccaesar.org/ontology/plm/rdl/PCA_100006184
rdl:PCA_100006184 rdf:type owl:Class ;
                  rdfs:subClassOf rdl:PCA_100004908 ;
                  rdl:PCA_100006763 "Schedule of planned activities from order entry to delivery. EPMS substantiates compliance with delivery requirements, and support planning of expediting activities." ;
                  rdl:PCA_100006765 rrdl:CFIHOS-20000001 ;
                  rdl:PCA_100006766 rdl:PCA_100006653 ;
                  rdl:PCA_100006768 "Schedule to include planned activities from order receipt, order entry to sub-suppliers, goods receipt, assembly, testing and shipping/delivery." ;
                  rdfs:comment "Schedule to include planned activities from order receipt, order entry to sub-suppliers, goods receipt, assembly, testing and shipping/delivery." ;
                  rdfs:label "Engineering, procurement and manufacturing schedule" ;
                  skos:broadMatch rdl:PCA_100006667 .


###  http://rds.posccaesar.org/ontology/plm/rdl/PCA_100006185
rdl:PCA_100006185 rdf:type owl:Class ;
                  rdfs:subClassOf rdl:PCA_100004908 ;
                  rdl:PCA_100006764 "Consists of:\n - Environmental Design Review report. This is the report from environmental design review performed. Could be a separate review report or a part of a HSE design Review report. \n - Environmental budget report. This report shall specify the yearly emissions to air (CO2, Nox, CH4, nmVOC, H2S, SOx, NH3 and particles) for the selected concept. The report shall also specify the yearly discharges to sea of process water, produced water, oil in water, chemicals in water and estimate of yearly waste fractions that must be handled.\n - BAT (Best Available Techniques) Evaluation Report. This report shall cover the BAT evaluations performed before the choice of technology was taken. Typical items will be power and heat generation, flare and vent systems, technology for reducing emission to air, material choice and use of chemicals, technology for reducing discharge to sea/water, e.g. cleaning technology." ;
                  rdl:PCA_100006765 rrdl:CFIHOS-20000010 ;
                  rdfs:label "Environment report" ;
                  skos:broadMatch rdl:PCA_100006728 ;
                  skos:broader rdl:PCA_100006756 .


###  http://rds.posccaesar.org/ontology/plm/rdl/PCA_100006186
rdl:PCA_100006186 rdf:type owl:Class ;
                  rdfs:subClassOf rdl:PCA_100004908 ;
                  rdl:PCA_100006763 "Description of heat emission from installed equipment shall be per room/area, tag based. The heat emission shall be stated in normal, emergency and UPS operation modes." ;
                  rdl:PCA_100006765 rrdl:CFIHOS-20000019 ;
                  rdl:PCA_100006766 rdl:PCA_100006653 ;
                  rdfs:label "Equipment heat emission" ;
                  skos:broadMatch rdl:PCA_100006687 ;
                  skos:broader rdl:PCA_100006741 .


###  http://rds.posccaesar.org/ontology/plm/rdl/PCA_100006187
rdl:PCA_100006187 rdf:type owl:Class ;
                  rdfs:subClassOf rdl:PCA_100004908 ;
                  rdl:PCA_100006763 "To give the installer instruction for installation of the equipment subsea." ;
                  rdl:PCA_100006765 rrdl:CFIHOS-20000031 ;
                  rdl:PCA_100006766 rdl:PCA_100006653 ;
                  rdl:PCA_100006768 "An equipment specific procedure providing the steps for installation and retrieval including limitations." ;
                  rdfs:comment "An equipment specific procedure providing the steps for installation and retrieval including limitations." ;
                  rdfs:label "Equipment installation & retrieval procedure" ;
                  skos:broadMatch rdl:PCA_100006688 ;
                  skos:broader rdl:PCA_100006751 .


###  http://rds.posccaesar.org/ontology/plm/rdl/PCA_100006188
rdl:PCA_100006188 rdf:type owl:Class ;
                  rdfs:subClassOf rdl:PCA_100004908 ;
                  rdl:PCA_100006765 rrdl:CFIHOS-20000020 ;
                  rdl:PCA_100006766 rdl:PCA_100006656 ;
                  rdl:PCA_100006768 "These drawings are relevant for offshore facilities and for the process plant and well pad area for onshore facilities.\n\nAt least one equipment layout drawing for each area or module deck level shall be produced. The size of the facility will determine the scale of the drawing, but normally a scale of 1:100 on A3 format shall be aimed for. If required several drawings per area can be necessary to achieve this scale. Equipment, which is covered by platforms above, shall be shown dotted or shown in separate figures. \n\nThe following content shall be included on the drawings:\n - Platform/plant northing and orientation with respect of true north;\n - Gridlines with north and east references;\n - Key plan;\n - Scale bar;\n - Match lines with drawing references;\n - Deck/area elevations;\n - Area segregation, with fire partitions indicated;\n - Maintenance/withdrawal areas for main components (compressor bundles, cooler internals, etc.);\n - Laydown areas;\n - Waste sorting stations;\n - Pipe racks;\n - Stairs, access and escape routes;\n - Material handling routes;\n - Manifold area arrangement;\n - Well head area, with number of wells and distance between wells indicated;\n - Drilling derrick extreme outlines indicated;\n - Location of temporary well intervention equipment;\n - Flare tower location and extreme outlines indicated;\n - HVAC, instrument and electrical rooms (relevant for offshore facility);\n - Control room (relevant for offshore facility);\n - Living Quarter outline. Reference to relevant Architectural layout drawings shall be included;\n - Main structures;\n - Location of all equipment as identified in MEL including identification of datum point;\n - Equipment shall be tagged according to MEL. An equipment index shall be included on the drawing. Datum point coordinates shall be included in this index;\n - Safety evacuation equipment, such as escape tunnels, lifeboats, escape chutes, etc. (relevant for offshore facility);\n - Hose loading station and tote tank area (relevant for offshore facility);\n - Utility stations;\n - Space allocation for risers, J-tubes and umbilicals including temporary equipment (pulling arrangement). (relevant for offshore facility);\n - Space for future areas/modules/equipment." ;
                  rdfs:comment "These drawings are relevant for offshore facilities and for the process plant and well pad area for onshore facilities.\n\nAt least one equipment layout drawing for each area or module deck level shall be produced. The size of the facility will determine the scale of the drawing, but normally a scale of 1:100 on A3 format shall be aimed for. If required several drawings per area can be necessary to achieve this scale. Equipment, which is covered by platforms above, shall be shown dotted or shown in separate figures. \n\nThe following content shall be included on the drawings:\n - Platform/plant northing and orientation with respect of true north;\n - Gridlines with north and east references;\n - Key plan;\n - Scale bar;\n - Match lines with drawing references;\n - Deck/area elevations;\n - Area segregation, with fire partitions indicated;\n - Maintenance/withdrawal areas for main components (compressor bundles, cooler internals, etc.);\n - Laydown areas;\n - Waste sorting stations;\n - Pipe racks;\n - Stairs, access and escape routes;\n - Material handling routes;\n - Manifold area arrangement;\n - Well head area, with number of wells and distance between wells indicated;\n - Drilling derrick extreme outlines indicated;\n - Location of temporary well intervention equipment;\n - Flare tower location and extreme outlines indicated;\n - HVAC, instrument and electrical rooms (relevant for offshore facility);\n - Control room (relevant for offshore facility);\n - Living Quarter outline. Reference to relevant Architectural layout drawings shall be included;\n - Main structures;\n - Location of all equipment as identified in MEL including identification of datum point;\n - Equipment shall be tagged according to MEL. An equipment index shall be included on the drawing. Datum point coordinates shall be included in this index;\n - Safety evacuation equipment, such as escape tunnels, lifeboats, escape chutes, etc. (relevant for offshore facility);\n - Hose loading station and tote tank area (relevant for offshore facility);\n - Utility stations;\n - Space allocation for risers, J-tubes and umbilicals including temporary equipment (pulling arrangement). (relevant for offshore facility);\n - Space for future areas/modules/equipment." ;
                  rdfs:label "Equipment layout drawings" ;
                  skos:broadMatch rdl:PCA_100006710 ;
                  skos:broader rdl:PCA_100006746 .


###  http://rds.posccaesar.org/ontology/plm/rdl/PCA_100006189
rdl:PCA_100006189 rdf:type owl:Class ;
                  rdfs:subClassOf rdl:PCA_100004908 ;
                  rdl:PCA_100006765 rrdl:CFIHOS-20000008 ,
                                    rrdl:CFIHOS-20000015 ,
                                    rrdl:CFIHOS-20000030 ;
                  rdl:PCA_100006766 rdl:PCA_100006656 ;
                  rdl:PCA_100006768 "Equipment room layout drawings shall be provided: \n - For areas equipped with instrument equipment cabinets/racks. Examples of such areas are: Central/ local equipment rooms (with instrument equipment cabinets/racks);\n - For electrical equipment room(s) in which switchgears, main distributions boards, transformers, UPS, etc. are located;\n - For areas equipped with telecommunication equipment, cabinets/racks. Examples of such areas are: Telecommunication equipment rooms and Local equipment rooms (with telecom equipment cabinets/racks.\n\nThe following information shall be shown:\n - Main Equipment with tag number (from all disciplines);\n - Reserved space for spare equipment;\n - Walls and doors;\n - Stairs and raised floor;\n - Equipment list including tag number, tag description and datum point coordinates." ;
                  rdfs:comment "Equipment room layout drawings shall be provided: \n - For areas equipped with instrument equipment cabinets/racks. Examples of such areas are: Central/ local equipment rooms (with instrument equipment cabinets/racks);\n - For electrical equipment room(s) in which switchgears, main distributions boards, transformers, UPS, etc. are located;\n - For areas equipped with telecommunication equipment, cabinets/racks. Examples of such areas are: Telecommunication equipment rooms and Local equipment rooms (with telecom equipment cabinets/racks.\n\nThe following information shall be shown:\n - Main Equipment with tag number (from all disciplines);\n - Reserved space for spare equipment;\n - Walls and doors;\n - Stairs and raised floor;\n - Equipment list including tag number, tag description and datum point coordinates." ;
                  rdfs:label "Equipment room layout drawings" ;
                  skos:broadMatch rdl:PCA_100006710 ;
                  skos:broader rdl:PCA_100006746 .


###  http://rds.posccaesar.org/ontology/plm/rdl/PCA_100006190
rdl:PCA_100006190 rdf:type owl:Class ;
                  rdfs:subClassOf rdl:PCA_100004908 ;
                  rdl:PCA_100006764 "Context specific information to be added" ;
                  rdl:PCA_100006765 rrdl:CFIHOS-20000015 ;
                  rdl:PCA_100006768 "Piping and Instrument Diagram (P&ID) includes the complete set of P&IDs, typicals and legends. Equipment supplier's drafting standard shall be used. Symbols used shall be described by a symbol legend on the P&ID, or as a separate document/drawing/P&ID sheet. All connections external to the supply shall be shown on the P&ID, marked with a unique number (N1, N2, etc.). Reference to the interfacing external P&IDs should also be given.\nAll interface signals to and from the plant’s safety and automation systems shall be shown \nwith reference to the interfacing external P&IDs. Control and monitoring functions shall be \ndrawn on the P&ID, this also applies for control panel locally within the supply.\nIdentical parallel items or systems shall be drawn in full detail, i.e. typical drawings with \nassociated tag number tables are not acceptable.\nUnique plant tags shall be used as assigned by the engineering contractor. Supplier’s \ninternal tag numbers shall be shown in addition where required for use of supplier’s standard\ndocumentation, preferably by use of tables on the P&ID/separate P&ID sheet, linking unique \nplant tag with supplier’s internal tag." ;
                  rdfs:comment "Piping and Instrument Diagram (P&ID) includes the complete set of P&IDs, typicals and legends. Equipment supplier's drafting standard shall be used. Symbols used shall be described by a symbol legend on the P&ID, or as a separate document/drawing/P&ID sheet. All connections external to the supply shall be shown on the P&ID, marked with a unique number (N1, N2, etc.). Reference to the interfacing external P&IDs should also be given.\nAll interface signals to and from the plant’s safety and automation systems shall be shown \nwith reference to the interfacing external P&IDs. Control and monitoring functions shall be \ndrawn on the P&ID, this also applies for control panel locally within the supply.\nIdentical parallel items or systems shall be drawn in full detail, i.e. typical drawings with \nassociated tag number tables are not acceptable.\nUnique plant tags shall be used as assigned by the engineering contractor. Supplier’s \ninternal tag numbers shall be shown in addition where required for use of supplier’s standard\ndocumentation, preferably by use of tables on the P&ID/separate P&ID sheet, linking unique \nplant tag with supplier’s internal tag." ;
                  rdfs:label "Equipment supplier piping and instrument diagram (P&ID)" ;
                  skos:broadMatch rdl:PCA_100006696 ;
                  skos:broader rdl:PCA_100006745 .


###  http://rds.posccaesar.org/ontology/plm/rdl/PCA_100006191
rdl:PCA_100006191 rdf:type owl:Class ;
                  rdfs:subClassOf rdl:PCA_100004908 ;
                  rdl:PCA_100006763 "Document compliance with applicable EU directives the equipment is designed to." ;
                  rdl:PCA_100006765 rrdl:CFIHOS-20000027 ;
                  rdl:PCA_100006766 rdl:PCA_100006653 ;
                  rdl:PCA_100006768 "The EU Declaration of conformity shall be written up by the manufacturer of the equipment or component, as the legal binding document from the manufacturer to the purchaser / user ensuring conformity with the relevant EU directive(s). \n\nEU declaration of Conformity shall be delivered according to requirements of the relevant EU - directives with respect to conformity assessment procedures and eventual necessary involvements of Notified Bodies. \n\nCertificate(s) of conformance, required by relevant directive(s), shall be available." ;
                  rdfs:comment "The EU Declaration of conformity shall be written up by the manufacturer of the equipment or component, as the legal binding document from the manufacturer to the purchaser / user ensuring conformity with the relevant EU directive(s). \n\nEU declaration of Conformity shall be delivered according to requirements of the relevant EU - directives with respect to conformity assessment procedures and eventual necessary involvements of Notified Bodies. \n\nCertificate(s) of conformance, required by relevant directive(s), shall be available." ;
                  rdfs:label "EU declaration of conformity" ;
                  skos:broadMatch rdl:PCA_100006724 ;
                  skos:broader rdl:PCA_100006756 .


###  http://rds.posccaesar.org/ontology/plm/rdl/PCA_100006192
rdl:PCA_100006192 rdf:type owl:Class ;
                  rdfs:subClassOf rdl:PCA_100004908 ;
                  rdl:PCA_100006763 "This document is required to allow use of equipment in hazardous areas." ;
                  rdl:PCA_100006764 "Attestation issued by a recognised independent authority certifying that a type test has satisfied the specified standards; e.g.  ATEX, BASEEFA, PTB, UL, CSA, NEMA, EX, etc. Examples of ratings include Intrinsically Safe & Explosion Proof. To include any special requirements for safe use, barrier/isolator to be used, etc." ;
                  rdl:PCA_100006765 rrdl:CFIHOS-20000013 ;
                  rdl:PCA_100006766 rdl:PCA_100006653 ;
                  rdl:PCA_100006768 "The equipment’s explosion protection certificate shall be delivered according to recognized standards.\n\nThis certificate proves that equipment conforms to the specific standard for the type of explosion protection, e.g. ATEX, IEC\nThis document shall provide input to IS-calculations, special requirements for safe use, barrier/isolator to be used, etc." ;
                  rdfs:comment "The equipment’s explosion protection certificate shall be delivered according to recognized standards.\n\nThis certificate proves that equipment conforms to the specific standard for the type of explosion protection, e.g. ATEX, IEC\nThis document shall provide input to IS-calculations, special requirements for safe use, barrier/isolator to be used, etc." ;
                  rdfs:label "EX certificate" ;
                  skos:broadMatch rdl:PCA_100006722 ,
                                  rdl:PCA_100006727 ;
                  skos:broader rdl:PCA_100006743 .


###  http://rds.posccaesar.org/ontology/plm/rdl/PCA_100006193
rdl:PCA_100006193 rdf:type owl:Class ;
                  rdfs:subClassOf rdl:PCA_100004908 ;
                  rdl:PCA_100006765 rrdl:CFIHOS-20000007 ;
                  rdl:PCA_100006766 rdl:PCA_100006656 ;
                  rdl:PCA_100006768 "All system, arrangement, layout, plan, section and detail drawings shall be included." ;
                  rdfs:comment "All system, arrangement, layout, plan, section and detail drawings shall be included." ;
                  rdfs:label "Excavation, fill and grading drawings" ;
                  skos:broadMatch rdl:PCA_100006706 ;
                  skos:broader rdl:PCA_100006746 .


###  http://rds.posccaesar.org/ontology/plm/rdl/PCA_100006194
rdl:PCA_100006194 rdf:type owl:Class ;
                  rdfs:subClassOf rdl:PCA_100004908 ;
                  rdl:PCA_100006763 "This document shall document deviations from standards and/or specifications, and issue of technical queries.\n\nThis document shall support the procurement process. Accepted exemptions must be incorporated in technical documentation for the equipment." ;
                  rdl:PCA_100006766 rdl:PCA_100006653 ;
                  rdl:PCA_100006768 "This document shall contain a list stating all deviations from the requirements in the inquiry, and proposed alternative requirements." ;
                  rdfs:comment "This document shall contain a list stating all deviations from the requirements in the inquiry, and proposed alternative requirements." ;
                  rdfs:label "Exemptions from specifications and other requirements in the inquiry" ;
                  skos:broadMatch rdl:PCA_100006722 ;
                  skos:broader rdl:PCA_100006756 .


###  http://rds.posccaesar.org/ontology/plm/rdl/PCA_100006195
rdl:PCA_100006195 rdf:type owl:Class ;
                  rdfs:subClassOf rdl:PCA_100004908 ;
                  rdl:PCA_100006763 "To document the expected pipeline expansion and to demonstrate sufficient pipeline design." ;
                  rdl:PCA_100006765 rrdl:CFIHOS-20000018 ;
                  rdl:PCA_100006766 rdl:PCA_100006653 ;
                  rdl:PCA_100006768 "Report documenting all calculations and analysis performed to show how pipeline is expected to expand during all conditions." ;
                  rdfs:comment "Report documenting all calculations and analysis performed to show how pipeline is expected to expand during all conditions." ;
                  rdfs:label "Expansion analysis" ;
                  skos:broadMatch rdl:PCA_100006687 ;
                  skos:broader rdl:PCA_100006741 .


###  http://rds.posccaesar.org/ontology/plm/rdl/PCA_100006196
rdl:PCA_100006196 rdf:type owl:Class ;
                  rdfs:subClassOf rdl:PCA_100004908 ;
                  rdl:PCA_100006763 "Ensure safe operation" ;
                  rdl:PCA_100006765 rrdl:CFIHOS-20000018 ;
                  rdl:PCA_100006766 rdl:PCA_100006654 ;
                  rdl:PCA_100006768 "Design report covering pipeline expansion and buckling analysis including pipeline soil interaction. Basis for analysis, assumptions and assessments not given in design basis shall be included." ;
                  rdfs:comment "Design report covering pipeline expansion and buckling analysis including pipeline soil interaction. Basis for analysis, assumptions and assessments not given in design basis shall be included." ;
                  rdfs:label "Expansion design report" ;
                  skos:broadMatch rdl:PCA_100006686 ;
                  skos:broader rdl:PCA_100006756 .


###  http://rds.posccaesar.org/ontology/plm/rdl/PCA_100006197
rdl:PCA_100006197 rdf:type owl:Class ;
                  rdfs:subClassOf rdl:PCA_100004908 ;
                  rdl:PCA_100006763 "Explosion protection certificates (ATEX , EX, NEMA). Applies to electrical devices and devices with electrical connections" ;
                  rdl:PCA_100006765 rrdl:CFIHOS-20000013 ;
                  rdfs:label "Explosion protection certificates" ;
                  skos:broadMatch rdl:PCA_100006722 ;
                  skos:broader rdl:PCA_100006743 .


###  http://rds.posccaesar.org/ontology/plm/rdl/PCA_100006198
rdl:PCA_100006198 rdf:type owl:Class ;
                  rdfs:subClassOf rdl:PCA_100004908 ;
                  rdl:PCA_100006763 "For  verfication purposes." ;
                  rdl:PCA_100006765 rrdl:CFIHOS-20000018 ;
                  rdl:PCA_100006766 rdl:PCA_100006654 ;
                  rdl:PCA_100006768 "The FRB shall contain welding procedures, relevant test certificates, heat treatment documentation and reference to requirements." ;
                  rdfs:comment "The FRB shall contain welding procedures, relevant test certificates, heat treatment documentation and reference to requirements." ;
                  rdfs:label "Fabrication record book (FRB)" ;
                  skos:broadMatch rdl:PCA_100006722 ;
                  skos:broader rdl:PCA_100006756 ,
                               rdl:PCA_100006762 .


###  http://rds.posccaesar.org/ontology/plm/rdl/PCA_100006199
rdl:PCA_100006199 rdf:type owl:Class ;
                  rdfs:subClassOf rdl:PCA_100004908 ;
                  rdl:PCA_100006763 "The FAT procedure will be used to ensure a common understanding of performed testing and acceptance criteria." ;
                  rdl:PCA_100006765 rrdl:CFIHOS-20000027 ;
                  rdl:PCA_100006766 rdl:PCA_100006653 ;
                  rdl:PCA_100006768 "This document shall include all testing activities and their acceptance criteria according to applicable standards, specifications and requirements,. to document the condition of the equipment as tested from factory. Test set-up and test equipment shall be defined. \n\nSuppliers standard (routine) test procedures should be used as far as possible" ;
                  rdfs:comment "This document shall include all testing activities and their acceptance criteria according to applicable standards, specifications and requirements,. to document the condition of the equipment as tested from factory. Test set-up and test equipment shall be defined. \n\nSuppliers standard (routine) test procedures should be used as far as possible" ;
                  rdfs:label "Factory acceptance test (FAT) procedures" ;
                  skos:broadMatch rdl:PCA_100006722 ;
                  skos:broader rdl:PCA_100006751 .


###  http://rds.posccaesar.org/ontology/plm/rdl/PCA_100006200
rdl:PCA_100006200 rdf:type owl:Class ;
                  rdfs:subClassOf rdl:PCA_100004908 ;
                  rdl:PCA_100006763 "The FAT report will be used to verify that the equipment has been tested according to FAT procedure.\nThe FAT report will be used for acceptance of the equipment delivery" ;
                  rdl:PCA_100006765 rrdl:CFIHOS-20000027 ;
                  rdl:PCA_100006766 rdl:PCA_100006653 ;
                  rdl:PCA_100006768 "This document shall record and document all activities performed and results from these, in accordance with the FAT procedure. \nThis document outline all testing activities and their acceptance criteria to document the condition of the equipment as tested from factory." ;
                  rdfs:comment "This document shall record and document all activities performed and results from these, in accordance with the FAT procedure. \nThis document outline all testing activities and their acceptance criteria to document the condition of the equipment as tested from factory." ;
                  rdfs:label "Factory acceptance test (FAT) report" ;
                  skos:broadMatch rdl:PCA_100006722 ;
                  skos:broader rdl:PCA_100006756 .


###  http://rds.posccaesar.org/ontology/plm/rdl/PCA_100006201
rdl:PCA_100006201 rdf:type owl:Class ;
                  rdfs:subClassOf rdl:PCA_100004908 ;
                  rdl:PCA_100006763 "Give clear test instructions and provide information to customers concerning test standards and acceptance criteria." ;
                  rdl:PCA_100006765 rrdl:CFIHOS-20000031 ;
                  rdl:PCA_100006766 rdl:PCA_100006653 ;
                  rdl:PCA_100006768 "A procedure describing the stepwise testing to be performed for the equipment after completed manufacturing. Test set-up and test equipment is defined" ;
                  rdfs:comment "A procedure describing the stepwise testing to be performed for the equipment after completed manufacturing. Test set-up and test equipment is defined" ;
                  rdfs:label "FAT procedure" ;
                  skos:broadMatch rdl:PCA_100006688 ;
                  skos:broader rdl:PCA_100006751 .


###  http://rds.posccaesar.org/ontology/plm/rdl/PCA_100006202
rdl:PCA_100006202 rdf:type owl:Class ;
                  rdfs:subClassOf rdl:PCA_100004908 ;
                  rdl:PCA_100006763 "To document the tests performed in accordance with the procedure." ;
                  rdl:PCA_100006764 "The Factory Acceptance Test (FAT) shall document and verify that acceptance testing has been performed in accordance with defined requirements and that these has been met successfully. In engineering and its various subdisciplines, acceptance testing is a test conducted to determine if the requirements of a specification or contract are met. It may involve chemical tests, physical tests, or performance tests." ;
                  rdl:PCA_100006765 rrdl:CFIHOS-20000031 ;
                  rdl:PCA_100006766 rdl:PCA_100006653 ;
                  rdl:PCA_100006768 "Report containing records from the FAT including pressure tests and flushing operations." ;
                  rdfs:comment "Report containing records from the FAT including pressure tests and flushing operations." ;
                  rdfs:label "FAT report" ;
                  skos:broadMatch rdl:PCA_100006722 ;
                  skos:broader rdl:PCA_100006756 .


###  http://rds.posccaesar.org/ontology/plm/rdl/PCA_100006203
rdl:PCA_100006203 rdf:type owl:Class ;
                  rdfs:subClassOf rdl:PCA_100004908 ;
                  rdl:PCA_100006763 "Design report describing the fatigue analysis and the fatigue service life for the pipeline." ;
                  rdl:PCA_100006765 rrdl:CFIHOS-20000018 ;
                  rdl:PCA_100006766 rdl:PCA_100006654 ;
                  rdl:PCA_100006768 "Basis for analysis, assumptions and assessments not given in design basis shall be included." ;
                  rdfs:comment "Basis for analysis, assumptions and assessments not given in design basis shall be included." ;
                  rdfs:label "Fatigue service life design report" ;
                  skos:broadMatch rdl:PCA_100006686 ;
                  skos:broader rdl:PCA_100006756 .


###  http://rds.posccaesar.org/ontology/plm/rdl/PCA_100006204
rdl:PCA_100006204 rdf:type owl:Class ;
                  rdfs:subClassOf rdl:PCA_100004908 ;
                  rdl:PCA_100006763 "Fibre optical long distance cable transmission budget calculations (attenuation in dB) that have been used for design of fibre optical cable and network equipment shall be provided." ;
                  rdl:PCA_100006764 "Discipline specific (telecom) content is missing" ;
                  rdl:PCA_100006765 rrdl:CFIHOS-20000030 ;
                  rdfs:label "Fiber optical long distance cable transmission budget calculations" ;
                  skos:broadMatch rdl:PCA_100006687 ;
                  skos:broader rdl:PCA_100006741 .


###  http://rds.posccaesar.org/ontology/plm/rdl/PCA_100006205
rdl:PCA_100006205 rdf:type owl:Class ;
                  rdfs:subClassOf rdl:PCA_100004908 ;
                  rdl:PCA_100006764 "Test reports for fibre optical cables (platform/facility internal) shall be provided. Test per fibre." ;
                  rdl:PCA_100006765 rrdl:CFIHOS-20000030 ;
                  rdl:PCA_100006766 rdl:PCA_100006653 ;
                  rdfs:label "Fibre optical cabling (platform / facility internal) test reports" ;
                  skos:broadMatch rdl:PCA_100006722 ;
                  skos:broader rdl:PCA_100006756 .


###  http://rds.posccaesar.org/ontology/plm/rdl/PCA_100006206
rdl:PCA_100006206 rdf:type owl:Class ;
                  rdfs:subClassOf rdl:PCA_100004908 ;
                  rdl:PCA_100006764 "Test reports for Fibre optical long-distance cable(s) shall be provided. Test per fibre." ;
                  rdl:PCA_100006765 rrdl:CFIHOS-20000030 ;
                  rdl:PCA_100006766 rdl:PCA_100006653 ;
                  rdfs:label "Fibre optical long-distance cable test report" ;
                  skos:broadMatch rdl:PCA_100006722 ;
                  skos:broader rdl:PCA_100006756 .


###  http://rds.posccaesar.org/ontology/plm/rdl/PCA_100006207
rdl:PCA_100006207 rdf:type owl:Class ;
                  rdfs:subClassOf rdl:PCA_100004908 ;
                  rdl:PCA_100006763 "An installation drawing shall indicate all details of the actual installation for the relevant instrument tag number (instruments and valves)" ;
                  rdl:PCA_100006764 "Drawing to include:\n - Field instrumentation part of process hook-up;\n - Structure and stands for field instrumentation.\n - A title to describe the process application;\n - All instrument/bulk material installed by Supplier, or to be installed by Purchaser;\n - Connections and dimensions of signal lines/tubing;\n - Material of instrument bulk;\n - A product code and quantity of instrument bulk;\n - Indicate split of responsibility instrument/piping.\nTypical installation drawings should be used as a guideline." ;
                  rdl:PCA_100006765 rrdl:CFIHOS-20000015 ;
                  rdl:PCA_100006766 rdl:PCA_100006653 ;
                  rdfs:label "Field instrument installation drawing typical" ;
                  skos:broadMatch rdl:PCA_100006731 ,
                                  rdl:PCA_100006732 ;
                  skos:broader rdl:PCA_100006746 .


###  http://rds.posccaesar.org/ontology/plm/rdl/PCA_100006208
rdl:PCA_100006208 rdf:type owl:Class ;
                  rdfs:subClassOf rdl:PCA_100004908 ;
                  rdl:PCA_100006763 "To give an overview of where assemblies will be/are installed on the seabed relative to other assemblies." ;
                  rdl:PCA_100006764 "For SURF this info is covered in GIS database" ;
                  rdl:PCA_100006765 rrdl:CFIHOS-20000031 ;
                  rdl:PCA_100006766 rdl:PCA_100006653 ;
                  rdl:PCA_100006768 "Geographic map outlining subsea assemblies on the seabed for a particular field with description." ;
                  rdfs:comment "Geographic map outlining subsea assemblies on the seabed for a particular field with description." ;
                  rdfs:label "Field layout drawing" ;
                  skos:broadMatch rdl:PCA_100006705 ;
                  skos:broader rdl:PCA_100006746 .


###  http://rds.posccaesar.org/ontology/plm/rdl/PCA_100006209
rdl:PCA_100006209 rdf:type owl:Class ;
                  rdfs:subClassOf rdl:PCA_100004908 ;
                  rdl:PCA_100006765 rrdl:CFIHOS-20000018 ;
                  rdl:PCA_100006766 rdl:PCA_100006654 ;
                  rdl:PCA_100006768 "Lay-out drawing comprising of all elements in the field such as templates, platforms, anchor patterns, pipelines, umbilicals, cables, pipeline structures etc." ;
                  rdfs:comment "Lay-out drawing comprising of all elements in the field such as templates, platforms, anchor patterns, pipelines, umbilicals, cables, pipeline structures etc." ;
                  rdfs:label "Field lay-out drawing" ;
                  skos:broadMatch rdl:PCA_100006705 ;
                  skos:broader rdl:PCA_100006746 .


###  http://rds.posccaesar.org/ontology/plm/rdl/PCA_100006210
rdl:PCA_100006210 rdf:type owl:Class ;
                  rdfs:subClassOf rdl:PCA_100004908 ;
                  rdl:PCA_100006765 rrdl:CFIHOS-20000031 ;
                  rdl:PCA_100006766 rdl:PCA_100006653 ;
                  rdl:PCA_100006768 "Final inspection reports:\n\nA final inspection program shall be performed for the subsea system prior to delivery to Company. The inspection program shall:\n - Identify status of all equipment upon delivery;\n - Valve status (shut/open);\n - Connection point status (permanent/temporary clamps);\n - Status hatches;\n - Pressure equalization system connection points;\n - Verification of tubular ventilation ports. \n\nTest reports:\n - All operations to be tested during assembly shall be identified with a test procedure;\n - The individual testing program operations shall be signed out by Contractor. Company shall sign the overall test program upon completion." ;
                  rdfs:comment "Final inspection reports:\n\nA final inspection program shall be performed for the subsea system prior to delivery to Company. The inspection program shall:\n - Identify status of all equipment upon delivery;\n - Valve status (shut/open);\n - Connection point status (permanent/temporary clamps);\n - Status hatches;\n - Pressure equalization system connection points;\n - Verification of tubular ventilation ports. \n\nTest reports:\n - All operations to be tested during assembly shall be identified with a test procedure;\n - The individual testing program operations shall be signed out by Contractor. Company shall sign the overall test program upon completion." ;
                  rdfs:label "Final inspection and test reports" ;
                  skos:broadMatch rdl:PCA_100006722 ;
                  skos:broader rdl:PCA_100006756 .


###  http://rds.posccaesar.org/ontology/plm/rdl/PCA_100006211
rdl:PCA_100006211 rdf:type owl:Class ;
                  rdfs:subClassOf rdl:PCA_100004908 ;
                  rdl:PCA_100006763 "Fire protection data sheets shall document the fire and explosion protection and detection design. Fire protection data sheets shall be maintained throughout the plant or installation lifetime and be consistent with information in other engineering/operational databases." ;
                  rdl:PCA_100006765 rrdl:CFIHOS-20000015 ;
                  rdl:PCA_100006766 rdl:PCA_100006626 ,
                                    rdl:PCA_100006627 ,
                                    rdl:PCA_100006628 ,
                                    rdl:PCA_100006633 ;
                  rdl:PCA_100006768 "A fire protection datasheet shall be produced for each of the defined fire detection areas. \n\nThe fire protection data sheets shall include the following main information elements:\n - Key characteristics of area barriers:\n   - Area classification references (zone 1, zone 2, non-hazardous by location, non-hazardous by ventilation);\n   - Ventilation of the area (natural, mechanical, overpressure, underpressure);\n   - Occupancy (permanent, intermittent, normally none, none);\n   - Construction of walls/floors/ceiling (none, wind shield, heat shield, steel walls, fire partitions with fire rating, explosion panels, suspended ceiling, false floor);\n   - Hazards in the area (e.g. crude oil, toxic gas, chemicals, fuel oil, electrical, radioactive, etc.);\n   - Type of fire and gas detection in the area;\n   - Type of fire protection with application design rates;\n - Basis for fire and gas detection design and fire protection:\n   - A listing of main equipment of the area which governs the fire and gas detection selection and location;\n   - A description of the basis for the selection of particular type and position of detectors including manual call points. This is an area specific detailing of the general fire and gas logic;\n   - A reference of area fire extinguishing facilities;\n - Fire and Gas Cause & Effect:\n   - This part shall be according to Cause & Effect requirements addressing the specific fire and gas detection logic including means for fire extinguishing control and monitoring and other specific output actions;\n   - The C&E sheet shall include a listing of all area tag numbers, i.e., fire and gas detectors and output devices." ;
                  rdfs:comment "A fire protection datasheet shall be produced for each of the defined fire detection areas. \n\nThe fire protection data sheets shall include the following main information elements:\n - Key characteristics of area barriers:\n   - Area classification references (zone 1, zone 2, non-hazardous by location, non-hazardous by ventilation);\n   - Ventilation of the area (natural, mechanical, overpressure, underpressure);\n   - Occupancy (permanent, intermittent, normally none, none);\n   - Construction of walls/floors/ceiling (none, wind shield, heat shield, steel walls, fire partitions with fire rating, explosion panels, suspended ceiling, false floor);\n   - Hazards in the area (e.g. crude oil, toxic gas, chemicals, fuel oil, electrical, radioactive, etc.);\n   - Type of fire and gas detection in the area;\n   - Type of fire protection with application design rates;\n - Basis for fire and gas detection design and fire protection:\n   - A listing of main equipment of the area which governs the fire and gas detection selection and location;\n   - A description of the basis for the selection of particular type and position of detectors including manual call points. This is an area specific detailing of the general fire and gas logic;\n   - A reference of area fire extinguishing facilities;\n - Fire and Gas Cause & Effect:\n   - This part shall be according to Cause & Effect requirements addressing the specific fire and gas detection logic including means for fire extinguishing control and monitoring and other specific output actions;\n   - The C&E sheet shall include a listing of all area tag numbers, i.e., fire and gas detectors and output devices." ;
                  rdfs:label "Fire protection data sheet (FPDS)" ;
                  skos:broadMatch rdl:PCA_100006727 ;
                  skos:broader rdl:PCA_100006747 .


###  http://rds.posccaesar.org/ontology/plm/rdl/PCA_100006212
rdl:PCA_100006212 rdf:type owl:Class ;
                  rdfs:subClassOf rdl:PCA_100004908 ;
                  rdl:PCA_100006763 "For compliance" ;
                  rdl:PCA_100006765 rrdl:CFIHOS-20000013 ;
                  rdl:PCA_100006766 rdl:PCA_100006653 ;
                  rdl:PCA_100006768 "Document fire test" ;
                  rdfs:comment "Document fire test" ;
                  rdfs:label "Fire test certificate" ;
                  skos:broadMatch rdl:PCA_100006722 ;
                  skos:broader rdl:PCA_100006743 .


###  http://rds.posccaesar.org/ontology/plm/rdl/PCA_100006213
rdl:PCA_100006213 rdf:type owl:Class ;
                  rdfs:subClassOf rdl:PCA_100004908 ;
                  rdl:PCA_100006763 "The basis for decision regarding selection of combustible materials shall be documented." ;
                  rdl:PCA_100006765 rrdl:CFIHOS-20000003 ;
                  rdl:PCA_100006766 rdl:PCA_100006630 ;
                  rdl:PCA_100006768 "Materials used in areas that may be exposed to a hydrocarbon fire shall be non-combustible. If it is justified from safety point of view to make use of materials that do not meet the requirements to non-combustibility, such materials shall have limited flame-spread properties, low smoke development and heat generation.\n\nAn assessment shall be made of the toxicity of gas emitted in the event of a fire." ;
                  rdfs:comment "Materials used in areas that may be exposed to a hydrocarbon fire shall be non-combustible. If it is justified from safety point of view to make use of materials that do not meet the requirements to non-combustibility, such materials shall have limited flame-spread properties, low smoke development and heat generation.\n\nAn assessment shall be made of the toxicity of gas emitted in the event of a fire." ;
                  rdfs:label "Fire test results reports" ;
                  skos:broadMatch rdl:PCA_100006722 ;
                  skos:broader rdl:PCA_100006756 .


###  http://rds.posccaesar.org/ontology/plm/rdl/PCA_100006214
rdl:PCA_100006214 rdf:type owl:Class ;
                  rdfs:subClassOf rdl:PCA_100004908 ;
                  rdl:PCA_100006764 "A document containing all calibration certificates for the fiscal metering system shall be provided." ;
                  rdl:PCA_100006765 rrdl:CFIHOS-20000015 ;
                  rdfs:label "Fiscal metering - Calibration certificates" ;
                  skos:broadMatch rdl:PCA_100006722 ;
                  skos:broader rdl:PCA_100006743 .


###  http://rds.posccaesar.org/ontology/plm/rdl/PCA_100006215
rdl:PCA_100006215 rdf:type owl:Class ;
                  rdfs:subClassOf rdl:PCA_100004908 ;
                  rdl:PCA_100006763 "All physical dimensions and parameters which will affect the measurement result shall have documented traceability to international standards." ;
                  rdl:PCA_100006764 "Document providing such traceability shall be provided." ;
                  rdl:PCA_100006765 rrdl:CFIHOS-20000015 ;
                  rdl:PCA_100006766 rdl:PCA_100006587 ,
                                    rdl:PCA_100006591 ;
                  rdfs:label "Fiscal metering - Configuration parameters" ;
                  skos:broadMatch rdl:PCA_100006687 ;
                  skos:broader rdl:PCA_100006741 ,
                               rdl:PCA_100006756 .


###  http://rds.posccaesar.org/ontology/plm/rdl/PCA_100006216
rdl:PCA_100006216 rdf:type owl:Class ;
                  rdfs:subClassOf rdl:PCA_100004908 ;
                  rdl:PCA_100006763 "A separate data exchange document shall be issued for each interface." ;
                  rdl:PCA_100006764 "Data content and interface shall be agreed between relevant parties." ;
                  rdl:PCA_100006765 rrdl:CFIHOS-20000015 ;
                  rdl:PCA_100006766 rdl:PCA_100006587 ,
                                    rdl:PCA_100006591 ;
                  rdfs:label "Fiscal metering - Data exchange specifications" ;
                  skos:broadMatch rdl:PCA_100006703 ;
                  skos:broader rdl:PCA_100006757 .


###  http://rds.posccaesar.org/ontology/plm/rdl/PCA_100006217
rdl:PCA_100006217 rdf:type owl:Class ;
                  rdfs:subClassOf rdl:PCA_100004908 ;
                  rdl:PCA_100006763 "All calculations needed for sizing and selection of metering equipment shall be documented." ;
                  rdl:PCA_100006764 "Such as, but not limited to:\n - Flow meters;\n - Prover sizing;\n - Mixing in accordance with ISO 3171;\n - Fast loops (pressure drop, flow rates required for isokinetic sampling;\n - Time lag for analyser system;\n - Dew point calculation for the sampling handling system;\n - Installation effects which may affect flowmeter performance such as:\n     - noise;\n     - low profile.\n - Pressure drop." ;
                  rdl:PCA_100006765 rrdl:CFIHOS-20000015 ;
                  rdl:PCA_100006766 rdl:PCA_100006587 ,
                                    rdl:PCA_100006591 ;
                  rdfs:label "Fiscal metering - Design calculations" ;
                  skos:broadMatch rdl:PCA_100006687 ;
                  skos:broader rdl:PCA_100006741 .


###  http://rds.posccaesar.org/ontology/plm/rdl/PCA_100006218
rdl:PCA_100006218 rdf:type owl:Class ;
                  rdfs:subClassOf rdl:PCA_100004908 ;
                  rdl:PCA_100006763 "The document shall provide the information needed for an independent verification of the calculations in the computer. All international standards used shall be referred to with version number, year and relevant section." ;
                  rdl:PCA_100006764 "A document unambiguously showing all calculations affecting the measurement result shall be provided." ;
                  rdl:PCA_100006765 rrdl:CFIHOS-20000015 ;
                  rdl:PCA_100006766 rdl:PCA_100006587 ,
                                    rdl:PCA_100006591 ;
                  rdfs:label "Fiscal metering - Fiscal metering calculations" ;
                  skos:broadMatch rdl:PCA_100006687 ;
                  skos:broader rdl:PCA_100006741 .


###  http://rds.posccaesar.org/ontology/plm/rdl/PCA_100006219
rdl:PCA_100006219 rdf:type owl:Class ;
                  rdfs:subClassOf rdl:PCA_100004908 ;
                  rdl:PCA_100006763 "The evaluation leading to the selection of flow meter principle and make shall be documented. Ref TR0814 section 4.1 Selection of flow meters." ;
                  rdl:PCA_100006765 rrdl:CFIHOS-20000015 ;
                  rdfs:label "Fiscal metering - Flow meter selection report" ;
                  skos:broadMatch rdl:PCA_100006691 ,
                                  rdl:PCA_100006698 ;
                  skos:broader rdl:PCA_100006756 .


###  http://rds.posccaesar.org/ontology/plm/rdl/PCA_100006220
rdl:PCA_100006220 rdf:type owl:Class ;
                  rdfs:subClassOf rdl:PCA_100004908 ;
                  rdl:PCA_100006764 "A document containing uncertainty analysis for the metering system shall be provided.  For Gas ultrasonic meters the influence of different pressure and temperature between calibration conditions and operational conditions shall be documented." ;
                  rdl:PCA_100006765 rrdl:CFIHOS-20000015 ;
                  rdl:PCA_100006766 rdl:PCA_100006587 ,
                                    rdl:PCA_100006591 ;
                  rdfs:label "Fiscal metering - Uncertainty analysis" ;
                  skos:broadMatch rdl:PCA_100006687 ;
                  skos:broader rdl:PCA_100006741 ,
                               rdl:PCA_100006756 .


###  http://rds.posccaesar.org/ontology/plm/rdl/PCA_100006221
rdl:PCA_100006221 rdf:type owl:Class ;
                  rdfs:subClassOf rdl:PCA_100004908 ;
                  rdl:PCA_100006763 "Provided for in API STD 521 chapter 4" ;
                  rdl:PCA_100006764 "The flare report shall be one common report for the plant (i.e. not split into several reports). Documentation of emergency depressurization may be issued as a separate report cross-referenced to the flare report.\n\nThe report should be named \"Flare report\". If the depressurization design is included, name the report \"Flare and Depressurization Report\"\n\nThe flare report shall describe the design of the flare and vent system, and as a minimum include:\n - Design basis for the system, e.g. system capacity and selection;\n-    Procedure for replacement of flare tip;\n - Description of the flare and vent system segregation and disposal, e.g. wet vs. dry streams, high vs. low temperature, high vs. low pressure, emergency vs. maintenance flare/vent, flaring vs. cold venting and common vent vs. local vent;\n     - For cold vents, selected/recommended methods to extinguish the flame (if the vent is ignited) shall be described;\n - Descriptions of flaring scenarios including flare rates, e.g. operational flaring, relief cases, emergency depressurization and simultaneous flaring (operational flaring + relief/depressurization). The simultaneous flaring cases shall be clearly defined. The selected base load (e.g. long-term operational flaring) shall be explained;\n     - The flare report shall list the largest flare sources, those that designs the flare headers/drums and the location of the flare tip;\n - Operation of the system during long duration cooldown, e.g. cold ambient temperature, flowline depressurization;\n - Description of the piping and equipment design, e.g.:\n     - Hydraulic design (sizing of pipes);\n     - Knock out drum;\n     - Flare tip design (e.g. hydraulic performance, soot emission, noise, purge requirements, expected lifetime, maintenance requirements);\n     - Flare gas recovery;\n     - Flare ignition;\n           - If flare gases are combusted for safety reasons (i.e. not only for environmental reasons), the reliability of the ignition system shall be documented to prove that the system has the required reliability and necessary requirements (assumptions) listed;\n - Documentation of system design calculations, where the input data, results and the calculations shall be included in the report and in simulation files, e.g.:\n     - Calculation of flare tip radiation to determine (a) the resulting heat exposure towards humans and (b) the resulting temperature on equipment, pipes and structures;\n     - Calculation of gas dispersion;\n     - The potential gas concentration resulting from an extinguished flare/vent shall be documented, and plant areas where operational activities are limited as a result (e.g. hot work) shall be defined;\n     - Hydraulic calculation (pipe sizing);\n     - Sizing of liquid knockout drums;\n     - The main results are documented in the main report, the details in appendices.\n\nThe various simulation files defined above shall be a part of the delivery as executable simulation files (simulation programs to be agreed) reflecting the As-built design.\n\nThe flare report, including the simulation files, shall be updated whenever relevant modifications to the plant are performed, i.e. parallel documents shall not be established.\n\n\nDocumentation of the depressurization design\n\nThe depressurization report shall specify the information required to repeat/re-establish all dimensioning cases both with respect to fire depressurization and cold depressurization. Typical required information is input streams, system geometry (see list above), initial conditions (e.g. pressure, temperature, liquid volumes, ambient conditions), orifice specification, any delayed opening of BDVs, material properties used, fire loads and durations, the plant specific intolerable ruptures, assumptions made and other relevant information.\n\nThe report shall tabulate the following:\n - Rupture conditions of pipes/equipment that will rupture during the dimensioning fire;\n     - Time to rupture;\n     - Pressure at rupture;\n     - Instantaneous release of hydrocarbon fluid at rupture (kg/s);\n     - Other relevant information;\n - The initial flare rate from fire depressurisation and cold depressurization;\n - System pressure 15 minutes after gas detection (no heat input, relevant delay of blowdown included);\n - The minimum vapour and liquid temperature resulting from the cold depressurization;\n - The minimum vapour wall and liquid wall temperatures resulting from the cold depressurization.\nThe report should contain the following:\n - The depressurisation rates for each depressurisation segment as function of time:\n     - cold depressurisation, fire depressurisation and depressurisation from normal conditions;\n - The total depressurisation rate (mass rate) for all segments that are feeding the disposal system simultaneously:\n     - fire depressurisation and depressurisation from normal conditions.\n\nThe following shall be available for Company during project execution and shall be handed over to Company at project close out.\n\n - A spreadsheet that describes the geometry of all depressurisation segments. See the below list for minimum content.\n - A spreadsheet tabulating the pressure profiles during fire exposure/fire depressurisation for all depressurization segments and for all segments containing hydrocarbons but without depressurization.\n - A spreadsheet tabulating the pressure profile for the flare header during depressurisation\n\nThe simulation file(s) used for calculation of temperature profile and stress/rupture (i.e. time to rupture calculations).\n\nA spreadsheet that describes the geometry of all depressurization segments shall be made. The spreadsheet shall always reflect the current process design, include date of last revision and corresponding P&ID revision(s) used, and shall as a minimum contain the following information for each pipe and equipment (it is recommended to use one sheet for each depressurization segment):\n - Line number or equipment tag number;\n - Length (note 3);\n - Inner and outer diameter;\n - Liquid volume (see note 1);\n - Gas volume (see note 1);\n - Total volume of the depressurisation segment and volume of each sub-segment (note 2);\n - Outside are:\n     - total outside area of the depressurisation segment and outside area of each sub-segment;\n - Dry area:\n     - total dry area of the depressurisation segment and dry area of each sub-segment. See note 1;\n - Wet area:\n     - total wet area of the depressurisation segment and wet area of each sub-segment. See note 1;\n - Insulated area and type of insulation;\n - Wall thickness;\n - Material;\n - Weight:\n     - total weight of depressurisation segment and weight of each sub segment.\n\nNote 1: Liquid in sloped pipes will be drain to its nearest low point. Pipes that will be drained are treated as “dry wall” pipes.\n\nNote 2: A sub-segment is e.g. a pipe or a vessel in a depressurization segment\n\nNote 3: Line sizes that do not contribute to the system volume/area/weight, typically sizes less than 1’’, need not to be listed with length and can be listed separately on the same sheet.\n\nThe spreadsheet should in addition contain the following information:\n - Name of depressurisation segment (e.g. 1ststage separator);\n - Tag-number of the BDV (and the orifice);\n - Which valves that determines the border of the depressurisation segment (PSD valves, ESD valves, PSVs, PV etc);\n - Information about what, when and by whom the spreadsheet was updated, i.e. a change log." ;
                  rdl:PCA_100006765 rrdl:CFIHOS-20000026 ;
                  rdl:PCA_100006766 rdl:PCA_100006654 ;
                  rdfs:label "Flare report/flare and depressurization report" ;
                  skos:broadMatch rdl:PCA_100006698 ;
                  skos:broader rdl:PCA_100006756 .


###  http://rds.posccaesar.org/ontology/plm/rdl/PCA_100006222
rdl:PCA_100006222 rdf:type owl:Class ;
                  rdfs:subClassOf rdl:PCA_100004908 ;
                  rdl:PCA_100006763 "Document the flow assurance analysis and calculations." ;
                  rdl:PCA_100006765 rrdl:CFIHOS-20000031 ;
                  rdl:PCA_100006766 rdl:PCA_100006657 ;
                  rdl:PCA_100006768 "A report providing the results from erosion analysis, pressure loss calculations, hydrate evaluations and analysis, flow induced vibration calculations and thermal analysis." ;
                  rdfs:comment "A report providing the results from erosion analysis, pressure loss calculations, hydrate evaluations and analysis, flow induced vibration calculations and thermal analysis." ;
                  rdfs:label "Flow assurance report" ;
                  skos:broadMatch rdl:PCA_100006696 ;
                  skos:broader rdl:PCA_100006756 .


###  http://rds.posccaesar.org/ontology/plm/rdl/PCA_100006223
rdl:PCA_100006223 rdf:type owl:Class ;
                  rdfs:subClassOf rdl:PCA_100004908 ;
                  rdl:PCA_100006763 "Schematic showing the flow path, line size, equipment and connections for process and utility systems. The schematic shall use standard symbols." ;
                  rdl:PCA_100006765 rrdl:CFIHOS-20000031 ;
                  rdl:PCA_100006766 rdl:PCA_100006657 ;
                  rdl:PCA_100006768 "Provide a simplified overview of connections, lines with sizes and equipment for a sub-system. Basis for piping design." ;
                  rdfs:comment "Provide a simplified overview of connections, lines with sizes and equipment for a sub-system. Basis for piping design." ;
                  rdfs:label "Flow schematic" ;
                  skos:broadMatch rdl:PCA_100006696 ;
                  skos:broader rdl:PCA_100006745 .


###  http://rds.posccaesar.org/ontology/plm/rdl/PCA_100006224
rdl:PCA_100006224 rdf:type owl:Class ;
                  rdfs:subClassOf rdl:PCA_100004908 ;
                  rdl:PCA_100006763 "Provide a simplified overview of connections, lines with sizes and equipment for a sub-system. Basis for piping design." ;
                  rdl:PCA_100006765 rrdl:CFIHOS-20000018 ;
                  rdl:PCA_100006766 rdl:PCA_100006657 ;
                  rdl:PCA_100006768 "Schematic showing the flow path, line size, equipment and connections for process and utility systems. The schematic shall use standard symbols." ;
                  rdfs:comment "Schematic showing the flow path, line size, equipment and connections for process and utility systems. The schematic shall use standard symbols." ;
                  rdfs:label "Flowline routing" ;
                  skos:broadMatch rdl:PCA_100006705 ;
                  skos:broader rdl:PCA_100006746 .


###  http://rds.posccaesar.org/ontology/plm/rdl/PCA_100006225
rdl:PCA_100006225 rdf:type owl:Class ;
                  rdfs:subClassOf rdl:PCA_100004908 ;
                  rdl:PCA_100006763 "Input to simulation models in project and operation phase." ;
                  rdl:PCA_100006764 "This report shall be prepared for the petroleum feed streams and shall include:\n - References to the experimental PVT (Pressure Volume Temperature) and fluid properties data;\n - Feed streams fluid compositions, including the properties of the C6+ hypothetical components;\n - A reasoning for the C6+ characterization, e.g. the selected equation of state and property models, the number of hypothetical components and the tuning of component properties;\n - Comparisons between experimental data and calculations in the characterization program and the process simulation program and a discussion of the differences;\n - Uncertainties in the fluid compositions and properties to be accommodated by the process design, including a reasoning of the selected uncertainties;\n - References to and relations to C6+ characterization(s) used by other disciplines, to demonstrate a consistent description throughout the value chain;\n - A description of the method used to predict the development of the feed stream compositions over the production lifetime, and the feed stream compositions to be accommodated by the process design.\n\nSimulation files from the characterization and process simulation programs shall be a part of the delivery, to allow execution in the simulation programs." ;
                  rdl:PCA_100006765 rrdl:CFIHOS-20000026 ;
                  rdl:PCA_100006766 rdl:PCA_100006654 ;
                  rdfs:label "Fluid description for process design" ;
                  skos:broadMatch rdl:PCA_100006696 ,
                                  rdl:PCA_100006698 ;
                  skos:broader rdl:PCA_100006756 .


###  http://rds.posccaesar.org/ontology/plm/rdl/PCA_100006226
rdl:PCA_100006226 rdf:type owl:Class ;
                  rdfs:subClassOf rdl:PCA_100004908 ;
                  rdl:PCA_100006763 "Identify possible failure modes and criticality for components and equipment assemblies as input to design and qualification program as well as OMM; inspection, maintenance and test plan, and spares program." ;
                  rdl:PCA_100006765 rrdl:CFIHOS-20000031 ;
                  rdl:PCA_100006766 rdl:PCA_100006653 ;
                  rdl:PCA_100006768 "The failure mode and effects analysis (FMEA) is a qualitative reliability technique for systematically analysing each possible failure mode for a component, equipment sub-assembly or assembly, and identifying the resulting effect. The criticality analysis (CA) is a quantitative procedure which ranks failure modes according to their probability and consequences (i.e. the resulting effect of the failure mode)." ;
                  rdfs:comment "The failure mode and effects analysis (FMEA) is a qualitative reliability technique for systematically analysing each possible failure mode for a component, equipment sub-assembly or assembly, and identifying the resulting effect. The criticality analysis (CA) is a quantitative procedure which ranks failure modes according to their probability and consequences (i.e. the resulting effect of the failure mode)." ;
                  rdfs:label "FMECA report" ;
                  skos:broadMatch rdl:PCA_100006727 ;
                  skos:broader rdl:PCA_100006756 .


###  http://rds.posccaesar.org/ontology/plm/rdl/PCA_100006227
rdl:PCA_100006227 rdf:type owl:Class ;
                  rdfs:subClassOf rdl:PCA_100004908 ;
                  rdl:PCA_100006765 rrdl:CFIHOS-20000018 ;
                  rdl:PCA_100006766 rdl:PCA_100006654 ;
                  rdl:PCA_100006768 "Drawing showing the footprint of the flexible risers on the seabed in normal and accidental situations." ;
                  rdfs:comment "Drawing showing the footprint of the flexible risers on the seabed in normal and accidental situations." ;
                  rdfs:label "Footprint drawing flexible risers" ;
                  skos:broadMatch rdl:PCA_100006731 ;
                  skos:broader rdl:PCA_100006746 .


###  http://rds.posccaesar.org/ontology/plm/rdl/PCA_100006228
rdl:PCA_100006228 rdf:type owl:Class ;
                  rdfs:subClassOf rdl:PCA_100004908 ;
                  rdl:PCA_100006763 "To give input to the design of structures installed on seabed." ;
                  rdl:PCA_100006765 rrdl:CFIHOS-20000031 ;
                  rdl:PCA_100006766 rdl:PCA_100006653 ;
                  rdl:PCA_100006768 "Report providing the results from geotechnical calculations and analysis for structures installed on seabed." ;
                  rdfs:comment "Report providing the results from geotechnical calculations and analysis for structures installed on seabed." ;
                  rdfs:label "Foundation design report" ;
                  skos:broadMatch rdl:PCA_100006686 ;
                  skos:broader rdl:PCA_100006756 .


###  http://rds.posccaesar.org/ontology/plm/rdl/PCA_100006229
rdl:PCA_100006229 rdf:type owl:Class ;
                  rdfs:subClassOf rdl:PCA_100004908 ;
                  rdl:PCA_100006763 "To document compliance with the PSA facilities regulations § 62 and NMA Regulations No. 878 in addition to IMO instruments and Class requirements, as applicable." ;
                  rdl:PCA_100006765 rrdl:CFIHOS-20000033 ;
                  rdl:PCA_100006766 rdl:PCA_100006657 ;
                  rdl:PCA_100006768 "The plan shall include the following information:\n - deepest draught for the vessel;\n - arrangement plan to show openings and closing appliances with the purpose of retaining the vessel's external watertight integrity, e.g.:\n   - external doors;\n   - cargo hatches service hatches;\n   - side scuttles and windows;\n   - sanitary discharges and garbage chutes;\n   - freeing ports and scuppers;\n   - sea water inlet and discharge valves;\n   - air pipes including vent heads;\n   - ventilators including closing appliances;\n - arrangement plan showing equipment for protection of the crew, e.g.:\n   - gangways, passageways, under deck passages and lifelines;\n   - guard rails and bulwarks." ;
                  rdfs:comment "The plan shall include the following information:\n - deepest draught for the vessel;\n - arrangement plan to show openings and closing appliances with the purpose of retaining the vessel's external watertight integrity, e.g.:\n   - external doors;\n   - cargo hatches service hatches;\n   - side scuttles and windows;\n   - sanitary discharges and garbage chutes;\n   - freeing ports and scuppers;\n   - sea water inlet and discharge valves;\n   - air pipes including vent heads;\n   - ventilators including closing appliances;\n - arrangement plan showing equipment for protection of the crew, e.g.:\n   - gangways, passageways, under deck passages and lifelines;\n   - guard rails and bulwarks." ;
                  rdfs:label "Freeboard plan" ;
                  skos:broadMatch rdl:PCA_100006707 ;
                  skos:broader rdl:PCA_100006753 .


###  http://rds.posccaesar.org/ontology/plm/rdl/PCA_100006230
rdl:PCA_100006230 rdf:type owl:Class ;
                  rdfs:subClassOf rdl:PCA_100004908 ;
                  rdl:PCA_100006763 "To verify the integrity of the pipelines and to enable required seabed intervention to support pipeline installation" ;
                  rdl:PCA_100006765 rrdl:CFIHOS-20000018 ;
                  rdl:PCA_100006766 rdl:PCA_100006653 ;
                  rdl:PCA_100006768 "Report documenting allowable freespans along pipeline route, primarily from fatigue (VIV) point of view." ;
                  rdfs:comment "Report documenting allowable freespans along pipeline route, primarily from fatigue (VIV) point of view." ;
                  rdfs:label "Freespan analysis report" ;
                  skos:broadMatch rdl:PCA_100006687 ;
                  skos:broader rdl:PCA_100006756 .


###  http://rds.posccaesar.org/ontology/plm/rdl/PCA_100006231
rdl:PCA_100006231 rdf:type owl:Class ;
                  rdfs:subClassOf rdl:PCA_100004908 ;
                  rdl:PCA_100006763 "The FDS shall give engineering a description of how the  functional requirement for the product is implemented. It will describe the function and not the design and contain sufficient information for the use." ;
                  rdl:PCA_100006766 rdl:PCA_100006653 ;
                  rdl:PCA_100006768 "The purpose of this document is, for the Supplier, to define all his requirements for safe and reliable control and monitoring function of his equipment. This document shall be used by the project to develop the control, interlocking, monitoring and sequences to be implemented in the switchgear, Electrical Network and Interface with the SAS." ;
                  rdfs:comment "The purpose of this document is, for the Supplier, to define all his requirements for safe and reliable control and monitoring function of his equipment. This document shall be used by the project to develop the control, interlocking, monitoring and sequences to be implemented in the switchgear, Electrical Network and Interface with the SAS." ;
                  rdfs:label "Function description" ;
                  skos:broadMatch rdl:PCA_100006698 ;
                  skos:broader rdl:PCA_100006757 .


###  http://rds.posccaesar.org/ontology/plm/rdl/PCA_100006232
rdl:PCA_100006232 rdf:type owl:Class ;
                  rdfs:subClassOf rdl:PCA_100004908 ;
                  rdl:PCA_100006763 "The document provides input for detailed design and describes equipment design and functional requirements." ;
                  rdl:PCA_100006765 rrdl:CFIHOS-20000031 ;
                  rdl:PCA_100006766 rdl:PCA_100006657 ;
                  rdl:PCA_100006768 "A document summarizing relevant design data and performance requirements for the sub-system and also containing specific design data and performance requirements for the equipment." ;
                  rdfs:comment "A document summarizing relevant design data and performance requirements for the sub-system and also containing specific design data and performance requirements for the equipment." ;
                  rdfs:label "Functional design specification" ;
                  skos:broadMatch rdl:PCA_100006687 ;
                  skos:broader rdl:PCA_100006757 .


###  http://rds.posccaesar.org/ontology/plm/rdl/PCA_100006233
rdl:PCA_100006233 rdf:type owl:Class ;
                  rdfs:subClassOf rdl:PCA_100004908 ;
                  rdl:PCA_100006763 "The manufacturer's standard general arrangement drawing shall be delivered. The content of the GA drawing must be adapted to the item described." ;
                  rdl:PCA_100006768 "Below are examples of expected level of detail. One or more examples may apply.\nFor Mechanical equipment:\n - Dimensions\n - Location and identification of piping and main components\n - Necessary space for disassembly and maintenance\n - Location of centre of gravity\n - Thermal expansion effect, when relevant\n - On the structural steel drawings, critical welds shall be included with a weld \nidentification number serving as a cross-reference to the weld summary index\n - Obstacles from other disciplines shall be included when relevant\n - Total weight, wet and dry and in operational condition\n - Weights, centre of gravity and main dimensions of disassembled units/components \nover 25 kg. Lifting lugs and runway beam for disassembling and their location shall \nbe shown\n - Identification and location of all nozzle and external pipe connections as well as \nrequirements for flexible connections and acceptable loads and moments. Locations \nshall be dimensioned and tolerances shown, if necessary in separate drawings\n - Identification and location of all external electrical and control monitoring connections \n(may be given in separate drawings describing the electrical arrangement and \ninstrumentation)\n - For pressure equipment: for projects at locations where EU regulations for pressure \nequipment apply, Category and Module shall be according to 2014/68/EU (PED)\n - Include bolt tension requirements for pressure equipment flanges\n - Iidentification of lubrication points\n - Foundation information shall include:\n     - The outer dimensions and footprint of the support frame or foundation supports\n     - The size, grade and location of the foundation bolts and torque where this is \nnecessary\n     - Forces and moments transferred to load bearing structures, both under normal \noperation and extreme conditions\n     - Details for adjustment and alignment\n     - Details for cut-outs inside outer limit of foundation\n     - Details for vibration dampening units (if installed)\n\nFor Electrical equipment:\n - Panel equipment layout - position of modules, cards, vacant slots and other \ninformation necessary for expansion or installation of new equipment in the same \ncabinet\n - Internal layout showing arrangement of auxiliary modules, cable trunks, etc.\n - All equipment including junction boxes, push buttons, light fittings, socket outlets, etc.\n - Dimensions\n - Necessary space for disassembly and maintenance\n - Location of centre of gravity\n - Possible thermal expansion\n - Obstacles from other disciplines shall be included when relevant\n\nFor Instrument equipment:\n - Dimensions\n - Location and identification of piping and main components\n - Necessary space for disassembly and maintenance\n - Location of centre of gravity\n - Possible thermal expansion\n - Obstacles from other disciplines shall be included when relevant\n - Panel equipment layout - position of modules, cards, vacant slots and other \ninformation necessary for expansion or installation of new equipment in the same \ncabinet\n - Internal/back layout showing arrangement of auxiliary modules, cable trunks, etc.\n - All equipment including technical network cabinets, junction boxes, push buttons, \nlight fittings, socket outlets, etc.\n - Reference to part list/SPIR\n\nFor Telecom equipment:\nA detailed drawing of the equipment shall be delivered. The drawing shall be to scale with \ndimensions included.\nFor Panel/cabinet/rack the following shall be included in addition:\n - Position of modules, cards, vacant slots and other information necessary for \nexpansion or installation of new equipment in the same cabinet/rack\n - Internal/back layout showing arrangement of auxiliary modules, cable trunks, etc.\n\nFor HVAC equipment:\n - Dimensions\n - Location and identification of piping, ducting, MCTs (Multi core transit) and main \ncomponents\n - Necessary space for disassembly and maintenance\n - Location of centre of gravity\n - Possible thermal expansion\n - Obstacles from other disciplines shall be included when relevant\nFoundation information shall include:\n     - The outer dimensions and footprint of the support frame or foundation supports\n     - The size, grade and location of the foundation bolts and torque where this is \nnecessary\n     - Forces and moments transferred to load bearing structures, both under normal \noperation and extreme conditions\n     - Details for adjustment and alignment\n     - Details for cut-outs inside outer limit of foundation\n     - Details for vibration dampening units (if installed)\n\nFor Lifting appliances:\nGeneral arrangement drawing of complete unit and foundation:\n - Dimensions\n - Location of centre of gravity\n - Total weight in operational condition\nFoundation:\n     - The outer dimensions and footprint of the support frame or foundation \nsupport\n     - The size, grade and location of the foundation bolts and torque where this is \nnecessary\n     - Forces and moments transferred to load bearing structures, both under \nnormal operation and extreme conditions\n     - Details for adjustment and alignment\nGeneral arrangement drawing for Crane cabin, machinery room, winches, crane boom, \nslewing drives, main drive, hook block, wire sheave arrangements, etc.:\n - Dimensions\n - Location and identification of bolting, piping and main components\n - Location of centre of gravity\n - Total weight in operational condition\nGeneral arrangement drawing for inspections for primary steel structures e.g. \npedestal/foundation, crane boom/traverse beams, A-frame, runway beams, winches, hook \nblock, etc.\n - Critical welds shall be included with a weld identification number including weld\nclassification. NDT procedures and intervals for each weld classification shall be \nincluded.\n\nFor Well completion equipment:\nElectrical submergible pump (ESP)\n - Dimensions\n - Weights, centre of gravity and main dimensions of disassembled \nunits/components over 25 kg\nWellhead penetrator\n - Dimensions\n - Necessary space for disassembly and maintenance\n - Obstacles from other disciplines shall be included when relevant\n - All equipment including technical network cabinets, junction boxes, push buttons, \nlight fittings, socket outlets, etc.\n - Parts list" ;
                  rdfs:comment "Below are examples of expected level of detail. One or more examples may apply.\nFor Mechanical equipment:\n - Dimensions\n - Location and identification of piping and main components\n - Necessary space for disassembly and maintenance\n - Location of centre of gravity\n - Thermal expansion effect, when relevant\n - On the structural steel drawings, critical welds shall be included with a weld \nidentification number serving as a cross-reference to the weld summary index\n - Obstacles from other disciplines shall be included when relevant\n - Total weight, wet and dry and in operational condition\n - Weights, centre of gravity and main dimensions of disassembled units/components \nover 25 kg. Lifting lugs and runway beam for disassembling and their location shall \nbe shown\n - Identification and location of all nozzle and external pipe connections as well as \nrequirements for flexible connections and acceptable loads and moments. Locations \nshall be dimensioned and tolerances shown, if necessary in separate drawings\n - Identification and location of all external electrical and control monitoring connections \n(may be given in separate drawings describing the electrical arrangement and \ninstrumentation)\n - For pressure equipment: for projects at locations where EU regulations for pressure \nequipment apply, Category and Module shall be according to 2014/68/EU (PED)\n - Include bolt tension requirements for pressure equipment flanges\n - Iidentification of lubrication points\n - Foundation information shall include:\n     - The outer dimensions and footprint of the support frame or foundation supports\n     - The size, grade and location of the foundation bolts and torque where this is \nnecessary\n     - Forces and moments transferred to load bearing structures, both under normal \noperation and extreme conditions\n     - Details for adjustment and alignment\n     - Details for cut-outs inside outer limit of foundation\n     - Details for vibration dampening units (if installed)\n\nFor Electrical equipment:\n - Panel equipment layout - position of modules, cards, vacant slots and other \ninformation necessary for expansion or installation of new equipment in the same \ncabinet\n - Internal layout showing arrangement of auxiliary modules, cable trunks, etc.\n - All equipment including junction boxes, push buttons, light fittings, socket outlets, etc.\n - Dimensions\n - Necessary space for disassembly and maintenance\n - Location of centre of gravity\n - Possible thermal expansion\n - Obstacles from other disciplines shall be included when relevant\n\nFor Instrument equipment:\n - Dimensions\n - Location and identification of piping and main components\n - Necessary space for disassembly and maintenance\n - Location of centre of gravity\n - Possible thermal expansion\n - Obstacles from other disciplines shall be included when relevant\n - Panel equipment layout - position of modules, cards, vacant slots and other \ninformation necessary for expansion or installation of new equipment in the same \ncabinet\n - Internal/back layout showing arrangement of auxiliary modules, cable trunks, etc.\n - All equipment including technical network cabinets, junction boxes, push buttons, \nlight fittings, socket outlets, etc.\n - Reference to part list/SPIR\n\nFor Telecom equipment:\nA detailed drawing of the equipment shall be delivered. The drawing shall be to scale with \ndimensions included.\nFor Panel/cabinet/rack the following shall be included in addition:\n - Position of modules, cards, vacant slots and other information necessary for \nexpansion or installation of new equipment in the same cabinet/rack\n - Internal/back layout showing arrangement of auxiliary modules, cable trunks, etc.\n\nFor HVAC equipment:\n - Dimensions\n - Location and identification of piping, ducting, MCTs (Multi core transit) and main \ncomponents\n - Necessary space for disassembly and maintenance\n - Location of centre of gravity\n - Possible thermal expansion\n - Obstacles from other disciplines shall be included when relevant\nFoundation information shall include:\n     - The outer dimensions and footprint of the support frame or foundation supports\n     - The size, grade and location of the foundation bolts and torque where this is \nnecessary\n     - Forces and moments transferred to load bearing structures, both under normal \noperation and extreme conditions\n     - Details for adjustment and alignment\n     - Details for cut-outs inside outer limit of foundation\n     - Details for vibration dampening units (if installed)\n\nFor Lifting appliances:\nGeneral arrangement drawing of complete unit and foundation:\n - Dimensions\n - Location of centre of gravity\n - Total weight in operational condition\nFoundation:\n     - The outer dimensions and footprint of the support frame or foundation \nsupport\n     - The size, grade and location of the foundation bolts and torque where this is \nnecessary\n     - Forces and moments transferred to load bearing structures, both under \nnormal operation and extreme conditions\n     - Details for adjustment and alignment\nGeneral arrangement drawing for Crane cabin, machinery room, winches, crane boom, \nslewing drives, main drive, hook block, wire sheave arrangements, etc.:\n - Dimensions\n - Location and identification of bolting, piping and main components\n - Location of centre of gravity\n - Total weight in operational condition\nGeneral arrangement drawing for inspections for primary steel structures e.g. \npedestal/foundation, crane boom/traverse beams, A-frame, runway beams, winches, hook \nblock, etc.\n - Critical welds shall be included with a weld identification number including weld\nclassification. NDT procedures and intervals for each weld classification shall be \nincluded.\n\nFor Well completion equipment:\nElectrical submergible pump (ESP)\n - Dimensions\n - Weights, centre of gravity and main dimensions of disassembled \nunits/components over 25 kg\nWellhead penetrator\n - Dimensions\n - Necessary space for disassembly and maintenance\n - Obstacles from other disciplines shall be included when relevant\n - All equipment including technical network cabinets, junction boxes, push buttons, \nlight fittings, socket outlets, etc.\n - Parts list" ;
                  rdfs:label "General arrangement drawing" ;
                  skos:broadMatch rdl:PCA_100006708 ,
                                  rdl:PCA_100006710 ;
                  skos:broader rdl:PCA_100006739 .


###  http://rds.posccaesar.org/ontology/plm/rdl/PCA_100006234
rdl:PCA_100006234 rdf:type owl:Class ;
                  rdfs:subClassOf rdl:PCA_100004908 ;
                  rdl:PCA_100006765 rrdl:CFIHOS-20000018 ;
                  rdl:PCA_100006766 rdl:PCA_100006654 ;
                  rdl:PCA_100006768 "Drawings of anchoring structures and wall penetrations shall cover materials, geometry, dimensions, position of pipeline in anchoring structure, minimum separation between pipeline and possible reinforcement and rockbolts, pipeline coating inside anchoring structure in addition to sealing and centring details for penetrations (such as concrete pits and –walls)." ;
                  rdfs:comment "Drawings of anchoring structures and wall penetrations shall cover materials, geometry, dimensions, position of pipeline in anchoring structure, minimum separation between pipeline and possible reinforcement and rockbolts, pipeline coating inside anchoring structure in addition to sealing and centring details for penetrations (such as concrete pits and –walls)." ;
                  rdfs:label "General arrangement drawing - Anchoring structures and wall penetrations" ;
                  skos:broadMatch rdl:PCA_100006708 ;
                  skos:broader rdl:PCA_100006739 .


###  http://rds.posccaesar.org/ontology/plm/rdl/PCA_100006235
rdl:PCA_100006235 rdf:type owl:Class ;
                  rdfs:subClassOf rdl:PCA_100004908 ;
                  rdl:PCA_100006763 "General arrangement drawing of anode bed including location, depth, backfill materials (such as coke and bentonite clay), geotextiles, cables and cable routing." ;
                  rdl:PCA_100006765 rrdl:CFIHOS-20000018 ;
                  rdl:PCA_100006766 rdl:PCA_100006657 ;
                  rdl:PCA_100006768 "Details showing anode arrangement (anode location and material, anode dimensions, cables, cable joints and cable to anode connections) shall also be included." ;
                  rdfs:comment "Details showing anode arrangement (anode location and material, anode dimensions, cables, cable joints and cable to anode connections) shall also be included." ;
                  rdfs:label "General arrangement drawing - Anode bed" ;
                  skos:broadMatch rdl:PCA_100006708 ;
                  skos:broader rdl:PCA_100006739 .


###  http://rds.posccaesar.org/ontology/plm/rdl/PCA_100006236
rdl:PCA_100006236 rdf:type owl:Class ;
                  rdfs:subClassOf rdl:PCA_100004908 ;
                  rdl:PCA_100006763 "Drawing showing anode cable sections and connection to tesposts/TR-units." ;
                  rdl:PCA_100006765 rrdl:CFIHOS-20000018 ;
                  rdl:PCA_100006766 rdl:PCA_100006657 ;
                  rdl:PCA_100006768 "Details shall show type and cross-section of anode cable and possible low resistivity backfill." ;
                  rdfs:comment "Details shall show type and cross-section of anode cable and possible low resistivity backfill." ;
                  rdfs:label "General arrangement drawing - Continuous anode cable" ;
                  skos:broadMatch rdl:PCA_100006708 ;
                  skos:broader rdl:PCA_100006739 .


###  http://rds.posccaesar.org/ontology/plm/rdl/PCA_100006237
rdl:PCA_100006237 rdf:type owl:Class ;
                  rdfs:subClassOf rdl:PCA_100004908 ;
                  rdl:PCA_100006765 rrdl:CFIHOS-20000031 ;
                  rdl:PCA_100006768 "The manufacturer's standard general arrangement drawing shall be delivered." ;
                  rdfs:comment "The manufacturer's standard general arrangement drawing shall be delivered." ;
                  rdfs:label "General arrangement drawing (subsea)" ;
                  skos:broadMatch rdl:PCA_100006708 ,
                                  rdl:PCA_100006710 ;
                  skos:broader rdl:PCA_100006739 .


###  http://rds.posccaesar.org/ontology/plm/rdl/PCA_100006238
rdl:PCA_100006238 rdf:type owl:Class ;
                  rdfs:subClassOf rdl:PCA_100004908 ;
                  rdl:PCA_100006763 "General arrangement drawings for borehole and casing shall cover routing and longitudinal profile of borehole with pipeline installed." ;
                  rdl:PCA_100006765 rrdl:CFIHOS-20000018 ;
                  rdl:PCA_100006766 rdl:PCA_100006657 ;
                  rdl:PCA_100006768 "Cross sections, entry and exit point, possible casing pipes, bellmouth, entry- and exit point sealing, location of pipeline spacers and anodes in borehole, position of pipeline sections with different types of coatings shall be included.\n\nDetails shall include but not be limited to casing pipe, bellmouth, sealing arrangements, pipeline spacers and anodes, access arrangements for water sampling, exchange of water, location and details of CP-monitoring equipment, type and extent of possible infill material (such as grout and inhibited water)." ;
                  rdfs:comment "Cross sections, entry and exit point, possible casing pipes, bellmouth, entry- and exit point sealing, location of pipeline spacers and anodes in borehole, position of pipeline sections with different types of coatings shall be included.\n\nDetails shall include but not be limited to casing pipe, bellmouth, sealing arrangements, pipeline spacers and anodes, access arrangements for water sampling, exchange of water, location and details of CP-monitoring equipment, type and extent of possible infill material (such as grout and inhibited water)." ;
                  rdfs:label "General arrangement drawings - Bore hole and casing" ;
                  skos:broadMatch rdl:PCA_100006708 ;
                  skos:broader rdl:PCA_100006739 .


###  http://rds.posccaesar.org/ontology/plm/rdl/PCA_100006239
rdl:PCA_100006239 rdf:type owl:Class ;
                  rdfs:subClassOf rdl:PCA_100004908 ;
                  rdl:PCA_100006763 "General arrangement drawings for landfall shall cover routing and longitudinal profile of landfall with pipeline installed." ;
                  rdl:PCA_100006765 rrdl:CFIHOS-20000018 ;
                  rdl:PCA_100006766 rdl:PCA_100006657 ;
                  rdl:PCA_100006768 "Cross sections detailing the landfall protection such as rock protection, micro tunnel etc. shall be included." ;
                  rdfs:comment "Cross sections detailing the landfall protection such as rock protection, micro tunnel etc. shall be included." ;
                  rdfs:label "General arrangement drawings - Landfall" ;
                  skos:broadMatch rdl:PCA_100006708 ;
                  skos:broader rdl:PCA_100006739 .


###  http://rds.posccaesar.org/ontology/plm/rdl/PCA_100006240
rdl:PCA_100006240 rdf:type owl:Class ;
                  rdfs:subClassOf rdl:PCA_100004908 ;
                  rdl:PCA_100006763 "General arrangement drawings for pipeline structures such as riser bases, pipeline protection structures, tee/wye assemblies, anchor blocks, valve stations, pump stations, pig traps etc." ;
                  rdl:PCA_100006765 rrdl:CFIHOS-20000018 ;
                  rdl:PCA_100006766 rdl:PCA_100006653 ;
                  rdl:PCA_100006768 "These drawings shall contain the following information:\n - Dimensions\n - Location and identification of piping and main components\n - Necessary space for disassembly and maintenance\n - Location of centre of gravity\n - Possible thermal expansion.\n - On the structural steel drawings, critical welds shall be included with a weld identification number serving as a cross-reference to the weld summary index\n - Obstacles from other disciplines shall be included when relevant\n - Total weight, wet and dry and in operational condition\n - Weights, centre of gravity and main dimensions of disassembled units/components over 25 kg. Lifting lugs and runway beam for disassembling and their location shall be shown\n - Identification and location of all external pipeline connections as well as requirements for flexible connections and acceptable loads and moments. Locations shall be dimensioned, and tolerances shown, if necessary, in separate drawings\n - Identification and location of all external electrical and control monitoring connections (may be given in separate drawings describing the electrical arrangement and instrumentation)\n - For pressure equipment: For projects within the EU, Category and Module shall be according to PED (Pressure equipment directive)\n - Include bolt tension requirements for pressure equipment flanges\n - identification of lubrication points\n\nFoundation information (such as support frame, support structure) shall include:\n - The outer dimensions and footprint of the support frame or foundation supports\n - The size, grade and location of the foundation bolts and torque where this is necessary\n - Forces and moments transferred to load bearing structures, both under normal operation and extreme conditions\n - Details for adjustment and alignment\n - Details for cut-outs inside outer limit of foundation\n - Details for vibration dampening units (if installed)" ;
                  rdfs:comment "These drawings shall contain the following information:\n - Dimensions\n - Location and identification of piping and main components\n - Necessary space for disassembly and maintenance\n - Location of centre of gravity\n - Possible thermal expansion.\n - On the structural steel drawings, critical welds shall be included with a weld identification number serving as a cross-reference to the weld summary index\n - Obstacles from other disciplines shall be included when relevant\n - Total weight, wet and dry and in operational condition\n - Weights, centre of gravity and main dimensions of disassembled units/components over 25 kg. Lifting lugs and runway beam for disassembling and their location shall be shown\n - Identification and location of all external pipeline connections as well as requirements for flexible connections and acceptable loads and moments. Locations shall be dimensioned, and tolerances shown, if necessary, in separate drawings\n - Identification and location of all external electrical and control monitoring connections (may be given in separate drawings describing the electrical arrangement and instrumentation)\n - For pressure equipment: For projects within the EU, Category and Module shall be according to PED (Pressure equipment directive)\n - Include bolt tension requirements for pressure equipment flanges\n - identification of lubrication points\n\nFoundation information (such as support frame, support structure) shall include:\n - The outer dimensions and footprint of the support frame or foundation supports\n - The size, grade and location of the foundation bolts and torque where this is necessary\n - Forces and moments transferred to load bearing structures, both under normal operation and extreme conditions\n - Details for adjustment and alignment\n - Details for cut-outs inside outer limit of foundation\n - Details for vibration dampening units (if installed)" ;
                  rdfs:label "General arrangement drawings - Pipeline structures" ;
                  skos:broadMatch rdl:PCA_100006707 ;
                  skos:broader rdl:PCA_100006739 .


###  http://rds.posccaesar.org/ontology/plm/rdl/PCA_100006241
rdl:PCA_100006241 rdf:type owl:Class ;
                  rdfs:subClassOf rdl:PCA_100004908 ;
                  rdl:PCA_100006763 "This documentation shall provide information about the physical dimensions of the unit, needed to integrate the product into a system design." ;
                  rdl:PCA_100006764 "[ELECTRICAL]\nTorque on connections in main circuit shall be specified" ;
                  rdl:PCA_100006766 rdl:PCA_100006653 ;
                  rdl:PCA_100006768 "The manufacturer's standard general arrangement should be used as far as possible.\n\nA drawing showing overall dimensions, critical interface dimensions, part references and weight of assemblies, equipment and components. The drawing shall\ncontain reference to main specifications and standards  For equipment / components the drawing may include cross sectional views.\nDocument may contain the following information:\n - Main dimensions\n - Interface connections\n - Weight\n - Centre of gravity\n - Withdrawal/installation and maintenance space.\n - Installation and mounting details\n - Lifting arrangement" ;
                  rdfs:comment "The manufacturer's standard general arrangement should be used as far as possible.\n\nA drawing showing overall dimensions, critical interface dimensions, part references and weight of assemblies, equipment and components. The drawing shall\ncontain reference to main specifications and standards  For equipment / components the drawing may include cross sectional views.\nDocument may contain the following information:\n - Main dimensions\n - Interface connections\n - Weight\n - Centre of gravity\n - Withdrawal/installation and maintenance space.\n - Installation and mounting details\n - Lifting arrangement" ;
                  rdfs:label "General arrangment drawing" ;
                  skos:broadMatch rdl:PCA_100006708 ,
                                  rdl:PCA_100006709 ,
                                  rdl:PCA_100006710 ;
                  skos:broader rdl:PCA_100006739 .


###  http://rds.posccaesar.org/ontology/plm/rdl/PCA_100006242
rdl:PCA_100006242 rdf:type owl:Class ;
                  rdfs:subClassOf rdl:PCA_100004908 ;
                  rdl:PCA_100006763 "The requirement shall apply to field investigations, laboratory tests and analyses and cover facilities in rock." ;
                  rdl:PCA_100006765 rrdl:CFIHOS-20000018 ;
                  rdl:PCA_100006766 rdl:PCA_100006654 ;
                  rdl:PCA_100006768 "The content and structure of the reports shall comply with the requirements in EN1997 or equivalent standard." ;
                  rdfs:comment "The content and structure of the reports shall comply with the requirements in EN1997 or equivalent standard." ;
                  rdfs:label "Geotechnical - Geotechnical reports" ;
                  skos:broadMatch rdl:PCA_100006689 ;
                  skos:broader rdl:PCA_100006756 .


###  http://rds.posccaesar.org/ontology/plm/rdl/PCA_100006243
rdl:PCA_100006243 rdf:type owl:Class ;
                  rdfs:subClassOf rdl:PCA_100004908 ;
                  rdl:PCA_100006763 "The results from the Topographical Survey shall be reported in a written document describing the various task and findings in a systematic way including appendices and data samples where applicable." ;
                  rdl:PCA_100006765 rrdl:CFIHOS-20000007 ;
                  rdl:PCA_100006766 rdl:PCA_100006656 ;
                  rdl:PCA_100006768 "The general content of the report shall as a minimum include the following items:\nDescriptive front page with dates and document numbers.\nComplete and systematic index, including appendices.\nRevision history with description of actions.\n - Introduction.\n   - General Project or Survey description (abstract)\n   - Scope, Objective and Responsibilities.\n   - Definitions and abbreviations.\n   - References.\n - Project or Survey description.\n   - Scope of work.\n   - Key maps - Overview of work area.\n   - Summary of results, task by task.\n   - Quality evaluation of achieved results.\n   - Geodesy.\n - Detailed results. \n   - Systematic detailed description of performed activities in same order as in Summary of results.\n   - Listing of data and observations.\n   - Used equipment and data acquisition parameters.\n   - Used references.\n   - Processing systems, methods and parameters.\n   - Reporting method and references.\n - Data Index of deliverables.\n   - Maps / drawings.\n   - Pictures.\n   - DTM.\n   - Etc.\n - Appendices.\n   - All relevant data.\n   - Data samples.\n   - Maps.\n - Etc." ;
                  rdfs:comment "The general content of the report shall as a minimum include the following items:\nDescriptive front page with dates and document numbers.\nComplete and systematic index, including appendices.\nRevision history with description of actions.\n - Introduction.\n   - General Project or Survey description (abstract)\n   - Scope, Objective and Responsibilities.\n   - Definitions and abbreviations.\n   - References.\n - Project or Survey description.\n   - Scope of work.\n   - Key maps - Overview of work area.\n   - Summary of results, task by task.\n   - Quality evaluation of achieved results.\n   - Geodesy.\n - Detailed results. \n   - Systematic detailed description of performed activities in same order as in Summary of results.\n   - Listing of data and observations.\n   - Used equipment and data acquisition parameters.\n   - Used references.\n   - Processing systems, methods and parameters.\n   - Reporting method and references.\n - Data Index of deliverables.\n   - Maps / drawings.\n   - Pictures.\n   - DTM.\n   - Etc.\n - Appendices.\n   - All relevant data.\n   - Data samples.\n   - Maps.\n - Etc." ;
                  rdfs:label "GIS mapping - Survey reports" ;
                  skos:broadMatch rdl:PCA_100006722 ;
                  skos:broader rdl:PCA_100006756 .


###  http://rds.posccaesar.org/ontology/plm/rdl/PCA_100006244
rdl:PCA_100006244 rdf:type owl:Class ;
                  rdfs:subClassOf rdl:PCA_100004908 ;
                  rdl:PCA_100006763 "The requirement shall apply to field investigations, laboratory tests and analyses. \n\nISO 14688, ISO 14689, ISO 17892 Geotechnical investigations and testing;\nEN 1997 Geotechnical design;\nBS6031 Code of practice for earthworks." ;
                  rdl:PCA_100006765 rrdl:CFIHOS-20000007 ;
                  rdl:PCA_100006766 rdl:PCA_100006656 ;
                  rdl:PCA_100006768 "The content and structure of the reports shall comply with the requirements in EN1997 or equivalent standard." ;
                  rdfs:comment "The content and structure of the reports shall comply with the requirements in EN1997 or equivalent standard." ;
                  rdfs:label "Ground investigation reports" ;
                  skos:broadMatch rdl:PCA_100006722 ;
                  skos:broader rdl:PCA_100006756 .


###  http://rds.posccaesar.org/ontology/plm/rdl/PCA_100006245
rdl:PCA_100006245 rdf:type owl:Class ;
                  rdfs:subClassOf rdl:PCA_100004908 ;
                  rdl:PCA_100006765 rrdl:CFIHOS-20000015 ;
                  rdl:PCA_100006766 rdl:PCA_100006626 ,
                                    rdl:PCA_100006627 ,
                                    rdl:PCA_100006633 ,
                                    rdl:PCA_100006641 ;
                  rdl:PCA_100006768 "Hardware loop typicals shall cover:\n - Typicals for all field instrument interfaces.\n\nDrawing should contain the following information:\n - Input/output from I/O-cards, barriers.\n - Field instrument information." ;
                  rdfs:comment "Hardware loop typicals shall cover:\n - Typicals for all field instrument interfaces.\n\nDrawing should contain the following information:\n - Input/output from I/O-cards, barriers.\n - Field instrument information." ;
                  rdfs:label "Hardware loop typicals" ;
                  skos:broadMatch rdl:PCA_100006712 ,
                                  rdl:PCA_100006713 ,
                                  rdl:PCA_100006734 ;
                  skos:broader rdl:PCA_100006746 .


###  http://rds.posccaesar.org/ontology/plm/rdl/PCA_100006246
rdl:PCA_100006246 rdf:type owl:Class ;
                  rdfs:subClassOf rdl:PCA_100004908 ;
                  rdl:PCA_100006763 "Identify, evaluate, control or correct the operational hazards in the system or operation. The HAZOP/HAZID is input to the design." ;
                  rdl:PCA_100006765 rrdl:CFIHOS-20000031 ;
                  rdl:PCA_100006766 rdl:PCA_100006657 ;
                  rdl:PCA_100006768 "A report summarizing the results from a systematic review of the system or operation with respect to operational hazards after the system is installed." ;
                  rdfs:comment "A report summarizing the results from a systematic review of the system or operation with respect to operational hazards after the system is installed." ;
                  rdfs:label "Hazid / hazop report" ;
                  skos:broadMatch rdl:PCA_100006726 ;
                  skos:broader rdl:PCA_100006756 .


###  http://rds.posccaesar.org/ontology/plm/rdl/PCA_100006247
rdl:PCA_100006247 rdf:type owl:Class ;
                  rdfs:subClassOf rdl:PCA_100004908 ;
                  rdl:PCA_100006765 rrdl:CFIHOS-20000008 ;
                  rdl:PCA_100006766 rdl:PCA_100006627 ,
                                    rdl:PCA_100006636 ,
                                    rdl:PCA_100006637 ,
                                    rdl:PCA_100006638 ;
                  rdl:PCA_100006768 "The heat tracing block diagram shall show the connection between the following:\n - Distribution board with circuit number;\n - Power supply cable numbers;\n - Junction boxes with tag number;\n - Heat tracing cable numbers." ;
                  rdfs:comment "The heat tracing block diagram shall show the connection between the following:\n - Distribution board with circuit number;\n - Power supply cable numbers;\n - Junction boxes with tag number;\n - Heat tracing cable numbers." ;
                  rdfs:label "Heat tracing block diagram" ;
                  skos:broadMatch rdl:PCA_100006695 ,
                                  rdl:PCA_100006696 ,
                                  rdl:PCA_100006699 ;
                  skos:broader rdl:PCA_100006740 .


###  http://rds.posccaesar.org/ontology/plm/rdl/PCA_100006248
rdl:PCA_100006248 rdf:type owl:Class ;
                  rdfs:subClassOf rdl:PCA_100004908 ;
                  rdl:PCA_100006763 "All lines including instrument tubing subject to heat tracing shall be shown on heat tracing isometrics." ;
                  rdl:PCA_100006765 rrdl:CFIHOS-20000008 ;
                  rdl:PCA_100006766 rdl:PCA_100006656 ;
                  rdl:PCA_100006768 "The isometrics can be based on piping isometrics, and shall include necessary information such as insulation type/thickness, temperature requirements, material of pipes and extent of heat tracing shall be clearly identified, including:\n - Graphical presentation of heat tracing cable (where installed);\n - Heat tracing cable numbers;\n - Junction boxes with tag code;\n - Distribution boards with circuits\n - End seal of heat tracing cable;\n - Splice of heat tracing;\n - Type and length of heat trace cables;\n - Minimum maintain temperature of heated medium;\n - Maximum medium temperatures;\n - Temperature control (where thermostat required) including set point of thermostat." ;
                  rdfs:comment "The isometrics can be based on piping isometrics, and shall include necessary information such as insulation type/thickness, temperature requirements, material of pipes and extent of heat tracing shall be clearly identified, including:\n - Graphical presentation of heat tracing cable (where installed);\n - Heat tracing cable numbers;\n - Junction boxes with tag code;\n - Distribution boards with circuits\n - End seal of heat tracing cable;\n - Splice of heat tracing;\n - Type and length of heat trace cables;\n - Minimum maintain temperature of heated medium;\n - Maximum medium temperatures;\n - Temperature control (where thermostat required) including set point of thermostat." ;
                  rdfs:label "Heat tracing isometrics" ;
                  skos:broadMatch rdl:PCA_100006710 ,
                                  rdl:PCA_100006732 ,
                                  rdl:PCA_100006733 ;
                  skos:broader rdl:PCA_100006746 .


###  http://rds.posccaesar.org/ontology/plm/rdl/PCA_100006249
rdl:PCA_100006249 rdf:type owl:Class ;
                  rdfs:subClassOf rdl:PCA_100004908 ;
                  rdl:PCA_100006763 "Provide a clear procedure to heat treat shop to ensure repeatability." ;
                  rdl:PCA_100006765 rrdl:CFIHOS-20000031 ;
                  rdl:PCA_100006766 rdl:PCA_100006653 ;
                  rdl:PCA_100006768 "Document specifying heating and cooling procedures to obtain specified conditions or properties." ;
                  rdfs:comment "Document specifying heating and cooling procedures to obtain specified conditions or properties." ;
                  rdfs:label "Heat treatment procedure" ;
                  skos:broadMatch rdl:PCA_100006688 ;
                  skos:broader rdl:PCA_100006751 .


###  http://rds.posccaesar.org/ontology/plm/rdl/PCA_100006250
rdl:PCA_100006250 rdf:type owl:Class ;
                  rdfs:subClassOf rdl:PCA_100004908 ;
                  rdl:PCA_100006763 "To document that the heat treatment performed meets specified requirements." ;
                  rdl:PCA_100006765 rrdl:CFIHOS-20000031 ;
                  rdl:PCA_100006766 rdl:PCA_100006653 ;
                  rdl:PCA_100006768 "Documents containing records of performed heat treatment." ;
                  rdfs:comment "Documents containing records of performed heat treatment." ;
                  rdfs:label "Heat treatment report" ;
                  skos:broadMatch rdl:PCA_100006722 ;
                  skos:broader rdl:PCA_100006756 .


###  http://rds.posccaesar.org/ontology/plm/rdl/PCA_100006251
rdl:PCA_100006251 rdf:type owl:Class ;
                  rdfs:subClassOf rdl:PCA_100004908 ;
                  rdl:PCA_100006763 "As required in FOR-2007-10-26-1181:" ;
                  rdl:PCA_100006765 rrdl:CFIHOS-20000010 ,
                                    rrdl:CFIHOS-20000011 ,
                                    rrdl:CFIHOS-20000013 ;
                  rdl:PCA_100006766 rdl:PCA_100006656 ;
                  rdl:PCA_100006768 "The following drawings shall be provided:\n\n1. Entire installation, profile view - all four quadrants\n\nThe drawings shall be prepared in accordance with the following requirements:\n - Showing entire structure from sea level to highest point;\n - Indication of sea level;\n - Elevation of helideck above sea level;\n - Elevation of highest point above sea level;\n - Location of obstacle lights;\n - Location of turbine exhaust outlet(s);\n - Location of cold emission source(s);\n - Location of anemometer(s);\n - Scales indicating metres and feet.\n\n\n2. Entire installation, plan view (looking from above)\n\nThe drawings shall be prepared in accordance with the following requirements:\n - Reference to platform and true north;\n - Location of obstacle lights;\n - Location of turbine exhaust outlet(s);\n - Location of cold emission source(s);\n - Location of anemometer(s);\n - Location of windsock(s);\n - Scales indicating metres and feet.\n\n\n3.  Helideck with surroundings (can included as a part of 2.)\n\nThe drawings shall be prepared in accordance with the following requirements:\n - Reference to platform and true north;\n - Latitude/Longitude (WGS84) of centre helideck;\n - Helideck magnetic direction, degrees True;\n - Helideck marking;\n - Helideck lighting;\n - Helideck firefighting equipment;\n - HTCC;\n - Antenna tower;\n - Lowered walkway/Perimeter net;\n - Accesses;\n - Depiction of Obstacle Free Sectors (180 and 210 degree);\n - Depiction of Limited Obstacle Sector (150 degree), including the extent of segment 1 and 2;\n - Elevation of structures in 150 LOS segment 1 and 2;\n - Elevation of structures close to 210 degree OFS;\n - Helicopter fuelling plant;\n - Scales indicating metres and feet." ;
                  rdfs:comment "The following drawings shall be provided:\n\n1. Entire installation, profile view - all four quadrants\n\nThe drawings shall be prepared in accordance with the following requirements:\n - Showing entire structure from sea level to highest point;\n - Indication of sea level;\n - Elevation of helideck above sea level;\n - Elevation of highest point above sea level;\n - Location of obstacle lights;\n - Location of turbine exhaust outlet(s);\n - Location of cold emission source(s);\n - Location of anemometer(s);\n - Scales indicating metres and feet.\n\n\n2. Entire installation, plan view (looking from above)\n\nThe drawings shall be prepared in accordance with the following requirements:\n - Reference to platform and true north;\n - Location of obstacle lights;\n - Location of turbine exhaust outlet(s);\n - Location of cold emission source(s);\n - Location of anemometer(s);\n - Location of windsock(s);\n - Scales indicating metres and feet.\n\n\n3.  Helideck with surroundings (can included as a part of 2.)\n\nThe drawings shall be prepared in accordance with the following requirements:\n - Reference to platform and true north;\n - Latitude/Longitude (WGS84) of centre helideck;\n - Helideck magnetic direction, degrees True;\n - Helideck marking;\n - Helideck lighting;\n - Helideck firefighting equipment;\n - HTCC;\n - Antenna tower;\n - Lowered walkway/Perimeter net;\n - Accesses;\n - Depiction of Obstacle Free Sectors (180 and 210 degree);\n - Depiction of Limited Obstacle Sector (150 degree), including the extent of segment 1 and 2;\n - Elevation of structures in 150 LOS segment 1 and 2;\n - Elevation of structures close to 210 degree OFS;\n - Helicopter fuelling plant;\n - Scales indicating metres and feet." ;
                  rdfs:label "Helideck drawings (offshore)" ;
                  skos:broadMatch rdl:PCA_100006707 ,
                                  rdl:PCA_100006731 ,
                                  rdl:PCA_100006732 ,
                                  rdl:PCA_100006733 ,
                                  rdl:PCA_100006734 ;
                  skos:broader rdl:PCA_100006746 .


###  http://rds.posccaesar.org/ontology/plm/rdl/PCA_100006252
rdl:PCA_100006252 rdf:type owl:Class ;
                  rdfs:subClassOf rdl:PCA_100004908 ;
                  rdl:PCA_100006763 "A drawing providing necessary information for an installation contractor to perform lifting and installation." ;
                  rdl:PCA_100006765 rrdl:CFIHOS-20000031 ;
                  rdl:PCA_100006766 rdl:PCA_100006653 ;
                  rdl:PCA_100006768 "Schematic drawing showing mechanical and connection interfaces on equipment." ;
                  rdfs:comment "Schematic drawing showing mechanical and connection interfaces on equipment." ;
                  rdfs:label "Hook-up /installation drawing" ;
                  skos:broadMatch rdl:PCA_100006708 ;
                  skos:broader rdl:PCA_100006746 .


###  http://rds.posccaesar.org/ontology/plm/rdl/PCA_100006253
rdl:PCA_100006253 rdf:type owl:Class ;
                  rdfs:subClassOf rdl:PCA_100004908 ;
                  rdl:PCA_100006763 "Information shall be given concerning health, safety and environment" ;
                  rdl:PCA_100006765 rrdl:CFIHOS-20000011 ,
                                    rrdl:CFIHOS-20000014 ;
                  rdl:PCA_100006766 rdl:PCA_100006653 ;
                  rdl:PCA_100006768 "Chemical substances that may be hazardous to personnel or environment. For all these chemicals datasheets shall be available during installation, operation and maintenance substances that in connection with maintenance, discarding or similar, require special precautions forsake destruction noise vibration radiation and/or radioactivity dust ergonomics in operation and maintenance risk and criticality analyses." ;
                  rdfs:comment "Chemical substances that may be hazardous to personnel or environment. For all these chemicals datasheets shall be available during installation, operation and maintenance substances that in connection with maintenance, discarding or similar, require special precautions forsake destruction noise vibration radiation and/or radioactivity dust ergonomics in operation and maintenance risk and criticality analyses." ;
                  rdfs:label "HSE activity plan/program" ;
                  skos:broadMatch rdl:PCA_100006726 ,
                                  rdl:PCA_100006727 ,
                                  rdl:PCA_100006728 ,
                                  rdl:PCA_100006729 ;
                  skos:broader rdl:PCA_100006756 .


###  http://rds.posccaesar.org/ontology/plm/rdl/PCA_100006254
rdl:PCA_100006254 rdf:type owl:Class ;
                  rdfs:subClassOf rdl:PCA_100004908 ;
                  rdl:PCA_100006765 rrdl:CFIHOS-20000019 ;
                  rdl:PCA_100006766 rdl:PCA_100006653 ;
                  rdl:PCA_100006768 "The HVAC Bulk item index will include the following information for standard inline off-the-shelf HVAC items without electric, instrument or pneumatic connection and with no regular operation or maintenance requirements.\n - HVAC Bulk item number (according to ENS);\n - Functional service description;\n - Area;\n - Real manufacturer;\n - Variant/type/real manufacture part number." ;
                  rdfs:comment "The HVAC Bulk item index will include the following information for standard inline off-the-shelf HVAC items without electric, instrument or pneumatic connection and with no regular operation or maintenance requirements.\n - HVAC Bulk item number (according to ENS);\n - Functional service description;\n - Area;\n - Real manufacturer;\n - Variant/type/real manufacture part number." ;
                  rdfs:label "HVAC bulk items index" ;
                  skos:broadMatch rdl:PCA_100006716 ;
                  skos:broader rdl:PCA_100006748 .


###  http://rds.posccaesar.org/ontology/plm/rdl/PCA_100006255
rdl:PCA_100006255 rdf:type owl:Class ;
                  rdfs:subClassOf rdl:PCA_100004908 ;
                  rdl:PCA_100006763 "Numerical analyses:\nIf required to clarify wind effects on air inlets and outlets and to determine possible contamination of the air intake from other sources, a numerical analysis shall be carried out, preferably computerized on software agreed with Company.\nNumerical analysis shall also provide pressure coefficients for calculation of the natural ventilation and make a visualization of the natural ventilation in naturally ventilated areas. \n\nVentilation Air Volumes:\nCalculations carried out and documented to determine ventilation in naturally ventilated areas for different wind velocities and directions shall be transferred.\n\nNecessary ventilation volumes shall be determined and documented with regard to potential gas leaks and other contaminations in the ventilated area. \n\nOther calculations/analyses to be transferred (as required):\n\nConsumption calculations of current and energy.\n\nHeating and cooling capacity calculations, performance calculations for air supply/external devices, pressure drop calculations, sound level calculations." ;
                  rdl:PCA_100006764 "Rename to Calculation/analyses. Discipline specific content to be defined." ;
                  rdl:PCA_100006765 rrdl:CFIHOS-20000019 ;
                  rdl:PCA_100006766 rdl:PCA_100006650 ;
                  rdfs:label "HVAC calculations / analyses" ;
                  skos:broadMatch rdl:PCA_100006687 ;
                  skos:broader rdl:PCA_100006741 .


###  http://rds.posccaesar.org/ontology/plm/rdl/PCA_100006256
rdl:PCA_100006256 rdf:type owl:Class ;
                  rdfs:subClassOf rdl:PCA_100004908 ;
                  rdl:PCA_100006765 rrdl:CFIHOS-20000019 ;
                  rdl:PCA_100006766 rdl:PCA_100006650 ;
                  rdl:PCA_100006768 "The HVAC control philosophy shall as a minimum include: \n - Heating/cooling control;\n - Fan control;\n - Start/stop sequence;\n - Vibration monitoring;\n - Flow control;\n - Shut down;\n - Gas/fire/smoke control;\n - Operational modes;\n - Central control system;\n - Local control/indicators." ;
                  rdfs:comment "The HVAC control philosophy shall as a minimum include: \n - Heating/cooling control;\n - Fan control;\n - Start/stop sequence;\n - Vibration monitoring;\n - Flow control;\n - Shut down;\n - Gas/fire/smoke control;\n - Operational modes;\n - Central control system;\n - Local control/indicators." ;
                  rdfs:label "HVAC control philosophy" ;
                  skos:broadMatch rdl:PCA_100006695 ,
                                  rdl:PCA_100006698 ;
                  skos:broader rdl:PCA_100006752 .


###  http://rds.posccaesar.org/ontology/plm/rdl/PCA_100006257
rdl:PCA_100006257 rdf:type owl:Class ;
                  rdfs:subClassOf rdl:PCA_100004908 ;
                  rdl:PCA_100006765 rrdl:CFIHOS-20000019 ;
                  rdl:PCA_100006766 rdl:PCA_100006650 ;
                  rdl:PCA_100006768 "The HVAC design philosophy shall as a minimum include: \n - Purpose of HVAC installation;\n - Ambient conditions;\n - Indoor conditions;\n - Utilities for HVAC;\n - Natural ventilation;\n - Mechanical ventilation;\n - Sparing philosophy;\n - Pressurization;\n - Fire damper installation (LRA & HRA);\n - Smoke ventilation;\n - Air inlets/outlets;\n - Black Start;\n - Ductwork;\n - Local cooling/heating." ;
                  rdfs:comment "The HVAC design philosophy shall as a minimum include: \n - Purpose of HVAC installation;\n - Ambient conditions;\n - Indoor conditions;\n - Utilities for HVAC;\n - Natural ventilation;\n - Mechanical ventilation;\n - Sparing philosophy;\n - Pressurization;\n - Fire damper installation (LRA & HRA);\n - Smoke ventilation;\n - Air inlets/outlets;\n - Black Start;\n - Ductwork;\n - Local cooling/heating." ;
                  rdfs:label "HVAC design philosophy" ;
                  skos:broadMatch rdl:PCA_100006695 ,
                                  rdl:PCA_100006698 ;
                  skos:broader rdl:PCA_100006752 .


###  http://rds.posccaesar.org/ontology/plm/rdl/PCA_100006258
rdl:PCA_100006258 rdf:type owl:Class ;
                  rdfs:subClassOf rdl:PCA_100004908 ;
                  rdl:PCA_100006765 rrdl:CFIHOS-20000019 ;
                  rdl:PCA_100006768 "HVAC Layout drawings shall include: \n - Duct size\n - Duct location\n - HVAC Bulk item(s) (numbered according to ENS)\n - Tagged equipment\n - Ductwork and insulation classification\n - Penetrations\n - Inspection hatches, ladders, etc\n - Measuring points for system balancing\n - Relevant instruments\n - Service areas for HVAC equipment\n - Walls and grid lines" ;
                  rdfs:comment "HVAC Layout drawings shall include: \n - Duct size\n - Duct location\n - HVAC Bulk item(s) (numbered according to ENS)\n - Tagged equipment\n - Ductwork and insulation classification\n - Penetrations\n - Inspection hatches, ladders, etc\n - Measuring points for system balancing\n - Relevant instruments\n - Service areas for HVAC equipment\n - Walls and grid lines" ;
                  rdfs:label "HVAC layout drawings" ;
                  skos:broadMatch rdl:PCA_100006709 ;
                  skos:broader rdl:PCA_100006746 .


###  http://rds.posccaesar.org/ontology/plm/rdl/PCA_100006259
rdl:PCA_100006259 rdf:type owl:Class ;
                  rdfs:subClassOf rdl:PCA_100004908 ;
                  rdl:PCA_100006765 rrdl:CFIHOS-20000019 ;
                  rdl:PCA_100006766 rdl:PCA_100006650 ;
                  rdl:PCA_100006768 "The HVAC system description shall as a minimum include: \n - System split-up;\n - System description;\n - Sparing;\n - Equipment description;\n - Utilities for HVAC/interface with other systems;\n - System interlock;\n - Pressurization;\n - Fire damper installation (LRA & HRA);\n - Smoke ventilation;\n - Air inlets/outlets;\n - Black Start;\n - Ductwork;\n - Local cooling/heating;\n - Heating/cooling control;\n - Start/stop sequence;\n - Shut down;\n - Gas/fire/smoke control;\n - Operational modes;\n - Central control system;\n - Local control/indicators." ;
                  rdfs:comment "The HVAC system description shall as a minimum include: \n - System split-up;\n - System description;\n - Sparing;\n - Equipment description;\n - Utilities for HVAC/interface with other systems;\n - System interlock;\n - Pressurization;\n - Fire damper installation (LRA & HRA);\n - Smoke ventilation;\n - Air inlets/outlets;\n - Black Start;\n - Ductwork;\n - Local cooling/heating;\n - Heating/cooling control;\n - Start/stop sequence;\n - Shut down;\n - Gas/fire/smoke control;\n - Operational modes;\n - Central control system;\n - Local control/indicators." ;
                  rdfs:label "HVAC system description" ;
                  skos:broadMatch rdl:PCA_100006695 ,
                                  rdl:PCA_100006698 ;
                  skos:broader rdl:PCA_100006754 ,
                               rdl:PCA_100006756 .


###  http://rds.posccaesar.org/ontology/plm/rdl/PCA_100006260
rdl:PCA_100006260 rdf:type owl:Class ;
                  rdfs:subClassOf rdl:PCA_100004908 ;
                  rdl:PCA_100006768 "The hydraulic circuit diagrams shall include: \n - All components with identification \n - Port sizes \n - Pressure settings \n - Cross reference to Circuit wiring diagrams \n - Bulkhead connectors, pipes with dimensions \n - Hoses id with dimensions" ;
                  rdfs:comment "The hydraulic circuit diagrams shall include: \n - All components with identification \n - Port sizes \n - Pressure settings \n - Cross reference to Circuit wiring diagrams \n - Bulkhead connectors, pipes with dimensions \n - Hoses id with dimensions" ;
                  rdfs:label "Hydraulic circuit diagrams - lifting appliances" ;
                  skos:broadMatch rdl:PCA_100006702 ,
                                  rdl:PCA_100006712 ;
                  skos:broader rdl:PCA_100006745 .


###  http://rds.posccaesar.org/ontology/plm/rdl/PCA_100006261
rdl:PCA_100006261 rdf:type owl:Class ;
                  rdfs:subClassOf rdl:PCA_100004908 ;
                  rdl:PCA_100006763 "The purpose of this document is to cover hydraulic distribution from ring main or a hydraulic manifold to all hydraulic connections on a mechanical package, and to include all other individual hydraulic consumers for the actual hydraulic pressure unit." ;
                  rdl:PCA_100006765 rrdl:CFIHOS-20000015 ,
                                    rrdl:CFIHOS-20000031 ;
                  rdl:PCA_100006766 rdl:PCA_100006653 ;
                  rdfs:label "Hydraulic connection diagram" ;
                  skos:broadMatch rdl:PCA_100006712 ;
                  skos:broader rdl:PCA_100006745 .


###  http://rds.posccaesar.org/ontology/plm/rdl/PCA_100006262
rdl:PCA_100006262 rdf:type owl:Class ;
                  rdfs:subClassOf rdl:PCA_100004908 ;
                  rdl:PCA_100006768 "The hydraulic hose list shall include the following information:\n - Hose id (corresponding to hose id on Hydraulic circuit diagram)\n - Type (e.g. EN norm or SAE norm)\n - Length in mm\n - Fittings on A & B end\n - Max pressure rating for the hose\n - System pressure" ;
                  rdfs:comment "The hydraulic hose list shall include the following information:\n - Hose id (corresponding to hose id on Hydraulic circuit diagram)\n - Type (e.g. EN norm or SAE norm)\n - Length in mm\n - Fittings on A & B end\n - Max pressure rating for the hose\n - System pressure" ;
                  rdfs:label "Hydraulic hose list -lifting appliances" ;
                  skos:broadMatch rdl:PCA_100006716 ;
                  skos:broader rdl:PCA_100006748 .


###  http://rds.posccaesar.org/ontology/plm/rdl/PCA_100006263
rdl:PCA_100006263 rdf:type owl:Class ;
                  rdfs:subClassOf rdl:PCA_100004908 ;
                  rdl:PCA_100006763 "To provide an overview of hydraulic equipment and their connections." ;
                  rdl:PCA_100006765 rrdl:CFIHOS-20000031 ;
                  rdl:PCA_100006766 rdl:PCA_100006653 ;
                  rdl:PCA_100006768 "A diagram showing hydraulic connections between equipment and components." ;
                  rdfs:comment "A diagram showing hydraulic connections between equipment and components." ;
                  rdfs:label "Hydraulic schematic" ;
                  skos:broadMatch rdl:PCA_100006696 ;
                  skos:broader rdl:PCA_100006745 .


###  http://rds.posccaesar.org/ontology/plm/rdl/PCA_100006264
rdl:PCA_100006264 rdf:type owl:Class ;
                  rdfs:subClassOf rdl:PCA_100004908 ;
                  rdl:PCA_100006763 "Document that the hydraulic system has been adequately designed and sized in accordance with shut down and operational requirements as per design basis." ;
                  rdl:PCA_100006765 rrdl:CFIHOS-20000031 ;
                  rdl:PCA_100006766 rdl:PCA_100006657 ;
                  rdl:PCA_100006768 "The results from the hydraulic response analysis including sizing of hydraulic and chemical lines, subsea compensation, valve signatures as spring forces and volumes to verify for the system performance." ;
                  rdfs:comment "The results from the hydraulic response analysis including sizing of hydraulic and chemical lines, subsea compensation, valve signatures as spring forces and volumes to verify for the system performance." ;
                  rdfs:label "Hydraulic system calculation analysis" ;
                  skos:broadMatch rdl:PCA_100006687 ;
                  skos:broader rdl:PCA_100006741 .


###  http://rds.posccaesar.org/ontology/plm/rdl/PCA_100006265
rdl:PCA_100006265 rdf:type owl:Class ;
                  rdfs:subClassOf rdl:PCA_100004908 ;
                  rdl:PCA_100006763 "For liquid systems such as heating medium, cooling medium, fire water, offloading, loading, hydraulic power systems, drain, etc., hydraulics design shall be documented by hydraulic system calculations demonstrating as a minimum:" ;
                  rdl:PCA_100006765 rrdl:CFIHOS-20000010 ,
                                    rrdl:CFIHOS-20000011 ,
                                    rrdl:CFIHOS-20000013 ,
                                    rrdl:CFIHOS-20000026 ;
                  rdl:PCA_100006766 rdl:PCA_100006578 ,
                                    rdl:PCA_100006579 ,
                                    rdl:PCA_100006580 ,
                                    rdl:PCA_100006581 ,
                                    rdl:PCA_100006582 ,
                                    rdl:PCA_100006583 ,
                                    rdl:PCA_100006584 ,
                                    rdl:PCA_100006585 ,
                                    rdl:PCA_100006586 ,
                                    rdl:PCA_100006587 ,
                                    rdl:PCA_100006588 ,
                                    rdl:PCA_100006589 ,
                                    rdl:PCA_100006590 ,
                                    rdl:PCA_100006591 ,
                                    rdl:PCA_100006592 ,
                                    rdl:PCA_100006593 ,
                                    rdl:PCA_100006594 ,
                                    rdl:PCA_100006595 ,
                                    rdl:PCA_100006596 ,
                                    rdl:PCA_100006597 ,
                                    rdl:PCA_100006598 ,
                                    rdl:PCA_100006599 ,
                                    rdl:PCA_100006600 ,
                                    rdl:PCA_100006601 ,
                                    rdl:PCA_100006602 ,
                                    rdl:PCA_100006603 ,
                                    rdl:PCA_100006604 ,
                                    rdl:PCA_100006605 ,
                                    rdl:PCA_100006608 ,
                                    rdl:PCA_100006612 ,
                                    rdl:PCA_100006613 ,
                                    rdl:PCA_100006614 ,
                                    rdl:PCA_100006616 ,
                                    rdl:PCA_100006617 ,
                                    rdl:PCA_100006619 ,
                                    rdl:PCA_100006620 ,
                                    rdl:PCA_100006623 ,
                                    rdl:PCA_100006624 ,
                                    rdl:PCA_100006625 ,
                                    rdl:PCA_100006627 ,
                                    rdl:PCA_100006628 ;
                  rdl:PCA_100006768 " - The required hydraulic system (network) capacity, and correct design for in-line equipment, such as control valves, hydraulic/pneumatic actuators, etc.\n - For liquid systems where water hammering can be an issue, such as fire water and offloading systems, dynamic calculations shall be included as a part of the hydraulic system calculations. \n - Firewater:\n   - Results/evaluation from transient firewater hammer effect for ringmain high points in distribution system shall also be included.\n   - Piping and nozzle diagrams as well as Commissioning test reports and results shall be included as separate files.\n\nHydraulic system calculation reports and corresponding executable simulation files (preferably embedded in the report)." ;
                  rdfs:comment " - The required hydraulic system (network) capacity, and correct design for in-line equipment, such as control valves, hydraulic/pneumatic actuators, etc.\n - For liquid systems where water hammering can be an issue, such as fire water and offloading systems, dynamic calculations shall be included as a part of the hydraulic system calculations. \n - Firewater:\n   - Results/evaluation from transient firewater hammer effect for ringmain high points in distribution system shall also be included.\n   - Piping and nozzle diagrams as well as Commissioning test reports and results shall be included as separate files.\n\nHydraulic system calculation reports and corresponding executable simulation files (preferably embedded in the report)." ;
                  rdfs:label "Hydraulic system calculations" ;
                  skos:broadMatch rdl:PCA_100006687 ;
                  skos:broader rdl:PCA_100006741 .


###  http://rds.posccaesar.org/ontology/plm/rdl/PCA_100006266
rdl:PCA_100006266 rdf:type owl:Class ;
                  rdfs:subClassOf rdl:PCA_100004908 ;
                  rdl:PCA_100006763 "Hydraulic system calculation reports and input files/parameters shall be delivered. The report or collection of reports shall be self-contained, i.e. provide all information required to re-produce the results.\n\nCalculations shall include references to basis of design and explanatory text (system description, etc.). All calculations shall be described thoroughly and shown by sketches, inclusive references to third parts equipment (strainers, etc.) calculations, if any.\n\nAll hydraulic calculations shall include system characteristics, where normal operation conditions and reserves are analysed and documented. For tunnels, sensitivity calculations shall be made to identify uncertainties in roughness, and tunnel profiles, and presented as above." ;
                  rdl:PCA_100006765 rrdl:CFIHOS-20000007 ;
                  rdl:PCA_100006766 rdl:PCA_100006579 ,
                                    rdl:PCA_100006580 ,
                                    rdl:PCA_100006581 ,
                                    rdl:PCA_100006582 ,
                                    rdl:PCA_100006583 ,
                                    rdl:PCA_100006584 ,
                                    rdl:PCA_100006585 ,
                                    rdl:PCA_100006616 ;
                  rdl:PCA_100006768 "The calculations shall include:\n - Head loss calculations during normal operation, including definition\n - Head loss calculations during various climatic conditions, such as storm rain, snow melting (if applicable), etc.\n - Variation in sea level if the system has intake or discharge to sea\n - Surge calculations shall be performed for all pump systems" ;
                  rdfs:comment "The calculations shall include:\n - Head loss calculations during normal operation, including definition\n - Head loss calculations during various climatic conditions, such as storm rain, snow melting (if applicable), etc.\n - Variation in sea level if the system has intake or discharge to sea\n - Surge calculations shall be performed for all pump systems" ;
                  rdfs:label "Hydraulic systems calculations for open drain and tunnel systems" ;
                  skos:broadMatch rdl:PCA_100006687 ;
                  skos:broader rdl:PCA_100006741 .


###  http://rds.posccaesar.org/ontology/plm/rdl/PCA_100006267
rdl:PCA_100006267 rdf:type owl:Class ;
                  rdfs:subClassOf rdl:PCA_100004908 ;
                  rdl:PCA_100006763 "To verify the integrity of the components exposed to hyperbaric pressure and to provide traceability and quality assurance by recording all test results within the procedure." ;
                  rdl:PCA_100006765 rrdl:CFIHOS-20000031 ;
                  rdl:PCA_100006766 rdl:PCA_100006653 ;
                  rdl:PCA_100006768 "Procedure for hyperbaric testing of equipment as part of the qualification." ;
                  rdfs:comment "Procedure for hyperbaric testing of equipment as part of the qualification." ;
                  rdfs:label "Hyperbaric test procedure" ;
                  skos:broadMatch rdl:PCA_100006688 ;
                  skos:broader rdl:PCA_100006751 .


###  http://rds.posccaesar.org/ontology/plm/rdl/PCA_100006268
rdl:PCA_100006268 rdf:type owl:Class ;
                  rdfs:subClassOf rdl:PCA_100004908 ;
                  rdl:PCA_100006763 "The report shall document the weight and centre of gravity for the lightship weight of the vessel." ;
                  rdl:PCA_100006765 rrdl:CFIHOS-20000033 ;
                  rdl:PCA_100006766 rdl:PCA_100006657 ;
                  rdl:PCA_100006768 "The report shall give a thorough description of the inclining experiment, including method and weights." ;
                  rdfs:comment "The report shall give a thorough description of the inclining experiment, including method and weights." ;
                  rdfs:label "Inclination test report" ;
                  skos:broadMatch rdl:PCA_100006722 ;
                  skos:broader rdl:PCA_100006756 .


###  http://rds.posccaesar.org/ontology/plm/rdl/PCA_100006269
rdl:PCA_100006269 rdf:type owl:Class ;
                  rdfs:subClassOf rdl:PCA_100004908 ;
                  rdl:PCA_100006766 rdl:PCA_100006654 ;
                  rdfs:label "Index information" ;
                  skos:broader rdl:PCA_100006748 .


###  http://rds.posccaesar.org/ontology/plm/rdl/PCA_100006270
rdl:PCA_100006270 rdf:type owl:Class ;
                  rdfs:subClassOf rdl:PCA_100004908 ;
                  rdl:PCA_100006763 "A report verifying that equipment will remain in in-place condition." ;
                  rdl:PCA_100006765 rrdl:CFIHOS-20000031 ;
                  rdl:PCA_100006766 rdl:PCA_100006653 ;
                  rdl:PCA_100006768 "A report containing design analysis/calculations for in-place condition, including loads and load cases." ;
                  rdfs:comment "A report containing design analysis/calculations for in-place condition, including loads and load cases." ;
                  rdfs:label "In-place analysis report" ;
                  skos:broadMatch rdl:PCA_100006687 ;
                  skos:broader rdl:PCA_100006756 .


###  http://rds.posccaesar.org/ontology/plm/rdl/PCA_100006271
rdl:PCA_100006271 rdf:type owl:Class ;
                  rdfs:subClassOf rdl:PCA_100004908 ;
                  rdl:PCA_100006763 "The philosophy shall reccommend methods, technics and/or routines to reveal and prevent typical failures that can influence the integrity or the purpose of the pipeline, ref also Barrier matrix." ;
                  rdl:PCA_100006765 rrdl:CFIHOS-20000018 ;
                  rdl:PCA_100006766 rdl:PCA_100006654 ;
                  rdl:PCA_100006768 "The philosophy shall recommend follow up frequency and methods based on assumptions made during design and expected challenges and areas that require special focus." ;
                  rdfs:comment "The philosophy shall recommend follow up frequency and methods based on assumptions made during design and expected challenges and areas that require special focus." ;
                  rdfs:label "Inspection and maintenance philosophy for pipelines" ;
                  skos:broadMatch rdl:PCA_100006688 ;
                  skos:broader rdl:PCA_100006752 .


###  http://rds.posccaesar.org/ontology/plm/rdl/PCA_100006272
rdl:PCA_100006272 rdf:type owl:Class ;
                  rdfs:subClassOf rdl:PCA_100004908 ;
                  rdl:PCA_100006763 "A document with recommended inspection and monitoring program addressing the items in Section 11 of API 17B and integrity management for ancillary components addressed in API 17L2 Recommended practice for flexible pipe ancillary equipment. The inspection and monitoring program minimum requirements shall be in accordance with Sections 11.2 and 11.5 of API 17B." ;
                  rdl:PCA_100006765 rrdl:CFIHOS-20000018 ;
                  rdl:PCA_100006766 rdl:PCA_100006654 ;
                  rdl:PCA_100006768 "The document shall take into consideration the experience from the actual design and manufacturing of the flexible pipe and ancillary components not limited to addressing non-conformances and critical design issues." ;
                  rdfs:comment "The document shall take into consideration the experience from the actual design and manufacturing of the flexible pipe and ancillary components not limited to addressing non-conformances and critical design issues." ;
                  rdfs:label "Inspection and monitoring program flexible pipeline and riser" ;
                  skos:broadMatch rdl:PCA_100006688 ;
                  skos:broader rdl:PCA_100006750 .


###  http://rds.posccaesar.org/ontology/plm/rdl/PCA_100006273
rdl:PCA_100006273 rdf:type owl:Class ;
                  rdfs:subClassOf rdl:PCA_100004908 ;
                  rdl:PCA_100006763 "This document shall support both the procurement process and quality controlling activities to assure that the equipment will be delivered according to specification." ;
                  rdl:PCA_100006766 rdl:PCA_100006653 ;
                  rdl:PCA_100006768 "The ITP shall list scheduled inspection or verification activities in the production process, from purchase order to delivery. Reference to applicable standard or procedure and acceptance criteria shall be included. Inspection items that needs to be controlled/witnessed by purchaser, 3rd parties etc. shall be identified." ;
                  rdfs:comment "The ITP shall list scheduled inspection or verification activities in the production process, from purchase order to delivery. Reference to applicable standard or procedure and acceptance criteria shall be included. Inspection items that needs to be controlled/witnessed by purchaser, 3rd parties etc. shall be identified." ;
                  rdfs:label "Inspection and test plan" ;
                  skos:broadMatch rdl:PCA_100006722 ;
                  skos:broader rdl:PCA_100006756 .


###  http://rds.posccaesar.org/ontology/plm/rdl/PCA_100006274
rdl:PCA_100006274 rdf:type owl:Class ;
                  rdfs:subClassOf rdl:PCA_100004908 ;
                  rdl:PCA_100006763 "IOM documents shall, in an organized manner, provide sufficient information to install, operate and maintain the equipment in a safe, economical and functionally correct manner." ;
                  rdl:PCA_100006765 rrdl:CFIHOS-20000022 ;
                  rdl:PCA_100006768 "Requirements for receipt, storage, installation, operation and maintenance of supplied valves. The document shall include, but not be limited to:\n - Instructions for un-packing, handling, lifting of consignment and components.\n - Requirements for storage and preservation/de-preservation/re-preservation during installation and commissioning.\n - Preservation maintenance to be carried out by the user during storage, installation and in the period prior to start-up for the intended use\n - Procedure and necessary documentation for installation, including any additional measures that Purchaser need to observe prior to and during installation\n - Information about valve functions, operating and maintenance instructions\n - Bolt tightening procedures, including lubrication requirements\n - Procedure for maintenance of packing boxes, including recommended compression\n - Procedure for dismantle and reassembly of actuator/gearbox\n - Information regarding lubrication\n - Technical and functional descriptions\n - Consumption data\n - Restrictions in use" ;
                  rdfs:comment "Requirements for receipt, storage, installation, operation and maintenance of supplied valves. The document shall include, but not be limited to:\n - Instructions for un-packing, handling, lifting of consignment and components.\n - Requirements for storage and preservation/de-preservation/re-preservation during installation and commissioning.\n - Preservation maintenance to be carried out by the user during storage, installation and in the period prior to start-up for the intended use\n - Procedure and necessary documentation for installation, including any additional measures that Purchaser need to observe prior to and during installation\n - Information about valve functions, operating and maintenance instructions\n - Bolt tightening procedures, including lubrication requirements\n - Procedure for maintenance of packing boxes, including recommended compression\n - Procedure for dismantle and reassembly of actuator/gearbox\n - Information regarding lubrication\n - Technical and functional descriptions\n - Consumption data\n - Restrictions in use" ;
                  rdfs:label "Installation , operating and maintenance instructions for valves" ;
                  skos:broadMatch rdl:PCA_100006688 ;
                  skos:broader rdl:PCA_100006749 .


###  http://rds.posccaesar.org/ontology/plm/rdl/PCA_100006275
rdl:PCA_100006275 rdf:type owl:Class ;
                  rdfs:subClassOf rdl:PCA_100004908 ;
                  rdl:PCA_100006765 rrdl:CFIHOS-20000018 ;
                  rdl:PCA_100006766 rdl:PCA_100006657 ;
                  rdl:PCA_100006768 "The installation and handling manual shall include:\n - installation,\n - load-out facilities at manufactures premises,\n - recommendations related to seawater fill or dry during installation,\n - outline installation method including main sequences,\n - allowable installation loads,\n - deformation,\n - capacities and limitations,\n - handling and lifting recommendations,\n - installation tolerances,\n - assembly and handling procedures for all accessories (ancillary equipment),\n - description of markings,\n - tolerances related to mounting positions of accessories along the flexible pipeline,\n - use of mounting tools, torque moments etc.,\n - relevant certificates." ;
                  rdfs:comment "The installation and handling manual shall include:\n - installation,\n - load-out facilities at manufactures premises,\n - recommendations related to seawater fill or dry during installation,\n - outline installation method including main sequences,\n - allowable installation loads,\n - deformation,\n - capacities and limitations,\n - handling and lifting recommendations,\n - installation tolerances,\n - assembly and handling procedures for all accessories (ancillary equipment),\n - description of markings,\n - tolerances related to mounting positions of accessories along the flexible pipeline,\n - use of mounting tools, torque moments etc.,\n - relevant certificates." ;
                  rdfs:label "Installation and handling manual flexible pipeline and riser" ;
                  skos:broadMatch rdl:PCA_100006688 ;
                  skos:broader rdl:PCA_100006751 .


###  http://rds.posccaesar.org/ontology/plm/rdl/PCA_100006276
rdl:PCA_100006276 rdf:type owl:Class ;
                  rdfs:subClassOf rdl:PCA_100004908 ;
                  rdl:PCA_100006763 "Design report covering pipeline installation. Basis for analysis, assumptions and assessments not given in design basis shall be included." ;
                  rdl:PCA_100006765 rrdl:CFIHOS-20000018 ;
                  rdl:PCA_100006766 rdl:PCA_100006654 ;
                  rdfs:label "Installation design report" ;
                  skos:broadMatch rdl:PCA_100006686 ;
                  skos:broader rdl:PCA_100006756 .


###  http://rds.posccaesar.org/ontology/plm/rdl/PCA_100006277
rdl:PCA_100006277 rdf:type owl:Class ;
                  rdfs:subClassOf rdl:PCA_100004908 ;
                  rdl:PCA_100006763 "Installation procedures shall be according to ISO15589-1 Section 13.1.2." ;
                  rdl:PCA_100006765 rrdl:CFIHOS-20000018 ;
                  rdl:PCA_100006766 rdl:PCA_100006657 ;
                  rdl:PCA_100006768 "The pipeline installation procedures shall reflect and take into account the CP-system." ;
                  rdfs:comment "The pipeline installation procedures shall reflect and take into account the CP-system." ;
                  rdfs:label "Installation procedures onshore CP system" ;
                  skos:broadMatch rdl:PCA_100006688 ;
                  skos:broader rdl:PCA_100006751 .


###  http://rds.posccaesar.org/ontology/plm/rdl/PCA_100006278
rdl:PCA_100006278 rdf:type owl:Class ;
                  rdfs:subClassOf rdl:PCA_100004908 ;
                  rdl:PCA_100006763 "To describe how to install, operate and maintain the equipment in a safe and functionally correct manner according to the specified maintenance philosophy." ;
                  rdl:PCA_100006766 rdl:PCA_100006653 ;
                  rdl:PCA_100006768 "The manufacturer's standard IOM  should be used as far as possible.\nThis document shall provide sufficient information to install, operate and maintain the equipment.\nThis document shall also provide sufficient information for troubleshooting." ;
                  rdfs:comment "The manufacturer's standard IOM  should be used as far as possible.\nThis document shall provide sufficient information to install, operate and maintain the equipment.\nThis document shall also provide sufficient information for troubleshooting." ;
                  rdfs:label "Installation, operation and maintenance instructions" ;
                  skos:broadMatch rdl:PCA_100006688 ;
                  skos:broader rdl:PCA_100006750 .


###  http://rds.posccaesar.org/ontology/plm/rdl/PCA_100006279
rdl:PCA_100006279 rdf:type owl:Class ;
                  rdfs:subClassOf rdl:PCA_100004908 ;
                  rdl:PCA_100006763 "IOM documents shall, in an organized manner, provide sufficient information to install, operate and maintain the equipment in a safe, economical and functionally correct manner according to the agreed maintenance philosophy. The equipment manufacturer’s standard IOM manual shall be delivered if it fulfils the intentions of this document, either as a complete IOM manual or split in two or more separate manuals. For assemblies/skids/packages the IOM manual shall cover the complete assembly." ;
                  rdl:PCA_100006768 "An IOM manual shall normally include the following information: \n\nMain Data \nInformation for the complete equipment showing all data necessary for the understanding of the equipment's mode of operation shall be given. Information regarding health, environment and safety shall be emphasized. Other data may be:\n - Restrictions in guarantee\n - Performance data\n - Restrictions in use\n - Main connections and requirements on connected systems\n - Weight and outline dimensions \nTechnical description \nDesign and function shall be described to facilitate a better understanding of the different parts of the operating and maintenance instructions. If the complete equipment package consists of several systems, the main system should be described first, followed by descriptions of each subsystem and their interconnections. \n\nPreparations \nAll preparations to be made from the moment the installation is completed until the equipment is ready for normal operation shall be described. The description shall include tests, adjustments, calibrations and necessary inspections. The sequence of the activities shall be stated as well as all tools, auxiliary equipment, consumables and spare parts that may be needed. If necessary, references to detailed technical information (e.g. performance and operational data) in other parts of the manual shall be made. \n\nOperating instructions \nStart, normal operation, stop and emergency stop The information shall be given in a logical sequence and shall include all operations and observations which the operator shall undertake. These may be:\n - Check list for prestart preparations\n - Prestart settings and precautions\n - The starting sequence shall include all modes of operation (manual, automatic, remote control, etc.)\n - Observations which shall be made during the starting sequence\n - Precautions concerning interruption of the starting sequence\n - Operations and observations during normal operation\n - Normal stop\n - Emergency stop\n - Start after emergency stop \n\nDisturbance of operation \nDescription of the various forms of disturbance of operation that may occur, how they can be identified and the consequences they may have for the operation, shall be given. \n\nCorrective measures \nA description shall be available of the necessary actions after a disturbance has occurred. For actions which cannot be taken by the operator, it may be necessary to refer to the maintenance instructions. The manual shall state all requirements for reports to the supplier in the form of registrations and observations. \n\nHazards and protective measures \nA description shall be given of all known hazards that may occur during operation. This also applies to hazards which are due to lack of observation of the supplier's procedures as well as to external causes, e. g. lack of cooling water, loss of electrical power, etc. The manual shall give detailed information about protective measures, how to reduce the consequences to a minimum and what procedures to follow in the event of an accident. Product data sheets for chemical substances shall be attached. \n\nQualification requirements and training program for operators \nThe supplier shall state the qualifications required of the operator and the training programs that can be offered. \n\nMaintenance \nGeneral Maintenance includes all inspections, measurements, adjustments and operations carried out directly on the equipment in order to ensure safe, reliable and economical operation. Maintenance documentation shall cover the maintenance which can normally be done by the user and the maintenance which is not expected to be done by the user. If the maintenance documentation shall be the basis of a maintenance system for the complete plant where the equipment is a part, then the customer shall state all necessary information and specify all special requests in the inquiry and order documentation. \n\nStructure and contents of operating instructions \nInstructions should contain a minimum of elements and shall be constructed as follows:\n - Introduction, scope and possible limitations of the instruction\n - Necessary safety precautions before and during maintenance\n - Detailed description of the procedure to be followed with references to relevant supplementary documentation\n - Necessary data and arrangement for lifting\n - List of necessary tools and equipment\n - Recommended spare parts and consumables\n - Control and measurement points with limits during maintenance and after completion prior to restart\n - Requirements for special skills and minimum crew for the maintenance\n - Registrations which should be part of a specially defined maintenance log \nMaintenance instructions \nThese shall be divided into the following separate instructions: \n\nRoutine inspection \nThis part of the maintenance consists of the regular inspections carried out by the operation and/or maintenance personnel. The inspections consist of what can be measured, seen, heard or felt without interference in the equipment both during an operation and while at standstill. The supplier shall give instructions concerning inspection points based on his own experience and the selected monitoring system. \n\nPeriodic maintenance \nIt shall cover all planned and expected maintenance based on operation time, calendar time or certain operational observations. This type of maintenance may e.g. include: \n - Cleaning\n - Lubrication schedule\n - Adjustments\n - Calibrations\n - Replacement of wear parts\n - Replenishments \n\nCorrections and minor repairs \nThe most comprehensive maintenance possible on site shall be described under this clause, e.g.:\n - Replacement of broken parts\n - Repairs which can be done on site or in a normally equipped maintenance shop\n - Dismantling parts of or the whole equipment for shipment to a special repair or overhaul shop Major repairs and modifications \nIt is not normally required that this shall be covered by the instructions at the user's disposal. However the supplier shall keep and upon request provide instructions concerning overhaul and repairs at special shops. If agreed, the supplier shall also keep all documentation for modification or rebuilding of the equipment. \n\nFault finding and correction of irregularities\n For heavy machinery, complicated equipment or if the equipment is considered critical for the total operation of the plant, the supplier shall include a fault finding diagram in his documentation. The diagram shall list possible faults and irregularities, and refer to possible causes. The diagram shall cover faults which may be discovered during operation and maintenance. Furthermore it shall be described how the fault is to be corrected, if necessary by referring to other maintenance instructions. The supplier should prepare a registration form where the results of measurements and observations can be noted systematically in order to give the supplier a better basis for diagnosis when the user requests supplier's assistance. \n\nStoring, preservation and maintenance of preservation\nThis clause shall describe storing of equipment removed from use. The description of the preparations for storage shall include preservation and other protection against external influences. The description of maintenance during storage shall include preventive and corrective measures to ensure that the functionality of the equipment is taken care of. The clause shall also describe how the equipment is prepared for operation after storage. The supplier shall also state how spare parts are to be stored and preserved. \n\n(reprint from NS5820, annex A2  - A6, with permission) \n\nLocal language: YES for lifting appliances" ;
                  rdfs:comment "An IOM manual shall normally include the following information: \n\nMain Data \nInformation for the complete equipment showing all data necessary for the understanding of the equipment's mode of operation shall be given. Information regarding health, environment and safety shall be emphasized. Other data may be:\n - Restrictions in guarantee\n - Performance data\n - Restrictions in use\n - Main connections and requirements on connected systems\n - Weight and outline dimensions \nTechnical description \nDesign and function shall be described to facilitate a better understanding of the different parts of the operating and maintenance instructions. If the complete equipment package consists of several systems, the main system should be described first, followed by descriptions of each subsystem and their interconnections. \n\nPreparations \nAll preparations to be made from the moment the installation is completed until the equipment is ready for normal operation shall be described. The description shall include tests, adjustments, calibrations and necessary inspections. The sequence of the activities shall be stated as well as all tools, auxiliary equipment, consumables and spare parts that may be needed. If necessary, references to detailed technical information (e.g. performance and operational data) in other parts of the manual shall be made. \n\nOperating instructions \nStart, normal operation, stop and emergency stop The information shall be given in a logical sequence and shall include all operations and observations which the operator shall undertake. These may be:\n - Check list for prestart preparations\n - Prestart settings and precautions\n - The starting sequence shall include all modes of operation (manual, automatic, remote control, etc.)\n - Observations which shall be made during the starting sequence\n - Precautions concerning interruption of the starting sequence\n - Operations and observations during normal operation\n - Normal stop\n - Emergency stop\n - Start after emergency stop \n\nDisturbance of operation \nDescription of the various forms of disturbance of operation that may occur, how they can be identified and the consequences they may have for the operation, shall be given. \n\nCorrective measures \nA description shall be available of the necessary actions after a disturbance has occurred. For actions which cannot be taken by the operator, it may be necessary to refer to the maintenance instructions. The manual shall state all requirements for reports to the supplier in the form of registrations and observations. \n\nHazards and protective measures \nA description shall be given of all known hazards that may occur during operation. This also applies to hazards which are due to lack of observation of the supplier's procedures as well as to external causes, e. g. lack of cooling water, loss of electrical power, etc. The manual shall give detailed information about protective measures, how to reduce the consequences to a minimum and what procedures to follow in the event of an accident. Product data sheets for chemical substances shall be attached. \n\nQualification requirements and training program for operators \nThe supplier shall state the qualifications required of the operator and the training programs that can be offered. \n\nMaintenance \nGeneral Maintenance includes all inspections, measurements, adjustments and operations carried out directly on the equipment in order to ensure safe, reliable and economical operation. Maintenance documentation shall cover the maintenance which can normally be done by the user and the maintenance which is not expected to be done by the user. If the maintenance documentation shall be the basis of a maintenance system for the complete plant where the equipment is a part, then the customer shall state all necessary information and specify all special requests in the inquiry and order documentation. \n\nStructure and contents of operating instructions \nInstructions should contain a minimum of elements and shall be constructed as follows:\n - Introduction, scope and possible limitations of the instruction\n - Necessary safety precautions before and during maintenance\n - Detailed description of the procedure to be followed with references to relevant supplementary documentation\n - Necessary data and arrangement for lifting\n - List of necessary tools and equipment\n - Recommended spare parts and consumables\n - Control and measurement points with limits during maintenance and after completion prior to restart\n - Requirements for special skills and minimum crew for the maintenance\n - Registrations which should be part of a specially defined maintenance log \nMaintenance instructions \nThese shall be divided into the following separate instructions: \n\nRoutine inspection \nThis part of the maintenance consists of the regular inspections carried out by the operation and/or maintenance personnel. The inspections consist of what can be measured, seen, heard or felt without interference in the equipment both during an operation and while at standstill. The supplier shall give instructions concerning inspection points based on his own experience and the selected monitoring system. \n\nPeriodic maintenance \nIt shall cover all planned and expected maintenance based on operation time, calendar time or certain operational observations. This type of maintenance may e.g. include: \n - Cleaning\n - Lubrication schedule\n - Adjustments\n - Calibrations\n - Replacement of wear parts\n - Replenishments \n\nCorrections and minor repairs \nThe most comprehensive maintenance possible on site shall be described under this clause, e.g.:\n - Replacement of broken parts\n - Repairs which can be done on site or in a normally equipped maintenance shop\n - Dismantling parts of or the whole equipment for shipment to a special repair or overhaul shop Major repairs and modifications \nIt is not normally required that this shall be covered by the instructions at the user's disposal. However the supplier shall keep and upon request provide instructions concerning overhaul and repairs at special shops. If agreed, the supplier shall also keep all documentation for modification or rebuilding of the equipment. \n\nFault finding and correction of irregularities\n For heavy machinery, complicated equipment or if the equipment is considered critical for the total operation of the plant, the supplier shall include a fault finding diagram in his documentation. The diagram shall list possible faults and irregularities, and refer to possible causes. The diagram shall cover faults which may be discovered during operation and maintenance. Furthermore it shall be described how the fault is to be corrected, if necessary by referring to other maintenance instructions. The supplier should prepare a registration form where the results of measurements and observations can be noted systematically in order to give the supplier a better basis for diagnosis when the user requests supplier's assistance. \n\nStoring, preservation and maintenance of preservation\nThis clause shall describe storing of equipment removed from use. The description of the preparations for storage shall include preservation and other protection against external influences. The description of maintenance during storage shall include preventive and corrective measures to ensure that the functionality of the equipment is taken care of. The clause shall also describe how the equipment is prepared for operation after storage. The supplier shall also state how spare parts are to be stored and preserved. \n\n(reprint from NS5820, annex A2  - A6, with permission) \n\nLocal language: YES for lifting appliances" ;
                  rdfs:label "Installation, operation and maintenance manual (IOM manual)" ;
                  skos:broadMatch rdl:PCA_100006688 ;
                  skos:broader rdl:PCA_100006749 .


###  http://rds.posccaesar.org/ontology/plm/rdl/PCA_100006280
rdl:PCA_100006280 rdf:type owl:Class ;
                  rdfs:subClassOf rdl:PCA_100004908 ;
                  rdl:PCA_100006763 "Ensure safe and efficient operation" ;
                  rdl:PCA_100006765 rrdl:CFIHOS-20000018 ;
                  rdl:PCA_100006766 rdl:PCA_100006657 ;
                  rdl:PCA_100006768 "IOM manual requirements:\n - The equipment manufacturers standard IOM manual shall be delivered.\n - For assemblies/skids/packages an IOM manual covering the complete assembly shall be delivered.\n - An IOM manual shall as a minimum include the following information:\n\nIntroduction\n - The Vendor’s address, telephone no., e-mail and web addresses\n - Subcontractor’s address, telephone no., e-mail and web addresses\n\nMain Data\nInformation for the complete equipment showing all data necessary for the understanding of the equipment's mode of operation shall be given. Information regarding health, environment and safety shall be emphasized. Other data may be:\n - restrictions in guarantee;\n - performance data;\n - restrictions in use;\n - main connections and requirements on connected systems;\n - weight and outline dimensions.\n\nTechnical description\nDesign and function shall be described to facilitate a better understanding of the different parts of the operating and maintenance instructions. If the complete equipment package consists of several systems, the main system should be described first, followed by descriptions of each subsystem and their interconnections.\n\nPreparations\nAll preparations to be made from the moment the installation is completed until the equipment is ready for normal operation shall be described. The description shall include tests, adjustments, calibrations and necessary inspections. The sequence of the activities shall be stated as well as all tools, auxiliary equipment, consumables and spare parts that may be needed. If necessary, references to detailed technical information (e.g. performance and operational data) in other parts of the manual shall be made.\n\nDisturbance of operation\nDescription of the various forms of disturbance of operation that may occur, how they can be identified and the consequences they may have for the operation, shall be given.\n\nCorrective measures\nA description shall be available of the necessary actions after a disturbance has occurred. For actions which cannot be taken by the operator, it may be necessary to refer to the maintenance instructions. The manual shall state all requirements for reports to the supplier in the form of registrations and observations.\n\nHazards and protective measures\nA description shall be given of all known hazards that may occur during operation. This also applies to hazards which are due to lack of observation of the supplier's procedures as well as to external causes, e. g. lack of cooling water, loss of electrical power, etc. The manual shall give detailed information about protective measures, how to reduce the consequences to a minimum and what procedures to follow in the event of an accident. Product data sheets for chemical substances shall be attached.\n\nQualification requirements and training program for operators\nThe supplier shall state the qualifications required of the operator and the training programs that can be offered.\n\n\nMaintenance\n\nGeneral\nMaintenance includes all inspections, measurements, adjustments and operations carried out directly on the equipment in order to ensure safe, reliable and economical operation. Maintenance documentation shall cover the maintenance which can normally be done by the user and the maintenance which is not expected to be done by the user. If the maintenance documentation shall be the basis of a maintenance system for the complete plant where the equipment is a part, then the customer shall state all necessary information and specify all special requests in the inquiry and order documentation.\n\nStructure and contents of operating instructions\nInstructions should contain a minimum of elements and shall be constructed as follows:\n1.introduction, scope and possible limitations of the instruction;\n2.a list of drawings or other necessary supplementary documentation;\n3.necessary safety precautions before and during maintenance;\n4.detailed description of the procedure to be followed with references to relevant supplementary documentation;\n5.necessary data and arrangement for lifting;\n6.list of necessary tools and equipment;\n7.recommended spare parts and consumables;\n8.control and measurement points with limits during maintenance and after completion prior to restart;\n9.requirements for special skills and minimum crew for the maintenance;\n10.registrations which should be part of a specially defined maintenance log.\n\nMaintenance instructions\nThese shall be divided into the following separate instructions:\n\nRoutine inspection\nThis part of the maintenance consists of the regular inspections carried out by the operation and/or maintenance personnel. The inspections consist of what can be measured, seen, heard or felt without interference in the equipment both during an operation and while at standstill. The supplier shall give instructions concerning inspection points based on his own experience and the selected monitoring system.\n\nPeriodic maintenance\nIt shall cover all planned and expected maintenance based on operation time, calendar time or certain operational observations. This type of maintenance may e.g. include:\n - cleaning;\n - lubrication schedule;\n - adjustments;\n - calibrations;\n - replacement of wear parts;\n - replenishments.\n\nCorrections and minor repairs\nThe most comprehensive maintenance possible on site shall be described under this clause, e.g.:\n - replacement of broken parts;\n - repairs which can be done on site or in a normally equipped maintenance shop;\n - dismantling parts of or the whole equipment for shipment to a special repair or overhaul shop.\n\nMajor repairs and modifications\nIt is not normally required that this shall be covered by the instructions at the user's disposal. However, the supplier shall keep and upon request provide instructions concerning overhaul and repairs at special shops. If agreed, the supplier shall also keep all documentation for modification or rebuilding of the equipment." ;
                  rdfs:comment "IOM manual requirements:\n - The equipment manufacturers standard IOM manual shall be delivered.\n - For assemblies/skids/packages an IOM manual covering the complete assembly shall be delivered.\n - An IOM manual shall as a minimum include the following information:\n\nIntroduction\n - The Vendor’s address, telephone no., e-mail and web addresses\n - Subcontractor’s address, telephone no., e-mail and web addresses\n\nMain Data\nInformation for the complete equipment showing all data necessary for the understanding of the equipment's mode of operation shall be given. Information regarding health, environment and safety shall be emphasized. Other data may be:\n - restrictions in guarantee;\n - performance data;\n - restrictions in use;\n - main connections and requirements on connected systems;\n - weight and outline dimensions.\n\nTechnical description\nDesign and function shall be described to facilitate a better understanding of the different parts of the operating and maintenance instructions. If the complete equipment package consists of several systems, the main system should be described first, followed by descriptions of each subsystem and their interconnections.\n\nPreparations\nAll preparations to be made from the moment the installation is completed until the equipment is ready for normal operation shall be described. The description shall include tests, adjustments, calibrations and necessary inspections. The sequence of the activities shall be stated as well as all tools, auxiliary equipment, consumables and spare parts that may be needed. If necessary, references to detailed technical information (e.g. performance and operational data) in other parts of the manual shall be made.\n\nDisturbance of operation\nDescription of the various forms of disturbance of operation that may occur, how they can be identified and the consequences they may have for the operation, shall be given.\n\nCorrective measures\nA description shall be available of the necessary actions after a disturbance has occurred. For actions which cannot be taken by the operator, it may be necessary to refer to the maintenance instructions. The manual shall state all requirements for reports to the supplier in the form of registrations and observations.\n\nHazards and protective measures\nA description shall be given of all known hazards that may occur during operation. This also applies to hazards which are due to lack of observation of the supplier's procedures as well as to external causes, e. g. lack of cooling water, loss of electrical power, etc. The manual shall give detailed information about protective measures, how to reduce the consequences to a minimum and what procedures to follow in the event of an accident. Product data sheets for chemical substances shall be attached.\n\nQualification requirements and training program for operators\nThe supplier shall state the qualifications required of the operator and the training programs that can be offered.\n\n\nMaintenance\n\nGeneral\nMaintenance includes all inspections, measurements, adjustments and operations carried out directly on the equipment in order to ensure safe, reliable and economical operation. Maintenance documentation shall cover the maintenance which can normally be done by the user and the maintenance which is not expected to be done by the user. If the maintenance documentation shall be the basis of a maintenance system for the complete plant where the equipment is a part, then the customer shall state all necessary information and specify all special requests in the inquiry and order documentation.\n\nStructure and contents of operating instructions\nInstructions should contain a minimum of elements and shall be constructed as follows:\n1.introduction, scope and possible limitations of the instruction;\n2.a list of drawings or other necessary supplementary documentation;\n3.necessary safety precautions before and during maintenance;\n4.detailed description of the procedure to be followed with references to relevant supplementary documentation;\n5.necessary data and arrangement for lifting;\n6.list of necessary tools and equipment;\n7.recommended spare parts and consumables;\n8.control and measurement points with limits during maintenance and after completion prior to restart;\n9.requirements for special skills and minimum crew for the maintenance;\n10.registrations which should be part of a specially defined maintenance log.\n\nMaintenance instructions\nThese shall be divided into the following separate instructions:\n\nRoutine inspection\nThis part of the maintenance consists of the regular inspections carried out by the operation and/or maintenance personnel. The inspections consist of what can be measured, seen, heard or felt without interference in the equipment both during an operation and while at standstill. The supplier shall give instructions concerning inspection points based on his own experience and the selected monitoring system.\n\nPeriodic maintenance\nIt shall cover all planned and expected maintenance based on operation time, calendar time or certain operational observations. This type of maintenance may e.g. include:\n - cleaning;\n - lubrication schedule;\n - adjustments;\n - calibrations;\n - replacement of wear parts;\n - replenishments.\n\nCorrections and minor repairs\nThe most comprehensive maintenance possible on site shall be described under this clause, e.g.:\n - replacement of broken parts;\n - repairs which can be done on site or in a normally equipped maintenance shop;\n - dismantling parts of or the whole equipment for shipment to a special repair or overhaul shop.\n\nMajor repairs and modifications\nIt is not normally required that this shall be covered by the instructions at the user's disposal. However, the supplier shall keep and upon request provide instructions concerning overhaul and repairs at special shops. If agreed, the supplier shall also keep all documentation for modification or rebuilding of the equipment." ;
                  rdfs:label "Installation, operation and maintenance manual (IOM manual) for CP" ;
                  skos:broadMatch rdl:PCA_100006688 ;
                  skos:broader rdl:PCA_100006751 .


###  http://rds.posccaesar.org/ontology/plm/rdl/PCA_100006281
rdl:PCA_100006281 rdf:type owl:Class ;
                  rdfs:subClassOf rdl:PCA_100004908 ;
                  rdl:PCA_100006763 "This document shall support verification of component design according to applicable design standards." ;
                  rdl:PCA_100006765 rrdl:CFIHOS-20000015 ;
                  rdl:PCA_100006766 rdl:PCA_100006653 ;
                  rdl:PCA_100006768 "Document content will depend on which equipment is supplied. Calculations will be done according to applicable standards.\nExamples of Instrument Calculations are:\n - Thermowell frequency calculation\n - dP flow element sizing calculation" ;
                  rdfs:comment "Document content will depend on which equipment is supplied. Calculations will be done according to applicable standards.\nExamples of Instrument Calculations are:\n - Thermowell frequency calculation\n - dP flow element sizing calculation" ;
                  rdfs:label "Instrument calculations" ;
                  skos:broadMatch rdl:PCA_100006687 ;
                  skos:broader rdl:PCA_100006741 .


###  http://rds.posccaesar.org/ontology/plm/rdl/PCA_100006282
rdl:PCA_100006282 rdf:type owl:Class ;
                  rdfs:subClassOf rdl:PCA_100004908 ;
                  rdl:PCA_100006763 "Used in engineering process to verify compliance with plant and process design. Used in operational phase for verification purposes, and in case replacement/modification of equipment is required." ;
                  rdl:PCA_100006765 rrdl:CFIHOS-20000015 ;
                  rdl:PCA_100006766 rdl:PCA_100006653 ;
                  rdl:PCA_100006768 "Supplier shall complete the data sheets as specified by customer. Content and data format to be solved in inquiry phase. Not required for commodity valves and manual on/off valves" ;
                  rdfs:comment "Supplier shall complete the data sheets as specified by customer. Content and data format to be solved in inquiry phase. Not required for commodity valves and manual on/off valves" ;
                  rdfs:label "Instrument data sheet" ;
                  skos:broadMatch rdl:PCA_100006686 ;
                  skos:broader rdl:PCA_100006747 .


###  http://rds.posccaesar.org/ontology/plm/rdl/PCA_100006283
rdl:PCA_100006283 rdf:type owl:Class ;
                  rdfs:subClassOf rdl:PCA_100004908 ;
                  rdl:PCA_100006765 rrdl:CFIHOS-20000015 ;
                  rdl:PCA_100006766 rdl:PCA_100006656 ;
                  rdl:PCA_100006768 "At least one field equipment layout drawing for each area or module deck level shall be produced.\n\nThe following content shall be included on the drawings:\n - Tagged field equipment including junction boxes and cabinets;\n - Sufficient main equipment on the drawing to easily identify the location of the field equipment;\n - Platform/plant northing and orientation with respect of true north;\n - Gridlines with north and east references;\n - Key plan;\n - Scale bar;\n - Match lines with drawing references;\n - Deck/area elevations." ;
                  rdfs:comment "At least one field equipment layout drawing for each area or module deck level shall be produced.\n\nThe following content shall be included on the drawings:\n - Tagged field equipment including junction boxes and cabinets;\n - Sufficient main equipment on the drawing to easily identify the location of the field equipment;\n - Platform/plant northing and orientation with respect of true north;\n - Gridlines with north and east references;\n - Key plan;\n - Scale bar;\n - Match lines with drawing references;\n - Deck/area elevations." ;
                  rdfs:label "Instrument field equipment layout drawings" ;
                  skos:broadMatch rdl:PCA_100006709 ;
                  skos:broader rdl:PCA_100006746 .


###  http://rds.posccaesar.org/ontology/plm/rdl/PCA_100006284
rdl:PCA_100006284 rdf:type owl:Class ;
                  rdfs:subClassOf rdl:PCA_100004908 ;
                  rdl:PCA_100006763 "The general earthing principles shall be included to ensure correct earthing of systems, equipment (cabinets, junction boxes and field devices) and cables." ;
                  rdl:PCA_100006765 rrdl:CFIHOS-20000015 ;
                  rdl:PCA_100006766 rdl:PCA_100006640 ;
                  rdl:PCA_100006768 "This diagram shall typically include:\n - Main equipment like system cabinets, termination cabinets, junction boxes and field devices;\n - Location of main equipment;\n - Signal type and function (typ. RS232, control signal) if applicable;\n - Typical interface, wiring and termination details from system cabinets and main earth bars to field devices;\n - Main earth bars for instrument and telecommunications;\n - Earthing electrodes;\n - Identification of PE bars and IE bars;\n - Identification of cable armour and screen." ;
                  rdfs:comment "This diagram shall typically include:\n - Main equipment like system cabinets, termination cabinets, junction boxes and field devices;\n - Location of main equipment;\n - Signal type and function (typ. RS232, control signal) if applicable;\n - Typical interface, wiring and termination details from system cabinets and main earth bars to field devices;\n - Main earth bars for instrument and telecommunications;\n - Earthing electrodes;\n - Identification of PE bars and IE bars;\n - Identification of cable armour and screen." ;
                  rdfs:label "Instrument/telecom. earthing distribution. schematic diagram" ;
                  skos:broadMatch rdl:PCA_100006702 ,
                                  rdl:PCA_100006712 ;
                  skos:broader rdl:PCA_100006745 .


###  http://rds.posccaesar.org/ontology/plm/rdl/PCA_100006285
rdl:PCA_100006285 rdf:type owl:Class ;
                  rdfs:subClassOf rdl:PCA_100004908 ;
                  rdl:PCA_100006763 "The procedure shall describe how to load an empty SAS system (assuming total black out), where to find the last version of the system (backup), and how to start up the system." ;
                  rdl:PCA_100006765 rrdl:CFIHOS-20000015 ;
                  rdl:PCA_100006766 rdl:PCA_100006657 ;
                  rdl:PCA_100006768 "Start-up description includes in what order the system should be started, focusing on safety first." ;
                  rdfs:comment "Start-up description includes in what order the system should be started, focusing on safety first." ;
                  rdfs:label "Instrumented systems - loading and start up procedures" ;
                  skos:broadMatch rdl:PCA_100006688 ;
                  skos:broader rdl:PCA_100006751 .


###  http://rds.posccaesar.org/ontology/plm/rdl/PCA_100006286
rdl:PCA_100006286 rdf:type owl:Class ;
                  rdfs:subClassOf rdl:PCA_100004908 ;
                  rdl:PCA_100006763 "Performance of components in SAS shall be documented. Refer to NORSOK I-002 for details about which parameter that shall be measured." ;
                  rdl:PCA_100006765 rrdl:CFIHOS-20000015 ;
                  rdl:PCA_100006766 rdl:PCA_100006657 ;
                  rdfs:label "Instrumented systems - performance data" ;
                  skos:broadMatch rdl:PCA_100006698 ;
                  skos:broader rdl:PCA_100006750 .


###  http://rds.posccaesar.org/ontology/plm/rdl/PCA_100006287
rdl:PCA_100006287 rdf:type owl:Class ;
                  rdfs:subClassOf rdl:PCA_100004908 ;
                  rdl:PCA_100006763 "Design report covering insulation joint design and requirements. The Insulating joints design report shall reflect the requirements for design in ISO 15589-1." ;
                  rdl:PCA_100006765 rrdl:CFIHOS-20000018 ;
                  rdl:PCA_100006766 rdl:PCA_100006657 ;
                  rdl:PCA_100006768 "The report shall cover, but not be limited to:\n - Selection of internal coating (coating type, -thickness, wear resistance regarding cleaning and inspection pigging, calculation of extent of coating based on fluid conductivity in pipeline during construction, commissioning and operational phase).\n - Mechanical design (such as allowable forces and moments).\n - Support and anchoring of insulating joint (electrical insulation)\n - External coating, field joints, thermal insulation and/or encapsulation.\n - Location (in pit below ground, above ground).\n - Spark gaps / high voltage protection (such as type, location, cable to pipeline connection, cable length)." ;
                  rdfs:comment "The report shall cover, but not be limited to:\n - Selection of internal coating (coating type, -thickness, wear resistance regarding cleaning and inspection pigging, calculation of extent of coating based on fluid conductivity in pipeline during construction, commissioning and operational phase).\n - Mechanical design (such as allowable forces and moments).\n - Support and anchoring of insulating joint (electrical insulation)\n - External coating, field joints, thermal insulation and/or encapsulation.\n - Location (in pit below ground, above ground).\n - Spark gaps / high voltage protection (such as type, location, cable to pipeline connection, cable length)." ;
                  rdfs:label "Insulating joints design report" ;
                  skos:broadMatch rdl:PCA_100006686 ;
                  skos:broader rdl:PCA_100006756 .


###  http://rds.posccaesar.org/ontology/plm/rdl/PCA_100006288
rdl:PCA_100006288 rdf:type owl:Class ;
                  rdfs:subClassOf rdl:PCA_100004908 ;
                  rdl:PCA_100006766 rdl:PCA_100006653 ;
                  rdl:PCA_100006768 "Drawings of insulating joints shall cover materials, geometry, dimensions, tolerances, weld bevel, internal and external coating, weld-in direction, spark gap attachment details and connection points, cables and cable connections." ;
                  rdfs:comment "Drawings of insulating joints shall cover materials, geometry, dimensions, tolerances, weld bevel, internal and external coating, weld-in direction, spark gap attachment details and connection points, cables and cable connections." ;
                  rdfs:label "Insulating joints drawing" ;
                  skos:broadMatch rdl:PCA_100006732 ;
                  skos:broader rdl:PCA_100006746 .


###  http://rds.posccaesar.org/ontology/plm/rdl/PCA_100006289
rdl:PCA_100006289 rdf:type owl:Class ;
                  rdfs:subClassOf rdl:PCA_100004908 ;
                  rdl:PCA_100006763 "Provide information to suppliers of interfacing equipment." ;
                  rdl:PCA_100006765 rrdl:CFIHOS-20000031 ;
                  rdl:PCA_100006766 rdl:PCA_100006653 ;
                  rdl:PCA_100006768 "A drawing showing information for an assembly of parts or sub-assemblies (co-functioning components, equipment or assemblies), including key interface dimensions, weight, assembly information and design limitations." ;
                  rdfs:comment "A drawing showing information for an assembly of parts or sub-assemblies (co-functioning components, equipment or assemblies), including key interface dimensions, weight, assembly information and design limitations." ;
                  rdfs:label "Interface drawing" ;
                  skos:broadMatch rdl:PCA_100006713 ;
                  skos:broader rdl:PCA_100006746 .


###  http://rds.posccaesar.org/ontology/plm/rdl/PCA_100006290
rdl:PCA_100006290 rdf:type owl:Class ;
                  rdfs:subClassOf rdl:PCA_100004908 ;
                  rdl:PCA_100006763 "Atex requirement for all intrinsically safe instrument/telecom-equipment.\n- IS / FISCO (Fieldbus Intrinsically Safe Concept) calculations.\n\n- Not required for wireless loops. For a IS wireless instrument, IS-calculation must be available in atex certificate/vendor standard documentation." ;
                  rdl:PCA_100006765 rrdl:CFIHOS-20000015 ,
                                    rrdl:CFIHOS-20000030 ;
                  rdl:PCA_100006766 rdl:PCA_100006655 ;
                  rdl:PCA_100006768 "Complete calculations according to IEC60079" ;
                  rdfs:comment "Complete calculations according to IEC60079" ;
                  rdfs:label "IS calculations" ;
                  skos:broadMatch rdl:PCA_100006687 ;
                  skos:broader rdl:PCA_100006741 .


###  http://rds.posccaesar.org/ontology/plm/rdl/PCA_100006291
rdl:PCA_100006291 rdf:type owl:Class ;
                  rdfs:subClassOf rdl:PCA_100004908 ;
                  rdl:PCA_100006765 rrdl:CFIHOS-20000018 ;
                  rdl:PCA_100006766 rdl:PCA_100006657 ;
                  rdl:PCA_100006768 "Drawings of isolating components shall cover material, geometry, dimensions, coating, location of electrical insulating materials for items such as, but not limited to, supports, casings and spacers." ;
                  rdfs:comment "Drawings of isolating components shall cover material, geometry, dimensions, coating, location of electrical insulating materials for items such as, but not limited to, supports, casings and spacers." ;
                  rdfs:label "Isolating component drawings" ;
                  skos:broadMatch rdl:PCA_100006732 ;
                  skos:broader rdl:PCA_100006746 .


###  http://rds.posccaesar.org/ontology/plm/rdl/PCA_100006292
rdl:PCA_100006292 rdf:type owl:Class ;
                  rdfs:subClassOf rdl:PCA_100004908 ;
                  rdl:PCA_100006765 rrdl:CFIHOS-20000018 ;
                  rdl:PCA_100006766 rdl:PCA_100006657 ;
                  rdl:PCA_100006768 "Documentation for construction done according to design" ;
                  rdfs:comment "Documentation for construction done according to design" ;
                  rdfs:label "Landfall construction drawings" ;
                  skos:broadMatch rdl:PCA_100006732 ;
                  skos:broader rdl:PCA_100006746 .


###  http://rds.posccaesar.org/ontology/plm/rdl/PCA_100006293
rdl:PCA_100006293 rdf:type owl:Class ;
                  rdfs:subClassOf rdl:PCA_100004908 ;
                  rdl:PCA_100006765 rrdl:CFIHOS-20000018 ;
                  rdl:PCA_100006766 rdl:PCA_100006657 ;
                  rdl:PCA_100006768 "Basis for design, assumptions and assessments not given in design basis shall be included." ;
                  rdfs:comment "Basis for design, assumptions and assessments not given in design basis shall be included." ;
                  rdfs:label "Landfall design report" ;
                  skos:broadMatch rdl:PCA_100006686 ;
                  skos:broader rdl:PCA_100006756 .


###  http://rds.posccaesar.org/ontology/plm/rdl/PCA_100006294
rdl:PCA_100006294 rdf:type owl:Class ;
                  rdfs:subClassOf rdl:PCA_100004908 ;
                  rdl:PCA_100006765 rrdl:CFIHOS-20000007 ;
                  rdl:PCA_100006766 rdl:PCA_100006656 ;
                  rdl:PCA_100006768 "All arrangement, layout, plan, section and detail drawings shall be included." ;
                  rdfs:comment "All arrangement, layout, plan, section and detail drawings shall be included." ;
                  rdfs:label "Landscaping drawings" ;
                  skos:broadMatch rdl:PCA_100006705 ;
                  skos:broader rdl:PCA_100006746 .


###  http://rds.posccaesar.org/ontology/plm/rdl/PCA_100006295
rdl:PCA_100006295 rdf:type owl:Class ;
                  rdfs:subClassOf rdl:PCA_100004908 ;
                  rdl:PCA_100006763 "For the purpose of documenting the engineering of level measurements, a \"Level measurement arrangement drawing\" per vessel shall be issued." ;
                  rdl:PCA_100006765 rrdl:CFIHOS-20000015 ;
                  rdl:PCA_100006766 rdl:PCA_100006656 ;
                  rdl:PCA_100006768 "A \"Level measurement arrangement drawing\" per vessel shall be issued, encompassing:\n - Dimensions;\n - Nozzles (including nozzles for pressure and temperature measurements);\n - Level glasses;\n - Location of measurement elements;\n - Calibration and measurement ranges;\n - Alarm levels;\n - Correlation between engineering units of measure (e.g. mm and %, with calculations);\n - ENS Tag number." ;
                  rdfs:comment "A \"Level measurement arrangement drawing\" per vessel shall be issued, encompassing:\n - Dimensions;\n - Nozzles (including nozzles for pressure and temperature measurements);\n - Level glasses;\n - Location of measurement elements;\n - Calibration and measurement ranges;\n - Alarm levels;\n - Correlation between engineering units of measure (e.g. mm and %, with calculations);\n - ENS Tag number." ;
                  rdfs:label "Level instrument arrangement drawings" ;
                  skos:broadMatch rdl:PCA_100006710 ;
                  skos:broader rdl:PCA_100006739 .


###  http://rds.posccaesar.org/ontology/plm/rdl/PCA_100006296
rdl:PCA_100006296 rdf:type owl:Class ;
                  rdfs:subClassOf rdl:PCA_100004908 ;
                  rdl:PCA_100006763 "Certificate to prove that the item can be used as lifting gear in accordance with an applicable standard. This will include slings, shackles, lugs, lifting frames, lifting instructions etc." ;
                  rdl:PCA_100006766 rdl:PCA_100006653 ;
                  rdl:PCA_100006768 "To confirm that the equipment can be safely used for lifting and handling for the applicable load stated.\n\nVALVES\nContent according to Norsok R-002, section F.7.8. (related to lifting points)" ;
                  rdfs:comment "To confirm that the equipment can be safely used for lifting and handling for the applicable load stated.\n\nVALVES\nContent according to Norsok R-002, section F.7.8. (related to lifting points)" ;
                  rdfs:label "Lifting certificate" ;
                  skos:broadMatch rdl:PCA_100006722 ;
                  skos:broader rdl:PCA_100006743 .


###  http://rds.posccaesar.org/ontology/plm/rdl/PCA_100006297
rdl:PCA_100006297 rdf:type owl:Class ;
                  rdfs:subClassOf rdl:PCA_100004908 ;
                  rdl:PCA_100006763 "A drawing containing information necessary for rigging and lifting of equipment." ;
                  rdl:PCA_100006765 rrdl:CFIHOS-20000031 ;
                  rdl:PCA_100006766 rdl:PCA_100006653 ;
                  rdl:PCA_100006768 "A drawing showing necessary arrangements for rigging and lifting, including lifting points and centre of gravity for equipment." ;
                  rdfs:comment "A drawing showing necessary arrangements for rigging and lifting, including lifting points and centre of gravity for equipment." ;
                  rdfs:label "Lifting drawing" ;
                  skos:broadMatch rdl:PCA_100006731 ;
                  skos:broader rdl:PCA_100006746 .


###  http://rds.posccaesar.org/ontology/plm/rdl/PCA_100006298
rdl:PCA_100006298 rdf:type owl:Class ;
                  rdfs:subClassOf rdl:PCA_100004908 ;
                  rdl:PCA_100006765 rrdl:CFIHOS-20000008 ;
                  rdl:PCA_100006766 rdl:PCA_100006656 ;
                  rdl:PCA_100006768 "These drawings are relevant for offshore facilities and for the process plant and well pad area for onshore facilities. \n\nAt least one lighting and small power layout drawing for each area or module deck level shall be produced. The size of the facility will determine the scale of the drawing, but normally a scale of 1:100 on A3 format shall be aimed for. If required several drawings per area can be necessary to achieve this scale. Equipment which is covered by platforms above shall be shown dotted or shown in separate figures.\n\nThe lighting and small power layout drawing should be based on the equipment layout drawing, and the following electrical field equipment shall be included:\nLighting fixture, flood lights, socket outlet and junction boxes. These shall be tagged according to ENS." ;
                  rdfs:comment "These drawings are relevant for offshore facilities and for the process plant and well pad area for onshore facilities. \n\nAt least one lighting and small power layout drawing for each area or module deck level shall be produced. The size of the facility will determine the scale of the drawing, but normally a scale of 1:100 on A3 format shall be aimed for. If required several drawings per area can be necessary to achieve this scale. Equipment which is covered by platforms above shall be shown dotted or shown in separate figures.\n\nThe lighting and small power layout drawing should be based on the equipment layout drawing, and the following electrical field equipment shall be included:\nLighting fixture, flood lights, socket outlet and junction boxes. These shall be tagged according to ENS." ;
                  rdfs:label "Lighting and small power layout drawings" ;
                  skos:broadMatch rdl:PCA_100006709 ;
                  skos:broader rdl:PCA_100006746 .


###  http://rds.posccaesar.org/ontology/plm/rdl/PCA_100006299
rdl:PCA_100006299 rdf:type owl:Class ;
                  rdfs:subClassOf rdl:PCA_100004908 ;
                  rdl:PCA_100006765 rrdl:CFIHOS-20000018 ;
                  rdl:PCA_100006766 rdl:PCA_100006657 ;
                  rdl:PCA_100006768 "Liner system information shall contain as a minimum:\n - Liner system identification \n - Manufacturer's material data \n - Material pre-qualification information \n - Type and thickness of liner material \n - Expected short-term and long-term volumetric swelling or shrinkage for the range of operating conditions\n - Expected thermal deformations due to operating temperatures \n - Liner manufacturing procedure \n - Liner installation procedure \n - Anticipated insertion forces for each liner section in relation to the liner strength capabilities \n - Maximum allowable weld penetration of carbon steel pipeline girth welds" ;
                  rdfs:comment "Liner system information shall contain as a minimum:\n - Liner system identification \n - Manufacturer's material data \n - Material pre-qualification information \n - Type and thickness of liner material \n - Expected short-term and long-term volumetric swelling or shrinkage for the range of operating conditions\n - Expected thermal deformations due to operating temperatures \n - Liner manufacturing procedure \n - Liner installation procedure \n - Anticipated insertion forces for each liner section in relation to the liner strength capabilities \n - Maximum allowable weld penetration of carbon steel pipeline girth welds" ;
                  rdfs:label "Liner system information" ;
                  skos:broadMatch rdl:PCA_100006686 ;
                  skos:broader rdl:PCA_100006762 .


###  http://rds.posccaesar.org/ontology/plm/rdl/PCA_100006300
rdl:PCA_100006300 rdf:type owl:Class ;
                  rdfs:subClassOf rdl:PCA_100004908 ;
                  rdl:PCA_100006763 "Information sufficient to enable generation of complete loop diagrams as graphical representations from Company’s Loop system for instrument loops, fire & gas, telecom, and electrical interface to SAS shall be provided." ;
                  rdl:PCA_100006765 rrdl:CFIHOS-20000015 ;
                  rdl:PCA_100006766 rdl:PCA_100006655 ;
                  rdfs:label "Loop information" ;
                  skos:broadMatch rdl:PCA_100006698 ,
                                  rdl:PCA_100006699 ,
                                  rdl:PCA_100006700 ;
                  skos:broader rdl:PCA_100006762 .


###  http://rds.posccaesar.org/ontology/plm/rdl/PCA_100006301
rdl:PCA_100006301 rdf:type owl:Class ;
                  rdfs:subClassOf rdl:PCA_100004908 ;
                  rdl:PCA_100006768 "A lubrication index shall be provided containing the following information:\n - Tag code\n - Location of sampling point\n - Lubrication point sequence number (allocated by Company and referred to as TAS number) Supplier lubricant (product type)\n - Company equivalent lubricant\n - Quantity first fill\n - Quantity normal\n - Interval or monitoring frequency and parameters (particles, water content and additives) \n\nThe above lubrication information shall be provided in the Excel template linked below.\n Lubrication information template for SAP uploading" ;
                  rdfs:comment "A lubrication index shall be provided containing the following information:\n - Tag code\n - Location of sampling point\n - Lubrication point sequence number (allocated by Company and referred to as TAS number) Supplier lubricant (product type)\n - Company equivalent lubricant\n - Quantity first fill\n - Quantity normal\n - Interval or monitoring frequency and parameters (particles, water content and additives) \n\nThe above lubrication information shall be provided in the Excel template linked below.\n Lubrication information template for SAP uploading" ;
                  rdfs:label "Lubrication index" ;
                  skos:broadMatch rdl:PCA_100006717 ;
                  skos:broader rdl:PCA_100006748 .


###  http://rds.posccaesar.org/ontology/plm/rdl/PCA_100006302
rdl:PCA_100006302 rdf:type owl:Class ;
                  rdfs:subClassOf rdl:PCA_100004908 ;
                  rdl:PCA_100006763 "This document shall support verification of compliance" ;
                  rdl:PCA_100006766 rdl:PCA_100006653 ;
                  rdl:PCA_100006768 "Provides list of chemicals" ;
                  rdfs:comment "Provides list of chemicals" ;
                  rdfs:label "Lubrication list" ;
                  skos:broadMatch rdl:PCA_100006722 ;
                  skos:broader rdl:PCA_100006748 .


###  http://rds.posccaesar.org/ontology/plm/rdl/PCA_100006303
rdl:PCA_100006303 rdf:type owl:Class ;
                  rdfs:subClassOf rdl:PCA_100004908 ;
                  rdl:PCA_100006763 "The master equipment list shall be prepared for all types of assembled equipment." ;
                  rdl:PCA_100006766 rdl:PCA_100006653 ;
                  rdl:PCA_100006768 "The list should include, but not be limited to, the following information: \n - part number/material number (complete designation) \n - part number/material number (complete designation) \n - part number/material number (complete designation) \n - reference to catalogue and/or data sheets\n - tag number" ;
                  rdfs:comment "The list should include, but not be limited to, the following information: \n - part number/material number (complete designation) \n - part number/material number (complete designation) \n - part number/material number (complete designation) \n - reference to catalogue and/or data sheets\n - tag number" ;
                  rdfs:label "Main equipment list" ;
                  skos:broadMatch rdl:PCA_100006716 ;
                  skos:broader rdl:PCA_100006748 .


###  http://rds.posccaesar.org/ontology/plm/rdl/PCA_100006304
rdl:PCA_100006304 rdf:type owl:Class ;
                  rdfs:subClassOf rdl:PCA_100004908 ;
                  rdl:PCA_100006763 "Ensuring evidence and traceability on construction, manufacturing, testing, reporting and certification for equipment or material." ;
                  rdl:PCA_100006765 rrdl:CFIHOS-20000031 ;
                  rdl:PCA_100006766 rdl:PCA_100006653 ;
                  rdl:PCA_100006768 "A compiled document containing as-built records/documents, signed reports, certificates and drawings." ;
                  rdfs:comment "A compiled document containing as-built records/documents, signed reports, certificates and drawings." ;
                  rdfs:label "Manufacturing and quality control records" ;
                  skos:broadMatch rdl:PCA_100006722 ;
                  skos:broader rdl:PCA_100006756 ,
                               rdl:PCA_100006762 .


###  http://rds.posccaesar.org/ontology/plm/rdl/PCA_100006305
rdl:PCA_100006305 rdf:type owl:Class ;
                  rdfs:subClassOf rdl:PCA_100004908 ;
                  rdl:PCA_100006763 "Provide the manufacturer with information enable them to produce as specified." ;
                  rdl:PCA_100006765 rrdl:CFIHOS-20000031 ;
                  rdl:PCA_100006766 rdl:PCA_100006653 ;
                  rdl:PCA_100006768 "Detailed drawings including manufacturing information such as dimensions, tolerances, materials, sling angles, lifting heights etc." ;
                  rdfs:comment "Detailed drawings including manufacturing information such as dimensions, tolerances, materials, sling angles, lifting heights etc." ;
                  rdfs:label "Manufacturing drawing" ;
                  skos:broadMatch rdl:PCA_100006733 ;
                  skos:broader rdl:PCA_100006746 .


###  http://rds.posccaesar.org/ontology/plm/rdl/PCA_100006306
rdl:PCA_100006306 rdf:type owl:Class ;
                  rdfs:subClassOf rdl:PCA_100004908 ;
                  rdl:PCA_100006763 "Provide clear specification to manufacturer to ensure repeatability." ;
                  rdl:PCA_100006765 rrdl:CFIHOS-20000031 ;
                  rdl:PCA_100006766 rdl:PCA_100006653 ;
                  rdl:PCA_100006768 "Document describing how specified material properties may be achieved and verified through the proposed manufacturing route." ;
                  rdfs:comment "Document describing how specified material properties may be achieved and verified through the proposed manufacturing route." ;
                  rdfs:label "Manufacturing procedure specification (MPS)" ;
                  skos:broadMatch rdl:PCA_100006688 ;
                  skos:broader rdl:PCA_100006757 .


###  http://rds.posccaesar.org/ontology/plm/rdl/PCA_100006307
rdl:PCA_100006307 rdf:type owl:Class ;
                  rdfs:subClassOf rdl:PCA_100004908 ;
                  rdl:PCA_100006763 "A compiled document containing as-built records/documents, signed reports, certificates and drawings." ;
                  rdl:PCA_100006766 rdl:PCA_100006653 ;
                  rdl:PCA_100006768 "Ensuring evidence and traceability on construction, manufacturing, testing, reporting and certification for equipment or material." ;
                  rdfs:comment "Ensuring evidence and traceability on construction, manufacturing, testing, reporting and certification for equipment or material." ;
                  rdfs:label "Manufacturing record book" ;
                  skos:broadMatch rdl:PCA_100006733 ;
                  skos:broader rdl:PCA_100006749 .


###  http://rds.posccaesar.org/ontology/plm/rdl/PCA_100006308
rdl:PCA_100006308 rdf:type owl:Class ;
                  rdfs:subClassOf rdl:PCA_100004908 ;
                  rdl:PCA_100006763 "MRB is a collection of necessary documents to demonstrate that the requirements with respect to design, calculation, production, testing and possible specified traceability requirements for materials and fabrication, are fulfilled.If the documentation normally contained in MRB is issued separately, a reference to such documents is sufficient in the MRB." ;
                  rdl:PCA_100006768 "MRB requirements:\n - The Manufacturers standard MRB can be delivered\n - If additional documents required by Company, they should be submitted as separate \ndeliverables.\n\nAn MRB shall include:\n(depending on the equipment it describes some of the below listed documents may not be \napplicable)\n - Introduction and MRB index\n - List of certificates\n - Analysis, tests, calculations, curves and tables (*)\n - Balancing certificates\n - Calibration certificates\n - Certificates needed for re-certification of equipment\n - Certificates of conformance (*)\n - Documentation for CE marking\n - Final inspection, preservation, packing and dispatch\n - Final test/acceptance reports (FAT reports)\n - Instrument calculations (safety and relief valves) (*)\n - Lifting certificates\n - Manufacturing procedures and reports\n - Material certificates (*)\n - Material testing and control\n - Material traceability list\n - Mechanical/structural calculations and analyses\n - NDE drawings, sketches and other NDE doc.\n - Non-conformance reports\n - Painting procedure\n - Performance / functional test procedures and reports\n - Photos of equipment/inspections\n - PMI report\n - Pressure test certificates\n - Telecommunication test report(s), Vendor reports, MC&C reports\n - Third party verification reports\n - Type Cert.’s/EX Certificates/Product Cert.’s. issued by third party (*)\n - Weight certificates (*)\n - Weld Summary Index and NDE log\n - Welding procedures\n - Welding procedure qualification records (where applicable)\n\n(*) Documents that may be required as separate documents. See chapter 4 for equipment \ntype specific requirements." ;
                  rdfs:comment "MRB requirements:\n - The Manufacturers standard MRB can be delivered\n - If additional documents required by Company, they should be submitted as separate \ndeliverables.\n\nAn MRB shall include:\n(depending on the equipment it describes some of the below listed documents may not be \napplicable)\n - Introduction and MRB index\n - List of certificates\n - Analysis, tests, calculations, curves and tables (*)\n - Balancing certificates\n - Calibration certificates\n - Certificates needed for re-certification of equipment\n - Certificates of conformance (*)\n - Documentation for CE marking\n - Final inspection, preservation, packing and dispatch\n - Final test/acceptance reports (FAT reports)\n - Instrument calculations (safety and relief valves) (*)\n - Lifting certificates\n - Manufacturing procedures and reports\n - Material certificates (*)\n - Material testing and control\n - Material traceability list\n - Mechanical/structural calculations and analyses\n - NDE drawings, sketches and other NDE doc.\n - Non-conformance reports\n - Painting procedure\n - Performance / functional test procedures and reports\n - Photos of equipment/inspections\n - PMI report\n - Pressure test certificates\n - Telecommunication test report(s), Vendor reports, MC&C reports\n - Third party verification reports\n - Type Cert.’s/EX Certificates/Product Cert.’s. issued by third party (*)\n - Weight certificates (*)\n - Weld Summary Index and NDE log\n - Welding procedures\n - Welding procedure qualification records (where applicable)\n\n(*) Documents that may be required as separate documents. See chapter 4 for equipment \ntype specific requirements." ;
                  rdfs:label "Manufacturing record book (MRB)" ;
                  skos:broadMatch rdl:PCA_100006722 ;
                  skos:broader rdl:PCA_100006749 .


###  http://rds.posccaesar.org/ontology/plm/rdl/PCA_100006309
rdl:PCA_100006309 rdf:type owl:Class ;
                  rdfs:subClassOf rdl:PCA_100004908 ;
                  rdl:PCA_100006763 "To demonstrate that the requirements with respect to design, calculation, production, testing and possible specified traceability requirements for materials and fabrication, are fulfilled." ;
                  rdl:PCA_100006765 rrdl:CFIHOS-20000018 ;
                  rdl:PCA_100006766 rdl:PCA_100006654 ;
                  rdl:PCA_100006768 "The MRB for flexible pipelines shall be in accordance with API 17J 4th edition section 8.8 (As-built documentation)." ;
                  rdfs:comment "The MRB for flexible pipelines shall be in accordance with API 17J 4th edition section 8.8 (As-built documentation)." ;
                  rdfs:label "Manufacturing record book (MRB) flexible pipeline and riser" ;
                  skos:broadMatch rdl:PCA_100006722 ;
                  skos:broader rdl:PCA_100006756 ,
                               rdl:PCA_100006762 .


###  http://rds.posccaesar.org/ontology/plm/rdl/PCA_100006310
rdl:PCA_100006310 rdf:type owl:Class ;
                  rdfs:subClassOf rdl:PCA_100004908 ;
                  rdl:PCA_100006763 "To demonstrate that the requirements with respect to design, calculation, production, testing and possible specified traceability requirements for materials and fabrication, are fulfilled." ;
                  rdl:PCA_100006765 rrdl:CFIHOS-20000020 ,
                                    rrdl:CFIHOS-20000031 ;
                  rdl:PCA_100006766 rdl:PCA_100006653 ;
                  rdl:PCA_100006768 "If the documentation normally contained in MRB is issued separately, a reference to such documents is sufficient in the MRB.\n\nMRB requirements:\n - The manufacturer's standard MRB shall be delivered.\n - If additional documents required by Company, then they should be submitted as separate deliverables.\n\n<Please see Word-document for table/akva>\n\nAny of the sections that are not applicable shall be marked “N/A”. The structure and the numbering shall remain as shown above.\n\nNote:\n\nSection 1: The MRB sections shall be delivered as one document (ref SR-15819 - PDF). Each section can be delivered as separate files, named \"Doc. No.-sectionx\"\n(Dxxx-xx-...-section1.pdf, Dxxx-xx-…-section9.xlsx, Dxxx-xx-…-section9.pdf, etc).\n\nSection 4 and 9: Reference to SPTS in the MDR index\n\nSection 3: Shall as a minimum refer to Company requirements contained in latest revision of the following documents:\n - Applicable Frame Agreement and purchase order\n - Applicable Specifications, Project-specific Material Data Sheet (PMDS) and Technical Changes (TC)\n - Reference standard (if specified: DNVGL-ST-F101, including amendments and corrections\n - Applicable SPTS specifications" ;
                  rdfs:comment "If the documentation normally contained in MRB is issued separately, a reference to such documents is sufficient in the MRB.\n\nMRB requirements:\n - The manufacturer's standard MRB shall be delivered.\n - If additional documents required by Company, then they should be submitted as separate deliverables.\n\n<Please see Word-document for table/akva>\n\nAny of the sections that are not applicable shall be marked “N/A”. The structure and the numbering shall remain as shown above.\n\nNote:\n\nSection 1: The MRB sections shall be delivered as one document (ref SR-15819 - PDF). Each section can be delivered as separate files, named \"Doc. No.-sectionx\"\n(Dxxx-xx-...-section1.pdf, Dxxx-xx-…-section9.xlsx, Dxxx-xx-…-section9.pdf, etc).\n\nSection 4 and 9: Reference to SPTS in the MDR index\n\nSection 3: Shall as a minimum refer to Company requirements contained in latest revision of the following documents:\n - Applicable Frame Agreement and purchase order\n - Applicable Specifications, Project-specific Material Data Sheet (PMDS) and Technical Changes (TC)\n - Reference standard (if specified: DNVGL-ST-F101, including amendments and corrections\n - Applicable SPTS specifications" ;
                  rdfs:label "Manufacturing record book (MRB) for linepipe" ;
                  skos:broadMatch rdl:PCA_100006722 ;
                  skos:broader rdl:PCA_100006756 ,
                               rdl:PCA_100006762 .


###  http://rds.posccaesar.org/ontology/plm/rdl/PCA_100006311
rdl:PCA_100006311 rdf:type owl:Class ;
                  rdfs:subClassOf rdl:PCA_100004908 ;
                  rdl:PCA_100006763 "A drawing illustrating necessary marking and labelling of equipment." ;
                  rdl:PCA_100006765 rrdl:CFIHOS-20000031 ;
                  rdl:PCA_100006766 rdl:PCA_100006653 ;
                  rdl:PCA_100006768 "A drawing identifying equipment for operational purposes (e.g. ROV navigation). The information can be covered by the General Arrangement Drawing." ;
                  rdfs:comment "A drawing identifying equipment for operational purposes (e.g. ROV navigation). The information can be covered by the General Arrangement Drawing." ;
                  rdfs:label "Marking drawing" ;
                  skos:broadMatch rdl:PCA_100006732 ;
                  skos:broader rdl:PCA_100006746 .


###  http://rds.posccaesar.org/ontology/plm/rdl/PCA_100006312
rdl:PCA_100006312 rdf:type owl:Class ;
                  rdfs:subClassOf rdl:PCA_100004908 ;
                  rdl:PCA_100006763 "Give a full overview of the equipment in scope." ;
                  rdl:PCA_100006765 rrdl:CFIHOS-20000001 ;
                  rdl:PCA_100006766 rdl:PCA_100006654 ;
                  rdl:PCA_100006768 "List of scope of supply for an contract with identification and quantity (broken down to stand alone equipment)." ;
                  rdfs:comment "List of scope of supply for an contract with identification and quantity (broken down to stand alone equipment)." ;
                  rdfs:label "Master equipment list (MEL)" ;
                  skos:broadMatch rdl:PCA_100006716 ;
                  skos:broader rdl:PCA_100006748 .


###  http://rds.posccaesar.org/ontology/plm/rdl/PCA_100006313
rdl:PCA_100006313 rdf:type owl:Class ;
                  rdfs:subClassOf rdl:PCA_100004908 ;
                  rdl:PCA_100006763 "The objective of Master Grid is to facilitate the availability of trusted spatial information throughout the installation life cycle." ;
                  rdl:PCA_100006766 rdl:PCA_100006656 ;
                  rdl:PCA_100006768 "The Master grid report shall include following information:\n - Master grid ID;\n - Easting;\n - Northing;\n - Elevation;\n - Count (number of measurements for each MG);\n - Root mean square (RMS) error for each MG point.\n\nSecondary Grid data shall be included in the Master Grid report as an attachment." ;
                  rdfs:comment "The Master grid report shall include following information:\n - Master grid ID;\n - Easting;\n - Northing;\n - Elevation;\n - Count (number of measurements for each MG);\n - Root mean square (RMS) error for each MG point.\n\nSecondary Grid data shall be included in the Master Grid report as an attachment." ;
                  rdfs:label "Master grid report" ;
                  skos:broadMatch rdl:PCA_100006705 ;
                  skos:broader rdl:PCA_100006756 .


###  http://rds.posccaesar.org/ontology/plm/rdl/PCA_100006314
rdl:PCA_100006314 rdf:type owl:Class ;
                  rdfs:subClassOf rdl:PCA_100004908 ;
                  rdl:PCA_100006763 "This document shall support verification of compliance." ;
                  rdl:PCA_100006765 rrdl:CFIHOS-20000027 ;
                  rdl:PCA_100006766 rdl:PCA_100006653 ;
                  rdl:PCA_100006768 "This document declares that the material properties for the products supplied are in compliance with the requirements of the purchase order.\n\nFor metallic materials, the material certificate shall be delivered according to ISO 10474 / EN 10204." ;
                  rdfs:comment "This document declares that the material properties for the products supplied are in compliance with the requirements of the purchase order.\n\nFor metallic materials, the material certificate shall be delivered according to ISO 10474 / EN 10204." ;
                  rdfs:label "Material certificate" ;
                  skos:broadMatch rdl:PCA_100006722 ;
                  skos:broader rdl:PCA_100006743 .


###  http://rds.posccaesar.org/ontology/plm/rdl/PCA_100006315
rdl:PCA_100006315 rdf:type owl:Class ;
                  rdfs:subClassOf rdl:PCA_100004908 ;
                  rdl:PCA_100006765 rrdl:CFIHOS-20000020 ;
                  rdl:PCA_100006766 rdl:PCA_100006653 ;
                  rdl:PCA_100006768 "For Offshore facilities, the material handling report which shall contain the following:\n - Description of all material handling equipment, e.g. offshore cranes, personnel and goods lift, forklift truck, trolleys, air film transporters, elephant cranes, A-frames, mobile cranes, etc., including tag numbers (where required), sizes and capacities. \n - Description of standardized sizes of typical lifting beams, pad eyes and lifting equipment, as applicable.\n - Requirements for certification and marking of lifting equipment including foundation and suspension.\n - Description of function, size and location, maximum allowable loads, point loads of lay down and storage areas including areas for the handling of temporary, Company provided and hired equipment., (Laydown area chart).\n - Requirements for transportation routes including maximum allowable loads, point loads, width and height in the different areas. (Transport routes chart).\n - Description and drawings of goods handling to/from helideck.\n - Description of loading hose handling including hose replacement.\n - Description and drawings of areas where special protection of equipment is required e.g. dropped object protection, truck barriers, swinging load protection etc.\n - Description and drawings of handling for all goods to and from the LQ.\n - Table /index containing all tags to be handled with corresponding identification number to the Material Handling Data Sheet.\n\nFor Onshore facilities, the material handling report which shall contain the following:\n - Description of all material handling equipment, e.g. forklift truck, trolleys, air film transporters, elephant cranes, A-frames, mobile cranes etc. including tag numbers, sizes and capacities, storage location, installation method and requirements for certification, marking and re-certification period. \n - Description of function, size and location of lay down and storage.\n - Description of all items above 25 kg (55 lbs.) to be handled, including tag numbers, location, weight, size, type of lifting equipment/ arrangement, lifting/ handling procedure, transport route etc. In cases where the equipment vendor has established thorough handling procedures in the maintenance manual, this can be referred to in the report. The material handling description for such equipment can be reduced to just defining the required lifting/ transportation equipment and transport route. \n - Requirements for transportation ways/roads including width and height in the different areas.\n - Description of areas where special protection of equipment is required e.g. dropped object protection, truck barriers, swinging load protection etc.\n - Material handling drawings based on equipment arrangement drawings or 3D plots including piping and valves containing the following:\n    - All equipment to be handled including lifting lugs, monorails, access ways etc.\n    - Table containing all tags to be handled with corresponding tags for the lifting equipment to be used." ;
                  rdfs:comment "For Offshore facilities, the material handling report which shall contain the following:\n - Description of all material handling equipment, e.g. offshore cranes, personnel and goods lift, forklift truck, trolleys, air film transporters, elephant cranes, A-frames, mobile cranes, etc., including tag numbers (where required), sizes and capacities. \n - Description of standardized sizes of typical lifting beams, pad eyes and lifting equipment, as applicable.\n - Requirements for certification and marking of lifting equipment including foundation and suspension.\n - Description of function, size and location, maximum allowable loads, point loads of lay down and storage areas including areas for the handling of temporary, Company provided and hired equipment., (Laydown area chart).\n - Requirements for transportation routes including maximum allowable loads, point loads, width and height in the different areas. (Transport routes chart).\n - Description and drawings of goods handling to/from helideck.\n - Description of loading hose handling including hose replacement.\n - Description and drawings of areas where special protection of equipment is required e.g. dropped object protection, truck barriers, swinging load protection etc.\n - Description and drawings of handling for all goods to and from the LQ.\n - Table /index containing all tags to be handled with corresponding identification number to the Material Handling Data Sheet.\n\nFor Onshore facilities, the material handling report which shall contain the following:\n - Description of all material handling equipment, e.g. forklift truck, trolleys, air film transporters, elephant cranes, A-frames, mobile cranes etc. including tag numbers, sizes and capacities, storage location, installation method and requirements for certification, marking and re-certification period. \n - Description of function, size and location of lay down and storage.\n - Description of all items above 25 kg (55 lbs.) to be handled, including tag numbers, location, weight, size, type of lifting equipment/ arrangement, lifting/ handling procedure, transport route etc. In cases where the equipment vendor has established thorough handling procedures in the maintenance manual, this can be referred to in the report. The material handling description for such equipment can be reduced to just defining the required lifting/ transportation equipment and transport route. \n - Requirements for transportation ways/roads including width and height in the different areas.\n - Description of areas where special protection of equipment is required e.g. dropped object protection, truck barriers, swinging load protection etc.\n - Material handling drawings based on equipment arrangement drawings or 3D plots including piping and valves containing the following:\n    - All equipment to be handled including lifting lugs, monorails, access ways etc.\n    - Table containing all tags to be handled with corresponding tags for the lifting equipment to be used." ;
                  rdfs:label "Material handling report" ;
                  skos:broadMatch rdl:PCA_100006687 ,
                                  rdl:PCA_100006695 ,
                                  rdl:PCA_100006697 ,
                                  rdl:PCA_100006726 ,
                                  rdl:PCA_100006727 ;
                  skos:broader rdl:PCA_100006756 .


###  http://rds.posccaesar.org/ontology/plm/rdl/PCA_100006316
rdl:PCA_100006316 rdf:type owl:Class ;
                  rdfs:subClassOf rdl:PCA_100004908 ;
                  rdl:PCA_100006763 "Identify materials proposed used and document fluid compatibility for material selected." ;
                  rdl:PCA_100006765 rrdl:CFIHOS-20000031 ;
                  rdl:PCA_100006766 rdl:PCA_100006653 ;
                  rdl:PCA_100006768 "Summarise materials selected for the various components and their compatibility with fluids." ;
                  rdfs:comment "Summarise materials selected for the various components and their compatibility with fluids." ;
                  rdfs:label "Material selection" ;
                  skos:broadMatch rdl:PCA_100006686 ;
                  skos:broader rdl:PCA_100006756 .


###  http://rds.posccaesar.org/ontology/plm/rdl/PCA_100006317
rdl:PCA_100006317 rdf:type owl:Class ;
                  rdfs:subClassOf rdl:PCA_100004908 ;
                  rdl:PCA_100006763 "Summarise materials selected for the various components and their compatibility with fluids." ;
                  rdl:PCA_100006765 rrdl:CFIHOS-20000031 ;
                  rdl:PCA_100006766 rdl:PCA_100006653 ;
                  rdl:PCA_100006768 "Identify materials proposed used and document fluid compatibility for material selected." ;
                  rdfs:comment "Identify materials proposed used and document fluid compatibility for material selected." ;
                  rdfs:label "Material selection report" ;
                  skos:broadMatch rdl:PCA_100006686 ;
                  skos:broader rdl:PCA_100006756 .


###  http://rds.posccaesar.org/ontology/plm/rdl/PCA_100006318
rdl:PCA_100006318 rdf:type owl:Class ;
                  rdfs:subClassOf rdl:PCA_100004908 ;
                  rdl:PCA_100006763 "Give instructions concerning material requirements." ;
                  rdl:PCA_100006765 rrdl:CFIHOS-20000031 ;
                  rdl:PCA_100006766 rdl:PCA_100006653 ;
                  rdl:PCA_100006768 "Document stating requirements for materials, e.g. mechanical properties and NDT." ;
                  rdfs:comment "Document stating requirements for materials, e.g. mechanical properties and NDT." ;
                  rdfs:label "Material specification" ;
                  skos:broadMatch rdl:PCA_100006687 ;
                  skos:broader rdl:PCA_100006757 .


###  http://rds.posccaesar.org/ontology/plm/rdl/PCA_100006319
rdl:PCA_100006319 rdf:type owl:Class ;
                  rdfs:subClassOf rdl:PCA_100004908 ;
                  rdl:PCA_100006763 "Document material traceability for assemblies, components and materials." ;
                  rdl:PCA_100006765 rrdl:CFIHOS-20000031 ;
                  rdl:PCA_100006766 rdl:PCA_100006653 ;
                  rdl:PCA_100006768 "List containing main materials of an assembly with reference to part, serial and batch numbers. List shall contain references to material certificate, heat treatment batch / report and NDT reports where applicable. Mostly used for pressure containing equipment and load bearing elements." ;
                  rdfs:comment "List containing main materials of an assembly with reference to part, serial and batch numbers. List shall contain references to material certificate, heat treatment batch / report and NDT reports where applicable. Mostly used for pressure containing equipment and load bearing elements." ;
                  rdfs:label "Material traceability list" ;
                  skos:broadMatch rdl:PCA_100006715 ;
                  skos:broader rdl:PCA_100006748 .


###  http://rds.posccaesar.org/ontology/plm/rdl/PCA_100006320
rdl:PCA_100006320 rdf:type owl:Class ;
                  rdfs:subClassOf rdl:PCA_100004908 ;
                  rdl:PCA_100006763 "Provide instructions for preparation of the material traceability list." ;
                  rdl:PCA_100006765 rrdl:CFIHOS-20000031 ;
                  rdl:PCA_100006766 rdl:PCA_100006653 ;
                  rdl:PCA_100006768 "Procedure describing the requirements for material traceability for different components and equipment." ;
                  rdfs:comment "Procedure describing the requirements for material traceability for different components and equipment." ;
                  rdfs:label "Material traceability procedure" ;
                  skos:broadMatch rdl:PCA_100006688 ;
                  skos:broader rdl:PCA_100006751 .


###  http://rds.posccaesar.org/ontology/plm/rdl/PCA_100006321
rdl:PCA_100006321 rdf:type owl:Class ;
                  rdfs:subClassOf rdl:PCA_100004908 ;
                  rdl:PCA_100006763 "Summarise materials selected for the various components and their compatibility with fluids. List containing main materials of an assembly with reference to part, serial and batch numbers. List shall contain references to material certificate, heat treatment batch / report and NDT reports where applicable. Mostly used for pressure containing equipment and load bearing elements." ;
                  rdl:PCA_100006765 rrdl:CFIHOS-20000027 ;
                  rdl:PCA_100006766 rdl:PCA_100006653 ;
                  rdl:PCA_100006768 "Identify materials proposed used and document fluid compatibility for material selected." ;
                  rdfs:comment "Identify materials proposed used and document fluid compatibility for material selected." ;
                  rdfs:label "Material traceability report" ;
                  skos:broadMatch rdl:PCA_100006715 ,
                                  rdl:PCA_100006716 ;
                  skos:broader rdl:PCA_100006756 .


###  http://rds.posccaesar.org/ontology/plm/rdl/PCA_100006322
rdl:PCA_100006322 rdf:type owl:Class ;
                  rdfs:subClassOf rdl:PCA_100004908 ;
                  rdl:PCA_100006768 "A circuit distribution schedule shall be provided inside each panel. This schedule shall include both circuits for internal control voltage and circuits for external consumers." ;
                  rdfs:comment "A circuit distribution schedule shall be provided inside each panel. This schedule shall include both circuits for internal control voltage and circuits for external consumers." ;
                  rdfs:label "MCB/fuse schedule" ;
                  skos:broadMatch rdl:PCA_100006702 ,
                                  rdl:PCA_100006716 ;
                  skos:broader rdl:PCA_100006748 .


###  http://rds.posccaesar.org/ontology/plm/rdl/PCA_100006323
rdl:PCA_100006323 rdf:type owl:Class ;
                  rdfs:subClassOf rdl:PCA_100004908 ;
                  rdl:PCA_100006763 "To verify that the products and components have been manufactured in accordance with drawings, procedures and specifications." ;
                  rdl:PCA_100006765 rrdl:CFIHOS-20000031 ;
                  rdl:PCA_100006766 rdl:PCA_100006653 ;
                  rdl:PCA_100006768 "Final inspection check list for products and components with signature fields for Supplier, customer and third party, and list of all applicable punch items." ;
                  rdfs:comment "Final inspection check list for products and components with signature fields for Supplier, customer and third party, and list of all applicable punch items." ;
                  rdfs:label "MCCR - mechanical completion check record" ;
                  skos:broadMatch rdl:PCA_100006722 ;
                  skos:broader rdl:PCA_100006756 .


###  http://rds.posccaesar.org/ontology/plm/rdl/PCA_100006324
rdl:PCA_100006324 rdf:type owl:Class ;
                  rdfs:subClassOf rdl:PCA_100004908 ;
                  rdl:PCA_100006763 "To verify that the products and components have been manufactured in accordance with drawings, procedures and specifications." ;
                  rdl:PCA_100006765 rrdl:CFIHOS-20000023 ;
                  rdl:PCA_100006766 rdl:PCA_100006653 ;
                  rdl:PCA_100006768 "Final inspection check list for products and components with signature fields for Supplier, customer and third party, and list of all applicable punch items." ;
                  rdfs:comment "Final inspection check list for products and components with signature fields for Supplier, customer and third party, and list of all applicable punch items." ;
                  rdfs:label "Mechanical completion check record (MCCR) / software check record (SWCR) dossier" ;
                  skos:broadMatch rdl:PCA_100006722 ;
                  skos:broader rdl:PCA_100006748 .


###  http://rds.posccaesar.org/ontology/plm/rdl/PCA_100006325
rdl:PCA_100006325 rdf:type owl:Class ;
                  rdfs:subClassOf rdl:PCA_100004908 ;
                  rdl:PCA_100006763 "The reports shall comply with requirements in: \nWMO 1995 Technical regulation manual on codes, Vol I.1, WMO No. 306 Genova;\nISO 19901-1 Petroleum and natural gas industries – Specific requirements for offshore structures – Part 1: Metocean design and operating considerations." ;
                  rdl:PCA_100006765 rrdl:CFIHOS-20000007 ;
                  rdl:PCA_100006766 rdl:PCA_100006656 ;
                  rdfs:label "Metocean - meterological and oceanographical reports" ;
                  skos:broadMatch rdl:PCA_100006691 ,
                                  rdl:PCA_100006698 ;
                  skos:broader rdl:PCA_100006756 .


###  http://rds.posccaesar.org/ontology/plm/rdl/PCA_100006326
rdl:PCA_100006326 rdf:type owl:Class ;
                  rdfs:subClassOf rdl:PCA_100004908 ;
                  rdl:PCA_100006763 "The report or collection of reports shall document the model test and describe the results of the testing." ;
                  rdl:PCA_100006765 rrdl:CFIHOS-20000033 ;
                  rdl:PCA_100006766 rdl:PCA_100006657 ;
                  rdl:PCA_100006768 "Model test report shall be delivered." ;
                  rdfs:comment "Model test report shall be delivered." ;
                  rdfs:label "Model test reports" ;
                  skos:broadMatch rdl:PCA_100006722 ;
                  skos:broader rdl:PCA_100006756 .


###  http://rds.posccaesar.org/ontology/plm/rdl/PCA_100006327
rdl:PCA_100006327 rdf:type owl:Class ;
                  rdfs:subClassOf rdl:PCA_100004908 ;
                  rdl:PCA_100006765 rrdl:CFIHOS-20000033 ;
                  rdl:PCA_100006766 rdl:PCA_100006647 ;
                  rdl:PCA_100006768 "A complete mooring analysis model shall be delivered in native format. The model shall be delivered with all necessary information required to perform a re-analysis." ;
                  rdfs:comment "A complete mooring analysis model shall be delivered in native format. The model shall be delivered with all necessary information required to perform a re-analysis." ;
                  rdfs:label "Mooring analysis model" ;
                  skos:broadMatch rdl:PCA_100006687 ;
                  skos:broader rdl:PCA_100006741 ,
                               rdl:PCA_100006762 .


###  http://rds.posccaesar.org/ontology/plm/rdl/PCA_100006328
rdl:PCA_100006328 rdf:type owl:Class ;
                  rdfs:subClassOf rdl:PCA_100004908 ;
                  rdl:PCA_100006763 "Mooring analysis reports shall be delivered. The report or collection of reports shall contain the final documentation of the mooring system." ;
                  rdl:PCA_100006765 rrdl:CFIHOS-20000033 ;
                  rdl:PCA_100006766 rdl:PCA_100006647 ;
                  rdl:PCA_100006768 "The report shall typically contain:\n - Design basis including rules and regulations, design life, location, water depth, environmental conditions, corrosion allowance and marine growth;\n - Design criteria including safety factors, offset requirements and fatigue;\n - Vessel particulars;\n - Design method and input parameters;\n - Analysis results;\n - Description for final mooring system layout and components." ;
                  rdfs:comment "The report shall typically contain:\n - Design basis including rules and regulations, design life, location, water depth, environmental conditions, corrosion allowance and marine growth;\n - Design criteria including safety factors, offset requirements and fatigue;\n - Vessel particulars;\n - Design method and input parameters;\n - Analysis results;\n - Description for final mooring system layout and components." ;
                  rdfs:label "Mooring analysis reports" ;
                  skos:broadMatch rdl:PCA_100006687 ;
                  skos:broader rdl:PCA_100006756 .


###  http://rds.posccaesar.org/ontology/plm/rdl/PCA_100006329
rdl:PCA_100006329 rdf:type owl:Class ;
                  rdfs:subClassOf rdl:PCA_100004908 ;
                  rdl:PCA_100006765 rrdl:CFIHOS-20000033 ;
                  rdl:PCA_100006766 rdl:PCA_100006647 ;
                  rdl:PCA_100006768 "Mooring component certificates and fabrication documentation collection report shall be delivered. All certificates and other relevant documentation issued during manufacturing of mooring components shall be organised in a logical manner (including welding filler material) along with traceability data." ;
                  rdfs:comment "Mooring component certificates and fabrication documentation collection report shall be delivered. All certificates and other relevant documentation issued during manufacturing of mooring components shall be organised in a logical manner (including welding filler material) along with traceability data." ;
                  rdfs:label "Mooring component certificate and fabrication documentation" ;
                  skos:broadMatch rdl:PCA_100006722 ;
                  skos:broader rdl:PCA_100006743 .


###  http://rds.posccaesar.org/ontology/plm/rdl/PCA_100006330
rdl:PCA_100006330 rdf:type owl:Class ;
                  rdfs:subClassOf rdl:PCA_100004908 ;
                  rdl:PCA_100006763 "The collection of reports and drawings shall provide information on mooring system layout and component design." ;
                  rdl:PCA_100006765 rrdl:CFIHOS-20000033 ;
                  rdl:PCA_100006766 rdl:PCA_100006647 ;
                  rdl:PCA_100006768 "The report shall contain a complete description of the entire mooring system: \n - Arrangement drawings;\n - Component drawings;\n - Design analyses of all mooring components from onboard systems to anchors." ;
                  rdfs:comment "The report shall contain a complete description of the entire mooring system: \n - Arrangement drawings;\n - Component drawings;\n - Design analyses of all mooring components from onboard systems to anchors." ;
                  rdfs:label "Mooring system design" ;
                  skos:broadMatch rdl:PCA_100006698 ,
                                  rdl:PCA_100006708 ,
                                  rdl:PCA_100006732 ;
                  skos:broader rdl:PCA_100006756 .


###  http://rds.posccaesar.org/ontology/plm/rdl/PCA_100006331
rdl:PCA_100006331 rdf:type owl:Class ;
                  rdfs:subClassOf rdl:PCA_100004908 ;
                  rdl:PCA_100006765 rrdl:CFIHOS-20000033 ;
                  rdl:PCA_100006766 rdl:PCA_100006647 ;
                  rdl:PCA_100006768 "Mooring systems procedures shall be delivered. The report or collection of reports shall contain all procedures necessary to safely operate, maintain and replace any component of the mooring system." ;
                  rdfs:comment "Mooring systems procedures shall be delivered. The report or collection of reports shall contain all procedures necessary to safely operate, maintain and replace any component of the mooring system." ;
                  rdfs:label "Mooring system procedures" ;
                  skos:broadMatch rdl:PCA_100006688 ;
                  skos:broader rdl:PCA_100006751 .


###  http://rds.posccaesar.org/ontology/plm/rdl/PCA_100006332
rdl:PCA_100006332 rdf:type owl:Class ;
                  rdfs:subClassOf rdl:PCA_100004908 ;
                  rdl:PCA_100006765 rrdl:CFIHOS-20000033 ;
                  rdl:PCA_100006766 rdl:PCA_100006647 ;
                  rdl:PCA_100006768 "A complete motion analyses model shall be delivered with all necessary information required to perform a re-analysis." ;
                  rdfs:comment "A complete motion analyses model shall be delivered with all necessary information required to perform a re-analysis." ;
                  rdfs:label "Motion analysis model" ;
                  skos:broadMatch rdl:PCA_100006687 ;
                  skos:broader rdl:PCA_100006741 ,
                               rdl:PCA_100006762 .


###  http://rds.posccaesar.org/ontology/plm/rdl/PCA_100006333
rdl:PCA_100006333 rdf:type owl:Class ;
                  rdfs:subClassOf rdl:PCA_100004908 ;
                  rdl:PCA_100006765 rrdl:CFIHOS-20000033 ;
                  rdl:PCA_100006766 rdl:PCA_100006647 ;
                  rdl:PCA_100006768 "Motion design reports shall be delivered. The report or collection of reports shall contain the final documentation of:\n - Dimensioning environmental conditions;\n - Vessel response characteristics;\n - Extreme motion response;\n - Dimensioning accelerations;\n - Air gap / slamming / green sea analyses;\n - Model test verification analyses." ;
                  rdfs:comment "Motion design reports shall be delivered. The report or collection of reports shall contain the final documentation of:\n - Dimensioning environmental conditions;\n - Vessel response characteristics;\n - Extreme motion response;\n - Dimensioning accelerations;\n - Air gap / slamming / green sea analyses;\n - Model test verification analyses." ;
                  rdfs:label "Motion design reports" ;
                  skos:broadMatch rdl:PCA_100006691 ,
                                  rdl:PCA_100006698 ;
                  skos:broader rdl:PCA_100006756 .


###  http://rds.posccaesar.org/ontology/plm/rdl/PCA_100006334
rdl:PCA_100006334 rdf:type owl:Class ;
                  rdfs:subClassOf rdl:PCA_100004908 ;
                  rdl:PCA_100006763 "Document that the NDT operator has the necessary qualifications for the relevant NDT method." ;
                  rdl:PCA_100006765 rrdl:CFIHOS-20000031 ;
                  rdl:PCA_100006766 rdl:PCA_100006653 ;
                  rdl:PCA_100006768 "Official certificates for operators performing NDT. NDT certificates are issued per method in e.g. UT, MT, PT, RT, ET and VT at three different levels." ;
                  rdfs:comment "Official certificates for operators performing NDT. NDT certificates are issued per method in e.g. UT, MT, PT, RT, ET and VT at three different levels." ;
                  rdfs:label "NDT operator certificates" ;
                  skos:broadMatch rdl:PCA_100006722 ;
                  skos:broader rdl:PCA_100006743 .


###  http://rds.posccaesar.org/ontology/plm/rdl/PCA_100006335
rdl:PCA_100006335 rdf:type owl:Class ;
                  rdfs:subClassOf rdl:PCA_100004908 ;
                  rdl:PCA_100006763 "Provide clear procedure to NDT operator to ensure repeatability." ;
                  rdl:PCA_100006765 rrdl:CFIHOS-20000031 ;
                  rdl:PCA_100006766 rdl:PCA_100006653 ;
                  rdl:PCA_100006768 "Document describing how to perform NDT (i.e. MT, PT, RT, UT, VT or ET) for a given object, including acceptance criteria and reporting." ;
                  rdfs:comment "Document describing how to perform NDT (i.e. MT, PT, RT, UT, VT or ET) for a given object, including acceptance criteria and reporting." ;
                  rdfs:label "NDT procedures" ;
                  skos:broadMatch rdl:PCA_100006688 ;
                  skos:broader rdl:PCA_100006751 .


###  http://rds.posccaesar.org/ontology/plm/rdl/PCA_100006336
rdl:PCA_100006336 rdf:type owl:Class ;
                  rdfs:subClassOf rdl:PCA_100004908 ;
                  rdl:PCA_100006763 "To document that the NDT performed meets specified requirements." ;
                  rdl:PCA_100006765 rrdl:CFIHOS-20000031 ;
                  rdl:PCA_100006766 rdl:PCA_100006653 ;
                  rdl:PCA_100006768 "Documents containing records of performed NDT (in typical NDT methodse.g. MT, PT, RT, UT, ET and VT)." ;
                  rdfs:comment "Documents containing records of performed NDT (in typical NDT methodse.g. MT, PT, RT, UT, ET and VT)." ;
                  rdfs:label "NDT reports" ;
                  skos:broadMatch rdl:PCA_100006722 ;
                  skos:broader rdl:PCA_100006755 .


###  http://rds.posccaesar.org/ontology/plm/rdl/PCA_100006337
rdl:PCA_100006337 rdf:type owl:Class ;
                  rdfs:subClassOf rdl:PCA_100004908 ;
                  rdl:PCA_100006763 "Overall network topology shall show topology of technical network and subnetwork to give a functional understanding and a foundation for a risk and vulnerability analysis." ;
                  rdl:PCA_100006765 rrdl:CFIHOS-20000015 ;
                  rdl:PCA_100006766 rdl:PCA_100006626 ,
                                    rdl:PCA_100006633 ,
                                    rdl:PCA_100006634 ,
                                    rdl:PCA_100006635 ,
                                    rdl:PCA_100006636 ,
                                    rdl:PCA_100006637 ;
                  rdl:PCA_100006768 "Typical contents shall be:\n - Related servers, switches, routers, firewalls and computers represented by a relevant symbol, marked with its identification and description of function;\n - Location of the equipment identifying the zone for the system;\n - Communication between units shall be indicated, also wireless interfaces;\n - Reference to information concerning IP/MAC addresses (restricted information);\n - Reference to information concerning firewall rules (restricted information);\n - Signal type, protocol and function (typ. RS232, control signal) if applicable;\n - Colour coding to indicate criticality level of the system.\n\nFor smaller technical networks the information from the subsystem block diagram can be integrated in the overall system topology, provided the readability of the drawing are maintained." ;
                  rdfs:comment "Typical contents shall be:\n - Related servers, switches, routers, firewalls and computers represented by a relevant symbol, marked with its identification and description of function;\n - Location of the equipment identifying the zone for the system;\n - Communication between units shall be indicated, also wireless interfaces;\n - Reference to information concerning IP/MAC addresses (restricted information);\n - Reference to information concerning firewall rules (restricted information);\n - Signal type, protocol and function (typ. RS232, control signal) if applicable;\n - Colour coding to indicate criticality level of the system.\n\nFor smaller technical networks the information from the subsystem block diagram can be integrated in the overall system topology, provided the readability of the drawing are maintained." ;
                  rdfs:label "Network topology diagram" ;
                  skos:broadMatch rdl:PCA_100006695 ;
                  skos:broader rdl:PCA_100006745 .


###  http://rds.posccaesar.org/ontology/plm/rdl/PCA_100006338
rdl:PCA_100006338 rdf:type owl:Class ;
                  rdfs:subClassOf rdl:PCA_100004908 ;
                  rdl:PCA_100006765 rrdl:CFIHOS-20000008 ;
                  rdl:PCA_100006766 rdl:PCA_100006656 ;
                  rdl:PCA_100006768 "Isometric non scaled view of routing of cable ladders including penetration transits and jumps shall be provided.  Following information shall typically be included:\n - Node number;\n - Segment name;\n - Length of segment;\n - Location/module number;\n - Cable segregation level;\n - Penetration identification;\n - References to other drawings where the cable ladder continued." ;
                  rdfs:comment "Isometric non scaled view of routing of cable ladders including penetration transits and jumps shall be provided.  Following information shall typically be included:\n - Node number;\n - Segment name;\n - Length of segment;\n - Location/module number;\n - Cable segregation level;\n - Penetration identification;\n - References to other drawings where the cable ladder continued." ;
                  rdfs:label "Nodal diagrams" ;
                  skos:broadMatch rdl:PCA_100006708 ;
                  skos:broader rdl:PCA_100006745 .


###  http://rds.posccaesar.org/ontology/plm/rdl/PCA_100006339
rdl:PCA_100006339 rdf:type owl:Class ;
                  rdfs:subClassOf rdl:PCA_100004908 ;
                  rdl:PCA_100006763 "Document providing information about noise levels." ;
                  rdl:PCA_100006766 rdl:PCA_100006653 ;
                  rdl:PCA_100006768 "Noise and vibration data shall be delivered according to NORSOK S-002.\n\nThe datasheet shall as a minimum contain the information specified in the applicable datasheet template." ;
                  rdfs:comment "Noise and vibration data shall be delivered according to NORSOK S-002.\n\nThe datasheet shall as a minimum contain the information specified in the applicable datasheet template." ;
                  rdfs:label "Noise data sheet" ;
                  skos:broadMatch rdl:PCA_100006686 ;
                  skos:broader rdl:PCA_100006747 .


###  http://rds.posccaesar.org/ontology/plm/rdl/PCA_100006340
rdl:PCA_100006340 rdf:type owl:Class ;
                  rdfs:subClassOf rdl:PCA_100004908 ;
                  rdl:PCA_100006763 "To document deviations and clarify technical issues." ;
                  rdl:PCA_100006765 rrdl:CFIHOS-20000031 ;
                  rdl:PCA_100006766 rdl:PCA_100006653 ;
                  rdl:PCA_100006768 "Report stating a deviation from standards and/or specifications, and issue of technical queries." ;
                  rdfs:comment "Report stating a deviation from standards and/or specifications, and issue of technical queries." ;
                  rdfs:label "Non-conformance / concession reports / technical queries" ;
                  skos:broadMatch rdl:PCA_100006724 .


###  http://rds.posccaesar.org/ontology/plm/rdl/PCA_100006341
rdl:PCA_100006341 rdf:type owl:Class ;
                  rdfs:subClassOf rdl:PCA_100004908 ;
                  rdl:PCA_100006763 "This document shall  document deviations from standards and/or specifications, and issue of\ntechnical queries." ;
                  rdl:PCA_100006765 rrdl:CFIHOS-20000027 ;
                  rdl:PCA_100006766 rdl:PCA_100006653 ;
                  rdl:PCA_100006768 "This document shall contain a list stating all deviations from the requirements in the inquiry, and proposed alternative requirements." ;
                  rdfs:comment "This document shall contain a list stating all deviations from the requirements in the inquiry, and proposed alternative requirements." ;
                  rdfs:label "Non-conformity report" ;
                  skos:broadMatch rdl:PCA_100006724 ;
                  skos:broader rdl:PCA_100006756 .


###  http://rds.posccaesar.org/ontology/plm/rdl/PCA_100006342
rdl:PCA_100006342 rdf:type owl:Class ;
                  rdfs:subClassOf rdl:PCA_100004908 ;
                  rdl:PCA_100006763 "This document is a part of the Quality Assurance Plan, and herein the Quality Assurance work process and verification.\nThis document provides a procedure for NDT operator to ensure repeatability and formalism and hence prove the quality of the NDT work." ;
                  rdl:PCA_100006765 rrdl:CFIHOS-20000028 ;
                  rdl:PCA_100006766 rdl:PCA_100006653 ;
                  rdl:PCA_100006768 "Document describing how to perform NDT (i.e. MT, PT, RT, UT, VT or ET) for a given object, including acceptance criteria and reporting." ;
                  rdfs:comment "Document describing how to perform NDT (i.e. MT, PT, RT, UT, VT or ET) for a given object, including acceptance criteria and reporting." ;
                  rdfs:label "Non-destructive examination (NDE) procedure" ;
                  skos:broadMatch rdl:PCA_100006672 ,
                                  rdl:PCA_100006722 ;
                  skos:broader rdl:PCA_100006751 .


###  http://rds.posccaesar.org/ontology/plm/rdl/PCA_100006343
rdl:PCA_100006343 rdf:type owl:Class ;
                  rdfs:subClassOf rdl:PCA_100004908 ;
                  rdl:PCA_100006763 "A document containing data which records compliance with specified procedure." ;
                  rdl:PCA_100006765 rrdl:CFIHOS-20000028 ;
                  rdl:PCA_100006766 rdl:PCA_100006653 ;
                  rdl:PCA_100006768 "Documents containing records of performed NDT (in typical NDT methods e.g. MT, PT, RT, UT, ET and VT)." ;
                  rdfs:comment "Documents containing records of performed NDT (in typical NDT methods e.g. MT, PT, RT, UT, ET and VT)." ;
                  rdfs:label "Non-destructive examination (NDE) report" ;
                  skos:broadMatch rdl:PCA_100006722 ;
                  skos:broader rdl:PCA_100006756 .


###  http://rds.posccaesar.org/ontology/plm/rdl/PCA_100006344
rdl:PCA_100006344 rdf:type owl:Class ;
                  rdfs:subClassOf rdl:PCA_100004908 ;
                  rdl:PCA_100006763 "Subsea equipment Supplier shall provide an Obsolescence Management Plan describing the strategies for identification and mitigation of the effects of obsolescence through all stages of the life of the product. This document shall be maintained throughout the product lifecycle." ;
                  rdfs:label "Obsolescence management plan" ;
                  skos:broader rdl:PCA_100006753 .


###  http://rds.posccaesar.org/ontology/plm/rdl/PCA_100006345
rdl:PCA_100006345 rdf:type owl:Class ;
                  rdfs:subClassOf rdl:PCA_100004908 ;
                  rdl:PCA_100006763 "The report or collection of reports shall contain a complete description of the offloading arrangement." ;
                  rdl:PCA_100006765 rrdl:CFIHOS-20000033 ;
                  rdl:PCA_100006766 rdl:PCA_100006603 ;
                  rdl:PCA_100006768 "The report shall typically contain:\n - Overall description of the functionality of the offloading system;\n - Design analyses and drawings of the offloading system;\n - Overall description of hose maintenance and replacement method." ;
                  rdfs:comment "The report shall typically contain:\n - Overall description of the functionality of the offloading system;\n - Design analyses and drawings of the offloading system;\n - Overall description of hose maintenance and replacement method." ;
                  rdfs:label "Offloading system arrangement report" ;
                  skos:broadMatch rdl:PCA_100006687 ;
                  skos:broader rdl:PCA_100006756 .


###  http://rds.posccaesar.org/ontology/plm/rdl/PCA_100006346
rdl:PCA_100006346 rdf:type owl:Class ;
                  rdfs:subClassOf rdl:PCA_100004908 ;
                  rdl:PCA_100006765 rrdl:CFIHOS-20000018 ;
                  rdl:PCA_100006766 rdl:PCA_100006657 ;
                  rdl:PCA_100006768 "including PVT file updated with as laid pipeline profile to DG4." ;
                  rdfs:comment "including PVT file updated with as laid pipeline profile to DG4." ;
                  rdfs:label "OLGA as laid models" ;
                  skos:broadMatch rdl:PCA_100006731 .


###  http://rds.posccaesar.org/ontology/plm/rdl/PCA_100006347
rdl:PCA_100006347 rdf:type owl:Class ;
                  rdfs:subClassOf rdl:PCA_100004908 ;
                  rdl:PCA_100006763 "To document that the pipeline, riser or umbilical will be stable on the sea bottom during all conditions." ;
                  rdl:PCA_100006765 rrdl:CFIHOS-20000018 ;
                  rdl:PCA_100006766 rdl:PCA_100006657 ;
                  rdl:PCA_100006768 "Report documenting all calculations and analysis performed to prove pipeline, riser or umbilical on bottom stability design." ;
                  rdfs:comment "Report documenting all calculations and analysis performed to prove pipeline, riser or umbilical on bottom stability design." ;
                  rdfs:label "On-bottom stability report" ;
                  skos:broadMatch rdl:PCA_100006687 ;
                  skos:broader rdl:PCA_100006756 .


###  http://rds.posccaesar.org/ontology/plm/rdl/PCA_100006348
rdl:PCA_100006348 rdf:type owl:Class ;
                  rdfs:subClassOf rdl:PCA_100004908 ;
                  rdl:PCA_100006763 "To describe how to operate and maintain the equipment in a safe and functionally correct manner according to the specified maintenance philosophy." ;
                  rdl:PCA_100006765 rrdl:CFIHOS-20000031 ;
                  rdl:PCA_100006766 rdl:PCA_100006653 ;
                  rdl:PCA_100006768 "A compiled document providing sufficient information to operate, maintain and preserve the equipment." ;
                  rdfs:comment "A compiled document providing sufficient information to operate, maintain and preserve the equipment." ;
                  rdfs:label "Operation and maintenance manual (OMM)" ;
                  skos:broadMatch rdl:PCA_100006688 ;
                  skos:broader rdl:PCA_100006751 .


###  http://rds.posccaesar.org/ontology/plm/rdl/PCA_100006349
rdl:PCA_100006349 rdf:type owl:Class ;
                  rdfs:subClassOf rdl:PCA_100004908 ;
                  rdl:PCA_100006763 "Ensure safe operation" ;
                  rdl:PCA_100006765 rrdl:CFIHOS-20000018 ;
                  rdl:PCA_100006766 rdl:PCA_100006654 ;
                  rdl:PCA_100006768 "Content shall be according to Section 8.9 in API 17J, and the following additional requirements:\n - Values for operational parameter critical for service life including operational pressure and temperatures with description of effect if exceeding these values.\n - Drawings of riser configuration from topside hang-off to the seabed connection to interface structure identifying section lengths, ancillary components, characteristic water depths for the configuration including identification of values for normal operation maximum/minimum density, maximum and minimum offset and temporary water filled condition.\n - List of situations that could be potentially detrimental to the flexible pipe including plan of action for such situations." ;
                  rdfs:comment "Content shall be according to Section 8.9 in API 17J, and the following additional requirements:\n - Values for operational parameter critical for service life including operational pressure and temperatures with description of effect if exceeding these values.\n - Drawings of riser configuration from topside hang-off to the seabed connection to interface structure identifying section lengths, ancillary components, characteristic water depths for the configuration including identification of values for normal operation maximum/minimum density, maximum and minimum offset and temporary water filled condition.\n - List of situations that could be potentially detrimental to the flexible pipe including plan of action for such situations." ;
                  rdfs:label "Operation manual flexible pipeline and riser" ;
                  skos:broadMatch rdl:PCA_100006688 ;
                  skos:broader rdl:PCA_100006751 .


###  http://rds.posccaesar.org/ontology/plm/rdl/PCA_100006350
rdl:PCA_100006350 rdf:type owl:Class ;
                  rdfs:subClassOf rdl:PCA_100004908 ;
                  rdl:PCA_100006765 rrdl:CFIHOS-20000018 ;
                  rdl:PCA_100006766 rdl:PCA_100006657 ;
                  rdl:PCA_100006768 "This procedure shall as a minimum address the following aspects: \n - System description.\n - Operating envelope.\n - Pigging.\n - Start-up procedure.\n - Routine operations.\n - De-pressurising." ;
                  rdfs:comment "This procedure shall as a minimum address the following aspects: \n - System description.\n - Operating envelope.\n - Pigging.\n - Start-up procedure.\n - Routine operations.\n - De-pressurising." ;
                  rdfs:label "Operational procedure for a lined pipeline" ;
                  skos:broadMatch rdl:PCA_100006688 ;
                  skos:broader rdl:PCA_100006751 .


###  http://rds.posccaesar.org/ontology/plm/rdl/PCA_100006351
rdl:PCA_100006351 rdf:type owl:Class ;
                  rdfs:subClassOf rdl:PCA_100004908 ;
                  rdl:PCA_100006763 "Outline procedure for the pre-commission activities and schedule." ;
                  rdl:PCA_100006765 rrdl:CFIHOS-20000031 ;
                  rdl:PCA_100006766 rdl:PCA_100006657 ;
                  rdl:PCA_100006768 "Input to design basis for pipeline and risers design and installation methodology." ;
                  rdfs:comment "Input to design basis for pipeline and risers design and installation methodology." ;
                  rdfs:label "Outline precommissioning procedure" ;
                  skos:broadMatch rdl:PCA_100006688 ;
                  skos:broader rdl:PCA_100006751 .


###  http://rds.posccaesar.org/ontology/plm/rdl/PCA_100006352
rdl:PCA_100006352 rdf:type owl:Class ;
                  rdfs:subClassOf rdl:PCA_100004908 ;
                  rdl:PCA_100006763 "The diagrams shall include all power distribution units (generators, eventual external grid, switchgears, transformers, distribution boards, rectifiers, batteries etc.) throughout the distribution system. End consumers shall be included for high voltage consumers. Only generators, transformers, switchgears, main distribution boards shall be shown on the low voltage level.\n\nSeparate single line diagrams shall be prepared showing UPSs including main and sub distribution boards as well as lighting and small power, typical 400/230 V system.\n\nSeparate earthing overall single line diagrams, including all main equipment, shall be provided for the electrical, instrument and telecommunication installations. The general earthing principles shall be included to ensure correct earthing of systems, equipment and cables." ;
                  rdl:PCA_100006765 rrdl:CFIHOS-20000008 ;
                  rdl:PCA_100006766 rdl:PCA_100006634 ,
                                    rdl:PCA_100006635 ,
                                    rdl:PCA_100006636 ,
                                    rdl:PCA_100006637 ,
                                    rdl:PCA_100006638 ,
                                    rdl:PCA_100006639 ;
                  rdl:PCA_100006768 "This single diagram shall typically include:\n - Main earth bars for electrical, instrument and telecommunications;\n - Earthing electrode;\n - Lightning system;\n - Earthing of electrical main equipment as switchboards, transformers and generators. System earthing shall be included." ;
                  rdfs:comment "This single diagram shall typically include:\n - Main earth bars for electrical, instrument and telecommunications;\n - Earthing electrode;\n - Lightning system;\n - Earthing of electrical main equipment as switchboards, transformers and generators. System earthing shall be included." ;
                  rdfs:label "Overall single line diagram" ;
                  skos:broadMatch rdl:PCA_100006702 ;
                  skos:broader rdl:PCA_100006745 .


###  http://rds.posccaesar.org/ontology/plm/rdl/PCA_100006353
rdl:PCA_100006353 rdf:type owl:Class ;
                  rdfs:subClassOf rdl:PCA_100004908 ;
                  rdl:PCA_100006763 "Overview of all permanent installation used for construction and installation along the pipeline, such as, but not limited to turn point and foundation for winches." ;
                  rdl:PCA_100006765 rrdl:CFIHOS-20000018 ;
                  rdl:PCA_100006766 rdl:PCA_100006654 ;
                  rdl:PCA_100006768 "Info to be recorded in the  As-Built revision of the Field Layout (GIS database)" ;
                  rdfs:comment "Info to be recorded in the  As-Built revision of the Field Layout (GIS database)" ;
                  rdfs:label "Overview of permanent auxiliary installations" ;
                  skos:broadMatch rdl:PCA_100006705 ,
                                  rdl:PCA_100006731 ;
                  skos:broader rdl:PCA_100006746 .


###  http://rds.posccaesar.org/ontology/plm/rdl/PCA_100006354
rdl:PCA_100006354 rdf:type owl:Class ;
                  rdfs:subClassOf rdl:PCA_100004908 ;
                  rdl:PCA_100006763 "This document shall provide requirements for storage, transport, lifting and preservation to maintain functionality and guarantees." ;
                  rdl:PCA_100006765 rrdl:CFIHOS-20000029 ;
                  rdl:PCA_100006766 rdl:PCA_100006653 ;
                  rdl:PCA_100006768 "A compound document that may contain: \n - Packing lists\n - Instructions for transport\n - Handling\n - Lifting\n - Storage location and requirements\n - Preservation of the equipment during short- and long term storage\n - Maintenance intervals\n - Inspection intervals\n - Instructions for unpacking if applicable\n - Completed applicable forms for mechanical completion\n - Certificate of conformity, data sheets\n - Preservation log\n - Certificate for lifting equipment\n - Material certificates" ;
                  rdfs:comment "A compound document that may contain: \n - Packing lists\n - Instructions for transport\n - Handling\n - Lifting\n - Storage location and requirements\n - Preservation of the equipment during short- and long term storage\n - Maintenance intervals\n - Inspection intervals\n - Instructions for unpacking if applicable\n - Completed applicable forms for mechanical completion\n - Certificate of conformity, data sheets\n - Preservation log\n - Certificate for lifting equipment\n - Material certificates" ;
                  rdfs:label "Packing, storage, preservation, lifting, transportation and handling procedure" ;
                  skos:broadMatch rdl:PCA_100006668 ;
                  skos:broader rdl:PCA_100006751 .


###  http://rds.posccaesar.org/ontology/plm/rdl/PCA_100006355
rdl:PCA_100006355 rdf:type owl:Class ;
                  rdfs:subClassOf rdl:PCA_100004908 ;
                  rdl:PCA_100006765 rrdl:CFIHOS-20000030 ;
                  rdl:PCA_100006766 rdl:PCA_100006640 ;
                  rdl:PCA_100006768 "Load list for PAGA amplifiers." ;
                  rdfs:comment "Load list for PAGA amplifiers." ;
                  rdfs:label "PAGA amplifier load list" ;
                  skos:broadMatch rdl:PCA_100006716 ;
                  skos:broader rdl:PCA_100006748 .


###  http://rds.posccaesar.org/ontology/plm/rdl/PCA_100006356
rdl:PCA_100006356 rdf:type owl:Class ;
                  rdfs:subClassOf rdl:PCA_100004908 ;
                  rdl:PCA_100006765 rrdl:CFIHOS-20000030 ;
                  rdl:PCA_100006766 rdl:PCA_100006653 ;
                  rdl:PCA_100006768 "PAGA coverage (STIPA or STI according to NORSOK T-101 measurements report shall be provided." ;
                  rdfs:comment "PAGA coverage (STIPA or STI according to NORSOK T-101 measurements report shall be provided." ;
                  rdfs:label "PAGA coverage measurements reports" ;
                  skos:broadMatch rdl:PCA_100006722 ;
                  skos:broader rdl:PCA_100006756 .


###  http://rds.posccaesar.org/ontology/plm/rdl/PCA_100006357
rdl:PCA_100006357 rdf:type owl:Class ;
                  rdfs:subClassOf rdl:PCA_100004908 ;
                  rdl:PCA_100006765 rrdl:CFIHOS-20000008 ;
                  rdl:PCA_100006766 rdl:PCA_100006634 ,
                                    rdl:PCA_100006635 ,
                                    rdl:PCA_100006636 ,
                                    rdl:PCA_100006637 ,
                                    rdl:PCA_100006638 ,
                                    rdl:PCA_100006639 ;
                  rdl:PCA_100006768 "The document shall contain a template including all adjustable parameters, indicating which parameters are fixed by the project. For parameters which have individual setting the criteria/formula for defining/calculating the individual setting shall be given. In addition, the document shall include a table listing all individual settings. This table shall on one axis list all equipment (tags) and the other all parameter requiring individual setting.\n\nExamples of relevant equipment are: VSD (Variable Speed Drive), Soft starter, Synchronising Equipment, OLTC control (On Load Tap Changer), Insulation Monitoring equipment, Intelligent electrical devices (IED)." ;
                  rdfs:comment "The document shall contain a template including all adjustable parameters, indicating which parameters are fixed by the project. For parameters which have individual setting the criteria/formula for defining/calculating the individual setting shall be given. In addition, the document shall include a table listing all individual settings. This table shall on one axis list all equipment (tags) and the other all parameter requiring individual setting.\n\nExamples of relevant equipment are: VSD (Variable Speed Drive), Soft starter, Synchronising Equipment, OLTC control (On Load Tap Changer), Insulation Monitoring equipment, Intelligent electrical devices (IED)." ;
                  rdfs:label "Parameter setting tables" ;
                  skos:broadMatch rdl:PCA_100006701 ;
                  skos:broader rdl:PCA_100006762 .


###  http://rds.posccaesar.org/ontology/plm/rdl/PCA_100006358
rdl:PCA_100006358 rdf:type owl:Class ;
                  rdfs:subClassOf rdl:PCA_100004908 ;
                  rdl:PCA_100006763 "List for an object containing list items specifying the sub-objects in the product aspect (parts, components, software, equipment, etc.) that constitute an assembly (or sub-assembly) or system and, if necessary, reference documents.\n\nNOTE - Class A indicates that each list item represents a type of constituent object and specifies the quantity of this." ;
                  rdl:PCA_100006766 rdl:PCA_100006653 ;
                  rdl:PCA_100006768 "Mandatory content of information:\nFor each list item:\n - Item reference number\n - Quantity\n - Part number or global identifier (together with manufacturer / supplier)\n - Part name.\n\nOptional content of information:\nFor each list item:\n - List of reference designations\n - Type designation\n - Specifying technical data\n - Descriptive technical data\n - Mass, dimensions\n - Reference to document\n - Remark." ;
                  rdfs:comment "Mandatory content of information:\nFor each list item:\n - Item reference number\n - Quantity\n - Part number or global identifier (together with manufacturer / supplier)\n - Part name.\n\nOptional content of information:\nFor each list item:\n - List of reference designations\n - Type designation\n - Specifying technical data\n - Descriptive technical data\n - Mass, dimensions\n - Reference to document\n - Remark." ;
                  rdfs:label "Part list" ;
                  skos:broadMatch rdl:PCA_100006716 ;
                  skos:broader rdl:PCA_100006748 .


###  http://rds.posccaesar.org/ontology/plm/rdl/PCA_100006359
rdl:PCA_100006359 rdf:type owl:Class ;
                  rdfs:subClassOf rdl:PCA_100004908 ;
                  rdl:PCA_100006763 "The penetration dossier shall give an overview of all penetrations (including penetrations in packages/skids)" ;
                  rdl:PCA_100006765 rrdl:CFIHOS-20000010 ,
                                    rrdl:CFIHOS-20000011 ,
                                    rrdl:CFIHOS-20000013 ;
                  rdl:PCA_100006766 rdl:PCA_100006656 ;
                  rdl:PCA_100006768 "The penetration dossier shall contain the following:\n - Location (e.g. coordinates);\n - Type of penetration;\n - Supplier;\n - Dimension (hole);\n - Dimension (sleeve);\n - Drawing references;\n - Fire rating;\n - Fire loads (include only if the information is available);\n - Penetration number/tag number as relevant." ;
                  rdfs:comment "The penetration dossier shall contain the following:\n - Location (e.g. coordinates);\n - Type of penetration;\n - Supplier;\n - Dimension (hole);\n - Dimension (sleeve);\n - Drawing references;\n - Fire rating;\n - Fire loads (include only if the information is available);\n - Penetration number/tag number as relevant." ;
                  rdfs:label "Penetration dossier" ;
                  skos:broadMatch rdl:PCA_100006716 ;
                  skos:broader rdl:PCA_100006748 .


###  http://rds.posccaesar.org/ontology/plm/rdl/PCA_100006360
rdl:PCA_100006360 rdf:type owl:Class ;
                  rdfs:subClassOf rdl:PCA_100004908 ;
                  rdl:PCA_100006765 rrdl:CFIHOS-20000031 ;
                  rdl:PCA_100006766 rdl:PCA_100006653 ;
                  rdl:PCA_100006768 "A photo archive with pictures of the delivered item(s). \n\n - Pictures shall be in JPEG format.\n - The file name for each picture shall describe the item in the picture.\n - There shall in general be taken picture of each tagged item (or each material/serial-numbered item if untagged), with focus on showing the tagged item in a best possible manner and with enough of its surroundings to get a picture of the location. Several pictures of the same item may be taken for clarity.\n - For a module or structure that contains many tagged items (such as valves, instruments, pumps, hatches, etc.) there shall be taken overview pictures of the module/structure from all sides and top, as well of each tagged item within the module/structure." ;
                  rdfs:comment "A photo archive with pictures of the delivered item(s). \n\n - Pictures shall be in JPEG format.\n - The file name for each picture shall describe the item in the picture.\n - There shall in general be taken picture of each tagged item (or each material/serial-numbered item if untagged), with focus on showing the tagged item in a best possible manner and with enough of its surroundings to get a picture of the location. Several pictures of the same item may be taken for clarity.\n - For a module or structure that contains many tagged items (such as valves, instruments, pumps, hatches, etc.) there shall be taken overview pictures of the module/structure from all sides and top, as well of each tagged item within the module/structure." ;
                  rdfs:label "Photo archive - subsea systems" .


###  http://rds.posccaesar.org/ontology/plm/rdl/PCA_100006361
rdl:PCA_100006361 rdf:type owl:Class ;
                  rdfs:subClassOf rdl:PCA_100004908 ;
                  rdl:PCA_100006763 "Pigability data describes relevant data and drawings for the complete pipeline system, from pigtrap to pigtrap that should be checked out prior to a pigging operation in order to ensure that the pipeline system is in a condition such that it can be pigged, and that the necessary equipment is correctly configured and will work as intended during the pigging operation. Furthermore, the purpose is to ensure that the work carried out is documented." ;
                  rdl:PCA_100006765 rrdl:CFIHOS-20000018 ;
                  rdl:PCA_100006766 rdl:PCA_100006654 ;
                  rdl:PCA_100006768 "Piggable Item List / Bore Map Overview document listing all bore sizes to confirm piggability througout each line\n\n(Template in TR is unavailable to S7 and has not been used)" ;
                  rdfs:comment "Piggable Item List / Bore Map Overview document listing all bore sizes to confirm piggability througout each line\n\n(Template in TR is unavailable to S7 and has not been used)" ;
                  rdfs:label "Pigability data" ;
                  skos:broadMatch rdl:PCA_100006717 ;
                  skos:broader rdl:PCA_100006748 ,
                               rdl:PCA_100006762 .


###  http://rds.posccaesar.org/ontology/plm/rdl/PCA_100006362
rdl:PCA_100006362 rdf:type owl:Class ;
                  rdfs:subClassOf rdl:PCA_100004908 ;
                  rdl:PCA_100006763 "The operational procedure shall describe the necessary activities required for safe pigging operations." ;
                  rdl:PCA_100006765 rrdl:CFIHOS-20000018 ;
                  rdl:PCA_100006766 rdl:PCA_100006654 ;
                  rdl:PCA_100006768 "The procedure shall describe:\n - planned pig type(s)\n - the main steps needed to launch pig into pig launcher and further into the pipeline\n - how to run it into the receiver and take it out\n - equipment needed for pigging\n - preparation for pigging\n - special precautions to be aware of (e.g. block valves, in-line instrumentations, Tees, Wyes etc.) and what corresponding actions to be taken before, during and/or after pigging." ;
                  rdfs:comment "The procedure shall describe:\n - planned pig type(s)\n - the main steps needed to launch pig into pig launcher and further into the pipeline\n - how to run it into the receiver and take it out\n - equipment needed for pigging\n - preparation for pigging\n - special precautions to be aware of (e.g. block valves, in-line instrumentations, Tees, Wyes etc.) and what corresponding actions to be taken before, during and/or after pigging." ;
                  rdfs:label "Pigging procedures" ;
                  skos:broadMatch rdl:PCA_100006688 ;
                  skos:broader rdl:PCA_100006751 .


###  http://rds.posccaesar.org/ontology/plm/rdl/PCA_100006363
rdl:PCA_100006363 rdf:type owl:Class ;
                  rdfs:subClassOf rdl:PCA_100004908 ;
                  rdl:PCA_100006765 rrdl:CFIHOS-20000020 ;
                  rdl:PCA_100006766 rdl:PCA_100006653 ;
                  rdl:PCA_100006768 "Electronic input files for pipe stress program to be delivered for each calculation no.\n\nNOTE: For equipment packages where the amount and size of piping is moderate, or the piping might be mostly for support functions (cooling, lubrication, drain etc.), pipe stress calculations from the manufacturer are not necessary.  For large packages with a considerable amount of larger piping, pipe stress calculations for the main piping should be delivered or optionally retained. Decision/selection should be done early in the project." ;
                  rdfs:comment "Electronic input files for pipe stress program to be delivered for each calculation no.\n\nNOTE: For equipment packages where the amount and size of piping is moderate, or the piping might be mostly for support functions (cooling, lubrication, drain etc.), pipe stress calculations from the manufacturer are not necessary.  For large packages with a considerable amount of larger piping, pipe stress calculations for the main piping should be delivered or optionally retained. Decision/selection should be done early in the project." ;
                  rdfs:label "Pipe stress calculations" ;
                  skos:broadMatch rdl:PCA_100006687 ;
                  skos:broader rdl:PCA_100006741 .


###  http://rds.posccaesar.org/ontology/plm/rdl/PCA_100006364
rdl:PCA_100006364 rdf:type owl:Class ;
                  rdfs:subClassOf rdl:PCA_100004908 ;
                  rdl:PCA_100006763 "The document shall describe the design data for the pipe stress work, and ensure that all applicable codes, standards, guidelines and regulations that are relevant at the commencement of detail engineering are fulfilled. For modification projects the existing procedure for the plant may be used if this is available.\n\nNOTE: For equipment packages where the amount and size of piping is moderate, or the piping might be mostly for support functions (cooling, lubrication, drain etc.), pipe stress procedure from the manufacturer is not necessary.  For large packages with a considerable amount of larger piping, where pipe stress isometrics will be delivered, pipe stress procedure should also be delivered." ;
                  rdl:PCA_100006765 rrdl:CFIHOS-20000020 ;
                  rdl:PCA_100006766 rdl:PCA_100006653 ;
                  rdfs:label "Pipe stress procedure" ;
                  skos:broadMatch rdl:PCA_100006688 ;
                  skos:broader rdl:PCA_100006751 .


###  http://rds.posccaesar.org/ontology/plm/rdl/PCA_100006365
rdl:PCA_100006365 rdf:type owl:Class ;
                  rdfs:subClassOf rdl:PCA_100004908 ;
                  rdl:PCA_100006763 "Detail drawings describing the support installed shall be provided for all pipe supports (pipe support assemblies and spring support assemblies)." ;
                  rdl:PCA_100006765 rrdl:CFIHOS-20000020 ;
                  rdl:PCA_100006766 rdl:PCA_100006653 ;
                  rdl:PCA_100006768 "The following information shall be included:\n - Dimensioned plan, elevation, sectional and iso views as required;\n - Centre of gravity location and coordinates;\n - Weight;\n - Material identification and description (bill of material);\n - Line numbers for all supported lines;\n - Reference to stress isometric if relevant;\n - Reference to support calculations if relevant;\n - Reference to connected pipe support assemblies / spring support assemblies;\n - The drawing title shall include the pipe support number.\n\nNOTE: For equipment packages where the amount and size of piping is moderate, or the piping might be mostly for support functions (cooling, lubrication, drain etc.), pipe support drawings from the manufacturer are not necessary.  For large packages with a considerable amount of larger piping, pipe support drawings for the main piping should be delivered.  Selection should be done early in the project." ;
                  rdfs:comment "The following information shall be included:\n - Dimensioned plan, elevation, sectional and iso views as required;\n - Centre of gravity location and coordinates;\n - Weight;\n - Material identification and description (bill of material);\n - Line numbers for all supported lines;\n - Reference to stress isometric if relevant;\n - Reference to support calculations if relevant;\n - Reference to connected pipe support assemblies / spring support assemblies;\n - The drawing title shall include the pipe support number.\n\nNOTE: For equipment packages where the amount and size of piping is moderate, or the piping might be mostly for support functions (cooling, lubrication, drain etc.), pipe support drawings from the manufacturer are not necessary.  For large packages with a considerable amount of larger piping, pipe support drawings for the main piping should be delivered.  Selection should be done early in the project." ;
                  rdfs:label "Pipe support drawings" ;
                  skos:broadMatch rdl:PCA_100006731 ,
                                  rdl:PCA_100006732 ,
                                  rdl:PCA_100006733 ,
                                  rdl:PCA_100006734 ;
                  skos:broader rdl:PCA_100006746 .


###  http://rds.posccaesar.org/ontology/plm/rdl/PCA_100006366
rdl:PCA_100006366 rdf:type owl:Class ;
                  rdfs:subClassOf rdl:PCA_100004908 ;
                  rdl:PCA_100006765 rrdl:CFIHOS-20000020 ;
                  rdl:PCA_100006766 rdl:PCA_100006653 ;
                  rdl:PCA_100006768 "Index to contain:\n - Pipe support number;\n - Pipe support drawing number;\n - Line number;\n - Piping stress isometric drawing number;\n - Welded attachment (Yes/No);\n - Fire Protection (Yes/No);\n - Hook-up (Yes/No);\n - Temporary pipe support (Yes/No)." ;
                  rdfs:comment "Index to contain:\n - Pipe support number;\n - Pipe support drawing number;\n - Line number;\n - Piping stress isometric drawing number;\n - Welded attachment (Yes/No);\n - Fire Protection (Yes/No);\n - Hook-up (Yes/No);\n - Temporary pipe support (Yes/No)." ;
                  rdfs:label "Pipe support index" ;
                  skos:broadMatch rdl:PCA_100006716 ;
                  skos:broader rdl:PCA_100006748 .


###  http://rds.posccaesar.org/ontology/plm/rdl/PCA_100006367
rdl:PCA_100006367 rdf:type owl:Class ;
                  rdfs:subClassOf rdl:PCA_100004908 ;
                  rdl:PCA_100006763 "DNV-OS-F101 Submarine Pipeline Systems, states  “a system for ensuring correct traceability to the material shall be established”" ;
                  rdl:PCA_100006765 rrdl:CFIHOS-20000020 ,
                                    rrdl:CFIHOS-20000031 ;
                  rdl:PCA_100006766 rdl:PCA_100006653 ;
                  rdl:PCA_100006768 "Pipe tracking data shall be in accordance with Company’s requirements." ;
                  rdfs:comment "Pipe tracking data shall be in accordance with Company’s requirements." ;
                  rdfs:label "Pipe tracking data" ;
                  skos:broadMatch rdl:PCA_100006722 ;
                  skos:broader rdl:PCA_100006756 ,
                               rdl:PCA_100006762 .


###  http://rds.posccaesar.org/ontology/plm/rdl/PCA_100006368
rdl:PCA_100006368 rdf:type owl:Class ;
                  rdfs:subClassOf rdl:PCA_100004908 ;
                  rdl:PCA_100006765 rrdl:CFIHOS-20000018 ;
                  rdl:PCA_100006766 rdl:PCA_100006654 ;
                  rdfs:label "Pipeline index" ;
                  skos:broadMatch rdl:PCA_100006717 ;
                  skos:broader rdl:PCA_100006748 .


###  http://rds.posccaesar.org/ontology/plm/rdl/PCA_100006369
rdl:PCA_100006369 rdf:type owl:Class ;
                  rdfs:subClassOf rdl:PCA_100004908 ;
                  rdl:PCA_100006763 "Documentation of installations to ensure safe operation" ;
                  rdl:PCA_100006765 rrdl:CFIHOS-20000018 ;
                  rdl:PCA_100006766 rdl:PCA_100006654 ;
                  rdl:PCA_100006768 "Pipeline protection drawings of protection not covered by rock installation, trenching or crossings such as use of concrete mattresses or covers" ;
                  rdfs:comment "Pipeline protection drawings of protection not covered by rock installation, trenching or crossings such as use of concrete mattresses or covers" ;
                  rdfs:label "Pipeline protection drawing" ;
                  skos:broadMatch rdl:PCA_100006732 ;
                  skos:broader rdl:PCA_100006746 .


###  http://rds.posccaesar.org/ontology/plm/rdl/PCA_100006370
rdl:PCA_100006370 rdf:type owl:Class ;
                  rdfs:subClassOf rdl:PCA_100004908 ;
                  rdl:PCA_100006763 "Ensure safe operation" ;
                  rdl:PCA_100006765 rrdl:CFIHOS-20000018 ;
                  rdl:PCA_100006766 rdl:PCA_100006654 ;
                  rdl:PCA_100006768 "It includes but it is not limited to: list/description of the surveys available, seabed features, geotechnics, routing restrictions including third party requirements, routing selection criteria and process, stress analysis evaluations, results in terms of reference to routing layout(s) and coordinates' file(s)." ;
                  rdfs:comment "It includes but it is not limited to: list/description of the surveys available, seabed features, geotechnics, routing restrictions including third party requirements, routing selection criteria and process, stress analysis evaluations, results in terms of reference to routing layout(s) and coordinates' file(s)." ;
                  rdfs:label "Pipeline route design report" ;
                  skos:broadMatch rdl:PCA_100006686 ;
                  skos:broader rdl:PCA_100006756 .


###  http://rds.posccaesar.org/ontology/plm/rdl/PCA_100006371
rdl:PCA_100006371 rdf:type owl:Class ;
                  rdfs:subClassOf rdl:PCA_100004908 ;
                  rdl:PCA_100006763 "Ensure safe operation" ;
                  rdl:PCA_100006765 rrdl:CFIHOS-20000018 ;
                  rdl:PCA_100006766 rdl:PCA_100006654 ;
                  rdl:PCA_100006768 "Survey reports and data shall comply with Company's requirements for Offshore surveys." ;
                  rdfs:comment "Survey reports and data shall comply with Company's requirements for Offshore surveys." ;
                  rdfs:label "Pipeline survey reports and data" ;
                  skos:broadMatch rdl:PCA_100006705 ;
                  skos:broader rdl:PCA_100006756 ,
                               rdl:PCA_100006762 .


###  http://rds.posccaesar.org/ontology/plm/rdl/PCA_100006372
rdl:PCA_100006372 rdf:type owl:Class ;
                  rdfs:subClassOf rdl:PCA_100004908 ;
                  rdl:PCA_100006763 "The symbols used for the P&IDs shall be explained by a legend which shall be a part of the total P&ID set. The P&IDs shall use the coding and numbering standard in ENS, and the plant legend and drawing standard in accordance to NORSOK Z-005.\n\nNorsok S-001 \"Tecnical safety\"" ;
                  rdl:PCA_100006765 rrdl:CFIHOS-20000026 ,
                                    rrdl:CFIHOS-20000031 ;
                  rdl:PCA_100006766 rdl:PCA_100006578 ,
                                    rdl:PCA_100006579 ,
                                    rdl:PCA_100006580 ,
                                    rdl:PCA_100006581 ,
                                    rdl:PCA_100006582 ,
                                    rdl:PCA_100006583 ,
                                    rdl:PCA_100006584 ,
                                    rdl:PCA_100006585 ,
                                    rdl:PCA_100006586 ,
                                    rdl:PCA_100006587 ,
                                    rdl:PCA_100006588 ,
                                    rdl:PCA_100006589 ,
                                    rdl:PCA_100006590 ,
                                    rdl:PCA_100006591 ,
                                    rdl:PCA_100006592 ,
                                    rdl:PCA_100006593 ,
                                    rdl:PCA_100006594 ,
                                    rdl:PCA_100006595 ,
                                    rdl:PCA_100006596 ,
                                    rdl:PCA_100006597 ,
                                    rdl:PCA_100006598 ,
                                    rdl:PCA_100006599 ,
                                    rdl:PCA_100006600 ,
                                    rdl:PCA_100006601 ,
                                    rdl:PCA_100006602 ,
                                    rdl:PCA_100006603 ,
                                    rdl:PCA_100006604 ,
                                    rdl:PCA_100006605 ,
                                    rdl:PCA_100006606 ,
                                    rdl:PCA_100006607 ,
                                    rdl:PCA_100006608 ,
                                    rdl:PCA_100006609 ,
                                    rdl:PCA_100006610 ,
                                    rdl:PCA_100006611 ,
                                    rdl:PCA_100006612 ,
                                    rdl:PCA_100006613 ,
                                    rdl:PCA_100006614 ,
                                    rdl:PCA_100006615 ,
                                    rdl:PCA_100006616 ,
                                    rdl:PCA_100006617 ,
                                    rdl:PCA_100006618 ,
                                    rdl:PCA_100006619 ,
                                    rdl:PCA_100006620 ,
                                    rdl:PCA_100006621 ,
                                    rdl:PCA_100006622 ,
                                    rdl:PCA_100006623 ,
                                    rdl:PCA_100006624 ,
                                    rdl:PCA_100006625 ,
                                    rdl:PCA_100006627 ,
                                    rdl:PCA_100006628 ;
                  rdl:PCA_100006768 "P&IDs shall be prepared for drilling+C402:C440 systems, main process (production, injection and export) systems, process support and utility systems and safety systems, including subsea parts of the systems (if any). \n\nAll equipment, piping, valves, orifices and blinds and instrumentation shall be shown on the P&IDs. Identical/parallel items, equipment or systems shall be drawn in full detail, i.e. typical drawings with associated tag number tables are not permitted. \n\nThe number of equipment units on one P&ID shall typically be limited to (a) one vessel or compressor and (b) parallel pumps or heat exchangers. For all connections (e.g. lines and instrument signals) between P&IDs/P&ID sheets, a descriptive text and the connected drawing number shall be included. \n\nThe P&IDs shall include boundary lines for interfaces to an equipment supplier’s scope. Unique numbers shall be included for the connections crossing these boundary lines. The equipment supplier prepares P&IDs for the supplier scope. The P&ID shall include a reference to the equipment supplier P&ID(s), preferably within the boundary lines. Where the equipment supplier scope is on several P&IDs/P&ID sheets, a cross reference between connection number and P&ID/P&ID sheet shall also be included. \n\nRegarding equipment, the following shall as a minimum be included:\n - Tag number;\n - Equipment (main) data in a table on the P&ID;\n - Elevation;\n - Equipment internals that is important to understand the functionality such as weir plate, sections of packing/plates, heat bundle, static mixers etc. shall be shown schematically;\n - Isolation and spading of equipment;\n - Manholes incl. nozzle size;\n - Insulation and heat tracing;\n - Open drains and drip trays;\n - Equipment connections such as connections for instruments, purge, steam out, vent and drains;\n - Inline equipment such as silencers, straightening vanes and strainers. A note shall describe the purpose and requirements for strainers (temporary/permanent, maximum allowable pressure drop etc.\n\nRegarding lines the following shall as a minimum be included: \n - Line number;\n - Direction of flow;\n - Requirements to layout/routing such as line slope and no pockets, symmetrical piping, branch entry to header (e.g. top of header), minimum straight length and minimum and maximum distances;\n - Height/elevation data where required for sumps;\n - Line size change (reducers);\n - Piping specification break;\n - Insulation break;\n - Heat tracing and heat trace break;\n - Blind flanges, caps, plugs or other at end of headers;\n - Spool pieces and flanges required for maintenance and operation;\n - Underground/aboveground breaks;\n - Floor/module breaks;\n - Area breaks;\n - Liquid or gas seal traps and goose necks;\n - Line connections such as connections for instruments, hoses, sampling, chemical injection, probes, pulsation damper, cleaning, drain, vent and temporary uses (to be described in a note).\n\nRegarding valves, orifices and blinds the following shall as a minimum be included: \n - Tag number for all valves, orifices and blinds;\n - For manual valves:\n    - All manual piping valves shall be tagged with nominal pipe size and valve specification reference/VDS-number (or piping special item tag number if applicable). Individual valve tag numbers shall be added on the \"issued for construction\" revision at the latest Locking/interlocking to secure correct operational position (e.g. KILO/KILC = mechanical key interlock open/closed, or CSO/CSC car seal open/closed);\n    - Position indication on valves where relevant (normally open or normally closed);\n\nFor actuated valves:\n   - All on/off actuated valves such as ESV, XSV, XV and HV shall be shown with nominal pipe size and VDS-number in addition to tag number;\n   - Leakage class of all actuated valves;\n   - Fail positions of all actuated valves (i.e. open/closed/maintained position);\n   - Limit switches of actuated valves;\n   - Position indication on valves (normally open or normally closed) where relevant;\n - Relief valve size and set pressure;\n - Spectacle blinds and spade/spacers, shown in normal position;\n - Special requirements to be note.\n\nRegarding instrumentation the following shall as a minimum be included: \n - Tag number;\n - Connections to local control and SAS (ESD, PSD or PCS);\n - Requirement for local reading of instrument;\n - Control power (pneumatic/hydraulic fluid or electrical power);\n - Alarm and trip functions (H, L, HH, LL) shall be indicated and set points shall be shown for trip functions;\n - Port identification when 3-way valves are used;\n - Heat tracing and insulation on instruments;\n - Type of level and flow instruments;\n - The piping valves connecting the instruments to the process, i.e. the valves required for isolation from the process shall be shown specifically. Detailed information about the instrument hook-up, however, will be found on the instrument hook-up drawings." ;
                  rdfs:comment "P&IDs shall be prepared for drilling+C402:C440 systems, main process (production, injection and export) systems, process support and utility systems and safety systems, including subsea parts of the systems (if any). \n\nAll equipment, piping, valves, orifices and blinds and instrumentation shall be shown on the P&IDs. Identical/parallel items, equipment or systems shall be drawn in full detail, i.e. typical drawings with associated tag number tables are not permitted. \n\nThe number of equipment units on one P&ID shall typically be limited to (a) one vessel or compressor and (b) parallel pumps or heat exchangers. For all connections (e.g. lines and instrument signals) between P&IDs/P&ID sheets, a descriptive text and the connected drawing number shall be included. \n\nThe P&IDs shall include boundary lines for interfaces to an equipment supplier’s scope. Unique numbers shall be included for the connections crossing these boundary lines. The equipment supplier prepares P&IDs for the supplier scope. The P&ID shall include a reference to the equipment supplier P&ID(s), preferably within the boundary lines. Where the equipment supplier scope is on several P&IDs/P&ID sheets, a cross reference between connection number and P&ID/P&ID sheet shall also be included. \n\nRegarding equipment, the following shall as a minimum be included:\n - Tag number;\n - Equipment (main) data in a table on the P&ID;\n - Elevation;\n - Equipment internals that is important to understand the functionality such as weir plate, sections of packing/plates, heat bundle, static mixers etc. shall be shown schematically;\n - Isolation and spading of equipment;\n - Manholes incl. nozzle size;\n - Insulation and heat tracing;\n - Open drains and drip trays;\n - Equipment connections such as connections for instruments, purge, steam out, vent and drains;\n - Inline equipment such as silencers, straightening vanes and strainers. A note shall describe the purpose and requirements for strainers (temporary/permanent, maximum allowable pressure drop etc.\n\nRegarding lines the following shall as a minimum be included: \n - Line number;\n - Direction of flow;\n - Requirements to layout/routing such as line slope and no pockets, symmetrical piping, branch entry to header (e.g. top of header), minimum straight length and minimum and maximum distances;\n - Height/elevation data where required for sumps;\n - Line size change (reducers);\n - Piping specification break;\n - Insulation break;\n - Heat tracing and heat trace break;\n - Blind flanges, caps, plugs or other at end of headers;\n - Spool pieces and flanges required for maintenance and operation;\n - Underground/aboveground breaks;\n - Floor/module breaks;\n - Area breaks;\n - Liquid or gas seal traps and goose necks;\n - Line connections such as connections for instruments, hoses, sampling, chemical injection, probes, pulsation damper, cleaning, drain, vent and temporary uses (to be described in a note).\n\nRegarding valves, orifices and blinds the following shall as a minimum be included: \n - Tag number for all valves, orifices and blinds;\n - For manual valves:\n    - All manual piping valves shall be tagged with nominal pipe size and valve specification reference/VDS-number (or piping special item tag number if applicable). Individual valve tag numbers shall be added on the \"issued for construction\" revision at the latest Locking/interlocking to secure correct operational position (e.g. KILO/KILC = mechanical key interlock open/closed, or CSO/CSC car seal open/closed);\n    - Position indication on valves where relevant (normally open or normally closed);\n\nFor actuated valves:\n   - All on/off actuated valves such as ESV, XSV, XV and HV shall be shown with nominal pipe size and VDS-number in addition to tag number;\n   - Leakage class of all actuated valves;\n   - Fail positions of all actuated valves (i.e. open/closed/maintained position);\n   - Limit switches of actuated valves;\n   - Position indication on valves (normally open or normally closed) where relevant;\n - Relief valve size and set pressure;\n - Spectacle blinds and spade/spacers, shown in normal position;\n - Special requirements to be note.\n\nRegarding instrumentation the following shall as a minimum be included: \n - Tag number;\n - Connections to local control and SAS (ESD, PSD or PCS);\n - Requirement for local reading of instrument;\n - Control power (pneumatic/hydraulic fluid or electrical power);\n - Alarm and trip functions (H, L, HH, LL) shall be indicated and set points shall be shown for trip functions;\n - Port identification when 3-way valves are used;\n - Heat tracing and insulation on instruments;\n - Type of level and flow instruments;\n - The piping valves connecting the instruments to the process, i.e. the valves required for isolation from the process shall be shown specifically. Detailed information about the instrument hook-up, however, will be found on the instrument hook-up drawings." ;
                  rdfs:label "Piping and instrument diagram (P&ID)" ;
                  skos:broadMatch rdl:PCA_100006696 ;
                  skos:broader rdl:PCA_100006745 .


###  http://rds.posccaesar.org/ontology/plm/rdl/PCA_100006373
rdl:PCA_100006373 rdf:type owl:Class ;
                  rdfs:subClassOf rdl:PCA_100004908 ;
                  rdl:PCA_100006765 rrdl:CFIHOS-20000020 ;
                  rdl:PCA_100006766 rdl:PCA_100006653 ;
                  rdl:PCA_100006768 "The document shall include drawings and strength calculations of piping components, typical: weldolets, nipoflanges etc." ;
                  rdfs:comment "The document shall include drawings and strength calculations of piping components, typical: weldolets, nipoflanges etc." ;
                  rdfs:label "Piping component calculations" ;
                  skos:broadMatch rdl:PCA_100006687 ;
                  skos:broader rdl:PCA_100006741 .


###  http://rds.posccaesar.org/ontology/plm/rdl/PCA_100006374
rdl:PCA_100006374 rdf:type owl:Class ;
                  rdfs:subClassOf rdl:PCA_100004908 ;
                  rdl:PCA_100006763 "Specify fabrication requirements for piping." ;
                  rdl:PCA_100006765 rrdl:CFIHOS-20000031 ;
                  rdl:PCA_100006766 rdl:PCA_100006653 ;
                  rdl:PCA_100006768 "Document specifying the methods for fabrication of piping. Includes references to specifications for welding, NDT, assembly, dimensional control, FAT, painting etc." ;
                  rdfs:comment "Document specifying the methods for fabrication of piping. Includes references to specifications for welding, NDT, assembly, dimensional control, FAT, painting etc." ;
                  rdfs:label "Piping fabrication procedure" ;
                  skos:broadMatch rdl:PCA_100006688 ;
                  skos:broader rdl:PCA_100006751 .


###  http://rds.posccaesar.org/ontology/plm/rdl/PCA_100006375
rdl:PCA_100006375 rdf:type owl:Class ;
                  rdfs:subClassOf rdl:PCA_100004908 ;
                  rdl:PCA_100006763 "FRB User guide - Describes the content of each deliverable in the FRB and how they relate and refer to each other. Include examples (images) of how to trace welds and material certificates from fabrication drawings/ISOs;" ;
                  rdl:PCA_100006765 rrdl:CFIHOS-20000020 ;
                  rdl:PCA_100006766 rdl:PCA_100006653 ;
                  rdl:PCA_100006768 "The following list shows the deliverables and structure of the fabrication records for piping:\n - Index of design drawings with reference to relevant fabrication drawings (Index of design drawings to be delivered in XLS format additionally to PDF);\n - Index of design-, material-, fabrication specifications, documents and data sheets (*);\n - Welding procedure specifications (*);\n - Welding procedure qualification records (*);\n - Repair procedures and specifications (*);\n - Repair and deviation reports. All alternative testing shall be documented with full traceability to the applicable welds;\n - Weld summary index;\n - Material identification system (*);\n - Material certificates (apply for pressurized Piping materials) (*);\n - Pressure test certificates/documentation (*);\n - PMI reports (*);\n - PWHT reports (*);\n - As-built Design Contractor originated design drawings, mark-ups;\n - As-built fabrication drawings/ISOs mark-ups;\n - Third Party verification reports;\n - Procedure for:\n    - Tensioning/torqueing of flange stud bolts (*);\n    - Flushing and cleaning (*);\n    - Hydro testing (*);\n    - Hydro flushing of riser- and pipeline valves (*);\n    - Pneumatic flushing (*);\n    - Pressurised air shock blowing (PAS) (*);\n    - Soft Pigging (*);\n    - Chemical cleaning (*);\n    - Hot oil flushing (*);\n    - Internal cleaning of pipe after completed fabrication (*);\n    - Bending/flaring (*);\n - Chemical cleaning documentation (*);\n - Hot oil flushing documentation (*).\n\n(*) Can be omitted in modifications if retained by modification Contractor" ;
                  rdfs:comment "The following list shows the deliverables and structure of the fabrication records for piping:\n - Index of design drawings with reference to relevant fabrication drawings (Index of design drawings to be delivered in XLS format additionally to PDF);\n - Index of design-, material-, fabrication specifications, documents and data sheets (*);\n - Welding procedure specifications (*);\n - Welding procedure qualification records (*);\n - Repair procedures and specifications (*);\n - Repair and deviation reports. All alternative testing shall be documented with full traceability to the applicable welds;\n - Weld summary index;\n - Material identification system (*);\n - Material certificates (apply for pressurized Piping materials) (*);\n - Pressure test certificates/documentation (*);\n - PMI reports (*);\n - PWHT reports (*);\n - As-built Design Contractor originated design drawings, mark-ups;\n - As-built fabrication drawings/ISOs mark-ups;\n - Third Party verification reports;\n - Procedure for:\n    - Tensioning/torqueing of flange stud bolts (*);\n    - Flushing and cleaning (*);\n    - Hydro testing (*);\n    - Hydro flushing of riser- and pipeline valves (*);\n    - Pneumatic flushing (*);\n    - Pressurised air shock blowing (PAS) (*);\n    - Soft Pigging (*);\n    - Chemical cleaning (*);\n    - Hot oil flushing (*);\n    - Internal cleaning of pipe after completed fabrication (*);\n    - Bending/flaring (*);\n - Chemical cleaning documentation (*);\n - Hot oil flushing documentation (*).\n\n(*) Can be omitted in modifications if retained by modification Contractor" ;
                  rdfs:label "Piping fabrication records" ;
                  skos:broadMatch rdl:PCA_100006722 ,
                                  rdl:PCA_100006733 ;
                  skos:broader rdl:PCA_100006749 .


###  http://rds.posccaesar.org/ontology/plm/rdl/PCA_100006376
rdl:PCA_100006376 rdf:type owl:Class ;
                  rdfs:subClassOf rdl:PCA_100004908 ;
                  rdl:PCA_100006763 "Applies to piping systems that require special attention during installation, typical for piping connected to strain sensitive equipment such as compressors." ;
                  rdl:PCA_100006765 rrdl:CFIHOS-20000020 ;
                  rdl:PCA_100006766 rdl:PCA_100006653 ;
                  rdfs:label "Piping installation procedure" ;
                  skos:broadMatch rdl:PCA_100006688 ;
                  skos:broader rdl:PCA_100006751 .


###  http://rds.posccaesar.org/ontology/plm/rdl/PCA_100006377
rdl:PCA_100006377 rdf:type owl:Class ;
                  rdfs:subClassOf rdl:PCA_100004908 ;
                  rdl:PCA_100006765 rrdl:CFIHOS-20000020 ;
                  rdl:PCA_100006766 rdl:PCA_100006653 ;
                  rdl:PCA_100006768 "The piping isometric shall be arranged such that it gives a clear readability. The piping line shall be split into reasonable large sections such that the drawing is not too crowded and at the same time avoid unnecessary small sections.\n\nThe following information shall be included:\n - Position numbers for each piping item;\n - Weld locations and numbers (field welds to be identified);\n - Flow arrow;\n - All inline equipment and instrument connections with tag numbers;\n - Special items with coding;\n - Dimensioned pipe support locations and support numbers including spring supports, etc.;\n - Penetrations;\n - Dimensions (including slope if relevant);\n - Reference to connecting isometric drawings;\n - Reference to attached equipment with tag number and nozzle number;\n - Bill of material including position numbers;\n - Line number (according to ENS);\n - Design pressures and temperatures;\n - Pressure test requirements;\n - NDT requirements;\n - Insulation requirements;\n - Heat trace requirements;\n - Surface treatment and topcoat colour requirements;\n - Service colour coding requirements;\n - Post weld heat treatment (PWHT) requirements;\n - Chemical cleaning requirements;\n - Pressure directive (PED) category (for EU countries);\n - Critical line and reference to Stress ISO no.;\n - Reference to P&ID;\n - Area code;\n - Material type;\n - Dry weight, wet weight (content) and CoG.\n\nNOTE: For equipment packages where the amount and size of piping is moderate, or the piping might be mostly for support functions (cooling, lubrication, drain etc.), piping isometrics from the manufacturer are not necessary. For large packages with a considerable amount of larger piping, isometrics for the main piping should be delivered. Selection should be done early in the project." ;
                  rdfs:comment "The piping isometric shall be arranged such that it gives a clear readability. The piping line shall be split into reasonable large sections such that the drawing is not too crowded and at the same time avoid unnecessary small sections.\n\nThe following information shall be included:\n - Position numbers for each piping item;\n - Weld locations and numbers (field welds to be identified);\n - Flow arrow;\n - All inline equipment and instrument connections with tag numbers;\n - Special items with coding;\n - Dimensioned pipe support locations and support numbers including spring supports, etc.;\n - Penetrations;\n - Dimensions (including slope if relevant);\n - Reference to connecting isometric drawings;\n - Reference to attached equipment with tag number and nozzle number;\n - Bill of material including position numbers;\n - Line number (according to ENS);\n - Design pressures and temperatures;\n - Pressure test requirements;\n - NDT requirements;\n - Insulation requirements;\n - Heat trace requirements;\n - Surface treatment and topcoat colour requirements;\n - Service colour coding requirements;\n - Post weld heat treatment (PWHT) requirements;\n - Chemical cleaning requirements;\n - Pressure directive (PED) category (for EU countries);\n - Critical line and reference to Stress ISO no.;\n - Reference to P&ID;\n - Area code;\n - Material type;\n - Dry weight, wet weight (content) and CoG.\n\nNOTE: For equipment packages where the amount and size of piping is moderate, or the piping might be mostly for support functions (cooling, lubrication, drain etc.), piping isometrics from the manufacturer are not necessary. For large packages with a considerable amount of larger piping, isometrics for the main piping should be delivered. Selection should be done early in the project." ;
                  rdfs:label "Piping isometrics" ;
                  skos:broadMatch rdl:PCA_100006708 ,
                                  rdl:PCA_100006732 ,
                                  rdl:PCA_100006733 ,
                                  rdl:PCA_100006734 ;
                  skos:broader rdl:PCA_100006746 .


###  http://rds.posccaesar.org/ontology/plm/rdl/PCA_100006378
rdl:PCA_100006378 rdf:type owl:Class ;
                  rdfs:subClassOf rdl:PCA_100004908 ;
                  rdl:PCA_100006763 "Piping stress isometrics shall be provided for all lines for which stress calculations or evaluation have been made." ;
                  rdl:PCA_100006765 rrdl:CFIHOS-20000020 ;
                  rdl:PCA_100006766 rdl:PCA_100006653 ;
                  rdl:PCA_100006768 "Piping stress isometrics shall include the following information:\n - Line number;\n - Process data (temp. and pressure);\n - Valve weights;\n - Equipment nozzle loads;\n - Stress summary;\n - Reference to P&ID;\n - Restraint loading and displacement;\n - Spring summary;\n - Calculation No.;\n - Separate document no with revision code on each stress iso (not stress report number);\n - Special supports, typical: gap, adjustable, PTFE;\n - Equipment nozzle with tag no;\n - Pipe specification break;\n - Reference to adjacent isometric drawings;\n - Special items;\n - Penetrations;\n - Pipe stress report no;\n - Dimensioned pipe support locations and support numbers including spring supports, etc.;\n - Node numbers from calculation model (as a minimum for each pipe support, valve, equipment nozzle, interface to other lines/sheets/isometrics and location for max utilisation).\n- Support function\n\nNOTE: For equipment packages where the amount and size of piping is moderate, or the piping might be mostly for support functions (cooling, lubrication, drain etc.), piping stress isometrics from the manufacturer are not necessary.  For large packages with a considerable amount of larger piping, piping stress isometrics for the main piping should be delivered.  Selection should be done early in the project." ;
                  rdfs:comment "Piping stress isometrics shall include the following information:\n - Line number;\n - Process data (temp. and pressure);\n - Valve weights;\n - Equipment nozzle loads;\n - Stress summary;\n - Reference to P&ID;\n - Restraint loading and displacement;\n - Spring summary;\n - Calculation No.;\n - Separate document no with revision code on each stress iso (not stress report number);\n - Special supports, typical: gap, adjustable, PTFE;\n - Equipment nozzle with tag no;\n - Pipe specification break;\n - Reference to adjacent isometric drawings;\n - Special items;\n - Penetrations;\n - Pipe stress report no;\n - Dimensioned pipe support locations and support numbers including spring supports, etc.;\n - Node numbers from calculation model (as a minimum for each pipe support, valve, equipment nozzle, interface to other lines/sheets/isometrics and location for max utilisation).\n- Support function\n\nNOTE: For equipment packages where the amount and size of piping is moderate, or the piping might be mostly for support functions (cooling, lubrication, drain etc.), piping stress isometrics from the manufacturer are not necessary.  For large packages with a considerable amount of larger piping, piping stress isometrics for the main piping should be delivered.  Selection should be done early in the project." ;
                  rdfs:label "Piping stress isometrics" ;
                  skos:broadMatch rdl:PCA_100006708 ,
                                  rdl:PCA_100006732 ;
                  skos:broader rdl:PCA_100006746 .


###  http://rds.posccaesar.org/ontology/plm/rdl/PCA_100006379
rdl:PCA_100006379 rdf:type owl:Class ;
                  rdfs:subClassOf rdl:PCA_100004908 ;
                  rdl:PCA_100006763 "The Piping Stress Report shall document that the critical lines meet the code, authority requirements and project requirements. Piping stress calculations shall be provided for all critical piping. The piping stress report shall include reference to the Piping Stress Isometric drawings." ;
                  rdl:PCA_100006765 rrdl:CFIHOS-20000020 ;
                  rdl:PCA_100006766 rdl:PCA_100006653 ;
                  rdfs:label "Piping stress report" ;
                  skos:broadMatch rdl:PCA_100006687 ;
                  skos:broader rdl:PCA_100006756 .


###  http://rds.posccaesar.org/ontology/plm/rdl/PCA_100006380
rdl:PCA_100006380 rdf:type owl:Class ;
                  rdfs:subClassOf rdl:PCA_100004908 ;
                  rdl:PCA_100006765 rrdl:CFIHOS-20000020 ;
                  rdl:PCA_100006766 rdl:PCA_100006656 ;
                  rdl:PCA_100006768 "These drawings are relevant for offshore facilities and for the process plant for onshore facilities.\n\nOne plot plan drawing for each area/deck level shall be produced. The plot plan drawing shall cover the entire process plant/deck area. The size of the facility will determine the scale of the drawing, but normally a scale of 1:500 on an A3 format shall be aimed for.\n\nThe following content shall be included on the drawings:\n - Plant/Platform Northing and orientation with respect of true north;\n - Gridlines with north and east references;\n - Scale bar;\n - Elevations of all decks/platforms;\n - Area segregation, with fire partitions indicated;\n - Safety evacuation equipment, such as escape tunnels, lifeboats (offshore), escape chutes (offshore), etc.;\n - MOB boat location (offshore);\n - Helideck location;\n - Location of cranes, with boom rests and maintenance platforms. Lifting capacity radiuses to be indicated;\n - Hose loading station and tote tank area (offshore);\n - Laydown areas;\n - Waste sorting stations;\n - Main pipe racks;\n - Main stairs, access and escape routes;\n - Main material handling routes;\n - Manifold area arrangement;\n - Wellhead area including well slots;\n - Drilling derrick extreme outlines indicated;\n - Location of temporary well intervention equipment;\n - Flare tower location and extreme outlines indicated;\n - HVAC, instrument and electrical rooms (offshore);\n - Control room (offshore);\n - Living Quarter (offshore);\n - Main structures;\n - Location of all major equipment as identified in MEL;\n - Main equipment shall be tagged according to MEL. An equipment index shall be included on the drawing;\n - Space allocation for risers, J-tubes and umbilicals including temporary equipment (pulling arrangement) (offshore);\n - Space for future modules/equipment." ;
                  rdfs:comment "These drawings are relevant for offshore facilities and for the process plant for onshore facilities.\n\nOne plot plan drawing for each area/deck level shall be produced. The plot plan drawing shall cover the entire process plant/deck area. The size of the facility will determine the scale of the drawing, but normally a scale of 1:500 on an A3 format shall be aimed for.\n\nThe following content shall be included on the drawings:\n - Plant/Platform Northing and orientation with respect of true north;\n - Gridlines with north and east references;\n - Scale bar;\n - Elevations of all decks/platforms;\n - Area segregation, with fire partitions indicated;\n - Safety evacuation equipment, such as escape tunnels, lifeboats (offshore), escape chutes (offshore), etc.;\n - MOB boat location (offshore);\n - Helideck location;\n - Location of cranes, with boom rests and maintenance platforms. Lifting capacity radiuses to be indicated;\n - Hose loading station and tote tank area (offshore);\n - Laydown areas;\n - Waste sorting stations;\n - Main pipe racks;\n - Main stairs, access and escape routes;\n - Main material handling routes;\n - Manifold area arrangement;\n - Wellhead area including well slots;\n - Drilling derrick extreme outlines indicated;\n - Location of temporary well intervention equipment;\n - Flare tower location and extreme outlines indicated;\n - HVAC, instrument and electrical rooms (offshore);\n - Control room (offshore);\n - Living Quarter (offshore);\n - Main structures;\n - Location of all major equipment as identified in MEL;\n - Main equipment shall be tagged according to MEL. An equipment index shall be included on the drawing;\n - Space allocation for risers, J-tubes and umbilicals including temporary equipment (pulling arrangement) (offshore);\n - Space for future modules/equipment." ;
                  rdfs:label "Plot plan drawings" ;
                  skos:broadMatch rdl:PCA_100006708 ;
                  skos:broader rdl:PCA_100006746 .


###  http://rds.posccaesar.org/ontology/plm/rdl/PCA_100006381
rdl:PCA_100006381 rdf:type owl:Class ;
                  rdfs:subClassOf rdl:PCA_100004908 ;
                  rdl:PCA_100006763 "Document use of correct material." ;
                  rdl:PCA_100006765 rrdl:CFIHOS-20000031 ;
                  rdl:PCA_100006766 rdl:PCA_100006653 ;
                  rdl:PCA_100006768 "Document containing records of material identification by chemical analysis." ;
                  rdfs:comment "Document containing records of material identification by chemical analysis." ;
                  rdfs:label "PMI reports" ;
                  skos:broadMatch rdl:PCA_100006722 ;
                  skos:broader rdl:PCA_100006756 .


###  http://rds.posccaesar.org/ontology/plm/rdl/PCA_100006382
rdl:PCA_100006382 rdf:type owl:Class ;
                  rdfs:subClassOf rdl:PCA_100004908 ;
                  rdl:PCA_100006765 rrdl:CFIHOS-20000023 ;
                  rdl:PCA_100006766 rdl:PCA_100006653 ;
                  rdl:PCA_100006768 "The diagram shall identify all pneumatic connections." ;
                  rdfs:comment "The diagram shall identify all pneumatic connections." ;
                  rdfs:label "Pneumatic connection diagram" ;
                  skos:broadMatch rdl:PCA_100006712 ;
                  skos:broader rdl:PCA_100006745 .


###  http://rds.posccaesar.org/ontology/plm/rdl/PCA_100006383
rdl:PCA_100006383 rdf:type owl:Class ;
                  rdfs:subClassOf rdl:PCA_100004908 ;
                  rdl:PCA_100006765 rrdl:CFIHOS-20000015 ;
                  rdl:PCA_100006766 rdl:PCA_100006653 ;
                  rdl:PCA_100006768 "For pneumatic and hydraulic consumers, the supplier shall work out hook-up drawings.\n\nA typical hook-up drawing shall indicate details such as:\n - All instrument/bulk material installed by Supplier;\n - Connections and dimensions of signal lines/tubing;\n - Material of instrument bulk.\n\nTypical hook-up drawings should be used as a guideline.\n\nThe drawing shall indicate split of responsibilities between Supplier and Purchaser." ;
                  rdfs:comment "For pneumatic and hydraulic consumers, the supplier shall work out hook-up drawings.\n\nA typical hook-up drawing shall indicate details such as:\n - All instrument/bulk material installed by Supplier;\n - Connections and dimensions of signal lines/tubing;\n - Material of instrument bulk.\n\nTypical hook-up drawings should be used as a guideline.\n\nThe drawing shall indicate split of responsibilities between Supplier and Purchaser." ;
                  rdfs:label "Pneumatic/hydraulic hook-up drawing" ;
                  skos:broadMatch rdl:PCA_100006713 ,
                                  rdl:PCA_100006731 ,
                                  rdl:PCA_100006732 ;
                  skos:broader rdl:PCA_100006746 .


###  http://rds.posccaesar.org/ontology/plm/rdl/PCA_100006384
rdl:PCA_100006384 rdf:type owl:Class ;
                  rdfs:subClassOf rdl:PCA_100004908 ;
                  rdl:PCA_100006763 "Certificate to confirm compliance with contract / purchase order with reference to standards, technical specifications and requirements for the product." ;
                  rdl:PCA_100006765 rrdl:CFIHOS-20000027 ;
                  rdl:PCA_100006766 rdl:PCA_100006653 ;
                  rdl:PCA_100006768 "The manufacture’s or other party’s confirmation that the product is designed, manufactured and tested as specified." ;
                  rdfs:comment "The manufacture’s or other party’s confirmation that the product is designed, manufactured and tested as specified." ;
                  rdfs:label "PO declaration of compliance" ;
                  skos:broadMatch rdl:PCA_100006722 ;
                  skos:broader rdl:PCA_100006743 .


###  http://rds.posccaesar.org/ontology/plm/rdl/PCA_100006385
rdl:PCA_100006385 rdf:type owl:Class ;
                  rdfs:subClassOf rdl:PCA_100004908 ;
                  rdl:PCA_100006763 "Procedure describing the method for material identification by elemental analysis." ;
                  rdl:PCA_100006766 rdl:PCA_100006653 ;
                  rdl:PCA_100006768 "Provide instructions to the PMI operator." ;
                  rdfs:comment "Provide instructions to the PMI operator." ;
                  rdfs:label "Positive material identification (PMI) procedure" ;
                  skos:broadMatch rdl:PCA_100006722 ;
                  skos:broader rdl:PCA_100006751 .


###  http://rds.posccaesar.org/ontology/plm/rdl/PCA_100006386
rdl:PCA_100006386 rdf:type owl:Class ;
                  rdfs:subClassOf rdl:PCA_100004908 ;
                  rdl:PCA_100006763 "Document use of correct material." ;
                  rdl:PCA_100006765 rrdl:CFIHOS-20000031 ;
                  rdl:PCA_100006766 rdl:PCA_100006653 ;
                  rdl:PCA_100006768 "Document containing records of material identification by chemical analysis." ;
                  rdfs:comment "Document containing records of material identification by chemical analysis." ;
                  rdfs:label "Positive material identification (PMI) reports" ;
                  skos:broadMatch rdl:PCA_100006722 ;
                  skos:broader rdl:PCA_100006756 .


###  http://rds.posccaesar.org/ontology/plm/rdl/PCA_100006387
rdl:PCA_100006387 rdf:type owl:Class ;
                  rdfs:subClassOf rdl:PCA_100004908 ;
                  rdl:PCA_100006763 "Verification that the product is manufactured with materials from pre-qualified material suppliers\n\nFor use by purchaser" ;
                  rdl:PCA_100006766 rdl:PCA_100006653 ;
                  rdl:PCA_100006768 "Suppliers own format. Manufacturer's Qualification Test Record may be required if specified by client\n\nList of Sub-suppliers" ;
                  rdfs:comment "Suppliers own format. Manufacturer's Qualification Test Record may be required if specified by client\n\nList of Sub-suppliers" ;
                  rdfs:label "Pre qualified manufacturers list (NORSOK M650)" ;
                  skos:broader rdl:PCA_100006748 .


###  http://rds.posccaesar.org/ontology/plm/rdl/PCA_100006388
rdl:PCA_100006388 rdf:type owl:Class ;
                  rdfs:subClassOf rdl:PCA_100004908 ;
                  rdl:PCA_100006763 "Describe how to preserve and store equipment in a safe and economical manner" ;
                  rdl:PCA_100006765 rrdl:CFIHOS-20000031 ;
                  rdl:PCA_100006766 rdl:PCA_100006653 ;
                  rdl:PCA_100006768 "Information for preservation of the equipment during short- and long term storage." ;
                  rdfs:comment "Information for preservation of the equipment during short- and long term storage." ;
                  rdfs:label "Preservation and storage instructions" ;
                  skos:broadMatch rdl:PCA_100006668 ;
                  skos:broader rdl:PCA_100006751 .


###  http://rds.posccaesar.org/ontology/plm/rdl/PCA_100006389
rdl:PCA_100006389 rdf:type owl:Class ;
                  rdfs:subClassOf rdl:PCA_100004908 ;
                  rdl:PCA_100006763 "To keep track of all pressure test charts performed during drilling/completion phase. Test data/chart documents the performance for each well barrier element installed during well construction phase" ;
                  rdl:PCA_100006765 rrdl:CFIHOS-20000042 ;
                  rdl:PCA_100006768 "Documentation of all leak/pressure test performed during the construction of the well, shall contain: \n - Time and date\n - Equipment tested\n - Volumes pumped and bleed back\n - Holding time\n - Pressure drop over holding time\n - Which pump used\n - Signature" ;
                  rdfs:comment "Documentation of all leak/pressure test performed during the construction of the well, shall contain: \n - Time and date\n - Equipment tested\n - Volumes pumped and bleed back\n - Holding time\n - Pressure drop over holding time\n - Which pump used\n - Signature" ;
                  rdfs:label "Pressure chart dossier (drilling / completion )" ;
                  skos:broadMatch rdl:PCA_100006722 ;
                  skos:broader rdl:PCA_100006748 .


###  http://rds.posccaesar.org/ontology/plm/rdl/PCA_100006390
rdl:PCA_100006390 rdf:type owl:Class ;
                  rdfs:subClassOf rdl:PCA_100004908 ;
                  rdl:PCA_100006763 "A document containing data which records compliance with specified requirements." ;
                  rdl:PCA_100006765 rrdl:CFIHOS-20000027 ;
                  rdl:PCA_100006766 rdl:PCA_100006653 ;
                  rdl:PCA_100006768 "Document shall contain or link to the proven requirements and results. It shall carry date and approvals (Signatures.)" ;
                  rdfs:comment "Document shall contain or link to the proven requirements and results. It shall carry date and approvals (Signatures.)" ;
                  rdfs:label "Pressure test certificate" ;
                  skos:broadMatch rdl:PCA_100006722 ;
                  skos:broader rdl:PCA_100006743 .


###  http://rds.posccaesar.org/ontology/plm/rdl/PCA_100006391
rdl:PCA_100006391 rdf:type owl:Class ;
                  rdfs:subClassOf rdl:PCA_100004908 ;
                  rdl:PCA_100006763 "This document is used for verification of compliance" ;
                  rdl:PCA_100006766 rdl:PCA_100006653 ;
                  rdl:PCA_100006768 "Pickling, passivation, flushing and visual cleanliness check to be documented" ;
                  rdfs:comment "Pickling, passivation, flushing and visual cleanliness check to be documented" ;
                  rdfs:label "Procedure - pickling / passivation / flushing / visual cleanliness check - multi" ;
                  skos:broadMatch rdl:PCA_100006722 ;
                  skos:broader rdl:PCA_100006751 .


###  http://rds.posccaesar.org/ontology/plm/rdl/PCA_100006392
rdl:PCA_100006392 rdf:type owl:Class ;
                  rdfs:subClassOf rdl:PCA_100004908 ;
                  rdl:PCA_100006763 "No standardized description is presently available." ;
                  rdl:PCA_100006765 rrdl:CFIHOS-20000026 ;
                  rdl:PCA_100006766 rdl:PCA_100006653 ;
                  rdl:PCA_100006768 "No standardized description is presently available." ;
                  rdfs:comment "No standardized description is presently available." ;
                  rdfs:label "Process datasheet" ;
                  skos:broadMatch rdl:PCA_100006686 ;
                  skos:broader rdl:PCA_100006747 .


###  http://rds.posccaesar.org/ontology/plm/rdl/PCA_100006393
rdl:PCA_100006393 rdf:type owl:Class ;
                  rdfs:subClassOf rdl:PCA_100004908 ;
                  rdl:PCA_100006763 "The symbols used for the PFDs shall be explained by a legend which shall be a part of the total PFD set. The PFDs shall use the coding and numbering standard in ENS, and the plant legend and drawing standard in accordance with NORSOK Z-005.\n\nNorsok S-001 \"Technical safety\"" ;
                  rdl:PCA_100006765 rrdl:CFIHOS-20000026 ,
                                    rrdl:CFIHOS-20000031 ;
                  rdl:PCA_100006766 rdl:PCA_100006578 ,
                                    rdl:PCA_100006579 ,
                                    rdl:PCA_100006580 ,
                                    rdl:PCA_100006581 ,
                                    rdl:PCA_100006582 ,
                                    rdl:PCA_100006583 ,
                                    rdl:PCA_100006584 ,
                                    rdl:PCA_100006585 ,
                                    rdl:PCA_100006586 ,
                                    rdl:PCA_100006587 ,
                                    rdl:PCA_100006588 ,
                                    rdl:PCA_100006589 ,
                                    rdl:PCA_100006590 ,
                                    rdl:PCA_100006591 ,
                                    rdl:PCA_100006592 ,
                                    rdl:PCA_100006593 ,
                                    rdl:PCA_100006594 ,
                                    rdl:PCA_100006595 ,
                                    rdl:PCA_100006596 ,
                                    rdl:PCA_100006597 ,
                                    rdl:PCA_100006598 ,
                                    rdl:PCA_100006599 ,
                                    rdl:PCA_100006600 ,
                                    rdl:PCA_100006601 ,
                                    rdl:PCA_100006602 ,
                                    rdl:PCA_100006603 ,
                                    rdl:PCA_100006604 ,
                                    rdl:PCA_100006605 ,
                                    rdl:PCA_100006606 ,
                                    rdl:PCA_100006607 ,
                                    rdl:PCA_100006608 ,
                                    rdl:PCA_100006609 ,
                                    rdl:PCA_100006610 ,
                                    rdl:PCA_100006611 ,
                                    rdl:PCA_100006612 ,
                                    rdl:PCA_100006613 ,
                                    rdl:PCA_100006614 ,
                                    rdl:PCA_100006615 ,
                                    rdl:PCA_100006616 ,
                                    rdl:PCA_100006617 ,
                                    rdl:PCA_100006618 ,
                                    rdl:PCA_100006619 ,
                                    rdl:PCA_100006620 ,
                                    rdl:PCA_100006621 ,
                                    rdl:PCA_100006622 ,
                                    rdl:PCA_100006623 ,
                                    rdl:PCA_100006624 ,
                                    rdl:PCA_100006625 ,
                                    rdl:PCA_100006627 ,
                                    rdl:PCA_100006628 ;
                  rdl:PCA_100006768 "PFDs shall be prepared for drilling systems, main process (production, injection and export) systems, process support and utility systems and safety systems, including subsea parts of the systems (if any). For systems with significantly different operating modes/phases, separate PFDs shall be prepared for each mode/phase. \n\nProcess equipment shall be shown schematically on the PFDs with equipment tag numbers and operating pressure and temperature. Equipment name, sparing (for parallel equipment) and main equipment operating/characteristic data (e.g. operating duty for a compressor) shall be included. \n \nProcess streams to/from the process equipment essential for understanding the operating principle and the heat and material balance shall be included on the PFDs with a stream number. Stream data describing the process fluid flow shall be included in a table on the PFD or on a separate drawing/sheet referred from the PFD. \n \nControl loops shall be shown schematically on the PFDs, including utility streams where these are a part of the control loops." ;
                  rdfs:comment "PFDs shall be prepared for drilling systems, main process (production, injection and export) systems, process support and utility systems and safety systems, including subsea parts of the systems (if any). For systems with significantly different operating modes/phases, separate PFDs shall be prepared for each mode/phase. \n\nProcess equipment shall be shown schematically on the PFDs with equipment tag numbers and operating pressure and temperature. Equipment name, sparing (for parallel equipment) and main equipment operating/characteristic data (e.g. operating duty for a compressor) shall be included. \n \nProcess streams to/from the process equipment essential for understanding the operating principle and the heat and material balance shall be included on the PFDs with a stream number. Stream data describing the process fluid flow shall be included in a table on the PFD or on a separate drawing/sheet referred from the PFD. \n \nControl loops shall be shown schematically on the PFDs, including utility streams where these are a part of the control loops." ;
                  rdfs:label "Process flow diagrams (PFD)" ;
                  skos:broadMatch rdl:PCA_100006696 ;
                  skos:broader rdl:PCA_100006745 .


###  http://rds.posccaesar.org/ontology/plm/rdl/PCA_100006394
rdl:PCA_100006394 rdf:type owl:Class ;
                  rdfs:subClassOf rdl:PCA_100004908 ;
                  rdl:PCA_100006763 "Individual close-out answer for each finding/recommendation from the HAZOP session(s) shall be issued." ;
                  rdl:PCA_100006765 rrdl:CFIHOS-20000026 ;
                  rdl:PCA_100006766 rdl:PCA_100006578 ,
                                    rdl:PCA_100006579 ,
                                    rdl:PCA_100006580 ,
                                    rdl:PCA_100006581 ,
                                    rdl:PCA_100006582 ,
                                    rdl:PCA_100006583 ,
                                    rdl:PCA_100006584 ,
                                    rdl:PCA_100006585 ,
                                    rdl:PCA_100006586 ,
                                    rdl:PCA_100006587 ,
                                    rdl:PCA_100006588 ,
                                    rdl:PCA_100006589 ,
                                    rdl:PCA_100006590 ,
                                    rdl:PCA_100006591 ,
                                    rdl:PCA_100006592 ,
                                    rdl:PCA_100006593 ,
                                    rdl:PCA_100006594 ,
                                    rdl:PCA_100006595 ,
                                    rdl:PCA_100006596 ,
                                    rdl:PCA_100006597 ,
                                    rdl:PCA_100006598 ,
                                    rdl:PCA_100006599 ,
                                    rdl:PCA_100006600 ,
                                    rdl:PCA_100006601 ,
                                    rdl:PCA_100006602 ,
                                    rdl:PCA_100006603 ,
                                    rdl:PCA_100006604 ,
                                    rdl:PCA_100006605 ,
                                    rdl:PCA_100006606 ,
                                    rdl:PCA_100006607 ,
                                    rdl:PCA_100006608 ,
                                    rdl:PCA_100006609 ,
                                    rdl:PCA_100006610 ,
                                    rdl:PCA_100006611 ,
                                    rdl:PCA_100006612 ,
                                    rdl:PCA_100006613 ,
                                    rdl:PCA_100006614 ,
                                    rdl:PCA_100006615 ,
                                    rdl:PCA_100006616 ,
                                    rdl:PCA_100006617 ,
                                    rdl:PCA_100006618 ,
                                    rdl:PCA_100006619 ,
                                    rdl:PCA_100006620 ,
                                    rdl:PCA_100006621 ,
                                    rdl:PCA_100006622 ,
                                    rdl:PCA_100006623 ,
                                    rdl:PCA_100006624 ,
                                    rdl:PCA_100006625 ,
                                    rdl:PCA_100006627 ,
                                    rdl:PCA_100006633 ;
                  rdl:PCA_100006768 "All answers shall be collected in a close-out report." ;
                  rdfs:comment "All answers shall be collected in a close-out report." ;
                  rdfs:label "Process hazop close-out report" ;
                  skos:broadMatch rdl:PCA_100006687 ,
                                  rdl:PCA_100006688 ;
                  skos:broader rdl:PCA_100006756 .


###  http://rds.posccaesar.org/ontology/plm/rdl/PCA_100006395
rdl:PCA_100006395 rdf:type owl:Class ;
                  rdfs:subClassOf rdl:PCA_100004908 ;
                  rdl:PCA_100006763 "In accordance with API 521 chapter 4.7, and authority regulation \"Aktivitetsforskriften\" §20." ;
                  rdl:PCA_100006765 rrdl:CFIHOS-20000026 ;
                  rdl:PCA_100006766 rdl:PCA_100006654 ;
                  rdl:PCA_100006768 "The process safety report shall be one single report for the plant (i.e. not split into several reports), and this report shall be updated whenever relevant modifications to the plant are performed.\n\nThe process safety report shall as a minimum include/describe:\n - The philosophy for process safety functions, i.e. pressure protection, level protection, temperature protection and overflow protection;\n - Process safety functions including premises for the design of the safety function:\n    - Documentation of how these premises are fulfilled in design and shall be maintained, so that future modifications will not compromise the design intention;\n    - Relief cases (all) for relief valves including the dimensioning ‘required capacity’ and the; ‘rated capacity’\n    - Instrumented shutdown:\n    - The structured review of the required instrumented shut down functions:\n   - Documentation of the performed structured analysis utilizing SAT, SAC and SAFEs in accordance with ISO 10418/API RP 14 C;\n   - Documentation of the structured review carried out to determine required instrumented shutdown functions, e.g. LOPA (if applicable); \n - The philosophy for leakage detection;\n - Listing of valves that need to be secured in the correct position as a part of the process safety design, including reasoning for securing the valve position and the choice of method;\n - Heat conservation philosophy for safety critical heat conservation including operating and maintenance practice to ensure proper reliability of the heat conservation systems;\n - Safety critical procedures (administrative control);\n - Safety critical check valves;\n - Pipeline protection (if relevant);\n - The reasoning for the chosen sectionalisation of the process;\n - The relief valve schedule;\n - PSD response time.\n\nThe dynamic simulation model(s) used for the simulations of the Inadvertent valve opening (IVO) and Choke collapse (CC) scenarios, e.g. the Olga model, shall be delivered and shall represent the As built design of wells, flowlines and topside piping." ;
                  rdfs:comment "The process safety report shall be one single report for the plant (i.e. not split into several reports), and this report shall be updated whenever relevant modifications to the plant are performed.\n\nThe process safety report shall as a minimum include/describe:\n - The philosophy for process safety functions, i.e. pressure protection, level protection, temperature protection and overflow protection;\n - Process safety functions including premises for the design of the safety function:\n    - Documentation of how these premises are fulfilled in design and shall be maintained, so that future modifications will not compromise the design intention;\n    - Relief cases (all) for relief valves including the dimensioning ‘required capacity’ and the; ‘rated capacity’\n    - Instrumented shutdown:\n    - The structured review of the required instrumented shut down functions:\n   - Documentation of the performed structured analysis utilizing SAT, SAC and SAFEs in accordance with ISO 10418/API RP 14 C;\n   - Documentation of the structured review carried out to determine required instrumented shutdown functions, e.g. LOPA (if applicable); \n - The philosophy for leakage detection;\n - Listing of valves that need to be secured in the correct position as a part of the process safety design, including reasoning for securing the valve position and the choice of method;\n - Heat conservation philosophy for safety critical heat conservation including operating and maintenance practice to ensure proper reliability of the heat conservation systems;\n - Safety critical procedures (administrative control);\n - Safety critical check valves;\n - Pipeline protection (if relevant);\n - The reasoning for the chosen sectionalisation of the process;\n - The relief valve schedule;\n - PSD response time.\n\nThe dynamic simulation model(s) used for the simulations of the Inadvertent valve opening (IVO) and Choke collapse (CC) scenarios, e.g. the Olga model, shall be delivered and shall represent the As built design of wells, flowlines and topside piping." ;
                  rdfs:label "Process safety report" ;
                  skos:broadMatch rdl:PCA_100006687 ,
                                  rdl:PCA_100006688 ,
                                  rdl:PCA_100006726 ,
                                  rdl:PCA_100006727 ,
                                  rdl:PCA_100006728 ,
                                  rdl:PCA_100006729 ;
                  skos:broader rdl:PCA_100006756 .


###  http://rds.posccaesar.org/ontology/plm/rdl/PCA_100006396
rdl:PCA_100006396 rdf:type owl:Class ;
                  rdfs:subClassOf rdl:PCA_100004908 ;
                  rdl:PCA_100006765 rrdl:CFIHOS-20000013 ,
                                    rrdl:CFIHOS-20000026 ;
                  rdl:PCA_100006768 "The minimum required information for main process safety schematics shall be:\n- Relevant main process equipment\n- Sectionalization valves\n- Pressure protection devices (PRV, PSE, other) with set-point and dimensioning case indicated\n- PSD transmitters\n- Non-return valves of relevance for process safety\n- Depressurization valves\n- Fail safe position of valves\n- Control functions relevant for process safety\n- Pressure and temperature specification\n- Line design pressure and temperature (breaks)\n- Actuated block valves other than ESV and XSV valves (XV)\n- Which disposal system streams are routed to\n- Chemical injection points\n- Drain points (CD)\n- Future system included\n- It is recommended to visualize the blowdown segments (by color-codes)." ;
                  rdfs:comment "The minimum required information for main process safety schematics shall be:\n- Relevant main process equipment\n- Sectionalization valves\n- Pressure protection devices (PRV, PSE, other) with set-point and dimensioning case indicated\n- PSD transmitters\n- Non-return valves of relevance for process safety\n- Depressurization valves\n- Fail safe position of valves\n- Control functions relevant for process safety\n- Pressure and temperature specification\n- Line design pressure and temperature (breaks)\n- Actuated block valves other than ESV and XSV valves (XV)\n- Which disposal system streams are routed to\n- Chemical injection points\n- Drain points (CD)\n- Future system included\n- It is recommended to visualize the blowdown segments (by color-codes)." ;
                  rdfs:label "Process safety schematics" ;
                  skos:broadMatch rdl:PCA_100006727 ;
                  skos:broader rdl:PCA_100006745 .


###  http://rds.posccaesar.org/ontology/plm/rdl/PCA_100006397
rdl:PCA_100006397 rdf:type owl:Class ;
                  rdfs:subClassOf rdl:PCA_100004908 ;
                  rdl:PCA_100006763 "Documentation of the process simulations defining the heat and material balances as basis for design of the plant shall consist of the following two parts:\n1. Executable process simulation files;\n2. The process simulation report.\n\nAll process design cases, i.e. all cases where stream data are used for equipment and line/valve sizing, shall be documented by 1. and 2. above." ;
                  rdl:PCA_100006765 rrdl:CFIHOS-20000026 ;
                  rdl:PCA_100006766 rdl:PCA_100006578 ,
                                    rdl:PCA_100006579 ,
                                    rdl:PCA_100006580 ,
                                    rdl:PCA_100006581 ,
                                    rdl:PCA_100006582 ,
                                    rdl:PCA_100006583 ,
                                    rdl:PCA_100006584 ,
                                    rdl:PCA_100006585 ,
                                    rdl:PCA_100006586 ,
                                    rdl:PCA_100006587 ,
                                    rdl:PCA_100006588 ,
                                    rdl:PCA_100006589 ,
                                    rdl:PCA_100006590 ,
                                    rdl:PCA_100006591 ,
                                    rdl:PCA_100006592 ,
                                    rdl:PCA_100006593 ,
                                    rdl:PCA_100006594 ,
                                    rdl:PCA_100006595 ,
                                    rdl:PCA_100006596 ,
                                    rdl:PCA_100006597 ,
                                    rdl:PCA_100006598 ,
                                    rdl:PCA_100006599 ,
                                    rdl:PCA_100006600 ,
                                    rdl:PCA_100006601 ,
                                    rdl:PCA_100006602 ,
                                    rdl:PCA_100006603 ,
                                    rdl:PCA_100006604 ,
                                    rdl:PCA_100006605 ,
                                    rdl:PCA_100006606 ,
                                    rdl:PCA_100006607 ,
                                    rdl:PCA_100006608 ,
                                    rdl:PCA_100006609 ,
                                    rdl:PCA_100006610 ,
                                    rdl:PCA_100006611 ,
                                    rdl:PCA_100006612 ,
                                    rdl:PCA_100006613 ,
                                    rdl:PCA_100006614 ,
                                    rdl:PCA_100006615 ,
                                    rdl:PCA_100006616 ,
                                    rdl:PCA_100006617 ,
                                    rdl:PCA_100006618 ,
                                    rdl:PCA_100006619 ,
                                    rdl:PCA_100006620 ,
                                    rdl:PCA_100006621 ,
                                    rdl:PCA_100006622 ,
                                    rdl:PCA_100006623 ,
                                    rdl:PCA_100006624 ,
                                    rdl:PCA_100006625 ;
                  rdl:PCA_100006768 "The process simulation report shall as a minimum include:\n - Feed stream descriptions, including the development over the production lifetime;\n - Product specifications;\n - A reasoning for the defined process design cases, e.g.:\n    - Which production situation is represented by each case, and how do the cases together represent the expected operation envelope;\n    - If applicable, which variations are included in the feed stream descriptions to accommodate uncertainties in the feed stream properties and conditions;\n - A description of the calculation models used in the process simulation;\n - Specifications for each unit operation in the process simulations;\n - Summary tables with resulting stream and equipment data. The stream numbers shall coincide with the stream numbers on the PFD's." ;
                  rdfs:comment "The process simulation report shall as a minimum include:\n - Feed stream descriptions, including the development over the production lifetime;\n - Product specifications;\n - A reasoning for the defined process design cases, e.g.:\n    - Which production situation is represented by each case, and how do the cases together represent the expected operation envelope;\n    - If applicable, which variations are included in the feed stream descriptions to accommodate uncertainties in the feed stream properties and conditions;\n - A description of the calculation models used in the process simulation;\n - Specifications for each unit operation in the process simulations;\n - Summary tables with resulting stream and equipment data. The stream numbers shall coincide with the stream numbers on the PFD's." ;
                  rdfs:label "Process simulation reports" ;
                  skos:broadMatch rdl:PCA_100006698 ;
                  skos:broader rdl:PCA_100006756 .


###  http://rds.posccaesar.org/ontology/plm/rdl/PCA_100006398
rdl:PCA_100006398 rdf:type owl:Class ;
                  rdfs:subClassOf rdl:PCA_100004908 ;
                  rdl:PCA_100006763 "One process system engineering manual shall be written for each process system (e.g. oil separation system, gas compression system, open drain system, freshwater system, flare system, etc.). The objective of the manuals is to describe and document the design and operation of the system." ;
                  rdl:PCA_100006765 rrdl:CFIHOS-20000026 ;
                  rdl:PCA_100006766 rdl:PCA_100006578 ,
                                    rdl:PCA_100006579 ,
                                    rdl:PCA_100006580 ,
                                    rdl:PCA_100006581 ,
                                    rdl:PCA_100006582 ,
                                    rdl:PCA_100006583 ,
                                    rdl:PCA_100006584 ,
                                    rdl:PCA_100006585 ,
                                    rdl:PCA_100006586 ,
                                    rdl:PCA_100006587 ,
                                    rdl:PCA_100006588 ,
                                    rdl:PCA_100006589 ,
                                    rdl:PCA_100006590 ,
                                    rdl:PCA_100006591 ,
                                    rdl:PCA_100006592 ,
                                    rdl:PCA_100006593 ,
                                    rdl:PCA_100006594 ,
                                    rdl:PCA_100006595 ,
                                    rdl:PCA_100006596 ,
                                    rdl:PCA_100006597 ,
                                    rdl:PCA_100006598 ,
                                    rdl:PCA_100006599 ,
                                    rdl:PCA_100006600 ,
                                    rdl:PCA_100006601 ,
                                    rdl:PCA_100006602 ,
                                    rdl:PCA_100006603 ,
                                    rdl:PCA_100006604 ,
                                    rdl:PCA_100006605 ,
                                    rdl:PCA_100006606 ,
                                    rdl:PCA_100006607 ,
                                    rdl:PCA_100006608 ,
                                    rdl:PCA_100006609 ,
                                    rdl:PCA_100006610 ,
                                    rdl:PCA_100006611 ,
                                    rdl:PCA_100006612 ,
                                    rdl:PCA_100006613 ,
                                    rdl:PCA_100006614 ,
                                    rdl:PCA_100006615 ,
                                    rdl:PCA_100006616 ,
                                    rdl:PCA_100006617 ,
                                    rdl:PCA_100006618 ,
                                    rdl:PCA_100006619 ,
                                    rdl:PCA_100006620 ,
                                    rdl:PCA_100006621 ,
                                    rdl:PCA_100006622 ,
                                    rdl:PCA_100006623 ,
                                    rdl:PCA_100006624 ,
                                    rdl:PCA_100006625 ,
                                    rdl:PCA_100006627 ,
                                    rdl:PCA_100006628 ;
                  rdl:PCA_100006768 "Table of contents:\n\n1    Objective and target group\n2    System description \n2.1    Introduction\n2.2    Design basis\n2.3    Process description\n2.4    Utility systems, chemicals and catalyst requirements\n2.5    Analysis (sampling points, etc.)\n2.6    HSE requirements\n3    System operation, including process control \n3.1    Normal operation\n3.2    Normal start-up\n3.3    Normal shut down\n3.4    Special operations\n3.5    Routine operations\n4    Maintenance\n4.1    Depressurization and flushing\n4.2    Maintenance\n5    System protection \n5.1    Premises\n5.2    Process and emergency shut-down functions\n5.3    Specific equipment protection\n5.4    Pressure safety equipment (relief valves, rupture disks, etc.)\n5.5    Car seals, key locks and key interlocks\n6    Specific design solutions\n7    Technical data, calculations and drawings \n8    Additional information \n8.1    Definitions and abbreviations\n8.2    Changes from previous version\n8.3    References\n\nSection 4 shall describe maintenance sequence, including how to shut down and drain equipment and parts of the system, relevant conclusions from HAZOP and other evaluations, and any other relevant considerations; reference to supplier documentation for individual equipment maintenance procedures can be done in addition.\n\nSection 5 shall include a list of all the isolation valves located in the pressure-relief system piping which could isolate pressure relief valves in the system. The required position and the reason for the lock or the seal shall be included.\n\nSection 6 shall give details about the specific design solutions chosen for equipment, instrumentation and materials. The reasoning behind the specific design solutions shall also be given in this section, e.g. the reason for choosing a specific level control instrument, the specific compressor configuration, the specific heat exchanger configuration etc. Any limitations to the operation caused by the e.g. the material selection or e.g. the design capacity shall be explained in this section. This could be low or high temperature limitations, throughput limitations for heat exchangers, operating conditions which reduce the lifetime of an equipment unit etc.\n\nSection 7 shall include the relevant technical data, calculations and drawings not covered by a reference to a separate document in section 8.3.\n\nSection 8.2 shall be used to log the performed modifications affecting the described system design and operation. For a new built installation this section will be empty. For a modification this section shall describe the changes resulting from the modification only once, i.e. changes between the versions issued internally throughout the modification project shall not be commented." ;
                  rdfs:comment "Table of contents:\n\n1    Objective and target group\n2    System description \n2.1    Introduction\n2.2    Design basis\n2.3    Process description\n2.4    Utility systems, chemicals and catalyst requirements\n2.5    Analysis (sampling points, etc.)\n2.6    HSE requirements\n3    System operation, including process control \n3.1    Normal operation\n3.2    Normal start-up\n3.3    Normal shut down\n3.4    Special operations\n3.5    Routine operations\n4    Maintenance\n4.1    Depressurization and flushing\n4.2    Maintenance\n5    System protection \n5.1    Premises\n5.2    Process and emergency shut-down functions\n5.3    Specific equipment protection\n5.4    Pressure safety equipment (relief valves, rupture disks, etc.)\n5.5    Car seals, key locks and key interlocks\n6    Specific design solutions\n7    Technical data, calculations and drawings \n8    Additional information \n8.1    Definitions and abbreviations\n8.2    Changes from previous version\n8.3    References\n\nSection 4 shall describe maintenance sequence, including how to shut down and drain equipment and parts of the system, relevant conclusions from HAZOP and other evaluations, and any other relevant considerations; reference to supplier documentation for individual equipment maintenance procedures can be done in addition.\n\nSection 5 shall include a list of all the isolation valves located in the pressure-relief system piping which could isolate pressure relief valves in the system. The required position and the reason for the lock or the seal shall be included.\n\nSection 6 shall give details about the specific design solutions chosen for equipment, instrumentation and materials. The reasoning behind the specific design solutions shall also be given in this section, e.g. the reason for choosing a specific level control instrument, the specific compressor configuration, the specific heat exchanger configuration etc. Any limitations to the operation caused by the e.g. the material selection or e.g. the design capacity shall be explained in this section. This could be low or high temperature limitations, throughput limitations for heat exchangers, operating conditions which reduce the lifetime of an equipment unit etc.\n\nSection 7 shall include the relevant technical data, calculations and drawings not covered by a reference to a separate document in section 8.3.\n\nSection 8.2 shall be used to log the performed modifications affecting the described system design and operation. For a new built installation this section will be empty. For a modification this section shall describe the changes resulting from the modification only once, i.e. changes between the versions issued internally throughout the modification project shall not be commented." ;
                  rdfs:label "Process system engineering manuals" ;
                  skos:broadMatch rdl:PCA_100006688 ;
                  skos:broader rdl:PCA_100006749 ,
                               rdl:PCA_100006754 .


###  http://rds.posccaesar.org/ontology/plm/rdl/PCA_100006399
rdl:PCA_100006399 rdf:type owl:Class ;
                  rdfs:subClassOf rdl:PCA_100004908 ;
                  rdl:PCA_100006763 "To summarize the equipment’s capacities and limitations." ;
                  rdl:PCA_100006765 rrdl:CFIHOS-20000031 ;
                  rdl:PCA_100006766 rdl:PCA_100006653 ;
                  rdl:PCA_100006768 "A structured data form containing part number/model, design information, operational data and limitations of the equipment. Data sheets are only applicable for instruments and valves." ;
                  rdfs:comment "A structured data form containing part number/model, design information, operational data and limitations of the equipment. Data sheets are only applicable for instruments and valves." ;
                  rdfs:label "Product data sheet" ;
                  skos:broadMatch rdl:PCA_100006686 ;
                  skos:broader rdl:PCA_100006747 .


###  http://rds.posccaesar.org/ontology/plm/rdl/PCA_100006400
rdl:PCA_100006400 rdf:type owl:Class ;
                  rdfs:subClassOf rdl:PCA_100004908 ;
                  rdl:PCA_100006763 "Document shall give the user a structured setup on how to document the setting of parameters for given protection." ;
                  rdl:PCA_100006765 rrdl:CFIHOS-20000013 ;
                  rdl:PCA_100006766 rdl:PCA_100006653 ;
                  rdl:PCA_100006768 "The document shall contain a template including all adjustable parameters, indicating which parameters are fixed by the project. For parameters which have individual setting the criteria/formula for defining/calculating the individual setting shall be given. In addition the document shall include a table listing all individual settings. This table shall on one axis list all equipment and the other all parameter requiring individual setting." ;
                  rdfs:comment "The document shall contain a template including all adjustable parameters, indicating which parameters are fixed by the project. For parameters which have individual setting the criteria/formula for defining/calculating the individual setting shall be given. In addition the document shall include a table listing all individual settings. This table shall on one axis list all equipment and the other all parameter requiring individual setting." ;
                  rdfs:label "Protective device setting list" ;
                  skos:broadMatch rdl:PCA_100006716 ;
                  skos:broader rdl:PCA_100006748 .


###  http://rds.posccaesar.org/ontology/plm/rdl/PCA_100006401
rdl:PCA_100006401 rdf:type owl:Class ;
                  rdfs:subClassOf rdl:PCA_100004908 ;
                  rdl:PCA_100006763 "Assembled report for verification of procedures followed and delivery according to bending procedure" ;
                  rdl:PCA_100006766 rdl:PCA_100006653 ;
                  rdl:PCA_100006768 "Bending results/report (including dimensions and material)" ;
                  rdfs:comment "Bending results/report (including dimensions and material)" ;
                  rdfs:label "Qualification dossier for bending" ;
                  skos:broadMatch rdl:PCA_100006722 ;
                  skos:broader rdl:PCA_100006756 .


###  http://rds.posccaesar.org/ontology/plm/rdl/PCA_100006402
rdl:PCA_100006402 rdf:type owl:Class ;
                  rdfs:subClassOf rdl:PCA_100004908 ;
                  rdl:PCA_100006763 "Describe the tests in sufficient detail enabling the test team to execute the tests." ;
                  rdl:PCA_100006765 rrdl:CFIHOS-20000031 ;
                  rdl:PCA_100006766 rdl:PCA_100006653 ;
                  rdl:PCA_100006768 "Procedure describing the tests to be performed to qualify equipment in accordance design requirements and specified acceptance criteria. In many equipment standards this is called Performance Validation Test (PVT)." ;
                  rdfs:comment "Procedure describing the tests to be performed to qualify equipment in accordance design requirements and specified acceptance criteria. In many equipment standards this is called Performance Validation Test (PVT)." ;
                  rdfs:label "Qualification test procedure" ;
                  skos:broadMatch rdl:PCA_100006688 ;
                  skos:broader rdl:PCA_100006751 .


###  http://rds.posccaesar.org/ontology/plm/rdl/PCA_100006403
rdl:PCA_100006403 rdf:type owl:Class ;
                  rdfs:subClassOf rdl:PCA_100004908 ;
                  rdl:PCA_100006763 "Document the qualification test results." ;
                  rdl:PCA_100006765 rrdl:CFIHOS-20000031 ;
                  rdl:PCA_100006766 rdl:PCA_100006653 ;
                  rdl:PCA_100006768 "Report from the qualification tests based on the procedure." ;
                  rdfs:comment "Report from the qualification tests based on the procedure." ;
                  rdfs:label "Qualification test records / report" ;
                  skos:broadMatch rdl:PCA_100006722 ;
                  skos:broader rdl:PCA_100006756 .


###  http://rds.posccaesar.org/ontology/plm/rdl/PCA_100006404
rdl:PCA_100006404 rdf:type owl:Class ;
                  rdfs:subClassOf rdl:PCA_100004908 ;
                  rdl:PCA_100006763 "Describes the quantitative risk analysis performed for the pipeline system, covering all risk elements related to the pipeline. The reason for location and spacing of safety valves shall be included." ;
                  rdl:PCA_100006765 rrdl:CFIHOS-20000018 ;
                  rdl:PCA_100006766 rdl:PCA_100006654 ;
                  rdfs:label "Qualitative risk analysis report" ;
                  skos:broadMatch rdl:PCA_100006664 ;
                  skos:broader rdl:PCA_100006756 .


###  http://rds.posccaesar.org/ontology/plm/rdl/PCA_100006405
rdl:PCA_100006405 rdf:type owl:Class ;
                  rdfs:subClassOf rdl:PCA_100004908 ;
                  rdl:PCA_100006763 "This document provides information concerning the planned verification activities performed by manufacturer, purchaser and third party." ;
                  rdl:PCA_100006765 rrdl:CFIHOS-20000027 ;
                  rdl:PCA_100006766 rdl:PCA_100006653 ;
                  rdl:PCA_100006768 "The Quality Plan shall provide manufacturer compliance with quality standards, procedures and specifications" ;
                  rdfs:comment "The Quality Plan shall provide manufacturer compliance with quality standards, procedures and specifications" ;
                  rdfs:label "Quality plan" ;
                  skos:broadMatch rdl:PCA_100006672 .


###  http://rds.posccaesar.org/ontology/plm/rdl/PCA_100006406
rdl:PCA_100006406 rdf:type owl:Class ;
                  rdfs:subClassOf rdl:PCA_100004908 ;
                  rdl:PCA_100006765 rrdl:CFIHOS-20000030 ;
                  rdl:PCA_100006766 rdl:PCA_100006640 ;
                  rdl:PCA_100006768 "Calculation of radar coverage." ;
                  rdfs:comment "Calculation of radar coverage." ;
                  rdfs:label "Radar coverage calculations" ;
                  skos:broadMatch rdl:PCA_100006687 ;
                  skos:broader rdl:PCA_100006741 .


###  http://rds.posccaesar.org/ontology/plm/rdl/PCA_100006407
rdl:PCA_100006407 rdf:type owl:Class ;
                  rdfs:subClassOf rdl:PCA_100004908 ;
                  rdl:PCA_100006763 "Radio link budget calculations that have been used for design of radio links shall be provided." ;
                  rdl:PCA_100006765 rrdl:CFIHOS-20000030 ;
                  rdfs:label "Radio link budget calculations" ;
                  skos:broadMatch rdl:PCA_100006687 ;
                  skos:broader rdl:PCA_100006741 .


###  http://rds.posccaesar.org/ontology/plm/rdl/PCA_100006408
rdl:PCA_100006408 rdf:type owl:Class ;
                  rdfs:subClassOf rdl:PCA_100004908 ;
                  rdl:PCA_100006763 "Document reliability availability and maintainability for selected equipment and components to meet the levels of intended use as specified." ;
                  rdl:PCA_100006765 rrdl:CFIHOS-20000031 ;
                  rdl:PCA_100006766 rdl:PCA_100006653 ;
                  rdl:PCA_100006768 "Report providing the reliability availability and maintainability analysis performed for equipment and components." ;
                  rdfs:comment "Report providing the reliability availability and maintainability analysis performed for equipment and components." ;
                  rdfs:label "RAM analysis" ;
                  skos:broadMatch rdl:PCA_100006727 .


###  http://rds.posccaesar.org/ontology/plm/rdl/PCA_100006409
rdl:PCA_100006409 rdf:type owl:Class ;
                  rdfs:subClassOf rdl:PCA_100004908 ;
                  rdl:PCA_100006763 "A close out report shall be delivered to document the work performed." ;
                  rdl:PCA_100006765 rrdl:CFIHOS-20000018 ;
                  rdl:PCA_100006766 rdl:PCA_100006654 ;
                  rdl:PCA_100006768 "All records and documents produced as a result of the monitoring and control requirements and the acceptance criteria shall, on completion of the work, be compiled into a Closeout Report.\n\nThe Closeout Report shall be divided into sections as follows:\nSection 1\nThis section shall give an introduction, general description of the system made ready for operation, list the chemicals used and describe the purpose of - and the structure of the Closeout Report.\nSection 2\nThis section shall contain the reports from the RFO operations. It shall contain summaries of events for all the operations and associated field operational paperwork.\nSection 3\nThis section shall contain all the operational procedures and field queries (FQs) for the operations associated with the RFO operations.\nSection 4\nThis section shall contain the RFO Contractors daily reports generated at the different sites where activities have been performed. These reports shall contain the day-by-day activities, , an environmental report listing the volumes of chemicals on site and a radioactive isotope form, listing the amount of isotopes in the field." ;
                  rdfs:comment "All records and documents produced as a result of the monitoring and control requirements and the acceptance criteria shall, on completion of the work, be compiled into a Closeout Report.\n\nThe Closeout Report shall be divided into sections as follows:\nSection 1\nThis section shall give an introduction, general description of the system made ready for operation, list the chemicals used and describe the purpose of - and the structure of the Closeout Report.\nSection 2\nThis section shall contain the reports from the RFO operations. It shall contain summaries of events for all the operations and associated field operational paperwork.\nSection 3\nThis section shall contain all the operational procedures and field queries (FQs) for the operations associated with the RFO operations.\nSection 4\nThis section shall contain the RFO Contractors daily reports generated at the different sites where activities have been performed. These reports shall contain the day-by-day activities, , an environmental report listing the volumes of chemicals on site and a radioactive isotope form, listing the amount of isotopes in the field." ;
                  rdfs:label "Ready for operation (RFO) close out report" ;
                  skos:broader rdl:PCA_100006756 .


###  http://rds.posccaesar.org/ontology/plm/rdl/PCA_100006410
rdl:PCA_100006410 rdf:type owl:Class ;
                  rdfs:subClassOf rdl:PCA_100004908 ;
                  rdl:PCA_100006763 "See requirement for protection and discrimination coordination study, ref. (Z-001-0052 - Electrical calculations / analyses)." ;
                  rdl:PCA_100006765 rrdl:CFIHOS-20000008 ;
                  rdl:PCA_100006766 rdl:PCA_100006634 ,
                                    rdl:PCA_100006635 ,
                                    rdl:PCA_100006636 ,
                                    rdl:PCA_100006637 ,
                                    rdl:PCA_100006638 ,
                                    rdl:PCA_100006639 ;
                  rdl:PCA_100006768 "The Relay setting table is part of the \"Protection and discrimination study\" \n\nWhere practical, the relay setting table shall be made similar as \"Parameter setting tables\", i.e. combination of templates and setting tables for parameters with individual setting." ;
                  rdfs:comment "The Relay setting table is part of the \"Protection and discrimination study\" \n\nWhere practical, the relay setting table shall be made similar as \"Parameter setting tables\", i.e. combination of templates and setting tables for parameters with individual setting." ;
                  rdfs:label "Relay setting table" ;
                  skos:broadMatch rdl:PCA_100006701 ;
                  skos:broader rdl:PCA_100006762 .


###  http://rds.posccaesar.org/ontology/plm/rdl/PCA_100006411
rdl:PCA_100006411 rdf:type owl:Class ;
                  rdfs:subClassOf rdl:PCA_100004908 ;
                  rdl:PCA_100006763 "To define the detailed steps required to repair or abandon a pipeline, riser or umbilical." ;
                  rdl:PCA_100006765 rrdl:CFIHOS-20000031 ;
                  rdl:PCA_100006766 rdl:PCA_100006657 ;
                  rdl:PCA_100006768 "Outline description and method statement for required actions to repair or abandon a pipeline, riser or umbilical during or after installation." ;
                  rdfs:comment "Outline description and method statement for required actions to repair or abandon a pipeline, riser or umbilical during or after installation." ;
                  rdfs:label "Repair & abandonment procedure" ;
                  skos:broadMatch rdl:PCA_100006688 ;
                  skos:broader rdl:PCA_100006751 .


###  http://rds.posccaesar.org/ontology/plm/rdl/PCA_100006412
rdl:PCA_100006412 rdf:type owl:Class ;
                  rdfs:subClassOf rdl:PCA_100004908 ;
                  rdl:PCA_100006763 "Ensure safe operation" ;
                  rdl:PCA_100006765 rrdl:CFIHOS-20000018 ;
                  rdl:PCA_100006766 rdl:PCA_100006654 ;
                  rdl:PCA_100006768 "Repair philosophy for pipelines shall be delivered, fulfilling the requirements DVGL-ST-F101." ;
                  rdfs:comment "Repair philosophy for pipelines shall be delivered, fulfilling the requirements DVGL-ST-F101." ;
                  rdfs:label "Repair philosophy" ;
                  skos:broader rdl:PCA_100006752 .


###  http://rds.posccaesar.org/ontology/plm/rdl/PCA_100006413
rdl:PCA_100006413 rdf:type owl:Class ;
                  rdfs:subClassOf rdl:PCA_100004908 ;
                  rdl:PCA_100006763 "Document providing information about noise levels." ;
                  rdl:PCA_100006765 rrdl:CFIHOS-20000011 ,
                                    rrdl:CFIHOS-20000014 ;
                  rdl:PCA_100006766 rdl:PCA_100006653 ;
                  rdl:PCA_100006768 "Noise and vibration data shall be reported" ;
                  rdfs:comment "Noise and vibration data shall be reported" ;
                  rdfs:label "Report - Noise test - HSE" ;
                  skos:broadMatch rdl:PCA_100006722 ;
                  skos:broader rdl:PCA_100006756 .


###  http://rds.posccaesar.org/ontology/plm/rdl/PCA_100006414
rdl:PCA_100006414 rdf:type owl:Class ;
                  rdfs:subClassOf rdl:PCA_100004908 ;
                  rdl:PCA_100006763 "Ensure safe operation" ;
                  rdl:PCA_100006765 rrdl:CFIHOS-20000018 ;
                  rdl:PCA_100006766 rdl:PCA_100006657 ;
                  rdl:PCA_100006768 "Riser hang off drawings covering hang off of subsea lines to offshore installations." ;
                  rdfs:comment "Riser hang off drawings covering hang off of subsea lines to offshore installations." ;
                  rdfs:label "Riser hang off drawings" ;
                  skos:broader rdl:PCA_100006746 .


###  http://rds.posccaesar.org/ontology/plm/rdl/PCA_100006415
rdl:PCA_100006415 rdf:type owl:Class ;
                  rdfs:subClassOf rdl:PCA_100004908 ;
                  rdl:PCA_100006765 rrdl:CFIHOS-20000010 ,
                                    rrdl:CFIHOS-20000011 ,
                                    rrdl:CFIHOS-20000013 ;
                  rdl:PCA_100006766 rdl:PCA_100006654 ;
                  rdl:PCA_100006768 "The report shall contain a full quantitative risk assessment of all identified hazards contributing to the total risk picture for personnel, environment and third party, for the facility in operations (including Area Risk charts)." ;
                  rdfs:comment "The report shall contain a full quantitative risk assessment of all identified hazards contributing to the total risk picture for personnel, environment and third party, for the facility in operations (including Area Risk charts)." ;
                  rdfs:label "Risk analysis" ;
                  skos:broadMatch rdl:PCA_100006726 ,
                                  rdl:PCA_100006727 ,
                                  rdl:PCA_100006728 ;
                  skos:broader rdl:PCA_100006756 .


###  http://rds.posccaesar.org/ontology/plm/rdl/PCA_100006416
rdl:PCA_100006416 rdf:type owl:Class ;
                  rdfs:subClassOf rdl:PCA_100004908 ;
                  rdl:PCA_100006765 rrdl:CFIHOS-20000007 ;
                  rdl:PCA_100006766 rdl:PCA_100006656 ;
                  rdl:PCA_100006768 "All system, arrangement, layout, plan, alignment, section and detail drawings shall be included.  Location, direction, type of signpost and reference to signpost data sheet shall be shown on layout drawings." ;
                  rdfs:comment "All system, arrangement, layout, plan, alignment, section and detail drawings shall be included.  Location, direction, type of signpost and reference to signpost data sheet shall be shown on layout drawings." ;
                  rdfs:label "Road drawings" ;
                  skos:broadMatch rdl:PCA_100006708 ;
                  skos:broader rdl:PCA_100006746 .


###  http://rds.posccaesar.org/ontology/plm/rdl/PCA_100006417
rdl:PCA_100006417 rdf:type owl:Class ;
                  rdfs:subClassOf rdl:PCA_100004908 ;
                  rdl:PCA_100006763 "Ensure safe operation" ;
                  rdl:PCA_100006765 rrdl:CFIHOS-20000018 ;
                  rdl:PCA_100006766 rdl:PCA_100006654 ;
                  rdl:PCA_100006768 "Survey reports and data shall comply with Company's requirements." ;
                  rdfs:comment "Survey reports and data shall comply with Company's requirements." ;
                  rdfs:label "Rock installation survey reports and data" ;
                  skos:broadMatch rdl:PCA_100006705 ;
                  skos:broader rdl:PCA_100006756 ,
                               rdl:PCA_100006762 .


###  http://rds.posccaesar.org/ontology/plm/rdl/PCA_100006418
rdl:PCA_100006418 rdf:type owl:Class ;
                  rdfs:subClassOf rdl:PCA_100004908 ;
                  rdl:PCA_100006763 "Document verifying tested characteristics of a certain object." ;
                  rdl:PCA_100006766 rdl:PCA_100006653 ;
                  rdl:PCA_100006768 "Mandatory content of information:\n - Date of testing\n - Signature of person responsible for test\n - Object identification (type, series number, etc.)\n - Measured values.\n\nOptional content of information:\n - Test equipment / instruments used\n - Reference to test procedure\n - Conclusion." ;
                  rdfs:comment "Mandatory content of information:\n - Date of testing\n - Signature of person responsible for test\n - Object identification (type, series number, etc.)\n - Measured values.\n\nOptional content of information:\n - Test equipment / instruments used\n - Reference to test procedure\n - Conclusion." ;
                  rdfs:label "Routine test report" ;
                  skos:broadMatch rdl:PCA_100006722 ;
                  skos:broader rdl:PCA_100006756 .


###  http://rds.posccaesar.org/ontology/plm/rdl/PCA_100006419
rdl:PCA_100006419 rdf:type owl:Class ;
                  rdfs:subClassOf rdl:PCA_100004908 ;
                  rdl:PCA_100006763 "To provide basis for laying and seabed intervention design report." ;
                  rdl:PCA_100006765 rrdl:CFIHOS-20000031 ;
                  rdl:PCA_100006766 rdl:PCA_100006656 ;
                  rdl:PCA_100006768 "Drawing showing the pipeline, riser or umbilical route." ;
                  rdfs:comment "Drawing showing the pipeline, riser or umbilical route." ;
                  rdfs:label "Routing design" ;
                  skos:broadMatch rdl:PCA_100006689 ;
                  skos:broader rdl:PCA_100006756 .


###  http://rds.posccaesar.org/ontology/plm/rdl/PCA_100006420
rdl:PCA_100006420 rdf:type owl:Class ;
                  rdfs:subClassOf rdl:PCA_100004908 ;
                  rdl:PCA_100006763 "To verify ROV access for subsea operations defined in the ROV task list." ;
                  rdl:PCA_100006765 rrdl:CFIHOS-20000031 ;
                  rdl:PCA_100006766 rdl:PCA_100006654 ;
                  rdl:PCA_100006768 "Report based on verification of ROV access in the 3D design model. The report includes 3D model pictures." ;
                  rdfs:comment "Report based on verification of ROV access in the 3D design model. The report includes 3D model pictures." ;
                  rdfs:label "ROV access verification report" ;
                  skos:broader rdl:PCA_100006756 .


###  http://rds.posccaesar.org/ontology/plm/rdl/PCA_100006421
rdl:PCA_100006421 rdf:type owl:Class ;
                  rdfs:subClassOf rdl:PCA_100004908 ;
                  rdl:PCA_100006763 "The ROV marking drawing shall identify all marking on the specified objects that are applicable for the ROV intervention work. The ROV marking shall be easily readable on an A3 drawing." ;
                  rdl:PCA_100006765 rrdl:CFIHOS-20000031 ;
                  rdfs:label "ROV marking drawings" ;
                  skos:broadMatch rdl:PCA_100006710 ;
                  skos:broader rdl:PCA_100006746 .


###  http://rds.posccaesar.org/ontology/plm/rdl/PCA_100006422
rdl:PCA_100006422 rdf:type owl:Class ;
                  rdfs:subClassOf rdl:PCA_100004908 ;
                  rdl:PCA_100006763 "Give an overview of all foreseen ROV intervention to enable planning of intervention and ROV access verification." ;
                  rdl:PCA_100006765 rrdl:CFIHOS-20000031 ;
                  rdl:PCA_100006766 rdl:PCA_100006654 ;
                  rdl:PCA_100006768 "A list documenting all foreseen subsea operations requiring ROV intervention." ;
                  rdfs:comment "A list documenting all foreseen subsea operations requiring ROV intervention." ;
                  rdfs:label "ROV task list" ;
                  skos:broadMatch rdl:PCA_100006688 ;
                  skos:broader rdl:PCA_100006751 .


###  http://rds.posccaesar.org/ontology/plm/rdl/PCA_100006423
rdl:PCA_100006423 rdf:type owl:Class ;
                  rdfs:subClassOf rdl:PCA_100004908 ;
                  rdl:PCA_100006763 "Required by the SAS supplier to configure his communication lines prior to test activities" ;
                  rdl:PCA_100006765 rrdl:CFIHOS-20000027 ;
                  rdl:PCA_100006766 rdl:PCA_100006653 ;
                  rdl:PCA_100006768 "This document shall include SAS communication interface test procedure (UFAT)" ;
                  rdfs:comment "This document shall include SAS communication interface test procedure (UFAT)" ;
                  rdfs:label "Safety and automation system (SAS) communication interface test procedure (UFAT)" ;
                  skos:broadMatch rdl:PCA_100006722 ;
                  skos:broader rdl:PCA_100006751 .


###  http://rds.posccaesar.org/ontology/plm/rdl/PCA_100006424
rdl:PCA_100006424 rdf:type owl:Class ;
                  rdfs:subClassOf rdl:PCA_100004908 ;
                  rdl:PCA_100006763 "Required by the SAS supplier to configure his communication lines prior to test activities" ;
                  rdl:PCA_100006765 rrdl:CFIHOS-20000027 ;
                  rdl:PCA_100006766 rdl:PCA_100006653 ;
                  rdl:PCA_100006768 "This document shall include SAS communication test report (UFAT)" ;
                  rdfs:comment "This document shall include SAS communication test report (UFAT)" ;
                  rdfs:label "Safety and automation system (SAS) communication test report (UFAT)" ;
                  skos:broadMatch rdl:PCA_100006722 ;
                  skos:broader rdl:PCA_100006756 .


###  http://rds.posccaesar.org/ontology/plm/rdl/PCA_100006425
rdl:PCA_100006425 rdf:type owl:Class ;
                  rdfs:subClassOf rdl:PCA_100004908 ;
                  rdl:PCA_100006763 "A structured form containing information on the safety, health and environmental protection aspects of the chemical, including protective measures and emergency actions.\n\nISO 11014 Safety data sheet for chemical products." ;
                  rdl:PCA_100006765 rrdl:CFIHOS-20000013 ;
                  rdl:PCA_100006766 rdl:PCA_100006653 ;
                  rdl:PCA_100006768 "A structured form containing information on the safety, health and environmental protection aspects of the material, including protective measures and\nemergency actions.\nSDS shall be according to local/national regulations  and in the official language plant is/will be operated, or in English if accepted by local authorities.\nA collection of Safety Data Sheets (SDS) shall be delivered to Company, for chemicals delivered as part of equipment, as first fill or used for preservation before operation.\nExceptions are\n - grease\n - fat\n - surface preservatives\n - coatings\n - oils in volume per equipment below 10 litres.\nThe report shall include one SDS per unique chemical trade name. A cross reference table with each unique chemical trade name, equipment tag number(s) and SDS file name shall also be included." ;
                  rdfs:comment "A structured form containing information on the safety, health and environmental protection aspects of the material, including protective measures and\nemergency actions.\nSDS shall be according to local/national regulations  and in the official language plant is/will be operated, or in English if accepted by local authorities.\nA collection of Safety Data Sheets (SDS) shall be delivered to Company, for chemicals delivered as part of equipment, as first fill or used for preservation before operation.\nExceptions are\n - grease\n - fat\n - surface preservatives\n - coatings\n - oils in volume per equipment below 10 litres.\nThe report shall include one SDS per unique chemical trade name. A cross reference table with each unique chemical trade name, equipment tag number(s) and SDS file name shall also be included." ;
                  rdfs:label "Safety data sheet" ;
                  skos:broadMatch rdl:PCA_100006686 ;
                  skos:broader rdl:PCA_100006747 .


###  http://rds.posccaesar.org/ontology/plm/rdl/PCA_100006426
rdl:PCA_100006426 rdf:type owl:Class ;
                  rdfs:subClassOf rdl:PCA_100004908 ;
                  rdl:PCA_100006765 rrdl:CFIHOS-20000010 ,
                                    rrdl:CFIHOS-20000011 ,
                                    rrdl:CFIHOS-20000013 ;
                  rdl:PCA_100006766 rdl:PCA_100006656 ;
                  rdl:PCA_100006768 "The drawings shall be prepared in accordance with the requirements below.\n\nThere shall be sufficient main equipment on the drawing to easily identify the location of the equipment in question. Safety layout drawings should as far as possible use the same basis/background as other layout drawings. All equipment listed below shall be identified by:\n - Tag code;\n - Approximate dimension and geometrical form of tag.\n\nThe following safety arrangement drawings and diagrams shall be produced as follows:\n - Escape route drawings; shall include:\n    - Primary escape routes with arrows indicating escape direction;\n    - Secondary escape routes with direction;\n    - Muster and embarkment areas;\n    - Evacuation means (e.g.: lifeboats, escape chutes and rafts);\n    - Areas for first aid treatment;\n - Safety equipment layout:\n    - First aid equipment;\n    - Safety equipment (e.g.: life jackets, life buoys, rescue equipment, MOB boat);\n    - Emergency showers;\n    - Emergency phones;\n - Safety sign layout:\n    - Location of signs;\n    - Signpost schedule including fixing details for signposts and signs;\n - Active fire protection equipment layout:\n    - Location of active fire protection units (e.g. deluge, sprinkler, foam, gaseous units);\n    - Manual firefighting equipment (e.g.: hydrants, hose reels, extinguishers);\n    - Monitor;\n - Passive fire protection and blast protection:\n    - Location of fire divisions (fire walls, deck segregation) including size and direction of dimensioning load;\n    - Location of explosion resistant walls including size and direction of dimensioning load;\n    - Location of explosion overpressure ventilation outlet;\n - Fire and gas detection layout:\n    - Fire and gas detectors with elevation and in addition direction of view including angle up/down for flame detectors;\n    - Manual Call buttons;\n    - Manual active fire protection release buttons;\n    - Manual ESD buttons;\n    - Manual Electrical Isolation buttons (MEI), isolation of high voltage electrical equipment;\n    - Warning lights, and other alarm devices." ;
                  rdfs:comment "The drawings shall be prepared in accordance with the requirements below.\n\nThere shall be sufficient main equipment on the drawing to easily identify the location of the equipment in question. Safety layout drawings should as far as possible use the same basis/background as other layout drawings. All equipment listed below shall be identified by:\n - Tag code;\n - Approximate dimension and geometrical form of tag.\n\nThe following safety arrangement drawings and diagrams shall be produced as follows:\n - Escape route drawings; shall include:\n    - Primary escape routes with arrows indicating escape direction;\n    - Secondary escape routes with direction;\n    - Muster and embarkment areas;\n    - Evacuation means (e.g.: lifeboats, escape chutes and rafts);\n    - Areas for first aid treatment;\n - Safety equipment layout:\n    - First aid equipment;\n    - Safety equipment (e.g.: life jackets, life buoys, rescue equipment, MOB boat);\n    - Emergency showers;\n    - Emergency phones;\n - Safety sign layout:\n    - Location of signs;\n    - Signpost schedule including fixing details for signposts and signs;\n - Active fire protection equipment layout:\n    - Location of active fire protection units (e.g. deluge, sprinkler, foam, gaseous units);\n    - Manual firefighting equipment (e.g.: hydrants, hose reels, extinguishers);\n    - Monitor;\n - Passive fire protection and blast protection:\n    - Location of fire divisions (fire walls, deck segregation) including size and direction of dimensioning load;\n    - Location of explosion resistant walls including size and direction of dimensioning load;\n    - Location of explosion overpressure ventilation outlet;\n - Fire and gas detection layout:\n    - Fire and gas detectors with elevation and in addition direction of view including angle up/down for flame detectors;\n    - Manual Call buttons;\n    - Manual active fire protection release buttons;\n    - Manual ESD buttons;\n    - Manual Electrical Isolation buttons (MEI), isolation of high voltage electrical equipment;\n    - Warning lights, and other alarm devices." ;
                  rdfs:label "Safety layout drawings" ;
                  skos:broadMatch rdl:PCA_100006708 ;
                  skos:broader rdl:PCA_100006746 .


###  http://rds.posccaesar.org/ontology/plm/rdl/PCA_100006427
rdl:PCA_100006427 rdf:type owl:Class ;
                  rdfs:subClassOf rdl:PCA_100004908 ;
                  rdl:PCA_100006763 "Supplier SIL documentation (Safety Manual, Certificate, etc) shall be provided for devices and assemblies/SIS sub-systems when part of a Safety Instrumented Function.\n\nThe supplier SIL documentation provides the necessary information about how to safely apply a device or assembly/SIS-subsystem and integrate it into a complete safety instrumented function. It addresses operation, maintenance, failure rates and other reliability data, fault detection and constraints associated with the device or assembly for the intended configurations and operating environment." ;
                  rdl:PCA_100006765 rrdl:CFIHOS-20000013 ;
                  rdl:PCA_100006768 "For standard off-the-shelf devices and assemblies/SIS sub-systems, the above documents should be delivered as supplier standard documents (project specific content minimized). Traceability between specific model/variant/configuration delivered with those covered in the standard document shall be ensured. To achieve this, it is good practice to mark-up the relevant parts of the standard document that apply to the specific delivery. \n\nDevice/component: \nFor IEC 61508 compliant devices the following supplier SIL documentation shall be delivered:\n - Safety Manual in accordance with IEC 61508\n - Certificate of compliance with IEC 61508 from recognized 3rd party certification body\n - Assessment report from 3rd party (as referred to in the certificate)\n\n For non-compliant devices, a Safety Manual (and evt. other complementary documents) shall be delivered in accordance with IEC 61511 and including underlying information supporting the claimed performance. For components claimed to be proven in use in accordance with IEC 61508, the documentary evidence shall be supplied (ref IEC 61508-2 sub clause 7.4.10).\n\n Assembly /SIS sub-system: For assemblies/SIS sub-systems within scope of delivery, a Safety Manual in accordance with IEC 61511 shall address the complete assembly. The SIL documentation for the devices forming part of the assembly shall be delivered (incl. from sub-suppliers) and all referred device SIL documents shall be delivered or attached to the assembly safety manual." ;
                  rdfs:comment "For standard off-the-shelf devices and assemblies/SIS sub-systems, the above documents should be delivered as supplier standard documents (project specific content minimized). Traceability between specific model/variant/configuration delivered with those covered in the standard document shall be ensured. To achieve this, it is good practice to mark-up the relevant parts of the standard document that apply to the specific delivery. \n\nDevice/component: \nFor IEC 61508 compliant devices the following supplier SIL documentation shall be delivered:\n - Safety Manual in accordance with IEC 61508\n - Certificate of compliance with IEC 61508 from recognized 3rd party certification body\n - Assessment report from 3rd party (as referred to in the certificate)\n\n For non-compliant devices, a Safety Manual (and evt. other complementary documents) shall be delivered in accordance with IEC 61511 and including underlying information supporting the claimed performance. For components claimed to be proven in use in accordance with IEC 61508, the documentary evidence shall be supplied (ref IEC 61508-2 sub clause 7.4.10).\n\n Assembly /SIS sub-system: For assemblies/SIS sub-systems within scope of delivery, a Safety Manual in accordance with IEC 61511 shall address the complete assembly. The SIL documentation for the devices forming part of the assembly shall be delivered (incl. from sub-suppliers) and all referred device SIL documents shall be delivered or attached to the assembly safety manual." ;
                  rdfs:label "Safety manual" ;
                  skos:broadMatch rdl:PCA_100006727 ;
                  skos:broader rdl:PCA_100006749 .


###  http://rds.posccaesar.org/ontology/plm/rdl/PCA_100006428
rdl:PCA_100006428 rdf:type owl:Class ;
                  rdfs:subClassOf rdl:PCA_100004908 ;
                  rdl:PCA_100006763 "The Safety Strategy describes how risks are to be managed based on the outcome of a systematic identification and evaluation of the hazards and effects which may arise on the actual installation." ;
                  rdl:PCA_100006765 rrdl:CFIHOS-20000010 ,
                                    rrdl:CFIHOS-20000011 ,
                                    rrdl:CFIHOS-20000013 ;
                  rdl:PCA_100006766 rdl:PCA_100006654 ;
                  rdl:PCA_100006768 "The Safety Strategy shall outline the design principles for layout, configuration, arrangement and the selection and role of safety barriers to be implemented to manage risk. The strategy shall include the Fire and Explosion Strategy (FES), the Emergency, Evacuation and Rescue Strategy (EER), the ESD philosophy, F&G detection philosophy and other high-level design and operational aspects related to safety barriers.\n\nThe Safety Strategy shall reflect installation specific conditions, including, but not limited to, environment and climate, competence of staff, cultural elements, infrastructure such as transport, external emergency preparedness resources, telecommunications, health care, availability of water supplies and electricity etc. The Safety Strategy shall document both general and area-specific strategies to manage risk." ;
                  rdfs:comment "The Safety Strategy shall outline the design principles for layout, configuration, arrangement and the selection and role of safety barriers to be implemented to manage risk. The strategy shall include the Fire and Explosion Strategy (FES), the Emergency, Evacuation and Rescue Strategy (EER), the ESD philosophy, F&G detection philosophy and other high-level design and operational aspects related to safety barriers.\n\nThe Safety Strategy shall reflect installation specific conditions, including, but not limited to, environment and climate, competence of staff, cultural elements, infrastructure such as transport, external emergency preparedness resources, telecommunications, health care, availability of water supplies and electricity etc. The Safety Strategy shall document both general and area-specific strategies to manage risk." ;
                  rdfs:label "Safety strategy and performance standards" ;
                  skos:broadMatch rdl:PCA_100006726 ,
                                  rdl:PCA_100006727 ,
                                  rdl:PCA_100006728 ;
                  skos:broader rdl:PCA_100006758 ,
                               rdl:PCA_100006759 .


###  http://rds.posccaesar.org/ontology/plm/rdl/PCA_100006429
rdl:PCA_100006429 rdf:type owl:Class ;
                  rdfs:subClassOf rdl:PCA_100004908 ;
                  rdl:PCA_100006763 "Satellite link budget calculations (signal level and attenuation in dB) that have been used for design of satellite hops shall be provided." ;
                  rdl:PCA_100006765 rrdl:CFIHOS-20000030 ;
                  rdfs:label "Satellite link budget calculations" ;
                  skos:broadMatch rdl:PCA_100006687 ;
                  skos:broader rdl:PCA_100006741 .


###  http://rds.posccaesar.org/ontology/plm/rdl/PCA_100006430
rdl:PCA_100006430 rdf:type owl:Class ;
                  rdfs:subClassOf rdl:PCA_100004908 ;
                  rdl:PCA_100006763 "This document shall provide Electrical/Electronic/Pneumatic/Hydraulic functionality  information e.g. to provide hook-up information and  component details for e.g. modifications/replacement." ;
                  rdl:PCA_100006766 rdl:PCA_100006653 ;
                  rdl:PCA_100006768 "To be prepared for valve assemblies with instrumentation, and control panels. All components and interconnection between units to be identified. External connections and interfaces shall be identified with type and size." ;
                  rdfs:comment "To be prepared for valve assemblies with instrumentation, and control panels. All components and interconnection between units to be identified. External connections and interfaces shall be identified with type and size." ;
                  rdfs:label "Schematics including hook-up information" ;
                  skos:broadMatch rdl:PCA_100006712 ,
                                  rdl:PCA_100006713 ;
                  skos:broader rdl:PCA_100006744 ,
                               rdl:PCA_100006746 .


###  http://rds.posccaesar.org/ontology/plm/rdl/PCA_100006431
rdl:PCA_100006431 rdf:type owl:Class ;
                  rdfs:subClassOf rdl:PCA_100004908 ;
                  rdl:PCA_100006763 "A drawing showing equipment and tools supplied including part numbers." ;
                  rdl:PCA_100006765 rrdl:CFIHOS-20000031 ;
                  rdl:PCA_100006766 rdl:PCA_100006653 ;
                  rdl:PCA_100006768 "An illustration providing holistic understanding of equipment, listing quantity and type" ;
                  rdfs:comment "An illustration providing holistic understanding of equipment, listing quantity and type" ;
                  rdfs:label "Scope of supply" ;
                  skos:broader rdl:PCA_100006748 .


###  http://rds.posccaesar.org/ontology/plm/rdl/PCA_100006432
rdl:PCA_100006432 rdf:type owl:Class ;
                  rdfs:subClassOf rdl:PCA_100004908 ;
                  rdl:PCA_100006763 "An illustration providing holistic understanding of equipment, listing quantity and type." ;
                  rdl:PCA_100006764 "The scope of supply / work drawing contain an overview of equipments and the borderline between contractor' s scope of supply / work and others." ;
                  rdl:PCA_100006765 rrdl:CFIHOS-20000031 ;
                  rdl:PCA_100006766 rdl:PCA_100006653 ;
                  rdl:PCA_100006768 "A drawing showing equipment and tools supplied including part numbers." ;
                  rdfs:comment "A drawing showing equipment and tools supplied including part numbers." ;
                  rdfs:label "Scope of supply drawing" ;
                  skos:broader rdl:PCA_100006746 .


###  http://rds.posccaesar.org/ontology/plm/rdl/PCA_100006433
rdl:PCA_100006433 rdf:type owl:Class ;
                  rdfs:subClassOf rdl:PCA_100004908 ;
                  rdl:PCA_100006763 "Design report describing all seabed intervention, pre-and post lay, along the pipeline route including crossings and intervention related to pipeline structures." ;
                  rdl:PCA_100006764 "More details. Survey reports and data shall comply with Company's requirements for Onshore/Offshore surveys." ;
                  rdl:PCA_100006765 rrdl:CFIHOS-20000018 ;
                  rdl:PCA_100006766 rdl:PCA_100006654 ;
                  rdfs:label "Seabed & topographic survey reports and data" ;
                  skos:broadMatch rdl:PCA_100006705 ;
                  skos:broader rdl:PCA_100006756 ,
                               rdl:PCA_100006762 .


###  http://rds.posccaesar.org/ontology/plm/rdl/PCA_100006434
rdl:PCA_100006434 rdf:type owl:Class ;
                  rdfs:subClassOf rdl:PCA_100004908 ;
                  rdl:PCA_100006763 "To provide basis for planning pipeline, riser or umbilical installation. Provide input to analysis and installation procedure." ;
                  rdl:PCA_100006765 rrdl:CFIHOS-20000018 ;
                  rdl:PCA_100006766 rdl:PCA_100006657 ;
                  rdl:PCA_100006768 "Report describing the required seabed intervention for the chosen routing." ;
                  rdfs:comment "Report describing the required seabed intervention for the chosen routing." ;
                  rdfs:label "Seabed intervention design report" ;
                  skos:broadMatch rdl:PCA_100006686 ;
                  skos:broader rdl:PCA_100006756 .


###  http://rds.posccaesar.org/ontology/plm/rdl/PCA_100006435
rdl:PCA_100006435 rdf:type owl:Class ;
                  rdfs:subClassOf rdl:PCA_100004908 ;
                  rdl:PCA_100006763 "To provide basis for planning pipeline, riser or umbilical installation. Provide input to analysis and installation procedure." ;
                  rdl:PCA_100006765 rrdl:CFIHOS-20000018 ;
                  rdl:PCA_100006766 rdl:PCA_100006657 ;
                  rdl:PCA_100006768 "Report describing the required seabed intervention for the chosen routing." ;
                  rdfs:comment "Report describing the required seabed intervention for the chosen routing." ;
                  rdfs:label "Seebed intervention report" ;
                  skos:broader rdl:PCA_100006756 .


###  http://rds.posccaesar.org/ontology/plm/rdl/PCA_100006436
rdl:PCA_100006436 rdf:type owl:Class ;
                  rdfs:subClassOf rdl:PCA_100004908 ;
                  rdl:PCA_100006763 "To provide basis for laying operations and seabed intervention report." ;
                  rdl:PCA_100006765 rrdl:CFIHOS-20000031 ;
                  rdl:PCA_100006766 rdl:PCA_100006657 ;
                  rdl:PCA_100006768 "Document how a pipeline or umbilical approaches onshore." ;
                  rdfs:comment "Document how a pipeline or umbilical approaches onshore." ;
                  rdfs:label "Shore approach" ;
                  skos:broader rdl:PCA_100006746 .


###  http://rds.posccaesar.org/ontology/plm/rdl/PCA_100006437
rdl:PCA_100006437 rdf:type owl:Class ;
                  rdfs:subClassOf rdl:PCA_100004908 ;
                  rdl:PCA_100006763 "The purpose of the \"Shutdown hierarchy\" diagrams is to give an overview of the different shutdown levels and present the levels in a hierarchical way.  Refer to NORSOK S-001 chapter 11.4.3 fig. 4 for a typical shutdown hierarchy for ESD." ;
                  rdl:PCA_100006765 rrdl:CFIHOS-20000015 ;
                  rdl:PCA_100006766 rdl:PCA_100006626 ,
                                    rdl:PCA_100006633 ,
                                    rdl:PCA_100006634 ,
                                    rdl:PCA_100006635 ,
                                    rdl:PCA_100006636 ,
                                    rdl:PCA_100006637 ,
                                    rdl:PCA_100006638 ,
                                    rdl:PCA_100006639 ,
                                    rdl:PCA_100006641 ;
                  rdfs:label "Shutdown hierarchy" ;
                  skos:broadMatch rdl:PCA_100006727 ;
                  skos:broader rdl:PCA_100006745 .


###  http://rds.posccaesar.org/ontology/plm/rdl/PCA_100006438
rdl:PCA_100006438 rdf:type owl:Class ;
                  rdfs:subClassOf rdl:PCA_100004908 ;
                  rdl:PCA_100006763 "Document acceptable level of SIL according to requirements." ;
                  rdl:PCA_100006765 rrdl:CFIHOS-20000031 ;
                  rdl:PCA_100006766 rdl:PCA_100006657 ;
                  rdl:PCA_100006768 "Document the assessments and input provided to establish required safety integrity levels." ;
                  rdfs:comment "Document the assessments and input provided to establish required safety integrity levels." ;
                  rdfs:label "SIL report" ;
                  skos:broader rdl:PCA_100006756 .


###  http://rds.posccaesar.org/ontology/plm/rdl/PCA_100006439
rdl:PCA_100006439 rdf:type owl:Class ;
                  rdfs:subClassOf rdl:PCA_100004908 ;
                  rdl:PCA_100006763 "For equipment packages the single line diagram shall show the main circuits and components in the electrical distribution system." ;
                  rdl:PCA_100006765 rrdl:CFIHOS-20000008 ;
                  rdl:PCA_100006768 "The drawing shall contain identification of and main data for the components within the equipment." ;
                  rdfs:comment "The drawing shall contain identification of and main data for the components within the equipment." ;
                  rdfs:label "Single line diagram (supplier)" ;
                  skos:broadMatch rdl:PCA_100006702 ;
                  skos:broader rdl:PCA_100006745 .


###  http://rds.posccaesar.org/ontology/plm/rdl/PCA_100006440
rdl:PCA_100006440 rdf:type owl:Class ;
                  rdfs:subClassOf rdl:PCA_100004908 ;
                  rdl:PCA_100006763 "The single line index shall cover all voltage levels including \"no break\" system (UPS), instrumentation and telecommunication. The index shall include all necessary information to enable the complete tracing of power distribution network, up/down and between main distribution boards to the consumer, including transformers, UPS, Central telecom equipment and instrument panels/cabinets/controls.\n\nThis shall include sub-distribution boards and junction boxes." ;
                  rdl:PCA_100006765 rrdl:CFIHOS-20000008 ;
                  rdl:PCA_100006766 rdl:PCA_100006634 ,
                                    rdl:PCA_100006635 ,
                                    rdl:PCA_100006636 ,
                                    rdl:PCA_100006637 ,
                                    rdl:PCA_100006638 ,
                                    rdl:PCA_100006639 ;
                  rdl:PCA_100006768 "The following information shall be included:\n - Switchboard or distribution board tag number;\n - Bus id;\n - Circuit id/feeder id;\n - Circuit type;\n - Consumer tag number;\n - Fuse/breaker type and size;\n - Type of consumer;\n - Spare circuits to be registered as such (type: Spare);\n - Description of circuit/feeder. Shall include location / address of consumer as relevant;\n - Cable number;\n - Termination details (including phase) - only for small power distribution;\n - Power and current rating according to datasheets." ;
                  rdfs:comment "The following information shall be included:\n - Switchboard or distribution board tag number;\n - Bus id;\n - Circuit id/feeder id;\n - Circuit type;\n - Consumer tag number;\n - Fuse/breaker type and size;\n - Type of consumer;\n - Spare circuits to be registered as such (type: Spare);\n - Description of circuit/feeder. Shall include location / address of consumer as relevant;\n - Cable number;\n - Termination details (including phase) - only for small power distribution;\n - Power and current rating according to datasheets." ;
                  rdfs:label "Single line index" ;
                  skos:broadMatch rdl:PCA_100006702 ,
                                  rdl:PCA_100006716 ;
                  skos:broader rdl:PCA_100006748 .


###  http://rds.posccaesar.org/ontology/plm/rdl/PCA_100006441
rdl:PCA_100006441 rdf:type owl:Class ;
                  rdfs:subClassOf rdl:PCA_100004908 ;
                  rdl:PCA_100006763 "Documentation shall fulfil the requirements in the standards IEC 61511 and IEC 61508 or Norwegian Oil and Gas guideline 070 as relevant and be developed to suit any lifecycle of a Safety Instrumented System (SIS)." ;
                  rdl:PCA_100006765 rrdl:CFIHOS-20000010 ,
                                    rrdl:CFIHOS-20000011 ,
                                    rrdl:CFIHOS-20000013 ;
                  rdl:PCA_100006766 rdl:PCA_100006626 ,
                                    rdl:PCA_100006627 ,
                                    rdl:PCA_100006628 ,
                                    rdl:PCA_100006633 ;
                  rdl:PCA_100006768 "Functional Safety management Plan (FSMP).\n\nFSMP shall be established addressing all activities of the SIS lifecycle and detailing each phase due to be performed (e.g. project development or operation phase). This shall include a plan for when the activities shall be performed and responsibilities for the different activities. The document shall be made available by the overall SIS compliance responsible, i.e., integrator. \n\n\nSIL Allocation Report.\n\nWith references in analysis of hazards, risks and risks reduction, the determined Safety Instrumented Functions (SIF), allocated Safety Integrity Levels and identified SIS respectively shall be documented in a \"SIL allocation report\" file including an index of all SIF/SIS. \n\n\nLOPA Report.\n\nLayer Of Protection Analysis (LOPA) is a simplified risk-based method that can be applied to allocate SIL requirement to the Safety Instrumented Functions (SIF). LOPA is the preferred method for the SIL allocation of preventive Safety Instrumented Functions. LOPA analysis shall be documented in a report. \n\n\nSafety Requirements Specification (SRS).\n\nSafety Instrumented System (SIS) is developed throughout different lifecycle phases providing an extract of relevant information. The SRS shall focus on main requirements and performance parameters of the SIS while references are made to other documents in order to accomplish a complete overview of all SIS properties.\n\n\nSIL Compliance Report.\n\nThis report including Calculation and Data Dossier (CDD), shall describe methodologies, all data sources applied, calculations and reporting the status of each SIS conformance with main requirements. \n\n\nFunctional Safety Assessment reports. \n\nFSA shall be planned, performed and reported at the relevant project stages as indicated by IEC 61511.\n\nMiscellaneous SIS specific information, examples: \n - Premises for SIS operating and maintenance activities. \n - Identify particular prerequisites and assumptions made as part of SIS design which has to be complied with during the phase of operating the SIS. This shall also include description and procedures of required proof testing (to be prepared prior to and verified during commissioning, readily available to incorporate in plant maintenance program). \n - Guideline for delivery of suppliers SIL documentation (e.g. IEC 61508 compliance certificate, Safety Manual). See also 5.186 SR-2740 Supplier SIL documentation. \n - Reports from the various validation and verification activities including Factory Acceptance Test (FAT) and Site Acceptance test (SAT), a SIS validation record normally issued upon completion of the engineering (by system integrator). \n\n\nFormats for calculation files:\nReports: DOC+ PDF.\nCalculation files (LOPA, SRS, SIL compliance including CDD): Excel (+TBA if commercial software applied)" ;
                  rdfs:comment "Functional Safety management Plan (FSMP).\n\nFSMP shall be established addressing all activities of the SIS lifecycle and detailing each phase due to be performed (e.g. project development or operation phase). This shall include a plan for when the activities shall be performed and responsibilities for the different activities. The document shall be made available by the overall SIS compliance responsible, i.e., integrator. \n\n\nSIL Allocation Report.\n\nWith references in analysis of hazards, risks and risks reduction, the determined Safety Instrumented Functions (SIF), allocated Safety Integrity Levels and identified SIS respectively shall be documented in a \"SIL allocation report\" file including an index of all SIF/SIS. \n\n\nLOPA Report.\n\nLayer Of Protection Analysis (LOPA) is a simplified risk-based method that can be applied to allocate SIL requirement to the Safety Instrumented Functions (SIF). LOPA is the preferred method for the SIL allocation of preventive Safety Instrumented Functions. LOPA analysis shall be documented in a report. \n\n\nSafety Requirements Specification (SRS).\n\nSafety Instrumented System (SIS) is developed throughout different lifecycle phases providing an extract of relevant information. The SRS shall focus on main requirements and performance parameters of the SIS while references are made to other documents in order to accomplish a complete overview of all SIS properties.\n\n\nSIL Compliance Report.\n\nThis report including Calculation and Data Dossier (CDD), shall describe methodologies, all data sources applied, calculations and reporting the status of each SIS conformance with main requirements. \n\n\nFunctional Safety Assessment reports. \n\nFSA shall be planned, performed and reported at the relevant project stages as indicated by IEC 61511.\n\nMiscellaneous SIS specific information, examples: \n - Premises for SIS operating and maintenance activities. \n - Identify particular prerequisites and assumptions made as part of SIS design which has to be complied with during the phase of operating the SIS. This shall also include description and procedures of required proof testing (to be prepared prior to and verified during commissioning, readily available to incorporate in plant maintenance program). \n - Guideline for delivery of suppliers SIL documentation (e.g. IEC 61508 compliance certificate, Safety Manual). See also 5.186 SR-2740 Supplier SIL documentation. \n - Reports from the various validation and verification activities including Factory Acceptance Test (FAT) and Site Acceptance test (SAT), a SIS validation record normally issued upon completion of the engineering (by system integrator). \n\n\nFormats for calculation files:\nReports: DOC+ PDF.\nCalculation files (LOPA, SRS, SIL compliance including CDD): Excel (+TBA if commercial software applied)" ;
                  rdfs:label "SIS functional safety information" ;
                  skos:broadMatch rdl:PCA_100006727 ;
                  skos:broader rdl:PCA_100006753 ,
                               rdl:PCA_100006756 .


###  http://rds.posccaesar.org/ontology/plm/rdl/PCA_100006442
rdl:PCA_100006442 rdf:type owl:Class ;
                  rdfs:subClassOf rdl:PCA_100004908 ;
                  rdl:PCA_100006763 "Provide a step by step procedure and acceptance criteria which will enable user to complete all steps of SIT in logical order." ;
                  rdl:PCA_100006765 rrdl:CFIHOS-20000031 ;
                  rdl:PCA_100006766 rdl:PCA_100006657 ;
                  rdl:PCA_100006768 "Procedure outlining detailed steps and acceptance criteria for all tasks in a system integration test (mechanical fit, verify procedures and personnel familiarization)." ;
                  rdfs:comment "Procedure outlining detailed steps and acceptance criteria for all tasks in a system integration test (mechanical fit, verify procedures and personnel familiarization)." ;
                  rdfs:label "SIT procedure" ;
                  skos:broadMatch rdl:PCA_100006688 ;
                  skos:broader rdl:PCA_100006751 .


###  http://rds.posccaesar.org/ontology/plm/rdl/PCA_100006443
rdl:PCA_100006443 rdf:type owl:Class ;
                  rdfs:subClassOf rdl:PCA_100004908 ;
                  rdl:PCA_100006763 "Document results of SIT." ;
                  rdl:PCA_100006765 rrdl:CFIHOS-20000031 ;
                  rdl:PCA_100006766 rdl:PCA_100006657 ;
                  rdl:PCA_100006768 "The System Integration Testing (SIT) shall document and verify that acceptance testing has been performed in accordance with defined requirements and that these has been met successfully." ;
                  rdfs:comment "The System Integration Testing (SIT) shall document and verify that acceptance testing has been performed in accordance with defined requirements and that these has been met successfully." ;
                  rdfs:label "SIT report" ;
                  skos:broader rdl:PCA_100006756 .


###  http://rds.posccaesar.org/ontology/plm/rdl/PCA_100006444
rdl:PCA_100006444 rdf:type owl:Class ;
                  rdfs:subClassOf rdl:PCA_100004908 ;
                  rdl:PCA_100006765 rrdl:CFIHOS-20000007 ;
                  rdl:PCA_100006766 rdl:PCA_100006656 ;
                  rdl:PCA_100006768 "The Site plan shall be based on a digital terrain model and shall include necessary layers to present (often provided as 2D input):\n - Geotechnical and geological features/strata;\n - Areas with registration of contaminated soil;\n - All plant functional areas/blocks including offsite;\n - Cavern, tunnel and shaft systems;\n - Areas defined for future plant development;\n - Areas that will have to be controlled or restricted during plant operations;\n - Levelled areas as a result of cut and fill;\n - Protective structures at sea, towards river and hinterland;\n - Plant road system including escape routes;\n - Plant main interconnecting pipe racks;\n - Plant fence lines and gates;\n - Outside plant local infrastructure and plant battery limits (roads, railways, port, pipelines, cables and overhead lines, etc.);\n - Permanent lay down and rig areas for future construction and turnaround activities;\n - Construction lay down areas and areas for temporary construction workshops, offices, accommodation, parking and holding areas;\n - Areas for permanent and temporary disposal of surplus materials;\n - Neighbouring settlements and use of land;\n - Areas that shall remain protected or with restriction to access (like nature reserves, historical monuments, archaeological sites);\n - Property borders;\n - Industrial zoning as per authority approvals." ;
                  rdfs:comment "The Site plan shall be based on a digital terrain model and shall include necessary layers to present (often provided as 2D input):\n - Geotechnical and geological features/strata;\n - Areas with registration of contaminated soil;\n - All plant functional areas/blocks including offsite;\n - Cavern, tunnel and shaft systems;\n - Areas defined for future plant development;\n - Areas that will have to be controlled or restricted during plant operations;\n - Levelled areas as a result of cut and fill;\n - Protective structures at sea, towards river and hinterland;\n - Plant road system including escape routes;\n - Plant main interconnecting pipe racks;\n - Plant fence lines and gates;\n - Outside plant local infrastructure and plant battery limits (roads, railways, port, pipelines, cables and overhead lines, etc.);\n - Permanent lay down and rig areas for future construction and turnaround activities;\n - Construction lay down areas and areas for temporary construction workshops, offices, accommodation, parking and holding areas;\n - Areas for permanent and temporary disposal of surplus materials;\n - Neighbouring settlements and use of land;\n - Areas that shall remain protected or with restriction to access (like nature reserves, historical monuments, archaeological sites);\n - Property borders;\n - Industrial zoning as per authority approvals." ;
                  rdfs:label "Site plan" ;
                  skos:broadMatch rdl:PCA_100006705 ;
                  skos:broader rdl:PCA_100006753 .


###  http://rds.posccaesar.org/ontology/plm/rdl/PCA_100006445
rdl:PCA_100006445 rdf:type owl:Class ;
                  rdfs:subClassOf rdl:PCA_100004908 ;
                  rdl:PCA_100006763 "No standardized description is presently available." ;
                  rdl:PCA_100006766 rdl:PCA_100006653 ;
                  rdl:PCA_100006768 "No standardized description is presently available." ;
                  rdfs:comment "No standardized description is presently available." ;
                  rdfs:label "Slewing ring / foundation bolts tension table" .


###  http://rds.posccaesar.org/ontology/plm/rdl/PCA_100006446
rdl:PCA_100006446 rdf:type owl:Class ;
                  rdfs:subClassOf rdl:PCA_100004908 ;
                  rdl:PCA_100006763 "A table showing pre-tensioning / extension for each slewing ring / pedestal adapter / foundation bolts after final assembly shall be delivered." ;
                  rdl:PCA_100006768 "For bolts using pre-tensioning, the table shall include length measurements before and after pre-tensioning including allowable tolerances." ;
                  rdfs:comment "For bolts using pre-tensioning, the table shall include length measurements before and after pre-tensioning including allowable tolerances." ;
                  rdfs:label "Slewing ring/foundation bolts tension table - lifting appliances" ;
                  skos:broadMatch rdl:PCA_100006710 ;
                  skos:broader rdl:PCA_100006748 .


###  http://rds.posccaesar.org/ontology/plm/rdl/PCA_100006447
rdl:PCA_100006447 rdf:type owl:Class ;
                  rdfs:subClassOf rdl:PCA_100004908 ;
                  rdl:PCA_100006763 "Specification that shall provide high level software design information necessary to meet the functional requirements (for a unit or equipment). The specification may include function descriptions, communication protocols, computer system network etc." ;
                  rdl:PCA_100006765 rrdl:CFIHOS-20000031 ;
                  rdl:PCA_100006766 rdl:PCA_100006653 ;
                  rdl:PCA_100006768 "It shall cover the system functionality provided by the software applications, and when necessary also provide hardware details in order to identify direct relationship between hardware and software." ;
                  rdfs:comment "It shall cover the system functionality provided by the software applications, and when necessary also provide hardware details in order to identify direct relationship between hardware and software." ;
                  rdfs:label "Software documentation" ;
                  skos:broadMatch rdl:PCA_100006703 .


###  http://rds.posccaesar.org/ontology/plm/rdl/PCA_100006448
rdl:PCA_100006448 rdf:type owl:Class ;
                  rdfs:subClassOf rdl:PCA_100004908 ;
                  rdl:PCA_100006763 "The Software documentation shall specifically identify the target systems that have been tested." ;
                  rdl:PCA_100006768 "Listing specific HW type, serial numbers, and specific SW version identification." ;
                  rdfs:comment "Listing specific HW type, serial numbers, and specific SW version identification." ;
                  rdfs:label "Software documentation - lifting appliances" .


###  http://rds.posccaesar.org/ontology/plm/rdl/PCA_100006449
rdl:PCA_100006449 rdf:type owl:Class ;
                  rdfs:subClassOf rdl:PCA_100004908 ;
                  rdl:PCA_100006763 "This document shall support design and verification of compliance. Documenting functionality and SW replacement" ;
                  rdl:PCA_100006766 rdl:PCA_100006653 ;
                  rdl:PCA_100006768 "Example of content:\n - Overall system description\n - Subsystem descriptions\n - Program descriptions\n - Module descriptions\n - Data structure descriptions\n - Software environment description." ;
                  rdfs:comment "Example of content:\n - Overall system description\n - Subsystem descriptions\n - Program descriptions\n - Module descriptions\n - Data structure descriptions\n - Software environment description." ;
                  rdfs:label "Software function description" ;
                  skos:broadMatch rdl:PCA_100006703 ;
                  skos:broader rdl:PCA_100006756 .


###  http://rds.posccaesar.org/ontology/plm/rdl/PCA_100006450
rdl:PCA_100006450 rdf:type owl:Class ;
                  rdfs:subClassOf rdl:PCA_100004908 ;
                  rdl:PCA_100006763 "To provide input to pipeline, riser or umbilical design with respect to soil interaction." ;
                  rdl:PCA_100006765 rrdl:CFIHOS-20000018 ;
                  rdl:PCA_100006766 rdl:PCA_100006653 ;
                  rdl:PCA_100006768 "Report documenting all calculations and analysis performed to show how equipment interacts with seabed / soil." ;
                  rdfs:comment "Report documenting all calculations and analysis performed to show how equipment interacts with seabed / soil." ;
                  rdfs:label "Soil interaction report" ;
                  skos:broader rdl:PCA_100006756 .


###  http://rds.posccaesar.org/ontology/plm/rdl/PCA_100006451
rdl:PCA_100006451 rdf:type owl:Class ;
                  rdfs:subClassOf rdl:PCA_100004908 ;
                  rdl:PCA_100006763 "Overview of all spare parts and tools required for operation and maintenance." ;
                  rdl:PCA_100006765 rrdl:CFIHOS-20000018 ;
                  rdl:PCA_100006766 rdl:PCA_100006654 ;
                  rdl:PCA_100006768 "Overview of all spare parts and tools required for operation and maintenance.\nE.g. spare linepipe (with or without coating), spare flexible pipe sections, tools needed during operation such as tools for valve operation." ;
                  rdfs:comment "Overview of all spare parts and tools required for operation and maintenance.\nE.g. spare linepipe (with or without coating), spare flexible pipe sections, tools needed during operation such as tools for valve operation." ;
                  rdfs:label "Spare and tools overview" ;
                  skos:broadMatch rdl:PCA_100006716 ;
                  skos:broader rdl:PCA_100006760 .


###  http://rds.posccaesar.org/ontology/plm/rdl/PCA_100006452
rdl:PCA_100006452 rdf:type owl:Class ;
                  rdfs:subClassOf rdl:PCA_100004908 ;
                  rdl:PCA_100006763 "Table containing list of items specifying the objects (parts, components, software, equipment, etc.) that are available or delivered as spare parts for later use." ;
                  rdl:PCA_100006766 rdl:PCA_100006653 ;
                  rdl:PCA_100006768 "Mandatory content of information:\n - Item reference number\n - Quantity\n - Part number or global identifier (together with manufacturer / supplier)\n - Part name.\n\nOptional content of information:\n - Type designation\n - Specifying technical data\n - Descriptive technical data\n - Mass, dimensions\n - Reference to document\n - Remark." ;
                  rdfs:comment "Mandatory content of information:\n - Item reference number\n - Quantity\n - Part number or global identifier (together with manufacturer / supplier)\n - Part name.\n\nOptional content of information:\n - Type designation\n - Specifying technical data\n - Descriptive technical data\n - Mass, dimensions\n - Reference to document\n - Remark." ;
                  rdfs:label "Spare part list" ;
                  skos:broadMatch rdl:PCA_100006716 ;
                  skos:broader rdl:PCA_100006760 .


###  http://rds.posccaesar.org/ontology/plm/rdl/PCA_100006453
rdl:PCA_100006453 rdf:type owl:Class ;
                  rdfs:subClassOf rdl:PCA_100004908 ;
                  rdl:PCA_100006763 "A spare parts interchangeability record (SPIR) shall be provided for all parts potentially requiring replacement/repair. The SPIR shall support the repair strategy for the equipment units. For bulk and other equipment unit with repair strategy “scrap and replace” only the complete replacement equipment shall be listed in the SPIR." ;
                  rdl:PCA_100006768 "Content shall be in accordance with Company specific requirements." ;
                  rdfs:comment "Content shall be in accordance with Company specific requirements." ;
                  rdfs:label "Spare parts interchangeability register (SPIR)" ;
                  skos:broadMatch rdl:PCA_100006716 ;
                  skos:broader rdl:PCA_100006760 .


###  http://rds.posccaesar.org/ontology/plm/rdl/PCA_100006454
rdl:PCA_100006454 rdf:type owl:Class ;
                  rdfs:subClassOf rdl:PCA_100004908 ;
                  rdl:PCA_100006763 "To verify compliance with the PSA facilities regulations § 62 and NMA Regulations No. 878 in addition to IMO instruments and Class requirements, as applicable." ;
                  rdl:PCA_100006765 rrdl:CFIHOS-20000033 ;
                  rdl:PCA_100006766 rdl:PCA_100006654 ;
                  rdl:PCA_100006768 "A complete stability analyses model shall be delivered with all necessary information required to perform a re-analysis." ;
                  rdfs:comment "A complete stability analyses model shall be delivered with all necessary information required to perform a re-analysis." ;
                  rdfs:label "Stability analysis model" ;
                  skos:broadMatch rdl:PCA_100006687 ;
                  skos:broader rdl:PCA_100006741 ,
                               rdl:PCA_100006762 .


###  http://rds.posccaesar.org/ontology/plm/rdl/PCA_100006455
rdl:PCA_100006455 rdf:type owl:Class ;
                  rdfs:subClassOf rdl:PCA_100004908 ;
                  rdl:PCA_100006763 "The report or collection of reports shall contain the final documentation of intact and damaged stability." ;
                  rdl:PCA_100006765 rrdl:CFIHOS-20000033 ;
                  rdl:PCA_100006766 rdl:PCA_100006654 ;
                  rdl:PCA_100006768 "The report shall typically contain:\n - Vessel particulars and geometrical reference system;\n - Description of watertight integrity and tank arrangement;\n - Lightship weight / weight information;\n - External openings;\n - Densities of liquids in tanks;\n - Applied computer programs;\n - Applicable stability regulations/criteria;\n - Summary of loading conditions;\n - Summary of stability and strength results;\n - Allowable KG limit curves;\n - Hydrostatic table(s);\n - Intact stability documentation;\n - Damage stability documentation." ;
                  rdfs:comment "The report shall typically contain:\n - Vessel particulars and geometrical reference system;\n - Description of watertight integrity and tank arrangement;\n - Lightship weight / weight information;\n - External openings;\n - Densities of liquids in tanks;\n - Applied computer programs;\n - Applicable stability regulations/criteria;\n - Summary of loading conditions;\n - Summary of stability and strength results;\n - Allowable KG limit curves;\n - Hydrostatic table(s);\n - Intact stability documentation;\n - Damage stability documentation." ;
                  rdfs:label "Stability design reports" ;
                  skos:broadMatch rdl:PCA_100006691 ,
                                  rdl:PCA_100006698 ;
                  skos:broader rdl:PCA_100006756 .


###  http://rds.posccaesar.org/ontology/plm/rdl/PCA_100006456
rdl:PCA_100006456 rdf:type owl:Class ;
                  rdfs:subClassOf rdl:PCA_100004908 ;
                  rdl:PCA_100006763 "To document compliance with the PSA facilities regulations § 62 and NMA Regulations No. 878 in addition to IMO instruments and Class requirements, as applicable." ;
                  rdl:PCA_100006765 rrdl:CFIHOS-20000033 ;
                  rdl:PCA_100006766 rdl:PCA_100006654 ;
                  rdl:PCA_100006768 "The manual shall provide the means to calculate the daily loading condition as well as describe the use of the onboard loading computer, if applicable." ;
                  rdfs:comment "The manual shall provide the means to calculate the daily loading condition as well as describe the use of the onboard loading computer, if applicable." ;
                  rdfs:label "Stability operation manual" ;
                  skos:broadMatch rdl:PCA_100006688 ;
                  skos:broader rdl:PCA_100006749 .


###  http://rds.posccaesar.org/ontology/plm/rdl/PCA_100006457
rdl:PCA_100006457 rdf:type owl:Class ;
                  rdfs:subClassOf rdl:PCA_100004908 ;
                  rdl:PCA_100006765 rrdl:CFIHOS-20000031 ;
                  rdl:PCA_100006766 rdl:PCA_100006653 ;
                  rdl:PCA_100006768 "A drawing showing critical interfaces and dimensions for testing, installation and offshore operations." ;
                  rdfs:comment "A drawing showing critical interfaces and dimensions for testing, installation and offshore operations." ;
                  rdfs:label "Stack-up-drawing" ;
                  skos:broadMatch rdl:PCA_100006731 ;
                  skos:broader rdl:PCA_100006746 .


###  http://rds.posccaesar.org/ontology/plm/rdl/PCA_100006458
rdl:PCA_100006458 rdf:type owl:Class ;
                  rdfs:subClassOf rdl:PCA_100004908 ;
                  rdl:PCA_100006763 "If engineering contractor or 3rd party verification body have made a global structural analysis model, then a zip file with input files and FEM files shall be delivered with a short description of each input file." ;
                  rdl:PCA_100006765 rrdl:CFIHOS-20000006 ;
                  rdl:PCA_100006766 rdl:PCA_100006643 ,
                                    rdl:PCA_100006644 ;
                  rdl:PCA_100006768 "It shall be possible to import the files and re-run the entire analysis following a provided step-by-step list. A description on how to import the zip file and run the analysis shall be delivered." ;
                  rdfs:comment "It shall be possible to import the files and re-run the entire analysis following a provided step-by-step list. A description on how to import the zip file and run the analysis shall be delivered." ;
                  rdfs:label "Structural analysis model" ;
                  skos:broadMatch rdl:PCA_100006687 ;
                  skos:broader rdl:PCA_100006741 ,
                               rdl:PCA_100006762 .


###  http://rds.posccaesar.org/ontology/plm/rdl/PCA_100006459
rdl:PCA_100006459 rdf:type owl:Class ;
                  rdfs:subClassOf rdl:PCA_100004908 ;
                  rdl:PCA_100006763 "Structural design reports and input files/parameters shall be delivered. The report or collection of reports shall be self-contained, i.e. provide all information required to re-produce the results." ;
                  rdl:PCA_100006765 rrdl:CFIHOS-20000006 ;
                  rdl:PCA_100006766 rdl:PCA_100006643 ,
                                    rdl:PCA_100006644 ;
                  rdl:PCA_100006768 "The structural design report shall have specific and detailed references to drawings and relevant part of regulations and referenced standards." ;
                  rdfs:comment "The structural design report shall have specific and detailed references to drawings and relevant part of regulations and referenced standards." ;
                  rdfs:label "Structural design report" ;
                  skos:broadMatch rdl:PCA_100006698 ;
                  skos:broader rdl:PCA_100006756 .


###  http://rds.posccaesar.org/ontology/plm/rdl/PCA_100006460
rdl:PCA_100006460 rdf:type owl:Class ;
                  rdfs:subClassOf rdl:PCA_100004908 ;
                  rdl:PCA_100006765 rrdl:CFIHOS-20000006 ;
                  rdl:PCA_100006766 rdl:PCA_100006653 ;
                  rdl:PCA_100006768 "Fabrication drawings for primary and secondary loadbearing structural members including supports for appurtenances (e.g. caissons, conductors, risers) shall be delivered including welds with reference to weld summary index." ;
                  rdfs:comment "Fabrication drawings for primary and secondary loadbearing structural members including supports for appurtenances (e.g. caissons, conductors, risers) shall be delivered including welds with reference to weld summary index." ;
                  rdfs:label "Structural fabrication drawings" ;
                  skos:broadMatch rdl:PCA_100006731 ,
                                  rdl:PCA_100006732 ,
                                  rdl:PCA_100006733 ,
                                  rdl:PCA_100006734 ;
                  skos:broader rdl:PCA_100006746 .


###  http://rds.posccaesar.org/ontology/plm/rdl/PCA_100006461
rdl:PCA_100006461 rdf:type owl:Class ;
                  rdfs:subClassOf rdl:PCA_100004908 ;
                  rdl:PCA_100006765 rrdl:CFIHOS-20000006 ;
                  rdl:PCA_100006766 rdl:PCA_100006653 ;
                  rdl:PCA_100006768 "The following list shows the deliverables and structure of the fabrication records for structural steel and aluminium:\n - As-built Users Guide;\n - Index of design drawings with reference to fabrication drawings;\n - Index of material, design, fabrication, specifications and documents, used by Contractor;\n - Welding procedure specifications;\n - Welding procedure qualification records;\n - Repair procedures and specifications;\n - Weld summary index;\n - Material specification system;\n - Assembly procedures;\n - Production test reports;\n - PWHT reports;\n - Repair and deviation reports;\n - As-built Design Contractor originated design drawings, mark-ups;\n - List of fabrication drawings containing Main Weld numbers;\n - Documentation of rubber coating of j-tubes shall include the following: \n    - Detailed design calculations of thermal insulation requirements, and the development of the insulation aspects of the product, during its lifetime expectancy in service. These calculations shall apply for the components and field joints and take into consideration all the necessary properties including application and installation.\n    - Detailed information about properties of the coating and coating system qualification.\n    - All materials data, test certificates and product data sheets (PDS).\n    - Detailed coating procedure, as a minimum including the information listed in the APS.\n    - Detailed field jointing procedure.\n    - Detailed repair procedure.\n    - Detailed procedures for handling and storage of line-pipe.\n    - Detailed Quality plans / Inspection and Test Plan (ITP). All witness and hold points shall be identified.\n    - Test records and results.\n    - Inspection reports and records.\n    - Repair and recoating records.\n    - All relevant coating application variables.\n    - The personnel qualification record shall constitute proof that the personnel designated to carry out the work are properly qualified to do so.\n\nThe following list shows the deliverables and structure of the fabrication records for Concrete structures:\n - FRB User guide - Describes the content of each deliverable in the FRB and how they relate and refer to each other. Include examples (images) of how to trace welds and material certificates from fabrication drawings;\n - Index of Concrete fabrication and detail drawings;  \n - Index of material, design, fabrication specifications and documents used by Contractor;   \n - Index of Construction sequence drawings, e.g. dry dock, inshore, tow-to field and installation;\n - Reinforcement bar lists;\n - Concrete mix specification (cement, aggregate, inhibitors, etc.);\n - Test records of compression- and tension capacity of actual fabricated concrete;\n - Material certificates reinforcement." ;
                  rdfs:comment "The following list shows the deliverables and structure of the fabrication records for structural steel and aluminium:\n - As-built Users Guide;\n - Index of design drawings with reference to fabrication drawings;\n - Index of material, design, fabrication, specifications and documents, used by Contractor;\n - Welding procedure specifications;\n - Welding procedure qualification records;\n - Repair procedures and specifications;\n - Weld summary index;\n - Material specification system;\n - Assembly procedures;\n - Production test reports;\n - PWHT reports;\n - Repair and deviation reports;\n - As-built Design Contractor originated design drawings, mark-ups;\n - List of fabrication drawings containing Main Weld numbers;\n - Documentation of rubber coating of j-tubes shall include the following: \n    - Detailed design calculations of thermal insulation requirements, and the development of the insulation aspects of the product, during its lifetime expectancy in service. These calculations shall apply for the components and field joints and take into consideration all the necessary properties including application and installation.\n    - Detailed information about properties of the coating and coating system qualification.\n    - All materials data, test certificates and product data sheets (PDS).\n    - Detailed coating procedure, as a minimum including the information listed in the APS.\n    - Detailed field jointing procedure.\n    - Detailed repair procedure.\n    - Detailed procedures for handling and storage of line-pipe.\n    - Detailed Quality plans / Inspection and Test Plan (ITP). All witness and hold points shall be identified.\n    - Test records and results.\n    - Inspection reports and records.\n    - Repair and recoating records.\n    - All relevant coating application variables.\n    - The personnel qualification record shall constitute proof that the personnel designated to carry out the work are properly qualified to do so.\n\nThe following list shows the deliverables and structure of the fabrication records for Concrete structures:\n - FRB User guide - Describes the content of each deliverable in the FRB and how they relate and refer to each other. Include examples (images) of how to trace welds and material certificates from fabrication drawings;\n - Index of Concrete fabrication and detail drawings;  \n - Index of material, design, fabrication specifications and documents used by Contractor;   \n - Index of Construction sequence drawings, e.g. dry dock, inshore, tow-to field and installation;\n - Reinforcement bar lists;\n - Concrete mix specification (cement, aggregate, inhibitors, etc.);\n - Test records of compression- and tension capacity of actual fabricated concrete;\n - Material certificates reinforcement." ;
                  rdfs:label "Structural fabrication records" ;
                  skos:broadMatch rdl:PCA_100006722 ,
                                  rdl:PCA_100006733 ;
                  skos:broader rdl:PCA_100006749 .


###  http://rds.posccaesar.org/ontology/plm/rdl/PCA_100006462
rdl:PCA_100006462 rdf:type owl:Class ;
                  rdfs:subClassOf rdl:PCA_100004908 ;
                  rdl:PCA_100006765 rrdl:CFIHOS-20000006 ;
                  rdl:PCA_100006766 rdl:PCA_100006656 ;
                  rdl:PCA_100006768 "Drawings shall include the following minimum information:\n - Extent and thickness of fireproofing, including description of coating/paint for fire protection systems." ;
                  rdfs:comment "Drawings shall include the following minimum information:\n - Extent and thickness of fireproofing, including description of coating/paint for fire protection systems." ;
                  rdfs:label "Structural fire protection drawings" ;
                  skos:broadMatch rdl:PCA_100006727 ,
                                  rdl:PCA_100006731 ,
                                  rdl:PCA_100006732 ,
                                  rdl:PCA_100006733 ,
                                  rdl:PCA_100006734 ;
                  skos:broader rdl:PCA_100006746 .


###  http://rds.posccaesar.org/ontology/plm/rdl/PCA_100006463
rdl:PCA_100006463 rdf:type owl:Class ;
                  rdfs:subClassOf rdl:PCA_100004908 ;
                  rdl:PCA_100006765 rrdl:CFIHOS-20000006 ;
                  rdl:PCA_100006766 rdl:PCA_100006643 ,
                                    rdl:PCA_100006644 ;
                  rdl:PCA_100006768 "Structural load plans shall be produced." ;
                  rdfs:comment "Structural load plans shall be produced." ;
                  rdfs:label "Structural load plans" ;
                  skos:broadMatch rdl:PCA_100006708 ;
                  skos:broader rdl:PCA_100006753 .


###  http://rds.posccaesar.org/ontology/plm/rdl/PCA_100006464
rdl:PCA_100006464 rdf:type owl:Class ;
                  rdfs:subClassOf rdl:PCA_100004908 ;
                  rdl:PCA_100006765 rrdl:CFIHOS-20000007 ;
                  rdl:PCA_100006766 rdl:PCA_100006643 ;
                  rdl:PCA_100006768 "Structural design reports and input files/parameters shall be delivered. The report or collection of reports shall be self-contained, i.e. provide all information required to re-produce the results.\n\nThe static analysis and calculations shall have specific and detailed references to drawings and relevant part of regulations and referenced standards." ;
                  rdfs:comment "Structural design reports and input files/parameters shall be delivered. The report or collection of reports shall be self-contained, i.e. provide all information required to re-produce the results.\n\nThe static analysis and calculations shall have specific and detailed references to drawings and relevant part of regulations and referenced standards." ;
                  rdfs:label "Structural steel and aluminium structural design report (civil)" ;
                  skos:broadMatch rdl:PCA_100006698 ;
                  skos:broader rdl:PCA_100006756 .


###  http://rds.posccaesar.org/ontology/plm/rdl/PCA_100006465
rdl:PCA_100006465 rdf:type owl:Class ;
                  rdfs:subClassOf rdl:PCA_100004908 ;
                  rdl:PCA_100006765 rrdl:CFIHOS-20000006 ;
                  rdl:PCA_100006766 rdl:PCA_100006656 ;
                  rdl:PCA_100006768 "The following drawings shall be delivered:\n - General notes and specifications;\n - Isometric view (one isometric view per module. Shall cover only main steel and include elevation, grid lines, key plan, north and east references, northing and orientation with respect of true north);\n - General Arrangement (plan and elevation view);\n - Plan, Sections and details;\n - Standard drawings (e.g. grating, railing, staircase, ladder).\n\nEach structural drawing shall contain the following information:\n - Dimensions;\n - Plate thicknesses and section properties;\n - Weld type and size;\n - Material properties;\n - Reference drawings number;\n - Reference to tag number (if relevant);\n - Weight and CoG." ;
                  rdfs:comment "The following drawings shall be delivered:\n - General notes and specifications;\n - Isometric view (one isometric view per module. Shall cover only main steel and include elevation, grid lines, key plan, north and east references, northing and orientation with respect of true north);\n - General Arrangement (plan and elevation view);\n - Plan, Sections and details;\n - Standard drawings (e.g. grating, railing, staircase, ladder).\n\nEach structural drawing shall contain the following information:\n - Dimensions;\n - Plate thicknesses and section properties;\n - Weld type and size;\n - Material properties;\n - Reference drawings number;\n - Reference to tag number (if relevant);\n - Weight and CoG." ;
                  rdfs:label "Structural steel and aluminium. main, secondary and outfitting drawings" ;
                  skos:broadMatch rdl:PCA_100006731 ,
                                  rdl:PCA_100006732 ,
                                  rdl:PCA_100006733 ,
                                  rdl:PCA_100006734 ;
                  skos:broader rdl:PCA_100006746 .


###  http://rds.posccaesar.org/ontology/plm/rdl/PCA_100006466
rdl:PCA_100006466 rdf:type owl:Class ;
                  rdfs:subClassOf rdl:PCA_100004908 ;
                  rdl:PCA_100006768 "The following drawings shall be delivered:\n - Arrangement\n - Typicals\n - Sections and details \nThe drawings shall contain:\n - Dimensions\n - Plate thicknesses and section properties\n - Weld type and size\n - Material properties\n - Reference drawings number\n - Reference to tag number\nStructural load plans shall be produced." ;
                  rdfs:comment "The following drawings shall be delivered:\n - Arrangement\n - Typicals\n - Sections and details \nThe drawings shall contain:\n - Dimensions\n - Plate thicknesses and section properties\n - Weld type and size\n - Material properties\n - Reference drawings number\n - Reference to tag number\nStructural load plans shall be produced." ;
                  rdfs:label "Structural steel and aluminium. main, secondary and outfitting drawings (civil)" ;
                  skos:broadMatch rdl:PCA_100006731 ,
                                  rdl:PCA_100006732 ,
                                  rdl:PCA_100006733 ,
                                  rdl:PCA_100006734 ;
                  skos:broader rdl:PCA_100006746 .


###  http://rds.posccaesar.org/ontology/plm/rdl/PCA_100006467
rdl:PCA_100006467 rdf:type owl:Class ;
                  rdfs:subClassOf rdl:PCA_100004908 ;
                  rdl:PCA_100006765 rrdl:CFIHOS-20000007 ;
                  rdl:PCA_100006766 rdl:PCA_100006656 ;
                  rdl:PCA_100006768 "Drawings shall include the following minimum information:\n - Extent and thickness of fireproofing, including description of coating/paint for fire protection systems;\n - Structural details related to the fire protection;\n - Material properties." ;
                  rdfs:comment "Drawings shall include the following minimum information:\n - Extent and thickness of fireproofing, including description of coating/paint for fire protection systems;\n - Structural details related to the fire protection;\n - Material properties." ;
                  rdfs:label "Structural steel fire protection drawings (civil)" ;
                  skos:broadMatch rdl:PCA_100006727 ,
                                  rdl:PCA_100006731 ,
                                  rdl:PCA_100006732 ,
                                  rdl:PCA_100006733 ,
                                  rdl:PCA_100006734 ;
                  skos:broader rdl:PCA_100006746 .


###  http://rds.posccaesar.org/ontology/plm/rdl/PCA_100006468
rdl:PCA_100006468 rdf:type owl:Class ;
                  rdfs:subClassOf rdl:PCA_100004908 ;
                  rdl:PCA_100006763 "Ensure safe operation" ;
                  rdl:PCA_100006765 rrdl:CFIHOS-20000018 ;
                  rdl:PCA_100006766 rdl:PCA_100006643 ;
                  rdl:PCA_100006768 "Covering design and analysis of pipeline structures such as riser bases, pipeline protection structures, tee/wye assemblies, valve stations, anchor blocks etc.. Basis for analysis, assumptions and assessments not given in design basis shall be included." ;
                  rdfs:comment "Covering design and analysis of pipeline structures such as riser bases, pipeline protection structures, tee/wye assemblies, valve stations, anchor blocks etc.. Basis for analysis, assumptions and assessments not given in design basis shall be included." ;
                  rdfs:label "Structure design report" ;
                  skos:broadMatch rdl:PCA_100006686 ;
                  skos:broader rdl:PCA_100006756 .


###  http://rds.posccaesar.org/ontology/plm/rdl/PCA_100006469
rdl:PCA_100006469 rdf:type owl:Class ;
                  rdfs:subClassOf rdl:PCA_100004908 ;
                  rdl:PCA_100006763 "Specify fabrication requirements for structures." ;
                  rdl:PCA_100006765 rrdl:CFIHOS-20000031 ;
                  rdl:PCA_100006766 rdl:PCA_100006653 ;
                  rdl:PCA_100006768 "Document specifying the methods for fabrication of subsea structures. Includes references to specifications for welding, NDT, assembly, painting, dimensional control, FAT etc." ;
                  rdfs:comment "Document specifying the methods for fabrication of subsea structures. Includes references to specifications for welding, NDT, assembly, painting, dimensional control, FAT etc." ;
                  rdfs:label "Structure fabrication procedure" ;
                  skos:broadMatch rdl:PCA_100006688 ;
                  skos:broader rdl:PCA_100006751 .


###  http://rds.posccaesar.org/ontology/plm/rdl/PCA_100006470
rdl:PCA_100006470 rdf:type owl:Class ;
                  rdfs:subClassOf rdl:PCA_100004908 ;
                  rdl:PCA_100006763 "More details req. Study report for project specific conditions not covered by other design documentation, such as environmental studies, third party activity studies, influence on third party etc.." ;
                  rdl:PCA_100006765 rrdl:CFIHOS-20000018 ;
                  rdl:PCA_100006766 rdl:PCA_100006654 ;
                  rdl:PCA_100006768 "Study Report detailing the final results from the Study (e.g FEED Study Report)" ;
                  rdfs:comment "Study Report detailing the final results from the Study (e.g FEED Study Report)" ;
                  rdfs:label "Study report" ;
                  skos:broader rdl:PCA_100006756 .


###  http://rds.posccaesar.org/ontology/plm/rdl/PCA_100006471
rdl:PCA_100006471 rdf:type owl:Class ;
                  rdfs:subClassOf rdl:PCA_100004908 ;
                  rdl:PCA_100006765 rrdl:CFIHOS-20000031 ;
                  rdl:PCA_100006766 rdl:PCA_100006653 ;
                  rdfs:label "Subsea spool layout drawings" ;
                  skos:broadMatch rdl:PCA_100006708 ,
                                  rdl:PCA_100006731 ,
                                  rdl:PCA_100006732 ,
                                  rdl:PCA_100006733 ,
                                  rdl:PCA_100006734 ;
                  skos:broader rdl:PCA_100006746 .


###  http://rds.posccaesar.org/ontology/plm/rdl/PCA_100006472
rdl:PCA_100006472 rdf:type owl:Class ;
                  rdfs:subClassOf rdl:PCA_100004908 ;
                  rdl:PCA_100006763 "Supports selection of size and schedule (selection table)" ;
                  rdl:PCA_100006766 rdl:PCA_100006653 ;
                  rdl:PCA_100006768 "Divided per pipe class including dimensions and loads." ;
                  rdfs:comment "Divided per pipe class including dimensions and loads." ;
                  rdfs:label "Summary table for mechanical joints (size and type)" ;
                  skos:broadMatch rdl:PCA_100006687 ;
                  skos:broader rdl:PCA_100006748 .


###  http://rds.posccaesar.org/ontology/plm/rdl/PCA_100006473
rdl:PCA_100006473 rdf:type owl:Class ;
                  rdfs:subClassOf rdl:PCA_100004908 ;
                  rdl:PCA_100006763 "Can be input to system calculation and engineering" ;
                  rdl:PCA_100006766 rdl:PCA_100006653 ;
                  rdl:PCA_100006768 "Characteristics and functional parameters shall be documented and performance shall be shown to be probable. This shall include but not be limited to calculations, curves, tables, reference to similar applications and test data. This shall as a minimum be at a level customary for the equipment and to the extent such data are of importance for interfaces to plant and system.                     Lateral analyses and torsion analyses for compressors performance curves for pumps and compressors. Strength calculations, thermal performance and vibration calculations for heat exchangers/pressure vessels." ;
                  rdfs:comment "Characteristics and functional parameters shall be documented and performance shall be shown to be probable. This shall include but not be limited to calculations, curves, tables, reference to similar applications and test data. This shall as a minimum be at a level customary for the equipment and to the extent such data are of importance for interfaces to plant and system.                     Lateral analyses and torsion analyses for compressors performance curves for pumps and compressors. Strength calculations, thermal performance and vibration calculations for heat exchangers/pressure vessels." ;
                  rdfs:label "Supplier calculations" ;
                  skos:broadMatch rdl:PCA_100006687 ;
                  skos:broader rdl:PCA_100006741 .


###  http://rds.posccaesar.org/ontology/plm/rdl/PCA_100006474
rdl:PCA_100006474 rdf:type owl:Class ;
                  rdfs:subClassOf rdl:PCA_100004908 ;
                  rdl:PCA_100006763 "For use by purchaser" ;
                  rdl:PCA_100006766 rdl:PCA_100006653 ;
                  rdl:PCA_100006768 "List of Sub-suppliers" ;
                  rdfs:comment "List of Sub-suppliers" ;
                  rdfs:label "Supplier list" ;
                  skos:broadMatch rdl:PCA_100006663 ;
                  skos:broader rdl:PCA_100006748 .


###  http://rds.posccaesar.org/ontology/plm/rdl/PCA_100006475
rdl:PCA_100006475 rdf:type owl:Class ;
                  rdfs:subClassOf rdl:PCA_100004908 ;
                  rdl:PCA_100006763 "This document is developed by mutual agreement between the Buyer and Seller prior to placement of the Purchase Order (PO) and submitted for approval following PO placement to fully define the list of documents to be issued to Buyer by the Seller. \nThis document provides efficient follow up of documentation deliverables during all phases of manufacturing, installation, testing and handover to operations.\nThe schedule of the delivered documentation shall be aligned with project execution plans." ;
                  rdl:PCA_100006766 rdl:PCA_100006653 ;
                  rdl:PCA_100006768 "This document shall give an overview of documentation relevant for the delivered equipment (PO) and schedule of documents to be delivered.\nDocuments shall be identified with title and document number.\nTo be developed by mutual agreement between the Buyer and Seller prior to placement of the Purchase Order (PO) and submitted for approval following PO placement to fully define the list of documents to be issued to Buyer by the Seller." ;
                  rdfs:comment "This document shall give an overview of documentation relevant for the delivered equipment (PO) and schedule of documents to be delivered.\nDocuments shall be identified with title and document number.\nTo be developed by mutual agreement between the Buyer and Seller prior to placement of the Purchase Order (PO) and submitted for approval following PO placement to fully define the list of documents to be issued to Buyer by the Seller." ;
                  rdfs:label "Supplier master document list" ;
                  skos:broadMatch rdl:PCA_100006660 ;
                  skos:broader rdl:PCA_100006748 .


###  http://rds.posccaesar.org/ontology/plm/rdl/PCA_100006476
rdl:PCA_100006476 rdf:type owl:Class ;
                  rdfs:subClassOf rdl:PCA_100004908 ;
                  rdl:PCA_100006763 "The supplier SIL documentation addresses the safety manual delivery as intended in IEC 61511 and 61508. It provides the necessary information about how to safely apply a component or assembly/system and integrate it into a complete SIS. It addresses design, operation, maintenance, failure rates and other reliability data, fault detection and constraints associated with the component or assembly/system for the intended configurations and operating environment." ;
                  rdl:PCA_100006766 rdl:PCA_100006653 ;
                  rdl:PCA_100006768 "The supplier SIL documentation shall be delivered if the component or system/assembly is part of realizing a safety instrumented function specified in the Safety Requirement Specification (SRS) with SIL requirement.Content requirement for the supplier SIL documentation are given in appendix E3 in NOROG - 070. \n\nSupplier SIL documentation may be delivered under various forms:\n - as single document called Safety Manual, \n - as several documents incl. e.g. a IEC61508 certificate and a Safety Manual \n - or as part of another document." ;
                  rdfs:comment "The supplier SIL documentation shall be delivered if the component or system/assembly is part of realizing a safety instrumented function specified in the Safety Requirement Specification (SRS) with SIL requirement.Content requirement for the supplier SIL documentation are given in appendix E3 in NOROG - 070. \n\nSupplier SIL documentation may be delivered under various forms:\n - as single document called Safety Manual, \n - as several documents incl. e.g. a IEC61508 certificate and a Safety Manual \n - or as part of another document." ;
                  rdfs:label "Supplier SIL documentation" .


###  http://rds.posccaesar.org/ontology/plm/rdl/PCA_100006477
rdl:PCA_100006477 rdf:type owl:Class ;
                  rdfs:subClassOf rdl:PCA_100004908 ;
                  rdl:PCA_100006765 rrdl:CFIHOS-20000033 ;
                  rdl:PCA_100006766 rdl:PCA_100006657 ;
                  rdl:PCA_100006768 "Technical documentation of the swivel stack and all mechanical components of the swivel shall be delivered. This documentation shall include the following:\n - General arrangement drawing;\n - Detail drawings of all major component;\n - Design analyses of all major component;\n - Material certificates for all components including welding filler material along with traceability data;\n - The design loads / swivel interface forces from piping, spools, flexible connections." ;
                  rdfs:comment "Technical documentation of the swivel stack and all mechanical components of the swivel shall be delivered. This documentation shall include the following:\n - General arrangement drawing;\n - Detail drawings of all major component;\n - Design analyses of all major component;\n - Material certificates for all components including welding filler material along with traceability data;\n - The design loads / swivel interface forces from piping, spools, flexible connections." ;
                  rdfs:label "Swivel system report" ;
                  skos:broadMatch rdl:PCA_100006698 ;
                  skos:broader rdl:PCA_100006756 .


###  http://rds.posccaesar.org/ontology/plm/rdl/PCA_100006478
rdl:PCA_100006478 rdf:type owl:Class ;
                  rdfs:subClassOf rdl:PCA_100004908 ;
                  rdl:PCA_100006763 "System documents:\nThe objective of the System documents is to describe the systems at a plant for learning purpose. The System document is a compilation of technical information (LCI), functional descriptions, reason for choice of design and describes the System characteristics, regulate how to operate and protect the System in various conditions. This shall apply to all disciplines within all systems.\n\nThe System documents (S-documents) apply for all systems, subsystems and assemblies. One document shall be produced for each system.\n\nThe main target group for System documents are mainly operational and maintenance personnel at a plant.\n\nThe System documents shall be produced in local language. \n\n\nOperation documents:\nThe objective of the operating documents is to describe how to operate a system and its equipment in a safe, reliable and effective way.\n\nOperation documents (O-documents) apply for all systems, subsystems and assemblies. One Main Operating document shall be produced for each system.\n\nThe \"Main Operating document \"shall contain a compilation (links to detailed O-documents) of operating procedures according to the index structure shown below.\n\nThe operating documents (check lists or operating rules) are formed as action points in tables.\n\nThe black start operating documents shall describe the complete sequence starting with \"black\" installation and ending with main power established. All involved auxiliary systems shall be included and each document shall be related to the Main operating document for each system.\n\nThe initial scenario shall be APS for offshore installations (Abandon Platform Shutdown) or Plant evacuation for onshore plants e.g. after a gas leakage, where gas may have entered non-hazardous areas and rooms. The two alternatives: Black start of emergency power /Essential power and black start of UPS shall be described. In case of cable from shore or other independent unit, such as a national grid, and this power is used as a source of emergency power, this alternative method of black start shall also be described. All Operating documents related to Black start shall be provided with a unique Node number.\n\nThe main target group for Operational document is mainly operational personnel at a plant." ;
                  rdl:PCA_100006765 rrdl:CFIHOS-20000033 ;
                  rdl:PCA_100006766 rdl:PCA_100006578 ,
                                    rdl:PCA_100006579 ,
                                    rdl:PCA_100006580 ,
                                    rdl:PCA_100006581 ,
                                    rdl:PCA_100006582 ,
                                    rdl:PCA_100006583 ,
                                    rdl:PCA_100006584 ,
                                    rdl:PCA_100006585 ,
                                    rdl:PCA_100006586 ,
                                    rdl:PCA_100006587 ,
                                    rdl:PCA_100006588 ,
                                    rdl:PCA_100006589 ,
                                    rdl:PCA_100006590 ,
                                    rdl:PCA_100006591 ,
                                    rdl:PCA_100006592 ,
                                    rdl:PCA_100006593 ,
                                    rdl:PCA_100006594 ,
                                    rdl:PCA_100006595 ,
                                    rdl:PCA_100006596 ,
                                    rdl:PCA_100006597 ,
                                    rdl:PCA_100006598 ,
                                    rdl:PCA_100006599 ,
                                    rdl:PCA_100006600 ,
                                    rdl:PCA_100006601 ,
                                    rdl:PCA_100006602 ,
                                    rdl:PCA_100006603 ,
                                    rdl:PCA_100006604 ,
                                    rdl:PCA_100006605 ,
                                    rdl:PCA_100006606 ,
                                    rdl:PCA_100006607 ,
                                    rdl:PCA_100006608 ,
                                    rdl:PCA_100006609 ,
                                    rdl:PCA_100006610 ,
                                    rdl:PCA_100006611 ,
                                    rdl:PCA_100006612 ,
                                    rdl:PCA_100006613 ,
                                    rdl:PCA_100006614 ,
                                    rdl:PCA_100006615 ,
                                    rdl:PCA_100006616 ,
                                    rdl:PCA_100006617 ,
                                    rdl:PCA_100006618 ,
                                    rdl:PCA_100006619 ,
                                    rdl:PCA_100006620 ,
                                    rdl:PCA_100006621 ,
                                    rdl:PCA_100006622 ,
                                    rdl:PCA_100006623 ,
                                    rdl:PCA_100006624 ,
                                    rdl:PCA_100006625 ,
                                    rdl:PCA_100006626 ,
                                    rdl:PCA_100006627 ,
                                    rdl:PCA_100006628 ,
                                    rdl:PCA_100006629 ,
                                    rdl:PCA_100006630 ,
                                    rdl:PCA_100006631 ,
                                    rdl:PCA_100006632 ,
                                    rdl:PCA_100006633 ,
                                    rdl:PCA_100006634 ,
                                    rdl:PCA_100006635 ,
                                    rdl:PCA_100006636 ,
                                    rdl:PCA_100006637 ,
                                    rdl:PCA_100006638 ,
                                    rdl:PCA_100006639 ,
                                    rdl:PCA_100006640 ,
                                    rdl:PCA_100006641 ,
                                    rdl:PCA_100006642 ;
                  rdl:PCA_100006768 "The index structure of the System documents shall be as follows:\n1  Objective and target group\n2  System description \n2.1  Introduction \n2.2  Design basis \n2.3  Process description \n2.4  Process control\n3  System operation (Opr) (Link to main Operation document for the actual system)\n4  System protection \n4.2  System control\n4.3  Equipment protection \n5  Technical data and drawings\n6  Additional information \n6.1  Definitions and abbreviations \n6.2  Changes from previous version\n6.3  References\n\n\nThe index structure of the main operating document shall be as follows:\nLink to S-document for the actual system\n3    System operation\n3.1  Normal operation\n3.2  Normal start-up\n3.3  Normal shut down\n3.4  Special operations\n3.5  Operational routines \n\nLocal language: YES" ;
                  rdfs:comment "The index structure of the System documents shall be as follows:\n1  Objective and target group\n2  System description \n2.1  Introduction \n2.2  Design basis \n2.3  Process description \n2.4  Process control\n3  System operation (Opr) (Link to main Operation document for the actual system)\n4  System protection \n4.2  System control\n4.3  Equipment protection \n5  Technical data and drawings\n6  Additional information \n6.1  Definitions and abbreviations \n6.2  Changes from previous version\n6.3  References\n\n\nThe index structure of the main operating document shall be as follows:\nLink to S-document for the actual system\n3    System operation\n3.1  Normal operation\n3.2  Normal start-up\n3.3  Normal shut down\n3.4  Special operations\n3.5  Operational routines \n\nLocal language: YES" ;
                  rdfs:label "System and operation documents" ;
                  skos:broadMatch rdl:PCA_100006695 ,
                                  rdl:PCA_100006698 ;
                  skos:broader rdl:PCA_100006750 .


###  http://rds.posccaesar.org/ontology/plm/rdl/PCA_100006479
rdl:PCA_100006479 rdf:type owl:Class ;
                  rdfs:subClassOf rdl:PCA_100004908 ;
                  rdl:PCA_100006763 "System Control Diagram shall be used to specify and document process control and process shutdown application within the control systems.\n\nThe method consists in principle of two parts.\n\n(1) Use of a defined set of function blocks, and\n(2) a diagram representation of usage of these function blocks and its interconnections.\n\nThe diagram has a presentation of the process as background. The content of multiple P&ID’s is simplified and combined into the SCD’s as the control and shutdown logic is laid out there.\n\nSystem Control Diagrams shall be in accordance with the standard referred to in IEC 63131.\n\nThe SCD standard also covers sequential control." ;
                  rdl:PCA_100006765 rrdl:CFIHOS-20000015 ;
                  rdl:PCA_100006766 rdl:PCA_100006578 ,
                                    rdl:PCA_100006579 ,
                                    rdl:PCA_100006580 ,
                                    rdl:PCA_100006581 ,
                                    rdl:PCA_100006582 ,
                                    rdl:PCA_100006583 ,
                                    rdl:PCA_100006584 ,
                                    rdl:PCA_100006585 ,
                                    rdl:PCA_100006586 ,
                                    rdl:PCA_100006587 ,
                                    rdl:PCA_100006588 ,
                                    rdl:PCA_100006589 ,
                                    rdl:PCA_100006590 ,
                                    rdl:PCA_100006591 ,
                                    rdl:PCA_100006592 ,
                                    rdl:PCA_100006593 ,
                                    rdl:PCA_100006594 ,
                                    rdl:PCA_100006595 ,
                                    rdl:PCA_100006596 ,
                                    rdl:PCA_100006597 ,
                                    rdl:PCA_100006598 ,
                                    rdl:PCA_100006599 ,
                                    rdl:PCA_100006600 ,
                                    rdl:PCA_100006601 ,
                                    rdl:PCA_100006602 ,
                                    rdl:PCA_100006603 ,
                                    rdl:PCA_100006604 ,
                                    rdl:PCA_100006605 ,
                                    rdl:PCA_100006606 ,
                                    rdl:PCA_100006607 ,
                                    rdl:PCA_100006608 ,
                                    rdl:PCA_100006609 ,
                                    rdl:PCA_100006610 ,
                                    rdl:PCA_100006611 ,
                                    rdl:PCA_100006612 ,
                                    rdl:PCA_100006613 ,
                                    rdl:PCA_100006614 ,
                                    rdl:PCA_100006615 ,
                                    rdl:PCA_100006616 ,
                                    rdl:PCA_100006617 ,
                                    rdl:PCA_100006618 ,
                                    rdl:PCA_100006619 ,
                                    rdl:PCA_100006620 ,
                                    rdl:PCA_100006621 ,
                                    rdl:PCA_100006622 ,
                                    rdl:PCA_100006623 ,
                                    rdl:PCA_100006624 ,
                                    rdl:PCA_100006625 ,
                                    rdl:PCA_100006626 ,
                                    rdl:PCA_100006627 ,
                                    rdl:PCA_100006628 ,
                                    rdl:PCA_100006633 ;
                  rdl:PCA_100006768 "Main components of a sequence are:\n - Steps with associated actions;\n - Transitions with associated logic conditions;\n - Directed links between steps and transitions.\n\nThe sequential function chart may be presented on separate pages to avoid cluttering the main SCD. \n\nThe SCD’s shall be made per process system and supported by a functional specification." ;
                  rdfs:comment "Main components of a sequence are:\n - Steps with associated actions;\n - Transitions with associated logic conditions;\n - Directed links between steps and transitions.\n\nThe sequential function chart may be presented on separate pages to avoid cluttering the main SCD. \n\nThe SCD’s shall be made per process system and supported by a functional specification." ;
                  rdfs:label "System control diagram (SCD)" ;
                  skos:broadMatch rdl:PCA_100006695 ;
                  skos:broader rdl:PCA_100006745 .


###  http://rds.posccaesar.org/ontology/plm/rdl/PCA_100006480
rdl:PCA_100006480 rdf:type owl:Class ;
                  rdfs:subClassOf rdl:PCA_100004908 ;
                  rdl:PCA_100006763 "The document provides input to the sub-system design and also acts as a verification of operator’s requirements." ;
                  rdl:PCA_100006765 rrdl:CFIHOS-20000031 ;
                  rdl:PCA_100006766 rdl:PCA_100006657 ;
                  rdl:PCA_100006768 "The system design basis includes the overall functional and performance requirements based on operator’s requirements." ;
                  rdfs:comment "The system design basis includes the overall functional and performance requirements based on operator’s requirements." ;
                  rdfs:label "System design basis" ;
                  skos:broadMatch rdl:PCA_100006687 .


###  http://rds.posccaesar.org/ontology/plm/rdl/PCA_100006481
rdl:PCA_100006481 rdf:type owl:Class ;
                  rdfs:subClassOf rdl:PCA_100004908 ;
                  rdl:PCA_100006763 "The complete System Duct & Instrumentation Diagram (D&ID) shall be in accordance with the plants’ process typicals and drafting standard.\n\nThe level of detail within packages shall be identical to that outside.\n\nTag number shall be shown for all tagged components." ;
                  rdl:PCA_100006765 rrdl:CFIHOS-20000019 ;
                  rdl:PCA_100006766 rdl:PCA_100006650 ;
                  rdl:PCA_100006768 "System Duct & Instrument Diagram (D&ID) shall be provided by system and include the following information:\n - All HVAC equipment with their tag number and all HVAC bulk items with their item number;\n - Equipment data summary with tag number for all main equipment such as filters, fans, coils, etc.;\n - All ductwork identified with system no., sizes, duct classes, insulation classes;\n - All inline equipment;\n - Air flow to main areas;\n - Area breaks and duct class breaks;\n - All instrumentation/F&G reflecting the control functions;\n - All instrument locations shall be indicated and completed with tag numbers;\n - Connections to other systems e.g. sea water, heating, cooling, drain, etc.;\n - Airflow in and out of diagram with references." ;
                  rdfs:comment "System Duct & Instrument Diagram (D&ID) shall be provided by system and include the following information:\n - All HVAC equipment with their tag number and all HVAC bulk items with their item number;\n - Equipment data summary with tag number for all main equipment such as filters, fans, coils, etc.;\n - All ductwork identified with system no., sizes, duct classes, insulation classes;\n - All inline equipment;\n - Air flow to main areas;\n - Area breaks and duct class breaks;\n - All instrumentation/F&G reflecting the control functions;\n - All instrument locations shall be indicated and completed with tag numbers;\n - Connections to other systems e.g. sea water, heating, cooling, drain, etc.;\n - Airflow in and out of diagram with references." ;
                  rdfs:label "System duct & instrumentation diagrams (D&ID)" ;
                  skos:broadMatch rdl:PCA_100006696 ;
                  skos:broader rdl:PCA_100006745 .


###  http://rds.posccaesar.org/ontology/plm/rdl/PCA_100006482
rdl:PCA_100006482 rdf:type owl:Class ;
                  rdfs:subClassOf rdl:PCA_100004908 ;
                  rdl:PCA_100006763 "System topology diagram shall show the structure of systems and subsystems to give a functional understanding.\n\nSystem topology diagram shall as a minimum be produced for the following systems:\n - Safety and Automation System;\n - Turbine control system;\n - Fiscal metering system;\n - Drilling system;\n - Subsea system.\n\nIf it is not possible to present all detailed information in a system on one topology drawing, the information shall be split in different detail levels as follows:\n - Overall topology diagram;\n - Detailed topology diagram." ;
                  rdl:PCA_100006765 rrdl:CFIHOS-20000015 ;
                  rdl:PCA_100006766 rdl:PCA_100006594 ,
                                    rdl:PCA_100006595 ,
                                    rdl:PCA_100006596 ,
                                    rdl:PCA_100006597 ,
                                    rdl:PCA_100006598 ,
                                    rdl:PCA_100006599 ,
                                    rdl:PCA_100006600 ,
                                    rdl:PCA_100006601 ,
                                    rdl:PCA_100006602 ,
                                    rdl:PCA_100006603 ,
                                    rdl:PCA_100006604 ,
                                    rdl:PCA_100006605 ,
                                    rdl:PCA_100006606 ,
                                    rdl:PCA_100006607 ,
                                    rdl:PCA_100006608 ,
                                    rdl:PCA_100006609 ,
                                    rdl:PCA_100006610 ,
                                    rdl:PCA_100006611 ,
                                    rdl:PCA_100006612 ,
                                    rdl:PCA_100006613 ,
                                    rdl:PCA_100006614 ,
                                    rdl:PCA_100006615 ,
                                    rdl:PCA_100006616 ,
                                    rdl:PCA_100006617 ,
                                    rdl:PCA_100006618 ,
                                    rdl:PCA_100006619 ,
                                    rdl:PCA_100006620 ,
                                    rdl:PCA_100006621 ,
                                    rdl:PCA_100006622 ,
                                    rdl:PCA_100006623 ,
                                    rdl:PCA_100006624 ,
                                    rdl:PCA_100006625 ,
                                    rdl:PCA_100006626 ,
                                    rdl:PCA_100006627 ,
                                    rdl:PCA_100006628 ,
                                    rdl:PCA_100006631 ,
                                    rdl:PCA_100006633 ,
                                    rdl:PCA_100006634 ,
                                    rdl:PCA_100006635 ,
                                    rdl:PCA_100006636 ,
                                    rdl:PCA_100006637 ,
                                    rdl:PCA_100006638 ,
                                    rdl:PCA_100006639 ,
                                    rdl:PCA_100006641 ;
                  rdl:PCA_100006768 "Typical contents of a detailed topology diagram shall be:\n - All related functional units and subunits represented by blocks including unit tag no and description;\n - Location of units;\n - Interface and network between units shall be indicated;\n - Interface from units to other external systems;\n - Protocol shall be indicated for serial links and for network connections to external system.\n\nBy units is meant but not limited to:\n - Logic solver;\n - Server;\n - Client;\n - Network component (Router, Switch, Firewall);\n - Remote IO." ;
                  rdfs:comment "Typical contents of a detailed topology diagram shall be:\n - All related functional units and subunits represented by blocks including unit tag no and description;\n - Location of units;\n - Interface and network between units shall be indicated;\n - Interface from units to other external systems;\n - Protocol shall be indicated for serial links and for network connections to external system.\n\nBy units is meant but not limited to:\n - Logic solver;\n - Server;\n - Client;\n - Network component (Router, Switch, Firewall);\n - Remote IO." ;
                  rdfs:label "System topology diagrams" ;
                  skos:broadMatch rdl:PCA_100006695 ;
                  skos:broader rdl:PCA_100006745 .


###  http://rds.posccaesar.org/ontology/plm/rdl/PCA_100006483
rdl:PCA_100006483 rdf:type owl:Class ;
                  rdfs:subClassOf rdl:PCA_100004908 ;
                  rdl:PCA_100006763 "Ensure traceability of components" ;
                  rdl:PCA_100006765 rrdl:CFIHOS-20000018 ;
                  rdl:PCA_100006766 rdl:PCA_100006654 ;
                  rdl:PCA_100006768 "To be delivered in accordance with Companys' requirements." ;
                  rdfs:comment "To be delivered in accordance with Companys' requirements." ;
                  rdfs:label "Tag - document cross reference" ;
                  skos:broadMatch rdl:PCA_100006660 ;
                  skos:broader rdl:PCA_100006748 .


###  http://rds.posccaesar.org/ontology/plm/rdl/PCA_100006484
rdl:PCA_100006484 rdf:type owl:Class ;
                  rdfs:subClassOf rdl:PCA_100004908 ;
                  rdl:PCA_100006763 "No standardized description is presently available." ;
                  rdl:PCA_100006766 rdl:PCA_100006653 ;
                  rdl:PCA_100006768 "No standardized description is presently available." ;
                  rdfs:comment "No standardized description is presently available." ;
                  rdfs:label "Tag and equipment list" ;
                  skos:broadMatch rdl:PCA_100006716 ;
                  skos:broader rdl:PCA_100006748 .


###  http://rds.posccaesar.org/ontology/plm/rdl/PCA_100006485
rdl:PCA_100006485 rdf:type owl:Class ;
                  rdfs:subClassOf rdl:PCA_100004908 ;
                  rdl:PCA_100006763 "A list prepared to keep track of all the pipes installed in the wellbore and at which depth they are installed" ;
                  rdl:PCA_100006765 rrdl:CFIHOS-20000042 ;
                  rdl:PCA_100006768 "A list containing details of tubulars that have been prepared for running, or that have been retrieved from the wellbore. \nThe minimum information to be included for the pipe and connection is:\n - Date installed\n - Revision \n - Size \n - Material Grade\n - Prepared by\n - Centralizer depth and type\n - Tubing clamp depht and type\n - Thread type \n - Makeup tourque\n - OD (Outer diameter)\n - ID (Inner diameter)\n - Volumes\n - Run number\n - Description\n - Pipe/Heat number per joint (to ensure full traceability to material certificates) \n - Joint length\n - Cumulative length\n - Depht joint" ;
                  rdfs:comment "A list containing details of tubulars that have been prepared for running, or that have been retrieved from the wellbore. \nThe minimum information to be included for the pipe and connection is:\n - Date installed\n - Revision \n - Size \n - Material Grade\n - Prepared by\n - Centralizer depth and type\n - Tubing clamp depht and type\n - Thread type \n - Makeup tourque\n - OD (Outer diameter)\n - ID (Inner diameter)\n - Volumes\n - Run number\n - Description\n - Pipe/Heat number per joint (to ensure full traceability to material certificates) \n - Joint length\n - Cumulative length\n - Depht joint" ;
                  rdfs:label "Tally" ;
                  skos:broadMatch rdl:PCA_100006722 ;
                  skos:broader rdl:PCA_100006748 .


###  http://rds.posccaesar.org/ontology/plm/rdl/PCA_100006486
rdl:PCA_100006486 rdf:type owl:Class ;
                  rdfs:subClassOf rdl:PCA_100004908 ;
                  rdl:PCA_100006763 "To document compliance with the PSA facilities regulations § 62 and NMA Regulations No. 878 in addition to IMO instruments and Class requirements, as applicable." ;
                  rdl:PCA_100006765 rrdl:CFIHOS-20000033 ;
                  rdl:PCA_100006766 rdl:PCA_100006654 ;
                  rdl:PCA_100006768 "The plan shall include information about capacity and boundaries of all tanks and compartments." ;
                  rdfs:comment "The plan shall include information about capacity and boundaries of all tanks and compartments." ;
                  rdfs:label "Tank plan" ;
                  skos:broadMatch rdl:PCA_100006707 ;
                  skos:broader rdl:PCA_100006753 .


###  http://rds.posccaesar.org/ontology/plm/rdl/PCA_100006487
rdl:PCA_100006487 rdf:type owl:Class ;
                  rdfs:subClassOf rdl:PCA_100004908 ;
                  rdl:PCA_100006763 "Overview of requirements used for design" ;
                  rdl:PCA_100006765 rrdl:CFIHOS-20000018 ;
                  rdl:PCA_100006766 rdl:PCA_100006654 ;
                  rdl:PCA_100006768 "The report shall include requirements not covered by design basis or codes." ;
                  rdfs:comment "The report shall include requirements not covered by design basis or codes." ;
                  rdfs:label "Technical and functional requirements for unbonded flexible pipeline and riser" ;
                  skos:broadMatch rdl:PCA_100006688 ;
                  skos:broader rdl:PCA_100006757 .


###  http://rds.posccaesar.org/ontology/plm/rdl/PCA_100006488
rdl:PCA_100006488 rdf:type owl:Class ;
                  rdfs:subClassOf rdl:PCA_100004908 ;
                  rdl:PCA_100006763 "A technical tag hierarchy shall be established according to Company’s requirements.\n\nThe technical hierarchy describes the technical structure of the installation.  The hierarchy provides an overview of equipment units that belong together technically, and shows the relationship between main equipment, instruments, valves and other related equipment." ;
                  rdl:PCA_100006765 rrdl:CFIHOS-20000001 ;
                  rdl:PCA_100006766 rdl:PCA_100006653 ;
                  rdfs:label "Technical tag hierarchy (TTH)" .


###  http://rds.posccaesar.org/ontology/plm/rdl/PCA_100006489
rdl:PCA_100006489 rdf:type owl:Class ;
                  rdfs:subClassOf rdl:PCA_100004908 ;
                  rdl:PCA_100006763 "Overview of technology development and new technology used in design" ;
                  rdl:PCA_100006765 rrdl:CFIHOS-20000018 ;
                  rdl:PCA_100006766 rdl:PCA_100006654 ;
                  rdl:PCA_100006768 "To  descibe all planned qualification activities and acceptance criteria." ;
                  rdfs:comment "To  descibe all planned qualification activities and acceptance criteria." ;
                  rdfs:label "Technology qualification program" ;
                  skos:broadMatch rdl:PCA_100006672 ;
                  skos:broader rdl:PCA_100006759 .


###  http://rds.posccaesar.org/ontology/plm/rdl/PCA_100006490
rdl:PCA_100006490 rdf:type owl:Class ;
                  rdfs:subClassOf rdl:PCA_100004908 ;
                  rdl:PCA_100006763 "Ensure safe operation" ;
                  rdl:PCA_100006765 rrdl:CFIHOS-20000018 ;
                  rdl:PCA_100006766 rdl:PCA_100006654 ;
                  rdl:PCA_100006768 "To give  the result of all planned qualification activities." ;
                  rdfs:comment "To give  the result of all planned qualification activities." ;
                  rdfs:label "Technology qualification report" ;
                  skos:broadMatch rdl:PCA_100006722 ;
                  skos:broader rdl:PCA_100006756 .


###  http://rds.posccaesar.org/ontology/plm/rdl/PCA_100006491
rdl:PCA_100006491 rdf:type owl:Class ;
                  rdfs:subClassOf rdl:PCA_100004908 ;
                  rdl:PCA_100006765 rrdl:CFIHOS-20000030 ;
                  rdl:PCA_100006766 rdl:PCA_100006653 ;
                  rdl:PCA_100006768 "Calculations of telecommunication battery and charger capacity." ;
                  rdfs:comment "Calculations of telecommunication battery and charger capacity." ;
                  rdfs:label "Telecommunication battery and charger capacity calculations" ;
                  skos:broadMatch rdl:PCA_100006687 ;
                  skos:broader rdl:PCA_100006741 .


###  http://rds.posccaesar.org/ontology/plm/rdl/PCA_100006492
rdl:PCA_100006492 rdf:type owl:Class ;
                  rdfs:subClassOf rdl:PCA_100004908 ;
                  rdl:PCA_100006763 "At least one Telecommunication field equipment layout drawing for each area or module deck level shall be produced. The size of the facility will determine the scale of the drawing, but normally a scale of 1:100 on A3 format shall be aimed for. If required several drawings per area can be necessary to achieve this scale. Equipment which is covered by platforms above shall be shown dotted or shown in separate figures." ;
                  rdl:PCA_100006765 rrdl:CFIHOS-20000030 ;
                  rdl:PCA_100006766 rdl:PCA_100006653 ;
                  rdl:PCA_100006768 "The following content shall be included on the drawings:\n - All tagged telecommunication field equipment like PAGA loudspeakers, flashing lights, Ex telephones, fixed radios, CCTV cameras, antennas, junction boxes, etc.;\n - Other telecommunication equipment installed outside telecommunication equipment rooms;\n - Telecommunication outlets;\n - Platform/plant northing and orientation with respect of true north;\n - Gridlines with north and east references;\n - Key plan;\n - Scale bar;\n - Match lines with drawing references;\n - Deck/area elevations." ;
                  rdfs:comment "The following content shall be included on the drawings:\n - All tagged telecommunication field equipment like PAGA loudspeakers, flashing lights, Ex telephones, fixed radios, CCTV cameras, antennas, junction boxes, etc.;\n - Other telecommunication equipment installed outside telecommunication equipment rooms;\n - Telecommunication outlets;\n - Platform/plant northing and orientation with respect of true north;\n - Gridlines with north and east references;\n - Key plan;\n - Scale bar;\n - Match lines with drawing references;\n - Deck/area elevations." ;
                  rdfs:label "Telecommunication field equipment layout drawings" ;
                  skos:broadMatch rdl:PCA_100006708 ;
                  skos:broader rdl:PCA_100006746 .


###  http://rds.posccaesar.org/ontology/plm/rdl/PCA_100006493
rdl:PCA_100006493 rdf:type owl:Class ;
                  rdfs:subClassOf rdl:PCA_100004908 ;
                  rdl:PCA_100006765 rrdl:CFIHOS-20000030 ;
                  rdl:PCA_100006766 rdl:PCA_100006640 ;
                  rdl:PCA_100006768 "Load list for telecommunication power supply." ;
                  rdfs:comment "Load list for telecommunication power supply." ;
                  rdfs:label "Telecommunication power supply load list" ;
                  skos:broadMatch rdl:PCA_100006702 ,
                                  rdl:PCA_100006716 ;
                  skos:broader rdl:PCA_100006748 .


###  http://rds.posccaesar.org/ontology/plm/rdl/PCA_100006494
rdl:PCA_100006494 rdf:type owl:Class ;
                  rdfs:subClassOf rdl:PCA_100004908 ;
                  rdl:PCA_100006765 rrdl:CFIHOS-20000030 ;
                  rdl:PCA_100006766 rdl:PCA_100006640 ;
                  rdl:PCA_100006768 "Signal level diagrams shall be made for:\n - The feeder arrangement of all radio systems including transceivers ports and antennas;\n - Audio and video entertainment distribution network (coaxial cable);\n - Interconnection signal lines between subsystems and to other systems;\n - External lines where signal level is not set by standard.\n\nLevels shall be given in dBm in conjunction with standardised impedances. If impedance is non-standard or undefined, voltage levels shall be given.\n\nWhere applicable, impedances and wire configuration should be indicated. (2-wire, 4-wire, coax, E&M lines, etc.)." ;
                  rdfs:comment "Signal level diagrams shall be made for:\n - The feeder arrangement of all radio systems including transceivers ports and antennas;\n - Audio and video entertainment distribution network (coaxial cable);\n - Interconnection signal lines between subsystems and to other systems;\n - External lines where signal level is not set by standard.\n\nLevels shall be given in dBm in conjunction with standardised impedances. If impedance is non-standard or undefined, voltage levels shall be given.\n\nWhere applicable, impedances and wire configuration should be indicated. (2-wire, 4-wire, coax, E&M lines, etc.)." ;
                  rdfs:label "Telecommunication signal level diagram" ;
                  skos:broadMatch rdl:PCA_100006700 ;
                  skos:broader rdl:PCA_100006745 .


###  http://rds.posccaesar.org/ontology/plm/rdl/PCA_100006495
rdl:PCA_100006495 rdf:type owl:Class ;
                  rdfs:subClassOf rdl:PCA_100004908 ;
                  rdl:PCA_100006763 "The overall telecommunication system topology diagram shall show an overall configuration of all telecommunication systems to give a functional understanding.\n\nTelecommunication topology diagram per telecommunication system shall show the relation between functional units within a telecommunication system/subsystem." ;
                  rdl:PCA_100006765 rrdl:CFIHOS-20000030 ;
                  rdl:PCA_100006766 rdl:PCA_100006640 ;
                  rdl:PCA_100006768 "The following telecommunication system topology diagrams shall be provided:\n - Overall telecommunication topology diagram;\n - Telecommunication topology diagram per telecommunication system (according to NORSOK T-101.\n\nThe overall telecommunication system topology diagram typical contents shall be:\n - All related telecommunication systems/subsystems represented by blocks;\n - Location;\n - Interface and wiring between blocks shall be indicated.\n\nTelecommunication topology diagram per telecommunication system typical information shall be:\n - The function of each unit (block): Short description, supplied with function identification code if applicable;\n - Interface between blocks and interface to other equipment/systems;\n - Signal type and function (Ethernet, 2/4 W E&M, G.703, RS232, control signals, etc.) if applicable;\n - Location of the equipment, either by text labelling of each block or by blocks located in dotted area boxes." ;
                  rdfs:comment "The following telecommunication system topology diagrams shall be provided:\n - Overall telecommunication topology diagram;\n - Telecommunication topology diagram per telecommunication system (according to NORSOK T-101.\n\nThe overall telecommunication system topology diagram typical contents shall be:\n - All related telecommunication systems/subsystems represented by blocks;\n - Location;\n - Interface and wiring between blocks shall be indicated.\n\nTelecommunication topology diagram per telecommunication system typical information shall be:\n - The function of each unit (block): Short description, supplied with function identification code if applicable;\n - Interface between blocks and interface to other equipment/systems;\n - Signal type and function (Ethernet, 2/4 W E&M, G.703, RS232, control signals, etc.) if applicable;\n - Location of the equipment, either by text labelling of each block or by blocks located in dotted area boxes." ;
                  rdfs:label "Telecommunication system topology diagram" ;
                  skos:broadMatch rdl:PCA_100006695 ;
                  skos:broader rdl:PCA_100006745 .


###  http://rds.posccaesar.org/ontology/plm/rdl/PCA_100006496
rdl:PCA_100006496 rdf:type owl:Class ;
                  rdfs:subClassOf rdl:PCA_100004908 ;
                  rdl:PCA_100006763 "This document shall provide input to electrical hook-up with respect to power, input/output signals and communication." ;
                  rdl:PCA_100006765 rrdl:CFIHOS-20000008 ;
                  rdl:PCA_100006766 rdl:PCA_100006653 ;
                  rdl:PCA_100006768 "Document to identify terminals for external connection, including marking (if applicable) and signal/power description. Cable entry information may be included in this drawing or part of valve drawing.  The  supplier standard drawing to be delivered if existing." ;
                  rdfs:comment "Document to identify terminals for external connection, including marking (if applicable) and signal/power description. Cable entry information may be included in this drawing or part of valve drawing.  The  supplier standard drawing to be delivered if existing." ;
                  rdfs:label "Termination and wiring diagram" ;
                  skos:broadMatch rdl:PCA_100006712 ;
                  skos:broader rdl:PCA_100006745 .


###  http://rds.posccaesar.org/ontology/plm/rdl/PCA_100006497
rdl:PCA_100006497 rdf:type owl:Class ;
                  rdfs:subClassOf rdl:PCA_100004908 ;
                  rdl:PCA_100006763 "Ensure safe operation" ;
                  rdl:PCA_100006765 rrdl:CFIHOS-20000018 ;
                  rdl:PCA_100006766 rdl:PCA_100006657 ;
                  rdl:PCA_100006768 "Shall be according to ISO 15589-1." ;
                  rdfs:comment "Shall be according to ISO 15589-1." ;
                  rdfs:label "Test procedures onshore CP system, coating quality and insulating joint" ;
                  skos:broadMatch rdl:PCA_100006688 ;
                  skos:broader rdl:PCA_100006751 .


###  http://rds.posccaesar.org/ontology/plm/rdl/PCA_100006498
rdl:PCA_100006498 rdf:type owl:Class ;
                  rdfs:subClassOf rdl:PCA_100004908 ;
                  rdl:PCA_100006763 "Ensure safe operation" ;
                  rdl:PCA_100006765 rrdl:CFIHOS-20000018 ;
                  rdl:PCA_100006766 rdl:PCA_100006657 ;
                  rdl:PCA_100006768 "Shall be according to ISO 15589-1." ;
                  rdfs:comment "Shall be according to ISO 15589-1." ;
                  rdfs:label "Test results onshore CP system, coating quality and insulating joint" ;
                  skos:broadMatch rdl:PCA_100006722 ;
                  skos:broader rdl:PCA_100006756 .


###  http://rds.posccaesar.org/ontology/plm/rdl/PCA_100006499
rdl:PCA_100006499 rdf:type owl:Class ;
                  rdfs:subClassOf rdl:PCA_100004908 ;
                  rdl:PCA_100006763 "Calculation of heat-transfer-related properties. This document gives a simplified approach for the treatment of thermal bridges." ;
                  rdl:PCA_100006766 rdl:PCA_100006653 ;
                  rdl:PCA_100006768 "ISO 12241\nCalculation methods of heat transfer." ;
                  rdfs:comment "ISO 12241\nCalculation methods of heat transfer." ;
                  rdfs:label "Thermal calculations" ;
                  skos:broadMatch rdl:PCA_100006687 ;
                  skos:broader rdl:PCA_100006741 .


###  http://rds.posccaesar.org/ontology/plm/rdl/PCA_100006500
rdl:PCA_100006500 rdf:type owl:Class ;
                  rdfs:subClassOf rdl:PCA_100004908 ;
                  rdl:PCA_100006763 "To secure independent verification of compliance" ;
                  rdl:PCA_100006765 rrdl:CFIHOS-20000027 ;
                  rdl:PCA_100006766 rdl:PCA_100006653 ;
                  rdl:PCA_100006768 "The document shall clearly describe the object(s) for which the certificate applies" ;
                  rdfs:comment "The document shall clearly describe the object(s) for which the certificate applies" ;
                  rdfs:label "Third party certificate" ;
                  skos:broadMatch rdl:PCA_100006722 ;
                  skos:broader rdl:PCA_100006743 .


###  http://rds.posccaesar.org/ontology/plm/rdl/PCA_100006501
rdl:PCA_100006501 rdf:type owl:Class ;
                  rdfs:subClassOf rdl:PCA_100004908 ;
                  rdl:PCA_100006765 rrdl:CFIHOS-20000020 ;
                  rdl:PCA_100006766 rdl:PCA_100006653 ;
                  rdl:PCA_100006768 "Third Party verification report" ;
                  rdfs:comment "Third Party verification report" ;
                  rdfs:label "Third party verifications" ;
                  skos:broadMatch rdl:PCA_100006722 ;
                  skos:broader rdl:PCA_100006756 .


###  http://rds.posccaesar.org/ontology/plm/rdl/PCA_100006502
rdl:PCA_100006502 rdf:type owl:Class ;
                  rdfs:subClassOf rdl:PCA_100004908 ;
                  rdl:PCA_100006763 "Ensure safe operation" ;
                  rdl:PCA_100006765 rrdl:CFIHOS-20000018 ;
                  rdl:PCA_100006766 rdl:PCA_100006654 ;
                  rdl:PCA_100006768 "Covering pipeline tie-in operations construction.\nBasis for analysis, assumptions and assessments not given in design basis shall be included." ;
                  rdfs:comment "Covering pipeline tie-in operations construction.\nBasis for analysis, assumptions and assessments not given in design basis shall be included." ;
                  rdfs:label "Tie-in design report" ;
                  skos:broadMatch rdl:PCA_100006686 ;
                  skos:broader rdl:PCA_100006756 .


###  http://rds.posccaesar.org/ontology/plm/rdl/PCA_100006503
rdl:PCA_100006503 rdf:type owl:Class ;
                  rdfs:subClassOf rdl:PCA_100004908 ;
                  rdl:PCA_100006768 "The tie-in and diving operations manuals shall give a detailed description of the following items and operations:\n - Description of tie-in tools to be used for the alternative operations\n - Drawings of tie-in tools with weights, size, operational requirements and operational limitations \n - Identification of ROV specific operations with outline descriptions of the ROV operation\n - Identification of critical items in relation to the above listed operations\n - Specify operations planned to be performed by divers\n - Identify access for divers, outline description of work tasks, work area and tools to be used\n - Identification of critical operations in relation to the diving programme." ;
                  rdfs:comment "The tie-in and diving operations manuals shall give a detailed description of the following items and operations:\n - Description of tie-in tools to be used for the alternative operations\n - Drawings of tie-in tools with weights, size, operational requirements and operational limitations \n - Identification of ROV specific operations with outline descriptions of the ROV operation\n - Identification of critical items in relation to the above listed operations\n - Specify operations planned to be performed by divers\n - Identify access for divers, outline description of work tasks, work area and tools to be used\n - Identification of critical operations in relation to the diving programme." ;
                  rdfs:label "Tie-in manual" ;
                  skos:broadMatch rdl:PCA_100006688 ,
                                  rdl:PCA_100006712 ,
                                  rdl:PCA_100006713 ;
                  skos:broader rdl:PCA_100006749 .


###  http://rds.posccaesar.org/ontology/plm/rdl/PCA_100006504
rdl:PCA_100006504 rdf:type owl:Class ;
                  rdfs:subClassOf rdl:PCA_100004908 ;
                  rdl:PCA_100006763 "Documentation of tie-in" ;
                  rdl:PCA_100006765 rrdl:CFIHOS-20000018 ;
                  rdl:PCA_100006766 rdl:PCA_100006654 ;
                  rdl:PCA_100006768 "Documentation of procedures used for tie-in" ;
                  rdfs:comment "Documentation of procedures used for tie-in" ;
                  rdfs:label "Tie-in procedures" ;
                  skos:broadMatch rdl:PCA_100006688 ;
                  skos:broader rdl:PCA_100006751 .


###  http://rds.posccaesar.org/ontology/plm/rdl/PCA_100006505
rdl:PCA_100006505 rdf:type owl:Class ;
                  rdfs:subClassOf rdl:PCA_100004908 ;
                  rdl:PCA_100006763 "Describe how to transport and handle equipment safely from delivery to final installation." ;
                  rdl:PCA_100006765 rrdl:CFIHOS-20000031 ;
                  rdl:PCA_100006766 rdl:PCA_100006653 ;
                  rdl:PCA_100006768 "Information for safe handling of equipment during transportation, lifting and handling." ;
                  rdfs:comment "Information for safe handling of equipment during transportation, lifting and handling." ;
                  rdfs:label "Transport and handling instructions" ;
                  skos:broadMatch rdl:PCA_100006668 ;
                  skos:broader rdl:PCA_100006751 .


###  http://rds.posccaesar.org/ontology/plm/rdl/PCA_100006506
rdl:PCA_100006506 rdf:type owl:Class ;
                  rdfs:subClassOf rdl:PCA_100004908 ;
                  rdl:PCA_100006763 "To give input to the design of a structure or assembly including seafastening." ;
                  rdl:PCA_100006765 rrdl:CFIHOS-20000031 ;
                  rdl:PCA_100006766 rdl:PCA_100006653 ;
                  rdl:PCA_100006768 "A report providing the results from sea transport analysis of a structure or equipment assembly." ;
                  rdfs:comment "A report providing the results from sea transport analysis of a structure or equipment assembly." ;
                  rdfs:label "Transportation analysis report" ;
                  skos:broadMatch rdl:PCA_100006668 ;
                  skos:broader rdl:PCA_100006756 .


###  http://rds.posccaesar.org/ontology/plm/rdl/PCA_100006507
rdl:PCA_100006507 rdf:type owl:Class ;
                  rdfs:subClassOf rdl:PCA_100004908 ;
                  rdl:PCA_100006763 "Basis for analysis, assumptions and assessments not given in design basis shall be included." ;
                  rdl:PCA_100006765 rrdl:CFIHOS-20000018 ;
                  rdl:PCA_100006766 rdl:PCA_100006654 ;
                  rdl:PCA_100006768 "More details Design report covering trawl impact, hooking and pull-over assessment and performed analyses." ;
                  rdfs:comment "More details Design report covering trawl impact, hooking and pull-over assessment and performed analyses." ;
                  rdfs:label "Trawl interference design report" ;
                  skos:broadMatch rdl:PCA_100006686 ;
                  skos:broader rdl:PCA_100006756 .


###  http://rds.posccaesar.org/ontology/plm/rdl/PCA_100006508
rdl:PCA_100006508 rdf:type owl:Class ;
                  rdfs:subClassOf rdl:PCA_100004908 ;
                  rdl:PCA_100006763 "To provide input to weight coating design and protection requirements." ;
                  rdl:PCA_100006765 rrdl:CFIHOS-20000031 ;
                  rdl:PCA_100006766 rdl:PCA_100006653 ;
                  rdl:PCA_100006768 "Document potential impact from trawl equipment towards pipeline." ;
                  rdfs:comment "Document potential impact from trawl equipment towards pipeline." ;
                  rdfs:label "Trawling interaction" ;
                  skos:broadMatch rdl:PCA_100006686 ,
                                  rdl:PCA_100006713 ;
                  skos:broader rdl:PCA_100006756 .


###  http://rds.posccaesar.org/ontology/plm/rdl/PCA_100006509
rdl:PCA_100006509 rdf:type owl:Class ;
                  rdfs:subClassOf rdl:PCA_100004908 ;
                  rdl:PCA_100006763 "The design loads used to dimension the turret shall be documented." ;
                  rdl:PCA_100006765 rrdl:CFIHOS-20000033 ;
                  rdl:PCA_100006766 rdl:PCA_100006657 ;
                  rdl:PCA_100006768 "The report or collection of reports shall contain a complete description of the turret design." ;
                  rdfs:comment "The report or collection of reports shall contain a complete description of the turret design." ;
                  rdfs:label "Turret design analysis report" ;
                  skos:broadMatch rdl:PCA_100006698 ;
                  skos:broader rdl:PCA_100006756 .


###  http://rds.posccaesar.org/ontology/plm/rdl/PCA_100006510
rdl:PCA_100006510 rdf:type owl:Class ;
                  rdfs:subClassOf rdl:PCA_100004908 ;
                  rdl:PCA_100006763 "Technical documentation of all mechanical and structural components of the turret shall be delivered." ;
                  rdl:PCA_100006765 rrdl:CFIHOS-20000033 ;
                  rdl:PCA_100006766 rdl:PCA_100006657 ;
                  rdl:PCA_100006768 "This documentation shall include the following:\n - General arrangement drawings;\n - Detail drawings of all major components;\n - Design analyses of all major components;\n - Material certificates for all components including welding filler material along with traceability data;\n - Turret / turning system procedures (if relevant);\n - Procedures necessary to safely operate, maintain and replace mechanical components." ;
                  rdfs:comment "This documentation shall include the following:\n - General arrangement drawings;\n - Detail drawings of all major components;\n - Design analyses of all major components;\n - Material certificates for all components including welding filler material along with traceability data;\n - Turret / turning system procedures (if relevant);\n - Procedures necessary to safely operate, maintain and replace mechanical components." ;
                  rdfs:label "Turret system report" ;
                  skos:broadMatch rdl:PCA_100006698 ;
                  skos:broader rdl:PCA_100006756 .


###  http://rds.posccaesar.org/ontology/plm/rdl/PCA_100006511
rdl:PCA_100006511 rdf:type owl:Class ;
                  rdfs:subClassOf rdl:PCA_100004908 ;
                  rdl:PCA_100006763 "This document is used for verification of compliance" ;
                  rdl:PCA_100006765 rrdl:CFIHOS-20000027 ;
                  rdl:PCA_100006766 rdl:PCA_100006653 ;
                  rdl:PCA_100006768 "Document compliance" ;
                  rdfs:comment "Document compliance" ;
                  rdfs:label "Type approval certificate" ;
                  skos:broadMatch rdl:PCA_100006722 ;
                  skos:broader rdl:PCA_100006743 .


###  http://rds.posccaesar.org/ontology/plm/rdl/PCA_100006512
rdl:PCA_100006512 rdf:type owl:Class ;
                  rdfs:subClassOf rdl:PCA_100004908 ;
                  rdl:PCA_100006765 rrdl:CFIHOS-20000030 ;
                  rdl:PCA_100006766 rdl:PCA_100006640 ;
                  rdl:PCA_100006768 "UHF/VHF radio (platform/facility internal) coverage chart/test report shall be provided." ;
                  rdfs:comment "UHF/VHF radio (platform/facility internal) coverage chart/test report shall be provided." ;
                  rdfs:label "UHF/VHF radio coverage" ;
                  skos:broadMatch rdl:PCA_100006705 ,
                                  rdl:PCA_100006722 ;
                  skos:broader rdl:PCA_100006756 .


###  http://rds.posccaesar.org/ontology/plm/rdl/PCA_100006513
rdl:PCA_100006513 rdf:type owl:Class ;
                  rdfs:subClassOf rdl:PCA_100004908 ;
                  rdl:PCA_100006763 "The drawings shall fully cover all construction and temporary underground piping and cable systems and their status if the system is not fully removed." ;
                  rdl:PCA_100006765 rrdl:CFIHOS-20000007 ;
                  rdl:PCA_100006766 rdl:PCA_100006656 ;
                  rdl:PCA_100006768 "All system, arrangement, layout, plan, alignment, section and detail drawings shall be included." ;
                  rdfs:comment "All system, arrangement, layout, plan, alignment, section and detail drawings shall be included." ;
                  rdfs:label "Underground piping and cables drawings" ;
                  skos:broadMatch rdl:PCA_100006708 ;
                  skos:broader rdl:PCA_100006746 .


###  http://rds.posccaesar.org/ontology/plm/rdl/PCA_100006514
rdl:PCA_100006514 rdf:type owl:Class ;
                  rdfs:subClassOf rdl:PCA_100004908 ;
                  rdl:PCA_100006763 "Hydraulic system calculation reports and input files/parameters shall be delivered. The report or collection of reports shall be self-contained, i.e. provide all information required to re-produce the results.\n\nThe design shall be documented by calculations. Calculations shall include references to basis of design (fire water quantities, maximum rainfall, etc.) and explanatory text (system description, etc.)" ;
                  rdl:PCA_100006765 rrdl:CFIHOS-20000007 ;
                  rdl:PCA_100006766 rdl:PCA_100006648 ;
                  rdl:PCA_100006768 "The calculations shall include:\n - Head loss calculations during fire situations;\n - Head loss calculations during various climatic conditions, such as storm rain, snow melting (if applicable) etc.;\n - Surge calculations for start/stop of pumps, valve operations, etc. shall be performed for all pump systems;\n - For drain systems with water traps, sensitivity calculations shall be made to identify uncertainties in head losses in manholes.\n\nIf existing calculation models exist, these models shall be updated." ;
                  rdfs:comment "The calculations shall include:\n - Head loss calculations during fire situations;\n - Head loss calculations during various climatic conditions, such as storm rain, snow melting (if applicable) etc.;\n - Surge calculations for start/stop of pumps, valve operations, etc. shall be performed for all pump systems;\n - For drain systems with water traps, sensitivity calculations shall be made to identify uncertainties in head losses in manholes.\n\nIf existing calculation models exist, these models shall be updated." ;
                  rdfs:label "Underground piping hydraulic system calculation" ;
                  skos:broadMatch rdl:PCA_100006687 ;
                  skos:broader rdl:PCA_100006741 .


###  http://rds.posccaesar.org/ontology/plm/rdl/PCA_100006515
rdl:PCA_100006515 rdf:type owl:Class ;
                  rdfs:subClassOf rdl:PCA_100004908 ;
                  rdl:PCA_100006765 rrdl:CFIHOS-20000007 ;
                  rdl:PCA_100006766 rdl:PCA_100006656 ;
                  rdl:PCA_100006768 "All system, arrangement, layout, plan, alignment, section and detail drawings shall be delivered including drawings showing details for rock support." ;
                  rdfs:comment "All system, arrangement, layout, plan, alignment, section and detail drawings shall be delivered including drawings showing details for rock support." ;
                  rdfs:label "Underground rock facilities drawings" ;
                  skos:broadMatch rdl:PCA_100006707 ,
                                  rdl:PCA_100006708 ,
                                  rdl:PCA_100006732 ;
                  skos:broader rdl:PCA_100006746 .


###  http://rds.posccaesar.org/ontology/plm/rdl/PCA_100006516
rdl:PCA_100006516 rdf:type owl:Class ;
                  rdfs:subClassOf rdl:PCA_100004908 ;
                  rdl:PCA_100006763 "The unique equipment ID is the key information element to retrieve standard documentation for standard equipment in Company's solution for standard documentation for equipment and materials. The unique equipment ID shall be in approved status at milestone LCI 1, and thus also required approved standard documentation is provided." ;
                  rdfs:label "Unique equipment ID for standard equipment" .


###  http://rds.posccaesar.org/ontology/plm/rdl/PCA_100006517
rdl:PCA_100006517 rdf:type owl:Class ;
                  rdfs:subClassOf rdl:PCA_100004908 ;
                  rdl:PCA_100006763 "Consumption data e.g. for diesel oil, compressed air, heating/cooling media etc." ;
                  rdl:PCA_100006768 "The following generalised index shall be used:\n - Equipment tag no.\n - Type of consumption\n - Volume m3 and time unit\n - Net weight (kg) and time unit\n - Specific weight (kg)\n - Storage temperature oC\n - Storage humidity %\n - Storage max pressure (barg)\n - Storage capacity m3\n - Storage location/area\n - Specification\n - Supplier\n - Data sheet\n - Notes" ;
                  rdfs:comment "The following generalised index shall be used:\n - Equipment tag no.\n - Type of consumption\n - Volume m3 and time unit\n - Net weight (kg) and time unit\n - Specific weight (kg)\n - Storage temperature oC\n - Storage humidity %\n - Storage max pressure (barg)\n - Storage capacity m3\n - Storage location/area\n - Specification\n - Supplier\n - Data sheet\n - Notes" ;
                  rdfs:label "Utility consumption index" ;
                  skos:broadMatch rdl:PCA_100006716 ;
                  skos:broader rdl:PCA_100006748 .


###  http://rds.posccaesar.org/ontology/plm/rdl/PCA_100006518
rdl:PCA_100006518 rdf:type owl:Class ;
                  rdfs:subClassOf rdl:PCA_100004908 ;
                  rdl:PCA_100006763 "Input to procurement and multi-discipline design. Information to operation regarding utility system design." ;
                  rdl:PCA_100006765 rrdl:CFIHOS-20000026 ;
                  rdl:PCA_100006766 rdl:PCA_100006583 ,
                                    rdl:PCA_100006604 ,
                                    rdl:PCA_100006605 ,
                                    rdl:PCA_100006606 ,
                                    rdl:PCA_100006607 ,
                                    rdl:PCA_100006608 ,
                                    rdl:PCA_100006609 ,
                                    rdl:PCA_100006610 ,
                                    rdl:PCA_100006611 ,
                                    rdl:PCA_100006612 ,
                                    rdl:PCA_100006613 ,
                                    rdl:PCA_100006614 ,
                                    rdl:PCA_100006615 ,
                                    rdl:PCA_100006616 ,
                                    rdl:PCA_100006617 ,
                                    rdl:PCA_100006618 ,
                                    rdl:PCA_100006619 ,
                                    rdl:PCA_100006620 ,
                                    rdl:PCA_100006621 ,
                                    rdl:PCA_100006622 ,
                                    rdl:PCA_100006623 ,
                                    rdl:PCA_100006624 ,
                                    rdl:PCA_100006625 ,
                                    rdl:PCA_100006627 ,
                                    rdl:PCA_100006628 ;
                  rdl:PCA_100006768 "For all utility systems the following shall be included in the utility consumption report:\n - For the total system:\n    - Total system capacity (duty, flow rate and/or other parameter relevant for capacity);\n    - Maximum coincident consumer load (duty, flow rate and/or other parameter relevant for capacity);\n    - Description of utility characteristic/quality prior to distribution to consumers (pressure, temperature, composition and/or other relevant parameters);\n    - Storage capacity;\n - For the consumers:\n    - Tag number;\n    - Continuous or intermittent consumer;\n    - Required consumption, both maximum, normal and minimum consumption;\n    - Description of utility characteristic/quality at consumer." ;
                  rdfs:comment "For all utility systems the following shall be included in the utility consumption report:\n - For the total system:\n    - Total system capacity (duty, flow rate and/or other parameter relevant for capacity);\n    - Maximum coincident consumer load (duty, flow rate and/or other parameter relevant for capacity);\n    - Description of utility characteristic/quality prior to distribution to consumers (pressure, temperature, composition and/or other relevant parameters);\n    - Storage capacity;\n - For the consumers:\n    - Tag number;\n    - Continuous or intermittent consumer;\n    - Required consumption, both maximum, normal and minimum consumption;\n    - Description of utility characteristic/quality at consumer." ;
                  rdfs:label "Utility consumption report" ;
                  skos:broadMatch rdl:PCA_100006687 ;
                  skos:broader rdl:PCA_100006756 .


###  http://rds.posccaesar.org/ontology/plm/rdl/PCA_100006519
rdl:PCA_100006519 rdf:type owl:Class ;
                  rdfs:subClassOf rdl:PCA_100004908 ;
                  rdl:PCA_100006763 "This document shall support verification of component function according to company/project requirements, Information to be used into system engineering." ;
                  rdl:PCA_100006765 rrdl:CFIHOS-20000022 ;
                  rdl:PCA_100006766 rdl:PCA_100006653 ;
                  rdl:PCA_100006768 "Characteristics and functional parameters shall be documented and performance shall be shown to be probable. This shall include but not be limited to calculations, curves, tables, reference to similar applications and test data. This shall as a minimum be at a level customary for the equipment and to the extent such data are of importance for interfaces to plant and system.\n\nValve and actuator should include: \n-Torque table showing safety factor for: Break to close ,run to close , end to close, break to open, run to open & end to open. \n-The table shall include Maximum Allowable Valve Input Torque (MAVIT).                      \n-Manufacturers standard calculation report can be used\n-Capacity calculations, Noise calculations," ;
                  rdfs:comment "Characteristics and functional parameters shall be documented and performance shall be shown to be probable. This shall include but not be limited to calculations, curves, tables, reference to similar applications and test data. This shall as a minimum be at a level customary for the equipment and to the extent such data are of importance for interfaces to plant and system.\n\nValve and actuator should include: \n-Torque table showing safety factor for: Break to close ,run to close , end to close, break to open, run to open & end to open. \n-The table shall include Maximum Allowable Valve Input Torque (MAVIT).                      \n-Manufacturers standard calculation report can be used\n-Capacity calculations, Noise calculations," ;
                  rdfs:label "Valve and operator calculations" ;
                  skos:broadMatch rdl:PCA_100006687 ;
                  skos:broader rdl:PCA_100006741 .


###  http://rds.posccaesar.org/ontology/plm/rdl/PCA_100006520
rdl:PCA_100006520 rdf:type owl:Class ;
                  rdfs:subClassOf rdl:PCA_100004908 ;
                  rdl:PCA_100006765 rrdl:CFIHOS-20000022 ;
                  rdl:PCA_100006768 "Drawings of the following are required:\n - Detail / cross sectional drawings (details of manual/bare stem valve/actuator/control panel, etc.)\n - Arrangement drawings of assemblies (assemblies of valve/gearbox/actuator/control panel, etc.)\n Arrangement drawings and detail/cross sectional drawings may be supplied as separate drawings or combined in one drawing. Drawings shall show all components in the same scale. \n\nDetail/cross sectional drawings shall at least include:\n - VDS reference (Valves)\n - All welds including hard facing and overlaying (Valves)\n - Bore (Valves)\n - Outline dimensions\n - Weight, as built\n - Lifting lugs\n - Parts list including all parts with functional part description and material standard used (real manufacturer’s part number is not required on the drawings). MDS reference to be included when specified in the requirements \nArrangement drawings of assemblies shall at least include: \n - Outline dimensions \n - Material selection for adaptor stool, coupling (connection between valve and actuator shafts), actuator/valve connection bolts and valve stem if modified from specified requirement (including CR reference) \n - Weight, as built (weights shall be listed separately for valve, actuator, control panel or cabinet and total assembly) \n - Principles for assembly (maintenance envelopes) \n - All power and signal connection points with entry details \nFor valves not specified according to TR2000 (e.g. control, choke and safety relief valves), real manufacturer's part number shall be included on the valve drawing or a separate BOM." ;
                  rdfs:comment "Drawings of the following are required:\n - Detail / cross sectional drawings (details of manual/bare stem valve/actuator/control panel, etc.)\n - Arrangement drawings of assemblies (assemblies of valve/gearbox/actuator/control panel, etc.)\n Arrangement drawings and detail/cross sectional drawings may be supplied as separate drawings or combined in one drawing. Drawings shall show all components in the same scale. \n\nDetail/cross sectional drawings shall at least include:\n - VDS reference (Valves)\n - All welds including hard facing and overlaying (Valves)\n - Bore (Valves)\n - Outline dimensions\n - Weight, as built\n - Lifting lugs\n - Parts list including all parts with functional part description and material standard used (real manufacturer’s part number is not required on the drawings). MDS reference to be included when specified in the requirements \nArrangement drawings of assemblies shall at least include: \n - Outline dimensions \n - Material selection for adaptor stool, coupling (connection between valve and actuator shafts), actuator/valve connection bolts and valve stem if modified from specified requirement (including CR reference) \n - Weight, as built (weights shall be listed separately for valve, actuator, control panel or cabinet and total assembly) \n - Principles for assembly (maintenance envelopes) \n - All power and signal connection points with entry details \nFor valves not specified according to TR2000 (e.g. control, choke and safety relief valves), real manufacturer's part number shall be included on the valve drawing or a separate BOM." ;
                  rdfs:label "Valve and operator drawings" ;
                  skos:broadMatch rdl:PCA_100006686 ,
                                  rdl:PCA_100006731 ,
                                  rdl:PCA_100006732 ,
                                  rdl:PCA_100006733 ,
                                  rdl:PCA_100006734 ;
                  skos:broader rdl:PCA_100006746 .


###  http://rds.posccaesar.org/ontology/plm/rdl/PCA_100006521
rdl:PCA_100006521 rdf:type owl:Class ;
                  rdfs:subClassOf rdl:PCA_100004908 ;
                  rdl:PCA_100006765 rrdl:CFIHOS-20000027 ;
                  rdl:PCA_100006768 "The following test reports are required: 1. Fugitive emission test reports when specified by Purchaser 2. Test reports from qualification of non-collapsible choke valves when specified by Purchaser 3. For intelligent positioner with 4-20 mA input and HART or Fieldbus communication and diagnostic possibilities, a documented footprint/valve signature from FAT shall be delivered in a file with ZIP format (containing the data in native format) in addition to PDF. 4. FAT reports 5. FAT reports for actuators according to TR0038 Valve and operator test reports shall be delivered in PDF format with the addition described above for the intelligent positioner." ;
                  rdfs:comment "The following test reports are required: 1. Fugitive emission test reports when specified by Purchaser 2. Test reports from qualification of non-collapsible choke valves when specified by Purchaser 3. For intelligent positioner with 4-20 mA input and HART or Fieldbus communication and diagnostic possibilities, a documented footprint/valve signature from FAT shall be delivered in a file with ZIP format (containing the data in native format) in addition to PDF. 4. FAT reports 5. FAT reports for actuators according to TR0038 Valve and operator test reports shall be delivered in PDF format with the addition described above for the intelligent positioner." ;
                  rdfs:label "Valve and operator test reports" ;
                  skos:broadMatch rdl:PCA_100006722 ;
                  skos:broader rdl:PCA_100006756 .


###  http://rds.posccaesar.org/ontology/plm/rdl/PCA_100006522
rdl:PCA_100006522 rdf:type owl:Class ;
                  rdfs:subClassOf rdl:PCA_100004908 ;
                  rdl:PCA_100006763 "Report documenting all calculations and analysis performed with regards to bursting, propagating buckling and collapse to prove correct wall thickness design." ;
                  rdl:PCA_100006765 rrdl:CFIHOS-20000031 ;
                  rdl:PCA_100006766 rdl:PCA_100006657 ;
                  rdl:PCA_100006768 "To document the correct wall thickness design of the pipeline." ;
                  rdfs:comment "To document the correct wall thickness design of the pipeline." ;
                  rdfs:label "Wall thickness design (bursting, propagating buckling, collapse)" ;
                  skos:broadMatch rdl:PCA_100006686 ;
                  skos:broader rdl:PCA_100006756 .


###  http://rds.posccaesar.org/ontology/plm/rdl/PCA_100006523
rdl:PCA_100006523 rdf:type owl:Class ;
                  rdfs:subClassOf rdl:PCA_100004908 ;
                  rdl:PCA_100006765 rrdl:CFIHOS-20000018 ;
                  rdl:PCA_100006766 rdl:PCA_100006657 ;
                  rdfs:label "Wall thickness design report" ;
                  skos:broadMatch rdl:PCA_100006686 ;
                  skos:broader rdl:PCA_100006756 .


###  http://rds.posccaesar.org/ontology/plm/rdl/PCA_100006524
rdl:PCA_100006524 rdf:type owl:Class ;
                  rdfs:subClassOf rdl:PCA_100004908 ;
                  rdl:PCA_100006763 "To document compliance with the PSA facilities regulations § 62 and NMA Regulations No. 878 in addition to IMO instruments and Class requirements, as applicable." ;
                  rdl:PCA_100006765 rrdl:CFIHOS-20000033 ;
                  rdl:PCA_100006766 rdl:PCA_100006654 ;
                  rdl:PCA_100006768 "The plan shall include information on all internal and external openings (air pipes, ventilators, hatches, doors, etc.) of volumes affecting stability calculations." ;
                  rdfs:comment "The plan shall include information on all internal and external openings (air pipes, ventilators, hatches, doors, etc.) of volumes affecting stability calculations." ;
                  rdfs:label "Watertight integrity plan" ;
                  skos:broadMatch rdl:PCA_100006708 ;
                  skos:broader rdl:PCA_100006753 .


###  http://rds.posccaesar.org/ontology/plm/rdl/PCA_100006525
rdl:PCA_100006525 rdf:type owl:Class ;
                  rdfs:subClassOf rdl:PCA_100004908 ;
                  rdl:PCA_100006763 "Provide instructions for weighing of an object / product." ;
                  rdl:PCA_100006764 "The Weight Test Procedure shall describe requirements for methods and equipment to be used to obtain the correct gross weight of the goods being shipped. It shall cover each separately installed item of equipment or skid to enable safe lifting operations and structural load calculations or components for which weight is a critical property." ;
                  rdl:PCA_100006765 rrdl:CFIHOS-20000031 ;
                  rdl:PCA_100006766 rdl:PCA_100006653 ;
                  rdl:PCA_100006768 "Procedure to describe methods for verifying weight of an object / product." ;
                  rdfs:comment "Procedure to describe methods for verifying weight of an object / product." ;
                  rdfs:label "Weighing procedure" ;
                  skos:broadMatch rdl:PCA_100006688 ;
                  skos:broader rdl:PCA_100006751 .


###  http://rds.posccaesar.org/ontology/plm/rdl/PCA_100006526
rdl:PCA_100006526 rdf:type owl:Class ;
                  rdfs:subClassOf rdl:PCA_100004908 ;
                  rdl:PCA_100006763 "To document actual weight." ;
                  rdl:PCA_100006765 rrdl:CFIHOS-20000031 ;
                  rdl:PCA_100006766 rdl:PCA_100006653 ;
                  rdl:PCA_100006768 "Report to verify weight of an object / product." ;
                  rdfs:comment "Report to verify weight of an object / product." ;
                  rdfs:label "Weighing report" ;
                  skos:broadMatch rdl:PCA_100006722 ;
                  skos:broader rdl:PCA_100006756 .


###  http://rds.posccaesar.org/ontology/plm/rdl/PCA_100006527
rdl:PCA_100006527 rdf:type owl:Class ;
                  rdfs:subClassOf rdl:PCA_100004908 ;
                  rdl:PCA_100006763 "This document is used to provide final weight both for transport/installation and design calculations." ;
                  rdl:PCA_100006765 rrdl:CFIHOS-20000027 ;
                  rdl:PCA_100006766 rdl:PCA_100006653 ;
                  rdl:PCA_100006768 "This document shall follow ISO 19901-5." ;
                  rdfs:comment "This document shall follow ISO 19901-5." ;
                  rdfs:label "Weight certificate" ;
                  skos:broadMatch rdl:PCA_100006722 ;
                  skos:broader rdl:PCA_100006743 .


###  http://rds.posccaesar.org/ontology/plm/rdl/PCA_100006528
rdl:PCA_100006528 rdf:type owl:Class ;
                  rdfs:subClassOf rdl:PCA_100004908 ;
                  rdl:PCA_100006765 rrdl:CFIHOS-20000006 ;
                  rdl:PCA_100006766 rdl:PCA_100006654 ;
                  rdl:PCA_100006768 "Content to be in accordance with ISO 19901-5. Handover format is plant specific." ;
                  rdfs:comment "Content to be in accordance with ISO 19901-5. Handover format is plant specific." ;
                  rdfs:label "Weight control database" ;
                  skos:broadMatch rdl:PCA_100006715 ,
                                  rdl:PCA_100006716 ,
                                  rdl:PCA_100006717 ,
                                  rdl:PCA_100006722 ;
                  skos:broader rdl:PCA_100006762 .


###  http://rds.posccaesar.org/ontology/plm/rdl/PCA_100006529
rdl:PCA_100006529 rdf:type owl:Class ;
                  rdfs:subClassOf rdl:PCA_100004908 ;
                  rdl:PCA_100006763 "Procedure to describe methods for verifying weight of an object / product." ;
                  rdl:PCA_100006765 rrdl:CFIHOS-20000027 ;
                  rdl:PCA_100006766 rdl:PCA_100006653 ;
                  rdl:PCA_100006768 "Provide instructions for weighing of an object / product." ;
                  rdfs:comment "Provide instructions for weighing of an object / product." ;
                  rdfs:label "Weight control procedure" ;
                  skos:broadMatch rdl:PCA_100006722 ;
                  skos:broader rdl:PCA_100006751 .


###  http://rds.posccaesar.org/ontology/plm/rdl/PCA_100006530
rdl:PCA_100006530 rdf:type owl:Class ;
                  rdfs:subClassOf rdl:PCA_100004908 ;
                  rdl:PCA_100006763 "Weight report according to ISO 19901-5." ;
                  rdl:PCA_100006765 rrdl:CFIHOS-20000006 ;
                  rdl:PCA_100006766 rdl:PCA_100006654 ;
                  rdfs:label "Weight report" ;
                  skos:broadMatch rdl:PCA_100006716 ,
                                  rdl:PCA_100006717 ;
                  skos:broader rdl:PCA_100006756 .


###  http://rds.posccaesar.org/ontology/plm/rdl/PCA_100006531
rdl:PCA_100006531 rdf:type owl:Class ;
                  rdfs:subClassOf rdl:PCA_100004908 ;
                  rdl:PCA_100006763 "It shall be prepared on basis of the weld numbering system, starting with the lowest weld number. The list shall be prepared prior to start of welding and NDE, and updating shall be parallel to execution of welding and NDE." ;
                  rdl:PCA_100006768 "The minimum requirements for this index are described below: 1. Weld no. inclusive Weld repair no. 2. Welder no. 3. Ref. to fabrication-, shop- and/or isometric drawing 4. Piping system and line no. 5. PWHT (Post Weld Heat Treatment); i.e. procedures and temperature-time records 6. WPS no. (with reference to WPQR no.) 7. Weld repair log 8. Non-Destructive Test (NDT) extent in % for different methods (e.g. UT, RT, MT, PT) 9. Visual inspection (e.g. on completed weld) 10. Weld inspection (e.g. QC activities; weld preparation, tack welding, parameter verification, consumable control, field metallographic verification, etc.) 11. NDT report number / Inspection report number 12. Weld completion time/date and NDT time/date 13. PMI (Positive Material Identification) report 14. Production tests (destructive testing when applicable) 15. Special procedures (e.g. cleaning/pickling, grinding or hammer peening of weld toe, straightening)" ;
                  rdfs:comment "The minimum requirements for this index are described below: 1. Weld no. inclusive Weld repair no. 2. Welder no. 3. Ref. to fabrication-, shop- and/or isometric drawing 4. Piping system and line no. 5. PWHT (Post Weld Heat Treatment); i.e. procedures and temperature-time records 6. WPS no. (with reference to WPQR no.) 7. Weld repair log 8. Non-Destructive Test (NDT) extent in % for different methods (e.g. UT, RT, MT, PT) 9. Visual inspection (e.g. on completed weld) 10. Weld inspection (e.g. QC activities; weld preparation, tack welding, parameter verification, consumable control, field metallographic verification, etc.) 11. NDT report number / Inspection report number 12. Weld completion time/date and NDT time/date 13. PMI (Positive Material Identification) report 14. Production tests (destructive testing when applicable) 15. Special procedures (e.g. cleaning/pickling, grinding or hammer peening of weld toe, straightening)" ;
                  rdfs:label "Weld summary index" ;
                  skos:broadMatch rdl:PCA_100006716 ,
                                  rdl:PCA_100006717 ;
                  skos:broader rdl:PCA_100006748 .


###  http://rds.posccaesar.org/ontology/plm/rdl/PCA_100006532
rdl:PCA_100006532 rdf:type owl:Class ;
                  rdfs:subClassOf rdl:PCA_100004908 ;
                  rdl:PCA_100006763 "Official certificates for welders which records compliance with specified requirements." ;
                  rdl:PCA_100006764 "Requirements related to assurance and check of quality in manufacturing phase will very much depend on Purchaser’s knowledge of supplier. Well known supplier, with proven track record, delivering products based on industry standards, will typically deliver less verification documentation to Purchaser than unknown/new supplier delivering the same product. Therefore, this deliverable should be evaluated as candidate for being available in digital format to Purchaser, for information only." ;
                  rdl:PCA_100006766 rdl:PCA_100006653 ;
                  rdl:PCA_100006768 "This document shall include welder(-s) certificate which shall clearly state that the welder(-s) is approved for the relevant welding process." ;
                  rdfs:comment "This document shall include welder(-s) certificate which shall clearly state that the welder(-s) is approved for the relevant welding process." ;
                  rdfs:label "Welders certificate" ;
                  skos:broadMatch rdl:PCA_100006722 ;
                  skos:broader rdl:PCA_100006743 .


###  http://rds.posccaesar.org/ontology/plm/rdl/PCA_100006533
rdl:PCA_100006533 rdf:type owl:Class ;
                  rdfs:subClassOf rdl:PCA_100004908 ;
                  rdl:PCA_100006763 "To document weld traceability." ;
                  rdl:PCA_100006766 rdl:PCA_100006653 ;
                  rdl:PCA_100006768 "Report containing all weld numbers in a series or an assembly with reference\nto WPS, WPQR, welder, PWHT, NDT etc." ;
                  rdfs:comment "Report containing all weld numbers in a series or an assembly with reference\nto WPS, WPQR, welder, PWHT, NDT etc." ;
                  rdfs:label "Welding plan" ;
                  skos:broadMatch rdl:PCA_100006733 ;
                  skos:broader rdl:PCA_100006756 .


###  http://rds.posccaesar.org/ontology/plm/rdl/PCA_100006534
rdl:PCA_100006534 rdf:type owl:Class ;
                  rdfs:subClassOf rdl:PCA_100004908 ;
                  rdl:PCA_100006763 "A document containing data which records compliance with specified procedure. \n* This document is a part of the Quality Assurance Plan, and herein the Quality Control  work process and verification." ;
                  rdl:PCA_100006764 "Requirements related to assurance and check of quality in manufacturing phase will very much depend on Purchaser’s knowledge of supplier. Well known supplier, with proven track record, delivering products based on industry standards, will typically deliver less verification documentation to Purchaser than unknown/new supplier delivering the same product. Therefore, this deliverable should be evaluated as candidate for being available in digital format to Purchaser, for information only." ;
                  rdl:PCA_100006766 rdl:PCA_100006653 ;
                  rdl:PCA_100006768 "Welding and material test records as set out by the welding procedure qualification\nThis record  shall contain all necessary data needed for qualification of a welding procedure specification." ;
                  rdfs:comment "Welding and material test records as set out by the welding procedure qualification\nThis record  shall contain all necessary data needed for qualification of a welding procedure specification." ;
                  rdfs:label "Welding procedure qualification record" ;
                  skos:broadMatch rdl:PCA_100006672 ,
                                  rdl:PCA_100006722 ;
                  skos:broader rdl:PCA_100006751 .


###  http://rds.posccaesar.org/ontology/plm/rdl/PCA_100006535
rdl:PCA_100006535 rdf:type owl:Class ;
                  rdfs:subClassOf rdl:PCA_100004908 ;
                  rdl:PCA_100006763 "Document the qualified welding processes and materials within defined limitations." ;
                  rdl:PCA_100006765 rrdl:CFIHOS-20000031 ;
                  rdl:PCA_100006766 rdl:PCA_100006653 ;
                  rdl:PCA_100006768 "Record comprising all necessary data needed for qualification of a preliminary welding procedure specification." ;
                  rdfs:comment "Record comprising all necessary data needed for qualification of a preliminary welding procedure specification." ;
                  rdfs:label "Welding procedure qualification record (WPQR)" ;
                  skos:broadMatch rdl:PCA_100006688 ;
                  skos:broader rdl:PCA_100006756 .


###  http://rds.posccaesar.org/ontology/plm/rdl/PCA_100006536
rdl:PCA_100006536 rdf:type owl:Class ;
                  rdfs:subClassOf rdl:PCA_100004908 ;
                  rdl:PCA_100006763 "This document is a part of the Quality Assurance Plan, and herein the Quality Assurance work process and verification.\nThis document provides a procedure for welding operator to ensure repeatability and formalism and hence prove the quality of the welding work." ;
                  rdl:PCA_100006764 "Minor weld procedures are not required for Norsok M-650 approved manufacturers (covered by approval).\n \nRequirements related to assurance and check of quality in manufacturing phase will very much depend on Purchaser’s knowledge of supplier. Well known supplier, with proven track record, delivering products based on industry standards, will typically deliver less verification documentation to Purchaser than unknown/new supplier delivering the same product. Therefore, this deliverable should be evaluated as candidate for being available in digital format to Purchaser, for information only." ;
                  rdl:PCA_100006766 rdl:PCA_100006653 ;
                  rdl:PCA_100006768 "Procedure in accordance with international standards." ;
                  rdfs:comment "Procedure in accordance with international standards." ;
                  rdfs:label "Welding procedure specification" ;
                  skos:broadMatch rdl:PCA_100006687 ;
                  skos:broader rdl:PCA_100006757 .


###  http://rds.posccaesar.org/ontology/plm/rdl/PCA_100006537
rdl:PCA_100006537 rdf:type owl:Class ;
                  rdfs:subClassOf rdl:PCA_100004908 ;
                  rdl:PCA_100006763 "Provide clear specification to welder to ensure repeatability of acceptable results." ;
                  rdl:PCA_100006764 "A Welding Procedure or Welding Procedure Specification (WPS) is generic information which is a written instruction that specifies materials, consumables and edge preparations for a given joint.\nIt lists the pre- and post-weld operations including heat treatments; machining, grinding and dressing of the weld; details the welding variables and the run sequence; and may specify the acceptance criteria and inspection methods.\n\nThe purpose of the WPS is to ensure that acceptance criteria can be met consistently, including mechanical properties and defect levels. It is also useful in enforcing quality control procedures, in standardising on welding methods, production times and costs and in controlling production schedules. Its prime purpose, however, is to give the welder clear, unequivocal nstructions on howa weld is to be made." ;
                  rdl:PCA_100006765 rrdl:CFIHOS-20000031 ;
                  rdl:PCA_100006766 rdl:PCA_100006653 ;
                  rdl:PCA_100006768 "Document that has been qualified and provides the required variables of the welding procedure." ;
                  rdfs:comment "Document that has been qualified and provides the required variables of the welding procedure." ;
                  rdfs:label "Welding procedure specification (WPS)" ;
                  skos:broadMatch rdl:PCA_100006688 ;
                  skos:broader rdl:PCA_100006757 .


###  http://rds.posccaesar.org/ontology/plm/rdl/PCA_100006538
rdl:PCA_100006538 rdf:type owl:Class ;
                  rdfs:subClassOf rdl:PCA_100004908 ;
                  rdl:PCA_100006763 "To document weld traceability." ;
                  rdl:PCA_100006765 rrdl:CFIHOS-20000031 ;
                  rdl:PCA_100006766 rdl:PCA_100006653 ;
                  rdl:PCA_100006768 "Report containing all weld numbers in a series or an assembly with reference to WPS, WPQR, welder, PWHT, NDT etc." ;
                  rdfs:comment "Report containing all weld numbers in a series or an assembly with reference to WPS, WPQR, welder, PWHT, NDT etc." ;
                  rdfs:label "Welding report / log" ;
                  skos:broadMatch rdl:PCA_100006722 ;
                  skos:broader rdl:PCA_100006748 .


###  http://rds.posccaesar.org/ontology/plm/rdl/PCA_100006539
rdl:PCA_100006539 rdf:type owl:Class ;
                  rdfs:subClassOf rdl:PCA_100004908 ;
                  rdl:PCA_100006763 "Precise determination of the well direction/path is important due to:\n - Position of well within defined target(s)\n - Avoid penetrating another well\n - Facilitate intersection of the wellbore with a relief well\n - Facilitate geological modelling\n - Facilitate anti-collision assessment for new wells\n - Input Intervention design simulation for wireline/coil tubing /snubbing\n - Input to casing design\n - Input to tubing design" ;
                  rdl:PCA_100006764 "Master data for survey data is stored in Wellview/compass" ;
                  rdl:PCA_100006765 rrdl:CFIHOS-20000042 ;
                  rdl:PCA_100006768 "The well trajectory documents the direction in which the well is drilled. It shall be defined in accordance with TCD 6501 and should as a minimum contain:\n - Measured depht \n - Inclination\n - Azimuth\n - True vertical depht" ;
                  rdfs:comment "The well trajectory documents the direction in which the well is drilled. It shall be defined in accordance with TCD 6501 and should as a minimum contain:\n - Measured depht \n - Inclination\n - Azimuth\n - True vertical depht" ;
                  rdfs:label "Well tracjectory" ;
                  skos:broadMatch rdl:PCA_100006727 ,
                                  rdl:PCA_100006728 ;
                  skos:broader rdl:PCA_100006748 .


###  http://rds.posccaesar.org/ontology/plm/rdl/PCA_100006540
rdl:PCA_100006540 rdf:type owl:Class ;
                  rdfs:subClassOf rdl:PCA_100004908 ;
                  rdl:PCA_100006763 "The report or collection of reports shall document the wind tunnel test and describe the results of the testing." ;
                  rdl:PCA_100006765 rrdl:CFIHOS-20000033 ;
                  rdl:PCA_100006766 rdl:PCA_100006653 ;
                  rdfs:label "Wind tunnel test report" ;
                  skos:broadMatch rdl:PCA_100006722 ;
                  skos:broader rdl:PCA_100006756 .


###  http://rds.posccaesar.org/ontology/plm/rdl/PCA_100006541
rdl:PCA_100006541 rdf:type owl:Class ;
                  rdfs:subClassOf rdl:PCA_100004908 ;
                  rdl:PCA_100006763 "This document describes use of WSN (Wireless Sensor Network) in the process plant." ;
                  rdl:PCA_100006765 rrdl:CFIHOS-20000015 ;
                  rdl:PCA_100006766 rdl:PCA_100006640 ;
                  rdl:PCA_100006768 "Shall include:\n - WSN topology;\n - WSN standard;\n - Coverage chart/maps of WSN with identified sensor and access point locations (gateways);\n - Expected latency time (normal/max);\n - Expected battery lifetime (normal/min);\n - Type and ENS tag number of sensors connected to one gateway;\n - Spare availability (number of sensors) to one gateway;\n - A frequency plan for co-existence of WLAN and WSN with specification of dedicated channels for WSN;\n - Any requirements for radio silence due to special operations (e.g. well perforation);\n - Recommended precautions due to radio silence;\n - Recommended precautions due to loss of one gateway." ;
                  rdfs:comment "Shall include:\n - WSN topology;\n - WSN standard;\n - Coverage chart/maps of WSN with identified sensor and access point locations (gateways);\n - Expected latency time (normal/max);\n - Expected battery lifetime (normal/min);\n - Type and ENS tag number of sensors connected to one gateway;\n - Spare availability (number of sensors) to one gateway;\n - A frequency plan for co-existence of WLAN and WSN with specification of dedicated channels for WSN;\n - Any requirements for radio silence due to special operations (e.g. well perforation);\n - Recommended precautions due to radio silence;\n - Recommended precautions due to loss of one gateway." ;
                  rdfs:label "Wireless network coverage" ;
                  skos:broadMatch rdl:PCA_100006705 ,
                                  rdl:PCA_100006722 ;
                  skos:broader rdl:PCA_100006756 .


###  http://rds.posccaesar.org/ontology/plm/rdl/PCA_100006542
rdl:PCA_100006542 rdf:type owl:Class ;
                  rdfs:subClassOf rdl:PCA_100004908 ;
                  rdl:PCA_100006763 "Ensure safe operation" ;
                  rdl:PCA_100006765 rrdl:CFIHOS-20000018 ;
                  rdl:PCA_100006766 rdl:PCA_100006657 ;
                  rdl:PCA_100006768 "The wiring diagrams for onshore cathodic protection shall cover wire colour, -type, -dimension and -connections." ;
                  rdfs:comment "The wiring diagrams for onshore cathodic protection shall cover wire colour, -type, -dimension and -connections." ;
                  rdfs:label "Wiring diagrams for onshore cathodic protection" ;
                  skos:broadMatch rdl:PCA_100006708 ;
                  skos:broader rdl:PCA_100006745 .


###  http://rds.posccaesar.org/ontology/plm/rdl/PCA_100006543
rdl:PCA_100006543 rdf:type owl:Class ;
                  rdfs:subClassOf rdl:PCA_100004908 ;
                  rdl:PCA_100006765 rrdl:CFIHOS-20000030 ;
                  rdl:PCA_100006766 rdl:PCA_100006640 ;
                  rdl:PCA_100006768 "Wireless Local Area Network (WLAN) coverage chart/test report shall be provided." ;
                  rdfs:comment "Wireless Local Area Network (WLAN) coverage chart/test report shall be provided." ;
                  rdfs:label "WLAN coverage" ;
                  skos:broadMatch rdl:PCA_100006705 ,
                                  rdl:PCA_100006722 ;
                  skos:broader rdl:PCA_100006756 .


###  http://rds.posccaesar.org/ontology/plm/rdl/PCA_100006544
rdl:PCA_100006544 rdf:type owl:Class ;
                  rdfs:subClassOf rdl:PCA_100004908 ;
                  rdl:PCA_100006763 "Measurements and documentation on risk assessments and risk mitigation in design for the WE Factors; noise, vibrations, chemical and biological exposure, access, ergonomics, outdoor operations, illumination and radiation. The information shall be linked to relevant tag numbers and/or area codes." ;
                  rdl:PCA_100006765 rrdl:CFIHOS-20000010 ,
                                    rrdl:CFIHOS-20000011 ,
                                    rrdl:CFIHOS-20000013 ;
                  rdl:PCA_100006766 rdl:PCA_100006654 ;
                  rdfs:label "Working environment status" ;
                  skos:broadMatch rdl:PCA_100006716 ;
                  skos:broader rdl:PCA_100006748 .


###  http://rds.posccaesar.org/ontology/plm/rdl/PCA_100006545
rdl:PCA_100006545 rdf:type owl:Class ;
                  rdfs:subClassOf rdl:PCA_100004908 ;
                  rdl:PCA_100006765 rrdl:CFIHOS-20000010 ,
                                    rrdl:CFIHOS-20000011 ,
                                    rrdl:CFIHOS-20000013 ;
                  rdl:PCA_100006766 rdl:PCA_100006654 ;
                  rdl:PCA_100006768 "The report shall include: \n - Documentation of all remaining risks not eliminated through design solutions and relevant for normal operations, inspection and maintenance\n - Updated WEHRA\n - Working Environment Area Charts" ;
                  rdfs:comment "The report shall include: \n - Documentation of all remaining risks not eliminated through design solutions and relevant for normal operations, inspection and maintenance\n - Updated WEHRA\n - Working Environment Area Charts" ;
                  rdfs:label "Working environment summary report" ;
                  skos:broadMatch rdl:PCA_100006726 ;
                  skos:broader rdl:PCA_100006756 .


###  http://rds.posccaesar.org/ontology/plm/rdl/PCA_100006546
rdl:PCA_100006546 rdf:type owl:Class ;
                  rdfs:subClassOf rdl:PCA_100004908 ;
                  rdl:PCA_100006764 "Tabell tilhørende 5.248, SR-2800, Workshop maintenance manuals" ;
                  rdl:PCA_100006768 "The Workshop maintenance manuals shall be used for subsea equipment, and equipment related to the subsea equipment. The Workshop maintenance manuals shall include: 1. All necessary procedures to perform Mobilisation & demobilisation 2. All necessary procedures to perform component replacement 3. All necessary procedures to perform Main overhaul\n\nGeneral \nMain overhaul includes all inspections, measurements, acceptance criteria’s, adjustments and operations carried out directly on the equipment in order to ensure safe, reliable and economical operation. This item must be seen in combination with the installation, operation and maintenance manual (IOM manual). Typical equipment and operations this is relevant for see table below. The O marked section(s,) the required workshop maintenance manual section shall be retained by vendor and made available upon request for Company." ;
                  rdfs:comment "The Workshop maintenance manuals shall be used for subsea equipment, and equipment related to the subsea equipment. The Workshop maintenance manuals shall include: 1. All necessary procedures to perform Mobilisation & demobilisation 2. All necessary procedures to perform component replacement 3. All necessary procedures to perform Main overhaul\n\nGeneral \nMain overhaul includes all inspections, measurements, acceptance criteria’s, adjustments and operations carried out directly on the equipment in order to ensure safe, reliable and economical operation. This item must be seen in combination with the installation, operation and maintenance manual (IOM manual). Typical equipment and operations this is relevant for see table below. The O marked section(s,) the required workshop maintenance manual section shall be retained by vendor and made available upon request for Company." ;
                  rdfs:label "Workshop maintenance manuals" .


#################################################################
#    Individuals
#################################################################

###  http://rds.posccaesar.org/ontology/plm/rdl/PCA_100006578
rdl:PCA_100006578 rdf:type owl:NamedIndividual ,
                           rdl:PCA_100001503 ;
                  rdl:PCA_100004924 "10" ;
                  rdfs:label "Drilling" .


###  http://rds.posccaesar.org/ontology/plm/rdl/PCA_100006579
rdl:PCA_100006579 rdf:type owl:NamedIndividual ,
                           rdl:PCA_100001503 ;
                  rdl:PCA_100004924 "11" ;
                  rdfs:label "Drilling process" .


###  http://rds.posccaesar.org/ontology/plm/rdl/PCA_100006580
rdl:PCA_100006580 rdf:type owl:NamedIndividual ,
                           rdl:PCA_100001503 ;
                  rdl:PCA_100004924 "12" ;
                  rdfs:label "Drilling well control" .


###  http://rds.posccaesar.org/ontology/plm/rdl/PCA_100006581
rdl:PCA_100006581 rdf:type owl:NamedIndividual ,
                           rdl:PCA_100001503 ;
                  rdl:PCA_100004924 "13" ;
                  rdfs:label "Riser and well topside" .


###  http://rds.posccaesar.org/ontology/plm/rdl/PCA_100006582
rdl:PCA_100006582 rdf:type owl:NamedIndividual ,
                           rdl:PCA_100001503 ;
                  rdl:PCA_100004924 "14" ;
                  rdfs:label "Drilling control and monitoring" .


###  http://rds.posccaesar.org/ontology/plm/rdl/PCA_100006583
rdl:PCA_100006583 rdf:type owl:NamedIndividual ,
                           rdl:PCA_100001503 ;
                  rdl:PCA_100004924 "15" ;
                  rdfs:label "Drilling drain" .


###  http://rds.posccaesar.org/ontology/plm/rdl/PCA_100006584
rdl:PCA_100006584 rdf:type owl:NamedIndividual ,
                           rdl:PCA_100001503 ;
                  rdl:PCA_100004924 "18" ;
                  rdfs:label "Well and riser subsea" .


###  http://rds.posccaesar.org/ontology/plm/rdl/PCA_100006585
rdl:PCA_100006585 rdf:type owl:NamedIndividual ,
                           rdl:PCA_100001503 ;
                  rdl:PCA_100004924 "19" ;
                  rdfs:label "Subsea installation - maintenance and work over" .


###  http://rds.posccaesar.org/ontology/plm/rdl/PCA_100006586
rdl:PCA_100006586 rdf:type owl:NamedIndividual ,
                           rdl:PCA_100001503 ;
                  rdl:PCA_100004924 "20" ;
                  rdfs:label "Separation and stabilisation" .


###  http://rds.posccaesar.org/ontology/plm/rdl/PCA_100006587
rdl:PCA_100006587 rdf:type owl:NamedIndividual ,
                           rdl:PCA_100001503 ;
                  rdl:PCA_100004924 "21" ;
                  rdfs:label "Crude handling and metering" .


###  http://rds.posccaesar.org/ontology/plm/rdl/PCA_100006588
rdl:PCA_100006588 rdf:type owl:NamedIndividual ,
                           rdl:PCA_100001503 ;
                  rdl:PCA_100004924 "23" ;
                  rdfs:label "Gas compression and re-injection" .


###  http://rds.posccaesar.org/ontology/plm/rdl/PCA_100006589
rdl:PCA_100006589 rdf:type owl:NamedIndividual ,
                           rdl:PCA_100001503 ;
                  rdl:PCA_100004924 "24" ;
                  rdfs:label "Gas treatment" .


###  http://rds.posccaesar.org/ontology/plm/rdl/PCA_100006590
rdl:PCA_100006590 rdf:type owl:NamedIndividual ,
                           rdl:PCA_100001503 ;
                  rdl:PCA_100004924 "25" ;
                  rdfs:label "Gas conditioning" .


###  http://rds.posccaesar.org/ontology/plm/rdl/PCA_100006591
rdl:PCA_100006591 rdf:type owl:NamedIndividual ,
                           rdl:PCA_100001503 ;
                  rdl:PCA_100004924 "27" ;
                  rdfs:label "Gas export and metering" .


###  http://rds.posccaesar.org/ontology/plm/rdl/PCA_100006592
rdl:PCA_100006592 rdf:type owl:NamedIndividual ,
                           rdl:PCA_100001503 ;
                  rdl:PCA_100004924 "28" ;
                  rdfs:label "Gas sweetening" .


###  http://rds.posccaesar.org/ontology/plm/rdl/PCA_100006593
rdl:PCA_100006593 rdf:type owl:NamedIndividual ,
                           rdl:PCA_100001503 ;
                  rdl:PCA_100004924 "29" ;
                  rdfs:label "Water injection" .


###  http://rds.posccaesar.org/ontology/plm/rdl/PCA_100006594
rdl:PCA_100006594 rdf:type owl:NamedIndividual ,
                           rdl:PCA_100001503 ;
                  rdl:PCA_100004924 "30" ;
                  rdfs:label "Oil export line" .


###  http://rds.posccaesar.org/ontology/plm/rdl/PCA_100006595
rdl:PCA_100006595 rdf:type owl:NamedIndividual ,
                           rdl:PCA_100001503 ;
                  rdl:PCA_100004924 "31" ;
                  rdfs:label "Condensate export line" .


###  http://rds.posccaesar.org/ontology/plm/rdl/PCA_100006596
rdl:PCA_100006596 rdf:type owl:NamedIndividual ,
                           rdl:PCA_100001503 ;
                  rdl:PCA_100004924 "32" ;
                  rdfs:label "Gas export pipeline" .


###  http://rds.posccaesar.org/ontology/plm/rdl/PCA_100006597
rdl:PCA_100006597 rdf:type owl:NamedIndividual ,
                           rdl:PCA_100001503 ;
                  rdl:PCA_100004924 "33" ;
                  rdfs:label "Oil storage" .


###  http://rds.posccaesar.org/ontology/plm/rdl/PCA_100006598
rdl:PCA_100006598 rdf:type owl:NamedIndividual ,
                           rdl:PCA_100001503 ;
                  rdl:PCA_100004924 "34" ;
                  rdfs:label "Injection water pipeline" .


###  http://rds.posccaesar.org/ontology/plm/rdl/PCA_100006599
rdl:PCA_100006599 rdf:type owl:NamedIndividual ,
                           rdl:PCA_100001503 ;
                  rdl:PCA_100004924 "35" ;
                  rdfs:label "Chemical injection pipeline" .


###  http://rds.posccaesar.org/ontology/plm/rdl/PCA_100006600
rdl:PCA_100006600 rdf:type owl:NamedIndividual ,
                           rdl:PCA_100001503 ;
                  rdl:PCA_100004924 "36" ;
                  rdfs:label "Wellstream pipeline" .


###  http://rds.posccaesar.org/ontology/plm/rdl/PCA_100006601
rdl:PCA_100006601 rdf:type owl:NamedIndividual ,
                           rdl:PCA_100001503 ;
                  rdl:PCA_100004924 "37" ;
                  rdfs:label "Gas injection pipeline" .


###  http://rds.posccaesar.org/ontology/plm/rdl/PCA_100006602
rdl:PCA_100006602 rdf:type owl:NamedIndividual ,
                           rdl:PCA_100001503 ;
                  rdl:PCA_100004924 "38" ;
                  rdfs:label "Glycol / methanol regeneration" .


###  http://rds.posccaesar.org/ontology/plm/rdl/PCA_100006603
rdl:PCA_100006603 rdf:type owl:NamedIndividual ,
                           rdl:PCA_100001503 ;
                  rdl:PCA_100004924 "39" ;
                  rdfs:label "Loading" .


###  http://rds.posccaesar.org/ontology/plm/rdl/PCA_100006604
rdl:PCA_100006604 rdf:type owl:NamedIndividual ,
                           rdl:PCA_100001503 ;
                  rdl:PCA_100004924 "40" ;
                  rdfs:label "Cooling medium" .


###  http://rds.posccaesar.org/ontology/plm/rdl/PCA_100006605
rdl:PCA_100006605 rdf:type owl:NamedIndividual ,
                           rdl:PCA_100001503 ;
                  rdl:PCA_100004924 "41" ;
                  rdfs:label "Heating medium" .


###  http://rds.posccaesar.org/ontology/plm/rdl/PCA_100006606
rdl:PCA_100006606 rdf:type owl:NamedIndividual ,
                           rdl:PCA_100001503 ;
                  rdl:PCA_100004924 "42" ;
                  rdfs:label "Chemical injection" .


###  http://rds.posccaesar.org/ontology/plm/rdl/PCA_100006607
rdl:PCA_100006607 rdf:type owl:NamedIndividual ,
                           rdl:PCA_100001503 ;
                  rdl:PCA_100004924 "43" ;
                  rdfs:label "Flare" .


###  http://rds.posccaesar.org/ontology/plm/rdl/PCA_100006608
rdl:PCA_100006608 rdf:type owl:NamedIndividual ,
                           rdl:PCA_100001503 ;
                  rdl:PCA_100004924 "44" ;
                  rdfs:label "Oily water" .


###  http://rds.posccaesar.org/ontology/plm/rdl/PCA_100006609
rdl:PCA_100006609 rdf:type owl:NamedIndividual ,
                           rdl:PCA_100001503 ;
                  rdl:PCA_100004924 "45" ;
                  rdfs:label "Fuel gas" .


###  http://rds.posccaesar.org/ontology/plm/rdl/PCA_100006610
rdl:PCA_100006610 rdf:type owl:NamedIndividual ,
                           rdl:PCA_100001503 ;
                  rdl:PCA_100004924 "46" ;
                  rdfs:label "Methanol injection" .


###  http://rds.posccaesar.org/ontology/plm/rdl/PCA_100006611
rdl:PCA_100006611 rdf:type owl:NamedIndividual ,
                           rdl:PCA_100001503 ;
                  rdl:PCA_100004924 "47" ;
                  rdfs:label "Chlorination" .


###  http://rds.posccaesar.org/ontology/plm/rdl/PCA_100006612
rdl:PCA_100006612 rdf:type owl:NamedIndividual ,
                           rdl:PCA_100001503 ;
                  rdl:PCA_100004924 "50" ;
                  rdfs:label "Sea water" .


###  http://rds.posccaesar.org/ontology/plm/rdl/PCA_100006613
rdl:PCA_100006613 rdf:type owl:NamedIndividual ,
                           rdl:PCA_100001503 ;
                  rdl:PCA_100004924 "52" ;
                  rdfs:label "Ballast water" .


###  http://rds.posccaesar.org/ontology/plm/rdl/PCA_100006614
rdl:PCA_100006614 rdf:type owl:NamedIndividual ,
                           rdl:PCA_100001503 ;
                  rdl:PCA_100004924 "53" ;
                  rdfs:label "Fresh water" .


###  http://rds.posccaesar.org/ontology/plm/rdl/PCA_100006615
rdl:PCA_100006615 rdf:type owl:NamedIndividual ,
                           rdl:PCA_100001503 ;
                  rdl:PCA_100004924 "55" ;
                  rdfs:label "Steam" .


###  http://rds.posccaesar.org/ontology/plm/rdl/PCA_100006616
rdl:PCA_100006616 rdf:type owl:NamedIndividual ,
                           rdl:PCA_100001503 ;
                  rdl:PCA_100004924 "56" ;
                  rdfs:label "Open drain" .


###  http://rds.posccaesar.org/ontology/plm/rdl/PCA_100006617
rdl:PCA_100006617 rdf:type owl:NamedIndividual ,
                           rdl:PCA_100001503 ;
                  rdl:PCA_100004924 "57" ;
                  rdfs:label "Closed drain" .


###  http://rds.posccaesar.org/ontology/plm/rdl/PCA_100006618
rdl:PCA_100006618 rdf:type owl:NamedIndividual ,
                           rdl:PCA_100001503 ;
                  rdl:PCA_100004924 "58" ;
                  rdfs:label "Thruster and propulsion" .


###  http://rds.posccaesar.org/ontology/plm/rdl/PCA_100006619
rdl:PCA_100006619 rdf:type owl:NamedIndividual ,
                           rdl:PCA_100001503 ;
                  rdl:PCA_100004924 "61" ;
                  rdfs:label "Jet fuel" .


###  http://rds.posccaesar.org/ontology/plm/rdl/PCA_100006620
rdl:PCA_100006620 rdf:type owl:NamedIndividual ,
                           rdl:PCA_100001503 ;
                  rdl:PCA_100004924 "62" ;
                  rdfs:label "Diesel oil" .


###  http://rds.posccaesar.org/ontology/plm/rdl/PCA_100006621
rdl:PCA_100006621 rdf:type owl:NamedIndividual ,
                           rdl:PCA_100001503 ;
                  rdl:PCA_100004924 "63" ;
                  rdfs:label "Compressed air" .


###  http://rds.posccaesar.org/ontology/plm/rdl/PCA_100006622
rdl:PCA_100006622 rdf:type owl:NamedIndividual ,
                           rdl:PCA_100001503 ;
                  rdl:PCA_100004924 "64" ;
                  rdfs:label "Inert gas" .


###  http://rds.posccaesar.org/ontology/plm/rdl/PCA_100006623
rdl:PCA_100006623 rdf:type owl:NamedIndividual ,
                           rdl:PCA_100001503 ;
                  rdl:PCA_100004924 "65" ;
                  rdfs:label "Hydraulic power" .


###  http://rds.posccaesar.org/ontology/plm/rdl/PCA_100006624
rdl:PCA_100006624 rdf:type owl:NamedIndividual ,
                           rdl:PCA_100001503 ;
                  rdl:PCA_100004924 "66" ;
                  rdfs:label "Sewage treatment" .


###  http://rds.posccaesar.org/ontology/plm/rdl/PCA_100006625
rdl:PCA_100006625 rdf:type owl:NamedIndividual ,
                           rdl:PCA_100001503 ;
                  rdl:PCA_100004924 "69" ;
                  rdfs:label "Lubrication oil" .


###  http://rds.posccaesar.org/ontology/plm/rdl/PCA_100006626
rdl:PCA_100006626 rdf:type owl:NamedIndividual ,
                           rdl:PCA_100001503 ;
                  rdl:PCA_100004924 "70" ;
                  rdfs:label "Fire and gas detection" .


###  http://rds.posccaesar.org/ontology/plm/rdl/PCA_100006627
rdl:PCA_100006627 rdf:type owl:NamedIndividual ,
                           rdl:PCA_100001503 ;
                  rdl:PCA_100004924 "71" ;
                  rdfs:label "Fire water" .


###  http://rds.posccaesar.org/ontology/plm/rdl/PCA_100006628
rdl:PCA_100006628 rdf:type owl:NamedIndividual ,
                           rdl:PCA_100001503 ;
                  rdl:PCA_100004924 "72" ;
                  rdfs:label "Fire fighting" .


###  http://rds.posccaesar.org/ontology/plm/rdl/PCA_100006629
rdl:PCA_100006629 rdf:type owl:NamedIndividual ,
                           rdl:PCA_100001503 ;
                  rdl:PCA_100004924 "73" ;
                  rdfs:label "Material handling" .


###  http://rds.posccaesar.org/ontology/plm/rdl/PCA_100006630
rdl:PCA_100006630 rdf:type owl:NamedIndividual ,
                           rdl:PCA_100001503 ;
                  rdl:PCA_100004924 "75" ;
                  rdfs:label "Passive fire protection" .


###  http://rds.posccaesar.org/ontology/plm/rdl/PCA_100006631
rdl:PCA_100006631 rdf:type owl:NamedIndividual ,
                           rdl:PCA_100001503 ;
                  rdl:PCA_100004924 "76" ;
                  rdfs:label "Emergency preparedness" .


###  http://rds.posccaesar.org/ontology/plm/rdl/PCA_100006632
rdl:PCA_100006632 rdf:type owl:NamedIndividual ,
                           rdl:PCA_100001503 ;
                  rdl:PCA_100004924 "77" ;
                  rdfs:label "Environment protection" .


###  http://rds.posccaesar.org/ontology/plm/rdl/PCA_100006633
rdl:PCA_100006633 rdf:type owl:NamedIndividual ,
                           rdl:PCA_100001503 ;
                  rdl:PCA_100004924 "79" ;
                  rdfs:label "Emergency shutdown and blow down" .


###  http://rds.posccaesar.org/ontology/plm/rdl/PCA_100006634
rdl:PCA_100006634 rdf:type owl:NamedIndividual ,
                           rdl:PCA_100001503 ;
                  rdl:PCA_100004924 "80" ;
                  rdfs:label "Main power (u =or >6.6 kV)" .


###  http://rds.posccaesar.org/ontology/plm/rdl/PCA_100006635
rdl:PCA_100006635 rdf:type owl:NamedIndividual ,
                           rdl:PCA_100001503 ;
                  rdl:PCA_100004924 "81" ;
                  rdfs:label "Main power (1.0 kV< u < 6.6 kV)" .


###  http://rds.posccaesar.org/ontology/plm/rdl/PCA_100006636
rdl:PCA_100006636 rdf:type owl:NamedIndividual ,
                           rdl:PCA_100001503 ;
                  rdl:PCA_100004924 "82" ;
                  rdfs:label "Main power (u = or <1.0 kV)" .


###  http://rds.posccaesar.org/ontology/plm/rdl/PCA_100006637
rdl:PCA_100006637 rdf:type owl:NamedIndividual ,
                           rdl:PCA_100001503 ;
                  rdl:PCA_100004924 "83" ;
                  rdfs:label "Emergency power (u = or >1.0 kV)" .


###  http://rds.posccaesar.org/ontology/plm/rdl/PCA_100006638
rdl:PCA_100006638 rdf:type owl:NamedIndividual ,
                           rdl:PCA_100001503 ;
                  rdl:PCA_100004924 "84" ;
                  rdfs:label "Emergency power (u<1.0 kV)" .


###  http://rds.posccaesar.org/ontology/plm/rdl/PCA_100006639
rdl:PCA_100006639 rdf:type owl:NamedIndividual ,
                           rdl:PCA_100001503 ;
                  rdl:PCA_100004924 "85" ;
                  rdfs:label "Battery and no-break" .


###  http://rds.posccaesar.org/ontology/plm/rdl/PCA_100006640
rdl:PCA_100006640 rdf:type owl:NamedIndividual ,
                           rdl:PCA_100001503 ;
                  rdl:PCA_100004924 "86" ;
                  rdfs:label "Telecommunication" .


###  http://rds.posccaesar.org/ontology/plm/rdl/PCA_100006641
rdl:PCA_100006641 rdf:type owl:NamedIndividual ,
                           rdl:PCA_100001503 ;
                  rdl:PCA_100004924 "87" ;
                  rdfs:label "Control" .


###  http://rds.posccaesar.org/ontology/plm/rdl/PCA_100006642
rdl:PCA_100006642 rdf:type owl:NamedIndividual ,
                           rdl:PCA_100001503 ;
                  rdl:PCA_100004924 "88" ;
                  rdfs:label "Earthing and lightning" .


###  http://rds.posccaesar.org/ontology/plm/rdl/PCA_100006643
rdl:PCA_100006643 rdf:type owl:NamedIndividual ,
                           rdl:PCA_100001503 ;
                  rdl:PCA_100004924 "90" ;
                  rdfs:label "Topside structure" .


###  http://rds.posccaesar.org/ontology/plm/rdl/PCA_100006644
rdl:PCA_100006644 rdf:type owl:NamedIndividual ,
                           rdl:PCA_100001503 ;
                  rdl:PCA_100004924 "91" ;
                  rdfs:label "Sub structure" .


###  http://rds.posccaesar.org/ontology/plm/rdl/PCA_100006645
rdl:PCA_100006645 rdf:type owl:NamedIndividual ,
                           rdl:PCA_100001503 ;
                  rdl:PCA_100004924 "92" ;
                  rdfs:label "Temporary" .


###  http://rds.posccaesar.org/ontology/plm/rdl/PCA_100006646
rdl:PCA_100006646 rdf:type owl:NamedIndividual ,
                           rdl:PCA_100001503 ;
                  rdl:PCA_100004924 "93" ;
                  rdfs:label "Architectural incl. Workshop and storage" .


###  http://rds.posccaesar.org/ontology/plm/rdl/PCA_100006647
rdl:PCA_100006647 rdf:type owl:NamedIndividual ,
                           rdl:PCA_100001503 ;
                  rdl:PCA_100004924 "94" ;
                  rdfs:label "Mooring and positioning" .


###  http://rds.posccaesar.org/ontology/plm/rdl/PCA_100006648
rdl:PCA_100006648 rdf:type owl:NamedIndividual ,
                           rdl:PCA_100001503 ;
                  rdl:PCA_100004924 "95" ;
                  rdfs:label "Onshore/civil" .


###  http://rds.posccaesar.org/ontology/plm/rdl/PCA_100006649
rdl:PCA_100006649 rdf:type owl:NamedIndividual ,
                           rdl:PCA_100001503 ;
                  rdl:PCA_100004924 "96" ;
                  rdfs:label "Subsea structure and template" .


###  http://rds.posccaesar.org/ontology/plm/rdl/PCA_100006650
rdl:PCA_100006650 rdf:type owl:NamedIndividual ,
                           rdl:PCA_100001503 ;
                  rdl:PCA_100004924 "97" ;
                  rdfs:label "HVAC" .


###  http://rds.posccaesar.org/ontology/plm/rdl/PCA_100006651
rdl:PCA_100006651 rdf:type owl:NamedIndividual ,
                           rdl:PCA_100001503 ;
                  rdl:PCA_100004924 "98" ;
                  rdfs:label "Corrosion protection" .


###  http://rds.posccaesar.org/ontology/plm/rdl/PCA_100006652
rdl:PCA_100006652 rdf:type owl:NamedIndividual ,
                           rdl:PCA_100001503 ;
                  rdl:PCA_100004924 "99" ;
                  rdfs:label "Area Completion" .


###  http://rds.posccaesar.org/ontology/plm/rdl/PCA_100006653
rdl:PCA_100006653 rdf:type owl:NamedIndividual ,
                           rdl:PCA_100001503 ;
                  rdfs:label "Equipment" .


###  http://rds.posccaesar.org/ontology/plm/rdl/PCA_100006654
rdl:PCA_100006654 rdf:type owl:NamedIndividual ,
                           rdl:PCA_100001503 ;
                  rdfs:label "Facility" .


###  http://rds.posccaesar.org/ontology/plm/rdl/PCA_100006655
rdl:PCA_100006655 rdf:type owl:NamedIndividual ,
                           rdl:PCA_100001503 ;
                  rdfs:label "Function" .


###  http://rds.posccaesar.org/ontology/plm/rdl/PCA_100006656
rdl:PCA_100006656 rdf:type owl:NamedIndividual ,
                           rdl:PCA_100001503 ;
                  rdfs:label "Location" .


###  http://rds.posccaesar.org/ontology/plm/rdl/PCA_100006657
rdl:PCA_100006657 rdf:type owl:NamedIndividual ,
                           rdl:PCA_100001503 ;
                  rdfs:label "System" .


###  http://rds.posccaesar.org/ontology/plm/rdl/PCA_100006658
rdl:PCA_100006658 rdf:type owl:NamedIndividual ,
                           rdl:PCA_100001503 ;
                  rdl:PCA_100004924 "A" ;
                  rdfs:label "meta" .


###  http://rds.posccaesar.org/ontology/plm/rdl/PCA_100006659
rdl:PCA_100006659 rdf:type owl:NamedIndividual ,
                           rdl:PCA_100001503 ;
                  rdl:PCA_100004924 "AA" ;
                  rdfs:label "identification information" .


###  http://rds.posccaesar.org/ontology/plm/rdl/PCA_100006660
rdl:PCA_100006660 rdf:type owl:NamedIndividual ,
                           rdl:PCA_100001503 ;
                  rdl:PCA_100004924 "AB" ;
                  rdfs:label "reference information" .


###  http://rds.posccaesar.org/ontology/plm/rdl/PCA_100006661
rdl:PCA_100006661 rdf:type owl:NamedIndividual ,
                           rdl:PCA_100001503 ;
                  rdl:PCA_100004924 "AC" ;
                  rdfs:label "descriptive meta information" .


###  http://rds.posccaesar.org/ontology/plm/rdl/PCA_100006662
rdl:PCA_100006662 rdf:type owl:NamedIndividual ,
                           rdl:PCA_100001503 ;
                  rdl:PCA_100004924 "B" ;
                  rdfs:label "management" .


###  http://rds.posccaesar.org/ontology/plm/rdl/PCA_100006663
rdl:PCA_100006663 rdf:type owl:NamedIndividual ,
                           rdl:PCA_100001503 ;
                  rdl:PCA_100004924 "BA" ;
                  rdfs:label "stakeholder information" .


###  http://rds.posccaesar.org/ontology/plm/rdl/PCA_100006664
rdl:PCA_100006664 rdf:type owl:NamedIndividual ,
                           rdl:PCA_100001503 ;
                  rdl:PCA_100004924 "BB" ;
                  rdfs:label "observation management information" .


###  http://rds.posccaesar.org/ontology/plm/rdl/PCA_100006665
rdl:PCA_100006665 rdf:type owl:NamedIndividual ,
                           rdl:PCA_100001503 ;
                  rdl:PCA_100004924 "BC" ;
                  rdfs:label "correspondence information" .


###  http://rds.posccaesar.org/ontology/plm/rdl/PCA_100006666
rdl:PCA_100006666 rdf:type owl:NamedIndividual ,
                           rdl:PCA_100001503 ;
                  rdl:PCA_100004924 "BD" ;
                  rdfs:label "project control information" .


###  http://rds.posccaesar.org/ontology/plm/rdl/PCA_100006667
rdl:PCA_100006667 rdf:type owl:NamedIndividual ,
                           rdl:PCA_100001503 ;
                  rdl:PCA_100004924 "BE" ;
                  rdfs:label "planning information" .


###  http://rds.posccaesar.org/ontology/plm/rdl/PCA_100006668
rdl:PCA_100006668 rdf:type owl:NamedIndividual ,
                           rdl:PCA_100001503 ;
                  rdl:PCA_100004924 "BF" ;
                  rdfs:label "logistic information" .


###  http://rds.posccaesar.org/ontology/plm/rdl/PCA_100006669
rdl:PCA_100006669 rdf:type owl:NamedIndividual ,
                           rdl:PCA_100001503 ;
                  rdl:PCA_100004924 "BG" ;
                  rdfs:label "organizational information" .


###  http://rds.posccaesar.org/ontology/plm/rdl/PCA_100006670
rdl:PCA_100006670 rdf:type owl:NamedIndividual ,
                           rdl:PCA_100001503 ;
                  rdl:PCA_100004924 "BH" ;
                  rdfs:label "change management information" .


###  http://rds.posccaesar.org/ontology/plm/rdl/PCA_100006671
rdl:PCA_100006671 rdf:type owl:NamedIndividual ,
                           rdl:PCA_100001503 ;
                  rdl:PCA_100004924 "BJ" ;
                  rdfs:label "economy information" .


###  http://rds.posccaesar.org/ontology/plm/rdl/PCA_100006672
rdl:PCA_100006672 rdf:type owl:NamedIndividual ,
                           rdl:PCA_100001503 ;
                  rdl:PCA_100004924 "BQ" ;
                  rdfs:label "quality management information" .


###  http://rds.posccaesar.org/ontology/plm/rdl/PCA_100006673
rdl:PCA_100006673 rdf:type owl:NamedIndividual ,
                           rdl:PCA_100001503 ;
                  rdl:PCA_100004924 "BU" ;
                  rdfs:label "training information" .


###  http://rds.posccaesar.org/ontology/plm/rdl/PCA_100006674
rdl:PCA_100006674 rdf:type owl:NamedIndividual ,
                           rdl:PCA_100001503 ;
                  rdl:PCA_100004924 "BW" ;
                  rdfs:label "information control management" .


###  http://rds.posccaesar.org/ontology/plm/rdl/PCA_100006675
rdl:PCA_100006675 rdf:type owl:NamedIndividual ,
                           rdl:PCA_100001503 ;
                  rdl:PCA_100004924 "C" ;
                  rdfs:label "contractual" .


###  http://rds.posccaesar.org/ontology/plm/rdl/PCA_100006676
rdl:PCA_100006676 rdf:type owl:NamedIndividual ,
                           rdl:PCA_100001503 ;
                  rdl:PCA_100004924 "CA" ;
                  rdfs:label "tender information" .


###  http://rds.posccaesar.org/ontology/plm/rdl/PCA_100006677
rdl:PCA_100006677 rdf:type owl:NamedIndividual ,
                           rdl:PCA_100001503 ;
                  rdl:PCA_100004924 "CB" ;
                  rdfs:label "authority approval information" .


###  http://rds.posccaesar.org/ontology/plm/rdl/PCA_100006678
rdl:PCA_100006678 rdf:type owl:NamedIndividual ,
                           rdl:PCA_100001503 ;
                  rdl:PCA_100004924 "CC" ;
                  rdfs:label "agreement information" .


###  http://rds.posccaesar.org/ontology/plm/rdl/PCA_100006679
rdl:PCA_100006679 rdf:type owl:NamedIndividual ,
                           rdl:PCA_100001503 ;
                  rdl:PCA_100004924 "CD" ;
                  rdfs:label "order information" .


###  http://rds.posccaesar.org/ontology/plm/rdl/PCA_100006680
rdl:PCA_100006680 rdf:type owl:NamedIndividual ,
                           rdl:PCA_100001503 ;
                  rdl:PCA_100004924 "CE" ;
                  rdfs:label "payment information" .


###  http://rds.posccaesar.org/ontology/plm/rdl/PCA_100006681
rdl:PCA_100006681 rdf:type owl:NamedIndividual ,
                           rdl:PCA_100001503 ;
                  rdl:PCA_100004924 "CF" ;
                  rdfs:label "insurance information" .


###  http://rds.posccaesar.org/ontology/plm/rdl/PCA_100006682
rdl:PCA_100006682 rdf:type owl:NamedIndividual ,
                           rdl:PCA_100001503 ;
                  rdl:PCA_100004924 "CG" ;
                  rdfs:label "warranty information" .


###  http://rds.posccaesar.org/ontology/plm/rdl/PCA_100006683
rdl:PCA_100006683 rdf:type owl:NamedIndividual ,
                           rdl:PCA_100001503 ;
                  rdl:PCA_100004924 "CH" ;
                  rdfs:label "expertise information" .


###  http://rds.posccaesar.org/ontology/plm/rdl/PCA_100006684
rdl:PCA_100006684 rdf:type owl:NamedIndividual ,
                           rdl:PCA_100001503 ;
                  rdl:PCA_100004924 "CJ" ;
                  rdfs:label "ownership information" .


###  http://rds.posccaesar.org/ontology/plm/rdl/PCA_100006685
rdl:PCA_100006685 rdf:type owl:NamedIndividual ,
                           rdl:PCA_100001503 ;
                  rdl:PCA_100004924 "D" ;
                  rdfs:label "capability" .


###  http://rds.posccaesar.org/ontology/plm/rdl/PCA_100006686
rdl:PCA_100006686 rdf:type owl:NamedIndividual ,
                           rdl:PCA_100001503 ;
                  rdl:PCA_100004924 "DA" ;
                  rdfs:label "technical property information" .


###  http://rds.posccaesar.org/ontology/plm/rdl/PCA_100006687
rdl:PCA_100006687 rdf:type owl:NamedIndividual ,
                           rdl:PCA_100001503 ;
                  rdl:PCA_100004924 "DB" ;
                  rdfs:label "explanatory technical information" .


###  http://rds.posccaesar.org/ontology/plm/rdl/PCA_100006688
rdl:PCA_100006688 rdf:type owl:NamedIndividual ,
                           rdl:PCA_100001503 ;
                  rdl:PCA_100004924 "DC" ;
                  rdfs:label "instructive information" .


###  http://rds.posccaesar.org/ontology/plm/rdl/PCA_100006689
rdl:PCA_100006689 rdf:type owl:NamedIndividual ,
                           rdl:PCA_100001503 ;
                  rdl:PCA_100004924 "DD" ;
                  rdfs:label "technical observation information" .


###  http://rds.posccaesar.org/ontology/plm/rdl/PCA_100006690
rdl:PCA_100006690 rdf:type owl:NamedIndividual ,
                           rdl:PCA_100001503 ;
                  rdl:PCA_100004924 "DE" ;
                  rdfs:label "advertising information" .


###  http://rds.posccaesar.org/ontology/plm/rdl/PCA_100006691
rdl:PCA_100006691 rdf:type owl:NamedIndividual ,
                           rdl:PCA_100001503 ;
                  rdl:PCA_100004924 "DF" ;
                  rdfs:label "scientific information" .


###  http://rds.posccaesar.org/ontology/plm/rdl/PCA_100006692
rdl:PCA_100006692 rdf:type owl:NamedIndividual ,
                           rdl:PCA_100001503 ;
                  rdl:PCA_100004924 "DG" ;
                  rdfs:label "regulatory requirement information" .


###  http://rds.posccaesar.org/ontology/plm/rdl/PCA_100006693
rdl:PCA_100006693 rdf:type owl:NamedIndividual ,
                           rdl:PCA_100001503 ;
                  rdl:PCA_100004924 "DH" ;
                  rdfs:label "standard" .


###  http://rds.posccaesar.org/ontology/plm/rdl/PCA_100006694
rdl:PCA_100006694 rdf:type owl:NamedIndividual ,
                           rdl:PCA_100001503 ;
                  rdl:PCA_100004924 "F" ;
                  rdfs:label "functionality" .


###  http://rds.posccaesar.org/ontology/plm/rdl/PCA_100006695
rdl:PCA_100006695 rdf:type owl:NamedIndividual ,
                           rdl:PCA_100001503 ;
                  rdl:PCA_100004924 "FA" ;
                  rdfs:label "system overview information" .


###  http://rds.posccaesar.org/ontology/plm/rdl/PCA_100006696
rdl:PCA_100006696 rdf:type owl:NamedIndividual ,
                           rdl:PCA_100001503 ;
                  rdl:PCA_100004924 "FB" ;
                  rdfs:label "flow information" .


###  http://rds.posccaesar.org/ontology/plm/rdl/PCA_100006697
rdl:PCA_100006697 rdf:type owl:NamedIndividual ,
                           rdl:PCA_100001503 ;
                  rdl:PCA_100004924 "FC" ;
                  rdfs:label "human-machine interface information" .


###  http://rds.posccaesar.org/ontology/plm/rdl/PCA_100006698
rdl:PCA_100006698 rdf:type owl:NamedIndividual ,
                           rdl:PCA_100001503 ;
                  rdl:PCA_100004924 "FE" ;
                  rdfs:label "function describing information" .


###  http://rds.posccaesar.org/ontology/plm/rdl/PCA_100006699
rdl:PCA_100006699 rdf:type owl:NamedIndividual ,
                           rdl:PCA_100001503 ;
                  rdl:PCA_100004924 "FF" ;
                  rdfs:label "functional time and sequence information" .


###  http://rds.posccaesar.org/ontology/plm/rdl/PCA_100006700
rdl:PCA_100006700 rdf:type owl:NamedIndividual ,
                           rdl:PCA_100001503 ;
                  rdl:PCA_100004924 "FP" ;
                  rdfs:label "signal information" .


###  http://rds.posccaesar.org/ontology/plm/rdl/PCA_100006701
rdl:PCA_100006701 rdf:type owl:NamedIndividual ,
                           rdl:PCA_100001503 ;
                  rdl:PCA_100004924 "FQ" ;
                  rdfs:label "set value information" .


###  http://rds.posccaesar.org/ontology/plm/rdl/PCA_100006702
rdl:PCA_100006702 rdf:type owl:NamedIndividual ,
                           rdl:PCA_100001503 ;
                  rdl:PCA_100004924 "FS" ;
                  rdfs:label "circuitry information" .


###  http://rds.posccaesar.org/ontology/plm/rdl/PCA_100006703
rdl:PCA_100006703 rdf:type owl:NamedIndividual ,
                           rdl:PCA_100001503 ;
                  rdl:PCA_100004924 "FT" ;
                  rdfs:label "software information" .


###  http://rds.posccaesar.org/ontology/plm/rdl/PCA_100006704
rdl:PCA_100006704 rdf:type owl:NamedIndividual ,
                           rdl:PCA_100001503 ;
                  rdl:PCA_100004924 "L" ;
                  rdfs:label "layout" .


###  http://rds.posccaesar.org/ontology/plm/rdl/PCA_100006705
rdl:PCA_100006705 rdf:type owl:NamedIndividual ,
                           rdl:PCA_100001503 ;
                  rdl:PCA_100004924 "LA" ;
                  rdfs:label "site information" .


###  http://rds.posccaesar.org/ontology/plm/rdl/PCA_100006706
rdl:PCA_100006706 rdf:type owl:NamedIndividual ,
                           rdl:PCA_100001503 ;
                  rdl:PCA_100004924 "LB" ;
                  rdfs:label "foundation information" .


###  http://rds.posccaesar.org/ontology/plm/rdl/PCA_100006707
rdl:PCA_100006707 rdf:type owl:NamedIndividual ,
                           rdl:PCA_100001503 ;
                  rdl:PCA_100004924 "LC" ;
                  rdfs:label "construction entity information" .


###  http://rds.posccaesar.org/ontology/plm/rdl/PCA_100006708
rdl:PCA_100006708 rdf:type owl:NamedIndividual ,
                           rdl:PCA_100001503 ;
                  rdl:PCA_100004924 "LD" ;
                  rdfs:label "on-site location information" .


###  http://rds.posccaesar.org/ontology/plm/rdl/PCA_100006709
rdl:PCA_100006709 rdf:type owl:NamedIndividual ,
                           rdl:PCA_100001503 ;
                  rdl:PCA_100004924 "LH" ;
                  rdfs:label "in-construction entity location information" .


###  http://rds.posccaesar.org/ontology/plm/rdl/PCA_100006710
rdl:PCA_100006710 rdf:type owl:NamedIndividual ,
                           rdl:PCA_100001503 ;
                  rdl:PCA_100004924 "LU" ;
                  rdfs:label "in/on-equipment location information" .


###  http://rds.posccaesar.org/ontology/plm/rdl/PCA_100006711
rdl:PCA_100006711 rdf:type owl:NamedIndividual ,
                           rdl:PCA_100001503 ;
                  rdl:PCA_100004924 "M" ;
                  rdfs:label "interface" .


###  http://rds.posccaesar.org/ontology/plm/rdl/PCA_100006712
rdl:PCA_100006712 rdf:type owl:NamedIndividual ,
                           rdl:PCA_100001503 ;
                  rdl:PCA_100004924 "MA" ;
                  rdfs:label "termination information" .


###  http://rds.posccaesar.org/ontology/plm/rdl/PCA_100006713
rdl:PCA_100006713 rdf:type owl:NamedIndividual ,
                           rdl:PCA_100001503 ;
                  rdl:PCA_100004924 "MB" ;
                  rdfs:label "interaction information" .


###  http://rds.posccaesar.org/ontology/plm/rdl/PCA_100006714
rdl:PCA_100006714 rdf:type owl:NamedIndividual ,
                           rdl:PCA_100001503 ;
                  rdl:PCA_100004924 "P" ;
                  rdfs:label "enumeration" .


###  http://rds.posccaesar.org/ontology/plm/rdl/PCA_100006715
rdl:PCA_100006715 rdf:type owl:NamedIndividual ,
                           rdl:PCA_100001503 ;
                  rdl:PCA_100004924 "PA" ;
                  rdfs:label "material listing" .


###  http://rds.posccaesar.org/ontology/plm/rdl/PCA_100006716
rdl:PCA_100006716 rdf:type owl:NamedIndividual ,
                           rdl:PCA_100001503 ;
                  rdl:PCA_100004924 "PB" ;
                  rdfs:label "objects listing" .


###  http://rds.posccaesar.org/ontology/plm/rdl/PCA_100006717
rdl:PCA_100006717 rdf:type owl:NamedIndividual ,
                           rdl:PCA_100001503 ;
                  rdl:PCA_100004924 "PC" ;
                  rdfs:label "items listing" .


###  http://rds.posccaesar.org/ontology/plm/rdl/PCA_100006718
rdl:PCA_100006718 rdf:type owl:NamedIndividual ,
                           rdl:PCA_100001503 ;
                  rdl:PCA_100004924 "PD" ;
                  rdfs:label "product listing" .


###  http://rds.posccaesar.org/ontology/plm/rdl/PCA_100006719
rdl:PCA_100006719 rdf:type owl:NamedIndividual ,
                           rdl:PCA_100001503 ;
                  rdl:PCA_100004924 "PF" ;
                  rdfs:label "function listing" .


###  http://rds.posccaesar.org/ontology/plm/rdl/PCA_100006720
rdl:PCA_100006720 rdf:type owl:NamedIndividual ,
                           rdl:PCA_100001503 ;
                  rdl:PCA_100004924 "PL" ;
                  rdfs:label "location listing" .


###  http://rds.posccaesar.org/ontology/plm/rdl/PCA_100006721
rdl:PCA_100006721 rdf:type owl:NamedIndividual ,
                           rdl:PCA_100001503 ;
                  rdl:PCA_100004924 "Q" ;
                  rdfs:label "quality" .


###  http://rds.posccaesar.org/ontology/plm/rdl/PCA_100006722
rdl:PCA_100006722 rdf:type owl:NamedIndividual ,
                           rdl:PCA_100001503 ;
                  rdl:PCA_100004924 "QC" ;
                  rdfs:label "validation and verification information" .


###  http://rds.posccaesar.org/ontology/plm/rdl/PCA_100006723
rdl:PCA_100006723 rdf:type owl:NamedIndividual ,
                           rdl:PCA_100001503 ;
                  rdl:PCA_100004924 "QD" ;
                  rdfs:label "quality action information" .


###  http://rds.posccaesar.org/ontology/plm/rdl/PCA_100006724
rdl:PCA_100006724 rdf:type owl:NamedIndividual ,
                           rdl:PCA_100001503 ;
                  rdl:PCA_100004924 "QE" ;
                  rdfs:label "conformity information" .


###  http://rds.posccaesar.org/ontology/plm/rdl/PCA_100006725
rdl:PCA_100006725 rdf:type owl:NamedIndividual ,
                           rdl:PCA_100001503 ;
                  rdl:PCA_100004924 "R" ;
                  rdfs:label "safety" .


###  http://rds.posccaesar.org/ontology/plm/rdl/PCA_100006726
rdl:PCA_100006726 rdf:type owl:NamedIndividual ,
                           rdl:PCA_100001503 ;
                  rdl:PCA_100004924 "RA" ;
                  rdfs:label "health protection information" .


###  http://rds.posccaesar.org/ontology/plm/rdl/PCA_100006727
rdl:PCA_100006727 rdf:type owl:NamedIndividual ,
                           rdl:PCA_100001503 ;
                  rdl:PCA_100004924 "RB" ;
                  rdfs:label "equipment protection information" .


###  http://rds.posccaesar.org/ontology/plm/rdl/PCA_100006728
rdl:PCA_100006728 rdf:type owl:NamedIndividual ,
                           rdl:PCA_100001503 ;
                  rdl:PCA_100004924 "RC" ;
                  rdfs:label "environment protection information" .


###  http://rds.posccaesar.org/ontology/plm/rdl/PCA_100006729
rdl:PCA_100006729 rdf:type owl:NamedIndividual ,
                           rdl:PCA_100001503 ;
                  rdl:PCA_100004924 "RD" ;
                  rdfs:label "security information" .


###  http://rds.posccaesar.org/ontology/plm/rdl/PCA_100006730
rdl:PCA_100006730 rdf:type owl:NamedIndividual ,
                           rdl:PCA_100001503 ;
                  rdl:PCA_100004924 "T" ;
                  rdfs:label "geometrical form" .


###  http://rds.posccaesar.org/ontology/plm/rdl/PCA_100006731
rdl:PCA_100006731 rdf:type owl:NamedIndividual ,
                           rdl:PCA_100001503 ;
                  rdl:PCA_100004924 "TA" ;
                  rdfs:label "geometrical outline information" .


###  http://rds.posccaesar.org/ontology/plm/rdl/PCA_100006732
rdl:PCA_100006732 rdf:type owl:NamedIndividual ,
                           rdl:PCA_100001503 ;
                  rdl:PCA_100004924 "TB" ;
                  rdfs:label "geometrical detail information" .


###  http://rds.posccaesar.org/ontology/plm/rdl/PCA_100006733
rdl:PCA_100006733 rdf:type owl:NamedIndividual ,
                           rdl:PCA_100001503 ;
                  rdl:PCA_100004924 "TC" ;
                  rdfs:label "manufacturing information" .


###  http://rds.posccaesar.org/ontology/plm/rdl/PCA_100006734
rdl:PCA_100006734 rdf:type owl:NamedIndividual ,
                           rdl:PCA_100001503 ;
                  rdl:PCA_100004924 "TL" ;
                  rdfs:label "assembly information" .


###  http://rds.posccaesar.org/ontology/plm/rdl/PCA_100006735
rdl:PCA_100006735 rdf:type owl:NamedIndividual ,
                           rdl:PCA_100001503 ;
                  rdl:PCA_100004924 "W" ;
                  rdfs:label "operational" .


###  http://rds.posccaesar.org/ontology/plm/rdl/PCA_100006736
rdl:PCA_100006736 rdf:type owl:NamedIndividual ,
                           rdl:PCA_100001503 ;
                  rdl:PCA_100004924 "WA" ;
                  rdfs:label "processing information" .


###  http://rds.posccaesar.org/ontology/plm/rdl/PCA_100006737
rdl:PCA_100006737 rdf:type owl:NamedIndividual ,
                           rdl:PCA_100001503 ;
                  rdl:PCA_100004924 "WT" ;
                  rdfs:label "recording information" .


###  http://rds.posccaesar.org/ontology/plm/rdl/PCA_100006738
rdl:PCA_100006738 rdf:type owl:NamedIndividual ,
                           rdl:PCA_100001503 ;
                  rdl:PCA_100004924 "3D" ;
                  rdfs:label "3D/CAD model" .


###  http://rds.posccaesar.org/ontology/plm/rdl/PCA_100006739
rdl:PCA_100006739 rdf:type owl:NamedIndividual ,
                           rdl:PCA_100001503 ;
                  rdl:PCA_100004924 "AD" ;
                  rdfs:label "Arrangement Drawing" .


###  http://rds.posccaesar.org/ontology/plm/rdl/PCA_100006740
rdl:PCA_100006740 rdf:type owl:NamedIndividual ,
                           rdl:PCA_100001503 ;
                  rdl:PCA_100004924 "BD" ;
                  rdfs:label "Block Diagram" .


###  http://rds.posccaesar.org/ontology/plm/rdl/PCA_100006741
rdl:PCA_100006741 rdf:type owl:NamedIndividual ,
                           rdl:PCA_100001503 ;
                  rdl:PCA_100004924 "CA" ;
                  rdfs:label "Calculation" .


###  http://rds.posccaesar.org/ontology/plm/rdl/PCA_100006742
rdl:PCA_100006742 rdf:type owl:NamedIndividual ,
                           rdl:PCA_100001503 ;
                  rdl:PCA_100004924 "CE" ;
                  rdfs:label "Cause and effect" .


###  http://rds.posccaesar.org/ontology/plm/rdl/PCA_100006743
rdl:PCA_100006743 rdf:type owl:NamedIndividual ,
                           rdl:PCA_100001503 ;
                  rdl:PCA_100004924 "CF" ;
                  rdfs:label "Certificate" .


###  http://rds.posccaesar.org/ontology/plm/rdl/PCA_100006744
rdl:PCA_100006744 rdf:type owl:NamedIndividual ,
                           rdl:PCA_100001503 ;
                  rdl:PCA_100004924 "CO" ;
                  rdfs:label "Connection" .


###  http://rds.posccaesar.org/ontology/plm/rdl/PCA_100006745
rdl:PCA_100006745 rdf:type owl:NamedIndividual ,
                           rdl:PCA_100001503 ;
                  rdl:PCA_100004924 "DI" ;
                  rdfs:label "Diagram" .


###  http://rds.posccaesar.org/ontology/plm/rdl/PCA_100006746
rdl:PCA_100006746 rdf:type owl:NamedIndividual ,
                           rdl:PCA_100001503 ;
                  rdl:PCA_100004924 "DR" ;
                  rdfs:label "Drawing" .


###  http://rds.posccaesar.org/ontology/plm/rdl/PCA_100006747
rdl:PCA_100006747 rdf:type owl:NamedIndividual ,
                           rdl:PCA_100001503 ;
                  rdl:PCA_100004924 "DS" ;
                  rdfs:label "Data sheet" .


###  http://rds.posccaesar.org/ontology/plm/rdl/PCA_100006748
rdl:PCA_100006748 rdf:type owl:NamedIndividual ,
                           rdl:PCA_100001503 ;
                  rdl:PCA_100004924 "LI" ;
                  rdfs:label "List/Index" .


###  http://rds.posccaesar.org/ontology/plm/rdl/PCA_100006749
rdl:PCA_100006749 rdf:type owl:NamedIndividual ,
                           rdl:PCA_100001503 ;
                  rdl:PCA_100004924 "MA" ;
                  rdfs:label "Manuals" .


###  http://rds.posccaesar.org/ontology/plm/rdl/PCA_100006750
rdl:PCA_100006750 rdf:type owl:NamedIndividual ,
                           rdl:PCA_100001503 ;
                  rdl:PCA_100004924 "OI" ;
                  rdfs:label "Operational information" .


###  http://rds.posccaesar.org/ontology/plm/rdl/PCA_100006751
rdl:PCA_100006751 rdf:type owl:NamedIndividual ,
                           rdl:PCA_100001503 ;
                  rdl:PCA_100004924 "PD" ;
                  rdfs:label "Procedure" .


###  http://rds.posccaesar.org/ontology/plm/rdl/PCA_100006752
rdl:PCA_100006752 rdf:type owl:NamedIndividual ,
                           rdl:PCA_100001503 ;
                  rdl:PCA_100004924 "PH" ;
                  rdfs:label "Philosophy" .


###  http://rds.posccaesar.org/ontology/plm/rdl/PCA_100006753
rdl:PCA_100006753 rdf:type owl:NamedIndividual ,
                           rdl:PCA_100001503 ;
                  rdl:PCA_100004924 "PL" ;
                  rdfs:label "Plan (Drawing not project planning)" .


###  http://rds.posccaesar.org/ontology/plm/rdl/PCA_100006754
rdl:PCA_100006754 rdf:type owl:NamedIndividual ,
                           rdl:PCA_100001503 ;
                  rdl:PCA_100004924 "PS" ;
                  rdfs:label "Process" .


###  http://rds.posccaesar.org/ontology/plm/rdl/PCA_100006755
rdl:PCA_100006755 rdf:type owl:NamedIndividual ,
                           rdl:PCA_100001503 ;
                  rdl:PCA_100004924 "RG" ;
                  rdfs:label "Regulations" .


###  http://rds.posccaesar.org/ontology/plm/rdl/PCA_100006756
rdl:PCA_100006756 rdf:type owl:NamedIndividual ,
                           rdl:PCA_100001503 ;
                  rdl:PCA_100004924 "RP" ;
                  rdfs:label "Report" .


###  http://rds.posccaesar.org/ontology/plm/rdl/PCA_100006757
rdl:PCA_100006757 rdf:type owl:NamedIndividual ,
                           rdl:PCA_100001503 ;
                  rdl:PCA_100004924 "SC" ;
                  rdfs:label "Specification" .


###  http://rds.posccaesar.org/ontology/plm/rdl/PCA_100006758
rdl:PCA_100006758 rdf:type owl:NamedIndividual ,
                           rdl:PCA_100001503 ;
                  rdl:PCA_100004924 "SD" ;
                  rdfs:label "Standards" .


###  http://rds.posccaesar.org/ontology/plm/rdl/PCA_100006759
rdl:PCA_100006759 rdf:type owl:NamedIndividual ,
                           rdl:PCA_100001503 ;
                  rdl:PCA_100004924 "SG" ;
                  rdfs:label "Strategy" .


###  http://rds.posccaesar.org/ontology/plm/rdl/PCA_100006760
rdl:PCA_100006760 rdf:type owl:NamedIndividual ,
                           rdl:PCA_100001503 ;
                  rdl:PCA_100004924 "SP" ;
                  rdfs:label "Spare-/Part list" .


###  http://rds.posccaesar.org/ontology/plm/rdl/PCA_100006761
rdl:PCA_100006761 rdf:type owl:NamedIndividual ,
                           rdl:PCA_100001503 ;
                  rdl:PCA_100004924 "SW" ;
                  rdfs:label "Software" .


###  http://rds.posccaesar.org/ontology/plm/rdl/PCA_100006762
rdl:PCA_100006762 rdf:type owl:NamedIndividual ,
                           rdl:PCA_100001503 ;
                  rdl:PCA_100004924 "TD" ;
                  rdfs:label "Technical data" .


###  http://w3id.org/readi/rdl/CFIHOS-20000001
rrdl:CFIHOS-20000001 rdf:type owl:NamedIndividual ,
                              rdl:PCA_100001503 ;
                     rdl:PCA_100004924 "AA" ;
                     rdfs:label "project management and engineering" .


###  http://w3id.org/readi/rdl/CFIHOS-20000002
rrdl:CFIHOS-20000002 rdf:type owl:NamedIndividual ,
                              rdl:PCA_100001503 ;
                     rdl:PCA_100004924 "BA" ;
                     rdfs:label "construction" .


###  http://w3id.org/readi/rdl/CFIHOS-20000003
rrdl:CFIHOS-20000003 rdf:type owl:NamedIndividual ,
                              rdl:PCA_100001503 ;
                     rdl:PCA_100004924 "CB" ;
                     rdfs:label "architectural engineering" .


###  http://w3id.org/readi/rdl/CFIHOS-20000004
rrdl:CFIHOS-20000004 rdf:type owl:NamedIndividual ,
                              rdl:PCA_100001503 ;
                     rdl:PCA_100004924 "CG" ;
                     rdfs:label "geotechnical engineering" .


###  http://w3id.org/readi/rdl/CFIHOS-20000005
rrdl:CFIHOS-20000005 rdf:type owl:NamedIndividual ,
                              rdl:PCA_100001503 ;
                     rdl:PCA_100004924 "CI" ;
                     rdfs:label "infrastructure engineering" .


###  http://w3id.org/readi/rdl/CFIHOS-20000006
rrdl:CFIHOS-20000006 rdf:type owl:NamedIndividual ,
                              rdl:PCA_100001503 ;
                     rdl:PCA_100004924 "CS" ;
                     rdfs:label "structural engineering" .


###  http://w3id.org/readi/rdl/CFIHOS-20000007
rrdl:CFIHOS-20000007 rdf:type owl:NamedIndividual ,
                              rdl:PCA_100001503 ;
                     rdl:PCA_100004924 "CX" ;
                     rdfs:label "civil engineering" .


###  http://w3id.org/readi/rdl/CFIHOS-20000008
rrdl:CFIHOS-20000008 rdf:type owl:NamedIndividual ,
                              rdl:PCA_100001503 ;
                     rdl:PCA_100004924 "EA" ;
                     rdfs:label "electrical engineering" .


###  http://w3id.org/readi/rdl/CFIHOS-20000009
rrdl:CFIHOS-20000009 rdf:type owl:NamedIndividual ,
                              rdl:PCA_100001503 ;
                     rdl:PCA_100004924 "FA" ;
                     rdfs:label "cost and planning management" .


###  http://w3id.org/readi/rdl/CFIHOS-20000010
rrdl:CFIHOS-20000010 rdf:type owl:NamedIndividual ,
                              rdl:PCA_100001503 ;
                     rdl:PCA_100004924 "HE" ;
                     rdfs:label "environmental" .


###  http://w3id.org/readi/rdl/CFIHOS-20000011
rrdl:CFIHOS-20000011 rdf:type owl:NamedIndividual ,
                              rdl:PCA_100001503 ;
                     rdl:PCA_100004924 "HH" ;
                     rdfs:label "health" .


###  http://w3id.org/readi/rdl/CFIHOS-20000012
rrdl:CFIHOS-20000012 rdf:type owl:NamedIndividual ,
                              rdl:PCA_100001503 ;
                     rdl:PCA_100004924 "HP" ;
                     rdfs:label "security" .


###  http://w3id.org/readi/rdl/CFIHOS-20000013
rrdl:CFIHOS-20000013 rdf:type owl:NamedIndividual ,
                              rdl:PCA_100001503 ;
                     rdl:PCA_100004924 "HS" ;
                     rdfs:label "safety" .


###  http://w3id.org/readi/rdl/CFIHOS-20000014
rrdl:CFIHOS-20000014 rdf:type owl:NamedIndividual ,
                              rdl:PCA_100001503 ;
                     rdl:PCA_100004924 "HX" ;
                     rdfs:label "health, safety, environmental and security" .


###  http://w3id.org/readi/rdl/CFIHOS-20000015
rrdl:CFIHOS-20000015 rdf:type owl:NamedIndividual ,
                              rdl:PCA_100001503 ;
                     rdl:PCA_100004924 "IN" ;
                     rdfs:label "instrumentation engineering" .


###  http://w3id.org/readi/rdl/CFIHOS-20000016
rrdl:CFIHOS-20000016 rdf:type owl:NamedIndividual ,
                              rdl:PCA_100001503 ;
                     rdl:PCA_100004924 "JA" ;
                     rdfs:label "information management" .


###  http://w3id.org/readi/rdl/CFIHOS-20000017
rrdl:CFIHOS-20000017 rdf:type owl:NamedIndividual ,
                              rdl:PCA_100001503 ;
                     rdl:PCA_100004924 "KA" ;
                     rdfs:label "information technology" .


###  http://w3id.org/readi/rdl/CFIHOS-20000018
rrdl:CFIHOS-20000018 rdf:type owl:NamedIndividual ,
                              rdl:PCA_100001503 ;
                     rdl:PCA_100004924 "LA" ;
                     rdfs:label "pipeline engineering" .


###  http://w3id.org/readi/rdl/CFIHOS-20000019
rrdl:CFIHOS-20000019 rdf:type owl:NamedIndividual ,
                              rdl:PCA_100001503 ;
                     rdl:PCA_100004924 "MH" ;
                     rdfs:label "heating, ventilating, and air conditioning" .


###  http://w3id.org/readi/rdl/CFIHOS-20000020
rrdl:CFIHOS-20000020 rdf:type owl:NamedIndividual ,
                              rdl:PCA_100001503 ;
                     rdl:PCA_100004924 "MP" ;
                     rdfs:label "piping engineering" .


###  http://w3id.org/readi/rdl/CFIHOS-20000021
rrdl:CFIHOS-20000021 rdf:type owl:NamedIndividual ,
                              rdl:PCA_100001503 ;
                     rdl:PCA_100004924 "MR" ;
                     rdfs:label "mechanical rotating engineering" .


###  http://w3id.org/readi/rdl/CFIHOS-20000022
rrdl:CFIHOS-20000022 rdf:type owl:NamedIndividual ,
                              rdl:PCA_100001503 ;
                     rdl:PCA_100004924 "MS" ;
                     rdfs:label "mechanical static engineering" .


###  http://w3id.org/readi/rdl/CFIHOS-20000023
rrdl:CFIHOS-20000023 rdf:type owl:NamedIndividual ,
                              rdl:PCA_100001503 ;
                     rdl:PCA_100004924 "MX" ;
                     rdfs:label "mechanical engineering" .


###  http://w3id.org/readi/rdl/CFIHOS-20000024
rrdl:CFIHOS-20000024 rdf:type owl:NamedIndividual ,
                              rdl:PCA_100001503 ;
                     rdl:PCA_100004924 "NA" ;
                     rdfs:label "maintenance management" .


###  http://w3id.org/readi/rdl/CFIHOS-20000025
rrdl:CFIHOS-20000025 rdf:type owl:NamedIndividual ,
                              rdl:PCA_100001503 ;
                     rdl:PCA_100004924 "OA" ;
                     rdfs:label "operations management" .


###  http://w3id.org/readi/rdl/CFIHOS-20000026
rrdl:CFIHOS-20000026 rdf:type owl:NamedIndividual ,
                              rdl:PCA_100001503 ;
                     rdl:PCA_100004924 "PX" ;
                     rdfs:label "process engineering" .


###  http://w3id.org/readi/rdl/CFIHOS-20000027
rrdl:CFIHOS-20000027 rdf:type owl:NamedIndividual ,
                              rdl:PCA_100001503 ;
                     rdl:PCA_100004924 "QA" ;
                     rdfs:label "quality management" .


###  http://w3id.org/readi/rdl/CFIHOS-20000028
rrdl:CFIHOS-20000028 rdf:type owl:NamedIndividual ,
                              rdl:PCA_100001503 ;
                     rdl:PCA_100004924 "RA" ;
                     rdfs:label "materials engineering" .


###  http://w3id.org/readi/rdl/CFIHOS-20000029
rrdl:CFIHOS-20000029 rdf:type owl:NamedIndividual ,
                              rdl:PCA_100001503 ;
                     rdl:PCA_100004924 "SA" ;
                     rdfs:label "logistics management" .


###  http://w3id.org/readi/rdl/CFIHOS-20000030
rrdl:CFIHOS-20000030 rdf:type owl:NamedIndividual ,
                              rdl:PCA_100001503 ;
                     rdl:PCA_100004924 "TA" ;
                     rdfs:label "telecommunications" .


###  http://w3id.org/readi/rdl/CFIHOS-20000031
rrdl:CFIHOS-20000031 rdf:type owl:NamedIndividual ,
                              rdl:PCA_100001503 ;
                     rdl:PCA_100004924 "UA" ;
                     rdfs:label "subsea engineering" .


###  http://w3id.org/readi/rdl/CFIHOS-20000032
rrdl:CFIHOS-20000032 rdf:type owl:NamedIndividual ,
                              rdl:PCA_100001503 ;
                     rdl:PCA_100004924 "VA" ;
                     rdfs:label "contracting and procurement management" .


###  http://w3id.org/readi/rdl/CFIHOS-20000033
rrdl:CFIHOS-20000033 rdf:type owl:NamedIndividual ,
                              rdl:PCA_100001503 ;
                     rdl:PCA_100004924 "WA" ;
                     rdfs:label "ocean engineering" .


###  http://w3id.org/readi/rdl/CFIHOS-20000034
rrdl:CFIHOS-20000034 rdf:type owl:NamedIndividual ,
                              rdl:PCA_100001503 ;
                     rdl:PCA_100004924 "ZE" ;
                     rdfs:label "geology" .


###  http://w3id.org/readi/rdl/CFIHOS-20000035
rrdl:CFIHOS-20000035 rdf:type owl:NamedIndividual ,
                              rdl:PCA_100001503 ;
                     rdl:PCA_100004924 "ZF" ;
                     rdfs:label "finance" .


###  http://w3id.org/readi/rdl/CFIHOS-20000036
rrdl:CFIHOS-20000036 rdf:type owl:NamedIndividual ,
                              rdl:PCA_100001503 ;
                     rdl:PCA_100004924 "ZG" ;
                     rdfs:label "geomatics" .


###  http://w3id.org/readi/rdl/CFIHOS-20000037
rrdl:CFIHOS-20000037 rdf:type owl:NamedIndividual ,
                              rdl:PCA_100001503 ;
                     rdl:PCA_100004924 "ZH" ;
                     rdfs:label "human resources" .


###  http://w3id.org/readi/rdl/CFIHOS-20000038
rrdl:CFIHOS-20000038 rdf:type owl:NamedIndividual ,
                              rdl:PCA_100001503 ;
                     rdl:PCA_100004924 "ZP" ;
                     rdfs:label "petrophysics" .


###  http://w3id.org/readi/rdl/CFIHOS-20000039
rrdl:CFIHOS-20000039 rdf:type owl:NamedIndividual ,
                              rdl:PCA_100001503 ;
                     rdl:PCA_100004924 "ZR" ;
                     rdfs:label "reservoir engineering" .


###  http://w3id.org/readi/rdl/CFIHOS-20000040
rrdl:CFIHOS-20000040 rdf:type owl:NamedIndividual ,
                              rdl:PCA_100001503 ;
                     rdl:PCA_100004924 "ZS" ;
                     rdfs:label "geophysics" .


###  http://w3id.org/readi/rdl/CFIHOS-20000041
rrdl:CFIHOS-20000041 rdf:type owl:NamedIndividual ,
                              rdl:PCA_100001503 ;
                     rdl:PCA_100004924 "ZT" ;
                     rdfs:label "production technology" .


###  http://w3id.org/readi/rdl/CFIHOS-20000042
rrdl:CFIHOS-20000042 rdf:type owl:NamedIndividual ,
                              rdl:PCA_100001503 ;
                     rdl:PCA_100004924 "ZW" ;
                     rdfs:label "well engineering" .


###  http://w3id.org/readi/rdl/CFIHOS-20000043
rrdl:CFIHOS-20000043 rdf:type owl:NamedIndividual ,
                              rdl:PCA_100001503 ;
                     rdl:PCA_100004924 "BC" ;
                     rdfs:label "commissioning" .


#################################################################
#    Annotations
#################################################################

rdl:PCA_100006769 skos:member rdl:PCA_100006578 ,
                              rdl:PCA_100006579 ,
                              rdl:PCA_100006580 ,
                              rdl:PCA_100006581 ,
                              rdl:PCA_100006582 ,
                              rdl:PCA_100006583 ,
                              rdl:PCA_100006584 ,
                              rdl:PCA_100006585 ,
                              rdl:PCA_100006586 ,
                              rdl:PCA_100006587 ,
                              rdl:PCA_100006588 ,
                              rdl:PCA_100006589 ,
                              rdl:PCA_100006590 ,
                              rdl:PCA_100006591 ,
                              rdl:PCA_100006592 ,
                              rdl:PCA_100006593 ,
                              rdl:PCA_100006594 ,
                              rdl:PCA_100006595 ,
                              rdl:PCA_100006596 ,
                              rdl:PCA_100006597 ,
                              rdl:PCA_100006598 ,
                              rdl:PCA_100006599 ,
                              rdl:PCA_100006600 ,
                              rdl:PCA_100006601 ,
                              rdl:PCA_100006602 ,
                              rdl:PCA_100006603 ,
                              rdl:PCA_100006604 ,
                              rdl:PCA_100006605 ,
                              rdl:PCA_100006606 ,
                              rdl:PCA_100006607 ,
                              rdl:PCA_100006608 ,
                              rdl:PCA_100006609 ,
                              rdl:PCA_100006610 ,
                              rdl:PCA_100006611 ,
                              rdl:PCA_100006612 ,
                              rdl:PCA_100006613 ,
                              rdl:PCA_100006614 ,
                              rdl:PCA_100006615 ,
                              rdl:PCA_100006616 ,
                              rdl:PCA_100006617 ,
                              rdl:PCA_100006618 ,
                              rdl:PCA_100006619 ,
                              rdl:PCA_100006620 ,
                              rdl:PCA_100006621 ,
                              rdl:PCA_100006622 ,
                              rdl:PCA_100006623 ,
                              rdl:PCA_100006624 ,
                              rdl:PCA_100006625 ,
                              rdl:PCA_100006626 ,
                              rdl:PCA_100006627 ,
                              rdl:PCA_100006628 ,
                              rdl:PCA_100006629 ,
                              rdl:PCA_100006630 ,
                              rdl:PCA_100006631 ,
                              rdl:PCA_100006632 ,
                              rdl:PCA_100006633 ,
                              rdl:PCA_100006634 ,
                              rdl:PCA_100006635 ,
                              rdl:PCA_100006636 ,
                              rdl:PCA_100006637 ,
                              rdl:PCA_100006638 ,
                              rdl:PCA_100006639 ,
                              rdl:PCA_100006640 ,
                              rdl:PCA_100006641 ,
                              rdl:PCA_100006642 ,
                              rdl:PCA_100006643 ,
                              rdl:PCA_100006644 ,
                              rdl:PCA_100006645 ,
                              rdl:PCA_100006646 ,
                              rdl:PCA_100006647 ,
                              rdl:PCA_100006648 ,
                              rdl:PCA_100006649 ,
                              rdl:PCA_100006650 ,
                              rdl:PCA_100006651 ,
                              rdl:PCA_100006652 ,
                              rdl:PCA_100006653 ,
                              rdl:PCA_100006654 ,
                              rdl:PCA_100006655 ,
                              rdl:PCA_100006656 ,
                              rdl:PCA_100006657 .


rdl:PCA_100006770 skos:member rdl:PCA_100006658 ,
                              rdl:PCA_100006659 ,
                              rdl:PCA_100006660 ,
                              rdl:PCA_100006661 ,
                              rdl:PCA_100006662 ,
                              rdl:PCA_100006663 ,
                              rdl:PCA_100006664 ,
                              rdl:PCA_100006665 ,
                              rdl:PCA_100006666 ,
                              rdl:PCA_100006667 ,
                              rdl:PCA_100006668 ,
                              rdl:PCA_100006669 ,
                              rdl:PCA_100006670 ,
                              rdl:PCA_100006671 ,
                              rdl:PCA_100006672 ,
                              rdl:PCA_100006673 ,
                              rdl:PCA_100006674 ,
                              rdl:PCA_100006675 ,
                              rdl:PCA_100006676 ,
                              rdl:PCA_100006677 ,
                              rdl:PCA_100006678 ,
                              rdl:PCA_100006679 ,
                              rdl:PCA_100006680 ,
                              rdl:PCA_100006681 ,
                              rdl:PCA_100006682 ,
                              rdl:PCA_100006683 ,
                              rdl:PCA_100006684 ,
                              rdl:PCA_100006685 ,
                              rdl:PCA_100006686 ,
                              rdl:PCA_100006687 ,
                              rdl:PCA_100006688 ,
                              rdl:PCA_100006689 ,
                              rdl:PCA_100006690 ,
                              rdl:PCA_100006691 ,
                              rdl:PCA_100006692 ,
                              rdl:PCA_100006693 ,
                              rdl:PCA_100006694 ,
                              rdl:PCA_100006695 ,
                              rdl:PCA_100006696 ,
                              rdl:PCA_100006697 ,
                              rdl:PCA_100006698 ,
                              rdl:PCA_100006699 ,
                              rdl:PCA_100006700 ,
                              rdl:PCA_100006701 ,
                              rdl:PCA_100006702 ,
                              rdl:PCA_100006703 ,
                              rdl:PCA_100006704 ,
                              rdl:PCA_100006705 ,
                              rdl:PCA_100006706 ,
                              rdl:PCA_100006707 ,
                              rdl:PCA_100006708 ,
                              rdl:PCA_100006709 ,
                              rdl:PCA_100006710 ,
                              rdl:PCA_100006711 ,
                              rdl:PCA_100006712 ,
                              rdl:PCA_100006713 ,
                              rdl:PCA_100006714 ,
                              rdl:PCA_100006715 ,
                              rdl:PCA_100006716 ,
                              rdl:PCA_100006717 ,
                              rdl:PCA_100006718 ,
                              rdl:PCA_100006719 ,
                              rdl:PCA_100006720 ,
                              rdl:PCA_100006721 ,
                              rdl:PCA_100006722 ,
                              rdl:PCA_100006723 ,
                              rdl:PCA_100006724 ,
                              rdl:PCA_100006725 ,
                              rdl:PCA_100006726 ,
                              rdl:PCA_100006727 ,
                              rdl:PCA_100006728 ,
                              rdl:PCA_100006729 ,
                              rdl:PCA_100006730 ,
                              rdl:PCA_100006731 ,
                              rdl:PCA_100006732 ,
                              rdl:PCA_100006733 ,
                              rdl:PCA_100006734 ,
                              rdl:PCA_100006735 ,
                              rdl:PCA_100006736 ,
                              rdl:PCA_100006737 .


rdl:PCA_100006771 skos:member rdl:PCA_100006738 ,
                              rdl:PCA_100006739 ,
                              rdl:PCA_100006740 ,
                              rdl:PCA_100006741 ,
                              rdl:PCA_100006742 ,
                              rdl:PCA_100006743 ,
                              rdl:PCA_100006744 ,
                              rdl:PCA_100006745 ,
                              rdl:PCA_100006746 ,
                              rdl:PCA_100006747 ,
                              rdl:PCA_100006748 ,
                              rdl:PCA_100006749 ,
                              rdl:PCA_100006750 ,
                              rdl:PCA_100006751 ,
                              rdl:PCA_100006752 ,
                              rdl:PCA_100006753 ,
                              rdl:PCA_100006754 ,
                              rdl:PCA_100006755 ,
                              rdl:PCA_100006756 ,
                              rdl:PCA_100006757 ,
                              rdl:PCA_100006758 ,
                              rdl:PCA_100006759 ,
                              rdl:PCA_100006760 ,
                              rdl:PCA_100006761 ,
                              rdl:PCA_100006762 .


rdl:PCA_100006772 skos:member rrdl:CFIHOS-20000001 ,
                              rrdl:CFIHOS-20000002 ,
                              rrdl:CFIHOS-20000003 ,
                              rrdl:CFIHOS-20000004 ,
                              rrdl:CFIHOS-20000005 ,
                              rrdl:CFIHOS-20000006 ,
                              rrdl:CFIHOS-20000007 ,
                              rrdl:CFIHOS-20000008 ,
                              rrdl:CFIHOS-20000009 ,
                              rrdl:CFIHOS-20000010 ,
                              rrdl:CFIHOS-20000011 ,
                              rrdl:CFIHOS-20000012 ,
                              rrdl:CFIHOS-20000013 ,
                              rrdl:CFIHOS-20000014 ,
                              rrdl:CFIHOS-20000015 ,
                              rrdl:CFIHOS-20000016 ,
                              rrdl:CFIHOS-20000017 ,
                              rrdl:CFIHOS-20000018 ,
                              rrdl:CFIHOS-20000019 ,
                              rrdl:CFIHOS-20000020 ,
                              rrdl:CFIHOS-20000021 ,
                              rrdl:CFIHOS-20000022 ,
                              rrdl:CFIHOS-20000023 ,
                              rrdl:CFIHOS-20000024 ,
                              rrdl:CFIHOS-20000025 ,
                              rrdl:CFIHOS-20000026 ,
                              rrdl:CFIHOS-20000027 ,
                              rrdl:CFIHOS-20000028 ,
                              rrdl:CFIHOS-20000029 ,
                              rrdl:CFIHOS-20000030 ,
                              rrdl:CFIHOS-20000031 ,
                              rrdl:CFIHOS-20000032 ,
                              rrdl:CFIHOS-20000033 ,
                              rrdl:CFIHOS-20000034 ,
                              rrdl:CFIHOS-20000035 ,
                              rrdl:CFIHOS-20000036 ,
                              rrdl:CFIHOS-20000037 ,
                              rrdl:CFIHOS-20000038 ,
                              rrdl:CFIHOS-20000039 ,
                              rrdl:CFIHOS-20000040 ,
                              rrdl:CFIHOS-20000041 ,
                              rrdl:CFIHOS-20000042 ,
                              rrdl:CFIHOS-20000043 .


rdl:PCA_100006773 skos:member rdl:PCA_100006078 ,
                              rdl:PCA_100006079 ,
                              rdl:PCA_100006080 ,
                              rdl:PCA_100006081 ,
                              rdl:PCA_100006082 ,
                              rdl:PCA_100006083 ,
                              rdl:PCA_100006084 ,
                              rdl:PCA_100006085 ,
                              rdl:PCA_100006086 ,
                              rdl:PCA_100006087 ,
                              rdl:PCA_100006088 ,
                              rdl:PCA_100006089 ,
                              rdl:PCA_100006090 ,
                              rdl:PCA_100006091 ,
                              rdl:PCA_100006092 ,
                              rdl:PCA_100006093 ,
                              rdl:PCA_100006094 ,
                              rdl:PCA_100006095 ,
                              rdl:PCA_100006096 ,
                              rdl:PCA_100006097 ,
                              rdl:PCA_100006098 ,
                              rdl:PCA_100006099 ,
                              rdl:PCA_100006100 ,
                              rdl:PCA_100006101 ,
                              rdl:PCA_100006102 ,
                              rdl:PCA_100006103 ,
                              rdl:PCA_100006104 ,
                              rdl:PCA_100006105 ,
                              rdl:PCA_100006106 ,
                              rdl:PCA_100006107 ,
                              rdl:PCA_100006108 ,
                              rdl:PCA_100006109 ,
                              rdl:PCA_100006110 ,
                              rdl:PCA_100006111 ,
                              rdl:PCA_100006112 ,
                              rdl:PCA_100006113 ,
                              rdl:PCA_100006114 ,
                              rdl:PCA_100006115 ,
                              rdl:PCA_100006116 ,
                              rdl:PCA_100006117 ,
                              rdl:PCA_100006118 ,
                              rdl:PCA_100006119 ,
                              rdl:PCA_100006120 ,
                              rdl:PCA_100006121 ,
                              rdl:PCA_100006122 ,
                              rdl:PCA_100006123 ,
                              rdl:PCA_100006124 ,
                              rdl:PCA_100006125 ,
                              rdl:PCA_100006126 ,
                              rdl:PCA_100006127 ,
                              rdl:PCA_100006128 ,
                              rdl:PCA_100006129 ,
                              rdl:PCA_100006130 ,
                              rdl:PCA_100006131 ,
                              rdl:PCA_100006132 ,
                              rdl:PCA_100006133 ,
                              rdl:PCA_100006134 ,
                              rdl:PCA_100006135 ,
                              rdl:PCA_100006136 ,
                              rdl:PCA_100006137 ,
                              rdl:PCA_100006138 ,
                              rdl:PCA_100006139 ,
                              rdl:PCA_100006140 ,
                              rdl:PCA_100006141 ,
                              rdl:PCA_100006142 ,
                              rdl:PCA_100006143 ,
                              rdl:PCA_100006144 ,
                              rdl:PCA_100006145 ,
                              rdl:PCA_100006146 ,
                              rdl:PCA_100006147 ,
                              rdl:PCA_100006148 ,
                              rdl:PCA_100006149 ,
                              rdl:PCA_100006150 ,
                              rdl:PCA_100006151 ,
                              rdl:PCA_100006152 ,
                              rdl:PCA_100006153 ,
                              rdl:PCA_100006154 ,
                              rdl:PCA_100006155 ,
                              rdl:PCA_100006156 ,
                              rdl:PCA_100006157 ,
                              rdl:PCA_100006158 ,
                              rdl:PCA_100006159 ,
                              rdl:PCA_100006160 ,
                              rdl:PCA_100006161 ,
                              rdl:PCA_100006162 ,
                              rdl:PCA_100006163 ,
                              rdl:PCA_100006164 ,
                              rdl:PCA_100006165 ,
                              rdl:PCA_100006166 ,
                              rdl:PCA_100006167 ,
                              rdl:PCA_100006168 ,
                              rdl:PCA_100006169 ,
                              rdl:PCA_100006170 ,
                              rdl:PCA_100006171 ,
                              rdl:PCA_100006172 ,
                              rdl:PCA_100006173 ,
                              rdl:PCA_100006174 ,
                              rdl:PCA_100006175 ,
                              rdl:PCA_100006176 ,
                              rdl:PCA_100006177 ,
                              rdl:PCA_100006178 ,
                              rdl:PCA_100006179 ,
                              rdl:PCA_100006180 ,
                              rdl:PCA_100006181 ,
                              rdl:PCA_100006182 ,
                              rdl:PCA_100006183 ,
                              rdl:PCA_100006184 ,
                              rdl:PCA_100006185 ,
                              rdl:PCA_100006186 ,
                              rdl:PCA_100006187 ,
                              rdl:PCA_100006188 ,
                              rdl:PCA_100006189 ,
                              rdl:PCA_100006190 ,
                              rdl:PCA_100006191 ,
                              rdl:PCA_100006192 ,
                              rdl:PCA_100006193 ,
                              rdl:PCA_100006194 ,
                              rdl:PCA_100006195 ,
                              rdl:PCA_100006196 ,
                              rdl:PCA_100006197 ,
                              rdl:PCA_100006198 ,
                              rdl:PCA_100006199 ,
                              rdl:PCA_100006200 ,
                              rdl:PCA_100006201 ,
                              rdl:PCA_100006202 ,
                              rdl:PCA_100006203 ,
                              rdl:PCA_100006204 ,
                              rdl:PCA_100006205 ,
                              rdl:PCA_100006206 ,
                              rdl:PCA_100006207 ,
                              rdl:PCA_100006208 ,
                              rdl:PCA_100006209 ,
                              rdl:PCA_100006210 ,
                              rdl:PCA_100006211 ,
                              rdl:PCA_100006212 ,
                              rdl:PCA_100006213 ,
                              rdl:PCA_100006214 ,
                              rdl:PCA_100006215 ,
                              rdl:PCA_100006216 ,
                              rdl:PCA_100006217 ,
                              rdl:PCA_100006218 ,
                              rdl:PCA_100006219 ,
                              rdl:PCA_100006220 ,
                              rdl:PCA_100006221 ,
                              rdl:PCA_100006222 ,
                              rdl:PCA_100006223 ,
                              rdl:PCA_100006224 ,
                              rdl:PCA_100006225 ,
                              rdl:PCA_100006226 ,
                              rdl:PCA_100006227 ,
                              rdl:PCA_100006228 ,
                              rdl:PCA_100006229 ,
                              rdl:PCA_100006230 ,
                              rdl:PCA_100006231 ,
                              rdl:PCA_100006232 ,
                              rdl:PCA_100006233 ,
                              rdl:PCA_100006234 ,
                              rdl:PCA_100006235 ,
                              rdl:PCA_100006236 ,
                              rdl:PCA_100006237 ,
                              rdl:PCA_100006238 ,
                              rdl:PCA_100006239 ,
                              rdl:PCA_100006240 ,
                              rdl:PCA_100006241 ,
                              rdl:PCA_100006242 ,
                              rdl:PCA_100006243 ,
                              rdl:PCA_100006244 ,
                              rdl:PCA_100006245 ,
                              rdl:PCA_100006246 ,
                              rdl:PCA_100006247 ,
                              rdl:PCA_100006248 ,
                              rdl:PCA_100006249 ,
                              rdl:PCA_100006250 ,
                              rdl:PCA_100006251 ,
                              rdl:PCA_100006252 ,
                              rdl:PCA_100006253 ,
                              rdl:PCA_100006254 ,
                              rdl:PCA_100006255 ,
                              rdl:PCA_100006256 ,
                              rdl:PCA_100006257 ,
                              rdl:PCA_100006258 ,
                              rdl:PCA_100006259 ,
                              rdl:PCA_100006260 ,
                              rdl:PCA_100006261 ,
                              rdl:PCA_100006262 ,
                              rdl:PCA_100006263 ,
                              rdl:PCA_100006264 ,
                              rdl:PCA_100006265 ,
                              rdl:PCA_100006266 ,
                              rdl:PCA_100006267 ,
                              rdl:PCA_100006268 ,
                              rdl:PCA_100006269 ,
                              rdl:PCA_100006270 ,
                              rdl:PCA_100006271 ,
                              rdl:PCA_100006272 ,
                              rdl:PCA_100006273 ,
                              rdl:PCA_100006274 ,
                              rdl:PCA_100006275 ,
                              rdl:PCA_100006276 ,
                              rdl:PCA_100006277 ,
                              rdl:PCA_100006278 ,
                              rdl:PCA_100006279 ,
                              rdl:PCA_100006280 ,
                              rdl:PCA_100006281 ,
                              rdl:PCA_100006282 ,
                              rdl:PCA_100006283 ,
                              rdl:PCA_100006284 ,
                              rdl:PCA_100006285 ,
                              rdl:PCA_100006286 ,
                              rdl:PCA_100006287 ,
                              rdl:PCA_100006288 ,
                              rdl:PCA_100006289 ,
                              rdl:PCA_100006290 ,
                              rdl:PCA_100006291 ,
                              rdl:PCA_100006292 ,
                              rdl:PCA_100006293 ,
                              rdl:PCA_100006294 ,
                              rdl:PCA_100006295 ,
                              rdl:PCA_100006296 ,
                              rdl:PCA_100006297 ,
                              rdl:PCA_100006298 ,
                              rdl:PCA_100006299 ,
                              rdl:PCA_100006300 ,
                              rdl:PCA_100006301 ,
                              rdl:PCA_100006302 ,
                              rdl:PCA_100006303 ,
                              rdl:PCA_100006304 ,
                              rdl:PCA_100006305 ,
                              rdl:PCA_100006306 ,
                              rdl:PCA_100006307 ,
                              rdl:PCA_100006308 ,
                              rdl:PCA_100006309 ,
                              rdl:PCA_100006310 ,
                              rdl:PCA_100006311 ,
                              rdl:PCA_100006312 ,
                              rdl:PCA_100006313 ,
                              rdl:PCA_100006314 ,
                              rdl:PCA_100006315 ,
                              rdl:PCA_100006316 ,
                              rdl:PCA_100006317 ,
                              rdl:PCA_100006318 ,
                              rdl:PCA_100006319 ,
                              rdl:PCA_100006320 ,
                              rdl:PCA_100006321 ,
                              rdl:PCA_100006322 ,
                              rdl:PCA_100006323 ,
                              rdl:PCA_100006324 ,
                              rdl:PCA_100006325 ,
                              rdl:PCA_100006326 ,
                              rdl:PCA_100006327 ,
                              rdl:PCA_100006328 ,
                              rdl:PCA_100006329 ,
                              rdl:PCA_100006330 ,
                              rdl:PCA_100006331 ,
                              rdl:PCA_100006332 ,
                              rdl:PCA_100006333 ,
                              rdl:PCA_100006334 ,
                              rdl:PCA_100006335 ,
                              rdl:PCA_100006336 ,
                              rdl:PCA_100006337 ,
                              rdl:PCA_100006338 ,
                              rdl:PCA_100006339 ,
                              rdl:PCA_100006340 ,
                              rdl:PCA_100006341 ,
                              rdl:PCA_100006342 ,
                              rdl:PCA_100006343 ,
                              rdl:PCA_100006344 ,
                              rdl:PCA_100006345 ,
                              rdl:PCA_100006346 ,
                              rdl:PCA_100006347 ,
                              rdl:PCA_100006348 ,
                              rdl:PCA_100006349 ,
                              rdl:PCA_100006350 ,
                              rdl:PCA_100006351 ,
                              rdl:PCA_100006352 ,
                              rdl:PCA_100006353 ,
                              rdl:PCA_100006354 ,
                              rdl:PCA_100006355 ,
                              rdl:PCA_100006356 ,
                              rdl:PCA_100006357 ,
                              rdl:PCA_100006358 ,
                              rdl:PCA_100006359 ,
                              rdl:PCA_100006360 ,
                              rdl:PCA_100006361 ,
                              rdl:PCA_100006362 ,
                              rdl:PCA_100006363 ,
                              rdl:PCA_100006364 ,
                              rdl:PCA_100006365 ,
                              rdl:PCA_100006366 ,
                              rdl:PCA_100006367 ,
                              rdl:PCA_100006368 ,
                              rdl:PCA_100006369 ,
                              rdl:PCA_100006370 ,
                              rdl:PCA_100006371 ,
                              rdl:PCA_100006372 ,
                              rdl:PCA_100006373 ,
                              rdl:PCA_100006374 ,
                              rdl:PCA_100006375 ,
                              rdl:PCA_100006376 ,
                              rdl:PCA_100006377 ,
                              rdl:PCA_100006378 ,
                              rdl:PCA_100006379 ,
                              rdl:PCA_100006380 ,
                              rdl:PCA_100006381 ,
                              rdl:PCA_100006382 ,
                              rdl:PCA_100006383 ,
                              rdl:PCA_100006384 ,
                              rdl:PCA_100006385 ,
                              rdl:PCA_100006386 ,
                              rdl:PCA_100006387 ,
                              rdl:PCA_100006388 ,
                              rdl:PCA_100006389 ,
                              rdl:PCA_100006390 ,
                              rdl:PCA_100006391 ,
                              rdl:PCA_100006392 ,
                              rdl:PCA_100006393 ,
                              rdl:PCA_100006394 ,
                              rdl:PCA_100006395 ,
                              rdl:PCA_100006396 ,
                              rdl:PCA_100006397 ,
                              rdl:PCA_100006398 ,
                              rdl:PCA_100006399 ,
                              rdl:PCA_100006400 ,
                              rdl:PCA_100006401 ,
                              rdl:PCA_100006402 ,
                              rdl:PCA_100006403 ,
                              rdl:PCA_100006404 ,
                              rdl:PCA_100006405 ,
                              rdl:PCA_100006406 ,
                              rdl:PCA_100006407 ,
                              rdl:PCA_100006408 ,
                              rdl:PCA_100006409 ,
                              rdl:PCA_100006410 ,
                              rdl:PCA_100006411 ,
                              rdl:PCA_100006412 ,
                              rdl:PCA_100006413 ,
                              rdl:PCA_100006414 ,
                              rdl:PCA_100006415 ,
                              rdl:PCA_100006416 ,
                              rdl:PCA_100006417 ,
                              rdl:PCA_100006418 ,
                              rdl:PCA_100006419 ,
                              rdl:PCA_100006420 ,
                              rdl:PCA_100006421 ,
                              rdl:PCA_100006422 ,
                              rdl:PCA_100006423 ,
                              rdl:PCA_100006424 ,
                              rdl:PCA_100006425 ,
                              rdl:PCA_100006426 ,
                              rdl:PCA_100006427 ,
                              rdl:PCA_100006428 ,
                              rdl:PCA_100006429 ,
                              rdl:PCA_100006430 ,
                              rdl:PCA_100006431 ,
                              rdl:PCA_100006432 ,
                              rdl:PCA_100006433 ,
                              rdl:PCA_100006434 ,
                              rdl:PCA_100006435 ,
                              rdl:PCA_100006436 ,
                              rdl:PCA_100006437 ,
                              rdl:PCA_100006438 ,
                              rdl:PCA_100006439 ,
                              rdl:PCA_100006440 ,
                              rdl:PCA_100006441 ,
                              rdl:PCA_100006442 ,
                              rdl:PCA_100006443 ,
                              rdl:PCA_100006444 ,
                              rdl:PCA_100006445 ,
                              rdl:PCA_100006446 ,
                              rdl:PCA_100006447 ,
                              rdl:PCA_100006448 ,
                              rdl:PCA_100006449 ,
                              rdl:PCA_100006450 ,
                              rdl:PCA_100006451 ,
                              rdl:PCA_100006452 ,
                              rdl:PCA_100006453 ,
                              rdl:PCA_100006454 ,
                              rdl:PCA_100006455 ,
                              rdl:PCA_100006456 ,
                              rdl:PCA_100006457 ,
                              rdl:PCA_100006458 ,
                              rdl:PCA_100006459 ,
                              rdl:PCA_100006460 ,
                              rdl:PCA_100006461 ,
                              rdl:PCA_100006462 ,
                              rdl:PCA_100006463 ,
                              rdl:PCA_100006464 ,
                              rdl:PCA_100006465 ,
                              rdl:PCA_100006466 ,
                              rdl:PCA_100006467 ,
                              rdl:PCA_100006468 ,
                              rdl:PCA_100006469 ,
                              rdl:PCA_100006470 ,
                              rdl:PCA_100006471 ,
                              rdl:PCA_100006472 ,
                              rdl:PCA_100006473 ,
                              rdl:PCA_100006474 ,
                              rdl:PCA_100006475 ,
                              rdl:PCA_100006476 ,
                              rdl:PCA_100006477 ,
                              rdl:PCA_100006478 ,
                              rdl:PCA_100006479 ,
                              rdl:PCA_100006480 ,
                              rdl:PCA_100006481 ,
                              rdl:PCA_100006482 ,
                              rdl:PCA_100006483 ,
                              rdl:PCA_100006484 ,
                              rdl:PCA_100006485 ,
                              rdl:PCA_100006486 ,
                              rdl:PCA_100006487 ,
                              rdl:PCA_100006488 ,
                              rdl:PCA_100006489 ,
                              rdl:PCA_100006490 ,
                              rdl:PCA_100006491 ,
                              rdl:PCA_100006492 ,
                              rdl:PCA_100006493 ,
                              rdl:PCA_100006494 ,
                              rdl:PCA_100006495 ,
                              rdl:PCA_100006496 ,
                              rdl:PCA_100006497 ,
                              rdl:PCA_100006498 ,
                              rdl:PCA_100006499 ,
                              rdl:PCA_100006500 ,
                              rdl:PCA_100006501 ,
                              rdl:PCA_100006502 ,
                              rdl:PCA_100006503 ,
                              rdl:PCA_100006504 ,
                              rdl:PCA_100006505 ,
                              rdl:PCA_100006506 ,
                              rdl:PCA_100006507 ,
                              rdl:PCA_100006508 ,
                              rdl:PCA_100006509 ,
                              rdl:PCA_100006510 ,
                              rdl:PCA_100006511 ,
                              rdl:PCA_100006512 ,
                              rdl:PCA_100006513 ,
                              rdl:PCA_100006514 ,
                              rdl:PCA_100006515 ,
                              rdl:PCA_100006516 ,
                              rdl:PCA_100006517 ,
                              rdl:PCA_100006518 ,
                              rdl:PCA_100006519 ,
                              rdl:PCA_100006520 ,
                              rdl:PCA_100006521 ,
                              rdl:PCA_100006522 ,
                              rdl:PCA_100006523 ,
                              rdl:PCA_100006524 ,
                              rdl:PCA_100006525 ,
                              rdl:PCA_100006526 ,
                              rdl:PCA_100006527 ,
                              rdl:PCA_100006528 ,
                              rdl:PCA_100006529 ,
                              rdl:PCA_100006530 ,
                              rdl:PCA_100006531 ,
                              rdl:PCA_100006532 ,
                              rdl:PCA_100006533 ,
                              rdl:PCA_100006534 ,
                              rdl:PCA_100006535 ,
                              rdl:PCA_100006536 ,
                              rdl:PCA_100006537 ,
                              rdl:PCA_100006538 ,
                              rdl:PCA_100006539 ,
                              rdl:PCA_100006540 ,
                              rdl:PCA_100006541 ,
                              rdl:PCA_100006542 ,
                              rdl:PCA_100006543 ,
                              rdl:PCA_100006544 ,
                              rdl:PCA_100006545 ,
                              rdl:PCA_100006546 .


###  Generated by the OWL API (version 5.1.7) https://github.com/owlcs/owlapi/
