<rdf:RDF
    xmlns:req="https://w3id.org/requirement-ontology/rdl/"
    xmlns:o-owl-ax="http://tpl.ottr.xyz/owl/axiom/0.1/"
    xmlns:o-owl-dec="http://tpl.ottr.xyz/owl/declaration/0.1/"
    xmlns:o-docttr="http://tpl.ottr.xyz/p/docttr/0.1/"
    xmlns:o-owl-ma="http://tpl.ottr.xyz/owl/macro/0.1/"
    xmlns:ntpl="http://norsok.org/templates/"
    xmlns:dcterms="http://purl.org/dc/terms/"
    xmlns:dc="http://purl.org/dc/elements/1.1/"
    xmlns:pca="http://data.posccaesar.org/rdl/"
    xmlns:skos="http://www.w3.org/2004/02/skos/core#"
    xmlns:sd="http://www.w3.org/ns/sparql-service-description#"
    xmlns:vann="http://purl.org/vocab/vann/"
    xmlns:orcid="https://orcid.org/"
    xmlns:xsd="http://www.w3.org/2001/XMLSchema#"
    xmlns:lis="http://rds.posccaesar.org/ontology/lis14/rdl/"
    xmlns:rdf="http://www.w3.org/1999/02/22-rdf-syntax-ns#"
    xmlns:rdl="http://rds.posccaesar.org/ontology/plm/rdl/"
    xmlns:rdfs="http://www.w3.org/2000/01/rdf-schema#"
    xmlns:rrdl="http://w3id.org/readi/rdl/"
    xmlns:void="http://rdfs.org/ns/void#"
    xmlns:o-rdfs="http://tpl.ottr.xyz/rdfs/0.1/"
    xmlns:plmtpl="http://rds.posccaesar.org/ontology/plm/tpl/0.1/"
    xmlns:listpl="http://rds.posccaesar.org/ontology/lis14/tpl/0.1/"
    xmlns:ottr="http://ns.ottr.xyz/0.4/"
    xmlns:ex="http://example.org/"
    xmlns="http://www.semanticweb.org/owl/owlapi/turtle#"
    xmlns:owl="http://www.w3.org/2002/07/owl#"
    xmlns:o-owl-re="http://tpl.ottr.xyz/owl/restriction/0.1/"
    xmlns:pav="http://purl.org/pav/"
    xmlns:o-rdf="http://tpl.ottr.xyz/rdf/0.1/"
    xmlns:reqtpl="http://w3id.org/requirement-ontology/tpl/0.1/"
    xmlns:foaf="http://xmlns.com/foaf/0.1/"
    xmlns:om="http://www.ontology-of-units-of-measure.org/resource/om-2/"
    xmlns:o-owl-ut="http://tpl.ottr.xyz/owl/util/0.1/">
  <owl:Ontology rdf:about="http://rds.posccaesar.org/ontology/plm/ont/norsok-z001">
    <owl:imports rdf:resource="http://rds.posccaesar.org/ontology/plm/ont/document"/>
    <owl:versionIRI rdf:resource="http://rds.posccaesar.org/ontology/plm/ont/norsok-z001/0.1.1"/>
    <void:feature rdf:resource="http://www.w3.org/ns/formats/OWL_Manchester"/>
    <void:feature rdf:resource="http://www.w3.org/ns/formats/JSON-LD"/>
    <pav:lastUpdateOn rdf:datatype="http://www.w3.org/2001/XMLSchema#dateTime"
    >2022-09-26T23:40:00Z</pav:lastUpdateOn>
    <void:feature rdf:resource="http://www.w3.org/ns/formats/Turtle"/>
    <vann:preferredNamespacePrefix>rdl</vann:preferredNamespacePrefix>
    <dc:title>norsok-z001</dc:title>
    <dcterms:modified rdf:datatype="http://www.w3.org/2001/XMLSchema#date"
    >2022-09-26</dcterms:modified>
    <dcterms:publisher rdf:resource="http://www.posccaesar.org/"/>
    <pav:createdBy rdf:resource="https://orcid.org/0000-0002-7167-7321"/>
    <vann:preferredNamespaceUri rdf:resource="http://rds.posccaesar.org/ontology/plm/rdl/"/>
    <void:sparqlEndpoint rdf:resource="https://rds.posccaesar.org/ontology/sparql"/>
    <void:feature rdf:resource="http://www.w3.org/ns/formats/N-Triples"/>
    <dc:description>NORSOK Z-001 Information Item ontology</dc:description>
    <pav:hasPreviousVersion rdf:resource="http://rds.posccaesar.org/ontology/plm/ont/norsok-z001/0.1.0"/>
    <dc:creator rdf:resource="https://orcid.org/0000-0002-7167-7321"/>
    <void:feature rdf:resource="http://www.w3.org/ns/formats/RDF_XML"/>
    <rdfs:label>norsok-z001</rdfs:label>
    <owl:versionInfo>0.1.1</owl:versionInfo>
    <ottr:status rdf:resource="http://ns.ottr.xyz/0.4/incomplete"/>
    <skos:changeNote>Z-001 Item collection</skos:changeNote>
    <dcterms:issued rdf:datatype="http://www.w3.org/2001/XMLSchema#date"
    >2022-05-02</dcterms:issued>
    <rdfs:comment>NORSOK Z-001 Information Item ontology</rdfs:comment>
  </owl:Ontology>
  <owl:Class rdf:about="http://rds.posccaesar.org/ontology/plm/rdl/PCA_100006294">
    <skos:broader>
      <rdl:PCA_100001503 rdf:about="http://rds.posccaesar.org/ontology/plm/rdl/PCA_100006746">
        <rdfs:label>Drawing</rdfs:label>
        <rdl:PCA_100004924>DR</rdl:PCA_100004924>
        <rdf:type rdf:resource="http://www.w3.org/2002/07/owl#NamedIndividual"/>
      </rdl:PCA_100001503>
    </skos:broader>
    <skos:broadMatch>
      <rdl:PCA_100001503 rdf:about="http://rds.posccaesar.org/ontology/plm/rdl/PCA_100006705">
        <rdfs:label>site information</rdfs:label>
        <rdl:PCA_100004924>LA</rdl:PCA_100004924>
        <rdf:type rdf:resource="http://www.w3.org/2002/07/owl#NamedIndividual"/>
      </rdl:PCA_100001503>
    </skos:broadMatch>
    <rdfs:label>Landscaping drawings</rdfs:label>
    <rdfs:comment>All arrangement, layout, plan, section and detail drawings shall be included.</rdfs:comment>
    <rdl:PCA_100006768>All arrangement, layout, plan, section and detail drawings shall be included.</rdl:PCA_100006768>
    <rdl:PCA_100006766>
      <rdl:PCA_100001503 rdf:about="http://rds.posccaesar.org/ontology/plm/rdl/PCA_100006656">
        <rdfs:label>Location</rdfs:label>
        <rdf:type rdf:resource="http://www.w3.org/2002/07/owl#NamedIndividual"/>
      </rdl:PCA_100001503>
    </rdl:PCA_100006766>
    <rdl:PCA_100006765>
      <rdl:PCA_100001503 rdf:about="http://w3id.org/readi/rdl/CFIHOS-20000007">
        <rdfs:label>civil engineering</rdfs:label>
        <rdl:PCA_100004924>CX</rdl:PCA_100004924>
        <rdf:type rdf:resource="http://www.w3.org/2002/07/owl#NamedIndividual"/>
      </rdl:PCA_100001503>
    </rdl:PCA_100006765>
    <rdfs:subClassOf rdf:resource="http://rds.posccaesar.org/ontology/plm/rdl/PCA_100004908"/>
  </owl:Class>
  <owl:Class rdf:about="http://rds.posccaesar.org/ontology/plm/rdl/PCA_100006160">
    <skos:broader rdf:resource="http://rds.posccaesar.org/ontology/plm/rdl/PCA_100006746"/>
    <skos:broadMatch>
      <rdl:PCA_100001503 rdf:about="http://rds.posccaesar.org/ontology/plm/rdl/PCA_100006732">
        <rdfs:label>geometrical detail information</rdfs:label>
        <rdl:PCA_100004924>TB</rdl:PCA_100004924>
        <rdf:type rdf:resource="http://www.w3.org/2002/07/owl#NamedIndividual"/>
      </rdl:PCA_100001503>
    </skos:broadMatch>
    <rdfs:label>Detail cross sectional drawings with parts list</rdfs:label>
    <rdfs:comment>A view or drawing that shows what the inside of equipment looks like after a cross-sectional cut has been made.
The manufacturer's standard detail cross sectional drawing shall be delivered.
Typical information may be:
 - Items list with reference to supplier’s  part number.
 - Material definition with reference to relevant  standards</rdfs:comment>
    <rdl:PCA_100006768>A view or drawing that shows what the inside of equipment looks like after a cross-sectional cut has been made.
The manufacturer's standard detail cross sectional drawing shall be delivered.
Typical information may be:
 - Items list with reference to supplier’s  part number.
 - Material definition with reference to relevant  standards</rdl:PCA_100006768>
    <rdl:PCA_100006766>
      <rdl:PCA_100001503 rdf:about="http://rds.posccaesar.org/ontology/plm/rdl/PCA_100006653">
        <rdfs:label>Equipment</rdfs:label>
        <rdf:type rdf:resource="http://www.w3.org/2002/07/owl#NamedIndividual"/>
      </rdl:PCA_100001503>
    </rdl:PCA_100006766>
    <rdl:PCA_100006763>A detail and cross sectional drawing with parts list to facilitate dismantling, repair and assembly of parts and components shall be included. Relevant for assemblies and smaller components within assemblies.</rdl:PCA_100006763>
    <rdfs:subClassOf rdf:resource="http://rds.posccaesar.org/ontology/plm/rdl/PCA_100004908"/>
  </owl:Class>
  <owl:Class rdf:about="http://rds.posccaesar.org/ontology/plm/rdl/PCA_100006282">
    <rdl:PCA_100006766 rdf:resource="http://rds.posccaesar.org/ontology/plm/rdl/PCA_100006653"/>
    <skos:broader>
      <rdl:PCA_100001503 rdf:about="http://rds.posccaesar.org/ontology/plm/rdl/PCA_100006747">
        <rdfs:label>Data sheet</rdfs:label>
        <rdl:PCA_100004924>DS</rdl:PCA_100004924>
        <rdf:type rdf:resource="http://www.w3.org/2002/07/owl#NamedIndividual"/>
      </rdl:PCA_100001503>
    </skos:broader>
    <rdfs:subClassOf rdf:resource="http://rds.posccaesar.org/ontology/plm/rdl/PCA_100004908"/>
    <rdl:PCA_100006763>Used in engineering process to verify compliance with plant and process design. Used in operational phase for verification purposes, and in case replacement/modification of equipment is required.</rdl:PCA_100006763>
    <skos:broadMatch>
      <rdl:PCA_100001503 rdf:about="http://rds.posccaesar.org/ontology/plm/rdl/PCA_100006686">
        <rdfs:label>technical property information</rdfs:label>
        <rdl:PCA_100004924>DA</rdl:PCA_100004924>
        <rdf:type rdf:resource="http://www.w3.org/2002/07/owl#NamedIndividual"/>
      </rdl:PCA_100001503>
    </skos:broadMatch>
    <rdl:PCA_100006768>Supplier shall complete the data sheets as specified by customer. Content and data format to be solved in inquiry phase. Not required for commodity valves and manual on/off valves</rdl:PCA_100006768>
    <rdfs:comment>Supplier shall complete the data sheets as specified by customer. Content and data format to be solved in inquiry phase. Not required for commodity valves and manual on/off valves</rdfs:comment>
    <rdl:PCA_100006765>
      <rdl:PCA_100001503 rdf:about="http://w3id.org/readi/rdl/CFIHOS-20000015">
        <rdfs:label>instrumentation engineering</rdfs:label>
        <rdl:PCA_100004924>IN</rdl:PCA_100004924>
        <rdf:type rdf:resource="http://www.w3.org/2002/07/owl#NamedIndividual"/>
      </rdl:PCA_100001503>
    </rdl:PCA_100006765>
    <rdfs:label>Instrument data sheet</rdfs:label>
  </owl:Class>
  <owl:Class rdf:about="http://rds.posccaesar.org/ontology/plm/rdl/PCA_100006391">
    <skos:broader>
      <rdl:PCA_100001503 rdf:about="http://rds.posccaesar.org/ontology/plm/rdl/PCA_100006751">
        <rdfs:label>Procedure</rdfs:label>
        <rdl:PCA_100004924>PD</rdl:PCA_100004924>
        <rdf:type rdf:resource="http://www.w3.org/2002/07/owl#NamedIndividual"/>
      </rdl:PCA_100001503>
    </skos:broader>
    <skos:broadMatch>
      <rdl:PCA_100001503 rdf:about="http://rds.posccaesar.org/ontology/plm/rdl/PCA_100006722">
        <rdfs:label>validation and verification information</rdfs:label>
        <rdl:PCA_100004924>QC</rdl:PCA_100004924>
        <rdf:type rdf:resource="http://www.w3.org/2002/07/owl#NamedIndividual"/>
      </rdl:PCA_100001503>
    </skos:broadMatch>
    <rdfs:label>Procedure - pickling / passivation / flushing / visual cleanliness check - multi</rdfs:label>
    <rdfs:comment>Pickling, passivation, flushing and visual cleanliness check to be documented</rdfs:comment>
    <rdl:PCA_100006768>Pickling, passivation, flushing and visual cleanliness check to be documented</rdl:PCA_100006768>
    <rdl:PCA_100006766 rdf:resource="http://rds.posccaesar.org/ontology/plm/rdl/PCA_100006653"/>
    <rdl:PCA_100006763>This document is used for verification of compliance</rdl:PCA_100006763>
    <rdfs:subClassOf rdf:resource="http://rds.posccaesar.org/ontology/plm/rdl/PCA_100004908"/>
  </owl:Class>
  <owl:Class rdf:about="http://rds.posccaesar.org/ontology/plm/rdl/PCA_100006172">
    <rdfs:comment>Report containing results from the EFAT including check records and pictures from the procedure steps.</rdfs:comment>
    <rdl:PCA_100006766 rdf:resource="http://rds.posccaesar.org/ontology/plm/rdl/PCA_100006653"/>
    <rdfs:label>EFAT report</rdfs:label>
    <rdl:PCA_100006768>Report containing results from the EFAT including check records and pictures from the procedure steps.</rdl:PCA_100006768>
    <rdl:PCA_100006763>Document the tests performed in accordance with the procedure.</rdl:PCA_100006763>
    <skos:broadMatch rdf:resource="http://rds.posccaesar.org/ontology/plm/rdl/PCA_100006722"/>
    <rdl:PCA_100006765>
      <rdl:PCA_100001503 rdf:about="http://w3id.org/readi/rdl/CFIHOS-20000031">
        <rdfs:label>subsea engineering</rdfs:label>
        <rdl:PCA_100004924>UA</rdl:PCA_100004924>
        <rdf:type rdf:resource="http://www.w3.org/2002/07/owl#NamedIndividual"/>
      </rdl:PCA_100001503>
    </rdl:PCA_100006765>
    <skos:broader>
      <rdl:PCA_100001503 rdf:about="http://rds.posccaesar.org/ontology/plm/rdl/PCA_100006756">
        <rdfs:label>Report</rdfs:label>
        <rdl:PCA_100004924>RP</rdl:PCA_100004924>
        <rdf:type rdf:resource="http://www.w3.org/2002/07/owl#NamedIndividual"/>
      </rdl:PCA_100001503>
    </skos:broader>
    <rdfs:subClassOf rdf:resource="http://rds.posccaesar.org/ontology/plm/rdl/PCA_100004908"/>
  </owl:Class>
  <owl:Class rdf:about="http://rds.posccaesar.org/ontology/plm/rdl/PCA_100006270">
    <skos:broader rdf:resource="http://rds.posccaesar.org/ontology/plm/rdl/PCA_100006756"/>
    <rdfs:subClassOf rdf:resource="http://rds.posccaesar.org/ontology/plm/rdl/PCA_100004908"/>
    <skos:broadMatch>
      <rdl:PCA_100001503 rdf:about="http://rds.posccaesar.org/ontology/plm/rdl/PCA_100006687">
        <rdfs:label>explanatory technical information</rdfs:label>
        <rdl:PCA_100004924>DB</rdl:PCA_100004924>
        <rdf:type rdf:resource="http://www.w3.org/2002/07/owl#NamedIndividual"/>
      </rdl:PCA_100001503>
    </skos:broadMatch>
    <rdl:PCA_100006763>A report verifying that equipment will remain in in-place condition.</rdl:PCA_100006763>
    <rdl:PCA_100006766 rdf:resource="http://rds.posccaesar.org/ontology/plm/rdl/PCA_100006653"/>
    <rdfs:label>In-place analysis report</rdfs:label>
    <rdl:PCA_100006765 rdf:resource="http://w3id.org/readi/rdl/CFIHOS-20000031"/>
    <rdl:PCA_100006768>A report containing design analysis/calculations for in-place condition, including loads and load cases.</rdl:PCA_100006768>
    <rdfs:comment>A report containing design analysis/calculations for in-place condition, including loads and load cases.</rdfs:comment>
  </owl:Class>
  <owl:Class rdf:about="http://rds.posccaesar.org/ontology/plm/rdl/PCA_100006184">
    <skos:broadMatch>
      <rdl:PCA_100001503 rdf:about="http://rds.posccaesar.org/ontology/plm/rdl/PCA_100006667">
        <rdfs:label>planning information</rdfs:label>
        <rdl:PCA_100004924>BE</rdl:PCA_100004924>
        <rdf:type rdf:resource="http://www.w3.org/2002/07/owl#NamedIndividual"/>
      </rdl:PCA_100001503>
    </skos:broadMatch>
    <rdfs:label>Engineering, procurement and manufacturing schedule</rdfs:label>
    <rdfs:comment>Schedule to include planned activities from order receipt, order entry to sub-suppliers, goods receipt, assembly, testing and shipping/delivery.</rdfs:comment>
    <rdl:PCA_100006768>Schedule to include planned activities from order receipt, order entry to sub-suppliers, goods receipt, assembly, testing and shipping/delivery.</rdl:PCA_100006768>
    <rdl:PCA_100006766 rdf:resource="http://rds.posccaesar.org/ontology/plm/rdl/PCA_100006653"/>
    <rdl:PCA_100006765>
      <rdl:PCA_100001503 rdf:about="http://w3id.org/readi/rdl/CFIHOS-20000001">
        <rdfs:label>project management and engineering</rdfs:label>
        <rdl:PCA_100004924>AA</rdl:PCA_100004924>
        <rdf:type rdf:resource="http://www.w3.org/2002/07/owl#NamedIndividual"/>
      </rdl:PCA_100001503>
    </rdl:PCA_100006765>
    <rdl:PCA_100006763>Schedule of planned activities from order entry to delivery. EPMS substantiates compliance with delivery requirements, and support planning of expediting activities.</rdl:PCA_100006763>
    <rdfs:subClassOf rdf:resource="http://rds.posccaesar.org/ontology/plm/rdl/PCA_100004908"/>
  </owl:Class>
  <owl:Class rdf:about="http://rds.posccaesar.org/ontology/plm/rdl/PCA_100006196">
    <rdl:PCA_100006763>Ensure safe operation</rdl:PCA_100006763>
    <skos:broader rdf:resource="http://rds.posccaesar.org/ontology/plm/rdl/PCA_100006756"/>
    <rdfs:label>Expansion design report</rdfs:label>
    <rdl:PCA_100006766>
      <rdl:PCA_100001503 rdf:about="http://rds.posccaesar.org/ontology/plm/rdl/PCA_100006654">
        <rdfs:label>Facility</rdfs:label>
        <rdf:type rdf:resource="http://www.w3.org/2002/07/owl#NamedIndividual"/>
      </rdl:PCA_100001503>
    </rdl:PCA_100006766>
    <rdfs:subClassOf rdf:resource="http://rds.posccaesar.org/ontology/plm/rdl/PCA_100004908"/>
    <rdfs:comment>Design report covering pipeline expansion and buckling analysis including pipeline soil interaction. Basis for analysis, assumptions and assessments not given in design basis shall be included.</rdfs:comment>
    <skos:broadMatch rdf:resource="http://rds.posccaesar.org/ontology/plm/rdl/PCA_100006686"/>
    <rdl:PCA_100006768>Design report covering pipeline expansion and buckling analysis including pipeline soil interaction. Basis for analysis, assumptions and assessments not given in design basis shall be included.</rdl:PCA_100006768>
    <rdl:PCA_100006765>
      <rdl:PCA_100001503 rdf:about="http://w3id.org/readi/rdl/CFIHOS-20000018">
        <rdfs:label>pipeline engineering</rdfs:label>
        <rdl:PCA_100004924>LA</rdl:PCA_100004924>
        <rdf:type rdf:resource="http://www.w3.org/2002/07/owl#NamedIndividual"/>
      </rdl:PCA_100001503>
    </rdl:PCA_100006765>
  </owl:Class>
  <owl:Class rdf:about="http://rds.posccaesar.org/ontology/plm/rdl/PCA_100006087">
    <rdl:PCA_100006766>
      <rdl:PCA_100001503 rdf:about="http://rds.posccaesar.org/ontology/plm/rdl/PCA_100006629">
        <rdfs:label>Material handling</rdfs:label>
        <rdl:PCA_100004924>73</rdl:PCA_100004924>
        <rdf:type rdf:resource="http://www.w3.org/2002/07/owl#NamedIndividual"/>
      </rdl:PCA_100001503>
    </rdl:PCA_100006766>
    <rdl:PCA_100006768>An ALARP register could contain the following information fields:
 - Unique identification number;
 - Source of identification, e.g. Hazop;
 - Cross reference to other databases/registers, for instance the uncertainty management register;
 - Description of the hazard/risk to be prevented or mitigated;
 - Description of the risk reducing measure;
 - Relevant DSHA(s);
 - Relevant safety barrier(s);
 - Coarse risk evaluation;
 - Decision based on coarse risk evaluation;
 - Date and signature for coarse risk evaluation/decision;
 - Detailed risk evaluation, if applicable;
 - Decision based on detailed risk evaluation, if applicable;
 - Date and signature for detailed risk evaluation/decision, if applicable.</rdl:PCA_100006768>
    <rdl:PCA_100006765>
      <rdl:PCA_100001503 rdf:about="http://w3id.org/readi/rdl/CFIHOS-20000010">
        <rdfs:label>environmental</rdfs:label>
        <rdl:PCA_100004924>HE</rdl:PCA_100004924>
        <rdf:type rdf:resource="http://www.w3.org/2002/07/owl#NamedIndividual"/>
      </rdl:PCA_100001503>
    </rdl:PCA_100006765>
    <rdl:PCA_100006766>
      <rdl:PCA_100001503 rdf:about="http://rds.posccaesar.org/ontology/plm/rdl/PCA_100006633">
        <rdfs:label>Emergency shutdown and blow down</rdfs:label>
        <rdl:PCA_100004924>79</rdl:PCA_100004924>
        <rdf:type rdf:resource="http://www.w3.org/2002/07/owl#NamedIndividual"/>
      </rdl:PCA_100001503>
    </rdl:PCA_100006766>
    <rdfs:subClassOf rdf:resource="http://rds.posccaesar.org/ontology/plm/rdl/PCA_100004908"/>
    <rdl:PCA_100006763>The ALARP register should be established to keep track of identification, evaluation and decision regarding risk reducing measures.</rdl:PCA_100006763>
    <rdl:PCA_100006765>
      <rdl:PCA_100001503 rdf:about="http://w3id.org/readi/rdl/CFIHOS-20000013">
        <rdfs:label>safety</rdfs:label>
        <rdl:PCA_100004924>HS</rdl:PCA_100004924>
        <rdf:type rdf:resource="http://www.w3.org/2002/07/owl#NamedIndividual"/>
      </rdl:PCA_100001503>
    </rdl:PCA_100006765>
    <skos:broader>
      <rdl:PCA_100001503 rdf:about="http://rds.posccaesar.org/ontology/plm/rdl/PCA_100006748">
        <rdfs:label>List/Index</rdfs:label>
        <rdl:PCA_100004924>LI</rdl:PCA_100004924>
        <rdf:type rdf:resource="http://www.w3.org/2002/07/owl#NamedIndividual"/>
      </rdl:PCA_100001503>
    </skos:broader>
    <rdl:PCA_100006766>
      <rdl:PCA_100001503 rdf:about="http://rds.posccaesar.org/ontology/plm/rdl/PCA_100006631">
        <rdfs:label>Emergency preparedness</rdfs:label>
        <rdl:PCA_100004924>76</rdl:PCA_100004924>
        <rdf:type rdf:resource="http://www.w3.org/2002/07/owl#NamedIndividual"/>
      </rdl:PCA_100001503>
    </rdl:PCA_100006766>
    <skos:broadMatch>
      <rdl:PCA_100001503 rdf:about="http://rds.posccaesar.org/ontology/plm/rdl/PCA_100006727">
        <rdfs:label>equipment protection information</rdfs:label>
        <rdl:PCA_100004924>RB</rdl:PCA_100004924>
        <rdf:type rdf:resource="http://www.w3.org/2002/07/owl#NamedIndividual"/>
      </rdl:PCA_100001503>
    </skos:broadMatch>
    <rdfs:comment>An ALARP register could contain the following information fields:
 - Unique identification number;
 - Source of identification, e.g. Hazop;
 - Cross reference to other databases/registers, for instance the uncertainty management register;
 - Description of the hazard/risk to be prevented or mitigated;
 - Description of the risk reducing measure;
 - Relevant DSHA(s);
 - Relevant safety barrier(s);
 - Coarse risk evaluation;
 - Decision based on coarse risk evaluation;
 - Date and signature for coarse risk evaluation/decision;
 - Detailed risk evaluation, if applicable;
 - Decision based on detailed risk evaluation, if applicable;
 - Date and signature for detailed risk evaluation/decision, if applicable.</rdfs:comment>
    <rdl:PCA_100006766>
      <rdl:PCA_100001503 rdf:about="http://rds.posccaesar.org/ontology/plm/rdl/PCA_100006630">
        <rdfs:label>Passive fire protection</rdfs:label>
        <rdl:PCA_100004924>75</rdl:PCA_100004924>
        <rdf:type rdf:resource="http://www.w3.org/2002/07/owl#NamedIndividual"/>
      </rdl:PCA_100001503>
    </rdl:PCA_100006766>
    <rdl:PCA_100006765>
      <rdl:PCA_100001503 rdf:about="http://w3id.org/readi/rdl/CFIHOS-20000011">
        <rdfs:label>health</rdfs:label>
        <rdl:PCA_100004924>HH</rdl:PCA_100004924>
        <rdf:type rdf:resource="http://www.w3.org/2002/07/owl#NamedIndividual"/>
      </rdl:PCA_100001503>
    </rdl:PCA_100006765>
    <rdl:PCA_100006766>
      <rdl:PCA_100001503 rdf:about="http://rds.posccaesar.org/ontology/plm/rdl/PCA_100006626">
        <rdfs:label>Fire and gas detection</rdfs:label>
        <rdl:PCA_100004924>70</rdl:PCA_100004924>
        <rdf:type rdf:resource="http://www.w3.org/2002/07/owl#NamedIndividual"/>
      </rdl:PCA_100001503>
    </rdl:PCA_100006766>
    <rdl:PCA_100006766>
      <rdl:PCA_100001503 rdf:about="http://rds.posccaesar.org/ontology/plm/rdl/PCA_100006628">
        <rdfs:label>Fire fighting</rdfs:label>
        <rdl:PCA_100004924>72</rdl:PCA_100004924>
        <rdf:type rdf:resource="http://www.w3.org/2002/07/owl#NamedIndividual"/>
      </rdl:PCA_100001503>
    </rdl:PCA_100006766>
    <rdfs:label>ALARP register</rdfs:label>
    <rdl:PCA_100006766>
      <rdl:PCA_100001503 rdf:about="http://rds.posccaesar.org/ontology/plm/rdl/PCA_100006632">
        <rdfs:label>Environment protection</rdfs:label>
        <rdl:PCA_100004924>77</rdl:PCA_100004924>
        <rdf:type rdf:resource="http://www.w3.org/2002/07/owl#NamedIndividual"/>
      </rdl:PCA_100001503>
    </rdl:PCA_100006766>
    <skos:broadMatch>
      <rdl:PCA_100001503 rdf:about="http://rds.posccaesar.org/ontology/plm/rdl/PCA_100006726">
        <rdfs:label>health protection information</rdfs:label>
        <rdl:PCA_100004924>RA</rdl:PCA_100004924>
        <rdf:type rdf:resource="http://www.w3.org/2002/07/owl#NamedIndividual"/>
      </rdl:PCA_100001503>
    </skos:broadMatch>
    <rdl:PCA_100006766>
      <rdl:PCA_100001503 rdf:about="http://rds.posccaesar.org/ontology/plm/rdl/PCA_100006627">
        <rdfs:label>Fire water</rdfs:label>
        <rdl:PCA_100004924>71</rdl:PCA_100004924>
        <rdf:type rdf:resource="http://www.w3.org/2002/07/owl#NamedIndividual"/>
      </rdl:PCA_100001503>
    </rdl:PCA_100006766>
  </owl:Class>
  <owl:Class rdf:about="http://rds.posccaesar.org/ontology/plm/rdl/PCA_100006099">
    <rdl:PCA_100006766 rdf:resource="http://rds.posccaesar.org/ontology/plm/rdl/PCA_100006626"/>
    <rdl:PCA_100006766 rdf:resource="http://rds.posccaesar.org/ontology/plm/rdl/PCA_100006629"/>
    <rdl:PCA_100006766 rdf:resource="http://rds.posccaesar.org/ontology/plm/rdl/PCA_100006628"/>
    <rdfs:subClassOf rdf:resource="http://rds.posccaesar.org/ontology/plm/rdl/PCA_100004908"/>
    <rdfs:comment>A complete list to identify of all potential ignition sources that could come into contact with explosive atmosphere and the likelihood of occurrence of the potential ignition source to become effective.  

Reference is made to EN 1127-1.</rdfs:comment>
    <rdl:PCA_100006763>The document shall be result of a systematic mapping of all potential ignition sources both electrical and non-electrical, including risk assessment and risk reduction measures in order to reduce ignition probability of an explosive atmosphere occurring in both hazardous and non-hazardous areas. The equipment shall be categorized as non-essential, essential and safety critical equipment respectively.</rdl:PCA_100006763>
    <rdl:PCA_100006765 rdf:resource="http://w3id.org/readi/rdl/CFIHOS-20000013"/>
    <rdl:PCA_100006766>
      <rdl:PCA_100001503 rdf:about="http://rds.posccaesar.org/ontology/plm/rdl/PCA_100006641">
        <rdfs:label>Control</rdfs:label>
        <rdl:PCA_100004924>87</rdl:PCA_100004924>
        <rdf:type rdf:resource="http://www.w3.org/2002/07/owl#NamedIndividual"/>
      </rdl:PCA_100001503>
    </rdl:PCA_100006766>
    <rdl:PCA_100006766>
      <rdl:PCA_100001503 rdf:about="http://rds.posccaesar.org/ontology/plm/rdl/PCA_100006638">
        <rdfs:label>Emergency power (u&lt;1.0 kV)</rdfs:label>
        <rdl:PCA_100004924>84</rdl:PCA_100004924>
        <rdf:type rdf:resource="http://www.w3.org/2002/07/owl#NamedIndividual"/>
      </rdl:PCA_100001503>
    </rdl:PCA_100006766>
    <rdl:PCA_100006766>
      <rdl:PCA_100001503 rdf:about="http://rds.posccaesar.org/ontology/plm/rdl/PCA_100006637">
        <rdfs:label>Emergency power (u = or &gt;1.0 kV)</rdfs:label>
        <rdl:PCA_100004924>83</rdl:PCA_100004924>
        <rdf:type rdf:resource="http://www.w3.org/2002/07/owl#NamedIndividual"/>
      </rdl:PCA_100001503>
    </rdl:PCA_100006766>
    <skos:broadMatch>
      <rdl:PCA_100001503 rdf:about="http://rds.posccaesar.org/ontology/plm/rdl/PCA_100006718">
        <rdfs:label>product listing</rdfs:label>
        <rdl:PCA_100004924>PD</rdl:PCA_100004924>
        <rdf:type rdf:resource="http://www.w3.org/2002/07/owl#NamedIndividual"/>
      </rdl:PCA_100001503>
    </skos:broadMatch>
    <skos:broadMatch>
      <rdl:PCA_100001503 rdf:about="http://rds.posccaesar.org/ontology/plm/rdl/PCA_100006717">
        <rdfs:label>items listing</rdfs:label>
        <rdl:PCA_100004924>PC</rdl:PCA_100004924>
        <rdf:type rdf:resource="http://www.w3.org/2002/07/owl#NamedIndividual"/>
      </rdl:PCA_100001503>
    </skos:broadMatch>
    <rdl:PCA_100006766>
      <rdl:PCA_100001503 rdf:about="http://rds.posccaesar.org/ontology/plm/rdl/PCA_100006640">
        <rdfs:label>Telecommunication</rdfs:label>
        <rdl:PCA_100004924>86</rdl:PCA_100004924>
        <rdf:type rdf:resource="http://www.w3.org/2002/07/owl#NamedIndividual"/>
      </rdl:PCA_100001503>
    </rdl:PCA_100006766>
    <rdl:PCA_100006766>
      <rdl:PCA_100001503 rdf:about="http://rds.posccaesar.org/ontology/plm/rdl/PCA_100006636">
        <rdfs:label>Main power (u = or &lt;1.0 kV)</rdfs:label>
        <rdl:PCA_100004924>82</rdl:PCA_100004924>
        <rdf:type rdf:resource="http://www.w3.org/2002/07/owl#NamedIndividual"/>
      </rdl:PCA_100001503>
    </rdl:PCA_100006766>
    <rdl:PCA_100006765 rdf:resource="http://w3id.org/readi/rdl/CFIHOS-20000011"/>
    <rdl:PCA_100006766 rdf:resource="http://rds.posccaesar.org/ontology/plm/rdl/PCA_100006630"/>
    <rdl:PCA_100006766>
      <rdl:PCA_100001503 rdf:about="http://rds.posccaesar.org/ontology/plm/rdl/PCA_100006635">
        <rdfs:label>Main power (1.0 kV&lt; u &lt; 6.6 kV)</rdfs:label>
        <rdl:PCA_100004924>81</rdl:PCA_100004924>
        <rdf:type rdf:resource="http://www.w3.org/2002/07/owl#NamedIndividual"/>
      </rdl:PCA_100001503>
    </rdl:PCA_100006766>
    <rdl:PCA_100006766>
      <rdl:PCA_100001503 rdf:about="http://rds.posccaesar.org/ontology/plm/rdl/PCA_100006639">
        <rdfs:label>Battery and no-break</rdfs:label>
        <rdl:PCA_100004924>85</rdl:PCA_100004924>
        <rdf:type rdf:resource="http://www.w3.org/2002/07/owl#NamedIndividual"/>
      </rdl:PCA_100001503>
    </rdl:PCA_100006766>
    <rdl:PCA_100006765 rdf:resource="http://w3id.org/readi/rdl/CFIHOS-20000010"/>
    <rdfs:label>ATEX ignition source mapping report</rdfs:label>
    <rdl:PCA_100006766>
      <rdl:PCA_100001503 rdf:about="http://rds.posccaesar.org/ontology/plm/rdl/PCA_100006634">
        <rdfs:label>Main power (u =or &gt;6.6 kV)</rdfs:label>
        <rdl:PCA_100004924>80</rdl:PCA_100004924>
        <rdf:type rdf:resource="http://www.w3.org/2002/07/owl#NamedIndividual"/>
      </rdl:PCA_100001503>
    </rdl:PCA_100006766>
    <rdl:PCA_100006766 rdf:resource="http://rds.posccaesar.org/ontology/plm/rdl/PCA_100006633"/>
    <skos:broadMatch>
      <rdl:PCA_100001503 rdf:about="http://rds.posccaesar.org/ontology/plm/rdl/PCA_100006716">
        <rdfs:label>objects listing</rdfs:label>
        <rdl:PCA_100004924>PB</rdl:PCA_100004924>
        <rdf:type rdf:resource="http://www.w3.org/2002/07/owl#NamedIndividual"/>
      </rdl:PCA_100001503>
    </skos:broadMatch>
    <skos:broader rdf:resource="http://rds.posccaesar.org/ontology/plm/rdl/PCA_100006756"/>
    <rdl:PCA_100006766 rdf:resource="http://rds.posccaesar.org/ontology/plm/rdl/PCA_100006632"/>
    <rdl:PCA_100006768>A complete list to identify of all potential ignition sources that could come into contact with explosive atmosphere and the likelihood of occurrence of the potential ignition source to become effective.  

Reference is made to EN 1127-1.</rdl:PCA_100006768>
    <rdl:PCA_100006766 rdf:resource="http://rds.posccaesar.org/ontology/plm/rdl/PCA_100006627"/>
    <rdl:PCA_100006766>
      <rdl:PCA_100001503 rdf:about="http://rds.posccaesar.org/ontology/plm/rdl/PCA_100006642">
        <rdfs:label>Earthing and lightning</rdfs:label>
        <rdl:PCA_100004924>88</rdl:PCA_100004924>
        <rdf:type rdf:resource="http://www.w3.org/2002/07/owl#NamedIndividual"/>
      </rdl:PCA_100001503>
    </rdl:PCA_100006766>
    <rdl:PCA_100006766 rdf:resource="http://rds.posccaesar.org/ontology/plm/rdl/PCA_100006631"/>
  </owl:Class>
  <owl:Class rdf:about="http://rds.posccaesar.org/ontology/plm/rdl/PCA_100006295">
    <rdfs:subClassOf rdf:resource="http://rds.posccaesar.org/ontology/plm/rdl/PCA_100004908"/>
    <rdl:PCA_100006766 rdf:resource="http://rds.posccaesar.org/ontology/plm/rdl/PCA_100006656"/>
    <rdl:PCA_100006768>A "Level measurement arrangement drawing" per vessel shall be issued, encompassing:
 - Dimensions;
 - Nozzles (including nozzles for pressure and temperature measurements);
 - Level glasses;
 - Location of measurement elements;
 - Calibration and measurement ranges;
 - Alarm levels;
 - Correlation between engineering units of measure (e.g. mm and %, with calculations);
 - ENS Tag number.</rdl:PCA_100006768>
    <rdfs:comment>A "Level measurement arrangement drawing" per vessel shall be issued, encompassing:
 - Dimensions;
 - Nozzles (including nozzles for pressure and temperature measurements);
 - Level glasses;
 - Location of measurement elements;
 - Calibration and measurement ranges;
 - Alarm levels;
 - Correlation between engineering units of measure (e.g. mm and %, with calculations);
 - ENS Tag number.</rdfs:comment>
    <rdl:PCA_100006763>For the purpose of documenting the engineering of level measurements, a "Level measurement arrangement drawing" per vessel shall be issued.</rdl:PCA_100006763>
    <rdfs:label>Level instrument arrangement drawings</rdfs:label>
    <skos:broadMatch>
      <rdl:PCA_100001503 rdf:about="http://rds.posccaesar.org/ontology/plm/rdl/PCA_100006710">
        <rdfs:label>in/on-equipment location information</rdfs:label>
        <rdl:PCA_100004924>LU</rdl:PCA_100004924>
        <rdf:type rdf:resource="http://www.w3.org/2002/07/owl#NamedIndividual"/>
      </rdl:PCA_100001503>
    </skos:broadMatch>
    <skos:broader>
      <rdl:PCA_100001503 rdf:about="http://rds.posccaesar.org/ontology/plm/rdl/PCA_100006739">
        <rdfs:label>Arrangement Drawing</rdfs:label>
        <rdl:PCA_100004924>AD</rdl:PCA_100004924>
        <rdf:type rdf:resource="http://www.w3.org/2002/07/owl#NamedIndividual"/>
      </rdl:PCA_100001503>
    </skos:broader>
    <rdl:PCA_100006765 rdf:resource="http://w3id.org/readi/rdl/CFIHOS-20000015"/>
  </owl:Class>
  <owl:Class rdf:about="http://rds.posccaesar.org/ontology/plm/rdl/PCA_100006283">
    <skos:broader rdf:resource="http://rds.posccaesar.org/ontology/plm/rdl/PCA_100006746"/>
    <skos:broadMatch>
      <rdl:PCA_100001503 rdf:about="http://rds.posccaesar.org/ontology/plm/rdl/PCA_100006709">
        <rdfs:label>in-construction entity location information</rdfs:label>
        <rdl:PCA_100004924>LH</rdl:PCA_100004924>
        <rdf:type rdf:resource="http://www.w3.org/2002/07/owl#NamedIndividual"/>
      </rdl:PCA_100001503>
    </skos:broadMatch>
    <rdfs:label>Instrument field equipment layout drawings</rdfs:label>
    <rdfs:comment>At least one field equipment layout drawing for each area or module deck level shall be produced.

The following content shall be included on the drawings:
 - Tagged field equipment including junction boxes and cabinets;
 - Sufficient main equipment on the drawing to easily identify the location of the field equipment;
 - Platform/plant northing and orientation with respect of true north;
 - Gridlines with north and east references;
 - Key plan;
 - Scale bar;
 - Match lines with drawing references;
 - Deck/area elevations.</rdfs:comment>
    <rdl:PCA_100006768>At least one field equipment layout drawing for each area or module deck level shall be produced.

The following content shall be included on the drawings:
 - Tagged field equipment including junction boxes and cabinets;
 - Sufficient main equipment on the drawing to easily identify the location of the field equipment;
 - Platform/plant northing and orientation with respect of true north;
 - Gridlines with north and east references;
 - Key plan;
 - Scale bar;
 - Match lines with drawing references;
 - Deck/area elevations.</rdl:PCA_100006768>
    <rdl:PCA_100006766 rdf:resource="http://rds.posccaesar.org/ontology/plm/rdl/PCA_100006656"/>
    <rdl:PCA_100006765 rdf:resource="http://w3id.org/readi/rdl/CFIHOS-20000015"/>
    <rdfs:subClassOf rdf:resource="http://rds.posccaesar.org/ontology/plm/rdl/PCA_100004908"/>
  </owl:Class>
  <owl:Class rdf:about="http://rds.posccaesar.org/ontology/plm/rdl/PCA_100006171">
    <rdfs:subClassOf rdf:resource="http://rds.posccaesar.org/ontology/plm/rdl/PCA_100004908"/>
    <rdfs:label>EFAT procedure</rdfs:label>
    <skos:broader rdf:resource="http://rds.posccaesar.org/ontology/plm/rdl/PCA_100006751"/>
    <rdl:PCA_100006765 rdf:resource="http://w3id.org/readi/rdl/CFIHOS-20000031"/>
    <skos:broadMatch>
      <rdl:PCA_100001503 rdf:about="http://rds.posccaesar.org/ontology/plm/rdl/PCA_100006688">
        <rdfs:label>instructive information</rdfs:label>
        <rdl:PCA_100004924>DC</rdl:PCA_100004924>
        <rdf:type rdf:resource="http://www.w3.org/2002/07/owl#NamedIndividual"/>
      </rdl:PCA_100001503>
    </skos:broadMatch>
    <rdl:PCA_100006766 rdf:resource="http://rds.posccaesar.org/ontology/plm/rdl/PCA_100006653"/>
    <rdl:PCA_100006763>Give clear instructions for testing of interfaces between different assemblies and equipment and to verify the sub-system performance and functionality.</rdl:PCA_100006763>
    <rdl:PCA_100006768>Extended factory acceptance test (EFAT) procedure contains detailed instructions and descriptions for test setup, methods, steps, activities and acceptance criteria for sub-systems. EFAT covers sub-system functionality and equipment interface testing.</rdl:PCA_100006768>
    <rdfs:comment>Extended factory acceptance test (EFAT) procedure contains detailed instructions and descriptions for test setup, methods, steps, activities and acceptance criteria for sub-systems. EFAT covers sub-system functionality and equipment interface testing.</rdfs:comment>
  </owl:Class>
  <owl:Class rdf:about="http://rds.posccaesar.org/ontology/plm/rdl/PCA_100006392">
    <rdfs:subClassOf rdf:resource="http://rds.posccaesar.org/ontology/plm/rdl/PCA_100004908"/>
    <rdfs:label>Process datasheet</rdfs:label>
    <rdl:PCA_100006763>No standardized description is presently available.</rdl:PCA_100006763>
    <rdl:PCA_100006765>
      <rdl:PCA_100001503 rdf:about="http://w3id.org/readi/rdl/CFIHOS-20000026">
        <rdfs:label>process engineering</rdfs:label>
        <rdl:PCA_100004924>PX</rdl:PCA_100004924>
        <rdf:type rdf:resource="http://www.w3.org/2002/07/owl#NamedIndividual"/>
      </rdl:PCA_100001503>
    </rdl:PCA_100006765>
    <skos:broadMatch rdf:resource="http://rds.posccaesar.org/ontology/plm/rdl/PCA_100006686"/>
    <skos:broader rdf:resource="http://rds.posccaesar.org/ontology/plm/rdl/PCA_100006747"/>
    <rdl:PCA_100006766 rdf:resource="http://rds.posccaesar.org/ontology/plm/rdl/PCA_100006653"/>
    <rdfs:comment>No standardized description is presently available.</rdfs:comment>
    <rdl:PCA_100006768>No standardized description is presently available.</rdl:PCA_100006768>
  </owl:Class>
  <owl:Class rdf:about="http://rds.posccaesar.org/ontology/plm/rdl/PCA_100006271">
    <rdl:PCA_100006765 rdf:resource="http://w3id.org/readi/rdl/CFIHOS-20000018"/>
    <rdl:PCA_100006766 rdf:resource="http://rds.posccaesar.org/ontology/plm/rdl/PCA_100006654"/>
    <rdfs:label>Inspection and maintenance philosophy for pipelines</rdfs:label>
    <skos:broadMatch rdf:resource="http://rds.posccaesar.org/ontology/plm/rdl/PCA_100006688"/>
    <rdl:PCA_100006768>The philosophy shall recommend follow up frequency and methods based on assumptions made during design and expected challenges and areas that require special focus.</rdl:PCA_100006768>
    <rdfs:comment>The philosophy shall recommend follow up frequency and methods based on assumptions made during design and expected challenges and areas that require special focus.</rdfs:comment>
    <rdfs:subClassOf rdf:resource="http://rds.posccaesar.org/ontology/plm/rdl/PCA_100004908"/>
    <rdl:PCA_100006763>The philosophy shall reccommend methods, technics and/or routines to reveal and prevent typical failures that can influence the integrity or the purpose of the pipeline, ref also Barrier matrix.</rdl:PCA_100006763>
    <skos:broader>
      <rdl:PCA_100001503 rdf:about="http://rds.posccaesar.org/ontology/plm/rdl/PCA_100006752">
        <rdfs:label>Philosophy</rdfs:label>
        <rdl:PCA_100004924>PH</rdl:PCA_100004924>
        <rdf:type rdf:resource="http://www.w3.org/2002/07/owl#NamedIndividual"/>
      </rdl:PCA_100001503>
    </skos:broader>
  </owl:Class>
  <owl:Class rdf:about="http://rds.posccaesar.org/ontology/plm/rdl/PCA_100006183">
    <skos:broadMatch>
      <rdl:PCA_100001503 rdf:about="http://rds.posccaesar.org/ontology/plm/rdl/PCA_100006729">
        <rdfs:label>security information</rdfs:label>
        <rdl:PCA_100004924>RD</rdl:PCA_100004924>
        <rdf:type rdf:resource="http://www.w3.org/2002/07/owl#NamedIndividual"/>
      </rdl:PCA_100001503>
    </skos:broadMatch>
    <rdfs:subClassOf rdf:resource="http://rds.posccaesar.org/ontology/plm/rdl/PCA_100004908"/>
    <rdl:PCA_100006766 rdf:resource="http://rds.posccaesar.org/ontology/plm/rdl/PCA_100006654"/>
    <rdl:PCA_100006763>The Emergency preparedness analysis report shall reflect the current operating conditions and experience and be written in a way to facilitate the use by the operating organization. See NORSOK Z-013 for further details.</rdl:PCA_100006763>
    <rdl:PCA_100006765 rdf:resource="http://w3id.org/readi/rdl/CFIHOS-20000010"/>
    <rdl:PCA_100006765 rdf:resource="http://w3id.org/readi/rdl/CFIHOS-20000013"/>
    <skos:broader rdf:resource="http://rds.posccaesar.org/ontology/plm/rdl/PCA_100006756"/>
    <rdl:PCA_100006765 rdf:resource="http://w3id.org/readi/rdl/CFIHOS-20000011"/>
    <rdfs:label>Emergency preparedness analysis</rdfs:label>
  </owl:Class>
  <owl:Class rdf:about="http://rds.posccaesar.org/ontology/plm/rdl/PCA_100006380">
    <skos:broader rdf:resource="http://rds.posccaesar.org/ontology/plm/rdl/PCA_100006746"/>
    <skos:broadMatch>
      <rdl:PCA_100001503 rdf:about="http://rds.posccaesar.org/ontology/plm/rdl/PCA_100006708">
        <rdfs:label>on-site location information</rdfs:label>
        <rdl:PCA_100004924>LD</rdl:PCA_100004924>
        <rdf:type rdf:resource="http://www.w3.org/2002/07/owl#NamedIndividual"/>
      </rdl:PCA_100001503>
    </skos:broadMatch>
    <rdfs:label>Plot plan drawings</rdfs:label>
    <rdfs:comment>These drawings are relevant for offshore facilities and for the process plant for onshore facilities.

One plot plan drawing for each area/deck level shall be produced. The plot plan drawing shall cover the entire process plant/deck area. The size of the facility will determine the scale of the drawing, but normally a scale of 1:500 on an A3 format shall be aimed for.

The following content shall be included on the drawings:
 - Plant/Platform Northing and orientation with respect of true north;
 - Gridlines with north and east references;
 - Scale bar;
 - Elevations of all decks/platforms;
 - Area segregation, with fire partitions indicated;
 - Safety evacuation equipment, such as escape tunnels, lifeboats (offshore), escape chutes (offshore), etc.;
 - MOB boat location (offshore);
 - Helideck location;
 - Location of cranes, with boom rests and maintenance platforms. Lifting capacity radiuses to be indicated;
 - Hose loading station and tote tank area (offshore);
 - Laydown areas;
 - Waste sorting stations;
 - Main pipe racks;
 - Main stairs, access and escape routes;
 - Main material handling routes;
 - Manifold area arrangement;
 - Wellhead area including well slots;
 - Drilling derrick extreme outlines indicated;
 - Location of temporary well intervention equipment;
 - Flare tower location and extreme outlines indicated;
 - HVAC, instrument and electrical rooms (offshore);
 - Control room (offshore);
 - Living Quarter (offshore);
 - Main structures;
 - Location of all major equipment as identified in MEL;
 - Main equipment shall be tagged according to MEL. An equipment index shall be included on the drawing;
 - Space allocation for risers, J-tubes and umbilicals including temporary equipment (pulling arrangement) (offshore);
 - Space for future modules/equipment.</rdfs:comment>
    <rdl:PCA_100006768>These drawings are relevant for offshore facilities and for the process plant for onshore facilities.

One plot plan drawing for each area/deck level shall be produced. The plot plan drawing shall cover the entire process plant/deck area. The size of the facility will determine the scale of the drawing, but normally a scale of 1:500 on an A3 format shall be aimed for.

The following content shall be included on the drawings:
 - Plant/Platform Northing and orientation with respect of true north;
 - Gridlines with north and east references;
 - Scale bar;
 - Elevations of all decks/platforms;
 - Area segregation, with fire partitions indicated;
 - Safety evacuation equipment, such as escape tunnels, lifeboats (offshore), escape chutes (offshore), etc.;
 - MOB boat location (offshore);
 - Helideck location;
 - Location of cranes, with boom rests and maintenance platforms. Lifting capacity radiuses to be indicated;
 - Hose loading station and tote tank area (offshore);
 - Laydown areas;
 - Waste sorting stations;
 - Main pipe racks;
 - Main stairs, access and escape routes;
 - Main material handling routes;
 - Manifold area arrangement;
 - Wellhead area including well slots;
 - Drilling derrick extreme outlines indicated;
 - Location of temporary well intervention equipment;
 - Flare tower location and extreme outlines indicated;
 - HVAC, instrument and electrical rooms (offshore);
 - Control room (offshore);
 - Living Quarter (offshore);
 - Main structures;
 - Location of all major equipment as identified in MEL;
 - Main equipment shall be tagged according to MEL. An equipment index shall be included on the drawing;
 - Space allocation for risers, J-tubes and umbilicals including temporary equipment (pulling arrangement) (offshore);
 - Space for future modules/equipment.</rdl:PCA_100006768>
    <rdl:PCA_100006766 rdf:resource="http://rds.posccaesar.org/ontology/plm/rdl/PCA_100006656"/>
    <rdl:PCA_100006765>
      <rdl:PCA_100001503 rdf:about="http://w3id.org/readi/rdl/CFIHOS-20000020">
        <rdfs:label>piping engineering</rdfs:label>
        <rdl:PCA_100004924>MP</rdl:PCA_100004924>
        <rdf:type rdf:resource="http://www.w3.org/2002/07/owl#NamedIndividual"/>
      </rdl:PCA_100001503>
    </rdl:PCA_100006765>
    <rdfs:subClassOf rdf:resource="http://rds.posccaesar.org/ontology/plm/rdl/PCA_100004908"/>
  </owl:Class>
  <owl:Class rdf:about="http://rds.posccaesar.org/ontology/plm/rdl/PCA_100006195">
    <skos:broader>
      <rdl:PCA_100001503 rdf:about="http://rds.posccaesar.org/ontology/plm/rdl/PCA_100006741">
        <rdfs:label>Calculation</rdfs:label>
        <rdl:PCA_100004924>CA</rdl:PCA_100004924>
        <rdf:type rdf:resource="http://www.w3.org/2002/07/owl#NamedIndividual"/>
      </rdl:PCA_100001503>
    </skos:broader>
    <skos:broadMatch rdf:resource="http://rds.posccaesar.org/ontology/plm/rdl/PCA_100006687"/>
    <rdl:PCA_100006768>Report documenting all calculations and analysis performed to show how pipeline is expected to expand during all conditions.</rdl:PCA_100006768>
    <rdfs:subClassOf rdf:resource="http://rds.posccaesar.org/ontology/plm/rdl/PCA_100004908"/>
    <rdl:PCA_100006763>To document the expected pipeline expansion and to demonstrate sufficient pipeline design.</rdl:PCA_100006763>
    <rdfs:label>Expansion analysis</rdfs:label>
    <rdl:PCA_100006766 rdf:resource="http://rds.posccaesar.org/ontology/plm/rdl/PCA_100006653"/>
    <rdl:PCA_100006765 rdf:resource="http://w3id.org/readi/rdl/CFIHOS-20000018"/>
    <rdfs:comment>Report documenting all calculations and analysis performed to show how pipeline is expected to expand during all conditions.</rdfs:comment>
  </owl:Class>
  <owl:Class rdf:about="http://rds.posccaesar.org/ontology/plm/rdl/PCA_100006086">
    <rdl:PCA_100006765 rdf:resource="http://w3id.org/readi/rdl/CFIHOS-20000015"/>
    <skos:broader rdf:resource="http://rds.posccaesar.org/ontology/plm/rdl/PCA_100006748"/>
    <rdl:PCA_100006766 rdf:resource="http://rds.posccaesar.org/ontology/plm/rdl/PCA_100006637"/>
    <rdl:PCA_100006766 rdf:resource="http://rds.posccaesar.org/ontology/plm/rdl/PCA_100006627"/>
    <rdl:PCA_100006766 rdf:resource="http://rds.posccaesar.org/ontology/plm/rdl/PCA_100006641"/>
    <rdl:PCA_100006766 rdf:resource="http://rds.posccaesar.org/ontology/plm/rdl/PCA_100006635"/>
    <rdl:PCA_100006766 rdf:resource="http://rds.posccaesar.org/ontology/plm/rdl/PCA_100006638"/>
    <rdl:PCA_100006766 rdf:resource="http://rds.posccaesar.org/ontology/plm/rdl/PCA_100006628"/>
    <rdl:PCA_100006763>A list containing necessary information for alarm handling such that it can be understood and handled in time for required safe operations of equipment.</rdl:PCA_100006763>
    <rdl:PCA_100006766 rdf:resource="http://rds.posccaesar.org/ontology/plm/rdl/PCA_100006633"/>
    <rdfs:subClassOf rdf:resource="http://rds.posccaesar.org/ontology/plm/rdl/PCA_100004908"/>
    <rdl:PCA_100006768>A list suggesting alarms and alarm priorities based on signals from equipment. Alarms shall be documented in accordance with IEC 62682 Ch 9 Rationalization.</rdl:PCA_100006768>
    <rdfs:comment>A list suggesting alarms and alarm priorities based on signals from equipment. Alarms shall be documented in accordance with IEC 62682 Ch 9 Rationalization.</rdfs:comment>
    <skos:broadMatch>
      <rdl:PCA_100001503 rdf:about="http://rds.posccaesar.org/ontology/plm/rdl/PCA_100006700">
        <rdfs:label>signal information</rdfs:label>
        <rdl:PCA_100004924>FP</rdl:PCA_100004924>
        <rdf:type rdf:resource="http://www.w3.org/2002/07/owl#NamedIndividual"/>
      </rdl:PCA_100001503>
    </skos:broadMatch>
    <rdl:PCA_100006766 rdf:resource="http://rds.posccaesar.org/ontology/plm/rdl/PCA_100006639"/>
    <rdl:PCA_100006766 rdf:resource="http://rds.posccaesar.org/ontology/plm/rdl/PCA_100006636"/>
    <rdl:PCA_100006765 rdf:resource="http://w3id.org/readi/rdl/CFIHOS-20000031"/>
    <rdl:PCA_100006766 rdf:resource="http://rds.posccaesar.org/ontology/plm/rdl/PCA_100006626"/>
    <rdl:PCA_100006766 rdf:resource="http://rds.posccaesar.org/ontology/plm/rdl/PCA_100006640"/>
    <rdl:PCA_100006766 rdf:resource="http://rds.posccaesar.org/ontology/plm/rdl/PCA_100006634"/>
    <rdfs:label>Alarm classification</rdfs:label>
  </owl:Class>
  <owl:Class rdf:about="http://rds.posccaesar.org/ontology/plm/rdl/PCA_100006098">
    <skos:broader rdf:resource="http://rds.posccaesar.org/ontology/plm/rdl/PCA_100006751"/>
    <rdl:PCA_100006766 rdf:resource="http://rds.posccaesar.org/ontology/plm/rdl/PCA_100006653"/>
    <skos:broadMatch rdf:resource="http://rds.posccaesar.org/ontology/plm/rdl/PCA_100006688"/>
    <rdl:PCA_100006768>Provide the assembly site with sufficient information to assemble the equipment correctly.</rdl:PCA_100006768>
    <rdfs:subClassOf rdf:resource="http://rds.posccaesar.org/ontology/plm/rdl/PCA_100004908"/>
    <rdl:PCA_100006764>The Assembly Procedure shall describe all actions, equipments and tools required to perform assembly of equipments including any lubricants or service materials.
This procedure shall include all HSE and safety precautions necessary to ensure safe operation.</rdl:PCA_100006764>
    <rdl:PCA_100006763>Procedure for assembly of individual components.</rdl:PCA_100006763>
    <rdfs:label>Assembly procedure</rdfs:label>
    <rdl:PCA_100006765 rdf:resource="http://w3id.org/readi/rdl/CFIHOS-20000031"/>
    <rdfs:comment>Provide the assembly site with sufficient information to assemble the equipment correctly.</rdfs:comment>
  </owl:Class>
  <owl:Class rdf:about="http://rds.posccaesar.org/ontology/plm/rdl/PCA_100006296">
    <skos:broader>
      <rdl:PCA_100001503 rdf:about="http://rds.posccaesar.org/ontology/plm/rdl/PCA_100006743">
        <rdfs:label>Certificate</rdfs:label>
        <rdl:PCA_100004924>CF</rdl:PCA_100004924>
        <rdf:type rdf:resource="http://www.w3.org/2002/07/owl#NamedIndividual"/>
      </rdl:PCA_100001503>
    </skos:broader>
    <skos:broadMatch rdf:resource="http://rds.posccaesar.org/ontology/plm/rdl/PCA_100006722"/>
    <rdfs:label>Lifting certificate</rdfs:label>
    <rdfs:comment>To confirm that the equipment can be safely used for lifting and handling for the applicable load stated.

VALVES
Content according to Norsok R-002, section F.7.8. (related to lifting points)</rdfs:comment>
    <rdl:PCA_100006768>To confirm that the equipment can be safely used for lifting and handling for the applicable load stated.

VALVES
Content according to Norsok R-002, section F.7.8. (related to lifting points)</rdl:PCA_100006768>
    <rdl:PCA_100006766 rdf:resource="http://rds.posccaesar.org/ontology/plm/rdl/PCA_100006653"/>
    <rdl:PCA_100006763>Certificate to prove that the item can be used as lifting gear in accordance with an applicable standard. This will include slings, shackles, lugs, lifting frames, lifting instructions etc.</rdl:PCA_100006763>
    <rdfs:subClassOf rdf:resource="http://rds.posccaesar.org/ontology/plm/rdl/PCA_100004908"/>
  </owl:Class>
  <owl:Class rdf:about="http://rds.posccaesar.org/ontology/plm/rdl/PCA_100006284">
    <rdl:PCA_100006765 rdf:resource="http://w3id.org/readi/rdl/CFIHOS-20000015"/>
    <rdfs:subClassOf rdf:resource="http://rds.posccaesar.org/ontology/plm/rdl/PCA_100004908"/>
    <rdl:PCA_100006763>The general earthing principles shall be included to ensure correct earthing of systems, equipment (cabinets, junction boxes and field devices) and cables.</rdl:PCA_100006763>
    <rdl:PCA_100006768>This diagram shall typically include:
 - Main equipment like system cabinets, termination cabinets, junction boxes and field devices;
 - Location of main equipment;
 - Signal type and function (typ. RS232, control signal) if applicable;
 - Typical interface, wiring and termination details from system cabinets and main earth bars to field devices;
 - Main earth bars for instrument and telecommunications;
 - Earthing electrodes;
 - Identification of PE bars and IE bars;
 - Identification of cable armour and screen.</rdl:PCA_100006768>
    <skos:broader>
      <rdl:PCA_100001503 rdf:about="http://rds.posccaesar.org/ontology/plm/rdl/PCA_100006745">
        <rdfs:label>Diagram</rdfs:label>
        <rdl:PCA_100004924>DI</rdl:PCA_100004924>
        <rdf:type rdf:resource="http://www.w3.org/2002/07/owl#NamedIndividual"/>
      </rdl:PCA_100001503>
    </skos:broader>
    <rdfs:comment>This diagram shall typically include:
 - Main equipment like system cabinets, termination cabinets, junction boxes and field devices;
 - Location of main equipment;
 - Signal type and function (typ. RS232, control signal) if applicable;
 - Typical interface, wiring and termination details from system cabinets and main earth bars to field devices;
 - Main earth bars for instrument and telecommunications;
 - Earthing electrodes;
 - Identification of PE bars and IE bars;
 - Identification of cable armour and screen.</rdfs:comment>
    <rdfs:label>Instrument/telecom. earthing distribution. schematic diagram</rdfs:label>
    <skos:broadMatch>
      <rdl:PCA_100001503 rdf:about="http://rds.posccaesar.org/ontology/plm/rdl/PCA_100006712">
        <rdfs:label>termination information</rdfs:label>
        <rdl:PCA_100004924>MA</rdl:PCA_100004924>
        <rdf:type rdf:resource="http://www.w3.org/2002/07/owl#NamedIndividual"/>
      </rdl:PCA_100001503>
    </skos:broadMatch>
    <rdl:PCA_100006766 rdf:resource="http://rds.posccaesar.org/ontology/plm/rdl/PCA_100006640"/>
    <skos:broadMatch>
      <rdl:PCA_100001503 rdf:about="http://rds.posccaesar.org/ontology/plm/rdl/PCA_100006702">
        <rdfs:label>circuitry information</rdfs:label>
        <rdl:PCA_100004924>FS</rdl:PCA_100004924>
        <rdf:type rdf:resource="http://www.w3.org/2002/07/owl#NamedIndividual"/>
      </rdl:PCA_100001503>
    </skos:broadMatch>
  </owl:Class>
  <owl:Class rdf:about="http://rds.posccaesar.org/ontology/plm/rdl/PCA_100006272">
    <rdfs:comment>The document shall take into consideration the experience from the actual design and manufacturing of the flexible pipe and ancillary components not limited to addressing non-conformances and critical design issues.</rdfs:comment>
    <skos:broadMatch rdf:resource="http://rds.posccaesar.org/ontology/plm/rdl/PCA_100006688"/>
    <rdfs:subClassOf rdf:resource="http://rds.posccaesar.org/ontology/plm/rdl/PCA_100004908"/>
    <rdl:PCA_100006768>The document shall take into consideration the experience from the actual design and manufacturing of the flexible pipe and ancillary components not limited to addressing non-conformances and critical design issues.</rdl:PCA_100006768>
    <skos:broader>
      <rdl:PCA_100001503 rdf:about="http://rds.posccaesar.org/ontology/plm/rdl/PCA_100006750">
        <rdfs:label>Operational information</rdfs:label>
        <rdl:PCA_100004924>OI</rdl:PCA_100004924>
        <rdf:type rdf:resource="http://www.w3.org/2002/07/owl#NamedIndividual"/>
      </rdl:PCA_100001503>
    </skos:broader>
    <rdl:PCA_100006765 rdf:resource="http://w3id.org/readi/rdl/CFIHOS-20000018"/>
    <rdfs:label>Inspection and monitoring program flexible pipeline and riser</rdfs:label>
    <rdl:PCA_100006766 rdf:resource="http://rds.posccaesar.org/ontology/plm/rdl/PCA_100006654"/>
    <rdl:PCA_100006763>A document with recommended inspection and monitoring program addressing the items in Section 11 of API 17B and integrity management for ancillary components addressed in API 17L2 Recommended practice for flexible pipe ancillary equipment. The inspection and monitoring program minimum requirements shall be in accordance with Sections 11.2 and 11.5 of API 17B.</rdl:PCA_100006763>
  </owl:Class>
  <owl:Class rdf:about="http://rds.posccaesar.org/ontology/plm/rdl/PCA_100006170">
    <rdl:PCA_100006763>To determine maximum sea state for installation of equipment.</rdl:PCA_100006763>
    <rdfs:comment>Report documenting all calculations and analysis performed for dynamic installation load cases.</rdfs:comment>
    <skos:broadMatch rdf:resource="http://rds.posccaesar.org/ontology/plm/rdl/PCA_100006687"/>
    <rdl:PCA_100006765 rdf:resource="http://w3id.org/readi/rdl/CFIHOS-20000031"/>
    <rdfs:subClassOf rdf:resource="http://rds.posccaesar.org/ontology/plm/rdl/PCA_100004908"/>
    <rdfs:label>Dynamic (installation) load case analysis</rdfs:label>
    <skos:broader rdf:resource="http://rds.posccaesar.org/ontology/plm/rdl/PCA_100006741"/>
    <rdl:PCA_100006766 rdf:resource="http://rds.posccaesar.org/ontology/plm/rdl/PCA_100006653"/>
    <rdl:PCA_100006768>Report documenting all calculations and analysis performed for dynamic installation load cases.</rdl:PCA_100006768>
  </owl:Class>
  <owl:Class rdf:about="http://rds.posccaesar.org/ontology/plm/rdl/PCA_100006393">
    <rdl:PCA_100006766>
      <rdl:PCA_100001503 rdf:about="http://rds.posccaesar.org/ontology/plm/rdl/PCA_100006581">
        <rdfs:label>Riser and well topside</rdfs:label>
        <rdl:PCA_100004924>13</rdl:PCA_100004924>
        <rdf:type rdf:resource="http://www.w3.org/2002/07/owl#NamedIndividual"/>
      </rdl:PCA_100001503>
    </rdl:PCA_100006766>
    <rdl:PCA_100006766>
      <rdl:PCA_100001503 rdf:about="http://rds.posccaesar.org/ontology/plm/rdl/PCA_100006622">
        <rdfs:label>Inert gas</rdfs:label>
        <rdl:PCA_100004924>64</rdl:PCA_100004924>
        <rdf:type rdf:resource="http://www.w3.org/2002/07/owl#NamedIndividual"/>
      </rdl:PCA_100001503>
    </rdl:PCA_100006766>
    <rdl:PCA_100006766>
      <rdl:PCA_100001503 rdf:about="http://rds.posccaesar.org/ontology/plm/rdl/PCA_100006598">
        <rdfs:label>Injection water pipeline</rdfs:label>
        <rdl:PCA_100004924>34</rdl:PCA_100004924>
        <rdf:type rdf:resource="http://www.w3.org/2002/07/owl#NamedIndividual"/>
      </rdl:PCA_100001503>
    </rdl:PCA_100006766>
    <rdl:PCA_100006766>
      <rdl:PCA_100001503 rdf:about="http://rds.posccaesar.org/ontology/plm/rdl/PCA_100006606">
        <rdfs:label>Chemical injection</rdfs:label>
        <rdl:PCA_100004924>42</rdl:PCA_100004924>
        <rdf:type rdf:resource="http://www.w3.org/2002/07/owl#NamedIndividual"/>
      </rdl:PCA_100001503>
    </rdl:PCA_100006766>
    <rdl:PCA_100006766>
      <rdl:PCA_100001503 rdf:about="http://rds.posccaesar.org/ontology/plm/rdl/PCA_100006597">
        <rdfs:label>Oil storage</rdfs:label>
        <rdl:PCA_100004924>33</rdl:PCA_100004924>
        <rdf:type rdf:resource="http://www.w3.org/2002/07/owl#NamedIndividual"/>
      </rdl:PCA_100001503>
    </rdl:PCA_100006766>
    <rdl:PCA_100006766>
      <rdl:PCA_100001503 rdf:about="http://rds.posccaesar.org/ontology/plm/rdl/PCA_100006605">
        <rdfs:label>Heating medium</rdfs:label>
        <rdl:PCA_100004924>41</rdl:PCA_100004924>
        <rdf:type rdf:resource="http://www.w3.org/2002/07/owl#NamedIndividual"/>
      </rdl:PCA_100001503>
    </rdl:PCA_100006766>
    <rdl:PCA_100006766>
      <rdl:PCA_100001503 rdf:about="http://rds.posccaesar.org/ontology/plm/rdl/PCA_100006594">
        <rdfs:label>Oil export line</rdfs:label>
        <rdl:PCA_100004924>30</rdl:PCA_100004924>
        <rdf:type rdf:resource="http://www.w3.org/2002/07/owl#NamedIndividual"/>
      </rdl:PCA_100001503>
    </rdl:PCA_100006766>
    <rdl:PCA_100006766>
      <rdl:PCA_100001503 rdf:about="http://rds.posccaesar.org/ontology/plm/rdl/PCA_100006593">
        <rdfs:label>Water injection</rdfs:label>
        <rdl:PCA_100004924>29</rdl:PCA_100004924>
        <rdf:type rdf:resource="http://www.w3.org/2002/07/owl#NamedIndividual"/>
      </rdl:PCA_100001503>
    </rdl:PCA_100006766>
    <rdl:PCA_100006766>
      <rdl:PCA_100001503 rdf:about="http://rds.posccaesar.org/ontology/plm/rdl/PCA_100006601">
        <rdfs:label>Gas injection pipeline</rdfs:label>
        <rdl:PCA_100004924>37</rdl:PCA_100004924>
        <rdf:type rdf:resource="http://www.w3.org/2002/07/owl#NamedIndividual"/>
      </rdl:PCA_100001503>
    </rdl:PCA_100006766>
    <rdl:PCA_100006766>
      <rdl:PCA_100001503 rdf:about="http://rds.posccaesar.org/ontology/plm/rdl/PCA_100006618">
        <rdfs:label>Thruster and propulsion</rdfs:label>
        <rdl:PCA_100004924>58</rdl:PCA_100004924>
        <rdf:type rdf:resource="http://www.w3.org/2002/07/owl#NamedIndividual"/>
      </rdl:PCA_100001503>
    </rdl:PCA_100006766>
    <rdl:PCA_100006766>
      <rdl:PCA_100001503 rdf:about="http://rds.posccaesar.org/ontology/plm/rdl/PCA_100006580">
        <rdfs:label>Drilling well control</rdfs:label>
        <rdl:PCA_100004924>12</rdl:PCA_100004924>
        <rdf:type rdf:resource="http://www.w3.org/2002/07/owl#NamedIndividual"/>
      </rdl:PCA_100001503>
    </rdl:PCA_100006766>
    <rdl:PCA_100006766>
      <rdl:PCA_100001503 rdf:about="http://rds.posccaesar.org/ontology/plm/rdl/PCA_100006621">
        <rdfs:label>Compressed air</rdfs:label>
        <rdl:PCA_100004924>63</rdl:PCA_100004924>
        <rdf:type rdf:resource="http://www.w3.org/2002/07/owl#NamedIndividual"/>
      </rdl:PCA_100001503>
    </rdl:PCA_100006766>
    <skos:broadMatch>
      <rdl:PCA_100001503 rdf:about="http://rds.posccaesar.org/ontology/plm/rdl/PCA_100006696">
        <rdfs:label>flow information</rdfs:label>
        <rdl:PCA_100004924>FB</rdl:PCA_100004924>
        <rdf:type rdf:resource="http://www.w3.org/2002/07/owl#NamedIndividual"/>
      </rdl:PCA_100001503>
    </skos:broadMatch>
    <rdl:PCA_100006766>
      <rdl:PCA_100001503 rdf:about="http://rds.posccaesar.org/ontology/plm/rdl/PCA_100006608">
        <rdfs:label>Oily water</rdfs:label>
        <rdl:PCA_100004924>44</rdl:PCA_100004924>
        <rdf:type rdf:resource="http://www.w3.org/2002/07/owl#NamedIndividual"/>
      </rdl:PCA_100001503>
    </rdl:PCA_100006766>
    <rdl:PCA_100006766>
      <rdl:PCA_100001503 rdf:about="http://rds.posccaesar.org/ontology/plm/rdl/PCA_100006607">
        <rdfs:label>Flare</rdfs:label>
        <rdl:PCA_100004924>43</rdl:PCA_100004924>
        <rdf:type rdf:resource="http://www.w3.org/2002/07/owl#NamedIndividual"/>
      </rdl:PCA_100001503>
    </rdl:PCA_100006766>
    <rdl:PCA_100006766>
      <rdl:PCA_100001503 rdf:about="http://rds.posccaesar.org/ontology/plm/rdl/PCA_100006586">
        <rdfs:label>Separation and stabilisation</rdfs:label>
        <rdl:PCA_100004924>20</rdl:PCA_100004924>
        <rdf:type rdf:resource="http://www.w3.org/2002/07/owl#NamedIndividual"/>
      </rdl:PCA_100001503>
    </rdl:PCA_100006766>
    <rdl:PCA_100006766 rdf:resource="http://rds.posccaesar.org/ontology/plm/rdl/PCA_100006628"/>
    <rdl:PCA_100006766 rdf:resource="http://rds.posccaesar.org/ontology/plm/rdl/PCA_100006627"/>
    <rdl:PCA_100006766>
      <rdl:PCA_100001503 rdf:about="http://rds.posccaesar.org/ontology/plm/rdl/PCA_100006582">
        <rdfs:label>Drilling control and monitoring</rdfs:label>
        <rdl:PCA_100004924>14</rdl:PCA_100004924>
        <rdf:type rdf:resource="http://www.w3.org/2002/07/owl#NamedIndividual"/>
      </rdl:PCA_100001503>
    </rdl:PCA_100006766>
    <rdl:PCA_100006766>
      <rdl:PCA_100001503 rdf:about="http://rds.posccaesar.org/ontology/plm/rdl/PCA_100006623">
        <rdfs:label>Hydraulic power</rdfs:label>
        <rdl:PCA_100004924>65</rdl:PCA_100004924>
        <rdf:type rdf:resource="http://www.w3.org/2002/07/owl#NamedIndividual"/>
      </rdl:PCA_100001503>
    </rdl:PCA_100006766>
    <rdl:PCA_100006766>
      <rdl:PCA_100001503 rdf:about="http://rds.posccaesar.org/ontology/plm/rdl/PCA_100006602">
        <rdfs:label>Glycol / methanol regeneration</rdfs:label>
        <rdl:PCA_100004924>38</rdl:PCA_100004924>
        <rdf:type rdf:resource="http://www.w3.org/2002/07/owl#NamedIndividual"/>
      </rdl:PCA_100001503>
    </rdl:PCA_100006766>
    <rdl:PCA_100006766>
      <rdl:PCA_100001503 rdf:about="http://rds.posccaesar.org/ontology/plm/rdl/PCA_100006579">
        <rdfs:label>Drilling process</rdfs:label>
        <rdl:PCA_100004924>11</rdl:PCA_100004924>
        <rdf:type rdf:resource="http://www.w3.org/2002/07/owl#NamedIndividual"/>
      </rdl:PCA_100001503>
    </rdl:PCA_100006766>
    <rdl:PCA_100006766>
      <rdl:PCA_100001503 rdf:about="http://rds.posccaesar.org/ontology/plm/rdl/PCA_100006615">
        <rdfs:label>Steam</rdfs:label>
        <rdl:PCA_100004924>55</rdl:PCA_100004924>
        <rdf:type rdf:resource="http://www.w3.org/2002/07/owl#NamedIndividual"/>
      </rdl:PCA_100001503>
    </rdl:PCA_100006766>
    <rdl:PCA_100006766>
      <rdl:PCA_100001503 rdf:about="http://rds.posccaesar.org/ontology/plm/rdl/PCA_100006587">
        <rdfs:label>Crude handling and metering</rdfs:label>
        <rdl:PCA_100004924>21</rdl:PCA_100004924>
        <rdf:type rdf:resource="http://www.w3.org/2002/07/owl#NamedIndividual"/>
      </rdl:PCA_100001503>
    </rdl:PCA_100006766>
    <rdl:PCA_100006766>
      <rdl:PCA_100001503 rdf:about="http://rds.posccaesar.org/ontology/plm/rdl/PCA_100006614">
        <rdfs:label>Fresh water</rdfs:label>
        <rdl:PCA_100004924>53</rdl:PCA_100004924>
        <rdf:type rdf:resource="http://www.w3.org/2002/07/owl#NamedIndividual"/>
      </rdl:PCA_100001503>
    </rdl:PCA_100006766>
    <rdl:PCA_100006766>
      <rdl:PCA_100001503 rdf:about="http://rds.posccaesar.org/ontology/plm/rdl/PCA_100006583">
        <rdfs:label>Drilling drain</rdfs:label>
        <rdl:PCA_100004924>15</rdl:PCA_100004924>
        <rdf:type rdf:resource="http://www.w3.org/2002/07/owl#NamedIndividual"/>
      </rdl:PCA_100001503>
    </rdl:PCA_100006766>
    <rdl:PCA_100006766>
      <rdl:PCA_100001503 rdf:about="http://rds.posccaesar.org/ontology/plm/rdl/PCA_100006611">
        <rdfs:label>Chlorination</rdfs:label>
        <rdl:PCA_100004924>47</rdl:PCA_100004924>
        <rdf:type rdf:resource="http://www.w3.org/2002/07/owl#NamedIndividual"/>
      </rdl:PCA_100001503>
    </rdl:PCA_100006766>
    <skos:broader rdf:resource="http://rds.posccaesar.org/ontology/plm/rdl/PCA_100006745"/>
    <rdl:PCA_100006766>
      <rdl:PCA_100001503 rdf:about="http://rds.posccaesar.org/ontology/plm/rdl/PCA_100006610">
        <rdfs:label>Methanol injection</rdfs:label>
        <rdl:PCA_100004924>46</rdl:PCA_100004924>
        <rdf:type rdf:resource="http://www.w3.org/2002/07/owl#NamedIndividual"/>
      </rdl:PCA_100001503>
    </rdl:PCA_100006766>
    <rdl:PCA_100006766>
      <rdl:PCA_100001503 rdf:about="http://rds.posccaesar.org/ontology/plm/rdl/PCA_100006624">
        <rdfs:label>Sewage treatment</rdfs:label>
        <rdl:PCA_100004924>66</rdl:PCA_100004924>
        <rdf:type rdf:resource="http://www.w3.org/2002/07/owl#NamedIndividual"/>
      </rdl:PCA_100001503>
    </rdl:PCA_100006766>
    <rdl:PCA_100006766>
      <rdl:PCA_100001503 rdf:about="http://rds.posccaesar.org/ontology/plm/rdl/PCA_100006599">
        <rdfs:label>Chemical injection pipeline</rdfs:label>
        <rdl:PCA_100004924>35</rdl:PCA_100004924>
        <rdf:type rdf:resource="http://www.w3.org/2002/07/owl#NamedIndividual"/>
      </rdl:PCA_100001503>
    </rdl:PCA_100006766>
    <rdl:PCA_100006765 rdf:resource="http://w3id.org/readi/rdl/CFIHOS-20000026"/>
    <rdl:PCA_100006766>
      <rdl:PCA_100001503 rdf:about="http://rds.posccaesar.org/ontology/plm/rdl/PCA_100006596">
        <rdfs:label>Gas export pipeline</rdfs:label>
        <rdl:PCA_100004924>32</rdl:PCA_100004924>
        <rdf:type rdf:resource="http://www.w3.org/2002/07/owl#NamedIndividual"/>
      </rdl:PCA_100001503>
    </rdl:PCA_100006766>
    <rdl:PCA_100006766>
      <rdl:PCA_100001503 rdf:about="http://rds.posccaesar.org/ontology/plm/rdl/PCA_100006595">
        <rdfs:label>Condensate export line</rdfs:label>
        <rdl:PCA_100004924>31</rdl:PCA_100004924>
        <rdf:type rdf:resource="http://www.w3.org/2002/07/owl#NamedIndividual"/>
      </rdl:PCA_100001503>
    </rdl:PCA_100006766>
    <rdl:PCA_100006766>
      <rdl:PCA_100001503 rdf:about="http://rds.posccaesar.org/ontology/plm/rdl/PCA_100006590">
        <rdfs:label>Gas conditioning</rdfs:label>
        <rdl:PCA_100004924>25</rdl:PCA_100004924>
        <rdf:type rdf:resource="http://www.w3.org/2002/07/owl#NamedIndividual"/>
      </rdl:PCA_100001503>
    </rdl:PCA_100006766>
    <rdfs:label>Process flow diagrams (PFD)</rdfs:label>
    <rdl:PCA_100006766>
      <rdl:PCA_100001503 rdf:about="http://rds.posccaesar.org/ontology/plm/rdl/PCA_100006589">
        <rdfs:label>Gas treatment</rdfs:label>
        <rdl:PCA_100004924>24</rdl:PCA_100004924>
        <rdf:type rdf:resource="http://www.w3.org/2002/07/owl#NamedIndividual"/>
      </rdl:PCA_100001503>
    </rdl:PCA_100006766>
    <rdl:PCA_100006766>
      <rdl:PCA_100001503 rdf:about="http://rds.posccaesar.org/ontology/plm/rdl/PCA_100006609">
        <rdfs:label>Fuel gas</rdfs:label>
        <rdl:PCA_100004924>45</rdl:PCA_100004924>
        <rdf:type rdf:resource="http://www.w3.org/2002/07/owl#NamedIndividual"/>
      </rdl:PCA_100001503>
    </rdl:PCA_100006766>
    <rdl:PCA_100006766>
      <rdl:PCA_100001503 rdf:about="http://rds.posccaesar.org/ontology/plm/rdl/PCA_100006603">
        <rdfs:label>Loading</rdfs:label>
        <rdl:PCA_100004924>39</rdl:PCA_100004924>
        <rdf:type rdf:resource="http://www.w3.org/2002/07/owl#NamedIndividual"/>
      </rdl:PCA_100001503>
    </rdl:PCA_100006766>
    <rdl:PCA_100006765 rdf:resource="http://w3id.org/readi/rdl/CFIHOS-20000031"/>
    <rdl:PCA_100006763>The symbols used for the PFDs shall be explained by a legend which shall be a part of the total PFD set. The PFDs shall use the coding and numbering standard in ENS, and the plant legend and drawing standard in accordance with NORSOK Z-005.

Norsok S-001 "Technical safety"</rdl:PCA_100006763>
    <rdl:PCA_100006766>
      <rdl:PCA_100001503 rdf:about="http://rds.posccaesar.org/ontology/plm/rdl/PCA_100006588">
        <rdfs:label>Gas compression and re-injection</rdfs:label>
        <rdl:PCA_100004924>23</rdl:PCA_100004924>
        <rdf:type rdf:resource="http://www.w3.org/2002/07/owl#NamedIndividual"/>
      </rdl:PCA_100001503>
    </rdl:PCA_100006766>
    <rdl:PCA_100006768>PFDs shall be prepared for drilling systems, main process (production, injection and export) systems, process support and utility systems and safety systems, including subsea parts of the systems (if any). For systems with significantly different operating modes/phases, separate PFDs shall be prepared for each mode/phase. 

Process equipment shall be shown schematically on the PFDs with equipment tag numbers and operating pressure and temperature. Equipment name, sparing (for parallel equipment) and main equipment operating/characteristic data (e.g. operating duty for a compressor) shall be included. 
 
Process streams to/from the process equipment essential for understanding the operating principle and the heat and material balance shall be included on the PFDs with a stream number. Stream data describing the process fluid flow shall be included in a table on the PFD or on a separate drawing/sheet referred from the PFD. 
 
Control loops shall be shown schematically on the PFDs, including utility streams where these are a part of the control loops.</rdl:PCA_100006768>
    <rdl:PCA_100006766>
      <rdl:PCA_100001503 rdf:about="http://rds.posccaesar.org/ontology/plm/rdl/PCA_100006584">
        <rdfs:label>Well and riser subsea</rdfs:label>
        <rdl:PCA_100004924>18</rdl:PCA_100004924>
        <rdf:type rdf:resource="http://www.w3.org/2002/07/owl#NamedIndividual"/>
      </rdl:PCA_100001503>
    </rdl:PCA_100006766>
    <rdl:PCA_100006766>
      <rdl:PCA_100001503 rdf:about="http://rds.posccaesar.org/ontology/plm/rdl/PCA_100006625">
        <rdfs:label>Lubrication oil</rdfs:label>
        <rdl:PCA_100004924>69</rdl:PCA_100004924>
        <rdf:type rdf:resource="http://www.w3.org/2002/07/owl#NamedIndividual"/>
      </rdl:PCA_100001503>
    </rdl:PCA_100006766>
    <rdl:PCA_100006766>
      <rdl:PCA_100001503 rdf:about="http://rds.posccaesar.org/ontology/plm/rdl/PCA_100006604">
        <rdfs:label>Cooling medium</rdfs:label>
        <rdl:PCA_100004924>40</rdl:PCA_100004924>
        <rdf:type rdf:resource="http://www.w3.org/2002/07/owl#NamedIndividual"/>
      </rdl:PCA_100001503>
    </rdl:PCA_100006766>
    <rdl:PCA_100006766>
      <rdl:PCA_100001503 rdf:about="http://rds.posccaesar.org/ontology/plm/rdl/PCA_100006600">
        <rdfs:label>Wellstream pipeline</rdfs:label>
        <rdl:PCA_100004924>36</rdl:PCA_100004924>
        <rdf:type rdf:resource="http://www.w3.org/2002/07/owl#NamedIndividual"/>
      </rdl:PCA_100001503>
    </rdl:PCA_100006766>
    <rdl:PCA_100006766>
      <rdl:PCA_100001503 rdf:about="http://rds.posccaesar.org/ontology/plm/rdl/PCA_100006617">
        <rdfs:label>Closed drain</rdfs:label>
        <rdl:PCA_100004924>57</rdl:PCA_100004924>
        <rdf:type rdf:resource="http://www.w3.org/2002/07/owl#NamedIndividual"/>
      </rdl:PCA_100001503>
    </rdl:PCA_100006766>
    <rdl:PCA_100006766>
      <rdl:PCA_100001503 rdf:about="http://rds.posccaesar.org/ontology/plm/rdl/PCA_100006616">
        <rdfs:label>Open drain</rdfs:label>
        <rdl:PCA_100004924>56</rdl:PCA_100004924>
        <rdf:type rdf:resource="http://www.w3.org/2002/07/owl#NamedIndividual"/>
      </rdl:PCA_100001503>
    </rdl:PCA_100006766>
    <rdl:PCA_100006766>
      <rdl:PCA_100001503 rdf:about="http://rds.posccaesar.org/ontology/plm/rdl/PCA_100006613">
        <rdfs:label>Ballast water</rdfs:label>
        <rdl:PCA_100004924>52</rdl:PCA_100004924>
        <rdf:type rdf:resource="http://www.w3.org/2002/07/owl#NamedIndividual"/>
      </rdl:PCA_100001503>
    </rdl:PCA_100006766>
    <rdl:PCA_100006766>
      <rdl:PCA_100001503 rdf:about="http://rds.posccaesar.org/ontology/plm/rdl/PCA_100006612">
        <rdfs:label>Sea water</rdfs:label>
        <rdl:PCA_100004924>50</rdl:PCA_100004924>
        <rdf:type rdf:resource="http://www.w3.org/2002/07/owl#NamedIndividual"/>
      </rdl:PCA_100001503>
    </rdl:PCA_100006766>
    <rdl:PCA_100006766>
      <rdl:PCA_100001503 rdf:about="http://rds.posccaesar.org/ontology/plm/rdl/PCA_100006620">
        <rdfs:label>Diesel oil</rdfs:label>
        <rdl:PCA_100004924>62</rdl:PCA_100004924>
        <rdf:type rdf:resource="http://www.w3.org/2002/07/owl#NamedIndividual"/>
      </rdl:PCA_100001503>
    </rdl:PCA_100006766>
    <rdfs:comment>PFDs shall be prepared for drilling systems, main process (production, injection and export) systems, process support and utility systems and safety systems, including subsea parts of the systems (if any). For systems with significantly different operating modes/phases, separate PFDs shall be prepared for each mode/phase. 

Process equipment shall be shown schematically on the PFDs with equipment tag numbers and operating pressure and temperature. Equipment name, sparing (for parallel equipment) and main equipment operating/characteristic data (e.g. operating duty for a compressor) shall be included. 
 
Process streams to/from the process equipment essential for understanding the operating principle and the heat and material balance shall be included on the PFDs with a stream number. Stream data describing the process fluid flow shall be included in a table on the PFD or on a separate drawing/sheet referred from the PFD. 
 
Control loops shall be shown schematically on the PFDs, including utility streams where these are a part of the control loops.</rdfs:comment>
    <rdl:PCA_100006766>
      <rdl:PCA_100001503 rdf:about="http://rds.posccaesar.org/ontology/plm/rdl/PCA_100006592">
        <rdfs:label>Gas sweetening</rdfs:label>
        <rdl:PCA_100004924>28</rdl:PCA_100004924>
        <rdf:type rdf:resource="http://www.w3.org/2002/07/owl#NamedIndividual"/>
      </rdl:PCA_100001503>
    </rdl:PCA_100006766>
    <rdl:PCA_100006766>
      <rdl:PCA_100001503 rdf:about="http://rds.posccaesar.org/ontology/plm/rdl/PCA_100006591">
        <rdfs:label>Gas export and metering</rdfs:label>
        <rdl:PCA_100004924>27</rdl:PCA_100004924>
        <rdf:type rdf:resource="http://www.w3.org/2002/07/owl#NamedIndividual"/>
      </rdl:PCA_100001503>
    </rdl:PCA_100006766>
    <rdfs:subClassOf rdf:resource="http://rds.posccaesar.org/ontology/plm/rdl/PCA_100004908"/>
    <rdl:PCA_100006766>
      <rdl:PCA_100001503 rdf:about="http://rds.posccaesar.org/ontology/plm/rdl/PCA_100006578">
        <rdfs:label>Drilling</rdfs:label>
        <rdl:PCA_100004924>10</rdl:PCA_100004924>
        <rdf:type rdf:resource="http://www.w3.org/2002/07/owl#NamedIndividual"/>
      </rdl:PCA_100001503>
    </rdl:PCA_100006766>
    <rdl:PCA_100006766>
      <rdl:PCA_100001503 rdf:about="http://rds.posccaesar.org/ontology/plm/rdl/PCA_100006619">
        <rdfs:label>Jet fuel</rdfs:label>
        <rdl:PCA_100004924>61</rdl:PCA_100004924>
        <rdf:type rdf:resource="http://www.w3.org/2002/07/owl#NamedIndividual"/>
      </rdl:PCA_100001503>
    </rdl:PCA_100006766>
    <rdl:PCA_100006766>
      <rdl:PCA_100001503 rdf:about="http://rds.posccaesar.org/ontology/plm/rdl/PCA_100006585">
        <rdfs:label>Subsea installation - maintenance and work over</rdfs:label>
        <rdl:PCA_100004924>19</rdl:PCA_100004924>
        <rdf:type rdf:resource="http://www.w3.org/2002/07/owl#NamedIndividual"/>
      </rdl:PCA_100001503>
    </rdl:PCA_100006766>
  </owl:Class>
  <owl:Class rdf:about="http://rds.posccaesar.org/ontology/plm/rdl/PCA_100006381">
    <rdl:PCA_100006765 rdf:resource="http://w3id.org/readi/rdl/CFIHOS-20000031"/>
    <rdl:PCA_100006768>Document containing records of material identification by chemical analysis.</rdl:PCA_100006768>
    <rdfs:label>PMI reports</rdfs:label>
    <rdfs:comment>Document containing records of material identification by chemical analysis.</rdfs:comment>
    <skos:broader rdf:resource="http://rds.posccaesar.org/ontology/plm/rdl/PCA_100006756"/>
    <skos:broadMatch rdf:resource="http://rds.posccaesar.org/ontology/plm/rdl/PCA_100006722"/>
    <rdl:PCA_100006766 rdf:resource="http://rds.posccaesar.org/ontology/plm/rdl/PCA_100006653"/>
    <rdfs:subClassOf rdf:resource="http://rds.posccaesar.org/ontology/plm/rdl/PCA_100004908"/>
    <rdl:PCA_100006763>Document use of correct material.</rdl:PCA_100006763>
  </owl:Class>
  <owl:Class rdf:about="http://rds.posccaesar.org/ontology/plm/rdl/PCA_100006260">
    <skos:broader rdf:resource="http://rds.posccaesar.org/ontology/plm/rdl/PCA_100006745"/>
    <skos:broadMatch rdf:resource="http://rds.posccaesar.org/ontology/plm/rdl/PCA_100006712"/>
    <skos:broadMatch rdf:resource="http://rds.posccaesar.org/ontology/plm/rdl/PCA_100006702"/>
    <rdfs:label>Hydraulic circuit diagrams - lifting appliances</rdfs:label>
    <rdfs:comment>The hydraulic circuit diagrams shall include: 
 - All components with identification 
 - Port sizes 
 - Pressure settings 
 - Cross reference to Circuit wiring diagrams 
 - Bulkhead connectors, pipes with dimensions 
 - Hoses id with dimensions</rdfs:comment>
    <rdl:PCA_100006768>The hydraulic circuit diagrams shall include: 
 - All components with identification 
 - Port sizes 
 - Pressure settings 
 - Cross reference to Circuit wiring diagrams 
 - Bulkhead connectors, pipes with dimensions 
 - Hoses id with dimensions</rdl:PCA_100006768>
    <rdfs:subClassOf rdf:resource="http://rds.posccaesar.org/ontology/plm/rdl/PCA_100004908"/>
  </owl:Class>
  <owl:Class rdf:about="http://rds.posccaesar.org/ontology/plm/rdl/PCA_100006182">
    <skos:broadMatch>
      <rdl:PCA_100001503 rdf:about="http://rds.posccaesar.org/ontology/plm/rdl/PCA_100006731">
        <rdfs:label>geometrical outline information</rdfs:label>
        <rdl:PCA_100004924>TA</rdl:PCA_100004924>
        <rdf:type rdf:resource="http://www.w3.org/2002/07/owl#NamedIndividual"/>
      </rdl:PCA_100001503>
    </skos:broadMatch>
    <rdfs:label>Electrical/fiberoptical hook-up drawing - well completion</rdfs:label>
    <rdfs:subClassOf rdf:resource="http://rds.posccaesar.org/ontology/plm/rdl/PCA_100004908"/>
    <skos:broadMatch rdf:resource="http://rds.posccaesar.org/ontology/plm/rdl/PCA_100006712"/>
    <rdl:PCA_100006765>
      <rdl:PCA_100001503 rdf:about="http://w3id.org/readi/rdl/CFIHOS-20000008">
        <rdfs:label>electrical engineering</rdfs:label>
        <rdl:PCA_100004924>EA</rdl:PCA_100004924>
        <rdf:type rdf:resource="http://www.w3.org/2002/07/owl#NamedIndividual"/>
      </rdl:PCA_100001503>
    </rdl:PCA_100006765>
    <rdl:PCA_100006763>For electrical and fiber-optical downhole instruments the supplier shall work out hook-up drawings. The drawing shall visualize the instrumentation in an entire well.</rdl:PCA_100006763>
    <skos:broader rdf:resource="http://rds.posccaesar.org/ontology/plm/rdl/PCA_100006746"/>
    <rdl:PCA_100006764>A typical hook-up drawing shall indicate details such as:
 - All instruments/type installed by Supplier
 - Location in well relative to zones/branches
 - Measuring point relative to tubing/annulus (gauges only)
 - Connections and interconnections of signal lines
The drawing shall indicate split of responsibilities between Supplier and Purchaser.</rdl:PCA_100006764>
    <skos:broadMatch rdf:resource="http://rds.posccaesar.org/ontology/plm/rdl/PCA_100006732"/>
  </owl:Class>
  <owl:Class rdf:about="http://rds.posccaesar.org/ontology/plm/rdl/PCA_100006194">
    <skos:broader rdf:resource="http://rds.posccaesar.org/ontology/plm/rdl/PCA_100006756"/>
    <skos:broadMatch rdf:resource="http://rds.posccaesar.org/ontology/plm/rdl/PCA_100006722"/>
    <rdfs:label>Exemptions from specifications and other requirements in the inquiry</rdfs:label>
    <rdfs:comment>This document shall contain a list stating all deviations from the requirements in the inquiry, and proposed alternative requirements.</rdfs:comment>
    <rdl:PCA_100006768>This document shall contain a list stating all deviations from the requirements in the inquiry, and proposed alternative requirements.</rdl:PCA_100006768>
    <rdl:PCA_100006766 rdf:resource="http://rds.posccaesar.org/ontology/plm/rdl/PCA_100006653"/>
    <rdl:PCA_100006763>This document shall document deviations from standards and/or specifications, and issue of technical queries.

This document shall support the procurement process. Accepted exemptions must be incorporated in technical documentation for the equipment.</rdl:PCA_100006763>
    <rdfs:subClassOf rdf:resource="http://rds.posccaesar.org/ontology/plm/rdl/PCA_100004908"/>
  </owl:Class>
  <owl:Class rdf:about="http://rds.posccaesar.org/ontology/plm/rdl/PCA_100006085">
    <rdfs:subClassOf rdf:resource="http://rds.posccaesar.org/ontology/plm/rdl/PCA_100004908"/>
    <rdl:PCA_100006765 rdf:resource="http://w3id.org/readi/rdl/CFIHOS-20000015"/>
    <rdl:PCA_100006766 rdf:resource="http://rds.posccaesar.org/ontology/plm/rdl/PCA_100006633"/>
    <skos:broader rdf:resource="http://rds.posccaesar.org/ontology/plm/rdl/PCA_100006748"/>
    <rdl:PCA_100006766 rdf:resource="http://rds.posccaesar.org/ontology/plm/rdl/PCA_100006626"/>
    <rdl:PCA_100006763>The context and hiding charts shall be prepared as a matrix between initiating and actuated elements to be hidden. Both initiating and hidden elements shall be identified by ENS tag numbers.</rdl:PCA_100006763>
    <rdfs:label>Alarm C&amp;H (context &amp; hiding)</rdfs:label>
    <skos:broadMatch>
      <rdl:PCA_100001503 rdf:about="http://rds.posccaesar.org/ontology/plm/rdl/PCA_100006699">
        <rdfs:label>functional time and sequence information</rdfs:label>
        <rdl:PCA_100004924>FF</rdl:PCA_100004924>
        <rdf:type rdf:resource="http://www.w3.org/2002/07/owl#NamedIndividual"/>
      </rdl:PCA_100001503>
    </skos:broadMatch>
    <rdl:PCA_100006766 rdf:resource="http://rds.posccaesar.org/ontology/plm/rdl/PCA_100006628"/>
    <rdl:PCA_100006768>The context and hiding charts shall be prepared as a matrix between initiating and actuated elements to be hidden. Both initiating and hidden elements shall be identified by ENS tag numbers.</rdl:PCA_100006768>
    <rdfs:comment>The context and hiding charts shall be prepared as a matrix between initiating and actuated elements to be hidden. Both initiating and hidden elements shall be identified by ENS tag numbers.</rdfs:comment>
    <rdl:PCA_100006766 rdf:resource="http://rds.posccaesar.org/ontology/plm/rdl/PCA_100006627"/>
  </owl:Class>
  <owl:Class rdf:about="http://rds.posccaesar.org/ontology/plm/rdl/PCA_100006490">
    <rdl:PCA_100006763>Ensure safe operation</rdl:PCA_100006763>
    <rdfs:label>Technology qualification report</rdfs:label>
    <rdfs:subClassOf rdf:resource="http://rds.posccaesar.org/ontology/plm/rdl/PCA_100004908"/>
    <rdl:PCA_100006768>To give  the result of all planned qualification activities.</rdl:PCA_100006768>
    <rdl:PCA_100006766 rdf:resource="http://rds.posccaesar.org/ontology/plm/rdl/PCA_100006654"/>
    <rdfs:comment>To give  the result of all planned qualification activities.</rdfs:comment>
    <skos:broader rdf:resource="http://rds.posccaesar.org/ontology/plm/rdl/PCA_100006756"/>
    <skos:broadMatch rdf:resource="http://rds.posccaesar.org/ontology/plm/rdl/PCA_100006722"/>
    <rdl:PCA_100006765 rdf:resource="http://w3id.org/readi/rdl/CFIHOS-20000018"/>
  </owl:Class>
  <owl:Class rdf:about="http://rds.posccaesar.org/ontology/plm/rdl/PCA_100006097">
    <rdfs:label>Assembly drawing</rdfs:label>
    <rdl:PCA_100006763>A drawing including an overview of main parts of the equipment used for manufacturing. The drawing includes reference to sub-assemblies, dimensions, interface information, weights, service supply details and reference to design documents.</rdl:PCA_100006763>
    <rdl:PCA_100006766 rdf:resource="http://rds.posccaesar.org/ontology/plm/rdl/PCA_100006653"/>
    <rdfs:subClassOf rdf:resource="http://rds.posccaesar.org/ontology/plm/rdl/PCA_100004908"/>
    <rdl:PCA_100006765 rdf:resource="http://w3id.org/readi/rdl/CFIHOS-20000031"/>
    <rdfs:comment>Provides overview of the main parts of the equipment including part numbers and references to specifications and other design documentation. Drawing is used for manufacturing of assemblies.</rdfs:comment>
    <skos:broader rdf:resource="http://rds.posccaesar.org/ontology/plm/rdl/PCA_100006746"/>
    <skos:broadMatch>
      <rdl:PCA_100001503 rdf:about="http://rds.posccaesar.org/ontology/plm/rdl/PCA_100006734">
        <rdfs:label>assembly information</rdfs:label>
        <rdl:PCA_100004924>TL</rdl:PCA_100004924>
        <rdf:type rdf:resource="http://www.w3.org/2002/07/owl#NamedIndividual"/>
      </rdl:PCA_100001503>
    </skos:broadMatch>
    <rdl:PCA_100006768>Provides overview of the main parts of the equipment including part numbers and references to specifications and other design documentation. Drawing is used for manufacturing of assemblies.</rdl:PCA_100006768>
  </owl:Class>
  <owl:Class rdf:about="http://rds.posccaesar.org/ontology/plm/rdl/PCA_100006297">
    <rdfs:comment>A drawing showing necessary arrangements for rigging and lifting, including lifting points and centre of gravity for equipment.</rdfs:comment>
    <rdl:PCA_100006768>A drawing showing necessary arrangements for rigging and lifting, including lifting points and centre of gravity for equipment.</rdl:PCA_100006768>
    <skos:broader rdf:resource="http://rds.posccaesar.org/ontology/plm/rdl/PCA_100006746"/>
    <rdfs:label>Lifting drawing</rdfs:label>
    <rdl:PCA_100006763>A drawing containing information necessary for rigging and lifting of equipment.</rdl:PCA_100006763>
    <rdl:PCA_100006766 rdf:resource="http://rds.posccaesar.org/ontology/plm/rdl/PCA_100006653"/>
    <skos:broadMatch rdf:resource="http://rds.posccaesar.org/ontology/plm/rdl/PCA_100006731"/>
    <rdfs:subClassOf rdf:resource="http://rds.posccaesar.org/ontology/plm/rdl/PCA_100004908"/>
    <rdl:PCA_100006765 rdf:resource="http://w3id.org/readi/rdl/CFIHOS-20000031"/>
  </owl:Class>
  <owl:Class rdf:about="http://rds.posccaesar.org/ontology/plm/rdl/PCA_100006285">
    <skos:broader rdf:resource="http://rds.posccaesar.org/ontology/plm/rdl/PCA_100006751"/>
    <rdl:PCA_100006766>
      <rdl:PCA_100001503 rdf:about="http://rds.posccaesar.org/ontology/plm/rdl/PCA_100006657">
        <rdfs:label>System</rdfs:label>
        <rdf:type rdf:resource="http://www.w3.org/2002/07/owl#NamedIndividual"/>
      </rdl:PCA_100001503>
    </rdl:PCA_100006766>
    <rdl:PCA_100006763>The procedure shall describe how to load an empty SAS system (assuming total black out), where to find the last version of the system (backup), and how to start up the system.</rdl:PCA_100006763>
    <rdfs:comment>Start-up description includes in what order the system should be started, focusing on safety first.</rdfs:comment>
    <skos:broadMatch rdf:resource="http://rds.posccaesar.org/ontology/plm/rdl/PCA_100006688"/>
    <rdl:PCA_100006765 rdf:resource="http://w3id.org/readi/rdl/CFIHOS-20000015"/>
    <rdfs:label>Instrumented systems - loading and start up procedures</rdfs:label>
    <rdl:PCA_100006768>Start-up description includes in what order the system should be started, focusing on safety first.</rdl:PCA_100006768>
    <rdfs:subClassOf rdf:resource="http://rds.posccaesar.org/ontology/plm/rdl/PCA_100004908"/>
  </owl:Class>
  <owl:Class rdf:about="http://rds.posccaesar.org/ontology/plm/rdl/PCA_100006394">
    <rdl:PCA_100006766 rdf:resource="http://rds.posccaesar.org/ontology/plm/rdl/PCA_100006606"/>
    <rdl:PCA_100006766 rdf:resource="http://rds.posccaesar.org/ontology/plm/rdl/PCA_100006612"/>
    <rdl:PCA_100006766 rdf:resource="http://rds.posccaesar.org/ontology/plm/rdl/PCA_100006594"/>
    <rdl:PCA_100006766 rdf:resource="http://rds.posccaesar.org/ontology/plm/rdl/PCA_100006593"/>
    <rdl:PCA_100006766 rdf:resource="http://rds.posccaesar.org/ontology/plm/rdl/PCA_100006620"/>
    <rdl:PCA_100006766 rdf:resource="http://rds.posccaesar.org/ontology/plm/rdl/PCA_100006618"/>
    <rdl:PCA_100006766 rdf:resource="http://rds.posccaesar.org/ontology/plm/rdl/PCA_100006633"/>
    <rdfs:label>Process hazop close-out report</rdfs:label>
    <rdl:PCA_100006766 rdf:resource="http://rds.posccaesar.org/ontology/plm/rdl/PCA_100006580"/>
    <rdl:PCA_100006766 rdf:resource="http://rds.posccaesar.org/ontology/plm/rdl/PCA_100006578"/>
    <rdl:PCA_100006766 rdf:resource="http://rds.posccaesar.org/ontology/plm/rdl/PCA_100006608"/>
    <rdl:PCA_100006766 rdf:resource="http://rds.posccaesar.org/ontology/plm/rdl/PCA_100006607"/>
    <rdl:PCA_100006766 rdf:resource="http://rds.posccaesar.org/ontology/plm/rdl/PCA_100006622"/>
    <rdl:PCA_100006765 rdf:resource="http://w3id.org/readi/rdl/CFIHOS-20000026"/>
    <rdl:PCA_100006766 rdf:resource="http://rds.posccaesar.org/ontology/plm/rdl/PCA_100006598"/>
    <rdl:PCA_100006766 rdf:resource="http://rds.posccaesar.org/ontology/plm/rdl/PCA_100006605"/>
    <rdl:PCA_100006766 rdf:resource="http://rds.posccaesar.org/ontology/plm/rdl/PCA_100006586"/>
    <rdl:PCA_100006766 rdf:resource="http://rds.posccaesar.org/ontology/plm/rdl/PCA_100006601"/>
    <rdl:PCA_100006766 rdf:resource="http://rds.posccaesar.org/ontology/plm/rdl/PCA_100006582"/>
    <rdl:PCA_100006766 rdf:resource="http://rds.posccaesar.org/ontology/plm/rdl/PCA_100006621"/>
    <rdl:PCA_100006766 rdf:resource="http://rds.posccaesar.org/ontology/plm/rdl/PCA_100006583"/>
    <rdl:PCA_100006766 rdf:resource="http://rds.posccaesar.org/ontology/plm/rdl/PCA_100006596"/>
    <rdl:PCA_100006766 rdf:resource="http://rds.posccaesar.org/ontology/plm/rdl/PCA_100006595"/>
    <rdl:PCA_100006766 rdf:resource="http://rds.posccaesar.org/ontology/plm/rdl/PCA_100006590"/>
    <rdl:PCA_100006766 rdf:resource="http://rds.posccaesar.org/ontology/plm/rdl/PCA_100006627"/>
    <skos:broadMatch rdf:resource="http://rds.posccaesar.org/ontology/plm/rdl/PCA_100006687"/>
    <rdl:PCA_100006766 rdf:resource="http://rds.posccaesar.org/ontology/plm/rdl/PCA_100006623"/>
    <rdl:PCA_100006766 rdf:resource="http://rds.posccaesar.org/ontology/plm/rdl/PCA_100006602"/>
    <rdl:PCA_100006766 rdf:resource="http://rds.posccaesar.org/ontology/plm/rdl/PCA_100006579"/>
    <rdl:PCA_100006766 rdf:resource="http://rds.posccaesar.org/ontology/plm/rdl/PCA_100006615"/>
    <rdl:PCA_100006766 rdf:resource="http://rds.posccaesar.org/ontology/plm/rdl/PCA_100006587"/>
    <rdl:PCA_100006766 rdf:resource="http://rds.posccaesar.org/ontology/plm/rdl/PCA_100006614"/>
    <rdl:PCA_100006766 rdf:resource="http://rds.posccaesar.org/ontology/plm/rdl/PCA_100006609"/>
    <rdl:PCA_100006766 rdf:resource="http://rds.posccaesar.org/ontology/plm/rdl/PCA_100006611"/>
    <rdl:PCA_100006766 rdf:resource="http://rds.posccaesar.org/ontology/plm/rdl/PCA_100006610"/>
    <rdl:PCA_100006766 rdf:resource="http://rds.posccaesar.org/ontology/plm/rdl/PCA_100006624"/>
    <rdl:PCA_100006766 rdf:resource="http://rds.posccaesar.org/ontology/plm/rdl/PCA_100006599"/>
    <rdl:PCA_100006766 rdf:resource="http://rds.posccaesar.org/ontology/plm/rdl/PCA_100006584"/>
    <rdl:PCA_100006766 rdf:resource="http://rds.posccaesar.org/ontology/plm/rdl/PCA_100006617"/>
    <rdl:PCA_100006766 rdf:resource="http://rds.posccaesar.org/ontology/plm/rdl/PCA_100006589"/>
    <rdl:PCA_100006766 rdf:resource="http://rds.posccaesar.org/ontology/plm/rdl/PCA_100006592"/>
    <rdl:PCA_100006766 rdf:resource="http://rds.posccaesar.org/ontology/plm/rdl/PCA_100006591"/>
    <rdl:PCA_100006766 rdf:resource="http://rds.posccaesar.org/ontology/plm/rdl/PCA_100006603"/>
    <skos:broadMatch rdf:resource="http://rds.posccaesar.org/ontology/plm/rdl/PCA_100006688"/>
    <rdl:PCA_100006768>All answers shall be collected in a close-out report.</rdl:PCA_100006768>
    <rdl:PCA_100006766 rdf:resource="http://rds.posccaesar.org/ontology/plm/rdl/PCA_100006588"/>
    <rdfs:comment>All answers shall be collected in a close-out report.</rdfs:comment>
    <rdl:PCA_100006766 rdf:resource="http://rds.posccaesar.org/ontology/plm/rdl/PCA_100006625"/>
    <rdfs:subClassOf rdf:resource="http://rds.posccaesar.org/ontology/plm/rdl/PCA_100004908"/>
    <rdl:PCA_100006766 rdf:resource="http://rds.posccaesar.org/ontology/plm/rdl/PCA_100006619"/>
    <rdl:PCA_100006766 rdf:resource="http://rds.posccaesar.org/ontology/plm/rdl/PCA_100006604"/>
    <rdl:PCA_100006766 rdf:resource="http://rds.posccaesar.org/ontology/plm/rdl/PCA_100006585"/>
    <rdl:PCA_100006766 rdf:resource="http://rds.posccaesar.org/ontology/plm/rdl/PCA_100006600"/>
    <rdl:PCA_100006763>Individual close-out answer for each finding/recommendation from the HAZOP session(s) shall be issued.</rdl:PCA_100006763>
    <rdl:PCA_100006766 rdf:resource="http://rds.posccaesar.org/ontology/plm/rdl/PCA_100006581"/>
    <rdl:PCA_100006766 rdf:resource="http://rds.posccaesar.org/ontology/plm/rdl/PCA_100006616"/>
    <skos:broader rdf:resource="http://rds.posccaesar.org/ontology/plm/rdl/PCA_100006756"/>
    <rdl:PCA_100006766 rdf:resource="http://rds.posccaesar.org/ontology/plm/rdl/PCA_100006597"/>
    <rdl:PCA_100006766 rdf:resource="http://rds.posccaesar.org/ontology/plm/rdl/PCA_100006613"/>
  </owl:Class>
  <owl:Class rdf:about="http://rds.posccaesar.org/ontology/plm/rdl/PCA_100006273">
    <skos:broader rdf:resource="http://rds.posccaesar.org/ontology/plm/rdl/PCA_100006756"/>
    <skos:broadMatch rdf:resource="http://rds.posccaesar.org/ontology/plm/rdl/PCA_100006722"/>
    <rdfs:label>Inspection and test plan</rdfs:label>
    <rdfs:comment>The ITP shall list scheduled inspection or verification activities in the production process, from purchase order to delivery. Reference to applicable standard or procedure and acceptance criteria shall be included. Inspection items that needs to be controlled/witnessed by purchaser, 3rd parties etc. shall be identified.</rdfs:comment>
    <rdl:PCA_100006768>The ITP shall list scheduled inspection or verification activities in the production process, from purchase order to delivery. Reference to applicable standard or procedure and acceptance criteria shall be included. Inspection items that needs to be controlled/witnessed by purchaser, 3rd parties etc. shall be identified.</rdl:PCA_100006768>
    <rdl:PCA_100006766 rdf:resource="http://rds.posccaesar.org/ontology/plm/rdl/PCA_100006653"/>
    <rdl:PCA_100006763>This document shall support both the procurement process and quality controlling activities to assure that the equipment will be delivered according to specification.</rdl:PCA_100006763>
    <rdfs:subClassOf rdf:resource="http://rds.posccaesar.org/ontology/plm/rdl/PCA_100004908"/>
  </owl:Class>
  <owl:Class rdf:about="http://rds.posccaesar.org/ontology/plm/rdl/PCA_100006261">
    <skos:broader rdf:resource="http://rds.posccaesar.org/ontology/plm/rdl/PCA_100006745"/>
    <skos:broadMatch rdf:resource="http://rds.posccaesar.org/ontology/plm/rdl/PCA_100006712"/>
    <rdfs:label>Hydraulic connection diagram</rdfs:label>
    <rdl:PCA_100006766 rdf:resource="http://rds.posccaesar.org/ontology/plm/rdl/PCA_100006653"/>
    <rdl:PCA_100006765 rdf:resource="http://w3id.org/readi/rdl/CFIHOS-20000031"/>
    <rdl:PCA_100006765 rdf:resource="http://w3id.org/readi/rdl/CFIHOS-20000015"/>
    <rdl:PCA_100006763>The purpose of this document is to cover hydraulic distribution from ring main or a hydraulic manifold to all hydraulic connections on a mechanical package, and to include all other individual hydraulic consumers for the actual hydraulic pressure unit.</rdl:PCA_100006763>
    <rdfs:subClassOf rdf:resource="http://rds.posccaesar.org/ontology/plm/rdl/PCA_100004908"/>
  </owl:Class>
  <owl:Class rdf:about="http://rds.posccaesar.org/ontology/plm/rdl/PCA_100006181">
    <skos:broader rdf:resource="http://rds.posccaesar.org/ontology/plm/rdl/PCA_100006745"/>
    <rdl:PCA_100006764>Electrical Circuit/Schematics shall be prepared for all feeders and control circuits (except for small components ). This diagram shall include all internal
connections for control, alarms, protection, interlocks, trip functions, monitoring, etc.</rdl:PCA_100006764>
    <rdfs:label>Electrical schematics</rdfs:label>
    <rdl:PCA_100006766 rdf:resource="http://rds.posccaesar.org/ontology/plm/rdl/PCA_100006653"/>
    <skos:broadMatch rdf:resource="http://rds.posccaesar.org/ontology/plm/rdl/PCA_100006702"/>
    <rdfs:comment>A diagram showing electrical and fiber optical connections between different equipment and components.</rdfs:comment>
    <rdfs:subClassOf rdf:resource="http://rds.posccaesar.org/ontology/plm/rdl/PCA_100004908"/>
    <rdl:PCA_100006768>A diagram showing electrical and fiber optical connections between different equipment and components.</rdl:PCA_100006768>
    <rdl:PCA_100006765 rdf:resource="http://w3id.org/readi/rdl/CFIHOS-20000031"/>
    <rdl:PCA_100006763>Illustrate electrical equipment with lines and connections.</rdl:PCA_100006763>
  </owl:Class>
  <owl:Class rdf:about="http://rds.posccaesar.org/ontology/plm/rdl/PCA_100006382">
    <skos:broader rdf:resource="http://rds.posccaesar.org/ontology/plm/rdl/PCA_100006745"/>
    <skos:broadMatch rdf:resource="http://rds.posccaesar.org/ontology/plm/rdl/PCA_100006712"/>
    <rdfs:label>Pneumatic connection diagram</rdfs:label>
    <rdfs:comment>The diagram shall identify all pneumatic connections.</rdfs:comment>
    <rdl:PCA_100006768>The diagram shall identify all pneumatic connections.</rdl:PCA_100006768>
    <rdl:PCA_100006766 rdf:resource="http://rds.posccaesar.org/ontology/plm/rdl/PCA_100006653"/>
    <rdl:PCA_100006765>
      <rdl:PCA_100001503 rdf:about="http://w3id.org/readi/rdl/CFIHOS-20000023">
        <rdfs:label>mechanical engineering</rdfs:label>
        <rdl:PCA_100004924>MX</rdl:PCA_100004924>
        <rdf:type rdf:resource="http://www.w3.org/2002/07/owl#NamedIndividual"/>
      </rdl:PCA_100001503>
    </rdl:PCA_100006765>
    <rdfs:subClassOf rdf:resource="http://rds.posccaesar.org/ontology/plm/rdl/PCA_100004908"/>
  </owl:Class>
  <owl:Class rdf:about="http://rds.posccaesar.org/ontology/plm/rdl/PCA_100006491">
    <skos:broader rdf:resource="http://rds.posccaesar.org/ontology/plm/rdl/PCA_100006741"/>
    <skos:broadMatch rdf:resource="http://rds.posccaesar.org/ontology/plm/rdl/PCA_100006687"/>
    <rdfs:label>Telecommunication battery and charger capacity calculations</rdfs:label>
    <rdfs:comment>Calculations of telecommunication battery and charger capacity.</rdfs:comment>
    <rdl:PCA_100006768>Calculations of telecommunication battery and charger capacity.</rdl:PCA_100006768>
    <rdl:PCA_100006766 rdf:resource="http://rds.posccaesar.org/ontology/plm/rdl/PCA_100006653"/>
    <rdl:PCA_100006765>
      <rdl:PCA_100001503 rdf:about="http://w3id.org/readi/rdl/CFIHOS-20000030">
        <rdfs:label>telecommunications</rdfs:label>
        <rdl:PCA_100004924>TA</rdl:PCA_100004924>
        <rdf:type rdf:resource="http://www.w3.org/2002/07/owl#NamedIndividual"/>
      </rdl:PCA_100001503>
    </rdl:PCA_100006765>
    <rdfs:subClassOf rdf:resource="http://rds.posccaesar.org/ontology/plm/rdl/PCA_100004908"/>
  </owl:Class>
  <owl:Class rdf:about="http://rds.posccaesar.org/ontology/plm/rdl/PCA_100006370">
    <skos:broadMatch rdf:resource="http://rds.posccaesar.org/ontology/plm/rdl/PCA_100006686"/>
    <rdl:PCA_100006768>It includes but it is not limited to: list/description of the surveys available, seabed features, geotechnics, routing restrictions including third party requirements, routing selection criteria and process, stress analysis evaluations, results in terms of reference to routing layout(s) and coordinates' file(s).</rdl:PCA_100006768>
    <rdfs:comment>It includes but it is not limited to: list/description of the surveys available, seabed features, geotechnics, routing restrictions including third party requirements, routing selection criteria and process, stress analysis evaluations, results in terms of reference to routing layout(s) and coordinates' file(s).</rdfs:comment>
    <rdl:PCA_100006766 rdf:resource="http://rds.posccaesar.org/ontology/plm/rdl/PCA_100006654"/>
    <rdfs:label>Pipeline route design report</rdfs:label>
    <skos:broader rdf:resource="http://rds.posccaesar.org/ontology/plm/rdl/PCA_100006756"/>
    <rdl:PCA_100006763>Ensure safe operation</rdl:PCA_100006763>
    <rdfs:subClassOf rdf:resource="http://rds.posccaesar.org/ontology/plm/rdl/PCA_100004908"/>
    <rdl:PCA_100006765 rdf:resource="http://w3id.org/readi/rdl/CFIHOS-20000018"/>
  </owl:Class>
  <owl:Class rdf:about="http://rds.posccaesar.org/ontology/plm/rdl/PCA_100006193">
    <skos:broader rdf:resource="http://rds.posccaesar.org/ontology/plm/rdl/PCA_100006746"/>
    <skos:broadMatch>
      <rdl:PCA_100001503 rdf:about="http://rds.posccaesar.org/ontology/plm/rdl/PCA_100006706">
        <rdfs:label>foundation information</rdfs:label>
        <rdl:PCA_100004924>LB</rdl:PCA_100004924>
        <rdf:type rdf:resource="http://www.w3.org/2002/07/owl#NamedIndividual"/>
      </rdl:PCA_100001503>
    </skos:broadMatch>
    <rdfs:label>Excavation, fill and grading drawings</rdfs:label>
    <rdfs:comment>All system, arrangement, layout, plan, section and detail drawings shall be included.</rdfs:comment>
    <rdl:PCA_100006768>All system, arrangement, layout, plan, section and detail drawings shall be included.</rdl:PCA_100006768>
    <rdl:PCA_100006766 rdf:resource="http://rds.posccaesar.org/ontology/plm/rdl/PCA_100006656"/>
    <rdl:PCA_100006765 rdf:resource="http://w3id.org/readi/rdl/CFIHOS-20000007"/>
    <rdfs:subClassOf rdf:resource="http://rds.posccaesar.org/ontology/plm/rdl/PCA_100004908"/>
  </owl:Class>
  <owl:Class rdf:about="http://rds.posccaesar.org/ontology/plm/rdl/PCA_100006084">
    <skos:broader rdf:resource="http://rds.posccaesar.org/ontology/plm/rdl/PCA_100006745"/>
    <rdl:PCA_100006763>Air distribution diagrams (HVAC flow diagrams) shall be provided per system</rdl:PCA_100006763>
    <rdfs:label>Air flow diagrams</rdfs:label>
    <rdfs:subClassOf rdf:resource="http://rds.posccaesar.org/ontology/plm/rdl/PCA_100004908"/>
    <rdfs:comment>Air distribution diagrams (HVAC flow diagrams) shall be provided per system and include the following information: 
 - Tag codes for supply and extract fans (air handling units);
 - Flow rates for supply and extract fans (air handling units);
 - Flow rates for all serviced areas and air flows necessary for system balancing;
 - Temperature range requirements for all serviced areas;
 - Air change rates for all serviced areas;
 - HVAC noise range requirements for all serviced areas;
 - Area code and description for fan rooms and serviced areas;
 - Notes regarding main design parameters, such as fan standby philosophy, emergency operation, shall be given.</rdfs:comment>
    <rdl:PCA_100006765>
      <rdl:PCA_100001503 rdf:about="http://w3id.org/readi/rdl/CFIHOS-20000019">
        <rdfs:label>heating, ventilating, and air conditioning</rdfs:label>
        <rdl:PCA_100004924>MH</rdl:PCA_100004924>
        <rdf:type rdf:resource="http://www.w3.org/2002/07/owl#NamedIndividual"/>
      </rdl:PCA_100001503>
    </rdl:PCA_100006765>
    <skos:broadMatch rdf:resource="http://rds.posccaesar.org/ontology/plm/rdl/PCA_100006696"/>
    <rdl:PCA_100006766>
      <rdl:PCA_100001503 rdf:about="http://rds.posccaesar.org/ontology/plm/rdl/PCA_100006650">
        <rdfs:label>HVAC</rdfs:label>
        <rdl:PCA_100004924>97</rdl:PCA_100004924>
        <rdf:type rdf:resource="http://www.w3.org/2002/07/owl#NamedIndividual"/>
      </rdl:PCA_100001503>
    </rdl:PCA_100006766>
    <rdl:PCA_100006768>Air distribution diagrams (HVAC flow diagrams) shall be provided per system and include the following information: 
 - Tag codes for supply and extract fans (air handling units);
 - Flow rates for supply and extract fans (air handling units);
 - Flow rates for all serviced areas and air flows necessary for system balancing;
 - Temperature range requirements for all serviced areas;
 - Air change rates for all serviced areas;
 - HVAC noise range requirements for all serviced areas;
 - Area code and description for fan rooms and serviced areas;
 - Notes regarding main design parameters, such as fan standby philosophy, emergency operation, shall be given.</rdl:PCA_100006768>
  </owl:Class>
  <owl:Class rdf:about="http://rds.posccaesar.org/ontology/plm/rdl/PCA_100006096">
    <rdfs:comment>To document actual manufacturing with reference to individual serial number.</rdfs:comment>
    <rdfs:subClassOf rdf:resource="http://rds.posccaesar.org/ontology/plm/rdl/PCA_100004908"/>
    <rdfs:label>As-built drawings (info)</rdfs:label>
    <rdl:PCA_100006766 rdf:resource="http://rds.posccaesar.org/ontology/plm/rdl/PCA_100006653"/>
    <rdl:PCA_100006764>An As-built drawing is a red-marked up and stamped copy of the IFC version of an drawing, that will be part of the MRB.</rdl:PCA_100006764>
    <rdl:PCA_100006768>To document actual manufacturing with reference to individual serial number.</rdl:PCA_100006768>
    <rdl:PCA_100006765 rdf:resource="http://w3id.org/readi/rdl/CFIHOS-20000031"/>
    <rdl:PCA_100006763>Drawing documenting the changes between issued for construction and as- built version of the product. Not used for standard and non-engineered products.</rdl:PCA_100006763>
    <skos:broadMatch>
      <rdl:PCA_100001503 rdf:about="http://rds.posccaesar.org/ontology/plm/rdl/PCA_100006733">
        <rdfs:label>manufacturing information</rdfs:label>
        <rdl:PCA_100004924>TC</rdl:PCA_100004924>
        <rdf:type rdf:resource="http://www.w3.org/2002/07/owl#NamedIndividual"/>
      </rdl:PCA_100001503>
    </skos:broadMatch>
    <skos:broader rdf:resource="http://rds.posccaesar.org/ontology/plm/rdl/PCA_100006746"/>
  </owl:Class>
  <owl:Class rdf:about="http://rds.posccaesar.org/ontology/plm/rdl/PCA_100006505">
    <rdl:PCA_100006763>Describe how to transport and handle equipment safely from delivery to final installation.</rdl:PCA_100006763>
    <rdl:PCA_100006768>Information for safe handling of equipment during transportation, lifting and handling.</rdl:PCA_100006768>
    <rdfs:comment>Information for safe handling of equipment during transportation, lifting and handling.</rdfs:comment>
    <rdl:PCA_100006766 rdf:resource="http://rds.posccaesar.org/ontology/plm/rdl/PCA_100006653"/>
    <rdl:PCA_100006765 rdf:resource="http://w3id.org/readi/rdl/CFIHOS-20000031"/>
    <skos:broadMatch>
      <rdl:PCA_100001503 rdf:about="http://rds.posccaesar.org/ontology/plm/rdl/PCA_100006668">
        <rdfs:label>logistic information</rdfs:label>
        <rdl:PCA_100004924>BF</rdl:PCA_100004924>
        <rdf:type rdf:resource="http://www.w3.org/2002/07/owl#NamedIndividual"/>
      </rdl:PCA_100001503>
    </skos:broadMatch>
    <rdfs:label>Transport and handling instructions</rdfs:label>
    <skos:broader rdf:resource="http://rds.posccaesar.org/ontology/plm/rdl/PCA_100006751"/>
    <rdfs:subClassOf rdf:resource="http://rds.posccaesar.org/ontology/plm/rdl/PCA_100004908"/>
  </owl:Class>
  <owl:Class rdf:about="http://rds.posccaesar.org/ontology/plm/rdl/PCA_100006517">
    <skos:broader rdf:resource="http://rds.posccaesar.org/ontology/plm/rdl/PCA_100006748"/>
    <skos:broadMatch rdf:resource="http://rds.posccaesar.org/ontology/plm/rdl/PCA_100006716"/>
    <rdfs:label>Utility consumption index</rdfs:label>
    <rdfs:comment>The following generalised index shall be used:
 - Equipment tag no.
 - Type of consumption
 - Volume m3 and time unit
 - Net weight (kg) and time unit
 - Specific weight (kg)
 - Storage temperature oC
 - Storage humidity %
 - Storage max pressure (barg)
 - Storage capacity m3
 - Storage location/area
 - Specification
 - Supplier
 - Data sheet
 - Notes</rdfs:comment>
    <rdl:PCA_100006768>The following generalised index shall be used:
 - Equipment tag no.
 - Type of consumption
 - Volume m3 and time unit
 - Net weight (kg) and time unit
 - Specific weight (kg)
 - Storage temperature oC
 - Storage humidity %
 - Storage max pressure (barg)
 - Storage capacity m3
 - Storage location/area
 - Specification
 - Supplier
 - Data sheet
 - Notes</rdl:PCA_100006768>
    <rdl:PCA_100006763>Consumption data e.g. for diesel oil, compressed air, heating/cooling media etc.</rdl:PCA_100006763>
    <rdfs:subClassOf rdf:resource="http://rds.posccaesar.org/ontology/plm/rdl/PCA_100004908"/>
  </owl:Class>
  <owl:Class rdf:about="http://rds.posccaesar.org/ontology/plm/rdl/PCA_100006140">
    <rdl:PCA_100006768>A view or drawing that shows what the inside of equipment looks like after a cross-sectional cut has been made, including key parameter capacities for the cross- section.</rdl:PCA_100006768>
    <rdfs:comment>A view or drawing that shows what the inside of equipment looks like after a cross-sectional cut has been made, including key parameter capacities for the cross- section.</rdfs:comment>
    <rdfs:label>Cross-sectional drawing</rdfs:label>
    <skos:broadMatch rdf:resource="http://rds.posccaesar.org/ontology/plm/rdl/PCA_100006732"/>
    <rdl:PCA_100006765 rdf:resource="http://w3id.org/readi/rdl/CFIHOS-20000031"/>
    <rdl:PCA_100006763>To show internals. Used in engineering and operations.</rdl:PCA_100006763>
    <rdl:PCA_100006766 rdf:resource="http://rds.posccaesar.org/ontology/plm/rdl/PCA_100006653"/>
    <skos:broader rdf:resource="http://rds.posccaesar.org/ontology/plm/rdl/PCA_100006746"/>
    <rdfs:subClassOf rdf:resource="http://rds.posccaesar.org/ontology/plm/rdl/PCA_100004908"/>
  </owl:Class>
  <owl:Class rdf:about="http://rds.posccaesar.org/ontology/plm/rdl/PCA_100006152">
    <skos:broader rdf:resource="http://rds.posccaesar.org/ontology/plm/rdl/PCA_100006746"/>
    <skos:broadMatch>
      <rdl:PCA_100001503 rdf:about="http://rds.posccaesar.org/ontology/plm/rdl/PCA_100006695">
        <rdfs:label>system overview information</rdfs:label>
        <rdl:PCA_100004924>FA</rdl:PCA_100004924>
        <rdf:type rdf:resource="http://www.w3.org/2002/07/owl#NamedIndividual"/>
      </rdl:PCA_100001503>
    </skos:broadMatch>
    <rdl:PCA_100006763>Documentation of the systems</rdl:PCA_100006763>
    <rdfs:comment>Drawing of the DEH system showing all the building blocks the system consists of.</rdfs:comment>
    <skos:broadMatch rdf:resource="http://rds.posccaesar.org/ontology/plm/rdl/PCA_100006705"/>
    <rdl:PCA_100006768>Drawing of the DEH system showing all the building blocks the system consists of.</rdl:PCA_100006768>
    <rdfs:subClassOf rdf:resource="http://rds.posccaesar.org/ontology/plm/rdl/PCA_100004908"/>
    <rdl:PCA_100006766 rdf:resource="http://rds.posccaesar.org/ontology/plm/rdl/PCA_100006657"/>
    <rdfs:label>DEH system overview (delivery overview)</rdfs:label>
    <rdl:PCA_100006765 rdf:resource="http://w3id.org/readi/rdl/CFIHOS-20000018"/>
  </owl:Class>
  <owl:Class rdf:about="http://rds.posccaesar.org/ontology/plm/rdl/PCA_100006290">
    <rdfs:label>IS calculations</rdfs:label>
    <rdl:PCA_100006765 rdf:resource="http://w3id.org/readi/rdl/CFIHOS-20000015"/>
    <rdfs:subClassOf rdf:resource="http://rds.posccaesar.org/ontology/plm/rdl/PCA_100004908"/>
    <skos:broader rdf:resource="http://rds.posccaesar.org/ontology/plm/rdl/PCA_100006741"/>
    <rdl:PCA_100006766>
      <rdl:PCA_100001503 rdf:about="http://rds.posccaesar.org/ontology/plm/rdl/PCA_100006655">
        <rdfs:label>Function</rdfs:label>
        <rdf:type rdf:resource="http://www.w3.org/2002/07/owl#NamedIndividual"/>
      </rdl:PCA_100001503>
    </rdl:PCA_100006766>
    <rdfs:comment>Complete calculations according to IEC60079</rdfs:comment>
    <rdl:PCA_100006768>Complete calculations according to IEC60079</rdl:PCA_100006768>
    <skos:broadMatch rdf:resource="http://rds.posccaesar.org/ontology/plm/rdl/PCA_100006687"/>
    <rdl:PCA_100006763>Atex requirement for all intrinsically safe instrument/telecom-equipment.
- IS / FISCO (Fieldbus Intrinsically Safe Concept) calculations.

- Not required for wireless loops. For a IS wireless instrument, IS-calculation must be available in atex certificate/vendor standard documentation.</rdl:PCA_100006763>
    <rdl:PCA_100006765 rdf:resource="http://w3id.org/readi/rdl/CFIHOS-20000030"/>
  </owl:Class>
  <owl:Class rdf:about="http://rds.posccaesar.org/ontology/plm/rdl/PCA_100006164">
    <rdl:PCA_100006764>The Dimensional Control Report shall document and verify that specified dimensional and tolerance requirements has been met. The control of dimensions is fundamental to the mechanical engineering discipline, and without which no mechanism could work, no parts would be interchangeable. It is achieved by specifying tolerances – limits to the deviation from nominal dimension. No mechanical drawing is complete without tolerances on all dimensions, limits and fits on mating parts, and flatness tolerances on surfaces.</rdl:PCA_100006764>
    <skos:broader rdf:resource="http://rds.posccaesar.org/ontology/plm/rdl/PCA_100006756"/>
    <skos:broadMatch rdf:resource="http://rds.posccaesar.org/ontology/plm/rdl/PCA_100006722"/>
    <rdl:PCA_100006763>Report including verification of critical dimensions specified on drawings.</rdl:PCA_100006763>
    <rdl:PCA_100006765 rdf:resource="http://w3id.org/readi/rdl/CFIHOS-20000031"/>
    <rdfs:subClassOf rdf:resource="http://rds.posccaesar.org/ontology/plm/rdl/PCA_100004908"/>
    <rdl:PCA_100006766 rdf:resource="http://rds.posccaesar.org/ontology/plm/rdl/PCA_100006653"/>
    <rdfs:comment>The Dimensional Control Report shall document and verify that specified dimensional and tolerance requirements has been met.</rdfs:comment>
    <rdfs:label>Dimensional control reports</rdfs:label>
    <rdl:PCA_100006768>The Dimensional Control Report shall document and verify that specified dimensional and tolerance requirements has been met.</rdl:PCA_100006768>
  </owl:Class>
  <owl:Class rdf:about="http://rds.posccaesar.org/ontology/plm/rdl/PCA_100006176">
    <skos:broader rdf:resource="http://rds.posccaesar.org/ontology/plm/rdl/PCA_100006745"/>
    <skos:broadMatch rdf:resource="http://rds.posccaesar.org/ontology/plm/rdl/PCA_100006712"/>
    <skos:broadMatch rdf:resource="http://rds.posccaesar.org/ontology/plm/rdl/PCA_100006702"/>
    <rdfs:label>Electrical connection and wiring diagram – well completion</rdfs:label>
    <rdl:PCA_100006765 rdf:resource="http://w3id.org/readi/rdl/CFIHOS-20000008"/>
    <rdl:PCA_100006764>The external connection diagram shall typically include:
 - Tag number of equipment
 - External cable tag number
 - Earthing details
Internal wiring diagrams shall be supplied when relevant e.g. to show the wiring between different electrical equipment within a package, and shall typically include:
 - Terminal block/socket number
 - Destination for internal cables
 - Earthing details</rdl:PCA_100006764>
    <rdfs:subClassOf rdf:resource="http://rds.posccaesar.org/ontology/plm/rdl/PCA_100004908"/>
  </owl:Class>
  <owl:Class rdf:about="http://rds.posccaesar.org/ontology/plm/rdl/PCA_100006188">
    <skos:broader rdf:resource="http://rds.posccaesar.org/ontology/plm/rdl/PCA_100006746"/>
    <skos:broadMatch rdf:resource="http://rds.posccaesar.org/ontology/plm/rdl/PCA_100006710"/>
    <rdfs:label>Equipment layout drawings</rdfs:label>
    <rdfs:comment>These drawings are relevant for offshore facilities and for the process plant and well pad area for onshore facilities.

At least one equipment layout drawing for each area or module deck level shall be produced. The size of the facility will determine the scale of the drawing, but normally a scale of 1:100 on A3 format shall be aimed for. If required several drawings per area can be necessary to achieve this scale. Equipment, which is covered by platforms above, shall be shown dotted or shown in separate figures. 

The following content shall be included on the drawings:
 - Platform/plant northing and orientation with respect of true north;
 - Gridlines with north and east references;
 - Key plan;
 - Scale bar;
 - Match lines with drawing references;
 - Deck/area elevations;
 - Area segregation, with fire partitions indicated;
 - Maintenance/withdrawal areas for main components (compressor bundles, cooler internals, etc.);
 - Laydown areas;
 - Waste sorting stations;
 - Pipe racks;
 - Stairs, access and escape routes;
 - Material handling routes;
 - Manifold area arrangement;
 - Well head area, with number of wells and distance between wells indicated;
 - Drilling derrick extreme outlines indicated;
 - Location of temporary well intervention equipment;
 - Flare tower location and extreme outlines indicated;
 - HVAC, instrument and electrical rooms (relevant for offshore facility);
 - Control room (relevant for offshore facility);
 - Living Quarter outline. Reference to relevant Architectural layout drawings shall be included;
 - Main structures;
 - Location of all equipment as identified in MEL including identification of datum point;
 - Equipment shall be tagged according to MEL. An equipment index shall be included on the drawing. Datum point coordinates shall be included in this index;
 - Safety evacuation equipment, such as escape tunnels, lifeboats, escape chutes, etc. (relevant for offshore facility);
 - Hose loading station and tote tank area (relevant for offshore facility);
 - Utility stations;
 - Space allocation for risers, J-tubes and umbilicals including temporary equipment (pulling arrangement). (relevant for offshore facility);
 - Space for future areas/modules/equipment.</rdfs:comment>
    <rdl:PCA_100006768>These drawings are relevant for offshore facilities and for the process plant and well pad area for onshore facilities.

At least one equipment layout drawing for each area or module deck level shall be produced. The size of the facility will determine the scale of the drawing, but normally a scale of 1:100 on A3 format shall be aimed for. If required several drawings per area can be necessary to achieve this scale. Equipment, which is covered by platforms above, shall be shown dotted or shown in separate figures. 

The following content shall be included on the drawings:
 - Platform/plant northing and orientation with respect of true north;
 - Gridlines with north and east references;
 - Key plan;
 - Scale bar;
 - Match lines with drawing references;
 - Deck/area elevations;
 - Area segregation, with fire partitions indicated;
 - Maintenance/withdrawal areas for main components (compressor bundles, cooler internals, etc.);
 - Laydown areas;
 - Waste sorting stations;
 - Pipe racks;
 - Stairs, access and escape routes;
 - Material handling routes;
 - Manifold area arrangement;
 - Well head area, with number of wells and distance between wells indicated;
 - Drilling derrick extreme outlines indicated;
 - Location of temporary well intervention equipment;
 - Flare tower location and extreme outlines indicated;
 - HVAC, instrument and electrical rooms (relevant for offshore facility);
 - Control room (relevant for offshore facility);
 - Living Quarter outline. Reference to relevant Architectural layout drawings shall be included;
 - Main structures;
 - Location of all equipment as identified in MEL including identification of datum point;
 - Equipment shall be tagged according to MEL. An equipment index shall be included on the drawing. Datum point coordinates shall be included in this index;
 - Safety evacuation equipment, such as escape tunnels, lifeboats, escape chutes, etc. (relevant for offshore facility);
 - Hose loading station and tote tank area (relevant for offshore facility);
 - Utility stations;
 - Space allocation for risers, J-tubes and umbilicals including temporary equipment (pulling arrangement). (relevant for offshore facility);
 - Space for future areas/modules/equipment.</rdl:PCA_100006768>
    <rdl:PCA_100006766 rdf:resource="http://rds.posccaesar.org/ontology/plm/rdl/PCA_100006656"/>
    <rdl:PCA_100006765 rdf:resource="http://w3id.org/readi/rdl/CFIHOS-20000020"/>
    <rdfs:subClassOf rdf:resource="http://rds.posccaesar.org/ontology/plm/rdl/PCA_100004908"/>
  </owl:Class>
  <owl:Class rdf:about="http://rds.posccaesar.org/ontology/plm/rdl/PCA_100006079">
    <skos:broadMatch rdf:resource="http://rds.posccaesar.org/ontology/plm/rdl/PCA_100006732"/>
    <skos:broadMatch rdf:resource="http://rds.posccaesar.org/ontology/plm/rdl/PCA_100006708"/>
    <rdfs:subClassOf rdf:resource="http://rds.posccaesar.org/ontology/plm/rdl/PCA_100004908"/>
    <rdl:PCA_100006765 rdf:resource="http://w3id.org/readi/rdl/CFIHOS-20000013"/>
    <rdfs:label>3D noise simulation model</rdfs:label>
    <skos:broadMatch rdf:resource="http://rds.posccaesar.org/ontology/plm/rdl/PCA_100006731"/>
    <rdl:PCA_100006765 rdf:resource="http://w3id.org/readi/rdl/CFIHOS-20000011"/>
    <skos:broader>
      <rdl:PCA_100001503 rdf:about="http://rds.posccaesar.org/ontology/plm/rdl/PCA_100006738">
        <rdfs:label>3D/CAD model</rdfs:label>
        <rdl:PCA_100004924>3D</rdl:PCA_100004924>
        <rdf:type rdf:resource="http://www.w3.org/2002/07/owl#NamedIndividual"/>
      </rdl:PCA_100001503>
    </skos:broader>
    <rdfs:comment>The Noise Simulation Model shall include all noise sources, piping and reflection from adjacent equipment and structure (walls, floor, ceiling, etc). Noise reducing measures, as absorption, noise hoods, etc. shall be included in the simulation model. The software to be used requires use of point sources, line sources, areas sources and box sources, both directly from sources and from reflections. The handover format to be agreed. All necessary files to run the model shall be handed over, including maps and/or plot plans.</rdfs:comment>
    <rdl:PCA_100006765 rdf:resource="http://w3id.org/readi/rdl/CFIHOS-20000010"/>
    <skos:broadMatch rdf:resource="http://rds.posccaesar.org/ontology/plm/rdl/PCA_100006709"/>
    <rdl:PCA_100006766 rdf:resource="http://rds.posccaesar.org/ontology/plm/rdl/PCA_100006656"/>
    <skos:broadMatch>
      <rdl:PCA_100001503 rdf:about="http://rds.posccaesar.org/ontology/plm/rdl/PCA_100006707">
        <rdfs:label>construction entity information</rdfs:label>
        <rdl:PCA_100004924>LC</rdl:PCA_100004924>
        <rdf:type rdf:resource="http://www.w3.org/2002/07/owl#NamedIndividual"/>
      </rdl:PCA_100001503>
    </skos:broadMatch>
    <rdl:PCA_100006768>The Noise Simulation Model shall include all noise sources, piping and reflection from adjacent equipment and structure (walls, floor, ceiling, etc). Noise reducing measures, as absorption, noise hoods, etc. shall be included in the simulation model. The software to be used requires use of point sources, line sources, areas sources and box sources, both directly from sources and from reflections. The handover format to be agreed. All necessary files to run the model shall be handed over, including maps and/or plot plans.</rdl:PCA_100006768>
    <skos:broadMatch rdf:resource="http://rds.posccaesar.org/ontology/plm/rdl/PCA_100006710"/>
  </owl:Class>
  <owl:Class rdf:about="http://rds.posccaesar.org/ontology/plm/rdl/PCA_100006409">
    <skos:broader rdf:resource="http://rds.posccaesar.org/ontology/plm/rdl/PCA_100006756"/>
    <rdfs:label>Ready for operation (RFO) close out report</rdfs:label>
    <rdfs:comment>All records and documents produced as a result of the monitoring and control requirements and the acceptance criteria shall, on completion of the work, be compiled into a Closeout Report.

The Closeout Report shall be divided into sections as follows:
Section 1
This section shall give an introduction, general description of the system made ready for operation, list the chemicals used and describe the purpose of - and the structure of the Closeout Report.
Section 2
This section shall contain the reports from the RFO operations. It shall contain summaries of events for all the operations and associated field operational paperwork.
Section 3
This section shall contain all the operational procedures and field queries (FQs) for the operations associated with the RFO operations.
Section 4
This section shall contain the RFO Contractors daily reports generated at the different sites where activities have been performed. These reports shall contain the day-by-day activities, , an environmental report listing the volumes of chemicals on site and a radioactive isotope form, listing the amount of isotopes in the field.</rdfs:comment>
    <rdl:PCA_100006768>All records and documents produced as a result of the monitoring and control requirements and the acceptance criteria shall, on completion of the work, be compiled into a Closeout Report.

The Closeout Report shall be divided into sections as follows:
Section 1
This section shall give an introduction, general description of the system made ready for operation, list the chemicals used and describe the purpose of - and the structure of the Closeout Report.
Section 2
This section shall contain the reports from the RFO operations. It shall contain summaries of events for all the operations and associated field operational paperwork.
Section 3
This section shall contain all the operational procedures and field queries (FQs) for the operations associated with the RFO operations.
Section 4
This section shall contain the RFO Contractors daily reports generated at the different sites where activities have been performed. These reports shall contain the day-by-day activities, , an environmental report listing the volumes of chemicals on site and a radioactive isotope form, listing the amount of isotopes in the field.</rdl:PCA_100006768>
    <rdl:PCA_100006766 rdf:resource="http://rds.posccaesar.org/ontology/plm/rdl/PCA_100006654"/>
    <rdl:PCA_100006765 rdf:resource="http://w3id.org/readi/rdl/CFIHOS-20000018"/>
    <rdl:PCA_100006763>A close out report shall be delivered to document the work performed.</rdl:PCA_100006763>
    <rdfs:subClassOf rdf:resource="http://rds.posccaesar.org/ontology/plm/rdl/PCA_100004908"/>
  </owl:Class>
  <owl:Class rdf:about="http://rds.posccaesar.org/ontology/plm/rdl/PCA_100006518">
    <rdfs:comment>For all utility systems the following shall be included in the utility consumption report:
 - For the total system:
    - Total system capacity (duty, flow rate and/or other parameter relevant for capacity);
    - Maximum coincident consumer load (duty, flow rate and/or other parameter relevant for capacity);
    - Description of utility characteristic/quality prior to distribution to consumers (pressure, temperature, composition and/or other relevant parameters);
    - Storage capacity;
 - For the consumers:
    - Tag number;
    - Continuous or intermittent consumer;
    - Required consumption, both maximum, normal and minimum consumption;
    - Description of utility characteristic/quality at consumer.</rdfs:comment>
    <rdl:PCA_100006766 rdf:resource="http://rds.posccaesar.org/ontology/plm/rdl/PCA_100006622"/>
    <rdl:PCA_100006766 rdf:resource="http://rds.posccaesar.org/ontology/plm/rdl/PCA_100006613"/>
    <rdl:PCA_100006766 rdf:resource="http://rds.posccaesar.org/ontology/plm/rdl/PCA_100006610"/>
    <rdl:PCA_100006765 rdf:resource="http://w3id.org/readi/rdl/CFIHOS-20000026"/>
    <rdl:PCA_100006766 rdf:resource="http://rds.posccaesar.org/ontology/plm/rdl/PCA_100006620"/>
    <skos:broadMatch rdf:resource="http://rds.posccaesar.org/ontology/plm/rdl/PCA_100006687"/>
    <rdl:PCA_100006768>For all utility systems the following shall be included in the utility consumption report:
 - For the total system:
    - Total system capacity (duty, flow rate and/or other parameter relevant for capacity);
    - Maximum coincident consumer load (duty, flow rate and/or other parameter relevant for capacity);
    - Description of utility characteristic/quality prior to distribution to consumers (pressure, temperature, composition and/or other relevant parameters);
    - Storage capacity;
 - For the consumers:
    - Tag number;
    - Continuous or intermittent consumer;
    - Required consumption, both maximum, normal and minimum consumption;
    - Description of utility characteristic/quality at consumer.</rdl:PCA_100006768>
    <rdl:PCA_100006766 rdf:resource="http://rds.posccaesar.org/ontology/plm/rdl/PCA_100006618"/>
    <rdl:PCA_100006766 rdf:resource="http://rds.posccaesar.org/ontology/plm/rdl/PCA_100006616"/>
    <rdl:PCA_100006766 rdf:resource="http://rds.posccaesar.org/ontology/plm/rdl/PCA_100006608"/>
    <rdl:PCA_100006766 rdf:resource="http://rds.posccaesar.org/ontology/plm/rdl/PCA_100006583"/>
    <rdl:PCA_100006766 rdf:resource="http://rds.posccaesar.org/ontology/plm/rdl/PCA_100006606"/>
    <skos:broader rdf:resource="http://rds.posccaesar.org/ontology/plm/rdl/PCA_100006756"/>
    <rdl:PCA_100006766 rdf:resource="http://rds.posccaesar.org/ontology/plm/rdl/PCA_100006623"/>
    <rdl:PCA_100006766 rdf:resource="http://rds.posccaesar.org/ontology/plm/rdl/PCA_100006604"/>
    <rdl:PCA_100006766 rdf:resource="http://rds.posccaesar.org/ontology/plm/rdl/PCA_100006628"/>
    <rdl:PCA_100006766 rdf:resource="http://rds.posccaesar.org/ontology/plm/rdl/PCA_100006614"/>
    <rdl:PCA_100006766 rdf:resource="http://rds.posccaesar.org/ontology/plm/rdl/PCA_100006621"/>
    <rdl:PCA_100006766 rdf:resource="http://rds.posccaesar.org/ontology/plm/rdl/PCA_100006611"/>
    <rdl:PCA_100006763>Input to procurement and multi-discipline design. Information to operation regarding utility system design.</rdl:PCA_100006763>
    <rdl:PCA_100006766 rdf:resource="http://rds.posccaesar.org/ontology/plm/rdl/PCA_100006624"/>
    <rdl:PCA_100006766 rdf:resource="http://rds.posccaesar.org/ontology/plm/rdl/PCA_100006609"/>
    <rdfs:subClassOf rdf:resource="http://rds.posccaesar.org/ontology/plm/rdl/PCA_100004908"/>
    <rdl:PCA_100006766 rdf:resource="http://rds.posccaesar.org/ontology/plm/rdl/PCA_100006605"/>
    <rdl:PCA_100006766 rdf:resource="http://rds.posccaesar.org/ontology/plm/rdl/PCA_100006619"/>
    <rdl:PCA_100006766 rdf:resource="http://rds.posccaesar.org/ontology/plm/rdl/PCA_100006607"/>
    <rdl:PCA_100006766 rdf:resource="http://rds.posccaesar.org/ontology/plm/rdl/PCA_100006627"/>
    <rdfs:label>Utility consumption report</rdfs:label>
    <rdl:PCA_100006766 rdf:resource="http://rds.posccaesar.org/ontology/plm/rdl/PCA_100006612"/>
    <rdl:PCA_100006766 rdf:resource="http://rds.posccaesar.org/ontology/plm/rdl/PCA_100006617"/>
    <rdl:PCA_100006766 rdf:resource="http://rds.posccaesar.org/ontology/plm/rdl/PCA_100006625"/>
    <rdl:PCA_100006766 rdf:resource="http://rds.posccaesar.org/ontology/plm/rdl/PCA_100006615"/>
  </owl:Class>
  <owl:Class rdf:about="http://rds.posccaesar.org/ontology/plm/rdl/PCA_100006506">
    <rdl:PCA_100006763>To give input to the design of a structure or assembly including seafastening.</rdl:PCA_100006763>
    <rdl:PCA_100006768>A report providing the results from sea transport analysis of a structure or equipment assembly.</rdl:PCA_100006768>
    <rdfs:subClassOf rdf:resource="http://rds.posccaesar.org/ontology/plm/rdl/PCA_100004908"/>
    <rdfs:comment>A report providing the results from sea transport analysis of a structure or equipment assembly.</rdfs:comment>
    <rdl:PCA_100006765 rdf:resource="http://w3id.org/readi/rdl/CFIHOS-20000031"/>
    <rdfs:label>Transportation analysis report</rdfs:label>
    <skos:broader rdf:resource="http://rds.posccaesar.org/ontology/plm/rdl/PCA_100006756"/>
    <skos:broadMatch rdf:resource="http://rds.posccaesar.org/ontology/plm/rdl/PCA_100006668"/>
    <rdl:PCA_100006766 rdf:resource="http://rds.posccaesar.org/ontology/plm/rdl/PCA_100006653"/>
  </owl:Class>
  <owl:Class rdf:about="http://rds.posccaesar.org/ontology/plm/rdl/PCA_100006291">
    <skos:broader rdf:resource="http://rds.posccaesar.org/ontology/plm/rdl/PCA_100006746"/>
    <skos:broadMatch rdf:resource="http://rds.posccaesar.org/ontology/plm/rdl/PCA_100006732"/>
    <rdfs:label>Isolating component drawings</rdfs:label>
    <rdfs:comment>Drawings of isolating components shall cover material, geometry, dimensions, coating, location of electrical insulating materials for items such as, but not limited to, supports, casings and spacers.</rdfs:comment>
    <rdl:PCA_100006768>Drawings of isolating components shall cover material, geometry, dimensions, coating, location of electrical insulating materials for items such as, but not limited to, supports, casings and spacers.</rdl:PCA_100006768>
    <rdl:PCA_100006766 rdf:resource="http://rds.posccaesar.org/ontology/plm/rdl/PCA_100006657"/>
    <rdl:PCA_100006765 rdf:resource="http://w3id.org/readi/rdl/CFIHOS-20000018"/>
    <rdfs:subClassOf rdf:resource="http://rds.posccaesar.org/ontology/plm/rdl/PCA_100004908"/>
  </owl:Class>
  <owl:Class rdf:about="http://rds.posccaesar.org/ontology/plm/rdl/PCA_100006151">
    <rdfs:subClassOf rdf:resource="http://rds.posccaesar.org/ontology/plm/rdl/PCA_100004908"/>
    <rdfs:comment>The DEH rating report shall give the electrical and thermal rating of the DEH system. Parameters such as current, voltage, system impedance and power are to be calculated for all design modes. Similarly, the thermal performance shall be documented for both steady state and transient conditions.</rdfs:comment>
    <rdl:PCA_100006763>Documentation of ratings</rdl:PCA_100006763>
    <skos:broader rdf:resource="http://rds.posccaesar.org/ontology/plm/rdl/PCA_100006756"/>
    <rdl:PCA_100006765 rdf:resource="http://w3id.org/readi/rdl/CFIHOS-20000018"/>
    <rdl:PCA_100006766 rdf:resource="http://rds.posccaesar.org/ontology/plm/rdl/PCA_100006657"/>
    <skos:broadMatch rdf:resource="http://rds.posccaesar.org/ontology/plm/rdl/PCA_100006686"/>
    <rdfs:label>DEH rating report</rdfs:label>
    <rdl:PCA_100006768>The DEH rating report shall give the electrical and thermal rating of the DEH system. Parameters such as current, voltage, system impedance and power are to be calculated for all design modes. Similarly, the thermal performance shall be documented for both steady state and transient conditions.</rdl:PCA_100006768>
  </owl:Class>
  <owl:Class rdf:about="http://rds.posccaesar.org/ontology/plm/rdl/PCA_100006163">
    <rdl:PCA_100006768>A procedure describing the dimensional control methods for different equipment.</rdl:PCA_100006768>
    <rdl:PCA_100006763>Provide clear instructions for how to perform dimensional control including acceptance criteria and reporting.</rdl:PCA_100006763>
    <rdfs:comment>A procedure describing the dimensional control methods for different equipment.</rdfs:comment>
    <rdfs:label>Dimensional control procedure</rdfs:label>
    <rdfs:subClassOf rdf:resource="http://rds.posccaesar.org/ontology/plm/rdl/PCA_100004908"/>
    <rdl:PCA_100006766 rdf:resource="http://rds.posccaesar.org/ontology/plm/rdl/PCA_100006653"/>
    <skos:broadMatch rdf:resource="http://rds.posccaesar.org/ontology/plm/rdl/PCA_100006688"/>
    <rdl:PCA_100006765 rdf:resource="http://w3id.org/readi/rdl/CFIHOS-20000031"/>
    <skos:broader rdf:resource="http://rds.posccaesar.org/ontology/plm/rdl/PCA_100006751"/>
  </owl:Class>
  <owl:Class rdf:about="http://rds.posccaesar.org/ontology/plm/rdl/PCA_100006175">
    <skos:broader rdf:resource="http://rds.posccaesar.org/ontology/plm/rdl/PCA_100006745"/>
    <skos:broadMatch rdf:resource="http://rds.posccaesar.org/ontology/plm/rdl/PCA_100006712"/>
    <skos:broadMatch rdf:resource="http://rds.posccaesar.org/ontology/plm/rdl/PCA_100006702"/>
    <rdfs:label>Electrical connection and wiring diagram - instrument</rdfs:label>
    <rdl:PCA_100006765 rdf:resource="http://w3id.org/readi/rdl/CFIHOS-20000008"/>
    <rdl:PCA_100006764>The equipment supplier standard drawing to be delivered. The external connection diagram should typically include:
 - Terminal/pin number
 - Earthing details 
Internal wiring diagrams shall be supplied when relevant e.g. to show the wiring between different electrical equipment within a package, and should typically include: 
 - Terminal block/socket number
 - Terminal/pin number (including spares)
 - Internal cable numbers with pair and core colour details
 - Destination for internal cables
 - Earthing details
 - Equipment and equipment connections
 - External cables with pair and core colour details</rdl:PCA_100006764>
    <rdfs:subClassOf rdf:resource="http://rds.posccaesar.org/ontology/plm/rdl/PCA_100004908"/>
  </owl:Class>
  <owl:Class rdf:about="http://rds.posccaesar.org/ontology/plm/rdl/PCA_100006187">
    <rdfs:comment>An equipment specific procedure providing the steps for installation and retrieval including limitations.</rdfs:comment>
    <rdfs:subClassOf rdf:resource="http://rds.posccaesar.org/ontology/plm/rdl/PCA_100004908"/>
    <rdfs:label>Equipment installation &amp; retrieval procedure</rdfs:label>
    <rdl:PCA_100006766 rdf:resource="http://rds.posccaesar.org/ontology/plm/rdl/PCA_100006653"/>
    <skos:broadMatch rdf:resource="http://rds.posccaesar.org/ontology/plm/rdl/PCA_100006688"/>
    <rdl:PCA_100006768>An equipment specific procedure providing the steps for installation and retrieval including limitations.</rdl:PCA_100006768>
    <skos:broader rdf:resource="http://rds.posccaesar.org/ontology/plm/rdl/PCA_100006751"/>
    <rdl:PCA_100006763>To give the installer instruction for installation of the equipment subsea.</rdl:PCA_100006763>
    <rdl:PCA_100006765 rdf:resource="http://w3id.org/readi/rdl/CFIHOS-20000031"/>
  </owl:Class>
  <owl:Class rdf:about="http://rds.posccaesar.org/ontology/plm/rdl/PCA_100006199">
    <rdl:PCA_100006768>This document shall include all testing activities and their acceptance criteria according to applicable standards, specifications and requirements,. to document the condition of the equipment as tested from factory. Test set-up and test equipment shall be defined. 

Suppliers standard (routine) test procedures should be used as far as possible</rdl:PCA_100006768>
    <rdfs:subClassOf rdf:resource="http://rds.posccaesar.org/ontology/plm/rdl/PCA_100004908"/>
    <rdfs:label>Factory acceptance test (FAT) procedures</rdfs:label>
    <rdfs:comment>This document shall include all testing activities and their acceptance criteria according to applicable standards, specifications and requirements,. to document the condition of the equipment as tested from factory. Test set-up and test equipment shall be defined. 

Suppliers standard (routine) test procedures should be used as far as possible</rdfs:comment>
    <rdl:PCA_100006766 rdf:resource="http://rds.posccaesar.org/ontology/plm/rdl/PCA_100006653"/>
    <skos:broadMatch rdf:resource="http://rds.posccaesar.org/ontology/plm/rdl/PCA_100006722"/>
    <skos:broader rdf:resource="http://rds.posccaesar.org/ontology/plm/rdl/PCA_100006751"/>
    <rdl:PCA_100006765>
      <rdl:PCA_100001503 rdf:about="http://w3id.org/readi/rdl/CFIHOS-20000027">
        <rdfs:label>quality management</rdfs:label>
        <rdl:PCA_100004924>QA</rdl:PCA_100004924>
        <rdf:type rdf:resource="http://www.w3.org/2002/07/owl#NamedIndividual"/>
      </rdl:PCA_100001503>
    </rdl:PCA_100006765>
    <rdl:PCA_100006763>The FAT procedure will be used to ensure a common understanding of performed testing and acceptance criteria.</rdl:PCA_100006763>
  </owl:Class>
  <owl:Class rdf:about="http://rds.posccaesar.org/ontology/plm/rdl/PCA_100006078">
    <skos:broader rdf:resource="http://rds.posccaesar.org/ontology/plm/rdl/PCA_100006738"/>
    <skos:broadMatch rdf:resource="http://rds.posccaesar.org/ontology/plm/rdl/PCA_100006710"/>
    <rdl:PCA_100006763>The documentation enabling visualisation of design and easier verification of design, dimensions, space (envelopes) and interfaces.</rdl:PCA_100006763>
    <skos:broadMatch rdf:resource="http://rds.posccaesar.org/ontology/plm/rdl/PCA_100006732"/>
    <rdfs:label>3D CAD model - offshore, onshore and subsea</rdfs:label>
    <skos:broadMatch rdf:resource="http://rds.posccaesar.org/ontology/plm/rdl/PCA_100006731"/>
    <rdl:PCA_100006768>The 3D model shall be prepared according to Company's requirements.</rdl:PCA_100006768>
    <rdl:PCA_100006764>The model must be complete in order to check interface and possible interference with other equipments. All final dimensions and external geometry must be defined in the 3D model. Weight and center of gravity shall be defined in the 3D model and in the assembly drawing.</rdl:PCA_100006764>
    <rdfs:comment>The 3D model shall be prepared according to Company's requirements.</rdfs:comment>
    <skos:broadMatch rdf:resource="http://rds.posccaesar.org/ontology/plm/rdl/PCA_100006709"/>
    <rdl:PCA_100006766 rdf:resource="http://rds.posccaesar.org/ontology/plm/rdl/PCA_100006656"/>
    <rdfs:subClassOf rdf:resource="http://rds.posccaesar.org/ontology/plm/rdl/PCA_100004908"/>
    <skos:broadMatch rdf:resource="http://rds.posccaesar.org/ontology/plm/rdl/PCA_100006707"/>
    <skos:broadMatch rdf:resource="http://rds.posccaesar.org/ontology/plm/rdl/PCA_100006708"/>
  </owl:Class>
  <owl:Class rdf:about="http://rds.posccaesar.org/ontology/plm/rdl/PCA_100006507">
    <rdl:PCA_100006766 rdf:resource="http://rds.posccaesar.org/ontology/plm/rdl/PCA_100006654"/>
    <rdl:PCA_100006763>Basis for analysis, assumptions and assessments not given in design basis shall be included.</rdl:PCA_100006763>
    <rdfs:label>Trawl interference design report</rdfs:label>
    <skos:broadMatch rdf:resource="http://rds.posccaesar.org/ontology/plm/rdl/PCA_100006686"/>
    <rdfs:subClassOf rdf:resource="http://rds.posccaesar.org/ontology/plm/rdl/PCA_100004908"/>
    <rdfs:comment>More details Design report covering trawl impact, hooking and pull-over assessment and performed analyses.</rdfs:comment>
    <rdl:PCA_100006768>More details Design report covering trawl impact, hooking and pull-over assessment and performed analyses.</rdl:PCA_100006768>
    <skos:broader rdf:resource="http://rds.posccaesar.org/ontology/plm/rdl/PCA_100006756"/>
    <rdl:PCA_100006765 rdf:resource="http://w3id.org/readi/rdl/CFIHOS-20000018"/>
  </owl:Class>
  <owl:Class rdf:about="http://rds.posccaesar.org/ontology/plm/rdl/PCA_100006519">
    <rdl:PCA_100006765>
      <rdl:PCA_100001503 rdf:about="http://w3id.org/readi/rdl/CFIHOS-20000022">
        <rdfs:label>mechanical static engineering</rdfs:label>
        <rdl:PCA_100004924>MS</rdl:PCA_100004924>
        <rdf:type rdf:resource="http://www.w3.org/2002/07/owl#NamedIndividual"/>
      </rdl:PCA_100001503>
    </rdl:PCA_100006765>
    <rdl:PCA_100006763>This document shall support verification of component function according to company/project requirements, Information to be used into system engineering.</rdl:PCA_100006763>
    <rdl:PCA_100006766 rdf:resource="http://rds.posccaesar.org/ontology/plm/rdl/PCA_100006653"/>
    <skos:broader rdf:resource="http://rds.posccaesar.org/ontology/plm/rdl/PCA_100006741"/>
    <rdfs:subClassOf rdf:resource="http://rds.posccaesar.org/ontology/plm/rdl/PCA_100004908"/>
    <rdfs:label>Valve and operator calculations</rdfs:label>
    <skos:broadMatch rdf:resource="http://rds.posccaesar.org/ontology/plm/rdl/PCA_100006687"/>
    <rdl:PCA_100006768>Characteristics and functional parameters shall be documented and performance shall be shown to be probable. This shall include but not be limited to calculations, curves, tables, reference to similar applications and test data. This shall as a minimum be at a level customary for the equipment and to the extent such data are of importance for interfaces to plant and system.

Valve and actuator should include: 
-Torque table showing safety factor for: Break to close ,run to close , end to close, break to open, run to open &amp; end to open. 
-The table shall include Maximum Allowable Valve Input Torque (MAVIT).                      
-Manufacturers standard calculation report can be used
-Capacity calculations, Noise calculations,</rdl:PCA_100006768>
    <rdfs:comment>Characteristics and functional parameters shall be documented and performance shall be shown to be probable. This shall include but not be limited to calculations, curves, tables, reference to similar applications and test data. This shall as a minimum be at a level customary for the equipment and to the extent such data are of importance for interfaces to plant and system.

Valve and actuator should include: 
-Torque table showing safety factor for: Break to close ,run to close , end to close, break to open, run to open &amp; end to open. 
-The table shall include Maximum Allowable Valve Input Torque (MAVIT).                      
-Manufacturers standard calculation report can be used
-Capacity calculations, Noise calculations,</rdfs:comment>
  </owl:Class>
  <owl:Class rdf:about="http://rds.posccaesar.org/ontology/plm/rdl/PCA_100006292">
    <skos:broader rdf:resource="http://rds.posccaesar.org/ontology/plm/rdl/PCA_100006746"/>
    <skos:broadMatch rdf:resource="http://rds.posccaesar.org/ontology/plm/rdl/PCA_100006732"/>
    <rdfs:label>Landfall construction drawings</rdfs:label>
    <rdfs:comment>Documentation for construction done according to design</rdfs:comment>
    <rdl:PCA_100006768>Documentation for construction done according to design</rdl:PCA_100006768>
    <rdl:PCA_100006766 rdf:resource="http://rds.posccaesar.org/ontology/plm/rdl/PCA_100006657"/>
    <rdl:PCA_100006765 rdf:resource="http://w3id.org/readi/rdl/CFIHOS-20000018"/>
    <rdfs:subClassOf rdf:resource="http://rds.posccaesar.org/ontology/plm/rdl/PCA_100004908"/>
  </owl:Class>
  <owl:Class rdf:about="http://rds.posccaesar.org/ontology/plm/rdl/PCA_100006150">
    <skos:broadMatch rdf:resource="http://rds.posccaesar.org/ontology/plm/rdl/PCA_100006688"/>
    <rdl:PCA_100006768>Proposed maintenance interval and method is to be outlined. In addition, the document shall describe the repair philosophy for the cables with illustrating sketches.</rdl:PCA_100006768>
    <rdl:PCA_100006763>The document shall describe all inspection and maintenance to be performed to the DEH equipment to ensure safe, reliable and economical operation.</rdl:PCA_100006763>
    <rdfs:comment>Proposed maintenance interval and method is to be outlined. In addition, the document shall describe the repair philosophy for the cables with illustrating sketches.</rdfs:comment>
    <rdfs:subClassOf rdf:resource="http://rds.posccaesar.org/ontology/plm/rdl/PCA_100004908"/>
    <rdl:PCA_100006765 rdf:resource="http://w3id.org/readi/rdl/CFIHOS-20000018"/>
    <rdl:PCA_100006766 rdf:resource="http://rds.posccaesar.org/ontology/plm/rdl/PCA_100006657"/>
    <rdfs:label>DEH maintenance and repair procedure</rdfs:label>
    <skos:broader rdf:resource="http://rds.posccaesar.org/ontology/plm/rdl/PCA_100006751"/>
  </owl:Class>
  <owl:Class rdf:about="http://rds.posccaesar.org/ontology/plm/rdl/PCA_100006280">
    <rdl:PCA_100006766 rdf:resource="http://rds.posccaesar.org/ontology/plm/rdl/PCA_100006657"/>
    <rdl:PCA_100006768>IOM manual requirements:
 - The equipment manufacturers standard IOM manual shall be delivered.
 - For assemblies/skids/packages an IOM manual covering the complete assembly shall be delivered.
 - An IOM manual shall as a minimum include the following information:

Introduction
 - The Vendor’s address, telephone no., e-mail and web addresses
 - Subcontractor’s address, telephone no., e-mail and web addresses

Main Data
Information for the complete equipment showing all data necessary for the understanding of the equipment's mode of operation shall be given. Information regarding health, environment and safety shall be emphasized. Other data may be:
 - restrictions in guarantee;
 - performance data;
 - restrictions in use;
 - main connections and requirements on connected systems;
 - weight and outline dimensions.

Technical description
Design and function shall be described to facilitate a better understanding of the different parts of the operating and maintenance instructions. If the complete equipment package consists of several systems, the main system should be described first, followed by descriptions of each subsystem and their interconnections.

Preparations
All preparations to be made from the moment the installation is completed until the equipment is ready for normal operation shall be described. The description shall include tests, adjustments, calibrations and necessary inspections. The sequence of the activities shall be stated as well as all tools, auxiliary equipment, consumables and spare parts that may be needed. If necessary, references to detailed technical information (e.g. performance and operational data) in other parts of the manual shall be made.

Disturbance of operation
Description of the various forms of disturbance of operation that may occur, how they can be identified and the consequences they may have for the operation, shall be given.

Corrective measures
A description shall be available of the necessary actions after a disturbance has occurred. For actions which cannot be taken by the operator, it may be necessary to refer to the maintenance instructions. The manual shall state all requirements for reports to the supplier in the form of registrations and observations.

Hazards and protective measures
A description shall be given of all known hazards that may occur during operation. This also applies to hazards which are due to lack of observation of the supplier's procedures as well as to external causes, e. g. lack of cooling water, loss of electrical power, etc. The manual shall give detailed information about protective measures, how to reduce the consequences to a minimum and what procedures to follow in the event of an accident. Product data sheets for chemical substances shall be attached.

Qualification requirements and training program for operators
The supplier shall state the qualifications required of the operator and the training programs that can be offered.


Maintenance

General
Maintenance includes all inspections, measurements, adjustments and operations carried out directly on the equipment in order to ensure safe, reliable and economical operation. Maintenance documentation shall cover the maintenance which can normally be done by the user and the maintenance which is not expected to be done by the user. If the maintenance documentation shall be the basis of a maintenance system for the complete plant where the equipment is a part, then the customer shall state all necessary information and specify all special requests in the inquiry and order documentation.

Structure and contents of operating instructions
Instructions should contain a minimum of elements and shall be constructed as follows:
1.introduction, scope and possible limitations of the instruction;
2.a list of drawings or other necessary supplementary documentation;
3.necessary safety precautions before and during maintenance;
4.detailed description of the procedure to be followed with references to relevant supplementary documentation;
5.necessary data and arrangement for lifting;
6.list of necessary tools and equipment;
7.recommended spare parts and consumables;
8.control and measurement points with limits during maintenance and after completion prior to restart;
9.requirements for special skills and minimum crew for the maintenance;
10.registrations which should be part of a specially defined maintenance log.

Maintenance instructions
These shall be divided into the following separate instructions:

Routine inspection
This part of the maintenance consists of the regular inspections carried out by the operation and/or maintenance personnel. The inspections consist of what can be measured, seen, heard or felt without interference in the equipment both during an operation and while at standstill. The supplier shall give instructions concerning inspection points based on his own experience and the selected monitoring system.

Periodic maintenance
It shall cover all planned and expected maintenance based on operation time, calendar time or certain operational observations. This type of maintenance may e.g. include:
 - cleaning;
 - lubrication schedule;
 - adjustments;
 - calibrations;
 - replacement of wear parts;
 - replenishments.

Corrections and minor repairs
The most comprehensive maintenance possible on site shall be described under this clause, e.g.:
 - replacement of broken parts;
 - repairs which can be done on site or in a normally equipped maintenance shop;
 - dismantling parts of or the whole equipment for shipment to a special repair or overhaul shop.

Major repairs and modifications
It is not normally required that this shall be covered by the instructions at the user's disposal. However, the supplier shall keep and upon request provide instructions concerning overhaul and repairs at special shops. If agreed, the supplier shall also keep all documentation for modification or rebuilding of the equipment.</rdl:PCA_100006768>
    <rdl:PCA_100006765 rdf:resource="http://w3id.org/readi/rdl/CFIHOS-20000018"/>
    <rdfs:label>Installation, operation and maintenance manual (IOM manual) for CP</rdfs:label>
    <rdfs:subClassOf rdf:resource="http://rds.posccaesar.org/ontology/plm/rdl/PCA_100004908"/>
    <rdl:PCA_100006763>Ensure safe and efficient operation</rdl:PCA_100006763>
    <skos:broader rdf:resource="http://rds.posccaesar.org/ontology/plm/rdl/PCA_100006751"/>
    <rdfs:comment>IOM manual requirements:
 - The equipment manufacturers standard IOM manual shall be delivered.
 - For assemblies/skids/packages an IOM manual covering the complete assembly shall be delivered.
 - An IOM manual shall as a minimum include the following information:

Introduction
 - The Vendor’s address, telephone no., e-mail and web addresses
 - Subcontractor’s address, telephone no., e-mail and web addresses

Main Data
Information for the complete equipment showing all data necessary for the understanding of the equipment's mode of operation shall be given. Information regarding health, environment and safety shall be emphasized. Other data may be:
 - restrictions in guarantee;
 - performance data;
 - restrictions in use;
 - main connections and requirements on connected systems;
 - weight and outline dimensions.

Technical description
Design and function shall be described to facilitate a better understanding of the different parts of the operating and maintenance instructions. If the complete equipment package consists of several systems, the main system should be described first, followed by descriptions of each subsystem and their interconnections.

Preparations
All preparations to be made from the moment the installation is completed until the equipment is ready for normal operation shall be described. The description shall include tests, adjustments, calibrations and necessary inspections. The sequence of the activities shall be stated as well as all tools, auxiliary equipment, consumables and spare parts that may be needed. If necessary, references to detailed technical information (e.g. performance and operational data) in other parts of the manual shall be made.

Disturbance of operation
Description of the various forms of disturbance of operation that may occur, how they can be identified and the consequences they may have for the operation, shall be given.

Corrective measures
A description shall be available of the necessary actions after a disturbance has occurred. For actions which cannot be taken by the operator, it may be necessary to refer to the maintenance instructions. The manual shall state all requirements for reports to the supplier in the form of registrations and observations.

Hazards and protective measures
A description shall be given of all known hazards that may occur during operation. This also applies to hazards which are due to lack of observation of the supplier's procedures as well as to external causes, e. g. lack of cooling water, loss of electrical power, etc. The manual shall give detailed information about protective measures, how to reduce the consequences to a minimum and what procedures to follow in the event of an accident. Product data sheets for chemical substances shall be attached.

Qualification requirements and training program for operators
The supplier shall state the qualifications required of the operator and the training programs that can be offered.


Maintenance

General
Maintenance includes all inspections, measurements, adjustments and operations carried out directly on the equipment in order to ensure safe, reliable and economical operation. Maintenance documentation shall cover the maintenance which can normally be done by the user and the maintenance which is not expected to be done by the user. If the maintenance documentation shall be the basis of a maintenance system for the complete plant where the equipment is a part, then the customer shall state all necessary information and specify all special requests in the inquiry and order documentation.

Structure and contents of operating instructions
Instructions should contain a minimum of elements and shall be constructed as follows:
1.introduction, scope and possible limitations of the instruction;
2.a list of drawings or other necessary supplementary documentation;
3.necessary safety precautions before and during maintenance;
4.detailed description of the procedure to be followed with references to relevant supplementary documentation;
5.necessary data and arrangement for lifting;
6.list of necessary tools and equipment;
7.recommended spare parts and consumables;
8.control and measurement points with limits during maintenance and after completion prior to restart;
9.requirements for special skills and minimum crew for the maintenance;
10.registrations which should be part of a specially defined maintenance log.

Maintenance instructions
These shall be divided into the following separate instructions:

Routine inspection
This part of the maintenance consists of the regular inspections carried out by the operation and/or maintenance personnel. The inspections consist of what can be measured, seen, heard or felt without interference in the equipment both during an operation and while at standstill. The supplier shall give instructions concerning inspection points based on his own experience and the selected monitoring system.

Periodic maintenance
It shall cover all planned and expected maintenance based on operation time, calendar time or certain operational observations. This type of maintenance may e.g. include:
 - cleaning;
 - lubrication schedule;
 - adjustments;
 - calibrations;
 - replacement of wear parts;
 - replenishments.

Corrections and minor repairs
The most comprehensive maintenance possible on site shall be described under this clause, e.g.:
 - replacement of broken parts;
 - repairs which can be done on site or in a normally equipped maintenance shop;
 - dismantling parts of or the whole equipment for shipment to a special repair or overhaul shop.

Major repairs and modifications
It is not normally required that this shall be covered by the instructions at the user's disposal. However, the supplier shall keep and upon request provide instructions concerning overhaul and repairs at special shops. If agreed, the supplier shall also keep all documentation for modification or rebuilding of the equipment.</rdfs:comment>
    <skos:broadMatch rdf:resource="http://rds.posccaesar.org/ontology/plm/rdl/PCA_100006688"/>
  </owl:Class>
  <owl:Class rdf:about="http://rds.posccaesar.org/ontology/plm/rdl/PCA_100006162">
    <rdl:PCA_100006765 rdf:resource="http://w3id.org/readi/rdl/CFIHOS-20000031"/>
    <skos:broader>
      <rdl:PCA_100001503 rdf:about="http://rds.posccaesar.org/ontology/plm/rdl/PCA_100006749">
        <rdfs:label>Manuals</rdfs:label>
        <rdl:PCA_100004924>MA</rdl:PCA_100004924>
        <rdf:type rdf:resource="http://www.w3.org/2002/07/owl#NamedIndividual"/>
      </rdl:PCA_100001503>
    </skos:broader>
    <rdfs:subClassOf rdf:resource="http://rds.posccaesar.org/ontology/plm/rdl/PCA_100004908"/>
    <rdl:PCA_100006763>The Design, Fabrication and Installation (DFI) resumés shall provide Operations with a general summary of the installation based on the most relevant information from the design, fabrication and installation phases, and contain information required for plant integrity management and maintenance planning of the facilities throughout the entire lifetime of the installation.

The document shall also serve as an aid in the consideration of measures to be taken if the condition monitoring reveals that the installation is damaged or deviates from the acceptance criteria.</rdl:PCA_100006763>
    <rdl:PCA_100006768>DFI resumes shall be produced in English and in accordance with this standard. The requirement for DFI resume applies to all locations.

Independent resumes to be made for each major unit or system of the installation, dependant of size and complexity. The Contractor shall incorporate relevant material from their sub-contractors. 

The Fabrication- and Installation-parts shall mainly concentrate on non-conformances from design/fabrication criteria, specifications, etc. Further, areas should be highlighted where special attention in the operational phase is recommended due to e.g. difficult repairs, unexpected large loads or other unforeseen events. Only a brief description of the work performed shall be included.

Information of foundation performance during installation being relevant for lifetime extension and/or removal shall be included. The required information will depend on foundation system (e.g. pile driving records, suction during penetration, drag lengths vs. tension, penetration during pre-loading).

DFI resumés shall be prepared for:
 - Load bearing structures, such as: Jackets, Gravity Based Structures, Tension Leg Platforms, Semi submersibles, Ships, Jack-Ups, Spars, Subsea structures, Module Support Frames, Modules, Living quarters, Integrated Topsides, Derricks, Flares, Riser support systems and Mooring systems.
 - Pipeline System, including submarine and connected onshore pipelines and risers transporting hydrocarbons and other commodities, with associated safety systems, valves, tool launchers/receivers, internal and external corrosion protection systems, other accessory equipment, and all applied intervention works.</rdl:PCA_100006768>
    <rdl:PCA_100006766 rdf:resource="http://rds.posccaesar.org/ontology/plm/rdl/PCA_100006653"/>
    <rdfs:label>DFI resumes</rdfs:label>
    <rdl:PCA_100006765>
      <rdl:PCA_100001503 rdf:about="http://w3id.org/readi/rdl/CFIHOS-20000006">
        <rdfs:label>structural engineering</rdfs:label>
        <rdl:PCA_100004924>CS</rdl:PCA_100004924>
        <rdf:type rdf:resource="http://www.w3.org/2002/07/owl#NamedIndividual"/>
      </rdl:PCA_100001503>
    </rdl:PCA_100006765>
    <rdfs:comment>DFI resumes shall be produced in English and in accordance with this standard. The requirement for DFI resume applies to all locations.

Independent resumes to be made for each major unit or system of the installation, dependant of size and complexity. The Contractor shall incorporate relevant material from their sub-contractors. 

The Fabrication- and Installation-parts shall mainly concentrate on non-conformances from design/fabrication criteria, specifications, etc. Further, areas should be highlighted where special attention in the operational phase is recommended due to e.g. difficult repairs, unexpected large loads or other unforeseen events. Only a brief description of the work performed shall be included.

Information of foundation performance during installation being relevant for lifetime extension and/or removal shall be included. The required information will depend on foundation system (e.g. pile driving records, suction during penetration, drag lengths vs. tension, penetration during pre-loading).

DFI resumés shall be prepared for:
 - Load bearing structures, such as: Jackets, Gravity Based Structures, Tension Leg Platforms, Semi submersibles, Ships, Jack-Ups, Spars, Subsea structures, Module Support Frames, Modules, Living quarters, Integrated Topsides, Derricks, Flares, Riser support systems and Mooring systems.
 - Pipeline System, including submarine and connected onshore pipelines and risers transporting hydrocarbons and other commodities, with associated safety systems, valves, tool launchers/receivers, internal and external corrosion protection systems, other accessory equipment, and all applied intervention works.</rdfs:comment>
  </owl:Class>
  <owl:Class rdf:about="http://rds.posccaesar.org/ontology/plm/rdl/PCA_100006174">
    <rdl:PCA_100006766 rdf:resource="http://rds.posccaesar.org/ontology/plm/rdl/PCA_100006639"/>
    <rdl:PCA_100006763>Electrical calculations / analyses are required to be done according to IEC 61892-2 to confirm the design of the electrical system and corresponding ratings of the equipment:

General EMC planning shall be in accordance with IEC 60533, Annex B(Offshore) or IEC 61000-2-5 (onshore).

Arc flash study is required to be done according to IEEE Std 1584 to calculate arc incident energy.</rdl:PCA_100006763>
    <rdl:PCA_100006766 rdf:resource="http://rds.posccaesar.org/ontology/plm/rdl/PCA_100006638"/>
    <skos:broadMatch rdf:resource="http://rds.posccaesar.org/ontology/plm/rdl/PCA_100006687"/>
    <skos:broader rdf:resource="http://rds.posccaesar.org/ontology/plm/rdl/PCA_100006741"/>
    <rdl:PCA_100006764>The following studies are required to be done:
 - Electrical load study:
     - The electrical load study shall be done to determine major equipment ratings.
     - An allowance and contingency multiplication factor shall be applied to the estimated load to select the rating of generators and transformers.
 - Load flow calculations:
     - Load flow calculations shall be done to check the voltage profile and circuit loading under steady state conditions. Calculations shall include:
     - All general modes (such as main power mode, essential mode, emergency mode).
           - Different network configuration (such as open bus tie breaker, closed bus tie breaker with single incomer supply).
           - Different load scenarios (maximum load, no load).
 - Short circuit analysis calculations:
     - Short circuit calculations shall be done to determine maximum stresses during fault conditions. The results shall be used for specifying equipment ratings and to determine setting of protection.
 - Protection and discrimination study:
     - The protection and discrimination study shall be done to provide correct protection and discrimination.
     - The study shall include the following main subjects:
           - Network description.
           - Short overview of plant, with a subchapter per voltage level and system.
           - Operational modes description.
           - Full production mode, drilling mode, essential mode, emergency mode, UPS mode.
           - Protection relays and functions per circuit type.
           - Description of each individual protective device for the plant.
           - Fuse selection.
           - Fuse selection criteria, short circuit protection of consumer and contactor in starter/feeder, starting current versus starting time, load current and overload protection.
           - Protection principles.
           - Protection principles per system and operational mode.
           - This to include phase-phase faults and phase-earth faults in separate subsections.
           - Coordination of earth fault relays with different operating characteristic to be handled especially.
           - Protection principles per equipment type (equipment protection).
           - Protection relay templates.
           - Template per make/type of protection and per type of equipment to be protected.
           - Setting tables.
           - All individual setting parameters to be included. This shall also include protective relay settings on mechanical packages (e.g. firefighting system).
           - Current - time diagrams.
           - Logarithms current versus time curves (for visually documenting selectivity in the system and proper protection of equipment and cables).
           - All cases where curves indicate conflict with defined principles or criteria shall be explained.
 - Power system dynamic study:
     - The dynamic study shall be done to analyse the transient and dynamic performance of the power system.
     - Calculations shall include (as applicable) the dynamic performance when:
           - Starting/ energising largest motor/ consumer at each main switchboard.
           - Stopping/deenergising the largest possible group of consumers (due to e.g. process shut down).
           - Trip of one generator (or power source), with and without load shedding.
           - Short circuit in the primary distribution system, cleared by short circuit protection.
           - Other as required.
           - Calculations shall be done for different preconditions as follows:
           - All power modes (such as main power mode, essential mode, emergency mode, testing of the essential and emergency generator).
           - Different network configuration (especially those giving the extreme dynamic disturbance conditions).
 - Calculations of harmonic voltages:
     - Calculations shall be done to verify that harmonic distortions in all operating modes are within defined limitations.
 - Switching/equipment insulation study:
     - A switching/equipment insulation study shall when necessary be performed in order to specify the correct equipment insulation levels and to determine whether additional protections are required.
 - Electromagnetic compatibility (EMC):
 
     - The above referred standards as well as the manufacturer’s and supplier’s instructions with regards to EMC shall be followed and taken into account in the design.
 - Cable selection and sizing criteria:
     - An electrical cable sizing study shall be performed in order to establish cable sizing criteria.
     - The following subjects shall be taken into account when making general cable sizing criteria:
           - Consumer/ circuit nominal current.
           - Motor start current (motor circuits).
           - For voltage drop from generator terminals (in primary distribution system) or transformer secondary terminals (in secondary distribution system), stationary and transient.
           - Cables’ short circuits withstand capabilities (both mechanical and thermal). To be coordinated with short circuit protection.
           - Short circuit (phase to phase) at the end of the power cable supplying small power and lighting should cause instantaneous trip of the protective device.
           - The type of cable to be used for each purpose and area shall be fully described (e.g. mud/oil resistant, fire resistant etc.).
           - Current ratings for cables and de-rating factors for ambient temperature and cable grouping.
           - The study shall as a minimum summarise the following results:
                 - Cable current capacity (maximum current) per type and size of cable.
                 
Studies shall be done according to relevant IEC standards and more detailed company specific requirements. 

If electrical power system design and simulation software is used, all modified or new files shall be transferred to Company as files of the software that is used. The report from the system study shall be delivered as a text file.</rdl:PCA_100006764>
    <rdl:PCA_100006765 rdf:resource="http://w3id.org/readi/rdl/CFIHOS-20000008"/>
    <rdl:PCA_100006766 rdf:resource="http://rds.posccaesar.org/ontology/plm/rdl/PCA_100006636"/>
    <rdfs:label>Electrical calculations / analyses</rdfs:label>
    <rdl:PCA_100006766 rdf:resource="http://rds.posccaesar.org/ontology/plm/rdl/PCA_100006634"/>
    <rdl:PCA_100006766 rdf:resource="http://rds.posccaesar.org/ontology/plm/rdl/PCA_100006637"/>
    <rdfs:subClassOf rdf:resource="http://rds.posccaesar.org/ontology/plm/rdl/PCA_100004908"/>
    <rdl:PCA_100006766 rdf:resource="http://rds.posccaesar.org/ontology/plm/rdl/PCA_100006635"/>
  </owl:Class>
  <owl:Class rdf:about="http://rds.posccaesar.org/ontology/plm/rdl/PCA_100006186">
    <skos:broader rdf:resource="http://rds.posccaesar.org/ontology/plm/rdl/PCA_100006741"/>
    <skos:broadMatch rdf:resource="http://rds.posccaesar.org/ontology/plm/rdl/PCA_100006687"/>
    <rdfs:label>Equipment heat emission</rdfs:label>
    <rdl:PCA_100006766 rdf:resource="http://rds.posccaesar.org/ontology/plm/rdl/PCA_100006653"/>
    <rdl:PCA_100006765 rdf:resource="http://w3id.org/readi/rdl/CFIHOS-20000019"/>
    <rdl:PCA_100006763>Description of heat emission from installed equipment shall be per room/area, tag based. The heat emission shall be stated in normal, emergency and UPS operation modes.</rdl:PCA_100006763>
    <rdfs:subClassOf rdf:resource="http://rds.posccaesar.org/ontology/plm/rdl/PCA_100004908"/>
  </owl:Class>
  <owl:Class rdf:about="http://rds.posccaesar.org/ontology/plm/rdl/PCA_100006198">
    <skos:broader rdf:resource="http://rds.posccaesar.org/ontology/plm/rdl/PCA_100006756"/>
    <skos:broader>
      <rdl:PCA_100001503 rdf:about="http://rds.posccaesar.org/ontology/plm/rdl/PCA_100006762">
        <rdfs:label>Technical data</rdfs:label>
        <rdl:PCA_100004924>TD</rdl:PCA_100004924>
        <rdf:type rdf:resource="http://www.w3.org/2002/07/owl#NamedIndividual"/>
      </rdl:PCA_100001503>
    </skos:broader>
    <rdfs:subClassOf rdf:resource="http://rds.posccaesar.org/ontology/plm/rdl/PCA_100004908"/>
    <rdl:PCA_100006763>For  verfication purposes.</rdl:PCA_100006763>
    <skos:broadMatch rdf:resource="http://rds.posccaesar.org/ontology/plm/rdl/PCA_100006722"/>
    <rdfs:comment>The FRB shall contain welding procedures, relevant test certificates, heat treatment documentation and reference to requirements.</rdfs:comment>
    <rdl:PCA_100006768>The FRB shall contain welding procedures, relevant test certificates, heat treatment documentation and reference to requirements.</rdl:PCA_100006768>
    <rdl:PCA_100006766 rdf:resource="http://rds.posccaesar.org/ontology/plm/rdl/PCA_100006654"/>
    <rdfs:label>Fabrication record book (FRB)</rdfs:label>
    <rdl:PCA_100006765 rdf:resource="http://w3id.org/readi/rdl/CFIHOS-20000018"/>
  </owl:Class>
  <owl:Class rdf:about="http://rds.posccaesar.org/ontology/plm/rdl/PCA_100006089">
    <rdl:PCA_100006765 rdf:resource="http://w3id.org/readi/rdl/CFIHOS-20000006"/>
    <skos:broader rdf:resource="http://rds.posccaesar.org/ontology/plm/rdl/PCA_100006746"/>
    <rdl:PCA_100006768>Drawing of anodes shall be provided for the structural discipline with the following information: 
 - Location where the anode is attached;
 - Number off;
 - Type/weight/dimension;
 - Attachment to structure.</rdl:PCA_100006768>
    <rdfs:label>Anode details and layout</rdfs:label>
    <rdl:PCA_100006763>To give an overview of location of the anodes on equipment</rdl:PCA_100006763>
    <rdfs:comment>Drawing of anodes shall be provided for the structural discipline with the following information: 
 - Location where the anode is attached;
 - Number off;
 - Type/weight/dimension;
 - Attachment to structure.</rdfs:comment>
    <skos:broadMatch rdf:resource="http://rds.posccaesar.org/ontology/plm/rdl/PCA_100006734"/>
    <rdl:PCA_100006766 rdf:resource="http://rds.posccaesar.org/ontology/plm/rdl/PCA_100006653"/>
    <skos:broadMatch rdf:resource="http://rds.posccaesar.org/ontology/plm/rdl/PCA_100006733"/>
    <rdfs:subClassOf rdf:resource="http://rds.posccaesar.org/ontology/plm/rdl/PCA_100004908"/>
    <skos:broadMatch rdf:resource="http://rds.posccaesar.org/ontology/plm/rdl/PCA_100006732"/>
  </owl:Class>
  <owl:Class rdf:about="http://rds.posccaesar.org/ontology/plm/rdl/PCA_100006508">
    <rdl:PCA_100006765 rdf:resource="http://w3id.org/readi/rdl/CFIHOS-20000031"/>
    <rdfs:label>Trawling interaction</rdfs:label>
    <rdl:PCA_100006768>Document potential impact from trawl equipment towards pipeline.</rdl:PCA_100006768>
    <rdfs:subClassOf rdf:resource="http://rds.posccaesar.org/ontology/plm/rdl/PCA_100004908"/>
    <skos:broadMatch rdf:resource="http://rds.posccaesar.org/ontology/plm/rdl/PCA_100006686"/>
    <skos:broadMatch>
      <rdl:PCA_100001503 rdf:about="http://rds.posccaesar.org/ontology/plm/rdl/PCA_100006713">
        <rdfs:label>interaction information</rdfs:label>
        <rdl:PCA_100004924>MB</rdl:PCA_100004924>
        <rdf:type rdf:resource="http://www.w3.org/2002/07/owl#NamedIndividual"/>
      </rdl:PCA_100001503>
    </skos:broadMatch>
    <rdl:PCA_100006766 rdf:resource="http://rds.posccaesar.org/ontology/plm/rdl/PCA_100006653"/>
    <rdl:PCA_100006763>To provide input to weight coating design and protection requirements.</rdl:PCA_100006763>
    <rdfs:comment>Document potential impact from trawl equipment towards pipeline.</rdfs:comment>
    <skos:broader rdf:resource="http://rds.posccaesar.org/ontology/plm/rdl/PCA_100006756"/>
  </owl:Class>
  <owl:Class rdf:about="http://rds.posccaesar.org/ontology/plm/rdl/PCA_100006293">
    <skos:broader rdf:resource="http://rds.posccaesar.org/ontology/plm/rdl/PCA_100006756"/>
    <skos:broadMatch rdf:resource="http://rds.posccaesar.org/ontology/plm/rdl/PCA_100006686"/>
    <rdfs:label>Landfall design report</rdfs:label>
    <rdfs:comment>Basis for design, assumptions and assessments not given in design basis shall be included.</rdfs:comment>
    <rdl:PCA_100006768>Basis for design, assumptions and assessments not given in design basis shall be included.</rdl:PCA_100006768>
    <rdl:PCA_100006766 rdf:resource="http://rds.posccaesar.org/ontology/plm/rdl/PCA_100006657"/>
    <rdl:PCA_100006765 rdf:resource="http://w3id.org/readi/rdl/CFIHOS-20000018"/>
    <rdfs:subClassOf rdf:resource="http://rds.posccaesar.org/ontology/plm/rdl/PCA_100004908"/>
  </owl:Class>
  <owl:Class rdf:about="http://rds.posccaesar.org/ontology/plm/rdl/PCA_100006281">
    <rdl:PCA_100006768>Document content will depend on which equipment is supplied. Calculations will be done according to applicable standards.
Examples of Instrument Calculations are:
 - Thermowell frequency calculation
 - dP flow element sizing calculation</rdl:PCA_100006768>
    <rdfs:subClassOf rdf:resource="http://rds.posccaesar.org/ontology/plm/rdl/PCA_100004908"/>
    <rdl:PCA_100006765 rdf:resource="http://w3id.org/readi/rdl/CFIHOS-20000015"/>
    <skos:broader rdf:resource="http://rds.posccaesar.org/ontology/plm/rdl/PCA_100006741"/>
    <rdfs:label>Instrument calculations</rdfs:label>
    <rdl:PCA_100006763>This document shall support verification of component design according to applicable design standards.</rdl:PCA_100006763>
    <rdl:PCA_100006766 rdf:resource="http://rds.posccaesar.org/ontology/plm/rdl/PCA_100006653"/>
    <skos:broadMatch rdf:resource="http://rds.posccaesar.org/ontology/plm/rdl/PCA_100006687"/>
    <rdfs:comment>Document content will depend on which equipment is supplied. Calculations will be done according to applicable standards.
Examples of Instrument Calculations are:
 - Thermowell frequency calculation
 - dP flow element sizing calculation</rdfs:comment>
  </owl:Class>
  <owl:Class rdf:about="http://rds.posccaesar.org/ontology/plm/rdl/PCA_100006161">
    <skos:broader rdf:resource="http://rds.posccaesar.org/ontology/plm/rdl/PCA_100006746"/>
    <skos:broadMatch rdf:resource="http://rds.posccaesar.org/ontology/plm/rdl/PCA_100006732"/>
    <rdfs:label>Detail drawing with parts list</rdfs:label>
    <rdfs:comment>A view or drawing that shows what the inside of equipment looks like after a cross-sectional cut has been made.

The manufacturer's standard detail cross sectional drawing shall be delivered, following content requirements are:
 - Part list with material description.
 - Part numbers can be included or delivered through recommended spare parts list, and is thus not required for all parts. 
 - Material definition shall include reference to relevant national/international standards - and material data sheet numbers if additional requirements applies
 - Top Work details in a separate view or sheet shall be included for on/off valves with intended use for gear box or actuator, and if applicable for control valves.
 - Bolt up torque table for pressure containing parts shall be included if not a part of IOM.</rdfs:comment>
    <rdl:PCA_100006768>A view or drawing that shows what the inside of equipment looks like after a cross-sectional cut has been made.

The manufacturer's standard detail cross sectional drawing shall be delivered, following content requirements are:
 - Part list with material description.
 - Part numbers can be included or delivered through recommended spare parts list, and is thus not required for all parts. 
 - Material definition shall include reference to relevant national/international standards - and material data sheet numbers if additional requirements applies
 - Top Work details in a separate view or sheet shall be included for on/off valves with intended use for gear box or actuator, and if applicable for control valves.
 - Bolt up torque table for pressure containing parts shall be included if not a part of IOM.</rdl:PCA_100006768>
    <rdl:PCA_100006766 rdf:resource="http://rds.posccaesar.org/ontology/plm/rdl/PCA_100006653"/>
    <rdl:PCA_100006763>This document shall support verification of supplier’s design with regards to functionality and material selection.

This document also supports other documents where a cross-sectional view or part list is necessary for clarity.</rdl:PCA_100006763>
    <rdfs:subClassOf rdf:resource="http://rds.posccaesar.org/ontology/plm/rdl/PCA_100004908"/>
  </owl:Class>
  <owl:Class rdf:about="http://rds.posccaesar.org/ontology/plm/rdl/PCA_100006173">
    <rdfs:label>Electrical block diagrams</rdfs:label>
    <skos:broadMatch rdf:resource="http://rds.posccaesar.org/ontology/plm/rdl/PCA_100006696"/>
    <rdl:PCA_100006766 rdf:resource="http://rds.posccaesar.org/ontology/plm/rdl/PCA_100006638"/>
    <skos:broadMatch rdf:resource="http://rds.posccaesar.org/ontology/plm/rdl/PCA_100006699"/>
    <rdl:PCA_100006768>Electrical block diagram typical contents shall be:
 - All related systems and subsystems or eventual packages and interfaces represented by blocks;
 - Short description;
 - Location of equipment;
 - Tag number (when applicable);
 - Interface cabling between blocks within the package and all interface cables towards other packages shall be indicated.</rdl:PCA_100006768>
    <rdl:PCA_100006766 rdf:resource="http://rds.posccaesar.org/ontology/plm/rdl/PCA_100006636"/>
    <rdl:PCA_100006766 rdf:resource="http://rds.posccaesar.org/ontology/plm/rdl/PCA_100006639"/>
    <rdl:PCA_100006763>Electrical block diagram shall show configuration of an electrical system/package and subsystems or relevant interfaces to give a functional understanding.</rdl:PCA_100006763>
    <skos:broader>
      <rdl:PCA_100001503 rdf:about="http://rds.posccaesar.org/ontology/plm/rdl/PCA_100006740">
        <rdfs:label>Block Diagram</rdfs:label>
        <rdl:PCA_100004924>BD</rdl:PCA_100004924>
        <rdf:type rdf:resource="http://www.w3.org/2002/07/owl#NamedIndividual"/>
      </rdl:PCA_100001503>
    </skos:broader>
    <rdl:PCA_100006766 rdf:resource="http://rds.posccaesar.org/ontology/plm/rdl/PCA_100006640"/>
    <rdfs:subClassOf rdf:resource="http://rds.posccaesar.org/ontology/plm/rdl/PCA_100004908"/>
    <rdl:PCA_100006766 rdf:resource="http://rds.posccaesar.org/ontology/plm/rdl/PCA_100006634"/>
    <rdl:PCA_100006766 rdf:resource="http://rds.posccaesar.org/ontology/plm/rdl/PCA_100006637"/>
    <rdl:PCA_100006766 rdf:resource="http://rds.posccaesar.org/ontology/plm/rdl/PCA_100006641"/>
    <skos:broadMatch rdf:resource="http://rds.posccaesar.org/ontology/plm/rdl/PCA_100006695"/>
    <rdfs:comment>Electrical block diagram typical contents shall be:
 - All related systems and subsystems or eventual packages and interfaces represented by blocks;
 - Short description;
 - Location of equipment;
 - Tag number (when applicable);
 - Interface cabling between blocks within the package and all interface cables towards other packages shall be indicated.</rdfs:comment>
    <rdl:PCA_100006766 rdf:resource="http://rds.posccaesar.org/ontology/plm/rdl/PCA_100006635"/>
    <rdl:PCA_100006766 rdf:resource="http://rds.posccaesar.org/ontology/plm/rdl/PCA_100006642"/>
    <rdl:PCA_100006765 rdf:resource="http://w3id.org/readi/rdl/CFIHOS-20000008"/>
  </owl:Class>
  <owl:Class rdf:about="http://rds.posccaesar.org/ontology/plm/rdl/PCA_100006390">
    <skos:broader rdf:resource="http://rds.posccaesar.org/ontology/plm/rdl/PCA_100006743"/>
    <rdl:PCA_100006763>A document containing data which records compliance with specified requirements.</rdl:PCA_100006763>
    <rdl:PCA_100006765 rdf:resource="http://w3id.org/readi/rdl/CFIHOS-20000027"/>
    <skos:broadMatch rdf:resource="http://rds.posccaesar.org/ontology/plm/rdl/PCA_100006722"/>
    <rdl:PCA_100006768>Document shall contain or link to the proven requirements and results. It shall carry date and approvals (Signatures.)</rdl:PCA_100006768>
    <rdfs:subClassOf rdf:resource="http://rds.posccaesar.org/ontology/plm/rdl/PCA_100004908"/>
    <rdfs:label>Pressure test certificate</rdfs:label>
    <rdl:PCA_100006766 rdf:resource="http://rds.posccaesar.org/ontology/plm/rdl/PCA_100006653"/>
    <rdfs:comment>Document shall contain or link to the proven requirements and results. It shall carry date and approvals (Signatures.)</rdfs:comment>
  </owl:Class>
  <owl:Class rdf:about="http://rds.posccaesar.org/ontology/plm/rdl/PCA_100006185">
    <skos:broader rdf:resource="http://rds.posccaesar.org/ontology/plm/rdl/PCA_100006756"/>
    <skos:broadMatch>
      <rdl:PCA_100001503 rdf:about="http://rds.posccaesar.org/ontology/plm/rdl/PCA_100006728">
        <rdfs:label>environment protection information</rdfs:label>
        <rdl:PCA_100004924>RC</rdl:PCA_100004924>
        <rdf:type rdf:resource="http://www.w3.org/2002/07/owl#NamedIndividual"/>
      </rdl:PCA_100001503>
    </skos:broadMatch>
    <rdfs:label>Environment report</rdfs:label>
    <rdl:PCA_100006765 rdf:resource="http://w3id.org/readi/rdl/CFIHOS-20000010"/>
    <rdl:PCA_100006764>Consists of:
 - Environmental Design Review report. This is the report from environmental design review performed. Could be a separate review report or a part of a HSE design Review report. 
 - Environmental budget report. This report shall specify the yearly emissions to air (CO2, Nox, CH4, nmVOC, H2S, SOx, NH3 and particles) for the selected concept. The report shall also specify the yearly discharges to sea of process water, produced water, oil in water, chemicals in water and estimate of yearly waste fractions that must be handled.
 - BAT (Best Available Techniques) Evaluation Report. This report shall cover the BAT evaluations performed before the choice of technology was taken. Typical items will be power and heat generation, flare and vent systems, technology for reducing emission to air, material choice and use of chemicals, technology for reducing discharge to sea/water, e.g. cleaning technology.</rdl:PCA_100006764>
    <rdfs:subClassOf rdf:resource="http://rds.posccaesar.org/ontology/plm/rdl/PCA_100004908"/>
  </owl:Class>
  <owl:Class rdf:about="http://rds.posccaesar.org/ontology/plm/rdl/PCA_100006197">
    <skos:broader rdf:resource="http://rds.posccaesar.org/ontology/plm/rdl/PCA_100006743"/>
    <skos:broadMatch rdf:resource="http://rds.posccaesar.org/ontology/plm/rdl/PCA_100006722"/>
    <rdfs:label>Explosion protection certificates</rdfs:label>
    <rdl:PCA_100006765 rdf:resource="http://w3id.org/readi/rdl/CFIHOS-20000013"/>
    <rdl:PCA_100006763>Explosion protection certificates (ATEX , EX, NEMA). Applies to electrical devices and devices with electrical connections</rdl:PCA_100006763>
    <rdfs:subClassOf rdf:resource="http://rds.posccaesar.org/ontology/plm/rdl/PCA_100004908"/>
  </owl:Class>
  <owl:Class rdf:about="http://rds.posccaesar.org/ontology/plm/rdl/PCA_100006088">
    <rdl:PCA_100006768>Anchor design reports shall be delivered. The report or collection of reports shall contain the final documentation of the anchors. The report shall typically contain: 
 - Geotechnical report;
 - Structural design report;
 - Arrangement and detail drawings.</rdl:PCA_100006768>
    <skos:broadMatch>
      <rdl:PCA_100001503 rdf:about="http://rds.posccaesar.org/ontology/plm/rdl/PCA_100006691">
        <rdfs:label>scientific information</rdfs:label>
        <rdl:PCA_100004924>DF</rdl:PCA_100004924>
        <rdf:type rdf:resource="http://www.w3.org/2002/07/owl#NamedIndividual"/>
      </rdl:PCA_100001503>
    </skos:broadMatch>
    <skos:broadMatch>
      <rdl:PCA_100001503 rdf:about="http://rds.posccaesar.org/ontology/plm/rdl/PCA_100006698">
        <rdfs:label>function describing information</rdfs:label>
        <rdl:PCA_100004924>FE</rdl:PCA_100004924>
        <rdf:type rdf:resource="http://www.w3.org/2002/07/owl#NamedIndividual"/>
      </rdl:PCA_100001503>
    </skos:broadMatch>
    <rdl:PCA_100006765>
      <rdl:PCA_100001503 rdf:about="http://w3id.org/readi/rdl/CFIHOS-20000033">
        <rdfs:label>ocean engineering</rdfs:label>
        <rdl:PCA_100004924>WA</rdl:PCA_100004924>
        <rdf:type rdf:resource="http://www.w3.org/2002/07/owl#NamedIndividual"/>
      </rdl:PCA_100001503>
    </rdl:PCA_100006765>
    <rdfs:subClassOf rdf:resource="http://rds.posccaesar.org/ontology/plm/rdl/PCA_100004908"/>
    <skos:broader rdf:resource="http://rds.posccaesar.org/ontology/plm/rdl/PCA_100006756"/>
    <rdfs:label>Anchor design reports</rdfs:label>
    <rdfs:comment>Anchor design reports shall be delivered. The report or collection of reports shall contain the final documentation of the anchors. The report shall typically contain: 
 - Geotechnical report;
 - Structural design report;
 - Arrangement and detail drawings.</rdfs:comment>
    <rdl:PCA_100006763>The report or collection of reports shall contain the final documentation of the anchors.</rdl:PCA_100006763>
    <rdl:PCA_100006766>
      <rdl:PCA_100001503 rdf:about="http://rds.posccaesar.org/ontology/plm/rdl/PCA_100006647">
        <rdfs:label>Mooring and positioning</rdfs:label>
        <rdl:PCA_100004924>94</rdl:PCA_100004924>
        <rdf:type rdf:resource="http://www.w3.org/2002/07/owl#NamedIndividual"/>
      </rdl:PCA_100001503>
    </rdl:PCA_100006766>
  </owl:Class>
  <owl:Class rdf:about="http://rds.posccaesar.org/ontology/plm/rdl/PCA_100006509">
    <rdl:PCA_100006763>The design loads used to dimension the turret shall be documented.</rdl:PCA_100006763>
    <rdl:PCA_100006766 rdf:resource="http://rds.posccaesar.org/ontology/plm/rdl/PCA_100006657"/>
    <rdfs:comment>The report or collection of reports shall contain a complete description of the turret design.</rdfs:comment>
    <skos:broader rdf:resource="http://rds.posccaesar.org/ontology/plm/rdl/PCA_100006756"/>
    <rdl:PCA_100006768>The report or collection of reports shall contain a complete description of the turret design.</rdl:PCA_100006768>
    <rdl:PCA_100006765 rdf:resource="http://w3id.org/readi/rdl/CFIHOS-20000033"/>
    <rdfs:subClassOf rdf:resource="http://rds.posccaesar.org/ontology/plm/rdl/PCA_100004908"/>
    <rdfs:label>Turret design analysis report</rdfs:label>
    <skos:broadMatch rdf:resource="http://rds.posccaesar.org/ontology/plm/rdl/PCA_100006698"/>
  </owl:Class>
  <owl:Class rdf:about="http://rds.posccaesar.org/ontology/plm/rdl/PCA_100006319">
    <rdl:PCA_100006768>List containing main materials of an assembly with reference to part, serial and batch numbers. List shall contain references to material certificate, heat treatment batch / report and NDT reports where applicable. Mostly used for pressure containing equipment and load bearing elements.</rdl:PCA_100006768>
    <rdl:PCA_100006766 rdf:resource="http://rds.posccaesar.org/ontology/plm/rdl/PCA_100006653"/>
    <rdfs:subClassOf rdf:resource="http://rds.posccaesar.org/ontology/plm/rdl/PCA_100004908"/>
    <rdl:PCA_100006765 rdf:resource="http://w3id.org/readi/rdl/CFIHOS-20000031"/>
    <rdfs:comment>List containing main materials of an assembly with reference to part, serial and batch numbers. List shall contain references to material certificate, heat treatment batch / report and NDT reports where applicable. Mostly used for pressure containing equipment and load bearing elements.</rdfs:comment>
    <skos:broader rdf:resource="http://rds.posccaesar.org/ontology/plm/rdl/PCA_100006748"/>
    <rdl:PCA_100006763>Document material traceability for assemblies, components and materials.</rdl:PCA_100006763>
    <skos:broadMatch>
      <rdl:PCA_100001503 rdf:about="http://rds.posccaesar.org/ontology/plm/rdl/PCA_100006715">
        <rdfs:label>material listing</rdfs:label>
        <rdl:PCA_100004924>PA</rdl:PCA_100004924>
        <rdf:type rdf:resource="http://www.w3.org/2002/07/owl#NamedIndividual"/>
      </rdl:PCA_100001503>
    </skos:broadMatch>
    <rdfs:label>Material traceability list</rdfs:label>
  </owl:Class>
  <owl:Class rdf:about="http://rds.posccaesar.org/ontology/plm/rdl/PCA_100006428">
    <rdl:PCA_100006766 rdf:resource="http://rds.posccaesar.org/ontology/plm/rdl/PCA_100006654"/>
    <skos:broader>
      <rdl:PCA_100001503 rdf:about="http://rds.posccaesar.org/ontology/plm/rdl/PCA_100006758">
        <rdfs:label>Standards</rdfs:label>
        <rdl:PCA_100004924>SD</rdl:PCA_100004924>
        <rdf:type rdf:resource="http://www.w3.org/2002/07/owl#NamedIndividual"/>
      </rdl:PCA_100001503>
    </skos:broader>
    <rdfs:comment>The Safety Strategy shall outline the design principles for layout, configuration, arrangement and the selection and role of safety barriers to be implemented to manage risk. The strategy shall include the Fire and Explosion Strategy (FES), the Emergency, Evacuation and Rescue Strategy (EER), the ESD philosophy, F&amp;G detection philosophy and other high-level design and operational aspects related to safety barriers.

The Safety Strategy shall reflect installation specific conditions, including, but not limited to, environment and climate, competence of staff, cultural elements, infrastructure such as transport, external emergency preparedness resources, telecommunications, health care, availability of water supplies and electricity etc. The Safety Strategy shall document both general and area-specific strategies to manage risk.</rdfs:comment>
    <rdl:PCA_100006765 rdf:resource="http://w3id.org/readi/rdl/CFIHOS-20000013"/>
    <rdl:PCA_100006763>The Safety Strategy describes how risks are to be managed based on the outcome of a systematic identification and evaluation of the hazards and effects which may arise on the actual installation.</rdl:PCA_100006763>
    <rdfs:label>Safety strategy and performance standards</rdfs:label>
    <skos:broader>
      <rdl:PCA_100001503 rdf:about="http://rds.posccaesar.org/ontology/plm/rdl/PCA_100006759">
        <rdfs:label>Strategy</rdfs:label>
        <rdl:PCA_100004924>SG</rdl:PCA_100004924>
        <rdf:type rdf:resource="http://www.w3.org/2002/07/owl#NamedIndividual"/>
      </rdl:PCA_100001503>
    </skos:broader>
    <skos:broadMatch rdf:resource="http://rds.posccaesar.org/ontology/plm/rdl/PCA_100006727"/>
    <rdl:PCA_100006765 rdf:resource="http://w3id.org/readi/rdl/CFIHOS-20000011"/>
    <rdfs:subClassOf rdf:resource="http://rds.posccaesar.org/ontology/plm/rdl/PCA_100004908"/>
    <rdl:PCA_100006768>The Safety Strategy shall outline the design principles for layout, configuration, arrangement and the selection and role of safety barriers to be implemented to manage risk. The strategy shall include the Fire and Explosion Strategy (FES), the Emergency, Evacuation and Rescue Strategy (EER), the ESD philosophy, F&amp;G detection philosophy and other high-level design and operational aspects related to safety barriers.

The Safety Strategy shall reflect installation specific conditions, including, but not limited to, environment and climate, competence of staff, cultural elements, infrastructure such as transport, external emergency preparedness resources, telecommunications, health care, availability of water supplies and electricity etc. The Safety Strategy shall document both general and area-specific strategies to manage risk.</rdl:PCA_100006768>
    <skos:broadMatch rdf:resource="http://rds.posccaesar.org/ontology/plm/rdl/PCA_100006726"/>
    <rdl:PCA_100006765 rdf:resource="http://w3id.org/readi/rdl/CFIHOS-20000010"/>
    <skos:broadMatch rdf:resource="http://rds.posccaesar.org/ontology/plm/rdl/PCA_100006728"/>
  </owl:Class>
  <owl:Class rdf:about="http://rds.posccaesar.org/ontology/plm/rdl/PCA_100006307">
    <skos:broader rdf:resource="http://rds.posccaesar.org/ontology/plm/rdl/PCA_100006749"/>
    <skos:broadMatch rdf:resource="http://rds.posccaesar.org/ontology/plm/rdl/PCA_100006733"/>
    <rdfs:label>Manufacturing record book</rdfs:label>
    <rdfs:comment>Ensuring evidence and traceability on construction, manufacturing, testing, reporting and certification for equipment or material.</rdfs:comment>
    <rdl:PCA_100006768>Ensuring evidence and traceability on construction, manufacturing, testing, reporting and certification for equipment or material.</rdl:PCA_100006768>
    <rdl:PCA_100006766 rdf:resource="http://rds.posccaesar.org/ontology/plm/rdl/PCA_100006653"/>
    <rdl:PCA_100006763>A compiled document containing as-built records/documents, signed reports, certificates and drawings.</rdl:PCA_100006763>
    <rdfs:subClassOf rdf:resource="http://rds.posccaesar.org/ontology/plm/rdl/PCA_100004908"/>
  </owl:Class>
  <owl:Class rdf:about="http://rds.posccaesar.org/ontology/plm/rdl/PCA_100006416">
    <skos:broader rdf:resource="http://rds.posccaesar.org/ontology/plm/rdl/PCA_100006746"/>
    <skos:broadMatch rdf:resource="http://rds.posccaesar.org/ontology/plm/rdl/PCA_100006708"/>
    <rdfs:label>Road drawings</rdfs:label>
    <rdfs:comment>All system, arrangement, layout, plan, alignment, section and detail drawings shall be included.  Location, direction, type of signpost and reference to signpost data sheet shall be shown on layout drawings.</rdfs:comment>
    <rdl:PCA_100006768>All system, arrangement, layout, plan, alignment, section and detail drawings shall be included.  Location, direction, type of signpost and reference to signpost data sheet shall be shown on layout drawings.</rdl:PCA_100006768>
    <rdl:PCA_100006766 rdf:resource="http://rds.posccaesar.org/ontology/plm/rdl/PCA_100006656"/>
    <rdl:PCA_100006765 rdf:resource="http://w3id.org/readi/rdl/CFIHOS-20000007"/>
    <rdfs:subClassOf rdf:resource="http://rds.posccaesar.org/ontology/plm/rdl/PCA_100004908"/>
  </owl:Class>
  <owl:Class rdf:about="http://rds.posccaesar.org/ontology/plm/rdl/PCA_100006525">
    <skos:broader rdf:resource="http://rds.posccaesar.org/ontology/plm/rdl/PCA_100006751"/>
    <rdfs:label>Weighing procedure</rdfs:label>
    <rdfs:subClassOf rdf:resource="http://rds.posccaesar.org/ontology/plm/rdl/PCA_100004908"/>
    <rdl:PCA_100006763>Provide instructions for weighing of an object / product.</rdl:PCA_100006763>
    <rdl:PCA_100006764>The Weight Test Procedure shall describe requirements for methods and equipment to be used to obtain the correct gross weight of the goods being shipped. It shall cover each separately installed item of equipment or skid to enable safe lifting operations and structural load calculations or components for which weight is a critical property.</rdl:PCA_100006764>
    <skos:broadMatch rdf:resource="http://rds.posccaesar.org/ontology/plm/rdl/PCA_100006688"/>
    <rdl:PCA_100006766 rdf:resource="http://rds.posccaesar.org/ontology/plm/rdl/PCA_100006653"/>
    <rdl:PCA_100006765 rdf:resource="http://w3id.org/readi/rdl/CFIHOS-20000031"/>
    <rdl:PCA_100006768>Procedure to describe methods for verifying weight of an object / product.</rdl:PCA_100006768>
    <rdfs:comment>Procedure to describe methods for verifying weight of an object / product.</rdfs:comment>
  </owl:Class>
  <owl:Class rdf:about="http://rds.posccaesar.org/ontology/plm/rdl/PCA_100006404">
    <skos:broader rdf:resource="http://rds.posccaesar.org/ontology/plm/rdl/PCA_100006756"/>
    <skos:broadMatch>
      <rdl:PCA_100001503 rdf:about="http://rds.posccaesar.org/ontology/plm/rdl/PCA_100006664">
        <rdfs:label>observation management information</rdfs:label>
        <rdl:PCA_100004924>BB</rdl:PCA_100004924>
        <rdf:type rdf:resource="http://www.w3.org/2002/07/owl#NamedIndividual"/>
      </rdl:PCA_100001503>
    </skos:broadMatch>
    <rdfs:label>Qualitative risk analysis report</rdfs:label>
    <rdl:PCA_100006766 rdf:resource="http://rds.posccaesar.org/ontology/plm/rdl/PCA_100006654"/>
    <rdl:PCA_100006765 rdf:resource="http://w3id.org/readi/rdl/CFIHOS-20000018"/>
    <rdl:PCA_100006763>Describes the quantitative risk analysis performed for the pipeline system, covering all risk elements related to the pipeline. The reason for location and spacing of safety valves shall be included.</rdl:PCA_100006763>
    <rdfs:subClassOf rdf:resource="http://rds.posccaesar.org/ontology/plm/rdl/PCA_100004908"/>
  </owl:Class>
  <owl:Class rdf:about="http://rds.posccaesar.org/ontology/plm/rdl/PCA_100006537">
    <rdl:PCA_100006768>Document that has been qualified and provides the required variables of the welding procedure.</rdl:PCA_100006768>
    <skos:broader>
      <rdl:PCA_100001503 rdf:about="http://rds.posccaesar.org/ontology/plm/rdl/PCA_100006757">
        <rdfs:label>Specification</rdfs:label>
        <rdl:PCA_100004924>SC</rdl:PCA_100004924>
        <rdf:type rdf:resource="http://www.w3.org/2002/07/owl#NamedIndividual"/>
      </rdl:PCA_100001503>
    </skos:broader>
    <rdfs:label>Welding procedure specification (WPS)</rdfs:label>
    <rdl:PCA_100006763>Provide clear specification to welder to ensure repeatability of acceptable results.</rdl:PCA_100006763>
    <rdl:PCA_100006764>A Welding Procedure or Welding Procedure Specification (WPS) is generic information which is a written instruction that specifies materials, consumables and edge preparations for a given joint.
It lists the pre- and post-weld operations including heat treatments; machining, grinding and dressing of the weld; details the welding variables and the run sequence; and may specify the acceptance criteria and inspection methods.

The purpose of the WPS is to ensure that acceptance criteria can be met consistently, including mechanical properties and defect levels. It is also useful in enforcing quality control procedures, in standardising on welding methods, production times and costs and in controlling production schedules. Its prime purpose, however, is to give the welder clear, unequivocal nstructions on howa weld is to be made.</rdl:PCA_100006764>
    <rdfs:subClassOf rdf:resource="http://rds.posccaesar.org/ontology/plm/rdl/PCA_100004908"/>
    <rdl:PCA_100006765 rdf:resource="http://w3id.org/readi/rdl/CFIHOS-20000031"/>
    <skos:broadMatch rdf:resource="http://rds.posccaesar.org/ontology/plm/rdl/PCA_100006688"/>
    <rdfs:comment>Document that has been qualified and provides the required variables of the welding procedure.</rdfs:comment>
    <rdl:PCA_100006766 rdf:resource="http://rds.posccaesar.org/ontology/plm/rdl/PCA_100006653"/>
  </owl:Class>
  <owl:Class rdf:about="http://rds.posccaesar.org/ontology/plm/rdl/PCA_100006501">
    <skos:broader rdf:resource="http://rds.posccaesar.org/ontology/plm/rdl/PCA_100006756"/>
    <skos:broadMatch rdf:resource="http://rds.posccaesar.org/ontology/plm/rdl/PCA_100006722"/>
    <rdfs:label>Third party verifications</rdfs:label>
    <rdfs:comment>Third Party verification report</rdfs:comment>
    <rdl:PCA_100006768>Third Party verification report</rdl:PCA_100006768>
    <rdl:PCA_100006766 rdf:resource="http://rds.posccaesar.org/ontology/plm/rdl/PCA_100006653"/>
    <rdl:PCA_100006765 rdf:resource="http://w3id.org/readi/rdl/CFIHOS-20000020"/>
    <rdfs:subClassOf rdf:resource="http://rds.posccaesar.org/ontology/plm/rdl/PCA_100004908"/>
  </owl:Class>
  <owl:Class rdf:about="http://rds.posccaesar.org/ontology/plm/rdl/PCA_100006513">
    <rdfs:subClassOf rdf:resource="http://rds.posccaesar.org/ontology/plm/rdl/PCA_100004908"/>
    <rdfs:comment>All system, arrangement, layout, plan, alignment, section and detail drawings shall be included.</rdfs:comment>
    <skos:broadMatch rdf:resource="http://rds.posccaesar.org/ontology/plm/rdl/PCA_100006708"/>
    <rdl:PCA_100006768>All system, arrangement, layout, plan, alignment, section and detail drawings shall be included.</rdl:PCA_100006768>
    <rdl:PCA_100006766 rdf:resource="http://rds.posccaesar.org/ontology/plm/rdl/PCA_100006656"/>
    <skos:broader rdf:resource="http://rds.posccaesar.org/ontology/plm/rdl/PCA_100006746"/>
    <rdl:PCA_100006763>The drawings shall fully cover all construction and temporary underground piping and cable systems and their status if the system is not fully removed.</rdl:PCA_100006763>
    <rdfs:label>Underground piping and cables drawings</rdfs:label>
    <rdl:PCA_100006765 rdf:resource="http://w3id.org/readi/rdl/CFIHOS-20000007"/>
  </owl:Class>
  <owl:Class rdf:about="http://rds.posccaesar.org/ontology/plm/rdl/PCA_100006091">
    <skos:broader rdf:resource="http://rds.posccaesar.org/ontology/plm/rdl/PCA_100006746"/>
    <skos:broadMatch rdf:resource="http://rds.posccaesar.org/ontology/plm/rdl/PCA_100006710"/>
    <rdfs:label>Antenna tower layout drawings</rdfs:label>
    <rdfs:comment>Antenna tower layout drawings shall be provided. Drawings shall include location of antennas in antenna tower, the type of antenna, associated equipment and the vertical and horizontal distance between the different antennas.</rdfs:comment>
    <rdl:PCA_100006768>Antenna tower layout drawings shall be provided. Drawings shall include location of antennas in antenna tower, the type of antenna, associated equipment and the vertical and horizontal distance between the different antennas.</rdl:PCA_100006768>
    <rdl:PCA_100006766 rdf:resource="http://rds.posccaesar.org/ontology/plm/rdl/PCA_100006653"/>
    <rdl:PCA_100006765 rdf:resource="http://w3id.org/readi/rdl/CFIHOS-20000030"/>
    <rdfs:subClassOf rdf:resource="http://rds.posccaesar.org/ontology/plm/rdl/PCA_100004908"/>
  </owl:Class>
  <owl:Class rdf:about="http://rds.posccaesar.org/ontology/plm/rdl/PCA_100006209">
    <skos:broader rdf:resource="http://rds.posccaesar.org/ontology/plm/rdl/PCA_100006746"/>
    <skos:broadMatch rdf:resource="http://rds.posccaesar.org/ontology/plm/rdl/PCA_100006705"/>
    <rdfs:label>Field lay-out drawing</rdfs:label>
    <rdfs:comment>Lay-out drawing comprising of all elements in the field such as templates, platforms, anchor patterns, pipelines, umbilicals, cables, pipeline structures etc.</rdfs:comment>
    <rdl:PCA_100006768>Lay-out drawing comprising of all elements in the field such as templates, platforms, anchor patterns, pipelines, umbilicals, cables, pipeline structures etc.</rdl:PCA_100006768>
    <rdl:PCA_100006766 rdf:resource="http://rds.posccaesar.org/ontology/plm/rdl/PCA_100006654"/>
    <rdl:PCA_100006765 rdf:resource="http://w3id.org/readi/rdl/CFIHOS-20000018"/>
    <rdfs:subClassOf rdf:resource="http://rds.posccaesar.org/ontology/plm/rdl/PCA_100004908"/>
  </owl:Class>
  <owl:Class rdf:about="http://rds.posccaesar.org/ontology/plm/rdl/PCA_100006308">
    <skos:broader rdf:resource="http://rds.posccaesar.org/ontology/plm/rdl/PCA_100006749"/>
    <skos:broadMatch rdf:resource="http://rds.posccaesar.org/ontology/plm/rdl/PCA_100006722"/>
    <rdfs:label>Manufacturing record book (MRB)</rdfs:label>
    <rdfs:comment>MRB requirements:
 - The Manufacturers standard MRB can be delivered
 - If additional documents required by Company, they should be submitted as separate 
deliverables.

An MRB shall include:
(depending on the equipment it describes some of the below listed documents may not be 
applicable)
 - Introduction and MRB index
 - List of certificates
 - Analysis, tests, calculations, curves and tables (*)
 - Balancing certificates
 - Calibration certificates
 - Certificates needed for re-certification of equipment
 - Certificates of conformance (*)
 - Documentation for CE marking
 - Final inspection, preservation, packing and dispatch
 - Final test/acceptance reports (FAT reports)
 - Instrument calculations (safety and relief valves) (*)
 - Lifting certificates
 - Manufacturing procedures and reports
 - Material certificates (*)
 - Material testing and control
 - Material traceability list
 - Mechanical/structural calculations and analyses
 - NDE drawings, sketches and other NDE doc.
 - Non-conformance reports
 - Painting procedure
 - Performance / functional test procedures and reports
 - Photos of equipment/inspections
 - PMI report
 - Pressure test certificates
 - Telecommunication test report(s), Vendor reports, MC&amp;C reports
 - Third party verification reports
 - Type Cert.’s/EX Certificates/Product Cert.’s. issued by third party (*)
 - Weight certificates (*)
 - Weld Summary Index and NDE log
 - Welding procedures
 - Welding procedure qualification records (where applicable)

(*) Documents that may be required as separate documents. See chapter 4 for equipment 
type specific requirements.</rdfs:comment>
    <rdl:PCA_100006768>MRB requirements:
 - The Manufacturers standard MRB can be delivered
 - If additional documents required by Company, they should be submitted as separate 
deliverables.

An MRB shall include:
(depending on the equipment it describes some of the below listed documents may not be 
applicable)
 - Introduction and MRB index
 - List of certificates
 - Analysis, tests, calculations, curves and tables (*)
 - Balancing certificates
 - Calibration certificates
 - Certificates needed for re-certification of equipment
 - Certificates of conformance (*)
 - Documentation for CE marking
 - Final inspection, preservation, packing and dispatch
 - Final test/acceptance reports (FAT reports)
 - Instrument calculations (safety and relief valves) (*)
 - Lifting certificates
 - Manufacturing procedures and reports
 - Material certificates (*)
 - Material testing and control
 - Material traceability list
 - Mechanical/structural calculations and analyses
 - NDE drawings, sketches and other NDE doc.
 - Non-conformance reports
 - Painting procedure
 - Performance / functional test procedures and reports
 - Photos of equipment/inspections
 - PMI report
 - Pressure test certificates
 - Telecommunication test report(s), Vendor reports, MC&amp;C reports
 - Third party verification reports
 - Type Cert.’s/EX Certificates/Product Cert.’s. issued by third party (*)
 - Weight certificates (*)
 - Weld Summary Index and NDE log
 - Welding procedures
 - Welding procedure qualification records (where applicable)

(*) Documents that may be required as separate documents. See chapter 4 for equipment 
type specific requirements.</rdl:PCA_100006768>
    <rdl:PCA_100006763>MRB is a collection of necessary documents to demonstrate that the requirements with respect to design, calculation, production, testing and possible specified traceability requirements for materials and fabrication, are fulfilled.If the documentation normally contained in MRB is issued separately, a reference to such documents is sufficient in the MRB.</rdl:PCA_100006763>
    <rdfs:subClassOf rdf:resource="http://rds.posccaesar.org/ontology/plm/rdl/PCA_100004908"/>
  </owl:Class>
  <owl:Class rdf:about="http://rds.posccaesar.org/ontology/plm/rdl/PCA_100006429">
    <skos:broader rdf:resource="http://rds.posccaesar.org/ontology/plm/rdl/PCA_100006741"/>
    <skos:broadMatch rdf:resource="http://rds.posccaesar.org/ontology/plm/rdl/PCA_100006687"/>
    <rdfs:label>Satellite link budget calculations</rdfs:label>
    <rdl:PCA_100006765 rdf:resource="http://w3id.org/readi/rdl/CFIHOS-20000030"/>
    <rdl:PCA_100006763>Satellite link budget calculations (signal level and attenuation in dB) that have been used for design of satellite hops shall be provided.</rdl:PCA_100006763>
    <rdfs:subClassOf rdf:resource="http://rds.posccaesar.org/ontology/plm/rdl/PCA_100004908"/>
  </owl:Class>
  <owl:Class rdf:about="http://rds.posccaesar.org/ontology/plm/rdl/PCA_100006538">
    <rdl:PCA_100006766 rdf:resource="http://rds.posccaesar.org/ontology/plm/rdl/PCA_100006653"/>
    <rdl:PCA_100006768>Report containing all weld numbers in a series or an assembly with reference to WPS, WPQR, welder, PWHT, NDT etc.</rdl:PCA_100006768>
    <rdfs:comment>Report containing all weld numbers in a series or an assembly with reference to WPS, WPQR, welder, PWHT, NDT etc.</rdfs:comment>
    <rdfs:label>Welding report / log</rdfs:label>
    <rdl:PCA_100006765 rdf:resource="http://w3id.org/readi/rdl/CFIHOS-20000031"/>
    <skos:broadMatch rdf:resource="http://rds.posccaesar.org/ontology/plm/rdl/PCA_100006722"/>
    <rdfs:subClassOf rdf:resource="http://rds.posccaesar.org/ontology/plm/rdl/PCA_100004908"/>
    <skos:broader rdf:resource="http://rds.posccaesar.org/ontology/plm/rdl/PCA_100006748"/>
    <rdl:PCA_100006763>To document weld traceability.</rdl:PCA_100006763>
  </owl:Class>
  <owl:Class rdf:about="http://rds.posccaesar.org/ontology/plm/rdl/PCA_100006417">
    <rdl:PCA_100006763>Ensure safe operation</rdl:PCA_100006763>
    <rdfs:comment>Survey reports and data shall comply with Company's requirements.</rdfs:comment>
    <skos:broader rdf:resource="http://rds.posccaesar.org/ontology/plm/rdl/PCA_100006762"/>
    <rdfs:label>Rock installation survey reports and data</rdfs:label>
    <rdl:PCA_100006768>Survey reports and data shall comply with Company's requirements.</rdl:PCA_100006768>
    <skos:broadMatch rdf:resource="http://rds.posccaesar.org/ontology/plm/rdl/PCA_100006705"/>
    <skos:broader rdf:resource="http://rds.posccaesar.org/ontology/plm/rdl/PCA_100006756"/>
    <rdfs:subClassOf rdf:resource="http://rds.posccaesar.org/ontology/plm/rdl/PCA_100004908"/>
    <rdl:PCA_100006765 rdf:resource="http://w3id.org/readi/rdl/CFIHOS-20000018"/>
    <rdl:PCA_100006766 rdf:resource="http://rds.posccaesar.org/ontology/plm/rdl/PCA_100006654"/>
  </owl:Class>
  <owl:Class rdf:about="http://rds.posccaesar.org/ontology/plm/rdl/PCA_100006405">
    <skos:broadMatch>
      <rdl:PCA_100001503 rdf:about="http://rds.posccaesar.org/ontology/plm/rdl/PCA_100006672">
        <rdfs:label>quality management information</rdfs:label>
        <rdl:PCA_100004924>BQ</rdl:PCA_100004924>
        <rdf:type rdf:resource="http://www.w3.org/2002/07/owl#NamedIndividual"/>
      </rdl:PCA_100001503>
    </skos:broadMatch>
    <rdfs:label>Quality plan</rdfs:label>
    <rdfs:comment>The Quality Plan shall provide manufacturer compliance with quality standards, procedures and specifications</rdfs:comment>
    <rdl:PCA_100006768>The Quality Plan shall provide manufacturer compliance with quality standards, procedures and specifications</rdl:PCA_100006768>
    <rdl:PCA_100006766 rdf:resource="http://rds.posccaesar.org/ontology/plm/rdl/PCA_100006653"/>
    <rdl:PCA_100006765 rdf:resource="http://w3id.org/readi/rdl/CFIHOS-20000027"/>
    <rdl:PCA_100006763>This document provides information concerning the planned verification activities performed by manufacturer, purchaser and third party.</rdl:PCA_100006763>
    <rdfs:subClassOf rdf:resource="http://rds.posccaesar.org/ontology/plm/rdl/PCA_100004908"/>
  </owl:Class>
  <owl:Class rdf:about="http://rds.posccaesar.org/ontology/plm/rdl/PCA_100006514">
    <rdfs:subClassOf rdf:resource="http://rds.posccaesar.org/ontology/plm/rdl/PCA_100004908"/>
    <rdl:PCA_100006765 rdf:resource="http://w3id.org/readi/rdl/CFIHOS-20000007"/>
    <rdfs:label>Underground piping hydraulic system calculation</rdfs:label>
    <rdl:PCA_100006768>The calculations shall include:
 - Head loss calculations during fire situations;
 - Head loss calculations during various climatic conditions, such as storm rain, snow melting (if applicable) etc.;
 - Surge calculations for start/stop of pumps, valve operations, etc. shall be performed for all pump systems;
 - For drain systems with water traps, sensitivity calculations shall be made to identify uncertainties in head losses in manholes.

If existing calculation models exist, these models shall be updated.</rdl:PCA_100006768>
    <skos:broadMatch rdf:resource="http://rds.posccaesar.org/ontology/plm/rdl/PCA_100006687"/>
    <rdfs:comment>The calculations shall include:
 - Head loss calculations during fire situations;
 - Head loss calculations during various climatic conditions, such as storm rain, snow melting (if applicable) etc.;
 - Surge calculations for start/stop of pumps, valve operations, etc. shall be performed for all pump systems;
 - For drain systems with water traps, sensitivity calculations shall be made to identify uncertainties in head losses in manholes.

If existing calculation models exist, these models shall be updated.</rdfs:comment>
    <rdl:PCA_100006763>Hydraulic system calculation reports and input files/parameters shall be delivered. The report or collection of reports shall be self-contained, i.e. provide all information required to re-produce the results.

The design shall be documented by calculations. Calculations shall include references to basis of design (fire water quantities, maximum rainfall, etc.) and explanatory text (system description, etc.)</rdl:PCA_100006763>
    <rdl:PCA_100006766>
      <rdl:PCA_100001503 rdf:about="http://rds.posccaesar.org/ontology/plm/rdl/PCA_100006648">
        <rdfs:label>Onshore/civil</rdfs:label>
        <rdl:PCA_100004924>95</rdl:PCA_100004924>
        <rdf:type rdf:resource="http://www.w3.org/2002/07/owl#NamedIndividual"/>
      </rdl:PCA_100001503>
    </rdl:PCA_100006766>
    <skos:broader rdf:resource="http://rds.posccaesar.org/ontology/plm/rdl/PCA_100006741"/>
  </owl:Class>
  <owl:Class rdf:about="http://rds.posccaesar.org/ontology/plm/rdl/PCA_100006526">
    <rdfs:subClassOf rdf:resource="http://rds.posccaesar.org/ontology/plm/rdl/PCA_100004908"/>
    <rdfs:label>Weighing report</rdfs:label>
    <rdl:PCA_100006763>To document actual weight.</rdl:PCA_100006763>
    <rdl:PCA_100006766 rdf:resource="http://rds.posccaesar.org/ontology/plm/rdl/PCA_100006653"/>
    <rdl:PCA_100006768>Report to verify weight of an object / product.</rdl:PCA_100006768>
    <skos:broadMatch rdf:resource="http://rds.posccaesar.org/ontology/plm/rdl/PCA_100006722"/>
    <rdfs:comment>Report to verify weight of an object / product.</rdfs:comment>
    <skos:broader rdf:resource="http://rds.posccaesar.org/ontology/plm/rdl/PCA_100006756"/>
    <rdl:PCA_100006765 rdf:resource="http://w3id.org/readi/rdl/CFIHOS-20000031"/>
  </owl:Class>
  <owl:Class rdf:about="http://rds.posccaesar.org/ontology/plm/rdl/PCA_100006502">
    <rdfs:subClassOf rdf:resource="http://rds.posccaesar.org/ontology/plm/rdl/PCA_100004908"/>
    <rdl:PCA_100006765 rdf:resource="http://w3id.org/readi/rdl/CFIHOS-20000018"/>
    <rdfs:label>Tie-in design report</rdfs:label>
    <rdl:PCA_100006766 rdf:resource="http://rds.posccaesar.org/ontology/plm/rdl/PCA_100006654"/>
    <rdl:PCA_100006763>Ensure safe operation</rdl:PCA_100006763>
    <rdfs:comment>Covering pipeline tie-in operations construction.
Basis for analysis, assumptions and assessments not given in design basis shall be included.</rdfs:comment>
    <skos:broadMatch rdf:resource="http://rds.posccaesar.org/ontology/plm/rdl/PCA_100006686"/>
    <skos:broader rdf:resource="http://rds.posccaesar.org/ontology/plm/rdl/PCA_100006756"/>
    <rdl:PCA_100006768>Covering pipeline tie-in operations construction.
Basis for analysis, assumptions and assessments not given in design basis shall be included.</rdl:PCA_100006768>
  </owl:Class>
  <owl:Class rdf:about="http://rds.posccaesar.org/ontology/plm/rdl/PCA_100006090">
    <rdl:PCA_100006763>An index describing the scope of Anodes for an installation, and reference related information.</rdl:PCA_100006763>
    <skos:broadMatch rdf:resource="http://rds.posccaesar.org/ontology/plm/rdl/PCA_100006718"/>
    <rdfs:subClassOf rdf:resource="http://rds.posccaesar.org/ontology/plm/rdl/PCA_100004908"/>
    <rdl:PCA_100006768>An anode/reference electrode index shall be provided containing the following information:
 - Anode/ref. electrode type (unique reference to applicable anode/ref. electrode datasheet);
 - Data sheet number (data sheet to include details of dimensions, weight, Ex. cert., potential (max/min), sacrificial material, steel insert quality;
 - PO number;
 - Manufacturer;
 - Manufacturer type;
 - Location;
 - Identification reference; cross reference to layout drawing for anode/ref. electrode;
 - Layout drawing number.</rdl:PCA_100006768>
    <rdfs:comment>An anode/reference electrode index shall be provided containing the following information:
 - Anode/ref. electrode type (unique reference to applicable anode/ref. electrode datasheet);
 - Data sheet number (data sheet to include details of dimensions, weight, Ex. cert., potential (max/min), sacrificial material, steel insert quality;
 - PO number;
 - Manufacturer;
 - Manufacturer type;
 - Location;
 - Identification reference; cross reference to layout drawing for anode/ref. electrode;
 - Layout drawing number.</rdfs:comment>
    <rdfs:label>Anode index</rdfs:label>
    <rdl:PCA_100006766 rdf:resource="http://rds.posccaesar.org/ontology/plm/rdl/PCA_100006653"/>
    <rdl:PCA_100006765 rdf:resource="http://w3id.org/readi/rdl/CFIHOS-20000031"/>
    <skos:broadMatch rdf:resource="http://rds.posccaesar.org/ontology/plm/rdl/PCA_100006716"/>
    <skos:broadMatch rdf:resource="http://rds.posccaesar.org/ontology/plm/rdl/PCA_100006717"/>
    <skos:broader rdf:resource="http://rds.posccaesar.org/ontology/plm/rdl/PCA_100006748"/>
  </owl:Class>
  <owl:Class rdf:about="http://rds.posccaesar.org/ontology/plm/rdl/PCA_100006208">
    <rdfs:comment>Geographic map outlining subsea assemblies on the seabed for a particular field with description.</rdfs:comment>
    <skos:broader rdf:resource="http://rds.posccaesar.org/ontology/plm/rdl/PCA_100006746"/>
    <skos:broadMatch rdf:resource="http://rds.posccaesar.org/ontology/plm/rdl/PCA_100006705"/>
    <rdfs:label>Field layout drawing</rdfs:label>
    <rdfs:subClassOf rdf:resource="http://rds.posccaesar.org/ontology/plm/rdl/PCA_100004908"/>
    <rdl:PCA_100006765 rdf:resource="http://w3id.org/readi/rdl/CFIHOS-20000031"/>
    <rdl:PCA_100006763>To give an overview of where assemblies will be/are installed on the seabed relative to other assemblies.</rdl:PCA_100006763>
    <rdl:PCA_100006768>Geographic map outlining subsea assemblies on the seabed for a particular field with description.</rdl:PCA_100006768>
    <rdl:PCA_100006766 rdf:resource="http://rds.posccaesar.org/ontology/plm/rdl/PCA_100006653"/>
    <rdl:PCA_100006764>For SURF this info is covered in GIS database</rdl:PCA_100006764>
  </owl:Class>
  <owl:Class rdf:about="http://rds.posccaesar.org/ontology/plm/rdl/PCA_100006309">
    <rdl:PCA_100006766 rdf:resource="http://rds.posccaesar.org/ontology/plm/rdl/PCA_100006654"/>
    <skos:broader rdf:resource="http://rds.posccaesar.org/ontology/plm/rdl/PCA_100006762"/>
    <skos:broadMatch rdf:resource="http://rds.posccaesar.org/ontology/plm/rdl/PCA_100006722"/>
    <rdl:PCA_100006765 rdf:resource="http://w3id.org/readi/rdl/CFIHOS-20000018"/>
    <rdfs:label>Manufacturing record book (MRB) flexible pipeline and riser</rdfs:label>
    <rdl:PCA_100006768>The MRB for flexible pipelines shall be in accordance with API 17J 4th edition section 8.8 (As-built documentation).</rdl:PCA_100006768>
    <skos:broader rdf:resource="http://rds.posccaesar.org/ontology/plm/rdl/PCA_100006756"/>
    <rdfs:subClassOf rdf:resource="http://rds.posccaesar.org/ontology/plm/rdl/PCA_100004908"/>
    <rdl:PCA_100006763>To demonstrate that the requirements with respect to design, calculation, production, testing and possible specified traceability requirements for materials and fabrication, are fulfilled.</rdl:PCA_100006763>
    <rdfs:comment>The MRB for flexible pipelines shall be in accordance with API 17J 4th edition section 8.8 (As-built documentation).</rdfs:comment>
  </owl:Class>
  <owl:Class rdf:about="http://rds.posccaesar.org/ontology/plm/rdl/PCA_100006418">
    <skos:broader rdf:resource="http://rds.posccaesar.org/ontology/plm/rdl/PCA_100006756"/>
    <skos:broadMatch rdf:resource="http://rds.posccaesar.org/ontology/plm/rdl/PCA_100006722"/>
    <rdfs:label>Routine test report</rdfs:label>
    <rdfs:comment>Mandatory content of information:
 - Date of testing
 - Signature of person responsible for test
 - Object identification (type, series number, etc.)
 - Measured values.

Optional content of information:
 - Test equipment / instruments used
 - Reference to test procedure
 - Conclusion.</rdfs:comment>
    <rdl:PCA_100006768>Mandatory content of information:
 - Date of testing
 - Signature of person responsible for test
 - Object identification (type, series number, etc.)
 - Measured values.

Optional content of information:
 - Test equipment / instruments used
 - Reference to test procedure
 - Conclusion.</rdl:PCA_100006768>
    <rdl:PCA_100006766 rdf:resource="http://rds.posccaesar.org/ontology/plm/rdl/PCA_100006653"/>
    <rdl:PCA_100006763>Document verifying tested characteristics of a certain object.</rdl:PCA_100006763>
    <rdfs:subClassOf rdf:resource="http://rds.posccaesar.org/ontology/plm/rdl/PCA_100004908"/>
  </owl:Class>
  <owl:Class rdf:about="http://rds.posccaesar.org/ontology/plm/rdl/PCA_100006527">
    <rdl:PCA_100006768>This document shall follow ISO 19901-5.</rdl:PCA_100006768>
    <rdl:PCA_100006763>This document is used to provide final weight both for transport/installation and design calculations.</rdl:PCA_100006763>
    <skos:broader rdf:resource="http://rds.posccaesar.org/ontology/plm/rdl/PCA_100006743"/>
    <rdfs:comment>This document shall follow ISO 19901-5.</rdfs:comment>
    <skos:broadMatch rdf:resource="http://rds.posccaesar.org/ontology/plm/rdl/PCA_100006722"/>
    <rdfs:label>Weight certificate</rdfs:label>
    <rdfs:subClassOf rdf:resource="http://rds.posccaesar.org/ontology/plm/rdl/PCA_100004908"/>
    <rdl:PCA_100006766 rdf:resource="http://rds.posccaesar.org/ontology/plm/rdl/PCA_100006653"/>
    <rdl:PCA_100006765 rdf:resource="http://w3id.org/readi/rdl/CFIHOS-20000027"/>
  </owl:Class>
  <owl:Class rdf:about="http://rds.posccaesar.org/ontology/plm/rdl/PCA_100006406">
    <skos:broader rdf:resource="http://rds.posccaesar.org/ontology/plm/rdl/PCA_100006741"/>
    <skos:broadMatch rdf:resource="http://rds.posccaesar.org/ontology/plm/rdl/PCA_100006687"/>
    <rdfs:label>Radar coverage calculations</rdfs:label>
    <rdfs:comment>Calculation of radar coverage.</rdfs:comment>
    <rdl:PCA_100006768>Calculation of radar coverage.</rdl:PCA_100006768>
    <rdl:PCA_100006766 rdf:resource="http://rds.posccaesar.org/ontology/plm/rdl/PCA_100006640"/>
    <rdl:PCA_100006765 rdf:resource="http://w3id.org/readi/rdl/CFIHOS-20000030"/>
    <rdfs:subClassOf rdf:resource="http://rds.posccaesar.org/ontology/plm/rdl/PCA_100004908"/>
  </owl:Class>
  <owl:Class rdf:about="http://rds.posccaesar.org/ontology/plm/rdl/PCA_100006539">
    <skos:broader rdf:resource="http://rds.posccaesar.org/ontology/plm/rdl/PCA_100006748"/>
    <rdl:PCA_100006768>The well trajectory documents the direction in which the well is drilled. It shall be defined in accordance with TCD 6501 and should as a minimum contain:
 - Measured depht 
 - Inclination
 - Azimuth
 - True vertical depht</rdl:PCA_100006768>
    <rdl:PCA_100006764>Master data for survey data is stored in Wellview/compass</rdl:PCA_100006764>
    <skos:broadMatch rdf:resource="http://rds.posccaesar.org/ontology/plm/rdl/PCA_100006728"/>
    <rdl:PCA_100006765>
      <rdl:PCA_100001503 rdf:about="http://w3id.org/readi/rdl/CFIHOS-20000042">
        <rdfs:label>well engineering</rdfs:label>
        <rdl:PCA_100004924>ZW</rdl:PCA_100004924>
        <rdf:type rdf:resource="http://www.w3.org/2002/07/owl#NamedIndividual"/>
      </rdl:PCA_100001503>
    </rdl:PCA_100006765>
    <rdl:PCA_100006763>Precise determination of the well direction/path is important due to:
 - Position of well within defined target(s)
 - Avoid penetrating another well
 - Facilitate intersection of the wellbore with a relief well
 - Facilitate geological modelling
 - Facilitate anti-collision assessment for new wells
 - Input Intervention design simulation for wireline/coil tubing /snubbing
 - Input to casing design
 - Input to tubing design</rdl:PCA_100006763>
    <rdfs:comment>The well trajectory documents the direction in which the well is drilled. It shall be defined in accordance with TCD 6501 and should as a minimum contain:
 - Measured depht 
 - Inclination
 - Azimuth
 - True vertical depht</rdfs:comment>
    <skos:broadMatch rdf:resource="http://rds.posccaesar.org/ontology/plm/rdl/PCA_100006727"/>
    <rdfs:label>Well tracjectory</rdfs:label>
    <rdfs:subClassOf rdf:resource="http://rds.posccaesar.org/ontology/plm/rdl/PCA_100004908"/>
  </owl:Class>
  <owl:Class rdf:about="http://rds.posccaesar.org/ontology/plm/rdl/PCA_100006503">
    <skos:broader rdf:resource="http://rds.posccaesar.org/ontology/plm/rdl/PCA_100006749"/>
    <skos:broadMatch rdf:resource="http://rds.posccaesar.org/ontology/plm/rdl/PCA_100006713"/>
    <skos:broadMatch rdf:resource="http://rds.posccaesar.org/ontology/plm/rdl/PCA_100006712"/>
    <skos:broadMatch rdf:resource="http://rds.posccaesar.org/ontology/plm/rdl/PCA_100006688"/>
    <rdfs:label>Tie-in manual</rdfs:label>
    <rdfs:comment>The tie-in and diving operations manuals shall give a detailed description of the following items and operations:
 - Description of tie-in tools to be used for the alternative operations
 - Drawings of tie-in tools with weights, size, operational requirements and operational limitations 
 - Identification of ROV specific operations with outline descriptions of the ROV operation
 - Identification of critical items in relation to the above listed operations
 - Specify operations planned to be performed by divers
 - Identify access for divers, outline description of work tasks, work area and tools to be used
 - Identification of critical operations in relation to the diving programme.</rdfs:comment>
    <rdl:PCA_100006768>The tie-in and diving operations manuals shall give a detailed description of the following items and operations:
 - Description of tie-in tools to be used for the alternative operations
 - Drawings of tie-in tools with weights, size, operational requirements and operational limitations 
 - Identification of ROV specific operations with outline descriptions of the ROV operation
 - Identification of critical items in relation to the above listed operations
 - Specify operations planned to be performed by divers
 - Identify access for divers, outline description of work tasks, work area and tools to be used
 - Identification of critical operations in relation to the diving programme.</rdl:PCA_100006768>
    <rdfs:subClassOf rdf:resource="http://rds.posccaesar.org/ontology/plm/rdl/PCA_100004908"/>
  </owl:Class>
  <owl:Class rdf:about="http://rds.posccaesar.org/ontology/plm/rdl/PCA_100006515">
    <rdfs:comment>All system, arrangement, layout, plan, alignment, section and detail drawings shall be delivered including drawings showing details for rock support.</rdfs:comment>
    <rdfs:label>Underground rock facilities drawings</rdfs:label>
    <skos:broadMatch rdf:resource="http://rds.posccaesar.org/ontology/plm/rdl/PCA_100006708"/>
    <rdl:PCA_100006766 rdf:resource="http://rds.posccaesar.org/ontology/plm/rdl/PCA_100006656"/>
    <skos:broadMatch rdf:resource="http://rds.posccaesar.org/ontology/plm/rdl/PCA_100006707"/>
    <skos:broadMatch rdf:resource="http://rds.posccaesar.org/ontology/plm/rdl/PCA_100006732"/>
    <rdl:PCA_100006768>All system, arrangement, layout, plan, alignment, section and detail drawings shall be delivered including drawings showing details for rock support.</rdl:PCA_100006768>
    <skos:broader rdf:resource="http://rds.posccaesar.org/ontology/plm/rdl/PCA_100006746"/>
    <rdfs:subClassOf rdf:resource="http://rds.posccaesar.org/ontology/plm/rdl/PCA_100004908"/>
    <rdl:PCA_100006765 rdf:resource="http://w3id.org/readi/rdl/CFIHOS-20000007"/>
  </owl:Class>
  <owl:Class rdf:about="http://rds.posccaesar.org/ontology/plm/rdl/PCA_100006207">
    <rdl:PCA_100006763>An installation drawing shall indicate all details of the actual installation for the relevant instrument tag number (instruments and valves)</rdl:PCA_100006763>
    <rdl:PCA_100006766 rdf:resource="http://rds.posccaesar.org/ontology/plm/rdl/PCA_100006653"/>
    <rdl:PCA_100006765 rdf:resource="http://w3id.org/readi/rdl/CFIHOS-20000015"/>
    <skos:broader rdf:resource="http://rds.posccaesar.org/ontology/plm/rdl/PCA_100006746"/>
    <skos:broadMatch rdf:resource="http://rds.posccaesar.org/ontology/plm/rdl/PCA_100006732"/>
    <rdl:PCA_100006764>Drawing to include:
 - Field instrumentation part of process hook-up;
 - Structure and stands for field instrumentation.
 - A title to describe the process application;
 - All instrument/bulk material installed by Supplier, or to be installed by Purchaser;
 - Connections and dimensions of signal lines/tubing;
 - Material of instrument bulk;
 - A product code and quantity of instrument bulk;
 - Indicate split of responsibility instrument/piping.
Typical installation drawings should be used as a guideline.</rdl:PCA_100006764>
    <rdfs:label>Field instrument installation drawing typical</rdfs:label>
    <rdfs:subClassOf rdf:resource="http://rds.posccaesar.org/ontology/plm/rdl/PCA_100004908"/>
    <skos:broadMatch rdf:resource="http://rds.posccaesar.org/ontology/plm/rdl/PCA_100006731"/>
  </owl:Class>
  <owl:Class rdf:about="http://rds.posccaesar.org/ontology/plm/rdl/PCA_100006219">
    <skos:broader rdf:resource="http://rds.posccaesar.org/ontology/plm/rdl/PCA_100006756"/>
    <skos:broadMatch rdf:resource="http://rds.posccaesar.org/ontology/plm/rdl/PCA_100006698"/>
    <skos:broadMatch rdf:resource="http://rds.posccaesar.org/ontology/plm/rdl/PCA_100006691"/>
    <rdfs:label>Fiscal metering - Flow meter selection report</rdfs:label>
    <rdl:PCA_100006765 rdf:resource="http://w3id.org/readi/rdl/CFIHOS-20000015"/>
    <rdl:PCA_100006763>The evaluation leading to the selection of flow meter principle and make shall be documented. Ref TR0814 section 4.1 Selection of flow meters.</rdl:PCA_100006763>
    <rdfs:subClassOf rdf:resource="http://rds.posccaesar.org/ontology/plm/rdl/PCA_100004908"/>
  </owl:Class>
  <owl:Class rdf:about="http://rds.posccaesar.org/ontology/plm/rdl/PCA_100006419">
    <skos:broader rdf:resource="http://rds.posccaesar.org/ontology/plm/rdl/PCA_100006756"/>
    <rdl:PCA_100006763>To provide basis for laying and seabed intervention design report.</rdl:PCA_100006763>
    <rdfs:comment>Drawing showing the pipeline, riser or umbilical route.</rdfs:comment>
    <rdl:PCA_100006765 rdf:resource="http://w3id.org/readi/rdl/CFIHOS-20000031"/>
    <skos:broadMatch>
      <rdl:PCA_100001503 rdf:about="http://rds.posccaesar.org/ontology/plm/rdl/PCA_100006689">
        <rdfs:label>technical observation information</rdfs:label>
        <rdl:PCA_100004924>DD</rdl:PCA_100004924>
        <rdf:type rdf:resource="http://www.w3.org/2002/07/owl#NamedIndividual"/>
      </rdl:PCA_100001503>
    </skos:broadMatch>
    <rdl:PCA_100006766 rdf:resource="http://rds.posccaesar.org/ontology/plm/rdl/PCA_100006656"/>
    <rdfs:label>Routing design</rdfs:label>
    <rdl:PCA_100006768>Drawing showing the pipeline, riser or umbilical route.</rdl:PCA_100006768>
    <rdfs:subClassOf rdf:resource="http://rds.posccaesar.org/ontology/plm/rdl/PCA_100004908"/>
  </owl:Class>
  <owl:Class rdf:about="http://rds.posccaesar.org/ontology/plm/rdl/PCA_100006407">
    <skos:broader rdf:resource="http://rds.posccaesar.org/ontology/plm/rdl/PCA_100006741"/>
    <skos:broadMatch rdf:resource="http://rds.posccaesar.org/ontology/plm/rdl/PCA_100006687"/>
    <rdfs:label>Radio link budget calculations</rdfs:label>
    <rdl:PCA_100006765 rdf:resource="http://w3id.org/readi/rdl/CFIHOS-20000030"/>
    <rdl:PCA_100006763>Radio link budget calculations that have been used for design of radio links shall be provided.</rdl:PCA_100006763>
    <rdfs:subClassOf rdf:resource="http://rds.posccaesar.org/ontology/plm/rdl/PCA_100004908"/>
  </owl:Class>
  <owl:Class rdf:about="http://rds.posccaesar.org/ontology/plm/rdl/PCA_100006516">
    <rdfs:label>Unique equipment ID for standard equipment</rdfs:label>
    <rdl:PCA_100006763>The unique equipment ID is the key information element to retrieve standard documentation for standard equipment in Company's solution for standard documentation for equipment and materials. The unique equipment ID shall be in approved status at milestone LCI 1, and thus also required approved standard documentation is provided.</rdl:PCA_100006763>
    <rdfs:subClassOf rdf:resource="http://rds.posccaesar.org/ontology/plm/rdl/PCA_100004908"/>
  </owl:Class>
  <owl:Class rdf:about="http://rds.posccaesar.org/ontology/plm/rdl/PCA_100006528">
    <skos:broadMatch rdf:resource="http://rds.posccaesar.org/ontology/plm/rdl/PCA_100006717"/>
    <skos:broadMatch rdf:resource="http://rds.posccaesar.org/ontology/plm/rdl/PCA_100006716"/>
    <rdfs:subClassOf rdf:resource="http://rds.posccaesar.org/ontology/plm/rdl/PCA_100004908"/>
    <rdfs:label>Weight control database</rdfs:label>
    <skos:broadMatch rdf:resource="http://rds.posccaesar.org/ontology/plm/rdl/PCA_100006715"/>
    <rdl:PCA_100006766 rdf:resource="http://rds.posccaesar.org/ontology/plm/rdl/PCA_100006654"/>
    <skos:broader rdf:resource="http://rds.posccaesar.org/ontology/plm/rdl/PCA_100006762"/>
    <rdfs:comment>Content to be in accordance with ISO 19901-5. Handover format is plant specific.</rdfs:comment>
    <skos:broadMatch rdf:resource="http://rds.posccaesar.org/ontology/plm/rdl/PCA_100006722"/>
    <rdl:PCA_100006768>Content to be in accordance with ISO 19901-5. Handover format is plant specific.</rdl:PCA_100006768>
    <rdl:PCA_100006765 rdf:resource="http://w3id.org/readi/rdl/CFIHOS-20000006"/>
  </owl:Class>
  <owl:Class rdf:about="http://rds.posccaesar.org/ontology/plm/rdl/PCA_100006504">
    <skos:broadMatch rdf:resource="http://rds.posccaesar.org/ontology/plm/rdl/PCA_100006688"/>
    <rdl:PCA_100006766 rdf:resource="http://rds.posccaesar.org/ontology/plm/rdl/PCA_100006654"/>
    <rdl:PCA_100006763>Documentation of tie-in</rdl:PCA_100006763>
    <rdl:PCA_100006765 rdf:resource="http://w3id.org/readi/rdl/CFIHOS-20000018"/>
    <skos:broader rdf:resource="http://rds.posccaesar.org/ontology/plm/rdl/PCA_100006751"/>
    <rdfs:comment>Documentation of procedures used for tie-in</rdfs:comment>
    <rdfs:label>Tie-in procedures</rdfs:label>
    <rdfs:subClassOf rdf:resource="http://rds.posccaesar.org/ontology/plm/rdl/PCA_100004908"/>
    <rdl:PCA_100006768>Documentation of procedures used for tie-in</rdl:PCA_100006768>
  </owl:Class>
  <owl:Class rdf:about="http://rds.posccaesar.org/ontology/plm/rdl/PCA_100006206">
    <skos:broader rdf:resource="http://rds.posccaesar.org/ontology/plm/rdl/PCA_100006756"/>
    <skos:broadMatch rdf:resource="http://rds.posccaesar.org/ontology/plm/rdl/PCA_100006722"/>
    <rdfs:label>Fibre optical long-distance cable test report</rdfs:label>
    <rdl:PCA_100006766 rdf:resource="http://rds.posccaesar.org/ontology/plm/rdl/PCA_100006653"/>
    <rdl:PCA_100006765 rdf:resource="http://w3id.org/readi/rdl/CFIHOS-20000030"/>
    <rdl:PCA_100006764>Test reports for Fibre optical long-distance cable(s) shall be provided. Test per fibre.</rdl:PCA_100006764>
    <rdfs:subClassOf rdf:resource="http://rds.posccaesar.org/ontology/plm/rdl/PCA_100004908"/>
  </owl:Class>
  <owl:Class rdf:about="http://rds.posccaesar.org/ontology/plm/rdl/PCA_100006218">
    <skos:broadMatch rdf:resource="http://rds.posccaesar.org/ontology/plm/rdl/PCA_100006687"/>
    <skos:broader rdf:resource="http://rds.posccaesar.org/ontology/plm/rdl/PCA_100006741"/>
    <rdl:PCA_100006765 rdf:resource="http://w3id.org/readi/rdl/CFIHOS-20000015"/>
    <rdfs:subClassOf rdf:resource="http://rds.posccaesar.org/ontology/plm/rdl/PCA_100004908"/>
    <rdl:PCA_100006766 rdf:resource="http://rds.posccaesar.org/ontology/plm/rdl/PCA_100006587"/>
    <rdfs:label>Fiscal metering - Fiscal metering calculations</rdfs:label>
    <rdl:PCA_100006766 rdf:resource="http://rds.posccaesar.org/ontology/plm/rdl/PCA_100006591"/>
    <rdl:PCA_100006763>The document shall provide the information needed for an independent verification of the calculations in the computer. All international standards used shall be referred to with version number, year and relevant section.</rdl:PCA_100006763>
    <rdl:PCA_100006764>A document unambiguously showing all calculations affecting the measurement result shall be provided.</rdl:PCA_100006764>
  </owl:Class>
  <owl:Class rdf:about="http://rds.posccaesar.org/ontology/plm/rdl/PCA_100006529">
    <rdl:PCA_100006768>Provide instructions for weighing of an object / product.</rdl:PCA_100006768>
    <rdfs:label>Weight control procedure</rdfs:label>
    <rdl:PCA_100006766 rdf:resource="http://rds.posccaesar.org/ontology/plm/rdl/PCA_100006653"/>
    <skos:broader rdf:resource="http://rds.posccaesar.org/ontology/plm/rdl/PCA_100006751"/>
    <rdl:PCA_100006765 rdf:resource="http://w3id.org/readi/rdl/CFIHOS-20000027"/>
    <rdfs:subClassOf rdf:resource="http://rds.posccaesar.org/ontology/plm/rdl/PCA_100004908"/>
    <rdfs:comment>Provide instructions for weighing of an object / product.</rdfs:comment>
    <skos:broadMatch rdf:resource="http://rds.posccaesar.org/ontology/plm/rdl/PCA_100006722"/>
    <rdl:PCA_100006763>Procedure to describe methods for verifying weight of an object / product.</rdl:PCA_100006763>
  </owl:Class>
  <owl:Class rdf:about="http://rds.posccaesar.org/ontology/plm/rdl/PCA_100006109">
    <rdl:PCA_100006763>Required for system understanding, functionality, and troubleshooting</rdl:PCA_100006763>
    <rdl:PCA_100006766 rdf:resource="http://rds.posccaesar.org/ontology/plm/rdl/PCA_100006653"/>
    <rdfs:subClassOf rdf:resource="http://rds.posccaesar.org/ontology/plm/rdl/PCA_100004908"/>
    <rdfs:comment>Show configuration of a system/package and subsystems or relevant interfaces to give a functional understanding.</rdfs:comment>
    <skos:broadMatch rdf:resource="http://rds.posccaesar.org/ontology/plm/rdl/PCA_100006695"/>
    <rdfs:label>Block diagram</rdfs:label>
    <rdl:PCA_100006764>This is a schematic diagram which shows connections between simple figures (rectangles etc.) in order to set out the sequence of pieces of equipment or functions. It includes the "Process block diagram".
NOTE! This type of block diagrams shall not be used to present logic.</rdl:PCA_100006764>
    <rdl:PCA_100006765 rdf:resource="http://w3id.org/readi/rdl/CFIHOS-20000031"/>
    <rdl:PCA_100006768>Show configuration of a system/package and subsystems or relevant interfaces to give a functional understanding.</rdl:PCA_100006768>
    <skos:broader rdf:resource="http://rds.posccaesar.org/ontology/plm/rdl/PCA_100006745"/>
  </owl:Class>
  <owl:Class rdf:about="http://rds.posccaesar.org/ontology/plm/rdl/PCA_100006408">
    <skos:broadMatch rdf:resource="http://rds.posccaesar.org/ontology/plm/rdl/PCA_100006727"/>
    <rdfs:label>RAM analysis</rdfs:label>
    <rdfs:comment>Report providing the reliability availability and maintainability analysis performed for equipment and components.</rdfs:comment>
    <rdl:PCA_100006768>Report providing the reliability availability and maintainability analysis performed for equipment and components.</rdl:PCA_100006768>
    <rdl:PCA_100006766 rdf:resource="http://rds.posccaesar.org/ontology/plm/rdl/PCA_100006653"/>
    <rdl:PCA_100006765 rdf:resource="http://w3id.org/readi/rdl/CFIHOS-20000031"/>
    <rdl:PCA_100006763>Document reliability availability and maintainability for selected equipment and components to meet the levels of intended use as specified.</rdl:PCA_100006763>
    <rdfs:subClassOf rdf:resource="http://rds.posccaesar.org/ontology/plm/rdl/PCA_100004908"/>
  </owl:Class>
  <owl:Class rdf:about="http://rds.posccaesar.org/ontology/plm/rdl/PCA_100006339">
    <skos:broader rdf:resource="http://rds.posccaesar.org/ontology/plm/rdl/PCA_100006747"/>
    <skos:broadMatch rdf:resource="http://rds.posccaesar.org/ontology/plm/rdl/PCA_100006686"/>
    <rdfs:label>Noise data sheet</rdfs:label>
    <rdfs:comment>Noise and vibration data shall be delivered according to NORSOK S-002.

The datasheet shall as a minimum contain the information specified in the applicable datasheet template.</rdfs:comment>
    <rdl:PCA_100006768>Noise and vibration data shall be delivered according to NORSOK S-002.

The datasheet shall as a minimum contain the information specified in the applicable datasheet template.</rdl:PCA_100006768>
    <rdl:PCA_100006766 rdf:resource="http://rds.posccaesar.org/ontology/plm/rdl/PCA_100006653"/>
    <rdl:PCA_100006763>Document providing information about noise levels.</rdl:PCA_100006763>
    <rdfs:subClassOf rdf:resource="http://rds.posccaesar.org/ontology/plm/rdl/PCA_100004908"/>
  </owl:Class>
  <owl:Class rdf:about="http://rds.posccaesar.org/ontology/plm/rdl/PCA_100006327">
    <rdl:PCA_100006765 rdf:resource="http://w3id.org/readi/rdl/CFIHOS-20000033"/>
    <skos:broadMatch rdf:resource="http://rds.posccaesar.org/ontology/plm/rdl/PCA_100006687"/>
    <rdl:PCA_100006766 rdf:resource="http://rds.posccaesar.org/ontology/plm/rdl/PCA_100006647"/>
    <skos:broader rdf:resource="http://rds.posccaesar.org/ontology/plm/rdl/PCA_100006762"/>
    <rdfs:comment>A complete mooring analysis model shall be delivered in native format. The model shall be delivered with all necessary information required to perform a re-analysis.</rdfs:comment>
    <skos:broader rdf:resource="http://rds.posccaesar.org/ontology/plm/rdl/PCA_100006741"/>
    <rdfs:label>Mooring analysis model</rdfs:label>
    <rdl:PCA_100006768>A complete mooring analysis model shall be delivered in native format. The model shall be delivered with all necessary information required to perform a re-analysis.</rdl:PCA_100006768>
    <rdfs:subClassOf rdf:resource="http://rds.posccaesar.org/ontology/plm/rdl/PCA_100004908"/>
  </owl:Class>
  <owl:Class rdf:about="http://rds.posccaesar.org/ontology/plm/rdl/PCA_100006448">
    <rdfs:label>Software documentation - lifting appliances</rdfs:label>
    <rdfs:comment>Listing specific HW type, serial numbers, and specific SW version identification.</rdfs:comment>
    <rdl:PCA_100006768>Listing specific HW type, serial numbers, and specific SW version identification.</rdl:PCA_100006768>
    <rdl:PCA_100006763>The Software documentation shall specifically identify the target systems that have been tested.</rdl:PCA_100006763>
    <rdfs:subClassOf rdf:resource="http://rds.posccaesar.org/ontology/plm/rdl/PCA_100004908"/>
  </owl:Class>
  <owl:Class rdf:about="http://rds.posccaesar.org/ontology/plm/rdl/PCA_100006436">
    <skos:broader rdf:resource="http://rds.posccaesar.org/ontology/plm/rdl/PCA_100006746"/>
    <rdfs:label>Shore approach</rdfs:label>
    <rdfs:comment>Document how a pipeline or umbilical approaches onshore.</rdfs:comment>
    <rdl:PCA_100006768>Document how a pipeline or umbilical approaches onshore.</rdl:PCA_100006768>
    <rdl:PCA_100006766 rdf:resource="http://rds.posccaesar.org/ontology/plm/rdl/PCA_100006657"/>
    <rdl:PCA_100006765 rdf:resource="http://w3id.org/readi/rdl/CFIHOS-20000031"/>
    <rdl:PCA_100006763>To provide basis for laying operations and seabed intervention report.</rdl:PCA_100006763>
    <rdfs:subClassOf rdf:resource="http://rds.posccaesar.org/ontology/plm/rdl/PCA_100004908"/>
  </owl:Class>
  <owl:Class rdf:about="http://rds.posccaesar.org/ontology/plm/rdl/PCA_100006545">
    <rdl:PCA_100006765 rdf:resource="http://w3id.org/readi/rdl/CFIHOS-20000013"/>
    <rdl:PCA_100006765 rdf:resource="http://w3id.org/readi/rdl/CFIHOS-20000010"/>
    <rdfs:subClassOf rdf:resource="http://rds.posccaesar.org/ontology/plm/rdl/PCA_100004908"/>
    <skos:broader rdf:resource="http://rds.posccaesar.org/ontology/plm/rdl/PCA_100006756"/>
    <rdl:PCA_100006766 rdf:resource="http://rds.posccaesar.org/ontology/plm/rdl/PCA_100006654"/>
    <rdl:PCA_100006765 rdf:resource="http://w3id.org/readi/rdl/CFIHOS-20000011"/>
    <rdfs:comment>The report shall include: 
 - Documentation of all remaining risks not eliminated through design solutions and relevant for normal operations, inspection and maintenance
 - Updated WEHRA
 - Working Environment Area Charts</rdfs:comment>
    <rdfs:label>Working environment summary report</rdfs:label>
    <skos:broadMatch rdf:resource="http://rds.posccaesar.org/ontology/plm/rdl/PCA_100006726"/>
    <rdl:PCA_100006768>The report shall include: 
 - Documentation of all remaining risks not eliminated through design solutions and relevant for normal operations, inspection and maintenance
 - Updated WEHRA
 - Working Environment Area Charts</rdl:PCA_100006768>
  </owl:Class>
  <owl:Class rdf:about="http://rds.posccaesar.org/ontology/plm/rdl/PCA_100006315">
    <rdfs:comment>For Offshore facilities, the material handling report which shall contain the following:
 - Description of all material handling equipment, e.g. offshore cranes, personnel and goods lift, forklift truck, trolleys, air film transporters, elephant cranes, A-frames, mobile cranes, etc., including tag numbers (where required), sizes and capacities. 
 - Description of standardized sizes of typical lifting beams, pad eyes and lifting equipment, as applicable.
 - Requirements for certification and marking of lifting equipment including foundation and suspension.
 - Description of function, size and location, maximum allowable loads, point loads of lay down and storage areas including areas for the handling of temporary, Company provided and hired equipment., (Laydown area chart).
 - Requirements for transportation routes including maximum allowable loads, point loads, width and height in the different areas. (Transport routes chart).
 - Description and drawings of goods handling to/from helideck.
 - Description of loading hose handling including hose replacement.
 - Description and drawings of areas where special protection of equipment is required e.g. dropped object protection, truck barriers, swinging load protection etc.
 - Description and drawings of handling for all goods to and from the LQ.
 - Table /index containing all tags to be handled with corresponding identification number to the Material Handling Data Sheet.

For Onshore facilities, the material handling report which shall contain the following:
 - Description of all material handling equipment, e.g. forklift truck, trolleys, air film transporters, elephant cranes, A-frames, mobile cranes etc. including tag numbers, sizes and capacities, storage location, installation method and requirements for certification, marking and re-certification period. 
 - Description of function, size and location of lay down and storage.
 - Description of all items above 25 kg (55 lbs.) to be handled, including tag numbers, location, weight, size, type of lifting equipment/ arrangement, lifting/ handling procedure, transport route etc. In cases where the equipment vendor has established thorough handling procedures in the maintenance manual, this can be referred to in the report. The material handling description for such equipment can be reduced to just defining the required lifting/ transportation equipment and transport route. 
 - Requirements for transportation ways/roads including width and height in the different areas.
 - Description of areas where special protection of equipment is required e.g. dropped object protection, truck barriers, swinging load protection etc.
 - Material handling drawings based on equipment arrangement drawings or 3D plots including piping and valves containing the following:
    - All equipment to be handled including lifting lugs, monorails, access ways etc.
    - Table containing all tags to be handled with corresponding tags for the lifting equipment to be used.</rdfs:comment>
    <skos:broader rdf:resource="http://rds.posccaesar.org/ontology/plm/rdl/PCA_100006756"/>
    <rdfs:label>Material handling report</rdfs:label>
    <rdl:PCA_100006766 rdf:resource="http://rds.posccaesar.org/ontology/plm/rdl/PCA_100006653"/>
    <rdl:PCA_100006768>For Offshore facilities, the material handling report which shall contain the following:
 - Description of all material handling equipment, e.g. offshore cranes, personnel and goods lift, forklift truck, trolleys, air film transporters, elephant cranes, A-frames, mobile cranes, etc., including tag numbers (where required), sizes and capacities. 
 - Description of standardized sizes of typical lifting beams, pad eyes and lifting equipment, as applicable.
 - Requirements for certification and marking of lifting equipment including foundation and suspension.
 - Description of function, size and location, maximum allowable loads, point loads of lay down and storage areas including areas for the handling of temporary, Company provided and hired equipment., (Laydown area chart).
 - Requirements for transportation routes including maximum allowable loads, point loads, width and height in the different areas. (Transport routes chart).
 - Description and drawings of goods handling to/from helideck.
 - Description of loading hose handling including hose replacement.
 - Description and drawings of areas where special protection of equipment is required e.g. dropped object protection, truck barriers, swinging load protection etc.
 - Description and drawings of handling for all goods to and from the LQ.
 - Table /index containing all tags to be handled with corresponding identification number to the Material Handling Data Sheet.

For Onshore facilities, the material handling report which shall contain the following:
 - Description of all material handling equipment, e.g. forklift truck, trolleys, air film transporters, elephant cranes, A-frames, mobile cranes etc. including tag numbers, sizes and capacities, storage location, installation method and requirements for certification, marking and re-certification period. 
 - Description of function, size and location of lay down and storage.
 - Description of all items above 25 kg (55 lbs.) to be handled, including tag numbers, location, weight, size, type of lifting equipment/ arrangement, lifting/ handling procedure, transport route etc. In cases where the equipment vendor has established thorough handling procedures in the maintenance manual, this can be referred to in the report. The material handling description for such equipment can be reduced to just defining the required lifting/ transportation equipment and transport route. 
 - Requirements for transportation ways/roads including width and height in the different areas.
 - Description of areas where special protection of equipment is required e.g. dropped object protection, truck barriers, swinging load protection etc.
 - Material handling drawings based on equipment arrangement drawings or 3D plots including piping and valves containing the following:
    - All equipment to be handled including lifting lugs, monorails, access ways etc.
    - Table containing all tags to be handled with corresponding tags for the lifting equipment to be used.</rdl:PCA_100006768>
    <rdfs:subClassOf rdf:resource="http://rds.posccaesar.org/ontology/plm/rdl/PCA_100004908"/>
    <skos:broadMatch rdf:resource="http://rds.posccaesar.org/ontology/plm/rdl/PCA_100006695"/>
    <skos:broadMatch>
      <rdl:PCA_100001503 rdf:about="http://rds.posccaesar.org/ontology/plm/rdl/PCA_100006697">
        <rdfs:label>human-machine interface information</rdfs:label>
        <rdl:PCA_100004924>FC</rdl:PCA_100004924>
        <rdf:type rdf:resource="http://www.w3.org/2002/07/owl#NamedIndividual"/>
      </rdl:PCA_100001503>
    </skos:broadMatch>
    <skos:broadMatch rdf:resource="http://rds.posccaesar.org/ontology/plm/rdl/PCA_100006687"/>
    <skos:broadMatch rdf:resource="http://rds.posccaesar.org/ontology/plm/rdl/PCA_100006726"/>
    <rdl:PCA_100006765 rdf:resource="http://w3id.org/readi/rdl/CFIHOS-20000020"/>
    <skos:broadMatch rdf:resource="http://rds.posccaesar.org/ontology/plm/rdl/PCA_100006727"/>
  </owl:Class>
  <owl:Class rdf:about="http://rds.posccaesar.org/ontology/plm/rdl/PCA_100006303">
    <skos:broader rdf:resource="http://rds.posccaesar.org/ontology/plm/rdl/PCA_100006748"/>
    <skos:broadMatch rdf:resource="http://rds.posccaesar.org/ontology/plm/rdl/PCA_100006716"/>
    <rdfs:label>Main equipment list</rdfs:label>
    <rdfs:comment>The list should include, but not be limited to, the following information: 
 - part number/material number (complete designation) 
 - part number/material number (complete designation) 
 - part number/material number (complete designation) 
 - reference to catalogue and/or data sheets
 - tag number</rdfs:comment>
    <rdl:PCA_100006768>The list should include, but not be limited to, the following information: 
 - part number/material number (complete designation) 
 - part number/material number (complete designation) 
 - part number/material number (complete designation) 
 - reference to catalogue and/or data sheets
 - tag number</rdl:PCA_100006768>
    <rdl:PCA_100006766 rdf:resource="http://rds.posccaesar.org/ontology/plm/rdl/PCA_100006653"/>
    <rdl:PCA_100006763>The master equipment list shall be prepared for all types of assembled equipment.</rdl:PCA_100006763>
    <rdfs:subClassOf rdf:resource="http://rds.posccaesar.org/ontology/plm/rdl/PCA_100004908"/>
  </owl:Class>
  <owl:Class rdf:about="http://rds.posccaesar.org/ontology/plm/rdl/PCA_100006424">
    <rdl:PCA_100006766 rdf:resource="http://rds.posccaesar.org/ontology/plm/rdl/PCA_100006653"/>
    <rdfs:label>Safety and automation system (SAS) communication test report (UFAT)</rdfs:label>
    <rdl:PCA_100006768>This document shall include SAS communication test report (UFAT)</rdl:PCA_100006768>
    <rdl:PCA_100006765 rdf:resource="http://w3id.org/readi/rdl/CFIHOS-20000027"/>
    <rdfs:comment>This document shall include SAS communication test report (UFAT)</rdfs:comment>
    <skos:broader rdf:resource="http://rds.posccaesar.org/ontology/plm/rdl/PCA_100006756"/>
    <rdl:PCA_100006763>Required by the SAS supplier to configure his communication lines prior to test activities</rdl:PCA_100006763>
    <skos:broadMatch rdf:resource="http://rds.posccaesar.org/ontology/plm/rdl/PCA_100006722"/>
    <rdfs:subClassOf rdf:resource="http://rds.posccaesar.org/ontology/plm/rdl/PCA_100004908"/>
  </owl:Class>
  <owl:Class rdf:about="http://rds.posccaesar.org/ontology/plm/rdl/PCA_100006412">
    <skos:broader rdf:resource="http://rds.posccaesar.org/ontology/plm/rdl/PCA_100006752"/>
    <rdfs:label>Repair philosophy</rdfs:label>
    <rdfs:comment>Repair philosophy for pipelines shall be delivered, fulfilling the requirements DVGL-ST-F101.</rdfs:comment>
    <rdl:PCA_100006768>Repair philosophy for pipelines shall be delivered, fulfilling the requirements DVGL-ST-F101.</rdl:PCA_100006768>
    <rdl:PCA_100006766 rdf:resource="http://rds.posccaesar.org/ontology/plm/rdl/PCA_100006654"/>
    <rdl:PCA_100006765 rdf:resource="http://w3id.org/readi/rdl/CFIHOS-20000018"/>
    <rdl:PCA_100006763>Ensure safe operation</rdl:PCA_100006763>
    <rdfs:subClassOf rdf:resource="http://rds.posccaesar.org/ontology/plm/rdl/PCA_100004908"/>
  </owl:Class>
  <owl:Class rdf:about="http://rds.posccaesar.org/ontology/plm/rdl/PCA_100006521">
    <skos:broader rdf:resource="http://rds.posccaesar.org/ontology/plm/rdl/PCA_100006756"/>
    <skos:broadMatch rdf:resource="http://rds.posccaesar.org/ontology/plm/rdl/PCA_100006722"/>
    <rdfs:label>Valve and operator test reports</rdfs:label>
    <rdfs:comment>The following test reports are required: 1. Fugitive emission test reports when specified by Purchaser 2. Test reports from qualification of non-collapsible choke valves when specified by Purchaser 3. For intelligent positioner with 4-20 mA input and HART or Fieldbus communication and diagnostic possibilities, a documented footprint/valve signature from FAT shall be delivered in a file with ZIP format (containing the data in native format) in addition to PDF. 4. FAT reports 5. FAT reports for actuators according to TR0038 Valve and operator test reports shall be delivered in PDF format with the addition described above for the intelligent positioner.</rdfs:comment>
    <rdl:PCA_100006768>The following test reports are required: 1. Fugitive emission test reports when specified by Purchaser 2. Test reports from qualification of non-collapsible choke valves when specified by Purchaser 3. For intelligent positioner with 4-20 mA input and HART or Fieldbus communication and diagnostic possibilities, a documented footprint/valve signature from FAT shall be delivered in a file with ZIP format (containing the data in native format) in addition to PDF. 4. FAT reports 5. FAT reports for actuators according to TR0038 Valve and operator test reports shall be delivered in PDF format with the addition described above for the intelligent positioner.</rdl:PCA_100006768>
    <rdl:PCA_100006765 rdf:resource="http://w3id.org/readi/rdl/CFIHOS-20000027"/>
    <rdfs:subClassOf rdf:resource="http://rds.posccaesar.org/ontology/plm/rdl/PCA_100004908"/>
  </owl:Class>
  <owl:Class rdf:about="http://rds.posccaesar.org/ontology/plm/rdl/PCA_100006400">
    <rdl:PCA_100006765 rdf:resource="http://w3id.org/readi/rdl/CFIHOS-20000013"/>
    <skos:broadMatch rdf:resource="http://rds.posccaesar.org/ontology/plm/rdl/PCA_100006716"/>
    <rdl:PCA_100006763>Document shall give the user a structured setup on how to document the setting of parameters for given protection.</rdl:PCA_100006763>
    <rdfs:subClassOf rdf:resource="http://rds.posccaesar.org/ontology/plm/rdl/PCA_100004908"/>
    <skos:broader rdf:resource="http://rds.posccaesar.org/ontology/plm/rdl/PCA_100006748"/>
    <rdl:PCA_100006766 rdf:resource="http://rds.posccaesar.org/ontology/plm/rdl/PCA_100006653"/>
    <rdl:PCA_100006768>The document shall contain a template including all adjustable parameters, indicating which parameters are fixed by the project. For parameters which have individual setting the criteria/formula for defining/calculating the individual setting shall be given. In addition the document shall include a table listing all individual settings. This table shall on one axis list all equipment and the other all parameter requiring individual setting.</rdl:PCA_100006768>
    <rdfs:label>Protective device setting list</rdfs:label>
    <rdfs:comment>The document shall contain a template including all adjustable parameters, indicating which parameters are fixed by the project. For parameters which have individual setting the criteria/formula for defining/calculating the individual setting shall be given. In addition the document shall include a table listing all individual settings. This table shall on one axis list all equipment and the other all parameter requiring individual setting.</rdfs:comment>
  </owl:Class>
  <owl:Class rdf:about="http://rds.posccaesar.org/ontology/plm/rdl/PCA_100006533">
    <skos:broader rdf:resource="http://rds.posccaesar.org/ontology/plm/rdl/PCA_100006756"/>
    <skos:broadMatch rdf:resource="http://rds.posccaesar.org/ontology/plm/rdl/PCA_100006733"/>
    <rdfs:label>Welding plan</rdfs:label>
    <rdfs:comment>Report containing all weld numbers in a series or an assembly with reference
to WPS, WPQR, welder, PWHT, NDT etc.</rdfs:comment>
    <rdl:PCA_100006768>Report containing all weld numbers in a series or an assembly with reference
to WPS, WPQR, welder, PWHT, NDT etc.</rdl:PCA_100006768>
    <rdl:PCA_100006766 rdf:resource="http://rds.posccaesar.org/ontology/plm/rdl/PCA_100006653"/>
    <rdl:PCA_100006763>To document weld traceability.</rdl:PCA_100006763>
    <rdfs:subClassOf rdf:resource="http://rds.posccaesar.org/ontology/plm/rdl/PCA_100004908"/>
  </owl:Class>
  <owl:Class rdf:about="http://rds.posccaesar.org/ontology/plm/rdl/PCA_100006180">
    <rdl:PCA_100006763>Power System Philosophy shall outline the design and operation of the electrical power supply and distribution systems. The document shall be the guideline for the electrical system detail design, supplier equipment and software deliveries to the power systems like switchboards, generators, variable speed drives etc.</rdl:PCA_100006763>
    <rdl:PCA_100006768>The document shall include an overview of:
 - The overall power system;
 - The hardwired electrical interlock/inter-tripping principles throughout the electrical distribution system;
 - An overview of the control philosophy;
 - The general principles for the Power Distribution Control System (PDCS);
 - The power management functions;
 - The operating requirements and interface between control facilities and electrical equipment;
 - The principles for remote access and monitoring of the electrical equipment.

The document shall further describe the various operating modes of the power system like:
 - Normal modes;
 - Emergency modes;
 - Maintenance modes;
 - Others (as applicable).

The reliability of the grid supply shall be assessed (if applicable).</rdl:PCA_100006768>
    <rdl:PCA_100006766 rdf:resource="http://rds.posccaesar.org/ontology/plm/rdl/PCA_100006634"/>
    <rdl:PCA_100006766 rdf:resource="http://rds.posccaesar.org/ontology/plm/rdl/PCA_100006639"/>
    <skos:broadMatch rdf:resource="http://rds.posccaesar.org/ontology/plm/rdl/PCA_100006698"/>
    <skos:broader rdf:resource="http://rds.posccaesar.org/ontology/plm/rdl/PCA_100006752"/>
    <rdl:PCA_100006766 rdf:resource="http://rds.posccaesar.org/ontology/plm/rdl/PCA_100006636"/>
    <rdl:PCA_100006765 rdf:resource="http://w3id.org/readi/rdl/CFIHOS-20000008"/>
    <rdfs:label>Electrical power system philosophy</rdfs:label>
    <skos:broadMatch rdf:resource="http://rds.posccaesar.org/ontology/plm/rdl/PCA_100006695"/>
    <rdl:PCA_100006766 rdf:resource="http://rds.posccaesar.org/ontology/plm/rdl/PCA_100006638"/>
    <rdfs:comment>The document shall include an overview of:
 - The overall power system;
 - The hardwired electrical interlock/inter-tripping principles throughout the electrical distribution system;
 - An overview of the control philosophy;
 - The general principles for the Power Distribution Control System (PDCS);
 - The power management functions;
 - The operating requirements and interface between control facilities and electrical equipment;
 - The principles for remote access and monitoring of the electrical equipment.

The document shall further describe the various operating modes of the power system like:
 - Normal modes;
 - Emergency modes;
 - Maintenance modes;
 - Others (as applicable).

The reliability of the grid supply shall be assessed (if applicable).</rdfs:comment>
    <rdfs:subClassOf rdf:resource="http://rds.posccaesar.org/ontology/plm/rdl/PCA_100004908"/>
    <rdl:PCA_100006766 rdf:resource="http://rds.posccaesar.org/ontology/plm/rdl/PCA_100006635"/>
    <rdl:PCA_100006766 rdf:resource="http://rds.posccaesar.org/ontology/plm/rdl/PCA_100006641"/>
    <rdl:PCA_100006766 rdf:resource="http://rds.posccaesar.org/ontology/plm/rdl/PCA_100006637"/>
  </owl:Class>
  <owl:Class rdf:about="http://rds.posccaesar.org/ontology/plm/rdl/PCA_100006192">
    <rdl:PCA_100006763>This document is required to allow use of equipment in hazardous areas.</rdl:PCA_100006763>
    <rdfs:comment>The equipment’s explosion protection certificate shall be delivered according to recognized standards.

This certificate proves that equipment conforms to the specific standard for the type of explosion protection, e.g. ATEX, IEC
This document shall provide input to IS-calculations, special requirements for safe use, barrier/isolator to be used, etc.</rdfs:comment>
    <rdl:PCA_100006765 rdf:resource="http://w3id.org/readi/rdl/CFIHOS-20000013"/>
    <rdl:PCA_100006766 rdf:resource="http://rds.posccaesar.org/ontology/plm/rdl/PCA_100006653"/>
    <rdl:PCA_100006764>Attestation issued by a recognised independent authority certifying that a type test has satisfied the specified standards; e.g.  ATEX, BASEEFA, PTB, UL, CSA, NEMA, EX, etc. Examples of ratings include Intrinsically Safe &amp; Explosion Proof. To include any special requirements for safe use, barrier/isolator to be used, etc.</rdl:PCA_100006764>
    <skos:broader rdf:resource="http://rds.posccaesar.org/ontology/plm/rdl/PCA_100006743"/>
    <rdfs:subClassOf rdf:resource="http://rds.posccaesar.org/ontology/plm/rdl/PCA_100004908"/>
    <skos:broadMatch rdf:resource="http://rds.posccaesar.org/ontology/plm/rdl/PCA_100006722"/>
    <rdfs:label>EX certificate</rdfs:label>
    <rdl:PCA_100006768>The equipment’s explosion protection certificate shall be delivered according to recognized standards.

This certificate proves that equipment conforms to the specific standard for the type of explosion protection, e.g. ATEX, IEC
This document shall provide input to IS-calculations, special requirements for safe use, barrier/isolator to be used, etc.</rdl:PCA_100006768>
    <skos:broadMatch rdf:resource="http://rds.posccaesar.org/ontology/plm/rdl/PCA_100006727"/>
  </owl:Class>
  <owl:Class rdf:about="http://rds.posccaesar.org/ontology/plm/rdl/PCA_100006083">
    <rdfs:label>Additional studies</rdfs:label>
    <rdfs:comment>All additional studies required for the specific scope for the project/plant shall be delivered. This may include:
 - Technology qualification studies;
 - 3rd party studies, e.g. special studies and verification studies.
These studies shall be delivered as LCI also when performed in project phases prior to the execution phase.</rdfs:comment>
    <rdl:PCA_100006768>All additional studies required for the specific scope for the project/plant shall be delivered. This may include:
 - Technology qualification studies;
 - 3rd party studies, e.g. special studies and verification studies.
These studies shall be delivered as LCI also when performed in project phases prior to the execution phase.</rdl:PCA_100006768>
    <rdl:PCA_100006766 rdf:resource="http://rds.posccaesar.org/ontology/plm/rdl/PCA_100006654"/>
    <rdfs:subClassOf rdf:resource="http://rds.posccaesar.org/ontology/plm/rdl/PCA_100004908"/>
  </owl:Class>
  <owl:Class rdf:about="http://rds.posccaesar.org/ontology/plm/rdl/PCA_100006095">
    <skos:broader rdf:resource="http://rds.posccaesar.org/ontology/plm/rdl/PCA_100006745"/>
    <skos:broadMatch rdf:resource="http://rds.posccaesar.org/ontology/plm/rdl/PCA_100006696"/>
    <rdfs:label>Area duct &amp; and instrumentation diagrams (D&amp;ID)</rdfs:label>
    <rdfs:comment>The complete Area Duct &amp; and Instrumentation Diagrams (D&amp;ID) shall be in accordance with the plants’ process typicals and drafting standard.

The level of detail within packages shall be identical to that outside.
Tag number shall be shown for all tagged components including manual valves.

Area Duct &amp; Instrumentation Diagram (D&amp;ID) shall be provided by area and include the following information:
 - All relevant HVAC system within the defined area;
 - All HVAC equipment with their tag number and all HVAC bulk items with their item number;
 - Equipment data summary with tag number for all equipment such as filters, fans, coils, etc.;
 - All ductwork identified with system no., sizes, duct classes, insulation classes;
 - All inline equipment;
 - Air flow to all serviced areas;
 - Area breaks and duct class breaks;
 - All areas/rooms served to be identified;
 - All instrument locations shall be indicated and completed with tag numbers;
 - Connections to other systems e.g. sea water, heating, cooling, drain, etc.;
 - Airflow in and out of diagram with references;
 - Fire partitions with fire rating.</rdfs:comment>
    <rdl:PCA_100006768>The complete Area Duct &amp; and Instrumentation Diagrams (D&amp;ID) shall be in accordance with the plants’ process typicals and drafting standard.

The level of detail within packages shall be identical to that outside.
Tag number shall be shown for all tagged components including manual valves.

Area Duct &amp; Instrumentation Diagram (D&amp;ID) shall be provided by area and include the following information:
 - All relevant HVAC system within the defined area;
 - All HVAC equipment with their tag number and all HVAC bulk items with their item number;
 - Equipment data summary with tag number for all equipment such as filters, fans, coils, etc.;
 - All ductwork identified with system no., sizes, duct classes, insulation classes;
 - All inline equipment;
 - Air flow to all serviced areas;
 - Area breaks and duct class breaks;
 - All areas/rooms served to be identified;
 - All instrument locations shall be indicated and completed with tag numbers;
 - Connections to other systems e.g. sea water, heating, cooling, drain, etc.;
 - Airflow in and out of diagram with references;
 - Fire partitions with fire rating.</rdl:PCA_100006768>
    <rdl:PCA_100006766 rdf:resource="http://rds.posccaesar.org/ontology/plm/rdl/PCA_100006650"/>
    <rdl:PCA_100006765 rdf:resource="http://w3id.org/readi/rdl/CFIHOS-20000019"/>
    <rdfs:subClassOf rdf:resource="http://rds.posccaesar.org/ontology/plm/rdl/PCA_100004908"/>
  </owl:Class>
  <owl:Class rdf:about="http://rds.posccaesar.org/ontology/plm/rdl/PCA_100006449">
    <skos:broader rdf:resource="http://rds.posccaesar.org/ontology/plm/rdl/PCA_100006756"/>
    <skos:broadMatch>
      <rdl:PCA_100001503 rdf:about="http://rds.posccaesar.org/ontology/plm/rdl/PCA_100006703">
        <rdfs:label>software information</rdfs:label>
        <rdl:PCA_100004924>FT</rdl:PCA_100004924>
        <rdf:type rdf:resource="http://www.w3.org/2002/07/owl#NamedIndividual"/>
      </rdl:PCA_100001503>
    </skos:broadMatch>
    <rdfs:label>Software function description</rdfs:label>
    <rdfs:comment>Example of content:
 - Overall system description
 - Subsystem descriptions
 - Program descriptions
 - Module descriptions
 - Data structure descriptions
 - Software environment description.</rdfs:comment>
    <rdl:PCA_100006768>Example of content:
 - Overall system description
 - Subsystem descriptions
 - Program descriptions
 - Module descriptions
 - Data structure descriptions
 - Software environment description.</rdl:PCA_100006768>
    <rdl:PCA_100006766 rdf:resource="http://rds.posccaesar.org/ontology/plm/rdl/PCA_100006653"/>
    <rdl:PCA_100006763>This document shall support design and verification of compliance. Documenting functionality and SW replacement</rdl:PCA_100006763>
    <rdfs:subClassOf rdf:resource="http://rds.posccaesar.org/ontology/plm/rdl/PCA_100004908"/>
  </owl:Class>
  <owl:Class rdf:about="http://rds.posccaesar.org/ontology/plm/rdl/PCA_100006328">
    <rdl:PCA_100006766 rdf:resource="http://rds.posccaesar.org/ontology/plm/rdl/PCA_100006647"/>
    <rdfs:label>Mooring analysis reports</rdfs:label>
    <rdl:PCA_100006763>Mooring analysis reports shall be delivered. The report or collection of reports shall contain the final documentation of the mooring system.</rdl:PCA_100006763>
    <rdfs:comment>The report shall typically contain:
 - Design basis including rules and regulations, design life, location, water depth, environmental conditions, corrosion allowance and marine growth;
 - Design criteria including safety factors, offset requirements and fatigue;
 - Vessel particulars;
 - Design method and input parameters;
 - Analysis results;
 - Description for final mooring system layout and components.</rdfs:comment>
    <rdl:PCA_100006765 rdf:resource="http://w3id.org/readi/rdl/CFIHOS-20000033"/>
    <rdl:PCA_100006768>The report shall typically contain:
 - Design basis including rules and regulations, design life, location, water depth, environmental conditions, corrosion allowance and marine growth;
 - Design criteria including safety factors, offset requirements and fatigue;
 - Vessel particulars;
 - Design method and input parameters;
 - Analysis results;
 - Description for final mooring system layout and components.</rdl:PCA_100006768>
    <skos:broadMatch rdf:resource="http://rds.posccaesar.org/ontology/plm/rdl/PCA_100006687"/>
    <rdfs:subClassOf rdf:resource="http://rds.posccaesar.org/ontology/plm/rdl/PCA_100004908"/>
    <skos:broader rdf:resource="http://rds.posccaesar.org/ontology/plm/rdl/PCA_100006756"/>
  </owl:Class>
  <owl:Class rdf:about="http://rds.posccaesar.org/ontology/plm/rdl/PCA_100006316">
    <rdfs:comment>Summarise materials selected for the various components and their compatibility with fluids.</rdfs:comment>
    <rdl:PCA_100006765 rdf:resource="http://w3id.org/readi/rdl/CFIHOS-20000031"/>
    <rdfs:label>Material selection</rdfs:label>
    <rdfs:subClassOf rdf:resource="http://rds.posccaesar.org/ontology/plm/rdl/PCA_100004908"/>
    <rdl:PCA_100006768>Summarise materials selected for the various components and their compatibility with fluids.</rdl:PCA_100006768>
    <skos:broadMatch rdf:resource="http://rds.posccaesar.org/ontology/plm/rdl/PCA_100006686"/>
    <rdl:PCA_100006763>Identify materials proposed used and document fluid compatibility for material selected.</rdl:PCA_100006763>
    <rdl:PCA_100006766 rdf:resource="http://rds.posccaesar.org/ontology/plm/rdl/PCA_100006653"/>
    <skos:broader rdf:resource="http://rds.posccaesar.org/ontology/plm/rdl/PCA_100006756"/>
  </owl:Class>
  <owl:Class rdf:about="http://rds.posccaesar.org/ontology/plm/rdl/PCA_100006437">
    <rdl:PCA_100006766 rdf:resource="http://rds.posccaesar.org/ontology/plm/rdl/PCA_100006636"/>
    <rdl:PCA_100006766 rdf:resource="http://rds.posccaesar.org/ontology/plm/rdl/PCA_100006638"/>
    <rdl:PCA_100006766 rdf:resource="http://rds.posccaesar.org/ontology/plm/rdl/PCA_100006633"/>
    <rdl:PCA_100006765 rdf:resource="http://w3id.org/readi/rdl/CFIHOS-20000015"/>
    <rdfs:label>Shutdown hierarchy</rdfs:label>
    <rdl:PCA_100006766 rdf:resource="http://rds.posccaesar.org/ontology/plm/rdl/PCA_100006639"/>
    <rdl:PCA_100006766 rdf:resource="http://rds.posccaesar.org/ontology/plm/rdl/PCA_100006634"/>
    <rdl:PCA_100006766 rdf:resource="http://rds.posccaesar.org/ontology/plm/rdl/PCA_100006635"/>
    <rdl:PCA_100006763>The purpose of the "Shutdown hierarchy" diagrams is to give an overview of the different shutdown levels and present the levels in a hierarchical way.  Refer to NORSOK S-001 chapter 11.4.3 fig. 4 for a typical shutdown hierarchy for ESD.</rdl:PCA_100006763>
    <rdl:PCA_100006766 rdf:resource="http://rds.posccaesar.org/ontology/plm/rdl/PCA_100006637"/>
    <skos:broadMatch rdf:resource="http://rds.posccaesar.org/ontology/plm/rdl/PCA_100006727"/>
    <rdfs:subClassOf rdf:resource="http://rds.posccaesar.org/ontology/plm/rdl/PCA_100004908"/>
    <skos:broader rdf:resource="http://rds.posccaesar.org/ontology/plm/rdl/PCA_100006745"/>
    <rdl:PCA_100006766 rdf:resource="http://rds.posccaesar.org/ontology/plm/rdl/PCA_100006626"/>
    <rdl:PCA_100006766 rdf:resource="http://rds.posccaesar.org/ontology/plm/rdl/PCA_100006641"/>
  </owl:Class>
  <owl:Class rdf:about="http://rds.posccaesar.org/ontology/plm/rdl/PCA_100006425">
    <skos:broader rdf:resource="http://rds.posccaesar.org/ontology/plm/rdl/PCA_100006747"/>
    <rdfs:label>Safety data sheet</rdfs:label>
    <rdl:PCA_100006763>A structured form containing information on the safety, health and environmental protection aspects of the chemical, including protective measures and emergency actions.

ISO 11014 Safety data sheet for chemical products.</rdl:PCA_100006763>
    <rdfs:subClassOf rdf:resource="http://rds.posccaesar.org/ontology/plm/rdl/PCA_100004908"/>
    <rdl:PCA_100006765 rdf:resource="http://w3id.org/readi/rdl/CFIHOS-20000013"/>
    <rdl:PCA_100006768>A structured form containing information on the safety, health and environmental protection aspects of the material, including protective measures and
emergency actions.
SDS shall be according to local/national regulations  and in the official language plant is/will be operated, or in English if accepted by local authorities.
A collection of Safety Data Sheets (SDS) shall be delivered to Company, for chemicals delivered as part of equipment, as first fill or used for preservation before operation.
Exceptions are
 - grease
 - fat
 - surface preservatives
 - coatings
 - oils in volume per equipment below 10 litres.
The report shall include one SDS per unique chemical trade name. A cross reference table with each unique chemical trade name, equipment tag number(s) and SDS file name shall also be included.</rdl:PCA_100006768>
    <skos:broadMatch rdf:resource="http://rds.posccaesar.org/ontology/plm/rdl/PCA_100006686"/>
    <rdfs:comment>A structured form containing information on the safety, health and environmental protection aspects of the material, including protective measures and
emergency actions.
SDS shall be according to local/national regulations  and in the official language plant is/will be operated, or in English if accepted by local authorities.
A collection of Safety Data Sheets (SDS) shall be delivered to Company, for chemicals delivered as part of equipment, as first fill or used for preservation before operation.
Exceptions are
 - grease
 - fat
 - surface preservatives
 - coatings
 - oils in volume per equipment below 10 litres.
The report shall include one SDS per unique chemical trade name. A cross reference table with each unique chemical trade name, equipment tag number(s) and SDS file name shall also be included.</rdfs:comment>
    <rdl:PCA_100006766 rdf:resource="http://rds.posccaesar.org/ontology/plm/rdl/PCA_100006653"/>
  </owl:Class>
  <owl:Class rdf:about="http://rds.posccaesar.org/ontology/plm/rdl/PCA_100006534">
    <rdl:PCA_100006768>Welding and material test records as set out by the welding procedure qualification
This record  shall contain all necessary data needed for qualification of a welding procedure specification.</rdl:PCA_100006768>
    <skos:broadMatch rdf:resource="http://rds.posccaesar.org/ontology/plm/rdl/PCA_100006672"/>
    <rdl:PCA_100006763>A document containing data which records compliance with specified procedure. 
* This document is a part of the Quality Assurance Plan, and herein the Quality Control  work process and verification.</rdl:PCA_100006763>
    <rdfs:label>Welding procedure qualification record</rdfs:label>
    <skos:broadMatch rdf:resource="http://rds.posccaesar.org/ontology/plm/rdl/PCA_100006722"/>
    <rdfs:comment>Welding and material test records as set out by the welding procedure qualification
This record  shall contain all necessary data needed for qualification of a welding procedure specification.</rdfs:comment>
    <rdl:PCA_100006766 rdf:resource="http://rds.posccaesar.org/ontology/plm/rdl/PCA_100006653"/>
    <rdl:PCA_100006764>Requirements related to assurance and check of quality in manufacturing phase will very much depend on Purchaser’s knowledge of supplier. Well known supplier, with proven track record, delivering products based on industry standards, will typically deliver less verification documentation to Purchaser than unknown/new supplier delivering the same product. Therefore, this deliverable should be evaluated as candidate for being available in digital format to Purchaser, for information only.</rdl:PCA_100006764>
    <rdfs:subClassOf rdf:resource="http://rds.posccaesar.org/ontology/plm/rdl/PCA_100004908"/>
    <skos:broader rdf:resource="http://rds.posccaesar.org/ontology/plm/rdl/PCA_100006751"/>
  </owl:Class>
  <owl:Class rdf:about="http://rds.posccaesar.org/ontology/plm/rdl/PCA_100006304">
    <skos:broadMatch rdf:resource="http://rds.posccaesar.org/ontology/plm/rdl/PCA_100006722"/>
    <skos:broader rdf:resource="http://rds.posccaesar.org/ontology/plm/rdl/PCA_100006762"/>
    <rdl:PCA_100006765 rdf:resource="http://w3id.org/readi/rdl/CFIHOS-20000031"/>
    <rdfs:label>Manufacturing and quality control records</rdfs:label>
    <rdfs:comment>A compiled document containing as-built records/documents, signed reports, certificates and drawings.</rdfs:comment>
    <rdfs:subClassOf rdf:resource="http://rds.posccaesar.org/ontology/plm/rdl/PCA_100004908"/>
    <rdl:PCA_100006768>A compiled document containing as-built records/documents, signed reports, certificates and drawings.</rdl:PCA_100006768>
    <rdl:PCA_100006766 rdf:resource="http://rds.posccaesar.org/ontology/plm/rdl/PCA_100006653"/>
    <skos:broader rdf:resource="http://rds.posccaesar.org/ontology/plm/rdl/PCA_100006756"/>
    <rdl:PCA_100006763>Ensuring evidence and traceability on construction, manufacturing, testing, reporting and certification for equipment or material.</rdl:PCA_100006763>
  </owl:Class>
  <owl:Class rdf:about="http://rds.posccaesar.org/ontology/plm/rdl/PCA_100006413">
    <skos:broader rdf:resource="http://rds.posccaesar.org/ontology/plm/rdl/PCA_100006756"/>
    <rdl:PCA_100006768>Noise and vibration data shall be reported</rdl:PCA_100006768>
    <rdl:PCA_100006763>Document providing information about noise levels.</rdl:PCA_100006763>
    <skos:broadMatch rdf:resource="http://rds.posccaesar.org/ontology/plm/rdl/PCA_100006722"/>
    <rdl:PCA_100006765 rdf:resource="http://w3id.org/readi/rdl/CFIHOS-20000011"/>
    <rdl:PCA_100006765>
      <rdl:PCA_100001503 rdf:about="http://w3id.org/readi/rdl/CFIHOS-20000014">
        <rdfs:label>health, safety, environmental and security</rdfs:label>
        <rdl:PCA_100004924>HX</rdl:PCA_100004924>
        <rdf:type rdf:resource="http://www.w3.org/2002/07/owl#NamedIndividual"/>
      </rdl:PCA_100001503>
    </rdl:PCA_100006765>
    <rdl:PCA_100006766 rdf:resource="http://rds.posccaesar.org/ontology/plm/rdl/PCA_100006653"/>
    <rdfs:comment>Noise and vibration data shall be reported</rdfs:comment>
    <rdfs:subClassOf rdf:resource="http://rds.posccaesar.org/ontology/plm/rdl/PCA_100004908"/>
    <rdfs:label>Report - Noise test - HSE</rdfs:label>
  </owl:Class>
  <owl:Class rdf:about="http://rds.posccaesar.org/ontology/plm/rdl/PCA_100006546">
    <rdfs:label>Workshop maintenance manuals</rdfs:label>
    <rdfs:comment>The Workshop maintenance manuals shall be used for subsea equipment, and equipment related to the subsea equipment. The Workshop maintenance manuals shall include: 1. All necessary procedures to perform Mobilisation &amp; demobilisation 2. All necessary procedures to perform component replacement 3. All necessary procedures to perform Main overhaul

General 
Main overhaul includes all inspections, measurements, acceptance criteria’s, adjustments and operations carried out directly on the equipment in order to ensure safe, reliable and economical operation. This item must be seen in combination with the installation, operation and maintenance manual (IOM manual). Typical equipment and operations this is relevant for see table below. The O marked section(s,) the required workshop maintenance manual section shall be retained by vendor and made available upon request for Company.</rdfs:comment>
    <rdl:PCA_100006768>The Workshop maintenance manuals shall be used for subsea equipment, and equipment related to the subsea equipment. The Workshop maintenance manuals shall include: 1. All necessary procedures to perform Mobilisation &amp; demobilisation 2. All necessary procedures to perform component replacement 3. All necessary procedures to perform Main overhaul

General 
Main overhaul includes all inspections, measurements, acceptance criteria’s, adjustments and operations carried out directly on the equipment in order to ensure safe, reliable and economical operation. This item must be seen in combination with the installation, operation and maintenance manual (IOM manual). Typical equipment and operations this is relevant for see table below. The O marked section(s,) the required workshop maintenance manual section shall be retained by vendor and made available upon request for Company.</rdl:PCA_100006768>
    <rdl:PCA_100006764>Tabell tilhørende 5.248, SR-2800, Workshop maintenance manuals</rdl:PCA_100006764>
    <rdfs:subClassOf rdf:resource="http://rds.posccaesar.org/ontology/plm/rdl/PCA_100004908"/>
  </owl:Class>
  <owl:Class rdf:about="http://rds.posccaesar.org/ontology/plm/rdl/PCA_100006401">
    <skos:broader rdf:resource="http://rds.posccaesar.org/ontology/plm/rdl/PCA_100006756"/>
    <skos:broadMatch rdf:resource="http://rds.posccaesar.org/ontology/plm/rdl/PCA_100006722"/>
    <rdfs:label>Qualification dossier for bending</rdfs:label>
    <rdfs:comment>Bending results/report (including dimensions and material)</rdfs:comment>
    <rdl:PCA_100006768>Bending results/report (including dimensions and material)</rdl:PCA_100006768>
    <rdl:PCA_100006766 rdf:resource="http://rds.posccaesar.org/ontology/plm/rdl/PCA_100006653"/>
    <rdl:PCA_100006763>Assembled report for verification of procedures followed and delivery according to bending procedure</rdl:PCA_100006763>
    <rdfs:subClassOf rdf:resource="http://rds.posccaesar.org/ontology/plm/rdl/PCA_100004908"/>
  </owl:Class>
  <owl:Class rdf:about="http://rds.posccaesar.org/ontology/plm/rdl/PCA_100006510">
    <rdfs:subClassOf rdf:resource="http://rds.posccaesar.org/ontology/plm/rdl/PCA_100004908"/>
    <rdfs:label>Turret system report</rdfs:label>
    <skos:broader rdf:resource="http://rds.posccaesar.org/ontology/plm/rdl/PCA_100006756"/>
    <rdl:PCA_100006763>Technical documentation of all mechanical and structural components of the turret shall be delivered.</rdl:PCA_100006763>
    <rdl:PCA_100006766 rdf:resource="http://rds.posccaesar.org/ontology/plm/rdl/PCA_100006657"/>
    <rdfs:comment>This documentation shall include the following:
 - General arrangement drawings;
 - Detail drawings of all major components;
 - Design analyses of all major components;
 - Material certificates for all components including welding filler material along with traceability data;
 - Turret / turning system procedures (if relevant);
 - Procedures necessary to safely operate, maintain and replace mechanical components.</rdfs:comment>
    <rdl:PCA_100006765 rdf:resource="http://w3id.org/readi/rdl/CFIHOS-20000033"/>
    <rdl:PCA_100006768>This documentation shall include the following:
 - General arrangement drawings;
 - Detail drawings of all major components;
 - Design analyses of all major components;
 - Material certificates for all components including welding filler material along with traceability data;
 - Turret / turning system procedures (if relevant);
 - Procedures necessary to safely operate, maintain and replace mechanical components.</rdl:PCA_100006768>
    <skos:broadMatch rdf:resource="http://rds.posccaesar.org/ontology/plm/rdl/PCA_100006698"/>
  </owl:Class>
  <owl:Class rdf:about="http://rds.posccaesar.org/ontology/plm/rdl/PCA_100006522">
    <skos:broader rdf:resource="http://rds.posccaesar.org/ontology/plm/rdl/PCA_100006756"/>
    <rdl:PCA_100006763>Report documenting all calculations and analysis performed with regards to bursting, propagating buckling and collapse to prove correct wall thickness design.</rdl:PCA_100006763>
    <rdfs:subClassOf rdf:resource="http://rds.posccaesar.org/ontology/plm/rdl/PCA_100004908"/>
    <rdl:PCA_100006765 rdf:resource="http://w3id.org/readi/rdl/CFIHOS-20000031"/>
    <skos:broadMatch rdf:resource="http://rds.posccaesar.org/ontology/plm/rdl/PCA_100006686"/>
    <rdl:PCA_100006766 rdf:resource="http://rds.posccaesar.org/ontology/plm/rdl/PCA_100006657"/>
    <rdfs:comment>To document the correct wall thickness design of the pipeline.</rdfs:comment>
    <rdl:PCA_100006768>To document the correct wall thickness design of the pipeline.</rdl:PCA_100006768>
    <rdfs:label>Wall thickness design (bursting, propagating buckling, collapse)</rdfs:label>
  </owl:Class>
  <owl:Class rdf:about="http://rds.posccaesar.org/ontology/plm/rdl/PCA_100006191">
    <rdl:PCA_100006766 rdf:resource="http://rds.posccaesar.org/ontology/plm/rdl/PCA_100006653"/>
    <rdfs:subClassOf rdf:resource="http://rds.posccaesar.org/ontology/plm/rdl/PCA_100004908"/>
    <skos:broadMatch>
      <rdl:PCA_100001503 rdf:about="http://rds.posccaesar.org/ontology/plm/rdl/PCA_100006724">
        <rdfs:label>conformity information</rdfs:label>
        <rdl:PCA_100004924>QE</rdl:PCA_100004924>
        <rdf:type rdf:resource="http://www.w3.org/2002/07/owl#NamedIndividual"/>
      </rdl:PCA_100001503>
    </skos:broadMatch>
    <rdfs:comment>The EU Declaration of conformity shall be written up by the manufacturer of the equipment or component, as the legal binding document from the manufacturer to the purchaser / user ensuring conformity with the relevant EU directive(s). 

EU declaration of Conformity shall be delivered according to requirements of the relevant EU - directives with respect to conformity assessment procedures and eventual necessary involvements of Notified Bodies. 

Certificate(s) of conformance, required by relevant directive(s), shall be available.</rdfs:comment>
    <skos:broader rdf:resource="http://rds.posccaesar.org/ontology/plm/rdl/PCA_100006756"/>
    <rdfs:label>EU declaration of conformity</rdfs:label>
    <rdl:PCA_100006763>Document compliance with applicable EU directives the equipment is designed to.</rdl:PCA_100006763>
    <rdl:PCA_100006768>The EU Declaration of conformity shall be written up by the manufacturer of the equipment or component, as the legal binding document from the manufacturer to the purchaser / user ensuring conformity with the relevant EU directive(s). 

EU declaration of Conformity shall be delivered according to requirements of the relevant EU - directives with respect to conformity assessment procedures and eventual necessary involvements of Notified Bodies. 

Certificate(s) of conformance, required by relevant directive(s), shall be available.</rdl:PCA_100006768>
    <rdl:PCA_100006765 rdf:resource="http://w3id.org/readi/rdl/CFIHOS-20000027"/>
  </owl:Class>
  <owl:Class rdf:about="http://rds.posccaesar.org/ontology/plm/rdl/PCA_100006082">
    <rdfs:label>Additional documentation for gas turbine exhaust systems</rdfs:label>
    <rdl:PCA_100006765 rdf:resource="http://w3id.org/readi/rdl/CFIHOS-20000023"/>
    <rdl:PCA_100006765 rdf:resource="http://w3id.org/readi/rdl/CFIHOS-20000022"/>
    <rdl:PCA_100006765>
      <rdl:PCA_100001503 rdf:about="http://w3id.org/readi/rdl/CFIHOS-20000021">
        <rdfs:label>mechanical rotating engineering</rdfs:label>
        <rdl:PCA_100004924>MR</rdl:PCA_100004924>
        <rdf:type rdf:resource="http://www.w3.org/2002/07/owl#NamedIndividual"/>
      </rdl:PCA_100001503>
    </rdl:PCA_100006765>
    <rdl:PCA_100006763>Documentation shall be in accordance with requirements in ISO21905.</rdl:PCA_100006763>
    <rdfs:subClassOf rdf:resource="http://rds.posccaesar.org/ontology/plm/rdl/PCA_100004908"/>
  </owl:Class>
  <owl:Class rdf:about="http://rds.posccaesar.org/ontology/plm/rdl/PCA_100006094">
    <rdfs:label>Area classification source of release</rdfs:label>
    <skos:broader rdf:resource="http://rds.posccaesar.org/ontology/plm/rdl/PCA_100006756"/>
    <rdfs:comment>The Area classification source of release shall describe all sources of release, medium causing hazardous area, extent of hazardous area from the release source, ventilation conditions for the area. The Area classification source of release shall be prepared in accordance with recognized area classification standards.  Examples of Area classification source of release can be found in IEC60079 and IP15.</rdfs:comment>
    <rdl:PCA_100006768>The Area classification source of release shall describe all sources of release, medium causing hazardous area, extent of hazardous area from the release source, ventilation conditions for the area. The Area classification source of release shall be prepared in accordance with recognized area classification standards.  Examples of Area classification source of release can be found in IEC60079 and IP15.</rdl:PCA_100006768>
    <rdfs:subClassOf rdf:resource="http://rds.posccaesar.org/ontology/plm/rdl/PCA_100004908"/>
    <skos:broadMatch rdf:resource="http://rds.posccaesar.org/ontology/plm/rdl/PCA_100006687"/>
    <rdl:PCA_100006766 rdf:resource="http://rds.posccaesar.org/ontology/plm/rdl/PCA_100006656"/>
    <skos:broadMatch rdf:resource="http://rds.posccaesar.org/ontology/plm/rdl/PCA_100006727"/>
    <rdl:PCA_100006765 rdf:resource="http://w3id.org/readi/rdl/CFIHOS-20000011"/>
    <rdl:PCA_100006765 rdf:resource="http://w3id.org/readi/rdl/CFIHOS-20000013"/>
    <rdl:PCA_100006765 rdf:resource="http://w3id.org/readi/rdl/CFIHOS-20000010"/>
  </owl:Class>
  <owl:Class rdf:about="http://rds.posccaesar.org/ontology/plm/rdl/PCA_100006329">
    <skos:broader rdf:resource="http://rds.posccaesar.org/ontology/plm/rdl/PCA_100006743"/>
    <skos:broadMatch rdf:resource="http://rds.posccaesar.org/ontology/plm/rdl/PCA_100006722"/>
    <rdfs:label>Mooring component certificate and fabrication documentation</rdfs:label>
    <rdfs:comment>Mooring component certificates and fabrication documentation collection report shall be delivered. All certificates and other relevant documentation issued during manufacturing of mooring components shall be organised in a logical manner (including welding filler material) along with traceability data.</rdfs:comment>
    <rdl:PCA_100006768>Mooring component certificates and fabrication documentation collection report shall be delivered. All certificates and other relevant documentation issued during manufacturing of mooring components shall be organised in a logical manner (including welding filler material) along with traceability data.</rdl:PCA_100006768>
    <rdl:PCA_100006766 rdf:resource="http://rds.posccaesar.org/ontology/plm/rdl/PCA_100006647"/>
    <rdl:PCA_100006765 rdf:resource="http://w3id.org/readi/rdl/CFIHOS-20000033"/>
    <rdfs:subClassOf rdf:resource="http://rds.posccaesar.org/ontology/plm/rdl/PCA_100004908"/>
  </owl:Class>
  <owl:Class rdf:about="http://rds.posccaesar.org/ontology/plm/rdl/PCA_100006438">
    <skos:broader rdf:resource="http://rds.posccaesar.org/ontology/plm/rdl/PCA_100006756"/>
    <rdfs:label>SIL report</rdfs:label>
    <rdfs:comment>Document the assessments and input provided to establish required safety integrity levels.</rdfs:comment>
    <rdl:PCA_100006768>Document the assessments and input provided to establish required safety integrity levels.</rdl:PCA_100006768>
    <rdl:PCA_100006766 rdf:resource="http://rds.posccaesar.org/ontology/plm/rdl/PCA_100006657"/>
    <rdl:PCA_100006765 rdf:resource="http://w3id.org/readi/rdl/CFIHOS-20000031"/>
    <rdl:PCA_100006763>Document acceptable level of SIL according to requirements.</rdl:PCA_100006763>
    <rdfs:subClassOf rdf:resource="http://rds.posccaesar.org/ontology/plm/rdl/PCA_100004908"/>
  </owl:Class>
  <owl:Class rdf:about="http://rds.posccaesar.org/ontology/plm/rdl/PCA_100006317">
    <rdfs:subClassOf rdf:resource="http://rds.posccaesar.org/ontology/plm/rdl/PCA_100004908"/>
    <rdl:PCA_100006763>Summarise materials selected for the various components and their compatibility with fluids.</rdl:PCA_100006763>
    <rdfs:label>Material selection report</rdfs:label>
    <rdl:PCA_100006765 rdf:resource="http://w3id.org/readi/rdl/CFIHOS-20000031"/>
    <rdl:PCA_100006766 rdf:resource="http://rds.posccaesar.org/ontology/plm/rdl/PCA_100006653"/>
    <rdl:PCA_100006768>Identify materials proposed used and document fluid compatibility for material selected.</rdl:PCA_100006768>
    <rdfs:comment>Identify materials proposed used and document fluid compatibility for material selected.</rdfs:comment>
    <skos:broader rdf:resource="http://rds.posccaesar.org/ontology/plm/rdl/PCA_100006756"/>
    <skos:broadMatch rdf:resource="http://rds.posccaesar.org/ontology/plm/rdl/PCA_100006686"/>
  </owl:Class>
  <owl:Class rdf:about="http://rds.posccaesar.org/ontology/plm/rdl/PCA_100006305">
    <rdfs:comment>Detailed drawings including manufacturing information such as dimensions, tolerances, materials, sling angles, lifting heights etc.</rdfs:comment>
    <skos:broader rdf:resource="http://rds.posccaesar.org/ontology/plm/rdl/PCA_100006746"/>
    <rdl:PCA_100006766 rdf:resource="http://rds.posccaesar.org/ontology/plm/rdl/PCA_100006653"/>
    <rdfs:label>Manufacturing drawing</rdfs:label>
    <rdl:PCA_100006763>Provide the manufacturer with information enable them to produce as specified.</rdl:PCA_100006763>
    <rdfs:subClassOf rdf:resource="http://rds.posccaesar.org/ontology/plm/rdl/PCA_100004908"/>
    <skos:broadMatch rdf:resource="http://rds.posccaesar.org/ontology/plm/rdl/PCA_100006733"/>
    <rdl:PCA_100006765 rdf:resource="http://w3id.org/readi/rdl/CFIHOS-20000031"/>
    <rdl:PCA_100006768>Detailed drawings including manufacturing information such as dimensions, tolerances, materials, sling angles, lifting heights etc.</rdl:PCA_100006768>
  </owl:Class>
  <owl:Class rdf:about="http://rds.posccaesar.org/ontology/plm/rdl/PCA_100006426">
    <rdl:PCA_100006765 rdf:resource="http://w3id.org/readi/rdl/CFIHOS-20000013"/>
    <rdl:PCA_100006768>The drawings shall be prepared in accordance with the requirements below.

There shall be sufficient main equipment on the drawing to easily identify the location of the equipment in question. Safety layout drawings should as far as possible use the same basis/background as other layout drawings. All equipment listed below shall be identified by:
 - Tag code;
 - Approximate dimension and geometrical form of tag.

The following safety arrangement drawings and diagrams shall be produced as follows:
 - Escape route drawings; shall include:
    - Primary escape routes with arrows indicating escape direction;
    - Secondary escape routes with direction;
    - Muster and embarkment areas;
    - Evacuation means (e.g.: lifeboats, escape chutes and rafts);
    - Areas for first aid treatment;
 - Safety equipment layout:
    - First aid equipment;
    - Safety equipment (e.g.: life jackets, life buoys, rescue equipment, MOB boat);
    - Emergency showers;
    - Emergency phones;
 - Safety sign layout:
    - Location of signs;
    - Signpost schedule including fixing details for signposts and signs;
 - Active fire protection equipment layout:
    - Location of active fire protection units (e.g. deluge, sprinkler, foam, gaseous units);
    - Manual firefighting equipment (e.g.: hydrants, hose reels, extinguishers);
    - Monitor;
 - Passive fire protection and blast protection:
    - Location of fire divisions (fire walls, deck segregation) including size and direction of dimensioning load;
    - Location of explosion resistant walls including size and direction of dimensioning load;
    - Location of explosion overpressure ventilation outlet;
 - Fire and gas detection layout:
    - Fire and gas detectors with elevation and in addition direction of view including angle up/down for flame detectors;
    - Manual Call buttons;
    - Manual active fire protection release buttons;
    - Manual ESD buttons;
    - Manual Electrical Isolation buttons (MEI), isolation of high voltage electrical equipment;
    - Warning lights, and other alarm devices.</rdl:PCA_100006768>
    <rdl:PCA_100006766 rdf:resource="http://rds.posccaesar.org/ontology/plm/rdl/PCA_100006656"/>
    <rdfs:comment>The drawings shall be prepared in accordance with the requirements below.

There shall be sufficient main equipment on the drawing to easily identify the location of the equipment in question. Safety layout drawings should as far as possible use the same basis/background as other layout drawings. All equipment listed below shall be identified by:
 - Tag code;
 - Approximate dimension and geometrical form of tag.

The following safety arrangement drawings and diagrams shall be produced as follows:
 - Escape route drawings; shall include:
    - Primary escape routes with arrows indicating escape direction;
    - Secondary escape routes with direction;
    - Muster and embarkment areas;
    - Evacuation means (e.g.: lifeboats, escape chutes and rafts);
    - Areas for first aid treatment;
 - Safety equipment layout:
    - First aid equipment;
    - Safety equipment (e.g.: life jackets, life buoys, rescue equipment, MOB boat);
    - Emergency showers;
    - Emergency phones;
 - Safety sign layout:
    - Location of signs;
    - Signpost schedule including fixing details for signposts and signs;
 - Active fire protection equipment layout:
    - Location of active fire protection units (e.g. deluge, sprinkler, foam, gaseous units);
    - Manual firefighting equipment (e.g.: hydrants, hose reels, extinguishers);
    - Monitor;
 - Passive fire protection and blast protection:
    - Location of fire divisions (fire walls, deck segregation) including size and direction of dimensioning load;
    - Location of explosion resistant walls including size and direction of dimensioning load;
    - Location of explosion overpressure ventilation outlet;
 - Fire and gas detection layout:
    - Fire and gas detectors with elevation and in addition direction of view including angle up/down for flame detectors;
    - Manual Call buttons;
    - Manual active fire protection release buttons;
    - Manual ESD buttons;
    - Manual Electrical Isolation buttons (MEI), isolation of high voltage electrical equipment;
    - Warning lights, and other alarm devices.</rdfs:comment>
    <skos:broader rdf:resource="http://rds.posccaesar.org/ontology/plm/rdl/PCA_100006746"/>
    <rdfs:subClassOf rdf:resource="http://rds.posccaesar.org/ontology/plm/rdl/PCA_100004908"/>
    <rdl:PCA_100006765 rdf:resource="http://w3id.org/readi/rdl/CFIHOS-20000011"/>
    <rdl:PCA_100006765 rdf:resource="http://w3id.org/readi/rdl/CFIHOS-20000010"/>
    <skos:broadMatch rdf:resource="http://rds.posccaesar.org/ontology/plm/rdl/PCA_100006708"/>
    <rdfs:label>Safety layout drawings</rdfs:label>
  </owl:Class>
  <owl:Class rdf:about="http://rds.posccaesar.org/ontology/plm/rdl/PCA_100006414">
    <skos:broader rdf:resource="http://rds.posccaesar.org/ontology/plm/rdl/PCA_100006746"/>
    <rdfs:label>Riser hang off drawings</rdfs:label>
    <rdfs:comment>Riser hang off drawings covering hang off of subsea lines to offshore installations.</rdfs:comment>
    <rdl:PCA_100006768>Riser hang off drawings covering hang off of subsea lines to offshore installations.</rdl:PCA_100006768>
    <rdl:PCA_100006766 rdf:resource="http://rds.posccaesar.org/ontology/plm/rdl/PCA_100006657"/>
    <rdl:PCA_100006765 rdf:resource="http://w3id.org/readi/rdl/CFIHOS-20000018"/>
    <rdl:PCA_100006763>Ensure safe operation</rdl:PCA_100006763>
    <rdfs:subClassOf rdf:resource="http://rds.posccaesar.org/ontology/plm/rdl/PCA_100004908"/>
  </owl:Class>
  <owl:Class rdf:about="http://rds.posccaesar.org/ontology/plm/rdl/PCA_100006523">
    <skos:broader rdf:resource="http://rds.posccaesar.org/ontology/plm/rdl/PCA_100006756"/>
    <skos:broadMatch rdf:resource="http://rds.posccaesar.org/ontology/plm/rdl/PCA_100006686"/>
    <rdfs:label>Wall thickness design report</rdfs:label>
    <rdl:PCA_100006766 rdf:resource="http://rds.posccaesar.org/ontology/plm/rdl/PCA_100006657"/>
    <rdl:PCA_100006765 rdf:resource="http://w3id.org/readi/rdl/CFIHOS-20000018"/>
    <rdfs:subClassOf rdf:resource="http://rds.posccaesar.org/ontology/plm/rdl/PCA_100004908"/>
  </owl:Class>
  <owl:Class rdf:about="http://rds.posccaesar.org/ontology/plm/rdl/PCA_100006402">
    <rdl:PCA_100006763>Describe the tests in sufficient detail enabling the test team to execute the tests.</rdl:PCA_100006763>
    <skos:broader rdf:resource="http://rds.posccaesar.org/ontology/plm/rdl/PCA_100006751"/>
    <skos:broadMatch rdf:resource="http://rds.posccaesar.org/ontology/plm/rdl/PCA_100006688"/>
    <rdl:PCA_100006768>Procedure describing the tests to be performed to qualify equipment in accordance design requirements and specified acceptance criteria. In many equipment standards this is called Performance Validation Test (PVT).</rdl:PCA_100006768>
    <rdfs:comment>Procedure describing the tests to be performed to qualify equipment in accordance design requirements and specified acceptance criteria. In many equipment standards this is called Performance Validation Test (PVT).</rdfs:comment>
    <rdl:PCA_100006765 rdf:resource="http://w3id.org/readi/rdl/CFIHOS-20000031"/>
    <rdl:PCA_100006766 rdf:resource="http://rds.posccaesar.org/ontology/plm/rdl/PCA_100006653"/>
    <rdfs:subClassOf rdf:resource="http://rds.posccaesar.org/ontology/plm/rdl/PCA_100004908"/>
    <rdfs:label>Qualification test procedure</rdfs:label>
  </owl:Class>
  <owl:Class rdf:about="http://rds.posccaesar.org/ontology/plm/rdl/PCA_100006535">
    <rdl:PCA_100006763>Document the qualified welding processes and materials within defined limitations.</rdl:PCA_100006763>
    <rdl:PCA_100006765 rdf:resource="http://w3id.org/readi/rdl/CFIHOS-20000031"/>
    <rdl:PCA_100006768>Record comprising all necessary data needed for qualification of a preliminary welding procedure specification.</rdl:PCA_100006768>
    <rdfs:comment>Record comprising all necessary data needed for qualification of a preliminary welding procedure specification.</rdfs:comment>
    <skos:broadMatch rdf:resource="http://rds.posccaesar.org/ontology/plm/rdl/PCA_100006688"/>
    <rdfs:label>Welding procedure qualification record (WPQR)</rdfs:label>
    <rdl:PCA_100006766 rdf:resource="http://rds.posccaesar.org/ontology/plm/rdl/PCA_100006653"/>
    <rdfs:subClassOf rdf:resource="http://rds.posccaesar.org/ontology/plm/rdl/PCA_100004908"/>
    <skos:broader rdf:resource="http://rds.posccaesar.org/ontology/plm/rdl/PCA_100006756"/>
  </owl:Class>
  <owl:Class rdf:about="http://rds.posccaesar.org/ontology/plm/rdl/PCA_100006511">
    <rdfs:comment>Document compliance</rdfs:comment>
    <rdl:PCA_100006763>This document is used for verification of compliance</rdl:PCA_100006763>
    <skos:broadMatch rdf:resource="http://rds.posccaesar.org/ontology/plm/rdl/PCA_100006722"/>
    <rdl:PCA_100006765 rdf:resource="http://w3id.org/readi/rdl/CFIHOS-20000027"/>
    <rdl:PCA_100006766 rdf:resource="http://rds.posccaesar.org/ontology/plm/rdl/PCA_100006653"/>
    <rdl:PCA_100006768>Document compliance</rdl:PCA_100006768>
    <rdfs:label>Type approval certificate</rdfs:label>
    <skos:broader rdf:resource="http://rds.posccaesar.org/ontology/plm/rdl/PCA_100006743"/>
    <rdfs:subClassOf rdf:resource="http://rds.posccaesar.org/ontology/plm/rdl/PCA_100004908"/>
  </owl:Class>
  <owl:Class rdf:about="http://rds.posccaesar.org/ontology/plm/rdl/PCA_100006190">
    <skos:broader rdf:resource="http://rds.posccaesar.org/ontology/plm/rdl/PCA_100006745"/>
    <skos:broadMatch rdf:resource="http://rds.posccaesar.org/ontology/plm/rdl/PCA_100006696"/>
    <rdfs:label>Equipment supplier piping and instrument diagram (P&amp;ID)</rdfs:label>
    <rdfs:comment>Piping and Instrument Diagram (P&amp;ID) includes the complete set of P&amp;IDs, typicals and legends. Equipment supplier's drafting standard shall be used. Symbols used shall be described by a symbol legend on the P&amp;ID, or as a separate document/drawing/P&amp;ID sheet. All connections external to the supply shall be shown on the P&amp;ID, marked with a unique number (N1, N2, etc.). Reference to the interfacing external P&amp;IDs should also be given.
All interface signals to and from the plant’s safety and automation systems shall be shown 
with reference to the interfacing external P&amp;IDs. Control and monitoring functions shall be 
drawn on the P&amp;ID, this also applies for control panel locally within the supply.
Identical parallel items or systems shall be drawn in full detail, i.e. typical drawings with 
associated tag number tables are not acceptable.
Unique plant tags shall be used as assigned by the engineering contractor. Supplier’s 
internal tag numbers shall be shown in addition where required for use of supplier’s standard
documentation, preferably by use of tables on the P&amp;ID/separate P&amp;ID sheet, linking unique 
plant tag with supplier’s internal tag.</rdfs:comment>
    <rdl:PCA_100006768>Piping and Instrument Diagram (P&amp;ID) includes the complete set of P&amp;IDs, typicals and legends. Equipment supplier's drafting standard shall be used. Symbols used shall be described by a symbol legend on the P&amp;ID, or as a separate document/drawing/P&amp;ID sheet. All connections external to the supply shall be shown on the P&amp;ID, marked with a unique number (N1, N2, etc.). Reference to the interfacing external P&amp;IDs should also be given.
All interface signals to and from the plant’s safety and automation systems shall be shown 
with reference to the interfacing external P&amp;IDs. Control and monitoring functions shall be 
drawn on the P&amp;ID, this also applies for control panel locally within the supply.
Identical parallel items or systems shall be drawn in full detail, i.e. typical drawings with 
associated tag number tables are not acceptable.
Unique plant tags shall be used as assigned by the engineering contractor. Supplier’s 
internal tag numbers shall be shown in addition where required for use of supplier’s standard
documentation, preferably by use of tables on the P&amp;ID/separate P&amp;ID sheet, linking unique 
plant tag with supplier’s internal tag.</rdl:PCA_100006768>
    <rdl:PCA_100006765 rdf:resource="http://w3id.org/readi/rdl/CFIHOS-20000015"/>
    <rdl:PCA_100006764>Context specific information to be added</rdl:PCA_100006764>
    <rdfs:subClassOf rdf:resource="http://rds.posccaesar.org/ontology/plm/rdl/PCA_100004908"/>
  </owl:Class>
  <owl:Class rdf:about="http://rds.posccaesar.org/ontology/plm/rdl/PCA_100006081">
    <skos:broader>
      <rdl:PCA_100001503 rdf:about="http://rds.posccaesar.org/ontology/plm/rdl/PCA_100006753">
        <rdfs:label>Plan (Drawing not project planning)</rdfs:label>
        <rdl:PCA_100004924>PL</rdl:PCA_100004924>
        <rdf:type rdf:resource="http://www.w3.org/2002/07/owl#NamedIndividual"/>
      </rdl:PCA_100001503>
    </skos:broader>
    <rdl:PCA_100006766 rdf:resource="http://rds.posccaesar.org/ontology/plm/rdl/PCA_100006654"/>
    <rdl:PCA_100006768>These drawings shall be based on equipment layout drawings or architectural layout drawings and shall include acoustic insulation, thermal insulation and fire protection details as follows: 
 - All doors and windows;
 - All insulation in ceiling, floors and walls;
 - Blast/fire walls;
 - All penetrations in blast/fire wall.</rdl:PCA_100006768>
    <rdl:PCA_100006765>
      <rdl:PCA_100001503 rdf:about="http://w3id.org/readi/rdl/CFIHOS-20000003">
        <rdfs:label>architectural engineering</rdfs:label>
        <rdl:PCA_100004924>CB</rdl:PCA_100004924>
        <rdf:type rdf:resource="http://www.w3.org/2002/07/owl#NamedIndividual"/>
      </rdl:PCA_100001503>
    </rdl:PCA_100006765>
    <skos:broadMatch rdf:resource="http://rds.posccaesar.org/ontology/plm/rdl/PCA_100006707"/>
    <skos:broadMatch rdf:resource="http://rds.posccaesar.org/ontology/plm/rdl/PCA_100006729"/>
    <rdl:PCA_100006763>These drawings shall be based on equipment layout drawings or architectural layout drawings and shall include acoustic insulation, thermal insulation and fire protection details</rdl:PCA_100006763>
    <rdfs:label>Acoustic/thermal insulation and fire protection plan</rdfs:label>
    <rdfs:comment>These drawings shall be based on equipment layout drawings or architectural layout drawings and shall include acoustic insulation, thermal insulation and fire protection details as follows: 
 - All doors and windows;
 - All insulation in ceiling, floors and walls;
 - Blast/fire walls;
 - All penetrations in blast/fire wall.</rdfs:comment>
    <rdfs:subClassOf rdf:resource="http://rds.posccaesar.org/ontology/plm/rdl/PCA_100004908"/>
  </owl:Class>
  <owl:Class rdf:about="http://rds.posccaesar.org/ontology/plm/rdl/PCA_100006093">
    <rdl:PCA_100006768>Fire walls, other gas tight barriers, hazardous area classification of zones and each fire area to be shown with fire area identification. All air intakes and ventilation air outlets to/from all areas shall be shown on the area classification drawings. All sources of releases shall be identified. Area classification drawings shall be scaled and prepared in accordance with regulatory requirements for area classification.</rdl:PCA_100006768>
    <rdfs:subClassOf rdf:resource="http://rds.posccaesar.org/ontology/plm/rdl/PCA_100004908"/>
    <skos:broader rdf:resource="http://rds.posccaesar.org/ontology/plm/rdl/PCA_100006746"/>
    <rdl:PCA_100006765 rdf:resource="http://w3id.org/readi/rdl/CFIHOS-20000011"/>
    <rdl:PCA_100006766 rdf:resource="http://rds.posccaesar.org/ontology/plm/rdl/PCA_100006656"/>
    <rdl:PCA_100006765 rdf:resource="http://w3id.org/readi/rdl/CFIHOS-20000013"/>
    <rdfs:comment>Fire walls, other gas tight barriers, hazardous area classification of zones and each fire area to be shown with fire area identification. All air intakes and ventilation air outlets to/from all areas shall be shown on the area classification drawings. All sources of releases shall be identified. Area classification drawings shall be scaled and prepared in accordance with regulatory requirements for area classification.</rdfs:comment>
    <rdl:PCA_100006765 rdf:resource="http://w3id.org/readi/rdl/CFIHOS-20000010"/>
    <rdfs:label>Area classification drawings</rdfs:label>
    <rdl:PCA_100006764>Area classification drawings should be based on Safety layout drawings</rdl:PCA_100006764>
    <skos:broadMatch rdf:resource="http://rds.posccaesar.org/ontology/plm/rdl/PCA_100006727"/>
  </owl:Class>
  <owl:Class rdf:about="http://rds.posccaesar.org/ontology/plm/rdl/PCA_100006318">
    <rdl:PCA_100006768>Document stating requirements for materials, e.g. mechanical properties and NDT.</rdl:PCA_100006768>
    <skos:broadMatch rdf:resource="http://rds.posccaesar.org/ontology/plm/rdl/PCA_100006687"/>
    <rdfs:label>Material specification</rdfs:label>
    <rdl:PCA_100006765 rdf:resource="http://w3id.org/readi/rdl/CFIHOS-20000031"/>
    <rdfs:subClassOf rdf:resource="http://rds.posccaesar.org/ontology/plm/rdl/PCA_100004908"/>
    <rdl:PCA_100006763>Give instructions concerning material requirements.</rdl:PCA_100006763>
    <rdl:PCA_100006766 rdf:resource="http://rds.posccaesar.org/ontology/plm/rdl/PCA_100006653"/>
    <rdfs:comment>Document stating requirements for materials, e.g. mechanical properties and NDT.</rdfs:comment>
    <skos:broader rdf:resource="http://rds.posccaesar.org/ontology/plm/rdl/PCA_100006757"/>
  </owl:Class>
  <owl:Class rdf:about="http://rds.posccaesar.org/ontology/plm/rdl/PCA_100006439">
    <skos:broader rdf:resource="http://rds.posccaesar.org/ontology/plm/rdl/PCA_100006745"/>
    <skos:broadMatch rdf:resource="http://rds.posccaesar.org/ontology/plm/rdl/PCA_100006702"/>
    <rdfs:label>Single line diagram (supplier)</rdfs:label>
    <rdfs:comment>The drawing shall contain identification of and main data for the components within the equipment.</rdfs:comment>
    <rdl:PCA_100006768>The drawing shall contain identification of and main data for the components within the equipment.</rdl:PCA_100006768>
    <rdl:PCA_100006765 rdf:resource="http://w3id.org/readi/rdl/CFIHOS-20000008"/>
    <rdl:PCA_100006763>For equipment packages the single line diagram shall show the main circuits and components in the electrical distribution system.</rdl:PCA_100006763>
    <rdfs:subClassOf rdf:resource="http://rds.posccaesar.org/ontology/plm/rdl/PCA_100004908"/>
  </owl:Class>
  <owl:Class rdf:about="http://rds.posccaesar.org/ontology/plm/rdl/PCA_100006427">
    <skos:broader rdf:resource="http://rds.posccaesar.org/ontology/plm/rdl/PCA_100006749"/>
    <skos:broadMatch rdf:resource="http://rds.posccaesar.org/ontology/plm/rdl/PCA_100006727"/>
    <rdfs:label>Safety manual</rdfs:label>
    <rdfs:comment>For standard off-the-shelf devices and assemblies/SIS sub-systems, the above documents should be delivered as supplier standard documents (project specific content minimized). Traceability between specific model/variant/configuration delivered with those covered in the standard document shall be ensured. To achieve this, it is good practice to mark-up the relevant parts of the standard document that apply to the specific delivery. 

Device/component: 
For IEC 61508 compliant devices the following supplier SIL documentation shall be delivered:
 - Safety Manual in accordance with IEC 61508
 - Certificate of compliance with IEC 61508 from recognized 3rd party certification body
 - Assessment report from 3rd party (as referred to in the certificate)

 For non-compliant devices, a Safety Manual (and evt. other complementary documents) shall be delivered in accordance with IEC 61511 and including underlying information supporting the claimed performance. For components claimed to be proven in use in accordance with IEC 61508, the documentary evidence shall be supplied (ref IEC 61508-2 sub clause 7.4.10).

 Assembly /SIS sub-system: For assemblies/SIS sub-systems within scope of delivery, a Safety Manual in accordance with IEC 61511 shall address the complete assembly. The SIL documentation for the devices forming part of the assembly shall be delivered (incl. from sub-suppliers) and all referred device SIL documents shall be delivered or attached to the assembly safety manual.</rdfs:comment>
    <rdl:PCA_100006768>For standard off-the-shelf devices and assemblies/SIS sub-systems, the above documents should be delivered as supplier standard documents (project specific content minimized). Traceability between specific model/variant/configuration delivered with those covered in the standard document shall be ensured. To achieve this, it is good practice to mark-up the relevant parts of the standard document that apply to the specific delivery. 

Device/component: 
For IEC 61508 compliant devices the following supplier SIL documentation shall be delivered:
 - Safety Manual in accordance with IEC 61508
 - Certificate of compliance with IEC 61508 from recognized 3rd party certification body
 - Assessment report from 3rd party (as referred to in the certificate)

 For non-compliant devices, a Safety Manual (and evt. other complementary documents) shall be delivered in accordance with IEC 61511 and including underlying information supporting the claimed performance. For components claimed to be proven in use in accordance with IEC 61508, the documentary evidence shall be supplied (ref IEC 61508-2 sub clause 7.4.10).

 Assembly /SIS sub-system: For assemblies/SIS sub-systems within scope of delivery, a Safety Manual in accordance with IEC 61511 shall address the complete assembly. The SIL documentation for the devices forming part of the assembly shall be delivered (incl. from sub-suppliers) and all referred device SIL documents shall be delivered or attached to the assembly safety manual.</rdl:PCA_100006768>
    <rdl:PCA_100006765 rdf:resource="http://w3id.org/readi/rdl/CFIHOS-20000013"/>
    <rdl:PCA_100006763>Supplier SIL documentation (Safety Manual, Certificate, etc) shall be provided for devices and assemblies/SIS sub-systems when part of a Safety Instrumented Function.

The supplier SIL documentation provides the necessary information about how to safely apply a device or assembly/SIS-subsystem and integrate it into a complete safety instrumented function. It addresses operation, maintenance, failure rates and other reliability data, fault detection and constraints associated with the device or assembly for the intended configurations and operating environment.</rdl:PCA_100006763>
    <rdfs:subClassOf rdf:resource="http://rds.posccaesar.org/ontology/plm/rdl/PCA_100004908"/>
  </owl:Class>
  <owl:Class rdf:about="http://rds.posccaesar.org/ontology/plm/rdl/PCA_100006536">
    <rdl:PCA_100006764>Minor weld procedures are not required for Norsok M-650 approved manufacturers (covered by approval).
 
Requirements related to assurance and check of quality in manufacturing phase will very much depend on Purchaser’s knowledge of supplier. Well known supplier, with proven track record, delivering products based on industry standards, will typically deliver less verification documentation to Purchaser than unknown/new supplier delivering the same product. Therefore, this deliverable should be evaluated as candidate for being available in digital format to Purchaser, for information only.</rdl:PCA_100006764>
    <rdl:PCA_100006768>Procedure in accordance with international standards.</rdl:PCA_100006768>
    <rdl:PCA_100006766 rdf:resource="http://rds.posccaesar.org/ontology/plm/rdl/PCA_100006653"/>
    <rdfs:comment>Procedure in accordance with international standards.</rdfs:comment>
    <rdl:PCA_100006763>This document is a part of the Quality Assurance Plan, and herein the Quality Assurance work process and verification.
This document provides a procedure for welding operator to ensure repeatability and formalism and hence prove the quality of the welding work.</rdl:PCA_100006763>
    <rdfs:subClassOf rdf:resource="http://rds.posccaesar.org/ontology/plm/rdl/PCA_100004908"/>
    <skos:broader rdf:resource="http://rds.posccaesar.org/ontology/plm/rdl/PCA_100006757"/>
    <skos:broadMatch rdf:resource="http://rds.posccaesar.org/ontology/plm/rdl/PCA_100006687"/>
    <rdfs:label>Welding procedure specification</rdfs:label>
  </owl:Class>
  <owl:Class rdf:about="http://rds.posccaesar.org/ontology/plm/rdl/PCA_100006306">
    <rdl:PCA_100006766 rdf:resource="http://rds.posccaesar.org/ontology/plm/rdl/PCA_100006653"/>
    <rdfs:subClassOf rdf:resource="http://rds.posccaesar.org/ontology/plm/rdl/PCA_100004908"/>
    <rdl:PCA_100006768>Document describing how specified material properties may be achieved and verified through the proposed manufacturing route.</rdl:PCA_100006768>
    <rdl:PCA_100006763>Provide clear specification to manufacturer to ensure repeatability.</rdl:PCA_100006763>
    <skos:broadMatch rdf:resource="http://rds.posccaesar.org/ontology/plm/rdl/PCA_100006688"/>
    <rdfs:comment>Document describing how specified material properties may be achieved and verified through the proposed manufacturing route.</rdfs:comment>
    <rdfs:label>Manufacturing procedure specification (MPS)</rdfs:label>
    <skos:broader rdf:resource="http://rds.posccaesar.org/ontology/plm/rdl/PCA_100006757"/>
    <rdl:PCA_100006765 rdf:resource="http://w3id.org/readi/rdl/CFIHOS-20000031"/>
  </owl:Class>
  <owl:Class rdf:about="http://rds.posccaesar.org/ontology/plm/rdl/PCA_100006415">
    <rdl:PCA_100006768>The report shall contain a full quantitative risk assessment of all identified hazards contributing to the total risk picture for personnel, environment and third party, for the facility in operations (including Area Risk charts).</rdl:PCA_100006768>
    <rdl:PCA_100006766 rdf:resource="http://rds.posccaesar.org/ontology/plm/rdl/PCA_100006654"/>
    <rdl:PCA_100006765 rdf:resource="http://w3id.org/readi/rdl/CFIHOS-20000011"/>
    <skos:broadMatch rdf:resource="http://rds.posccaesar.org/ontology/plm/rdl/PCA_100006728"/>
    <rdl:PCA_100006765 rdf:resource="http://w3id.org/readi/rdl/CFIHOS-20000010"/>
    <skos:broadMatch rdf:resource="http://rds.posccaesar.org/ontology/plm/rdl/PCA_100006727"/>
    <skos:broadMatch rdf:resource="http://rds.posccaesar.org/ontology/plm/rdl/PCA_100006726"/>
    <rdfs:comment>The report shall contain a full quantitative risk assessment of all identified hazards contributing to the total risk picture for personnel, environment and third party, for the facility in operations (including Area Risk charts).</rdfs:comment>
    <rdl:PCA_100006765 rdf:resource="http://w3id.org/readi/rdl/CFIHOS-20000013"/>
    <rdfs:label>Risk analysis</rdfs:label>
    <rdfs:subClassOf rdf:resource="http://rds.posccaesar.org/ontology/plm/rdl/PCA_100004908"/>
    <skos:broader rdf:resource="http://rds.posccaesar.org/ontology/plm/rdl/PCA_100006756"/>
  </owl:Class>
  <owl:Class rdf:about="http://rds.posccaesar.org/ontology/plm/rdl/PCA_100006403">
    <rdl:PCA_100006768>Report from the qualification tests based on the procedure.</rdl:PCA_100006768>
    <rdl:PCA_100006763>Document the qualification test results.</rdl:PCA_100006763>
    <rdfs:label>Qualification test records / report</rdfs:label>
    <rdl:PCA_100006766 rdf:resource="http://rds.posccaesar.org/ontology/plm/rdl/PCA_100006653"/>
    <rdfs:subClassOf rdf:resource="http://rds.posccaesar.org/ontology/plm/rdl/PCA_100004908"/>
    <skos:broader rdf:resource="http://rds.posccaesar.org/ontology/plm/rdl/PCA_100006756"/>
    <rdfs:comment>Report from the qualification tests based on the procedure.</rdfs:comment>
    <skos:broadMatch rdf:resource="http://rds.posccaesar.org/ontology/plm/rdl/PCA_100006722"/>
    <rdl:PCA_100006765 rdf:resource="http://w3id.org/readi/rdl/CFIHOS-20000031"/>
  </owl:Class>
  <owl:Class rdf:about="http://rds.posccaesar.org/ontology/plm/rdl/PCA_100006512">
    <skos:broader rdf:resource="http://rds.posccaesar.org/ontology/plm/rdl/PCA_100006756"/>
    <skos:broadMatch rdf:resource="http://rds.posccaesar.org/ontology/plm/rdl/PCA_100006705"/>
    <rdfs:label>UHF/VHF radio coverage</rdfs:label>
    <rdl:PCA_100006765 rdf:resource="http://w3id.org/readi/rdl/CFIHOS-20000030"/>
    <rdfs:subClassOf rdf:resource="http://rds.posccaesar.org/ontology/plm/rdl/PCA_100004908"/>
    <rdl:PCA_100006766 rdf:resource="http://rds.posccaesar.org/ontology/plm/rdl/PCA_100006640"/>
    <rdfs:comment>UHF/VHF radio (platform/facility internal) coverage chart/test report shall be provided.</rdfs:comment>
    <rdl:PCA_100006768>UHF/VHF radio (platform/facility internal) coverage chart/test report shall be provided.</rdl:PCA_100006768>
    <skos:broadMatch rdf:resource="http://rds.posccaesar.org/ontology/plm/rdl/PCA_100006722"/>
  </owl:Class>
  <owl:Class rdf:about="http://rds.posccaesar.org/ontology/plm/rdl/PCA_100006524">
    <skos:broader rdf:resource="http://rds.posccaesar.org/ontology/plm/rdl/PCA_100006753"/>
    <rdfs:comment>The plan shall include information on all internal and external openings (air pipes, ventilators, hatches, doors, etc.) of volumes affecting stability calculations.</rdfs:comment>
    <rdl:PCA_100006768>The plan shall include information on all internal and external openings (air pipes, ventilators, hatches, doors, etc.) of volumes affecting stability calculations.</rdl:PCA_100006768>
    <rdfs:subClassOf rdf:resource="http://rds.posccaesar.org/ontology/plm/rdl/PCA_100004908"/>
    <rdl:PCA_100006766 rdf:resource="http://rds.posccaesar.org/ontology/plm/rdl/PCA_100006654"/>
    <skos:broadMatch rdf:resource="http://rds.posccaesar.org/ontology/plm/rdl/PCA_100006708"/>
    <rdl:PCA_100006765 rdf:resource="http://w3id.org/readi/rdl/CFIHOS-20000033"/>
    <rdl:PCA_100006763>To document compliance with the PSA facilities regulations § 62 and NMA Regulations No. 878 in addition to IMO instruments and Class requirements, as applicable.</rdl:PCA_100006763>
    <rdfs:label>Watertight integrity plan</rdfs:label>
  </owl:Class>
  <owl:Class rdf:about="http://rds.posccaesar.org/ontology/plm/rdl/PCA_100006500">
    <skos:broader rdf:resource="http://rds.posccaesar.org/ontology/plm/rdl/PCA_100006743"/>
    <rdl:PCA_100006763>To secure independent verification of compliance</rdl:PCA_100006763>
    <skos:broadMatch rdf:resource="http://rds.posccaesar.org/ontology/plm/rdl/PCA_100006722"/>
    <rdl:PCA_100006768>The document shall clearly describe the object(s) for which the certificate applies</rdl:PCA_100006768>
    <rdl:PCA_100006766 rdf:resource="http://rds.posccaesar.org/ontology/plm/rdl/PCA_100006653"/>
    <rdl:PCA_100006765 rdf:resource="http://w3id.org/readi/rdl/CFIHOS-20000027"/>
    <rdfs:comment>The document shall clearly describe the object(s) for which the certificate applies</rdfs:comment>
    <rdfs:label>Third party certificate</rdfs:label>
    <rdfs:subClassOf rdf:resource="http://rds.posccaesar.org/ontology/plm/rdl/PCA_100004908"/>
  </owl:Class>
  <owl:Class rdf:about="http://rds.posccaesar.org/ontology/plm/rdl/PCA_100006080">
    <skos:broader rdf:resource="http://rds.posccaesar.org/ontology/plm/rdl/PCA_100006738"/>
    <skos:broadMatch rdf:resource="http://rds.posccaesar.org/ontology/plm/rdl/PCA_100006732"/>
    <rdfs:label>3D view model</rdfs:label>
    <rdfs:comment>A view model in as-built status of all structures in adequate details, including panels, pipeline, cabling,
tees, wyes and valves, for intervention/inspection activities during operations shall be delivered</rdfs:comment>
    <rdl:PCA_100006768>A view model in as-built status of all structures in adequate details, including panels, pipeline, cabling,
tees, wyes and valves, for intervention/inspection activities during operations shall be delivered</rdl:PCA_100006768>
    <rdl:PCA_100006766 rdf:resource="http://rds.posccaesar.org/ontology/plm/rdl/PCA_100006656"/>
    <rdfs:subClassOf rdf:resource="http://rds.posccaesar.org/ontology/plm/rdl/PCA_100004908"/>
  </owl:Class>
  <owl:Class rdf:about="http://rds.posccaesar.org/ontology/plm/rdl/PCA_100006092">
    <skos:broader rdf:resource="http://rds.posccaesar.org/ontology/plm/rdl/PCA_100006746"/>
    <skos:broadMatch rdf:resource="http://rds.posccaesar.org/ontology/plm/rdl/PCA_100006710"/>
    <rdfs:label>Architectural layout drawings</rdfs:label>
    <rdfs:comment>Architectural layout drawings (plans and elevations) shall be produced for all architectural areas (living quarters, CCR, stores, workshops, etc.). The drawing scale shall normally be 1:100 on A3 format. However larger scales can be selected if required. The drawings shall include stairs, walls, doors, windows, furniture, access and escape routes and all tagged equipment.

Main dimensions shall be included. Elevations of all floors and platforms etc. shall be shown. Room areas shall be included. The area shall be noted in m2 and be positioned adjacent to or directly under the room or area name. A key plan, grid lines with north and east references and match lines with drawing references shall be included. Drawings from adjacent areas shall be referenced.</rdfs:comment>
    <rdl:PCA_100006768>Architectural layout drawings (plans and elevations) shall be produced for all architectural areas (living quarters, CCR, stores, workshops, etc.). The drawing scale shall normally be 1:100 on A3 format. However larger scales can be selected if required. The drawings shall include stairs, walls, doors, windows, furniture, access and escape routes and all tagged equipment.

Main dimensions shall be included. Elevations of all floors and platforms etc. shall be shown. Room areas shall be included. The area shall be noted in m2 and be positioned adjacent to or directly under the room or area name. A key plan, grid lines with north and east references and match lines with drawing references shall be included. Drawings from adjacent areas shall be referenced.</rdl:PCA_100006768>
    <rdl:PCA_100006766 rdf:resource="http://rds.posccaesar.org/ontology/plm/rdl/PCA_100006656"/>
    <rdl:PCA_100006765 rdf:resource="http://w3id.org/readi/rdl/CFIHOS-20000003"/>
    <rdfs:subClassOf rdf:resource="http://rds.posccaesar.org/ontology/plm/rdl/PCA_100004908"/>
  </owl:Class>
  <owl:Class rdf:about="http://rds.posccaesar.org/ontology/plm/rdl/PCA_100006359">
    <skos:broader rdf:resource="http://rds.posccaesar.org/ontology/plm/rdl/PCA_100006748"/>
    <rdl:PCA_100006768>The penetration dossier shall contain the following:
 - Location (e.g. coordinates);
 - Type of penetration;
 - Supplier;
 - Dimension (hole);
 - Dimension (sleeve);
 - Drawing references;
 - Fire rating;
 - Fire loads (include only if the information is available);
 - Penetration number/tag number as relevant.</rdl:PCA_100006768>
    <rdfs:comment>The penetration dossier shall contain the following:
 - Location (e.g. coordinates);
 - Type of penetration;
 - Supplier;
 - Dimension (hole);
 - Dimension (sleeve);
 - Drawing references;
 - Fire rating;
 - Fire loads (include only if the information is available);
 - Penetration number/tag number as relevant.</rdfs:comment>
    <rdl:PCA_100006763>The penetration dossier shall give an overview of all penetrations (including penetrations in packages/skids)</rdl:PCA_100006763>
    <skos:broadMatch rdf:resource="http://rds.posccaesar.org/ontology/plm/rdl/PCA_100006716"/>
    <rdl:PCA_100006765 rdf:resource="http://w3id.org/readi/rdl/CFIHOS-20000010"/>
    <rdl:PCA_100006765 rdf:resource="http://w3id.org/readi/rdl/CFIHOS-20000013"/>
    <rdl:PCA_100006766 rdf:resource="http://rds.posccaesar.org/ontology/plm/rdl/PCA_100006656"/>
    <rdfs:label>Penetration dossier</rdfs:label>
    <rdl:PCA_100006765 rdf:resource="http://w3id.org/readi/rdl/CFIHOS-20000011"/>
    <rdfs:subClassOf rdf:resource="http://rds.posccaesar.org/ontology/plm/rdl/PCA_100004908"/>
  </owl:Class>
  <owl:Class rdf:about="http://rds.posccaesar.org/ontology/plm/rdl/PCA_100006238">
    <rdl:PCA_100006765 rdf:resource="http://w3id.org/readi/rdl/CFIHOS-20000018"/>
    <rdl:PCA_100006766 rdf:resource="http://rds.posccaesar.org/ontology/plm/rdl/PCA_100006657"/>
    <rdl:PCA_100006763>General arrangement drawings for borehole and casing shall cover routing and longitudinal profile of borehole with pipeline installed.</rdl:PCA_100006763>
    <rdfs:comment>Cross sections, entry and exit point, possible casing pipes, bellmouth, entry- and exit point sealing, location of pipeline spacers and anodes in borehole, position of pipeline sections with different types of coatings shall be included.

Details shall include but not be limited to casing pipe, bellmouth, sealing arrangements, pipeline spacers and anodes, access arrangements for water sampling, exchange of water, location and details of CP-monitoring equipment, type and extent of possible infill material (such as grout and inhibited water).</rdfs:comment>
    <rdfs:label>General arrangement drawings - Bore hole and casing</rdfs:label>
    <rdl:PCA_100006768>Cross sections, entry and exit point, possible casing pipes, bellmouth, entry- and exit point sealing, location of pipeline spacers and anodes in borehole, position of pipeline sections with different types of coatings shall be included.

Details shall include but not be limited to casing pipe, bellmouth, sealing arrangements, pipeline spacers and anodes, access arrangements for water sampling, exchange of water, location and details of CP-monitoring equipment, type and extent of possible infill material (such as grout and inhibited water).</rdl:PCA_100006768>
    <skos:broader rdf:resource="http://rds.posccaesar.org/ontology/plm/rdl/PCA_100006739"/>
    <rdfs:subClassOf rdf:resource="http://rds.posccaesar.org/ontology/plm/rdl/PCA_100004908"/>
    <skos:broadMatch rdf:resource="http://rds.posccaesar.org/ontology/plm/rdl/PCA_100006708"/>
  </owl:Class>
  <owl:Class rdf:about="http://rds.posccaesar.org/ontology/plm/rdl/PCA_100006468">
    <rdl:PCA_100006768>Covering design and analysis of pipeline structures such as riser bases, pipeline protection structures, tee/wye assemblies, valve stations, anchor blocks etc.. Basis for analysis, assumptions and assessments not given in design basis shall be included.</rdl:PCA_100006768>
    <rdfs:subClassOf rdf:resource="http://rds.posccaesar.org/ontology/plm/rdl/PCA_100004908"/>
    <rdfs:label>Structure design report</rdfs:label>
    <rdfs:comment>Covering design and analysis of pipeline structures such as riser bases, pipeline protection structures, tee/wye assemblies, valve stations, anchor blocks etc.. Basis for analysis, assumptions and assessments not given in design basis shall be included.</rdfs:comment>
    <rdl:PCA_100006763>Ensure safe operation</rdl:PCA_100006763>
    <rdl:PCA_100006766>
      <rdl:PCA_100001503 rdf:about="http://rds.posccaesar.org/ontology/plm/rdl/PCA_100006643">
        <rdfs:label>Topside structure</rdfs:label>
        <rdl:PCA_100004924>90</rdl:PCA_100004924>
        <rdf:type rdf:resource="http://www.w3.org/2002/07/owl#NamedIndividual"/>
      </rdl:PCA_100001503>
    </rdl:PCA_100006766>
    <skos:broader rdf:resource="http://rds.posccaesar.org/ontology/plm/rdl/PCA_100006756"/>
    <rdl:PCA_100006765 rdf:resource="http://w3id.org/readi/rdl/CFIHOS-20000018"/>
    <skos:broadMatch rdf:resource="http://rds.posccaesar.org/ontology/plm/rdl/PCA_100006686"/>
  </owl:Class>
  <owl:Class rdf:about="http://rds.posccaesar.org/ontology/plm/rdl/PCA_100006347">
    <rdl:PCA_100006768>Report documenting all calculations and analysis performed to prove pipeline, riser or umbilical on bottom stability design.</rdl:PCA_100006768>
    <rdfs:label>On-bottom stability report</rdfs:label>
    <rdl:PCA_100006763>To document that the pipeline, riser or umbilical will be stable on the sea bottom during all conditions.</rdl:PCA_100006763>
    <rdl:PCA_100006766 rdf:resource="http://rds.posccaesar.org/ontology/plm/rdl/PCA_100006657"/>
    <rdl:PCA_100006765 rdf:resource="http://w3id.org/readi/rdl/CFIHOS-20000018"/>
    <skos:broadMatch rdf:resource="http://rds.posccaesar.org/ontology/plm/rdl/PCA_100006687"/>
    <skos:broader rdf:resource="http://rds.posccaesar.org/ontology/plm/rdl/PCA_100006756"/>
    <rdfs:comment>Report documenting all calculations and analysis performed to prove pipeline, riser or umbilical on bottom stability design.</rdfs:comment>
    <rdfs:subClassOf rdf:resource="http://rds.posccaesar.org/ontology/plm/rdl/PCA_100004908"/>
  </owl:Class>
  <owl:Class rdf:about="http://rds.posccaesar.org/ontology/plm/rdl/PCA_100006335">
    <rdfs:label>NDT procedures</rdfs:label>
    <skos:broadMatch rdf:resource="http://rds.posccaesar.org/ontology/plm/rdl/PCA_100006688"/>
    <rdl:PCA_100006766 rdf:resource="http://rds.posccaesar.org/ontology/plm/rdl/PCA_100006653"/>
    <rdl:PCA_100006765 rdf:resource="http://w3id.org/readi/rdl/CFIHOS-20000031"/>
    <skos:broader rdf:resource="http://rds.posccaesar.org/ontology/plm/rdl/PCA_100006751"/>
    <rdfs:subClassOf rdf:resource="http://rds.posccaesar.org/ontology/plm/rdl/PCA_100004908"/>
    <rdl:PCA_100006768>Document describing how to perform NDT (i.e. MT, PT, RT, UT, VT or ET) for a given object, including acceptance criteria and reporting.</rdl:PCA_100006768>
    <rdl:PCA_100006763>Provide clear procedure to NDT operator to ensure repeatability.</rdl:PCA_100006763>
    <rdfs:comment>Document describing how to perform NDT (i.e. MT, PT, RT, UT, VT or ET) for a given object, including acceptance criteria and reporting.</rdfs:comment>
  </owl:Class>
  <owl:Class rdf:about="http://rds.posccaesar.org/ontology/plm/rdl/PCA_100006456">
    <rdfs:label>Stability operation manual</rdfs:label>
    <rdl:PCA_100006768>The manual shall provide the means to calculate the daily loading condition as well as describe the use of the onboard loading computer, if applicable.</rdl:PCA_100006768>
    <skos:broader rdf:resource="http://rds.posccaesar.org/ontology/plm/rdl/PCA_100006749"/>
    <skos:broadMatch rdf:resource="http://rds.posccaesar.org/ontology/plm/rdl/PCA_100006688"/>
    <rdfs:subClassOf rdf:resource="http://rds.posccaesar.org/ontology/plm/rdl/PCA_100004908"/>
    <rdfs:comment>The manual shall provide the means to calculate the daily loading condition as well as describe the use of the onboard loading computer, if applicable.</rdfs:comment>
    <rdl:PCA_100006763>To document compliance with the PSA facilities regulations § 62 and NMA Regulations No. 878 in addition to IMO instruments and Class requirements, as applicable.</rdl:PCA_100006763>
    <rdl:PCA_100006765 rdf:resource="http://w3id.org/readi/rdl/CFIHOS-20000033"/>
    <rdl:PCA_100006766 rdf:resource="http://rds.posccaesar.org/ontology/plm/rdl/PCA_100006654"/>
  </owl:Class>
  <owl:Class rdf:about="http://rds.posccaesar.org/ontology/plm/rdl/PCA_100006444">
    <skos:broader rdf:resource="http://rds.posccaesar.org/ontology/plm/rdl/PCA_100006753"/>
    <skos:broadMatch rdf:resource="http://rds.posccaesar.org/ontology/plm/rdl/PCA_100006705"/>
    <rdfs:label>Site plan</rdfs:label>
    <rdfs:comment>The Site plan shall be based on a digital terrain model and shall include necessary layers to present (often provided as 2D input):
 - Geotechnical and geological features/strata;
 - Areas with registration of contaminated soil;
 - All plant functional areas/blocks including offsite;
 - Cavern, tunnel and shaft systems;
 - Areas defined for future plant development;
 - Areas that will have to be controlled or restricted during plant operations;
 - Levelled areas as a result of cut and fill;
 - Protective structures at sea, towards river and hinterland;
 - Plant road system including escape routes;
 - Plant main interconnecting pipe racks;
 - Plant fence lines and gates;
 - Outside plant local infrastructure and plant battery limits (roads, railways, port, pipelines, cables and overhead lines, etc.);
 - Permanent lay down and rig areas for future construction and turnaround activities;
 - Construction lay down areas and areas for temporary construction workshops, offices, accommodation, parking and holding areas;
 - Areas for permanent and temporary disposal of surplus materials;
 - Neighbouring settlements and use of land;
 - Areas that shall remain protected or with restriction to access (like nature reserves, historical monuments, archaeological sites);
 - Property borders;
 - Industrial zoning as per authority approvals.</rdfs:comment>
    <rdl:PCA_100006768>The Site plan shall be based on a digital terrain model and shall include necessary layers to present (often provided as 2D input):
 - Geotechnical and geological features/strata;
 - Areas with registration of contaminated soil;
 - All plant functional areas/blocks including offsite;
 - Cavern, tunnel and shaft systems;
 - Areas defined for future plant development;
 - Areas that will have to be controlled or restricted during plant operations;
 - Levelled areas as a result of cut and fill;
 - Protective structures at sea, towards river and hinterland;
 - Plant road system including escape routes;
 - Plant main interconnecting pipe racks;
 - Plant fence lines and gates;
 - Outside plant local infrastructure and plant battery limits (roads, railways, port, pipelines, cables and overhead lines, etc.);
 - Permanent lay down and rig areas for future construction and turnaround activities;
 - Construction lay down areas and areas for temporary construction workshops, offices, accommodation, parking and holding areas;
 - Areas for permanent and temporary disposal of surplus materials;
 - Neighbouring settlements and use of land;
 - Areas that shall remain protected or with restriction to access (like nature reserves, historical monuments, archaeological sites);
 - Property borders;
 - Industrial zoning as per authority approvals.</rdl:PCA_100006768>
    <rdl:PCA_100006766 rdf:resource="http://rds.posccaesar.org/ontology/plm/rdl/PCA_100006656"/>
    <rdl:PCA_100006765 rdf:resource="http://w3id.org/readi/rdl/CFIHOS-20000007"/>
    <rdfs:subClassOf rdf:resource="http://rds.posccaesar.org/ontology/plm/rdl/PCA_100004908"/>
  </owl:Class>
  <owl:Class rdf:about="http://rds.posccaesar.org/ontology/plm/rdl/PCA_100006323">
    <rdfs:label>MCCR - mechanical completion check record</rdfs:label>
    <skos:broader rdf:resource="http://rds.posccaesar.org/ontology/plm/rdl/PCA_100006756"/>
    <rdfs:subClassOf rdf:resource="http://rds.posccaesar.org/ontology/plm/rdl/PCA_100004908"/>
    <rdl:PCA_100006766 rdf:resource="http://rds.posccaesar.org/ontology/plm/rdl/PCA_100006653"/>
    <rdl:PCA_100006765 rdf:resource="http://w3id.org/readi/rdl/CFIHOS-20000031"/>
    <rdfs:comment>Final inspection check list for products and components with signature fields for Supplier, customer and third party, and list of all applicable punch items.</rdfs:comment>
    <rdl:PCA_100006763>To verify that the products and components have been manufactured in accordance with drawings, procedures and specifications.</rdl:PCA_100006763>
    <rdl:PCA_100006768>Final inspection check list for products and components with signature fields for Supplier, customer and third party, and list of all applicable punch items.</rdl:PCA_100006768>
    <skos:broadMatch rdf:resource="http://rds.posccaesar.org/ontology/plm/rdl/PCA_100006722"/>
  </owl:Class>
  <owl:Class rdf:about="http://rds.posccaesar.org/ontology/plm/rdl/PCA_100006311">
    <rdl:PCA_100006763>A drawing illustrating necessary marking and labelling of equipment.</rdl:PCA_100006763>
    <rdl:PCA_100006766 rdf:resource="http://rds.posccaesar.org/ontology/plm/rdl/PCA_100006653"/>
    <rdl:PCA_100006765 rdf:resource="http://w3id.org/readi/rdl/CFIHOS-20000031"/>
    <rdfs:subClassOf rdf:resource="http://rds.posccaesar.org/ontology/plm/rdl/PCA_100004908"/>
    <skos:broadMatch rdf:resource="http://rds.posccaesar.org/ontology/plm/rdl/PCA_100006732"/>
    <rdfs:label>Marking drawing</rdfs:label>
    <rdl:PCA_100006768>A drawing identifying equipment for operational purposes (e.g. ROV navigation). The information can be covered by the General Arrangement Drawing.</rdl:PCA_100006768>
    <skos:broader rdf:resource="http://rds.posccaesar.org/ontology/plm/rdl/PCA_100006746"/>
    <rdfs:comment>A drawing identifying equipment for operational purposes (e.g. ROV navigation). The information can be covered by the General Arrangement Drawing.</rdfs:comment>
  </owl:Class>
  <owl:Class rdf:about="http://rds.posccaesar.org/ontology/plm/rdl/PCA_100006432">
    <skos:broader rdf:resource="http://rds.posccaesar.org/ontology/plm/rdl/PCA_100006746"/>
    <rdfs:comment>A drawing showing equipment and tools supplied including part numbers.</rdfs:comment>
    <rdl:PCA_100006765 rdf:resource="http://w3id.org/readi/rdl/CFIHOS-20000031"/>
    <rdl:PCA_100006766 rdf:resource="http://rds.posccaesar.org/ontology/plm/rdl/PCA_100006653"/>
    <rdfs:subClassOf rdf:resource="http://rds.posccaesar.org/ontology/plm/rdl/PCA_100004908"/>
    <rdl:PCA_100006763>An illustration providing holistic understanding of equipment, listing quantity and type.</rdl:PCA_100006763>
    <rdl:PCA_100006768>A drawing showing equipment and tools supplied including part numbers.</rdl:PCA_100006768>
    <rdl:PCA_100006764>The scope of supply / work drawing contain an overview of equipments and the borderline between contractor' s scope of supply / work and others.</rdl:PCA_100006764>
    <rdfs:label>Scope of supply drawing</rdfs:label>
  </owl:Class>
  <owl:Class rdf:about="http://rds.posccaesar.org/ontology/plm/rdl/PCA_100006541">
    <rdl:PCA_100006763>This document describes use of WSN (Wireless Sensor Network) in the process plant.</rdl:PCA_100006763>
    <skos:broadMatch rdf:resource="http://rds.posccaesar.org/ontology/plm/rdl/PCA_100006705"/>
    <skos:broader rdf:resource="http://rds.posccaesar.org/ontology/plm/rdl/PCA_100006756"/>
    <rdl:PCA_100006768>Shall include:
 - WSN topology;
 - WSN standard;
 - Coverage chart/maps of WSN with identified sensor and access point locations (gateways);
 - Expected latency time (normal/max);
 - Expected battery lifetime (normal/min);
 - Type and ENS tag number of sensors connected to one gateway;
 - Spare availability (number of sensors) to one gateway;
 - A frequency plan for co-existence of WLAN and WSN with specification of dedicated channels for WSN;
 - Any requirements for radio silence due to special operations (e.g. well perforation);
 - Recommended precautions due to radio silence;
 - Recommended precautions due to loss of one gateway.</rdl:PCA_100006768>
    <skos:broadMatch rdf:resource="http://rds.posccaesar.org/ontology/plm/rdl/PCA_100006722"/>
    <rdl:PCA_100006765 rdf:resource="http://w3id.org/readi/rdl/CFIHOS-20000015"/>
    <rdl:PCA_100006766 rdf:resource="http://rds.posccaesar.org/ontology/plm/rdl/PCA_100006640"/>
    <rdfs:comment>Shall include:
 - WSN topology;
 - WSN standard;
 - Coverage chart/maps of WSN with identified sensor and access point locations (gateways);
 - Expected latency time (normal/max);
 - Expected battery lifetime (normal/min);
 - Type and ENS tag number of sensors connected to one gateway;
 - Spare availability (number of sensors) to one gateway;
 - A frequency plan for co-existence of WLAN and WSN with specification of dedicated channels for WSN;
 - Any requirements for radio silence due to special operations (e.g. well perforation);
 - Recommended precautions due to radio silence;
 - Recommended precautions due to loss of one gateway.</rdfs:comment>
    <rdfs:subClassOf rdf:resource="http://rds.posccaesar.org/ontology/plm/rdl/PCA_100004908"/>
    <rdfs:label>Wireless network coverage</rdfs:label>
  </owl:Class>
  <owl:Class rdf:about="http://rds.posccaesar.org/ontology/plm/rdl/PCA_100006420">
    <skos:broader rdf:resource="http://rds.posccaesar.org/ontology/plm/rdl/PCA_100006756"/>
    <rdfs:label>ROV access verification report</rdfs:label>
    <rdfs:comment>Report based on verification of ROV access in the 3D design model. The report includes 3D model pictures.</rdfs:comment>
    <rdl:PCA_100006768>Report based on verification of ROV access in the 3D design model. The report includes 3D model pictures.</rdl:PCA_100006768>
    <rdl:PCA_100006766 rdf:resource="http://rds.posccaesar.org/ontology/plm/rdl/PCA_100006654"/>
    <rdl:PCA_100006765 rdf:resource="http://w3id.org/readi/rdl/CFIHOS-20000031"/>
    <rdl:PCA_100006763>To verify ROV access for subsea operations defined in the ROV task list.</rdl:PCA_100006763>
    <rdfs:subClassOf rdf:resource="http://rds.posccaesar.org/ontology/plm/rdl/PCA_100004908"/>
  </owl:Class>
  <owl:Class rdf:about="http://rds.posccaesar.org/ontology/plm/rdl/PCA_100006201">
    <rdfs:subClassOf rdf:resource="http://rds.posccaesar.org/ontology/plm/rdl/PCA_100004908"/>
    <rdl:PCA_100006766 rdf:resource="http://rds.posccaesar.org/ontology/plm/rdl/PCA_100006653"/>
    <skos:broader rdf:resource="http://rds.posccaesar.org/ontology/plm/rdl/PCA_100006751"/>
    <rdfs:comment>A procedure describing the stepwise testing to be performed for the equipment after completed manufacturing. Test set-up and test equipment is defined</rdfs:comment>
    <rdl:PCA_100006768>A procedure describing the stepwise testing to be performed for the equipment after completed manufacturing. Test set-up and test equipment is defined</rdl:PCA_100006768>
    <rdl:PCA_100006765 rdf:resource="http://w3id.org/readi/rdl/CFIHOS-20000031"/>
    <rdfs:label>FAT procedure</rdfs:label>
    <rdl:PCA_100006763>Give clear test instructions and provide information to customers concerning test standards and acceptance criteria.</rdl:PCA_100006763>
    <skos:broadMatch rdf:resource="http://rds.posccaesar.org/ontology/plm/rdl/PCA_100006688"/>
  </owl:Class>
  <owl:Class rdf:about="http://rds.posccaesar.org/ontology/plm/rdl/PCA_100006213">
    <rdl:PCA_100006768>Materials used in areas that may be exposed to a hydrocarbon fire shall be non-combustible. If it is justified from safety point of view to make use of materials that do not meet the requirements to non-combustibility, such materials shall have limited flame-spread properties, low smoke development and heat generation.

An assessment shall be made of the toxicity of gas emitted in the event of a fire.</rdl:PCA_100006768>
    <rdfs:comment>Materials used in areas that may be exposed to a hydrocarbon fire shall be non-combustible. If it is justified from safety point of view to make use of materials that do not meet the requirements to non-combustibility, such materials shall have limited flame-spread properties, low smoke development and heat generation.

An assessment shall be made of the toxicity of gas emitted in the event of a fire.</rdfs:comment>
    <rdl:PCA_100006766 rdf:resource="http://rds.posccaesar.org/ontology/plm/rdl/PCA_100006630"/>
    <rdfs:label>Fire test results reports</rdfs:label>
    <skos:broader rdf:resource="http://rds.posccaesar.org/ontology/plm/rdl/PCA_100006756"/>
    <rdl:PCA_100006765 rdf:resource="http://w3id.org/readi/rdl/CFIHOS-20000003"/>
    <skos:broadMatch rdf:resource="http://rds.posccaesar.org/ontology/plm/rdl/PCA_100006722"/>
    <rdl:PCA_100006763>The basis for decision regarding selection of combustible materials shall be documented.</rdl:PCA_100006763>
    <rdfs:subClassOf rdf:resource="http://rds.posccaesar.org/ontology/plm/rdl/PCA_100004908"/>
  </owl:Class>
  <owl:Class rdf:about="http://rds.posccaesar.org/ontology/plm/rdl/PCA_100006225">
    <rdfs:subClassOf rdf:resource="http://rds.posccaesar.org/ontology/plm/rdl/PCA_100004908"/>
    <skos:broadMatch rdf:resource="http://rds.posccaesar.org/ontology/plm/rdl/PCA_100006696"/>
    <rdl:PCA_100006766 rdf:resource="http://rds.posccaesar.org/ontology/plm/rdl/PCA_100006654"/>
    <skos:broadMatch rdf:resource="http://rds.posccaesar.org/ontology/plm/rdl/PCA_100006698"/>
    <rdl:PCA_100006763>Input to simulation models in project and operation phase.</rdl:PCA_100006763>
    <rdfs:label>Fluid description for process design</rdfs:label>
    <skos:broader rdf:resource="http://rds.posccaesar.org/ontology/plm/rdl/PCA_100006756"/>
    <rdl:PCA_100006764>This report shall be prepared for the petroleum feed streams and shall include:
 - References to the experimental PVT (Pressure Volume Temperature) and fluid properties data;
 - Feed streams fluid compositions, including the properties of the C6+ hypothetical components;
 - A reasoning for the C6+ characterization, e.g. the selected equation of state and property models, the number of hypothetical components and the tuning of component properties;
 - Comparisons between experimental data and calculations in the characterization program and the process simulation program and a discussion of the differences;
 - Uncertainties in the fluid compositions and properties to be accommodated by the process design, including a reasoning of the selected uncertainties;
 - References to and relations to C6+ characterization(s) used by other disciplines, to demonstrate a consistent description throughout the value chain;
 - A description of the method used to predict the development of the feed stream compositions over the production lifetime, and the feed stream compositions to be accommodated by the process design.

Simulation files from the characterization and process simulation programs shall be a part of the delivery, to allow execution in the simulation programs.</rdl:PCA_100006764>
    <rdl:PCA_100006765 rdf:resource="http://w3id.org/readi/rdl/CFIHOS-20000026"/>
  </owl:Class>
  <owl:Class rdf:about="http://rds.posccaesar.org/ontology/plm/rdl/PCA_100006104">
    <rdfs:subClassOf rdf:resource="http://rds.posccaesar.org/ontology/plm/rdl/PCA_100004908"/>
    <rdl:PCA_100006765 rdf:resource="http://w3id.org/readi/rdl/CFIHOS-20000018"/>
    <rdfs:label>Battery limit drawings</rdfs:label>
    <rdfs:comment>Drawing covering interfaces towards elements such as, plants, platforms and other pipelines (tees/wyes), and other pipeline operators. Changes in standards, codes and authority requirements and testing interfaces along the pipeline system shall be included.</rdfs:comment>
    <skos:broader rdf:resource="http://rds.posccaesar.org/ontology/plm/rdl/PCA_100006746"/>
    <skos:broader rdf:resource="http://rds.posccaesar.org/ontology/plm/rdl/PCA_100006753"/>
    <rdl:PCA_100006766 rdf:resource="http://rds.posccaesar.org/ontology/plm/rdl/PCA_100006654"/>
    <rdl:PCA_100006763>A description of the overall pipeline system 'pig trap to pig trap' is needed to ensure a common understanding of where documentation will be authorized during the pipeline lifetime, including an overview of battery limits.</rdl:PCA_100006763>
    <rdl:PCA_100006768>Drawing covering interfaces towards elements such as, plants, platforms and other pipelines (tees/wyes), and other pipeline operators. Changes in standards, codes and authority requirements and testing interfaces along the pipeline system shall be included.</rdl:PCA_100006768>
    <skos:broadMatch rdf:resource="http://rds.posccaesar.org/ontology/plm/rdl/PCA_100006713"/>
  </owl:Class>
  <owl:Class rdf:about="http://rds.posccaesar.org/ontology/plm/rdl/PCA_100006116">
    <skos:broader>
      <rdl:PCA_100001503 rdf:about="http://rds.posccaesar.org/ontology/plm/rdl/PCA_100006742">
        <rdfs:label>Cause and effect</rdfs:label>
        <rdl:PCA_100004924>CE</rdl:PCA_100004924>
        <rdf:type rdf:resource="http://www.w3.org/2002/07/owl#NamedIndividual"/>
      </rdl:PCA_100001503>
    </skos:broader>
    <skos:broadMatch rdf:resource="http://rds.posccaesar.org/ontology/plm/rdl/PCA_100006699"/>
    <rdfs:label>Cause &amp; effect (C&amp;E) for interlock and intertrip</rdfs:label>
    <rdfs:comment>IEC 61850 / GOOSE address shall be included if relevant. Logical diagrams shall be included as part of Cause and Effect, or reference to relevant documents shall be given. There shall be one sheet per IED / breaker.</rdfs:comment>
    <rdl:PCA_100006768>IEC 61850 / GOOSE address shall be included if relevant. Logical diagrams shall be included as part of Cause and Effect, or reference to relevant documents shall be given. There shall be one sheet per IED / breaker.</rdl:PCA_100006768>
    <rdl:PCA_100006765 rdf:resource="http://w3id.org/readi/rdl/CFIHOS-20000015"/>
    <rdl:PCA_100006763>The purpose of the Cause and Effect (C&amp;E) is to give an overview over interlock and intertrip between IED / breakers.</rdl:PCA_100006763>
    <rdfs:subClassOf rdf:resource="http://rds.posccaesar.org/ontology/plm/rdl/PCA_100004908"/>
  </owl:Class>
  <owl:Class rdf:about="http://rds.posccaesar.org/ontology/plm/rdl/PCA_100006128">
    <skos:broader rdf:resource="http://rds.posccaesar.org/ontology/plm/rdl/PCA_100006746"/>
    <skos:broadMatch rdf:resource="http://rds.posccaesar.org/ontology/plm/rdl/PCA_100006731"/>
    <rdfs:label>Concrete detail drawings</rdfs:label>
    <rdfs:comment>The following concrete detail drawings shall be delivered: 
 - General Arrangements;
 - Typicals;
 - Sections and details;
 - Main Mechanical Outfitting (MMO) drawings.

The concrete detail drawings shall contain:
 - Concrete dimensions;
 - All reinforcement types (tensile-, shear, pretension reinforcement, other if applicable);
 - Reinforcement dimensions, quantity and location in concrete structure;
 - Material properties (concrete and reinforcement).</rdfs:comment>
    <rdl:PCA_100006768>The following concrete detail drawings shall be delivered: 
 - General Arrangements;
 - Typicals;
 - Sections and details;
 - Main Mechanical Outfitting (MMO) drawings.

The concrete detail drawings shall contain:
 - Concrete dimensions;
 - All reinforcement types (tensile-, shear, pretension reinforcement, other if applicable);
 - Reinforcement dimensions, quantity and location in concrete structure;
 - Material properties (concrete and reinforcement).</rdl:PCA_100006768>
    <rdl:PCA_100006766 rdf:resource="http://rds.posccaesar.org/ontology/plm/rdl/PCA_100006656"/>
    <rdl:PCA_100006765 rdf:resource="http://w3id.org/readi/rdl/CFIHOS-20000006"/>
    <rdfs:subClassOf rdf:resource="http://rds.posccaesar.org/ontology/plm/rdl/PCA_100004908"/>
  </owl:Class>
  <owl:Class rdf:about="http://rds.posccaesar.org/ontology/plm/rdl/PCA_100006239">
    <skos:broadMatch rdf:resource="http://rds.posccaesar.org/ontology/plm/rdl/PCA_100006708"/>
    <rdl:PCA_100006768>Cross sections detailing the landfall protection such as rock protection, micro tunnel etc. shall be included.</rdl:PCA_100006768>
    <rdfs:comment>Cross sections detailing the landfall protection such as rock protection, micro tunnel etc. shall be included.</rdfs:comment>
    <rdfs:label>General arrangement drawings - Landfall</rdfs:label>
    <skos:broader rdf:resource="http://rds.posccaesar.org/ontology/plm/rdl/PCA_100006739"/>
    <rdl:PCA_100006765 rdf:resource="http://w3id.org/readi/rdl/CFIHOS-20000018"/>
    <rdl:PCA_100006763>General arrangement drawings for landfall shall cover routing and longitudinal profile of landfall with pipeline installed.</rdl:PCA_100006763>
    <rdl:PCA_100006766 rdf:resource="http://rds.posccaesar.org/ontology/plm/rdl/PCA_100006657"/>
    <rdfs:subClassOf rdf:resource="http://rds.posccaesar.org/ontology/plm/rdl/PCA_100004908"/>
  </owl:Class>
  <owl:Class rdf:about="http://rds.posccaesar.org/ontology/plm/rdl/PCA_100006348">
    <rdfs:comment>A compiled document providing sufficient information to operate, maintain and preserve the equipment.</rdfs:comment>
    <rdl:PCA_100006765 rdf:resource="http://w3id.org/readi/rdl/CFIHOS-20000031"/>
    <rdfs:label>Operation and maintenance manual (OMM)</rdfs:label>
    <skos:broader rdf:resource="http://rds.posccaesar.org/ontology/plm/rdl/PCA_100006751"/>
    <rdfs:subClassOf rdf:resource="http://rds.posccaesar.org/ontology/plm/rdl/PCA_100004908"/>
    <rdl:PCA_100006768>A compiled document providing sufficient information to operate, maintain and preserve the equipment.</rdl:PCA_100006768>
    <rdl:PCA_100006763>To describe how to operate and maintain the equipment in a safe and functionally correct manner according to the specified maintenance philosophy.</rdl:PCA_100006763>
    <rdl:PCA_100006766 rdf:resource="http://rds.posccaesar.org/ontology/plm/rdl/PCA_100006653"/>
    <skos:broadMatch rdf:resource="http://rds.posccaesar.org/ontology/plm/rdl/PCA_100006688"/>
  </owl:Class>
  <owl:Class rdf:about="http://rds.posccaesar.org/ontology/plm/rdl/PCA_100006469">
    <skos:broadMatch rdf:resource="http://rds.posccaesar.org/ontology/plm/rdl/PCA_100006688"/>
    <rdl:PCA_100006765 rdf:resource="http://w3id.org/readi/rdl/CFIHOS-20000031"/>
    <rdl:PCA_100006768>Document specifying the methods for fabrication of subsea structures. Includes references to specifications for welding, NDT, assembly, painting, dimensional control, FAT etc.</rdl:PCA_100006768>
    <rdl:PCA_100006763>Specify fabrication requirements for structures.</rdl:PCA_100006763>
    <rdfs:comment>Document specifying the methods for fabrication of subsea structures. Includes references to specifications for welding, NDT, assembly, painting, dimensional control, FAT etc.</rdfs:comment>
    <rdl:PCA_100006766 rdf:resource="http://rds.posccaesar.org/ontology/plm/rdl/PCA_100006653"/>
    <skos:broader rdf:resource="http://rds.posccaesar.org/ontology/plm/rdl/PCA_100006751"/>
    <rdfs:label>Structure fabrication procedure</rdfs:label>
    <rdfs:subClassOf rdf:resource="http://rds.posccaesar.org/ontology/plm/rdl/PCA_100004908"/>
  </owl:Class>
  <owl:Class rdf:about="http://rds.posccaesar.org/ontology/plm/rdl/PCA_100006457">
    <skos:broader rdf:resource="http://rds.posccaesar.org/ontology/plm/rdl/PCA_100006746"/>
    <skos:broadMatch rdf:resource="http://rds.posccaesar.org/ontology/plm/rdl/PCA_100006731"/>
    <rdfs:label>Stack-up-drawing</rdfs:label>
    <rdfs:comment>A drawing showing critical interfaces and dimensions for testing, installation and offshore operations.</rdfs:comment>
    <rdl:PCA_100006768>A drawing showing critical interfaces and dimensions for testing, installation and offshore operations.</rdl:PCA_100006768>
    <rdl:PCA_100006766 rdf:resource="http://rds.posccaesar.org/ontology/plm/rdl/PCA_100006653"/>
    <rdl:PCA_100006765 rdf:resource="http://w3id.org/readi/rdl/CFIHOS-20000031"/>
    <rdfs:subClassOf rdf:resource="http://rds.posccaesar.org/ontology/plm/rdl/PCA_100004908"/>
  </owl:Class>
  <owl:Class rdf:about="http://rds.posccaesar.org/ontology/plm/rdl/PCA_100006336">
    <rdfs:comment>Documents containing records of performed NDT (in typical NDT methodse.g. MT, PT, RT, UT, ET and VT).</rdfs:comment>
    <skos:broader>
      <rdl:PCA_100001503 rdf:about="http://rds.posccaesar.org/ontology/plm/rdl/PCA_100006755">
        <rdfs:label>Regulations</rdfs:label>
        <rdl:PCA_100004924>RG</rdl:PCA_100004924>
        <rdf:type rdf:resource="http://www.w3.org/2002/07/owl#NamedIndividual"/>
      </rdl:PCA_100001503>
    </skos:broader>
    <rdfs:label>NDT reports</rdfs:label>
    <rdl:PCA_100006768>Documents containing records of performed NDT (in typical NDT methodse.g. MT, PT, RT, UT, ET and VT).</rdl:PCA_100006768>
    <rdl:PCA_100006765 rdf:resource="http://w3id.org/readi/rdl/CFIHOS-20000031"/>
    <rdl:PCA_100006766 rdf:resource="http://rds.posccaesar.org/ontology/plm/rdl/PCA_100006653"/>
    <skos:broadMatch rdf:resource="http://rds.posccaesar.org/ontology/plm/rdl/PCA_100006722"/>
    <rdfs:subClassOf rdf:resource="http://rds.posccaesar.org/ontology/plm/rdl/PCA_100004908"/>
    <rdl:PCA_100006763>To document that the NDT performed meets specified requirements.</rdl:PCA_100006763>
  </owl:Class>
  <owl:Class rdf:about="http://rds.posccaesar.org/ontology/plm/rdl/PCA_100006324">
    <skos:broader rdf:resource="http://rds.posccaesar.org/ontology/plm/rdl/PCA_100006748"/>
    <rdfs:subClassOf rdf:resource="http://rds.posccaesar.org/ontology/plm/rdl/PCA_100004908"/>
    <rdl:PCA_100006766 rdf:resource="http://rds.posccaesar.org/ontology/plm/rdl/PCA_100006653"/>
    <skos:broadMatch rdf:resource="http://rds.posccaesar.org/ontology/plm/rdl/PCA_100006722"/>
    <rdl:PCA_100006763>To verify that the products and components have been manufactured in accordance with drawings, procedures and specifications.</rdl:PCA_100006763>
    <rdl:PCA_100006768>Final inspection check list for products and components with signature fields for Supplier, customer and third party, and list of all applicable punch items.</rdl:PCA_100006768>
    <rdl:PCA_100006765 rdf:resource="http://w3id.org/readi/rdl/CFIHOS-20000023"/>
    <rdfs:label>Mechanical completion check record (MCCR) / software check record (SWCR) dossier</rdfs:label>
    <rdfs:comment>Final inspection check list for products and components with signature fields for Supplier, customer and third party, and list of all applicable punch items.</rdfs:comment>
  </owl:Class>
  <owl:Class rdf:about="http://rds.posccaesar.org/ontology/plm/rdl/PCA_100006445">
    <rdfs:label>Slewing ring / foundation bolts tension table</rdfs:label>
    <rdfs:comment>No standardized description is presently available.</rdfs:comment>
    <rdl:PCA_100006768>No standardized description is presently available.</rdl:PCA_100006768>
    <rdl:PCA_100006766 rdf:resource="http://rds.posccaesar.org/ontology/plm/rdl/PCA_100006653"/>
    <rdl:PCA_100006763>No standardized description is presently available.</rdl:PCA_100006763>
    <rdfs:subClassOf rdf:resource="http://rds.posccaesar.org/ontology/plm/rdl/PCA_100004908"/>
  </owl:Class>
  <owl:Class rdf:about="http://rds.posccaesar.org/ontology/plm/rdl/PCA_100006433">
    <skos:broader rdf:resource="http://rds.posccaesar.org/ontology/plm/rdl/PCA_100006762"/>
    <skos:broadMatch rdf:resource="http://rds.posccaesar.org/ontology/plm/rdl/PCA_100006705"/>
    <skos:broader rdf:resource="http://rds.posccaesar.org/ontology/plm/rdl/PCA_100006756"/>
    <rdfs:subClassOf rdf:resource="http://rds.posccaesar.org/ontology/plm/rdl/PCA_100004908"/>
    <rdfs:label>Seabed &amp; topographic survey reports and data</rdfs:label>
    <rdl:PCA_100006765 rdf:resource="http://w3id.org/readi/rdl/CFIHOS-20000018"/>
    <rdl:PCA_100006766 rdf:resource="http://rds.posccaesar.org/ontology/plm/rdl/PCA_100006654"/>
    <rdl:PCA_100006764>More details. Survey reports and data shall comply with Company's requirements for Onshore/Offshore surveys.</rdl:PCA_100006764>
    <rdl:PCA_100006763>Design report describing all seabed intervention, pre-and post lay, along the pipeline route including crossings and intervention related to pipeline structures.</rdl:PCA_100006763>
  </owl:Class>
  <owl:Class rdf:about="http://rds.posccaesar.org/ontology/plm/rdl/PCA_100006312">
    <skos:broadMatch rdf:resource="http://rds.posccaesar.org/ontology/plm/rdl/PCA_100006716"/>
    <rdl:PCA_100006765 rdf:resource="http://w3id.org/readi/rdl/CFIHOS-20000001"/>
    <rdfs:subClassOf rdf:resource="http://rds.posccaesar.org/ontology/plm/rdl/PCA_100004908"/>
    <rdfs:label>Master equipment list (MEL)</rdfs:label>
    <skos:broader rdf:resource="http://rds.posccaesar.org/ontology/plm/rdl/PCA_100006748"/>
    <rdfs:comment>List of scope of supply for an contract with identification and quantity (broken down to stand alone equipment).</rdfs:comment>
    <rdl:PCA_100006768>List of scope of supply for an contract with identification and quantity (broken down to stand alone equipment).</rdl:PCA_100006768>
    <rdl:PCA_100006766 rdf:resource="http://rds.posccaesar.org/ontology/plm/rdl/PCA_100006654"/>
    <rdl:PCA_100006763>Give a full overview of the equipment in scope.</rdl:PCA_100006763>
  </owl:Class>
  <owl:Class rdf:about="http://rds.posccaesar.org/ontology/plm/rdl/PCA_100006421">
    <skos:broader rdf:resource="http://rds.posccaesar.org/ontology/plm/rdl/PCA_100006746"/>
    <skos:broadMatch rdf:resource="http://rds.posccaesar.org/ontology/plm/rdl/PCA_100006710"/>
    <rdfs:label>ROV marking drawings</rdfs:label>
    <rdl:PCA_100006765 rdf:resource="http://w3id.org/readi/rdl/CFIHOS-20000031"/>
    <rdl:PCA_100006763>The ROV marking drawing shall identify all marking on the specified objects that are applicable for the ROV intervention work. The ROV marking shall be easily readable on an A3 drawing.</rdl:PCA_100006763>
    <rdfs:subClassOf rdf:resource="http://rds.posccaesar.org/ontology/plm/rdl/PCA_100004908"/>
  </owl:Class>
  <owl:Class rdf:about="http://rds.posccaesar.org/ontology/plm/rdl/PCA_100006530">
    <skos:broader rdf:resource="http://rds.posccaesar.org/ontology/plm/rdl/PCA_100006756"/>
    <skos:broadMatch rdf:resource="http://rds.posccaesar.org/ontology/plm/rdl/PCA_100006717"/>
    <skos:broadMatch rdf:resource="http://rds.posccaesar.org/ontology/plm/rdl/PCA_100006716"/>
    <rdfs:label>Weight report</rdfs:label>
    <rdl:PCA_100006766 rdf:resource="http://rds.posccaesar.org/ontology/plm/rdl/PCA_100006654"/>
    <rdl:PCA_100006765 rdf:resource="http://w3id.org/readi/rdl/CFIHOS-20000006"/>
    <rdl:PCA_100006763>Weight report according to ISO 19901-5.</rdl:PCA_100006763>
    <rdfs:subClassOf rdf:resource="http://rds.posccaesar.org/ontology/plm/rdl/PCA_100004908"/>
  </owl:Class>
  <owl:Class rdf:about="http://rds.posccaesar.org/ontology/plm/rdl/PCA_100006300">
    <rdfs:subClassOf rdf:resource="http://rds.posccaesar.org/ontology/plm/rdl/PCA_100004908"/>
    <skos:broader rdf:resource="http://rds.posccaesar.org/ontology/plm/rdl/PCA_100006762"/>
    <skos:broadMatch rdf:resource="http://rds.posccaesar.org/ontology/plm/rdl/PCA_100006698"/>
    <skos:broadMatch rdf:resource="http://rds.posccaesar.org/ontology/plm/rdl/PCA_100006700"/>
    <rdfs:label>Loop information</rdfs:label>
    <rdl:PCA_100006763>Information sufficient to enable generation of complete loop diagrams as graphical representations from Company’s Loop system for instrument loops, fire &amp; gas, telecom, and electrical interface to SAS shall be provided.</rdl:PCA_100006763>
    <rdl:PCA_100006765 rdf:resource="http://w3id.org/readi/rdl/CFIHOS-20000015"/>
    <skos:broadMatch rdf:resource="http://rds.posccaesar.org/ontology/plm/rdl/PCA_100006699"/>
    <rdl:PCA_100006766 rdf:resource="http://rds.posccaesar.org/ontology/plm/rdl/PCA_100006655"/>
  </owl:Class>
  <owl:Class rdf:about="http://rds.posccaesar.org/ontology/plm/rdl/PCA_100006542">
    <rdl:PCA_100006768>The wiring diagrams for onshore cathodic protection shall cover wire colour, -type, -dimension and -connections.</rdl:PCA_100006768>
    <rdfs:comment>The wiring diagrams for onshore cathodic protection shall cover wire colour, -type, -dimension and -connections.</rdfs:comment>
    <rdl:PCA_100006765 rdf:resource="http://w3id.org/readi/rdl/CFIHOS-20000018"/>
    <rdl:PCA_100006766 rdf:resource="http://rds.posccaesar.org/ontology/plm/rdl/PCA_100006657"/>
    <rdl:PCA_100006763>Ensure safe operation</rdl:PCA_100006763>
    <skos:broadMatch rdf:resource="http://rds.posccaesar.org/ontology/plm/rdl/PCA_100006708"/>
    <rdfs:label>Wiring diagrams for onshore cathodic protection</rdfs:label>
    <rdfs:subClassOf rdf:resource="http://rds.posccaesar.org/ontology/plm/rdl/PCA_100004908"/>
    <skos:broader rdf:resource="http://rds.posccaesar.org/ontology/plm/rdl/PCA_100006745"/>
  </owl:Class>
  <owl:Class rdf:about="http://rds.posccaesar.org/ontology/plm/rdl/PCA_100006200">
    <rdl:PCA_100006763>The FAT report will be used to verify that the equipment has been tested according to FAT procedure.
The FAT report will be used for acceptance of the equipment delivery</rdl:PCA_100006763>
    <skos:broader rdf:resource="http://rds.posccaesar.org/ontology/plm/rdl/PCA_100006756"/>
    <skos:broadMatch rdf:resource="http://rds.posccaesar.org/ontology/plm/rdl/PCA_100006722"/>
    <rdl:PCA_100006765 rdf:resource="http://w3id.org/readi/rdl/CFIHOS-20000027"/>
    <rdfs:label>Factory acceptance test (FAT) report</rdfs:label>
    <rdfs:subClassOf rdf:resource="http://rds.posccaesar.org/ontology/plm/rdl/PCA_100004908"/>
    <rdl:PCA_100006766 rdf:resource="http://rds.posccaesar.org/ontology/plm/rdl/PCA_100006653"/>
    <rdl:PCA_100006768>This document shall record and document all activities performed and results from these, in accordance with the FAT procedure. 
This document outline all testing activities and their acceptance criteria to document the condition of the equipment as tested from factory.</rdl:PCA_100006768>
    <rdfs:comment>This document shall record and document all activities performed and results from these, in accordance with the FAT procedure. 
This document outline all testing activities and their acceptance criteria to document the condition of the equipment as tested from factory.</rdfs:comment>
  </owl:Class>
  <owl:Class rdf:about="http://rds.posccaesar.org/ontology/plm/rdl/PCA_100006212">
    <rdl:PCA_100006768>Document fire test</rdl:PCA_100006768>
    <skos:broadMatch rdf:resource="http://rds.posccaesar.org/ontology/plm/rdl/PCA_100006722"/>
    <rdfs:subClassOf rdf:resource="http://rds.posccaesar.org/ontology/plm/rdl/PCA_100004908"/>
    <skos:broader rdf:resource="http://rds.posccaesar.org/ontology/plm/rdl/PCA_100006743"/>
    <rdl:PCA_100006765 rdf:resource="http://w3id.org/readi/rdl/CFIHOS-20000013"/>
    <rdl:PCA_100006763>For compliance</rdl:PCA_100006763>
    <rdfs:label>Fire test certificate</rdfs:label>
    <rdfs:comment>Document fire test</rdfs:comment>
    <rdl:PCA_100006766 rdf:resource="http://rds.posccaesar.org/ontology/plm/rdl/PCA_100006653"/>
  </owl:Class>
  <owl:Class rdf:about="http://rds.posccaesar.org/ontology/plm/rdl/PCA_100006103">
    <rdl:PCA_100006766 rdf:resource="http://rds.posccaesar.org/ontology/plm/rdl/PCA_100006657"/>
    <skos:broader rdf:resource="http://rds.posccaesar.org/ontology/plm/rdl/PCA_100006753"/>
    <rdfs:comment>A spreadsheet shall be prepared. This shall include all barrier system /element given in DNV-RP-F116:2019, table I-7. The spreadsheet shall also include function, reliability and robustness per barrier element/threat. (Template available in Equinor, however needs to be updated). .</rdfs:comment>
    <rdfs:subClassOf rdf:resource="http://rds.posccaesar.org/ontology/plm/rdl/PCA_100004908"/>
    <rdl:PCA_100006763>An overview of all barriers to prevent hazardous event, and barriers to control consequences and effects for a pipeline system is needed for safe operation. Reference is given to DNV-RP-F116:2019, figure I-1.</rdl:PCA_100006763>
    <rdl:PCA_100006765 rdf:resource="http://w3id.org/readi/rdl/CFIHOS-20000018"/>
    <rdl:PCA_100006768>A spreadsheet shall be prepared. This shall include all barrier system /element given in DNV-RP-F116:2019, table I-7. The spreadsheet shall also include function, reliability and robustness per barrier element/threat. (Template available in Equinor, however needs to be updated). .</rdl:PCA_100006768>
    <skos:broadMatch rdf:resource="http://rds.posccaesar.org/ontology/plm/rdl/PCA_100006699"/>
    <rdfs:label>Barrier matrix</rdfs:label>
  </owl:Class>
  <owl:Class rdf:about="http://rds.posccaesar.org/ontology/plm/rdl/PCA_100006224">
    <rdfs:subClassOf rdf:resource="http://rds.posccaesar.org/ontology/plm/rdl/PCA_100004908"/>
    <rdfs:label>Flowline routing</rdfs:label>
    <rdfs:comment>Schematic showing the flow path, line size, equipment and connections for process and utility systems. The schematic shall use standard symbols.</rdfs:comment>
    <rdl:PCA_100006765 rdf:resource="http://w3id.org/readi/rdl/CFIHOS-20000018"/>
    <skos:broader rdf:resource="http://rds.posccaesar.org/ontology/plm/rdl/PCA_100006746"/>
    <rdl:PCA_100006768>Schematic showing the flow path, line size, equipment and connections for process and utility systems. The schematic shall use standard symbols.</rdl:PCA_100006768>
    <skos:broadMatch rdf:resource="http://rds.posccaesar.org/ontology/plm/rdl/PCA_100006705"/>
    <rdl:PCA_100006766 rdf:resource="http://rds.posccaesar.org/ontology/plm/rdl/PCA_100006657"/>
    <rdl:PCA_100006763>Provide a simplified overview of connections, lines with sizes and equipment for a sub-system. Basis for piping design.</rdl:PCA_100006763>
  </owl:Class>
  <owl:Class rdf:about="http://rds.posccaesar.org/ontology/plm/rdl/PCA_100006115">
    <rdl:PCA_100006763>The purpose of Cause &amp; Effect (C&amp;E) Diagram is to define logic control and shutdown functions.</rdl:PCA_100006763>
    <rdl:PCA_100006766 rdf:resource="http://rds.posccaesar.org/ontology/plm/rdl/PCA_100006640"/>
    <rdl:PCA_100006766 rdf:resource="http://rds.posccaesar.org/ontology/plm/rdl/PCA_100006638"/>
    <rdl:PCA_100006765 rdf:resource="http://w3id.org/readi/rdl/CFIHOS-20000031"/>
    <rdl:PCA_100006766 rdf:resource="http://rds.posccaesar.org/ontology/plm/rdl/PCA_100006635"/>
    <rdl:PCA_100006766 rdf:resource="http://rds.posccaesar.org/ontology/plm/rdl/PCA_100006633"/>
    <rdl:PCA_100006766 rdf:resource="http://rds.posccaesar.org/ontology/plm/rdl/PCA_100006628"/>
    <rdl:PCA_100006766 rdf:resource="http://rds.posccaesar.org/ontology/plm/rdl/PCA_100006641"/>
    <rdl:PCA_100006766 rdf:resource="http://rds.posccaesar.org/ontology/plm/rdl/PCA_100006636"/>
    <rdl:PCA_100006765 rdf:resource="http://w3id.org/readi/rdl/CFIHOS-20000015"/>
    <rdl:PCA_100006766 rdf:resource="http://rds.posccaesar.org/ontology/plm/rdl/PCA_100006639"/>
    <skos:broader rdf:resource="http://rds.posccaesar.org/ontology/plm/rdl/PCA_100006742"/>
    <rdl:PCA_100006766 rdf:resource="http://rds.posccaesar.org/ontology/plm/rdl/PCA_100006634"/>
    <rdl:PCA_100006766 rdf:resource="http://rds.posccaesar.org/ontology/plm/rdl/PCA_100006626"/>
    <rdfs:comment>The C&amp;E Diagram shall be prepared as a matrix between initiating (input) and actuated elements (output) performing the corrective action. Both input and output shall be identified by ENS tag numbers. In addition, the following information shall be given for each input/output:
 - Tag number, Initiator/Actuator, Value, Note, Service description.
 - Reference drawing number (e.g. Piping &amp; instrument diagram).

Note: The cause and effect for the fire and gas detection system is included in the Fire protection data sheet (FPDS).</rdfs:comment>
    <rdfs:subClassOf rdf:resource="http://rds.posccaesar.org/ontology/plm/rdl/PCA_100004908"/>
    <rdl:PCA_100006766 rdf:resource="http://rds.posccaesar.org/ontology/plm/rdl/PCA_100006637"/>
    <skos:broadMatch rdf:resource="http://rds.posccaesar.org/ontology/plm/rdl/PCA_100006699"/>
    <rdl:PCA_100006766 rdf:resource="http://rds.posccaesar.org/ontology/plm/rdl/PCA_100006627"/>
    <rdl:PCA_100006768>The C&amp;E Diagram shall be prepared as a matrix between initiating (input) and actuated elements (output) performing the corrective action. Both input and output shall be identified by ENS tag numbers. In addition, the following information shall be given for each input/output:
 - Tag number, Initiator/Actuator, Value, Note, Service description.
 - Reference drawing number (e.g. Piping &amp; instrument diagram).

Note: The cause and effect for the fire and gas detection system is included in the Fire protection data sheet (FPDS).</rdl:PCA_100006768>
    <rdfs:label>Cause &amp; effect (C&amp;E)</rdfs:label>
  </owl:Class>
  <owl:Class rdf:about="http://rds.posccaesar.org/ontology/plm/rdl/PCA_100006127">
    <rdl:PCA_100006768>Commissioning report shall be according to ISO15589-1 Section 13.2</rdl:PCA_100006768>
    <rdfs:label>Commissioning report CP system (close out report)</rdfs:label>
    <rdl:PCA_100006766 rdf:resource="http://rds.posccaesar.org/ontology/plm/rdl/PCA_100006657"/>
    <rdl:PCA_100006765 rdf:resource="http://w3id.org/readi/rdl/CFIHOS-20000018"/>
    <skos:broadMatch>
      <rdl:PCA_100001503 rdf:about="http://rds.posccaesar.org/ontology/plm/rdl/PCA_100006663">
        <rdfs:label>stakeholder information</rdfs:label>
        <rdl:PCA_100004924>BA</rdl:PCA_100004924>
        <rdf:type rdf:resource="http://www.w3.org/2002/07/owl#NamedIndividual"/>
      </rdl:PCA_100001503>
    </skos:broadMatch>
    <skos:broader rdf:resource="http://rds.posccaesar.org/ontology/plm/rdl/PCA_100006756"/>
    <rdl:PCA_100006763>Document the performance of the CP system</rdl:PCA_100006763>
    <rdfs:comment>Commissioning report shall be according to ISO15589-1 Section 13.2</rdfs:comment>
    <rdfs:subClassOf rdf:resource="http://rds.posccaesar.org/ontology/plm/rdl/PCA_100004908"/>
  </owl:Class>
  <owl:Class rdf:about="http://rds.posccaesar.org/ontology/plm/rdl/PCA_100006139">
    <rdfs:subClassOf rdf:resource="http://rds.posccaesar.org/ontology/plm/rdl/PCA_100004908"/>
    <rdl:PCA_100006766 rdf:resource="http://rds.posccaesar.org/ontology/plm/rdl/PCA_100006654"/>
    <rdl:PCA_100006763>Overview of pipeline crossings</rdl:PCA_100006763>
    <rdfs:label>Crossing lists</rdfs:label>
    <rdl:PCA_100006765 rdf:resource="http://w3id.org/readi/rdl/CFIHOS-20000018"/>
    <skos:broadMatch>
      <rdl:PCA_100001503 rdf:about="http://rds.posccaesar.org/ontology/plm/rdl/PCA_100006720">
        <rdfs:label>location listing</rdfs:label>
        <rdl:PCA_100004924>PL</rdl:PCA_100004924>
        <rdf:type rdf:resource="http://www.w3.org/2002/07/owl#NamedIndividual"/>
      </rdl:PCA_100001503>
    </skos:broadMatch>
    <rdl:PCA_100006768>List of all crossings (pipelines, roads, road allowances, rivers, power line, cables, railway lines etc.) in chronological order along the pipeline (KP) with geographical position, type of crossing and crossing method. Also include reference to relevant crossing design drawings. Owner and content of the crossed object.</rdl:PCA_100006768>
    <skos:broader rdf:resource="http://rds.posccaesar.org/ontology/plm/rdl/PCA_100006748"/>
    <rdfs:comment>List of all crossings (pipelines, roads, road allowances, rivers, power line, cables, railway lines etc.) in chronological order along the pipeline (KP) with geographical position, type of crossing and crossing method. Also include reference to relevant crossing design drawings. Owner and content of the crossed object.</rdfs:comment>
  </owl:Class>
  <owl:Class rdf:about="http://rds.posccaesar.org/ontology/plm/rdl/PCA_100006349">
    <skos:broadMatch rdf:resource="http://rds.posccaesar.org/ontology/plm/rdl/PCA_100006688"/>
    <rdl:PCA_100006768>Content shall be according to Section 8.9 in API 17J, and the following additional requirements:
 - Values for operational parameter critical for service life including operational pressure and temperatures with description of effect if exceeding these values.
 - Drawings of riser configuration from topside hang-off to the seabed connection to interface structure identifying section lengths, ancillary components, characteristic water depths for the configuration including identification of values for normal operation maximum/minimum density, maximum and minimum offset and temporary water filled condition.
 - List of situations that could be potentially detrimental to the flexible pipe including plan of action for such situations.</rdl:PCA_100006768>
    <rdfs:comment>Content shall be according to Section 8.9 in API 17J, and the following additional requirements:
 - Values for operational parameter critical for service life including operational pressure and temperatures with description of effect if exceeding these values.
 - Drawings of riser configuration from topside hang-off to the seabed connection to interface structure identifying section lengths, ancillary components, characteristic water depths for the configuration including identification of values for normal operation maximum/minimum density, maximum and minimum offset and temporary water filled condition.
 - List of situations that could be potentially detrimental to the flexible pipe including plan of action for such situations.</rdfs:comment>
    <rdl:PCA_100006765 rdf:resource="http://w3id.org/readi/rdl/CFIHOS-20000018"/>
    <rdfs:subClassOf rdf:resource="http://rds.posccaesar.org/ontology/plm/rdl/PCA_100004908"/>
    <rdfs:label>Operation manual flexible pipeline and riser</rdfs:label>
    <rdl:PCA_100006763>Ensure safe operation</rdl:PCA_100006763>
    <skos:broader rdf:resource="http://rds.posccaesar.org/ontology/plm/rdl/PCA_100006751"/>
    <rdl:PCA_100006766 rdf:resource="http://rds.posccaesar.org/ontology/plm/rdl/PCA_100006654"/>
  </owl:Class>
  <owl:Class rdf:about="http://rds.posccaesar.org/ontology/plm/rdl/PCA_100006337">
    <rdl:PCA_100006766 rdf:resource="http://rds.posccaesar.org/ontology/plm/rdl/PCA_100006634"/>
    <rdl:PCA_100006766 rdf:resource="http://rds.posccaesar.org/ontology/plm/rdl/PCA_100006637"/>
    <rdfs:comment>Typical contents shall be:
 - Related servers, switches, routers, firewalls and computers represented by a relevant symbol, marked with its identification and description of function;
 - Location of the equipment identifying the zone for the system;
 - Communication between units shall be indicated, also wireless interfaces;
 - Reference to information concerning IP/MAC addresses (restricted information);
 - Reference to information concerning firewall rules (restricted information);
 - Signal type, protocol and function (typ. RS232, control signal) if applicable;
 - Colour coding to indicate criticality level of the system.

For smaller technical networks the information from the subsystem block diagram can be integrated in the overall system topology, provided the readability of the drawing are maintained.</rdfs:comment>
    <rdl:PCA_100006765 rdf:resource="http://w3id.org/readi/rdl/CFIHOS-20000015"/>
    <rdl:PCA_100006763>Overall network topology shall show topology of technical network and subnetwork to give a functional understanding and a foundation for a risk and vulnerability analysis.</rdl:PCA_100006763>
    <rdl:PCA_100006766 rdf:resource="http://rds.posccaesar.org/ontology/plm/rdl/PCA_100006635"/>
    <rdfs:label>Network topology diagram</rdfs:label>
    <rdl:PCA_100006766 rdf:resource="http://rds.posccaesar.org/ontology/plm/rdl/PCA_100006633"/>
    <rdfs:subClassOf rdf:resource="http://rds.posccaesar.org/ontology/plm/rdl/PCA_100004908"/>
    <skos:broadMatch rdf:resource="http://rds.posccaesar.org/ontology/plm/rdl/PCA_100006695"/>
    <skos:broader rdf:resource="http://rds.posccaesar.org/ontology/plm/rdl/PCA_100006745"/>
    <rdl:PCA_100006766 rdf:resource="http://rds.posccaesar.org/ontology/plm/rdl/PCA_100006626"/>
    <rdl:PCA_100006768>Typical contents shall be:
 - Related servers, switches, routers, firewalls and computers represented by a relevant symbol, marked with its identification and description of function;
 - Location of the equipment identifying the zone for the system;
 - Communication between units shall be indicated, also wireless interfaces;
 - Reference to information concerning IP/MAC addresses (restricted information);
 - Reference to information concerning firewall rules (restricted information);
 - Signal type, protocol and function (typ. RS232, control signal) if applicable;
 - Colour coding to indicate criticality level of the system.

For smaller technical networks the information from the subsystem block diagram can be integrated in the overall system topology, provided the readability of the drawing are maintained.</rdl:PCA_100006768>
    <rdl:PCA_100006766 rdf:resource="http://rds.posccaesar.org/ontology/plm/rdl/PCA_100006636"/>
  </owl:Class>
  <owl:Class rdf:about="http://rds.posccaesar.org/ontology/plm/rdl/PCA_100006458">
    <rdl:PCA_100006766 rdf:resource="http://rds.posccaesar.org/ontology/plm/rdl/PCA_100006643"/>
    <skos:broader rdf:resource="http://rds.posccaesar.org/ontology/plm/rdl/PCA_100006762"/>
    <skos:broader rdf:resource="http://rds.posccaesar.org/ontology/plm/rdl/PCA_100006741"/>
    <rdl:PCA_100006768>It shall be possible to import the files and re-run the entire analysis following a provided step-by-step list. A description on how to import the zip file and run the analysis shall be delivered.</rdl:PCA_100006768>
    <rdfs:comment>It shall be possible to import the files and re-run the entire analysis following a provided step-by-step list. A description on how to import the zip file and run the analysis shall be delivered.</rdfs:comment>
    <rdl:PCA_100006765 rdf:resource="http://w3id.org/readi/rdl/CFIHOS-20000006"/>
    <rdfs:subClassOf rdf:resource="http://rds.posccaesar.org/ontology/plm/rdl/PCA_100004908"/>
    <rdl:PCA_100006766>
      <rdl:PCA_100001503 rdf:about="http://rds.posccaesar.org/ontology/plm/rdl/PCA_100006644">
        <rdfs:label>Sub structure</rdfs:label>
        <rdl:PCA_100004924>91</rdl:PCA_100004924>
        <rdf:type rdf:resource="http://www.w3.org/2002/07/owl#NamedIndividual"/>
      </rdl:PCA_100001503>
    </rdl:PCA_100006766>
    <skos:broadMatch rdf:resource="http://rds.posccaesar.org/ontology/plm/rdl/PCA_100006687"/>
    <rdfs:label>Structural analysis model</rdfs:label>
    <rdl:PCA_100006763>If engineering contractor or 3rd party verification body have made a global structural analysis model, then a zip file with input files and FEM files shall be delivered with a short description of each input file.</rdl:PCA_100006763>
  </owl:Class>
  <owl:Class rdf:about="http://rds.posccaesar.org/ontology/plm/rdl/PCA_100006446">
    <skos:broader rdf:resource="http://rds.posccaesar.org/ontology/plm/rdl/PCA_100006748"/>
    <skos:broadMatch rdf:resource="http://rds.posccaesar.org/ontology/plm/rdl/PCA_100006710"/>
    <rdfs:label>Slewing ring/foundation bolts tension table - lifting appliances</rdfs:label>
    <rdfs:comment>For bolts using pre-tensioning, the table shall include length measurements before and after pre-tensioning including allowable tolerances.</rdfs:comment>
    <rdl:PCA_100006768>For bolts using pre-tensioning, the table shall include length measurements before and after pre-tensioning including allowable tolerances.</rdl:PCA_100006768>
    <rdl:PCA_100006763>A table showing pre-tensioning / extension for each slewing ring / pedestal adapter / foundation bolts after final assembly shall be delivered.</rdl:PCA_100006763>
    <rdfs:subClassOf rdf:resource="http://rds.posccaesar.org/ontology/plm/rdl/PCA_100004908"/>
  </owl:Class>
  <owl:Class rdf:about="http://rds.posccaesar.org/ontology/plm/rdl/PCA_100006325">
    <skos:broader rdf:resource="http://rds.posccaesar.org/ontology/plm/rdl/PCA_100006756"/>
    <skos:broadMatch rdf:resource="http://rds.posccaesar.org/ontology/plm/rdl/PCA_100006698"/>
    <skos:broadMatch rdf:resource="http://rds.posccaesar.org/ontology/plm/rdl/PCA_100006691"/>
    <rdfs:label>Metocean - meterological and oceanographical reports</rdfs:label>
    <rdl:PCA_100006766 rdf:resource="http://rds.posccaesar.org/ontology/plm/rdl/PCA_100006656"/>
    <rdl:PCA_100006765 rdf:resource="http://w3id.org/readi/rdl/CFIHOS-20000007"/>
    <rdl:PCA_100006763>The reports shall comply with requirements in: 
WMO 1995 Technical regulation manual on codes, Vol I.1, WMO No. 306 Genova;
ISO 19901-1 Petroleum and natural gas industries – Specific requirements for offshore structures – Part 1: Metocean design and operating considerations.</rdl:PCA_100006763>
    <rdfs:subClassOf rdf:resource="http://rds.posccaesar.org/ontology/plm/rdl/PCA_100004908"/>
  </owl:Class>
  <owl:Class rdf:about="http://rds.posccaesar.org/ontology/plm/rdl/PCA_100006434">
    <rdl:PCA_100006763>To provide basis for planning pipeline, riser or umbilical installation. Provide input to analysis and installation procedure.</rdl:PCA_100006763>
    <rdfs:subClassOf rdf:resource="http://rds.posccaesar.org/ontology/plm/rdl/PCA_100004908"/>
    <rdl:PCA_100006765 rdf:resource="http://w3id.org/readi/rdl/CFIHOS-20000018"/>
    <skos:broader rdf:resource="http://rds.posccaesar.org/ontology/plm/rdl/PCA_100006756"/>
    <rdl:PCA_100006768>Report describing the required seabed intervention for the chosen routing.</rdl:PCA_100006768>
    <rdfs:comment>Report describing the required seabed intervention for the chosen routing.</rdfs:comment>
    <rdl:PCA_100006766 rdf:resource="http://rds.posccaesar.org/ontology/plm/rdl/PCA_100006657"/>
    <rdfs:label>Seabed intervention design report</rdfs:label>
    <skos:broadMatch rdf:resource="http://rds.posccaesar.org/ontology/plm/rdl/PCA_100006686"/>
  </owl:Class>
  <owl:Class rdf:about="http://rds.posccaesar.org/ontology/plm/rdl/PCA_100006543">
    <rdl:PCA_100006766 rdf:resource="http://rds.posccaesar.org/ontology/plm/rdl/PCA_100006640"/>
    <skos:broader rdf:resource="http://rds.posccaesar.org/ontology/plm/rdl/PCA_100006756"/>
    <rdfs:label>WLAN coverage</rdfs:label>
    <rdl:PCA_100006768>Wireless Local Area Network (WLAN) coverage chart/test report shall be provided.</rdl:PCA_100006768>
    <skos:broadMatch rdf:resource="http://rds.posccaesar.org/ontology/plm/rdl/PCA_100006722"/>
    <skos:broadMatch rdf:resource="http://rds.posccaesar.org/ontology/plm/rdl/PCA_100006705"/>
    <rdfs:subClassOf rdf:resource="http://rds.posccaesar.org/ontology/plm/rdl/PCA_100004908"/>
    <rdl:PCA_100006765 rdf:resource="http://w3id.org/readi/rdl/CFIHOS-20000030"/>
    <rdfs:comment>Wireless Local Area Network (WLAN) coverage chart/test report shall be provided.</rdfs:comment>
  </owl:Class>
  <owl:Class rdf:about="http://rds.posccaesar.org/ontology/plm/rdl/PCA_100006313">
    <skos:broader rdf:resource="http://rds.posccaesar.org/ontology/plm/rdl/PCA_100006756"/>
    <skos:broadMatch rdf:resource="http://rds.posccaesar.org/ontology/plm/rdl/PCA_100006705"/>
    <rdfs:label>Master grid report</rdfs:label>
    <rdfs:comment>The Master grid report shall include following information:
 - Master grid ID;
 - Easting;
 - Northing;
 - Elevation;
 - Count (number of measurements for each MG);
 - Root mean square (RMS) error for each MG point.

Secondary Grid data shall be included in the Master Grid report as an attachment.</rdfs:comment>
    <rdl:PCA_100006768>The Master grid report shall include following information:
 - Master grid ID;
 - Easting;
 - Northing;
 - Elevation;
 - Count (number of measurements for each MG);
 - Root mean square (RMS) error for each MG point.

Secondary Grid data shall be included in the Master Grid report as an attachment.</rdl:PCA_100006768>
    <rdl:PCA_100006766 rdf:resource="http://rds.posccaesar.org/ontology/plm/rdl/PCA_100006656"/>
    <rdl:PCA_100006763>The objective of Master Grid is to facilitate the availability of trusted spatial information throughout the installation life cycle.</rdl:PCA_100006763>
    <rdfs:subClassOf rdf:resource="http://rds.posccaesar.org/ontology/plm/rdl/PCA_100004908"/>
  </owl:Class>
  <owl:Class rdf:about="http://rds.posccaesar.org/ontology/plm/rdl/PCA_100006301">
    <skos:broader rdf:resource="http://rds.posccaesar.org/ontology/plm/rdl/PCA_100006748"/>
    <skos:broadMatch rdf:resource="http://rds.posccaesar.org/ontology/plm/rdl/PCA_100006717"/>
    <rdfs:label>Lubrication index</rdfs:label>
    <rdfs:comment>A lubrication index shall be provided containing the following information:
 - Tag code
 - Location of sampling point
 - Lubrication point sequence number (allocated by Company and referred to as TAS number) Supplier lubricant (product type)
 - Company equivalent lubricant
 - Quantity first fill
 - Quantity normal
 - Interval or monitoring frequency and parameters (particles, water content and additives) 

The above lubrication information shall be provided in the Excel template linked below.
 Lubrication information template for SAP uploading</rdfs:comment>
    <rdl:PCA_100006768>A lubrication index shall be provided containing the following information:
 - Tag code
 - Location of sampling point
 - Lubrication point sequence number (allocated by Company and referred to as TAS number) Supplier lubricant (product type)
 - Company equivalent lubricant
 - Quantity first fill
 - Quantity normal
 - Interval or monitoring frequency and parameters (particles, water content and additives) 

The above lubrication information shall be provided in the Excel template linked below.
 Lubrication information template for SAP uploading</rdl:PCA_100006768>
    <rdfs:subClassOf rdf:resource="http://rds.posccaesar.org/ontology/plm/rdl/PCA_100004908"/>
  </owl:Class>
  <owl:Class rdf:about="http://rds.posccaesar.org/ontology/plm/rdl/PCA_100006422">
    <rdl:PCA_100006768>A list documenting all foreseen subsea operations requiring ROV intervention.</rdl:PCA_100006768>
    <rdl:PCA_100006765 rdf:resource="http://w3id.org/readi/rdl/CFIHOS-20000031"/>
    <rdfs:label>ROV task list</rdfs:label>
    <rdfs:comment>A list documenting all foreseen subsea operations requiring ROV intervention.</rdfs:comment>
    <rdfs:subClassOf rdf:resource="http://rds.posccaesar.org/ontology/plm/rdl/PCA_100004908"/>
    <skos:broadMatch rdf:resource="http://rds.posccaesar.org/ontology/plm/rdl/PCA_100006688"/>
    <skos:broader rdf:resource="http://rds.posccaesar.org/ontology/plm/rdl/PCA_100006751"/>
    <rdl:PCA_100006763>Give an overview of all foreseen ROV intervention to enable planning of intervention and ROV access verification.</rdl:PCA_100006763>
    <rdl:PCA_100006766 rdf:resource="http://rds.posccaesar.org/ontology/plm/rdl/PCA_100006654"/>
  </owl:Class>
  <owl:Class rdf:about="http://rds.posccaesar.org/ontology/plm/rdl/PCA_100006410">
    <rdl:PCA_100006768>The Relay setting table is part of the "Protection and discrimination study" 

Where practical, the relay setting table shall be made similar as "Parameter setting tables", i.e. combination of templates and setting tables for parameters with individual setting.</rdl:PCA_100006768>
    <rdl:PCA_100006765 rdf:resource="http://w3id.org/readi/rdl/CFIHOS-20000008"/>
    <rdfs:comment>The Relay setting table is part of the "Protection and discrimination study" 

Where practical, the relay setting table shall be made similar as "Parameter setting tables", i.e. combination of templates and setting tables for parameters with individual setting.</rdfs:comment>
    <rdfs:subClassOf rdf:resource="http://rds.posccaesar.org/ontology/plm/rdl/PCA_100004908"/>
    <rdl:PCA_100006766 rdf:resource="http://rds.posccaesar.org/ontology/plm/rdl/PCA_100006639"/>
    <rdl:PCA_100006766 rdf:resource="http://rds.posccaesar.org/ontology/plm/rdl/PCA_100006637"/>
    <rdl:PCA_100006766 rdf:resource="http://rds.posccaesar.org/ontology/plm/rdl/PCA_100006635"/>
    <rdfs:label>Relay setting table</rdfs:label>
    <rdl:PCA_100006766 rdf:resource="http://rds.posccaesar.org/ontology/plm/rdl/PCA_100006638"/>
    <rdl:PCA_100006766 rdf:resource="http://rds.posccaesar.org/ontology/plm/rdl/PCA_100006636"/>
    <skos:broader rdf:resource="http://rds.posccaesar.org/ontology/plm/rdl/PCA_100006762"/>
    <rdl:PCA_100006766 rdf:resource="http://rds.posccaesar.org/ontology/plm/rdl/PCA_100006634"/>
    <rdl:PCA_100006763>See requirement for protection and discrimination coordination study, ref. (Z-001-0052 - Electrical calculations / analyses).</rdl:PCA_100006763>
    <skos:broadMatch>
      <rdl:PCA_100001503 rdf:about="http://rds.posccaesar.org/ontology/plm/rdl/PCA_100006701">
        <rdfs:label>set value information</rdfs:label>
        <rdl:PCA_100004924>FQ</rdl:PCA_100004924>
        <rdf:type rdf:resource="http://www.w3.org/2002/07/owl#NamedIndividual"/>
      </rdl:PCA_100001503>
    </skos:broadMatch>
  </owl:Class>
  <owl:Class rdf:about="http://rds.posccaesar.org/ontology/plm/rdl/PCA_100006531">
    <skos:broader rdf:resource="http://rds.posccaesar.org/ontology/plm/rdl/PCA_100006748"/>
    <skos:broadMatch rdf:resource="http://rds.posccaesar.org/ontology/plm/rdl/PCA_100006717"/>
    <skos:broadMatch rdf:resource="http://rds.posccaesar.org/ontology/plm/rdl/PCA_100006716"/>
    <rdfs:label>Weld summary index</rdfs:label>
    <rdfs:comment>The minimum requirements for this index are described below: 1. Weld no. inclusive Weld repair no. 2. Welder no. 3. Ref. to fabrication-, shop- and/or isometric drawing 4. Piping system and line no. 5. PWHT (Post Weld Heat Treatment); i.e. procedures and temperature-time records 6. WPS no. (with reference to WPQR no.) 7. Weld repair log 8. Non-Destructive Test (NDT) extent in % for different methods (e.g. UT, RT, MT, PT) 9. Visual inspection (e.g. on completed weld) 10. Weld inspection (e.g. QC activities; weld preparation, tack welding, parameter verification, consumable control, field metallographic verification, etc.) 11. NDT report number / Inspection report number 12. Weld completion time/date and NDT time/date 13. PMI (Positive Material Identification) report 14. Production tests (destructive testing when applicable) 15. Special procedures (e.g. cleaning/pickling, grinding or hammer peening of weld toe, straightening)</rdfs:comment>
    <rdl:PCA_100006768>The minimum requirements for this index are described below: 1. Weld no. inclusive Weld repair no. 2. Welder no. 3. Ref. to fabrication-, shop- and/or isometric drawing 4. Piping system and line no. 5. PWHT (Post Weld Heat Treatment); i.e. procedures and temperature-time records 6. WPS no. (with reference to WPQR no.) 7. Weld repair log 8. Non-Destructive Test (NDT) extent in % for different methods (e.g. UT, RT, MT, PT) 9. Visual inspection (e.g. on completed weld) 10. Weld inspection (e.g. QC activities; weld preparation, tack welding, parameter verification, consumable control, field metallographic verification, etc.) 11. NDT report number / Inspection report number 12. Weld completion time/date and NDT time/date 13. PMI (Positive Material Identification) report 14. Production tests (destructive testing when applicable) 15. Special procedures (e.g. cleaning/pickling, grinding or hammer peening of weld toe, straightening)</rdl:PCA_100006768>
    <rdl:PCA_100006763>It shall be prepared on basis of the weld numbering system, starting with the lowest weld number. The list shall be prepared prior to start of welding and NDE, and updating shall be parallel to execution of welding and NDE.</rdl:PCA_100006763>
    <rdfs:subClassOf rdf:resource="http://rds.posccaesar.org/ontology/plm/rdl/PCA_100004908"/>
  </owl:Class>
  <owl:Class rdf:about="http://rds.posccaesar.org/ontology/plm/rdl/PCA_100006211">
    <rdl:PCA_100006766 rdf:resource="http://rds.posccaesar.org/ontology/plm/rdl/PCA_100006628"/>
    <rdfs:subClassOf rdf:resource="http://rds.posccaesar.org/ontology/plm/rdl/PCA_100004908"/>
    <skos:broadMatch rdf:resource="http://rds.posccaesar.org/ontology/plm/rdl/PCA_100006727"/>
    <rdl:PCA_100006768>A fire protection datasheet shall be produced for each of the defined fire detection areas. 

The fire protection data sheets shall include the following main information elements:
 - Key characteristics of area barriers:
   - Area classification references (zone 1, zone 2, non-hazardous by location, non-hazardous by ventilation);
   - Ventilation of the area (natural, mechanical, overpressure, underpressure);
   - Occupancy (permanent, intermittent, normally none, none);
   - Construction of walls/floors/ceiling (none, wind shield, heat shield, steel walls, fire partitions with fire rating, explosion panels, suspended ceiling, false floor);
   - Hazards in the area (e.g. crude oil, toxic gas, chemicals, fuel oil, electrical, radioactive, etc.);
   - Type of fire and gas detection in the area;
   - Type of fire protection with application design rates;
 - Basis for fire and gas detection design and fire protection:
   - A listing of main equipment of the area which governs the fire and gas detection selection and location;
   - A description of the basis for the selection of particular type and position of detectors including manual call points. This is an area specific detailing of the general fire and gas logic;
   - A reference of area fire extinguishing facilities;
 - Fire and Gas Cause &amp; Effect:
   - This part shall be according to Cause &amp; Effect requirements addressing the specific fire and gas detection logic including means for fire extinguishing control and monitoring and other specific output actions;
   - The C&amp;E sheet shall include a listing of all area tag numbers, i.e., fire and gas detectors and output devices.</rdl:PCA_100006768>
    <rdfs:comment>A fire protection datasheet shall be produced for each of the defined fire detection areas. 

The fire protection data sheets shall include the following main information elements:
 - Key characteristics of area barriers:
   - Area classification references (zone 1, zone 2, non-hazardous by location, non-hazardous by ventilation);
   - Ventilation of the area (natural, mechanical, overpressure, underpressure);
   - Occupancy (permanent, intermittent, normally none, none);
   - Construction of walls/floors/ceiling (none, wind shield, heat shield, steel walls, fire partitions with fire rating, explosion panels, suspended ceiling, false floor);
   - Hazards in the area (e.g. crude oil, toxic gas, chemicals, fuel oil, electrical, radioactive, etc.);
   - Type of fire and gas detection in the area;
   - Type of fire protection with application design rates;
 - Basis for fire and gas detection design and fire protection:
   - A listing of main equipment of the area which governs the fire and gas detection selection and location;
   - A description of the basis for the selection of particular type and position of detectors including manual call points. This is an area specific detailing of the general fire and gas logic;
   - A reference of area fire extinguishing facilities;
 - Fire and Gas Cause &amp; Effect:
   - This part shall be according to Cause &amp; Effect requirements addressing the specific fire and gas detection logic including means for fire extinguishing control and monitoring and other specific output actions;
   - The C&amp;E sheet shall include a listing of all area tag numbers, i.e., fire and gas detectors and output devices.</rdfs:comment>
    <rdl:PCA_100006763>Fire protection data sheets shall document the fire and explosion protection and detection design. Fire protection data sheets shall be maintained throughout the plant or installation lifetime and be consistent with information in other engineering/operational databases.</rdl:PCA_100006763>
    <skos:broader rdf:resource="http://rds.posccaesar.org/ontology/plm/rdl/PCA_100006747"/>
    <rdl:PCA_100006766 rdf:resource="http://rds.posccaesar.org/ontology/plm/rdl/PCA_100006633"/>
    <rdfs:label>Fire protection data sheet (FPDS)</rdfs:label>
    <rdl:PCA_100006766 rdf:resource="http://rds.posccaesar.org/ontology/plm/rdl/PCA_100006627"/>
    <rdl:PCA_100006765 rdf:resource="http://w3id.org/readi/rdl/CFIHOS-20000015"/>
    <rdl:PCA_100006766 rdf:resource="http://rds.posccaesar.org/ontology/plm/rdl/PCA_100006626"/>
  </owl:Class>
  <owl:Class rdf:about="http://rds.posccaesar.org/ontology/plm/rdl/PCA_100006223">
    <rdl:PCA_100006766 rdf:resource="http://rds.posccaesar.org/ontology/plm/rdl/PCA_100006657"/>
    <skos:broader rdf:resource="http://rds.posccaesar.org/ontology/plm/rdl/PCA_100006745"/>
    <rdfs:subClassOf rdf:resource="http://rds.posccaesar.org/ontology/plm/rdl/PCA_100004908"/>
    <skos:broadMatch rdf:resource="http://rds.posccaesar.org/ontology/plm/rdl/PCA_100006696"/>
    <rdfs:comment>Provide a simplified overview of connections, lines with sizes and equipment for a sub-system. Basis for piping design.</rdfs:comment>
    <rdl:PCA_100006763>Schematic showing the flow path, line size, equipment and connections for process and utility systems. The schematic shall use standard symbols.</rdl:PCA_100006763>
    <rdl:PCA_100006768>Provide a simplified overview of connections, lines with sizes and equipment for a sub-system. Basis for piping design.</rdl:PCA_100006768>
    <rdfs:label>Flow schematic</rdfs:label>
    <rdl:PCA_100006765 rdf:resource="http://w3id.org/readi/rdl/CFIHOS-20000031"/>
  </owl:Class>
  <owl:Class rdf:about="http://rds.posccaesar.org/ontology/plm/rdl/PCA_100006102">
    <rdfs:label>Balancing report</rdfs:label>
    <rdl:PCA_100006766 rdf:resource="http://rds.posccaesar.org/ontology/plm/rdl/PCA_100006653"/>
    <rdl:PCA_100006763>This document shall support verification of component or system function according to company/project requirements.</rdl:PCA_100006763>
    <rdl:PCA_100006765 rdf:resource="http://w3id.org/readi/rdl/CFIHOS-20000021"/>
    <rdfs:comment>Sufficient information to demonstrate balancing of delivered equipment</rdfs:comment>
    <rdfs:subClassOf rdf:resource="http://rds.posccaesar.org/ontology/plm/rdl/PCA_100004908"/>
    <skos:broadMatch rdf:resource="http://rds.posccaesar.org/ontology/plm/rdl/PCA_100006722"/>
    <rdl:PCA_100006768>Sufficient information to demonstrate balancing of delivered equipment</rdl:PCA_100006768>
    <skos:broader rdf:resource="http://rds.posccaesar.org/ontology/plm/rdl/PCA_100006756"/>
  </owl:Class>
  <owl:Class rdf:about="http://rds.posccaesar.org/ontology/plm/rdl/PCA_100006114">
    <rdl:PCA_100006768>Provides details about out-of-tolerance conditions, special measurement conditions, standard used, date and approvals etc. Each certificate includes a serial number that associates one calibration with one instrument.</rdl:PCA_100006768>
    <rdl:PCA_100006765 rdf:resource="http://w3id.org/readi/rdl/CFIHOS-20000015"/>
    <rdl:PCA_100006763>A document containing data which records compliance with specified requirements.</rdl:PCA_100006763>
    <skos:broader rdf:resource="http://rds.posccaesar.org/ontology/plm/rdl/PCA_100006743"/>
    <rdfs:subClassOf rdf:resource="http://rds.posccaesar.org/ontology/plm/rdl/PCA_100004908"/>
    <skos:broadMatch rdf:resource="http://rds.posccaesar.org/ontology/plm/rdl/PCA_100006722"/>
    <rdfs:comment>Provides details about out-of-tolerance conditions, special measurement conditions, standard used, date and approvals etc. Each certificate includes a serial number that associates one calibration with one instrument.</rdfs:comment>
    <rdfs:label>Calibration certificate</rdfs:label>
    <rdl:PCA_100006766 rdf:resource="http://rds.posccaesar.org/ontology/plm/rdl/PCA_100006653"/>
  </owl:Class>
  <owl:Class rdf:about="http://rds.posccaesar.org/ontology/plm/rdl/PCA_100006126">
    <skos:broadMatch rdf:resource="http://rds.posccaesar.org/ontology/plm/rdl/PCA_100006688"/>
    <rdfs:label>Commissioning instruction</rdfs:label>
    <rdfs:comment>These instructions should contain for example:

 - download program, software instructions according to IEC 61506
 - checking instructions
 - checks to be performed before connection to the supply network and before first operation
 - details of specifications to apply to acceptance, inspection and performance tests.</rdfs:comment>
    <rdl:PCA_100006768>These instructions should contain for example:

 - download program, software instructions according to IEC 61506
 - checking instructions
 - checks to be performed before connection to the supply network and before first operation
 - details of specifications to apply to acceptance, inspection and performance tests.</rdl:PCA_100006768>
    <rdl:PCA_100006766 rdf:resource="http://rds.posccaesar.org/ontology/plm/rdl/PCA_100006653"/>
    <rdl:PCA_100006763>Instruction providing information on the commissioning of the product. Instructions for commissioning are provided especially for large and highly complex products and for large industrial installations. The purpose of such instructions is to provide the user with the information needed for initial setting-up and start-up of the product.</rdl:PCA_100006763>
    <rdfs:subClassOf rdf:resource="http://rds.posccaesar.org/ontology/plm/rdl/PCA_100004908"/>
  </owl:Class>
  <owl:Class rdf:about="http://rds.posccaesar.org/ontology/plm/rdl/PCA_100006138">
    <rdl:PCA_100006768>To detail how crossings will be performed.</rdl:PCA_100006768>
    <rdfs:comment>To detail how crossings will be performed.</rdfs:comment>
    <rdfs:subClassOf rdf:resource="http://rds.posccaesar.org/ontology/plm/rdl/PCA_100004908"/>
    <rdl:PCA_100006765 rdf:resource="http://w3id.org/readi/rdl/CFIHOS-20000031"/>
    <skos:broader rdf:resource="http://rds.posccaesar.org/ontology/plm/rdl/PCA_100006756"/>
    <rdfs:label>Crossing design report</rdfs:label>
    <rdl:PCA_100006766 rdf:resource="http://rds.posccaesar.org/ontology/plm/rdl/PCA_100006653"/>
    <skos:broadMatch rdf:resource="http://rds.posccaesar.org/ontology/plm/rdl/PCA_100006686"/>
    <rdl:PCA_100006763>Report documenting seabed intervention required for separation between crossing pipeline, riser or umbilical and provides input to routing design.</rdl:PCA_100006763>
  </owl:Class>
  <owl:Class rdf:about="http://rds.posccaesar.org/ontology/plm/rdl/PCA_100006459">
    <rdl:PCA_100006766 rdf:resource="http://rds.posccaesar.org/ontology/plm/rdl/PCA_100006643"/>
    <rdl:PCA_100006766 rdf:resource="http://rds.posccaesar.org/ontology/plm/rdl/PCA_100006644"/>
    <skos:broadMatch rdf:resource="http://rds.posccaesar.org/ontology/plm/rdl/PCA_100006698"/>
    <rdl:PCA_100006765 rdf:resource="http://w3id.org/readi/rdl/CFIHOS-20000006"/>
    <rdfs:label>Structural design report</rdfs:label>
    <rdfs:subClassOf rdf:resource="http://rds.posccaesar.org/ontology/plm/rdl/PCA_100004908"/>
    <rdl:PCA_100006768>The structural design report shall have specific and detailed references to drawings and relevant part of regulations and referenced standards.</rdl:PCA_100006768>
    <rdfs:comment>The structural design report shall have specific and detailed references to drawings and relevant part of regulations and referenced standards.</rdfs:comment>
    <rdl:PCA_100006763>Structural design reports and input files/parameters shall be delivered. The report or collection of reports shall be self-contained, i.e. provide all information required to re-produce the results.</rdl:PCA_100006763>
    <skos:broader rdf:resource="http://rds.posccaesar.org/ontology/plm/rdl/PCA_100006756"/>
  </owl:Class>
  <owl:Class rdf:about="http://rds.posccaesar.org/ontology/plm/rdl/PCA_100006338">
    <skos:broader rdf:resource="http://rds.posccaesar.org/ontology/plm/rdl/PCA_100006745"/>
    <skos:broadMatch rdf:resource="http://rds.posccaesar.org/ontology/plm/rdl/PCA_100006708"/>
    <rdfs:label>Nodal diagrams</rdfs:label>
    <rdfs:comment>Isometric non scaled view of routing of cable ladders including penetration transits and jumps shall be provided.  Following information shall typically be included:
 - Node number;
 - Segment name;
 - Length of segment;
 - Location/module number;
 - Cable segregation level;
 - Penetration identification;
 - References to other drawings where the cable ladder continued.</rdfs:comment>
    <rdl:PCA_100006768>Isometric non scaled view of routing of cable ladders including penetration transits and jumps shall be provided.  Following information shall typically be included:
 - Node number;
 - Segment name;
 - Length of segment;
 - Location/module number;
 - Cable segregation level;
 - Penetration identification;
 - References to other drawings where the cable ladder continued.</rdl:PCA_100006768>
    <rdl:PCA_100006766 rdf:resource="http://rds.posccaesar.org/ontology/plm/rdl/PCA_100006656"/>
    <rdl:PCA_100006765 rdf:resource="http://w3id.org/readi/rdl/CFIHOS-20000008"/>
    <rdfs:subClassOf rdf:resource="http://rds.posccaesar.org/ontology/plm/rdl/PCA_100004908"/>
  </owl:Class>
  <owl:Class rdf:about="http://rds.posccaesar.org/ontology/plm/rdl/PCA_100006447">
    <skos:broadMatch rdf:resource="http://rds.posccaesar.org/ontology/plm/rdl/PCA_100006703"/>
    <rdfs:label>Software documentation</rdfs:label>
    <rdfs:comment>It shall cover the system functionality provided by the software applications, and when necessary also provide hardware details in order to identify direct relationship between hardware and software.</rdfs:comment>
    <rdl:PCA_100006768>It shall cover the system functionality provided by the software applications, and when necessary also provide hardware details in order to identify direct relationship between hardware and software.</rdl:PCA_100006768>
    <rdl:PCA_100006766 rdf:resource="http://rds.posccaesar.org/ontology/plm/rdl/PCA_100006653"/>
    <rdl:PCA_100006765 rdf:resource="http://w3id.org/readi/rdl/CFIHOS-20000031"/>
    <rdl:PCA_100006763>Specification that shall provide high level software design information necessary to meet the functional requirements (for a unit or equipment). The specification may include function descriptions, communication protocols, computer system network etc.</rdl:PCA_100006763>
    <rdfs:subClassOf rdf:resource="http://rds.posccaesar.org/ontology/plm/rdl/PCA_100004908"/>
  </owl:Class>
  <owl:Class rdf:about="http://rds.posccaesar.org/ontology/plm/rdl/PCA_100006326">
    <skos:broadMatch rdf:resource="http://rds.posccaesar.org/ontology/plm/rdl/PCA_100006722"/>
    <rdfs:subClassOf rdf:resource="http://rds.posccaesar.org/ontology/plm/rdl/PCA_100004908"/>
    <rdl:PCA_100006768>Model test report shall be delivered.</rdl:PCA_100006768>
    <rdl:PCA_100006763>The report or collection of reports shall document the model test and describe the results of the testing.</rdl:PCA_100006763>
    <skos:broader rdf:resource="http://rds.posccaesar.org/ontology/plm/rdl/PCA_100006756"/>
    <rdl:PCA_100006766 rdf:resource="http://rds.posccaesar.org/ontology/plm/rdl/PCA_100006657"/>
    <rdl:PCA_100006765 rdf:resource="http://w3id.org/readi/rdl/CFIHOS-20000033"/>
    <rdfs:comment>Model test report shall be delivered.</rdfs:comment>
    <rdfs:label>Model test reports</rdfs:label>
  </owl:Class>
  <owl:Class rdf:about="http://rds.posccaesar.org/ontology/plm/rdl/PCA_100006314">
    <rdl:PCA_100006763>This document shall support verification of compliance.</rdl:PCA_100006763>
    <rdl:PCA_100006765 rdf:resource="http://w3id.org/readi/rdl/CFIHOS-20000027"/>
    <rdfs:subClassOf rdf:resource="http://rds.posccaesar.org/ontology/plm/rdl/PCA_100004908"/>
    <skos:broadMatch rdf:resource="http://rds.posccaesar.org/ontology/plm/rdl/PCA_100006722"/>
    <skos:broader rdf:resource="http://rds.posccaesar.org/ontology/plm/rdl/PCA_100006743"/>
    <rdfs:label>Material certificate</rdfs:label>
    <rdl:PCA_100006766 rdf:resource="http://rds.posccaesar.org/ontology/plm/rdl/PCA_100006653"/>
    <rdl:PCA_100006768>This document declares that the material properties for the products supplied are in compliance with the requirements of the purchase order.

For metallic materials, the material certificate shall be delivered according to ISO 10474 / EN 10204.</rdl:PCA_100006768>
    <rdfs:comment>This document declares that the material properties for the products supplied are in compliance with the requirements of the purchase order.

For metallic materials, the material certificate shall be delivered according to ISO 10474 / EN 10204.</rdfs:comment>
  </owl:Class>
  <owl:Class rdf:about="http://rds.posccaesar.org/ontology/plm/rdl/PCA_100006435">
    <skos:broader rdf:resource="http://rds.posccaesar.org/ontology/plm/rdl/PCA_100006756"/>
    <rdfs:label>Seebed intervention report</rdfs:label>
    <rdfs:comment>Report describing the required seabed intervention for the chosen routing.</rdfs:comment>
    <rdl:PCA_100006768>Report describing the required seabed intervention for the chosen routing.</rdl:PCA_100006768>
    <rdl:PCA_100006766 rdf:resource="http://rds.posccaesar.org/ontology/plm/rdl/PCA_100006657"/>
    <rdl:PCA_100006765 rdf:resource="http://w3id.org/readi/rdl/CFIHOS-20000018"/>
    <rdl:PCA_100006763>To provide basis for planning pipeline, riser or umbilical installation. Provide input to analysis and installation procedure.</rdl:PCA_100006763>
    <rdfs:subClassOf rdf:resource="http://rds.posccaesar.org/ontology/plm/rdl/PCA_100004908"/>
  </owl:Class>
  <owl:Class rdf:about="http://rds.posccaesar.org/ontology/plm/rdl/PCA_100006423">
    <skos:broadMatch rdf:resource="http://rds.posccaesar.org/ontology/plm/rdl/PCA_100006722"/>
    <rdfs:subClassOf rdf:resource="http://rds.posccaesar.org/ontology/plm/rdl/PCA_100004908"/>
    <rdl:PCA_100006768>This document shall include SAS communication interface test procedure (UFAT)</rdl:PCA_100006768>
    <rdfs:comment>This document shall include SAS communication interface test procedure (UFAT)</rdfs:comment>
    <skos:broader rdf:resource="http://rds.posccaesar.org/ontology/plm/rdl/PCA_100006751"/>
    <rdfs:label>Safety and automation system (SAS) communication interface test procedure (UFAT)</rdfs:label>
    <rdl:PCA_100006766 rdf:resource="http://rds.posccaesar.org/ontology/plm/rdl/PCA_100006653"/>
    <rdl:PCA_100006765 rdf:resource="http://w3id.org/readi/rdl/CFIHOS-20000027"/>
    <rdl:PCA_100006763>Required by the SAS supplier to configure his communication lines prior to test activities</rdl:PCA_100006763>
  </owl:Class>
  <owl:Class rdf:about="http://rds.posccaesar.org/ontology/plm/rdl/PCA_100006532">
    <rdfs:label>Welders certificate</rdfs:label>
    <skos:broadMatch rdf:resource="http://rds.posccaesar.org/ontology/plm/rdl/PCA_100006722"/>
    <rdfs:subClassOf rdf:resource="http://rds.posccaesar.org/ontology/plm/rdl/PCA_100004908"/>
    <rdl:PCA_100006766 rdf:resource="http://rds.posccaesar.org/ontology/plm/rdl/PCA_100006653"/>
    <rdl:PCA_100006763>Official certificates for welders which records compliance with specified requirements.</rdl:PCA_100006763>
    <rdl:PCA_100006768>This document shall include welder(-s) certificate which shall clearly state that the welder(-s) is approved for the relevant welding process.</rdl:PCA_100006768>
    <rdl:PCA_100006764>Requirements related to assurance and check of quality in manufacturing phase will very much depend on Purchaser’s knowledge of supplier. Well known supplier, with proven track record, delivering products based on industry standards, will typically deliver less verification documentation to Purchaser than unknown/new supplier delivering the same product. Therefore, this deliverable should be evaluated as candidate for being available in digital format to Purchaser, for information only.</rdl:PCA_100006764>
    <rdfs:comment>This document shall include welder(-s) certificate which shall clearly state that the welder(-s) is approved for the relevant welding process.</rdfs:comment>
    <skos:broader rdf:resource="http://rds.posccaesar.org/ontology/plm/rdl/PCA_100006743"/>
  </owl:Class>
  <owl:Class rdf:about="http://rds.posccaesar.org/ontology/plm/rdl/PCA_100006302">
    <skos:broader rdf:resource="http://rds.posccaesar.org/ontology/plm/rdl/PCA_100006748"/>
    <skos:broadMatch rdf:resource="http://rds.posccaesar.org/ontology/plm/rdl/PCA_100006722"/>
    <rdfs:label>Lubrication list</rdfs:label>
    <rdfs:comment>Provides list of chemicals</rdfs:comment>
    <rdl:PCA_100006768>Provides list of chemicals</rdl:PCA_100006768>
    <rdl:PCA_100006766 rdf:resource="http://rds.posccaesar.org/ontology/plm/rdl/PCA_100006653"/>
    <rdl:PCA_100006763>This document shall support verification of compliance</rdl:PCA_100006763>
    <rdfs:subClassOf rdf:resource="http://rds.posccaesar.org/ontology/plm/rdl/PCA_100004908"/>
  </owl:Class>
  <owl:Class rdf:about="http://rds.posccaesar.org/ontology/plm/rdl/PCA_100006411">
    <rdl:PCA_100006768>Outline description and method statement for required actions to repair or abandon a pipeline, riser or umbilical during or after installation.</rdl:PCA_100006768>
    <rdfs:subClassOf rdf:resource="http://rds.posccaesar.org/ontology/plm/rdl/PCA_100004908"/>
    <rdfs:comment>Outline description and method statement for required actions to repair or abandon a pipeline, riser or umbilical during or after installation.</rdfs:comment>
    <rdfs:label>Repair &amp; abandonment procedure</rdfs:label>
    <skos:broader rdf:resource="http://rds.posccaesar.org/ontology/plm/rdl/PCA_100006751"/>
    <rdl:PCA_100006765 rdf:resource="http://w3id.org/readi/rdl/CFIHOS-20000031"/>
    <rdl:PCA_100006766 rdf:resource="http://rds.posccaesar.org/ontology/plm/rdl/PCA_100006657"/>
    <rdl:PCA_100006763>To define the detailed steps required to repair or abandon a pipeline, riser or umbilical.</rdl:PCA_100006763>
    <skos:broadMatch rdf:resource="http://rds.posccaesar.org/ontology/plm/rdl/PCA_100006688"/>
  </owl:Class>
  <owl:Class rdf:about="http://rds.posccaesar.org/ontology/plm/rdl/PCA_100006544">
    <skos:broadMatch rdf:resource="http://rds.posccaesar.org/ontology/plm/rdl/PCA_100006716"/>
    <rdfs:subClassOf rdf:resource="http://rds.posccaesar.org/ontology/plm/rdl/PCA_100004908"/>
    <skos:broader rdf:resource="http://rds.posccaesar.org/ontology/plm/rdl/PCA_100006748"/>
    <rdl:PCA_100006763>Measurements and documentation on risk assessments and risk mitigation in design for the WE Factors; noise, vibrations, chemical and biological exposure, access, ergonomics, outdoor operations, illumination and radiation. The information shall be linked to relevant tag numbers and/or area codes.</rdl:PCA_100006763>
    <rdfs:label>Working environment status</rdfs:label>
    <rdl:PCA_100006766 rdf:resource="http://rds.posccaesar.org/ontology/plm/rdl/PCA_100006654"/>
    <rdl:PCA_100006765 rdf:resource="http://w3id.org/readi/rdl/CFIHOS-20000010"/>
    <rdl:PCA_100006765 rdf:resource="http://w3id.org/readi/rdl/CFIHOS-20000013"/>
    <rdl:PCA_100006765 rdf:resource="http://w3id.org/readi/rdl/CFIHOS-20000011"/>
  </owl:Class>
  <owl:Class rdf:about="http://rds.posccaesar.org/ontology/plm/rdl/PCA_100006520">
    <skos:broadMatch rdf:resource="http://rds.posccaesar.org/ontology/plm/rdl/PCA_100006733"/>
    <rdfs:comment>Drawings of the following are required:
 - Detail / cross sectional drawings (details of manual/bare stem valve/actuator/control panel, etc.)
 - Arrangement drawings of assemblies (assemblies of valve/gearbox/actuator/control panel, etc.)
 Arrangement drawings and detail/cross sectional drawings may be supplied as separate drawings or combined in one drawing. Drawings shall show all components in the same scale. 

Detail/cross sectional drawings shall at least include:
 - VDS reference (Valves)
 - All welds including hard facing and overlaying (Valves)
 - Bore (Valves)
 - Outline dimensions
 - Weight, as built
 - Lifting lugs
 - Parts list including all parts with functional part description and material standard used (real manufacturer’s part number is not required on the drawings). MDS reference to be included when specified in the requirements 
Arrangement drawings of assemblies shall at least include: 
 - Outline dimensions 
 - Material selection for adaptor stool, coupling (connection between valve and actuator shafts), actuator/valve connection bolts and valve stem if modified from specified requirement (including CR reference) 
 - Weight, as built (weights shall be listed separately for valve, actuator, control panel or cabinet and total assembly) 
 - Principles for assembly (maintenance envelopes) 
 - All power and signal connection points with entry details 
For valves not specified according to TR2000 (e.g. control, choke and safety relief valves), real manufacturer's part number shall be included on the valve drawing or a separate BOM.</rdfs:comment>
    <skos:broadMatch rdf:resource="http://rds.posccaesar.org/ontology/plm/rdl/PCA_100006732"/>
    <skos:broadMatch rdf:resource="http://rds.posccaesar.org/ontology/plm/rdl/PCA_100006686"/>
    <skos:broader rdf:resource="http://rds.posccaesar.org/ontology/plm/rdl/PCA_100006746"/>
    <rdl:PCA_100006768>Drawings of the following are required:
 - Detail / cross sectional drawings (details of manual/bare stem valve/actuator/control panel, etc.)
 - Arrangement drawings of assemblies (assemblies of valve/gearbox/actuator/control panel, etc.)
 Arrangement drawings and detail/cross sectional drawings may be supplied as separate drawings or combined in one drawing. Drawings shall show all components in the same scale. 

Detail/cross sectional drawings shall at least include:
 - VDS reference (Valves)
 - All welds including hard facing and overlaying (Valves)
 - Bore (Valves)
 - Outline dimensions
 - Weight, as built
 - Lifting lugs
 - Parts list including all parts with functional part description and material standard used (real manufacturer’s part number is not required on the drawings). MDS reference to be included when specified in the requirements 
Arrangement drawings of assemblies shall at least include: 
 - Outline dimensions 
 - Material selection for adaptor stool, coupling (connection between valve and actuator shafts), actuator/valve connection bolts and valve stem if modified from specified requirement (including CR reference) 
 - Weight, as built (weights shall be listed separately for valve, actuator, control panel or cabinet and total assembly) 
 - Principles for assembly (maintenance envelopes) 
 - All power and signal connection points with entry details 
For valves not specified according to TR2000 (e.g. control, choke and safety relief valves), real manufacturer's part number shall be included on the valve drawing or a separate BOM.</rdl:PCA_100006768>
    <skos:broadMatch rdf:resource="http://rds.posccaesar.org/ontology/plm/rdl/PCA_100006731"/>
    <rdl:PCA_100006765 rdf:resource="http://w3id.org/readi/rdl/CFIHOS-20000022"/>
    <skos:broadMatch rdf:resource="http://rds.posccaesar.org/ontology/plm/rdl/PCA_100006734"/>
    <rdfs:subClassOf rdf:resource="http://rds.posccaesar.org/ontology/plm/rdl/PCA_100004908"/>
    <rdfs:label>Valve and operator drawings</rdfs:label>
  </owl:Class>
  <owl:Class rdf:about="http://rds.posccaesar.org/ontology/plm/rdl/PCA_100006210">
    <skos:broader rdf:resource="http://rds.posccaesar.org/ontology/plm/rdl/PCA_100006756"/>
    <skos:broadMatch rdf:resource="http://rds.posccaesar.org/ontology/plm/rdl/PCA_100006722"/>
    <rdfs:label>Final inspection and test reports</rdfs:label>
    <rdfs:comment>Final inspection reports:

A final inspection program shall be performed for the subsea system prior to delivery to Company. The inspection program shall:
 - Identify status of all equipment upon delivery;
 - Valve status (shut/open);
 - Connection point status (permanent/temporary clamps);
 - Status hatches;
 - Pressure equalization system connection points;
 - Verification of tubular ventilation ports. 

Test reports:
 - All operations to be tested during assembly shall be identified with a test procedure;
 - The individual testing program operations shall be signed out by Contractor. Company shall sign the overall test program upon completion.</rdfs:comment>
    <rdl:PCA_100006768>Final inspection reports:

A final inspection program shall be performed for the subsea system prior to delivery to Company. The inspection program shall:
 - Identify status of all equipment upon delivery;
 - Valve status (shut/open);
 - Connection point status (permanent/temporary clamps);
 - Status hatches;
 - Pressure equalization system connection points;
 - Verification of tubular ventilation ports. 

Test reports:
 - All operations to be tested during assembly shall be identified with a test procedure;
 - The individual testing program operations shall be signed out by Contractor. Company shall sign the overall test program upon completion.</rdl:PCA_100006768>
    <rdl:PCA_100006766 rdf:resource="http://rds.posccaesar.org/ontology/plm/rdl/PCA_100006653"/>
    <rdl:PCA_100006765 rdf:resource="http://w3id.org/readi/rdl/CFIHOS-20000031"/>
    <rdfs:subClassOf rdf:resource="http://rds.posccaesar.org/ontology/plm/rdl/PCA_100004908"/>
  </owl:Class>
  <owl:Class rdf:about="http://rds.posccaesar.org/ontology/plm/rdl/PCA_100006101">
    <rdl:PCA_100006763>To detailed the design and the implementation of the control and monitoring system.</rdl:PCA_100006763>
    <rdfs:comment>Individual Functional Specifications (FS) shall be developed for each process system to be controlled and/or monitored. A separate FS shall be developed for the control system itself.</rdfs:comment>
    <rdl:PCA_100006766 rdf:resource="http://rds.posccaesar.org/ontology/plm/rdl/PCA_100006627"/>
    <rdl:PCA_100006766 rdf:resource="http://rds.posccaesar.org/ontology/plm/rdl/PCA_100006626"/>
    <skos:broader rdf:resource="http://rds.posccaesar.org/ontology/plm/rdl/PCA_100006757"/>
    <rdfs:label>Automation functional specifications</rdfs:label>
    <skos:broadMatch rdf:resource="http://rds.posccaesar.org/ontology/plm/rdl/PCA_100006687"/>
    <rdl:PCA_100006766 rdf:resource="http://rds.posccaesar.org/ontology/plm/rdl/PCA_100006633"/>
    <rdl:PCA_100006765 rdf:resource="http://w3id.org/readi/rdl/CFIHOS-20000015"/>
    <rdl:PCA_100006768>Individual Functional Specifications (FS) shall be developed for each process system to be controlled and/or monitored. A separate FS shall be developed for the control system itself.</rdl:PCA_100006768>
    <rdfs:subClassOf rdf:resource="http://rds.posccaesar.org/ontology/plm/rdl/PCA_100004908"/>
    <rdl:PCA_100006766 rdf:resource="http://rds.posccaesar.org/ontology/plm/rdl/PCA_100006629"/>
    <rdl:PCA_100006766 rdf:resource="http://rds.posccaesar.org/ontology/plm/rdl/PCA_100006628"/>
  </owl:Class>
  <owl:Class rdf:about="http://rds.posccaesar.org/ontology/plm/rdl/PCA_100006222">
    <rdl:PCA_100006766 rdf:resource="http://rds.posccaesar.org/ontology/plm/rdl/PCA_100006657"/>
    <rdfs:label>Flow assurance report</rdfs:label>
    <rdl:PCA_100006763>Document the flow assurance analysis and calculations.</rdl:PCA_100006763>
    <skos:broader rdf:resource="http://rds.posccaesar.org/ontology/plm/rdl/PCA_100006756"/>
    <rdl:PCA_100006768>A report providing the results from erosion analysis, pressure loss calculations, hydrate evaluations and analysis, flow induced vibration calculations and thermal analysis.</rdl:PCA_100006768>
    <rdfs:subClassOf rdf:resource="http://rds.posccaesar.org/ontology/plm/rdl/PCA_100004908"/>
    <skos:broadMatch rdf:resource="http://rds.posccaesar.org/ontology/plm/rdl/PCA_100006696"/>
    <rdfs:comment>A report providing the results from erosion analysis, pressure loss calculations, hydrate evaluations and analysis, flow induced vibration calculations and thermal analysis.</rdfs:comment>
    <rdl:PCA_100006765 rdf:resource="http://w3id.org/readi/rdl/CFIHOS-20000031"/>
  </owl:Class>
  <owl:Class rdf:about="http://rds.posccaesar.org/ontology/plm/rdl/PCA_100006113">
    <skos:broader rdf:resource="http://rds.posccaesar.org/ontology/plm/rdl/PCA_100006741"/>
    <skos:broadMatch rdf:resource="http://rds.posccaesar.org/ontology/plm/rdl/PCA_100006687"/>
    <rdfs:label>Calculations, curves and tables</rdfs:label>
    <rdfs:comment>Lateral analyses and torsion analyses for compressors; performance curves for pumps and compressors. 

Strength calculations, thermal performance and vibration calculations for heat exchangers/pressure vessels.</rdfs:comment>
    <rdl:PCA_100006768>Lateral analyses and torsion analyses for compressors; performance curves for pumps and compressors. 

Strength calculations, thermal performance and vibration calculations for heat exchangers/pressure vessels.</rdl:PCA_100006768>
    <rdl:PCA_100006763>Characteristics and functional parameters shall be documented and performance shall be shown to be probable. This shall include but not be limited to calculations, curves, tables, reference to similar applications and test data. This shall as a minimum be at a level customary for the equipment and to the extent such data are of importance for interfaces to plant and system.</rdl:PCA_100006763>
    <rdfs:subClassOf rdf:resource="http://rds.posccaesar.org/ontology/plm/rdl/PCA_100004908"/>
  </owl:Class>
  <owl:Class rdf:about="http://rds.posccaesar.org/ontology/plm/rdl/PCA_100006125">
    <skos:broader rdf:resource="http://rds.posccaesar.org/ontology/plm/rdl/PCA_100006743"/>
    <rdl:PCA_100006763>Certificate to confirm compliance with contract / purchase order with reference to standards, technical specifications and requirements for the product.</rdl:PCA_100006763>
    <rdl:PCA_100006765 rdf:resource="http://w3id.org/readi/rdl/CFIHOS-20000031"/>
    <rdfs:label>COC - certificate of conformance</rdfs:label>
    <rdl:PCA_100006766 rdf:resource="http://rds.posccaesar.org/ontology/plm/rdl/PCA_100006653"/>
    <rdfs:subClassOf rdf:resource="http://rds.posccaesar.org/ontology/plm/rdl/PCA_100004908"/>
    <rdfs:comment>The manufacture’s or other party’s confirmation that the product is designed, manufactured and tested as specified.</rdfs:comment>
    <rdl:PCA_100006768>The manufacture’s or other party’s confirmation that the product is designed, manufactured and tested as specified.</rdl:PCA_100006768>
    <skos:broadMatch rdf:resource="http://rds.posccaesar.org/ontology/plm/rdl/PCA_100006724"/>
  </owl:Class>
  <owl:Class rdf:about="http://rds.posccaesar.org/ontology/plm/rdl/PCA_100006137">
    <rdfs:label>Critical line list</rdfs:label>
    <rdl:PCA_100006765 rdf:resource="http://w3id.org/readi/rdl/CFIHOS-20000020"/>
    <rdl:PCA_100006766 rdf:resource="http://rds.posccaesar.org/ontology/plm/rdl/PCA_100006654"/>
    <skos:broadMatch rdf:resource="http://rds.posccaesar.org/ontology/plm/rdl/PCA_100006716"/>
    <skos:broader rdf:resource="http://rds.posccaesar.org/ontology/plm/rdl/PCA_100006748"/>
    <rdl:PCA_100006768>The stress critical lines shall be listed in the document. The list shall include:
 - Line number;
 - Stress ISO document number (typically referenced on piping ISOs/support drawings);
 - Pipe size;
 - Pipe class;
 - Service;
 - Max design temp;
 - Min design temp;
 - Design pressure;
 - PED category (applicable for installations that require conformity with Pressure Equipment Directive);
 - P&amp;ID document number;
 - Pipe stress report document number;
 - Piping stress isometric drawing number;</rdl:PCA_100006768>
    <rdfs:comment>The stress critical lines shall be listed in the document. The list shall include:
 - Line number;
 - Stress ISO document number (typically referenced on piping ISOs/support drawings);
 - Pipe size;
 - Pipe class;
 - Service;
 - Max design temp;
 - Min design temp;
 - Design pressure;
 - PED category (applicable for installations that require conformity with Pressure Equipment Directive);
 - P&amp;ID document number;
 - Pipe stress report document number;
 - Piping stress isometric drawing number;</rdfs:comment>
    <skos:broadMatch rdf:resource="http://rds.posccaesar.org/ontology/plm/rdl/PCA_100006717"/>
    <rdfs:subClassOf rdf:resource="http://rds.posccaesar.org/ontology/plm/rdl/PCA_100004908"/>
  </owl:Class>
  <owl:Class rdf:about="http://rds.posccaesar.org/ontology/plm/rdl/PCA_100006149">
    <skos:broader rdf:resource="http://rds.posccaesar.org/ontology/plm/rdl/PCA_100006756"/>
    <skos:broadMatch rdf:resource="http://rds.posccaesar.org/ontology/plm/rdl/PCA_100006724"/>
    <rdfs:label>Declaration of conformity</rdfs:label>
    <rdfs:comment>The declaration of conformity shall be written up by the manufacturer of the equipment or component, as the legal binding document from the manufacturer / vendor to the purchaser / user ensuring conformity with the relevant EU directive( s). 

Local language: YES for lifting appliances</rdfs:comment>
    <rdl:PCA_100006768>The declaration of conformity shall be written up by the manufacturer of the equipment or component, as the legal binding document from the manufacturer / vendor to the purchaser / user ensuring conformity with the relevant EU directive( s). 

Local language: YES for lifting appliances</rdl:PCA_100006768>
    <rdl:PCA_100006765 rdf:resource="http://w3id.org/readi/rdl/CFIHOS-20000027"/>
    <rdl:PCA_100006763>Shall be provided for equipment and / or assemblies covered by EU Directives, delivered to projects within the EEA, according to requirements of the relevant EU - directives wrt conformity assessment procedures and eventual necessary involvements of Notified Bodies i.e for EU type examinations thereto , e.g.: EU Directive: 2006/42/EC Machinery Directive EU Directive: 2004/22/EC (MID) Measuring Instruments EU Directive: 2014/68/EU (PED) Pressure Equipment Directive EU Directive: 2014/34/EU (ATEX) Product Directive, EU Directive: 2014/30/EU (EMC) Electromagnetic Compatibility EU Directive: 89/686/EEC (PPE) Personal Protective Equipment EU Regulation: No 1272/2008 (CLP) on classification, labelling and packaging of substances and mixtures, amending and repealing Directives 67/548/EEC and 1999/45/EC, and amending Regulation (EC) No 1907/2006 LVD (2014/35-EU) The guidance of relevant directive shall be considered by the manufacturer when compiling the DoC.</rdl:PCA_100006763>
    <rdfs:subClassOf rdf:resource="http://rds.posccaesar.org/ontology/plm/rdl/PCA_100004908"/>
  </owl:Class>
  <owl:Class rdf:about="http://rds.posccaesar.org/ontology/plm/rdl/PCA_100006258">
    <skos:broader rdf:resource="http://rds.posccaesar.org/ontology/plm/rdl/PCA_100006746"/>
    <skos:broadMatch rdf:resource="http://rds.posccaesar.org/ontology/plm/rdl/PCA_100006709"/>
    <rdfs:label>HVAC layout drawings</rdfs:label>
    <rdfs:comment>HVAC Layout drawings shall include: 
 - Duct size
 - Duct location
 - HVAC Bulk item(s) (numbered according to ENS)
 - Tagged equipment
 - Ductwork and insulation classification
 - Penetrations
 - Inspection hatches, ladders, etc
 - Measuring points for system balancing
 - Relevant instruments
 - Service areas for HVAC equipment
 - Walls and grid lines</rdfs:comment>
    <rdl:PCA_100006768>HVAC Layout drawings shall include: 
 - Duct size
 - Duct location
 - HVAC Bulk item(s) (numbered according to ENS)
 - Tagged equipment
 - Ductwork and insulation classification
 - Penetrations
 - Inspection hatches, ladders, etc
 - Measuring points for system balancing
 - Relevant instruments
 - Service areas for HVAC equipment
 - Walls and grid lines</rdl:PCA_100006768>
    <rdl:PCA_100006765 rdf:resource="http://w3id.org/readi/rdl/CFIHOS-20000019"/>
    <rdfs:subClassOf rdf:resource="http://rds.posccaesar.org/ontology/plm/rdl/PCA_100004908"/>
  </owl:Class>
  <owl:Class rdf:about="http://rds.posccaesar.org/ontology/plm/rdl/PCA_100006379">
    <skos:broader rdf:resource="http://rds.posccaesar.org/ontology/plm/rdl/PCA_100006756"/>
    <skos:broadMatch rdf:resource="http://rds.posccaesar.org/ontology/plm/rdl/PCA_100006687"/>
    <rdfs:label>Piping stress report</rdfs:label>
    <rdl:PCA_100006766 rdf:resource="http://rds.posccaesar.org/ontology/plm/rdl/PCA_100006653"/>
    <rdl:PCA_100006765 rdf:resource="http://w3id.org/readi/rdl/CFIHOS-20000020"/>
    <rdl:PCA_100006763>The Piping Stress Report shall document that the critical lines meet the code, authority requirements and project requirements. Piping stress calculations shall be provided for all critical piping. The piping stress report shall include reference to the Piping Stress Isometric drawings.</rdl:PCA_100006763>
    <rdfs:subClassOf rdf:resource="http://rds.posccaesar.org/ontology/plm/rdl/PCA_100004908"/>
  </owl:Class>
  <owl:Class rdf:about="http://rds.posccaesar.org/ontology/plm/rdl/PCA_100006367">
    <rdfs:comment>Pipe tracking data shall be in accordance with Company’s requirements.</rdfs:comment>
    <rdl:PCA_100006766 rdf:resource="http://rds.posccaesar.org/ontology/plm/rdl/PCA_100006653"/>
    <skos:broadMatch rdf:resource="http://rds.posccaesar.org/ontology/plm/rdl/PCA_100006722"/>
    <skos:broader rdf:resource="http://rds.posccaesar.org/ontology/plm/rdl/PCA_100006762"/>
    <rdfs:label>Pipe tracking data</rdfs:label>
    <skos:broader rdf:resource="http://rds.posccaesar.org/ontology/plm/rdl/PCA_100006756"/>
    <rdfs:subClassOf rdf:resource="http://rds.posccaesar.org/ontology/plm/rdl/PCA_100004908"/>
    <rdl:PCA_100006768>Pipe tracking data shall be in accordance with Company’s requirements.</rdl:PCA_100006768>
    <rdl:PCA_100006765 rdf:resource="http://w3id.org/readi/rdl/CFIHOS-20000020"/>
    <rdl:PCA_100006765 rdf:resource="http://w3id.org/readi/rdl/CFIHOS-20000031"/>
    <rdl:PCA_100006763>DNV-OS-F101 Submarine Pipeline Systems, states  “a system for ensuring correct traceability to the material shall be established”</rdl:PCA_100006763>
  </owl:Class>
  <owl:Class rdf:about="http://rds.posccaesar.org/ontology/plm/rdl/PCA_100006246">
    <skos:broader rdf:resource="http://rds.posccaesar.org/ontology/plm/rdl/PCA_100006756"/>
    <rdl:PCA_100006766 rdf:resource="http://rds.posccaesar.org/ontology/plm/rdl/PCA_100006657"/>
    <rdl:PCA_100006768>A report summarizing the results from a systematic review of the system or operation with respect to operational hazards after the system is installed.</rdl:PCA_100006768>
    <rdfs:label>Hazid / hazop report</rdfs:label>
    <rdl:PCA_100006763>Identify, evaluate, control or correct the operational hazards in the system or operation. The HAZOP/HAZID is input to the design.</rdl:PCA_100006763>
    <rdfs:subClassOf rdf:resource="http://rds.posccaesar.org/ontology/plm/rdl/PCA_100004908"/>
    <rdfs:comment>A report summarizing the results from a systematic review of the system or operation with respect to operational hazards after the system is installed.</rdfs:comment>
    <skos:broadMatch rdf:resource="http://rds.posccaesar.org/ontology/plm/rdl/PCA_100006726"/>
    <rdl:PCA_100006765 rdf:resource="http://w3id.org/readi/rdl/CFIHOS-20000031"/>
  </owl:Class>
  <owl:Class rdf:about="http://rds.posccaesar.org/ontology/plm/rdl/PCA_100006488">
    <rdfs:label>Technical tag hierarchy (TTH)</rdfs:label>
    <rdl:PCA_100006766 rdf:resource="http://rds.posccaesar.org/ontology/plm/rdl/PCA_100006653"/>
    <rdl:PCA_100006765 rdf:resource="http://w3id.org/readi/rdl/CFIHOS-20000001"/>
    <rdl:PCA_100006763>A technical tag hierarchy shall be established according to Company’s requirements.

The technical hierarchy describes the technical structure of the installation.  The hierarchy provides an overview of equipment units that belong together technically, and shows the relationship between main equipment, instruments, valves and other related equipment.</rdl:PCA_100006763>
    <rdfs:subClassOf rdf:resource="http://rds.posccaesar.org/ontology/plm/rdl/PCA_100004908"/>
  </owl:Class>
  <owl:Class rdf:about="http://rds.posccaesar.org/ontology/plm/rdl/PCA_100006234">
    <skos:broader rdf:resource="http://rds.posccaesar.org/ontology/plm/rdl/PCA_100006739"/>
    <skos:broadMatch rdf:resource="http://rds.posccaesar.org/ontology/plm/rdl/PCA_100006708"/>
    <rdfs:label>General arrangement drawing - Anchoring structures and wall penetrations</rdfs:label>
    <rdfs:comment>Drawings of anchoring structures and wall penetrations shall cover materials, geometry, dimensions, position of pipeline in anchoring structure, minimum separation between pipeline and possible reinforcement and rockbolts, pipeline coating inside anchoring structure in addition to sealing and centring details for penetrations (such as concrete pits and –walls).</rdfs:comment>
    <rdl:PCA_100006768>Drawings of anchoring structures and wall penetrations shall cover materials, geometry, dimensions, position of pipeline in anchoring structure, minimum separation between pipeline and possible reinforcement and rockbolts, pipeline coating inside anchoring structure in addition to sealing and centring details for penetrations (such as concrete pits and –walls).</rdl:PCA_100006768>
    <rdl:PCA_100006766 rdf:resource="http://rds.posccaesar.org/ontology/plm/rdl/PCA_100006654"/>
    <rdl:PCA_100006765 rdf:resource="http://w3id.org/readi/rdl/CFIHOS-20000018"/>
    <rdfs:subClassOf rdf:resource="http://rds.posccaesar.org/ontology/plm/rdl/PCA_100004908"/>
  </owl:Class>
  <owl:Class rdf:about="http://rds.posccaesar.org/ontology/plm/rdl/PCA_100006476">
    <rdfs:label>Supplier SIL documentation</rdfs:label>
    <rdfs:comment>The supplier SIL documentation shall be delivered if the component or system/assembly is part of realizing a safety instrumented function specified in the Safety Requirement Specification (SRS) with SIL requirement.Content requirement for the supplier SIL documentation are given in appendix E3 in NOROG - 070. 

Supplier SIL documentation may be delivered under various forms:
 - as single document called Safety Manual, 
 - as several documents incl. e.g. a IEC61508 certificate and a Safety Manual 
 - or as part of another document.</rdfs:comment>
    <rdl:PCA_100006768>The supplier SIL documentation shall be delivered if the component or system/assembly is part of realizing a safety instrumented function specified in the Safety Requirement Specification (SRS) with SIL requirement.Content requirement for the supplier SIL documentation are given in appendix E3 in NOROG - 070. 

Supplier SIL documentation may be delivered under various forms:
 - as single document called Safety Manual, 
 - as several documents incl. e.g. a IEC61508 certificate and a Safety Manual 
 - or as part of another document.</rdl:PCA_100006768>
    <rdl:PCA_100006766 rdf:resource="http://rds.posccaesar.org/ontology/plm/rdl/PCA_100006653"/>
    <rdl:PCA_100006763>The supplier SIL documentation addresses the safety manual delivery as intended in IEC 61511 and 61508. It provides the necessary information about how to safely apply a component or assembly/system and integrate it into a complete SIS. It addresses design, operation, maintenance, failure rates and other reliability data, fault detection and constraints associated with the component or assembly/system for the intended configurations and operating environment.</rdl:PCA_100006763>
    <rdfs:subClassOf rdf:resource="http://rds.posccaesar.org/ontology/plm/rdl/PCA_100004908"/>
  </owl:Class>
  <owl:Class rdf:about="http://rds.posccaesar.org/ontology/plm/rdl/PCA_100006355">
    <skos:broader rdf:resource="http://rds.posccaesar.org/ontology/plm/rdl/PCA_100006748"/>
    <skos:broadMatch rdf:resource="http://rds.posccaesar.org/ontology/plm/rdl/PCA_100006716"/>
    <rdfs:label>PAGA amplifier load list</rdfs:label>
    <rdfs:comment>Load list for PAGA amplifiers.</rdfs:comment>
    <rdl:PCA_100006768>Load list for PAGA amplifiers.</rdl:PCA_100006768>
    <rdl:PCA_100006766 rdf:resource="http://rds.posccaesar.org/ontology/plm/rdl/PCA_100006640"/>
    <rdl:PCA_100006765 rdf:resource="http://w3id.org/readi/rdl/CFIHOS-20000030"/>
    <rdfs:subClassOf rdf:resource="http://rds.posccaesar.org/ontology/plm/rdl/PCA_100004908"/>
  </owl:Class>
  <owl:Class rdf:about="http://rds.posccaesar.org/ontology/plm/rdl/PCA_100006343">
    <rdl:PCA_100006765>
      <rdl:PCA_100001503 rdf:about="http://w3id.org/readi/rdl/CFIHOS-20000028">
        <rdfs:label>materials engineering</rdfs:label>
        <rdl:PCA_100004924>RA</rdl:PCA_100004924>
        <rdf:type rdf:resource="http://www.w3.org/2002/07/owl#NamedIndividual"/>
      </rdl:PCA_100001503>
    </rdl:PCA_100006765>
    <rdfs:label>Non-destructive examination (NDE) report</rdfs:label>
    <rdl:PCA_100006763>A document containing data which records compliance with specified procedure.</rdl:PCA_100006763>
    <skos:broadMatch rdf:resource="http://rds.posccaesar.org/ontology/plm/rdl/PCA_100006722"/>
    <rdl:PCA_100006768>Documents containing records of performed NDT (in typical NDT methods e.g. MT, PT, RT, UT, ET and VT).</rdl:PCA_100006768>
    <rdl:PCA_100006766 rdf:resource="http://rds.posccaesar.org/ontology/plm/rdl/PCA_100006653"/>
    <rdfs:comment>Documents containing records of performed NDT (in typical NDT methods e.g. MT, PT, RT, UT, ET and VT).</rdfs:comment>
    <rdfs:subClassOf rdf:resource="http://rds.posccaesar.org/ontology/plm/rdl/PCA_100004908"/>
    <skos:broader rdf:resource="http://rds.posccaesar.org/ontology/plm/rdl/PCA_100006756"/>
  </owl:Class>
  <owl:Class rdf:about="http://rds.posccaesar.org/ontology/plm/rdl/PCA_100006464">
    <skos:broader rdf:resource="http://rds.posccaesar.org/ontology/plm/rdl/PCA_100006756"/>
    <skos:broadMatch rdf:resource="http://rds.posccaesar.org/ontology/plm/rdl/PCA_100006698"/>
    <rdfs:label>Structural steel and aluminium structural design report (civil)</rdfs:label>
    <rdfs:comment>Structural design reports and input files/parameters shall be delivered. The report or collection of reports shall be self-contained, i.e. provide all information required to re-produce the results.

The static analysis and calculations shall have specific and detailed references to drawings and relevant part of regulations and referenced standards.</rdfs:comment>
    <rdl:PCA_100006768>Structural design reports and input files/parameters shall be delivered. The report or collection of reports shall be self-contained, i.e. provide all information required to re-produce the results.

The static analysis and calculations shall have specific and detailed references to drawings and relevant part of regulations and referenced standards.</rdl:PCA_100006768>
    <rdl:PCA_100006766 rdf:resource="http://rds.posccaesar.org/ontology/plm/rdl/PCA_100006643"/>
    <rdl:PCA_100006765 rdf:resource="http://w3id.org/readi/rdl/CFIHOS-20000007"/>
    <rdfs:subClassOf rdf:resource="http://rds.posccaesar.org/ontology/plm/rdl/PCA_100004908"/>
  </owl:Class>
  <owl:Class rdf:about="http://rds.posccaesar.org/ontology/plm/rdl/PCA_100006452">
    <skos:broader>
      <rdl:PCA_100001503 rdf:about="http://rds.posccaesar.org/ontology/plm/rdl/PCA_100006760">
        <rdfs:label>Spare-/Part list</rdfs:label>
        <rdl:PCA_100004924>SP</rdl:PCA_100004924>
        <rdf:type rdf:resource="http://www.w3.org/2002/07/owl#NamedIndividual"/>
      </rdl:PCA_100001503>
    </skos:broader>
    <skos:broadMatch rdf:resource="http://rds.posccaesar.org/ontology/plm/rdl/PCA_100006716"/>
    <rdfs:label>Spare part list</rdfs:label>
    <rdfs:comment>Mandatory content of information:
 - Item reference number
 - Quantity
 - Part number or global identifier (together with manufacturer / supplier)
 - Part name.

Optional content of information:
 - Type designation
 - Specifying technical data
 - Descriptive technical data
 - Mass, dimensions
 - Reference to document
 - Remark.</rdfs:comment>
    <rdl:PCA_100006768>Mandatory content of information:
 - Item reference number
 - Quantity
 - Part number or global identifier (together with manufacturer / supplier)
 - Part name.

Optional content of information:
 - Type designation
 - Specifying technical data
 - Descriptive technical data
 - Mass, dimensions
 - Reference to document
 - Remark.</rdl:PCA_100006768>
    <rdl:PCA_100006766 rdf:resource="http://rds.posccaesar.org/ontology/plm/rdl/PCA_100006653"/>
    <rdl:PCA_100006763>Table containing list of items specifying the objects (parts, components, software, equipment, etc.) that are available or delivered as spare parts for later use.</rdl:PCA_100006763>
    <rdfs:subClassOf rdf:resource="http://rds.posccaesar.org/ontology/plm/rdl/PCA_100004908"/>
  </owl:Class>
  <owl:Class rdf:about="http://rds.posccaesar.org/ontology/plm/rdl/PCA_100006331">
    <skos:broader rdf:resource="http://rds.posccaesar.org/ontology/plm/rdl/PCA_100006751"/>
    <skos:broadMatch rdf:resource="http://rds.posccaesar.org/ontology/plm/rdl/PCA_100006688"/>
    <rdfs:label>Mooring system procedures</rdfs:label>
    <rdfs:comment>Mooring systems procedures shall be delivered. The report or collection of reports shall contain all procedures necessary to safely operate, maintain and replace any component of the mooring system.</rdfs:comment>
    <rdl:PCA_100006768>Mooring systems procedures shall be delivered. The report or collection of reports shall contain all procedures necessary to safely operate, maintain and replace any component of the mooring system.</rdl:PCA_100006768>
    <rdl:PCA_100006766 rdf:resource="http://rds.posccaesar.org/ontology/plm/rdl/PCA_100006647"/>
    <rdl:PCA_100006765 rdf:resource="http://w3id.org/readi/rdl/CFIHOS-20000033"/>
    <rdfs:subClassOf rdf:resource="http://rds.posccaesar.org/ontology/plm/rdl/PCA_100004908"/>
  </owl:Class>
  <owl:Class rdf:about="http://rds.posccaesar.org/ontology/plm/rdl/PCA_100006440">
    <rdl:PCA_100006766 rdf:resource="http://rds.posccaesar.org/ontology/plm/rdl/PCA_100006639"/>
    <skos:broader rdf:resource="http://rds.posccaesar.org/ontology/plm/rdl/PCA_100006748"/>
    <rdl:PCA_100006765 rdf:resource="http://w3id.org/readi/rdl/CFIHOS-20000008"/>
    <skos:broadMatch rdf:resource="http://rds.posccaesar.org/ontology/plm/rdl/PCA_100006716"/>
    <rdl:PCA_100006766 rdf:resource="http://rds.posccaesar.org/ontology/plm/rdl/PCA_100006638"/>
    <rdl:PCA_100006766 rdf:resource="http://rds.posccaesar.org/ontology/plm/rdl/PCA_100006637"/>
    <rdl:PCA_100006768>The following information shall be included:
 - Switchboard or distribution board tag number;
 - Bus id;
 - Circuit id/feeder id;
 - Circuit type;
 - Consumer tag number;
 - Fuse/breaker type and size;
 - Type of consumer;
 - Spare circuits to be registered as such (type: Spare);
 - Description of circuit/feeder. Shall include location / address of consumer as relevant;
 - Cable number;
 - Termination details (including phase) - only for small power distribution;
 - Power and current rating according to datasheets.</rdl:PCA_100006768>
    <rdl:PCA_100006766 rdf:resource="http://rds.posccaesar.org/ontology/plm/rdl/PCA_100006636"/>
    <rdfs:label>Single line index</rdfs:label>
    <rdl:PCA_100006766 rdf:resource="http://rds.posccaesar.org/ontology/plm/rdl/PCA_100006635"/>
    <rdl:PCA_100006766 rdf:resource="http://rds.posccaesar.org/ontology/plm/rdl/PCA_100006634"/>
    <skos:broadMatch rdf:resource="http://rds.posccaesar.org/ontology/plm/rdl/PCA_100006702"/>
    <rdfs:subClassOf rdf:resource="http://rds.posccaesar.org/ontology/plm/rdl/PCA_100004908"/>
    <rdfs:comment>The following information shall be included:
 - Switchboard or distribution board tag number;
 - Bus id;
 - Circuit id/feeder id;
 - Circuit type;
 - Consumer tag number;
 - Fuse/breaker type and size;
 - Type of consumer;
 - Spare circuits to be registered as such (type: Spare);
 - Description of circuit/feeder. Shall include location / address of consumer as relevant;
 - Cable number;
 - Termination details (including phase) - only for small power distribution;
 - Power and current rating according to datasheets.</rdfs:comment>
    <rdl:PCA_100006763>The single line index shall cover all voltage levels including "no break" system (UPS), instrumentation and telecommunication. The index shall include all necessary information to enable the complete tracing of power distribution network, up/down and between main distribution boards to the consumer, including transformers, UPS, Central telecom equipment and instrument panels/cabinets/controls.

This shall include sub-distribution boards and junction boxes.</rdl:PCA_100006763>
  </owl:Class>
  <owl:Class rdf:about="http://rds.posccaesar.org/ontology/plm/rdl/PCA_100006205">
    <skos:broader rdf:resource="http://rds.posccaesar.org/ontology/plm/rdl/PCA_100006756"/>
    <skos:broadMatch rdf:resource="http://rds.posccaesar.org/ontology/plm/rdl/PCA_100006722"/>
    <rdfs:label>Fibre optical cabling (platform / facility internal) test reports</rdfs:label>
    <rdl:PCA_100006766 rdf:resource="http://rds.posccaesar.org/ontology/plm/rdl/PCA_100006653"/>
    <rdl:PCA_100006765 rdf:resource="http://w3id.org/readi/rdl/CFIHOS-20000030"/>
    <rdl:PCA_100006764>Test reports for fibre optical cables (platform/facility internal) shall be provided. Test per fibre.</rdl:PCA_100006764>
    <rdfs:subClassOf rdf:resource="http://rds.posccaesar.org/ontology/plm/rdl/PCA_100004908"/>
  </owl:Class>
  <owl:Class rdf:about="http://rds.posccaesar.org/ontology/plm/rdl/PCA_100006217">
    <skos:broadMatch rdf:resource="http://rds.posccaesar.org/ontology/plm/rdl/PCA_100006687"/>
    <rdl:PCA_100006764>Such as, but not limited to:
 - Flow meters;
 - Prover sizing;
 - Mixing in accordance with ISO 3171;
 - Fast loops (pressure drop, flow rates required for isokinetic sampling;
 - Time lag for analyser system;
 - Dew point calculation for the sampling handling system;
 - Installation effects which may affect flowmeter performance such as:
     - noise;
     - low profile.
 - Pressure drop.</rdl:PCA_100006764>
    <rdl:PCA_100006765 rdf:resource="http://w3id.org/readi/rdl/CFIHOS-20000015"/>
    <rdl:PCA_100006766 rdf:resource="http://rds.posccaesar.org/ontology/plm/rdl/PCA_100006591"/>
    <rdl:PCA_100006763>All calculations needed for sizing and selection of metering equipment shall be documented.</rdl:PCA_100006763>
    <skos:broader rdf:resource="http://rds.posccaesar.org/ontology/plm/rdl/PCA_100006741"/>
    <rdl:PCA_100006766 rdf:resource="http://rds.posccaesar.org/ontology/plm/rdl/PCA_100006587"/>
    <rdfs:label>Fiscal metering - Design calculations</rdfs:label>
    <rdfs:subClassOf rdf:resource="http://rds.posccaesar.org/ontology/plm/rdl/PCA_100004908"/>
  </owl:Class>
  <owl:Class rdf:about="http://rds.posccaesar.org/ontology/plm/rdl/PCA_100006108">
    <rdfs:subClassOf rdf:resource="http://rds.posccaesar.org/ontology/plm/rdl/PCA_100004908"/>
    <rdl:PCA_100006768>This calculation documents that the combined unit has sufficient strength for the explosion loads specified</rdl:PCA_100006768>
    <skos:broadMatch rdf:resource="http://rds.posccaesar.org/ontology/plm/rdl/PCA_100006687"/>
    <rdl:PCA_100006763>This document shall support verification of component function according to company/project requirements.

This document gives an input to DAL</rdl:PCA_100006763>
    <rdfs:label>Blast load calculation</rdfs:label>
    <rdl:PCA_100006766 rdf:resource="http://rds.posccaesar.org/ontology/plm/rdl/PCA_100006653"/>
    <rdfs:comment>This calculation documents that the combined unit has sufficient strength for the explosion loads specified</rdfs:comment>
    <rdl:PCA_100006765 rdf:resource="http://w3id.org/readi/rdl/CFIHOS-20000013"/>
    <skos:broader rdf:resource="http://rds.posccaesar.org/ontology/plm/rdl/PCA_100006741"/>
  </owl:Class>
  <owl:Class rdf:about="http://rds.posccaesar.org/ontology/plm/rdl/PCA_100006229">
    <rdl:PCA_100006765 rdf:resource="http://w3id.org/readi/rdl/CFIHOS-20000033"/>
    <rdfs:comment>The plan shall include the following information:
 - deepest draught for the vessel;
 - arrangement plan to show openings and closing appliances with the purpose of retaining the vessel's external watertight integrity, e.g.:
   - external doors;
   - cargo hatches service hatches;
   - side scuttles and windows;
   - sanitary discharges and garbage chutes;
   - freeing ports and scuppers;
   - sea water inlet and discharge valves;
   - air pipes including vent heads;
   - ventilators including closing appliances;
 - arrangement plan showing equipment for protection of the crew, e.g.:
   - gangways, passageways, under deck passages and lifelines;
   - guard rails and bulwarks.</rdfs:comment>
    <rdl:PCA_100006768>The plan shall include the following information:
 - deepest draught for the vessel;
 - arrangement plan to show openings and closing appliances with the purpose of retaining the vessel's external watertight integrity, e.g.:
   - external doors;
   - cargo hatches service hatches;
   - side scuttles and windows;
   - sanitary discharges and garbage chutes;
   - freeing ports and scuppers;
   - sea water inlet and discharge valves;
   - air pipes including vent heads;
   - ventilators including closing appliances;
 - arrangement plan showing equipment for protection of the crew, e.g.:
   - gangways, passageways, under deck passages and lifelines;
   - guard rails and bulwarks.</rdl:PCA_100006768>
    <rdl:PCA_100006763>To document compliance with the PSA facilities regulations § 62 and NMA Regulations No. 878 in addition to IMO instruments and Class requirements, as applicable.</rdl:PCA_100006763>
    <rdl:PCA_100006766 rdf:resource="http://rds.posccaesar.org/ontology/plm/rdl/PCA_100006657"/>
    <skos:broadMatch rdf:resource="http://rds.posccaesar.org/ontology/plm/rdl/PCA_100006707"/>
    <rdfs:label>Freeboard plan</rdfs:label>
    <skos:broader rdf:resource="http://rds.posccaesar.org/ontology/plm/rdl/PCA_100006753"/>
    <rdfs:subClassOf rdf:resource="http://rds.posccaesar.org/ontology/plm/rdl/PCA_100004908"/>
  </owl:Class>
  <owl:Class rdf:about="http://rds.posccaesar.org/ontology/plm/rdl/PCA_100006259">
    <skos:broadMatch rdf:resource="http://rds.posccaesar.org/ontology/plm/rdl/PCA_100006698"/>
    <rdl:PCA_100006768>The HVAC system description shall as a minimum include: 
 - System split-up;
 - System description;
 - Sparing;
 - Equipment description;
 - Utilities for HVAC/interface with other systems;
 - System interlock;
 - Pressurization;
 - Fire damper installation (LRA &amp; HRA);
 - Smoke ventilation;
 - Air inlets/outlets;
 - Black Start;
 - Ductwork;
 - Local cooling/heating;
 - Heating/cooling control;
 - Start/stop sequence;
 - Shut down;
 - Gas/fire/smoke control;
 - Operational modes;
 - Central control system;
 - Local control/indicators.</rdl:PCA_100006768>
    <skos:broader>
      <rdl:PCA_100001503 rdf:about="http://rds.posccaesar.org/ontology/plm/rdl/PCA_100006754">
        <rdfs:label>Process</rdfs:label>
        <rdl:PCA_100004924>PS</rdl:PCA_100004924>
        <rdf:type rdf:resource="http://www.w3.org/2002/07/owl#NamedIndividual"/>
      </rdl:PCA_100001503>
    </skos:broader>
    <rdl:PCA_100006765 rdf:resource="http://w3id.org/readi/rdl/CFIHOS-20000019"/>
    <rdfs:subClassOf rdf:resource="http://rds.posccaesar.org/ontology/plm/rdl/PCA_100004908"/>
    <skos:broadMatch rdf:resource="http://rds.posccaesar.org/ontology/plm/rdl/PCA_100006695"/>
    <rdl:PCA_100006766 rdf:resource="http://rds.posccaesar.org/ontology/plm/rdl/PCA_100006650"/>
    <rdfs:label>HVAC system description</rdfs:label>
    <skos:broader rdf:resource="http://rds.posccaesar.org/ontology/plm/rdl/PCA_100006756"/>
    <rdfs:comment>The HVAC system description shall as a minimum include: 
 - System split-up;
 - System description;
 - Sparing;
 - Equipment description;
 - Utilities for HVAC/interface with other systems;
 - System interlock;
 - Pressurization;
 - Fire damper installation (LRA &amp; HRA);
 - Smoke ventilation;
 - Air inlets/outlets;
 - Black Start;
 - Ductwork;
 - Local cooling/heating;
 - Heating/cooling control;
 - Start/stop sequence;
 - Shut down;
 - Gas/fire/smoke control;
 - Operational modes;
 - Central control system;
 - Local control/indicators.</rdfs:comment>
  </owl:Class>
  <owl:Class rdf:about="http://rds.posccaesar.org/ontology/plm/rdl/PCA_100006247">
    <rdfs:subClassOf rdf:resource="http://rds.posccaesar.org/ontology/plm/rdl/PCA_100004908"/>
    <skos:broader rdf:resource="http://rds.posccaesar.org/ontology/plm/rdl/PCA_100006740"/>
    <rdl:PCA_100006766 rdf:resource="http://rds.posccaesar.org/ontology/plm/rdl/PCA_100006636"/>
    <rdl:PCA_100006765 rdf:resource="http://w3id.org/readi/rdl/CFIHOS-20000008"/>
    <rdl:PCA_100006766 rdf:resource="http://rds.posccaesar.org/ontology/plm/rdl/PCA_100006637"/>
    <rdfs:comment>The heat tracing block diagram shall show the connection between the following:
 - Distribution board with circuit number;
 - Power supply cable numbers;
 - Junction boxes with tag number;
 - Heat tracing cable numbers.</rdfs:comment>
    <rdl:PCA_100006766 rdf:resource="http://rds.posccaesar.org/ontology/plm/rdl/PCA_100006627"/>
    <skos:broadMatch rdf:resource="http://rds.posccaesar.org/ontology/plm/rdl/PCA_100006696"/>
    <rdl:PCA_100006766 rdf:resource="http://rds.posccaesar.org/ontology/plm/rdl/PCA_100006638"/>
    <rdfs:label>Heat tracing block diagram</rdfs:label>
    <rdl:PCA_100006768>The heat tracing block diagram shall show the connection between the following:
 - Distribution board with circuit number;
 - Power supply cable numbers;
 - Junction boxes with tag number;
 - Heat tracing cable numbers.</rdl:PCA_100006768>
    <skos:broadMatch rdf:resource="http://rds.posccaesar.org/ontology/plm/rdl/PCA_100006699"/>
    <skos:broadMatch rdf:resource="http://rds.posccaesar.org/ontology/plm/rdl/PCA_100006695"/>
  </owl:Class>
  <owl:Class rdf:about="http://rds.posccaesar.org/ontology/plm/rdl/PCA_100006489">
    <rdl:PCA_100006765 rdf:resource="http://w3id.org/readi/rdl/CFIHOS-20000018"/>
    <rdfs:label>Technology qualification program</rdfs:label>
    <skos:broader rdf:resource="http://rds.posccaesar.org/ontology/plm/rdl/PCA_100006759"/>
    <rdfs:comment>To  descibe all planned qualification activities and acceptance criteria.</rdfs:comment>
    <skos:broadMatch rdf:resource="http://rds.posccaesar.org/ontology/plm/rdl/PCA_100006672"/>
    <rdl:PCA_100006768>To  descibe all planned qualification activities and acceptance criteria.</rdl:PCA_100006768>
    <rdl:PCA_100006766 rdf:resource="http://rds.posccaesar.org/ontology/plm/rdl/PCA_100006654"/>
    <rdl:PCA_100006763>Overview of technology development and new technology used in design</rdl:PCA_100006763>
    <rdfs:subClassOf rdf:resource="http://rds.posccaesar.org/ontology/plm/rdl/PCA_100004908"/>
  </owl:Class>
  <owl:Class rdf:about="http://rds.posccaesar.org/ontology/plm/rdl/PCA_100006368">
    <skos:broader rdf:resource="http://rds.posccaesar.org/ontology/plm/rdl/PCA_100006748"/>
    <skos:broadMatch rdf:resource="http://rds.posccaesar.org/ontology/plm/rdl/PCA_100006717"/>
    <rdfs:label>Pipeline index</rdfs:label>
    <rdl:PCA_100006766 rdf:resource="http://rds.posccaesar.org/ontology/plm/rdl/PCA_100006654"/>
    <rdl:PCA_100006765 rdf:resource="http://w3id.org/readi/rdl/CFIHOS-20000018"/>
    <rdfs:subClassOf rdf:resource="http://rds.posccaesar.org/ontology/plm/rdl/PCA_100004908"/>
  </owl:Class>
  <owl:Class rdf:about="http://rds.posccaesar.org/ontology/plm/rdl/PCA_100006356">
    <skos:broader rdf:resource="http://rds.posccaesar.org/ontology/plm/rdl/PCA_100006756"/>
    <skos:broadMatch rdf:resource="http://rds.posccaesar.org/ontology/plm/rdl/PCA_100006722"/>
    <rdfs:label>PAGA coverage measurements reports</rdfs:label>
    <rdfs:comment>PAGA coverage (STIPA or STI according to NORSOK T-101 measurements report shall be provided.</rdfs:comment>
    <rdl:PCA_100006768>PAGA coverage (STIPA or STI according to NORSOK T-101 measurements report shall be provided.</rdl:PCA_100006768>
    <rdl:PCA_100006766 rdf:resource="http://rds.posccaesar.org/ontology/plm/rdl/PCA_100006653"/>
    <rdl:PCA_100006765 rdf:resource="http://w3id.org/readi/rdl/CFIHOS-20000030"/>
    <rdfs:subClassOf rdf:resource="http://rds.posccaesar.org/ontology/plm/rdl/PCA_100004908"/>
  </owl:Class>
  <owl:Class rdf:about="http://rds.posccaesar.org/ontology/plm/rdl/PCA_100006235">
    <rdfs:comment>Details showing anode arrangement (anode location and material, anode dimensions, cables, cable joints and cable to anode connections) shall also be included.</rdfs:comment>
    <rdl:PCA_100006763>General arrangement drawing of anode bed including location, depth, backfill materials (such as coke and bentonite clay), geotextiles, cables and cable routing.</rdl:PCA_100006763>
    <rdl:PCA_100006765 rdf:resource="http://w3id.org/readi/rdl/CFIHOS-20000018"/>
    <skos:broader rdf:resource="http://rds.posccaesar.org/ontology/plm/rdl/PCA_100006739"/>
    <rdl:PCA_100006768>Details showing anode arrangement (anode location and material, anode dimensions, cables, cable joints and cable to anode connections) shall also be included.</rdl:PCA_100006768>
    <skos:broadMatch rdf:resource="http://rds.posccaesar.org/ontology/plm/rdl/PCA_100006708"/>
    <rdfs:label>General arrangement drawing - Anode bed</rdfs:label>
    <rdl:PCA_100006766 rdf:resource="http://rds.posccaesar.org/ontology/plm/rdl/PCA_100006657"/>
    <rdfs:subClassOf rdf:resource="http://rds.posccaesar.org/ontology/plm/rdl/PCA_100004908"/>
  </owl:Class>
  <owl:Class rdf:about="http://rds.posccaesar.org/ontology/plm/rdl/PCA_100006477">
    <skos:broader rdf:resource="http://rds.posccaesar.org/ontology/plm/rdl/PCA_100006756"/>
    <skos:broadMatch rdf:resource="http://rds.posccaesar.org/ontology/plm/rdl/PCA_100006698"/>
    <rdfs:label>Swivel system report</rdfs:label>
    <rdfs:comment>Technical documentation of the swivel stack and all mechanical components of the swivel shall be delivered. This documentation shall include the following:
 - General arrangement drawing;
 - Detail drawings of all major component;
 - Design analyses of all major component;
 - Material certificates for all components including welding filler material along with traceability data;
 - The design loads / swivel interface forces from piping, spools, flexible connections.</rdfs:comment>
    <rdl:PCA_100006768>Technical documentation of the swivel stack and all mechanical components of the swivel shall be delivered. This documentation shall include the following:
 - General arrangement drawing;
 - Detail drawings of all major component;
 - Design analyses of all major component;
 - Material certificates for all components including welding filler material along with traceability data;
 - The design loads / swivel interface forces from piping, spools, flexible connections.</rdl:PCA_100006768>
    <rdl:PCA_100006766 rdf:resource="http://rds.posccaesar.org/ontology/plm/rdl/PCA_100006657"/>
    <rdl:PCA_100006765 rdf:resource="http://w3id.org/readi/rdl/CFIHOS-20000033"/>
    <rdfs:subClassOf rdf:resource="http://rds.posccaesar.org/ontology/plm/rdl/PCA_100004908"/>
  </owl:Class>
  <owl:Class rdf:about="http://rds.posccaesar.org/ontology/plm/rdl/PCA_100006465">
    <skos:broadMatch rdf:resource="http://rds.posccaesar.org/ontology/plm/rdl/PCA_100006734"/>
    <rdl:PCA_100006766 rdf:resource="http://rds.posccaesar.org/ontology/plm/rdl/PCA_100006656"/>
    <skos:broader rdf:resource="http://rds.posccaesar.org/ontology/plm/rdl/PCA_100006746"/>
    <rdl:PCA_100006768>The following drawings shall be delivered:
 - General notes and specifications;
 - Isometric view (one isometric view per module. Shall cover only main steel and include elevation, grid lines, key plan, north and east references, northing and orientation with respect of true north);
 - General Arrangement (plan and elevation view);
 - Plan, Sections and details;
 - Standard drawings (e.g. grating, railing, staircase, ladder).

Each structural drawing shall contain the following information:
 - Dimensions;
 - Plate thicknesses and section properties;
 - Weld type and size;
 - Material properties;
 - Reference drawings number;
 - Reference to tag number (if relevant);
 - Weight and CoG.</rdl:PCA_100006768>
    <skos:broadMatch rdf:resource="http://rds.posccaesar.org/ontology/plm/rdl/PCA_100006732"/>
    <rdfs:label>Structural steel and aluminium. main, secondary and outfitting drawings</rdfs:label>
    <skos:broadMatch rdf:resource="http://rds.posccaesar.org/ontology/plm/rdl/PCA_100006733"/>
    <skos:broadMatch rdf:resource="http://rds.posccaesar.org/ontology/plm/rdl/PCA_100006731"/>
    <rdl:PCA_100006765 rdf:resource="http://w3id.org/readi/rdl/CFIHOS-20000006"/>
    <rdfs:comment>The following drawings shall be delivered:
 - General notes and specifications;
 - Isometric view (one isometric view per module. Shall cover only main steel and include elevation, grid lines, key plan, north and east references, northing and orientation with respect of true north);
 - General Arrangement (plan and elevation view);
 - Plan, Sections and details;
 - Standard drawings (e.g. grating, railing, staircase, ladder).

Each structural drawing shall contain the following information:
 - Dimensions;
 - Plate thicknesses and section properties;
 - Weld type and size;
 - Material properties;
 - Reference drawings number;
 - Reference to tag number (if relevant);
 - Weight and CoG.</rdfs:comment>
    <rdfs:subClassOf rdf:resource="http://rds.posccaesar.org/ontology/plm/rdl/PCA_100004908"/>
  </owl:Class>
  <owl:Class rdf:about="http://rds.posccaesar.org/ontology/plm/rdl/PCA_100006344">
    <skos:broader rdf:resource="http://rds.posccaesar.org/ontology/plm/rdl/PCA_100006753"/>
    <rdfs:label>Obsolescence management plan</rdfs:label>
    <rdl:PCA_100006763>Subsea equipment Supplier shall provide an Obsolescence Management Plan describing the strategies for identification and mitigation of the effects of obsolescence through all stages of the life of the product. This document shall be maintained throughout the product lifecycle.</rdl:PCA_100006763>
    <rdfs:subClassOf rdf:resource="http://rds.posccaesar.org/ontology/plm/rdl/PCA_100004908"/>
  </owl:Class>
  <owl:Class rdf:about="http://rds.posccaesar.org/ontology/plm/rdl/PCA_100006453">
    <skos:broader rdf:resource="http://rds.posccaesar.org/ontology/plm/rdl/PCA_100006760"/>
    <skos:broadMatch rdf:resource="http://rds.posccaesar.org/ontology/plm/rdl/PCA_100006716"/>
    <rdfs:label>Spare parts interchangeability register (SPIR)</rdfs:label>
    <rdfs:comment>Content shall be in accordance with Company specific requirements.</rdfs:comment>
    <rdl:PCA_100006768>Content shall be in accordance with Company specific requirements.</rdl:PCA_100006768>
    <rdl:PCA_100006763>A spare parts interchangeability record (SPIR) shall be provided for all parts potentially requiring replacement/repair. The SPIR shall support the repair strategy for the equipment units. For bulk and other equipment unit with repair strategy “scrap and replace” only the complete replacement equipment shall be listed in the SPIR.</rdl:PCA_100006763>
    <rdfs:subClassOf rdf:resource="http://rds.posccaesar.org/ontology/plm/rdl/PCA_100004908"/>
  </owl:Class>
  <owl:Class rdf:about="http://rds.posccaesar.org/ontology/plm/rdl/PCA_100006332">
    <rdfs:comment>A complete motion analyses model shall be delivered with all necessary information required to perform a re-analysis.</rdfs:comment>
    <skos:broader rdf:resource="http://rds.posccaesar.org/ontology/plm/rdl/PCA_100006741"/>
    <rdl:PCA_100006766 rdf:resource="http://rds.posccaesar.org/ontology/plm/rdl/PCA_100006647"/>
    <rdl:PCA_100006765 rdf:resource="http://w3id.org/readi/rdl/CFIHOS-20000033"/>
    <skos:broader rdf:resource="http://rds.posccaesar.org/ontology/plm/rdl/PCA_100006762"/>
    <skos:broadMatch rdf:resource="http://rds.posccaesar.org/ontology/plm/rdl/PCA_100006687"/>
    <rdl:PCA_100006768>A complete motion analyses model shall be delivered with all necessary information required to perform a re-analysis.</rdl:PCA_100006768>
    <rdfs:subClassOf rdf:resource="http://rds.posccaesar.org/ontology/plm/rdl/PCA_100004908"/>
    <rdfs:label>Motion analysis model</rdfs:label>
  </owl:Class>
  <owl:Class rdf:about="http://rds.posccaesar.org/ontology/plm/rdl/PCA_100006441">
    <rdl:PCA_100006768>Functional Safety management Plan (FSMP).

FSMP shall be established addressing all activities of the SIS lifecycle and detailing each phase due to be performed (e.g. project development or operation phase). This shall include a plan for when the activities shall be performed and responsibilities for the different activities. The document shall be made available by the overall SIS compliance responsible, i.e., integrator. 


SIL Allocation Report.

With references in analysis of hazards, risks and risks reduction, the determined Safety Instrumented Functions (SIF), allocated Safety Integrity Levels and identified SIS respectively shall be documented in a "SIL allocation report" file including an index of all SIF/SIS. 


LOPA Report.

Layer Of Protection Analysis (LOPA) is a simplified risk-based method that can be applied to allocate SIL requirement to the Safety Instrumented Functions (SIF). LOPA is the preferred method for the SIL allocation of preventive Safety Instrumented Functions. LOPA analysis shall be documented in a report. 


Safety Requirements Specification (SRS).

Safety Instrumented System (SIS) is developed throughout different lifecycle phases providing an extract of relevant information. The SRS shall focus on main requirements and performance parameters of the SIS while references are made to other documents in order to accomplish a complete overview of all SIS properties.


SIL Compliance Report.

This report including Calculation and Data Dossier (CDD), shall describe methodologies, all data sources applied, calculations and reporting the status of each SIS conformance with main requirements. 


Functional Safety Assessment reports. 

FSA shall be planned, performed and reported at the relevant project stages as indicated by IEC 61511.

Miscellaneous SIS specific information, examples: 
 - Premises for SIS operating and maintenance activities. 
 - Identify particular prerequisites and assumptions made as part of SIS design which has to be complied with during the phase of operating the SIS. This shall also include description and procedures of required proof testing (to be prepared prior to and verified during commissioning, readily available to incorporate in plant maintenance program). 
 - Guideline for delivery of suppliers SIL documentation (e.g. IEC 61508 compliance certificate, Safety Manual). See also 5.186 SR-2740 Supplier SIL documentation. 
 - Reports from the various validation and verification activities including Factory Acceptance Test (FAT) and Site Acceptance test (SAT), a SIS validation record normally issued upon completion of the engineering (by system integrator). 


Formats for calculation files:
Reports: DOC+ PDF.
Calculation files (LOPA, SRS, SIL compliance including CDD): Excel (+TBA if commercial software applied)</rdl:PCA_100006768>
    <rdl:PCA_100006766 rdf:resource="http://rds.posccaesar.org/ontology/plm/rdl/PCA_100006628"/>
    <rdl:PCA_100006765 rdf:resource="http://w3id.org/readi/rdl/CFIHOS-20000011"/>
    <rdfs:comment>Functional Safety management Plan (FSMP).

FSMP shall be established addressing all activities of the SIS lifecycle and detailing each phase due to be performed (e.g. project development or operation phase). This shall include a plan for when the activities shall be performed and responsibilities for the different activities. The document shall be made available by the overall SIS compliance responsible, i.e., integrator. 


SIL Allocation Report.

With references in analysis of hazards, risks and risks reduction, the determined Safety Instrumented Functions (SIF), allocated Safety Integrity Levels and identified SIS respectively shall be documented in a "SIL allocation report" file including an index of all SIF/SIS. 


LOPA Report.

Layer Of Protection Analysis (LOPA) is a simplified risk-based method that can be applied to allocate SIL requirement to the Safety Instrumented Functions (SIF). LOPA is the preferred method for the SIL allocation of preventive Safety Instrumented Functions. LOPA analysis shall be documented in a report. 


Safety Requirements Specification (SRS).

Safety Instrumented System (SIS) is developed throughout different lifecycle phases providing an extract of relevant information. The SRS shall focus on main requirements and performance parameters of the SIS while references are made to other documents in order to accomplish a complete overview of all SIS properties.


SIL Compliance Report.

This report including Calculation and Data Dossier (CDD), shall describe methodologies, all data sources applied, calculations and reporting the status of each SIS conformance with main requirements. 


Functional Safety Assessment reports. 

FSA shall be planned, performed and reported at the relevant project stages as indicated by IEC 61511.

Miscellaneous SIS specific information, examples: 
 - Premises for SIS operating and maintenance activities. 
 - Identify particular prerequisites and assumptions made as part of SIS design which has to be complied with during the phase of operating the SIS. This shall also include description and procedures of required proof testing (to be prepared prior to and verified during commissioning, readily available to incorporate in plant maintenance program). 
 - Guideline for delivery of suppliers SIL documentation (e.g. IEC 61508 compliance certificate, Safety Manual). See also 5.186 SR-2740 Supplier SIL documentation. 
 - Reports from the various validation and verification activities including Factory Acceptance Test (FAT) and Site Acceptance test (SAT), a SIS validation record normally issued upon completion of the engineering (by system integrator). 


Formats for calculation files:
Reports: DOC+ PDF.
Calculation files (LOPA, SRS, SIL compliance including CDD): Excel (+TBA if commercial software applied)</rdfs:comment>
    <skos:broadMatch rdf:resource="http://rds.posccaesar.org/ontology/plm/rdl/PCA_100006727"/>
    <rdl:PCA_100006765 rdf:resource="http://w3id.org/readi/rdl/CFIHOS-20000010"/>
    <rdl:PCA_100006763>Documentation shall fulfil the requirements in the standards IEC 61511 and IEC 61508 or Norwegian Oil and Gas guideline 070 as relevant and be developed to suit any lifecycle of a Safety Instrumented System (SIS).</rdl:PCA_100006763>
    <skos:broader rdf:resource="http://rds.posccaesar.org/ontology/plm/rdl/PCA_100006756"/>
    <rdfs:label>SIS functional safety information</rdfs:label>
    <rdl:PCA_100006766 rdf:resource="http://rds.posccaesar.org/ontology/plm/rdl/PCA_100006633"/>
    <rdfs:subClassOf rdf:resource="http://rds.posccaesar.org/ontology/plm/rdl/PCA_100004908"/>
    <skos:broader rdf:resource="http://rds.posccaesar.org/ontology/plm/rdl/PCA_100006753"/>
    <rdl:PCA_100006766 rdf:resource="http://rds.posccaesar.org/ontology/plm/rdl/PCA_100006627"/>
    <rdl:PCA_100006766 rdf:resource="http://rds.posccaesar.org/ontology/plm/rdl/PCA_100006626"/>
    <rdl:PCA_100006765 rdf:resource="http://w3id.org/readi/rdl/CFIHOS-20000013"/>
  </owl:Class>
  <owl:Class rdf:about="http://rds.posccaesar.org/ontology/plm/rdl/PCA_100006320">
    <rdl:PCA_100006765 rdf:resource="http://w3id.org/readi/rdl/CFIHOS-20000031"/>
    <rdfs:subClassOf rdf:resource="http://rds.posccaesar.org/ontology/plm/rdl/PCA_100004908"/>
    <skos:broadMatch rdf:resource="http://rds.posccaesar.org/ontology/plm/rdl/PCA_100006688"/>
    <rdfs:comment>Procedure describing the requirements for material traceability for different components and equipment.</rdfs:comment>
    <rdl:PCA_100006763>Provide instructions for preparation of the material traceability list.</rdl:PCA_100006763>
    <rdl:PCA_100006768>Procedure describing the requirements for material traceability for different components and equipment.</rdl:PCA_100006768>
    <skos:broader rdf:resource="http://rds.posccaesar.org/ontology/plm/rdl/PCA_100006751"/>
    <rdfs:label>Material traceability procedure</rdfs:label>
    <rdl:PCA_100006766 rdf:resource="http://rds.posccaesar.org/ontology/plm/rdl/PCA_100006653"/>
  </owl:Class>
  <owl:Class rdf:about="http://rds.posccaesar.org/ontology/plm/rdl/PCA_100006204">
    <skos:broader rdf:resource="http://rds.posccaesar.org/ontology/plm/rdl/PCA_100006741"/>
    <skos:broadMatch rdf:resource="http://rds.posccaesar.org/ontology/plm/rdl/PCA_100006687"/>
    <rdfs:label>Fiber optical long distance cable transmission budget calculations</rdfs:label>
    <rdl:PCA_100006765 rdf:resource="http://w3id.org/readi/rdl/CFIHOS-20000030"/>
    <rdl:PCA_100006764>Discipline specific (telecom) content is missing</rdl:PCA_100006764>
    <rdl:PCA_100006763>Fibre optical long distance cable transmission budget calculations (attenuation in dB) that have been used for design of fibre optical cable and network equipment shall be provided.</rdl:PCA_100006763>
    <rdfs:subClassOf rdf:resource="http://rds.posccaesar.org/ontology/plm/rdl/PCA_100004908"/>
  </owl:Class>
  <owl:Class rdf:about="http://rds.posccaesar.org/ontology/plm/rdl/PCA_100006216">
    <rdl:PCA_100006766 rdf:resource="http://rds.posccaesar.org/ontology/plm/rdl/PCA_100006587"/>
    <rdl:PCA_100006764>Data content and interface shall be agreed between relevant parties.</rdl:PCA_100006764>
    <skos:broader rdf:resource="http://rds.posccaesar.org/ontology/plm/rdl/PCA_100006757"/>
    <rdfs:label>Fiscal metering - Data exchange specifications</rdfs:label>
    <rdl:PCA_100006766 rdf:resource="http://rds.posccaesar.org/ontology/plm/rdl/PCA_100006591"/>
    <rdl:PCA_100006763>A separate data exchange document shall be issued for each interface.</rdl:PCA_100006763>
    <rdl:PCA_100006765 rdf:resource="http://w3id.org/readi/rdl/CFIHOS-20000015"/>
    <skos:broadMatch rdf:resource="http://rds.posccaesar.org/ontology/plm/rdl/PCA_100006703"/>
    <rdfs:subClassOf rdf:resource="http://rds.posccaesar.org/ontology/plm/rdl/PCA_100004908"/>
  </owl:Class>
  <owl:Class rdf:about="http://rds.posccaesar.org/ontology/plm/rdl/PCA_100006228">
    <skos:broadMatch rdf:resource="http://rds.posccaesar.org/ontology/plm/rdl/PCA_100006686"/>
    <rdl:PCA_100006765 rdf:resource="http://w3id.org/readi/rdl/CFIHOS-20000031"/>
    <rdfs:subClassOf rdf:resource="http://rds.posccaesar.org/ontology/plm/rdl/PCA_100004908"/>
    <rdfs:label>Foundation design report</rdfs:label>
    <rdl:PCA_100006768>Report providing the results from geotechnical calculations and analysis for structures installed on seabed.</rdl:PCA_100006768>
    <rdl:PCA_100006763>To give input to the design of structures installed on seabed.</rdl:PCA_100006763>
    <rdl:PCA_100006766 rdf:resource="http://rds.posccaesar.org/ontology/plm/rdl/PCA_100006653"/>
    <rdfs:comment>Report providing the results from geotechnical calculations and analysis for structures installed on seabed.</rdfs:comment>
    <skos:broader rdf:resource="http://rds.posccaesar.org/ontology/plm/rdl/PCA_100006756"/>
  </owl:Class>
  <owl:Class rdf:about="http://rds.posccaesar.org/ontology/plm/rdl/PCA_100006107">
    <rdfs:comment>All involved auxiliary systems shall be included.</rdfs:comment>
    <rdl:PCA_100006768>All involved auxiliary systems shall be included.</rdl:PCA_100006768>
    <rdl:PCA_100006766 rdf:resource="http://rds.posccaesar.org/ontology/plm/rdl/PCA_100006638"/>
    <skos:broadMatch rdf:resource="http://rds.posccaesar.org/ontology/plm/rdl/PCA_100006688"/>
    <rdl:PCA_100006766 rdf:resource="http://rds.posccaesar.org/ontology/plm/rdl/PCA_100006635"/>
    <skos:broadMatch rdf:resource="http://rds.posccaesar.org/ontology/plm/rdl/PCA_100006687"/>
    <rdl:PCA_100006766 rdf:resource="http://rds.posccaesar.org/ontology/plm/rdl/PCA_100006636"/>
    <rdl:PCA_100006766 rdf:resource="http://rds.posccaesar.org/ontology/plm/rdl/PCA_100006634"/>
    <rdfs:subClassOf rdf:resource="http://rds.posccaesar.org/ontology/plm/rdl/PCA_100004908"/>
    <skos:broader rdf:resource="http://rds.posccaesar.org/ontology/plm/rdl/PCA_100006752"/>
    <rdfs:label>Black start philosophy</rdfs:label>
    <rdl:PCA_100006763>To describe the complete sequence starting with "black" platform/plant and ending with main power established.</rdl:PCA_100006763>
    <rdl:PCA_100006765 rdf:resource="http://w3id.org/readi/rdl/CFIHOS-20000008"/>
    <rdl:PCA_100006766 rdf:resource="http://rds.posccaesar.org/ontology/plm/rdl/PCA_100006637"/>
    <rdl:PCA_100006766 rdf:resource="http://rds.posccaesar.org/ontology/plm/rdl/PCA_100006639"/>
  </owl:Class>
  <owl:Class rdf:about="http://rds.posccaesar.org/ontology/plm/rdl/PCA_100006119">
    <rdfs:label>Chemical management plan</rdfs:label>
    <rdl:PCA_100006768>Each field/plant should have a Chemical Management Plan that describes as a minimum:
 - Contact details for key personnel;
 - Roles &amp; Responsibilities;
 - Contract references;
 - Risk reviews;
 - Description of each and every chemical used (past, present and future), including:
   - Reason for use;
   - Mechanism &amp; application;
   - Imitations;
   - Injection system;
   - Monitoring programme
   - Troubleshooting guide;
   - HSE summary;
   - Supply chain description;
 - Description of processes where chemicals are currently not used, and why;
 - Description of data management;
 - Report references;
 - Reference to governing documents;
 - Reference to substitution plans;
 - Reference to improvement plans;
 - Key Performance Indicators.</rdl:PCA_100006768>
    <skos:broader rdf:resource="http://rds.posccaesar.org/ontology/plm/rdl/PCA_100006753"/>
    <skos:broadMatch rdf:resource="http://rds.posccaesar.org/ontology/plm/rdl/PCA_100006726"/>
    <rdfs:subClassOf rdf:resource="http://rds.posccaesar.org/ontology/plm/rdl/PCA_100004908"/>
    <skos:broadMatch rdf:resource="http://rds.posccaesar.org/ontology/plm/rdl/PCA_100006729"/>
    <rdl:PCA_100006763>Description of chemical treatment strategy for the project/asset, including strategy for modifications &amp; tie-ins;</rdl:PCA_100006763>
    <rdfs:comment>Each field/plant should have a Chemical Management Plan that describes as a minimum:
 - Contact details for key personnel;
 - Roles &amp; Responsibilities;
 - Contract references;
 - Risk reviews;
 - Description of each and every chemical used (past, present and future), including:
   - Reason for use;
   - Mechanism &amp; application;
   - Imitations;
   - Injection system;
   - Monitoring programme
   - Troubleshooting guide;
   - HSE summary;
   - Supply chain description;
 - Description of processes where chemicals are currently not used, and why;
 - Description of data management;
 - Report references;
 - Reference to governing documents;
 - Reference to substitution plans;
 - Reference to improvement plans;
 - Key Performance Indicators.</rdfs:comment>
    <rdl:PCA_100006766 rdf:resource="http://rds.posccaesar.org/ontology/plm/rdl/PCA_100006654"/>
    <skos:broadMatch rdf:resource="http://rds.posccaesar.org/ontology/plm/rdl/PCA_100006728"/>
    <rdl:PCA_100006765 rdf:resource="http://w3id.org/readi/rdl/CFIHOS-20000026"/>
  </owl:Class>
  <owl:Class rdf:about="http://rds.posccaesar.org/ontology/plm/rdl/PCA_100006369">
    <rdfs:comment>Pipeline protection drawings of protection not covered by rock installation, trenching or crossings such as use of concrete mattresses or covers</rdfs:comment>
    <rdl:PCA_100006763>Documentation of installations to ensure safe operation</rdl:PCA_100006763>
    <rdl:PCA_100006765 rdf:resource="http://w3id.org/readi/rdl/CFIHOS-20000018"/>
    <rdl:PCA_100006768>Pipeline protection drawings of protection not covered by rock installation, trenching or crossings such as use of concrete mattresses or covers</rdl:PCA_100006768>
    <rdfs:subClassOf rdf:resource="http://rds.posccaesar.org/ontology/plm/rdl/PCA_100004908"/>
    <skos:broadMatch rdf:resource="http://rds.posccaesar.org/ontology/plm/rdl/PCA_100006732"/>
    <rdl:PCA_100006766 rdf:resource="http://rds.posccaesar.org/ontology/plm/rdl/PCA_100006654"/>
    <skos:broader rdf:resource="http://rds.posccaesar.org/ontology/plm/rdl/PCA_100006746"/>
    <rdfs:label>Pipeline protection drawing</rdfs:label>
  </owl:Class>
  <owl:Class rdf:about="http://rds.posccaesar.org/ontology/plm/rdl/PCA_100006248">
    <rdfs:comment>The isometrics can be based on piping isometrics, and shall include necessary information such as insulation type/thickness, temperature requirements, material of pipes and extent of heat tracing shall be clearly identified, including:
 - Graphical presentation of heat tracing cable (where installed);
 - Heat tracing cable numbers;
 - Junction boxes with tag code;
 - Distribution boards with circuits
 - End seal of heat tracing cable;
 - Splice of heat tracing;
 - Type and length of heat trace cables;
 - Minimum maintain temperature of heated medium;
 - Maximum medium temperatures;
 - Temperature control (where thermostat required) including set point of thermostat.</rdfs:comment>
    <rdl:PCA_100006763>All lines including instrument tubing subject to heat tracing shall be shown on heat tracing isometrics.</rdl:PCA_100006763>
    <skos:broadMatch rdf:resource="http://rds.posccaesar.org/ontology/plm/rdl/PCA_100006710"/>
    <skos:broadMatch rdf:resource="http://rds.posccaesar.org/ontology/plm/rdl/PCA_100006733"/>
    <rdl:PCA_100006768>The isometrics can be based on piping isometrics, and shall include necessary information such as insulation type/thickness, temperature requirements, material of pipes and extent of heat tracing shall be clearly identified, including:
 - Graphical presentation of heat tracing cable (where installed);
 - Heat tracing cable numbers;
 - Junction boxes with tag code;
 - Distribution boards with circuits
 - End seal of heat tracing cable;
 - Splice of heat tracing;
 - Type and length of heat trace cables;
 - Minimum maintain temperature of heated medium;
 - Maximum medium temperatures;
 - Temperature control (where thermostat required) including set point of thermostat.</rdl:PCA_100006768>
    <rdl:PCA_100006766 rdf:resource="http://rds.posccaesar.org/ontology/plm/rdl/PCA_100006656"/>
    <rdfs:subClassOf rdf:resource="http://rds.posccaesar.org/ontology/plm/rdl/PCA_100004908"/>
    <rdfs:label>Heat tracing isometrics</rdfs:label>
    <skos:broader rdf:resource="http://rds.posccaesar.org/ontology/plm/rdl/PCA_100006746"/>
    <skos:broadMatch rdf:resource="http://rds.posccaesar.org/ontology/plm/rdl/PCA_100006732"/>
    <rdl:PCA_100006765 rdf:resource="http://w3id.org/readi/rdl/CFIHOS-20000008"/>
  </owl:Class>
  <owl:Class rdf:about="http://rds.posccaesar.org/ontology/plm/rdl/PCA_100006236">
    <rdl:PCA_100006765 rdf:resource="http://w3id.org/readi/rdl/CFIHOS-20000018"/>
    <rdl:PCA_100006763>Drawing showing anode cable sections and connection to tesposts/TR-units.</rdl:PCA_100006763>
    <skos:broadMatch rdf:resource="http://rds.posccaesar.org/ontology/plm/rdl/PCA_100006708"/>
    <skos:broader rdf:resource="http://rds.posccaesar.org/ontology/plm/rdl/PCA_100006739"/>
    <rdfs:comment>Details shall show type and cross-section of anode cable and possible low resistivity backfill.</rdfs:comment>
    <rdl:PCA_100006766 rdf:resource="http://rds.posccaesar.org/ontology/plm/rdl/PCA_100006657"/>
    <rdl:PCA_100006768>Details shall show type and cross-section of anode cable and possible low resistivity backfill.</rdl:PCA_100006768>
    <rdfs:subClassOf rdf:resource="http://rds.posccaesar.org/ontology/plm/rdl/PCA_100004908"/>
    <rdfs:label>General arrangement drawing - Continuous anode cable</rdfs:label>
  </owl:Class>
  <owl:Class rdf:about="http://rds.posccaesar.org/ontology/plm/rdl/PCA_100006478">
    <rdl:PCA_100006766 rdf:resource="http://rds.posccaesar.org/ontology/plm/rdl/PCA_100006614"/>
    <rdl:PCA_100006763>System documents:
The objective of the System documents is to describe the systems at a plant for learning purpose. The System document is a compilation of technical information (LCI), functional descriptions, reason for choice of design and describes the System characteristics, regulate how to operate and protect the System in various conditions. This shall apply to all disciplines within all systems.

The System documents (S-documents) apply for all systems, subsystems and assemblies. One document shall be produced for each system.

The main target group for System documents are mainly operational and maintenance personnel at a plant.

The System documents shall be produced in local language. 


Operation documents:
The objective of the operating documents is to describe how to operate a system and its equipment in a safe, reliable and effective way.

Operation documents (O-documents) apply for all systems, subsystems and assemblies. One Main Operating document shall be produced for each system.

The "Main Operating document "shall contain a compilation (links to detailed O-documents) of operating procedures according to the index structure shown below.

The operating documents (check lists or operating rules) are formed as action points in tables.

The black start operating documents shall describe the complete sequence starting with "black" installation and ending with main power established. All involved auxiliary systems shall be included and each document shall be related to the Main operating document for each system.

The initial scenario shall be APS for offshore installations (Abandon Platform Shutdown) or Plant evacuation for onshore plants e.g. after a gas leakage, where gas may have entered non-hazardous areas and rooms. The two alternatives: Black start of emergency power /Essential power and black start of UPS shall be described. In case of cable from shore or other independent unit, such as a national grid, and this power is used as a source of emergency power, this alternative method of black start shall also be described. All Operating documents related to Black start shall be provided with a unique Node number.

The main target group for Operational document is mainly operational personnel at a plant.</rdl:PCA_100006763>
    <rdl:PCA_100006766 rdf:resource="http://rds.posccaesar.org/ontology/plm/rdl/PCA_100006642"/>
    <rdl:PCA_100006766 rdf:resource="http://rds.posccaesar.org/ontology/plm/rdl/PCA_100006595"/>
    <rdl:PCA_100006766 rdf:resource="http://rds.posccaesar.org/ontology/plm/rdl/PCA_100006639"/>
    <rdl:PCA_100006766 rdf:resource="http://rds.posccaesar.org/ontology/plm/rdl/PCA_100006636"/>
    <rdl:PCA_100006766 rdf:resource="http://rds.posccaesar.org/ontology/plm/rdl/PCA_100006613"/>
    <rdl:PCA_100006766 rdf:resource="http://rds.posccaesar.org/ontology/plm/rdl/PCA_100006601"/>
    <rdl:PCA_100006766 rdf:resource="http://rds.posccaesar.org/ontology/plm/rdl/PCA_100006598"/>
    <rdl:PCA_100006766 rdf:resource="http://rds.posccaesar.org/ontology/plm/rdl/PCA_100006586"/>
    <rdl:PCA_100006766 rdf:resource="http://rds.posccaesar.org/ontology/plm/rdl/PCA_100006627"/>
    <rdl:PCA_100006766 rdf:resource="http://rds.posccaesar.org/ontology/plm/rdl/PCA_100006619"/>
    <rdl:PCA_100006766 rdf:resource="http://rds.posccaesar.org/ontology/plm/rdl/PCA_100006604"/>
    <rdl:PCA_100006766 rdf:resource="http://rds.posccaesar.org/ontology/plm/rdl/PCA_100006629"/>
    <rdl:PCA_100006766 rdf:resource="http://rds.posccaesar.org/ontology/plm/rdl/PCA_100006606"/>
    <rdl:PCA_100006766 rdf:resource="http://rds.posccaesar.org/ontology/plm/rdl/PCA_100006578"/>
    <rdl:PCA_100006766 rdf:resource="http://rds.posccaesar.org/ontology/plm/rdl/PCA_100006630"/>
    <rdl:PCA_100006766 rdf:resource="http://rds.posccaesar.org/ontology/plm/rdl/PCA_100006588"/>
    <rdl:PCA_100006766 rdf:resource="http://rds.posccaesar.org/ontology/plm/rdl/PCA_100006609"/>
    <rdl:PCA_100006766 rdf:resource="http://rds.posccaesar.org/ontology/plm/rdl/PCA_100006591"/>
    <rdl:PCA_100006766 rdf:resource="http://rds.posccaesar.org/ontology/plm/rdl/PCA_100006641"/>
    <rdl:PCA_100006766 rdf:resource="http://rds.posccaesar.org/ontology/plm/rdl/PCA_100006632"/>
    <rdl:PCA_100006766 rdf:resource="http://rds.posccaesar.org/ontology/plm/rdl/PCA_100006612"/>
    <rdl:PCA_100006766 rdf:resource="http://rds.posccaesar.org/ontology/plm/rdl/PCA_100006581"/>
    <rdl:PCA_100006766 rdf:resource="http://rds.posccaesar.org/ontology/plm/rdl/PCA_100006622"/>
    <rdl:PCA_100006766 rdf:resource="http://rds.posccaesar.org/ontology/plm/rdl/PCA_100006597"/>
    <rdfs:subClassOf rdf:resource="http://rds.posccaesar.org/ontology/plm/rdl/PCA_100004908"/>
    <rdl:PCA_100006766 rdf:resource="http://rds.posccaesar.org/ontology/plm/rdl/PCA_100006638"/>
    <rdl:PCA_100006766 rdf:resource="http://rds.posccaesar.org/ontology/plm/rdl/PCA_100006615"/>
    <skos:broadMatch rdf:resource="http://rds.posccaesar.org/ontology/plm/rdl/PCA_100006698"/>
    <rdl:PCA_100006766 rdf:resource="http://rds.posccaesar.org/ontology/plm/rdl/PCA_100006596"/>
    <rdl:PCA_100006766 rdf:resource="http://rds.posccaesar.org/ontology/plm/rdl/PCA_100006637"/>
    <rdl:PCA_100006766 rdf:resource="http://rds.posccaesar.org/ontology/plm/rdl/PCA_100006617"/>
    <rdl:PCA_100006766 rdf:resource="http://rds.posccaesar.org/ontology/plm/rdl/PCA_100006602"/>
    <rdl:PCA_100006766 rdf:resource="http://rds.posccaesar.org/ontology/plm/rdl/PCA_100006583"/>
    <rdl:PCA_100006766 rdf:resource="http://rds.posccaesar.org/ontology/plm/rdl/PCA_100006624"/>
    <rdl:PCA_100006766 rdf:resource="http://rds.posccaesar.org/ontology/plm/rdl/PCA_100006599"/>
    <rdl:PCA_100006765 rdf:resource="http://w3id.org/readi/rdl/CFIHOS-20000033"/>
    <rdl:PCA_100006766 rdf:resource="http://rds.posccaesar.org/ontology/plm/rdl/PCA_100006605"/>
    <rdl:PCA_100006766 rdf:resource="http://rds.posccaesar.org/ontology/plm/rdl/PCA_100006607"/>
    <rdl:PCA_100006766 rdf:resource="http://rds.posccaesar.org/ontology/plm/rdl/PCA_100006579"/>
    <rdl:PCA_100006766 rdf:resource="http://rds.posccaesar.org/ontology/plm/rdl/PCA_100006589"/>
    <skos:broader rdf:resource="http://rds.posccaesar.org/ontology/plm/rdl/PCA_100006750"/>
    <rdl:PCA_100006766 rdf:resource="http://rds.posccaesar.org/ontology/plm/rdl/PCA_100006592"/>
    <rdl:PCA_100006766 rdf:resource="http://rds.posccaesar.org/ontology/plm/rdl/PCA_100006633"/>
    <rdl:PCA_100006766 rdf:resource="http://rds.posccaesar.org/ontology/plm/rdl/PCA_100006610"/>
    <rdfs:comment>The index structure of the System documents shall be as follows:
1  Objective and target group
2  System description 
2.1  Introduction 
2.2  Design basis 
2.3  Process description 
2.4  Process control
3  System operation (Opr) (Link to main Operation document for the actual system)
4  System protection 
4.2  System control
4.3  Equipment protection 
5  Technical data and drawings
6  Additional information 
6.1  Definitions and abbreviations 
6.2  Changes from previous version
6.3  References


The index structure of the main operating document shall be as follows:
Link to S-document for the actual system
3    System operation
3.1  Normal operation
3.2  Normal start-up
3.3  Normal shut down
3.4  Special operations
3.5  Operational routines 

Local language: YES</rdfs:comment>
    <rdl:PCA_100006766 rdf:resource="http://rds.posccaesar.org/ontology/plm/rdl/PCA_100006620"/>
    <rdl:PCA_100006766 rdf:resource="http://rds.posccaesar.org/ontology/plm/rdl/PCA_100006594"/>
    <rdl:PCA_100006766 rdf:resource="http://rds.posccaesar.org/ontology/plm/rdl/PCA_100006635"/>
    <rdl:PCA_100006766 rdf:resource="http://rds.posccaesar.org/ontology/plm/rdl/PCA_100006582"/>
    <rdl:PCA_100006766 rdf:resource="http://rds.posccaesar.org/ontology/plm/rdl/PCA_100006623"/>
    <rdl:PCA_100006766 rdf:resource="http://rds.posccaesar.org/ontology/plm/rdl/PCA_100006600"/>
    <rdl:PCA_100006766 rdf:resource="http://rds.posccaesar.org/ontology/plm/rdl/PCA_100006616"/>
    <rdl:PCA_100006766 rdf:resource="http://rds.posccaesar.org/ontology/plm/rdl/PCA_100006585"/>
    <rdl:PCA_100006766 rdf:resource="http://rds.posccaesar.org/ontology/plm/rdl/PCA_100006626"/>
    <rdl:PCA_100006766 rdf:resource="http://rds.posccaesar.org/ontology/plm/rdl/PCA_100006618"/>
    <rdl:PCA_100006766 rdf:resource="http://rds.posccaesar.org/ontology/plm/rdl/PCA_100006603"/>
    <rdl:PCA_100006766 rdf:resource="http://rds.posccaesar.org/ontology/plm/rdl/PCA_100006584"/>
    <rdl:PCA_100006766 rdf:resource="http://rds.posccaesar.org/ontology/plm/rdl/PCA_100006628"/>
    <rdl:PCA_100006766 rdf:resource="http://rds.posccaesar.org/ontology/plm/rdl/PCA_100006625"/>
    <rdl:PCA_100006766 rdf:resource="http://rds.posccaesar.org/ontology/plm/rdl/PCA_100006587"/>
    <rdl:PCA_100006768>The index structure of the System documents shall be as follows:
1  Objective and target group
2  System description 
2.1  Introduction 
2.2  Design basis 
2.3  Process description 
2.4  Process control
3  System operation (Opr) (Link to main Operation document for the actual system)
4  System protection 
4.2  System control
4.3  Equipment protection 
5  Technical data and drawings
6  Additional information 
6.1  Definitions and abbreviations 
6.2  Changes from previous version
6.3  References


The index structure of the main operating document shall be as follows:
Link to S-document for the actual system
3    System operation
3.1  Normal operation
3.2  Normal start-up
3.3  Normal shut down
3.4  Special operations
3.5  Operational routines 

Local language: YES</rdl:PCA_100006768>
    <rdl:PCA_100006766 rdf:resource="http://rds.posccaesar.org/ontology/plm/rdl/PCA_100006608"/>
    <rdfs:label>System and operation documents</rdfs:label>
    <rdl:PCA_100006766 rdf:resource="http://rds.posccaesar.org/ontology/plm/rdl/PCA_100006590"/>
    <rdl:PCA_100006766 rdf:resource="http://rds.posccaesar.org/ontology/plm/rdl/PCA_100006640"/>
    <rdl:PCA_100006766 rdf:resource="http://rds.posccaesar.org/ontology/plm/rdl/PCA_100006631"/>
    <rdl:PCA_100006766 rdf:resource="http://rds.posccaesar.org/ontology/plm/rdl/PCA_100006593"/>
    <skos:broadMatch rdf:resource="http://rds.posccaesar.org/ontology/plm/rdl/PCA_100006695"/>
    <rdl:PCA_100006766 rdf:resource="http://rds.posccaesar.org/ontology/plm/rdl/PCA_100006634"/>
    <rdl:PCA_100006766 rdf:resource="http://rds.posccaesar.org/ontology/plm/rdl/PCA_100006611"/>
    <rdl:PCA_100006766 rdf:resource="http://rds.posccaesar.org/ontology/plm/rdl/PCA_100006580"/>
    <rdl:PCA_100006766 rdf:resource="http://rds.posccaesar.org/ontology/plm/rdl/PCA_100006621"/>
  </owl:Class>
  <owl:Class rdf:about="http://rds.posccaesar.org/ontology/plm/rdl/PCA_100006357">
    <skos:broader rdf:resource="http://rds.posccaesar.org/ontology/plm/rdl/PCA_100006762"/>
    <rdl:PCA_100006768>The document shall contain a template including all adjustable parameters, indicating which parameters are fixed by the project. For parameters which have individual setting the criteria/formula for defining/calculating the individual setting shall be given. In addition, the document shall include a table listing all individual settings. This table shall on one axis list all equipment (tags) and the other all parameter requiring individual setting.

Examples of relevant equipment are: VSD (Variable Speed Drive), Soft starter, Synchronising Equipment, OLTC control (On Load Tap Changer), Insulation Monitoring equipment, Intelligent electrical devices (IED).</rdl:PCA_100006768>
    <rdl:PCA_100006766 rdf:resource="http://rds.posccaesar.org/ontology/plm/rdl/PCA_100006636"/>
    <rdl:PCA_100006766 rdf:resource="http://rds.posccaesar.org/ontology/plm/rdl/PCA_100006639"/>
    <rdl:PCA_100006766 rdf:resource="http://rds.posccaesar.org/ontology/plm/rdl/PCA_100006634"/>
    <rdfs:label>Parameter setting tables</rdfs:label>
    <rdl:PCA_100006766 rdf:resource="http://rds.posccaesar.org/ontology/plm/rdl/PCA_100006637"/>
    <rdfs:subClassOf rdf:resource="http://rds.posccaesar.org/ontology/plm/rdl/PCA_100004908"/>
    <rdfs:comment>The document shall contain a template including all adjustable parameters, indicating which parameters are fixed by the project. For parameters which have individual setting the criteria/formula for defining/calculating the individual setting shall be given. In addition, the document shall include a table listing all individual settings. This table shall on one axis list all equipment (tags) and the other all parameter requiring individual setting.

Examples of relevant equipment are: VSD (Variable Speed Drive), Soft starter, Synchronising Equipment, OLTC control (On Load Tap Changer), Insulation Monitoring equipment, Intelligent electrical devices (IED).</rdfs:comment>
    <rdl:PCA_100006765 rdf:resource="http://w3id.org/readi/rdl/CFIHOS-20000008"/>
    <rdl:PCA_100006766 rdf:resource="http://rds.posccaesar.org/ontology/plm/rdl/PCA_100006638"/>
    <rdl:PCA_100006766 rdf:resource="http://rds.posccaesar.org/ontology/plm/rdl/PCA_100006635"/>
    <skos:broadMatch rdf:resource="http://rds.posccaesar.org/ontology/plm/rdl/PCA_100006701"/>
  </owl:Class>
  <owl:Class rdf:about="http://rds.posccaesar.org/ontology/plm/rdl/PCA_100006466">
    <skos:broadMatch rdf:resource="http://rds.posccaesar.org/ontology/plm/rdl/PCA_100006734"/>
    <skos:broadMatch rdf:resource="http://rds.posccaesar.org/ontology/plm/rdl/PCA_100006733"/>
    <skos:broader rdf:resource="http://rds.posccaesar.org/ontology/plm/rdl/PCA_100006746"/>
    <skos:broadMatch rdf:resource="http://rds.posccaesar.org/ontology/plm/rdl/PCA_100006731"/>
    <rdfs:comment>The following drawings shall be delivered:
 - Arrangement
 - Typicals
 - Sections and details 
The drawings shall contain:
 - Dimensions
 - Plate thicknesses and section properties
 - Weld type and size
 - Material properties
 - Reference drawings number
 - Reference to tag number
Structural load plans shall be produced.</rdfs:comment>
    <rdl:PCA_100006768>The following drawings shall be delivered:
 - Arrangement
 - Typicals
 - Sections and details 
The drawings shall contain:
 - Dimensions
 - Plate thicknesses and section properties
 - Weld type and size
 - Material properties
 - Reference drawings number
 - Reference to tag number
Structural load plans shall be produced.</rdl:PCA_100006768>
    <skos:broadMatch rdf:resource="http://rds.posccaesar.org/ontology/plm/rdl/PCA_100006732"/>
    <rdfs:label>Structural steel and aluminium. main, secondary and outfitting drawings (civil)</rdfs:label>
    <rdfs:subClassOf rdf:resource="http://rds.posccaesar.org/ontology/plm/rdl/PCA_100004908"/>
  </owl:Class>
  <owl:Class rdf:about="http://rds.posccaesar.org/ontology/plm/rdl/PCA_100006345">
    <rdl:PCA_100006763>The report or collection of reports shall contain a complete description of the offloading arrangement.</rdl:PCA_100006763>
    <rdl:PCA_100006766 rdf:resource="http://rds.posccaesar.org/ontology/plm/rdl/PCA_100006603"/>
    <skos:broadMatch rdf:resource="http://rds.posccaesar.org/ontology/plm/rdl/PCA_100006687"/>
    <rdl:PCA_100006768>The report shall typically contain:
 - Overall description of the functionality of the offloading system;
 - Design analyses and drawings of the offloading system;
 - Overall description of hose maintenance and replacement method.</rdl:PCA_100006768>
    <rdfs:label>Offloading system arrangement report</rdfs:label>
    <rdfs:subClassOf rdf:resource="http://rds.posccaesar.org/ontology/plm/rdl/PCA_100004908"/>
    <rdl:PCA_100006765 rdf:resource="http://w3id.org/readi/rdl/CFIHOS-20000033"/>
    <skos:broader rdf:resource="http://rds.posccaesar.org/ontology/plm/rdl/PCA_100006756"/>
    <rdfs:comment>The report shall typically contain:
 - Overall description of the functionality of the offloading system;
 - Design analyses and drawings of the offloading system;
 - Overall description of hose maintenance and replacement method.</rdfs:comment>
  </owl:Class>
  <owl:Class rdf:about="http://rds.posccaesar.org/ontology/plm/rdl/PCA_100006333">
    <rdl:PCA_100006766 rdf:resource="http://rds.posccaesar.org/ontology/plm/rdl/PCA_100006647"/>
    <rdl:PCA_100006768>Motion design reports shall be delivered. The report or collection of reports shall contain the final documentation of:
 - Dimensioning environmental conditions;
 - Vessel response characteristics;
 - Extreme motion response;
 - Dimensioning accelerations;
 - Air gap / slamming / green sea analyses;
 - Model test verification analyses.</rdl:PCA_100006768>
    <rdfs:comment>Motion design reports shall be delivered. The report or collection of reports shall contain the final documentation of:
 - Dimensioning environmental conditions;
 - Vessel response characteristics;
 - Extreme motion response;
 - Dimensioning accelerations;
 - Air gap / slamming / green sea analyses;
 - Model test verification analyses.</rdfs:comment>
    <skos:broader rdf:resource="http://rds.posccaesar.org/ontology/plm/rdl/PCA_100006756"/>
    <rdfs:label>Motion design reports</rdfs:label>
    <rdl:PCA_100006765 rdf:resource="http://w3id.org/readi/rdl/CFIHOS-20000033"/>
    <rdfs:subClassOf rdf:resource="http://rds.posccaesar.org/ontology/plm/rdl/PCA_100004908"/>
    <skos:broadMatch rdf:resource="http://rds.posccaesar.org/ontology/plm/rdl/PCA_100006691"/>
    <skos:broadMatch rdf:resource="http://rds.posccaesar.org/ontology/plm/rdl/PCA_100006698"/>
  </owl:Class>
  <owl:Class rdf:about="http://rds.posccaesar.org/ontology/plm/rdl/PCA_100006454">
    <skos:broadMatch rdf:resource="http://rds.posccaesar.org/ontology/plm/rdl/PCA_100006687"/>
    <rdl:PCA_100006766 rdf:resource="http://rds.posccaesar.org/ontology/plm/rdl/PCA_100006654"/>
    <skos:broader rdf:resource="http://rds.posccaesar.org/ontology/plm/rdl/PCA_100006762"/>
    <rdl:PCA_100006763>To verify compliance with the PSA facilities regulations § 62 and NMA Regulations No. 878 in addition to IMO instruments and Class requirements, as applicable.</rdl:PCA_100006763>
    <skos:broader rdf:resource="http://rds.posccaesar.org/ontology/plm/rdl/PCA_100006741"/>
    <rdl:PCA_100006768>A complete stability analyses model shall be delivered with all necessary information required to perform a re-analysis.</rdl:PCA_100006768>
    <rdl:PCA_100006765 rdf:resource="http://w3id.org/readi/rdl/CFIHOS-20000033"/>
    <rdfs:subClassOf rdf:resource="http://rds.posccaesar.org/ontology/plm/rdl/PCA_100004908"/>
    <rdfs:comment>A complete stability analyses model shall be delivered with all necessary information required to perform a re-analysis.</rdfs:comment>
    <rdfs:label>Stability analysis model</rdfs:label>
  </owl:Class>
  <owl:Class rdf:about="http://rds.posccaesar.org/ontology/plm/rdl/PCA_100006442">
    <rdfs:label>SIT procedure</rdfs:label>
    <rdfs:comment>Procedure outlining detailed steps and acceptance criteria for all tasks in a system integration test (mechanical fit, verify procedures and personnel familiarization).</rdfs:comment>
    <rdl:PCA_100006768>Procedure outlining detailed steps and acceptance criteria for all tasks in a system integration test (mechanical fit, verify procedures and personnel familiarization).</rdl:PCA_100006768>
    <skos:broader rdf:resource="http://rds.posccaesar.org/ontology/plm/rdl/PCA_100006751"/>
    <rdl:PCA_100006763>Provide a step by step procedure and acceptance criteria which will enable user to complete all steps of SIT in logical order.</rdl:PCA_100006763>
    <rdl:PCA_100006765 rdf:resource="http://w3id.org/readi/rdl/CFIHOS-20000031"/>
    <skos:broadMatch rdf:resource="http://rds.posccaesar.org/ontology/plm/rdl/PCA_100006688"/>
    <rdl:PCA_100006766 rdf:resource="http://rds.posccaesar.org/ontology/plm/rdl/PCA_100006657"/>
    <rdfs:subClassOf rdf:resource="http://rds.posccaesar.org/ontology/plm/rdl/PCA_100004908"/>
  </owl:Class>
  <owl:Class rdf:about="http://rds.posccaesar.org/ontology/plm/rdl/PCA_100006321">
    <rdl:PCA_100006768>Identify materials proposed used and document fluid compatibility for material selected.</rdl:PCA_100006768>
    <rdl:PCA_100006766 rdf:resource="http://rds.posccaesar.org/ontology/plm/rdl/PCA_100006653"/>
    <rdl:PCA_100006763>Summarise materials selected for the various components and their compatibility with fluids. List containing main materials of an assembly with reference to part, serial and batch numbers. List shall contain references to material certificate, heat treatment batch / report and NDT reports where applicable. Mostly used for pressure containing equipment and load bearing elements.</rdl:PCA_100006763>
    <skos:broadMatch rdf:resource="http://rds.posccaesar.org/ontology/plm/rdl/PCA_100006715"/>
    <skos:broader rdf:resource="http://rds.posccaesar.org/ontology/plm/rdl/PCA_100006756"/>
    <rdl:PCA_100006765 rdf:resource="http://w3id.org/readi/rdl/CFIHOS-20000027"/>
    <rdfs:subClassOf rdf:resource="http://rds.posccaesar.org/ontology/plm/rdl/PCA_100004908"/>
    <rdfs:label>Material traceability report</rdfs:label>
    <rdfs:comment>Identify materials proposed used and document fluid compatibility for material selected.</rdfs:comment>
    <skos:broadMatch rdf:resource="http://rds.posccaesar.org/ontology/plm/rdl/PCA_100006716"/>
  </owl:Class>
  <owl:Class rdf:about="http://rds.posccaesar.org/ontology/plm/rdl/PCA_100006430">
    <skos:broadMatch rdf:resource="http://rds.posccaesar.org/ontology/plm/rdl/PCA_100006712"/>
    <skos:broader rdf:resource="http://rds.posccaesar.org/ontology/plm/rdl/PCA_100006746"/>
    <skos:broadMatch rdf:resource="http://rds.posccaesar.org/ontology/plm/rdl/PCA_100006713"/>
    <rdl:PCA_100006763>This document shall provide Electrical/Electronic/Pneumatic/Hydraulic functionality  information e.g. to provide hook-up information and  component details for e.g. modifications/replacement.</rdl:PCA_100006763>
    <rdfs:subClassOf rdf:resource="http://rds.posccaesar.org/ontology/plm/rdl/PCA_100004908"/>
    <rdl:PCA_100006768>To be prepared for valve assemblies with instrumentation, and control panels. All components and interconnection between units to be identified. External connections and interfaces shall be identified with type and size.</rdl:PCA_100006768>
    <rdl:PCA_100006766 rdf:resource="http://rds.posccaesar.org/ontology/plm/rdl/PCA_100006653"/>
    <rdfs:comment>To be prepared for valve assemblies with instrumentation, and control panels. All components and interconnection between units to be identified. External connections and interfaces shall be identified with type and size.</rdfs:comment>
    <skos:broader>
      <rdl:PCA_100001503 rdf:about="http://rds.posccaesar.org/ontology/plm/rdl/PCA_100006744">
        <rdfs:label>Connection</rdfs:label>
        <rdl:PCA_100004924>CO</rdl:PCA_100004924>
        <rdf:type rdf:resource="http://www.w3.org/2002/07/owl#NamedIndividual"/>
      </rdl:PCA_100001503>
    </skos:broader>
    <rdfs:label>Schematics including hook-up information</rdfs:label>
  </owl:Class>
  <owl:Class rdf:about="http://rds.posccaesar.org/ontology/plm/rdl/PCA_100006203">
    <rdl:PCA_100006768>Basis for analysis, assumptions and assessments not given in design basis shall be included.</rdl:PCA_100006768>
    <rdl:PCA_100006766 rdf:resource="http://rds.posccaesar.org/ontology/plm/rdl/PCA_100006654"/>
    <rdfs:label>Fatigue service life design report</rdfs:label>
    <skos:broader rdf:resource="http://rds.posccaesar.org/ontology/plm/rdl/PCA_100006756"/>
    <skos:broadMatch rdf:resource="http://rds.posccaesar.org/ontology/plm/rdl/PCA_100006686"/>
    <rdfs:comment>Basis for analysis, assumptions and assessments not given in design basis shall be included.</rdfs:comment>
    <rdl:PCA_100006765 rdf:resource="http://w3id.org/readi/rdl/CFIHOS-20000018"/>
    <rdfs:subClassOf rdf:resource="http://rds.posccaesar.org/ontology/plm/rdl/PCA_100004908"/>
    <rdl:PCA_100006763>Design report describing the fatigue analysis and the fatigue service life for the pipeline.</rdl:PCA_100006763>
  </owl:Class>
  <owl:Class rdf:about="http://rds.posccaesar.org/ontology/plm/rdl/PCA_100006215">
    <rdfs:subClassOf rdf:resource="http://rds.posccaesar.org/ontology/plm/rdl/PCA_100004908"/>
    <skos:broadMatch rdf:resource="http://rds.posccaesar.org/ontology/plm/rdl/PCA_100006687"/>
    <rdl:PCA_100006766 rdf:resource="http://rds.posccaesar.org/ontology/plm/rdl/PCA_100006587"/>
    <rdl:PCA_100006766 rdf:resource="http://rds.posccaesar.org/ontology/plm/rdl/PCA_100006591"/>
    <rdl:PCA_100006763>All physical dimensions and parameters which will affect the measurement result shall have documented traceability to international standards.</rdl:PCA_100006763>
    <rdl:PCA_100006765 rdf:resource="http://w3id.org/readi/rdl/CFIHOS-20000015"/>
    <skos:broader rdf:resource="http://rds.posccaesar.org/ontology/plm/rdl/PCA_100006756"/>
    <skos:broader rdf:resource="http://rds.posccaesar.org/ontology/plm/rdl/PCA_100006741"/>
    <rdfs:label>Fiscal metering - Configuration parameters</rdfs:label>
    <rdl:PCA_100006764>Document providing such traceability shall be provided.</rdl:PCA_100006764>
  </owl:Class>
  <owl:Class rdf:about="http://rds.posccaesar.org/ontology/plm/rdl/PCA_100006106">
    <rdfs:label>Bill of material (BOM)</rdfs:label>
    <skos:broadMatch rdf:resource="http://rds.posccaesar.org/ontology/plm/rdl/PCA_100006715"/>
    <rdfs:comment>Provide purchase information on key parts of an assembly. Gives reference to sub-level parts. The BOM is used as part of the documents for manufacturing and accompanies the assembly drawings.</rdfs:comment>
    <rdl:PCA_100006765 rdf:resource="http://w3id.org/readi/rdl/CFIHOS-20000031"/>
    <skos:broader rdf:resource="http://rds.posccaesar.org/ontology/plm/rdl/PCA_100006748"/>
    <rdl:PCA_100006766 rdf:resource="http://rds.posccaesar.org/ontology/plm/rdl/PCA_100006653"/>
    <rdfs:subClassOf rdf:resource="http://rds.posccaesar.org/ontology/plm/rdl/PCA_100004908"/>
    <rdl:PCA_100006763>A list of parts, components and sub-assemblies for equipment with part numbers, item numbers, quantities, material designations and references to specifications.</rdl:PCA_100006763>
    <rdl:PCA_100006768>Provide purchase information on key parts of an assembly. Gives reference to sub-level parts. The BOM is used as part of the documents for manufacturing and accompanies the assembly drawings.</rdl:PCA_100006768>
  </owl:Class>
  <owl:Class rdf:about="http://rds.posccaesar.org/ontology/plm/rdl/PCA_100006227">
    <skos:broader rdf:resource="http://rds.posccaesar.org/ontology/plm/rdl/PCA_100006746"/>
    <skos:broadMatch rdf:resource="http://rds.posccaesar.org/ontology/plm/rdl/PCA_100006731"/>
    <rdfs:label>Footprint drawing flexible risers</rdfs:label>
    <rdfs:comment>Drawing showing the footprint of the flexible risers on the seabed in normal and accidental situations.</rdfs:comment>
    <rdl:PCA_100006768>Drawing showing the footprint of the flexible risers on the seabed in normal and accidental situations.</rdl:PCA_100006768>
    <rdl:PCA_100006766 rdf:resource="http://rds.posccaesar.org/ontology/plm/rdl/PCA_100006654"/>
    <rdl:PCA_100006765 rdf:resource="http://w3id.org/readi/rdl/CFIHOS-20000018"/>
    <rdfs:subClassOf rdf:resource="http://rds.posccaesar.org/ontology/plm/rdl/PCA_100004908"/>
  </owl:Class>
  <owl:Class rdf:about="http://rds.posccaesar.org/ontology/plm/rdl/PCA_100006118">
    <rdl:PCA_100006768>One document shall cover the complete contract/purchase order.</rdl:PCA_100006768>
    <rdfs:comment>One document shall cover the complete contract/purchase order.</rdfs:comment>
    <rdl:PCA_100006766 rdf:resource="http://rds.posccaesar.org/ontology/plm/rdl/PCA_100006640"/>
    <rdl:PCA_100006766 rdf:resource="http://rds.posccaesar.org/ontology/plm/rdl/PCA_100006638"/>
    <rdl:PCA_100006766 rdf:resource="http://rds.posccaesar.org/ontology/plm/rdl/PCA_100006635"/>
    <rdfs:label>Certificate of conformance</rdfs:label>
    <skos:broader rdf:resource="http://rds.posccaesar.org/ontology/plm/rdl/PCA_100006743"/>
    <rdl:PCA_100006765 rdf:resource="http://w3id.org/readi/rdl/CFIHOS-20000031"/>
    <rdl:PCA_100006766 rdf:resource="http://rds.posccaesar.org/ontology/plm/rdl/PCA_100006636"/>
    <rdl:PCA_100006766 rdf:resource="http://rds.posccaesar.org/ontology/plm/rdl/PCA_100006634"/>
    <rdl:PCA_100006766 rdf:resource="http://rds.posccaesar.org/ontology/plm/rdl/PCA_100006639"/>
    <rdfs:subClassOf rdf:resource="http://rds.posccaesar.org/ontology/plm/rdl/PCA_100004908"/>
    <skos:broadMatch rdf:resource="http://rds.posccaesar.org/ontology/plm/rdl/PCA_100006722"/>
    <rdl:PCA_100006763>A Certificate where Contractor/supplier confirms/verifies that the requirements in the contract/purchase order for design, calculations, production, testing and traceability requirements have been met;</rdl:PCA_100006763>
    <rdl:PCA_100006766 rdf:resource="http://rds.posccaesar.org/ontology/plm/rdl/PCA_100006642"/>
    <rdl:PCA_100006766 rdf:resource="http://rds.posccaesar.org/ontology/plm/rdl/PCA_100006641"/>
    <rdl:PCA_100006765 rdf:resource="http://w3id.org/readi/rdl/CFIHOS-20000008"/>
    <rdl:PCA_100006766 rdf:resource="http://rds.posccaesar.org/ontology/plm/rdl/PCA_100006637"/>
  </owl:Class>
  <owl:Class rdf:about="http://rds.posccaesar.org/ontology/plm/rdl/PCA_100006249">
    <skos:broadMatch rdf:resource="http://rds.posccaesar.org/ontology/plm/rdl/PCA_100006688"/>
    <rdfs:subClassOf rdf:resource="http://rds.posccaesar.org/ontology/plm/rdl/PCA_100004908"/>
    <rdl:PCA_100006765 rdf:resource="http://w3id.org/readi/rdl/CFIHOS-20000031"/>
    <rdl:PCA_100006766 rdf:resource="http://rds.posccaesar.org/ontology/plm/rdl/PCA_100006653"/>
    <skos:broader rdf:resource="http://rds.posccaesar.org/ontology/plm/rdl/PCA_100006751"/>
    <rdl:PCA_100006763>Provide a clear procedure to heat treat shop to ensure repeatability.</rdl:PCA_100006763>
    <rdfs:label>Heat treatment procedure</rdfs:label>
    <rdl:PCA_100006768>Document specifying heating and cooling procedures to obtain specified conditions or properties.</rdl:PCA_100006768>
    <rdfs:comment>Document specifying heating and cooling procedures to obtain specified conditions or properties.</rdfs:comment>
  </owl:Class>
  <owl:Class rdf:about="http://rds.posccaesar.org/ontology/plm/rdl/PCA_100006479">
    <rdl:PCA_100006766 rdf:resource="http://rds.posccaesar.org/ontology/plm/rdl/PCA_100006587"/>
    <rdl:PCA_100006766 rdf:resource="http://rds.posccaesar.org/ontology/plm/rdl/PCA_100006586"/>
    <rdl:PCA_100006766 rdf:resource="http://rds.posccaesar.org/ontology/plm/rdl/PCA_100006619"/>
    <rdl:PCA_100006766 rdf:resource="http://rds.posccaesar.org/ontology/plm/rdl/PCA_100006606"/>
    <skos:broadMatch rdf:resource="http://rds.posccaesar.org/ontology/plm/rdl/PCA_100006695"/>
    <rdl:PCA_100006766 rdf:resource="http://rds.posccaesar.org/ontology/plm/rdl/PCA_100006609"/>
    <rdl:PCA_100006766 rdf:resource="http://rds.posccaesar.org/ontology/plm/rdl/PCA_100006611"/>
    <skos:broader rdf:resource="http://rds.posccaesar.org/ontology/plm/rdl/PCA_100006745"/>
    <rdl:PCA_100006766 rdf:resource="http://rds.posccaesar.org/ontology/plm/rdl/PCA_100006621"/>
    <rdl:PCA_100006766 rdf:resource="http://rds.posccaesar.org/ontology/plm/rdl/PCA_100006591"/>
    <rdl:PCA_100006766 rdf:resource="http://rds.posccaesar.org/ontology/plm/rdl/PCA_100006614"/>
    <rdl:PCA_100006766 rdf:resource="http://rds.posccaesar.org/ontology/plm/rdl/PCA_100006613"/>
    <rdl:PCA_100006766 rdf:resource="http://rds.posccaesar.org/ontology/plm/rdl/PCA_100006601"/>
    <rdl:PCA_100006766 rdf:resource="http://rds.posccaesar.org/ontology/plm/rdl/PCA_100006598"/>
    <rdl:PCA_100006766 rdf:resource="http://rds.posccaesar.org/ontology/plm/rdl/PCA_100006627"/>
    <rdl:PCA_100006766 rdf:resource="http://rds.posccaesar.org/ontology/plm/rdl/PCA_100006581"/>
    <rdl:PCA_100006766 rdf:resource="http://rds.posccaesar.org/ontology/plm/rdl/PCA_100006604"/>
    <rdl:PCA_100006766 rdf:resource="http://rds.posccaesar.org/ontology/plm/rdl/PCA_100006597"/>
    <rdl:PCA_100006766 rdf:resource="http://rds.posccaesar.org/ontology/plm/rdl/PCA_100006578"/>
    <rdl:PCA_100006766 rdf:resource="http://rds.posccaesar.org/ontology/plm/rdl/PCA_100006596"/>
    <rdl:PCA_100006766 rdf:resource="http://rds.posccaesar.org/ontology/plm/rdl/PCA_100006617"/>
    <rdl:PCA_100006766 rdf:resource="http://rds.posccaesar.org/ontology/plm/rdl/PCA_100006588"/>
    <rdfs:subClassOf rdf:resource="http://rds.posccaesar.org/ontology/plm/rdl/PCA_100004908"/>
    <rdl:PCA_100006766 rdf:resource="http://rds.posccaesar.org/ontology/plm/rdl/PCA_100006583"/>
    <rdl:PCA_100006766 rdf:resource="http://rds.posccaesar.org/ontology/plm/rdl/PCA_100006607"/>
    <rdl:PCA_100006763>System Control Diagram shall be used to specify and document process control and process shutdown application within the control systems.

The method consists in principle of two parts.

(1) Use of a defined set of function blocks, and
(2) a diagram representation of usage of these function blocks and its interconnections.

The diagram has a presentation of the process as background. The content of multiple P&amp;ID’s is simplified and combined into the SCD’s as the control and shutdown logic is laid out there.

System Control Diagrams shall be in accordance with the standard referred to in IEC 63131.

The SCD standard also covers sequential control.</rdl:PCA_100006763>
    <rdl:PCA_100006766 rdf:resource="http://rds.posccaesar.org/ontology/plm/rdl/PCA_100006612"/>
    <rdfs:comment>Main components of a sequence are:
 - Steps with associated actions;
 - Transitions with associated logic conditions;
 - Directed links between steps and transitions.

The sequential function chart may be presented on separate pages to avoid cluttering the main SCD. 

The SCD’s shall be made per process system and supported by a functional specification.</rdfs:comment>
    <rdl:PCA_100006766 rdf:resource="http://rds.posccaesar.org/ontology/plm/rdl/PCA_100006622"/>
    <rdl:PCA_100006766 rdf:resource="http://rds.posccaesar.org/ontology/plm/rdl/PCA_100006592"/>
    <rdl:PCA_100006766 rdf:resource="http://rds.posccaesar.org/ontology/plm/rdl/PCA_100006615"/>
    <rdl:PCA_100006766 rdf:resource="http://rds.posccaesar.org/ontology/plm/rdl/PCA_100006602"/>
    <rdl:PCA_100006766 rdf:resource="http://rds.posccaesar.org/ontology/plm/rdl/PCA_100006624"/>
    <rdl:PCA_100006766 rdf:resource="http://rds.posccaesar.org/ontology/plm/rdl/PCA_100006599"/>
    <rdl:PCA_100006766 rdf:resource="http://rds.posccaesar.org/ontology/plm/rdl/PCA_100006594"/>
    <rdl:PCA_100006766 rdf:resource="http://rds.posccaesar.org/ontology/plm/rdl/PCA_100006582"/>
    <rdl:PCA_100006766 rdf:resource="http://rds.posccaesar.org/ontology/plm/rdl/PCA_100006605"/>
    <rdl:PCA_100006766 rdf:resource="http://rds.posccaesar.org/ontology/plm/rdl/PCA_100006579"/>
    <rdl:PCA_100006766 rdf:resource="http://rds.posccaesar.org/ontology/plm/rdl/PCA_100006585"/>
    <rdl:PCA_100006766 rdf:resource="http://rds.posccaesar.org/ontology/plm/rdl/PCA_100006618"/>
    <rdl:PCA_100006766 rdf:resource="http://rds.posccaesar.org/ontology/plm/rdl/PCA_100006589"/>
    <rdl:PCA_100006766 rdf:resource="http://rds.posccaesar.org/ontology/plm/rdl/PCA_100006584"/>
    <rdl:PCA_100006766 rdf:resource="http://rds.posccaesar.org/ontology/plm/rdl/PCA_100006628"/>
    <rdl:PCA_100006766 rdf:resource="http://rds.posccaesar.org/ontology/plm/rdl/PCA_100006633"/>
    <rdl:PCA_100006766 rdf:resource="http://rds.posccaesar.org/ontology/plm/rdl/PCA_100006608"/>
    <rdl:PCA_100006766 rdf:resource="http://rds.posccaesar.org/ontology/plm/rdl/PCA_100006610"/>
    <rdl:PCA_100006768>Main components of a sequence are:
 - Steps with associated actions;
 - Transitions with associated logic conditions;
 - Directed links between steps and transitions.

The sequential function chart may be presented on separate pages to avoid cluttering the main SCD. 

The SCD’s shall be made per process system and supported by a functional specification.</rdl:PCA_100006768>
    <rdl:PCA_100006766 rdf:resource="http://rds.posccaesar.org/ontology/plm/rdl/PCA_100006620"/>
    <rdl:PCA_100006766 rdf:resource="http://rds.posccaesar.org/ontology/plm/rdl/PCA_100006590"/>
    <rdfs:label>System control diagram (SCD)</rdfs:label>
    <rdl:PCA_100006766 rdf:resource="http://rds.posccaesar.org/ontology/plm/rdl/PCA_100006623"/>
    <rdl:PCA_100006766 rdf:resource="http://rds.posccaesar.org/ontology/plm/rdl/PCA_100006600"/>
    <rdl:PCA_100006766 rdf:resource="http://rds.posccaesar.org/ontology/plm/rdl/PCA_100006593"/>
    <rdl:PCA_100006766 rdf:resource="http://rds.posccaesar.org/ontology/plm/rdl/PCA_100006616"/>
    <rdl:PCA_100006766 rdf:resource="http://rds.posccaesar.org/ontology/plm/rdl/PCA_100006626"/>
    <rdl:PCA_100006766 rdf:resource="http://rds.posccaesar.org/ontology/plm/rdl/PCA_100006580"/>
    <rdl:PCA_100006766 rdf:resource="http://rds.posccaesar.org/ontology/plm/rdl/PCA_100006603"/>
    <rdl:PCA_100006765 rdf:resource="http://w3id.org/readi/rdl/CFIHOS-20000015"/>
    <rdl:PCA_100006766 rdf:resource="http://rds.posccaesar.org/ontology/plm/rdl/PCA_100006625"/>
    <rdl:PCA_100006766 rdf:resource="http://rds.posccaesar.org/ontology/plm/rdl/PCA_100006595"/>
  </owl:Class>
  <owl:Class rdf:about="http://rds.posccaesar.org/ontology/plm/rdl/PCA_100006358">
    <skos:broader rdf:resource="http://rds.posccaesar.org/ontology/plm/rdl/PCA_100006748"/>
    <skos:broadMatch rdf:resource="http://rds.posccaesar.org/ontology/plm/rdl/PCA_100006716"/>
    <rdfs:label>Part list</rdfs:label>
    <rdfs:comment>Mandatory content of information:
For each list item:
 - Item reference number
 - Quantity
 - Part number or global identifier (together with manufacturer / supplier)
 - Part name.

Optional content of information:
For each list item:
 - List of reference designations
 - Type designation
 - Specifying technical data
 - Descriptive technical data
 - Mass, dimensions
 - Reference to document
 - Remark.</rdfs:comment>
    <rdl:PCA_100006768>Mandatory content of information:
For each list item:
 - Item reference number
 - Quantity
 - Part number or global identifier (together with manufacturer / supplier)
 - Part name.

Optional content of information:
For each list item:
 - List of reference designations
 - Type designation
 - Specifying technical data
 - Descriptive technical data
 - Mass, dimensions
 - Reference to document
 - Remark.</rdl:PCA_100006768>
    <rdl:PCA_100006766 rdf:resource="http://rds.posccaesar.org/ontology/plm/rdl/PCA_100006653"/>
    <rdl:PCA_100006763>List for an object containing list items specifying the sub-objects in the product aspect (parts, components, software, equipment, etc.) that constitute an assembly (or sub-assembly) or system and, if necessary, reference documents.

NOTE - Class A indicates that each list item represents a type of constituent object and specifies the quantity of this.</rdl:PCA_100006763>
    <rdfs:subClassOf rdf:resource="http://rds.posccaesar.org/ontology/plm/rdl/PCA_100004908"/>
  </owl:Class>
  <owl:Class rdf:about="http://rds.posccaesar.org/ontology/plm/rdl/PCA_100006237">
    <skos:broader rdf:resource="http://rds.posccaesar.org/ontology/plm/rdl/PCA_100006739"/>
    <skos:broadMatch rdf:resource="http://rds.posccaesar.org/ontology/plm/rdl/PCA_100006710"/>
    <skos:broadMatch rdf:resource="http://rds.posccaesar.org/ontology/plm/rdl/PCA_100006708"/>
    <rdfs:label>General arrangement drawing (subsea)</rdfs:label>
    <rdfs:comment>The manufacturer's standard general arrangement drawing shall be delivered.</rdfs:comment>
    <rdl:PCA_100006768>The manufacturer's standard general arrangement drawing shall be delivered.</rdl:PCA_100006768>
    <rdl:PCA_100006765 rdf:resource="http://w3id.org/readi/rdl/CFIHOS-20000031"/>
    <rdfs:subClassOf rdf:resource="http://rds.posccaesar.org/ontology/plm/rdl/PCA_100004908"/>
  </owl:Class>
  <owl:Class rdf:about="http://rds.posccaesar.org/ontology/plm/rdl/PCA_100006346">
    <skos:broadMatch rdf:resource="http://rds.posccaesar.org/ontology/plm/rdl/PCA_100006731"/>
    <rdfs:label>OLGA as laid models</rdfs:label>
    <rdfs:comment>including PVT file updated with as laid pipeline profile to DG4.</rdfs:comment>
    <rdl:PCA_100006768>including PVT file updated with as laid pipeline profile to DG4.</rdl:PCA_100006768>
    <rdl:PCA_100006766 rdf:resource="http://rds.posccaesar.org/ontology/plm/rdl/PCA_100006657"/>
    <rdl:PCA_100006765 rdf:resource="http://w3id.org/readi/rdl/CFIHOS-20000018"/>
    <rdfs:subClassOf rdf:resource="http://rds.posccaesar.org/ontology/plm/rdl/PCA_100004908"/>
  </owl:Class>
  <owl:Class rdf:about="http://rds.posccaesar.org/ontology/plm/rdl/PCA_100006467">
    <rdfs:comment>Drawings shall include the following minimum information:
 - Extent and thickness of fireproofing, including description of coating/paint for fire protection systems;
 - Structural details related to the fire protection;
 - Material properties.</rdfs:comment>
    <skos:broadMatch rdf:resource="http://rds.posccaesar.org/ontology/plm/rdl/PCA_100006734"/>
    <skos:broadMatch rdf:resource="http://rds.posccaesar.org/ontology/plm/rdl/PCA_100006727"/>
    <skos:broadMatch rdf:resource="http://rds.posccaesar.org/ontology/plm/rdl/PCA_100006733"/>
    <skos:broader rdf:resource="http://rds.posccaesar.org/ontology/plm/rdl/PCA_100006746"/>
    <skos:broadMatch rdf:resource="http://rds.posccaesar.org/ontology/plm/rdl/PCA_100006731"/>
    <rdfs:subClassOf rdf:resource="http://rds.posccaesar.org/ontology/plm/rdl/PCA_100004908"/>
    <rdfs:label>Structural steel fire protection drawings (civil)</rdfs:label>
    <skos:broadMatch rdf:resource="http://rds.posccaesar.org/ontology/plm/rdl/PCA_100006732"/>
    <rdl:PCA_100006766 rdf:resource="http://rds.posccaesar.org/ontology/plm/rdl/PCA_100006656"/>
    <rdl:PCA_100006765 rdf:resource="http://w3id.org/readi/rdl/CFIHOS-20000007"/>
    <rdl:PCA_100006768>Drawings shall include the following minimum information:
 - Extent and thickness of fireproofing, including description of coating/paint for fire protection systems;
 - Structural details related to the fire protection;
 - Material properties.</rdl:PCA_100006768>
  </owl:Class>
  <owl:Class rdf:about="http://rds.posccaesar.org/ontology/plm/rdl/PCA_100006455">
    <rdl:PCA_100006766 rdf:resource="http://rds.posccaesar.org/ontology/plm/rdl/PCA_100006654"/>
    <skos:broader rdf:resource="http://rds.posccaesar.org/ontology/plm/rdl/PCA_100006756"/>
    <rdl:PCA_100006763>The report or collection of reports shall contain the final documentation of intact and damaged stability.</rdl:PCA_100006763>
    <skos:broadMatch rdf:resource="http://rds.posccaesar.org/ontology/plm/rdl/PCA_100006698"/>
    <rdfs:subClassOf rdf:resource="http://rds.posccaesar.org/ontology/plm/rdl/PCA_100004908"/>
    <skos:broadMatch rdf:resource="http://rds.posccaesar.org/ontology/plm/rdl/PCA_100006691"/>
    <rdfs:label>Stability design reports</rdfs:label>
    <rdl:PCA_100006765 rdf:resource="http://w3id.org/readi/rdl/CFIHOS-20000033"/>
    <rdfs:comment>The report shall typically contain:
 - Vessel particulars and geometrical reference system;
 - Description of watertight integrity and tank arrangement;
 - Lightship weight / weight information;
 - External openings;
 - Densities of liquids in tanks;
 - Applied computer programs;
 - Applicable stability regulations/criteria;
 - Summary of loading conditions;
 - Summary of stability and strength results;
 - Allowable KG limit curves;
 - Hydrostatic table(s);
 - Intact stability documentation;
 - Damage stability documentation.</rdfs:comment>
    <rdl:PCA_100006768>The report shall typically contain:
 - Vessel particulars and geometrical reference system;
 - Description of watertight integrity and tank arrangement;
 - Lightship weight / weight information;
 - External openings;
 - Densities of liquids in tanks;
 - Applied computer programs;
 - Applicable stability regulations/criteria;
 - Summary of loading conditions;
 - Summary of stability and strength results;
 - Allowable KG limit curves;
 - Hydrostatic table(s);
 - Intact stability documentation;
 - Damage stability documentation.</rdl:PCA_100006768>
  </owl:Class>
  <owl:Class rdf:about="http://rds.posccaesar.org/ontology/plm/rdl/PCA_100006334">
    <rdfs:label>NDT operator certificates</rdfs:label>
    <rdl:PCA_100006768>Official certificates for operators performing NDT. NDT certificates are issued per method in e.g. UT, MT, PT, RT, ET and VT at three different levels.</rdl:PCA_100006768>
    <rdl:PCA_100006763>Document that the NDT operator has the necessary qualifications for the relevant NDT method.</rdl:PCA_100006763>
    <rdl:PCA_100006765 rdf:resource="http://w3id.org/readi/rdl/CFIHOS-20000031"/>
    <rdfs:comment>Official certificates for operators performing NDT. NDT certificates are issued per method in e.g. UT, MT, PT, RT, ET and VT at three different levels.</rdfs:comment>
    <skos:broadMatch rdf:resource="http://rds.posccaesar.org/ontology/plm/rdl/PCA_100006722"/>
    <rdfs:subClassOf rdf:resource="http://rds.posccaesar.org/ontology/plm/rdl/PCA_100004908"/>
    <rdl:PCA_100006766 rdf:resource="http://rds.posccaesar.org/ontology/plm/rdl/PCA_100006653"/>
    <skos:broader rdf:resource="http://rds.posccaesar.org/ontology/plm/rdl/PCA_100006743"/>
  </owl:Class>
  <owl:Class rdf:about="http://rds.posccaesar.org/ontology/plm/rdl/PCA_100006322">
    <skos:broader rdf:resource="http://rds.posccaesar.org/ontology/plm/rdl/PCA_100006748"/>
    <skos:broadMatch rdf:resource="http://rds.posccaesar.org/ontology/plm/rdl/PCA_100006716"/>
    <skos:broadMatch rdf:resource="http://rds.posccaesar.org/ontology/plm/rdl/PCA_100006702"/>
    <rdfs:label>MCB/fuse schedule</rdfs:label>
    <rdfs:comment>A circuit distribution schedule shall be provided inside each panel. This schedule shall include both circuits for internal control voltage and circuits for external consumers.</rdfs:comment>
    <rdl:PCA_100006768>A circuit distribution schedule shall be provided inside each panel. This schedule shall include both circuits for internal control voltage and circuits for external consumers.</rdl:PCA_100006768>
    <rdfs:subClassOf rdf:resource="http://rds.posccaesar.org/ontology/plm/rdl/PCA_100004908"/>
  </owl:Class>
  <owl:Class rdf:about="http://rds.posccaesar.org/ontology/plm/rdl/PCA_100006443">
    <skos:broader rdf:resource="http://rds.posccaesar.org/ontology/plm/rdl/PCA_100006756"/>
    <rdfs:label>SIT report</rdfs:label>
    <rdfs:comment>The System Integration Testing (SIT) shall document and verify that acceptance testing has been performed in accordance with defined requirements and that these has been met successfully.</rdfs:comment>
    <rdl:PCA_100006768>The System Integration Testing (SIT) shall document and verify that acceptance testing has been performed in accordance with defined requirements and that these has been met successfully.</rdl:PCA_100006768>
    <rdl:PCA_100006766 rdf:resource="http://rds.posccaesar.org/ontology/plm/rdl/PCA_100006657"/>
    <rdl:PCA_100006765 rdf:resource="http://w3id.org/readi/rdl/CFIHOS-20000031"/>
    <rdl:PCA_100006763>Document results of SIT.</rdl:PCA_100006763>
    <rdfs:subClassOf rdf:resource="http://rds.posccaesar.org/ontology/plm/rdl/PCA_100004908"/>
  </owl:Class>
  <owl:Class rdf:about="http://rds.posccaesar.org/ontology/plm/rdl/PCA_100006431">
    <skos:broader rdf:resource="http://rds.posccaesar.org/ontology/plm/rdl/PCA_100006748"/>
    <rdfs:label>Scope of supply</rdfs:label>
    <rdfs:comment>An illustration providing holistic understanding of equipment, listing quantity and type</rdfs:comment>
    <rdl:PCA_100006768>An illustration providing holistic understanding of equipment, listing quantity and type</rdl:PCA_100006768>
    <rdl:PCA_100006766 rdf:resource="http://rds.posccaesar.org/ontology/plm/rdl/PCA_100006653"/>
    <rdl:PCA_100006765 rdf:resource="http://w3id.org/readi/rdl/CFIHOS-20000031"/>
    <rdl:PCA_100006763>A drawing showing equipment and tools supplied including part numbers.</rdl:PCA_100006763>
    <rdfs:subClassOf rdf:resource="http://rds.posccaesar.org/ontology/plm/rdl/PCA_100004908"/>
  </owl:Class>
  <owl:Class rdf:about="http://rds.posccaesar.org/ontology/plm/rdl/PCA_100006310">
    <rdl:PCA_100006765 rdf:resource="http://w3id.org/readi/rdl/CFIHOS-20000020"/>
    <skos:broader rdf:resource="http://rds.posccaesar.org/ontology/plm/rdl/PCA_100006756"/>
    <rdl:PCA_100006768>If the documentation normally contained in MRB is issued separately, a reference to such documents is sufficient in the MRB.

MRB requirements:
 - The manufacturer's standard MRB shall be delivered.
 - If additional documents required by Company, then they should be submitted as separate deliverables.

&lt;Please see Word-document for table/akva&gt;

Any of the sections that are not applicable shall be marked “N/A”. The structure and the numbering shall remain as shown above.

Note:

Section 1: The MRB sections shall be delivered as one document (ref SR-15819 - PDF). Each section can be delivered as separate files, named "Doc. No.-sectionx"
(Dxxx-xx-...-section1.pdf, Dxxx-xx-…-section9.xlsx, Dxxx-xx-…-section9.pdf, etc).

Section 4 and 9: Reference to SPTS in the MDR index

Section 3: Shall as a minimum refer to Company requirements contained in latest revision of the following documents:
 - Applicable Frame Agreement and purchase order
 - Applicable Specifications, Project-specific Material Data Sheet (PMDS) and Technical Changes (TC)
 - Reference standard (if specified: DNVGL-ST-F101, including amendments and corrections
 - Applicable SPTS specifications</rdl:PCA_100006768>
    <rdl:PCA_100006765 rdf:resource="http://w3id.org/readi/rdl/CFIHOS-20000031"/>
    <rdfs:comment>If the documentation normally contained in MRB is issued separately, a reference to such documents is sufficient in the MRB.

MRB requirements:
 - The manufacturer's standard MRB shall be delivered.
 - If additional documents required by Company, then they should be submitted as separate deliverables.

&lt;Please see Word-document for table/akva&gt;

Any of the sections that are not applicable shall be marked “N/A”. The structure and the numbering shall remain as shown above.

Note:

Section 1: The MRB sections shall be delivered as one document (ref SR-15819 - PDF). Each section can be delivered as separate files, named "Doc. No.-sectionx"
(Dxxx-xx-...-section1.pdf, Dxxx-xx-…-section9.xlsx, Dxxx-xx-…-section9.pdf, etc).

Section 4 and 9: Reference to SPTS in the MDR index

Section 3: Shall as a minimum refer to Company requirements contained in latest revision of the following documents:
 - Applicable Frame Agreement and purchase order
 - Applicable Specifications, Project-specific Material Data Sheet (PMDS) and Technical Changes (TC)
 - Reference standard (if specified: DNVGL-ST-F101, including amendments and corrections
 - Applicable SPTS specifications</rdfs:comment>
    <rdl:PCA_100006763>To demonstrate that the requirements with respect to design, calculation, production, testing and possible specified traceability requirements for materials and fabrication, are fulfilled.</rdl:PCA_100006763>
    <rdfs:subClassOf rdf:resource="http://rds.posccaesar.org/ontology/plm/rdl/PCA_100004908"/>
    <rdl:PCA_100006766 rdf:resource="http://rds.posccaesar.org/ontology/plm/rdl/PCA_100006653"/>
    <skos:broadMatch rdf:resource="http://rds.posccaesar.org/ontology/plm/rdl/PCA_100006722"/>
    <skos:broader rdf:resource="http://rds.posccaesar.org/ontology/plm/rdl/PCA_100006762"/>
    <rdfs:label>Manufacturing record book (MRB) for linepipe</rdfs:label>
  </owl:Class>
  <owl:Class rdf:about="http://rds.posccaesar.org/ontology/plm/rdl/PCA_100006540">
    <skos:broader rdf:resource="http://rds.posccaesar.org/ontology/plm/rdl/PCA_100006756"/>
    <skos:broadMatch rdf:resource="http://rds.posccaesar.org/ontology/plm/rdl/PCA_100006722"/>
    <rdfs:label>Wind tunnel test report</rdfs:label>
    <rdl:PCA_100006766 rdf:resource="http://rds.posccaesar.org/ontology/plm/rdl/PCA_100006653"/>
    <rdl:PCA_100006765 rdf:resource="http://w3id.org/readi/rdl/CFIHOS-20000033"/>
    <rdl:PCA_100006763>The report or collection of reports shall document the wind tunnel test and describe the results of the testing.</rdl:PCA_100006763>
    <rdfs:subClassOf rdf:resource="http://rds.posccaesar.org/ontology/plm/rdl/PCA_100004908"/>
  </owl:Class>
  <owl:Class rdf:about="http://rds.posccaesar.org/ontology/plm/rdl/PCA_100006202">
    <rdfs:subClassOf rdf:resource="http://rds.posccaesar.org/ontology/plm/rdl/PCA_100004908"/>
    <skos:broadMatch rdf:resource="http://rds.posccaesar.org/ontology/plm/rdl/PCA_100006722"/>
    <rdl:PCA_100006763>To document the tests performed in accordance with the procedure.</rdl:PCA_100006763>
    <rdl:PCA_100006764>The Factory Acceptance Test (FAT) shall document and verify that acceptance testing has been performed in accordance with defined requirements and that these has been met successfully. In engineering and its various subdisciplines, acceptance testing is a test conducted to determine if the requirements of a specification or contract are met. It may involve chemical tests, physical tests, or performance tests.</rdl:PCA_100006764>
    <rdfs:comment>Report containing records from the FAT including pressure tests and flushing operations.</rdfs:comment>
    <rdfs:label>FAT report</rdfs:label>
    <rdl:PCA_100006766 rdf:resource="http://rds.posccaesar.org/ontology/plm/rdl/PCA_100006653"/>
    <rdl:PCA_100006768>Report containing records from the FAT including pressure tests and flushing operations.</rdl:PCA_100006768>
    <rdl:PCA_100006765 rdf:resource="http://w3id.org/readi/rdl/CFIHOS-20000031"/>
    <skos:broader rdf:resource="http://rds.posccaesar.org/ontology/plm/rdl/PCA_100006756"/>
  </owl:Class>
  <owl:Class rdf:about="http://rds.posccaesar.org/ontology/plm/rdl/PCA_100006214">
    <skos:broader rdf:resource="http://rds.posccaesar.org/ontology/plm/rdl/PCA_100006743"/>
    <skos:broadMatch rdf:resource="http://rds.posccaesar.org/ontology/plm/rdl/PCA_100006722"/>
    <rdfs:label>Fiscal metering - Calibration certificates</rdfs:label>
    <rdl:PCA_100006765 rdf:resource="http://w3id.org/readi/rdl/CFIHOS-20000015"/>
    <rdl:PCA_100006764>A document containing all calibration certificates for the fiscal metering system shall be provided.</rdl:PCA_100006764>
    <rdfs:subClassOf rdf:resource="http://rds.posccaesar.org/ontology/plm/rdl/PCA_100004908"/>
  </owl:Class>
  <owl:Class rdf:about="http://rds.posccaesar.org/ontology/plm/rdl/PCA_100006226">
    <skos:broadMatch rdf:resource="http://rds.posccaesar.org/ontology/plm/rdl/PCA_100006727"/>
    <skos:broader rdf:resource="http://rds.posccaesar.org/ontology/plm/rdl/PCA_100006756"/>
    <rdfs:label>FMECA report</rdfs:label>
    <rdl:PCA_100006768>The failure mode and effects analysis (FMEA) is a qualitative reliability technique for systematically analysing each possible failure mode for a component, equipment sub-assembly or assembly, and identifying the resulting effect. The criticality analysis (CA) is a quantitative procedure which ranks failure modes according to their probability and consequences (i.e. the resulting effect of the failure mode).</rdl:PCA_100006768>
    <rdl:PCA_100006765 rdf:resource="http://w3id.org/readi/rdl/CFIHOS-20000031"/>
    <rdl:PCA_100006766 rdf:resource="http://rds.posccaesar.org/ontology/plm/rdl/PCA_100006653"/>
    <rdl:PCA_100006763>Identify possible failure modes and criticality for components and equipment assemblies as input to design and qualification program as well as OMM; inspection, maintenance and test plan, and spares program.</rdl:PCA_100006763>
    <rdfs:subClassOf rdf:resource="http://rds.posccaesar.org/ontology/plm/rdl/PCA_100004908"/>
    <rdfs:comment>The failure mode and effects analysis (FMEA) is a qualitative reliability technique for systematically analysing each possible failure mode for a component, equipment sub-assembly or assembly, and identifying the resulting effect. The criticality analysis (CA) is a quantitative procedure which ranks failure modes according to their probability and consequences (i.e. the resulting effect of the failure mode).</rdfs:comment>
  </owl:Class>
  <owl:Class rdf:about="http://rds.posccaesar.org/ontology/plm/rdl/PCA_100006105">
    <skos:broadMatch rdf:resource="http://rds.posccaesar.org/ontology/plm/rdl/PCA_100006722"/>
    <rdfs:label>Bending procedure</rdfs:label>
    <skos:broader rdf:resource="http://rds.posccaesar.org/ontology/plm/rdl/PCA_100006751"/>
    <rdl:PCA_100006763>Quality assurance of the product (incl. dimensions and materials)</rdl:PCA_100006763>
    <rdl:PCA_100006768>Describe parameters for bending, and expected bending results</rdl:PCA_100006768>
    <rdl:PCA_100006765 rdf:resource="http://w3id.org/readi/rdl/CFIHOS-20000027"/>
    <rdl:PCA_100006766 rdf:resource="http://rds.posccaesar.org/ontology/plm/rdl/PCA_100006653"/>
    <rdfs:subClassOf rdf:resource="http://rds.posccaesar.org/ontology/plm/rdl/PCA_100004908"/>
    <rdfs:comment>Describe parameters for bending, and expected bending results</rdfs:comment>
  </owl:Class>
  <owl:Class rdf:about="http://rds.posccaesar.org/ontology/plm/rdl/PCA_100006117">
    <skos:broader rdf:resource="http://rds.posccaesar.org/ontology/plm/rdl/PCA_100006743"/>
    <skos:broadMatch rdf:resource="http://rds.posccaesar.org/ontology/plm/rdl/PCA_100006722"/>
    <rdfs:label>Certificate for use - lifting appliances</rdfs:label>
    <rdl:PCA_100006763>Lifting appliances shall be accompanied by a certificate issued by an enterprise of competence prior to use in accordance with ILO C152 or Annex H of NORSOK R-003, or NORSOK R-005, as applicable.

This also includes manufacturers' ILO based certificates for loose Gear (hooks, hooks block, 
wire, shackles, links, etc.).</rdl:PCA_100006763>
    <rdfs:subClassOf rdf:resource="http://rds.posccaesar.org/ontology/plm/rdl/PCA_100004908"/>
  </owl:Class>
  <owl:Class rdf:about="http://rds.posccaesar.org/ontology/plm/rdl/PCA_100006129">
    <skos:broadMatch rdf:resource="http://rds.posccaesar.org/ontology/plm/rdl/PCA_100006691"/>
    <rdl:PCA_100006765 rdf:resource="http://w3id.org/readi/rdl/CFIHOS-20000007"/>
    <rdl:PCA_100006768>Ref. generic design report</rdl:PCA_100006768>
    <skos:broader rdf:resource="http://rds.posccaesar.org/ontology/plm/rdl/PCA_100006756"/>
    <rdfs:comment>Ref. generic design report</rdfs:comment>
    <rdl:PCA_100006766 rdf:resource="http://rds.posccaesar.org/ontology/plm/rdl/PCA_100006656"/>
    <rdfs:subClassOf rdf:resource="http://rds.posccaesar.org/ontology/plm/rdl/PCA_100004908"/>
    <skos:broadMatch rdf:resource="http://rds.posccaesar.org/ontology/plm/rdl/PCA_100006698"/>
    <rdfs:label>Concrete structural design report</rdfs:label>
    <rdl:PCA_100006764>Structural design reports and input files/parameters shall be delivered. The report or collection of reports shall be self-contained, i.e. provide all information required to reproduce the results.

The static analysis and calculations shall have specific and detailed references to drawings and relevant part of regulations and referenced standards.</rdl:PCA_100006764>
  </owl:Class>
  <owl:Class rdf:about="http://rds.posccaesar.org/ontology/plm/rdl/PCA_100006399">
    <rdfs:comment>A structured data form containing part number/model, design information, operational data and limitations of the equipment. Data sheets are only applicable for instruments and valves.</rdfs:comment>
    <rdfs:subClassOf rdf:resource="http://rds.posccaesar.org/ontology/plm/rdl/PCA_100004908"/>
    <rdl:PCA_100006765 rdf:resource="http://w3id.org/readi/rdl/CFIHOS-20000031"/>
    <rdl:PCA_100006768>A structured data form containing part number/model, design information, operational data and limitations of the equipment. Data sheets are only applicable for instruments and valves.</rdl:PCA_100006768>
    <skos:broadMatch rdf:resource="http://rds.posccaesar.org/ontology/plm/rdl/PCA_100006686"/>
    <rdfs:label>Product data sheet</rdfs:label>
    <rdl:PCA_100006766 rdf:resource="http://rds.posccaesar.org/ontology/plm/rdl/PCA_100006653"/>
    <rdl:PCA_100006763>To summarize the equipment’s capacities and limitations.</rdl:PCA_100006763>
    <skos:broader rdf:resource="http://rds.posccaesar.org/ontology/plm/rdl/PCA_100006747"/>
  </owl:Class>
  <owl:Class rdf:about="http://rds.posccaesar.org/ontology/plm/rdl/PCA_100006278">
    <skos:broader rdf:resource="http://rds.posccaesar.org/ontology/plm/rdl/PCA_100006750"/>
    <skos:broadMatch rdf:resource="http://rds.posccaesar.org/ontology/plm/rdl/PCA_100006688"/>
    <rdfs:label>Installation, operation and maintenance instructions</rdfs:label>
    <rdfs:comment>The manufacturer's standard IOM  should be used as far as possible.
This document shall provide sufficient information to install, operate and maintain the equipment.
This document shall also provide sufficient information for troubleshooting.</rdfs:comment>
    <rdl:PCA_100006768>The manufacturer's standard IOM  should be used as far as possible.
This document shall provide sufficient information to install, operate and maintain the equipment.
This document shall also provide sufficient information for troubleshooting.</rdl:PCA_100006768>
    <rdl:PCA_100006766 rdf:resource="http://rds.posccaesar.org/ontology/plm/rdl/PCA_100006653"/>
    <rdl:PCA_100006763>To describe how to install, operate and maintain the equipment in a safe and functionally correct manner according to the specified maintenance philosophy.</rdl:PCA_100006763>
    <rdfs:subClassOf rdf:resource="http://rds.posccaesar.org/ontology/plm/rdl/PCA_100004908"/>
  </owl:Class>
  <owl:Class rdf:about="http://rds.posccaesar.org/ontology/plm/rdl/PCA_100006266">
    <rdl:PCA_100006765 rdf:resource="http://w3id.org/readi/rdl/CFIHOS-20000007"/>
    <skos:broader rdf:resource="http://rds.posccaesar.org/ontology/plm/rdl/PCA_100006741"/>
    <rdl:PCA_100006766 rdf:resource="http://rds.posccaesar.org/ontology/plm/rdl/PCA_100006583"/>
    <rdfs:subClassOf rdf:resource="http://rds.posccaesar.org/ontology/plm/rdl/PCA_100004908"/>
    <rdfs:comment>The calculations shall include:
 - Head loss calculations during normal operation, including definition
 - Head loss calculations during various climatic conditions, such as storm rain, snow melting (if applicable), etc.
 - Variation in sea level if the system has intake or discharge to sea
 - Surge calculations shall be performed for all pump systems</rdfs:comment>
    <rdl:PCA_100006766 rdf:resource="http://rds.posccaesar.org/ontology/plm/rdl/PCA_100006580"/>
    <rdl:PCA_100006768>The calculations shall include:
 - Head loss calculations during normal operation, including definition
 - Head loss calculations during various climatic conditions, such as storm rain, snow melting (if applicable), etc.
 - Variation in sea level if the system has intake or discharge to sea
 - Surge calculations shall be performed for all pump systems</rdl:PCA_100006768>
    <skos:broadMatch rdf:resource="http://rds.posccaesar.org/ontology/plm/rdl/PCA_100006687"/>
    <rdl:PCA_100006766 rdf:resource="http://rds.posccaesar.org/ontology/plm/rdl/PCA_100006585"/>
    <rdl:PCA_100006766 rdf:resource="http://rds.posccaesar.org/ontology/plm/rdl/PCA_100006616"/>
    <rdl:PCA_100006766 rdf:resource="http://rds.posccaesar.org/ontology/plm/rdl/PCA_100006582"/>
    <rdl:PCA_100006763>Hydraulic system calculation reports and input files/parameters shall be delivered. The report or collection of reports shall be self-contained, i.e. provide all information required to re-produce the results.

Calculations shall include references to basis of design and explanatory text (system description, etc.). All calculations shall be described thoroughly and shown by sketches, inclusive references to third parts equipment (strainers, etc.) calculations, if any.

All hydraulic calculations shall include system characteristics, where normal operation conditions and reserves are analysed and documented. For tunnels, sensitivity calculations shall be made to identify uncertainties in roughness, and tunnel profiles, and presented as above.</rdl:PCA_100006763>
    <rdfs:label>Hydraulic systems calculations for open drain and tunnel systems</rdfs:label>
    <rdl:PCA_100006766 rdf:resource="http://rds.posccaesar.org/ontology/plm/rdl/PCA_100006579"/>
    <rdl:PCA_100006766 rdf:resource="http://rds.posccaesar.org/ontology/plm/rdl/PCA_100006581"/>
    <rdl:PCA_100006766 rdf:resource="http://rds.posccaesar.org/ontology/plm/rdl/PCA_100006584"/>
  </owl:Class>
  <owl:Class rdf:about="http://rds.posccaesar.org/ontology/plm/rdl/PCA_100006387">
    <skos:broader rdf:resource="http://rds.posccaesar.org/ontology/plm/rdl/PCA_100006748"/>
    <rdfs:label>Pre qualified manufacturers list (NORSOK M650)</rdfs:label>
    <rdfs:comment>Suppliers own format. Manufacturer's Qualification Test Record may be required if specified by client

List of Sub-suppliers</rdfs:comment>
    <rdl:PCA_100006768>Suppliers own format. Manufacturer's Qualification Test Record may be required if specified by client

List of Sub-suppliers</rdl:PCA_100006768>
    <rdl:PCA_100006766 rdf:resource="http://rds.posccaesar.org/ontology/plm/rdl/PCA_100006653"/>
    <rdl:PCA_100006763>Verification that the product is manufactured with materials from pre-qualified material suppliers

For use by purchaser</rdl:PCA_100006763>
    <rdfs:subClassOf rdf:resource="http://rds.posccaesar.org/ontology/plm/rdl/PCA_100004908"/>
  </owl:Class>
  <owl:Class rdf:about="http://rds.posccaesar.org/ontology/plm/rdl/PCA_100006375">
    <rdfs:subClassOf rdf:resource="http://rds.posccaesar.org/ontology/plm/rdl/PCA_100004908"/>
    <skos:broadMatch rdf:resource="http://rds.posccaesar.org/ontology/plm/rdl/PCA_100006733"/>
    <skos:broadMatch rdf:resource="http://rds.posccaesar.org/ontology/plm/rdl/PCA_100006722"/>
    <rdfs:label>Piping fabrication records</rdfs:label>
    <rdl:PCA_100006763>FRB User guide - Describes the content of each deliverable in the FRB and how they relate and refer to each other. Include examples (images) of how to trace welds and material certificates from fabrication drawings/ISOs;</rdl:PCA_100006763>
    <rdl:PCA_100006766 rdf:resource="http://rds.posccaesar.org/ontology/plm/rdl/PCA_100006653"/>
    <rdl:PCA_100006768>The following list shows the deliverables and structure of the fabrication records for piping:
 - Index of design drawings with reference to relevant fabrication drawings (Index of design drawings to be delivered in XLS format additionally to PDF);
 - Index of design-, material-, fabrication specifications, documents and data sheets (*);
 - Welding procedure specifications (*);
 - Welding procedure qualification records (*);
 - Repair procedures and specifications (*);
 - Repair and deviation reports. All alternative testing shall be documented with full traceability to the applicable welds;
 - Weld summary index;
 - Material identification system (*);
 - Material certificates (apply for pressurized Piping materials) (*);
 - Pressure test certificates/documentation (*);
 - PMI reports (*);
 - PWHT reports (*);
 - As-built Design Contractor originated design drawings, mark-ups;
 - As-built fabrication drawings/ISOs mark-ups;
 - Third Party verification reports;
 - Procedure for:
    - Tensioning/torqueing of flange stud bolts (*);
    - Flushing and cleaning (*);
    - Hydro testing (*);
    - Hydro flushing of riser- and pipeline valves (*);
    - Pneumatic flushing (*);
    - Pressurised air shock blowing (PAS) (*);
    - Soft Pigging (*);
    - Chemical cleaning (*);
    - Hot oil flushing (*);
    - Internal cleaning of pipe after completed fabrication (*);
    - Bending/flaring (*);
 - Chemical cleaning documentation (*);
 - Hot oil flushing documentation (*).

(*) Can be omitted in modifications if retained by modification Contractor</rdl:PCA_100006768>
    <skos:broader rdf:resource="http://rds.posccaesar.org/ontology/plm/rdl/PCA_100006749"/>
    <rdl:PCA_100006765 rdf:resource="http://w3id.org/readi/rdl/CFIHOS-20000020"/>
    <rdfs:comment>The following list shows the deliverables and structure of the fabrication records for piping:
 - Index of design drawings with reference to relevant fabrication drawings (Index of design drawings to be delivered in XLS format additionally to PDF);
 - Index of design-, material-, fabrication specifications, documents and data sheets (*);
 - Welding procedure specifications (*);
 - Welding procedure qualification records (*);
 - Repair procedures and specifications (*);
 - Repair and deviation reports. All alternative testing shall be documented with full traceability to the applicable welds;
 - Weld summary index;
 - Material identification system (*);
 - Material certificates (apply for pressurized Piping materials) (*);
 - Pressure test certificates/documentation (*);
 - PMI reports (*);
 - PWHT reports (*);
 - As-built Design Contractor originated design drawings, mark-ups;
 - As-built fabrication drawings/ISOs mark-ups;
 - Third Party verification reports;
 - Procedure for:
    - Tensioning/torqueing of flange stud bolts (*);
    - Flushing and cleaning (*);
    - Hydro testing (*);
    - Hydro flushing of riser- and pipeline valves (*);
    - Pneumatic flushing (*);
    - Pressurised air shock blowing (PAS) (*);
    - Soft Pigging (*);
    - Chemical cleaning (*);
    - Hot oil flushing (*);
    - Internal cleaning of pipe after completed fabrication (*);
    - Bending/flaring (*);
 - Chemical cleaning documentation (*);
 - Hot oil flushing documentation (*).

(*) Can be omitted in modifications if retained by modification Contractor</rdfs:comment>
  </owl:Class>
  <owl:Class rdf:about="http://rds.posccaesar.org/ontology/plm/rdl/PCA_100006254">
    <skos:broader rdf:resource="http://rds.posccaesar.org/ontology/plm/rdl/PCA_100006748"/>
    <skos:broadMatch rdf:resource="http://rds.posccaesar.org/ontology/plm/rdl/PCA_100006716"/>
    <rdfs:label>HVAC bulk items index</rdfs:label>
    <rdfs:comment>The HVAC Bulk item index will include the following information for standard inline off-the-shelf HVAC items without electric, instrument or pneumatic connection and with no regular operation or maintenance requirements.
 - HVAC Bulk item number (according to ENS);
 - Functional service description;
 - Area;
 - Real manufacturer;
 - Variant/type/real manufacture part number.</rdfs:comment>
    <rdl:PCA_100006768>The HVAC Bulk item index will include the following information for standard inline off-the-shelf HVAC items without electric, instrument or pneumatic connection and with no regular operation or maintenance requirements.
 - HVAC Bulk item number (according to ENS);
 - Functional service description;
 - Area;
 - Real manufacturer;
 - Variant/type/real manufacture part number.</rdl:PCA_100006768>
    <rdl:PCA_100006766 rdf:resource="http://rds.posccaesar.org/ontology/plm/rdl/PCA_100006653"/>
    <rdl:PCA_100006765 rdf:resource="http://w3id.org/readi/rdl/CFIHOS-20000019"/>
    <rdfs:subClassOf rdf:resource="http://rds.posccaesar.org/ontology/plm/rdl/PCA_100004908"/>
  </owl:Class>
  <owl:Class rdf:about="http://rds.posccaesar.org/ontology/plm/rdl/PCA_100006242">
    <skos:broadMatch rdf:resource="http://rds.posccaesar.org/ontology/plm/rdl/PCA_100006689"/>
    <rdl:PCA_100006763>The requirement shall apply to field investigations, laboratory tests and analyses and cover facilities in rock.</rdl:PCA_100006763>
    <rdl:PCA_100006766 rdf:resource="http://rds.posccaesar.org/ontology/plm/rdl/PCA_100006654"/>
    <rdfs:label>Geotechnical - Geotechnical reports</rdfs:label>
    <rdfs:comment>The content and structure of the reports shall comply with the requirements in EN1997 or equivalent standard.</rdfs:comment>
    <rdl:PCA_100006765 rdf:resource="http://w3id.org/readi/rdl/CFIHOS-20000018"/>
    <rdfs:subClassOf rdf:resource="http://rds.posccaesar.org/ontology/plm/rdl/PCA_100004908"/>
    <rdl:PCA_100006768>The content and structure of the reports shall comply with the requirements in EN1997 or equivalent standard.</rdl:PCA_100006768>
    <skos:broader rdf:resource="http://rds.posccaesar.org/ontology/plm/rdl/PCA_100006756"/>
  </owl:Class>
  <owl:Class rdf:about="http://rds.posccaesar.org/ontology/plm/rdl/PCA_100006484">
    <skos:broader rdf:resource="http://rds.posccaesar.org/ontology/plm/rdl/PCA_100006748"/>
    <skos:broadMatch rdf:resource="http://rds.posccaesar.org/ontology/plm/rdl/PCA_100006716"/>
    <rdfs:label>Tag and equipment list</rdfs:label>
    <rdfs:comment>No standardized description is presently available.</rdfs:comment>
    <rdl:PCA_100006768>No standardized description is presently available.</rdl:PCA_100006768>
    <rdl:PCA_100006766 rdf:resource="http://rds.posccaesar.org/ontology/plm/rdl/PCA_100006653"/>
    <rdl:PCA_100006763>No standardized description is presently available.</rdl:PCA_100006763>
    <rdfs:subClassOf rdf:resource="http://rds.posccaesar.org/ontology/plm/rdl/PCA_100004908"/>
  </owl:Class>
  <owl:Class rdf:about="http://rds.posccaesar.org/ontology/plm/rdl/PCA_100006363">
    <skos:broader rdf:resource="http://rds.posccaesar.org/ontology/plm/rdl/PCA_100006741"/>
    <skos:broadMatch rdf:resource="http://rds.posccaesar.org/ontology/plm/rdl/PCA_100006687"/>
    <rdfs:label>Pipe stress calculations</rdfs:label>
    <rdfs:comment>Electronic input files for pipe stress program to be delivered for each calculation no.

NOTE: For equipment packages where the amount and size of piping is moderate, or the piping might be mostly for support functions (cooling, lubrication, drain etc.), pipe stress calculations from the manufacturer are not necessary.  For large packages with a considerable amount of larger piping, pipe stress calculations for the main piping should be delivered or optionally retained. Decision/selection should be done early in the project.</rdfs:comment>
    <rdl:PCA_100006768>Electronic input files for pipe stress program to be delivered for each calculation no.

NOTE: For equipment packages where the amount and size of piping is moderate, or the piping might be mostly for support functions (cooling, lubrication, drain etc.), pipe stress calculations from the manufacturer are not necessary.  For large packages with a considerable amount of larger piping, pipe stress calculations for the main piping should be delivered or optionally retained. Decision/selection should be done early in the project.</rdl:PCA_100006768>
    <rdl:PCA_100006766 rdf:resource="http://rds.posccaesar.org/ontology/plm/rdl/PCA_100006653"/>
    <rdl:PCA_100006765 rdf:resource="http://w3id.org/readi/rdl/CFIHOS-20000020"/>
    <rdfs:subClassOf rdf:resource="http://rds.posccaesar.org/ontology/plm/rdl/PCA_100004908"/>
  </owl:Class>
  <owl:Class rdf:about="http://rds.posccaesar.org/ontology/plm/rdl/PCA_100006496">
    <rdfs:subClassOf rdf:resource="http://rds.posccaesar.org/ontology/plm/rdl/PCA_100004908"/>
    <rdl:PCA_100006765 rdf:resource="http://w3id.org/readi/rdl/CFIHOS-20000008"/>
    <rdl:PCA_100006763>This document shall provide input to electrical hook-up with respect to power, input/output signals and communication.</rdl:PCA_100006763>
    <skos:broader rdf:resource="http://rds.posccaesar.org/ontology/plm/rdl/PCA_100006745"/>
    <rdl:PCA_100006768>Document to identify terminals for external connection, including marking (if applicable) and signal/power description. Cable entry information may be included in this drawing or part of valve drawing.  The  supplier standard drawing to be delivered if existing.</rdl:PCA_100006768>
    <skos:broadMatch rdf:resource="http://rds.posccaesar.org/ontology/plm/rdl/PCA_100006712"/>
    <rdfs:comment>Document to identify terminals for external connection, including marking (if applicable) and signal/power description. Cable entry information may be included in this drawing or part of valve drawing.  The  supplier standard drawing to be delivered if existing.</rdfs:comment>
    <rdl:PCA_100006766 rdf:resource="http://rds.posccaesar.org/ontology/plm/rdl/PCA_100006653"/>
    <rdfs:label>Termination and wiring diagram</rdfs:label>
  </owl:Class>
  <owl:Class rdf:about="http://rds.posccaesar.org/ontology/plm/rdl/PCA_100006351">
    <rdfs:comment>Input to design basis for pipeline and risers design and installation methodology.</rdfs:comment>
    <rdl:PCA_100006768>Input to design basis for pipeline and risers design and installation methodology.</rdl:PCA_100006768>
    <rdl:PCA_100006766 rdf:resource="http://rds.posccaesar.org/ontology/plm/rdl/PCA_100006657"/>
    <rdl:PCA_100006765 rdf:resource="http://w3id.org/readi/rdl/CFIHOS-20000031"/>
    <rdfs:subClassOf rdf:resource="http://rds.posccaesar.org/ontology/plm/rdl/PCA_100004908"/>
    <rdfs:label>Outline precommissioning procedure</rdfs:label>
    <skos:broader rdf:resource="http://rds.posccaesar.org/ontology/plm/rdl/PCA_100006751"/>
    <rdl:PCA_100006763>Outline procedure for the pre-commission activities and schedule.</rdl:PCA_100006763>
    <skos:broadMatch rdf:resource="http://rds.posccaesar.org/ontology/plm/rdl/PCA_100006688"/>
  </owl:Class>
  <owl:Class rdf:about="http://rds.posccaesar.org/ontology/plm/rdl/PCA_100006230">
    <rdl:PCA_100006765 rdf:resource="http://w3id.org/readi/rdl/CFIHOS-20000018"/>
    <rdfs:comment>Report documenting allowable freespans along pipeline route, primarily from fatigue (VIV) point of view.</rdfs:comment>
    <skos:broadMatch rdf:resource="http://rds.posccaesar.org/ontology/plm/rdl/PCA_100006687"/>
    <rdl:PCA_100006766 rdf:resource="http://rds.posccaesar.org/ontology/plm/rdl/PCA_100006653"/>
    <rdfs:subClassOf rdf:resource="http://rds.posccaesar.org/ontology/plm/rdl/PCA_100004908"/>
    <rdl:PCA_100006763>To verify the integrity of the pipelines and to enable required seabed intervention to support pipeline installation</rdl:PCA_100006763>
    <rdfs:label>Freespan analysis report</rdfs:label>
    <skos:broader rdf:resource="http://rds.posccaesar.org/ontology/plm/rdl/PCA_100006756"/>
    <rdl:PCA_100006768>Report documenting allowable freespans along pipeline route, primarily from fatigue (VIV) point of view.</rdl:PCA_100006768>
  </owl:Class>
  <owl:Class rdf:about="http://rds.posccaesar.org/ontology/plm/rdl/PCA_100006472">
    <skos:broader rdf:resource="http://rds.posccaesar.org/ontology/plm/rdl/PCA_100006748"/>
    <skos:broadMatch rdf:resource="http://rds.posccaesar.org/ontology/plm/rdl/PCA_100006687"/>
    <rdfs:label>Summary table for mechanical joints (size and type)</rdfs:label>
    <rdfs:comment>Divided per pipe class including dimensions and loads.</rdfs:comment>
    <rdl:PCA_100006768>Divided per pipe class including dimensions and loads.</rdl:PCA_100006768>
    <rdl:PCA_100006766 rdf:resource="http://rds.posccaesar.org/ontology/plm/rdl/PCA_100006653"/>
    <rdl:PCA_100006763>Supports selection of size and schedule (selection table)</rdl:PCA_100006763>
    <rdfs:subClassOf rdf:resource="http://rds.posccaesar.org/ontology/plm/rdl/PCA_100004908"/>
  </owl:Class>
  <owl:Class rdf:about="http://rds.posccaesar.org/ontology/plm/rdl/PCA_100006460">
    <skos:broadMatch rdf:resource="http://rds.posccaesar.org/ontology/plm/rdl/PCA_100006733"/>
    <rdl:PCA_100006766 rdf:resource="http://rds.posccaesar.org/ontology/plm/rdl/PCA_100006653"/>
    <rdfs:comment>Fabrication drawings for primary and secondary loadbearing structural members including supports for appurtenances (e.g. caissons, conductors, risers) shall be delivered including welds with reference to weld summary index.</rdfs:comment>
    <skos:broadMatch rdf:resource="http://rds.posccaesar.org/ontology/plm/rdl/PCA_100006732"/>
    <rdfs:label>Structural fabrication drawings</rdfs:label>
    <skos:broadMatch rdf:resource="http://rds.posccaesar.org/ontology/plm/rdl/PCA_100006734"/>
    <rdl:PCA_100006768>Fabrication drawings for primary and secondary loadbearing structural members including supports for appurtenances (e.g. caissons, conductors, risers) shall be delivered including welds with reference to weld summary index.</rdl:PCA_100006768>
    <rdl:PCA_100006765 rdf:resource="http://w3id.org/readi/rdl/CFIHOS-20000006"/>
    <skos:broader rdf:resource="http://rds.posccaesar.org/ontology/plm/rdl/PCA_100006746"/>
    <rdfs:subClassOf rdf:resource="http://rds.posccaesar.org/ontology/plm/rdl/PCA_100004908"/>
    <skos:broadMatch rdf:resource="http://rds.posccaesar.org/ontology/plm/rdl/PCA_100006731"/>
  </owl:Class>
  <owl:Class rdf:about="http://rds.posccaesar.org/ontology/plm/rdl/PCA_100006120">
    <skos:broadMatch rdf:resource="http://rds.posccaesar.org/ontology/plm/rdl/PCA_100006712"/>
    <rdl:PCA_100006766 rdf:resource="http://rds.posccaesar.org/ontology/plm/rdl/PCA_100006634"/>
    <rdfs:label>Circuit / wiring diagram</rdfs:label>
    <rdfs:comment>Circuit/wiring diagram shall typically include the following (as relevant for the equipment):
 - All internal connections for control, alarms, protection, interlocks, trip functions, monitoring, etc.;
 - Component list for all internal components including control and protection units;
 - Switchgear/-board tag code;
 - Cubicle number;
 - Consumer tag code;
 - Type of external signals (fire and gas trip signal, etc.);
 - Power and current rating;
 - Terminal block/socket number;
 - Terminal/pin number (including spares);
 - Internal cable numbers with pair and core colour details;
 - Destination for internal cables;
 - Earthing details;
 - Equipment and equipment connections;
 - External cable numbers with pair and core colour details;
 - Signal tag number;
 - Reference drawings (Company document number);
 - Reference to loop database for signal interfaced to instrument/automation and telecommunication systems.</rdfs:comment>
    <rdl:PCA_100006768>Circuit/wiring diagram shall typically include the following (as relevant for the equipment):
 - All internal connections for control, alarms, protection, interlocks, trip functions, monitoring, etc.;
 - Component list for all internal components including control and protection units;
 - Switchgear/-board tag code;
 - Cubicle number;
 - Consumer tag code;
 - Type of external signals (fire and gas trip signal, etc.);
 - Power and current rating;
 - Terminal block/socket number;
 - Terminal/pin number (including spares);
 - Internal cable numbers with pair and core colour details;
 - Destination for internal cables;
 - Earthing details;
 - Equipment and equipment connections;
 - External cable numbers with pair and core colour details;
 - Signal tag number;
 - Reference drawings (Company document number);
 - Reference to loop database for signal interfaced to instrument/automation and telecommunication systems.</rdl:PCA_100006768>
    <rdfs:subClassOf rdf:resource="http://rds.posccaesar.org/ontology/plm/rdl/PCA_100004908"/>
    <skos:broader rdf:resource="http://rds.posccaesar.org/ontology/plm/rdl/PCA_100006745"/>
    <rdl:PCA_100006766 rdf:resource="http://rds.posccaesar.org/ontology/plm/rdl/PCA_100006636"/>
    <rdl:PCA_100006765 rdf:resource="http://w3id.org/readi/rdl/CFIHOS-20000008"/>
    <rdl:PCA_100006763>The circuit/wiring diagram shall be sufficient for all testing, troubleshooting and maintenance.

The principles of the circuit/wiring diagrams shall be in accordance with IEC 61082.

NOTE: For customized documentation, handover format shall be native 2D CAD (Z-005) + PDF.

The power circuit shall be shown to the extent necessary for the understanding of the circuit functions and for understanding how the components are wired. Contactor and terminal blocks shall be included. This means also including references to equipment not being part of scope of work. The documentation shall reflect the actual internal wiring. Terminal blocks and external references shall be included. Reference shall be made to the supplier's equipment and terminal marking.</rdl:PCA_100006763>
    <rdl:PCA_100006766 rdf:resource="http://rds.posccaesar.org/ontology/plm/rdl/PCA_100006635"/>
    <rdl:PCA_100006766 rdf:resource="http://rds.posccaesar.org/ontology/plm/rdl/PCA_100006639"/>
    <skos:broadMatch rdf:resource="http://rds.posccaesar.org/ontology/plm/rdl/PCA_100006702"/>
    <rdl:PCA_100006766 rdf:resource="http://rds.posccaesar.org/ontology/plm/rdl/PCA_100006638"/>
    <rdl:PCA_100006766 rdf:resource="http://rds.posccaesar.org/ontology/plm/rdl/PCA_100006637"/>
  </owl:Class>
  <owl:Class rdf:about="http://rds.posccaesar.org/ontology/plm/rdl/PCA_100006132">
    <skos:broadMatch rdf:resource="http://rds.posccaesar.org/ontology/plm/rdl/PCA_100006712"/>
    <rdl:PCA_100006766 rdf:resource="http://rds.posccaesar.org/ontology/plm/rdl/PCA_100006653"/>
    <rdfs:comment>(IEC 61082-1) Diagram providing information about the physical connections among components or units
Mandatory content of information:
 - Conductor or cable type information (e.g. recognized type designation, catalogue or part number, material, construction, size, insulation, voltage rating, colour, number of conductors, other technical data);
 - Reference designation or conductor or cable number;
 - Identification or representation of the connected objects (e.g. reference and/or terminal designation).</rdfs:comment>
    <rdfs:subClassOf rdf:resource="http://rds.posccaesar.org/ontology/plm/rdl/PCA_100004908"/>
    <skos:broadMatch rdf:resource="http://rds.posccaesar.org/ontology/plm/rdl/PCA_100006713"/>
    <skos:broader rdf:resource="http://rds.posccaesar.org/ontology/plm/rdl/PCA_100006745"/>
    <rdl:PCA_100006764>Separate diagrams shall be made for hydraulic, pneumatic and electrical connections, unless deemed not appropriate.</rdl:PCA_100006764>
    <rdl:PCA_100006768>(IEC 61082-1) Diagram providing information about the physical connections among components or units
Mandatory content of information:
 - Conductor or cable type information (e.g. recognized type designation, catalogue or part number, material, construction, size, insulation, voltage rating, colour, number of conductors, other technical data);
 - Reference designation or conductor or cable number;
 - Identification or representation of the connected objects (e.g. reference and/or terminal designation).</rdl:PCA_100006768>
    <rdfs:label>Connection diagram</rdfs:label>
    <rdl:PCA_100006763>Diagram providing information about the physical connections among components or units.</rdl:PCA_100006763>
  </owl:Class>
  <owl:Class rdf:about="http://rds.posccaesar.org/ontology/plm/rdl/PCA_100006144">
    <skos:broader rdf:resource="http://rds.posccaesar.org/ontology/plm/rdl/PCA_100006747"/>
    <skos:broadMatch rdf:resource="http://rds.posccaesar.org/ontology/plm/rdl/PCA_100006686"/>
    <rdfs:label>Data sheet</rdfs:label>
    <rdfs:comment>This document provides structured data form containing part number/model, design information,
operational data and limitations of the equipment. 
Document shall provide information on technical data and characteristics about material, products or systems and their environment for proper implementation.</rdfs:comment>
    <rdl:PCA_100006768>This document provides structured data form containing part number/model, design information,
operational data and limitations of the equipment. 
Document shall provide information on technical data and characteristics about material, products or systems and their environment for proper implementation.</rdl:PCA_100006768>
    <rdl:PCA_100006766 rdf:resource="http://rds.posccaesar.org/ontology/plm/rdl/PCA_100006653"/>
    <rdl:PCA_100006763>Document providing information on technical data and characteristics about material, products or systems and their environment for proper implementation.</rdl:PCA_100006763>
    <rdfs:subClassOf rdf:resource="http://rds.posccaesar.org/ontology/plm/rdl/PCA_100004908"/>
  </owl:Class>
  <owl:Class rdf:about="http://rds.posccaesar.org/ontology/plm/rdl/PCA_100006156">
    <rdl:PCA_100006766 rdf:resource="http://rds.posccaesar.org/ontology/plm/rdl/PCA_100006654"/>
    <skos:broader rdf:resource="http://rds.posccaesar.org/ontology/plm/rdl/PCA_100006746"/>
    <rdfs:comment>Design documentation (analysis and drawings) of all permanent installation used for construction and installation along the pipeline, such as, but not limited to, turn point and foundation for winches.</rdfs:comment>
    <skos:broadMatch rdf:resource="http://rds.posccaesar.org/ontology/plm/rdl/PCA_100006686"/>
    <skos:broader rdf:resource="http://rds.posccaesar.org/ontology/plm/rdl/PCA_100006741"/>
    <rdl:PCA_100006765 rdf:resource="http://w3id.org/readi/rdl/CFIHOS-20000018"/>
    <rdl:PCA_100006768>Design documentation (analysis and drawings) of all permanent installation used for construction and installation along the pipeline, such as, but not limited to, turn point and foundation for winches.</rdl:PCA_100006768>
    <rdfs:label>Design documentation of permanent auxiliary installations</rdfs:label>
    <rdfs:subClassOf rdf:resource="http://rds.posccaesar.org/ontology/plm/rdl/PCA_100004908"/>
  </owl:Class>
  <owl:Class rdf:about="http://rds.posccaesar.org/ontology/plm/rdl/PCA_100006168">
    <rdl:PCA_100006766 rdf:resource="http://rds.posccaesar.org/ontology/plm/rdl/PCA_100006657"/>
    <skos:broader rdf:resource="http://rds.posccaesar.org/ontology/plm/rdl/PCA_100006746"/>
    <rdfs:comment>The drawings for transformer rectifiers units, testposts and belonging components for onshore CP-system shall cover geometry, dimensions, materials, cable routing, cable penetrations for foundation and cabinets.</rdfs:comment>
    <rdl:PCA_100006768>The drawings for transformer rectifiers units, testposts and belonging components for onshore CP-system shall cover geometry, dimensions, materials, cable routing, cable penetrations for foundation and cabinets.</rdl:PCA_100006768>
    <rdl:PCA_100006763>Documentation of installed cathodic protection equipment to ensure safe operation</rdl:PCA_100006763>
    <rdfs:subClassOf rdf:resource="http://rds.posccaesar.org/ontology/plm/rdl/PCA_100004908"/>
    <rdl:PCA_100006765 rdf:resource="http://w3id.org/readi/rdl/CFIHOS-20000018"/>
    <skos:broadMatch rdf:resource="http://rds.posccaesar.org/ontology/plm/rdl/PCA_100006732"/>
    <rdfs:label>Drawings for onshore cp-system</rdfs:label>
  </owl:Class>
  <owl:Class rdf:about="http://rds.posccaesar.org/ontology/plm/rdl/PCA_100006279">
    <skos:broader rdf:resource="http://rds.posccaesar.org/ontology/plm/rdl/PCA_100006749"/>
    <skos:broadMatch rdf:resource="http://rds.posccaesar.org/ontology/plm/rdl/PCA_100006688"/>
    <rdfs:label>Installation, operation and maintenance manual (IOM manual)</rdfs:label>
    <rdfs:comment>An IOM manual shall normally include the following information: 

Main Data 
Information for the complete equipment showing all data necessary for the understanding of the equipment's mode of operation shall be given. Information regarding health, environment and safety shall be emphasized. Other data may be:
 - Restrictions in guarantee
 - Performance data
 - Restrictions in use
 - Main connections and requirements on connected systems
 - Weight and outline dimensions 
Technical description 
Design and function shall be described to facilitate a better understanding of the different parts of the operating and maintenance instructions. If the complete equipment package consists of several systems, the main system should be described first, followed by descriptions of each subsystem and their interconnections. 

Preparations 
All preparations to be made from the moment the installation is completed until the equipment is ready for normal operation shall be described. The description shall include tests, adjustments, calibrations and necessary inspections. The sequence of the activities shall be stated as well as all tools, auxiliary equipment, consumables and spare parts that may be needed. If necessary, references to detailed technical information (e.g. performance and operational data) in other parts of the manual shall be made. 

Operating instructions 
Start, normal operation, stop and emergency stop The information shall be given in a logical sequence and shall include all operations and observations which the operator shall undertake. These may be:
 - Check list for prestart preparations
 - Prestart settings and precautions
 - The starting sequence shall include all modes of operation (manual, automatic, remote control, etc.)
 - Observations which shall be made during the starting sequence
 - Precautions concerning interruption of the starting sequence
 - Operations and observations during normal operation
 - Normal stop
 - Emergency stop
 - Start after emergency stop 

Disturbance of operation 
Description of the various forms of disturbance of operation that may occur, how they can be identified and the consequences they may have for the operation, shall be given. 

Corrective measures 
A description shall be available of the necessary actions after a disturbance has occurred. For actions which cannot be taken by the operator, it may be necessary to refer to the maintenance instructions. The manual shall state all requirements for reports to the supplier in the form of registrations and observations. 

Hazards and protective measures 
A description shall be given of all known hazards that may occur during operation. This also applies to hazards which are due to lack of observation of the supplier's procedures as well as to external causes, e. g. lack of cooling water, loss of electrical power, etc. The manual shall give detailed information about protective measures, how to reduce the consequences to a minimum and what procedures to follow in the event of an accident. Product data sheets for chemical substances shall be attached. 

Qualification requirements and training program for operators 
The supplier shall state the qualifications required of the operator and the training programs that can be offered. 

Maintenance 
General Maintenance includes all inspections, measurements, adjustments and operations carried out directly on the equipment in order to ensure safe, reliable and economical operation. Maintenance documentation shall cover the maintenance which can normally be done by the user and the maintenance which is not expected to be done by the user. If the maintenance documentation shall be the basis of a maintenance system for the complete plant where the equipment is a part, then the customer shall state all necessary information and specify all special requests in the inquiry and order documentation. 

Structure and contents of operating instructions 
Instructions should contain a minimum of elements and shall be constructed as follows:
 - Introduction, scope and possible limitations of the instruction
 - Necessary safety precautions before and during maintenance
 - Detailed description of the procedure to be followed with references to relevant supplementary documentation
 - Necessary data and arrangement for lifting
 - List of necessary tools and equipment
 - Recommended spare parts and consumables
 - Control and measurement points with limits during maintenance and after completion prior to restart
 - Requirements for special skills and minimum crew for the maintenance
 - Registrations which should be part of a specially defined maintenance log 
Maintenance instructions 
These shall be divided into the following separate instructions: 

Routine inspection 
This part of the maintenance consists of the regular inspections carried out by the operation and/or maintenance personnel. The inspections consist of what can be measured, seen, heard or felt without interference in the equipment both during an operation and while at standstill. The supplier shall give instructions concerning inspection points based on his own experience and the selected monitoring system. 

Periodic maintenance 
It shall cover all planned and expected maintenance based on operation time, calendar time or certain operational observations. This type of maintenance may e.g. include: 
 - Cleaning
 - Lubrication schedule
 - Adjustments
 - Calibrations
 - Replacement of wear parts
 - Replenishments 

Corrections and minor repairs 
The most comprehensive maintenance possible on site shall be described under this clause, e.g.:
 - Replacement of broken parts
 - Repairs which can be done on site or in a normally equipped maintenance shop
 - Dismantling parts of or the whole equipment for shipment to a special repair or overhaul shop Major repairs and modifications 
It is not normally required that this shall be covered by the instructions at the user's disposal. However the supplier shall keep and upon request provide instructions concerning overhaul and repairs at special shops. If agreed, the supplier shall also keep all documentation for modification or rebuilding of the equipment. 

Fault finding and correction of irregularities
 For heavy machinery, complicated equipment or if the equipment is considered critical for the total operation of the plant, the supplier shall include a fault finding diagram in his documentation. The diagram shall list possible faults and irregularities, and refer to possible causes. The diagram shall cover faults which may be discovered during operation and maintenance. Furthermore it shall be described how the fault is to be corrected, if necessary by referring to other maintenance instructions. The supplier should prepare a registration form where the results of measurements and observations can be noted systematically in order to give the supplier a better basis for diagnosis when the user requests supplier's assistance. 

Storing, preservation and maintenance of preservation
This clause shall describe storing of equipment removed from use. The description of the preparations for storage shall include preservation and other protection against external influences. The description of maintenance during storage shall include preventive and corrective measures to ensure that the functionality of the equipment is taken care of. The clause shall also describe how the equipment is prepared for operation after storage. The supplier shall also state how spare parts are to be stored and preserved. 

(reprint from NS5820, annex A2  - A6, with permission) 

Local language: YES for lifting appliances</rdfs:comment>
    <rdl:PCA_100006768>An IOM manual shall normally include the following information: 

Main Data 
Information for the complete equipment showing all data necessary for the understanding of the equipment's mode of operation shall be given. Information regarding health, environment and safety shall be emphasized. Other data may be:
 - Restrictions in guarantee
 - Performance data
 - Restrictions in use
 - Main connections and requirements on connected systems
 - Weight and outline dimensions 
Technical description 
Design and function shall be described to facilitate a better understanding of the different parts of the operating and maintenance instructions. If the complete equipment package consists of several systems, the main system should be described first, followed by descriptions of each subsystem and their interconnections. 

Preparations 
All preparations to be made from the moment the installation is completed until the equipment is ready for normal operation shall be described. The description shall include tests, adjustments, calibrations and necessary inspections. The sequence of the activities shall be stated as well as all tools, auxiliary equipment, consumables and spare parts that may be needed. If necessary, references to detailed technical information (e.g. performance and operational data) in other parts of the manual shall be made. 

Operating instructions 
Start, normal operation, stop and emergency stop The information shall be given in a logical sequence and shall include all operations and observations which the operator shall undertake. These may be:
 - Check list for prestart preparations
 - Prestart settings and precautions
 - The starting sequence shall include all modes of operation (manual, automatic, remote control, etc.)
 - Observations which shall be made during the starting sequence
 - Precautions concerning interruption of the starting sequence
 - Operations and observations during normal operation
 - Normal stop
 - Emergency stop
 - Start after emergency stop 

Disturbance of operation 
Description of the various forms of disturbance of operation that may occur, how they can be identified and the consequences they may have for the operation, shall be given. 

Corrective measures 
A description shall be available of the necessary actions after a disturbance has occurred. For actions which cannot be taken by the operator, it may be necessary to refer to the maintenance instructions. The manual shall state all requirements for reports to the supplier in the form of registrations and observations. 

Hazards and protective measures 
A description shall be given of all known hazards that may occur during operation. This also applies to hazards which are due to lack of observation of the supplier's procedures as well as to external causes, e. g. lack of cooling water, loss of electrical power, etc. The manual shall give detailed information about protective measures, how to reduce the consequences to a minimum and what procedures to follow in the event of an accident. Product data sheets for chemical substances shall be attached. 

Qualification requirements and training program for operators 
The supplier shall state the qualifications required of the operator and the training programs that can be offered. 

Maintenance 
General Maintenance includes all inspections, measurements, adjustments and operations carried out directly on the equipment in order to ensure safe, reliable and economical operation. Maintenance documentation shall cover the maintenance which can normally be done by the user and the maintenance which is not expected to be done by the user. If the maintenance documentation shall be the basis of a maintenance system for the complete plant where the equipment is a part, then the customer shall state all necessary information and specify all special requests in the inquiry and order documentation. 

Structure and contents of operating instructions 
Instructions should contain a minimum of elements and shall be constructed as follows:
 - Introduction, scope and possible limitations of the instruction
 - Necessary safety precautions before and during maintenance
 - Detailed description of the procedure to be followed with references to relevant supplementary documentation
 - Necessary data and arrangement for lifting
 - List of necessary tools and equipment
 - Recommended spare parts and consumables
 - Control and measurement points with limits during maintenance and after completion prior to restart
 - Requirements for special skills and minimum crew for the maintenance
 - Registrations which should be part of a specially defined maintenance log 
Maintenance instructions 
These shall be divided into the following separate instructions: 

Routine inspection 
This part of the maintenance consists of the regular inspections carried out by the operation and/or maintenance personnel. The inspections consist of what can be measured, seen, heard or felt without interference in the equipment both during an operation and while at standstill. The supplier shall give instructions concerning inspection points based on his own experience and the selected monitoring system. 

Periodic maintenance 
It shall cover all planned and expected maintenance based on operation time, calendar time or certain operational observations. This type of maintenance may e.g. include: 
 - Cleaning
 - Lubrication schedule
 - Adjustments
 - Calibrations
 - Replacement of wear parts
 - Replenishments 

Corrections and minor repairs 
The most comprehensive maintenance possible on site shall be described under this clause, e.g.:
 - Replacement of broken parts
 - Repairs which can be done on site or in a normally equipped maintenance shop
 - Dismantling parts of or the whole equipment for shipment to a special repair or overhaul shop Major repairs and modifications 
It is not normally required that this shall be covered by the instructions at the user's disposal. However the supplier shall keep and upon request provide instructions concerning overhaul and repairs at special shops. If agreed, the supplier shall also keep all documentation for modification or rebuilding of the equipment. 

Fault finding and correction of irregularities
 For heavy machinery, complicated equipment or if the equipment is considered critical for the total operation of the plant, the supplier shall include a fault finding diagram in his documentation. The diagram shall list possible faults and irregularities, and refer to possible causes. The diagram shall cover faults which may be discovered during operation and maintenance. Furthermore it shall be described how the fault is to be corrected, if necessary by referring to other maintenance instructions. The supplier should prepare a registration form where the results of measurements and observations can be noted systematically in order to give the supplier a better basis for diagnosis when the user requests supplier's assistance. 

Storing, preservation and maintenance of preservation
This clause shall describe storing of equipment removed from use. The description of the preparations for storage shall include preservation and other protection against external influences. The description of maintenance during storage shall include preventive and corrective measures to ensure that the functionality of the equipment is taken care of. The clause shall also describe how the equipment is prepared for operation after storage. The supplier shall also state how spare parts are to be stored and preserved. 

(reprint from NS5820, annex A2  - A6, with permission) 

Local language: YES for lifting appliances</rdl:PCA_100006768>
    <rdl:PCA_100006763>IOM documents shall, in an organized manner, provide sufficient information to install, operate and maintain the equipment in a safe, economical and functionally correct manner according to the agreed maintenance philosophy. The equipment manufacturer’s standard IOM manual shall be delivered if it fulfils the intentions of this document, either as a complete IOM manual or split in two or more separate manuals. For assemblies/skids/packages the IOM manual shall cover the complete assembly.</rdl:PCA_100006763>
    <rdfs:subClassOf rdf:resource="http://rds.posccaesar.org/ontology/plm/rdl/PCA_100004908"/>
  </owl:Class>
  <owl:Class rdf:about="http://rds.posccaesar.org/ontology/plm/rdl/PCA_100006388">
    <rdfs:label>Preservation and storage instructions</rdfs:label>
    <rdfs:subClassOf rdf:resource="http://rds.posccaesar.org/ontology/plm/rdl/PCA_100004908"/>
    <skos:broadMatch rdf:resource="http://rds.posccaesar.org/ontology/plm/rdl/PCA_100006668"/>
    <rdl:PCA_100006768>Information for preservation of the equipment during short- and long term storage.</rdl:PCA_100006768>
    <rdl:PCA_100006763>Describe how to preserve and store equipment in a safe and economical manner</rdl:PCA_100006763>
    <rdfs:comment>Information for preservation of the equipment during short- and long term storage.</rdfs:comment>
    <rdl:PCA_100006766 rdf:resource="http://rds.posccaesar.org/ontology/plm/rdl/PCA_100006653"/>
    <skos:broader rdf:resource="http://rds.posccaesar.org/ontology/plm/rdl/PCA_100006751"/>
    <rdl:PCA_100006765 rdf:resource="http://w3id.org/readi/rdl/CFIHOS-20000031"/>
  </owl:Class>
  <owl:Class rdf:about="http://rds.posccaesar.org/ontology/plm/rdl/PCA_100006497">
    <skos:broadMatch rdf:resource="http://rds.posccaesar.org/ontology/plm/rdl/PCA_100006688"/>
    <rdl:PCA_100006765 rdf:resource="http://w3id.org/readi/rdl/CFIHOS-20000018"/>
    <rdfs:label>Test procedures onshore CP system, coating quality and insulating joint</rdfs:label>
    <rdl:PCA_100006763>Ensure safe operation</rdl:PCA_100006763>
    <rdfs:subClassOf rdf:resource="http://rds.posccaesar.org/ontology/plm/rdl/PCA_100004908"/>
    <skos:broader rdf:resource="http://rds.posccaesar.org/ontology/plm/rdl/PCA_100006751"/>
    <rdl:PCA_100006766 rdf:resource="http://rds.posccaesar.org/ontology/plm/rdl/PCA_100006657"/>
    <rdl:PCA_100006768>Shall be according to ISO 15589-1.</rdl:PCA_100006768>
    <rdfs:comment>Shall be according to ISO 15589-1.</rdfs:comment>
  </owl:Class>
  <owl:Class rdf:about="http://rds.posccaesar.org/ontology/plm/rdl/PCA_100006267">
    <skos:broadMatch rdf:resource="http://rds.posccaesar.org/ontology/plm/rdl/PCA_100006688"/>
    <rdl:PCA_100006763>To verify the integrity of the components exposed to hyperbaric pressure and to provide traceability and quality assurance by recording all test results within the procedure.</rdl:PCA_100006763>
    <rdfs:subClassOf rdf:resource="http://rds.posccaesar.org/ontology/plm/rdl/PCA_100004908"/>
    <rdl:PCA_100006768>Procedure for hyperbaric testing of equipment as part of the qualification.</rdl:PCA_100006768>
    <rdfs:comment>Procedure for hyperbaric testing of equipment as part of the qualification.</rdfs:comment>
    <rdl:PCA_100006766 rdf:resource="http://rds.posccaesar.org/ontology/plm/rdl/PCA_100006653"/>
    <rdfs:label>Hyperbaric test procedure</rdfs:label>
    <skos:broader rdf:resource="http://rds.posccaesar.org/ontology/plm/rdl/PCA_100006751"/>
    <rdl:PCA_100006765 rdf:resource="http://w3id.org/readi/rdl/CFIHOS-20000031"/>
  </owl:Class>
  <owl:Class rdf:about="http://rds.posccaesar.org/ontology/plm/rdl/PCA_100006255">
    <skos:broader rdf:resource="http://rds.posccaesar.org/ontology/plm/rdl/PCA_100006741"/>
    <skos:broadMatch rdf:resource="http://rds.posccaesar.org/ontology/plm/rdl/PCA_100006687"/>
    <rdfs:label>HVAC calculations / analyses</rdfs:label>
    <rdl:PCA_100006766 rdf:resource="http://rds.posccaesar.org/ontology/plm/rdl/PCA_100006650"/>
    <rdl:PCA_100006765 rdf:resource="http://w3id.org/readi/rdl/CFIHOS-20000019"/>
    <rdl:PCA_100006764>Rename to Calculation/analyses. Discipline specific content to be defined.</rdl:PCA_100006764>
    <rdl:PCA_100006763>Numerical analyses:
If required to clarify wind effects on air inlets and outlets and to determine possible contamination of the air intake from other sources, a numerical analysis shall be carried out, preferably computerized on software agreed with Company.
Numerical analysis shall also provide pressure coefficients for calculation of the natural ventilation and make a visualization of the natural ventilation in naturally ventilated areas. 

Ventilation Air Volumes:
Calculations carried out and documented to determine ventilation in naturally ventilated areas for different wind velocities and directions shall be transferred.

Necessary ventilation volumes shall be determined and documented with regard to potential gas leaks and other contaminations in the ventilated area. 

Other calculations/analyses to be transferred (as required):

Consumption calculations of current and energy.

Heating and cooling capacity calculations, performance calculations for air supply/external devices, pressure drop calculations, sound level calculations.</rdl:PCA_100006763>
    <rdfs:subClassOf rdf:resource="http://rds.posccaesar.org/ontology/plm/rdl/PCA_100004908"/>
  </owl:Class>
  <owl:Class rdf:about="http://rds.posccaesar.org/ontology/plm/rdl/PCA_100006376">
    <skos:broader rdf:resource="http://rds.posccaesar.org/ontology/plm/rdl/PCA_100006751"/>
    <skos:broadMatch rdf:resource="http://rds.posccaesar.org/ontology/plm/rdl/PCA_100006688"/>
    <rdfs:label>Piping installation procedure</rdfs:label>
    <rdl:PCA_100006766 rdf:resource="http://rds.posccaesar.org/ontology/plm/rdl/PCA_100006653"/>
    <rdl:PCA_100006765 rdf:resource="http://w3id.org/readi/rdl/CFIHOS-20000020"/>
    <rdl:PCA_100006763>Applies to piping systems that require special attention during installation, typical for piping connected to strain sensitive equipment such as compressors.</rdl:PCA_100006763>
    <rdfs:subClassOf rdf:resource="http://rds.posccaesar.org/ontology/plm/rdl/PCA_100004908"/>
  </owl:Class>
  <owl:Class rdf:about="http://rds.posccaesar.org/ontology/plm/rdl/PCA_100006485">
    <skos:broader rdf:resource="http://rds.posccaesar.org/ontology/plm/rdl/PCA_100006748"/>
    <skos:broadMatch rdf:resource="http://rds.posccaesar.org/ontology/plm/rdl/PCA_100006722"/>
    <rdfs:label>Tally</rdfs:label>
    <rdfs:comment>A list containing details of tubulars that have been prepared for running, or that have been retrieved from the wellbore. 
The minimum information to be included for the pipe and connection is:
 - Date installed
 - Revision 
 - Size 
 - Material Grade
 - Prepared by
 - Centralizer depth and type
 - Tubing clamp depht and type
 - Thread type 
 - Makeup tourque
 - OD (Outer diameter)
 - ID (Inner diameter)
 - Volumes
 - Run number
 - Description
 - Pipe/Heat number per joint (to ensure full traceability to material certificates) 
 - Joint length
 - Cumulative length
 - Depht joint</rdfs:comment>
    <rdl:PCA_100006768>A list containing details of tubulars that have been prepared for running, or that have been retrieved from the wellbore. 
The minimum information to be included for the pipe and connection is:
 - Date installed
 - Revision 
 - Size 
 - Material Grade
 - Prepared by
 - Centralizer depth and type
 - Tubing clamp depht and type
 - Thread type 
 - Makeup tourque
 - OD (Outer diameter)
 - ID (Inner diameter)
 - Volumes
 - Run number
 - Description
 - Pipe/Heat number per joint (to ensure full traceability to material certificates) 
 - Joint length
 - Cumulative length
 - Depht joint</rdl:PCA_100006768>
    <rdl:PCA_100006765 rdf:resource="http://w3id.org/readi/rdl/CFIHOS-20000042"/>
    <rdl:PCA_100006763>A list prepared to keep track of all the pipes installed in the wellbore and at which depth they are installed</rdl:PCA_100006763>
    <rdfs:subClassOf rdf:resource="http://rds.posccaesar.org/ontology/plm/rdl/PCA_100004908"/>
  </owl:Class>
  <owl:Class rdf:about="http://rds.posccaesar.org/ontology/plm/rdl/PCA_100006364">
    <skos:broader rdf:resource="http://rds.posccaesar.org/ontology/plm/rdl/PCA_100006751"/>
    <skos:broadMatch rdf:resource="http://rds.posccaesar.org/ontology/plm/rdl/PCA_100006688"/>
    <rdfs:label>Pipe stress procedure</rdfs:label>
    <rdl:PCA_100006766 rdf:resource="http://rds.posccaesar.org/ontology/plm/rdl/PCA_100006653"/>
    <rdl:PCA_100006765 rdf:resource="http://w3id.org/readi/rdl/CFIHOS-20000020"/>
    <rdl:PCA_100006763>The document shall describe the design data for the pipe stress work, and ensure that all applicable codes, standards, guidelines and regulations that are relevant at the commencement of detail engineering are fulfilled. For modification projects the existing procedure for the plant may be used if this is available.

NOTE: For equipment packages where the amount and size of piping is moderate, or the piping might be mostly for support functions (cooling, lubrication, drain etc.), pipe stress procedure from the manufacturer is not necessary.  For large packages with a considerable amount of larger piping, where pipe stress isometrics will be delivered, pipe stress procedure should also be delivered.</rdl:PCA_100006763>
    <rdfs:subClassOf rdf:resource="http://rds.posccaesar.org/ontology/plm/rdl/PCA_100004908"/>
  </owl:Class>
  <owl:Class rdf:about="http://rds.posccaesar.org/ontology/plm/rdl/PCA_100006243">
    <rdl:PCA_100006763>The results from the Topographical Survey shall be reported in a written document describing the various task and findings in a systematic way including appendices and data samples where applicable.</rdl:PCA_100006763>
    <skos:broader rdf:resource="http://rds.posccaesar.org/ontology/plm/rdl/PCA_100006756"/>
    <rdl:PCA_100006766 rdf:resource="http://rds.posccaesar.org/ontology/plm/rdl/PCA_100006656"/>
    <rdfs:comment>The general content of the report shall as a minimum include the following items:
Descriptive front page with dates and document numbers.
Complete and systematic index, including appendices.
Revision history with description of actions.
 - Introduction.
   - General Project or Survey description (abstract)
   - Scope, Objective and Responsibilities.
   - Definitions and abbreviations.
   - References.
 - Project or Survey description.
   - Scope of work.
   - Key maps - Overview of work area.
   - Summary of results, task by task.
   - Quality evaluation of achieved results.
   - Geodesy.
 - Detailed results. 
   - Systematic detailed description of performed activities in same order as in Summary of results.
   - Listing of data and observations.
   - Used equipment and data acquisition parameters.
   - Used references.
   - Processing systems, methods and parameters.
   - Reporting method and references.
 - Data Index of deliverables.
   - Maps / drawings.
   - Pictures.
   - DTM.
   - Etc.
 - Appendices.
   - All relevant data.
   - Data samples.
   - Maps.
 - Etc.</rdfs:comment>
    <skos:broadMatch rdf:resource="http://rds.posccaesar.org/ontology/plm/rdl/PCA_100006722"/>
    <rdfs:subClassOf rdf:resource="http://rds.posccaesar.org/ontology/plm/rdl/PCA_100004908"/>
    <rdl:PCA_100006768>The general content of the report shall as a minimum include the following items:
Descriptive front page with dates and document numbers.
Complete and systematic index, including appendices.
Revision history with description of actions.
 - Introduction.
   - General Project or Survey description (abstract)
   - Scope, Objective and Responsibilities.
   - Definitions and abbreviations.
   - References.
 - Project or Survey description.
   - Scope of work.
   - Key maps - Overview of work area.
   - Summary of results, task by task.
   - Quality evaluation of achieved results.
   - Geodesy.
 - Detailed results. 
   - Systematic detailed description of performed activities in same order as in Summary of results.
   - Listing of data and observations.
   - Used equipment and data acquisition parameters.
   - Used references.
   - Processing systems, methods and parameters.
   - Reporting method and references.
 - Data Index of deliverables.
   - Maps / drawings.
   - Pictures.
   - DTM.
   - Etc.
 - Appendices.
   - All relevant data.
   - Data samples.
   - Maps.
 - Etc.</rdl:PCA_100006768>
    <rdfs:label>GIS mapping - Survey reports</rdfs:label>
    <rdl:PCA_100006765 rdf:resource="http://w3id.org/readi/rdl/CFIHOS-20000007"/>
  </owl:Class>
  <owl:Class rdf:about="http://rds.posccaesar.org/ontology/plm/rdl/PCA_100006231">
    <skos:broader rdf:resource="http://rds.posccaesar.org/ontology/plm/rdl/PCA_100006757"/>
    <skos:broadMatch rdf:resource="http://rds.posccaesar.org/ontology/plm/rdl/PCA_100006698"/>
    <rdfs:label>Function description</rdfs:label>
    <rdfs:comment>The purpose of this document is, for the Supplier, to define all his requirements for safe and reliable control and monitoring function of his equipment. This document shall be used by the project to develop the control, interlocking, monitoring and sequences to be implemented in the switchgear, Electrical Network and Interface with the SAS.</rdfs:comment>
    <rdl:PCA_100006768>The purpose of this document is, for the Supplier, to define all his requirements for safe and reliable control and monitoring function of his equipment. This document shall be used by the project to develop the control, interlocking, monitoring and sequences to be implemented in the switchgear, Electrical Network and Interface with the SAS.</rdl:PCA_100006768>
    <rdl:PCA_100006766 rdf:resource="http://rds.posccaesar.org/ontology/plm/rdl/PCA_100006653"/>
    <rdl:PCA_100006763>The FDS shall give engineering a description of how the  functional requirement for the product is implemented. It will describe the function and not the design and contain sufficient information for the use.</rdl:PCA_100006763>
    <rdfs:subClassOf rdf:resource="http://rds.posccaesar.org/ontology/plm/rdl/PCA_100004908"/>
  </owl:Class>
  <owl:Class rdf:about="http://rds.posccaesar.org/ontology/plm/rdl/PCA_100006473">
    <skos:broader rdf:resource="http://rds.posccaesar.org/ontology/plm/rdl/PCA_100006741"/>
    <skos:broadMatch rdf:resource="http://rds.posccaesar.org/ontology/plm/rdl/PCA_100006687"/>
    <rdfs:label>Supplier calculations</rdfs:label>
    <rdfs:comment>Characteristics and functional parameters shall be documented and performance shall be shown to be probable. This shall include but not be limited to calculations, curves, tables, reference to similar applications and test data. This shall as a minimum be at a level customary for the equipment and to the extent such data are of importance for interfaces to plant and system.                     Lateral analyses and torsion analyses for compressors performance curves for pumps and compressors. Strength calculations, thermal performance and vibration calculations for heat exchangers/pressure vessels.</rdfs:comment>
    <rdl:PCA_100006768>Characteristics and functional parameters shall be documented and performance shall be shown to be probable. This shall include but not be limited to calculations, curves, tables, reference to similar applications and test data. This shall as a minimum be at a level customary for the equipment and to the extent such data are of importance for interfaces to plant and system.                     Lateral analyses and torsion analyses for compressors performance curves for pumps and compressors. Strength calculations, thermal performance and vibration calculations for heat exchangers/pressure vessels.</rdl:PCA_100006768>
    <rdl:PCA_100006766 rdf:resource="http://rds.posccaesar.org/ontology/plm/rdl/PCA_100006653"/>
    <rdl:PCA_100006763>Can be input to system calculation and engineering</rdl:PCA_100006763>
    <rdfs:subClassOf rdf:resource="http://rds.posccaesar.org/ontology/plm/rdl/PCA_100004908"/>
  </owl:Class>
  <owl:Class rdf:about="http://rds.posccaesar.org/ontology/plm/rdl/PCA_100006352">
    <skos:broadMatch rdf:resource="http://rds.posccaesar.org/ontology/plm/rdl/PCA_100006702"/>
    <rdl:PCA_100006766 rdf:resource="http://rds.posccaesar.org/ontology/plm/rdl/PCA_100006639"/>
    <rdfs:label>Overall single line diagram</rdfs:label>
    <rdl:PCA_100006766 rdf:resource="http://rds.posccaesar.org/ontology/plm/rdl/PCA_100006634"/>
    <rdl:PCA_100006766 rdf:resource="http://rds.posccaesar.org/ontology/plm/rdl/PCA_100006637"/>
    <rdl:PCA_100006765 rdf:resource="http://w3id.org/readi/rdl/CFIHOS-20000008"/>
    <rdfs:subClassOf rdf:resource="http://rds.posccaesar.org/ontology/plm/rdl/PCA_100004908"/>
    <skos:broader rdf:resource="http://rds.posccaesar.org/ontology/plm/rdl/PCA_100006745"/>
    <rdl:PCA_100006763>The diagrams shall include all power distribution units (generators, eventual external grid, switchgears, transformers, distribution boards, rectifiers, batteries etc.) throughout the distribution system. End consumers shall be included for high voltage consumers. Only generators, transformers, switchgears, main distribution boards shall be shown on the low voltage level.

Separate single line diagrams shall be prepared showing UPSs including main and sub distribution boards as well as lighting and small power, typical 400/230 V system.

Separate earthing overall single line diagrams, including all main equipment, shall be provided for the electrical, instrument and telecommunication installations. The general earthing principles shall be included to ensure correct earthing of systems, equipment and cables.</rdl:PCA_100006763>
    <rdl:PCA_100006768>This single diagram shall typically include:
 - Main earth bars for electrical, instrument and telecommunications;
 - Earthing electrode;
 - Lightning system;
 - Earthing of electrical main equipment as switchboards, transformers and generators. System earthing shall be included.</rdl:PCA_100006768>
    <rdfs:comment>This single diagram shall typically include:
 - Main earth bars for electrical, instrument and telecommunications;
 - Earthing electrode;
 - Lightning system;
 - Earthing of electrical main equipment as switchboards, transformers and generators. System earthing shall be included.</rdfs:comment>
    <rdl:PCA_100006766 rdf:resource="http://rds.posccaesar.org/ontology/plm/rdl/PCA_100006636"/>
    <rdl:PCA_100006766 rdf:resource="http://rds.posccaesar.org/ontology/plm/rdl/PCA_100006638"/>
    <rdl:PCA_100006766 rdf:resource="http://rds.posccaesar.org/ontology/plm/rdl/PCA_100006635"/>
  </owl:Class>
  <owl:Class rdf:about="http://rds.posccaesar.org/ontology/plm/rdl/PCA_100006461">
    <rdfs:label>Structural fabrication records</rdfs:label>
    <rdfs:comment>The following list shows the deliverables and structure of the fabrication records for structural steel and aluminium:
 - As-built Users Guide;
 - Index of design drawings with reference to fabrication drawings;
 - Index of material, design, fabrication, specifications and documents, used by Contractor;
 - Welding procedure specifications;
 - Welding procedure qualification records;
 - Repair procedures and specifications;
 - Weld summary index;
 - Material specification system;
 - Assembly procedures;
 - Production test reports;
 - PWHT reports;
 - Repair and deviation reports;
 - As-built Design Contractor originated design drawings, mark-ups;
 - List of fabrication drawings containing Main Weld numbers;
 - Documentation of rubber coating of j-tubes shall include the following: 
    - Detailed design calculations of thermal insulation requirements, and the development of the insulation aspects of the product, during its lifetime expectancy in service. These calculations shall apply for the components and field joints and take into consideration all the necessary properties including application and installation.
    - Detailed information about properties of the coating and coating system qualification.
    - All materials data, test certificates and product data sheets (PDS).
    - Detailed coating procedure, as a minimum including the information listed in the APS.
    - Detailed field jointing procedure.
    - Detailed repair procedure.
    - Detailed procedures for handling and storage of line-pipe.
    - Detailed Quality plans / Inspection and Test Plan (ITP). All witness and hold points shall be identified.
    - Test records and results.
    - Inspection reports and records.
    - Repair and recoating records.
    - All relevant coating application variables.
    - The personnel qualification record shall constitute proof that the personnel designated to carry out the work are properly qualified to do so.

The following list shows the deliverables and structure of the fabrication records for Concrete structures:
 - FRB User guide - Describes the content of each deliverable in the FRB and how they relate and refer to each other. Include examples (images) of how to trace welds and material certificates from fabrication drawings;
 - Index of Concrete fabrication and detail drawings;  
 - Index of material, design, fabrication specifications and documents used by Contractor;   
 - Index of Construction sequence drawings, e.g. dry dock, inshore, tow-to field and installation;
 - Reinforcement bar lists;
 - Concrete mix specification (cement, aggregate, inhibitors, etc.);
 - Test records of compression- and tension capacity of actual fabricated concrete;
 - Material certificates reinforcement.</rdfs:comment>
    <skos:broadMatch rdf:resource="http://rds.posccaesar.org/ontology/plm/rdl/PCA_100006733"/>
    <rdl:PCA_100006765 rdf:resource="http://w3id.org/readi/rdl/CFIHOS-20000006"/>
    <skos:broadMatch rdf:resource="http://rds.posccaesar.org/ontology/plm/rdl/PCA_100006722"/>
    <rdfs:subClassOf rdf:resource="http://rds.posccaesar.org/ontology/plm/rdl/PCA_100004908"/>
    <rdl:PCA_100006768>The following list shows the deliverables and structure of the fabrication records for structural steel and aluminium:
 - As-built Users Guide;
 - Index of design drawings with reference to fabrication drawings;
 - Index of material, design, fabrication, specifications and documents, used by Contractor;
 - Welding procedure specifications;
 - Welding procedure qualification records;
 - Repair procedures and specifications;
 - Weld summary index;
 - Material specification system;
 - Assembly procedures;
 - Production test reports;
 - PWHT reports;
 - Repair and deviation reports;
 - As-built Design Contractor originated design drawings, mark-ups;
 - List of fabrication drawings containing Main Weld numbers;
 - Documentation of rubber coating of j-tubes shall include the following: 
    - Detailed design calculations of thermal insulation requirements, and the development of the insulation aspects of the product, during its lifetime expectancy in service. These calculations shall apply for the components and field joints and take into consideration all the necessary properties including application and installation.
    - Detailed information about properties of the coating and coating system qualification.
    - All materials data, test certificates and product data sheets (PDS).
    - Detailed coating procedure, as a minimum including the information listed in the APS.
    - Detailed field jointing procedure.
    - Detailed repair procedure.
    - Detailed procedures for handling and storage of line-pipe.
    - Detailed Quality plans / Inspection and Test Plan (ITP). All witness and hold points shall be identified.
    - Test records and results.
    - Inspection reports and records.
    - Repair and recoating records.
    - All relevant coating application variables.
    - The personnel qualification record shall constitute proof that the personnel designated to carry out the work are properly qualified to do so.

The following list shows the deliverables and structure of the fabrication records for Concrete structures:
 - FRB User guide - Describes the content of each deliverable in the FRB and how they relate and refer to each other. Include examples (images) of how to trace welds and material certificates from fabrication drawings;
 - Index of Concrete fabrication and detail drawings;  
 - Index of material, design, fabrication specifications and documents used by Contractor;   
 - Index of Construction sequence drawings, e.g. dry dock, inshore, tow-to field and installation;
 - Reinforcement bar lists;
 - Concrete mix specification (cement, aggregate, inhibitors, etc.);
 - Test records of compression- and tension capacity of actual fabricated concrete;
 - Material certificates reinforcement.</rdl:PCA_100006768>
    <skos:broader rdf:resource="http://rds.posccaesar.org/ontology/plm/rdl/PCA_100006749"/>
    <rdl:PCA_100006766 rdf:resource="http://rds.posccaesar.org/ontology/plm/rdl/PCA_100006653"/>
  </owl:Class>
  <owl:Class rdf:about="http://rds.posccaesar.org/ontology/plm/rdl/PCA_100006340">
    <skos:broadMatch rdf:resource="http://rds.posccaesar.org/ontology/plm/rdl/PCA_100006724"/>
    <rdfs:label>Non-conformance / concession reports / technical queries</rdfs:label>
    <rdfs:comment>Report stating a deviation from standards and/or specifications, and issue of technical queries.</rdfs:comment>
    <rdl:PCA_100006768>Report stating a deviation from standards and/or specifications, and issue of technical queries.</rdl:PCA_100006768>
    <rdl:PCA_100006766 rdf:resource="http://rds.posccaesar.org/ontology/plm/rdl/PCA_100006653"/>
    <rdl:PCA_100006765 rdf:resource="http://w3id.org/readi/rdl/CFIHOS-20000031"/>
    <rdl:PCA_100006763>To document deviations and clarify technical issues.</rdl:PCA_100006763>
    <rdfs:subClassOf rdf:resource="http://rds.posccaesar.org/ontology/plm/rdl/PCA_100004908"/>
  </owl:Class>
  <owl:Class rdf:about="http://rds.posccaesar.org/ontology/plm/rdl/PCA_100006131">
    <rdl:PCA_100006765 rdf:resource="http://w3id.org/readi/rdl/CFIHOS-20000007"/>
    <skos:broadMatch rdf:resource="http://rds.posccaesar.org/ontology/plm/rdl/PCA_100006707"/>
    <rdl:PCA_100006766 rdf:resource="http://rds.posccaesar.org/ontology/plm/rdl/PCA_100006656"/>
    <rdl:PCA_100006764>The following drawings shall be delivered:
 - All reinforcement types (tensile-, shear, pretension reinforcement, other if applicable);
 - Reinforcement dimensions, quantity and location in concrete structure;
 - Material properties.</rdl:PCA_100006764>
    <rdl:PCA_100006768>Ref. generic general arrangement drawing</rdl:PCA_100006768>
    <skos:broadMatch rdf:resource="http://rds.posccaesar.org/ontology/plm/rdl/PCA_100006731"/>
    <skos:broadMatch rdf:resource="http://rds.posccaesar.org/ontology/plm/rdl/PCA_100006732"/>
    <rdfs:comment>Ref. generic general arrangement drawing</rdfs:comment>
    <rdfs:subClassOf rdf:resource="http://rds.posccaesar.org/ontology/plm/rdl/PCA_100004908"/>
    <rdfs:label>Concrete structures reinforcement drawings</rdfs:label>
    <skos:broader rdf:resource="http://rds.posccaesar.org/ontology/plm/rdl/PCA_100006746"/>
  </owl:Class>
  <owl:Class rdf:about="http://rds.posccaesar.org/ontology/plm/rdl/PCA_100006143">
    <skos:broader rdf:resource="http://rds.posccaesar.org/ontology/plm/rdl/PCA_100006756"/>
    <skos:broadMatch rdf:resource="http://rds.posccaesar.org/ontology/plm/rdl/PCA_100006722"/>
    <rdfs:label>Data and telephone cabling network test reports</rdfs:label>
    <rdfs:comment>Test reports for Data and telephone cabling network (category type copper cables) shall be provided. Test per outlet.</rdfs:comment>
    <rdl:PCA_100006768>Test reports for Data and telephone cabling network (category type copper cables) shall be provided. Test per outlet.</rdl:PCA_100006768>
    <rdl:PCA_100006766 rdf:resource="http://rds.posccaesar.org/ontology/plm/rdl/PCA_100006653"/>
    <rdl:PCA_100006765 rdf:resource="http://w3id.org/readi/rdl/CFIHOS-20000030"/>
    <rdfs:subClassOf rdf:resource="http://rds.posccaesar.org/ontology/plm/rdl/PCA_100004908"/>
  </owl:Class>
  <owl:Class rdf:about="http://rds.posccaesar.org/ontology/plm/rdl/PCA_100006155">
    <skos:broader rdf:resource="http://rds.posccaesar.org/ontology/plm/rdl/PCA_100006741"/>
    <rdfs:label>Design calculations and analyses report</rdfs:label>
    <rdfs:comment>A report providing calculations of the load cases defined for the equipment with reference to applicable standards.</rdfs:comment>
    <rdl:PCA_100006768>A report providing calculations of the load cases defined for the equipment with reference to applicable standards.</rdl:PCA_100006768>
    <rdl:PCA_100006766 rdf:resource="http://rds.posccaesar.org/ontology/plm/rdl/PCA_100006653"/>
    <rdl:PCA_100006763>A report providing calculations of the load cases defined for the equipment with reference to applicable standards. The report shall contain loads and load cases as per design basis.</rdl:PCA_100006763>
    <rdfs:subClassOf rdf:resource="http://rds.posccaesar.org/ontology/plm/rdl/PCA_100004908"/>
  </owl:Class>
  <owl:Class rdf:about="http://rds.posccaesar.org/ontology/plm/rdl/PCA_100006167">
    <skos:broader rdf:resource="http://rds.posccaesar.org/ontology/plm/rdl/PCA_100006749"/>
    <skos:broadMatch rdf:resource="http://rds.posccaesar.org/ontology/plm/rdl/PCA_100006668"/>
    <rdfs:label>Documentation for dispatch, receipt, storage and preservation</rdfs:label>
    <rdfs:comment>Documentation available to recipient prior to delivery The following documentation shall be available to the recipient prior to delivery of the equipment:
 - Procedure for receiving inspection required by the supplier
 - Guidelines for lifting and handling
 - Requirements for storage and preservation 

Documentation available to recipient at delivery The following documentation shall be available to the recipient no later than at delivery of the equipment:
 - Packing lists
 - Instructions for unpacking, if special precautions are required during unpacking
 - Completed forms for mechanical completion. This applies only if the order includes a clause stating that the supplier shall complete forms forming a part of the purchaser’s system for mechanical completion
 - Preservation log, if this is specified in the order
 - Certificate for temporary lifting equipment</rdfs:comment>
    <rdl:PCA_100006768>Documentation available to recipient prior to delivery The following documentation shall be available to the recipient prior to delivery of the equipment:
 - Procedure for receiving inspection required by the supplier
 - Guidelines for lifting and handling
 - Requirements for storage and preservation 

Documentation available to recipient at delivery The following documentation shall be available to the recipient no later than at delivery of the equipment:
 - Packing lists
 - Instructions for unpacking, if special precautions are required during unpacking
 - Completed forms for mechanical completion. This applies only if the order includes a clause stating that the supplier shall complete forms forming a part of the purchaser’s system for mechanical completion
 - Preservation log, if this is specified in the order
 - Certificate for temporary lifting equipment</rdl:PCA_100006768>
    <rdl:PCA_100006765>
      <rdl:PCA_100001503 rdf:about="http://w3id.org/readi/rdl/CFIHOS-20000029">
        <rdfs:label>logistics management</rdfs:label>
        <rdl:PCA_100004924>SA</rdl:PCA_100004924>
        <rdf:type rdf:resource="http://www.w3.org/2002/07/owl#NamedIndividual"/>
      </rdl:PCA_100001503>
    </rdl:PCA_100006765>
    <rdl:PCA_100006763>The supplier shall supply the documentation needed to enable the customer to evaluate the dispatch and make plans for receipt, storage and installation of the equipment. 

Documentation shall be available to the customer prior to dispatch. Documentation for preservation, packing and transportation method shall be available to the customer prior to dispatch of the equipment.</rdl:PCA_100006763>
    <rdfs:subClassOf rdf:resource="http://rds.posccaesar.org/ontology/plm/rdl/PCA_100004908"/>
  </owl:Class>
  <owl:Class rdf:about="http://rds.posccaesar.org/ontology/plm/rdl/PCA_100006179">
    <rdl:PCA_100006765 rdf:resource="http://w3id.org/readi/rdl/CFIHOS-20000008"/>
    <rdfs:label>Electrical load list</rdfs:label>
    <rdfs:subClassOf rdf:resource="http://rds.posccaesar.org/ontology/plm/rdl/PCA_100004908"/>
    <rdl:PCA_100006766 rdf:resource="http://rds.posccaesar.org/ontology/plm/rdl/PCA_100006637"/>
    <rdl:PCA_100006766 rdf:resource="http://rds.posccaesar.org/ontology/plm/rdl/PCA_100006639"/>
    <skos:broadMatch rdf:resource="http://rds.posccaesar.org/ontology/plm/rdl/PCA_100006716"/>
    <rdl:PCA_100006766 rdf:resource="http://rds.posccaesar.org/ontology/plm/rdl/PCA_100006636"/>
    <rdfs:comment>An electrical load list shall be worked out based on the Main Equipment List and emergency and/or essential consumers clearly marked as such in the list. Load list shall include individual consumers on high and low voltage switchboards (motor control centers) as well as assumed sum load on 400/230 V level. Sum UPS load per UPS system shall be listed. Allowance and contingency requirements for the load list shall be applied.</rdfs:comment>
    <rdl:PCA_100006768>An electrical load list shall be worked out based on the Main Equipment List and emergency and/or essential consumers clearly marked as such in the list. Load list shall include individual consumers on high and low voltage switchboards (motor control centers) as well as assumed sum load on 400/230 V level. Sum UPS load per UPS system shall be listed. Allowance and contingency requirements for the load list shall be applied.</rdl:PCA_100006768>
    <rdl:PCA_100006766 rdf:resource="http://rds.posccaesar.org/ontology/plm/rdl/PCA_100006638"/>
    <rdl:PCA_100006763>See requirements to load study, ref. (Z-001-0052 - Electrical calculations / analyses). 
The purpose of this document is to define the electrical loading of the electrical power system.</rdl:PCA_100006763>
    <skos:broader rdf:resource="http://rds.posccaesar.org/ontology/plm/rdl/PCA_100006748"/>
    <rdl:PCA_100006766 rdf:resource="http://rds.posccaesar.org/ontology/plm/rdl/PCA_100006635"/>
    <skos:broadMatch rdf:resource="http://rds.posccaesar.org/ontology/plm/rdl/PCA_100006717"/>
    <rdl:PCA_100006766 rdf:resource="http://rds.posccaesar.org/ontology/plm/rdl/PCA_100006634"/>
  </owl:Class>
  <owl:Class rdf:about="http://rds.posccaesar.org/ontology/plm/rdl/PCA_100006268">
    <skos:broader rdf:resource="http://rds.posccaesar.org/ontology/plm/rdl/PCA_100006756"/>
    <rdfs:subClassOf rdf:resource="http://rds.posccaesar.org/ontology/plm/rdl/PCA_100004908"/>
    <rdl:PCA_100006766 rdf:resource="http://rds.posccaesar.org/ontology/plm/rdl/PCA_100006657"/>
    <rdl:PCA_100006768>The report shall give a thorough description of the inclining experiment, including method and weights.</rdl:PCA_100006768>
    <skos:broadMatch rdf:resource="http://rds.posccaesar.org/ontology/plm/rdl/PCA_100006722"/>
    <rdl:PCA_100006763>The report shall document the weight and centre of gravity for the lightship weight of the vessel.</rdl:PCA_100006763>
    <rdfs:comment>The report shall give a thorough description of the inclining experiment, including method and weights.</rdfs:comment>
    <rdl:PCA_100006765 rdf:resource="http://w3id.org/readi/rdl/CFIHOS-20000033"/>
    <rdfs:label>Inclination test report</rdfs:label>
  </owl:Class>
  <owl:Class rdf:about="http://rds.posccaesar.org/ontology/plm/rdl/PCA_100006389">
    <skos:broader rdf:resource="http://rds.posccaesar.org/ontology/plm/rdl/PCA_100006748"/>
    <skos:broadMatch rdf:resource="http://rds.posccaesar.org/ontology/plm/rdl/PCA_100006722"/>
    <rdfs:label>Pressure chart dossier (drilling / completion )</rdfs:label>
    <rdfs:comment>Documentation of all leak/pressure test performed during the construction of the well, shall contain: 
 - Time and date
 - Equipment tested
 - Volumes pumped and bleed back
 - Holding time
 - Pressure drop over holding time
 - Which pump used
 - Signature</rdfs:comment>
    <rdl:PCA_100006768>Documentation of all leak/pressure test performed during the construction of the well, shall contain: 
 - Time and date
 - Equipment tested
 - Volumes pumped and bleed back
 - Holding time
 - Pressure drop over holding time
 - Which pump used
 - Signature</rdl:PCA_100006768>
    <rdl:PCA_100006765 rdf:resource="http://w3id.org/readi/rdl/CFIHOS-20000042"/>
    <rdl:PCA_100006763>To keep track of all pressure test charts performed during drilling/completion phase. Test data/chart documents the performance for each well barrier element installed during well construction phase</rdl:PCA_100006763>
    <rdfs:subClassOf rdf:resource="http://rds.posccaesar.org/ontology/plm/rdl/PCA_100004908"/>
  </owl:Class>
  <owl:Class rdf:about="http://rds.posccaesar.org/ontology/plm/rdl/PCA_100006377">
    <skos:broadMatch rdf:resource="http://rds.posccaesar.org/ontology/plm/rdl/PCA_100006733"/>
    <rdfs:subClassOf rdf:resource="http://rds.posccaesar.org/ontology/plm/rdl/PCA_100004908"/>
    <rdl:PCA_100006766 rdf:resource="http://rds.posccaesar.org/ontology/plm/rdl/PCA_100006653"/>
    <rdl:PCA_100006768>The piping isometric shall be arranged such that it gives a clear readability. The piping line shall be split into reasonable large sections such that the drawing is not too crowded and at the same time avoid unnecessary small sections.

The following information shall be included:
 - Position numbers for each piping item;
 - Weld locations and numbers (field welds to be identified);
 - Flow arrow;
 - All inline equipment and instrument connections with tag numbers;
 - Special items with coding;
 - Dimensioned pipe support locations and support numbers including spring supports, etc.;
 - Penetrations;
 - Dimensions (including slope if relevant);
 - Reference to connecting isometric drawings;
 - Reference to attached equipment with tag number and nozzle number;
 - Bill of material including position numbers;
 - Line number (according to ENS);
 - Design pressures and temperatures;
 - Pressure test requirements;
 - NDT requirements;
 - Insulation requirements;
 - Heat trace requirements;
 - Surface treatment and topcoat colour requirements;
 - Service colour coding requirements;
 - Post weld heat treatment (PWHT) requirements;
 - Chemical cleaning requirements;
 - Pressure directive (PED) category (for EU countries);
 - Critical line and reference to Stress ISO no.;
 - Reference to P&amp;ID;
 - Area code;
 - Material type;
 - Dry weight, wet weight (content) and CoG.

NOTE: For equipment packages where the amount and size of piping is moderate, or the piping might be mostly for support functions (cooling, lubrication, drain etc.), piping isometrics from the manufacturer are not necessary. For large packages with a considerable amount of larger piping, isometrics for the main piping should be delivered. Selection should be done early in the project.</rdl:PCA_100006768>
    <skos:broadMatch rdf:resource="http://rds.posccaesar.org/ontology/plm/rdl/PCA_100006732"/>
    <skos:broader rdf:resource="http://rds.posccaesar.org/ontology/plm/rdl/PCA_100006746"/>
    <rdfs:label>Piping isometrics</rdfs:label>
    <skos:broadMatch rdf:resource="http://rds.posccaesar.org/ontology/plm/rdl/PCA_100006734"/>
    <rdl:PCA_100006765 rdf:resource="http://w3id.org/readi/rdl/CFIHOS-20000020"/>
    <rdfs:comment>The piping isometric shall be arranged such that it gives a clear readability. The piping line shall be split into reasonable large sections such that the drawing is not too crowded and at the same time avoid unnecessary small sections.

The following information shall be included:
 - Position numbers for each piping item;
 - Weld locations and numbers (field welds to be identified);
 - Flow arrow;
 - All inline equipment and instrument connections with tag numbers;
 - Special items with coding;
 - Dimensioned pipe support locations and support numbers including spring supports, etc.;
 - Penetrations;
 - Dimensions (including slope if relevant);
 - Reference to connecting isometric drawings;
 - Reference to attached equipment with tag number and nozzle number;
 - Bill of material including position numbers;
 - Line number (according to ENS);
 - Design pressures and temperatures;
 - Pressure test requirements;
 - NDT requirements;
 - Insulation requirements;
 - Heat trace requirements;
 - Surface treatment and topcoat colour requirements;
 - Service colour coding requirements;
 - Post weld heat treatment (PWHT) requirements;
 - Chemical cleaning requirements;
 - Pressure directive (PED) category (for EU countries);
 - Critical line and reference to Stress ISO no.;
 - Reference to P&amp;ID;
 - Area code;
 - Material type;
 - Dry weight, wet weight (content) and CoG.

NOTE: For equipment packages where the amount and size of piping is moderate, or the piping might be mostly for support functions (cooling, lubrication, drain etc.), piping isometrics from the manufacturer are not necessary. For large packages with a considerable amount of larger piping, isometrics for the main piping should be delivered. Selection should be done early in the project.</rdfs:comment>
    <skos:broadMatch rdf:resource="http://rds.posccaesar.org/ontology/plm/rdl/PCA_100006708"/>
  </owl:Class>
  <owl:Class rdf:about="http://rds.posccaesar.org/ontology/plm/rdl/PCA_100006256">
    <rdfs:comment>The HVAC control philosophy shall as a minimum include: 
 - Heating/cooling control;
 - Fan control;
 - Start/stop sequence;
 - Vibration monitoring;
 - Flow control;
 - Shut down;
 - Gas/fire/smoke control;
 - Operational modes;
 - Central control system;
 - Local control/indicators.</rdfs:comment>
    <skos:broader rdf:resource="http://rds.posccaesar.org/ontology/plm/rdl/PCA_100006752"/>
    <rdl:PCA_100006768>The HVAC control philosophy shall as a minimum include: 
 - Heating/cooling control;
 - Fan control;
 - Start/stop sequence;
 - Vibration monitoring;
 - Flow control;
 - Shut down;
 - Gas/fire/smoke control;
 - Operational modes;
 - Central control system;
 - Local control/indicators.</rdl:PCA_100006768>
    <skos:broadMatch rdf:resource="http://rds.posccaesar.org/ontology/plm/rdl/PCA_100006695"/>
    <rdl:PCA_100006766 rdf:resource="http://rds.posccaesar.org/ontology/plm/rdl/PCA_100006650"/>
    <rdfs:label>HVAC control philosophy</rdfs:label>
    <rdl:PCA_100006765 rdf:resource="http://w3id.org/readi/rdl/CFIHOS-20000019"/>
    <rdfs:subClassOf rdf:resource="http://rds.posccaesar.org/ontology/plm/rdl/PCA_100004908"/>
    <skos:broadMatch rdf:resource="http://rds.posccaesar.org/ontology/plm/rdl/PCA_100006698"/>
  </owl:Class>
  <owl:Class rdf:about="http://rds.posccaesar.org/ontology/plm/rdl/PCA_100006365">
    <rdfs:label>Pipe support drawings</rdfs:label>
    <rdfs:comment>The following information shall be included:
 - Dimensioned plan, elevation, sectional and iso views as required;
 - Centre of gravity location and coordinates;
 - Weight;
 - Material identification and description (bill of material);
 - Line numbers for all supported lines;
 - Reference to stress isometric if relevant;
 - Reference to support calculations if relevant;
 - Reference to connected pipe support assemblies / spring support assemblies;
 - The drawing title shall include the pipe support number.

NOTE: For equipment packages where the amount and size of piping is moderate, or the piping might be mostly for support functions (cooling, lubrication, drain etc.), pipe support drawings from the manufacturer are not necessary.  For large packages with a considerable amount of larger piping, pipe support drawings for the main piping should be delivered.  Selection should be done early in the project.</rdfs:comment>
    <rdl:PCA_100006763>Detail drawings describing the support installed shall be provided for all pipe supports (pipe support assemblies and spring support assemblies).</rdl:PCA_100006763>
    <rdfs:subClassOf rdf:resource="http://rds.posccaesar.org/ontology/plm/rdl/PCA_100004908"/>
    <skos:broadMatch rdf:resource="http://rds.posccaesar.org/ontology/plm/rdl/PCA_100006733"/>
    <rdl:PCA_100006766 rdf:resource="http://rds.posccaesar.org/ontology/plm/rdl/PCA_100006653"/>
    <rdl:PCA_100006768>The following information shall be included:
 - Dimensioned plan, elevation, sectional and iso views as required;
 - Centre of gravity location and coordinates;
 - Weight;
 - Material identification and description (bill of material);
 - Line numbers for all supported lines;
 - Reference to stress isometric if relevant;
 - Reference to support calculations if relevant;
 - Reference to connected pipe support assemblies / spring support assemblies;
 - The drawing title shall include the pipe support number.

NOTE: For equipment packages where the amount and size of piping is moderate, or the piping might be mostly for support functions (cooling, lubrication, drain etc.), pipe support drawings from the manufacturer are not necessary.  For large packages with a considerable amount of larger piping, pipe support drawings for the main piping should be delivered.  Selection should be done early in the project.</rdl:PCA_100006768>
    <skos:broadMatch rdf:resource="http://rds.posccaesar.org/ontology/plm/rdl/PCA_100006732"/>
    <skos:broader rdf:resource="http://rds.posccaesar.org/ontology/plm/rdl/PCA_100006746"/>
    <rdl:PCA_100006765 rdf:resource="http://w3id.org/readi/rdl/CFIHOS-20000020"/>
    <skos:broadMatch rdf:resource="http://rds.posccaesar.org/ontology/plm/rdl/PCA_100006734"/>
    <skos:broadMatch rdf:resource="http://rds.posccaesar.org/ontology/plm/rdl/PCA_100006731"/>
  </owl:Class>
  <owl:Class rdf:about="http://rds.posccaesar.org/ontology/plm/rdl/PCA_100006498">
    <rdl:PCA_100006765 rdf:resource="http://w3id.org/readi/rdl/CFIHOS-20000018"/>
    <rdl:PCA_100006768>Shall be according to ISO 15589-1.</rdl:PCA_100006768>
    <rdfs:subClassOf rdf:resource="http://rds.posccaesar.org/ontology/plm/rdl/PCA_100004908"/>
    <skos:broader rdf:resource="http://rds.posccaesar.org/ontology/plm/rdl/PCA_100006756"/>
    <rdl:PCA_100006763>Ensure safe operation</rdl:PCA_100006763>
    <rdl:PCA_100006766 rdf:resource="http://rds.posccaesar.org/ontology/plm/rdl/PCA_100006657"/>
    <skos:broadMatch rdf:resource="http://rds.posccaesar.org/ontology/plm/rdl/PCA_100006722"/>
    <rdfs:comment>Shall be according to ISO 15589-1.</rdfs:comment>
    <rdfs:label>Test results onshore CP system, coating quality and insulating joint</rdfs:label>
  </owl:Class>
  <owl:Class rdf:about="http://rds.posccaesar.org/ontology/plm/rdl/PCA_100006244">
    <rdfs:subClassOf rdf:resource="http://rds.posccaesar.org/ontology/plm/rdl/PCA_100004908"/>
    <rdfs:label>Ground investigation reports</rdfs:label>
    <skos:broadMatch rdf:resource="http://rds.posccaesar.org/ontology/plm/rdl/PCA_100006722"/>
    <rdl:PCA_100006765 rdf:resource="http://w3id.org/readi/rdl/CFIHOS-20000007"/>
    <rdl:PCA_100006763>The requirement shall apply to field investigations, laboratory tests and analyses. 

ISO 14688, ISO 14689, ISO 17892 Geotechnical investigations and testing;
EN 1997 Geotechnical design;
BS6031 Code of practice for earthworks.</rdl:PCA_100006763>
    <rdl:PCA_100006766 rdf:resource="http://rds.posccaesar.org/ontology/plm/rdl/PCA_100006656"/>
    <skos:broader rdf:resource="http://rds.posccaesar.org/ontology/plm/rdl/PCA_100006756"/>
    <rdfs:comment>The content and structure of the reports shall comply with the requirements in EN1997 or equivalent standard.</rdfs:comment>
    <rdl:PCA_100006768>The content and structure of the reports shall comply with the requirements in EN1997 or equivalent standard.</rdl:PCA_100006768>
  </owl:Class>
  <owl:Class rdf:about="http://rds.posccaesar.org/ontology/plm/rdl/PCA_100006486">
    <rdfs:comment>The plan shall include information about capacity and boundaries of all tanks and compartments.</rdfs:comment>
    <rdl:PCA_100006766 rdf:resource="http://rds.posccaesar.org/ontology/plm/rdl/PCA_100006654"/>
    <rdl:PCA_100006763>To document compliance with the PSA facilities regulations § 62 and NMA Regulations No. 878 in addition to IMO instruments and Class requirements, as applicable.</rdl:PCA_100006763>
    <skos:broadMatch rdf:resource="http://rds.posccaesar.org/ontology/plm/rdl/PCA_100006707"/>
    <rdl:PCA_100006768>The plan shall include information about capacity and boundaries of all tanks and compartments.</rdl:PCA_100006768>
    <rdfs:label>Tank plan</rdfs:label>
    <skos:broader rdf:resource="http://rds.posccaesar.org/ontology/plm/rdl/PCA_100006753"/>
    <rdl:PCA_100006765 rdf:resource="http://w3id.org/readi/rdl/CFIHOS-20000033"/>
    <rdfs:subClassOf rdf:resource="http://rds.posccaesar.org/ontology/plm/rdl/PCA_100004908"/>
  </owl:Class>
  <owl:Class rdf:about="http://rds.posccaesar.org/ontology/plm/rdl/PCA_100006232">
    <rdfs:comment>A document summarizing relevant design data and performance requirements for the sub-system and also containing specific design data and performance requirements for the equipment.</rdfs:comment>
    <skos:broader rdf:resource="http://rds.posccaesar.org/ontology/plm/rdl/PCA_100006757"/>
    <rdfs:label>Functional design specification</rdfs:label>
    <skos:broadMatch rdf:resource="http://rds.posccaesar.org/ontology/plm/rdl/PCA_100006687"/>
    <rdfs:subClassOf rdf:resource="http://rds.posccaesar.org/ontology/plm/rdl/PCA_100004908"/>
    <rdl:PCA_100006763>The document provides input for detailed design and describes equipment design and functional requirements.</rdl:PCA_100006763>
    <rdl:PCA_100006766 rdf:resource="http://rds.posccaesar.org/ontology/plm/rdl/PCA_100006657"/>
    <rdl:PCA_100006765 rdf:resource="http://w3id.org/readi/rdl/CFIHOS-20000031"/>
    <rdl:PCA_100006768>A document summarizing relevant design data and performance requirements for the sub-system and also containing specific design data and performance requirements for the equipment.</rdl:PCA_100006768>
  </owl:Class>
  <owl:Class rdf:about="http://rds.posccaesar.org/ontology/plm/rdl/PCA_100006474">
    <skos:broader rdf:resource="http://rds.posccaesar.org/ontology/plm/rdl/PCA_100006748"/>
    <skos:broadMatch rdf:resource="http://rds.posccaesar.org/ontology/plm/rdl/PCA_100006663"/>
    <rdfs:label>Supplier list</rdfs:label>
    <rdfs:comment>List of Sub-suppliers</rdfs:comment>
    <rdl:PCA_100006768>List of Sub-suppliers</rdl:PCA_100006768>
    <rdl:PCA_100006766 rdf:resource="http://rds.posccaesar.org/ontology/plm/rdl/PCA_100006653"/>
    <rdl:PCA_100006763>For use by purchaser</rdl:PCA_100006763>
    <rdfs:subClassOf rdf:resource="http://rds.posccaesar.org/ontology/plm/rdl/PCA_100004908"/>
  </owl:Class>
  <owl:Class rdf:about="http://rds.posccaesar.org/ontology/plm/rdl/PCA_100006353">
    <rdl:PCA_100006763>Overview of all permanent installation used for construction and installation along the pipeline, such as, but not limited to turn point and foundation for winches.</rdl:PCA_100006763>
    <skos:broadMatch rdf:resource="http://rds.posccaesar.org/ontology/plm/rdl/PCA_100006705"/>
    <rdfs:subClassOf rdf:resource="http://rds.posccaesar.org/ontology/plm/rdl/PCA_100004908"/>
    <rdl:PCA_100006765 rdf:resource="http://w3id.org/readi/rdl/CFIHOS-20000018"/>
    <rdfs:comment>Info to be recorded in the  As-Built revision of the Field Layout (GIS database)</rdfs:comment>
    <skos:broader rdf:resource="http://rds.posccaesar.org/ontology/plm/rdl/PCA_100006746"/>
    <rdl:PCA_100006766 rdf:resource="http://rds.posccaesar.org/ontology/plm/rdl/PCA_100006654"/>
    <rdfs:label>Overview of permanent auxiliary installations</rdfs:label>
    <skos:broadMatch rdf:resource="http://rds.posccaesar.org/ontology/plm/rdl/PCA_100006731"/>
    <rdl:PCA_100006768>Info to be recorded in the  As-Built revision of the Field Layout (GIS database)</rdl:PCA_100006768>
  </owl:Class>
  <owl:Class rdf:about="http://rds.posccaesar.org/ontology/plm/rdl/PCA_100006341">
    <rdfs:subClassOf rdf:resource="http://rds.posccaesar.org/ontology/plm/rdl/PCA_100004908"/>
    <rdl:PCA_100006765 rdf:resource="http://w3id.org/readi/rdl/CFIHOS-20000027"/>
    <rdl:PCA_100006768>This document shall contain a list stating all deviations from the requirements in the inquiry, and proposed alternative requirements.</rdl:PCA_100006768>
    <skos:broadMatch rdf:resource="http://rds.posccaesar.org/ontology/plm/rdl/PCA_100006724"/>
    <rdl:PCA_100006763>This document shall  document deviations from standards and/or specifications, and issue of
technical queries.</rdl:PCA_100006763>
    <skos:broader rdf:resource="http://rds.posccaesar.org/ontology/plm/rdl/PCA_100006756"/>
    <rdl:PCA_100006766 rdf:resource="http://rds.posccaesar.org/ontology/plm/rdl/PCA_100006653"/>
    <rdfs:comment>This document shall contain a list stating all deviations from the requirements in the inquiry, and proposed alternative requirements.</rdfs:comment>
    <rdfs:label>Non-conformity report</rdfs:label>
  </owl:Class>
  <owl:Class rdf:about="http://rds.posccaesar.org/ontology/plm/rdl/PCA_100006462">
    <skos:broader rdf:resource="http://rds.posccaesar.org/ontology/plm/rdl/PCA_100006746"/>
    <skos:broadMatch rdf:resource="http://rds.posccaesar.org/ontology/plm/rdl/PCA_100006733"/>
    <rdfs:label>Structural fire protection drawings</rdfs:label>
    <skos:broadMatch rdf:resource="http://rds.posccaesar.org/ontology/plm/rdl/PCA_100006727"/>
    <rdl:PCA_100006766 rdf:resource="http://rds.posccaesar.org/ontology/plm/rdl/PCA_100006656"/>
    <rdl:PCA_100006765 rdf:resource="http://w3id.org/readi/rdl/CFIHOS-20000006"/>
    <rdfs:comment>Drawings shall include the following minimum information:
 - Extent and thickness of fireproofing, including description of coating/paint for fire protection systems.</rdfs:comment>
    <rdfs:subClassOf rdf:resource="http://rds.posccaesar.org/ontology/plm/rdl/PCA_100004908"/>
    <skos:broadMatch rdf:resource="http://rds.posccaesar.org/ontology/plm/rdl/PCA_100006732"/>
    <skos:broadMatch rdf:resource="http://rds.posccaesar.org/ontology/plm/rdl/PCA_100006734"/>
    <skos:broadMatch rdf:resource="http://rds.posccaesar.org/ontology/plm/rdl/PCA_100006731"/>
    <rdl:PCA_100006768>Drawings shall include the following minimum information:
 - Extent and thickness of fireproofing, including description of coating/paint for fire protection systems.</rdl:PCA_100006768>
  </owl:Class>
  <owl:Class rdf:about="http://rds.posccaesar.org/ontology/plm/rdl/PCA_100006450">
    <skos:broader rdf:resource="http://rds.posccaesar.org/ontology/plm/rdl/PCA_100006756"/>
    <rdfs:label>Soil interaction report</rdfs:label>
    <rdfs:comment>Report documenting all calculations and analysis performed to show how equipment interacts with seabed / soil.</rdfs:comment>
    <rdl:PCA_100006768>Report documenting all calculations and analysis performed to show how equipment interacts with seabed / soil.</rdl:PCA_100006768>
    <rdl:PCA_100006766 rdf:resource="http://rds.posccaesar.org/ontology/plm/rdl/PCA_100006653"/>
    <rdl:PCA_100006765 rdf:resource="http://w3id.org/readi/rdl/CFIHOS-20000018"/>
    <rdl:PCA_100006763>To provide input to pipeline, riser or umbilical design with respect to soil interaction.</rdl:PCA_100006763>
    <rdfs:subClassOf rdf:resource="http://rds.posccaesar.org/ontology/plm/rdl/PCA_100004908"/>
  </owl:Class>
  <owl:Class rdf:about="http://rds.posccaesar.org/ontology/plm/rdl/PCA_100006130">
    <skos:broadMatch rdf:resource="http://rds.posccaesar.org/ontology/plm/rdl/PCA_100006731"/>
    <skos:broadMatch rdf:resource="http://rds.posccaesar.org/ontology/plm/rdl/PCA_100006732"/>
    <skos:broadMatch rdf:resource="http://rds.posccaesar.org/ontology/plm/rdl/PCA_100006733"/>
    <skos:broadMatch rdf:resource="http://rds.posccaesar.org/ontology/plm/rdl/PCA_100006734"/>
    <rdl:PCA_100006765 rdf:resource="http://w3id.org/readi/rdl/CFIHOS-20000006"/>
    <skos:broader rdf:resource="http://rds.posccaesar.org/ontology/plm/rdl/PCA_100006746"/>
    <rdfs:subClassOf rdf:resource="http://rds.posccaesar.org/ontology/plm/rdl/PCA_100004908"/>
    <rdfs:comment>The following detail drawings shall be delivered
 - General Arrangements 
 - Typicals 
 - Sections and details 
 - Concrete dimensions 
 - Material properties 
Details related to embedded items, block-outs, pre-stressing and post-tensioning of structures shall be included. 
For embedded items for lifting operations documentation of certificates shall be included. Structural load plans shall also be included.</rdfs:comment>
    <rdfs:label>Concrete structures geometry drawings</rdfs:label>
    <rdl:PCA_100006768>The following detail drawings shall be delivered
 - General Arrangements 
 - Typicals 
 - Sections and details 
 - Concrete dimensions 
 - Material properties 
Details related to embedded items, block-outs, pre-stressing and post-tensioning of structures shall be included. 
For embedded items for lifting operations documentation of certificates shall be included. Structural load plans shall also be included.</rdl:PCA_100006768>
  </owl:Class>
  <owl:Class rdf:about="http://rds.posccaesar.org/ontology/plm/rdl/PCA_100006142">
    <rdl:PCA_100006763>To document compliance with the PSA facilities regulations § 62 and NMA Regulations No. 878 in addition to IMO instruments and Class requirements, as applicable.</rdl:PCA_100006763>
    <rdl:PCA_100006765 rdf:resource="http://w3id.org/readi/rdl/CFIHOS-20000033"/>
    <rdl:PCA_100006768>The damage control plan and damage control booklet are intended to provide information for actions to mitigate the loss of stability in the event of a damage causing flooding. The damage control plan should include inboard profile, plan views of each deck and transverse sections to the extent necessary to show amongst others watertight subdivision and equipment related to maintaining the boundaries and effectiveness of the subdivision.</rdl:PCA_100006768>
    <rdl:PCA_100006766 rdf:resource="http://rds.posccaesar.org/ontology/plm/rdl/PCA_100006657"/>
    <skos:broader rdf:resource="http://rds.posccaesar.org/ontology/plm/rdl/PCA_100006753"/>
    <rdfs:subClassOf rdf:resource="http://rds.posccaesar.org/ontology/plm/rdl/PCA_100004908"/>
    <rdfs:comment>The damage control plan and damage control booklet are intended to provide information for actions to mitigate the loss of stability in the event of a damage causing flooding. The damage control plan should include inboard profile, plan views of each deck and transverse sections to the extent necessary to show amongst others watertight subdivision and equipment related to maintaining the boundaries and effectiveness of the subdivision.</rdfs:comment>
    <rdfs:label>Damage control plan</rdfs:label>
    <skos:broadMatch rdf:resource="http://rds.posccaesar.org/ontology/plm/rdl/PCA_100006707"/>
  </owl:Class>
  <owl:Class rdf:about="http://rds.posccaesar.org/ontology/plm/rdl/PCA_100006154">
    <rdl:PCA_100006766 rdf:resource="http://rds.posccaesar.org/ontology/plm/rdl/PCA_100006654"/>
    <skos:broadMatch rdf:resource="http://rds.posccaesar.org/ontology/plm/rdl/PCA_100006686"/>
    <skos:broader rdf:resource="http://rds.posccaesar.org/ontology/plm/rdl/PCA_100006756"/>
    <rdl:PCA_100006765 rdf:resource="http://w3id.org/readi/rdl/CFIHOS-20000018"/>
    <rdl:PCA_100006768>Covering all possible loads along the pipeline route such as 3rd party activities (e.g. anchoring, trawling, construction, traffic). Could be a part of pipeline desig report.</rdl:PCA_100006768>
    <rdfs:label>Design accidental loads report</rdfs:label>
    <rdfs:subClassOf rdf:resource="http://rds.posccaesar.org/ontology/plm/rdl/PCA_100004908"/>
    <rdl:PCA_100006763>Accidential load chosen to be used as basis for design. In the design phase, the design accidental load could be more conservative (higher) than the dimensioning accidental load, but should never be lower.</rdl:PCA_100006763>
    <rdfs:comment>Covering all possible loads along the pipeline route such as 3rd party activities (e.g. anchoring, trawling, construction, traffic). Could be a part of pipeline desig report.</rdfs:comment>
  </owl:Class>
  <owl:Class rdf:about="http://rds.posccaesar.org/ontology/plm/rdl/PCA_100006166">
    <rdl:PCA_100006768>A document shipped with equipment, enabling correct handling, transport, receipt, storage and preservation. Normally is the dispatch dossier a short version of the full MRB.</rdl:PCA_100006768>
    <rdl:PCA_100006766 rdf:resource="http://rds.posccaesar.org/ontology/plm/rdl/PCA_100006653"/>
    <rdfs:label>Dispatch dossier</rdfs:label>
    <skos:broader rdf:resource="http://rds.posccaesar.org/ontology/plm/rdl/PCA_100006762"/>
    <skos:broadMatch rdf:resource="http://rds.posccaesar.org/ontology/plm/rdl/PCA_100006668"/>
    <rdfs:subClassOf rdf:resource="http://rds.posccaesar.org/ontology/plm/rdl/PCA_100004908"/>
    <rdl:PCA_100006763>A compound document typically containing the following;packing lists, instructions for transport, handling, lifting and preservation, instructions for unpacking if applicable, completed applicable forms for mechanical completion, certificate of conformity, data sheets, preservation log, certificate for lifting equipment, material certificates.</rdl:PCA_100006763>
    <rdfs:comment>A document shipped with equipment, enabling correct handling, transport, receipt, storage and preservation. Normally is the dispatch dossier a short version of the full MRB.</rdfs:comment>
    <rdl:PCA_100006765 rdf:resource="http://w3id.org/readi/rdl/CFIHOS-20000031"/>
  </owl:Class>
  <owl:Class rdf:about="http://rds.posccaesar.org/ontology/plm/rdl/PCA_100006178">
    <skos:broader rdf:resource="http://rds.posccaesar.org/ontology/plm/rdl/PCA_100006746"/>
    <skos:broadMatch rdf:resource="http://rds.posccaesar.org/ontology/plm/rdl/PCA_100006710"/>
    <rdfs:label>Electrical field equipment layout drawings</rdfs:label>
    <rdfs:comment>At least one field equipment layout drawing for each area or module deck level shall be produced. The size of the facility will determine the scale of the drawing, but normally a scale of 1:100 on A3 format shall be aimed for. If required several drawings per area can be necessary to achieve this scale. Equipment which is covered by platforms above shall be shown dotted or shown in separate figures.

The following content shall be included on the drawings:
 - Platform/plant northing and orientation with respect of true north;
 - Gridlines with north and east references;
 - Key plan;
 - Scale bar;
 - Match lines with drawing references;
 - Deck/area elevations;
 - Location of electrical field equipment as identified in MEL;
 - Equipment shall be tagged according to MEL.</rdfs:comment>
    <rdl:PCA_100006768>At least one field equipment layout drawing for each area or module deck level shall be produced. The size of the facility will determine the scale of the drawing, but normally a scale of 1:100 on A3 format shall be aimed for. If required several drawings per area can be necessary to achieve this scale. Equipment which is covered by platforms above shall be shown dotted or shown in separate figures.

The following content shall be included on the drawings:
 - Platform/plant northing and orientation with respect of true north;
 - Gridlines with north and east references;
 - Key plan;
 - Scale bar;
 - Match lines with drawing references;
 - Deck/area elevations;
 - Location of electrical field equipment as identified in MEL;
 - Equipment shall be tagged according to MEL.</rdl:PCA_100006768>
    <rdl:PCA_100006766 rdf:resource="http://rds.posccaesar.org/ontology/plm/rdl/PCA_100006656"/>
    <rdl:PCA_100006765 rdf:resource="http://w3id.org/readi/rdl/CFIHOS-20000008"/>
    <rdfs:subClassOf rdf:resource="http://rds.posccaesar.org/ontology/plm/rdl/PCA_100004908"/>
  </owl:Class>
  <owl:Class rdf:about="http://rds.posccaesar.org/ontology/plm/rdl/PCA_100006499">
    <skos:broader rdf:resource="http://rds.posccaesar.org/ontology/plm/rdl/PCA_100006741"/>
    <skos:broadMatch rdf:resource="http://rds.posccaesar.org/ontology/plm/rdl/PCA_100006687"/>
    <rdfs:label>Thermal calculations</rdfs:label>
    <rdfs:comment>ISO 12241
Calculation methods of heat transfer.</rdfs:comment>
    <rdl:PCA_100006768>ISO 12241
Calculation methods of heat transfer.</rdl:PCA_100006768>
    <rdl:PCA_100006766 rdf:resource="http://rds.posccaesar.org/ontology/plm/rdl/PCA_100006653"/>
    <rdl:PCA_100006763>Calculation of heat-transfer-related properties. This document gives a simplified approach for the treatment of thermal bridges.</rdl:PCA_100006763>
    <rdfs:subClassOf rdf:resource="http://rds.posccaesar.org/ontology/plm/rdl/PCA_100004908"/>
  </owl:Class>
  <owl:Class rdf:about="http://rds.posccaesar.org/ontology/plm/rdl/PCA_100006269">
    <skos:broader rdf:resource="http://rds.posccaesar.org/ontology/plm/rdl/PCA_100006748"/>
    <rdfs:label>Index information</rdfs:label>
    <rdl:PCA_100006766 rdf:resource="http://rds.posccaesar.org/ontology/plm/rdl/PCA_100006654"/>
    <rdfs:subClassOf rdf:resource="http://rds.posccaesar.org/ontology/plm/rdl/PCA_100004908"/>
  </owl:Class>
  <owl:Class rdf:about="http://rds.posccaesar.org/ontology/plm/rdl/PCA_100006378">
    <skos:broadMatch rdf:resource="http://rds.posccaesar.org/ontology/plm/rdl/PCA_100006708"/>
    <rdfs:subClassOf rdf:resource="http://rds.posccaesar.org/ontology/plm/rdl/PCA_100004908"/>
    <rdl:PCA_100006768>Piping stress isometrics shall include the following information:
 - Line number;
 - Process data (temp. and pressure);
 - Valve weights;
 - Equipment nozzle loads;
 - Stress summary;
 - Reference to P&amp;ID;
 - Restraint loading and displacement;
 - Spring summary;
 - Calculation No.;
 - Separate document no with revision code on each stress iso (not stress report number);
 - Special supports, typical: gap, adjustable, PTFE;
 - Equipment nozzle with tag no;
 - Pipe specification break;
 - Reference to adjacent isometric drawings;
 - Special items;
 - Penetrations;
 - Pipe stress report no;
 - Dimensioned pipe support locations and support numbers including spring supports, etc.;
 - Node numbers from calculation model (as a minimum for each pipe support, valve, equipment nozzle, interface to other lines/sheets/isometrics and location for max utilisation).
- Support function

NOTE: For equipment packages where the amount and size of piping is moderate, or the piping might be mostly for support functions (cooling, lubrication, drain etc.), piping stress isometrics from the manufacturer are not necessary.  For large packages with a considerable amount of larger piping, piping stress isometrics for the main piping should be delivered.  Selection should be done early in the project.</rdl:PCA_100006768>
    <rdl:PCA_100006765 rdf:resource="http://w3id.org/readi/rdl/CFIHOS-20000020"/>
    <rdfs:label>Piping stress isometrics</rdfs:label>
    <rdl:PCA_100006763>Piping stress isometrics shall be provided for all lines for which stress calculations or evaluation have been made.</rdl:PCA_100006763>
    <rdfs:comment>Piping stress isometrics shall include the following information:
 - Line number;
 - Process data (temp. and pressure);
 - Valve weights;
 - Equipment nozzle loads;
 - Stress summary;
 - Reference to P&amp;ID;
 - Restraint loading and displacement;
 - Spring summary;
 - Calculation No.;
 - Separate document no with revision code on each stress iso (not stress report number);
 - Special supports, typical: gap, adjustable, PTFE;
 - Equipment nozzle with tag no;
 - Pipe specification break;
 - Reference to adjacent isometric drawings;
 - Special items;
 - Penetrations;
 - Pipe stress report no;
 - Dimensioned pipe support locations and support numbers including spring supports, etc.;
 - Node numbers from calculation model (as a minimum for each pipe support, valve, equipment nozzle, interface to other lines/sheets/isometrics and location for max utilisation).
- Support function

NOTE: For equipment packages where the amount and size of piping is moderate, or the piping might be mostly for support functions (cooling, lubrication, drain etc.), piping stress isometrics from the manufacturer are not necessary.  For large packages with a considerable amount of larger piping, piping stress isometrics for the main piping should be delivered.  Selection should be done early in the project.</rdfs:comment>
    <skos:broadMatch rdf:resource="http://rds.posccaesar.org/ontology/plm/rdl/PCA_100006732"/>
    <skos:broader rdf:resource="http://rds.posccaesar.org/ontology/plm/rdl/PCA_100006746"/>
    <rdl:PCA_100006766 rdf:resource="http://rds.posccaesar.org/ontology/plm/rdl/PCA_100006653"/>
  </owl:Class>
  <owl:Class rdf:about="http://rds.posccaesar.org/ontology/plm/rdl/PCA_100006257">
    <rdfs:comment>The HVAC design philosophy shall as a minimum include: 
 - Purpose of HVAC installation;
 - Ambient conditions;
 - Indoor conditions;
 - Utilities for HVAC;
 - Natural ventilation;
 - Mechanical ventilation;
 - Sparing philosophy;
 - Pressurization;
 - Fire damper installation (LRA &amp; HRA);
 - Smoke ventilation;
 - Air inlets/outlets;
 - Black Start;
 - Ductwork;
 - Local cooling/heating.</rdfs:comment>
    <skos:broadMatch rdf:resource="http://rds.posccaesar.org/ontology/plm/rdl/PCA_100006698"/>
    <rdl:PCA_100006765 rdf:resource="http://w3id.org/readi/rdl/CFIHOS-20000019"/>
    <rdfs:subClassOf rdf:resource="http://rds.posccaesar.org/ontology/plm/rdl/PCA_100004908"/>
    <rdl:PCA_100006768>The HVAC design philosophy shall as a minimum include: 
 - Purpose of HVAC installation;
 - Ambient conditions;
 - Indoor conditions;
 - Utilities for HVAC;
 - Natural ventilation;
 - Mechanical ventilation;
 - Sparing philosophy;
 - Pressurization;
 - Fire damper installation (LRA &amp; HRA);
 - Smoke ventilation;
 - Air inlets/outlets;
 - Black Start;
 - Ductwork;
 - Local cooling/heating.</rdl:PCA_100006768>
    <skos:broader rdf:resource="http://rds.posccaesar.org/ontology/plm/rdl/PCA_100006752"/>
    <rdfs:label>HVAC design philosophy</rdfs:label>
    <skos:broadMatch rdf:resource="http://rds.posccaesar.org/ontology/plm/rdl/PCA_100006695"/>
    <rdl:PCA_100006766 rdf:resource="http://rds.posccaesar.org/ontology/plm/rdl/PCA_100006650"/>
  </owl:Class>
  <owl:Class rdf:about="http://rds.posccaesar.org/ontology/plm/rdl/PCA_100006245">
    <rdl:PCA_100006766 rdf:resource="http://rds.posccaesar.org/ontology/plm/rdl/PCA_100006633"/>
    <rdl:PCA_100006765 rdf:resource="http://w3id.org/readi/rdl/CFIHOS-20000015"/>
    <rdl:PCA_100006766 rdf:resource="http://rds.posccaesar.org/ontology/plm/rdl/PCA_100006626"/>
    <skos:broadMatch rdf:resource="http://rds.posccaesar.org/ontology/plm/rdl/PCA_100006734"/>
    <rdl:PCA_100006768>Hardware loop typicals shall cover:
 - Typicals for all field instrument interfaces.

Drawing should contain the following information:
 - Input/output from I/O-cards, barriers.
 - Field instrument information.</rdl:PCA_100006768>
    <skos:broadMatch rdf:resource="http://rds.posccaesar.org/ontology/plm/rdl/PCA_100006712"/>
    <rdl:PCA_100006766 rdf:resource="http://rds.posccaesar.org/ontology/plm/rdl/PCA_100006641"/>
    <rdfs:label>Hardware loop typicals</rdfs:label>
    <skos:broader rdf:resource="http://rds.posccaesar.org/ontology/plm/rdl/PCA_100006746"/>
    <rdfs:comment>Hardware loop typicals shall cover:
 - Typicals for all field instrument interfaces.

Drawing should contain the following information:
 - Input/output from I/O-cards, barriers.
 - Field instrument information.</rdfs:comment>
    <rdfs:subClassOf rdf:resource="http://rds.posccaesar.org/ontology/plm/rdl/PCA_100004908"/>
    <skos:broadMatch rdf:resource="http://rds.posccaesar.org/ontology/plm/rdl/PCA_100006713"/>
    <rdl:PCA_100006766 rdf:resource="http://rds.posccaesar.org/ontology/plm/rdl/PCA_100006627"/>
  </owl:Class>
  <owl:Class rdf:about="http://rds.posccaesar.org/ontology/plm/rdl/PCA_100006487">
    <skos:broadMatch rdf:resource="http://rds.posccaesar.org/ontology/plm/rdl/PCA_100006688"/>
    <rdl:PCA_100006768>The report shall include requirements not covered by design basis or codes.</rdl:PCA_100006768>
    <rdl:PCA_100006765 rdf:resource="http://w3id.org/readi/rdl/CFIHOS-20000018"/>
    <rdfs:label>Technical and functional requirements for unbonded flexible pipeline and riser</rdfs:label>
    <rdl:PCA_100006763>Overview of requirements used for design</rdl:PCA_100006763>
    <rdfs:comment>The report shall include requirements not covered by design basis or codes.</rdfs:comment>
    <rdfs:subClassOf rdf:resource="http://rds.posccaesar.org/ontology/plm/rdl/PCA_100004908"/>
    <skos:broader rdf:resource="http://rds.posccaesar.org/ontology/plm/rdl/PCA_100006757"/>
    <rdl:PCA_100006766 rdf:resource="http://rds.posccaesar.org/ontology/plm/rdl/PCA_100006654"/>
  </owl:Class>
  <owl:Class rdf:about="http://rds.posccaesar.org/ontology/plm/rdl/PCA_100006366">
    <skos:broader rdf:resource="http://rds.posccaesar.org/ontology/plm/rdl/PCA_100006748"/>
    <skos:broadMatch rdf:resource="http://rds.posccaesar.org/ontology/plm/rdl/PCA_100006716"/>
    <rdfs:label>Pipe support index</rdfs:label>
    <rdfs:comment>Index to contain:
 - Pipe support number;
 - Pipe support drawing number;
 - Line number;
 - Piping stress isometric drawing number;
 - Welded attachment (Yes/No);
 - Fire Protection (Yes/No);
 - Hook-up (Yes/No);
 - Temporary pipe support (Yes/No).</rdfs:comment>
    <rdl:PCA_100006768>Index to contain:
 - Pipe support number;
 - Pipe support drawing number;
 - Line number;
 - Piping stress isometric drawing number;
 - Welded attachment (Yes/No);
 - Fire Protection (Yes/No);
 - Hook-up (Yes/No);
 - Temporary pipe support (Yes/No).</rdl:PCA_100006768>
    <rdl:PCA_100006766 rdf:resource="http://rds.posccaesar.org/ontology/plm/rdl/PCA_100006653"/>
    <rdl:PCA_100006765 rdf:resource="http://w3id.org/readi/rdl/CFIHOS-20000020"/>
    <rdfs:subClassOf rdf:resource="http://rds.posccaesar.org/ontology/plm/rdl/PCA_100004908"/>
  </owl:Class>
  <owl:Class rdf:about="http://rds.posccaesar.org/ontology/plm/rdl/PCA_100006354">
    <rdl:PCA_100006763>This document shall provide requirements for storage, transport, lifting and preservation to maintain functionality and guarantees.</rdl:PCA_100006763>
    <rdfs:label>Packing, storage, preservation, lifting, transportation and handling procedure</rdfs:label>
    <rdl:PCA_100006768>A compound document that may contain: 
 - Packing lists
 - Instructions for transport
 - Handling
 - Lifting
 - Storage location and requirements
 - Preservation of the equipment during short- and long term storage
 - Maintenance intervals
 - Inspection intervals
 - Instructions for unpacking if applicable
 - Completed applicable forms for mechanical completion
 - Certificate of conformity, data sheets
 - Preservation log
 - Certificate for lifting equipment
 - Material certificates</rdl:PCA_100006768>
    <skos:broader rdf:resource="http://rds.posccaesar.org/ontology/plm/rdl/PCA_100006751"/>
    <skos:broadMatch rdf:resource="http://rds.posccaesar.org/ontology/plm/rdl/PCA_100006668"/>
    <rdfs:subClassOf rdf:resource="http://rds.posccaesar.org/ontology/plm/rdl/PCA_100004908"/>
    <rdl:PCA_100006766 rdf:resource="http://rds.posccaesar.org/ontology/plm/rdl/PCA_100006653"/>
    <rdfs:comment>A compound document that may contain: 
 - Packing lists
 - Instructions for transport
 - Handling
 - Lifting
 - Storage location and requirements
 - Preservation of the equipment during short- and long term storage
 - Maintenance intervals
 - Inspection intervals
 - Instructions for unpacking if applicable
 - Completed applicable forms for mechanical completion
 - Certificate of conformity, data sheets
 - Preservation log
 - Certificate for lifting equipment
 - Material certificates</rdfs:comment>
    <rdl:PCA_100006765 rdf:resource="http://w3id.org/readi/rdl/CFIHOS-20000029"/>
  </owl:Class>
  <owl:Class rdf:about="http://rds.posccaesar.org/ontology/plm/rdl/PCA_100006233">
    <skos:broader rdf:resource="http://rds.posccaesar.org/ontology/plm/rdl/PCA_100006739"/>
    <skos:broadMatch rdf:resource="http://rds.posccaesar.org/ontology/plm/rdl/PCA_100006710"/>
    <skos:broadMatch rdf:resource="http://rds.posccaesar.org/ontology/plm/rdl/PCA_100006708"/>
    <rdfs:label>General arrangement drawing</rdfs:label>
    <rdfs:comment>Below are examples of expected level of detail. One or more examples may apply.
For Mechanical equipment:
 - Dimensions
 - Location and identification of piping and main components
 - Necessary space for disassembly and maintenance
 - Location of centre of gravity
 - Thermal expansion effect, when relevant
 - On the structural steel drawings, critical welds shall be included with a weld 
identification number serving as a cross-reference to the weld summary index
 - Obstacles from other disciplines shall be included when relevant
 - Total weight, wet and dry and in operational condition
 - Weights, centre of gravity and main dimensions of disassembled units/components 
over 25 kg. Lifting lugs and runway beam for disassembling and their location shall 
be shown
 - Identification and location of all nozzle and external pipe connections as well as 
requirements for flexible connections and acceptable loads and moments. Locations 
shall be dimensioned and tolerances shown, if necessary in separate drawings
 - Identification and location of all external electrical and control monitoring connections 
(may be given in separate drawings describing the electrical arrangement and 
instrumentation)
 - For pressure equipment: for projects at locations where EU regulations for pressure 
equipment apply, Category and Module shall be according to 2014/68/EU (PED)
 - Include bolt tension requirements for pressure equipment flanges
 - Iidentification of lubrication points
 - Foundation information shall include:
     - The outer dimensions and footprint of the support frame or foundation supports
     - The size, grade and location of the foundation bolts and torque where this is 
necessary
     - Forces and moments transferred to load bearing structures, both under normal 
operation and extreme conditions
     - Details for adjustment and alignment
     - Details for cut-outs inside outer limit of foundation
     - Details for vibration dampening units (if installed)

For Electrical equipment:
 - Panel equipment layout - position of modules, cards, vacant slots and other 
information necessary for expansion or installation of new equipment in the same 
cabinet
 - Internal layout showing arrangement of auxiliary modules, cable trunks, etc.
 - All equipment including junction boxes, push buttons, light fittings, socket outlets, etc.
 - Dimensions
 - Necessary space for disassembly and maintenance
 - Location of centre of gravity
 - Possible thermal expansion
 - Obstacles from other disciplines shall be included when relevant

For Instrument equipment:
 - Dimensions
 - Location and identification of piping and main components
 - Necessary space for disassembly and maintenance
 - Location of centre of gravity
 - Possible thermal expansion
 - Obstacles from other disciplines shall be included when relevant
 - Panel equipment layout - position of modules, cards, vacant slots and other 
information necessary for expansion or installation of new equipment in the same 
cabinet
 - Internal/back layout showing arrangement of auxiliary modules, cable trunks, etc.
 - All equipment including technical network cabinets, junction boxes, push buttons, 
light fittings, socket outlets, etc.
 - Reference to part list/SPIR

For Telecom equipment:
A detailed drawing of the equipment shall be delivered. The drawing shall be to scale with 
dimensions included.
For Panel/cabinet/rack the following shall be included in addition:
 - Position of modules, cards, vacant slots and other information necessary for 
expansion or installation of new equipment in the same cabinet/rack
 - Internal/back layout showing arrangement of auxiliary modules, cable trunks, etc.

For HVAC equipment:
 - Dimensions
 - Location and identification of piping, ducting, MCTs (Multi core transit) and main 
components
 - Necessary space for disassembly and maintenance
 - Location of centre of gravity
 - Possible thermal expansion
 - Obstacles from other disciplines shall be included when relevant
Foundation information shall include:
     - The outer dimensions and footprint of the support frame or foundation supports
     - The size, grade and location of the foundation bolts and torque where this is 
necessary
     - Forces and moments transferred to load bearing structures, both under normal 
operation and extreme conditions
     - Details for adjustment and alignment
     - Details for cut-outs inside outer limit of foundation
     - Details for vibration dampening units (if installed)

For Lifting appliances:
General arrangement drawing of complete unit and foundation:
 - Dimensions
 - Location of centre of gravity
 - Total weight in operational condition
Foundation:
     - The outer dimensions and footprint of the support frame or foundation 
support
     - The size, grade and location of the foundation bolts and torque where this is 
necessary
     - Forces and moments transferred to load bearing structures, both under 
normal operation and extreme conditions
     - Details for adjustment and alignment
General arrangement drawing for Crane cabin, machinery room, winches, crane boom, 
slewing drives, main drive, hook block, wire sheave arrangements, etc.:
 - Dimensions
 - Location and identification of bolting, piping and main components
 - Location of centre of gravity
 - Total weight in operational condition
General arrangement drawing for inspections for primary steel structures e.g. 
pedestal/foundation, crane boom/traverse beams, A-frame, runway beams, winches, hook 
block, etc.
 - Critical welds shall be included with a weld identification number including weld
classification. NDT procedures and intervals for each weld classification shall be 
included.

For Well completion equipment:
Electrical submergible pump (ESP)
 - Dimensions
 - Weights, centre of gravity and main dimensions of disassembled 
units/components over 25 kg
Wellhead penetrator
 - Dimensions
 - Necessary space for disassembly and maintenance
 - Obstacles from other disciplines shall be included when relevant
 - All equipment including technical network cabinets, junction boxes, push buttons, 
light fittings, socket outlets, etc.
 - Parts list</rdfs:comment>
    <rdl:PCA_100006768>Below are examples of expected level of detail. One or more examples may apply.
For Mechanical equipment:
 - Dimensions
 - Location and identification of piping and main components
 - Necessary space for disassembly and maintenance
 - Location of centre of gravity
 - Thermal expansion effect, when relevant
 - On the structural steel drawings, critical welds shall be included with a weld 
identification number serving as a cross-reference to the weld summary index
 - Obstacles from other disciplines shall be included when relevant
 - Total weight, wet and dry and in operational condition
 - Weights, centre of gravity and main dimensions of disassembled units/components 
over 25 kg. Lifting lugs and runway beam for disassembling and their location shall 
be shown
 - Identification and location of all nozzle and external pipe connections as well as 
requirements for flexible connections and acceptable loads and moments. Locations 
shall be dimensioned and tolerances shown, if necessary in separate drawings
 - Identification and location of all external electrical and control monitoring connections 
(may be given in separate drawings describing the electrical arrangement and 
instrumentation)
 - For pressure equipment: for projects at locations where EU regulations for pressure 
equipment apply, Category and Module shall be according to 2014/68/EU (PED)
 - Include bolt tension requirements for pressure equipment flanges
 - Iidentification of lubrication points
 - Foundation information shall include:
     - The outer dimensions and footprint of the support frame or foundation supports
     - The size, grade and location of the foundation bolts and torque where this is 
necessary
     - Forces and moments transferred to load bearing structures, both under normal 
operation and extreme conditions
     - Details for adjustment and alignment
     - Details for cut-outs inside outer limit of foundation
     - Details for vibration dampening units (if installed)

For Electrical equipment:
 - Panel equipment layout - position of modules, cards, vacant slots and other 
information necessary for expansion or installation of new equipment in the same 
cabinet
 - Internal layout showing arrangement of auxiliary modules, cable trunks, etc.
 - All equipment including junction boxes, push buttons, light fittings, socket outlets, etc.
 - Dimensions
 - Necessary space for disassembly and maintenance
 - Location of centre of gravity
 - Possible thermal expansion
 - Obstacles from other disciplines shall be included when relevant

For Instrument equipment:
 - Dimensions
 - Location and identification of piping and main components
 - Necessary space for disassembly and maintenance
 - Location of centre of gravity
 - Possible thermal expansion
 - Obstacles from other disciplines shall be included when relevant
 - Panel equipment layout - position of modules, cards, vacant slots and other 
information necessary for expansion or installation of new equipment in the same 
cabinet
 - Internal/back layout showing arrangement of auxiliary modules, cable trunks, etc.
 - All equipment including technical network cabinets, junction boxes, push buttons, 
light fittings, socket outlets, etc.
 - Reference to part list/SPIR

For Telecom equipment:
A detailed drawing of the equipment shall be delivered. The drawing shall be to scale with 
dimensions included.
For Panel/cabinet/rack the following shall be included in addition:
 - Position of modules, cards, vacant slots and other information necessary for 
expansion or installation of new equipment in the same cabinet/rack
 - Internal/back layout showing arrangement of auxiliary modules, cable trunks, etc.

For HVAC equipment:
 - Dimensions
 - Location and identification of piping, ducting, MCTs (Multi core transit) and main 
components
 - Necessary space for disassembly and maintenance
 - Location of centre of gravity
 - Possible thermal expansion
 - Obstacles from other disciplines shall be included when relevant
Foundation information shall include:
     - The outer dimensions and footprint of the support frame or foundation supports
     - The size, grade and location of the foundation bolts and torque where this is 
necessary
     - Forces and moments transferred to load bearing structures, both under normal 
operation and extreme conditions
     - Details for adjustment and alignment
     - Details for cut-outs inside outer limit of foundation
     - Details for vibration dampening units (if installed)

For Lifting appliances:
General arrangement drawing of complete unit and foundation:
 - Dimensions
 - Location of centre of gravity
 - Total weight in operational condition
Foundation:
     - The outer dimensions and footprint of the support frame or foundation 
support
     - The size, grade and location of the foundation bolts and torque where this is 
necessary
     - Forces and moments transferred to load bearing structures, both under 
normal operation and extreme conditions
     - Details for adjustment and alignment
General arrangement drawing for Crane cabin, machinery room, winches, crane boom, 
slewing drives, main drive, hook block, wire sheave arrangements, etc.:
 - Dimensions
 - Location and identification of bolting, piping and main components
 - Location of centre of gravity
 - Total weight in operational condition
General arrangement drawing for inspections for primary steel structures e.g. 
pedestal/foundation, crane boom/traverse beams, A-frame, runway beams, winches, hook 
block, etc.
 - Critical welds shall be included with a weld identification number including weld
classification. NDT procedures and intervals for each weld classification shall be 
included.

For Well completion equipment:
Electrical submergible pump (ESP)
 - Dimensions
 - Weights, centre of gravity and main dimensions of disassembled 
units/components over 25 kg
Wellhead penetrator
 - Dimensions
 - Necessary space for disassembly and maintenance
 - Obstacles from other disciplines shall be included when relevant
 - All equipment including technical network cabinets, junction boxes, push buttons, 
light fittings, socket outlets, etc.
 - Parts list</rdl:PCA_100006768>
    <rdl:PCA_100006763>The manufacturer's standard general arrangement drawing shall be delivered. The content of the GA drawing must be adapted to the item described.</rdl:PCA_100006763>
    <rdfs:subClassOf rdf:resource="http://rds.posccaesar.org/ontology/plm/rdl/PCA_100004908"/>
  </owl:Class>
  <owl:Class rdf:about="http://rds.posccaesar.org/ontology/plm/rdl/PCA_100006475">
    <skos:broader rdf:resource="http://rds.posccaesar.org/ontology/plm/rdl/PCA_100006748"/>
    <skos:broadMatch>
      <rdl:PCA_100001503 rdf:about="http://rds.posccaesar.org/ontology/plm/rdl/PCA_100006660">
        <rdfs:label>reference information</rdfs:label>
        <rdl:PCA_100004924>AB</rdl:PCA_100004924>
        <rdf:type rdf:resource="http://www.w3.org/2002/07/owl#NamedIndividual"/>
      </rdl:PCA_100001503>
    </skos:broadMatch>
    <rdfs:label>Supplier master document list</rdfs:label>
    <rdfs:comment>This document shall give an overview of documentation relevant for the delivered equipment (PO) and schedule of documents to be delivered.
Documents shall be identified with title and document number.
To be developed by mutual agreement between the Buyer and Seller prior to placement of the Purchase Order (PO) and submitted for approval following PO placement to fully define the list of documents to be issued to Buyer by the Seller.</rdfs:comment>
    <rdl:PCA_100006768>This document shall give an overview of documentation relevant for the delivered equipment (PO) and schedule of documents to be delivered.
Documents shall be identified with title and document number.
To be developed by mutual agreement between the Buyer and Seller prior to placement of the Purchase Order (PO) and submitted for approval following PO placement to fully define the list of documents to be issued to Buyer by the Seller.</rdl:PCA_100006768>
    <rdl:PCA_100006766 rdf:resource="http://rds.posccaesar.org/ontology/plm/rdl/PCA_100006653"/>
    <rdl:PCA_100006763>This document is developed by mutual agreement between the Buyer and Seller prior to placement of the Purchase Order (PO) and submitted for approval following PO placement to fully define the list of documents to be issued to Buyer by the Seller. 
This document provides efficient follow up of documentation deliverables during all phases of manufacturing, installation, testing and handover to operations.
The schedule of the delivered documentation shall be aligned with project execution plans.</rdl:PCA_100006763>
    <rdfs:subClassOf rdf:resource="http://rds.posccaesar.org/ontology/plm/rdl/PCA_100004908"/>
  </owl:Class>
  <owl:Class rdf:about="http://rds.posccaesar.org/ontology/plm/rdl/PCA_100006463">
    <rdl:PCA_100006766 rdf:resource="http://rds.posccaesar.org/ontology/plm/rdl/PCA_100006643"/>
    <skos:broader rdf:resource="http://rds.posccaesar.org/ontology/plm/rdl/PCA_100006753"/>
    <rdl:PCA_100006765 rdf:resource="http://w3id.org/readi/rdl/CFIHOS-20000006"/>
    <rdl:PCA_100006768>Structural load plans shall be produced.</rdl:PCA_100006768>
    <rdfs:subClassOf rdf:resource="http://rds.posccaesar.org/ontology/plm/rdl/PCA_100004908"/>
    <skos:broadMatch rdf:resource="http://rds.posccaesar.org/ontology/plm/rdl/PCA_100006708"/>
    <rdl:PCA_100006766 rdf:resource="http://rds.posccaesar.org/ontology/plm/rdl/PCA_100006644"/>
    <rdfs:label>Structural load plans</rdfs:label>
    <rdfs:comment>Structural load plans shall be produced.</rdfs:comment>
  </owl:Class>
  <owl:Class rdf:about="http://rds.posccaesar.org/ontology/plm/rdl/PCA_100006342">
    <rdl:PCA_100006766 rdf:resource="http://rds.posccaesar.org/ontology/plm/rdl/PCA_100006653"/>
    <rdfs:comment>Document describing how to perform NDT (i.e. MT, PT, RT, UT, VT or ET) for a given object, including acceptance criteria and reporting.</rdfs:comment>
    <skos:broadMatch rdf:resource="http://rds.posccaesar.org/ontology/plm/rdl/PCA_100006722"/>
    <rdl:PCA_100006765 rdf:resource="http://w3id.org/readi/rdl/CFIHOS-20000028"/>
    <rdl:PCA_100006763>This document is a part of the Quality Assurance Plan, and herein the Quality Assurance work process and verification.
This document provides a procedure for NDT operator to ensure repeatability and formalism and hence prove the quality of the NDT work.</rdl:PCA_100006763>
    <skos:broadMatch rdf:resource="http://rds.posccaesar.org/ontology/plm/rdl/PCA_100006672"/>
    <rdfs:label>Non-destructive examination (NDE) procedure</rdfs:label>
    <rdfs:subClassOf rdf:resource="http://rds.posccaesar.org/ontology/plm/rdl/PCA_100004908"/>
    <rdl:PCA_100006768>Document describing how to perform NDT (i.e. MT, PT, RT, UT, VT or ET) for a given object, including acceptance criteria and reporting.</rdl:PCA_100006768>
    <skos:broader rdf:resource="http://rds.posccaesar.org/ontology/plm/rdl/PCA_100006751"/>
  </owl:Class>
  <owl:Class rdf:about="http://rds.posccaesar.org/ontology/plm/rdl/PCA_100006330">
    <skos:broadMatch rdf:resource="http://rds.posccaesar.org/ontology/plm/rdl/PCA_100006732"/>
    <rdfs:subClassOf rdf:resource="http://rds.posccaesar.org/ontology/plm/rdl/PCA_100004908"/>
    <skos:broadMatch rdf:resource="http://rds.posccaesar.org/ontology/plm/rdl/PCA_100006708"/>
    <rdfs:comment>The report shall contain a complete description of the entire mooring system: 
 - Arrangement drawings;
 - Component drawings;
 - Design analyses of all mooring components from onboard systems to anchors.</rdfs:comment>
    <rdl:PCA_100006766 rdf:resource="http://rds.posccaesar.org/ontology/plm/rdl/PCA_100006647"/>
    <rdl:PCA_100006763>The collection of reports and drawings shall provide information on mooring system layout and component design.</rdl:PCA_100006763>
    <rdfs:label>Mooring system design</rdfs:label>
    <skos:broader rdf:resource="http://rds.posccaesar.org/ontology/plm/rdl/PCA_100006756"/>
    <rdl:PCA_100006768>The report shall contain a complete description of the entire mooring system: 
 - Arrangement drawings;
 - Component drawings;
 - Design analyses of all mooring components from onboard systems to anchors.</rdl:PCA_100006768>
    <rdl:PCA_100006765 rdf:resource="http://w3id.org/readi/rdl/CFIHOS-20000033"/>
    <skos:broadMatch rdf:resource="http://rds.posccaesar.org/ontology/plm/rdl/PCA_100006698"/>
  </owl:Class>
  <owl:Class rdf:about="http://rds.posccaesar.org/ontology/plm/rdl/PCA_100006451">
    <rdfs:subClassOf rdf:resource="http://rds.posccaesar.org/ontology/plm/rdl/PCA_100004908"/>
    <skos:broadMatch rdf:resource="http://rds.posccaesar.org/ontology/plm/rdl/PCA_100006716"/>
    <rdfs:label>Spare and tools overview</rdfs:label>
    <rdl:PCA_100006765 rdf:resource="http://w3id.org/readi/rdl/CFIHOS-20000018"/>
    <rdl:PCA_100006763>Overview of all spare parts and tools required for operation and maintenance.</rdl:PCA_100006763>
    <rdfs:comment>Overview of all spare parts and tools required for operation and maintenance.
E.g. spare linepipe (with or without coating), spare flexible pipe sections, tools needed during operation such as tools for valve operation.</rdfs:comment>
    <rdl:PCA_100006766 rdf:resource="http://rds.posccaesar.org/ontology/plm/rdl/PCA_100006654"/>
    <skos:broader rdf:resource="http://rds.posccaesar.org/ontology/plm/rdl/PCA_100006760"/>
    <rdl:PCA_100006768>Overview of all spare parts and tools required for operation and maintenance.
E.g. spare linepipe (with or without coating), spare flexible pipe sections, tools needed during operation such as tools for valve operation.</rdl:PCA_100006768>
  </owl:Class>
  <owl:Class rdf:about="http://rds.posccaesar.org/ontology/plm/rdl/PCA_100006141">
    <rdfs:label>Damage control booklet</rdfs:label>
    <rdfs:comment>The damage control plan and damage control booklet are intended to provide information for actions to mitigate the loss of stability in the event of a damage causing flooding. The damage control booklet should include the same information as the damage control plan in addition to general instructions for controlling the effects of damage.</rdfs:comment>
    <rdl:PCA_100006768>The damage control plan and damage control booklet are intended to provide information for actions to mitigate the loss of stability in the event of a damage causing flooding. The damage control booklet should include the same information as the damage control plan in addition to general instructions for controlling the effects of damage.</rdl:PCA_100006768>
    <rdl:PCA_100006766 rdf:resource="http://rds.posccaesar.org/ontology/plm/rdl/PCA_100006657"/>
    <rdl:PCA_100006765 rdf:resource="http://w3id.org/readi/rdl/CFIHOS-20000033"/>
    <rdl:PCA_100006763>To document compliance with the PSA facilities regulations § 62 and NMA Regulations No. 878 in addition to IMO instruments and Class requirements, as applicable.</rdl:PCA_100006763>
    <rdfs:subClassOf rdf:resource="http://rds.posccaesar.org/ontology/plm/rdl/PCA_100004908"/>
  </owl:Class>
  <owl:Class rdf:about="http://rds.posccaesar.org/ontology/plm/rdl/PCA_100006153">
    <skos:broader rdf:resource="http://rds.posccaesar.org/ontology/plm/rdl/PCA_100006756"/>
    <skos:broadMatch rdf:resource="http://rds.posccaesar.org/ontology/plm/rdl/PCA_100006729"/>
    <skos:broadMatch rdf:resource="http://rds.posccaesar.org/ontology/plm/rdl/PCA_100006727"/>
    <skos:broadMatch rdf:resource="http://rds.posccaesar.org/ontology/plm/rdl/PCA_100006726"/>
    <rdfs:label>Design accidental load report</rdfs:label>
    <rdfs:subClassOf rdf:resource="http://rds.posccaesar.org/ontology/plm/rdl/PCA_100004908"/>
  </owl:Class>
  <owl:Class rdf:about="http://rds.posccaesar.org/ontology/plm/rdl/PCA_100006165">
    <skos:broader rdf:resource="http://rds.posccaesar.org/ontology/plm/rdl/PCA_100006756"/>
    <skos:broadMatch rdf:resource="http://rds.posccaesar.org/ontology/plm/rdl/PCA_100006722"/>
    <rdfs:label>Dimensional report</rdfs:label>
    <rdfs:comment>Measured real dimensions</rdfs:comment>
    <rdl:PCA_100006768>Measured real dimensions</rdl:PCA_100006768>
    <rdl:PCA_100006766 rdf:resource="http://rds.posccaesar.org/ontology/plm/rdl/PCA_100006653"/>
    <rdl:PCA_100006763>Verification of tolerances</rdl:PCA_100006763>
    <rdfs:subClassOf rdf:resource="http://rds.posccaesar.org/ontology/plm/rdl/PCA_100004908"/>
  </owl:Class>
  <owl:Class rdf:about="http://rds.posccaesar.org/ontology/plm/rdl/PCA_100006177">
    <rdfs:label>Electrical connection diagram</rdfs:label>
    <rdl:PCA_100006766 rdf:resource="http://rds.posccaesar.org/ontology/plm/rdl/PCA_100006637"/>
    <rdl:PCA_100006763>The diagram shall show the electrical connection between different electrical equipment and components within a package. The diagram shall also identify all connections to Company’s power supply and instrumented systems.</rdl:PCA_100006763>
    <rdl:PCA_100006766 rdf:resource="http://rds.posccaesar.org/ontology/plm/rdl/PCA_100006636"/>
    <rdl:PCA_100006766 rdf:resource="http://rds.posccaesar.org/ontology/plm/rdl/PCA_100006639"/>
    <rdl:PCA_100006765 rdf:resource="http://w3id.org/readi/rdl/CFIHOS-20000031"/>
    <rdl:PCA_100006765 rdf:resource="http://w3id.org/readi/rdl/CFIHOS-20000030"/>
    <rdl:PCA_100006764>Electrical connection diagram shall typical include the following:
 - Tag number of equipment to which the cable ends are terminated;
 - Signal tag number;
 - External cable tag number;
 - External cables with pair or wire number and core colour details;
 - Terminal block/socket number;
 - Earthing details;
 - Reference drawings.</rdl:PCA_100006764>
    <rdl:PCA_100006766 rdf:resource="http://rds.posccaesar.org/ontology/plm/rdl/PCA_100006638"/>
    <skos:broader rdf:resource="http://rds.posccaesar.org/ontology/plm/rdl/PCA_100006745"/>
    <skos:broadMatch rdf:resource="http://rds.posccaesar.org/ontology/plm/rdl/PCA_100006702"/>
    <rdl:PCA_100006766 rdf:resource="http://rds.posccaesar.org/ontology/plm/rdl/PCA_100006642"/>
    <rdl:PCA_100006766 rdf:resource="http://rds.posccaesar.org/ontology/plm/rdl/PCA_100006641"/>
    <skos:broadMatch rdf:resource="http://rds.posccaesar.org/ontology/plm/rdl/PCA_100006712"/>
    <rdl:PCA_100006766 rdf:resource="http://rds.posccaesar.org/ontology/plm/rdl/PCA_100006635"/>
    <rdl:PCA_100006765 rdf:resource="http://w3id.org/readi/rdl/CFIHOS-20000008"/>
    <rdl:PCA_100006766 rdf:resource="http://rds.posccaesar.org/ontology/plm/rdl/PCA_100006640"/>
    <rdfs:subClassOf rdf:resource="http://rds.posccaesar.org/ontology/plm/rdl/PCA_100004908"/>
    <rdl:PCA_100006766 rdf:resource="http://rds.posccaesar.org/ontology/plm/rdl/PCA_100006634"/>
  </owl:Class>
  <owl:Class rdf:about="http://rds.posccaesar.org/ontology/plm/rdl/PCA_100006189">
    <rdl:PCA_100006765 rdf:resource="http://w3id.org/readi/rdl/CFIHOS-20000030"/>
    <rdl:PCA_100006766 rdf:resource="http://rds.posccaesar.org/ontology/plm/rdl/PCA_100006656"/>
    <rdfs:comment>Equipment room layout drawings shall be provided: 
 - For areas equipped with instrument equipment cabinets/racks. Examples of such areas are: Central/ local equipment rooms (with instrument equipment cabinets/racks);
 - For electrical equipment room(s) in which switchgears, main distributions boards, transformers, UPS, etc. are located;
 - For areas equipped with telecommunication equipment, cabinets/racks. Examples of such areas are: Telecommunication equipment rooms and Local equipment rooms (with telecom equipment cabinets/racks.

The following information shall be shown:
 - Main Equipment with tag number (from all disciplines);
 - Reserved space for spare equipment;
 - Walls and doors;
 - Stairs and raised floor;
 - Equipment list including tag number, tag description and datum point coordinates.</rdfs:comment>
    <rdl:PCA_100006768>Equipment room layout drawings shall be provided: 
 - For areas equipped with instrument equipment cabinets/racks. Examples of such areas are: Central/ local equipment rooms (with instrument equipment cabinets/racks);
 - For electrical equipment room(s) in which switchgears, main distributions boards, transformers, UPS, etc. are located;
 - For areas equipped with telecommunication equipment, cabinets/racks. Examples of such areas are: Telecommunication equipment rooms and Local equipment rooms (with telecom equipment cabinets/racks.

The following information shall be shown:
 - Main Equipment with tag number (from all disciplines);
 - Reserved space for spare equipment;
 - Walls and doors;
 - Stairs and raised floor;
 - Equipment list including tag number, tag description and datum point coordinates.</rdl:PCA_100006768>
    <skos:broadMatch rdf:resource="http://rds.posccaesar.org/ontology/plm/rdl/PCA_100006710"/>
    <rdl:PCA_100006765 rdf:resource="http://w3id.org/readi/rdl/CFIHOS-20000008"/>
    <rdfs:label>Equipment room layout drawings</rdfs:label>
    <rdl:PCA_100006765 rdf:resource="http://w3id.org/readi/rdl/CFIHOS-20000015"/>
    <skos:broader rdf:resource="http://rds.posccaesar.org/ontology/plm/rdl/PCA_100006746"/>
    <rdfs:subClassOf rdf:resource="http://rds.posccaesar.org/ontology/plm/rdl/PCA_100004908"/>
  </owl:Class>
  <owl:Class rdf:about="http://rds.posccaesar.org/ontology/plm/rdl/PCA_100006298">
    <skos:broader rdf:resource="http://rds.posccaesar.org/ontology/plm/rdl/PCA_100006746"/>
    <skos:broadMatch rdf:resource="http://rds.posccaesar.org/ontology/plm/rdl/PCA_100006709"/>
    <rdfs:label>Lighting and small power layout drawings</rdfs:label>
    <rdfs:comment>These drawings are relevant for offshore facilities and for the process plant and well pad area for onshore facilities. 

At least one lighting and small power layout drawing for each area or module deck level shall be produced. The size of the facility will determine the scale of the drawing, but normally a scale of 1:100 on A3 format shall be aimed for. If required several drawings per area can be necessary to achieve this scale. Equipment which is covered by platforms above shall be shown dotted or shown in separate figures.

The lighting and small power layout drawing should be based on the equipment layout drawing, and the following electrical field equipment shall be included:
Lighting fixture, flood lights, socket outlet and junction boxes. These shall be tagged according to ENS.</rdfs:comment>
    <rdl:PCA_100006768>These drawings are relevant for offshore facilities and for the process plant and well pad area for onshore facilities. 

At least one lighting and small power layout drawing for each area or module deck level shall be produced. The size of the facility will determine the scale of the drawing, but normally a scale of 1:100 on A3 format shall be aimed for. If required several drawings per area can be necessary to achieve this scale. Equipment which is covered by platforms above shall be shown dotted or shown in separate figures.

The lighting and small power layout drawing should be based on the equipment layout drawing, and the following electrical field equipment shall be included:
Lighting fixture, flood lights, socket outlet and junction boxes. These shall be tagged according to ENS.</rdl:PCA_100006768>
    <rdl:PCA_100006766 rdf:resource="http://rds.posccaesar.org/ontology/plm/rdl/PCA_100006656"/>
    <rdl:PCA_100006765 rdf:resource="http://w3id.org/readi/rdl/CFIHOS-20000008"/>
    <rdfs:subClassOf rdf:resource="http://rds.posccaesar.org/ontology/plm/rdl/PCA_100004908"/>
  </owl:Class>
  <owl:Class rdf:about="http://rds.posccaesar.org/ontology/plm/rdl/PCA_100006286">
    <skos:broader rdf:resource="http://rds.posccaesar.org/ontology/plm/rdl/PCA_100006750"/>
    <skos:broadMatch rdf:resource="http://rds.posccaesar.org/ontology/plm/rdl/PCA_100006698"/>
    <rdfs:label>Instrumented systems - performance data</rdfs:label>
    <rdl:PCA_100006766 rdf:resource="http://rds.posccaesar.org/ontology/plm/rdl/PCA_100006657"/>
    <rdl:PCA_100006765 rdf:resource="http://w3id.org/readi/rdl/CFIHOS-20000015"/>
    <rdl:PCA_100006763>Performance of components in SAS shall be documented. Refer to NORSOK I-002 for details about which parameter that shall be measured.</rdl:PCA_100006763>
    <rdfs:subClassOf rdf:resource="http://rds.posccaesar.org/ontology/plm/rdl/PCA_100004908"/>
  </owl:Class>
  <owl:Class rdf:about="http://rds.posccaesar.org/ontology/plm/rdl/PCA_100006274">
    <skos:broader rdf:resource="http://rds.posccaesar.org/ontology/plm/rdl/PCA_100006749"/>
    <skos:broadMatch rdf:resource="http://rds.posccaesar.org/ontology/plm/rdl/PCA_100006688"/>
    <rdfs:label>Installation , operating and maintenance instructions for valves</rdfs:label>
    <rdfs:comment>Requirements for receipt, storage, installation, operation and maintenance of supplied valves. The document shall include, but not be limited to:
 - Instructions for un-packing, handling, lifting of consignment and components.
 - Requirements for storage and preservation/de-preservation/re-preservation during installation and commissioning.
 - Preservation maintenance to be carried out by the user during storage, installation and in the period prior to start-up for the intended use
 - Procedure and necessary documentation for installation, including any additional measures that Purchaser need to observe prior to and during installation
 - Information about valve functions, operating and maintenance instructions
 - Bolt tightening procedures, including lubrication requirements
 - Procedure for maintenance of packing boxes, including recommended compression
 - Procedure for dismantle and reassembly of actuator/gearbox
 - Information regarding lubrication
 - Technical and functional descriptions
 - Consumption data
 - Restrictions in use</rdfs:comment>
    <rdl:PCA_100006768>Requirements for receipt, storage, installation, operation and maintenance of supplied valves. The document shall include, but not be limited to:
 - Instructions for un-packing, handling, lifting of consignment and components.
 - Requirements for storage and preservation/de-preservation/re-preservation during installation and commissioning.
 - Preservation maintenance to be carried out by the user during storage, installation and in the period prior to start-up for the intended use
 - Procedure and necessary documentation for installation, including any additional measures that Purchaser need to observe prior to and during installation
 - Information about valve functions, operating and maintenance instructions
 - Bolt tightening procedures, including lubrication requirements
 - Procedure for maintenance of packing boxes, including recommended compression
 - Procedure for dismantle and reassembly of actuator/gearbox
 - Information regarding lubrication
 - Technical and functional descriptions
 - Consumption data
 - Restrictions in use</rdl:PCA_100006768>
    <rdl:PCA_100006765 rdf:resource="http://w3id.org/readi/rdl/CFIHOS-20000022"/>
    <rdl:PCA_100006763>IOM documents shall, in an organized manner, provide sufficient information to install, operate and maintain the equipment in a safe, economical and functionally correct manner.</rdl:PCA_100006763>
    <rdfs:subClassOf rdf:resource="http://rds.posccaesar.org/ontology/plm/rdl/PCA_100004908"/>
  </owl:Class>
  <owl:Class rdf:about="http://rds.posccaesar.org/ontology/plm/rdl/PCA_100006395">
    <rdfs:label>Process safety report</rdfs:label>
    <skos:broadMatch rdf:resource="http://rds.posccaesar.org/ontology/plm/rdl/PCA_100006727"/>
    <skos:broadMatch rdf:resource="http://rds.posccaesar.org/ontology/plm/rdl/PCA_100006728"/>
    <rdl:PCA_100006765 rdf:resource="http://w3id.org/readi/rdl/CFIHOS-20000026"/>
    <skos:broadMatch rdf:resource="http://rds.posccaesar.org/ontology/plm/rdl/PCA_100006729"/>
    <rdl:PCA_100006763>In accordance with API 521 chapter 4.7, and authority regulation "Aktivitetsforskriften" §20.</rdl:PCA_100006763>
    <rdfs:subClassOf rdf:resource="http://rds.posccaesar.org/ontology/plm/rdl/PCA_100004908"/>
    <skos:broader rdf:resource="http://rds.posccaesar.org/ontology/plm/rdl/PCA_100006756"/>
    <skos:broadMatch rdf:resource="http://rds.posccaesar.org/ontology/plm/rdl/PCA_100006687"/>
    <rdl:PCA_100006768>The process safety report shall be one single report for the plant (i.e. not split into several reports), and this report shall be updated whenever relevant modifications to the plant are performed.

The process safety report shall as a minimum include/describe:
 - The philosophy for process safety functions, i.e. pressure protection, level protection, temperature protection and overflow protection;
 - Process safety functions including premises for the design of the safety function:
    - Documentation of how these premises are fulfilled in design and shall be maintained, so that future modifications will not compromise the design intention;
    - Relief cases (all) for relief valves including the dimensioning ‘required capacity’ and the; ‘rated capacity’
    - Instrumented shutdown:
    - The structured review of the required instrumented shut down functions:
   - Documentation of the performed structured analysis utilizing SAT, SAC and SAFEs in accordance with ISO 10418/API RP 14 C;
   - Documentation of the structured review carried out to determine required instrumented shutdown functions, e.g. LOPA (if applicable); 
 - The philosophy for leakage detection;
 - Listing of valves that need to be secured in the correct position as a part of the process safety design, including reasoning for securing the valve position and the choice of method;
 - Heat conservation philosophy for safety critical heat conservation including operating and maintenance practice to ensure proper reliability of the heat conservation systems;
 - Safety critical procedures (administrative control);
 - Safety critical check valves;
 - Pipeline protection (if relevant);
 - The reasoning for the chosen sectionalisation of the process;
 - The relief valve schedule;
 - PSD response time.

The dynamic simulation model(s) used for the simulations of the Inadvertent valve opening (IVO) and Choke collapse (CC) scenarios, e.g. the Olga model, shall be delivered and shall represent the As built design of wells, flowlines and topside piping.</rdl:PCA_100006768>
    <rdfs:comment>The process safety report shall be one single report for the plant (i.e. not split into several reports), and this report shall be updated whenever relevant modifications to the plant are performed.

The process safety report shall as a minimum include/describe:
 - The philosophy for process safety functions, i.e. pressure protection, level protection, temperature protection and overflow protection;
 - Process safety functions including premises for the design of the safety function:
    - Documentation of how these premises are fulfilled in design and shall be maintained, so that future modifications will not compromise the design intention;
    - Relief cases (all) for relief valves including the dimensioning ‘required capacity’ and the; ‘rated capacity’
    - Instrumented shutdown:
    - The structured review of the required instrumented shut down functions:
   - Documentation of the performed structured analysis utilizing SAT, SAC and SAFEs in accordance with ISO 10418/API RP 14 C;
   - Documentation of the structured review carried out to determine required instrumented shutdown functions, e.g. LOPA (if applicable); 
 - The philosophy for leakage detection;
 - Listing of valves that need to be secured in the correct position as a part of the process safety design, including reasoning for securing the valve position and the choice of method;
 - Heat conservation philosophy for safety critical heat conservation including operating and maintenance practice to ensure proper reliability of the heat conservation systems;
 - Safety critical procedures (administrative control);
 - Safety critical check valves;
 - Pipeline protection (if relevant);
 - The reasoning for the chosen sectionalisation of the process;
 - The relief valve schedule;
 - PSD response time.

The dynamic simulation model(s) used for the simulations of the Inadvertent valve opening (IVO) and Choke collapse (CC) scenarios, e.g. the Olga model, shall be delivered and shall represent the As built design of wells, flowlines and topside piping.</rdfs:comment>
    <skos:broadMatch rdf:resource="http://rds.posccaesar.org/ontology/plm/rdl/PCA_100006688"/>
    <rdl:PCA_100006766 rdf:resource="http://rds.posccaesar.org/ontology/plm/rdl/PCA_100006654"/>
    <skos:broadMatch rdf:resource="http://rds.posccaesar.org/ontology/plm/rdl/PCA_100006726"/>
  </owl:Class>
  <owl:Class rdf:about="http://rds.posccaesar.org/ontology/plm/rdl/PCA_100006383">
    <skos:broader rdf:resource="http://rds.posccaesar.org/ontology/plm/rdl/PCA_100006746"/>
    <rdfs:comment>For pneumatic and hydraulic consumers, the supplier shall work out hook-up drawings.

A typical hook-up drawing shall indicate details such as:
 - All instrument/bulk material installed by Supplier;
 - Connections and dimensions of signal lines/tubing;
 - Material of instrument bulk.

Typical hook-up drawings should be used as a guideline.

The drawing shall indicate split of responsibilities between Supplier and Purchaser.</rdfs:comment>
    <rdfs:subClassOf rdf:resource="http://rds.posccaesar.org/ontology/plm/rdl/PCA_100004908"/>
    <skos:broadMatch rdf:resource="http://rds.posccaesar.org/ontology/plm/rdl/PCA_100006731"/>
    <rdl:PCA_100006765 rdf:resource="http://w3id.org/readi/rdl/CFIHOS-20000015"/>
    <rdl:PCA_100006768>For pneumatic and hydraulic consumers, the supplier shall work out hook-up drawings.

A typical hook-up drawing shall indicate details such as:
 - All instrument/bulk material installed by Supplier;
 - Connections and dimensions of signal lines/tubing;
 - Material of instrument bulk.

Typical hook-up drawings should be used as a guideline.

The drawing shall indicate split of responsibilities between Supplier and Purchaser.</rdl:PCA_100006768>
    <skos:broadMatch rdf:resource="http://rds.posccaesar.org/ontology/plm/rdl/PCA_100006732"/>
    <rdfs:label>Pneumatic/hydraulic hook-up drawing</rdfs:label>
    <rdl:PCA_100006766 rdf:resource="http://rds.posccaesar.org/ontology/plm/rdl/PCA_100006653"/>
    <skos:broadMatch rdf:resource="http://rds.posccaesar.org/ontology/plm/rdl/PCA_100006713"/>
  </owl:Class>
  <owl:Class rdf:about="http://rds.posccaesar.org/ontology/plm/rdl/PCA_100006262">
    <skos:broader rdf:resource="http://rds.posccaesar.org/ontology/plm/rdl/PCA_100006748"/>
    <skos:broadMatch rdf:resource="http://rds.posccaesar.org/ontology/plm/rdl/PCA_100006716"/>
    <rdfs:label>Hydraulic hose list -lifting appliances</rdfs:label>
    <rdfs:comment>The hydraulic hose list shall include the following information:
 - Hose id (corresponding to hose id on Hydraulic circuit diagram)
 - Type (e.g. EN norm or SAE norm)
 - Length in mm
 - Fittings on A &amp; B end
 - Max pressure rating for the hose
 - System pressure</rdfs:comment>
    <rdl:PCA_100006768>The hydraulic hose list shall include the following information:
 - Hose id (corresponding to hose id on Hydraulic circuit diagram)
 - Type (e.g. EN norm or SAE norm)
 - Length in mm
 - Fittings on A &amp; B end
 - Max pressure rating for the hose
 - System pressure</rdl:PCA_100006768>
    <rdfs:subClassOf rdf:resource="http://rds.posccaesar.org/ontology/plm/rdl/PCA_100004908"/>
  </owl:Class>
  <owl:Class rdf:about="http://rds.posccaesar.org/ontology/plm/rdl/PCA_100006250">
    <rdl:PCA_100006768>Documents containing records of performed heat treatment.</rdl:PCA_100006768>
    <skos:broader rdf:resource="http://rds.posccaesar.org/ontology/plm/rdl/PCA_100006756"/>
    <rdl:PCA_100006766 rdf:resource="http://rds.posccaesar.org/ontology/plm/rdl/PCA_100006653"/>
    <skos:broadMatch rdf:resource="http://rds.posccaesar.org/ontology/plm/rdl/PCA_100006722"/>
    <rdl:PCA_100006765 rdf:resource="http://w3id.org/readi/rdl/CFIHOS-20000031"/>
    <rdfs:comment>Documents containing records of performed heat treatment.</rdfs:comment>
    <rdfs:label>Heat treatment report</rdfs:label>
    <rdfs:subClassOf rdf:resource="http://rds.posccaesar.org/ontology/plm/rdl/PCA_100004908"/>
    <rdl:PCA_100006763>To document that the heat treatment performed meets specified requirements.</rdl:PCA_100006763>
  </owl:Class>
  <owl:Class rdf:about="http://rds.posccaesar.org/ontology/plm/rdl/PCA_100006371">
    <rdfs:subClassOf rdf:resource="http://rds.posccaesar.org/ontology/plm/rdl/PCA_100004908"/>
    <rdl:PCA_100006765 rdf:resource="http://w3id.org/readi/rdl/CFIHOS-20000018"/>
    <skos:broader rdf:resource="http://rds.posccaesar.org/ontology/plm/rdl/PCA_100006762"/>
    <skos:broadMatch rdf:resource="http://rds.posccaesar.org/ontology/plm/rdl/PCA_100006705"/>
    <rdfs:comment>Survey reports and data shall comply with Company's requirements for Offshore surveys.</rdfs:comment>
    <skos:broader rdf:resource="http://rds.posccaesar.org/ontology/plm/rdl/PCA_100006756"/>
    <rdfs:label>Pipeline survey reports and data</rdfs:label>
    <rdl:PCA_100006766 rdf:resource="http://rds.posccaesar.org/ontology/plm/rdl/PCA_100006654"/>
    <rdl:PCA_100006768>Survey reports and data shall comply with Company's requirements for Offshore surveys.</rdl:PCA_100006768>
    <rdl:PCA_100006763>Ensure safe operation</rdl:PCA_100006763>
  </owl:Class>
  <owl:Class rdf:about="http://rds.posccaesar.org/ontology/plm/rdl/PCA_100006480">
    <skos:broadMatch rdf:resource="http://rds.posccaesar.org/ontology/plm/rdl/PCA_100006687"/>
    <rdfs:label>System design basis</rdfs:label>
    <rdfs:comment>The system design basis includes the overall functional and performance requirements based on operator’s requirements.</rdfs:comment>
    <rdl:PCA_100006768>The system design basis includes the overall functional and performance requirements based on operator’s requirements.</rdl:PCA_100006768>
    <rdl:PCA_100006766 rdf:resource="http://rds.posccaesar.org/ontology/plm/rdl/PCA_100006657"/>
    <rdl:PCA_100006765 rdf:resource="http://w3id.org/readi/rdl/CFIHOS-20000031"/>
    <rdl:PCA_100006763>The document provides input to the sub-system design and also acts as a verification of operator’s requirements.</rdl:PCA_100006763>
    <rdfs:subClassOf rdf:resource="http://rds.posccaesar.org/ontology/plm/rdl/PCA_100004908"/>
  </owl:Class>
  <owl:Class rdf:about="http://rds.posccaesar.org/ontology/plm/rdl/PCA_100006492">
    <skos:broadMatch rdf:resource="http://rds.posccaesar.org/ontology/plm/rdl/PCA_100006708"/>
    <rdfs:comment>The following content shall be included on the drawings:
 - All tagged telecommunication field equipment like PAGA loudspeakers, flashing lights, Ex telephones, fixed radios, CCTV cameras, antennas, junction boxes, etc.;
 - Other telecommunication equipment installed outside telecommunication equipment rooms;
 - Telecommunication outlets;
 - Platform/plant northing and orientation with respect of true north;
 - Gridlines with north and east references;
 - Key plan;
 - Scale bar;
 - Match lines with drawing references;
 - Deck/area elevations.</rdfs:comment>
    <rdfs:subClassOf rdf:resource="http://rds.posccaesar.org/ontology/plm/rdl/PCA_100004908"/>
    <rdl:PCA_100006763>At least one Telecommunication field equipment layout drawing for each area or module deck level shall be produced. The size of the facility will determine the scale of the drawing, but normally a scale of 1:100 on A3 format shall be aimed for. If required several drawings per area can be necessary to achieve this scale. Equipment which is covered by platforms above shall be shown dotted or shown in separate figures.</rdl:PCA_100006763>
    <skos:broader rdf:resource="http://rds.posccaesar.org/ontology/plm/rdl/PCA_100006746"/>
    <rdl:PCA_100006766 rdf:resource="http://rds.posccaesar.org/ontology/plm/rdl/PCA_100006653"/>
    <rdfs:label>Telecommunication field equipment layout drawings</rdfs:label>
    <rdl:PCA_100006765 rdf:resource="http://w3id.org/readi/rdl/CFIHOS-20000030"/>
    <rdl:PCA_100006768>The following content shall be included on the drawings:
 - All tagged telecommunication field equipment like PAGA loudspeakers, flashing lights, Ex telephones, fixed radios, CCTV cameras, antennas, junction boxes, etc.;
 - Other telecommunication equipment installed outside telecommunication equipment rooms;
 - Telecommunication outlets;
 - Platform/plant northing and orientation with respect of true north;
 - Gridlines with north and east references;
 - Key plan;
 - Scale bar;
 - Match lines with drawing references;
 - Deck/area elevations.</rdl:PCA_100006768>
  </owl:Class>
  <owl:Class rdf:about="http://rds.posccaesar.org/ontology/plm/rdl/PCA_100006221">
    <skos:broader rdf:resource="http://rds.posccaesar.org/ontology/plm/rdl/PCA_100006756"/>
    <skos:broadMatch rdf:resource="http://rds.posccaesar.org/ontology/plm/rdl/PCA_100006698"/>
    <rdfs:label>Flare report/flare and depressurization report</rdfs:label>
    <rdl:PCA_100006766 rdf:resource="http://rds.posccaesar.org/ontology/plm/rdl/PCA_100006654"/>
    <rdl:PCA_100006765 rdf:resource="http://w3id.org/readi/rdl/CFIHOS-20000026"/>
    <rdl:PCA_100006764>The flare report shall be one common report for the plant (i.e. not split into several reports). Documentation of emergency depressurization may be issued as a separate report cross-referenced to the flare report.

The report should be named "Flare report". If the depressurization design is included, name the report "Flare and Depressurization Report"

The flare report shall describe the design of the flare and vent system, and as a minimum include:
 - Design basis for the system, e.g. system capacity and selection;
-    Procedure for replacement of flare tip;
 - Description of the flare and vent system segregation and disposal, e.g. wet vs. dry streams, high vs. low temperature, high vs. low pressure, emergency vs. maintenance flare/vent, flaring vs. cold venting and common vent vs. local vent;
     - For cold vents, selected/recommended methods to extinguish the flame (if the vent is ignited) shall be described;
 - Descriptions of flaring scenarios including flare rates, e.g. operational flaring, relief cases, emergency depressurization and simultaneous flaring (operational flaring + relief/depressurization). The simultaneous flaring cases shall be clearly defined. The selected base load (e.g. long-term operational flaring) shall be explained;
     - The flare report shall list the largest flare sources, those that designs the flare headers/drums and the location of the flare tip;
 - Operation of the system during long duration cooldown, e.g. cold ambient temperature, flowline depressurization;
 - Description of the piping and equipment design, e.g.:
     - Hydraulic design (sizing of pipes);
     - Knock out drum;
     - Flare tip design (e.g. hydraulic performance, soot emission, noise, purge requirements, expected lifetime, maintenance requirements);
     - Flare gas recovery;
     - Flare ignition;
           - If flare gases are combusted for safety reasons (i.e. not only for environmental reasons), the reliability of the ignition system shall be documented to prove that the system has the required reliability and necessary requirements (assumptions) listed;
 - Documentation of system design calculations, where the input data, results and the calculations shall be included in the report and in simulation files, e.g.:
     - Calculation of flare tip radiation to determine (a) the resulting heat exposure towards humans and (b) the resulting temperature on equipment, pipes and structures;
     - Calculation of gas dispersion;
     - The potential gas concentration resulting from an extinguished flare/vent shall be documented, and plant areas where operational activities are limited as a result (e.g. hot work) shall be defined;
     - Hydraulic calculation (pipe sizing);
     - Sizing of liquid knockout drums;
     - The main results are documented in the main report, the details in appendices.

The various simulation files defined above shall be a part of the delivery as executable simulation files (simulation programs to be agreed) reflecting the As-built design.

The flare report, including the simulation files, shall be updated whenever relevant modifications to the plant are performed, i.e. parallel documents shall not be established.


Documentation of the depressurization design

The depressurization report shall specify the information required to repeat/re-establish all dimensioning cases both with respect to fire depressurization and cold depressurization. Typical required information is input streams, system geometry (see list above), initial conditions (e.g. pressure, temperature, liquid volumes, ambient conditions), orifice specification, any delayed opening of BDVs, material properties used, fire loads and durations, the plant specific intolerable ruptures, assumptions made and other relevant information.

The report shall tabulate the following:
 - Rupture conditions of pipes/equipment that will rupture during the dimensioning fire;
     - Time to rupture;
     - Pressure at rupture;
     - Instantaneous release of hydrocarbon fluid at rupture (kg/s);
     - Other relevant information;
 - The initial flare rate from fire depressurisation and cold depressurization;
 - System pressure 15 minutes after gas detection (no heat input, relevant delay of blowdown included);
 - The minimum vapour and liquid temperature resulting from the cold depressurization;
 - The minimum vapour wall and liquid wall temperatures resulting from the cold depressurization.
The report should contain the following:
 - The depressurisation rates for each depressurisation segment as function of time:
     - cold depressurisation, fire depressurisation and depressurisation from normal conditions;
 - The total depressurisation rate (mass rate) for all segments that are feeding the disposal system simultaneously:
     - fire depressurisation and depressurisation from normal conditions.

The following shall be available for Company during project execution and shall be handed over to Company at project close out.

 - A spreadsheet that describes the geometry of all depressurisation segments. See the below list for minimum content.
 - A spreadsheet tabulating the pressure profiles during fire exposure/fire depressurisation for all depressurization segments and for all segments containing hydrocarbons but without depressurization.
 - A spreadsheet tabulating the pressure profile for the flare header during depressurisation

The simulation file(s) used for calculation of temperature profile and stress/rupture (i.e. time to rupture calculations).

A spreadsheet that describes the geometry of all depressurization segments shall be made. The spreadsheet shall always reflect the current process design, include date of last revision and corresponding P&amp;ID revision(s) used, and shall as a minimum contain the following information for each pipe and equipment (it is recommended to use one sheet for each depressurization segment):
 - Line number or equipment tag number;
 - Length (note 3);
 - Inner and outer diameter;
 - Liquid volume (see note 1);
 - Gas volume (see note 1);
 - Total volume of the depressurisation segment and volume of each sub-segment (note 2);
 - Outside are:
     - total outside area of the depressurisation segment and outside area of each sub-segment;
 - Dry area:
     - total dry area of the depressurisation segment and dry area of each sub-segment. See note 1;
 - Wet area:
     - total wet area of the depressurisation segment and wet area of each sub-segment. See note 1;
 - Insulated area and type of insulation;
 - Wall thickness;
 - Material;
 - Weight:
     - total weight of depressurisation segment and weight of each sub segment.

Note 1: Liquid in sloped pipes will be drain to its nearest low point. Pipes that will be drained are treated as “dry wall” pipes.

Note 2: A sub-segment is e.g. a pipe or a vessel in a depressurization segment

Note 3: Line sizes that do not contribute to the system volume/area/weight, typically sizes less than 1’’, need not to be listed with length and can be listed separately on the same sheet.

The spreadsheet should in addition contain the following information:
 - Name of depressurisation segment (e.g. 1ststage separator);
 - Tag-number of the BDV (and the orifice);
 - Which valves that determines the border of the depressurisation segment (PSD valves, ESD valves, PSVs, PV etc);
 - Information about what, when and by whom the spreadsheet was updated, i.e. a change log.</rdl:PCA_100006764>
    <rdl:PCA_100006763>Provided for in API STD 521 chapter 4</rdl:PCA_100006763>
    <rdfs:subClassOf rdf:resource="http://rds.posccaesar.org/ontology/plm/rdl/PCA_100004908"/>
  </owl:Class>
  <owl:Class rdf:about="http://rds.posccaesar.org/ontology/plm/rdl/PCA_100006100">
    <skos:broader rdf:resource="http://rds.posccaesar.org/ontology/plm/rdl/PCA_100006756"/>
    <skos:broadMatch rdf:resource="http://rds.posccaesar.org/ontology/plm/rdl/PCA_100006722"/>
    <rdfs:label>Audio and video entertainment distribution network (coaxial cable) test report</rdfs:label>
    <rdl:PCA_100006766 rdf:resource="http://rds.posccaesar.org/ontology/plm/rdl/PCA_100006653"/>
    <rdl:PCA_100006765 rdf:resource="http://w3id.org/readi/rdl/CFIHOS-20000030"/>
    <rdl:PCA_100006763>Test reports for Audio and video entertainment distribution network (coaxial cable) shall be provided. Test per outlet.</rdl:PCA_100006763>
    <rdfs:subClassOf rdf:resource="http://rds.posccaesar.org/ontology/plm/rdl/PCA_100004908"/>
  </owl:Class>
  <owl:Class rdf:about="http://rds.posccaesar.org/ontology/plm/rdl/PCA_100006112">
    <skos:broadMatch rdf:resource="http://rds.posccaesar.org/ontology/plm/rdl/PCA_100006709"/>
    <rdl:PCA_100006765 rdf:resource="http://w3id.org/readi/rdl/CFIHOS-20000031"/>
    <rdl:PCA_100006765 rdf:resource="http://w3id.org/readi/rdl/CFIHOS-20000008"/>
    <skos:broader rdf:resource="http://rds.posccaesar.org/ontology/plm/rdl/PCA_100006762"/>
    <skos:broadMatch rdf:resource="http://rds.posccaesar.org/ontology/plm/rdl/PCA_100006708"/>
    <rdfs:subClassOf rdf:resource="http://rds.posccaesar.org/ontology/plm/rdl/PCA_100004908"/>
    <rdl:PCA_100006768>Cable route and changes to network shall be delivered.

Cable routing shall document the following:
 - Cable route network:
   - Cable ladder/tray &gt;=300mm;
   - Cable tray &lt;300 mm if purpose to connect Cable ladders &gt;=300mm;
   - Penetrations;
   - Unsupported Jump between cable ladders;
 - Cables routed on network.</rdl:PCA_100006768>
    <rdl:PCA_100006765 rdf:resource="http://w3id.org/readi/rdl/CFIHOS-20000030"/>
    <rdl:PCA_100006765 rdf:resource="http://w3id.org/readi/rdl/CFIHOS-20000015"/>
    <rdfs:comment>Cable route and changes to network shall be delivered.

Cable routing shall document the following:
 - Cable route network:
   - Cable ladder/tray &gt;=300mm;
   - Cable tray &lt;300 mm if purpose to connect Cable ladders &gt;=300mm;
   - Penetrations;
   - Unsupported Jump between cable ladders;
 - Cables routed on network.</rdfs:comment>
    <rdl:PCA_100006766 rdf:resource="http://rds.posccaesar.org/ontology/plm/rdl/PCA_100006656"/>
    <rdfs:label>Cable routing</rdfs:label>
  </owl:Class>
  <owl:Class rdf:about="http://rds.posccaesar.org/ontology/plm/rdl/PCA_100006124">
    <skos:broader rdf:resource="http://rds.posccaesar.org/ontology/plm/rdl/PCA_100006756"/>
    <skos:broadMatch rdf:resource="http://rds.posccaesar.org/ontology/plm/rdl/PCA_100006722"/>
    <rdfs:label>Coaxial cable test reports</rdfs:label>
    <rdfs:comment>Test reports for coaxial cables (for radio systems) shall be provided.</rdfs:comment>
    <rdl:PCA_100006768>Test reports for coaxial cables (for radio systems) shall be provided.</rdl:PCA_100006768>
    <rdl:PCA_100006766 rdf:resource="http://rds.posccaesar.org/ontology/plm/rdl/PCA_100006653"/>
    <rdl:PCA_100006765 rdf:resource="http://w3id.org/readi/rdl/CFIHOS-20000030"/>
    <rdfs:subClassOf rdf:resource="http://rds.posccaesar.org/ontology/plm/rdl/PCA_100004908"/>
  </owl:Class>
  <owl:Class rdf:about="http://rds.posccaesar.org/ontology/plm/rdl/PCA_100006136">
    <rdl:PCA_100006765 rdf:resource="http://w3id.org/readi/rdl/CFIHOS-20000031"/>
    <rdl:PCA_100006766 rdf:resource="http://rds.posccaesar.org/ontology/plm/rdl/PCA_100006653"/>
    <rdfs:subClassOf rdf:resource="http://rds.posccaesar.org/ontology/plm/rdl/PCA_100004908"/>
    <rdl:PCA_100006763>A compound document containing information on capabilities, design details, features, and limitations of software.</rdl:PCA_100006763>
    <rdfs:label>Control system software documentation</rdfs:label>
    <rdfs:comment>A document describing logical and communicative functions including interfaces for a software system.</rdfs:comment>
    <rdl:PCA_100006768>A document describing logical and communicative functions including interfaces for a software system.</rdl:PCA_100006768>
    <skos:broader>
      <rdl:PCA_100001503 rdf:about="http://rds.posccaesar.org/ontology/plm/rdl/PCA_100006761">
        <rdfs:label>Software</rdfs:label>
        <rdl:PCA_100004924>SW</rdl:PCA_100004924>
        <rdf:type rdf:resource="http://www.w3.org/2002/07/owl#NamedIndividual"/>
      </rdl:PCA_100001503>
    </skos:broader>
    <skos:broadMatch rdf:resource="http://rds.posccaesar.org/ontology/plm/rdl/PCA_100006703"/>
  </owl:Class>
  <owl:Class rdf:about="http://rds.posccaesar.org/ontology/plm/rdl/PCA_100006148">
    <skos:broader rdf:resource="http://rds.posccaesar.org/ontology/plm/rdl/PCA_100006747"/>
    <skos:broadMatch rdf:resource="http://rds.posccaesar.org/ontology/plm/rdl/PCA_100006686"/>
    <rdfs:label>Data sheets -Weight</rdfs:label>
    <rdfs:comment>Content according to ISO 19901-5 ‘Weight control during engineering and construction’, Class A. For equipment packages, separate weight data sheets shall be issued for each piece of equipment shipped and installed separately comprising the total equipment package.</rdfs:comment>
    <rdl:PCA_100006768>Content according to ISO 19901-5 ‘Weight control during engineering and construction’, Class A. For equipment packages, separate weight data sheets shall be issued for each piece of equipment shipped and installed separately comprising the total equipment package.</rdl:PCA_100006768>
    <rdfs:subClassOf rdf:resource="http://rds.posccaesar.org/ontology/plm/rdl/PCA_100004908"/>
  </owl:Class>
  <owl:Class rdf:about="http://rds.posccaesar.org/ontology/plm/rdl/PCA_100006299">
    <skos:broader rdf:resource="http://rds.posccaesar.org/ontology/plm/rdl/PCA_100006762"/>
    <skos:broadMatch rdf:resource="http://rds.posccaesar.org/ontology/plm/rdl/PCA_100006686"/>
    <rdfs:label>Liner system information</rdfs:label>
    <rdfs:comment>Liner system information shall contain as a minimum:
 - Liner system identification 
 - Manufacturer's material data 
 - Material pre-qualification information 
 - Type and thickness of liner material 
 - Expected short-term and long-term volumetric swelling or shrinkage for the range of operating conditions
 - Expected thermal deformations due to operating temperatures 
 - Liner manufacturing procedure 
 - Liner installation procedure 
 - Anticipated insertion forces for each liner section in relation to the liner strength capabilities 
 - Maximum allowable weld penetration of carbon steel pipeline girth welds</rdfs:comment>
    <rdl:PCA_100006768>Liner system information shall contain as a minimum:
 - Liner system identification 
 - Manufacturer's material data 
 - Material pre-qualification information 
 - Type and thickness of liner material 
 - Expected short-term and long-term volumetric swelling or shrinkage for the range of operating conditions
 - Expected thermal deformations due to operating temperatures 
 - Liner manufacturing procedure 
 - Liner installation procedure 
 - Anticipated insertion forces for each liner section in relation to the liner strength capabilities 
 - Maximum allowable weld penetration of carbon steel pipeline girth welds</rdl:PCA_100006768>
    <rdl:PCA_100006766 rdf:resource="http://rds.posccaesar.org/ontology/plm/rdl/PCA_100006657"/>
    <rdl:PCA_100006765 rdf:resource="http://w3id.org/readi/rdl/CFIHOS-20000018"/>
    <rdfs:subClassOf rdf:resource="http://rds.posccaesar.org/ontology/plm/rdl/PCA_100004908"/>
  </owl:Class>
  <owl:Class rdf:about="http://rds.posccaesar.org/ontology/plm/rdl/PCA_100006287">
    <rdfs:subClassOf rdf:resource="http://rds.posccaesar.org/ontology/plm/rdl/PCA_100004908"/>
    <rdl:PCA_100006768>The report shall cover, but not be limited to:
 - Selection of internal coating (coating type, -thickness, wear resistance regarding cleaning and inspection pigging, calculation of extent of coating based on fluid conductivity in pipeline during construction, commissioning and operational phase).
 - Mechanical design (such as allowable forces and moments).
 - Support and anchoring of insulating joint (electrical insulation)
 - External coating, field joints, thermal insulation and/or encapsulation.
 - Location (in pit below ground, above ground).
 - Spark gaps / high voltage protection (such as type, location, cable to pipeline connection, cable length).</rdl:PCA_100006768>
    <rdfs:label>Insulating joints design report</rdfs:label>
    <rdfs:comment>The report shall cover, but not be limited to:
 - Selection of internal coating (coating type, -thickness, wear resistance regarding cleaning and inspection pigging, calculation of extent of coating based on fluid conductivity in pipeline during construction, commissioning and operational phase).
 - Mechanical design (such as allowable forces and moments).
 - Support and anchoring of insulating joint (electrical insulation)
 - External coating, field joints, thermal insulation and/or encapsulation.
 - Location (in pit below ground, above ground).
 - Spark gaps / high voltage protection (such as type, location, cable to pipeline connection, cable length).</rdfs:comment>
    <skos:broadMatch rdf:resource="http://rds.posccaesar.org/ontology/plm/rdl/PCA_100006686"/>
    <skos:broader rdf:resource="http://rds.posccaesar.org/ontology/plm/rdl/PCA_100006756"/>
    <rdl:PCA_100006763>Design report covering insulation joint design and requirements. The Insulating joints design report shall reflect the requirements for design in ISO 15589-1.</rdl:PCA_100006763>
    <rdl:PCA_100006766 rdf:resource="http://rds.posccaesar.org/ontology/plm/rdl/PCA_100006657"/>
    <rdl:PCA_100006765 rdf:resource="http://w3id.org/readi/rdl/CFIHOS-20000018"/>
  </owl:Class>
  <owl:Class rdf:about="http://rds.posccaesar.org/ontology/plm/rdl/PCA_100006396">
    <skos:broader rdf:resource="http://rds.posccaesar.org/ontology/plm/rdl/PCA_100006745"/>
    <skos:broadMatch rdf:resource="http://rds.posccaesar.org/ontology/plm/rdl/PCA_100006727"/>
    <rdfs:label>Process safety schematics</rdfs:label>
    <rdfs:comment>The minimum required information for main process safety schematics shall be:
- Relevant main process equipment
- Sectionalization valves
- Pressure protection devices (PRV, PSE, other) with set-point and dimensioning case indicated
- PSD transmitters
- Non-return valves of relevance for process safety
- Depressurization valves
- Fail safe position of valves
- Control functions relevant for process safety
- Pressure and temperature specification
- Line design pressure and temperature (breaks)
- Actuated block valves other than ESV and XSV valves (XV)
- Which disposal system streams are routed to
- Chemical injection points
- Drain points (CD)
- Future system included
- It is recommended to visualize the blowdown segments (by color-codes).</rdfs:comment>
    <rdl:PCA_100006768>The minimum required information for main process safety schematics shall be:
- Relevant main process equipment
- Sectionalization valves
- Pressure protection devices (PRV, PSE, other) with set-point and dimensioning case indicated
- PSD transmitters
- Non-return valves of relevance for process safety
- Depressurization valves
- Fail safe position of valves
- Control functions relevant for process safety
- Pressure and temperature specification
- Line design pressure and temperature (breaks)
- Actuated block valves other than ESV and XSV valves (XV)
- Which disposal system streams are routed to
- Chemical injection points
- Drain points (CD)
- Future system included
- It is recommended to visualize the blowdown segments (by color-codes).</rdl:PCA_100006768>
    <rdl:PCA_100006765 rdf:resource="http://w3id.org/readi/rdl/CFIHOS-20000026"/>
    <rdl:PCA_100006765 rdf:resource="http://w3id.org/readi/rdl/CFIHOS-20000013"/>
    <rdfs:subClassOf rdf:resource="http://rds.posccaesar.org/ontology/plm/rdl/PCA_100004908"/>
  </owl:Class>
  <owl:Class rdf:about="http://rds.posccaesar.org/ontology/plm/rdl/PCA_100006275">
    <skos:broader rdf:resource="http://rds.posccaesar.org/ontology/plm/rdl/PCA_100006751"/>
    <skos:broadMatch rdf:resource="http://rds.posccaesar.org/ontology/plm/rdl/PCA_100006688"/>
    <rdfs:label>Installation and handling manual flexible pipeline and riser</rdfs:label>
    <rdfs:comment>The installation and handling manual shall include:
 - installation,
 - load-out facilities at manufactures premises,
 - recommendations related to seawater fill or dry during installation,
 - outline installation method including main sequences,
 - allowable installation loads,
 - deformation,
 - capacities and limitations,
 - handling and lifting recommendations,
 - installation tolerances,
 - assembly and handling procedures for all accessories (ancillary equipment),
 - description of markings,
 - tolerances related to mounting positions of accessories along the flexible pipeline,
 - use of mounting tools, torque moments etc.,
 - relevant certificates.</rdfs:comment>
    <rdl:PCA_100006768>The installation and handling manual shall include:
 - installation,
 - load-out facilities at manufactures premises,
 - recommendations related to seawater fill or dry during installation,
 - outline installation method including main sequences,
 - allowable installation loads,
 - deformation,
 - capacities and limitations,
 - handling and lifting recommendations,
 - installation tolerances,
 - assembly and handling procedures for all accessories (ancillary equipment),
 - description of markings,
 - tolerances related to mounting positions of accessories along the flexible pipeline,
 - use of mounting tools, torque moments etc.,
 - relevant certificates.</rdl:PCA_100006768>
    <rdl:PCA_100006766 rdf:resource="http://rds.posccaesar.org/ontology/plm/rdl/PCA_100006657"/>
    <rdl:PCA_100006765 rdf:resource="http://w3id.org/readi/rdl/CFIHOS-20000018"/>
    <rdfs:subClassOf rdf:resource="http://rds.posccaesar.org/ontology/plm/rdl/PCA_100004908"/>
  </owl:Class>
  <owl:Class rdf:about="http://rds.posccaesar.org/ontology/plm/rdl/PCA_100006493">
    <skos:broadMatch rdf:resource="http://rds.posccaesar.org/ontology/plm/rdl/PCA_100006702"/>
    <rdfs:comment>Load list for telecommunication power supply.</rdfs:comment>
    <rdfs:label>Telecommunication power supply load list</rdfs:label>
    <rdl:PCA_100006766 rdf:resource="http://rds.posccaesar.org/ontology/plm/rdl/PCA_100006640"/>
    <rdfs:subClassOf rdf:resource="http://rds.posccaesar.org/ontology/plm/rdl/PCA_100004908"/>
    <rdl:PCA_100006765 rdf:resource="http://w3id.org/readi/rdl/CFIHOS-20000030"/>
    <rdl:PCA_100006768>Load list for telecommunication power supply.</rdl:PCA_100006768>
    <skos:broader rdf:resource="http://rds.posccaesar.org/ontology/plm/rdl/PCA_100006748"/>
    <skos:broadMatch rdf:resource="http://rds.posccaesar.org/ontology/plm/rdl/PCA_100006716"/>
  </owl:Class>
  <owl:Class rdf:about="http://rds.posccaesar.org/ontology/plm/rdl/PCA_100006263">
    <rdfs:comment>A diagram showing hydraulic connections between equipment and components.</rdfs:comment>
    <skos:broader rdf:resource="http://rds.posccaesar.org/ontology/plm/rdl/PCA_100006745"/>
    <rdfs:subClassOf rdf:resource="http://rds.posccaesar.org/ontology/plm/rdl/PCA_100004908"/>
    <rdfs:label>Hydraulic schematic</rdfs:label>
    <rdl:PCA_100006766 rdf:resource="http://rds.posccaesar.org/ontology/plm/rdl/PCA_100006653"/>
    <skos:broadMatch rdf:resource="http://rds.posccaesar.org/ontology/plm/rdl/PCA_100006696"/>
    <rdl:PCA_100006765 rdf:resource="http://w3id.org/readi/rdl/CFIHOS-20000031"/>
    <rdl:PCA_100006768>A diagram showing hydraulic connections between equipment and components.</rdl:PCA_100006768>
    <rdl:PCA_100006763>To provide an overview of hydraulic equipment and their connections.</rdl:PCA_100006763>
  </owl:Class>
  <owl:Class rdf:about="http://rds.posccaesar.org/ontology/plm/rdl/PCA_100006384">
    <rdl:PCA_100006763>Certificate to confirm compliance with contract / purchase order with reference to standards, technical specifications and requirements for the product.</rdl:PCA_100006763>
    <rdfs:subClassOf rdf:resource="http://rds.posccaesar.org/ontology/plm/rdl/PCA_100004908"/>
    <rdl:PCA_100006765 rdf:resource="http://w3id.org/readi/rdl/CFIHOS-20000027"/>
    <rdfs:comment>The manufacture’s or other party’s confirmation that the product is designed, manufactured and tested as specified.</rdfs:comment>
    <rdfs:label>PO declaration of compliance</rdfs:label>
    <rdl:PCA_100006766 rdf:resource="http://rds.posccaesar.org/ontology/plm/rdl/PCA_100006653"/>
    <skos:broader rdf:resource="http://rds.posccaesar.org/ontology/plm/rdl/PCA_100006743"/>
    <rdl:PCA_100006768>The manufacture’s or other party’s confirmation that the product is designed, manufactured and tested as specified.</rdl:PCA_100006768>
    <skos:broadMatch rdf:resource="http://rds.posccaesar.org/ontology/plm/rdl/PCA_100006722"/>
  </owl:Class>
  <owl:Class rdf:about="http://rds.posccaesar.org/ontology/plm/rdl/PCA_100006372">
    <rdl:PCA_100006766 rdf:resource="http://rds.posccaesar.org/ontology/plm/rdl/PCA_100006585"/>
    <rdl:PCA_100006766 rdf:resource="http://rds.posccaesar.org/ontology/plm/rdl/PCA_100006589"/>
    <rdl:PCA_100006766 rdf:resource="http://rds.posccaesar.org/ontology/plm/rdl/PCA_100006623"/>
    <rdl:PCA_100006766 rdf:resource="http://rds.posccaesar.org/ontology/plm/rdl/PCA_100006597"/>
    <rdfs:comment>P&amp;IDs shall be prepared for drilling+C402:C440 systems, main process (production, injection and export) systems, process support and utility systems and safety systems, including subsea parts of the systems (if any). 

All equipment, piping, valves, orifices and blinds and instrumentation shall be shown on the P&amp;IDs. Identical/parallel items, equipment or systems shall be drawn in full detail, i.e. typical drawings with associated tag number tables are not permitted. 

The number of equipment units on one P&amp;ID shall typically be limited to (a) one vessel or compressor and (b) parallel pumps or heat exchangers. For all connections (e.g. lines and instrument signals) between P&amp;IDs/P&amp;ID sheets, a descriptive text and the connected drawing number shall be included. 

The P&amp;IDs shall include boundary lines for interfaces to an equipment supplier’s scope. Unique numbers shall be included for the connections crossing these boundary lines. The equipment supplier prepares P&amp;IDs for the supplier scope. The P&amp;ID shall include a reference to the equipment supplier P&amp;ID(s), preferably within the boundary lines. Where the equipment supplier scope is on several P&amp;IDs/P&amp;ID sheets, a cross reference between connection number and P&amp;ID/P&amp;ID sheet shall also be included. 

Regarding equipment, the following shall as a minimum be included:
 - Tag number;
 - Equipment (main) data in a table on the P&amp;ID;
 - Elevation;
 - Equipment internals that is important to understand the functionality such as weir plate, sections of packing/plates, heat bundle, static mixers etc. shall be shown schematically;
 - Isolation and spading of equipment;
 - Manholes incl. nozzle size;
 - Insulation and heat tracing;
 - Open drains and drip trays;
 - Equipment connections such as connections for instruments, purge, steam out, vent and drains;
 - Inline equipment such as silencers, straightening vanes and strainers. A note shall describe the purpose and requirements for strainers (temporary/permanent, maximum allowable pressure drop etc.

Regarding lines the following shall as a minimum be included: 
 - Line number;
 - Direction of flow;
 - Requirements to layout/routing such as line slope and no pockets, symmetrical piping, branch entry to header (e.g. top of header), minimum straight length and minimum and maximum distances;
 - Height/elevation data where required for sumps;
 - Line size change (reducers);
 - Piping specification break;
 - Insulation break;
 - Heat tracing and heat trace break;
 - Blind flanges, caps, plugs or other at end of headers;
 - Spool pieces and flanges required for maintenance and operation;
 - Underground/aboveground breaks;
 - Floor/module breaks;
 - Area breaks;
 - Liquid or gas seal traps and goose necks;
 - Line connections such as connections for instruments, hoses, sampling, chemical injection, probes, pulsation damper, cleaning, drain, vent and temporary uses (to be described in a note).

Regarding valves, orifices and blinds the following shall as a minimum be included: 
 - Tag number for all valves, orifices and blinds;
 - For manual valves:
    - All manual piping valves shall be tagged with nominal pipe size and valve specification reference/VDS-number (or piping special item tag number if applicable). Individual valve tag numbers shall be added on the "issued for construction" revision at the latest Locking/interlocking to secure correct operational position (e.g. KILO/KILC = mechanical key interlock open/closed, or CSO/CSC car seal open/closed);
    - Position indication on valves where relevant (normally open or normally closed);

For actuated valves:
   - All on/off actuated valves such as ESV, XSV, XV and HV shall be shown with nominal pipe size and VDS-number in addition to tag number;
   - Leakage class of all actuated valves;
   - Fail positions of all actuated valves (i.e. open/closed/maintained position);
   - Limit switches of actuated valves;
   - Position indication on valves (normally open or normally closed) where relevant;
 - Relief valve size and set pressure;
 - Spectacle blinds and spade/spacers, shown in normal position;
 - Special requirements to be note.

Regarding instrumentation the following shall as a minimum be included: 
 - Tag number;
 - Connections to local control and SAS (ESD, PSD or PCS);
 - Requirement for local reading of instrument;
 - Control power (pneumatic/hydraulic fluid or electrical power);
 - Alarm and trip functions (H, L, HH, LL) shall be indicated and set points shall be shown for trip functions;
 - Port identification when 3-way valves are used;
 - Heat tracing and insulation on instruments;
 - Type of level and flow instruments;
 - The piping valves connecting the instruments to the process, i.e. the valves required for isolation from the process shall be shown specifically. Detailed information about the instrument hook-up, however, will be found on the instrument hook-up drawings.</rdfs:comment>
    <rdl:PCA_100006766 rdf:resource="http://rds.posccaesar.org/ontology/plm/rdl/PCA_100006610"/>
    <rdl:PCA_100006766 rdf:resource="http://rds.posccaesar.org/ontology/plm/rdl/PCA_100006580"/>
    <rdl:PCA_100006766 rdf:resource="http://rds.posccaesar.org/ontology/plm/rdl/PCA_100006628"/>
    <rdl:PCA_100006766 rdf:resource="http://rds.posccaesar.org/ontology/plm/rdl/PCA_100006604"/>
    <rdl:PCA_100006766 rdf:resource="http://rds.posccaesar.org/ontology/plm/rdl/PCA_100006611"/>
    <rdl:PCA_100006763>The symbols used for the P&amp;IDs shall be explained by a legend which shall be a part of the total P&amp;ID set. The P&amp;IDs shall use the coding and numbering standard in ENS, and the plant legend and drawing standard in accordance to NORSOK Z-005.

Norsok S-001 "Tecnical safety"</rdl:PCA_100006763>
    <rdl:PCA_100006766 rdf:resource="http://rds.posccaesar.org/ontology/plm/rdl/PCA_100006616"/>
    <rdl:PCA_100006766 rdf:resource="http://rds.posccaesar.org/ontology/plm/rdl/PCA_100006603"/>
    <rdl:PCA_100006766 rdf:resource="http://rds.posccaesar.org/ontology/plm/rdl/PCA_100006620"/>
    <rdl:PCA_100006766 rdf:resource="http://rds.posccaesar.org/ontology/plm/rdl/PCA_100006607"/>
    <rdl:PCA_100006766 rdf:resource="http://rds.posccaesar.org/ontology/plm/rdl/PCA_100006581"/>
    <rdl:PCA_100006766 rdf:resource="http://rds.posccaesar.org/ontology/plm/rdl/PCA_100006608"/>
    <rdl:PCA_100006766 rdf:resource="http://rds.posccaesar.org/ontology/plm/rdl/PCA_100006593"/>
    <rdl:PCA_100006765 rdf:resource="http://w3id.org/readi/rdl/CFIHOS-20000026"/>
    <rdl:PCA_100006766 rdf:resource="http://rds.posccaesar.org/ontology/plm/rdl/PCA_100006594"/>
    <rdl:PCA_100006766 rdf:resource="http://rds.posccaesar.org/ontology/plm/rdl/PCA_100006600"/>
    <rdl:PCA_100006766 rdf:resource="http://rds.posccaesar.org/ontology/plm/rdl/PCA_100006625"/>
    <rdl:PCA_100006766 rdf:resource="http://rds.posccaesar.org/ontology/plm/rdl/PCA_100006598"/>
    <rdl:PCA_100006766 rdf:resource="http://rds.posccaesar.org/ontology/plm/rdl/PCA_100006586"/>
    <skos:broader rdf:resource="http://rds.posccaesar.org/ontology/plm/rdl/PCA_100006745"/>
    <skos:broadMatch rdf:resource="http://rds.posccaesar.org/ontology/plm/rdl/PCA_100006696"/>
    <rdl:PCA_100006766 rdf:resource="http://rds.posccaesar.org/ontology/plm/rdl/PCA_100006612"/>
    <rdfs:subClassOf rdf:resource="http://rds.posccaesar.org/ontology/plm/rdl/PCA_100004908"/>
    <rdl:PCA_100006768>P&amp;IDs shall be prepared for drilling+C402:C440 systems, main process (production, injection and export) systems, process support and utility systems and safety systems, including subsea parts of the systems (if any). 

All equipment, piping, valves, orifices and blinds and instrumentation shall be shown on the P&amp;IDs. Identical/parallel items, equipment or systems shall be drawn in full detail, i.e. typical drawings with associated tag number tables are not permitted. 

The number of equipment units on one P&amp;ID shall typically be limited to (a) one vessel or compressor and (b) parallel pumps or heat exchangers. For all connections (e.g. lines and instrument signals) between P&amp;IDs/P&amp;ID sheets, a descriptive text and the connected drawing number shall be included. 

The P&amp;IDs shall include boundary lines for interfaces to an equipment supplier’s scope. Unique numbers shall be included for the connections crossing these boundary lines. The equipment supplier prepares P&amp;IDs for the supplier scope. The P&amp;ID shall include a reference to the equipment supplier P&amp;ID(s), preferably within the boundary lines. Where the equipment supplier scope is on several P&amp;IDs/P&amp;ID sheets, a cross reference between connection number and P&amp;ID/P&amp;ID sheet shall also be included. 

Regarding equipment, the following shall as a minimum be included:
 - Tag number;
 - Equipment (main) data in a table on the P&amp;ID;
 - Elevation;
 - Equipment internals that is important to understand the functionality such as weir plate, sections of packing/plates, heat bundle, static mixers etc. shall be shown schematically;
 - Isolation and spading of equipment;
 - Manholes incl. nozzle size;
 - Insulation and heat tracing;
 - Open drains and drip trays;
 - Equipment connections such as connections for instruments, purge, steam out, vent and drains;
 - Inline equipment such as silencers, straightening vanes and strainers. A note shall describe the purpose and requirements for strainers (temporary/permanent, maximum allowable pressure drop etc.

Regarding lines the following shall as a minimum be included: 
 - Line number;
 - Direction of flow;
 - Requirements to layout/routing such as line slope and no pockets, symmetrical piping, branch entry to header (e.g. top of header), minimum straight length and minimum and maximum distances;
 - Height/elevation data where required for sumps;
 - Line size change (reducers);
 - Piping specification break;
 - Insulation break;
 - Heat tracing and heat trace break;
 - Blind flanges, caps, plugs or other at end of headers;
 - Spool pieces and flanges required for maintenance and operation;
 - Underground/aboveground breaks;
 - Floor/module breaks;
 - Area breaks;
 - Liquid or gas seal traps and goose necks;
 - Line connections such as connections for instruments, hoses, sampling, chemical injection, probes, pulsation damper, cleaning, drain, vent and temporary uses (to be described in a note).

Regarding valves, orifices and blinds the following shall as a minimum be included: 
 - Tag number for all valves, orifices and blinds;
 - For manual valves:
    - All manual piping valves shall be tagged with nominal pipe size and valve specification reference/VDS-number (or piping special item tag number if applicable). Individual valve tag numbers shall be added on the "issued for construction" revision at the latest Locking/interlocking to secure correct operational position (e.g. KILO/KILC = mechanical key interlock open/closed, or CSO/CSC car seal open/closed);
    - Position indication on valves where relevant (normally open or normally closed);

For actuated valves:
   - All on/off actuated valves such as ESV, XSV, XV and HV shall be shown with nominal pipe size and VDS-number in addition to tag number;
   - Leakage class of all actuated valves;
   - Fail positions of all actuated valves (i.e. open/closed/maintained position);
   - Limit switches of actuated valves;
   - Position indication on valves (normally open or normally closed) where relevant;
 - Relief valve size and set pressure;
 - Spectacle blinds and spade/spacers, shown in normal position;
 - Special requirements to be note.

Regarding instrumentation the following shall as a minimum be included: 
 - Tag number;
 - Connections to local control and SAS (ESD, PSD or PCS);
 - Requirement for local reading of instrument;
 - Control power (pneumatic/hydraulic fluid or electrical power);
 - Alarm and trip functions (H, L, HH, LL) shall be indicated and set points shall be shown for trip functions;
 - Port identification when 3-way valves are used;
 - Heat tracing and insulation on instruments;
 - Type of level and flow instruments;
 - The piping valves connecting the instruments to the process, i.e. the valves required for isolation from the process shall be shown specifically. Detailed information about the instrument hook-up, however, will be found on the instrument hook-up drawings.</rdl:PCA_100006768>
    <rdl:PCA_100006766 rdf:resource="http://rds.posccaesar.org/ontology/plm/rdl/PCA_100006613"/>
    <rdl:PCA_100006766 rdf:resource="http://rds.posccaesar.org/ontology/plm/rdl/PCA_100006617"/>
    <rdl:PCA_100006766 rdf:resource="http://rds.posccaesar.org/ontology/plm/rdl/PCA_100006578"/>
    <rdl:PCA_100006766 rdf:resource="http://rds.posccaesar.org/ontology/plm/rdl/PCA_100006605"/>
    <rdl:PCA_100006766 rdf:resource="http://rds.posccaesar.org/ontology/plm/rdl/PCA_100006609"/>
    <rdl:PCA_100006766 rdf:resource="http://rds.posccaesar.org/ontology/plm/rdl/PCA_100006583"/>
    <rdl:PCA_100006766 rdf:resource="http://rds.posccaesar.org/ontology/plm/rdl/PCA_100006590"/>
    <rdl:PCA_100006766 rdf:resource="http://rds.posccaesar.org/ontology/plm/rdl/PCA_100006587"/>
    <rdl:PCA_100006766 rdf:resource="http://rds.posccaesar.org/ontology/plm/rdl/PCA_100006621"/>
    <rdl:PCA_100006766 rdf:resource="http://rds.posccaesar.org/ontology/plm/rdl/PCA_100006595"/>
    <rdl:PCA_100006766 rdf:resource="http://rds.posccaesar.org/ontology/plm/rdl/PCA_100006582"/>
    <rdl:PCA_100006766 rdf:resource="http://rds.posccaesar.org/ontology/plm/rdl/PCA_100006599"/>
    <rdfs:label>Piping and instrument diagram (P&amp;ID)</rdfs:label>
    <rdl:PCA_100006766 rdf:resource="http://rds.posccaesar.org/ontology/plm/rdl/PCA_100006596"/>
    <rdl:PCA_100006766 rdf:resource="http://rds.posccaesar.org/ontology/plm/rdl/PCA_100006601"/>
    <rdl:PCA_100006766 rdf:resource="http://rds.posccaesar.org/ontology/plm/rdl/PCA_100006622"/>
    <rdl:PCA_100006766 rdf:resource="http://rds.posccaesar.org/ontology/plm/rdl/PCA_100006579"/>
    <rdl:PCA_100006766 rdf:resource="http://rds.posccaesar.org/ontology/plm/rdl/PCA_100006606"/>
    <rdl:PCA_100006766 rdf:resource="http://rds.posccaesar.org/ontology/plm/rdl/PCA_100006591"/>
    <rdl:PCA_100006766 rdf:resource="http://rds.posccaesar.org/ontology/plm/rdl/PCA_100006618"/>
    <rdl:PCA_100006765 rdf:resource="http://w3id.org/readi/rdl/CFIHOS-20000031"/>
    <rdl:PCA_100006766 rdf:resource="http://rds.posccaesar.org/ontology/plm/rdl/PCA_100006592"/>
    <rdl:PCA_100006766 rdf:resource="http://rds.posccaesar.org/ontology/plm/rdl/PCA_100006602"/>
    <rdl:PCA_100006766 rdf:resource="http://rds.posccaesar.org/ontology/plm/rdl/PCA_100006627"/>
    <rdl:PCA_100006766 rdf:resource="http://rds.posccaesar.org/ontology/plm/rdl/PCA_100006614"/>
    <rdl:PCA_100006766 rdf:resource="http://rds.posccaesar.org/ontology/plm/rdl/PCA_100006584"/>
    <rdl:PCA_100006766 rdf:resource="http://rds.posccaesar.org/ontology/plm/rdl/PCA_100006588"/>
    <rdl:PCA_100006766 rdf:resource="http://rds.posccaesar.org/ontology/plm/rdl/PCA_100006615"/>
    <rdl:PCA_100006766 rdf:resource="http://rds.posccaesar.org/ontology/plm/rdl/PCA_100006619"/>
    <rdl:PCA_100006766 rdf:resource="http://rds.posccaesar.org/ontology/plm/rdl/PCA_100006624"/>
  </owl:Class>
  <owl:Class rdf:about="http://rds.posccaesar.org/ontology/plm/rdl/PCA_100006251">
    <rdfs:subClassOf rdf:resource="http://rds.posccaesar.org/ontology/plm/rdl/PCA_100004908"/>
    <skos:broadMatch rdf:resource="http://rds.posccaesar.org/ontology/plm/rdl/PCA_100006732"/>
    <skos:broader rdf:resource="http://rds.posccaesar.org/ontology/plm/rdl/PCA_100006746"/>
    <rdl:PCA_100006768>The following drawings shall be provided:

1. Entire installation, profile view - all four quadrants

The drawings shall be prepared in accordance with the following requirements:
 - Showing entire structure from sea level to highest point;
 - Indication of sea level;
 - Elevation of helideck above sea level;
 - Elevation of highest point above sea level;
 - Location of obstacle lights;
 - Location of turbine exhaust outlet(s);
 - Location of cold emission source(s);
 - Location of anemometer(s);
 - Scales indicating metres and feet.


2. Entire installation, plan view (looking from above)

The drawings shall be prepared in accordance with the following requirements:
 - Reference to platform and true north;
 - Location of obstacle lights;
 - Location of turbine exhaust outlet(s);
 - Location of cold emission source(s);
 - Location of anemometer(s);
 - Location of windsock(s);
 - Scales indicating metres and feet.


3.  Helideck with surroundings (can included as a part of 2.)

The drawings shall be prepared in accordance with the following requirements:
 - Reference to platform and true north;
 - Latitude/Longitude (WGS84) of centre helideck;
 - Helideck magnetic direction, degrees True;
 - Helideck marking;
 - Helideck lighting;
 - Helideck firefighting equipment;
 - HTCC;
 - Antenna tower;
 - Lowered walkway/Perimeter net;
 - Accesses;
 - Depiction of Obstacle Free Sectors (180 and 210 degree);
 - Depiction of Limited Obstacle Sector (150 degree), including the extent of segment 1 and 2;
 - Elevation of structures in 150 LOS segment 1 and 2;
 - Elevation of structures close to 210 degree OFS;
 - Helicopter fuelling plant;
 - Scales indicating metres and feet.</rdl:PCA_100006768>
    <skos:broadMatch rdf:resource="http://rds.posccaesar.org/ontology/plm/rdl/PCA_100006733"/>
    <skos:broadMatch rdf:resource="http://rds.posccaesar.org/ontology/plm/rdl/PCA_100006707"/>
    <skos:broadMatch rdf:resource="http://rds.posccaesar.org/ontology/plm/rdl/PCA_100006734"/>
    <rdl:PCA_100006765 rdf:resource="http://w3id.org/readi/rdl/CFIHOS-20000011"/>
    <rdl:PCA_100006763>As required in FOR-2007-10-26-1181:</rdl:PCA_100006763>
    <rdl:PCA_100006765 rdf:resource="http://w3id.org/readi/rdl/CFIHOS-20000013"/>
    <rdl:PCA_100006766 rdf:resource="http://rds.posccaesar.org/ontology/plm/rdl/PCA_100006656"/>
    <rdfs:comment>The following drawings shall be provided:

1. Entire installation, profile view - all four quadrants

The drawings shall be prepared in accordance with the following requirements:
 - Showing entire structure from sea level to highest point;
 - Indication of sea level;
 - Elevation of helideck above sea level;
 - Elevation of highest point above sea level;
 - Location of obstacle lights;
 - Location of turbine exhaust outlet(s);
 - Location of cold emission source(s);
 - Location of anemometer(s);
 - Scales indicating metres and feet.


2. Entire installation, plan view (looking from above)

The drawings shall be prepared in accordance with the following requirements:
 - Reference to platform and true north;
 - Location of obstacle lights;
 - Location of turbine exhaust outlet(s);
 - Location of cold emission source(s);
 - Location of anemometer(s);
 - Location of windsock(s);
 - Scales indicating metres and feet.


3.  Helideck with surroundings (can included as a part of 2.)

The drawings shall be prepared in accordance with the following requirements:
 - Reference to platform and true north;
 - Latitude/Longitude (WGS84) of centre helideck;
 - Helideck magnetic direction, degrees True;
 - Helideck marking;
 - Helideck lighting;
 - Helideck firefighting equipment;
 - HTCC;
 - Antenna tower;
 - Lowered walkway/Perimeter net;
 - Accesses;
 - Depiction of Obstacle Free Sectors (180 and 210 degree);
 - Depiction of Limited Obstacle Sector (150 degree), including the extent of segment 1 and 2;
 - Elevation of structures in 150 LOS segment 1 and 2;
 - Elevation of structures close to 210 degree OFS;
 - Helicopter fuelling plant;
 - Scales indicating metres and feet.</rdfs:comment>
    <rdfs:label>Helideck drawings (offshore)</rdfs:label>
    <rdl:PCA_100006765 rdf:resource="http://w3id.org/readi/rdl/CFIHOS-20000010"/>
    <skos:broadMatch rdf:resource="http://rds.posccaesar.org/ontology/plm/rdl/PCA_100006731"/>
  </owl:Class>
  <owl:Class rdf:about="http://rds.posccaesar.org/ontology/plm/rdl/PCA_100006360">
    <rdfs:label>Photo archive - subsea systems</rdfs:label>
    <rdfs:comment>A photo archive with pictures of the delivered item(s). 

 - Pictures shall be in JPEG format.
 - The file name for each picture shall describe the item in the picture.
 - There shall in general be taken picture of each tagged item (or each material/serial-numbered item if untagged), with focus on showing the tagged item in a best possible manner and with enough of its surroundings to get a picture of the location. Several pictures of the same item may be taken for clarity.
 - For a module or structure that contains many tagged items (such as valves, instruments, pumps, hatches, etc.) there shall be taken overview pictures of the module/structure from all sides and top, as well of each tagged item within the module/structure.</rdfs:comment>
    <rdl:PCA_100006768>A photo archive with pictures of the delivered item(s). 

 - Pictures shall be in JPEG format.
 - The file name for each picture shall describe the item in the picture.
 - There shall in general be taken picture of each tagged item (or each material/serial-numbered item if untagged), with focus on showing the tagged item in a best possible manner and with enough of its surroundings to get a picture of the location. Several pictures of the same item may be taken for clarity.
 - For a module or structure that contains many tagged items (such as valves, instruments, pumps, hatches, etc.) there shall be taken overview pictures of the module/structure from all sides and top, as well of each tagged item within the module/structure.</rdl:PCA_100006768>
    <rdl:PCA_100006766 rdf:resource="http://rds.posccaesar.org/ontology/plm/rdl/PCA_100006653"/>
    <rdl:PCA_100006765 rdf:resource="http://w3id.org/readi/rdl/CFIHOS-20000031"/>
    <rdfs:subClassOf rdf:resource="http://rds.posccaesar.org/ontology/plm/rdl/PCA_100004908"/>
  </owl:Class>
  <owl:Class rdf:about="http://rds.posccaesar.org/ontology/plm/rdl/PCA_100006481">
    <rdfs:label>System duct &amp; instrumentation diagrams (D&amp;ID)</rdfs:label>
    <rdl:PCA_100006765 rdf:resource="http://w3id.org/readi/rdl/CFIHOS-20000019"/>
    <rdfs:comment>System Duct &amp; Instrument Diagram (D&amp;ID) shall be provided by system and include the following information:
 - All HVAC equipment with their tag number and all HVAC bulk items with their item number;
 - Equipment data summary with tag number for all main equipment such as filters, fans, coils, etc.;
 - All ductwork identified with system no., sizes, duct classes, insulation classes;
 - All inline equipment;
 - Air flow to main areas;
 - Area breaks and duct class breaks;
 - All instrumentation/F&amp;G reflecting the control functions;
 - All instrument locations shall be indicated and completed with tag numbers;
 - Connections to other systems e.g. sea water, heating, cooling, drain, etc.;
 - Airflow in and out of diagram with references.</rdfs:comment>
    <rdl:PCA_100006763>The complete System Duct &amp; Instrumentation Diagram (D&amp;ID) shall be in accordance with the plants’ process typicals and drafting standard.

The level of detail within packages shall be identical to that outside.

Tag number shall be shown for all tagged components.</rdl:PCA_100006763>
    <skos:broadMatch rdf:resource="http://rds.posccaesar.org/ontology/plm/rdl/PCA_100006696"/>
    <rdl:PCA_100006766 rdf:resource="http://rds.posccaesar.org/ontology/plm/rdl/PCA_100006650"/>
    <rdfs:subClassOf rdf:resource="http://rds.posccaesar.org/ontology/plm/rdl/PCA_100004908"/>
    <skos:broader rdf:resource="http://rds.posccaesar.org/ontology/plm/rdl/PCA_100006745"/>
    <rdl:PCA_100006768>System Duct &amp; Instrument Diagram (D&amp;ID) shall be provided by system and include the following information:
 - All HVAC equipment with their tag number and all HVAC bulk items with their item number;
 - Equipment data summary with tag number for all main equipment such as filters, fans, coils, etc.;
 - All ductwork identified with system no., sizes, duct classes, insulation classes;
 - All inline equipment;
 - Air flow to main areas;
 - Area breaks and duct class breaks;
 - All instrumentation/F&amp;G reflecting the control functions;
 - All instrument locations shall be indicated and completed with tag numbers;
 - Connections to other systems e.g. sea water, heating, cooling, drain, etc.;
 - Airflow in and out of diagram with references.</rdl:PCA_100006768>
  </owl:Class>
  <owl:Class rdf:about="http://rds.posccaesar.org/ontology/plm/rdl/PCA_100006220">
    <rdl:PCA_100006766 rdf:resource="http://rds.posccaesar.org/ontology/plm/rdl/PCA_100006587"/>
    <skos:broader rdf:resource="http://rds.posccaesar.org/ontology/plm/rdl/PCA_100006756"/>
    <rdl:PCA_100006766 rdf:resource="http://rds.posccaesar.org/ontology/plm/rdl/PCA_100006591"/>
    <rdl:PCA_100006764>A document containing uncertainty analysis for the metering system shall be provided.  For Gas ultrasonic meters the influence of different pressure and temperature between calibration conditions and operational conditions shall be documented.</rdl:PCA_100006764>
    <rdfs:label>Fiscal metering - Uncertainty analysis</rdfs:label>
    <skos:broader rdf:resource="http://rds.posccaesar.org/ontology/plm/rdl/PCA_100006741"/>
    <skos:broadMatch rdf:resource="http://rds.posccaesar.org/ontology/plm/rdl/PCA_100006687"/>
    <rdl:PCA_100006765 rdf:resource="http://w3id.org/readi/rdl/CFIHOS-20000015"/>
    <rdfs:subClassOf rdf:resource="http://rds.posccaesar.org/ontology/plm/rdl/PCA_100004908"/>
  </owl:Class>
  <owl:Class rdf:about="http://rds.posccaesar.org/ontology/plm/rdl/PCA_100006111">
    <skos:broader rdf:resource="http://rds.posccaesar.org/ontology/plm/rdl/PCA_100006746"/>
    <skos:broadMatch rdf:resource="http://rds.posccaesar.org/ontology/plm/rdl/PCA_100006709"/>
    <rdfs:label>Cable ladder/trays &gt;=300 mm layout drawings</rdfs:label>
    <rdfs:comment>For the following, individual layout drawings shall be provided:   Cable ladders/trays &gt; =300 mm</rdfs:comment>
    <rdl:PCA_100006768>For the following, individual layout drawings shall be provided:   Cable ladders/trays &gt; =300 mm</rdl:PCA_100006768>
    <rdl:PCA_100006766 rdf:resource="http://rds.posccaesar.org/ontology/plm/rdl/PCA_100006656"/>
    <rdl:PCA_100006765 rdf:resource="http://w3id.org/readi/rdl/CFIHOS-20000008"/>
    <rdfs:subClassOf rdf:resource="http://rds.posccaesar.org/ontology/plm/rdl/PCA_100004908"/>
  </owl:Class>
  <owl:Class rdf:about="http://rds.posccaesar.org/ontology/plm/rdl/PCA_100006123">
    <rdl:PCA_100006768>Document containing records of performed surface protection and coating work.</rdl:PCA_100006768>
    <skos:broader rdf:resource="http://rds.posccaesar.org/ontology/plm/rdl/PCA_100006756"/>
    <rdfs:comment>Document containing records of performed surface protection and coating work.</rdfs:comment>
    <rdfs:subClassOf rdf:resource="http://rds.posccaesar.org/ontology/plm/rdl/PCA_100004908"/>
    <rdfs:label>Coating report</rdfs:label>
    <skos:broadMatch rdf:resource="http://rds.posccaesar.org/ontology/plm/rdl/PCA_100006722"/>
    <rdl:PCA_100006764>Requirements related to assurance and check of quality in manufacturing phase will very much depend on Purchaser’s knowledge of supplier. Well known supplier, with proven track record, delivering products based on industry standards, will typically deliver less verification documentation to Purchaser than unknown/new supplier delivering the same product. Therefore, this deliverable should be evaluated as candidate for being available in digital format to Purchaser, for information only.</rdl:PCA_100006764>
    <rdl:PCA_100006766 rdf:resource="http://rds.posccaesar.org/ontology/plm/rdl/PCA_100006653"/>
    <rdl:PCA_100006765 rdf:resource="http://w3id.org/readi/rdl/CFIHOS-20000028"/>
    <rdl:PCA_100006763>This document is used for verification of compliance with surface protection and coating requirements.</rdl:PCA_100006763>
  </owl:Class>
  <owl:Class rdf:about="http://rds.posccaesar.org/ontology/plm/rdl/PCA_100006135">
    <rdfs:comment>LCI strategy shall as a minimum include the following:
 - Contractor’s Life Cycle information management organization;
 - An overall strategy for interaction between internal parties, such as procurement and engineering.;
 - An overall integration strategy of life cycle information from all parties involved such as external contractors, subcontractors and suppliers;
 - Contractor shall describe their systems portfolio related to the production and administration of LCI including integration capabilities with the Company systems;
 - Training strategy of staff in both Company’s and Contractor's LCI tools;
 - LCI Handover strategy from MC to Commissioning;
 - Strategy for Material control and SPIR handling;
 - Contractor's method for LCI quality control and systematic correction of quality issues;
 - Contractor's method for ensuring delivery of 3D CAD design models throughout the project in compliance with Company’s requirements;
 - LCI procedures (including):
   - Procedure for collection, storage, processing, transfer and sharing of LCI;
   - The procedure for standard documentation handling;
   - Work procedures for 3D handling as described in Company’s requirements;
   - The procedure shall include transfer methods, information logistics, systems involved, responsibilities, milestones, quality control, error reporting and rectification;
   - The procedure for tag scoping for supplier packages;
   - The procedure for tag scoping for engineering;
   - List containing Contractors planned deliveries of LCI according to Company's requirements;
   - Time schedules showing LCI deliveries including 3D;
   - Procedures or method to ensure special attention to identify early access and QC milestones. The schedules shall reflect the project execution plan and time schedules;
   - Procedure for LCI progress reporting according to LCI time schedules;
   - Procedures and checklists to ensure quality and completeness of the LCI delivery including maintenance of LCI during MC &amp; commissioning;
   - Procedure for handling of "mark-ups" from construction and MC &amp; commissioning.

Describe work process for continuous transfer of LCI covering:
 - Project revisions of documents and drawings;
 - Tag information (including tag-doc references);
 - Continuous updates of 3D CAD information according to Company’s requirements;
 - Before issuing safety critical documents and single line diagram in IFC revision, tag information (in Company’s LCI systems) for tags shown on document/drawing shall as a minimum include tag no, description, area, discipline, system and PO references, cross references tag/tag, tag/doc relation.</rdfs:comment>
    <rdl:PCA_100006763>A document to describe the method and timeline to deliver the required LCI during project execution and final handover to operations,  in accordance with Client LCI requirments.</rdl:PCA_100006763>
    <rdfs:label>Contractor's LCI execution strategy</rdfs:label>
    <rdfs:subClassOf rdf:resource="http://rds.posccaesar.org/ontology/plm/rdl/PCA_100004908"/>
    <rdl:PCA_100006768>LCI strategy shall as a minimum include the following:
 - Contractor’s Life Cycle information management organization;
 - An overall strategy for interaction between internal parties, such as procurement and engineering.;
 - An overall integration strategy of life cycle information from all parties involved such as external contractors, subcontractors and suppliers;
 - Contractor shall describe their systems portfolio related to the production and administration of LCI including integration capabilities with the Company systems;
 - Training strategy of staff in both Company’s and Contractor's LCI tools;
 - LCI Handover strategy from MC to Commissioning;
 - Strategy for Material control and SPIR handling;
 - Contractor's method for LCI quality control and systematic correction of quality issues;
 - Contractor's method for ensuring delivery of 3D CAD design models throughout the project in compliance with Company’s requirements;
 - LCI procedures (including):
   - Procedure for collection, storage, processing, transfer and sharing of LCI;
   - The procedure for standard documentation handling;
   - Work procedures for 3D handling as described in Company’s requirements;
   - The procedure shall include transfer methods, information logistics, systems involved, responsibilities, milestones, quality control, error reporting and rectification;
   - The procedure for tag scoping for supplier packages;
   - The procedure for tag scoping for engineering;
   - List containing Contractors planned deliveries of LCI according to Company's requirements;
   - Time schedules showing LCI deliveries including 3D;
   - Procedures or method to ensure special attention to identify early access and QC milestones. The schedules shall reflect the project execution plan and time schedules;
   - Procedure for LCI progress reporting according to LCI time schedules;
   - Procedures and checklists to ensure quality and completeness of the LCI delivery including maintenance of LCI during MC &amp; commissioning;
   - Procedure for handling of "mark-ups" from construction and MC &amp; commissioning.

Describe work process for continuous transfer of LCI covering:
 - Project revisions of documents and drawings;
 - Tag information (including tag-doc references);
 - Continuous updates of 3D CAD information according to Company’s requirements;
 - Before issuing safety critical documents and single line diagram in IFC revision, tag information (in Company’s LCI systems) for tags shown on document/drawing shall as a minimum include tag no, description, area, discipline, system and PO references, cross references tag/tag, tag/doc relation.</rdl:PCA_100006768>
    <rdl:PCA_100006766 rdf:resource="http://rds.posccaesar.org/ontology/plm/rdl/PCA_100006654"/>
    <skos:broadMatch rdf:resource="http://rds.posccaesar.org/ontology/plm/rdl/PCA_100006667"/>
    <skos:broadMatch>
      <rdl:PCA_100001503 rdf:about="http://rds.posccaesar.org/ontology/plm/rdl/PCA_100006666">
        <rdfs:label>project control information</rdfs:label>
        <rdl:PCA_100004924>BD</rdl:PCA_100004924>
        <rdf:type rdf:resource="http://www.w3.org/2002/07/owl#NamedIndividual"/>
      </rdl:PCA_100001503>
    </skos:broadMatch>
    <skos:broader rdf:resource="http://rds.posccaesar.org/ontology/plm/rdl/PCA_100006759"/>
    <rdl:PCA_100006765 rdf:resource="http://w3id.org/readi/rdl/CFIHOS-20000001"/>
  </owl:Class>
  <owl:Class rdf:about="http://rds.posccaesar.org/ontology/plm/rdl/PCA_100006147">
    <skos:broader rdf:resource="http://rds.posccaesar.org/ontology/plm/rdl/PCA_100006747"/>
    <skos:broadMatch rdf:resource="http://rds.posccaesar.org/ontology/plm/rdl/PCA_100006686"/>
    <rdfs:label>Data sheets - Well completion equipment</rdfs:label>
    <rdfs:comment>The equipment supplier standard datasheet shall be delivered. · The datasheet shall as a minimum contain the information specified in the applicable datasheet template · Plant specific information (e.g. P.O. number, tag number, P&amp;ID, etc.) is not required · The data sheet shall only describe one equipment type and shall be identified by one document number</rdfs:comment>
    <rdl:PCA_100006768>The equipment supplier standard datasheet shall be delivered. · The datasheet shall as a minimum contain the information specified in the applicable datasheet template · Plant specific information (e.g. P.O. number, tag number, P&amp;ID, etc.) is not required · The data sheet shall only describe one equipment type and shall be identified by one document number</rdl:PCA_100006768>
    <rdl:PCA_100006765 rdf:resource="http://w3id.org/readi/rdl/CFIHOS-20000042"/>
    <rdfs:subClassOf rdf:resource="http://rds.posccaesar.org/ontology/plm/rdl/PCA_100004908"/>
  </owl:Class>
  <owl:Class rdf:about="http://rds.posccaesar.org/ontology/plm/rdl/PCA_100006159">
    <skos:broadMatch rdf:resource="http://rds.posccaesar.org/ontology/plm/rdl/PCA_100006687"/>
    <rdfs:label>Design specification</rdfs:label>
    <skos:broader rdf:resource="http://rds.posccaesar.org/ontology/plm/rdl/PCA_100006757"/>
    <rdl:PCA_100006768>Specification for design requirements used for equipment and components.</rdl:PCA_100006768>
    <rdfs:subClassOf rdf:resource="http://rds.posccaesar.org/ontology/plm/rdl/PCA_100004908"/>
    <rdl:PCA_100006763>Give instructions concerning design requirements.</rdl:PCA_100006763>
    <rdl:PCA_100006765 rdf:resource="http://w3id.org/readi/rdl/CFIHOS-20000031"/>
    <rdl:PCA_100006766 rdf:resource="http://rds.posccaesar.org/ontology/plm/rdl/PCA_100006653"/>
    <rdfs:comment>Specification for design requirements used for equipment and components.</rdfs:comment>
  </owl:Class>
  <owl:Class rdf:about="http://rds.posccaesar.org/ontology/plm/rdl/PCA_100006288">
    <skos:broader rdf:resource="http://rds.posccaesar.org/ontology/plm/rdl/PCA_100006746"/>
    <skos:broadMatch rdf:resource="http://rds.posccaesar.org/ontology/plm/rdl/PCA_100006732"/>
    <rdfs:label>Insulating joints drawing</rdfs:label>
    <rdfs:comment>Drawings of insulating joints shall cover materials, geometry, dimensions, tolerances, weld bevel, internal and external coating, weld-in direction, spark gap attachment details and connection points, cables and cable connections.</rdfs:comment>
    <rdl:PCA_100006768>Drawings of insulating joints shall cover materials, geometry, dimensions, tolerances, weld bevel, internal and external coating, weld-in direction, spark gap attachment details and connection points, cables and cable connections.</rdl:PCA_100006768>
    <rdl:PCA_100006766 rdf:resource="http://rds.posccaesar.org/ontology/plm/rdl/PCA_100006653"/>
    <rdfs:subClassOf rdf:resource="http://rds.posccaesar.org/ontology/plm/rdl/PCA_100004908"/>
  </owl:Class>
  <owl:Class rdf:about="http://rds.posccaesar.org/ontology/plm/rdl/PCA_100006397">
    <rdl:PCA_100006766 rdf:resource="http://rds.posccaesar.org/ontology/plm/rdl/PCA_100006589"/>
    <rdl:PCA_100006766 rdf:resource="http://rds.posccaesar.org/ontology/plm/rdl/PCA_100006607"/>
    <rdl:PCA_100006765 rdf:resource="http://w3id.org/readi/rdl/CFIHOS-20000026"/>
    <rdl:PCA_100006766 rdf:resource="http://rds.posccaesar.org/ontology/plm/rdl/PCA_100006592"/>
    <rdl:PCA_100006766 rdf:resource="http://rds.posccaesar.org/ontology/plm/rdl/PCA_100006579"/>
    <rdl:PCA_100006766 rdf:resource="http://rds.posccaesar.org/ontology/plm/rdl/PCA_100006600"/>
    <rdl:PCA_100006766 rdf:resource="http://rds.posccaesar.org/ontology/plm/rdl/PCA_100006595"/>
    <rdl:PCA_100006766 rdf:resource="http://rds.posccaesar.org/ontology/plm/rdl/PCA_100006582"/>
    <rdl:PCA_100006766 rdf:resource="http://rds.posccaesar.org/ontology/plm/rdl/PCA_100006623"/>
    <rdl:PCA_100006766 rdf:resource="http://rds.posccaesar.org/ontology/plm/rdl/PCA_100006613"/>
    <rdl:PCA_100006766 rdf:resource="http://rds.posccaesar.org/ontology/plm/rdl/PCA_100006610"/>
    <rdfs:label>Process simulation reports</rdfs:label>
    <rdl:PCA_100006766 rdf:resource="http://rds.posccaesar.org/ontology/plm/rdl/PCA_100006588"/>
    <rdl:PCA_100006766 rdf:resource="http://rds.posccaesar.org/ontology/plm/rdl/PCA_100006606"/>
    <rdl:PCA_100006766 rdf:resource="http://rds.posccaesar.org/ontology/plm/rdl/PCA_100006585"/>
    <rdl:PCA_100006766 rdf:resource="http://rds.posccaesar.org/ontology/plm/rdl/PCA_100006616"/>
    <rdl:PCA_100006766 rdf:resource="http://rds.posccaesar.org/ontology/plm/rdl/PCA_100006603"/>
    <rdl:PCA_100006766 rdf:resource="http://rds.posccaesar.org/ontology/plm/rdl/PCA_100006609"/>
    <rdl:PCA_100006766 rdf:resource="http://rds.posccaesar.org/ontology/plm/rdl/PCA_100006598"/>
    <rdl:PCA_100006766 rdf:resource="http://rds.posccaesar.org/ontology/plm/rdl/PCA_100006591"/>
    <rdl:PCA_100006766 rdf:resource="http://rds.posccaesar.org/ontology/plm/rdl/PCA_100006619"/>
    <rdl:PCA_100006766 rdf:resource="http://rds.posccaesar.org/ontology/plm/rdl/PCA_100006584"/>
    <rdl:PCA_100006766 rdf:resource="http://rds.posccaesar.org/ontology/plm/rdl/PCA_100006581"/>
    <rdl:PCA_100006766 rdf:resource="http://rds.posccaesar.org/ontology/plm/rdl/PCA_100006625"/>
    <rdl:PCA_100006766 rdf:resource="http://rds.posccaesar.org/ontology/plm/rdl/PCA_100006622"/>
    <rdl:PCA_100006766 rdf:resource="http://rds.posccaesar.org/ontology/plm/rdl/PCA_100006578"/>
    <rdl:PCA_100006766 rdf:resource="http://rds.posccaesar.org/ontology/plm/rdl/PCA_100006612"/>
    <skos:broadMatch rdf:resource="http://rds.posccaesar.org/ontology/plm/rdl/PCA_100006698"/>
    <rdl:PCA_100006766 rdf:resource="http://rds.posccaesar.org/ontology/plm/rdl/PCA_100006587"/>
    <rdl:PCA_100006766 rdf:resource="http://rds.posccaesar.org/ontology/plm/rdl/PCA_100006594"/>
    <rdl:PCA_100006766 rdf:resource="http://rds.posccaesar.org/ontology/plm/rdl/PCA_100006605"/>
    <rdl:PCA_100006766 rdf:resource="http://rds.posccaesar.org/ontology/plm/rdl/PCA_100006602"/>
    <rdl:PCA_100006766 rdf:resource="http://rds.posccaesar.org/ontology/plm/rdl/PCA_100006618"/>
    <rdl:PCA_100006766 rdf:resource="http://rds.posccaesar.org/ontology/plm/rdl/PCA_100006597"/>
    <rdl:PCA_100006766 rdf:resource="http://rds.posccaesar.org/ontology/plm/rdl/PCA_100006580"/>
    <rdl:PCA_100006766 rdf:resource="http://rds.posccaesar.org/ontology/plm/rdl/PCA_100006621"/>
    <rdfs:subClassOf rdf:resource="http://rds.posccaesar.org/ontology/plm/rdl/PCA_100004908"/>
    <rdl:PCA_100006766 rdf:resource="http://rds.posccaesar.org/ontology/plm/rdl/PCA_100006615"/>
    <rdl:PCA_100006763>Documentation of the process simulations defining the heat and material balances as basis for design of the plant shall consist of the following two parts:
1. Executable process simulation files;
2. The process simulation report.

All process design cases, i.e. all cases where stream data are used for equipment and line/valve sizing, shall be documented by 1. and 2. above.</rdl:PCA_100006763>
    <rdl:PCA_100006766 rdf:resource="http://rds.posccaesar.org/ontology/plm/rdl/PCA_100006608"/>
    <rdl:PCA_100006766 rdf:resource="http://rds.posccaesar.org/ontology/plm/rdl/PCA_100006583"/>
    <rdl:PCA_100006766 rdf:resource="http://rds.posccaesar.org/ontology/plm/rdl/PCA_100006590"/>
    <rdl:PCA_100006766 rdf:resource="http://rds.posccaesar.org/ontology/plm/rdl/PCA_100006624"/>
    <skos:broader rdf:resource="http://rds.posccaesar.org/ontology/plm/rdl/PCA_100006756"/>
    <rdfs:comment>The process simulation report shall as a minimum include:
 - Feed stream descriptions, including the development over the production lifetime;
 - Product specifications;
 - A reasoning for the defined process design cases, e.g.:
    - Which production situation is represented by each case, and how do the cases together represent the expected operation envelope;
    - If applicable, which variations are included in the feed stream descriptions to accommodate uncertainties in the feed stream properties and conditions;
 - A description of the calculation models used in the process simulation;
 - Specifications for each unit operation in the process simulations;
 - Summary tables with resulting stream and equipment data. The stream numbers shall coincide with the stream numbers on the PFD's.</rdfs:comment>
    <rdl:PCA_100006766 rdf:resource="http://rds.posccaesar.org/ontology/plm/rdl/PCA_100006601"/>
    <rdl:PCA_100006766 rdf:resource="http://rds.posccaesar.org/ontology/plm/rdl/PCA_100006596"/>
    <rdl:PCA_100006766 rdf:resource="http://rds.posccaesar.org/ontology/plm/rdl/PCA_100006593"/>
    <rdl:PCA_100006766 rdf:resource="http://rds.posccaesar.org/ontology/plm/rdl/PCA_100006604"/>
    <rdl:PCA_100006766 rdf:resource="http://rds.posccaesar.org/ontology/plm/rdl/PCA_100006611"/>
    <rdl:PCA_100006766 rdf:resource="http://rds.posccaesar.org/ontology/plm/rdl/PCA_100006599"/>
    <rdl:PCA_100006766 rdf:resource="http://rds.posccaesar.org/ontology/plm/rdl/PCA_100006617"/>
    <rdl:PCA_100006766 rdf:resource="http://rds.posccaesar.org/ontology/plm/rdl/PCA_100006586"/>
    <rdl:PCA_100006768>The process simulation report shall as a minimum include:
 - Feed stream descriptions, including the development over the production lifetime;
 - Product specifications;
 - A reasoning for the defined process design cases, e.g.:
    - Which production situation is represented by each case, and how do the cases together represent the expected operation envelope;
    - If applicable, which variations are included in the feed stream descriptions to accommodate uncertainties in the feed stream properties and conditions;
 - A description of the calculation models used in the process simulation;
 - Specifications for each unit operation in the process simulations;
 - Summary tables with resulting stream and equipment data. The stream numbers shall coincide with the stream numbers on the PFD's.</rdl:PCA_100006768>
    <rdl:PCA_100006766 rdf:resource="http://rds.posccaesar.org/ontology/plm/rdl/PCA_100006620"/>
    <rdl:PCA_100006766 rdf:resource="http://rds.posccaesar.org/ontology/plm/rdl/PCA_100006614"/>
  </owl:Class>
  <owl:Class rdf:about="http://rds.posccaesar.org/ontology/plm/rdl/PCA_100006276">
    <skos:broader rdf:resource="http://rds.posccaesar.org/ontology/plm/rdl/PCA_100006756"/>
    <skos:broadMatch rdf:resource="http://rds.posccaesar.org/ontology/plm/rdl/PCA_100006686"/>
    <rdfs:label>Installation design report</rdfs:label>
    <rdl:PCA_100006766 rdf:resource="http://rds.posccaesar.org/ontology/plm/rdl/PCA_100006654"/>
    <rdl:PCA_100006765 rdf:resource="http://w3id.org/readi/rdl/CFIHOS-20000018"/>
    <rdl:PCA_100006763>Design report covering pipeline installation. Basis for analysis, assumptions and assessments not given in design basis shall be included.</rdl:PCA_100006763>
    <rdfs:subClassOf rdf:resource="http://rds.posccaesar.org/ontology/plm/rdl/PCA_100004908"/>
  </owl:Class>
  <owl:Class rdf:about="http://rds.posccaesar.org/ontology/plm/rdl/PCA_100006385">
    <skos:broader rdf:resource="http://rds.posccaesar.org/ontology/plm/rdl/PCA_100006751"/>
    <skos:broadMatch rdf:resource="http://rds.posccaesar.org/ontology/plm/rdl/PCA_100006722"/>
    <rdfs:label>Positive material identification (PMI) procedure</rdfs:label>
    <rdfs:comment>Provide instructions to the PMI operator.</rdfs:comment>
    <rdl:PCA_100006768>Provide instructions to the PMI operator.</rdl:PCA_100006768>
    <rdl:PCA_100006766 rdf:resource="http://rds.posccaesar.org/ontology/plm/rdl/PCA_100006653"/>
    <rdl:PCA_100006763>Procedure describing the method for material identification by elemental analysis.</rdl:PCA_100006763>
    <rdfs:subClassOf rdf:resource="http://rds.posccaesar.org/ontology/plm/rdl/PCA_100004908"/>
  </owl:Class>
  <owl:Class rdf:about="http://rds.posccaesar.org/ontology/plm/rdl/PCA_100006264">
    <skos:broader rdf:resource="http://rds.posccaesar.org/ontology/plm/rdl/PCA_100006741"/>
    <rdfs:subClassOf rdf:resource="http://rds.posccaesar.org/ontology/plm/rdl/PCA_100004908"/>
    <rdfs:comment>The results from the hydraulic response analysis including sizing of hydraulic and chemical lines, subsea compensation, valve signatures as spring forces and volumes to verify for the system performance.</rdfs:comment>
    <rdfs:label>Hydraulic system calculation analysis</rdfs:label>
    <rdl:PCA_100006768>The results from the hydraulic response analysis including sizing of hydraulic and chemical lines, subsea compensation, valve signatures as spring forces and volumes to verify for the system performance.</rdl:PCA_100006768>
    <skos:broadMatch rdf:resource="http://rds.posccaesar.org/ontology/plm/rdl/PCA_100006687"/>
    <rdl:PCA_100006765 rdf:resource="http://w3id.org/readi/rdl/CFIHOS-20000031"/>
    <rdl:PCA_100006763>Document that the hydraulic system has been adequately designed and sized in accordance with shut down and operational requirements as per design basis.</rdl:PCA_100006763>
    <rdl:PCA_100006766 rdf:resource="http://rds.posccaesar.org/ontology/plm/rdl/PCA_100006657"/>
  </owl:Class>
  <owl:Class rdf:about="http://rds.posccaesar.org/ontology/plm/rdl/PCA_100006373">
    <skos:broader rdf:resource="http://rds.posccaesar.org/ontology/plm/rdl/PCA_100006741"/>
    <skos:broadMatch rdf:resource="http://rds.posccaesar.org/ontology/plm/rdl/PCA_100006687"/>
    <rdfs:label>Piping component calculations</rdfs:label>
    <rdfs:comment>The document shall include drawings and strength calculations of piping components, typical: weldolets, nipoflanges etc.</rdfs:comment>
    <rdl:PCA_100006768>The document shall include drawings and strength calculations of piping components, typical: weldolets, nipoflanges etc.</rdl:PCA_100006768>
    <rdl:PCA_100006766 rdf:resource="http://rds.posccaesar.org/ontology/plm/rdl/PCA_100006653"/>
    <rdl:PCA_100006765 rdf:resource="http://w3id.org/readi/rdl/CFIHOS-20000020"/>
    <rdfs:subClassOf rdf:resource="http://rds.posccaesar.org/ontology/plm/rdl/PCA_100004908"/>
  </owl:Class>
  <owl:Class rdf:about="http://rds.posccaesar.org/ontology/plm/rdl/PCA_100006252">
    <rdl:PCA_100006768>Schematic drawing showing mechanical and connection interfaces on equipment.</rdl:PCA_100006768>
    <rdfs:comment>Schematic drawing showing mechanical and connection interfaces on equipment.</rdfs:comment>
    <rdl:PCA_100006766 rdf:resource="http://rds.posccaesar.org/ontology/plm/rdl/PCA_100006653"/>
    <skos:broader rdf:resource="http://rds.posccaesar.org/ontology/plm/rdl/PCA_100006746"/>
    <skos:broadMatch rdf:resource="http://rds.posccaesar.org/ontology/plm/rdl/PCA_100006708"/>
    <rdfs:label>Hook-up /installation drawing</rdfs:label>
    <rdl:PCA_100006765 rdf:resource="http://w3id.org/readi/rdl/CFIHOS-20000031"/>
    <rdl:PCA_100006763>A drawing providing necessary information for an installation contractor to perform lifting and installation.</rdl:PCA_100006763>
    <rdfs:subClassOf rdf:resource="http://rds.posccaesar.org/ontology/plm/rdl/PCA_100004908"/>
  </owl:Class>
  <owl:Class rdf:about="http://rds.posccaesar.org/ontology/plm/rdl/PCA_100006240">
    <rdfs:subClassOf rdf:resource="http://rds.posccaesar.org/ontology/plm/rdl/PCA_100004908"/>
    <rdfs:comment>These drawings shall contain the following information:
 - Dimensions
 - Location and identification of piping and main components
 - Necessary space for disassembly and maintenance
 - Location of centre of gravity
 - Possible thermal expansion.
 - On the structural steel drawings, critical welds shall be included with a weld identification number serving as a cross-reference to the weld summary index
 - Obstacles from other disciplines shall be included when relevant
 - Total weight, wet and dry and in operational condition
 - Weights, centre of gravity and main dimensions of disassembled units/components over 25 kg. Lifting lugs and runway beam for disassembling and their location shall be shown
 - Identification and location of all external pipeline connections as well as requirements for flexible connections and acceptable loads and moments. Locations shall be dimensioned, and tolerances shown, if necessary, in separate drawings
 - Identification and location of all external electrical and control monitoring connections (may be given in separate drawings describing the electrical arrangement and instrumentation)
 - For pressure equipment: For projects within the EU, Category and Module shall be according to PED (Pressure equipment directive)
 - Include bolt tension requirements for pressure equipment flanges
 - identification of lubrication points

Foundation information (such as support frame, support structure) shall include:
 - The outer dimensions and footprint of the support frame or foundation supports
 - The size, grade and location of the foundation bolts and torque where this is necessary
 - Forces and moments transferred to load bearing structures, both under normal operation and extreme conditions
 - Details for adjustment and alignment
 - Details for cut-outs inside outer limit of foundation
 - Details for vibration dampening units (if installed)</rdfs:comment>
    <skos:broadMatch rdf:resource="http://rds.posccaesar.org/ontology/plm/rdl/PCA_100006707"/>
    <skos:broader rdf:resource="http://rds.posccaesar.org/ontology/plm/rdl/PCA_100006739"/>
    <rdl:PCA_100006765 rdf:resource="http://w3id.org/readi/rdl/CFIHOS-20000018"/>
    <rdl:PCA_100006768>These drawings shall contain the following information:
 - Dimensions
 - Location and identification of piping and main components
 - Necessary space for disassembly and maintenance
 - Location of centre of gravity
 - Possible thermal expansion.
 - On the structural steel drawings, critical welds shall be included with a weld identification number serving as a cross-reference to the weld summary index
 - Obstacles from other disciplines shall be included when relevant
 - Total weight, wet and dry and in operational condition
 - Weights, centre of gravity and main dimensions of disassembled units/components over 25 kg. Lifting lugs and runway beam for disassembling and their location shall be shown
 - Identification and location of all external pipeline connections as well as requirements for flexible connections and acceptable loads and moments. Locations shall be dimensioned, and tolerances shown, if necessary, in separate drawings
 - Identification and location of all external electrical and control monitoring connections (may be given in separate drawings describing the electrical arrangement and instrumentation)
 - For pressure equipment: For projects within the EU, Category and Module shall be according to PED (Pressure equipment directive)
 - Include bolt tension requirements for pressure equipment flanges
 - identification of lubrication points

Foundation information (such as support frame, support structure) shall include:
 - The outer dimensions and footprint of the support frame or foundation supports
 - The size, grade and location of the foundation bolts and torque where this is necessary
 - Forces and moments transferred to load bearing structures, both under normal operation and extreme conditions
 - Details for adjustment and alignment
 - Details for cut-outs inside outer limit of foundation
 - Details for vibration dampening units (if installed)</rdl:PCA_100006768>
    <rdl:PCA_100006763>General arrangement drawings for pipeline structures such as riser bases, pipeline protection structures, tee/wye assemblies, anchor blocks, valve stations, pump stations, pig traps etc.</rdl:PCA_100006763>
    <rdfs:label>General arrangement drawings - Pipeline structures</rdfs:label>
    <rdl:PCA_100006766 rdf:resource="http://rds.posccaesar.org/ontology/plm/rdl/PCA_100006653"/>
  </owl:Class>
  <owl:Class rdf:about="http://rds.posccaesar.org/ontology/plm/rdl/PCA_100006482">
    <rdl:PCA_100006766 rdf:resource="http://rds.posccaesar.org/ontology/plm/rdl/PCA_100006612"/>
    <rdfs:comment>Typical contents of a detailed topology diagram shall be:
 - All related functional units and subunits represented by blocks including unit tag no and description;
 - Location of units;
 - Interface and network between units shall be indicated;
 - Interface from units to other external systems;
 - Protocol shall be indicated for serial links and for network connections to external system.

By units is meant but not limited to:
 - Logic solver;
 - Server;
 - Client;
 - Network component (Router, Switch, Firewall);
 - Remote IO.</rdfs:comment>
    <rdl:PCA_100006766 rdf:resource="http://rds.posccaesar.org/ontology/plm/rdl/PCA_100006608"/>
    <rdl:PCA_100006766 rdf:resource="http://rds.posccaesar.org/ontology/plm/rdl/PCA_100006595"/>
    <rdl:PCA_100006766 rdf:resource="http://rds.posccaesar.org/ontology/plm/rdl/PCA_100006636"/>
    <skos:broadMatch rdf:resource="http://rds.posccaesar.org/ontology/plm/rdl/PCA_100006695"/>
    <rdl:PCA_100006766 rdf:resource="http://rds.posccaesar.org/ontology/plm/rdl/PCA_100006613"/>
    <rdl:PCA_100006766 rdf:resource="http://rds.posccaesar.org/ontology/plm/rdl/PCA_100006596"/>
    <rdl:PCA_100006766 rdf:resource="http://rds.posccaesar.org/ontology/plm/rdl/PCA_100006637"/>
    <rdl:PCA_100006766 rdf:resource="http://rds.posccaesar.org/ontology/plm/rdl/PCA_100006622"/>
    <rdl:PCA_100006766 rdf:resource="http://rds.posccaesar.org/ontology/plm/rdl/PCA_100006618"/>
    <rdl:PCA_100006766 rdf:resource="http://rds.posccaesar.org/ontology/plm/rdl/PCA_100006604"/>
    <rdl:PCA_100006766 rdf:resource="http://rds.posccaesar.org/ontology/plm/rdl/PCA_100006603"/>
    <rdl:PCA_100006766 rdf:resource="http://rds.posccaesar.org/ontology/plm/rdl/PCA_100006628"/>
    <rdl:PCA_100006766 rdf:resource="http://rds.posccaesar.org/ontology/plm/rdl/PCA_100006627"/>
    <rdfs:subClassOf rdf:resource="http://rds.posccaesar.org/ontology/plm/rdl/PCA_100004908"/>
    <rdl:PCA_100006766 rdf:resource="http://rds.posccaesar.org/ontology/plm/rdl/PCA_100006609"/>
    <rdl:PCA_100006766 rdf:resource="http://rds.posccaesar.org/ontology/plm/rdl/PCA_100006619"/>
    <rdl:PCA_100006766 rdf:resource="http://rds.posccaesar.org/ontology/plm/rdl/PCA_100006633"/>
    <rdl:PCA_100006766 rdf:resource="http://rds.posccaesar.org/ontology/plm/rdl/PCA_100006641"/>
    <rdl:PCA_100006766 rdf:resource="http://rds.posccaesar.org/ontology/plm/rdl/PCA_100006600"/>
    <rdl:PCA_100006766 rdf:resource="http://rds.posccaesar.org/ontology/plm/rdl/PCA_100006624"/>
    <rdl:PCA_100006766 rdf:resource="http://rds.posccaesar.org/ontology/plm/rdl/PCA_100006623"/>
    <rdl:PCA_100006766 rdf:resource="http://rds.posccaesar.org/ontology/plm/rdl/PCA_100006614"/>
    <rdl:PCA_100006766 rdf:resource="http://rds.posccaesar.org/ontology/plm/rdl/PCA_100006597"/>
    <rdl:PCA_100006766 rdf:resource="http://rds.posccaesar.org/ontology/plm/rdl/PCA_100006639"/>
    <rdl:PCA_100006766 rdf:resource="http://rds.posccaesar.org/ontology/plm/rdl/PCA_100006606"/>
    <rdl:PCA_100006766 rdf:resource="http://rds.posccaesar.org/ontology/plm/rdl/PCA_100006638"/>
    <rdl:PCA_100006766 rdf:resource="http://rds.posccaesar.org/ontology/plm/rdl/PCA_100006605"/>
    <rdl:PCA_100006766 rdf:resource="http://rds.posccaesar.org/ontology/plm/rdl/PCA_100006615"/>
    <rdl:PCA_100006766 rdf:resource="http://rds.posccaesar.org/ontology/plm/rdl/PCA_100006598"/>
    <rdl:PCA_100006766 rdf:resource="http://rds.posccaesar.org/ontology/plm/rdl/PCA_100006620"/>
    <rdl:PCA_100006768>Typical contents of a detailed topology diagram shall be:
 - All related functional units and subunits represented by blocks including unit tag no and description;
 - Location of units;
 - Interface and network between units shall be indicated;
 - Interface from units to other external systems;
 - Protocol shall be indicated for serial links and for network connections to external system.

By units is meant but not limited to:
 - Logic solver;
 - Server;
 - Client;
 - Network component (Router, Switch, Firewall);
 - Remote IO.</rdl:PCA_100006768>
    <rdl:PCA_100006766 rdf:resource="http://rds.posccaesar.org/ontology/plm/rdl/PCA_100006610"/>
    <skos:broader rdf:resource="http://rds.posccaesar.org/ontology/plm/rdl/PCA_100006745"/>
    <rdl:PCA_100006766 rdf:resource="http://rds.posccaesar.org/ontology/plm/rdl/PCA_100006634"/>
    <rdl:PCA_100006766 rdf:resource="http://rds.posccaesar.org/ontology/plm/rdl/PCA_100006601"/>
    <rdl:PCA_100006766 rdf:resource="http://rds.posccaesar.org/ontology/plm/rdl/PCA_100006611"/>
    <rdl:PCA_100006766 rdf:resource="http://rds.posccaesar.org/ontology/plm/rdl/PCA_100006594"/>
    <rdl:PCA_100006766 rdf:resource="http://rds.posccaesar.org/ontology/plm/rdl/PCA_100006635"/>
    <rdl:PCA_100006766 rdf:resource="http://rds.posccaesar.org/ontology/plm/rdl/PCA_100006625"/>
    <rdl:PCA_100006766 rdf:resource="http://rds.posccaesar.org/ontology/plm/rdl/PCA_100006617"/>
    <rdl:PCA_100006766 rdf:resource="http://rds.posccaesar.org/ontology/plm/rdl/PCA_100006616"/>
    <rdl:PCA_100006765 rdf:resource="http://w3id.org/readi/rdl/CFIHOS-20000015"/>
    <rdl:PCA_100006766 rdf:resource="http://rds.posccaesar.org/ontology/plm/rdl/PCA_100006599"/>
    <rdl:PCA_100006766 rdf:resource="http://rds.posccaesar.org/ontology/plm/rdl/PCA_100006602"/>
    <rdl:PCA_100006766 rdf:resource="http://rds.posccaesar.org/ontology/plm/rdl/PCA_100006626"/>
    <rdfs:label>System topology diagrams</rdfs:label>
    <rdl:PCA_100006763>System topology diagram shall show the structure of systems and subsystems to give a functional understanding.

System topology diagram shall as a minimum be produced for the following systems:
 - Safety and Automation System;
 - Turbine control system;
 - Fiscal metering system;
 - Drilling system;
 - Subsea system.

If it is not possible to present all detailed information in a system on one topology drawing, the information shall be split in different detail levels as follows:
 - Overall topology diagram;
 - Detailed topology diagram.</rdl:PCA_100006763>
    <rdl:PCA_100006766 rdf:resource="http://rds.posccaesar.org/ontology/plm/rdl/PCA_100006607"/>
    <rdl:PCA_100006766 rdf:resource="http://rds.posccaesar.org/ontology/plm/rdl/PCA_100006621"/>
    <rdl:PCA_100006766 rdf:resource="http://rds.posccaesar.org/ontology/plm/rdl/PCA_100006631"/>
  </owl:Class>
  <owl:Class rdf:about="http://rds.posccaesar.org/ontology/plm/rdl/PCA_100006361">
    <skos:broadMatch rdf:resource="http://rds.posccaesar.org/ontology/plm/rdl/PCA_100006717"/>
    <rdfs:subClassOf rdf:resource="http://rds.posccaesar.org/ontology/plm/rdl/PCA_100004908"/>
    <rdl:PCA_100006765 rdf:resource="http://w3id.org/readi/rdl/CFIHOS-20000018"/>
    <skos:broader rdf:resource="http://rds.posccaesar.org/ontology/plm/rdl/PCA_100006748"/>
    <rdfs:comment>Piggable Item List / Bore Map Overview document listing all bore sizes to confirm piggability througout each line

(Template in TR is unavailable to S7 and has not been used)</rdfs:comment>
    <rdl:PCA_100006763>Pigability data describes relevant data and drawings for the complete pipeline system, from pigtrap to pigtrap that should be checked out prior to a pigging operation in order to ensure that the pipeline system is in a condition such that it can be pigged, and that the necessary equipment is correctly configured and will work as intended during the pigging operation. Furthermore, the purpose is to ensure that the work carried out is documented.</rdl:PCA_100006763>
    <rdl:PCA_100006766 rdf:resource="http://rds.posccaesar.org/ontology/plm/rdl/PCA_100006654"/>
    <rdfs:label>Pigability data</rdfs:label>
    <rdl:PCA_100006768>Piggable Item List / Bore Map Overview document listing all bore sizes to confirm piggability througout each line

(Template in TR is unavailable to S7 and has not been used)</rdl:PCA_100006768>
    <skos:broader rdf:resource="http://rds.posccaesar.org/ontology/plm/rdl/PCA_100006762"/>
  </owl:Class>
  <owl:Class rdf:about="http://rds.posccaesar.org/ontology/plm/rdl/PCA_100006494">
    <skos:broader rdf:resource="http://rds.posccaesar.org/ontology/plm/rdl/PCA_100006745"/>
    <skos:broadMatch rdf:resource="http://rds.posccaesar.org/ontology/plm/rdl/PCA_100006700"/>
    <rdfs:label>Telecommunication signal level diagram</rdfs:label>
    <rdfs:comment>Signal level diagrams shall be made for:
 - The feeder arrangement of all radio systems including transceivers ports and antennas;
 - Audio and video entertainment distribution network (coaxial cable);
 - Interconnection signal lines between subsystems and to other systems;
 - External lines where signal level is not set by standard.

Levels shall be given in dBm in conjunction with standardised impedances. If impedance is non-standard or undefined, voltage levels shall be given.

Where applicable, impedances and wire configuration should be indicated. (2-wire, 4-wire, coax, E&amp;M lines, etc.).</rdfs:comment>
    <rdl:PCA_100006768>Signal level diagrams shall be made for:
 - The feeder arrangement of all radio systems including transceivers ports and antennas;
 - Audio and video entertainment distribution network (coaxial cable);
 - Interconnection signal lines between subsystems and to other systems;
 - External lines where signal level is not set by standard.

Levels shall be given in dBm in conjunction with standardised impedances. If impedance is non-standard or undefined, voltage levels shall be given.

Where applicable, impedances and wire configuration should be indicated. (2-wire, 4-wire, coax, E&amp;M lines, etc.).</rdl:PCA_100006768>
    <rdl:PCA_100006766 rdf:resource="http://rds.posccaesar.org/ontology/plm/rdl/PCA_100006640"/>
    <rdl:PCA_100006765 rdf:resource="http://w3id.org/readi/rdl/CFIHOS-20000030"/>
    <rdfs:subClassOf rdf:resource="http://rds.posccaesar.org/ontology/plm/rdl/PCA_100004908"/>
  </owl:Class>
  <owl:Class rdf:about="http://rds.posccaesar.org/ontology/plm/rdl/PCA_100006470">
    <skos:broader rdf:resource="http://rds.posccaesar.org/ontology/plm/rdl/PCA_100006756"/>
    <rdfs:label>Study report</rdfs:label>
    <rdfs:comment>Study Report detailing the final results from the Study (e.g FEED Study Report)</rdfs:comment>
    <rdl:PCA_100006768>Study Report detailing the final results from the Study (e.g FEED Study Report)</rdl:PCA_100006768>
    <rdl:PCA_100006766 rdf:resource="http://rds.posccaesar.org/ontology/plm/rdl/PCA_100006654"/>
    <rdl:PCA_100006765 rdf:resource="http://w3id.org/readi/rdl/CFIHOS-20000018"/>
    <rdl:PCA_100006763>More details req. Study report for project specific conditions not covered by other design documentation, such as environmental studies, third party activity studies, influence on third party etc..</rdl:PCA_100006763>
    <rdfs:subClassOf rdf:resource="http://rds.posccaesar.org/ontology/plm/rdl/PCA_100004908"/>
  </owl:Class>
  <owl:Class rdf:about="http://rds.posccaesar.org/ontology/plm/rdl/PCA_100006110">
    <skos:broader rdf:resource="http://rds.posccaesar.org/ontology/plm/rdl/PCA_100006746"/>
    <skos:broadMatch rdf:resource="http://rds.posccaesar.org/ontology/plm/rdl/PCA_100006710"/>
    <rdfs:label>Buildings architectural drawings</rdfs:label>
    <rdfs:comment>Architectural layout drawings (plans, elevations) and cross sections and details of all architectural components shall be produced.

Drawings showing extent and details for thermal and acoustic insulation and fire protection shall be included. All penetrations including windows and doors shall be shown.

Location, direction and type of signpost shall be shown on architectural layout drawings.

The drawing scale for architectural layout drawings shall normally be 1:100 in A3 format. However different scales can be used on A1 format if readable when reduced to A3 format. The drawings shall include stairs, walls, doors, windows, furniture, access and escape routes and all tagged equipment.

Main dimensions shall be included. Elevations of all floors and platforms etc. shall be shown. A key plan, grid lines with north and east references and match lines with drawing references shall be included. Relevant civil, structural, HVAC, etc. drawings be referenced. The drawings shall have a title block which contains all the information necessary to identify the drawing and its purpose.</rdfs:comment>
    <rdl:PCA_100006768>Architectural layout drawings (plans, elevations) and cross sections and details of all architectural components shall be produced.

Drawings showing extent and details for thermal and acoustic insulation and fire protection shall be included. All penetrations including windows and doors shall be shown.

Location, direction and type of signpost shall be shown on architectural layout drawings.

The drawing scale for architectural layout drawings shall normally be 1:100 in A3 format. However different scales can be used on A1 format if readable when reduced to A3 format. The drawings shall include stairs, walls, doors, windows, furniture, access and escape routes and all tagged equipment.

Main dimensions shall be included. Elevations of all floors and platforms etc. shall be shown. A key plan, grid lines with north and east references and match lines with drawing references shall be included. Relevant civil, structural, HVAC, etc. drawings be referenced. The drawings shall have a title block which contains all the information necessary to identify the drawing and its purpose.</rdl:PCA_100006768>
    <rdl:PCA_100006766 rdf:resource="http://rds.posccaesar.org/ontology/plm/rdl/PCA_100006656"/>
    <rdl:PCA_100006765 rdf:resource="http://w3id.org/readi/rdl/CFIHOS-20000003"/>
    <rdfs:subClassOf rdf:resource="http://rds.posccaesar.org/ontology/plm/rdl/PCA_100004908"/>
  </owl:Class>
  <owl:Class rdf:about="http://rds.posccaesar.org/ontology/plm/rdl/PCA_100006122">
    <rdfs:subClassOf rdf:resource="http://rds.posccaesar.org/ontology/plm/rdl/PCA_100004908"/>
    <skos:broader rdf:resource="http://rds.posccaesar.org/ontology/plm/rdl/PCA_100006751"/>
    <rdl:PCA_100006764>Requirements related to assurance and check of quality in manufacturing phase will very much depend on Purchaser’s knowledge of supplier. Well known supplier, with proven track record, delivering products based on industry standards, will typically deliver less verification documentation to Purchaser than unknown/new supplier delivering the same product. Therefore, this deliverable should be evaluated as candidate for being available in digital format to Purchaser, for information only.</rdl:PCA_100006764>
    <rdl:PCA_100006765 rdf:resource="http://w3id.org/readi/rdl/CFIHOS-20000028"/>
    <rdfs:comment>This document details the work process and how the defined requirements to surface treatment, application and quality control shall be met. 

A procedure may cover wet paint, powder coating, or metallic coatings. The document shall include reference to applied standards and the information about revision of the applied standard.</rdfs:comment>
    <rdl:PCA_100006763>Verification of suppliers compliance with surface protection and coating requirements.

(This document provides a procedure for coating operator to ensure repeatability and formalism and hence prove the quality of the coating work.)</rdl:PCA_100006763>
    <rdl:PCA_100006766 rdf:resource="http://rds.posccaesar.org/ontology/plm/rdl/PCA_100006653"/>
    <rdl:PCA_100006768>This document details the work process and how the defined requirements to surface treatment, application and quality control shall be met. 

A procedure may cover wet paint, powder coating, or metallic coatings. The document shall include reference to applied standards and the information about revision of the applied standard.</rdl:PCA_100006768>
    <rdfs:label>Coating procedure</rdfs:label>
    <skos:broadMatch rdf:resource="http://rds.posccaesar.org/ontology/plm/rdl/PCA_100006722"/>
  </owl:Class>
  <owl:Class rdf:about="http://rds.posccaesar.org/ontology/plm/rdl/PCA_100006134">
    <rdl:PCA_100006763>A document stating the normal and maximum consumption of the equipment.</rdl:PCA_100006763>
    <rdfs:label>Consumption/utilities list</rdfs:label>
    <rdl:PCA_100006765 rdf:resource="http://w3id.org/readi/rdl/CFIHOS-20000031"/>
    <rdfs:subClassOf rdf:resource="http://rds.posccaesar.org/ontology/plm/rdl/PCA_100004908"/>
    <skos:broadMatch rdf:resource="http://rds.posccaesar.org/ontology/plm/rdl/PCA_100006716"/>
    <rdfs:comment>The document provides input for sizing relevant supplying sources such as e.g. electrical, air.</rdfs:comment>
    <skos:broader rdf:resource="http://rds.posccaesar.org/ontology/plm/rdl/PCA_100006748"/>
    <rdl:PCA_100006766 rdf:resource="http://rds.posccaesar.org/ontology/plm/rdl/PCA_100006653"/>
    <rdl:PCA_100006768>The document provides input for sizing relevant supplying sources such as e.g. electrical, air.</rdl:PCA_100006768>
  </owl:Class>
  <owl:Class rdf:about="http://rds.posccaesar.org/ontology/plm/rdl/PCA_100006146">
    <skos:broader rdf:resource="http://rds.posccaesar.org/ontology/plm/rdl/PCA_100006747"/>
    <skos:broadMatch rdf:resource="http://rds.posccaesar.org/ontology/plm/rdl/PCA_100006686"/>
    <rdfs:label>Data sheets - Hose</rdfs:label>
    <rdfs:comment>Hose data, including pressure, medium, materials</rdfs:comment>
    <rdl:PCA_100006768>Hose data, including pressure, medium, materials</rdl:PCA_100006768>
    <rdl:PCA_100006766 rdf:resource="http://rds.posccaesar.org/ontology/plm/rdl/PCA_100006653"/>
    <rdl:PCA_100006763>This document shall support verification of compliance and provide necessary information</rdl:PCA_100006763>
    <rdfs:subClassOf rdf:resource="http://rds.posccaesar.org/ontology/plm/rdl/PCA_100004908"/>
  </owl:Class>
  <owl:Class rdf:about="http://rds.posccaesar.org/ontology/plm/rdl/PCA_100006158">
    <rdl:PCA_100006766 rdf:resource="http://rds.posccaesar.org/ontology/plm/rdl/PCA_100006654"/>
    <skos:broadMatch rdf:resource="http://rds.posccaesar.org/ontology/plm/rdl/PCA_100006698"/>
    <rdl:PCA_100006768>In general, requirements applicable for design of the plant are defined by design basis, Company specifications and international standard.</rdl:PCA_100006768>
    <skos:broadMatch>
      <rdl:PCA_100001503 rdf:about="http://rds.posccaesar.org/ontology/plm/rdl/PCA_100006693">
        <rdfs:label>standard</rdfs:label>
        <rdl:PCA_100004924>DH</rdl:PCA_100004924>
        <rdf:type rdf:resource="http://www.w3.org/2002/07/owl#NamedIndividual"/>
      </rdl:PCA_100001503>
    </skos:broadMatch>
    <skos:broader rdf:resource="http://rds.posccaesar.org/ontology/plm/rdl/PCA_100006757"/>
    <rdfs:label>Design requirements for process and utility systems</rdfs:label>
    <rdfs:comment>In general, requirements applicable for design of the plant are defined by design basis, Company specifications and international standard.</rdfs:comment>
    <rdl:PCA_100006765 rdf:resource="http://w3id.org/readi/rdl/CFIHOS-20000026"/>
    <skos:broadMatch rdf:resource="http://rds.posccaesar.org/ontology/plm/rdl/PCA_100006696"/>
    <skos:broadMatch rdf:resource="http://rds.posccaesar.org/ontology/plm/rdl/PCA_100006695"/>
    <rdfs:subClassOf rdf:resource="http://rds.posccaesar.org/ontology/plm/rdl/PCA_100004908"/>
    <rdl:PCA_100006763>For installation specific requirements to newbuilds and modifications.</rdl:PCA_100006763>
  </owl:Class>
  <owl:Class rdf:about="http://rds.posccaesar.org/ontology/plm/rdl/PCA_100006289">
    <rdl:PCA_100006766 rdf:resource="http://rds.posccaesar.org/ontology/plm/rdl/PCA_100006653"/>
    <rdl:PCA_100006768>A drawing showing information for an assembly of parts or sub-assemblies (co-functioning components, equipment or assemblies), including key interface dimensions, weight, assembly information and design limitations.</rdl:PCA_100006768>
    <rdfs:subClassOf rdf:resource="http://rds.posccaesar.org/ontology/plm/rdl/PCA_100004908"/>
    <rdl:PCA_100006765 rdf:resource="http://w3id.org/readi/rdl/CFIHOS-20000031"/>
    <skos:broader rdf:resource="http://rds.posccaesar.org/ontology/plm/rdl/PCA_100006746"/>
    <rdfs:label>Interface drawing</rdfs:label>
    <rdfs:comment>A drawing showing information for an assembly of parts or sub-assemblies (co-functioning components, equipment or assemblies), including key interface dimensions, weight, assembly information and design limitations.</rdfs:comment>
    <skos:broadMatch rdf:resource="http://rds.posccaesar.org/ontology/plm/rdl/PCA_100006713"/>
    <rdl:PCA_100006763>Provide information to suppliers of interfacing equipment.</rdl:PCA_100006763>
  </owl:Class>
  <owl:Class rdf:about="http://rds.posccaesar.org/ontology/plm/rdl/PCA_100006277">
    <rdl:PCA_100006765 rdf:resource="http://w3id.org/readi/rdl/CFIHOS-20000018"/>
    <rdfs:label>Installation procedures onshore CP system</rdfs:label>
    <rdfs:subClassOf rdf:resource="http://rds.posccaesar.org/ontology/plm/rdl/PCA_100004908"/>
    <rdl:PCA_100006763>Installation procedures shall be according to ISO15589-1 Section 13.1.2.</rdl:PCA_100006763>
    <rdl:PCA_100006768>The pipeline installation procedures shall reflect and take into account the CP-system.</rdl:PCA_100006768>
    <rdfs:comment>The pipeline installation procedures shall reflect and take into account the CP-system.</rdfs:comment>
    <skos:broader rdf:resource="http://rds.posccaesar.org/ontology/plm/rdl/PCA_100006751"/>
    <rdl:PCA_100006766 rdf:resource="http://rds.posccaesar.org/ontology/plm/rdl/PCA_100006657"/>
    <skos:broadMatch rdf:resource="http://rds.posccaesar.org/ontology/plm/rdl/PCA_100006688"/>
  </owl:Class>
  <owl:Class rdf:about="http://rds.posccaesar.org/ontology/plm/rdl/PCA_100006398">
    <rdl:PCA_100006766 rdf:resource="http://rds.posccaesar.org/ontology/plm/rdl/PCA_100006607"/>
    <rdl:PCA_100006766 rdf:resource="http://rds.posccaesar.org/ontology/plm/rdl/PCA_100006601"/>
    <rdl:PCA_100006766 rdf:resource="http://rds.posccaesar.org/ontology/plm/rdl/PCA_100006592"/>
    <skos:broader rdf:resource="http://rds.posccaesar.org/ontology/plm/rdl/PCA_100006749"/>
    <rdl:PCA_100006766 rdf:resource="http://rds.posccaesar.org/ontology/plm/rdl/PCA_100006604"/>
    <rdl:PCA_100006766 rdf:resource="http://rds.posccaesar.org/ontology/plm/rdl/PCA_100006611"/>
    <rdl:PCA_100006766 rdf:resource="http://rds.posccaesar.org/ontology/plm/rdl/PCA_100006595"/>
    <rdl:PCA_100006766 rdf:resource="http://rds.posccaesar.org/ontology/plm/rdl/PCA_100006582"/>
    <rdl:PCA_100006766 rdf:resource="http://rds.posccaesar.org/ontology/plm/rdl/PCA_100006599"/>
    <rdl:PCA_100006766 rdf:resource="http://rds.posccaesar.org/ontology/plm/rdl/PCA_100006627"/>
    <rdfs:label>Process system engineering manuals</rdfs:label>
    <rdl:PCA_100006766 rdf:resource="http://rds.posccaesar.org/ontology/plm/rdl/PCA_100006620"/>
    <rdl:PCA_100006766 rdf:resource="http://rds.posccaesar.org/ontology/plm/rdl/PCA_100006614"/>
    <rdl:PCA_100006768>Table of contents:

1    Objective and target group
2    System description 
2.1    Introduction
2.2    Design basis
2.3    Process description
2.4    Utility systems, chemicals and catalyst requirements
2.5    Analysis (sampling points, etc.)
2.6    HSE requirements
3    System operation, including process control 
3.1    Normal operation
3.2    Normal start-up
3.3    Normal shut down
3.4    Special operations
3.5    Routine operations
4    Maintenance
4.1    Depressurization and flushing
4.2    Maintenance
5    System protection 
5.1    Premises
5.2    Process and emergency shut-down functions
5.3    Specific equipment protection
5.4    Pressure safety equipment (relief valves, rupture disks, etc.)
5.5    Car seals, key locks and key interlocks
6    Specific design solutions
7    Technical data, calculations and drawings 
8    Additional information 
8.1    Definitions and abbreviations
8.2    Changes from previous version
8.3    References

Section 4 shall describe maintenance sequence, including how to shut down and drain equipment and parts of the system, relevant conclusions from HAZOP and other evaluations, and any other relevant considerations; reference to supplier documentation for individual equipment maintenance procedures can be done in addition.

Section 5 shall include a list of all the isolation valves located in the pressure-relief system piping which could isolate pressure relief valves in the system. The required position and the reason for the lock or the seal shall be included.

Section 6 shall give details about the specific design solutions chosen for equipment, instrumentation and materials. The reasoning behind the specific design solutions shall also be given in this section, e.g. the reason for choosing a specific level control instrument, the specific compressor configuration, the specific heat exchanger configuration etc. Any limitations to the operation caused by the e.g. the material selection or e.g. the design capacity shall be explained in this section. This could be low or high temperature limitations, throughput limitations for heat exchangers, operating conditions which reduce the lifetime of an equipment unit etc.

Section 7 shall include the relevant technical data, calculations and drawings not covered by a reference to a separate document in section 8.3.

Section 8.2 shall be used to log the performed modifications affecting the described system design and operation. For a new built installation this section will be empty. For a modification this section shall describe the changes resulting from the modification only once, i.e. changes between the versions issued internally throughout the modification project shall not be commented.</rdl:PCA_100006768>
    <rdl:PCA_100006766 rdf:resource="http://rds.posccaesar.org/ontology/plm/rdl/PCA_100006606"/>
    <rdl:PCA_100006766 rdf:resource="http://rds.posccaesar.org/ontology/plm/rdl/PCA_100006585"/>
    <rdl:PCA_100006766 rdf:resource="http://rds.posccaesar.org/ontology/plm/rdl/PCA_100006589"/>
    <skos:broadMatch rdf:resource="http://rds.posccaesar.org/ontology/plm/rdl/PCA_100006688"/>
    <rdl:PCA_100006766 rdf:resource="http://rds.posccaesar.org/ontology/plm/rdl/PCA_100006579"/>
    <rdl:PCA_100006763>One process system engineering manual shall be written for each process system (e.g. oil separation system, gas compression system, open drain system, freshwater system, flare system, etc.). The objective of the manuals is to describe and document the design and operation of the system.</rdl:PCA_100006763>
    <rdl:PCA_100006766 rdf:resource="http://rds.posccaesar.org/ontology/plm/rdl/PCA_100006609"/>
    <rdl:PCA_100006766 rdf:resource="http://rds.posccaesar.org/ontology/plm/rdl/PCA_100006600"/>
    <rdl:PCA_100006766 rdf:resource="http://rds.posccaesar.org/ontology/plm/rdl/PCA_100006591"/>
    <rdfs:comment>Table of contents:

1    Objective and target group
2    System description 
2.1    Introduction
2.2    Design basis
2.3    Process description
2.4    Utility systems, chemicals and catalyst requirements
2.5    Analysis (sampling points, etc.)
2.6    HSE requirements
3    System operation, including process control 
3.1    Normal operation
3.2    Normal start-up
3.3    Normal shut down
3.4    Special operations
3.5    Routine operations
4    Maintenance
4.1    Depressurization and flushing
4.2    Maintenance
5    System protection 
5.1    Premises
5.2    Process and emergency shut-down functions
5.3    Specific equipment protection
5.4    Pressure safety equipment (relief valves, rupture disks, etc.)
5.5    Car seals, key locks and key interlocks
6    Specific design solutions
7    Technical data, calculations and drawings 
8    Additional information 
8.1    Definitions and abbreviations
8.2    Changes from previous version
8.3    References

Section 4 shall describe maintenance sequence, including how to shut down and drain equipment and parts of the system, relevant conclusions from HAZOP and other evaluations, and any other relevant considerations; reference to supplier documentation for individual equipment maintenance procedures can be done in addition.

Section 5 shall include a list of all the isolation valves located in the pressure-relief system piping which could isolate pressure relief valves in the system. The required position and the reason for the lock or the seal shall be included.

Section 6 shall give details about the specific design solutions chosen for equipment, instrumentation and materials. The reasoning behind the specific design solutions shall also be given in this section, e.g. the reason for choosing a specific level control instrument, the specific compressor configuration, the specific heat exchanger configuration etc. Any limitations to the operation caused by the e.g. the material selection or e.g. the design capacity shall be explained in this section. This could be low or high temperature limitations, throughput limitations for heat exchangers, operating conditions which reduce the lifetime of an equipment unit etc.

Section 7 shall include the relevant technical data, calculations and drawings not covered by a reference to a separate document in section 8.3.

Section 8.2 shall be used to log the performed modifications affecting the described system design and operation. For a new built installation this section will be empty. For a modification this section shall describe the changes resulting from the modification only once, i.e. changes between the versions issued internally throughout the modification project shall not be commented.</rdfs:comment>
    <skos:broader rdf:resource="http://rds.posccaesar.org/ontology/plm/rdl/PCA_100006754"/>
    <rdl:PCA_100006766 rdf:resource="http://rds.posccaesar.org/ontology/plm/rdl/PCA_100006623"/>
    <rdl:PCA_100006766 rdf:resource="http://rds.posccaesar.org/ontology/plm/rdl/PCA_100006619"/>
    <rdl:PCA_100006766 rdf:resource="http://rds.posccaesar.org/ontology/plm/rdl/PCA_100006613"/>
    <rdl:PCA_100006766 rdf:resource="http://rds.posccaesar.org/ontology/plm/rdl/PCA_100006610"/>
    <rdl:PCA_100006766 rdf:resource="http://rds.posccaesar.org/ontology/plm/rdl/PCA_100006584"/>
    <rdl:PCA_100006766 rdf:resource="http://rds.posccaesar.org/ontology/plm/rdl/PCA_100006581"/>
    <rdl:PCA_100006766 rdf:resource="http://rds.posccaesar.org/ontology/plm/rdl/PCA_100006588"/>
    <rdl:PCA_100006766 rdf:resource="http://rds.posccaesar.org/ontology/plm/rdl/PCA_100006616"/>
    <rdl:PCA_100006766 rdf:resource="http://rds.posccaesar.org/ontology/plm/rdl/PCA_100006603"/>
    <rdl:PCA_100006766 rdf:resource="http://rds.posccaesar.org/ontology/plm/rdl/PCA_100006594"/>
    <rdl:PCA_100006766 rdf:resource="http://rds.posccaesar.org/ontology/plm/rdl/PCA_100006598"/>
    <rdl:PCA_100006766 rdf:resource="http://rds.posccaesar.org/ontology/plm/rdl/PCA_100006628"/>
    <rdl:PCA_100006766 rdf:resource="http://rds.posccaesar.org/ontology/plm/rdl/PCA_100006618"/>
    <rdl:PCA_100006766 rdf:resource="http://rds.posccaesar.org/ontology/plm/rdl/PCA_100006597"/>
    <rdl:PCA_100006766 rdf:resource="http://rds.posccaesar.org/ontology/plm/rdl/PCA_100006580"/>
    <rdl:PCA_100006766 rdf:resource="http://rds.posccaesar.org/ontology/plm/rdl/PCA_100006625"/>
    <rdl:PCA_100006766 rdf:resource="http://rds.posccaesar.org/ontology/plm/rdl/PCA_100006622"/>
    <rdl:PCA_100006766 rdf:resource="http://rds.posccaesar.org/ontology/plm/rdl/PCA_100006578"/>
    <rdl:PCA_100006766 rdf:resource="http://rds.posccaesar.org/ontology/plm/rdl/PCA_100006608"/>
    <rdl:PCA_100006766 rdf:resource="http://rds.posccaesar.org/ontology/plm/rdl/PCA_100006612"/>
    <rdfs:subClassOf rdf:resource="http://rds.posccaesar.org/ontology/plm/rdl/PCA_100004908"/>
    <rdl:PCA_100006766 rdf:resource="http://rds.posccaesar.org/ontology/plm/rdl/PCA_100006583"/>
    <rdl:PCA_100006766 rdf:resource="http://rds.posccaesar.org/ontology/plm/rdl/PCA_100006590"/>
    <rdl:PCA_100006766 rdf:resource="http://rds.posccaesar.org/ontology/plm/rdl/PCA_100006587"/>
    <rdl:PCA_100006766 rdf:resource="http://rds.posccaesar.org/ontology/plm/rdl/PCA_100006605"/>
    <rdl:PCA_100006766 rdf:resource="http://rds.posccaesar.org/ontology/plm/rdl/PCA_100006602"/>
    <rdl:PCA_100006766 rdf:resource="http://rds.posccaesar.org/ontology/plm/rdl/PCA_100006596"/>
    <rdl:PCA_100006766 rdf:resource="http://rds.posccaesar.org/ontology/plm/rdl/PCA_100006593"/>
    <rdl:PCA_100006765 rdf:resource="http://w3id.org/readi/rdl/CFIHOS-20000026"/>
    <rdl:PCA_100006766 rdf:resource="http://rds.posccaesar.org/ontology/plm/rdl/PCA_100006621"/>
    <rdl:PCA_100006766 rdf:resource="http://rds.posccaesar.org/ontology/plm/rdl/PCA_100006615"/>
    <rdl:PCA_100006766 rdf:resource="http://rds.posccaesar.org/ontology/plm/rdl/PCA_100006617"/>
    <rdl:PCA_100006766 rdf:resource="http://rds.posccaesar.org/ontology/plm/rdl/PCA_100006586"/>
    <rdl:PCA_100006766 rdf:resource="http://rds.posccaesar.org/ontology/plm/rdl/PCA_100006624"/>
  </owl:Class>
  <owl:Class rdf:about="http://rds.posccaesar.org/ontology/plm/rdl/PCA_100006386">
    <rdl:PCA_100006768>Document containing records of material identification by chemical analysis.</rdl:PCA_100006768>
    <rdfs:comment>Document containing records of material identification by chemical analysis.</rdfs:comment>
    <rdfs:label>Positive material identification (PMI) reports</rdfs:label>
    <rdl:PCA_100006763>Document use of correct material.</rdl:PCA_100006763>
    <skos:broadMatch rdf:resource="http://rds.posccaesar.org/ontology/plm/rdl/PCA_100006722"/>
    <skos:broader rdf:resource="http://rds.posccaesar.org/ontology/plm/rdl/PCA_100006756"/>
    <rdl:PCA_100006766 rdf:resource="http://rds.posccaesar.org/ontology/plm/rdl/PCA_100006653"/>
    <rdfs:subClassOf rdf:resource="http://rds.posccaesar.org/ontology/plm/rdl/PCA_100004908"/>
    <rdl:PCA_100006765 rdf:resource="http://w3id.org/readi/rdl/CFIHOS-20000031"/>
  </owl:Class>
  <owl:Class rdf:about="http://rds.posccaesar.org/ontology/plm/rdl/PCA_100006495">
    <rdfs:label>Telecommunication system topology diagram</rdfs:label>
    <rdfs:subClassOf rdf:resource="http://rds.posccaesar.org/ontology/plm/rdl/PCA_100004908"/>
    <rdl:PCA_100006768>The following telecommunication system topology diagrams shall be provided:
 - Overall telecommunication topology diagram;
 - Telecommunication topology diagram per telecommunication system (according to NORSOK T-101.

The overall telecommunication system topology diagram typical contents shall be:
 - All related telecommunication systems/subsystems represented by blocks;
 - Location;
 - Interface and wiring between blocks shall be indicated.

Telecommunication topology diagram per telecommunication system typical information shall be:
 - The function of each unit (block): Short description, supplied with function identification code if applicable;
 - Interface between blocks and interface to other equipment/systems;
 - Signal type and function (Ethernet, 2/4 W E&amp;M, G.703, RS232, control signals, etc.) if applicable;
 - Location of the equipment, either by text labelling of each block or by blocks located in dotted area boxes.</rdl:PCA_100006768>
    <rdl:PCA_100006763>The overall telecommunication system topology diagram shall show an overall configuration of all telecommunication systems to give a functional understanding.

Telecommunication topology diagram per telecommunication system shall show the relation between functional units within a telecommunication system/subsystem.</rdl:PCA_100006763>
    <skos:broadMatch rdf:resource="http://rds.posccaesar.org/ontology/plm/rdl/PCA_100006695"/>
    <rdl:PCA_100006765 rdf:resource="http://w3id.org/readi/rdl/CFIHOS-20000030"/>
    <rdl:PCA_100006766 rdf:resource="http://rds.posccaesar.org/ontology/plm/rdl/PCA_100006640"/>
    <rdfs:comment>The following telecommunication system topology diagrams shall be provided:
 - Overall telecommunication topology diagram;
 - Telecommunication topology diagram per telecommunication system (according to NORSOK T-101.

The overall telecommunication system topology diagram typical contents shall be:
 - All related telecommunication systems/subsystems represented by blocks;
 - Location;
 - Interface and wiring between blocks shall be indicated.

Telecommunication topology diagram per telecommunication system typical information shall be:
 - The function of each unit (block): Short description, supplied with function identification code if applicable;
 - Interface between blocks and interface to other equipment/systems;
 - Signal type and function (Ethernet, 2/4 W E&amp;M, G.703, RS232, control signals, etc.) if applicable;
 - Location of the equipment, either by text labelling of each block or by blocks located in dotted area boxes.</rdfs:comment>
    <skos:broader rdf:resource="http://rds.posccaesar.org/ontology/plm/rdl/PCA_100006745"/>
  </owl:Class>
  <owl:Class rdf:about="http://rds.posccaesar.org/ontology/plm/rdl/PCA_100006265">
    <rdfs:subClassOf rdf:resource="http://rds.posccaesar.org/ontology/plm/rdl/PCA_100004908"/>
    <rdl:PCA_100006766 rdf:resource="http://rds.posccaesar.org/ontology/plm/rdl/PCA_100006617"/>
    <rdl:PCA_100006766 rdf:resource="http://rds.posccaesar.org/ontology/plm/rdl/PCA_100006584"/>
    <rdl:PCA_100006766 rdf:resource="http://rds.posccaesar.org/ontology/plm/rdl/PCA_100006581"/>
    <rdl:PCA_100006765 rdf:resource="http://w3id.org/readi/rdl/CFIHOS-20000011"/>
    <rdl:PCA_100006766 rdf:resource="http://rds.posccaesar.org/ontology/plm/rdl/PCA_100006588"/>
    <rdl:PCA_100006766 rdf:resource="http://rds.posccaesar.org/ontology/plm/rdl/PCA_100006624"/>
    <rdl:PCA_100006766 rdf:resource="http://rds.posccaesar.org/ontology/plm/rdl/PCA_100006601"/>
    <rdl:PCA_100006766 rdf:resource="http://rds.posccaesar.org/ontology/plm/rdl/PCA_100006594"/>
    <rdl:PCA_100006766 rdf:resource="http://rds.posccaesar.org/ontology/plm/rdl/PCA_100006598"/>
    <rdfs:comment> - The required hydraulic system (network) capacity, and correct design for in-line equipment, such as control valves, hydraulic/pneumatic actuators, etc.
 - For liquid systems where water hammering can be an issue, such as fire water and offloading systems, dynamic calculations shall be included as a part of the hydraulic system calculations. 
 - Firewater:
   - Results/evaluation from transient firewater hammer effect for ringmain high points in distribution system shall also be included.
   - Piping and nozzle diagrams as well as Commissioning test reports and results shall be included as separate files.

Hydraulic system calculation reports and corresponding executable simulation files (preferably embedded in the report).</rdfs:comment>
    <rdl:PCA_100006766 rdf:resource="http://rds.posccaesar.org/ontology/plm/rdl/PCA_100006604"/>
    <rdl:PCA_100006766 rdf:resource="http://rds.posccaesar.org/ontology/plm/rdl/PCA_100006597"/>
    <rdl:PCA_100006766 rdf:resource="http://rds.posccaesar.org/ontology/plm/rdl/PCA_100006580"/>
    <rdl:PCA_100006766 rdf:resource="http://rds.posccaesar.org/ontology/plm/rdl/PCA_100006627"/>
    <rdl:PCA_100006766 rdf:resource="http://rds.posccaesar.org/ontology/plm/rdl/PCA_100006620"/>
    <rdl:PCA_100006766 rdf:resource="http://rds.posccaesar.org/ontology/plm/rdl/PCA_100006578"/>
    <rdl:PCA_100006766 rdf:resource="http://rds.posccaesar.org/ontology/plm/rdl/PCA_100006614"/>
    <rdl:PCA_100006763>For liquid systems such as heating medium, cooling medium, fire water, offloading, loading, hydraulic power systems, drain, etc., hydraulics design shall be documented by hydraulic system calculations demonstrating as a minimum:</rdl:PCA_100006763>
    <rdl:PCA_100006766 rdf:resource="http://rds.posccaesar.org/ontology/plm/rdl/PCA_100006583"/>
    <rdl:PCA_100006766 rdf:resource="http://rds.posccaesar.org/ontology/plm/rdl/PCA_100006590"/>
    <rdl:PCA_100006765 rdf:resource="http://w3id.org/readi/rdl/CFIHOS-20000013"/>
    <rdl:PCA_100006765 rdf:resource="http://w3id.org/readi/rdl/CFIHOS-20000010"/>
    <rdl:PCA_100006766 rdf:resource="http://rds.posccaesar.org/ontology/plm/rdl/PCA_100006587"/>
    <skos:broadMatch rdf:resource="http://rds.posccaesar.org/ontology/plm/rdl/PCA_100006687"/>
    <rdl:PCA_100006766 rdf:resource="http://rds.posccaesar.org/ontology/plm/rdl/PCA_100006600"/>
    <rdl:PCA_100006766 rdf:resource="http://rds.posccaesar.org/ontology/plm/rdl/PCA_100006596"/>
    <rdl:PCA_100006766 rdf:resource="http://rds.posccaesar.org/ontology/plm/rdl/PCA_100006593"/>
    <rdl:PCA_100006766 rdf:resource="http://rds.posccaesar.org/ontology/plm/rdl/PCA_100006623"/>
    <skos:broader rdf:resource="http://rds.posccaesar.org/ontology/plm/rdl/PCA_100006741"/>
    <rdl:PCA_100006766 rdf:resource="http://rds.posccaesar.org/ontology/plm/rdl/PCA_100006619"/>
    <rdl:PCA_100006766 rdf:resource="http://rds.posccaesar.org/ontology/plm/rdl/PCA_100006613"/>
    <rdl:PCA_100006766 rdf:resource="http://rds.posccaesar.org/ontology/plm/rdl/PCA_100006586"/>
    <rdfs:label>Hydraulic system calculations</rdfs:label>
    <rdl:PCA_100006766 rdf:resource="http://rds.posccaesar.org/ontology/plm/rdl/PCA_100006616"/>
    <rdl:PCA_100006766 rdf:resource="http://rds.posccaesar.org/ontology/plm/rdl/PCA_100006603"/>
    <rdl:PCA_100006765 rdf:resource="http://w3id.org/readi/rdl/CFIHOS-20000026"/>
    <rdl:PCA_100006766 rdf:resource="http://rds.posccaesar.org/ontology/plm/rdl/PCA_100006592"/>
    <rdl:PCA_100006766 rdf:resource="http://rds.posccaesar.org/ontology/plm/rdl/PCA_100006628"/>
    <rdl:PCA_100006766 rdf:resource="http://rds.posccaesar.org/ontology/plm/rdl/PCA_100006595"/>
    <rdl:PCA_100006766 rdf:resource="http://rds.posccaesar.org/ontology/plm/rdl/PCA_100006582"/>
    <rdl:PCA_100006768> - The required hydraulic system (network) capacity, and correct design for in-line equipment, such as control valves, hydraulic/pneumatic actuators, etc.
 - For liquid systems where water hammering can be an issue, such as fire water and offloading systems, dynamic calculations shall be included as a part of the hydraulic system calculations. 
 - Firewater:
   - Results/evaluation from transient firewater hammer effect for ringmain high points in distribution system shall also be included.
   - Piping and nozzle diagrams as well as Commissioning test reports and results shall be included as separate files.

Hydraulic system calculation reports and corresponding executable simulation files (preferably embedded in the report).</rdl:PCA_100006768>
    <rdl:PCA_100006766 rdf:resource="http://rds.posccaesar.org/ontology/plm/rdl/PCA_100006599"/>
    <rdl:PCA_100006766 rdf:resource="http://rds.posccaesar.org/ontology/plm/rdl/PCA_100006625"/>
    <rdl:PCA_100006766 rdf:resource="http://rds.posccaesar.org/ontology/plm/rdl/PCA_100006608"/>
    <rdl:PCA_100006766 rdf:resource="http://rds.posccaesar.org/ontology/plm/rdl/PCA_100006612"/>
    <rdl:PCA_100006766 rdf:resource="http://rds.posccaesar.org/ontology/plm/rdl/PCA_100006585"/>
    <rdl:PCA_100006766 rdf:resource="http://rds.posccaesar.org/ontology/plm/rdl/PCA_100006589"/>
    <rdl:PCA_100006766 rdf:resource="http://rds.posccaesar.org/ontology/plm/rdl/PCA_100006579"/>
    <rdl:PCA_100006766 rdf:resource="http://rds.posccaesar.org/ontology/plm/rdl/PCA_100006605"/>
    <rdl:PCA_100006766 rdf:resource="http://rds.posccaesar.org/ontology/plm/rdl/PCA_100006602"/>
    <rdl:PCA_100006766 rdf:resource="http://rds.posccaesar.org/ontology/plm/rdl/PCA_100006591"/>
  </owl:Class>
  <owl:Class rdf:about="http://rds.posccaesar.org/ontology/plm/rdl/PCA_100006253">
    <rdl:PCA_100006765 rdf:resource="http://w3id.org/readi/rdl/CFIHOS-20000011"/>
    <rdfs:label>HSE activity plan/program</rdfs:label>
    <skos:broadMatch rdf:resource="http://rds.posccaesar.org/ontology/plm/rdl/PCA_100006726"/>
    <skos:broadMatch rdf:resource="http://rds.posccaesar.org/ontology/plm/rdl/PCA_100006727"/>
    <skos:broadMatch rdf:resource="http://rds.posccaesar.org/ontology/plm/rdl/PCA_100006729"/>
    <rdl:PCA_100006763>Information shall be given concerning health, safety and environment</rdl:PCA_100006763>
    <skos:broader rdf:resource="http://rds.posccaesar.org/ontology/plm/rdl/PCA_100006756"/>
    <rdl:PCA_100006766 rdf:resource="http://rds.posccaesar.org/ontology/plm/rdl/PCA_100006653"/>
    <rdl:PCA_100006768>Chemical substances that may be hazardous to personnel or environment. For all these chemicals datasheets shall be available during installation, operation and maintenance substances that in connection with maintenance, discarding or similar, require special precautions forsake destruction noise vibration radiation and/or radioactivity dust ergonomics in operation and maintenance risk and criticality analyses.</rdl:PCA_100006768>
    <rdfs:subClassOf rdf:resource="http://rds.posccaesar.org/ontology/plm/rdl/PCA_100004908"/>
    <rdfs:comment>Chemical substances that may be hazardous to personnel or environment. For all these chemicals datasheets shall be available during installation, operation and maintenance substances that in connection with maintenance, discarding or similar, require special precautions forsake destruction noise vibration radiation and/or radioactivity dust ergonomics in operation and maintenance risk and criticality analyses.</rdfs:comment>
    <rdl:PCA_100006765 rdf:resource="http://w3id.org/readi/rdl/CFIHOS-20000014"/>
    <skos:broadMatch rdf:resource="http://rds.posccaesar.org/ontology/plm/rdl/PCA_100006728"/>
  </owl:Class>
  <owl:Class rdf:about="http://rds.posccaesar.org/ontology/plm/rdl/PCA_100006374">
    <rdfs:label>Piping fabrication procedure</rdfs:label>
    <rdl:PCA_100006765 rdf:resource="http://w3id.org/readi/rdl/CFIHOS-20000031"/>
    <rdfs:subClassOf rdf:resource="http://rds.posccaesar.org/ontology/plm/rdl/PCA_100004908"/>
    <skos:broadMatch rdf:resource="http://rds.posccaesar.org/ontology/plm/rdl/PCA_100006688"/>
    <rdl:PCA_100006766 rdf:resource="http://rds.posccaesar.org/ontology/plm/rdl/PCA_100006653"/>
    <rdl:PCA_100006768>Document specifying the methods for fabrication of piping. Includes references to specifications for welding, NDT, assembly, dimensional control, FAT, painting etc.</rdl:PCA_100006768>
    <rdfs:comment>Document specifying the methods for fabrication of piping. Includes references to specifications for welding, NDT, assembly, dimensional control, FAT, painting etc.</rdfs:comment>
    <skos:broader rdf:resource="http://rds.posccaesar.org/ontology/plm/rdl/PCA_100006751"/>
    <rdl:PCA_100006763>Specify fabrication requirements for piping.</rdl:PCA_100006763>
  </owl:Class>
  <owl:Class rdf:about="http://rds.posccaesar.org/ontology/plm/rdl/PCA_100006362">
    <rdl:PCA_100006765 rdf:resource="http://w3id.org/readi/rdl/CFIHOS-20000018"/>
    <skos:broader rdf:resource="http://rds.posccaesar.org/ontology/plm/rdl/PCA_100006751"/>
    <rdl:PCA_100006766 rdf:resource="http://rds.posccaesar.org/ontology/plm/rdl/PCA_100006654"/>
    <skos:broadMatch rdf:resource="http://rds.posccaesar.org/ontology/plm/rdl/PCA_100006688"/>
    <rdfs:comment>The procedure shall describe:
 - planned pig type(s)
 - the main steps needed to launch pig into pig launcher and further into the pipeline
 - how to run it into the receiver and take it out
 - equipment needed for pigging
 - preparation for pigging
 - special precautions to be aware of (e.g. block valves, in-line instrumentations, Tees, Wyes etc.) and what corresponding actions to be taken before, during and/or after pigging.</rdfs:comment>
    <rdfs:label>Pigging procedures</rdfs:label>
    <rdl:PCA_100006768>The procedure shall describe:
 - planned pig type(s)
 - the main steps needed to launch pig into pig launcher and further into the pipeline
 - how to run it into the receiver and take it out
 - equipment needed for pigging
 - preparation for pigging
 - special precautions to be aware of (e.g. block valves, in-line instrumentations, Tees, Wyes etc.) and what corresponding actions to be taken before, during and/or after pigging.</rdl:PCA_100006768>
    <rdl:PCA_100006763>The operational procedure shall describe the necessary activities required for safe pigging operations.</rdl:PCA_100006763>
    <rdfs:subClassOf rdf:resource="http://rds.posccaesar.org/ontology/plm/rdl/PCA_100004908"/>
  </owl:Class>
  <owl:Class rdf:about="http://rds.posccaesar.org/ontology/plm/rdl/PCA_100006241">
    <rdl:PCA_100006768>The manufacturer's standard general arrangement should be used as far as possible.

A drawing showing overall dimensions, critical interface dimensions, part references and weight of assemblies, equipment and components. The drawing shall
contain reference to main specifications and standards  For equipment / components the drawing may include cross sectional views.
Document may contain the following information:
 - Main dimensions
 - Interface connections
 - Weight
 - Centre of gravity
 - Withdrawal/installation and maintenance space.
 - Installation and mounting details
 - Lifting arrangement</rdl:PCA_100006768>
    <skos:broader rdf:resource="http://rds.posccaesar.org/ontology/plm/rdl/PCA_100006739"/>
    <rdfs:label>General arrangment drawing</rdfs:label>
    <rdl:PCA_100006763>This documentation shall provide information about the physical dimensions of the unit, needed to integrate the product into a system design.</rdl:PCA_100006763>
    <rdfs:comment>The manufacturer's standard general arrangement should be used as far as possible.

A drawing showing overall dimensions, critical interface dimensions, part references and weight of assemblies, equipment and components. The drawing shall
contain reference to main specifications and standards  For equipment / components the drawing may include cross sectional views.
Document may contain the following information:
 - Main dimensions
 - Interface connections
 - Weight
 - Centre of gravity
 - Withdrawal/installation and maintenance space.
 - Installation and mounting details
 - Lifting arrangement</rdfs:comment>
    <rdl:PCA_100006764>[ELECTRICAL]
Torque on connections in main circuit shall be specified</rdl:PCA_100006764>
    <rdl:PCA_100006766 rdf:resource="http://rds.posccaesar.org/ontology/plm/rdl/PCA_100006653"/>
    <skos:broadMatch rdf:resource="http://rds.posccaesar.org/ontology/plm/rdl/PCA_100006710"/>
    <skos:broadMatch rdf:resource="http://rds.posccaesar.org/ontology/plm/rdl/PCA_100006708"/>
    <rdfs:subClassOf rdf:resource="http://rds.posccaesar.org/ontology/plm/rdl/PCA_100004908"/>
    <skos:broadMatch rdf:resource="http://rds.posccaesar.org/ontology/plm/rdl/PCA_100006709"/>
  </owl:Class>
  <owl:Class rdf:about="http://rds.posccaesar.org/ontology/plm/rdl/PCA_100006483">
    <rdl:PCA_100006765 rdf:resource="http://w3id.org/readi/rdl/CFIHOS-20000018"/>
    <rdl:PCA_100006766 rdf:resource="http://rds.posccaesar.org/ontology/plm/rdl/PCA_100006654"/>
    <rdfs:comment>To be delivered in accordance with Companys' requirements.</rdfs:comment>
    <skos:broader rdf:resource="http://rds.posccaesar.org/ontology/plm/rdl/PCA_100006748"/>
    <skos:broadMatch rdf:resource="http://rds.posccaesar.org/ontology/plm/rdl/PCA_100006660"/>
    <rdfs:label>Tag - document cross reference</rdfs:label>
    <rdfs:subClassOf rdf:resource="http://rds.posccaesar.org/ontology/plm/rdl/PCA_100004908"/>
    <rdl:PCA_100006763>Ensure traceability of components</rdl:PCA_100006763>
    <rdl:PCA_100006768>To be delivered in accordance with Companys' requirements.</rdl:PCA_100006768>
  </owl:Class>
  <owl:Class rdf:about="http://rds.posccaesar.org/ontology/plm/rdl/PCA_100006471">
    <skos:broadMatch rdf:resource="http://rds.posccaesar.org/ontology/plm/rdl/PCA_100006734"/>
    <rdl:PCA_100006765 rdf:resource="http://w3id.org/readi/rdl/CFIHOS-20000031"/>
    <rdfs:label>Subsea spool layout drawings</rdfs:label>
    <skos:broadMatch rdf:resource="http://rds.posccaesar.org/ontology/plm/rdl/PCA_100006708"/>
    <skos:broader rdf:resource="http://rds.posccaesar.org/ontology/plm/rdl/PCA_100006746"/>
    <rdfs:subClassOf rdf:resource="http://rds.posccaesar.org/ontology/plm/rdl/PCA_100004908"/>
    <skos:broadMatch rdf:resource="http://rds.posccaesar.org/ontology/plm/rdl/PCA_100006731"/>
    <rdl:PCA_100006766 rdf:resource="http://rds.posccaesar.org/ontology/plm/rdl/PCA_100006653"/>
    <skos:broadMatch rdf:resource="http://rds.posccaesar.org/ontology/plm/rdl/PCA_100006732"/>
    <skos:broadMatch rdf:resource="http://rds.posccaesar.org/ontology/plm/rdl/PCA_100006733"/>
  </owl:Class>
  <owl:Class rdf:about="http://rds.posccaesar.org/ontology/plm/rdl/PCA_100006350">
    <skos:broader rdf:resource="http://rds.posccaesar.org/ontology/plm/rdl/PCA_100006751"/>
    <skos:broadMatch rdf:resource="http://rds.posccaesar.org/ontology/plm/rdl/PCA_100006688"/>
    <rdfs:label>Operational procedure for a lined pipeline</rdfs:label>
    <rdfs:comment>This procedure shall as a minimum address the following aspects: 
 - System description.
 - Operating envelope.
 - Pigging.
 - Start-up procedure.
 - Routine operations.
 - De-pressurising.</rdfs:comment>
    <rdl:PCA_100006768>This procedure shall as a minimum address the following aspects: 
 - System description.
 - Operating envelope.
 - Pigging.
 - Start-up procedure.
 - Routine operations.
 - De-pressurising.</rdl:PCA_100006768>
    <rdl:PCA_100006766 rdf:resource="http://rds.posccaesar.org/ontology/plm/rdl/PCA_100006657"/>
    <rdl:PCA_100006765 rdf:resource="http://w3id.org/readi/rdl/CFIHOS-20000018"/>
    <rdfs:subClassOf rdf:resource="http://rds.posccaesar.org/ontology/plm/rdl/PCA_100004908"/>
  </owl:Class>
  <owl:Class rdf:about="http://rds.posccaesar.org/ontology/plm/rdl/PCA_100006121">
    <rdfs:label>Cleanness documentation</rdfs:label>
    <rdfs:comment>Documentation of cleanness according to specification.</rdfs:comment>
    <rdl:PCA_100006768>Documentation of cleanness according to specification.</rdl:PCA_100006768>
    <rdl:PCA_100006766 rdf:resource="http://rds.posccaesar.org/ontology/plm/rdl/PCA_100006653"/>
    <rdl:PCA_100006763>Verification of cleanness off hydraulic system.</rdl:PCA_100006763>
    <rdfs:subClassOf rdf:resource="http://rds.posccaesar.org/ontology/plm/rdl/PCA_100004908"/>
  </owl:Class>
  <owl:Class rdf:about="http://rds.posccaesar.org/ontology/plm/rdl/PCA_100006133">
    <rdfs:comment>Description of consequences of switching off the logic solver, including both hardwired signals and software communicated signals, and suggestion to operational mitigating actions to avoid the consequences described to avoid further loss of plant operation covering both switching off and start-up. The document shall describe the general precautions and consequences and describe in detail signals found to be critical (regularity, safety and environmental) and the effect on these signals after switching off the logic solver.</rdfs:comment>
    <rdfs:subClassOf rdf:resource="http://rds.posccaesar.org/ontology/plm/rdl/PCA_100004908"/>
    <rdl:PCA_100006765 rdf:resource="http://w3id.org/readi/rdl/CFIHOS-20000015"/>
    <skos:broader rdf:resource="http://rds.posccaesar.org/ontology/plm/rdl/PCA_100006756"/>
    <skos:broadMatch rdf:resource="http://rds.posccaesar.org/ontology/plm/rdl/PCA_100006698"/>
    <rdl:PCA_100006768>Description of consequences of switching off the logic solver, including both hardwired signals and software communicated signals, and suggestion to operational mitigating actions to avoid the consequences described to avoid further loss of plant operation covering both switching off and start-up. The document shall describe the general precautions and consequences and describe in detail signals found to be critical (regularity, safety and environmental) and the effect on these signals after switching off the logic solver.</rdl:PCA_100006768>
    <rdl:PCA_100006763>There shall be a consequence analysis document for each individual logic solver.

This document shall give information about which process unit is affected if the logic solver is switched off.</rdl:PCA_100006763>
    <rdl:PCA_100006766 rdf:resource="http://rds.posccaesar.org/ontology/plm/rdl/PCA_100006633"/>
    <rdfs:label>Consequence analysis logic solver</rdfs:label>
    <rdl:PCA_100006766 rdf:resource="http://rds.posccaesar.org/ontology/plm/rdl/PCA_100006626"/>
  </owl:Class>
  <owl:Class rdf:about="http://rds.posccaesar.org/ontology/plm/rdl/PCA_100006145">
    <rdl:PCA_100006765 rdf:resource="http://w3id.org/readi/rdl/CFIHOS-20000011"/>
    <rdfs:comment>The datasheet shall as a minimum contain the information specified in the datasheet template. 

C999-ST-R-DS-0041 Template - Noise data sheet</rdfs:comment>
    <skos:broader rdf:resource="http://rds.posccaesar.org/ontology/plm/rdl/PCA_100006747"/>
    <skos:broadMatch rdf:resource="http://rds.posccaesar.org/ontology/plm/rdl/PCA_100006686"/>
    <rdl:PCA_100006765 rdf:resource="http://w3id.org/readi/rdl/CFIHOS-20000010"/>
    <rdl:PCA_100006763>The equipment supplier standard datasheet shall be delivered.</rdl:PCA_100006763>
    <rdfs:label>Data sheet - Noise</rdfs:label>
    <rdl:PCA_100006768>The datasheet shall as a minimum contain the information specified in the datasheet template. 

C999-ST-R-DS-0041 Template - Noise data sheet</rdl:PCA_100006768>
    <rdfs:subClassOf rdf:resource="http://rds.posccaesar.org/ontology/plm/rdl/PCA_100004908"/>
  </owl:Class>
  <owl:Class rdf:about="http://rds.posccaesar.org/ontology/plm/rdl/PCA_100006157">
    <rdl:PCA_100006765 rdf:resource="http://w3id.org/readi/rdl/CFIHOS-20000031"/>
    <rdl:PCA_100006764>If on System level, (i.e. System Design Report): 
The objective of the system design report is to give sufficient details arguing the reason for choice of design related to system parameters. This shall apply to all disciplines within all systems. Typical content may be:
 - System description
 - Operational data and limitations
 - Composition of medium
 - Material choice
 - Corrosion evaluations
 - Bases for choice and use of corrosion inhibitors
 - Location of injection points
 - Location of sampling points for analyses
 - Location of areas for corrosion control equipment
 - Project specific features and solutions
 - Hydraulic analysis (fire protection systems)
 - Seabed preparation and intervention work</rdl:PCA_100006764>
    <rdfs:comment>A report containing design analysis/calculations, including loads and load cases. It further summarizes design parameters, system integrity and operational limitations according to design specifications as given by the design basis.</rdfs:comment>
    <rdl:PCA_100006763>A report verifying conformance to design specifications.</rdl:PCA_100006763>
    <rdl:PCA_100006766 rdf:resource="http://rds.posccaesar.org/ontology/plm/rdl/PCA_100006653"/>
    <skos:broadMatch rdf:resource="http://rds.posccaesar.org/ontology/plm/rdl/PCA_100006686"/>
    <skos:broader rdf:resource="http://rds.posccaesar.org/ontology/plm/rdl/PCA_100006756"/>
    <rdfs:label>Design report</rdfs:label>
    <rdfs:subClassOf rdf:resource="http://rds.posccaesar.org/ontology/plm/rdl/PCA_100004908"/>
    <rdl:PCA_100006768>A report containing design analysis/calculations, including loads and load cases. It further summarizes design parameters, system integrity and operational limitations according to design specifications as given by the design basis.</rdl:PCA_100006768>
  </owl:Class>
  <owl:Class rdf:about="http://rds.posccaesar.org/ontology/plm/rdl/PCA_100006169">
    <rdl:PCA_100006765 rdf:resource="http://w3id.org/readi/rdl/CFIHOS-20000018"/>
    <rdl:PCA_100006766 rdf:resource="http://rds.posccaesar.org/ontology/plm/rdl/PCA_100006656"/>
    <rdfs:label>Dredging, trenching and ploughing survey reports and data</rdfs:label>
    <rdl:PCA_100006768>Data to be delivered in accordance with Companys' requirements</rdl:PCA_100006768>
    <rdl:PCA_100006763>Survey reports and data shall comply with requirements for Onshore/Offshore surveys.</rdl:PCA_100006763>
    <skos:broader rdf:resource="http://rds.posccaesar.org/ontology/plm/rdl/PCA_100006762"/>
    <rdfs:comment>Data to be delivered in accordance with Companys' requirements</rdfs:comment>
    <rdfs:subClassOf rdf:resource="http://rds.posccaesar.org/ontology/plm/rdl/PCA_100004908"/>
    <skos:broader rdf:resource="http://rds.posccaesar.org/ontology/plm/rdl/PCA_100006756"/>
    <skos:broadMatch rdf:resource="http://rds.posccaesar.org/ontology/plm/rdl/PCA_100006705"/>
  </owl:Class>
  <owl:AnnotationProperty rdf:about="http://www.w3.org/2004/02/skos/core#broadMatch"/>
  <owl:AnnotationProperty rdf:about="http://www.w3.org/2004/02/skos/core#member"/>
  <rdf:Description rdf:about="http://rds.posccaesar.org/ontology/plm/rdl/PCA_100006769">
    <skos:member rdf:resource="http://rds.posccaesar.org/ontology/plm/rdl/PCA_100006604"/>
    <skos:member rdf:resource="http://rds.posccaesar.org/ontology/plm/rdl/PCA_100006600"/>
    <skos:member rdf:resource="http://rds.posccaesar.org/ontology/plm/rdl/PCA_100006585"/>
    <skos:member rdf:resource="http://rds.posccaesar.org/ontology/plm/rdl/PCA_100006628"/>
    <skos:member rdf:resource="http://rds.posccaesar.org/ontology/plm/rdl/PCA_100006581"/>
    <skos:member rdf:resource="http://rds.posccaesar.org/ontology/plm/rdl/PCA_100006617"/>
    <skos:member rdf:resource="http://rds.posccaesar.org/ontology/plm/rdl/PCA_100006624"/>
    <skos:member rdf:resource="http://rds.posccaesar.org/ontology/plm/rdl/PCA_100006613"/>
    <skos:member rdf:resource="http://rds.posccaesar.org/ontology/plm/rdl/PCA_100006598"/>
    <skos:member rdf:resource="http://rds.posccaesar.org/ontology/plm/rdl/PCA_100006594"/>
    <skos:member rdf:resource="http://rds.posccaesar.org/ontology/plm/rdl/PCA_100006637"/>
    <skos:member rdf:resource="http://rds.posccaesar.org/ontology/plm/rdl/PCA_100006614"/>
    <skos:member rdf:resource="http://rds.posccaesar.org/ontology/plm/rdl/PCA_100006621"/>
    <skos:member rdf:resource="http://rds.posccaesar.org/ontology/plm/rdl/PCA_100006610"/>
    <skos:member rdf:resource="http://rds.posccaesar.org/ontology/plm/rdl/PCA_100006638"/>
    <skos:member rdf:resource="http://rds.posccaesar.org/ontology/plm/rdl/PCA_100006591"/>
    <skos:member rdf:resource="http://rds.posccaesar.org/ontology/plm/rdl/PCA_100006634"/>
    <skos:member rdf:resource="http://rds.posccaesar.org/ontology/plm/rdl/PCA_100006647"/>
    <skos:member rdf:resource="http://rds.posccaesar.org/ontology/plm/rdl/PCA_100006631"/>
    <skos:member>
      <rdl:PCA_100001503 rdf:about="http://rds.posccaesar.org/ontology/plm/rdl/PCA_100006652">
        <rdfs:label>Area Completion</rdfs:label>
        <rdl:PCA_100004924>99</rdl:PCA_100004924>
        <rdf:type rdf:resource="http://www.w3.org/2002/07/owl#NamedIndividual"/>
      </rdl:PCA_100001503>
    </skos:member>
    <skos:member rdf:resource="http://rds.posccaesar.org/ontology/plm/rdl/PCA_100006644"/>
    <skos:member rdf:resource="http://rds.posccaesar.org/ontology/plm/rdl/PCA_100006609"/>
    <skos:member rdf:resource="http://rds.posccaesar.org/ontology/plm/rdl/PCA_100006579"/>
    <skos:member rdf:resource="http://rds.posccaesar.org/ontology/plm/rdl/PCA_100006657"/>
    <skos:member rdf:resource="http://rds.posccaesar.org/ontology/plm/rdl/PCA_100006606"/>
    <skos:member rdf:resource="http://rds.posccaesar.org/ontology/plm/rdl/PCA_100006587"/>
    <skos:member rdf:resource="http://rds.posccaesar.org/ontology/plm/rdl/PCA_100006654"/>
    <skos:member rdf:resource="http://rds.posccaesar.org/ontology/plm/rdl/PCA_100006583"/>
    <skos:member rdf:resource="http://rds.posccaesar.org/ontology/plm/rdl/PCA_100006619"/>
    <skos:member rdf:resource="http://rds.posccaesar.org/ontology/plm/rdl/PCA_100006603"/>
    <skos:member rdf:resource="http://rds.posccaesar.org/ontology/plm/rdl/PCA_100006596"/>
    <skos:member rdf:resource="http://rds.posccaesar.org/ontology/plm/rdl/PCA_100006627"/>
    <skos:member rdf:resource="http://rds.posccaesar.org/ontology/plm/rdl/PCA_100006580"/>
    <skos:member rdf:resource="http://rds.posccaesar.org/ontology/plm/rdl/PCA_100006616"/>
    <skos:member rdf:resource="http://rds.posccaesar.org/ontology/plm/rdl/PCA_100006623"/>
    <skos:member rdf:resource="http://rds.posccaesar.org/ontology/plm/rdl/PCA_100006612"/>
    <skos:member rdf:resource="http://rds.posccaesar.org/ontology/plm/rdl/PCA_100006597"/>
    <skos:member rdf:resource="http://rds.posccaesar.org/ontology/plm/rdl/PCA_100006593"/>
    <skos:member rdf:resource="http://rds.posccaesar.org/ontology/plm/rdl/PCA_100006636"/>
    <skos:member rdf:resource="http://rds.posccaesar.org/ontology/plm/rdl/PCA_100006620"/>
    <skos:member rdf:resource="http://rds.posccaesar.org/ontology/plm/rdl/PCA_100006641"/>
    <skos:member>
      <rdl:PCA_100001503 rdf:about="http://rds.posccaesar.org/ontology/plm/rdl/PCA_100006649">
        <rdfs:label>Subsea structure and template</rdfs:label>
        <rdl:PCA_100004924>96</rdl:PCA_100004924>
        <rdf:type rdf:resource="http://www.w3.org/2002/07/owl#NamedIndividual"/>
      </rdl:PCA_100001503>
    </skos:member>
    <skos:member rdf:resource="http://rds.posccaesar.org/ontology/plm/rdl/PCA_100006590"/>
    <skos:member rdf:resource="http://rds.posccaesar.org/ontology/plm/rdl/PCA_100006633"/>
    <skos:member>
      <rdl:PCA_100001503 rdf:about="http://rds.posccaesar.org/ontology/plm/rdl/PCA_100006646">
        <rdfs:label>Architectural incl. Workshop and storage</rdfs:label>
        <rdl:PCA_100004924>93</rdl:PCA_100004924>
        <rdf:type rdf:resource="http://www.w3.org/2002/07/owl#NamedIndividual"/>
      </rdl:PCA_100001503>
    </skos:member>
    <skos:member rdf:resource="http://rds.posccaesar.org/ontology/plm/rdl/PCA_100006630"/>
    <skos:member>
      <rdl:PCA_100001503 rdf:about="http://rds.posccaesar.org/ontology/plm/rdl/PCA_100006651">
        <rdfs:label>Corrosion protection</rdfs:label>
        <rdl:PCA_100004924>98</rdl:PCA_100004924>
        <rdf:type rdf:resource="http://www.w3.org/2002/07/owl#NamedIndividual"/>
      </rdl:PCA_100001503>
    </skos:member>
    <skos:member rdf:resource="http://rds.posccaesar.org/ontology/plm/rdl/PCA_100006643"/>
    <skos:member rdf:resource="http://rds.posccaesar.org/ontology/plm/rdl/PCA_100006608"/>
    <skos:member rdf:resource="http://rds.posccaesar.org/ontology/plm/rdl/PCA_100006589"/>
    <skos:member rdf:resource="http://rds.posccaesar.org/ontology/plm/rdl/PCA_100006578"/>
    <skos:member rdf:resource="http://rds.posccaesar.org/ontology/plm/rdl/PCA_100006656"/>
    <skos:member rdf:resource="http://rds.posccaesar.org/ontology/plm/rdl/PCA_100006605"/>
    <skos:member rdf:resource="http://rds.posccaesar.org/ontology/plm/rdl/PCA_100006601"/>
    <skos:member rdf:resource="http://rds.posccaesar.org/ontology/plm/rdl/PCA_100006586"/>
    <skos:member rdf:resource="http://rds.posccaesar.org/ontology/plm/rdl/PCA_100006629"/>
    <skos:member rdf:resource="http://rds.posccaesar.org/ontology/plm/rdl/PCA_100006582"/>
    <skos:member rdf:resource="http://rds.posccaesar.org/ontology/plm/rdl/PCA_100006618"/>
    <skos:member rdf:resource="http://rds.posccaesar.org/ontology/plm/rdl/PCA_100006625"/>
    <skos:member rdf:resource="http://rds.posccaesar.org/ontology/plm/rdl/PCA_100006602"/>
    <skos:member rdf:resource="http://rds.posccaesar.org/ontology/plm/rdl/PCA_100006599"/>
    <skos:member rdf:resource="http://rds.posccaesar.org/ontology/plm/rdl/PCA_100006595"/>
    <skos:member rdf:resource="http://rds.posccaesar.org/ontology/plm/rdl/PCA_100006626"/>
    <skos:member rdf:resource="http://rds.posccaesar.org/ontology/plm/rdl/PCA_100006615"/>
    <skos:member rdf:resource="http://rds.posccaesar.org/ontology/plm/rdl/PCA_100006622"/>
    <skos:member rdf:resource="http://rds.posccaesar.org/ontology/plm/rdl/PCA_100006611"/>
    <skos:member rdf:resource="http://rds.posccaesar.org/ontology/plm/rdl/PCA_100006639"/>
    <skos:member rdf:resource="http://rds.posccaesar.org/ontology/plm/rdl/PCA_100006592"/>
    <skos:member rdf:resource="http://rds.posccaesar.org/ontology/plm/rdl/PCA_100006635"/>
    <skos:member rdf:resource="http://rds.posccaesar.org/ontology/plm/rdl/PCA_100006640"/>
    <skos:member rdf:resource="http://rds.posccaesar.org/ontology/plm/rdl/PCA_100006648"/>
    <skos:member rdf:resource="http://rds.posccaesar.org/ontology/plm/rdl/PCA_100006632"/>
    <skos:member rdf:resource="http://rds.posccaesar.org/ontology/plm/rdl/PCA_100006653"/>
    <skos:member>
      <rdl:PCA_100001503 rdf:about="http://rds.posccaesar.org/ontology/plm/rdl/PCA_100006645">
        <rdfs:label>Temporary</rdfs:label>
        <rdl:PCA_100004924>92</rdl:PCA_100004924>
        <rdf:type rdf:resource="http://www.w3.org/2002/07/owl#NamedIndividual"/>
      </rdl:PCA_100001503>
    </skos:member>
    <skos:member rdf:resource="http://rds.posccaesar.org/ontology/plm/rdl/PCA_100006650"/>
    <skos:member rdf:resource="http://rds.posccaesar.org/ontology/plm/rdl/PCA_100006642"/>
    <skos:member rdf:resource="http://rds.posccaesar.org/ontology/plm/rdl/PCA_100006607"/>
    <skos:member rdf:resource="http://rds.posccaesar.org/ontology/plm/rdl/PCA_100006588"/>
    <skos:member rdf:resource="http://rds.posccaesar.org/ontology/plm/rdl/PCA_100006584"/>
    <skos:member rdf:resource="http://rds.posccaesar.org/ontology/plm/rdl/PCA_100006655"/>
  </rdf:Description>
  <owl:AnnotationProperty rdf:about="http://www.w3.org/2004/02/skos/core#broader"/>
  <rdf:Description rdf:about="http://rds.posccaesar.org/ontology/plm/rdl/PCA_100006771">
    <skos:member rdf:resource="http://rds.posccaesar.org/ontology/plm/rdl/PCA_100006755"/>
    <skos:member rdf:resource="http://rds.posccaesar.org/ontology/plm/rdl/PCA_100006761"/>
    <skos:member rdf:resource="http://rds.posccaesar.org/ontology/plm/rdl/PCA_100006741"/>
    <skos:member rdf:resource="http://rds.posccaesar.org/ontology/plm/rdl/PCA_100006760"/>
    <skos:member rdf:resource="http://rds.posccaesar.org/ontology/plm/rdl/PCA_100006752"/>
    <skos:member rdf:resource="http://rds.posccaesar.org/ontology/plm/rdl/PCA_100006747"/>
    <skos:member rdf:resource="http://rds.posccaesar.org/ontology/plm/rdl/PCA_100006746"/>
    <skos:member rdf:resource="http://rds.posccaesar.org/ontology/plm/rdl/PCA_100006753"/>
    <skos:member rdf:resource="http://rds.posccaesar.org/ontology/plm/rdl/PCA_100006744"/>
    <skos:member rdf:resource="http://rds.posccaesar.org/ontology/plm/rdl/PCA_100006751"/>
    <skos:member rdf:resource="http://rds.posccaesar.org/ontology/plm/rdl/PCA_100006750"/>
    <skos:member rdf:resource="http://rds.posccaesar.org/ontology/plm/rdl/PCA_100006758"/>
    <skos:member rdf:resource="http://rds.posccaesar.org/ontology/plm/rdl/PCA_100006739"/>
    <skos:member rdf:resource="http://rds.posccaesar.org/ontology/plm/rdl/PCA_100006759"/>
    <skos:member rdf:resource="http://rds.posccaesar.org/ontology/plm/rdl/PCA_100006745"/>
    <skos:member rdf:resource="http://rds.posccaesar.org/ontology/plm/rdl/PCA_100006762"/>
    <skos:member rdf:resource="http://rds.posccaesar.org/ontology/plm/rdl/PCA_100006743"/>
    <skos:member rdf:resource="http://rds.posccaesar.org/ontology/plm/rdl/PCA_100006742"/>
    <skos:member rdf:resource="http://rds.posccaesar.org/ontology/plm/rdl/PCA_100006740"/>
    <skos:member rdf:resource="http://rds.posccaesar.org/ontology/plm/rdl/PCA_100006756"/>
    <skos:member rdf:resource="http://rds.posccaesar.org/ontology/plm/rdl/PCA_100006754"/>
    <skos:member rdf:resource="http://rds.posccaesar.org/ontology/plm/rdl/PCA_100006738"/>
    <skos:member rdf:resource="http://rds.posccaesar.org/ontology/plm/rdl/PCA_100006749"/>
    <skos:member rdf:resource="http://rds.posccaesar.org/ontology/plm/rdl/PCA_100006757"/>
    <skos:member rdf:resource="http://rds.posccaesar.org/ontology/plm/rdl/PCA_100006748"/>
  </rdf:Description>
  <rdf:Description rdf:about="http://rds.posccaesar.org/ontology/plm/rdl/PCA_100006772">
    <skos:member rdf:resource="http://w3id.org/readi/rdl/CFIHOS-20000014"/>
    <skos:member>
      <rdl:PCA_100001503 rdf:about="http://w3id.org/readi/rdl/CFIHOS-20000004">
        <rdfs:label>geotechnical engineering</rdfs:label>
        <rdl:PCA_100004924>CG</rdl:PCA_100004924>
        <rdf:type rdf:resource="http://www.w3.org/2002/07/owl#NamedIndividual"/>
      </rdl:PCA_100001503>
    </skos:member>
    <skos:member rdf:resource="http://w3id.org/readi/rdl/CFIHOS-20000018"/>
    <skos:member rdf:resource="http://w3id.org/readi/rdl/CFIHOS-20000008"/>
    <skos:member rdf:resource="http://w3id.org/readi/rdl/CFIHOS-20000021"/>
    <skos:member rdf:resource="http://w3id.org/readi/rdl/CFIHOS-20000030"/>
    <skos:member rdf:resource="http://w3id.org/readi/rdl/CFIHOS-20000020"/>
    <skos:member>
      <rdl:PCA_100001503 rdf:about="http://w3id.org/readi/rdl/CFIHOS-20000040">
        <rdfs:label>geophysics</rdfs:label>
        <rdl:PCA_100004924>ZS</rdl:PCA_100004924>
        <rdf:type rdf:resource="http://www.w3.org/2002/07/owl#NamedIndividual"/>
      </rdl:PCA_100001503>
    </skos:member>
    <skos:member rdf:resource="http://w3id.org/readi/rdl/CFIHOS-20000023"/>
    <skos:member rdf:resource="http://w3id.org/readi/rdl/CFIHOS-20000010"/>
    <skos:member rdf:resource="http://w3id.org/readi/rdl/CFIHOS-20000027"/>
    <skos:member rdf:resource="http://w3id.org/readi/rdl/CFIHOS-20000003"/>
    <skos:member rdf:resource="http://w3id.org/readi/rdl/CFIHOS-20000007"/>
    <skos:member>
      <rdl:PCA_100001503 rdf:about="http://w3id.org/readi/rdl/CFIHOS-20000037">
        <rdfs:label>human resources</rdfs:label>
        <rdl:PCA_100004924>ZH</rdl:PCA_100004924>
        <rdf:type rdf:resource="http://www.w3.org/2002/07/owl#NamedIndividual"/>
      </rdl:PCA_100001503>
    </skos:member>
    <skos:member>
      <rdl:PCA_100001503 rdf:about="http://w3id.org/readi/rdl/CFIHOS-20000012">
        <rdfs:label>security</rdfs:label>
        <rdl:PCA_100004924>HP</rdl:PCA_100004924>
        <rdf:type rdf:resource="http://www.w3.org/2002/07/owl#NamedIndividual"/>
      </rdl:PCA_100001503>
    </skos:member>
    <skos:member>
      <rdl:PCA_100001503 rdf:about="http://w3id.org/readi/rdl/CFIHOS-20000002">
        <rdfs:label>construction</rdfs:label>
        <rdl:PCA_100004924>BA</rdl:PCA_100004924>
        <rdf:type rdf:resource="http://www.w3.org/2002/07/owl#NamedIndividual"/>
      </rdl:PCA_100001503>
    </skos:member>
    <skos:member>
      <rdl:PCA_100001503 rdf:about="http://w3id.org/readi/rdl/CFIHOS-20000016">
        <rdfs:label>information management</rdfs:label>
        <rdl:PCA_100004924>JA</rdl:PCA_100004924>
        <rdf:type rdf:resource="http://www.w3.org/2002/07/owl#NamedIndividual"/>
      </rdl:PCA_100001503>
    </skos:member>
    <skos:member rdf:resource="http://w3id.org/readi/rdl/CFIHOS-20000006"/>
    <skos:member>
      <rdl:PCA_100001503 rdf:about="http://w3id.org/readi/rdl/CFIHOS-20000009">
        <rdfs:label>cost and planning management</rdfs:label>
        <rdl:PCA_100004924>FA</rdl:PCA_100004924>
        <rdf:type rdf:resource="http://www.w3.org/2002/07/owl#NamedIndividual"/>
      </rdl:PCA_100001503>
    </skos:member>
    <skos:member>
      <rdl:PCA_100001503 rdf:about="http://w3id.org/readi/rdl/CFIHOS-20000043">
        <rdfs:label>commissioning</rdfs:label>
        <rdl:PCA_100004924>BC</rdl:PCA_100004924>
        <rdf:type rdf:resource="http://www.w3.org/2002/07/owl#NamedIndividual"/>
      </rdl:PCA_100001503>
    </skos:member>
    <skos:member rdf:resource="http://w3id.org/readi/rdl/CFIHOS-20000033"/>
    <skos:member rdf:resource="http://w3id.org/readi/rdl/CFIHOS-20000042"/>
    <skos:member rdf:resource="http://w3id.org/readi/rdl/CFIHOS-20000001"/>
    <skos:member>
      <rdl:PCA_100001503 rdf:about="http://w3id.org/readi/rdl/CFIHOS-20000005">
        <rdfs:label>infrastructure engineering</rdfs:label>
        <rdl:PCA_100004924>CI</rdl:PCA_100004924>
        <rdf:type rdf:resource="http://www.w3.org/2002/07/owl#NamedIndividual"/>
      </rdl:PCA_100001503>
    </skos:member>
    <skos:member>
      <rdl:PCA_100001503 rdf:about="http://w3id.org/readi/rdl/CFIHOS-20000035">
        <rdfs:label>finance</rdfs:label>
        <rdl:PCA_100004924>ZF</rdl:PCA_100004924>
        <rdf:type rdf:resource="http://www.w3.org/2002/07/owl#NamedIndividual"/>
      </rdl:PCA_100001503>
    </skos:member>
    <skos:member>
      <rdl:PCA_100001503 rdf:about="http://w3id.org/readi/rdl/CFIHOS-20000039">
        <rdfs:label>reservoir engineering</rdfs:label>
        <rdl:PCA_100004924>ZR</rdl:PCA_100004924>
        <rdf:type rdf:resource="http://www.w3.org/2002/07/owl#NamedIndividual"/>
      </rdl:PCA_100001503>
    </skos:member>
    <skos:member>
      <rdl:PCA_100001503 rdf:about="http://w3id.org/readi/rdl/CFIHOS-20000036">
        <rdfs:label>geomatics</rdfs:label>
        <rdl:PCA_100004924>ZG</rdl:PCA_100004924>
        <rdf:type rdf:resource="http://www.w3.org/2002/07/owl#NamedIndividual"/>
      </rdl:PCA_100001503>
    </skos:member>
    <skos:member rdf:resource="http://w3id.org/readi/rdl/CFIHOS-20000026"/>
    <skos:member rdf:resource="http://w3id.org/readi/rdl/CFIHOS-20000015"/>
    <skos:member rdf:resource="http://w3id.org/readi/rdl/CFIHOS-20000019"/>
    <skos:member>
      <rdl:PCA_100001503 rdf:about="http://w3id.org/readi/rdl/CFIHOS-20000041">
        <rdfs:label>production technology</rdfs:label>
        <rdl:PCA_100004924>ZT</rdl:PCA_100004924>
        <rdf:type rdf:resource="http://www.w3.org/2002/07/owl#NamedIndividual"/>
      </rdl:PCA_100001503>
    </skos:member>
    <skos:member rdf:resource="http://w3id.org/readi/rdl/CFIHOS-20000031"/>
    <skos:member>
      <rdl:PCA_100001503 rdf:about="http://w3id.org/readi/rdl/CFIHOS-20000032">
        <rdfs:label>contracting and procurement management</rdfs:label>
        <rdl:PCA_100004924>VA</rdl:PCA_100004924>
        <rdf:type rdf:resource="http://www.w3.org/2002/07/owl#NamedIndividual"/>
      </rdl:PCA_100001503>
    </skos:member>
    <skos:member rdf:resource="http://w3id.org/readi/rdl/CFIHOS-20000022"/>
    <skos:member rdf:resource="http://w3id.org/readi/rdl/CFIHOS-20000011"/>
    <skos:member>
      <rdl:PCA_100001503 rdf:about="http://w3id.org/readi/rdl/CFIHOS-20000025">
        <rdfs:label>operations management</rdfs:label>
        <rdl:PCA_100004924>OA</rdl:PCA_100004924>
        <rdf:type rdf:resource="http://www.w3.org/2002/07/owl#NamedIndividual"/>
      </rdl:PCA_100001503>
    </skos:member>
    <skos:member rdf:resource="http://w3id.org/readi/rdl/CFIHOS-20000029"/>
    <skos:member>
      <rdl:PCA_100001503 rdf:about="http://w3id.org/readi/rdl/CFIHOS-20000034">
        <rdfs:label>geology</rdfs:label>
        <rdl:PCA_100004924>ZE</rdl:PCA_100004924>
        <rdf:type rdf:resource="http://www.w3.org/2002/07/owl#NamedIndividual"/>
      </rdl:PCA_100001503>
    </skos:member>
    <skos:member>
      <rdl:PCA_100001503 rdf:about="http://w3id.org/readi/rdl/CFIHOS-20000024">
        <rdfs:label>maintenance management</rdfs:label>
        <rdl:PCA_100004924>NA</rdl:PCA_100004924>
        <rdf:type rdf:resource="http://www.w3.org/2002/07/owl#NamedIndividual"/>
      </rdl:PCA_100001503>
    </skos:member>
    <skos:member rdf:resource="http://w3id.org/readi/rdl/CFIHOS-20000013"/>
    <skos:member>
      <rdl:PCA_100001503 rdf:about="http://w3id.org/readi/rdl/CFIHOS-20000038">
        <rdfs:label>petrophysics</rdfs:label>
        <rdl:PCA_100004924>ZP</rdl:PCA_100004924>
        <rdf:type rdf:resource="http://www.w3.org/2002/07/owl#NamedIndividual"/>
      </rdl:PCA_100001503>
    </skos:member>
    <skos:member rdf:resource="http://w3id.org/readi/rdl/CFIHOS-20000028"/>
    <skos:member>
      <rdl:PCA_100001503 rdf:about="http://w3id.org/readi/rdl/CFIHOS-20000017">
        <rdfs:label>information technology</rdfs:label>
        <rdl:PCA_100004924>KA</rdl:PCA_100004924>
        <rdf:type rdf:resource="http://www.w3.org/2002/07/owl#NamedIndividual"/>
      </rdl:PCA_100001503>
    </skos:member>
  </rdf:Description>
  <rdf:Description rdf:about="http://rds.posccaesar.org/ontology/plm/rdl/PCA_100006773">
    <skos:member rdf:resource="http://rds.posccaesar.org/ontology/plm/rdl/PCA_100006469"/>
    <skos:member rdf:resource="http://rds.posccaesar.org/ontology/plm/rdl/PCA_100006193"/>
    <skos:member rdf:resource="http://rds.posccaesar.org/ontology/plm/rdl/PCA_100006135"/>
    <skos:member rdf:resource="http://rds.posccaesar.org/ontology/plm/rdl/PCA_100006339"/>
    <skos:member rdf:resource="http://rds.posccaesar.org/ontology/plm/rdl/PCA_100006161"/>
    <skos:member rdf:resource="http://rds.posccaesar.org/ontology/plm/rdl/PCA_100006203"/>
    <skos:member rdf:resource="http://rds.posccaesar.org/ontology/plm/rdl/PCA_100006096"/>
    <skos:member rdf:resource="http://rds.posccaesar.org/ontology/plm/rdl/PCA_100006458"/>
    <skos:member rdf:resource="http://rds.posccaesar.org/ontology/plm/rdl/PCA_100006200"/>
    <skos:member rdf:resource="http://rds.posccaesar.org/ontology/plm/rdl/PCA_100006308"/>
    <skos:member rdf:resource="http://rds.posccaesar.org/ontology/plm/rdl/PCA_100006313"/>
    <skos:member rdf:resource="http://rds.posccaesar.org/ontology/plm/rdl/PCA_100006130"/>
    <skos:member rdf:resource="http://rds.posccaesar.org/ontology/plm/rdl/PCA_100006237"/>
    <skos:member rdf:resource="http://rds.posccaesar.org/ontology/plm/rdl/PCA_100006388"/>
    <skos:member rdf:resource="http://rds.posccaesar.org/ontology/plm/rdl/PCA_100006299"/>
    <skos:member rdf:resource="http://rds.posccaesar.org/ontology/plm/rdl/PCA_100006488"/>
    <skos:member rdf:resource="http://rds.posccaesar.org/ontology/plm/rdl/PCA_100006536"/>
    <skos:member rdf:resource="http://rds.posccaesar.org/ontology/plm/rdl/PCA_100006340"/>
    <skos:member rdf:resource="http://rds.posccaesar.org/ontology/plm/rdl/PCA_100006180"/>
    <skos:member rdf:resource="http://rds.posccaesar.org/ontology/plm/rdl/PCA_100006091"/>
    <skos:member rdf:resource="http://rds.posccaesar.org/ontology/plm/rdl/PCA_100006542"/>
    <skos:member rdf:resource="http://rds.posccaesar.org/ontology/plm/rdl/PCA_100006122"/>
    <skos:member rdf:resource="http://rds.posccaesar.org/ontology/plm/rdl/PCA_100006453"/>
    <skos:member rdf:resource="http://rds.posccaesar.org/ontology/plm/rdl/PCA_100006290"/>
    <skos:member rdf:resource="http://rds.posccaesar.org/ontology/plm/rdl/PCA_100006412"/>
    <skos:member rdf:resource="http://rds.posccaesar.org/ontology/plm/rdl/PCA_100006377"/>
    <skos:member rdf:resource="http://rds.posccaesar.org/ontology/plm/rdl/PCA_100006288"/>
    <skos:member rdf:resource="http://rds.posccaesar.org/ontology/plm/rdl/PCA_100006223"/>
    <skos:member rdf:resource="http://rds.posccaesar.org/ontology/plm/rdl/PCA_100006492"/>
    <skos:member rdf:resource="http://rds.posccaesar.org/ontology/plm/rdl/PCA_100006408"/>
    <skos:member rdf:resource="http://rds.posccaesar.org/ontology/plm/rdl/PCA_100006111"/>
    <skos:member rdf:resource="http://rds.posccaesar.org/ontology/plm/rdl/PCA_100006173"/>
    <skos:member rdf:resource="http://rds.posccaesar.org/ontology/plm/rdl/PCA_100006084"/>
    <skos:member rdf:resource="http://rds.posccaesar.org/ontology/plm/rdl/PCA_100006206"/>
    <skos:member rdf:resource="http://rds.posccaesar.org/ontology/plm/rdl/PCA_100006446"/>
    <skos:member rdf:resource="http://rds.posccaesar.org/ontology/plm/rdl/PCA_100006372"/>
    <skos:member rdf:resource="http://rds.posccaesar.org/ontology/plm/rdl/PCA_100006212"/>
    <skos:member rdf:resource="http://rds.posccaesar.org/ontology/plm/rdl/PCA_100006249"/>
    <skos:member rdf:resource="http://rds.posccaesar.org/ontology/plm/rdl/PCA_100006349"/>
    <skos:member rdf:resource="http://rds.posccaesar.org/ontology/plm/rdl/PCA_100006364"/>
    <skos:member rdf:resource="http://rds.posccaesar.org/ontology/plm/rdl/PCA_100006275"/>
    <skos:member rdf:resource="http://rds.posccaesar.org/ontology/plm/rdl/PCA_100006530"/>
    <skos:member rdf:resource="http://rds.posccaesar.org/ontology/plm/rdl/PCA_100006361"/>
    <skos:member rdf:resource="http://rds.posccaesar.org/ontology/plm/rdl/PCA_100006545"/>
    <skos:member rdf:resource="http://rds.posccaesar.org/ontology/plm/rdl/PCA_100006465"/>
    <skos:member rdf:resource="http://rds.posccaesar.org/ontology/plm/rdl/PCA_100006131"/>
    <skos:member rdf:resource="http://rds.posccaesar.org/ontology/plm/rdl/PCA_100006158"/>
    <skos:member rdf:resource="http://rds.posccaesar.org/ontology/plm/rdl/PCA_100006238"/>
    <skos:member rdf:resource="http://rds.posccaesar.org/ontology/plm/rdl/PCA_100006433"/>
    <skos:member rdf:resource="http://rds.posccaesar.org/ontology/plm/rdl/PCA_100006537"/>
    <skos:member rdf:resource="http://rds.posccaesar.org/ontology/plm/rdl/PCA_100006448"/>
    <skos:member rdf:resource="http://rds.posccaesar.org/ontology/plm/rdl/PCA_100006268"/>
    <skos:member rdf:resource="http://rds.posccaesar.org/ontology/plm/rdl/PCA_100006092"/>
    <skos:member rdf:resource="http://rds.posccaesar.org/ontology/plm/rdl/PCA_100006454"/>
    <skos:member rdf:resource="http://rds.posccaesar.org/ontology/plm/rdl/PCA_100006304"/>
    <skos:member rdf:resource="http://rds.posccaesar.org/ontology/plm/rdl/PCA_100006218"/>
    <skos:member rdf:resource="http://rds.posccaesar.org/ontology/plm/rdl/PCA_100006506"/>
    <skos:member rdf:resource="http://rds.posccaesar.org/ontology/plm/rdl/PCA_100006417"/>
    <skos:member rdf:resource="http://rds.posccaesar.org/ontology/plm/rdl/PCA_100006233"/>
    <skos:member rdf:resource="http://rds.posccaesar.org/ontology/plm/rdl/PCA_100006384"/>
    <skos:member rdf:resource="http://rds.posccaesar.org/ontology/plm/rdl/PCA_100006295"/>
    <skos:member rdf:resource="http://rds.posccaesar.org/ontology/plm/rdl/PCA_100006147"/>
    <skos:member rdf:resource="http://rds.posccaesar.org/ontology/plm/rdl/PCA_100006422"/>
    <skos:member rdf:resource="http://rds.posccaesar.org/ontology/plm/rdl/PCA_100006484"/>
    <skos:member rdf:resource="http://rds.posccaesar.org/ontology/plm/rdl/PCA_100006497"/>
    <skos:member rdf:resource="http://rds.posccaesar.org/ontology/plm/rdl/PCA_100006409"/>
    <skos:member rdf:resource="http://rds.posccaesar.org/ontology/plm/rdl/PCA_100006287"/>
    <skos:member rdf:resource="http://rds.posccaesar.org/ontology/plm/rdl/PCA_100006116"/>
    <skos:member rdf:resource="http://rds.posccaesar.org/ontology/plm/rdl/PCA_100006178"/>
    <skos:member rdf:resource="http://rds.posccaesar.org/ontology/plm/rdl/PCA_100006373"/>
    <skos:member rdf:resource="http://rds.posccaesar.org/ontology/plm/rdl/PCA_100006284"/>
    <skos:member rdf:resource="http://rds.posccaesar.org/ontology/plm/rdl/PCA_100006406"/>
    <skos:member rdf:resource="http://rds.posccaesar.org/ontology/plm/rdl/PCA_100006326"/>
    <skos:member rdf:resource="http://rds.posccaesar.org/ontology/plm/rdl/PCA_100006108"/>
    <skos:member rdf:resource="http://rds.posccaesar.org/ontology/plm/rdl/PCA_100006525"/>
    <skos:member rdf:resource="http://rds.posccaesar.org/ontology/plm/rdl/PCA_100006445"/>
    <skos:member rdf:resource="http://rds.posccaesar.org/ontology/plm/rdl/PCA_100006356"/>
    <skos:member rdf:resource="http://rds.posccaesar.org/ontology/plm/rdl/PCA_100006276"/>
    <skos:member rdf:resource="http://rds.posccaesar.org/ontology/plm/rdl/PCA_100006105"/>
    <skos:member rdf:resource="http://rds.posccaesar.org/ontology/plm/rdl/PCA_100006080"/>
    <skos:member rdf:resource="http://rds.posccaesar.org/ontology/plm/rdl/PCA_100006531"/>
    <skos:member rdf:resource="http://rds.posccaesar.org/ontology/plm/rdl/PCA_100006167"/>
    <skos:member rdf:resource="http://rds.posccaesar.org/ontology/plm/rdl/PCA_100006442"/>
    <skos:member rdf:resource="http://rds.posccaesar.org/ontology/plm/rdl/PCA_100006245"/>
    <skos:member rdf:resource="http://rds.posccaesar.org/ontology/plm/rdl/PCA_100006429"/>
    <skos:member rdf:resource="http://rds.posccaesar.org/ontology/plm/rdl/PCA_100006159"/>
    <skos:member rdf:resource="http://rds.posccaesar.org/ontology/plm/rdl/PCA_100006434"/>
    <skos:member rdf:resource="http://rds.posccaesar.org/ontology/plm/rdl/PCA_100006345"/>
    <skos:member rdf:resource="http://rds.posccaesar.org/ontology/plm/rdl/PCA_100006360"/>
    <skos:member rdf:resource="http://rds.posccaesar.org/ontology/plm/rdl/PCA_100006271"/>
    <skos:member rdf:resource="http://rds.posccaesar.org/ontology/plm/rdl/PCA_100006461"/>
    <skos:member rdf:resource="http://rds.posccaesar.org/ontology/plm/rdl/PCA_100006186"/>
    <skos:member rdf:resource="http://rds.posccaesar.org/ontology/plm/rdl/PCA_100006097"/>
    <skos:member rdf:resource="http://rds.posccaesar.org/ontology/plm/rdl/PCA_100006128"/>
    <skos:member rdf:resource="http://rds.posccaesar.org/ontology/plm/rdl/PCA_100006314"/>
    <skos:member rdf:resource="http://rds.posccaesar.org/ontology/plm/rdl/PCA_100006228"/>
    <skos:member rdf:resource="http://rds.posccaesar.org/ontology/plm/rdl/PCA_100006154"/>
    <skos:member rdf:resource="http://rds.posccaesar.org/ontology/plm/rdl/PCA_100006234"/>
    <skos:member rdf:resource="http://rds.posccaesar.org/ontology/plm/rdl/PCA_100006296"/>
    <skos:member rdf:resource="http://rds.posccaesar.org/ontology/plm/rdl/PCA_100006418"/>
    <skos:member rdf:resource="http://rds.posccaesar.org/ontology/plm/rdl/PCA_100006329"/>
    <skos:member rdf:resource="http://rds.posccaesar.org/ontology/plm/rdl/PCA_100006533"/>
    <skos:member rdf:resource="http://rds.posccaesar.org/ontology/plm/rdl/PCA_100006498"/>
    <skos:member rdf:resource="http://rds.posccaesar.org/ontology/plm/rdl/PCA_100006264"/>
    <skos:member rdf:resource="http://rds.posccaesar.org/ontology/plm/rdl/PCA_100006450"/>
    <skos:member rdf:resource="http://rds.posccaesar.org/ontology/plm/rdl/PCA_100006117"/>
    <skos:member rdf:resource="http://rds.posccaesar.org/ontology/plm/rdl/PCA_100006179"/>
    <skos:member rdf:resource="http://rds.posccaesar.org/ontology/plm/rdl/PCA_100006502"/>
    <skos:member rdf:resource="http://rds.posccaesar.org/ontology/plm/rdl/PCA_100006413"/>
    <skos:member rdf:resource="http://rds.posccaesar.org/ontology/plm/rdl/PCA_100006380"/>
    <skos:member rdf:resource="http://rds.posccaesar.org/ontology/plm/rdl/PCA_100006291"/>
    <skos:member rdf:resource="http://rds.posccaesar.org/ontology/plm/rdl/PCA_100006143"/>
    <skos:member rdf:resource="http://rds.posccaesar.org/ontology/plm/rdl/PCA_100006480"/>
    <skos:member rdf:resource="http://rds.posccaesar.org/ontology/plm/rdl/PCA_100006493"/>
    <skos:member rdf:resource="http://rds.posccaesar.org/ontology/plm/rdl/PCA_100006357"/>
    <skos:member rdf:resource="http://rds.posccaesar.org/ontology/plm/rdl/PCA_100006405"/>
    <skos:member rdf:resource="http://rds.posccaesar.org/ontology/plm/rdl/PCA_100006283"/>
    <skos:member rdf:resource="http://rds.posccaesar.org/ontology/plm/rdl/PCA_100006112"/>
    <skos:member rdf:resource="http://rds.posccaesar.org/ontology/plm/rdl/PCA_100006316"/>
    <skos:member rdf:resource="http://rds.posccaesar.org/ontology/plm/rdl/PCA_100006174"/>
    <skos:member rdf:resource="http://rds.posccaesar.org/ontology/plm/rdl/PCA_100006280"/>
    <skos:member rdf:resource="http://rds.posccaesar.org/ontology/plm/rdl/PCA_100006402"/>
    <skos:member rdf:resource="http://rds.posccaesar.org/ontology/plm/rdl/PCA_100006322"/>
    <skos:member rdf:resource="http://rds.posccaesar.org/ontology/plm/rdl/PCA_100006104"/>
    <skos:member rdf:resource="http://rds.posccaesar.org/ontology/plm/rdl/PCA_100006521"/>
    <skos:member rdf:resource="http://rds.posccaesar.org/ontology/plm/rdl/PCA_100006166"/>
    <skos:member rdf:resource="http://rds.posccaesar.org/ontology/plm/rdl/PCA_100006441"/>
    <skos:member rdf:resource="http://rds.posccaesar.org/ontology/plm/rdl/PCA_100006352"/>
    <skos:member rdf:resource="http://rds.posccaesar.org/ontology/plm/rdl/PCA_100006272"/>
    <skos:member rdf:resource="http://rds.posccaesar.org/ontology/plm/rdl/PCA_100006101"/>
    <skos:member rdf:resource="http://rds.posccaesar.org/ontology/plm/rdl/PCA_100006163"/>
    <skos:member rdf:resource="http://rds.posccaesar.org/ontology/plm/rdl/PCA_100006205"/>
    <skos:member rdf:resource="http://rds.posccaesar.org/ontology/plm/rdl/PCA_100006389"/>
    <skos:member rdf:resource="http://rds.posccaesar.org/ontology/plm/rdl/PCA_100006098"/>
    <skos:member rdf:resource="http://rds.posccaesar.org/ontology/plm/rdl/PCA_100006241"/>
    <skos:member rdf:resource="http://rds.posccaesar.org/ontology/plm/rdl/PCA_100006425"/>
    <skos:member rdf:resource="http://rds.posccaesar.org/ontology/plm/rdl/PCA_100006155"/>
    <skos:member rdf:resource="http://rds.posccaesar.org/ontology/plm/rdl/PCA_100006430"/>
    <skos:member rdf:resource="http://rds.posccaesar.org/ontology/plm/rdl/PCA_100006341"/>
    <skos:member rdf:resource="http://rds.posccaesar.org/ontology/plm/rdl/PCA_100006538"/>
    <skos:member rdf:resource="http://rds.posccaesar.org/ontology/plm/rdl/PCA_100006543"/>
    <skos:member rdf:resource="http://rds.posccaesar.org/ontology/plm/rdl/PCA_100006182"/>
    <skos:member rdf:resource="http://rds.posccaesar.org/ontology/plm/rdl/PCA_100006093"/>
    <skos:member rdf:resource="http://rds.posccaesar.org/ontology/plm/rdl/PCA_100006124"/>
    <skos:member rdf:resource="http://rds.posccaesar.org/ontology/plm/rdl/PCA_100006328"/>
    <skos:member rdf:resource="http://rds.posccaesar.org/ontology/plm/rdl/PCA_100006310"/>
    <skos:member rdf:resource="http://rds.posccaesar.org/ontology/plm/rdl/PCA_100006219"/>
    <skos:member rdf:resource="http://rds.posccaesar.org/ontology/plm/rdl/PCA_100006224"/>
    <skos:member rdf:resource="http://rds.posccaesar.org/ontology/plm/rdl/PCA_100006230"/>
    <skos:member rdf:resource="http://rds.posccaesar.org/ontology/plm/rdl/PCA_100006150"/>
    <skos:member rdf:resource="http://rds.posccaesar.org/ontology/plm/rdl/PCA_100006292"/>
    <skos:member rdf:resource="http://rds.posccaesar.org/ontology/plm/rdl/PCA_100006414"/>
    <skos:member rdf:resource="http://rds.posccaesar.org/ontology/plm/rdl/PCA_100006494"/>
    <skos:member rdf:resource="http://rds.posccaesar.org/ontology/plm/rdl/PCA_100006260"/>
    <skos:member rdf:resource="http://rds.posccaesar.org/ontology/plm/rdl/PCA_100006302"/>
    <skos:member rdf:resource="http://rds.posccaesar.org/ontology/plm/rdl/PCA_100006089"/>
    <skos:member rdf:resource="http://rds.posccaesar.org/ontology/plm/rdl/PCA_100006477"/>
    <skos:member rdf:resource="http://rds.posccaesar.org/ontology/plm/rdl/PCA_100006113"/>
    <skos:member rdf:resource="http://rds.posccaesar.org/ontology/plm/rdl/PCA_100006317"/>
    <skos:member rdf:resource="http://rds.posccaesar.org/ontology/plm/rdl/PCA_100006175"/>
    <skos:member rdf:resource="http://rds.posccaesar.org/ontology/plm/rdl/PCA_100006086"/>
    <skos:member rdf:resource="http://rds.posccaesar.org/ontology/plm/rdl/PCA_100006208"/>
    <skos:member rdf:resource="http://rds.posccaesar.org/ontology/plm/rdl/PCA_100006529"/>
    <skos:member rdf:resource="http://rds.posccaesar.org/ontology/plm/rdl/PCA_100006078"/>
    <skos:member rdf:resource="http://rds.posccaesar.org/ontology/plm/rdl/PCA_100006353"/>
    <skos:member rdf:resource="http://rds.posccaesar.org/ontology/plm/rdl/PCA_100006401"/>
    <skos:member rdf:resource="http://rds.posccaesar.org/ontology/plm/rdl/PCA_100006366"/>
    <skos:member rdf:resource="http://rds.posccaesar.org/ontology/plm/rdl/PCA_100006170"/>
    <skos:member rdf:resource="http://rds.posccaesar.org/ontology/plm/rdl/PCA_100006277"/>
    <skos:member rdf:resource="http://rds.posccaesar.org/ontology/plm/rdl/PCA_100006466"/>
    <skos:member rdf:resource="http://rds.posccaesar.org/ontology/plm/rdl/PCA_100006396"/>
    <skos:member rdf:resource="http://rds.posccaesar.org/ontology/plm/rdl/PCA_100006518"/>
    <skos:member rdf:resource="http://rds.posccaesar.org/ontology/plm/rdl/PCA_100006100"/>
    <skos:member rdf:resource="http://rds.posccaesar.org/ontology/plm/rdl/PCA_100006162"/>
    <skos:member rdf:resource="http://rds.posccaesar.org/ontology/plm/rdl/PCA_100006435"/>
    <skos:member rdf:resource="http://rds.posccaesar.org/ontology/plm/rdl/PCA_100006539"/>
    <skos:member rdf:resource="http://rds.posccaesar.org/ontology/plm/rdl/PCA_100006201"/>
    <skos:member rdf:resource="http://rds.posccaesar.org/ontology/plm/rdl/PCA_100006305"/>
    <skos:member rdf:resource="http://rds.posccaesar.org/ontology/plm/rdl/PCA_100006385"/>
    <skos:member rdf:resource="http://rds.posccaesar.org/ontology/plm/rdl/PCA_100006094"/>
    <skos:member rdf:resource="http://rds.posccaesar.org/ontology/plm/rdl/PCA_100006311"/>
    <skos:member rdf:resource="http://rds.posccaesar.org/ontology/plm/rdl/PCA_100006338"/>
    <skos:member rdf:resource="http://rds.posccaesar.org/ontology/plm/rdl/PCA_100006489"/>
    <skos:member rdf:resource="http://rds.posccaesar.org/ontology/plm/rdl/PCA_100006151"/>
    <skos:member rdf:resource="http://rds.posccaesar.org/ontology/plm/rdl/PCA_100006149"/>
    <skos:member rdf:resource="http://rds.posccaesar.org/ontology/plm/rdl/PCA_100006486"/>
    <skos:member rdf:resource="http://rds.posccaesar.org/ontology/plm/rdl/PCA_100006534"/>
    <skos:member rdf:resource="http://rds.posccaesar.org/ontology/plm/rdl/PCA_100006120"/>
    <skos:member rdf:resource="http://rds.posccaesar.org/ontology/plm/rdl/PCA_100006289"/>
    <skos:member rdf:resource="http://rds.posccaesar.org/ontology/plm/rdl/PCA_100006220"/>
    <skos:member rdf:resource="http://rds.posccaesar.org/ontology/plm/rdl/PCA_100006478"/>
    <skos:member rdf:resource="http://rds.posccaesar.org/ontology/plm/rdl/PCA_100006257"/>
    <skos:member rdf:resource="http://rds.posccaesar.org/ontology/plm/rdl/PCA_100006490"/>
    <skos:member rdf:resource="http://rds.posccaesar.org/ontology/plm/rdl/PCA_100006527"/>
    <skos:member rdf:resource="http://rds.posccaesar.org/ontology/plm/rdl/PCA_100006085"/>
    <skos:member rdf:resource="http://rds.posccaesar.org/ontology/plm/rdl/PCA_100006207"/>
    <skos:member rdf:resource="http://rds.posccaesar.org/ontology/plm/rdl/PCA_100006447"/>
    <skos:member rdf:resource="http://rds.posccaesar.org/ontology/plm/rdl/PCA_100006358"/>
    <skos:member rdf:resource="http://rds.posccaesar.org/ontology/plm/rdl/PCA_100006473"/>
    <skos:member rdf:resource="http://rds.posccaesar.org/ontology/plm/rdl/PCA_100006411"/>
    <skos:member rdf:resource="http://rds.posccaesar.org/ontology/plm/rdl/PCA_100006171"/>
    <skos:member rdf:resource="http://rds.posccaesar.org/ontology/plm/rdl/PCA_100006198"/>
    <skos:member rdf:resource="http://rds.posccaesar.org/ontology/plm/rdl/PCA_100006278"/>
    <skos:member rdf:resource="http://rds.posccaesar.org/ontology/plm/rdl/PCA_100006082"/>
    <skos:member rdf:resource="http://rds.posccaesar.org/ontology/plm/rdl/PCA_100006246"/>
    <skos:member rdf:resource="http://rds.posccaesar.org/ontology/plm/rdl/PCA_100006397"/>
    <skos:member rdf:resource="http://rds.posccaesar.org/ontology/plm/rdl/PCA_100006347"/>
    <skos:member rdf:resource="http://rds.posccaesar.org/ontology/plm/rdl/PCA_100006362"/>
    <skos:member rdf:resource="http://rds.posccaesar.org/ontology/plm/rdl/PCA_100006273"/>
    <skos:member rdf:resource="http://rds.posccaesar.org/ontology/plm/rdl/PCA_100006546"/>
    <skos:member rdf:resource="http://rds.posccaesar.org/ontology/plm/rdl/PCA_100006187"/>
    <skos:member rdf:resource="http://rds.posccaesar.org/ontology/plm/rdl/PCA_100006462"/>
    <skos:member rdf:resource="http://rds.posccaesar.org/ontology/plm/rdl/PCA_100006129"/>
    <skos:member rdf:resource="http://rds.posccaesar.org/ontology/plm/rdl/PCA_100006392"/>
    <skos:member rdf:resource="http://rds.posccaesar.org/ontology/plm/rdl/PCA_100006514"/>
    <skos:member rdf:resource="http://rds.posccaesar.org/ontology/plm/rdl/PCA_100006520"/>
    <skos:member rdf:resource="http://rds.posccaesar.org/ontology/plm/rdl/PCA_100006449"/>
    <skos:member rdf:resource="http://rds.posccaesar.org/ontology/plm/rdl/PCA_100006156"/>
    <skos:member rdf:resource="http://rds.posccaesar.org/ontology/plm/rdl/PCA_100006431"/>
    <skos:member rdf:resource="http://rds.posccaesar.org/ontology/plm/rdl/PCA_100006269"/>
    <skos:member rdf:resource="http://rds.posccaesar.org/ontology/plm/rdl/PCA_100006535"/>
    <skos:member rdf:resource="http://rds.posccaesar.org/ontology/plm/rdl/PCA_100006266"/>
    <skos:member rdf:resource="http://rds.posccaesar.org/ontology/plm/rdl/PCA_100006090"/>
    <skos:member rdf:resource="http://rds.posccaesar.org/ontology/plm/rdl/PCA_100006381"/>
    <skos:member rdf:resource="http://rds.posccaesar.org/ontology/plm/rdl/PCA_100006503"/>
    <skos:member rdf:resource="http://rds.posccaesar.org/ontology/plm/rdl/PCA_100006148"/>
    <skos:member rdf:resource="http://rds.posccaesar.org/ontology/plm/rdl/PCA_100006423"/>
    <skos:member rdf:resource="http://rds.posccaesar.org/ontology/plm/rdl/PCA_100006334"/>
    <skos:member rdf:resource="http://rds.posccaesar.org/ontology/plm/rdl/PCA_100006485"/>
    <skos:member rdf:resource="http://rds.posccaesar.org/ontology/plm/rdl/PCA_100006145"/>
    <skos:member rdf:resource="http://rds.posccaesar.org/ontology/plm/rdl/PCA_100006420"/>
    <skos:member rdf:resource="http://rds.posccaesar.org/ontology/plm/rdl/PCA_100006258"/>
    <skos:member rdf:resource="http://rds.posccaesar.org/ontology/plm/rdl/PCA_100006482"/>
    <skos:member rdf:resource="http://rds.posccaesar.org/ontology/plm/rdl/PCA_100006217"/>
    <skos:member rdf:resource="http://rds.posccaesar.org/ontology/plm/rdl/PCA_100006359"/>
    <skos:member rdf:resource="http://rds.posccaesar.org/ontology/plm/rdl/PCA_100006407"/>
    <skos:member rdf:resource="http://rds.posccaesar.org/ontology/plm/rdl/PCA_100006285"/>
    <skos:member rdf:resource="http://rds.posccaesar.org/ontology/plm/rdl/PCA_100006323"/>
    <skos:member rdf:resource="http://rds.posccaesar.org/ontology/plm/rdl/PCA_100006318"/>
    <skos:member rdf:resource="http://rds.posccaesar.org/ontology/plm/rdl/PCA_100006199"/>
    <skos:member rdf:resource="http://rds.posccaesar.org/ontology/plm/rdl/PCA_100006474"/>
    <skos:member rdf:resource="http://rds.posccaesar.org/ontology/plm/rdl/PCA_100006253"/>
    <skos:member rdf:resource="http://rds.posccaesar.org/ontology/plm/rdl/PCA_100006526"/>
    <skos:member rdf:resource="http://rds.posccaesar.org/ontology/plm/rdl/PCA_100006437"/>
    <skos:member rdf:resource="http://rds.posccaesar.org/ontology/plm/rdl/PCA_100006523"/>
    <skos:member rdf:resource="http://rds.posccaesar.org/ontology/plm/rdl/PCA_100006106"/>
    <skos:member rdf:resource="http://rds.posccaesar.org/ontology/plm/rdl/PCA_100006081"/>
    <skos:member rdf:resource="http://rds.posccaesar.org/ontology/plm/rdl/PCA_100006443"/>
    <skos:member rdf:resource="http://rds.posccaesar.org/ontology/plm/rdl/PCA_100006168"/>
    <skos:member rdf:resource="http://rds.posccaesar.org/ontology/plm/rdl/PCA_100006079"/>
    <skos:member rdf:resource="http://rds.posccaesar.org/ontology/plm/rdl/PCA_100006354"/>
    <skos:member rdf:resource="http://rds.posccaesar.org/ontology/plm/rdl/PCA_100006194"/>
    <skos:member rdf:resource="http://rds.posccaesar.org/ontology/plm/rdl/PCA_100006274"/>
    <skos:member rdf:resource="http://rds.posccaesar.org/ontology/plm/rdl/PCA_100006136"/>
    <skos:member rdf:resource="http://rds.posccaesar.org/ontology/plm/rdl/PCA_100006242"/>
    <skos:member rdf:resource="http://rds.posccaesar.org/ontology/plm/rdl/PCA_100006393"/>
    <skos:member rdf:resource="http://rds.posccaesar.org/ontology/plm/rdl/PCA_100006515"/>
    <skos:member rdf:resource="http://rds.posccaesar.org/ontology/plm/rdl/PCA_100006426"/>
    <skos:member rdf:resource="http://rds.posccaesar.org/ontology/plm/rdl/PCA_100006346"/>
    <skos:member rdf:resource="http://rds.posccaesar.org/ontology/plm/rdl/PCA_100006459"/>
    <skos:member rdf:resource="http://rds.posccaesar.org/ontology/plm/rdl/PCA_100006432"/>
    <skos:member rdf:resource="http://rds.posccaesar.org/ontology/plm/rdl/PCA_100006157"/>
    <skos:member rdf:resource="http://rds.posccaesar.org/ontology/plm/rdl/PCA_100006309"/>
    <skos:member rdf:resource="http://rds.posccaesar.org/ontology/plm/rdl/PCA_100006343"/>
    <skos:member rdf:resource="http://rds.posccaesar.org/ontology/plm/rdl/PCA_100006183"/>
    <skos:member rdf:resource="http://rds.posccaesar.org/ontology/plm/rdl/PCA_100006125"/>
    <skos:member rdf:resource="http://rds.posccaesar.org/ontology/plm/rdl/PCA_100006229"/>
    <skos:member rdf:resource="http://rds.posccaesar.org/ontology/plm/rdl/PCA_100006510"/>
    <skos:member rdf:resource="http://rds.posccaesar.org/ontology/plm/rdl/PCA_100006335"/>
    <skos:member rdf:resource="http://rds.posccaesar.org/ontology/plm/rdl/PCA_100006226"/>
    <skos:member rdf:resource="http://rds.posccaesar.org/ontology/plm/rdl/PCA_100006152"/>
    <skos:member rdf:resource="http://rds.posccaesar.org/ontology/plm/rdl/PCA_100006265"/>
    <skos:member rdf:resource="http://rds.posccaesar.org/ontology/plm/rdl/PCA_100006262"/>
    <skos:member rdf:resource="http://rds.posccaesar.org/ontology/plm/rdl/PCA_100006378"/>
    <skos:member rdf:resource="http://rds.posccaesar.org/ontology/plm/rdl/PCA_100006109"/>
    <skos:member rdf:resource="http://rds.posccaesar.org/ontology/plm/rdl/PCA_100006144"/>
    <skos:member rdf:resource="http://rds.posccaesar.org/ontology/plm/rdl/PCA_100006330"/>
    <skos:member rdf:resource="http://rds.posccaesar.org/ontology/plm/rdl/PCA_100006481"/>
    <skos:member rdf:resource="http://rds.posccaesar.org/ontology/plm/rdl/PCA_100006319"/>
    <skos:member rdf:resource="http://rds.posccaesar.org/ontology/plm/rdl/PCA_100006479"/>
    <skos:member rdf:resource="http://rds.posccaesar.org/ontology/plm/rdl/PCA_100006141"/>
    <skos:member rdf:resource="http://rds.posccaesar.org/ontology/plm/rdl/PCA_100006254"/>
    <skos:member rdf:resource="http://rds.posccaesar.org/ontology/plm/rdl/PCA_100006438"/>
    <skos:member rdf:resource="http://rds.posccaesar.org/ontology/plm/rdl/PCA_100006367"/>
    <skos:member rdf:resource="http://rds.posccaesar.org/ontology/plm/rdl/PCA_100006213"/>
    <skos:member rdf:resource="http://rds.posccaesar.org/ontology/plm/rdl/PCA_100006355"/>
    <skos:member rdf:resource="http://rds.posccaesar.org/ontology/plm/rdl/PCA_100006281"/>
    <skos:member rdf:resource="http://rds.posccaesar.org/ontology/plm/rdl/PCA_100006403"/>
    <skos:member rdf:resource="http://rds.posccaesar.org/ontology/plm/rdl/PCA_100006195"/>
    <skos:member rdf:resource="http://rds.posccaesar.org/ontology/plm/rdl/PCA_100006470"/>
    <skos:member rdf:resource="http://rds.posccaesar.org/ontology/plm/rdl/PCA_100006137"/>
    <skos:member rdf:resource="http://rds.posccaesar.org/ontology/plm/rdl/PCA_100006468"/>
    <skos:member rdf:resource="http://rds.posccaesar.org/ontology/plm/rdl/PCA_100006522"/>
    <skos:member rdf:resource="http://rds.posccaesar.org/ontology/plm/rdl/PCA_100006398"/>
    <skos:member rdf:resource="http://rds.posccaesar.org/ontology/plm/rdl/PCA_100006102"/>
    <skos:member rdf:resource="http://rds.posccaesar.org/ontology/plm/rdl/PCA_100006164"/>
    <skos:member rdf:resource="http://rds.posccaesar.org/ontology/plm/rdl/PCA_100006350"/>
    <skos:member rdf:resource="http://rds.posccaesar.org/ontology/plm/rdl/PCA_100006202"/>
    <skos:member rdf:resource="http://rds.posccaesar.org/ontology/plm/rdl/PCA_100006190"/>
    <skos:member rdf:resource="http://rds.posccaesar.org/ontology/plm/rdl/PCA_100006270"/>
    <skos:member rdf:resource="http://rds.posccaesar.org/ontology/plm/rdl/PCA_100006132"/>
    <skos:member rdf:resource="http://rds.posccaesar.org/ontology/plm/rdl/PCA_100006239"/>
    <skos:member rdf:resource="http://rds.posccaesar.org/ontology/plm/rdl/PCA_100006307"/>
    <skos:member rdf:resource="http://rds.posccaesar.org/ontology/plm/rdl/PCA_100006511"/>
    <skos:member rdf:resource="http://rds.posccaesar.org/ontology/plm/rdl/PCA_100006387"/>
    <skos:member rdf:resource="http://rds.posccaesar.org/ontology/plm/rdl/PCA_100006342"/>
    <skos:member rdf:resource="http://rds.posccaesar.org/ontology/plm/rdl/PCA_100006544"/>
    <skos:member rdf:resource="http://rds.posccaesar.org/ontology/plm/rdl/PCA_100006153"/>
    <skos:member rdf:resource="http://rds.posccaesar.org/ontology/plm/rdl/PCA_100006455"/>
    <skos:member rdf:resource="http://rds.posccaesar.org/ontology/plm/rdl/PCA_100006541"/>
    <skos:member rdf:resource="http://rds.posccaesar.org/ontology/plm/rdl/PCA_100006507"/>
    <skos:member rdf:resource="http://rds.posccaesar.org/ontology/plm/rdl/PCA_100006121"/>
    <skos:member rdf:resource="http://rds.posccaesar.org/ontology/plm/rdl/PCA_100006379"/>
    <skos:member rdf:resource="http://rds.posccaesar.org/ontology/plm/rdl/PCA_100006225"/>
    <skos:member rdf:resource="http://rds.posccaesar.org/ontology/plm/rdl/PCA_100006331"/>
    <skos:member rdf:resource="http://rds.posccaesar.org/ontology/plm/rdl/PCA_100006222"/>
    <skos:member rdf:resource="http://rds.posccaesar.org/ontology/plm/rdl/PCA_100006261"/>
    <skos:member rdf:resource="http://rds.posccaesar.org/ontology/plm/rdl/PCA_100006259"/>
    <skos:member rdf:resource="http://rds.posccaesar.org/ontology/plm/rdl/PCA_100006374"/>
    <skos:member rdf:resource="http://rds.posccaesar.org/ontology/plm/rdl/PCA_100006300"/>
    <skos:member rdf:resource="http://rds.posccaesar.org/ontology/plm/rdl/PCA_100006087"/>
    <skos:member rdf:resource="http://rds.posccaesar.org/ontology/plm/rdl/PCA_100006209"/>
    <skos:member rdf:resource="http://rds.posccaesar.org/ontology/plm/rdl/PCA_100006214"/>
    <skos:member rdf:resource="http://rds.posccaesar.org/ontology/plm/rdl/PCA_100006140"/>
    <skos:member rdf:resource="http://rds.posccaesar.org/ontology/plm/rdl/PCA_100006315"/>
    <skos:member rdf:resource="http://rds.posccaesar.org/ontology/plm/rdl/PCA_100006475"/>
    <skos:member rdf:resource="http://rds.posccaesar.org/ontology/plm/rdl/PCA_100006250"/>
    <skos:member rdf:resource="http://rds.posccaesar.org/ontology/plm/rdl/PCA_100006532"/>
    <skos:member rdf:resource="http://rds.posccaesar.org/ontology/plm/rdl/PCA_100006248"/>
    <skos:member rdf:resource="http://rds.posccaesar.org/ontology/plm/rdl/PCA_100006399"/>
    <skos:member rdf:resource="http://rds.posccaesar.org/ontology/plm/rdl/PCA_100006363"/>
    <skos:member rdf:resource="http://rds.posccaesar.org/ontology/plm/rdl/PCA_100006467"/>
    <skos:member rdf:resource="http://rds.posccaesar.org/ontology/plm/rdl/PCA_100006351"/>
    <skos:member rdf:resource="http://rds.posccaesar.org/ontology/plm/rdl/PCA_100006191"/>
    <skos:member rdf:resource="http://rds.posccaesar.org/ontology/plm/rdl/PCA_100006519"/>
    <skos:member rdf:resource="http://rds.posccaesar.org/ontology/plm/rdl/PCA_100006133"/>
    <skos:member rdf:resource="http://rds.posccaesar.org/ontology/plm/rdl/PCA_100006189"/>
    <skos:member rdf:resource="http://rds.posccaesar.org/ontology/plm/rdl/PCA_100006464"/>
    <skos:member rdf:resource="http://rds.posccaesar.org/ontology/plm/rdl/PCA_100006394"/>
    <skos:member rdf:resource="http://rds.posccaesar.org/ontology/plm/rdl/PCA_100006516"/>
    <skos:member rdf:resource="http://rds.posccaesar.org/ontology/plm/rdl/PCA_100006160"/>
    <skos:member rdf:resource="http://rds.posccaesar.org/ontology/plm/rdl/PCA_100006456"/>
    <skos:member rdf:resource="http://rds.posccaesar.org/ontology/plm/rdl/PCA_100006306"/>
    <skos:member rdf:resource="http://rds.posccaesar.org/ontology/plm/rdl/PCA_100006508"/>
    <skos:member rdf:resource="http://rds.posccaesar.org/ontology/plm/rdl/PCA_100006235"/>
    <skos:member rdf:resource="http://rds.posccaesar.org/ontology/plm/rdl/PCA_100006386"/>
    <skos:member rdf:resource="http://rds.posccaesar.org/ontology/plm/rdl/PCA_100006297"/>
    <skos:member rdf:resource="http://rds.posccaesar.org/ontology/plm/rdl/PCA_100006419"/>
    <skos:member rdf:resource="http://rds.posccaesar.org/ontology/plm/rdl/PCA_100006303"/>
    <skos:member rdf:resource="http://rds.posccaesar.org/ontology/plm/rdl/PCA_100006499"/>
    <skos:member rdf:resource="http://rds.posccaesar.org/ontology/plm/rdl/PCA_100006383"/>
    <skos:member rdf:resource="http://rds.posccaesar.org/ontology/plm/rdl/PCA_100006505"/>
    <skos:member rdf:resource="http://rds.posccaesar.org/ontology/plm/rdl/PCA_100006336"/>
    <skos:member rdf:resource="http://rds.posccaesar.org/ontology/plm/rdl/PCA_100006487"/>
    <skos:member rdf:resource="http://rds.posccaesar.org/ontology/plm/rdl/PCA_100006540"/>
    <skos:member rdf:resource="http://rds.posccaesar.org/ontology/plm/rdl/PCA_100006451"/>
    <skos:member rdf:resource="http://rds.posccaesar.org/ontology/plm/rdl/PCA_100006118"/>
    <skos:member rdf:resource="http://rds.posccaesar.org/ontology/plm/rdl/PCA_100006375"/>
    <skos:member rdf:resource="http://rds.posccaesar.org/ontology/plm/rdl/PCA_100006286"/>
    <skos:member rdf:resource="http://rds.posccaesar.org/ontology/plm/rdl/PCA_100006221"/>
    <skos:member rdf:resource="http://rds.posccaesar.org/ontology/plm/rdl/PCA_100006325"/>
    <skos:member rdf:resource="http://rds.posccaesar.org/ontology/plm/rdl/PCA_100006476"/>
    <skos:member rdf:resource="http://rds.posccaesar.org/ontology/plm/rdl/PCA_100006528"/>
    <skos:member rdf:resource="http://rds.posccaesar.org/ontology/plm/rdl/PCA_100006255"/>
    <skos:member rdf:resource="http://rds.posccaesar.org/ontology/plm/rdl/PCA_100006107"/>
    <skos:member rdf:resource="http://rds.posccaesar.org/ontology/plm/rdl/PCA_100006439"/>
    <skos:member rdf:resource="http://rds.posccaesar.org/ontology/plm/rdl/PCA_100006169"/>
    <skos:member rdf:resource="http://rds.posccaesar.org/ontology/plm/rdl/PCA_100006444"/>
    <skos:member rdf:resource="http://rds.posccaesar.org/ontology/plm/rdl/PCA_100006370"/>
    <skos:member rdf:resource="http://rds.posccaesar.org/ontology/plm/rdl/PCA_100006083"/>
    <skos:member rdf:resource="http://rds.posccaesar.org/ontology/plm/rdl/PCA_100006210"/>
    <skos:member rdf:resource="http://rds.posccaesar.org/ontology/plm/rdl/PCA_100006247"/>
    <skos:member rdf:resource="http://rds.posccaesar.org/ontology/plm/rdl/PCA_100006196"/>
    <skos:member rdf:resource="http://rds.posccaesar.org/ontology/plm/rdl/PCA_100006471"/>
    <skos:member rdf:resource="http://rds.posccaesar.org/ontology/plm/rdl/PCA_100006138"/>
    <skos:member rdf:resource="http://rds.posccaesar.org/ontology/plm/rdl/PCA_100006244"/>
    <skos:member rdf:resource="http://rds.posccaesar.org/ontology/plm/rdl/PCA_100006395"/>
    <skos:member rdf:resource="http://rds.posccaesar.org/ontology/plm/rdl/PCA_100006517"/>
    <skos:member rdf:resource="http://rds.posccaesar.org/ontology/plm/rdl/PCA_100006428"/>
    <skos:member rdf:resource="http://rds.posccaesar.org/ontology/plm/rdl/PCA_100006348"/>
    <skos:member rdf:resource="http://rds.posccaesar.org/ontology/plm/rdl/PCA_100006463"/>
    <skos:member rdf:resource="http://rds.posccaesar.org/ontology/plm/rdl/PCA_100006188"/>
    <skos:member rdf:resource="http://rds.posccaesar.org/ontology/plm/rdl/PCA_100006099"/>
    <skos:member rdf:resource="http://rds.posccaesar.org/ontology/plm/rdl/PCA_100006236"/>
    <skos:member rdf:resource="http://rds.posccaesar.org/ontology/plm/rdl/PCA_100006185"/>
    <skos:member rdf:resource="http://rds.posccaesar.org/ontology/plm/rdl/PCA_100006460"/>
    <skos:member rdf:resource="http://rds.posccaesar.org/ontology/plm/rdl/PCA_100006298"/>
    <skos:member rdf:resource="http://rds.posccaesar.org/ontology/plm/rdl/PCA_100006127"/>
    <skos:member rdf:resource="http://rds.posccaesar.org/ontology/plm/rdl/PCA_100006390"/>
    <skos:member rdf:resource="http://rds.posccaesar.org/ontology/plm/rdl/PCA_100006512"/>
    <skos:member rdf:resource="http://rds.posccaesar.org/ontology/plm/rdl/PCA_100006337"/>
    <skos:member rdf:resource="http://rds.posccaesar.org/ontology/plm/rdl/PCA_100006452"/>
    <skos:member rdf:resource="http://rds.posccaesar.org/ontology/plm/rdl/PCA_100006267"/>
    <skos:member rdf:resource="http://rds.posccaesar.org/ontology/plm/rdl/PCA_100006119"/>
    <skos:member rdf:resource="http://rds.posccaesar.org/ontology/plm/rdl/PCA_100006504"/>
    <skos:member rdf:resource="http://rds.posccaesar.org/ontology/plm/rdl/PCA_100006231"/>
    <skos:member rdf:resource="http://rds.posccaesar.org/ontology/plm/rdl/PCA_100006382"/>
    <skos:member rdf:resource="http://rds.posccaesar.org/ontology/plm/rdl/PCA_100006293"/>
    <skos:member rdf:resource="http://rds.posccaesar.org/ontology/plm/rdl/PCA_100006415"/>
    <skos:member rdf:resource="http://rds.posccaesar.org/ontology/plm/rdl/PCA_100006495"/>
    <skos:member rdf:resource="http://rds.posccaesar.org/ontology/plm/rdl/PCA_100006501"/>
    <skos:member rdf:resource="http://rds.posccaesar.org/ontology/plm/rdl/PCA_100006146"/>
    <skos:member rdf:resource="http://rds.posccaesar.org/ontology/plm/rdl/PCA_100006421"/>
    <skos:member rdf:resource="http://rds.posccaesar.org/ontology/plm/rdl/PCA_100006332"/>
    <skos:member rdf:resource="http://rds.posccaesar.org/ontology/plm/rdl/PCA_100006483"/>
    <skos:member rdf:resource="http://rds.posccaesar.org/ontology/plm/rdl/PCA_100006114"/>
    <skos:member rdf:resource="http://rds.posccaesar.org/ontology/plm/rdl/PCA_100006176"/>
    <skos:member rdf:resource="http://rds.posccaesar.org/ontology/plm/rdl/PCA_100006256"/>
    <skos:member rdf:resource="http://rds.posccaesar.org/ontology/plm/rdl/PCA_100006371"/>
    <skos:member rdf:resource="http://rds.posccaesar.org/ontology/plm/rdl/PCA_100006282"/>
    <skos:member rdf:resource="http://rds.posccaesar.org/ontology/plm/rdl/PCA_100006404"/>
    <skos:member rdf:resource="http://rds.posccaesar.org/ontology/plm/rdl/PCA_100006369"/>
    <skos:member rdf:resource="http://rds.posccaesar.org/ontology/plm/rdl/PCA_100006324"/>
    <skos:member rdf:resource="http://rds.posccaesar.org/ontology/plm/rdl/PCA_100006215"/>
    <skos:member rdf:resource="http://rds.posccaesar.org/ontology/plm/rdl/PCA_100006410"/>
    <skos:member rdf:resource="http://rds.posccaesar.org/ontology/plm/rdl/PCA_100006321"/>
    <skos:member rdf:resource="http://rds.posccaesar.org/ontology/plm/rdl/PCA_100006197"/>
    <skos:member rdf:resource="http://rds.posccaesar.org/ontology/plm/rdl/PCA_100006472"/>
    <skos:member rdf:resource="http://rds.posccaesar.org/ontology/plm/rdl/PCA_100006139"/>
    <skos:member rdf:resource="http://rds.posccaesar.org/ontology/plm/rdl/PCA_100006251"/>
    <skos:member rdf:resource="http://rds.posccaesar.org/ontology/plm/rdl/PCA_100006103"/>
    <skos:member rdf:resource="http://rds.posccaesar.org/ontology/plm/rdl/PCA_100006524"/>
    <skos:member rdf:resource="http://rds.posccaesar.org/ontology/plm/rdl/PCA_100006165"/>
    <skos:member rdf:resource="http://rds.posccaesar.org/ontology/plm/rdl/PCA_100006440"/>
    <skos:member rdf:resource="http://rds.posccaesar.org/ontology/plm/rdl/PCA_100006204"/>
    <skos:member rdf:resource="http://rds.posccaesar.org/ontology/plm/rdl/PCA_100006192"/>
    <skos:member rdf:resource="http://rds.posccaesar.org/ontology/plm/rdl/PCA_100006243"/>
    <skos:member rdf:resource="http://rds.posccaesar.org/ontology/plm/rdl/PCA_100006427"/>
    <skos:member rdf:resource="http://rds.posccaesar.org/ontology/plm/rdl/PCA_100006134"/>
    <skos:member rdf:resource="http://rds.posccaesar.org/ontology/plm/rdl/PCA_100006240"/>
    <skos:member rdf:resource="http://rds.posccaesar.org/ontology/plm/rdl/PCA_100006391"/>
    <skos:member rdf:resource="http://rds.posccaesar.org/ontology/plm/rdl/PCA_100006513"/>
    <skos:member rdf:resource="http://rds.posccaesar.org/ontology/plm/rdl/PCA_100006424"/>
    <skos:member rdf:resource="http://rds.posccaesar.org/ontology/plm/rdl/PCA_100006344"/>
    <skos:member rdf:resource="http://rds.posccaesar.org/ontology/plm/rdl/PCA_100006184"/>
    <skos:member rdf:resource="http://rds.posccaesar.org/ontology/plm/rdl/PCA_100006095"/>
    <skos:member rdf:resource="http://rds.posccaesar.org/ontology/plm/rdl/PCA_100006126"/>
    <skos:member rdf:resource="http://rds.posccaesar.org/ontology/plm/rdl/PCA_100006457"/>
    <skos:member rdf:resource="http://rds.posccaesar.org/ontology/plm/rdl/PCA_100006312"/>
    <skos:member rdf:resource="http://rds.posccaesar.org/ontology/plm/rdl/PCA_100006509"/>
    <skos:member rdf:resource="http://rds.posccaesar.org/ontology/plm/rdl/PCA_100006181"/>
    <skos:member rdf:resource="http://rds.posccaesar.org/ontology/plm/rdl/PCA_100006232"/>
    <skos:member rdf:resource="http://rds.posccaesar.org/ontology/plm/rdl/PCA_100006416"/>
    <skos:member rdf:resource="http://rds.posccaesar.org/ontology/plm/rdl/PCA_100006294"/>
    <skos:member rdf:resource="http://rds.posccaesar.org/ontology/plm/rdl/PCA_100006123"/>
    <skos:member rdf:resource="http://rds.posccaesar.org/ontology/plm/rdl/PCA_100006327"/>
    <skos:member rdf:resource="http://rds.posccaesar.org/ontology/plm/rdl/PCA_100006227"/>
    <skos:member rdf:resource="http://rds.posccaesar.org/ontology/plm/rdl/PCA_100006496"/>
    <skos:member rdf:resource="http://rds.posccaesar.org/ontology/plm/rdl/PCA_100006333"/>
    <skos:member rdf:resource="http://rds.posccaesar.org/ontology/plm/rdl/PCA_100006263"/>
    <skos:member rdf:resource="http://rds.posccaesar.org/ontology/plm/rdl/PCA_100006115"/>
    <skos:member rdf:resource="http://rds.posccaesar.org/ontology/plm/rdl/PCA_100006301"/>
    <skos:member rdf:resource="http://rds.posccaesar.org/ontology/plm/rdl/PCA_100006177"/>
    <skos:member rdf:resource="http://rds.posccaesar.org/ontology/plm/rdl/PCA_100006088"/>
    <skos:member rdf:resource="http://rds.posccaesar.org/ontology/plm/rdl/PCA_100006500"/>
    <skos:member rdf:resource="http://rds.posccaesar.org/ontology/plm/rdl/PCA_100006376"/>
    <skos:member rdf:resource="http://rds.posccaesar.org/ontology/plm/rdl/PCA_100006491"/>
    <skos:member rdf:resource="http://rds.posccaesar.org/ontology/plm/rdl/PCA_100006216"/>
    <skos:member rdf:resource="http://rds.posccaesar.org/ontology/plm/rdl/PCA_100006142"/>
    <skos:member rdf:resource="http://rds.posccaesar.org/ontology/plm/rdl/PCA_100006368"/>
    <skos:member rdf:resource="http://rds.posccaesar.org/ontology/plm/rdl/PCA_100006172"/>
    <skos:member rdf:resource="http://rds.posccaesar.org/ontology/plm/rdl/PCA_100006110"/>
    <skos:member rdf:resource="http://rds.posccaesar.org/ontology/plm/rdl/PCA_100006252"/>
    <skos:member rdf:resource="http://rds.posccaesar.org/ontology/plm/rdl/PCA_100006279"/>
    <skos:member rdf:resource="http://rds.posccaesar.org/ontology/plm/rdl/PCA_100006436"/>
    <skos:member rdf:resource="http://rds.posccaesar.org/ontology/plm/rdl/PCA_100006400"/>
    <skos:member rdf:resource="http://rds.posccaesar.org/ontology/plm/rdl/PCA_100006365"/>
    <skos:member rdf:resource="http://rds.posccaesar.org/ontology/plm/rdl/PCA_100006320"/>
    <skos:member rdf:resource="http://rds.posccaesar.org/ontology/plm/rdl/PCA_100006211"/>
  </rdf:Description>
  <rdf:Description rdf:about="http://rds.posccaesar.org/ontology/plm/rdl/PCA_100006770">
    <skos:member>
      <rdl:PCA_100001503 rdf:about="http://rds.posccaesar.org/ontology/plm/rdl/PCA_100006690">
        <rdfs:label>advertising information</rdfs:label>
        <rdl:PCA_100004924>DE</rdl:PCA_100004924>
        <rdf:type rdf:resource="http://www.w3.org/2002/07/owl#NamedIndividual"/>
      </rdl:PCA_100001503>
    </skos:member>
    <skos:member>
      <rdl:PCA_100001503 rdf:about="http://rds.posccaesar.org/ontology/plm/rdl/PCA_100006681">
        <rdfs:label>insurance information</rdfs:label>
        <rdl:PCA_100004924>CF</rdl:PCA_100004924>
        <rdf:type rdf:resource="http://www.w3.org/2002/07/owl#NamedIndividual"/>
      </rdl:PCA_100001503>
    </skos:member>
    <skos:member rdf:resource="http://rds.posccaesar.org/ontology/plm/rdl/PCA_100006691"/>
    <skos:member>
      <rdl:PCA_100001503 rdf:about="http://rds.posccaesar.org/ontology/plm/rdl/PCA_100006658">
        <rdfs:label>meta</rdfs:label>
        <rdl:PCA_100004924>A</rdl:PCA_100004924>
        <rdf:type rdf:resource="http://www.w3.org/2002/07/owl#NamedIndividual"/>
      </rdl:PCA_100001503>
    </skos:member>
    <skos:member>
      <rdl:PCA_100001503 rdf:about="http://rds.posccaesar.org/ontology/plm/rdl/PCA_100006659">
        <rdfs:label>identification information</rdfs:label>
        <rdl:PCA_100004924>AA</rdl:PCA_100004924>
        <rdf:type rdf:resource="http://www.w3.org/2002/07/owl#NamedIndividual"/>
      </rdl:PCA_100001503>
    </skos:member>
    <skos:member rdf:resource="http://rds.posccaesar.org/ontology/plm/rdl/PCA_100006706"/>
    <skos:member rdf:resource="http://rds.posccaesar.org/ontology/plm/rdl/PCA_100006707"/>
    <skos:member rdf:resource="http://rds.posccaesar.org/ontology/plm/rdl/PCA_100006732"/>
    <skos:member rdf:resource="http://rds.posccaesar.org/ontology/plm/rdl/PCA_100006731"/>
    <skos:member rdf:resource="http://rds.posccaesar.org/ontology/plm/rdl/PCA_100006693"/>
    <skos:member>
      <rdl:PCA_100001503 rdf:about="http://rds.posccaesar.org/ontology/plm/rdl/PCA_100006683">
        <rdfs:label>expertise information</rdfs:label>
        <rdl:PCA_100004924>CH</rdl:PCA_100004924>
        <rdf:type rdf:resource="http://www.w3.org/2002/07/owl#NamedIndividual"/>
      </rdl:PCA_100001503>
    </skos:member>
    <skos:member rdf:resource="http://rds.posccaesar.org/ontology/plm/rdl/PCA_100006722"/>
    <skos:member>
      <rdl:PCA_100001503 rdf:about="http://rds.posccaesar.org/ontology/plm/rdl/PCA_100006684">
        <rdfs:label>ownership information</rdfs:label>
        <rdl:PCA_100004924>CJ</rdl:PCA_100004924>
        <rdf:type rdf:resource="http://www.w3.org/2002/07/owl#NamedIndividual"/>
      </rdl:PCA_100001503>
    </skos:member>
    <skos:member>
      <rdl:PCA_100001503 rdf:about="http://rds.posccaesar.org/ontology/plm/rdl/PCA_100006674">
        <rdfs:label>information control management</rdfs:label>
        <rdl:PCA_100004924>BW</rdl:PCA_100004924>
        <rdf:type rdf:resource="http://www.w3.org/2002/07/owl#NamedIndividual"/>
      </rdl:PCA_100001503>
    </skos:member>
    <skos:member rdf:resource="http://rds.posccaesar.org/ontology/plm/rdl/PCA_100006697"/>
    <skos:member rdf:resource="http://rds.posccaesar.org/ontology/plm/rdl/PCA_100006687"/>
    <skos:member rdf:resource="http://rds.posccaesar.org/ontology/plm/rdl/PCA_100006688"/>
    <skos:member rdf:resource="http://rds.posccaesar.org/ontology/plm/rdl/PCA_100006709"/>
    <skos:member rdf:resource="http://rds.posccaesar.org/ontology/plm/rdl/PCA_100006663"/>
    <skos:member rdf:resource="http://rds.posccaesar.org/ontology/plm/rdl/PCA_100006666"/>
    <skos:member rdf:resource="http://rds.posccaesar.org/ontology/plm/rdl/PCA_100006734"/>
    <skos:member rdf:resource="http://rds.posccaesar.org/ontology/plm/rdl/PCA_100006724"/>
    <skos:member>
      <rdl:PCA_100001503 rdf:about="http://rds.posccaesar.org/ontology/plm/rdl/PCA_100006725">
        <rdfs:label>safety</rdfs:label>
        <rdl:PCA_100004924>R</rdl:PCA_100004924>
        <rdf:type rdf:resource="http://www.w3.org/2002/07/owl#NamedIndividual"/>
      </rdl:PCA_100001503>
    </skos:member>
    <skos:member rdf:resource="http://rds.posccaesar.org/ontology/plm/rdl/PCA_100006715"/>
    <skos:member>
      <rdl:PCA_100001503 rdf:about="http://rds.posccaesar.org/ontology/plm/rdl/PCA_100006704">
        <rdfs:label>layout</rdfs:label>
        <rdl:PCA_100004924>L</rdl:PCA_100004924>
        <rdf:type rdf:resource="http://www.w3.org/2002/07/owl#NamedIndividual"/>
      </rdl:PCA_100001503>
    </skos:member>
    <skos:member rdf:resource="http://rds.posccaesar.org/ontology/plm/rdl/PCA_100006668"/>
    <skos:member rdf:resource="http://rds.posccaesar.org/ontology/plm/rdl/PCA_100006716"/>
    <skos:member>
      <rdl:PCA_100001503 rdf:about="http://rds.posccaesar.org/ontology/plm/rdl/PCA_100006680">
        <rdfs:label>payment information</rdfs:label>
        <rdl:PCA_100004924>CE</rdl:PCA_100004924>
        <rdf:type rdf:resource="http://www.w3.org/2002/07/owl#NamedIndividual"/>
      </rdl:PCA_100001503>
    </skos:member>
    <skos:member>
      <rdl:PCA_100001503 rdf:about="http://rds.posccaesar.org/ontology/plm/rdl/PCA_100006670">
        <rdfs:label>change management information</rdfs:label>
        <rdl:PCA_100004924>BH</rdl:PCA_100004924>
        <rdf:type rdf:resource="http://www.w3.org/2002/07/owl#NamedIndividual"/>
      </rdl:PCA_100001503>
    </skos:member>
    <skos:member rdf:resource="http://rds.posccaesar.org/ontology/plm/rdl/PCA_100006705"/>
    <skos:member>
      <rdl:PCA_100001503 rdf:about="http://rds.posccaesar.org/ontology/plm/rdl/PCA_100006730">
        <rdfs:label>geometrical form</rdfs:label>
        <rdl:PCA_100004924>T</rdl:PCA_100004924>
        <rdf:type rdf:resource="http://www.w3.org/2002/07/owl#NamedIndividual"/>
      </rdl:PCA_100001503>
    </skos:member>
    <skos:member>
      <rdl:PCA_100001503 rdf:about="http://rds.posccaesar.org/ontology/plm/rdl/PCA_100006721">
        <rdfs:label>quality</rdfs:label>
        <rdl:PCA_100004924>Q</rdl:PCA_100004924>
        <rdf:type rdf:resource="http://www.w3.org/2002/07/owl#NamedIndividual"/>
      </rdl:PCA_100001503>
    </skos:member>
    <skos:member rdf:resource="http://rds.posccaesar.org/ontology/plm/rdl/PCA_100006720"/>
    <skos:member>
      <rdl:PCA_100001503 rdf:about="http://rds.posccaesar.org/ontology/plm/rdl/PCA_100006682">
        <rdfs:label>warranty information</rdfs:label>
        <rdl:PCA_100004924>CG</rdl:PCA_100004924>
        <rdf:type rdf:resource="http://www.w3.org/2002/07/owl#NamedIndividual"/>
      </rdl:PCA_100001503>
    </skos:member>
    <skos:member rdf:resource="http://rds.posccaesar.org/ontology/plm/rdl/PCA_100006672"/>
    <skos:member>
      <rdl:PCA_100001503 rdf:about="http://rds.posccaesar.org/ontology/plm/rdl/PCA_100006711">
        <rdfs:label>interface</rdfs:label>
        <rdl:PCA_100004924>M</rdl:PCA_100004924>
        <rdf:type rdf:resource="http://www.w3.org/2002/07/owl#NamedIndividual"/>
      </rdl:PCA_100001503>
    </skos:member>
    <skos:member>
      <rdl:PCA_100001503 rdf:about="http://rds.posccaesar.org/ontology/plm/rdl/PCA_100006673">
        <rdfs:label>training information</rdfs:label>
        <rdl:PCA_100004924>BU</rdl:PCA_100004924>
        <rdf:type rdf:resource="http://www.w3.org/2002/07/owl#NamedIndividual"/>
      </rdl:PCA_100001503>
    </skos:member>
    <skos:member rdf:resource="http://rds.posccaesar.org/ontology/plm/rdl/PCA_100006686"/>
    <skos:member>
      <rdl:PCA_100001503 rdf:about="http://rds.posccaesar.org/ontology/plm/rdl/PCA_100006676">
        <rdfs:label>tender information</rdfs:label>
        <rdl:PCA_100004924>CA</rdl:PCA_100004924>
        <rdf:type rdf:resource="http://www.w3.org/2002/07/owl#NamedIndividual"/>
      </rdl:PCA_100001503>
    </skos:member>
    <skos:member>
      <rdl:PCA_100001503 rdf:about="http://rds.posccaesar.org/ontology/plm/rdl/PCA_100006677">
        <rdfs:label>authority approval information</rdfs:label>
        <rdl:PCA_100004924>CB</rdl:PCA_100004924>
        <rdf:type rdf:resource="http://www.w3.org/2002/07/owl#NamedIndividual"/>
      </rdl:PCA_100001503>
    </skos:member>
    <skos:member>
      <rdl:PCA_100001503 rdf:about="http://rds.posccaesar.org/ontology/plm/rdl/PCA_100006661">
        <rdfs:label>descriptive meta information</rdfs:label>
        <rdl:PCA_100004924>AC</rdl:PCA_100004924>
        <rdf:type rdf:resource="http://www.w3.org/2002/07/owl#NamedIndividual"/>
      </rdl:PCA_100001503>
    </skos:member>
    <skos:member rdf:resource="http://rds.posccaesar.org/ontology/plm/rdl/PCA_100006700"/>
    <skos:member>
      <rdl:PCA_100001503 rdf:about="http://rds.posccaesar.org/ontology/plm/rdl/PCA_100006662">
        <rdfs:label>management</rdfs:label>
        <rdl:PCA_100004924>B</rdl:PCA_100004924>
        <rdf:type rdf:resource="http://www.w3.org/2002/07/owl#NamedIndividual"/>
      </rdl:PCA_100001503>
    </skos:member>
    <skos:member>
      <rdl:PCA_100001503 rdf:about="http://rds.posccaesar.org/ontology/plm/rdl/PCA_100006665">
        <rdfs:label>correspondence information</rdfs:label>
        <rdl:PCA_100004924>BC</rdl:PCA_100004924>
        <rdf:type rdf:resource="http://www.w3.org/2002/07/owl#NamedIndividual"/>
      </rdl:PCA_100001503>
    </skos:member>
    <skos:member>
      <rdl:PCA_100001503 rdf:about="http://rds.posccaesar.org/ontology/plm/rdl/PCA_100006723">
        <rdfs:label>quality action information</rdfs:label>
        <rdl:PCA_100004924>QD</rdl:PCA_100004924>
        <rdf:type rdf:resource="http://www.w3.org/2002/07/owl#NamedIndividual"/>
      </rdl:PCA_100001503>
    </skos:member>
    <skos:member rdf:resource="http://rds.posccaesar.org/ontology/plm/rdl/PCA_100006713"/>
    <skos:member rdf:resource="http://rds.posccaesar.org/ontology/plm/rdl/PCA_100006696"/>
    <skos:member>
      <rdl:PCA_100001503 rdf:about="http://rds.posccaesar.org/ontology/plm/rdl/PCA_100006714">
        <rdfs:label>enumeration</rdfs:label>
        <rdl:PCA_100004924>P</rdl:PCA_100004924>
        <rdf:type rdf:resource="http://www.w3.org/2002/07/owl#NamedIndividual"/>
      </rdl:PCA_100001503>
    </skos:member>
    <skos:member rdf:resource="http://rds.posccaesar.org/ontology/plm/rdl/PCA_100006702"/>
    <skos:member rdf:resource="http://rds.posccaesar.org/ontology/plm/rdl/PCA_100006703"/>
    <skos:member>
      <rdl:PCA_100001503 rdf:about="http://rds.posccaesar.org/ontology/plm/rdl/PCA_100006678">
        <rdfs:label>agreement information</rdfs:label>
        <rdl:PCA_100004924>CC</rdl:PCA_100004924>
        <rdf:type rdf:resource="http://www.w3.org/2002/07/owl#NamedIndividual"/>
      </rdl:PCA_100001503>
    </skos:member>
    <skos:member>
      <rdl:PCA_100001503 rdf:about="http://rds.posccaesar.org/ontology/plm/rdl/PCA_100006737">
        <rdfs:label>recording information</rdfs:label>
        <rdl:PCA_100004924>WT</rdl:PCA_100004924>
        <rdf:type rdf:resource="http://www.w3.org/2002/07/owl#NamedIndividual"/>
      </rdl:PCA_100001503>
    </skos:member>
    <skos:member rdf:resource="http://rds.posccaesar.org/ontology/plm/rdl/PCA_100006728"/>
    <skos:member rdf:resource="http://rds.posccaesar.org/ontology/plm/rdl/PCA_100006729"/>
    <skos:member>
      <rdl:PCA_100001503 rdf:about="http://rds.posccaesar.org/ontology/plm/rdl/PCA_100006719">
        <rdfs:label>function listing</rdfs:label>
        <rdl:PCA_100004924>PF</rdl:PCA_100004924>
        <rdf:type rdf:resource="http://www.w3.org/2002/07/owl#NamedIndividual"/>
      </rdl:PCA_100001503>
    </skos:member>
    <skos:member>
      <rdl:PCA_100001503 rdf:about="http://rds.posccaesar.org/ontology/plm/rdl/PCA_100006671">
        <rdfs:label>economy information</rdfs:label>
        <rdl:PCA_100004924>BJ</rdl:PCA_100004924>
        <rdf:type rdf:resource="http://www.w3.org/2002/07/owl#NamedIndividual"/>
      </rdl:PCA_100001503>
    </skos:member>
    <skos:member>
      <rdl:PCA_100001503 rdf:about="http://rds.posccaesar.org/ontology/plm/rdl/PCA_100006692">
        <rdfs:label>regulatory requirement information</rdfs:label>
        <rdl:PCA_100004924>DG</rdl:PCA_100004924>
        <rdf:type rdf:resource="http://www.w3.org/2002/07/owl#NamedIndividual"/>
      </rdl:PCA_100001503>
    </skos:member>
    <skos:member rdf:resource="http://rds.posccaesar.org/ontology/plm/rdl/PCA_100006710"/>
    <skos:member>
      <rdl:PCA_100001503 rdf:about="http://rds.posccaesar.org/ontology/plm/rdl/PCA_100006675">
        <rdfs:label>contractual</rdfs:label>
        <rdl:PCA_100004924>C</rdl:PCA_100004924>
        <rdf:type rdf:resource="http://www.w3.org/2002/07/owl#NamedIndividual"/>
      </rdl:PCA_100001503>
    </skos:member>
    <skos:member rdf:resource="http://rds.posccaesar.org/ontology/plm/rdl/PCA_100006708"/>
    <skos:member rdf:resource="http://rds.posccaesar.org/ontology/plm/rdl/PCA_100006660"/>
    <skos:member rdf:resource="http://rds.posccaesar.org/ontology/plm/rdl/PCA_100006664"/>
    <skos:member rdf:resource="http://rds.posccaesar.org/ontology/plm/rdl/PCA_100006733"/>
    <skos:member>
      <rdl:PCA_100001503 rdf:about="http://rds.posccaesar.org/ontology/plm/rdl/PCA_100006694">
        <rdfs:label>functionality</rdfs:label>
        <rdl:PCA_100004924>F</rdl:PCA_100004924>
        <rdf:type rdf:resource="http://www.w3.org/2002/07/owl#NamedIndividual"/>
      </rdl:PCA_100001503>
    </skos:member>
    <skos:member rdf:resource="http://rds.posccaesar.org/ontology/plm/rdl/PCA_100006712"/>
    <skos:member rdf:resource="http://rds.posccaesar.org/ontology/plm/rdl/PCA_100006695"/>
    <skos:member>
      <rdl:PCA_100001503 rdf:about="http://rds.posccaesar.org/ontology/plm/rdl/PCA_100006685">
        <rdfs:label>capability</rdfs:label>
        <rdl:PCA_100004924>D</rdl:PCA_100004924>
        <rdf:type rdf:resource="http://www.w3.org/2002/07/owl#NamedIndividual"/>
      </rdl:PCA_100001503>
    </skos:member>
    <skos:member rdf:resource="http://rds.posccaesar.org/ontology/plm/rdl/PCA_100006698"/>
    <skos:member rdf:resource="http://rds.posccaesar.org/ontology/plm/rdl/PCA_100006699"/>
    <skos:member rdf:resource="http://rds.posccaesar.org/ontology/plm/rdl/PCA_100006689"/>
    <skos:member rdf:resource="http://rds.posccaesar.org/ontology/plm/rdl/PCA_100006701"/>
    <skos:member rdf:resource="http://rds.posccaesar.org/ontology/plm/rdl/PCA_100006667"/>
    <skos:member>
      <rdl:PCA_100001503 rdf:about="http://rds.posccaesar.org/ontology/plm/rdl/PCA_100006735">
        <rdfs:label>operational</rdfs:label>
        <rdl:PCA_100004924>W</rdl:PCA_100004924>
        <rdf:type rdf:resource="http://www.w3.org/2002/07/owl#NamedIndividual"/>
      </rdl:PCA_100001503>
    </skos:member>
    <skos:member>
      <rdl:PCA_100001503 rdf:about="http://rds.posccaesar.org/ontology/plm/rdl/PCA_100006736">
        <rdfs:label>processing information</rdfs:label>
        <rdl:PCA_100004924>WA</rdl:PCA_100004924>
        <rdf:type rdf:resource="http://www.w3.org/2002/07/owl#NamedIndividual"/>
      </rdl:PCA_100001503>
    </skos:member>
    <skos:member rdf:resource="http://rds.posccaesar.org/ontology/plm/rdl/PCA_100006726"/>
    <skos:member>
      <rdl:PCA_100001503 rdf:about="http://rds.posccaesar.org/ontology/plm/rdl/PCA_100006679">
        <rdfs:label>order information</rdfs:label>
        <rdl:PCA_100004924>CD</rdl:PCA_100004924>
        <rdf:type rdf:resource="http://www.w3.org/2002/07/owl#NamedIndividual"/>
      </rdl:PCA_100001503>
    </skos:member>
    <skos:member>
      <rdl:PCA_100001503 rdf:about="http://rds.posccaesar.org/ontology/plm/rdl/PCA_100006669">
        <rdfs:label>organizational information</rdfs:label>
        <rdl:PCA_100004924>BG</rdl:PCA_100004924>
        <rdf:type rdf:resource="http://www.w3.org/2002/07/owl#NamedIndividual"/>
      </rdl:PCA_100001503>
    </skos:member>
    <skos:member rdf:resource="http://rds.posccaesar.org/ontology/plm/rdl/PCA_100006727"/>
    <skos:member rdf:resource="http://rds.posccaesar.org/ontology/plm/rdl/PCA_100006717"/>
    <skos:member rdf:resource="http://rds.posccaesar.org/ontology/plm/rdl/PCA_100006718"/>
  </rdf:Description>
</rdf:RDF>
